@prefix core:  <https://github.com/VCityTeam/UD-Graph/Ontologies/core#> .
@prefix iso19150-2: <http://def.isotc211.org/iso19150/-2/2012/base#> .
@prefix wtr:   <https://github.com/VCityTeam/UD-Graph/Ontologies/waterbody#> .
@prefix rdf:   <http://www.w3.org/1999/02/22-rdf-syntax-ns#> .
@prefix owl:   <http://www.w3.org/2002/07/owl#> .
@prefix xsd:   <http://www.w3.org/2001/XMLSchema#> .
@prefix skos:  <http://www.w3.org/2004/02/skos/core#> .
@prefix rdfs:  <http://www.w3.org/2000/01/rdf-schema#> .

wtr:WaterBodyClassValue
        a                owl:Class ;
        rdfs:subClassOf  skos:Concept ;
        skos:definition  "WaterBodyClassValue is a code list used to further classify a WaterBody."@en ;
        skos:prefLabel   "WaterBodyClassValue"@en .

wtr:WaterSurface.waterLevel
        a                owl:ObjectProperty ;
        rdfs:domain      wtr:WaterSurface ;
        rdfs:range       wtr:WaterLevelValue ;
        skos:definition  "Specifies the level of the WaterSurface."@en ;
        skos:prefLabel   "waterLevel"@en .

wtr:WaterLevelValue  a   owl:Class ;
        rdfs:subClassOf  skos:Concept ;
        skos:definition  "WaterLevelValue is a code list that enumerates the different levels of a water surface."@en ;
        skos:prefLabel   "WaterLevelValue"@en .

wtr:WaterBody.function
        a                owl:ObjectProperty ;
        rdfs:domain      wtr:WaterBody ;
        rdfs:range       wtr:WaterBodyFunctionValue ;
        skos:definition  "Specifies the intended purposes of the WaterBody."@en ;
        skos:prefLabel   "function"@en .

wtr:ADEOfWaterGroundSurface
        a                      owl:Class ;
        iso19150-2:isAbstract  true ;
        skos:definition        "ADEOfWaterGroundSurface acts as a hook to define properties within an ADE that are to be added to a WaterGroundSurface."@en ;
        skos:prefLabel         "ADEOfWaterGroundSurface"@en .

wtr:ADEOfAbstractWaterBoundarySurface
        a                      owl:Class ;
        iso19150-2:isAbstract  true ;
        skos:definition        "ADEOfAbstractWaterBoundarySurface acts as a hook to define properties within an ADE that are to be added to AbstractWaterBoundarySurface."@en ;
        skos:prefLabel         "ADEOfAbstractWaterBoundarySurface"@en .

<https://github.com/VCityTeam/UD-Graph/Ontologies/waterbody>
        a                owl:Ontology ;
        owl:imports      <https://github.com/VCityTeam/UD-Graph/Ontologies/core> , <http://def.isotc211.org/iso19150/-2/2012/base> ;
        owl:versionIRI   "https://github.com/VCityTeam/UD-Graph/Ontologies/waterbody/3.0.0" ;
        owl:versionInfo  "3.0.0" ;
        skos:definition  "The WaterBody module supports representation of the thematic aspects and 3D geometry of rivers, canals, lakes, and basins. It does, however, not inherit any hydrological or other dynamic aspects of fluid flow."@en ;
        skos:prefLabel   "WaterBody"@en .

wtr:WaterBody.usage  a   owl:ObjectProperty ;
        rdfs:domain      wtr:WaterBody ;
        rdfs:range       wtr:WaterBodyUsageValue ;
        skos:definition  "Specifies the actual uses of the WaterBody."@en ;
        skos:prefLabel   "usage"@en .

wtr:WaterBodyFunctionValue
        a                owl:Class ;
        rdfs:subClassOf  skos:Concept ;
        skos:definition  "WaterBodyFunctionValue is a code list that enumerates the different purposes of a WaterBody."@en ;
        skos:prefLabel   "WaterBodyFunctionValue"@en .

wtr:WaterBody.class  a   owl:ObjectProperty ;
        rdfs:domain      wtr:WaterBody ;
        rdfs:range       wtr:WaterBodyClassValue ;
        skos:definition  "Indicates the specific type of the WaterBody."@en ;
        skos:prefLabel   "class"@en .

wtr:ADEOfWaterBody  a          owl:Class ;
        iso19150-2:isAbstract  true ;
        skos:definition        "ADEOfWaterBody acts as a hook to define properties within an ADE that are to be added to a WaterBody."@en ;
        skos:prefLabel         "ADEOfWaterBody"@en .

wtr:WaterSurface  a      owl:Class ;
        rdfs:subClassOf  wtr:AbstractWaterBoundarySurface ;
        skos:definition  "A WaterSurface represents the upper exterior interface between a water body and the atmosphere."@en ;
        skos:prefLabel   "WaterSurface"@en .

wtr:WaterGroundSurface.adeOfWaterGroundSurface
        a                owl:ObjectProperty ;
        rdfs:domain      wtr:WaterGroundSurface ;
        rdfs:range       wtr:ADEOfWaterGroundSurface ;
        skos:definition  "Augments the WaterGroundSurface with properties defined in an ADE."@en ;
        skos:prefLabel   "adeOfWaterGroundSurface"@en .

wtr:AbstractWaterBoundarySurface.adeOfAbstractWaterBoundarySurface
        a                owl:ObjectProperty ;
        rdfs:domain      wtr:AbstractWaterBoundarySurface ;
        rdfs:range       wtr:ADEOfAbstractWaterBoundarySurface ;
        skos:definition  "Augments AbstractWaterBoundarySurface with properties defined in an ADE."@en ;
        skos:prefLabel   "adeOfAbstractWaterBoundarySurface"@en .

wtr:WaterBody.adeOfWaterBody
        a                owl:ObjectProperty ;
        rdfs:domain      wtr:WaterBody ;
        rdfs:range       wtr:ADEOfWaterBody ;
        skos:definition  "Augments the WaterBody with properties defined in an ADE."@en ;
        skos:prefLabel   "adeOfWaterBody"@en .

wtr:AbstractWaterBoundarySurface
        a                      owl:Class ;
        rdfs:subClassOf        core:AbstractThematicSurface ;
        iso19150-2:isAbstract  true ;
        skos:definition        "AbstractWaterBoundarySurface is the abstract superclass for all kinds of thematic surfaces bounding a water body."@en ;
        skos:prefLabel         "AbstractWaterBoundarySurface"@en .

wtr:WaterGroundSurface
        a                owl:Class ;
        rdfs:subClassOf  wtr:AbstractWaterBoundarySurface ;
        skos:definition  "A WaterGroundSurface represents the exterior boundary surface of the submerged bottom of a water body."@en ;
        skos:prefLabel   "WaterGroundSurface"@en .

wtr:WaterBodyUsageValue
        a                owl:Class ;
        rdfs:subClassOf  skos:Concept ;
        skos:definition  "WaterBodyUsageValue is a code list that enumerates the different uses of a WaterBody."@en ;
        skos:prefLabel   "WaterBodyUsageValue"@en .

wtr:ADEOfWaterSurface
        a                      owl:Class ;
        iso19150-2:isAbstract  true ;
        skos:definition        "ADEOfWaterSurface acts as a hook to define properties within an ADE that are to be added to a WaterSurface."@en ;
        skos:prefLabel         "ADEOfWaterSurface"@en .

wtr:WaterBody.boundary
        a               owl:ObjectProperty ;
        rdfs:domain     wtr:WaterBody ;
        rdfs:range      wtr:AbstractWaterBoundarySurface ;
        skos:prefLabel  "boundary"@en .

wtr:WaterBody  a         owl:Class ;
        rdfs:subClassOf  core:AbstractOccupiedSpace ;
        skos:definition  "A WaterBody represents significant and permanent or semi-permanent accumulations of surface water, usually covering a part of the Earth."@en ;
        skos:prefLabel   "WaterBody"@en .

wtr:WaterSurface.adeOfWaterSurface
        a                owl:ObjectProperty ;
        rdfs:domain      wtr:WaterSurface ;
        rdfs:range       wtr:ADEOfWaterSurface ;
        skos:definition  "Augments the WaterSurface with properties defined in an ADE."@en ;
        skos:prefLabel   "adeOfWaterSurface"@en .
