@prefix core:  <https://github.com/VCityTeam/UD-Graph/Ontologies/core#> .
@prefix frn:   <https://github.com/VCityTeam/UD-Graph/Ontologies/cityfurniture#> .
@prefix iso19150-2: <http://def.isotc211.org/iso19150/-2/2012/base#> .
@prefix rdf:   <http://www.w3.org/1999/02/22-rdf-syntax-ns#> .
@prefix owl:   <http://www.w3.org/2002/07/owl#> .
@prefix xsd:   <http://www.w3.org/2001/XMLSchema#> .
@prefix skos:  <http://www.w3.org/2004/02/skos/core#> .
@prefix rdfs:  <http://www.w3.org/2000/01/rdf-schema#> .

frn:CityFurniture.class
        a                owl:ObjectProperty ;
        rdfs:domain      frn:CityFurniture ;
        rdfs:range       frn:CityFurnitureClassValue ;
        skos:definition  "Indicates the specific type of the CityFurniture."@en ;
        skos:prefLabel   "class"@en .

<https://github.com/VCityTeam/UD-Graph/Ontologies/cityfurniture>
        a                owl:Ontology ;
        owl:imports      <https://github.com/VCityTeam/UD-Graph/Ontologies/core> , <http://def.isotc211.org/iso19150/-2/2012/base> ;
        owl:versionIRI   "https://github.com/VCityTeam/UD-Graph/Ontologies/cityfurniture/3.0.0" ;
        owl:versionInfo  "3.0.0" ;
        skos:definition  "The CityFurniture module supports representation of city furniture objects. City furniture objects are immovable objects like lanterns, traffic signs, advertising columns, benches, or bus stops that can be found in traffic areas, residential areas, on squares, or in built-up areas."@en ;
        skos:prefLabel   "CityFurniture"@en .

frn:ADEOfCityFurniture
        a                      owl:Class ;
        iso19150-2:isAbstract  true ;
        skos:definition        "ADEOfCityFurniture acts as a hook to define properties within an ADE that are to be added to a CityFurniture."@en ;
        skos:prefLabel         "ADEOfCityFurniture"@en .

frn:CityFurnitureUsageValue
        a                owl:Class ;
        rdfs:subClassOf  skos:Concept ;
        skos:definition  "CityFurnitureUsageValue is a code list that enumerates the different uses of a CityFurniture."@en ;
        skos:prefLabel   "CityFurnitureUsageValue"@en .

frn:CityFurniture.adeOfCityFurniture
        a                owl:ObjectProperty ;
        rdfs:domain      frn:CityFurniture ;
        rdfs:range       frn:ADEOfCityFurniture ;
        skos:definition  "Augments the CityFurniture with properties defined in an ADE."@en ;
        skos:prefLabel   "adeOfCityFurniture"@en .

frn:CityFurniture.usage
        a                owl:ObjectProperty ;
        rdfs:domain      frn:CityFurniture ;
        rdfs:range       frn:CityFurnitureUsageValue ;
        skos:definition  "Specifies the actual uses of the CityFurniture."@en ;
        skos:prefLabel   "usage"@en .

frn:CityFurnitureFunctionValue
        a                owl:Class ;
        rdfs:subClassOf  skos:Concept ;
        skos:definition  "CityFurnitureFunctionValue is a code list that enumerates the different purposes of a CityFurniture."@en ;
        skos:prefLabel   "CityFurnitureFunctionValue"@en .

frn:CityFurnitureClassValue
        a                owl:Class ;
        rdfs:subClassOf  skos:Concept ;
        skos:definition  "CityFurnitureClassValue is a code list used to further classify a CityFurniture."@en ;
        skos:prefLabel   "CityFurnitureClassValue"@en .

frn:CityFurniture.function
        a                owl:ObjectProperty ;
        rdfs:domain      frn:CityFurniture ;
        rdfs:range       frn:CityFurnitureFunctionValue ;
        skos:definition  "Specifies the intended purposes of the CityFurniture."@en ;
        skos:prefLabel   "function"@en .

frn:CityFurniture  a     owl:Class ;
        rdfs:subClassOf  core:AbstractOccupiedSpace ;
        skos:definition  "CityFurniture is an object or piece of equipment installed in the outdoor environment for various purposes. Examples include street signs, traffic signals, street lamps, benches, fountains."@en ;
        skos:prefLabel   "CityFurniture"@en .
