<rdf:RDF xmlns:math="http://www.w3.org/2005/xpath-functions/math" xmlns:owl="http://www.w3.org/2002/07/owl#" xmlns:rdf="http://www.w3.org/1999/02/22-rdf-syntax-ns#" xmlns:rdfs="http://www.w3.org/2000/01/rdf-schema#" xmlns:xs="http://www.w3.org/2001/XMLSchema" xmlns:xsd="http://www.w3.org/2001/XMLSchema">
   <owl:Ontology rdf:about="http://liris.cnrs.fr/ontologies/gmlBase">
      <owl:imports rdf:resource="http://liris.cnrs.fr/ontologies/gml"/>
      <owl:imports rdf:resource="http://liris.cnrs.fr/ontologies/basicTypes"/>
      <owl:imports rdf:resource="http://liris.cnrs.fr/ontologies/xlink"/>
      <rdfs:seeAlso>urn:opengis:specification:gml:schema-xsd:gmlBase:3.1.1</rdfs:seeAlso>
      <rdfs:comment>GML base schema for GML 3
			Components to support the GML encoding model.
			The abstract Schematron rules can be used by any schema that includes gmlBase.
			
			GML is an OGC Standard.
			Copyright (c) 2001,2005,2010 Open Geospatial Consortium.
			To obtain additional rights of use, visit http://www.opengeospatial.org/legal/ .
		</rdfs:comment>
   </owl:Ontology>
   <owl:Class rdf:about="http://www.opengis.net/gml#AbstractGMLType">
      <rdfs:comment>This is an abstract class</rdfs:comment>
      <rdfs:comment>All complexContent GML elements are directly or indirectly derived from this abstract supertype 
	to establish a hierarchy of GML types that may be distinguished from other XML types by their ancestry. 
	Elements in this hierarchy may have an ID and are thus referenceable.</rdfs:comment>
      <rdfs:subClassOf rdf:resource="http://www.opengis.net/gml#StandardObjectProperties"/>
      <rdfs:subClassOf>
         <owl:Class>
            <owl:intersectionOf rdf:parseType="Collection">
               <owl:Restriction>
                  <owl:onProperty rdf:resource="http://www.opengis.net/gml#hasid"/>
                  <owl:allValuesFrom rdf:resource="http://www.opengis.net/gml#id"/>
               </owl:Restriction>
            </owl:intersectionOf>
         </owl:Class>
      </rdfs:subClassOf>
   </owl:Class>
   <owl:Class rdf:about="http://www.opengis.net/gml#BagType">
      <rdfs:comment>A non-abstract generic collection type that can be used as a document element for a collection of any GML types - Geometries, Topologies, Features ...

FeatureCollections may only contain Features.  GeometryCollections may only contain Geometrys.  Bags are less constrained  they must contain objects that are substitutable for gml:_Object.  This may mix several levels, including Features, Definitions, Dictionaries, Geometries etc.  

The content model would ideally be 
   member 0..*
   members 0..1
   member 0..*
for maximum flexibility in building a collection from both homogeneous and distinct components: 
included "member" elements each contain a single Object
an included "members" element contains a set of Objects 

However, this is non-deterministic, thus prohibited by XSD.</rdfs:comment>
      <rdfs:subClassOf>
         <owl:Class>
            <owl:intersectionOf rdf:parseType="Collection">
               <owl:Restriction>
                  <owl:onProperty rdf:resource="http://www.opengis.net/gml#hasmember"/>
                  <owl:allValuesFrom rdf:resource="http://www.opengis.net/gml#member"/>
               </owl:Restriction>
               <owl:Restriction>
                  <owl:onProperty rdf:resource="http://www.opengis.net/gml#hasmember"/>
                  <owl:minCardinality rdf:datatype="http://www.w3.org/2001/XMLSchema#nonNegativeInteger">0</owl:minCardinality>
               </owl:Restriction>
               <owl:Restriction>
                  <owl:onProperty rdf:resource="http://www.opengis.net/gml#hasmembers"/>
                  <owl:allValuesFrom rdf:resource="http://www.opengis.net/gml#members"/>
               </owl:Restriction>
               <owl:Restriction>
                  <owl:onProperty rdf:resource="http://www.opengis.net/gml#hasmembers"/>
                  <owl:minCardinality rdf:datatype="http://www.w3.org/2001/XMLSchema#nonNegativeInteger">0</owl:minCardinality>
               </owl:Restriction>
            </owl:intersectionOf>
         </owl:Class>
      </rdfs:subClassOf>
      <rdfs:subClassOf rdf:resource="http://www.opengis.net/gml#AbstractGMLType"/>
   </owl:Class>
   <owl:Class rdf:about="http://www.opengis.net/gml#ArrayType">
      <rdfs:comment>A non-abstract generic collection type that can be used as a document element for a homogeneous collection of any GML types - Geometries, Topologies, Features ...</rdfs:comment>
      <rdfs:subClassOf>
         <owl:Class>
            <owl:intersectionOf rdf:parseType="Collection">
               <owl:Restriction>
                  <owl:onProperty rdf:resource="http://www.opengis.net/gml#hasmembers"/>
                  <owl:allValuesFrom rdf:resource="http://www.opengis.net/gml#members"/>
               </owl:Restriction>
               <owl:Restriction>
                  <owl:onProperty rdf:resource="http://www.opengis.net/gml#hasmembers"/>
                  <owl:minCardinality rdf:datatype="http://www.w3.org/2001/XMLSchema#nonNegativeInteger">0</owl:minCardinality>
               </owl:Restriction>
            </owl:intersectionOf>
         </owl:Class>
      </rdfs:subClassOf>
      <rdfs:subClassOf rdf:resource="http://www.opengis.net/gml#AbstractGMLType"/>
   </owl:Class>
   <owl:Class rdf:about="http://www.opengis.net/gml#AbstractMetaDataType">
      <rdfs:comment>This is an abstract class</rdfs:comment>
      <rdfs:comment>An abstract base type for complex metadata types.</rdfs:comment>
      <rdfs:subClassOf>
         <owl:Class>
            <owl:intersectionOf rdf:parseType="Collection">
               <owl:Restriction>
                  <owl:onProperty rdf:resource="http://www.opengis.net/gml#hasid"/>
                  <owl:allValuesFrom rdf:resource="http://www.opengis.net/gml#id"/>
               </owl:Restriction>
            </owl:intersectionOf>
         </owl:Class>
      </rdfs:subClassOf>
   </owl:Class>
   <owl:Class rdf:about="http://www.opengis.net/gml#GenericMetaDataType">
      <rdfs:comment>Deprecated with GML version 3.1.0.</rdfs:comment>
      <rdfs:subClassOf rdf:resource="http://www.opengis.net/gml#AbstractMetaDataType"/>
   </owl:Class>
   <owl:Class rdf:about="http://www.opengis.net/gml#AssociationType">
      <rdfs:comment>A pattern or base for derived types used to specify complex types corresponding to an  unspecified UML association - either composition or aggregation.  Restricts the cardinality of Objects contained in the association to a maximum of one.  An instance of this type can contain an element representing an Object, or serve as a pointer to a remote Object.  

Descendents of this type can be restricted in an application schema to 
* allow only specified classes as valid participants in the aggregation
* allow only association by reference (i.e. empty the content model) or by value (i.e. remove the xlinks).    

When used for association by reference, the value of the gml:remoteSchema attribute can be used to locate a schema fragment that constrains the target instance.   

In many cases it is desirable to impose the constraint prohibiting the occurence of both reference and value in the same instance, as that would be ambiguous.  This is accomplished by adding a directive in the annotation element of the element declaration.  This directive can be in the form of normative prose, or can use a Schematron pattern to automatically constrain co-occurrence - see the declaration for _strictAssociation below.   

If co-occurence is not prohibited, then both a link and content may be present.  If this occurs in an instance, then the rule for interpretation is that the instance found by traversing the href provides the normative value of the property, and should be used when possible.  The value(s) included as content may be used if the remote instance cannot be resolved.  This may be considered to be a "cached" version of the value(s).</rdfs:comment>
      <rdfs:subClassOf>
         <owl:Class>
            <owl:intersectionOf rdf:parseType="Collection">
               <owl:Restriction>
                  <owl:onProperty rdf:resource="http://www.opengis.net/gml#has_Object"/>
                  <owl:allValuesFrom rdf:resource="http://www.opengis.net/gml#_Object"/>
               </owl:Restriction>
            </owl:intersectionOf>
         </owl:Class>
      </rdfs:subClassOf>
   </owl:Class>
   <owl:Class rdf:about="http://www.opengis.net/gml#ReferenceType">
      <rdfs:comment>A pattern or base for derived types used to specify complex types corresponding to a UML aggregation association.  An instance of this type serves as a pointer to a remote Object.</rdfs:comment>
   </owl:Class>
   <owl:Class rdf:about="http://www.opengis.net/gml#ArrayAssociationType">
      <rdfs:comment>A base for derived types used to specify complex types containing an array of objects, by unspecified UML association - either composition or aggregation.  An instance of this type contains elements representing Objects.

Ideally this type would be derived by extension of AssociationType.  
However, this leads to a non-deterministic content model, since both the base and the extension have minOccurs="0", and is thus prohibited in XML Schema.</rdfs:comment>
      <rdfs:subClassOf>
         <owl:Class>
            <owl:intersectionOf rdf:parseType="Collection">
               <owl:Restriction>
                  <owl:onProperty rdf:resource="http://www.opengis.net/gml#has_Object"/>
                  <owl:allValuesFrom rdf:resource="http://www.opengis.net/gml#_Object"/>
               </owl:Restriction>
               <owl:Restriction>
                  <owl:onProperty rdf:resource="http://www.opengis.net/gml#has_Object"/>
                  <owl:minCardinality rdf:datatype="http://www.w3.org/2001/XMLSchema#nonNegativeInteger">0</owl:minCardinality>
               </owl:Restriction>
            </owl:intersectionOf>
         </owl:Class>
      </rdfs:subClassOf>
   </owl:Class>
   <owl:Class rdf:about="http://www.opengis.net/gml#MetaDataPropertyType">
      <rdfs:comment>Base type for complex metadata property types.</rdfs:comment>
      <rdfs:subClassOf>
         <owl:Class>
            <owl:intersectionOf rdf:parseType="Collection">
               <owl:Restriction>
                  <owl:onProperty rdf:resource="http://www.opengis.net/gml#about"/>
                  <owl:allValuesFrom rdf:resource="http://www.w3.org/2001/XMLSchema#anyURI"/>
               </owl:Restriction>
            </owl:intersectionOf>
         </owl:Class>
      </rdfs:subClassOf>
   </owl:Class>
   <owl:Class rdf:about="http://www.opengis.net/gml#StringOrRefType">
      <rdfs:comment>This type is available wherever there is a need for a "text" type property. It is of string type, so the text can be included inline, but the value can also be referenced remotely via xlinks from the AssociationAttributeGroup. If the remote reference is present, then the value obtained by traversing the link should be used, and the string content of the element can be used for an annotation.</rdfs:comment>
      <rdfs:subClassOf>
         <owl:Restriction>
            <owl:onProperty rdf:resource="http://www.opengis.net/gml#hasstring"/>
            <owl:someValuesFrom rdf:resource="http://www.w3.org/2001/XMLSchema#string"/>
         </owl:Restriction>
      </rdfs:subClassOf>
   </owl:Class>
   <owl:DatatypeProperty rdf:about="http://www.opengis.net/gml#hasstring">
      <rdfs:domain rdf:resource="http://www.opengis.net/gml#StringOrRefType"/>
      <rdfs:range rdf:resource="http://www.w3.org/2001/XMLSchema#string"/>
   </owl:DatatypeProperty>
   <owl:Class rdf:about="http://www.opengis.net/gml#StandardObjectProperties">
      <rdfs:subClassOf>
         <owl:Class>
            <owl:intersectionOf rdf:parseType="Collection">
               <owl:Restriction>
                  <owl:onProperty rdf:resource="http://www.opengis.net/gml#hasmetaDataProperty"/>
                  <owl:allValuesFrom rdf:resource="http://www.opengis.net/gml#metaDataProperty"/>
               </owl:Restriction>
               <owl:Restriction>
                  <owl:onProperty rdf:resource="http://www.opengis.net/gml#hasmetaDataProperty"/>
                  <owl:minCardinality rdf:datatype="http://www.w3.org/2001/XMLSchema#nonNegativeInteger">0</owl:minCardinality>
               </owl:Restriction>
               <owl:Restriction>
                  <owl:onProperty rdf:resource="http://www.opengis.net/gml#hasdescription"/>
                  <owl:allValuesFrom rdf:resource="http://www.opengis.net/gml#description"/>
               </owl:Restriction>
               <owl:Restriction>
                  <owl:onProperty rdf:resource="http://www.opengis.net/gml#hasdescription"/>
                  <owl:minCardinality rdf:datatype="http://www.w3.org/2001/XMLSchema#nonNegativeInteger">0</owl:minCardinality>
               </owl:Restriction>
               <owl:Restriction>
                  <owl:onProperty rdf:resource="http://www.opengis.net/gml#hasname"/>
                  <owl:allValuesFrom rdf:resource="http://www.opengis.net/gml#name"/>
               </owl:Restriction>
               <owl:Restriction>
                  <owl:onProperty rdf:resource="http://www.opengis.net/gml#hasname"/>
                  <owl:minCardinality rdf:datatype="http://www.w3.org/2001/XMLSchema#nonNegativeInteger">0</owl:minCardinality>
               </owl:Restriction>
            </owl:intersectionOf>
         </owl:Class>
      </rdfs:subClassOf>
      <rdfs:comment>This content model group makes it easier to construct types that 
      derive from AbstractGMLType and its descendents "by restriction".  
      A reference to the group saves having to enumerate the standard object properties.</rdfs:comment>
   </owl:Class>
   <owl:Class rdf:about="http://www.opengis.net/gml#AssociationAttributeGroup">
      <rdfs:subClassOf>
         <owl:Class>
            <owl:intersectionOf rdf:parseType="Collection">
               <owl:Restriction>
                  <owl:onProperty rdf:resource="http://www.opengis.net/gml#hasremoteSchema"/>
                  <owl:allValuesFrom rdf:resource="http://www.opengis.net/gml#remoteSchema"/>
               </owl:Restriction>
            </owl:intersectionOf>
         </owl:Class>
      </rdfs:subClassOf>
      <rdfs:comment>Attribute group used to enable property elements to refer to their value remotely. It contains the simple link components from xlinks.xsd, with all members optional, and the remoteSchema attribute, which is also optional.  These attributes can be attached to any element, thus allowing it to act as a pointer. The 'remoteSchema' attribute allows an element  that carries link attributes to indicate that the element is declared  in a remote schema rather than by the schema that constrains the current document instance.</rdfs:comment>
   </owl:Class>
   <owl:DatatypeProperty rdf:about="http://www.opengis.net/gml#hasid">
      <rdfs:domain rdf:resource="http://www.opengis.net/gml#AbstractGMLType"/>
      <rdfs:range rdf:resource="http://www.opengis.net/gml#id"/>
   </owl:DatatypeProperty>
   <owl:DatatypeProperty rdf:about="http://www.opengis.net/gml#hasid">
      <rdfs:domain rdf:resource="http://www.opengis.net/gml#AbstractMetaDataType"/>
      <rdfs:range rdf:resource="http://www.opengis.net/gml#id"/>
   </owl:DatatypeProperty>
   <owl:DatatypeProperty rdf:about="http://www.opengis.net/gml#about">
      <rdfs:domain rdf:resource="http://www.opengis.net/gml#MetaDataPropertyType"/>
      <rdfs:range rdf:resource="http://www.w3.org/2001/XMLSchema#anyURI"/>
   </owl:DatatypeProperty>
   <rdfs:Datatype rdf:about="http://www.opengis.net/gml#id">
      <rdfs:comment>Database handle for the object.  It is of XML type ID, so is constrained to be unique in the XML document within which it occurs.  An external identifier for the object in the form of a URI may be constructed using standard XML and XPointer methods.  This is done by concatenating the URI for the document, a fragment separator, and the value of the id attribute.</rdfs:comment>
      <owl:equivalentClass rdf:resource="http://www.w3.org/2001/XMLSchema#ID"/>
   </rdfs:Datatype>
   <rdfs:Datatype rdf:about="http://www.opengis.net/gml#remoteSchema">
      <rdfs:comment>Reference to an XML Schema fragment that specifies the content model of the propertys value. This is in conformance with the XML Schema Section 4.14 Referencing Schemas from Elsewhere.</rdfs:comment>
      <owl:equivalentClass rdf:resource="http://www.w3.org/2001/XMLSchema#anyURI"/>
   </rdfs:Datatype>
   <owl:DatatypeProperty rdf:about="http://www.opengis.net/gml#hasremoteSchema">
      <rdfs:domain rdf:resource="http://www.opengis.net/gml#AssociationAttributeGroup"/>
      <rdfs:range rdf:resource="http://www.opengis.net/gml#remoteSchema"/>
   </owl:DatatypeProperty>
   <owl:Class rdf:about="http://www.opengis.net/gml#_GML">
      <rdfs:subClassOf rdf:resource="http://www.opengis.net/gml#_Object"/>
      <rdfs:subClassOf rdf:resource="http://www.opengis.net/gml#AbstractGMLType"/>
   </owl:Class>
   <owl:Class rdf:about="http://www.opengis.net/gml#Bag">
      <rdfs:subClassOf rdf:resource="http://www.opengis.net/gml#_GML"/>
      <rdfs:subClassOf rdf:resource="http://www.opengis.net/gml#BagType"/>
   </owl:Class>
   <owl:Class rdf:about="http://www.opengis.net/gml#Array">
      <rdfs:subClassOf rdf:resource="http://www.opengis.net/gml#_GML"/>
      <rdfs:subClassOf rdf:resource="http://www.opengis.net/gml#ArrayType"/>
   </owl:Class>
   <owl:Class rdf:about="http://www.opengis.net/gml#_MetaData">
      <rdfs:subClassOf rdf:resource="http://www.opengis.net/gml#_Object"/>
      <rdfs:subClassOf rdf:resource="http://www.opengis.net/gml#AbstractMetaDataType"/>
   </owl:Class>
   <owl:Class rdf:about="http://www.opengis.net/gml#GenericMetaData">
      <rdfs:subClassOf rdf:resource="http://www.opengis.net/gml#_MetaData"/>
      <rdfs:subClassOf rdf:resource="http://www.opengis.net/gml#GenericMetaDataType"/>
   </owl:Class>
   <owl:Class rdf:about="http://www.opengis.net/gml#_association">
      <rdfs:subClassOf rdf:resource="http://www.opengis.net/gml#AssociationType"/>
   </owl:Class>
   <owl:Class rdf:about="http://www.opengis.net/gml#_strictAssociation">
      <rdfs:subClassOf rdf:resource="http://www.opengis.net/gml#AssociationType"/>
   </owl:Class>
   <owl:Class rdf:about="http://www.opengis.net/gml#member">
      <rdfs:subClassOf rdf:resource="http://www.opengis.net/gml#AssociationType"/>
   </owl:Class>
   <owl:Class rdf:about="http://www.opengis.net/gml#_reference">
      <rdfs:subClassOf rdf:resource="http://www.opengis.net/gml#ReferenceType"/>
   </owl:Class>
   <owl:Class rdf:about="http://www.opengis.net/gml#members">
      <rdfs:subClassOf rdf:resource="http://www.opengis.net/gml#ArrayAssociationType"/>
   </owl:Class>
   <owl:Class rdf:about="http://www.opengis.net/gml#metaDataProperty">
      <rdfs:subClassOf rdf:resource="http://www.opengis.net/gml#MetaDataPropertyType"/>
   </owl:Class>
   <owl:Class rdf:about="http://www.opengis.net/gml#name">
      <rdfs:subClassOf rdf:resource="CodeType"/>
      <rdfs:comment>Warning: This class type was declared outside of its original schema. This class may be declared incorrectly.</rdfs:comment>
   </owl:Class>
   <owl:Class rdf:about="http://www.opengis.net/gml#description">
      <rdfs:subClassOf rdf:resource="http://www.opengis.net/gml#StringOrRefType"/>
   </owl:Class>
   <owl:ObjectProperty rdf:about="http://www.opengis.net/gml#hasmetaDataProperty">
      <rdfs:comment>Warning: This ObjectProperty reference was declared outside of its original schema. This ObjectProperty may be declared incorrectly.</rdfs:comment>
      <rdfs:domain rdf:resource="http://www.opengis.net/gml#StandardObjectProperties"/>
      <rdfs:range rdf:resource="http://www.opengis.net/gml#metaDataProperty"/>
   </owl:ObjectProperty>
   <owl:ObjectProperty rdf:about="http://www.opengis.net/gml#hasdescription">
      <rdfs:comment>Warning: This ObjectProperty reference was declared outside of its original schema. This ObjectProperty may be declared incorrectly.</rdfs:comment>
      <rdfs:domain rdf:resource="http://www.opengis.net/gml#StandardObjectProperties"/>
      <rdfs:range rdf:resource="http://www.opengis.net/gml#description"/>
   </owl:ObjectProperty>
   <owl:ObjectProperty rdf:about="http://www.opengis.net/gml#hasname">
      <rdfs:comment>Warning: This ObjectProperty reference was declared outside of its original schema. This ObjectProperty may be declared incorrectly.</rdfs:comment>
      <rdfs:domain rdf:resource="http://www.opengis.net/gml#StandardObjectProperties"/>
      <rdfs:range rdf:resource="http://www.opengis.net/gml#name"/>
   </owl:ObjectProperty>
   <owl:ObjectProperty rdf:about="http://www.opengis.net/gml#hasmember">
      <rdfs:comment>Warning: This ObjectProperty reference was declared outside of its original schema. This ObjectProperty may be declared incorrectly.</rdfs:comment>
      <rdfs:domain rdf:resource="http://www.opengis.net/gml#BagType"/>
      <rdfs:range rdf:resource="http://www.opengis.net/gml#member"/>
   </owl:ObjectProperty>
   <owl:ObjectProperty rdf:about="http://www.opengis.net/gml#hasmembers">
      <rdfs:comment>Warning: This ObjectProperty reference was declared outside of its original schema. This ObjectProperty may be declared incorrectly.</rdfs:comment>
      <rdfs:domain rdf:resource="http://www.opengis.net/gml#BagType"/>
      <rdfs:range rdf:resource="http://www.opengis.net/gml#members"/>
   </owl:ObjectProperty>
   <owl:ObjectProperty rdf:about="http://www.opengis.net/gml#hasmembers">
      <rdfs:comment>Warning: This ObjectProperty reference was declared outside of its original schema. This ObjectProperty may be declared incorrectly.</rdfs:comment>
      <rdfs:domain rdf:resource="http://www.opengis.net/gml#ArrayType"/>
      <rdfs:range rdf:resource="http://www.opengis.net/gml#members"/>
   </owl:ObjectProperty>
   <owl:ObjectProperty rdf:about="http://www.opengis.net/gml#has_Object">
      <rdfs:comment>Warning: This ObjectProperty reference was declared outside of its original schema. This ObjectProperty may be declared incorrectly.</rdfs:comment>
      <rdfs:domain rdf:resource="http://www.opengis.net/gml#AssociationType"/>
      <rdfs:range rdf:resource="http://www.opengis.net/gml#_Object"/>
   </owl:ObjectProperty>
   <owl:ObjectProperty rdf:about="http://www.opengis.net/gml#has_Object">
      <rdfs:comment>Warning: This ObjectProperty reference was declared outside of its original schema. This ObjectProperty may be declared incorrectly.</rdfs:comment>
      <rdfs:domain rdf:resource="http://www.opengis.net/gml#ArrayAssociationType"/>
      <rdfs:range rdf:resource="http://www.opengis.net/gml#_Object"/>
   </owl:ObjectProperty>
</rdf:RDF>
