<rdf:RDF xmlns:math="http://www.w3.org/2005/xpath-functions/math" xmlns:owl="http://www.w3.org/2002/07/owl#" xmlns:rdf="http://www.w3.org/1999/02/22-rdf-syntax-ns#" xmlns:rdfs="http://www.w3.org/2000/01/rdf-schema#" xmlns:xs="http://www.w3.org/2001/XMLSchema" xmlns:xsd="http://www.w3.org/2001/XMLSchema">
   <owl:Ontology rdf:about="http://liris.cnrs.fr/ontologies/basicTypes">
      <owl:imports rdf:resource="http://liris.cnrs.fr/ontologies/gml"/>
      <rdfs:comment>basicTypes.xsd</rdfs:comment>
      <rdfs:seeAlso>urn:opengis:specification:gml:schema-xsd:basicTypes:3.1.1</rdfs:seeAlso>
      <rdfs:comment>
    Generic simpleContent components for use in GML
    
    GML is an OGC Standard.
    Copyright (c) 2001,2005,2010 Open Geospatial Consortium.
    To obtain additional rights of use, visit http://www.opengeospatial.org/legal/ .
    </rdfs:comment>
   </owl:Ontology>
   <owl:Class rdf:about="#CodeType">
      <rdfs:comment>Name or code with an (optional) authority.  Text token.  
      If the codeSpace attribute is present, then its value should identify a dictionary, thesaurus 
      or authority for the term, such as the organisation who assigned the value, 
      or the dictionary from which it is taken.  
      A text string with an optional codeSpace attribute. </rdfs:comment>
      <rdfs:subClassOf>
         <owl:Class>
            <owl:intersectionOf rdf:parseType="Collection">
               <owl:Restriction>
                  <owl:onProperty rdf:resource="#codeSpace"/>
                  <owl:allValuesFrom rdf:resource="http://www.w3.org/2001/XMLSchema#anyURI"/>
               </owl:Restriction>
            </owl:intersectionOf>
         </owl:Class>
      </rdfs:subClassOf>
   </owl:Class>
   <owl:DatatypeProperty rdf:about="#hasCodeType">
      <rdfs:domain rdf:resource="#CodeType"/>
      <rdfs:range rdf:resource="#string"/>
      <rdfs:subPropertyOf rdf:resource="#hasstring"/>
   </owl:DatatypeProperty>
   <owl:Class rdf:about="#CodeListType">
      <rdfs:comment>List of values on a uniform nominal scale.  List of text tokens.   
      In a list context a token should not include any spaces, so xsd:Name is used instead of xsd:string.   
      If a codeSpace attribute is present, then its value is a reference to 
      a Reference System for the value, a dictionary or code list.</rdfs:comment>
      <rdfs:subClassOf>
         <owl:Class>
            <owl:intersectionOf rdf:parseType="Collection">
               <owl:Restriction>
                  <owl:onProperty rdf:resource="#codeSpace"/>
                  <owl:allValuesFrom rdf:resource="http://www.w3.org/2001/XMLSchema#anyURI"/>
               </owl:Restriction>
            </owl:intersectionOf>
         </owl:Class>
      </rdfs:subClassOf>
      <rdfs:subClassOf rdf:resource="http://www.opengis.net/gml#NameList"/>
      <rdfs:comment>Warning: The parent class 'gml:NameList' is declared outside of this class' original schema. This class may be declared incorrectly.</rdfs:comment>
   </owl:Class>
   <owl:DatatypeProperty rdf:about="#hasCodeListType">
      <rdfs:domain rdf:resource="#CodeListType"/>
      <rdfs:range rdf:resource="http://www.opengis.net/gml#NameList"/>
      <rdfs:subPropertyOf rdf:resource="http://www.opengis.net/gml#hasNameList"/>
      <rdfs:comment>Warning: The parent property 'gml:hasNameList' is declared outside of this property's original schema. This property may be declared incorrectly.</rdfs:comment>
   </owl:DatatypeProperty>
   <owl:Class rdf:about="#CodeOrNullListType">
      <rdfs:comment>List of values on a uniform nominal scale.  List of text tokens.   
      In a list context a token should not include any spaces, so xsd:Name is used instead of xsd:string.  
      A member of the list may be a typed null.  
      If a codeSpace attribute is present, then its value is a reference to 
      a Reference System for the value, a dictionary or code list.</rdfs:comment>
      <rdfs:subClassOf>
         <owl:Class>
            <owl:intersectionOf rdf:parseType="Collection">
               <owl:Restriction>
                  <owl:onProperty rdf:resource="#codeSpace"/>
                  <owl:allValuesFrom rdf:resource="http://www.w3.org/2001/XMLSchema#anyURI"/>
               </owl:Restriction>
            </owl:intersectionOf>
         </owl:Class>
      </rdfs:subClassOf>
      <rdfs:subClassOf rdf:resource="http://www.opengis.net/gml#NameOrNullList"/>
      <rdfs:comment>Warning: The parent class 'gml:NameOrNullList' is declared outside of this class' original schema. This class may be declared incorrectly.</rdfs:comment>
   </owl:Class>
   <owl:DatatypeProperty rdf:about="#hasCodeOrNullListType">
      <rdfs:domain rdf:resource="#CodeOrNullListType"/>
      <rdfs:range rdf:resource="http://www.opengis.net/gml#NameOrNullList"/>
      <rdfs:subPropertyOf rdf:resource="http://www.opengis.net/gml#hasNameOrNullList"/>
      <rdfs:comment>Warning: The parent property 'gml:hasNameOrNullList' is declared outside of this property's original schema. This property may be declared incorrectly.</rdfs:comment>
   </owl:DatatypeProperty>
   <owl:Class rdf:about="#MeasureType">
      <rdfs:comment>Number with a scale.  
      The value of uom (Units Of Measure) attribute is a reference to a Reference System for the amount, either a ratio or position scale. </rdfs:comment>
      <rdfs:subClassOf>
         <owl:Class>
            <owl:intersectionOf rdf:parseType="Collection">
               <owl:Restriction>
                  <owl:onProperty rdf:resource="#uom"/>
                  <owl:allValuesFrom rdf:resource="http://www.w3.org/2001/XMLSchema#anyURI"/>
               </owl:Restriction>
            </owl:intersectionOf>
         </owl:Class>
      </rdfs:subClassOf>
   </owl:Class>
   <owl:DatatypeProperty rdf:about="#hasMeasureType">
      <rdfs:domain rdf:resource="#MeasureType"/>
      <rdfs:range rdf:resource="#double"/>
      <rdfs:subPropertyOf rdf:resource="#hasdouble"/>
   </owl:DatatypeProperty>
   <owl:Class rdf:about="#MeasureListType">
      <rdfs:comment>List of numbers with a uniform scale.  
      The value of uom (Units Of Measure) attribute is a reference to 
      a Reference System for the amount, either a ratio or position scale. </rdfs:comment>
      <rdfs:subClassOf>
         <owl:Class>
            <owl:intersectionOf rdf:parseType="Collection">
               <owl:Restriction>
                  <owl:onProperty rdf:resource="#uom"/>
                  <owl:allValuesFrom rdf:resource="http://www.w3.org/2001/XMLSchema#anyURI"/>
               </owl:Restriction>
            </owl:intersectionOf>
         </owl:Class>
      </rdfs:subClassOf>
      <rdfs:subClassOf rdf:resource="http://www.opengis.net/gml#doubleList"/>
      <rdfs:comment>Warning: The parent class 'gml:doubleList' is declared outside of this class' original schema. This class may be declared incorrectly.</rdfs:comment>
   </owl:Class>
   <owl:DatatypeProperty rdf:about="#hasMeasureListType">
      <rdfs:domain rdf:resource="#MeasureListType"/>
      <rdfs:range rdf:resource="http://www.opengis.net/gml#doubleList"/>
      <rdfs:subPropertyOf rdf:resource="http://www.opengis.net/gml#hasdoubleList"/>
      <rdfs:comment>Warning: The parent property 'gml:hasdoubleList' is declared outside of this property's original schema. This property may be declared incorrectly.</rdfs:comment>
   </owl:DatatypeProperty>
   <owl:Class rdf:about="#MeasureOrNullListType">
      <rdfs:comment>List of numbers with a uniform scale.  
      A member of the list may be a typed null. 
      The value of uom (Units Of Measure) attribute is a reference to 
      a Reference System for the amount, either a ratio or position scale. </rdfs:comment>
      <rdfs:subClassOf>
         <owl:Class>
            <owl:intersectionOf rdf:parseType="Collection">
               <owl:Restriction>
                  <owl:onProperty rdf:resource="#uom"/>
                  <owl:allValuesFrom rdf:resource="http://www.w3.org/2001/XMLSchema#anyURI"/>
               </owl:Restriction>
            </owl:intersectionOf>
         </owl:Class>
      </rdfs:subClassOf>
      <rdfs:subClassOf rdf:resource="http://www.opengis.net/gml#doubleOrNullList"/>
      <rdfs:comment>Warning: The parent class 'gml:doubleOrNullList' is declared outside of this class' original schema. This class may be declared incorrectly.</rdfs:comment>
   </owl:Class>
   <owl:DatatypeProperty rdf:about="#hasMeasureOrNullListType">
      <rdfs:domain rdf:resource="#MeasureOrNullListType"/>
      <rdfs:range rdf:resource="http://www.opengis.net/gml#doubleOrNullList"/>
      <rdfs:subPropertyOf rdf:resource="http://www.opengis.net/gml#hasdoubleOrNullList"/>
      <rdfs:comment>Warning: The parent property 'gml:hasdoubleOrNullList' is declared outside of this property's original schema. This property may be declared incorrectly.</rdfs:comment>
   </owl:DatatypeProperty>
   <owl:Class rdf:about="#CoordinatesType">
      <rdfs:comment>Tables or arrays of tuples.  
        May be used for text-encoding of values from a table.  
        Actually just a string, but allows the user to indicate which characters are used as separators.  
        The value of the 'cs' attribute is the separator for coordinate values, 
        and the value of the 'ts' attribute gives the tuple separator (a single space by default); 
        the default values may be changed to reflect local usage.
        Defaults to CSV within a tuple, space between tuples.  
        However, any string content will be schema-valid.  </rdfs:comment>
      <rdfs:subClassOf>
         <owl:Class>
            <owl:intersectionOf rdf:parseType="Collection">
               <owl:Restriction>
                  <owl:onProperty rdf:resource="#decimal"/>
                  <owl:allValuesFrom rdf:resource="http://www.w3.org/2001/XMLSchema#string"/>
               </owl:Restriction>
               <owl:Restriction>
                  <owl:onProperty rdf:resource="#cs"/>
                  <owl:allValuesFrom rdf:resource="http://www.w3.org/2001/XMLSchema#string"/>
               </owl:Restriction>
               <owl:Restriction>
                  <owl:onProperty rdf:resource="#ts"/>
                  <owl:allValuesFrom rdf:resource="http://www.w3.org/2001/XMLSchema#string"/>
               </owl:Restriction>
            </owl:intersectionOf>
         </owl:Class>
      </rdfs:subClassOf>
   </owl:Class>
   <owl:DatatypeProperty rdf:about="#hasCoordinatesType">
      <rdfs:domain rdf:resource="#CoordinatesType"/>
      <rdfs:range rdf:resource="#string"/>
      <rdfs:subPropertyOf rdf:resource="#hasstring"/>
   </owl:DatatypeProperty>
   <rdfs:Datatype rdf:about="#NullEnumeration">
      <rdfs:comment> Some common reasons for a null value:   
			
        innapplicable - the object does not have a value
        missing - The correct value is not readily available to the sender of this data.  
                           Furthermore, a correct value may not exist.
        template - the value will be available later
        unknown - The correct value is not known to, and not computable by, the sender of this data. 
                           However, a correct value probably exists.
        withheld - the value is not divulged 
        
        other:reason - as indicated by "reason" string
        
        Specific communities may agree to assign more strict semantics when these terms are used in a particular context.  
      </rdfs:comment>
   </rdfs:Datatype>
   <rdfs:Datatype rdf:about="#">
      <owl:equivalentClass>
         <rdfs:Datatype>
            <owl:oneOf>
               <rdf:Description rdf:type="http://www.w3.org/1999/02/22-rdf-syntax-ns#List">
                  <rdf:first rdf:datatype="string">inapplicable</rdf:first>
                  <rdf:rest>
                     <rdf:Description rdf:type="http://www.w3.org/1999/02/22-rdf-syntax-ns#List">
                        <rdf:first rdf:datatype="string">missing</rdf:first>
                        <rdf:rest>
                           <rdf:Description rdf:type="http://www.w3.org/1999/02/22-rdf-syntax-ns#List">
                              <rdf:first rdf:datatype="string">template</rdf:first>
                              <rdf:rest>
                                 <rdf:Description rdf:type="http://www.w3.org/1999/02/22-rdf-syntax-ns#List">
                                    <rdf:first rdf:datatype="string">unknown</rdf:first>
                                    <rdf:rest>
                                       <rdf:Description rdf:type="http://www.w3.org/1999/02/22-rdf-syntax-ns#List">
                                          <rdf:first rdf:datatype="string">withheld</rdf:first>
                                          <rdf:rest rdf:resource="http://www.w3.org/1999/02/22-rdf-syntax-ns#nil"/>
                                       </rdf:Description>
                                    </rdf:rest>
                                 </rdf:Description>
                              </rdf:rest>
                           </rdf:Description>
                        </rdf:rest>
                     </rdf:Description>
                  </rdf:rest>
               </rdf:Description>
            </owl:oneOf>
         </rdfs:Datatype>
      </owl:equivalentClass>
   </rdfs:Datatype>
   <rdfs:Datatype rdf:about="#"/>
   <rdfs:Datatype rdf:about="#NullType">
      <rdfs:comment>Utility type for null elements.  The value may be selected from one of the enumerated tokens, or may be a URI in which case this should identify a resource which describes the reason for the null. </rdfs:comment>
      <owl:equivalentClass rdf:resource="http://www.opengis.net/gml#NullEnumeration"/>
      <owl:equivalentClass rdf:resource="#anyURI"/>
   </rdfs:Datatype>
   <rdfs:Datatype rdf:about="#SignType">
      <rdfs:comment>Utility type used in various places 
      - e.g. to indicate the direction of topological objects;
      "+" for forwards, or "-" for backwards.</rdfs:comment>
      <owl:equivalentClass>
         <rdfs:Datatype>
            <owl:oneOf>
               <rdf:Description rdf:type="http://www.w3.org/1999/02/22-rdf-syntax-ns#List">
                  <rdf:first rdf:datatype="string">-</rdf:first>
                  <rdf:rest>
                     <rdf:Description rdf:type="http://www.w3.org/1999/02/22-rdf-syntax-ns#List">
                        <rdf:first rdf:datatype="string">+</rdf:first>
                        <rdf:rest rdf:resource="http://www.w3.org/1999/02/22-rdf-syntax-ns#nil"/>
                     </rdf:Description>
                  </rdf:rest>
               </rdf:Description>
            </owl:oneOf>
         </rdfs:Datatype>
      </owl:equivalentClass>
   </rdfs:Datatype>
   <rdfs:Datatype rdf:about="#booleanOrNull">
      <rdfs:comment>Union of the XML Schema boolean type and the GML Nulltype.  An element which uses this type may have content which is either a boolean {0,1,true,false} or a value from Nulltype</rdfs:comment>
      <owl:equivalentClass rdf:resource="http://www.opengis.net/gml#NullEnumeration"/>
      <owl:equivalentClass rdf:resource="#boolean"/>
      <owl:equivalentClass rdf:resource="#anyURI"/>
   </rdfs:Datatype>
   <rdfs:Datatype rdf:about="#booleanOrNullList">
      <rdfs:comment>XML List based on the union type defined above.  An element declared with this type contains a space-separated list of boolean values {0,1,true,false} with null values interspersed as needed</rdfs:comment>
      <owl:equivalentClass rdf:resource="http://www.w3.org/2000/01/rdf-schema#Literal"/>
   </rdfs:Datatype>
   <rdfs:Datatype rdf:about="#booleanList">
      <rdfs:comment>XML List based on XML Schema boolean type.  An element of this type contains a space-separated list of boolean values {0,1,true,false}</rdfs:comment>
      <owl:equivalentClass rdf:resource="http://www.w3.org/2000/01/rdf-schema#Literal"/>
   </rdfs:Datatype>
   <rdfs:Datatype rdf:about="#stringOrNull">
      <rdfs:comment>Union of the XML Schema string type and the GML Nulltype.  An element which uses this type may have content which is either a string or a value from Nulltype.  Note that a "string" may contain whitespace.  </rdfs:comment>
      <owl:equivalentClass rdf:resource="http://www.opengis.net/gml#NullEnumeration"/>
      <owl:equivalentClass rdf:resource="#string"/>
      <owl:equivalentClass rdf:resource="#anyURI"/>
   </rdfs:Datatype>
   <rdfs:Datatype rdf:about="#NameOrNull">
      <rdfs:comment>Union of the XML Schema Name type and the GML Nulltype.  An element which uses this type may have content which is either a Name or a value from Nulltype.  Note that a "Name" may not contain whitespace.  </rdfs:comment>
      <owl:equivalentClass rdf:resource="http://www.opengis.net/gml#NullEnumeration"/>
      <owl:equivalentClass rdf:resource="#Name"/>
      <owl:equivalentClass rdf:resource="#anyURI"/>
   </rdfs:Datatype>
   <rdfs:Datatype rdf:about="#NameOrNullList">
      <rdfs:comment>XML List based on the union type defined above.  An element declared with this type contains a space-separated list of Name values with null values interspersed as needed</rdfs:comment>
      <owl:equivalentClass rdf:resource="http://www.w3.org/2000/01/rdf-schema#Literal"/>
   </rdfs:Datatype>
   <rdfs:Datatype rdf:about="#NameList">
      <rdfs:comment>XML List based on XML Schema Name type.  An element of this type contains a space-separated list of Name values</rdfs:comment>
      <owl:equivalentClass rdf:resource="http://www.w3.org/2000/01/rdf-schema#Literal"/>
   </rdfs:Datatype>
   <rdfs:Datatype rdf:about="#doubleOrNull">
      <rdfs:comment>Union of the XML Schema double type and the GML Nulltype.  An element which uses this type may have content which is either a double or a value from Nulltype</rdfs:comment>
      <owl:equivalentClass rdf:resource="http://www.opengis.net/gml#NullEnumeration"/>
      <owl:equivalentClass rdf:resource="#double"/>
      <owl:equivalentClass rdf:resource="#anyURI"/>
   </rdfs:Datatype>
   <rdfs:Datatype rdf:about="#doubleOrNullList">
      <rdfs:comment>XML List based on the union type defined above.  An element declared with this type contains a space-separated list of double values with null values interspersed as needed</rdfs:comment>
      <owl:equivalentClass rdf:resource="http://www.w3.org/2000/01/rdf-schema#Literal"/>
   </rdfs:Datatype>
   <rdfs:Datatype rdf:about="#doubleList">
      <rdfs:comment>XML List based on XML Schema double type.  An element of this type contains a space-separated list of double values</rdfs:comment>
      <owl:equivalentClass rdf:resource="http://www.w3.org/2000/01/rdf-schema#Literal"/>
   </rdfs:Datatype>
   <rdfs:Datatype rdf:about="#integerOrNull">
      <rdfs:comment>Union of the XML Schema integer type and the GML Nulltype.  An element which uses this type may have content which is either an integer or a value from Nulltype</rdfs:comment>
      <owl:equivalentClass rdf:resource="http://www.opengis.net/gml#NullEnumeration"/>
      <owl:equivalentClass rdf:resource="#integer"/>
      <owl:equivalentClass rdf:resource="#anyURI"/>
   </rdfs:Datatype>
   <rdfs:Datatype rdf:about="#integerOrNullList">
      <rdfs:comment>XML List based on the union type defined above.  An element declared with this type contains a space-separated list of integer values with null values interspersed as needed</rdfs:comment>
      <owl:equivalentClass rdf:resource="http://www.w3.org/2000/01/rdf-schema#Literal"/>
   </rdfs:Datatype>
   <rdfs:Datatype rdf:about="#integerList">
      <rdfs:comment>XML List based on XML Schema integer type.  An element of this type contains a space-separated list of integer values</rdfs:comment>
      <owl:equivalentClass rdf:resource="http://www.w3.org/2000/01/rdf-schema#Literal"/>
   </rdfs:Datatype>
   <rdfs:Datatype rdf:about="#NCNameList">
      <rdfs:comment>A set of values, representing a list of token with the lexical value space of NCName. The tokens are seperated by whitespace.</rdfs:comment>
      <owl:equivalentClass rdf:resource="http://www.w3.org/2000/01/rdf-schema#Literal"/>
   </rdfs:Datatype>
   <rdfs:Datatype rdf:about="#QNameList">
      <rdfs:comment>A set of values, representing a list of token with the lexical value space of QName. The tokens are seperated by whitespace.</rdfs:comment>
      <owl:equivalentClass rdf:resource="http://www.w3.org/2000/01/rdf-schema#Literal"/>
   </rdfs:Datatype>
   <owl:DatatypeProperty rdf:about="#codeSpace">
      <rdfs:domain rdf:resource="#CodeType"/>
      <rdfs:range rdf:resource="#anyURI"/>
   </owl:DatatypeProperty>
   <owl:DatatypeProperty rdf:about="#codeSpace">
      <rdfs:domain rdf:resource="#CodeListType"/>
      <rdfs:range rdf:resource="#anyURI"/>
   </owl:DatatypeProperty>
   <owl:DatatypeProperty rdf:about="#codeSpace">
      <rdfs:domain rdf:resource="#CodeOrNullListType"/>
      <rdfs:range rdf:resource="#anyURI"/>
   </owl:DatatypeProperty>
   <owl:DatatypeProperty rdf:about="#uom">
      <rdfs:domain rdf:resource="#MeasureType"/>
      <rdfs:range rdf:resource="#anyURI"/>
   </owl:DatatypeProperty>
   <owl:DatatypeProperty rdf:about="#uom">
      <rdfs:domain rdf:resource="#MeasureListType"/>
      <rdfs:range rdf:resource="#anyURI"/>
   </owl:DatatypeProperty>
   <owl:DatatypeProperty rdf:about="#uom">
      <rdfs:domain rdf:resource="#MeasureOrNullListType"/>
      <rdfs:range rdf:resource="#anyURI"/>
   </owl:DatatypeProperty>
   <owl:DatatypeProperty rdf:about="#decimal">
      <rdfs:domain rdf:resource="#CoordinatesType"/>
      <rdfs:range rdf:resource="#string"/>
   </owl:DatatypeProperty>
   <owl:DatatypeProperty rdf:about="#cs">
      <rdfs:domain rdf:resource="#CoordinatesType"/>
      <rdfs:range rdf:resource="#string"/>
   </owl:DatatypeProperty>
   <owl:DatatypeProperty rdf:about="#ts">
      <rdfs:domain rdf:resource="#CoordinatesType"/>
      <rdfs:range rdf:resource="#string"/>
   </owl:DatatypeProperty>
   <owl:Class rdf:about="#Null">
      <rdfs:subClassOf rdf:resource="http://www.opengis.net/gml#NullType"/>
      <rdfs:comment>Warning: This class type was declared outside of its original schema. This class may be declared incorrectly.</rdfs:comment>
   </owl:Class>
</rdf:RDF>
