<rdf:RDF xmlns:math="http://www.w3.org/2005/xpath-functions/math" xmlns:owl="http://www.w3.org/2002/07/owl#" xmlns:rdf="http://www.w3.org/1999/02/22-rdf-syntax-ns#" xmlns:rdfs="http://www.w3.org/2000/01/rdf-schema#" xmlns:xs="http://www.w3.org/2001/XMLSchema" xmlns:xsd="http://www.w3.org/2001/XMLSchema">
   <owl:Ontology rdf:about="http://liris.cnrs.fr/ontologies/defaultStyle">
      <owl:imports rdf:resource="http://liris.cnrs.fr/ontologies/smil20"/>
      <owl:imports rdf:resource="http://liris.cnrs.fr/ontologies/gml"/>
      <owl:imports rdf:resource="http://liris.cnrs.fr/ontologies/measures"/>
      <rdfs:comment>defaultStyle.xsd</rdfs:comment>
      <rdfs:seeAlso>urn:opengis:specification:gml:schema-defaultStyle:v3.1.0</rdfs:seeAlso>
      <rdfs:comment>
			Default Style schema for GML 3.1.1
			
			GML is an OGC Standard.
			Copyright (c) 2001,2005,2010 Open Geospatial Consortium.
			To obtain additional rights of use, visit http://www.opengeospatial.org/legal/ .
		</rdfs:comment>
   </owl:Ontology>
   <owl:Class rdf:about="http://www.opengis.net/gml#DefaultStylePropertyType">
      <rdfs:comment>[complexType of] Top-level property. Used in application schemas to "attach" the styling information to GML data. The link between the data and the style should be established through this property only.</rdfs:comment>
      <rdfs:subClassOf>
         <owl:Class>
            <owl:intersectionOf rdf:parseType="Collection">
               <owl:Restriction>
                  <owl:onProperty rdf:resource="http://www.opengis.net/gml#has_Style"/>
                  <owl:allValuesFrom rdf:resource="http://www.opengis.net/gml#_Style"/>
               </owl:Restriction>
               <owl:Restriction>
                  <owl:onProperty rdf:resource="http://www.opengis.net/gml#has_Style"/>
                  <owl:minCardinality rdf:datatype="http://www.w3.org/2001/XMLSchema#nonNegativeInteger">0</owl:minCardinality>
               </owl:Restriction>
            </owl:intersectionOf>
         </owl:Class>
      </rdfs:subClassOf>
      <rdfs:subClassOf>
         <owl:Class>
            <owl:intersectionOf rdf:parseType="Collection">
               <owl:Restriction>
                  <owl:onProperty rdf:resource="http://www.opengis.net/gml#about"/>
                  <owl:allValuesFrom rdf:resource="http://www.w3.org/2001/XMLSchema#anyURI"/>
               </owl:Restriction>
            </owl:intersectionOf>
         </owl:Class>
      </rdfs:subClassOf>
   </owl:Class>
   <owl:Class rdf:about="http://www.opengis.net/gml#AbstractStyleType">
      <rdfs:comment>This is an abstract class</rdfs:comment>
      <rdfs:comment>[complexType of] The value of the top-level property. It is an abstract element. Used as the head element of the substitution group for extensibility purposes.</rdfs:comment>
      <rdfs:subClassOf rdf:resource="http://www.opengis.net/gml#AbstractGMLType"/>
      <rdfs:comment>Warning: The parent class 'gml:AbstractGMLType' is declared outside of this class' original schema. This class may be declared incorrectly.</rdfs:comment>
   </owl:Class>
   <owl:Class rdf:about="http://www.opengis.net/gml#StyleType">
      <rdfs:comment>[complexType of] Predefined concrete value of the top-level property. Encapsulates all other styling information.</rdfs:comment>
      <rdfs:subClassOf>
         <owl:Class>
            <owl:intersectionOf rdf:parseType="Collection">
               <owl:Restriction>
                  <owl:onProperty rdf:resource="http://www.opengis.net/gml#hasfeatureStyle"/>
                  <owl:allValuesFrom rdf:resource="http://www.opengis.net/gml#featureStyle"/>
               </owl:Restriction>
               <owl:Restriction>
                  <owl:onProperty rdf:resource="http://www.opengis.net/gml#hasgraphStyle"/>
                  <owl:allValuesFrom rdf:resource="http://www.opengis.net/gml#graphStyle"/>
               </owl:Restriction>
               <owl:Restriction>
                  <owl:onProperty rdf:resource="http://www.opengis.net/gml#hasgraphStyle"/>
                  <owl:minCardinality rdf:datatype="http://www.w3.org/2001/XMLSchema#nonNegativeInteger">0</owl:minCardinality>
               </owl:Restriction>
            </owl:intersectionOf>
         </owl:Class>
      </rdfs:subClassOf>
      <rdfs:subClassOf rdf:resource="http://www.opengis.net/gml#AbstractStyleType"/>
      <rdfs:comment>Warning: The parent class 'gml:AbstractStyleType' is declared outside of this class' original schema. This class may be declared incorrectly.</rdfs:comment>
   </owl:Class>
   <owl:Class rdf:about="http://www.opengis.net/gml#FeatureStylePropertyType">
      <rdfs:subClassOf>
         <owl:Class>
            <owl:intersectionOf rdf:parseType="Collection">
               <owl:Restriction>
                  <owl:onProperty rdf:resource="http://www.opengis.net/gml#hasFeatureStyle"/>
                  <owl:allValuesFrom rdf:resource="http://www.opengis.net/gml#FeatureStyle"/>
               </owl:Restriction>
               <owl:Restriction>
                  <owl:onProperty rdf:resource="http://www.opengis.net/gml#hasFeatureStyle"/>
                  <owl:minCardinality rdf:datatype="http://www.w3.org/2001/XMLSchema#nonNegativeInteger">0</owl:minCardinality>
               </owl:Restriction>
            </owl:intersectionOf>
         </owl:Class>
      </rdfs:subClassOf>
      <rdfs:subClassOf>
         <owl:Class>
            <owl:intersectionOf rdf:parseType="Collection">
               <owl:Restriction>
                  <owl:onProperty rdf:resource="http://www.opengis.net/gml#about"/>
                  <owl:allValuesFrom rdf:resource="http://www.w3.org/2001/XMLSchema#anyURI"/>
               </owl:Restriction>
            </owl:intersectionOf>
         </owl:Class>
      </rdfs:subClassOf>
   </owl:Class>
   <owl:Class rdf:about="http://www.opengis.net/gml#FeatureStyleType">
      <rdfs:comment>[complexType of] The style descriptor for features.</rdfs:comment>
      <rdfs:subClassOf>
         <owl:Class>
            <owl:intersectionOf rdf:parseType="Collection">
               <owl:Restriction>
                  <owl:onProperty rdf:resource="http://www.opengis.net/gml#featureConstraint"/>
                  <owl:allValuesFrom rdf:resource="http://www.w3.org/2001/XMLSchema#string"/>
               </owl:Restriction>
               <owl:Restriction>
                  <owl:onProperty rdf:resource="http://www.opengis.net/gml#featureConstraint"/>
                  <owl:minCardinality rdf:datatype="http://www.w3.org/2001/XMLSchema#nonNegativeInteger">0</owl:minCardinality>
               </owl:Restriction>
               <owl:Restriction>
                  <owl:onProperty rdf:resource="http://www.opengis.net/gml#hasgeometryStyle"/>
                  <owl:allValuesFrom rdf:resource="http://www.opengis.net/gml#geometryStyle"/>
               </owl:Restriction>
               <owl:Restriction>
                  <owl:onProperty rdf:resource="http://www.opengis.net/gml#hasgeometryStyle"/>
                  <owl:minCardinality rdf:datatype="http://www.w3.org/2001/XMLSchema#nonNegativeInteger">0</owl:minCardinality>
               </owl:Restriction>
               <owl:Restriction>
                  <owl:onProperty rdf:resource="http://www.opengis.net/gml#hastopologyStyle"/>
                  <owl:allValuesFrom rdf:resource="http://www.opengis.net/gml#topologyStyle"/>
               </owl:Restriction>
               <owl:Restriction>
                  <owl:onProperty rdf:resource="http://www.opengis.net/gml#hastopologyStyle"/>
                  <owl:minCardinality rdf:datatype="http://www.w3.org/2001/XMLSchema#nonNegativeInteger">0</owl:minCardinality>
               </owl:Restriction>
               <owl:Restriction>
                  <owl:onProperty rdf:resource="http://www.opengis.net/gml#haslabelStyle"/>
                  <owl:allValuesFrom rdf:resource="http://www.opengis.net/gml#labelStyle"/>
               </owl:Restriction>
               <owl:Restriction>
                  <owl:onProperty rdf:resource="http://www.opengis.net/gml#haslabelStyle"/>
                  <owl:minCardinality rdf:datatype="http://www.w3.org/2001/XMLSchema#nonNegativeInteger">0</owl:minCardinality>
               </owl:Restriction>
            </owl:intersectionOf>
         </owl:Class>
      </rdfs:subClassOf>
      <rdfs:subClassOf>
         <owl:Class>
            <owl:intersectionOf rdf:parseType="Collection">
               <owl:Restriction>
                  <owl:onProperty rdf:resource="http://www.opengis.net/gml#featureType"/>
                  <owl:allValuesFrom rdf:resource="http://www.w3.org/2001/XMLSchema#string"/>
               </owl:Restriction>
               <owl:Restriction>
                  <owl:onProperty rdf:resource="http://www.opengis.net/gml#baseType"/>
                  <owl:allValuesFrom rdf:resource="http://www.w3.org/2001/XMLSchema#string"/>
               </owl:Restriction>
               <owl:Restriction>
                  <owl:onProperty rdf:resource="http://www.opengis.net/gml#queryGrammar"/>
                  <owl:allValuesFrom rdf:resource="http://www.opengis.net/gml#QueryGrammarEnumeration"/>
               </owl:Restriction>
            </owl:intersectionOf>
         </owl:Class>
      </rdfs:subClassOf>
      <rdfs:subClassOf rdf:resource="http://www.opengis.net/gml#AbstractGMLType"/>
      <rdfs:comment>Warning: The parent class 'gml:AbstractGMLType' is declared outside of this class' original schema. This class may be declared incorrectly.</rdfs:comment>
   </owl:Class>
   <owl:Class rdf:about="http://www.opengis.net/gml#BaseStyleDescriptorType">
      <rdfs:comment>Base complex type for geometry, topology, label and graph styles.</rdfs:comment>
      <rdfs:subClassOf>
         <owl:Class>
            <owl:intersectionOf rdf:parseType="Collection">
               <owl:Restriction>
                  <owl:onProperty rdf:resource="http://www.opengis.net/gml#spatialResolution"/>
                  <owl:allValuesFrom rdf:resource="http://www.opengis.net/gml#ScaleType"/>
               </owl:Restriction>
               <owl:Restriction>
                  <owl:onProperty rdf:resource="http://www.opengis.net/gml#spatialResolution"/>
                  <owl:minCardinality rdf:datatype="http://www.w3.org/2001/XMLSchema#nonNegativeInteger">0</owl:minCardinality>
               </owl:Restriction>
               <owl:Restriction>
                  <owl:onProperty rdf:resource="http://www.opengis.net/gml#styleVariation"/>
                  <owl:allValuesFrom rdf:resource="http://www.opengis.net/gml#StyleVariationType"/>
               </owl:Restriction>
               <owl:Restriction>
                  <owl:onProperty rdf:resource="http://www.opengis.net/gml#styleVariation"/>
                  <owl:minCardinality rdf:datatype="http://www.w3.org/2001/XMLSchema#nonNegativeInteger">0</owl:minCardinality>
               </owl:Restriction>
               <owl:Restriction>
                  <owl:onProperty rdf:resource="http://www.w3.org/2001/SMIL20/#hasanimate"/>
                  <owl:allValuesFrom rdf:resource="http://www.w3.org/2001/SMIL20/#animate"/>
               </owl:Restriction>
               <owl:Restriction>
                  <owl:onProperty rdf:resource="http://www.w3.org/2001/SMIL20/#hasanimate"/>
                  <owl:minCardinality rdf:datatype="http://www.w3.org/2001/XMLSchema#nonNegativeInteger">0</owl:minCardinality>
               </owl:Restriction>
               <owl:Restriction>
                  <owl:onProperty rdf:resource="http://www.w3.org/2001/SMIL20/#hasanimateMotion"/>
                  <owl:allValuesFrom rdf:resource="http://www.w3.org/2001/SMIL20/#animateMotion"/>
               </owl:Restriction>
               <owl:Restriction>
                  <owl:onProperty rdf:resource="http://www.w3.org/2001/SMIL20/#hasanimateMotion"/>
                  <owl:minCardinality rdf:datatype="http://www.w3.org/2001/XMLSchema#nonNegativeInteger">0</owl:minCardinality>
               </owl:Restriction>
               <owl:Restriction>
                  <owl:onProperty rdf:resource="http://www.w3.org/2001/SMIL20/#hasanimateColor"/>
                  <owl:allValuesFrom rdf:resource="http://www.w3.org/2001/SMIL20/#animateColor"/>
               </owl:Restriction>
               <owl:Restriction>
                  <owl:onProperty rdf:resource="http://www.w3.org/2001/SMIL20/#hasanimateColor"/>
                  <owl:minCardinality rdf:datatype="http://www.w3.org/2001/XMLSchema#nonNegativeInteger">0</owl:minCardinality>
               </owl:Restriction>
               <owl:Restriction>
                  <owl:onProperty rdf:resource="http://www.w3.org/2001/SMIL20/#hasset"/>
                  <owl:allValuesFrom rdf:resource="http://www.w3.org/2001/SMIL20/#set"/>
               </owl:Restriction>
               <owl:Restriction>
                  <owl:onProperty rdf:resource="http://www.w3.org/2001/SMIL20/#hasset"/>
                  <owl:minCardinality rdf:datatype="http://www.w3.org/2001/XMLSchema#nonNegativeInteger">0</owl:minCardinality>
               </owl:Restriction>
            </owl:intersectionOf>
         </owl:Class>
      </rdfs:subClassOf>
      <rdfs:subClassOf rdf:resource="http://www.opengis.net/gml#AbstractGMLType"/>
      <rdfs:comment>Warning: The parent class 'gml:AbstractGMLType' is declared outside of this class' original schema. This class may be declared incorrectly.</rdfs:comment>
   </owl:Class>
   <owl:Class rdf:about="http://www.opengis.net/gml#GeometryStylePropertyType">
      <rdfs:subClassOf>
         <owl:Class>
            <owl:intersectionOf rdf:parseType="Collection">
               <owl:Restriction>
                  <owl:onProperty rdf:resource="http://www.opengis.net/gml#hasGeometryStyle"/>
                  <owl:allValuesFrom rdf:resource="http://www.opengis.net/gml#GeometryStyle"/>
               </owl:Restriction>
               <owl:Restriction>
                  <owl:onProperty rdf:resource="http://www.opengis.net/gml#hasGeometryStyle"/>
                  <owl:minCardinality rdf:datatype="http://www.w3.org/2001/XMLSchema#nonNegativeInteger">0</owl:minCardinality>
               </owl:Restriction>
            </owl:intersectionOf>
         </owl:Class>
      </rdfs:subClassOf>
      <rdfs:subClassOf>
         <owl:Class>
            <owl:intersectionOf rdf:parseType="Collection">
               <owl:Restriction>
                  <owl:onProperty rdf:resource="http://www.opengis.net/gml#about"/>
                  <owl:allValuesFrom rdf:resource="http://www.w3.org/2001/XMLSchema#anyURI"/>
               </owl:Restriction>
            </owl:intersectionOf>
         </owl:Class>
      </rdfs:subClassOf>
   </owl:Class>
   <owl:Class rdf:about="http://www.opengis.net/gml#GeometryStyleType">
      <rdfs:comment>[complexType of] The style descriptor for geometries of a feature.</rdfs:comment>
      <rdfs:subClassOf>
         <owl:Class>
            <owl:intersectionOf rdf:parseType="Collection">
               <owl:Restriction>
                  <owl:onProperty rdf:resource="http://www.opengis.net/gml#haslabelStyle"/>
                  <owl:allValuesFrom rdf:resource="http://www.opengis.net/gml#labelStyle"/>
               </owl:Restriction>
               <owl:Restriction>
                  <owl:onProperty rdf:resource="http://www.opengis.net/gml#haslabelStyle"/>
                  <owl:minCardinality rdf:datatype="http://www.w3.org/2001/XMLSchema#nonNegativeInteger">0</owl:minCardinality>
               </owl:Restriction>
            </owl:intersectionOf>
         </owl:Class>
      </rdfs:subClassOf>
      <owl:disjointUnionOf rdf:parseType="Collection">
         <owl:Restriction>
            <owl:onProperty rdf:resource="http://www.opengis.net/gml#hassymbol"/>
            <owl:allValuesFrom rdf:resource="http://www.opengis.net/gml#symbol"/>
         </owl:Restriction>
         <owl:Restriction>
            <owl:onProperty rdf:resource="http://www.opengis.net/gml#style"/>
            <owl:allValuesFrom rdf:resource="http://www.w3.org/2001/XMLSchema#string"/>
         </owl:Restriction>
      </owl:disjointUnionOf>
      <rdfs:subClassOf>
         <owl:Class>
            <owl:intersectionOf rdf:parseType="Collection">
               <owl:Restriction>
                  <owl:onProperty rdf:resource="http://www.opengis.net/gml#geometryProperty"/>
                  <owl:allValuesFrom rdf:resource="http://www.w3.org/2001/XMLSchema#string"/>
               </owl:Restriction>
               <owl:Restriction>
                  <owl:onProperty rdf:resource="http://www.opengis.net/gml#geometryType"/>
                  <owl:allValuesFrom rdf:resource="http://www.w3.org/2001/XMLSchema#string"/>
               </owl:Restriction>
            </owl:intersectionOf>
         </owl:Class>
      </rdfs:subClassOf>
      <rdfs:subClassOf rdf:resource="http://www.opengis.net/gml#BaseStyleDescriptorType"/>
      <rdfs:comment>Warning: The parent class 'gml:BaseStyleDescriptorType' is declared outside of this class' original schema. This class may be declared incorrectly.</rdfs:comment>
   </owl:Class>
   <owl:Class rdf:about="http://www.opengis.net/gml#TopologyStylePropertyType">
      <rdfs:subClassOf>
         <owl:Class>
            <owl:intersectionOf rdf:parseType="Collection">
               <owl:Restriction>
                  <owl:onProperty rdf:resource="http://www.opengis.net/gml#hasTopologyStyle"/>
                  <owl:allValuesFrom rdf:resource="http://www.opengis.net/gml#TopologyStyle"/>
               </owl:Restriction>
               <owl:Restriction>
                  <owl:onProperty rdf:resource="http://www.opengis.net/gml#hasTopologyStyle"/>
                  <owl:minCardinality rdf:datatype="http://www.w3.org/2001/XMLSchema#nonNegativeInteger">0</owl:minCardinality>
               </owl:Restriction>
            </owl:intersectionOf>
         </owl:Class>
      </rdfs:subClassOf>
      <rdfs:subClassOf>
         <owl:Class>
            <owl:intersectionOf rdf:parseType="Collection">
               <owl:Restriction>
                  <owl:onProperty rdf:resource="http://www.opengis.net/gml#about"/>
                  <owl:allValuesFrom rdf:resource="http://www.w3.org/2001/XMLSchema#anyURI"/>
               </owl:Restriction>
            </owl:intersectionOf>
         </owl:Class>
      </rdfs:subClassOf>
   </owl:Class>
   <owl:Class rdf:about="http://www.opengis.net/gml#TopologyStyleType">
      <rdfs:comment>[complexType of] The style descriptor for topologies of a feature. Describes individual topology elements styles.</rdfs:comment>
      <rdfs:subClassOf>
         <owl:Class>
            <owl:intersectionOf rdf:parseType="Collection">
               <owl:Restriction>
                  <owl:onProperty rdf:resource="http://www.opengis.net/gml#haslabelStyle"/>
                  <owl:allValuesFrom rdf:resource="http://www.opengis.net/gml#labelStyle"/>
               </owl:Restriction>
               <owl:Restriction>
                  <owl:onProperty rdf:resource="http://www.opengis.net/gml#haslabelStyle"/>
                  <owl:minCardinality rdf:datatype="http://www.w3.org/2001/XMLSchema#nonNegativeInteger">0</owl:minCardinality>
               </owl:Restriction>
            </owl:intersectionOf>
         </owl:Class>
      </rdfs:subClassOf>
      <owl:disjointUnionOf rdf:parseType="Collection">
         <owl:Restriction>
            <owl:onProperty rdf:resource="http://www.opengis.net/gml#hassymbol"/>
            <owl:allValuesFrom rdf:resource="http://www.opengis.net/gml#symbol"/>
         </owl:Restriction>
         <owl:Restriction>
            <owl:onProperty rdf:resource="http://www.opengis.net/gml#style"/>
            <owl:allValuesFrom rdf:resource="http://www.w3.org/2001/XMLSchema#string"/>
         </owl:Restriction>
      </owl:disjointUnionOf>
      <rdfs:subClassOf>
         <owl:Class>
            <owl:intersectionOf rdf:parseType="Collection">
               <owl:Restriction>
                  <owl:onProperty rdf:resource="http://www.opengis.net/gml#topologyProperty"/>
                  <owl:allValuesFrom rdf:resource="http://www.w3.org/2001/XMLSchema#string"/>
               </owl:Restriction>
               <owl:Restriction>
                  <owl:onProperty rdf:resource="http://www.opengis.net/gml#topologyType"/>
                  <owl:allValuesFrom rdf:resource="http://www.w3.org/2001/XMLSchema#string"/>
               </owl:Restriction>
            </owl:intersectionOf>
         </owl:Class>
      </rdfs:subClassOf>
      <rdfs:subClassOf rdf:resource="http://www.opengis.net/gml#BaseStyleDescriptorType"/>
      <rdfs:comment>Warning: The parent class 'gml:BaseStyleDescriptorType' is declared outside of this class' original schema. This class may be declared incorrectly.</rdfs:comment>
   </owl:Class>
   <owl:Class rdf:about="http://www.opengis.net/gml#LabelStylePropertyType">
      <rdfs:subClassOf>
         <owl:Class>
            <owl:intersectionOf rdf:parseType="Collection">
               <owl:Restriction>
                  <owl:onProperty rdf:resource="http://www.opengis.net/gml#hasLabelStyle"/>
                  <owl:allValuesFrom rdf:resource="http://www.opengis.net/gml#LabelStyle"/>
               </owl:Restriction>
               <owl:Restriction>
                  <owl:onProperty rdf:resource="http://www.opengis.net/gml#hasLabelStyle"/>
                  <owl:minCardinality rdf:datatype="http://www.w3.org/2001/XMLSchema#nonNegativeInteger">0</owl:minCardinality>
               </owl:Restriction>
            </owl:intersectionOf>
         </owl:Class>
      </rdfs:subClassOf>
      <rdfs:subClassOf>
         <owl:Class>
            <owl:intersectionOf rdf:parseType="Collection">
               <owl:Restriction>
                  <owl:onProperty rdf:resource="http://www.opengis.net/gml#about"/>
                  <owl:allValuesFrom rdf:resource="http://www.w3.org/2001/XMLSchema#anyURI"/>
               </owl:Restriction>
            </owl:intersectionOf>
         </owl:Class>
      </rdfs:subClassOf>
   </owl:Class>
   <owl:Class rdf:about="http://www.opengis.net/gml#LabelStyleType">
      <rdfs:comment>[complexType of] The style descriptor for labels of a feature, geometry or topology.</rdfs:comment>
      <rdfs:subClassOf>
         <owl:Class>
            <owl:intersectionOf rdf:parseType="Collection">
               <owl:Restriction>
                  <owl:onProperty rdf:resource="http://www.opengis.net/gml#style"/>
                  <owl:allValuesFrom rdf:resource="http://www.w3.org/2001/XMLSchema#string"/>
               </owl:Restriction>
               <owl:Restriction>
                  <owl:onProperty rdf:resource="http://www.opengis.net/gml#label"/>
                  <owl:allValuesFrom rdf:resource="http://www.opengis.net/gml#LabelType"/>
               </owl:Restriction>
            </owl:intersectionOf>
         </owl:Class>
      </rdfs:subClassOf>
      <rdfs:subClassOf rdf:resource="http://www.opengis.net/gml#BaseStyleDescriptorType"/>
      <rdfs:comment>Warning: The parent class 'gml:BaseStyleDescriptorType' is declared outside of this class' original schema. This class may be declared incorrectly.</rdfs:comment>
   </owl:Class>
   <owl:Class rdf:about="http://www.opengis.net/gml#GraphStylePropertyType">
      <rdfs:subClassOf>
         <owl:Class>
            <owl:intersectionOf rdf:parseType="Collection">
               <owl:Restriction>
                  <owl:onProperty rdf:resource="http://www.opengis.net/gml#hasGraphStyle"/>
                  <owl:allValuesFrom rdf:resource="http://www.opengis.net/gml#GraphStyle"/>
               </owl:Restriction>
               <owl:Restriction>
                  <owl:onProperty rdf:resource="http://www.opengis.net/gml#hasGraphStyle"/>
                  <owl:minCardinality rdf:datatype="http://www.w3.org/2001/XMLSchema#nonNegativeInteger">0</owl:minCardinality>
               </owl:Restriction>
            </owl:intersectionOf>
         </owl:Class>
      </rdfs:subClassOf>
      <rdfs:subClassOf>
         <owl:Class>
            <owl:intersectionOf rdf:parseType="Collection">
               <owl:Restriction>
                  <owl:onProperty rdf:resource="http://www.opengis.net/gml#about"/>
                  <owl:allValuesFrom rdf:resource="http://www.w3.org/2001/XMLSchema#anyURI"/>
               </owl:Restriction>
            </owl:intersectionOf>
         </owl:Class>
      </rdfs:subClassOf>
   </owl:Class>
   <owl:Class rdf:about="http://www.opengis.net/gml#GraphStyleType">
      <rdfs:comment>[complexType of] The style descriptor for a graph consisting of a number of features. Describes graph-specific style attributes.</rdfs:comment>
      <rdfs:subClassOf>
         <owl:Class>
            <owl:intersectionOf rdf:parseType="Collection">
               <owl:Restriction>
                  <owl:onProperty rdf:resource="http://www.opengis.net/gml#planar"/>
                  <owl:allValuesFrom rdf:resource="http://www.w3.org/2001/XMLSchema#boolean"/>
               </owl:Restriction>
               <owl:Restriction>
                  <owl:onProperty rdf:resource="http://www.opengis.net/gml#planar"/>
                  <owl:minCardinality rdf:datatype="http://www.w3.org/2001/XMLSchema#nonNegativeInteger">0</owl:minCardinality>
               </owl:Restriction>
               <owl:Restriction>
                  <owl:onProperty rdf:resource="http://www.opengis.net/gml#directed"/>
                  <owl:allValuesFrom rdf:resource="http://www.w3.org/2001/XMLSchema#boolean"/>
               </owl:Restriction>
               <owl:Restriction>
                  <owl:onProperty rdf:resource="http://www.opengis.net/gml#directed"/>
                  <owl:minCardinality rdf:datatype="http://www.w3.org/2001/XMLSchema#nonNegativeInteger">0</owl:minCardinality>
               </owl:Restriction>
               <owl:Restriction>
                  <owl:onProperty rdf:resource="http://www.opengis.net/gml#grid"/>
                  <owl:allValuesFrom rdf:resource="http://www.w3.org/2001/XMLSchema#boolean"/>
               </owl:Restriction>
               <owl:Restriction>
                  <owl:onProperty rdf:resource="http://www.opengis.net/gml#grid"/>
                  <owl:minCardinality rdf:datatype="http://www.w3.org/2001/XMLSchema#nonNegativeInteger">0</owl:minCardinality>
               </owl:Restriction>
               <owl:Restriction>
                  <owl:onProperty rdf:resource="http://www.opengis.net/gml#minDistance"/>
                  <owl:allValuesFrom rdf:resource="http://www.w3.org/2001/XMLSchema#double"/>
               </owl:Restriction>
               <owl:Restriction>
                  <owl:onProperty rdf:resource="http://www.opengis.net/gml#minDistance"/>
                  <owl:minCardinality rdf:datatype="http://www.w3.org/2001/XMLSchema#nonNegativeInteger">0</owl:minCardinality>
               </owl:Restriction>
               <owl:Restriction>
                  <owl:onProperty rdf:resource="http://www.opengis.net/gml#minAngle"/>
                  <owl:allValuesFrom rdf:resource="http://www.w3.org/2001/XMLSchema#double"/>
               </owl:Restriction>
               <owl:Restriction>
                  <owl:onProperty rdf:resource="http://www.opengis.net/gml#minAngle"/>
                  <owl:minCardinality rdf:datatype="http://www.w3.org/2001/XMLSchema#nonNegativeInteger">0</owl:minCardinality>
               </owl:Restriction>
               <owl:Restriction>
                  <owl:onProperty rdf:resource="http://www.opengis.net/gml#graphType"/>
                  <owl:allValuesFrom rdf:resource="http://www.opengis.net/gml#GraphTypeType"/>
               </owl:Restriction>
               <owl:Restriction>
                  <owl:onProperty rdf:resource="http://www.opengis.net/gml#graphType"/>
                  <owl:minCardinality rdf:datatype="http://www.w3.org/2001/XMLSchema#nonNegativeInteger">0</owl:minCardinality>
               </owl:Restriction>
               <owl:Restriction>
                  <owl:onProperty rdf:resource="http://www.opengis.net/gml#drawingType"/>
                  <owl:allValuesFrom rdf:resource="http://www.opengis.net/gml#DrawingTypeType"/>
               </owl:Restriction>
               <owl:Restriction>
                  <owl:onProperty rdf:resource="http://www.opengis.net/gml#drawingType"/>
                  <owl:minCardinality rdf:datatype="http://www.w3.org/2001/XMLSchema#nonNegativeInteger">0</owl:minCardinality>
               </owl:Restriction>
               <owl:Restriction>
                  <owl:onProperty rdf:resource="http://www.opengis.net/gml#lineType"/>
                  <owl:allValuesFrom rdf:resource="http://www.opengis.net/gml#LineTypeType"/>
               </owl:Restriction>
               <owl:Restriction>
                  <owl:onProperty rdf:resource="http://www.opengis.net/gml#lineType"/>
                  <owl:minCardinality rdf:datatype="http://www.w3.org/2001/XMLSchema#nonNegativeInteger">0</owl:minCardinality>
               </owl:Restriction>
               <owl:Restriction>
                  <owl:onProperty rdf:resource="http://www.opengis.net/gml#aestheticCriteria"/>
                  <owl:allValuesFrom rdf:resource="http://www.opengis.net/gml#AesheticCriteriaType"/>
               </owl:Restriction>
               <owl:Restriction>
                  <owl:onProperty rdf:resource="http://www.opengis.net/gml#aestheticCriteria"/>
                  <owl:minCardinality rdf:datatype="http://www.w3.org/2001/XMLSchema#nonNegativeInteger">0</owl:minCardinality>
               </owl:Restriction>
            </owl:intersectionOf>
         </owl:Class>
      </rdfs:subClassOf>
      <rdfs:subClassOf rdf:resource="http://www.opengis.net/gml#BaseStyleDescriptorType"/>
      <rdfs:comment>Warning: The parent class 'gml:BaseStyleDescriptorType' is declared outside of this class' original schema. This class may be declared incorrectly.</rdfs:comment>
   </owl:Class>
   <owl:Class rdf:about="http://www.opengis.net/gml#SymbolType">
      <rdfs:comment>[complexType of] The symbol property. Allows for remote referencing of symbols.</rdfs:comment>
      <rdfs:subClassOf>
         <owl:Class>
            <owl:intersectionOf rdf:parseType="Collection"/>
         </owl:Class>
      </rdfs:subClassOf>
      <rdfs:subClassOf>
         <owl:Class>
            <owl:intersectionOf rdf:parseType="Collection">
               <owl:Restriction>
                  <owl:onProperty rdf:resource="http://www.opengis.net/gml#symbolType"/>
                  <owl:allValuesFrom rdf:resource="http://www.opengis.net/gml#SymbolTypeEnumeration"/>
               </owl:Restriction>
               <owl:Restriction>
                  <owl:onProperty rdf:resource="http://www.opengis.net/gml#hastransform"/>
                  <owl:allValuesFrom rdf:resource="http://www.opengis.net/gml#transform"/>
               </owl:Restriction>
               <owl:Restriction>
                  <owl:onProperty rdf:resource="http://www.opengis.net/gml#about"/>
                  <owl:allValuesFrom rdf:resource="http://www.w3.org/2001/XMLSchema#anyURI"/>
               </owl:Restriction>
            </owl:intersectionOf>
         </owl:Class>
      </rdfs:subClassOf>
   </owl:Class>
   <owl:Class rdf:about="http://www.opengis.net/gml#LabelType">
      <rdfs:comment>Label is mixed -- composed of text and XPath expressions used to extract the useful information from the feature.</rdfs:comment>
      <rdfs:subClassOf>
         <owl:Class>
            <owl:intersectionOf rdf:parseType="Collection">
               <owl:Restriction>
                  <owl:onProperty rdf:resource="http://www.opengis.net/gml#LabelExpression"/>
                  <owl:allValuesFrom rdf:resource="http://www.w3.org/2001/XMLSchema#string"/>
               </owl:Restriction>
               <owl:Restriction>
                  <owl:onProperty rdf:resource="http://www.opengis.net/gml#LabelExpression"/>
                  <owl:minCardinality rdf:datatype="http://www.w3.org/2001/XMLSchema#nonNegativeInteger">0</owl:minCardinality>
               </owl:Restriction>
            </owl:intersectionOf>
         </owl:Class>
      </rdfs:subClassOf>
      <rdfs:subClassOf>
         <owl:Class>
            <owl:intersectionOf rdf:parseType="Collection">
               <owl:Restriction>
                  <owl:onProperty rdf:resource="http://www.opengis.net/gml#hastransform"/>
                  <owl:allValuesFrom rdf:resource="http://www.opengis.net/gml#transform"/>
               </owl:Restriction>
            </owl:intersectionOf>
         </owl:Class>
      </rdfs:subClassOf>
   </owl:Class>
   <owl:Class rdf:about="http://www.opengis.net/gml#StyleVariationType">
      <rdfs:comment>Used to vary individual graphic parameters and attributes of the style, symbol or text.</rdfs:comment>
      <rdfs:subClassOf>
         <owl:Class>
            <owl:intersectionOf rdf:parseType="Collection">
               <owl:Restriction>
                  <owl:onProperty rdf:resource="http://www.opengis.net/gml#styleProperty"/>
                  <owl:allValuesFrom rdf:resource="http://www.w3.org/2001/XMLSchema#string"/>
               </owl:Restriction>
               <owl:Restriction>
                  <owl:onProperty rdf:resource="http://www.opengis.net/gml#featurePropertyRange"/>
                  <owl:allValuesFrom rdf:resource="http://www.w3.org/2001/XMLSchema#string"/>
               </owl:Restriction>
            </owl:intersectionOf>
         </owl:Class>
      </rdfs:subClassOf>
   </owl:Class>
   <owl:DatatypeProperty rdf:about="http://www.opengis.net/gml#hasStyleVariationType">
      <rdfs:domain rdf:resource="http://www.opengis.net/gml#StyleVariationType"/>
      <rdfs:range rdf:resource="http://www.opengis.net/gml#string"/>
      <rdfs:subPropertyOf rdf:resource="http://www.opengis.net/gml#hasstring"/>
   </owl:DatatypeProperty>
   <owl:ObjectProperty rdf:about="http://www.opengis.net/gml#hasAssociationAttributeGroup">
      <rdfs:domain rdf:resource="http://www.opengis.net/gml#DefaultStylePropertyType"/>
      <rdfs:range rdf:resource="http://www.opengis.net/gml#AssociationAttributeGroup"/>
   </owl:ObjectProperty>
   <owl:ObjectProperty rdf:about="http://www.opengis.net/gml#hasAssociationAttributeGroup">
      <rdfs:domain rdf:resource="http://www.opengis.net/gml#FeatureStylePropertyType"/>
      <rdfs:range rdf:resource="http://www.opengis.net/gml#AssociationAttributeGroup"/>
   </owl:ObjectProperty>
   <owl:ObjectProperty rdf:about="http://www.opengis.net/gml#hasAssociationAttributeGroup">
      <rdfs:domain rdf:resource="http://www.opengis.net/gml#GeometryStylePropertyType"/>
      <rdfs:range rdf:resource="http://www.opengis.net/gml#AssociationAttributeGroup"/>
   </owl:ObjectProperty>
   <owl:ObjectProperty rdf:about="http://www.opengis.net/gml#hasAssociationAttributeGroup">
      <rdfs:domain rdf:resource="http://www.opengis.net/gml#TopologyStylePropertyType"/>
      <rdfs:range rdf:resource="http://www.opengis.net/gml#AssociationAttributeGroup"/>
   </owl:ObjectProperty>
   <owl:ObjectProperty rdf:about="http://www.opengis.net/gml#hasAssociationAttributeGroup">
      <rdfs:domain rdf:resource="http://www.opengis.net/gml#LabelStylePropertyType"/>
      <rdfs:range rdf:resource="http://www.opengis.net/gml#AssociationAttributeGroup"/>
   </owl:ObjectProperty>
   <owl:ObjectProperty rdf:about="http://www.opengis.net/gml#hasAssociationAttributeGroup">
      <rdfs:domain rdf:resource="http://www.opengis.net/gml#GraphStylePropertyType"/>
      <rdfs:range rdf:resource="http://www.opengis.net/gml#AssociationAttributeGroup"/>
   </owl:ObjectProperty>
   <owl:ObjectProperty rdf:about="http://www.opengis.net/gml#hasAssociationAttributeGroup">
      <rdfs:domain rdf:resource="http://www.opengis.net/gml#SymbolType"/>
      <rdfs:range rdf:resource="http://www.opengis.net/gml#AssociationAttributeGroup"/>
   </owl:ObjectProperty>
   <rdfs:Datatype rdf:about="http://www.opengis.net/gml#QueryGrammarEnumeration">
      <rdfs:comment>Used to specify the grammar of the feature query mechanism.</rdfs:comment>
      <owl:equivalentClass>
         <rdfs:Datatype>
            <owl:oneOf>
               <rdf:Description rdf:type="http://www.w3.org/1999/02/22-rdf-syntax-ns#List">
                  <rdf:first rdf:datatype="string">xpath</rdf:first>
                  <rdf:rest>
                     <rdf:Description rdf:type="http://www.w3.org/1999/02/22-rdf-syntax-ns#List">
                        <rdf:first rdf:datatype="string">xquery</rdf:first>
                        <rdf:rest>
                           <rdf:Description rdf:type="http://www.w3.org/1999/02/22-rdf-syntax-ns#List">
                              <rdf:first rdf:datatype="string">other</rdf:first>
                              <rdf:rest rdf:resource="http://www.w3.org/1999/02/22-rdf-syntax-ns#nil"/>
                           </rdf:Description>
                        </rdf:rest>
                     </rdf:Description>
                  </rdf:rest>
               </rdf:Description>
            </owl:oneOf>
         </rdfs:Datatype>
      </owl:equivalentClass>
   </rdfs:Datatype>
   <rdfs:Datatype rdf:about="http://www.opengis.net/gml#SymbolTypeEnumeration">
      <rdfs:comment>Used to specify the type of the symbol used.</rdfs:comment>
      <owl:equivalentClass>
         <rdfs:Datatype>
            <owl:oneOf>
               <rdf:Description rdf:type="http://www.w3.org/1999/02/22-rdf-syntax-ns#List">
                  <rdf:first rdf:datatype="string">svg</rdf:first>
                  <rdf:rest>
                     <rdf:Description rdf:type="http://www.w3.org/1999/02/22-rdf-syntax-ns#List">
                        <rdf:first rdf:datatype="string">xpath</rdf:first>
                        <rdf:rest>
                           <rdf:Description rdf:type="http://www.w3.org/1999/02/22-rdf-syntax-ns#List">
                              <rdf:first rdf:datatype="string">other</rdf:first>
                              <rdf:rest rdf:resource="http://www.w3.org/1999/02/22-rdf-syntax-ns#nil"/>
                           </rdf:Description>
                        </rdf:rest>
                     </rdf:Description>
                  </rdf:rest>
               </rdf:Description>
            </owl:oneOf>
         </rdfs:Datatype>
      </owl:equivalentClass>
   </rdfs:Datatype>
   <rdfs:Datatype rdf:about="http://www.opengis.net/gml#GraphTypeType">
      <rdfs:comment>Graph-specific styling property.</rdfs:comment>
      <owl:equivalentClass>
         <rdfs:Datatype>
            <owl:oneOf>
               <rdf:Description rdf:type="http://www.w3.org/1999/02/22-rdf-syntax-ns#List">
                  <rdf:first rdf:datatype="string">TREE</rdf:first>
                  <rdf:rest>
                     <rdf:Description rdf:type="http://www.w3.org/1999/02/22-rdf-syntax-ns#List">
                        <rdf:first rdf:datatype="string">BICONNECTED</rdf:first>
                        <rdf:rest rdf:resource="http://www.w3.org/1999/02/22-rdf-syntax-ns#nil"/>
                     </rdf:Description>
                  </rdf:rest>
               </rdf:Description>
            </owl:oneOf>
         </rdfs:Datatype>
      </owl:equivalentClass>
   </rdfs:Datatype>
   <rdfs:Datatype rdf:about="http://www.opengis.net/gml#DrawingTypeType">
      <rdfs:comment>Graph-specific styling property.</rdfs:comment>
      <owl:equivalentClass>
         <rdfs:Datatype>
            <owl:oneOf>
               <rdf:Description rdf:type="http://www.w3.org/1999/02/22-rdf-syntax-ns#List">
                  <rdf:first rdf:datatype="string">POLYLINE</rdf:first>
                  <rdf:rest>
                     <rdf:Description rdf:type="http://www.w3.org/1999/02/22-rdf-syntax-ns#List">
                        <rdf:first rdf:datatype="string">ORTHOGONAL</rdf:first>
                        <rdf:rest rdf:resource="http://www.w3.org/1999/02/22-rdf-syntax-ns#nil"/>
                     </rdf:Description>
                  </rdf:rest>
               </rdf:Description>
            </owl:oneOf>
         </rdfs:Datatype>
      </owl:equivalentClass>
   </rdfs:Datatype>
   <rdfs:Datatype rdf:about="http://www.opengis.net/gml#LineTypeType">
      <rdfs:comment>Graph-specific styling property.</rdfs:comment>
      <owl:equivalentClass>
         <rdfs:Datatype>
            <owl:oneOf>
               <rdf:Description rdf:type="http://www.w3.org/1999/02/22-rdf-syntax-ns#List">
                  <rdf:first rdf:datatype="string">STRAIGHT</rdf:first>
                  <rdf:rest>
                     <rdf:Description rdf:type="http://www.w3.org/1999/02/22-rdf-syntax-ns#List">
                        <rdf:first rdf:datatype="string">BENT</rdf:first>
                        <rdf:rest rdf:resource="http://www.w3.org/1999/02/22-rdf-syntax-ns#nil"/>
                     </rdf:Description>
                  </rdf:rest>
               </rdf:Description>
            </owl:oneOf>
         </rdfs:Datatype>
      </owl:equivalentClass>
   </rdfs:Datatype>
   <rdfs:Datatype rdf:about="http://www.opengis.net/gml#AesheticCriteriaType">
      <rdfs:comment>Graph-specific styling property.</rdfs:comment>
      <owl:equivalentClass>
         <rdfs:Datatype>
            <owl:oneOf>
               <rdf:Description rdf:type="http://www.w3.org/1999/02/22-rdf-syntax-ns#List">
                  <rdf:first rdf:datatype="string">MIN_CROSSINGS</rdf:first>
                  <rdf:rest>
                     <rdf:Description rdf:type="http://www.w3.org/1999/02/22-rdf-syntax-ns#List">
                        <rdf:first rdf:datatype="string">MIN_AREA</rdf:first>
                        <rdf:rest>
                           <rdf:Description rdf:type="http://www.w3.org/1999/02/22-rdf-syntax-ns#List">
                              <rdf:first rdf:datatype="string">MIN_BENDS</rdf:first>
                              <rdf:rest>
                                 <rdf:Description rdf:type="http://www.w3.org/1999/02/22-rdf-syntax-ns#List">
                                    <rdf:first rdf:datatype="string">MAX_BENDS</rdf:first>
                                    <rdf:rest>
                                       <rdf:Description rdf:type="http://www.w3.org/1999/02/22-rdf-syntax-ns#List">
                                          <rdf:first rdf:datatype="string">UNIFORM_BENDS</rdf:first>
                                          <rdf:rest>
                                             <rdf:Description rdf:type="http://www.w3.org/1999/02/22-rdf-syntax-ns#List">
                                                <rdf:first rdf:datatype="string">MIN_SLOPES</rdf:first>
                                                <rdf:rest>
                                                   <rdf:Description rdf:type="http://www.w3.org/1999/02/22-rdf-syntax-ns#List">
                                                      <rdf:first rdf:datatype="string">MIN_EDGE_LENGTH</rdf:first>
                                                      <rdf:rest>
                                                         <rdf:Description rdf:type="http://www.w3.org/1999/02/22-rdf-syntax-ns#List">
                                                            <rdf:first rdf:datatype="string">MAX_EDGE_LENGTH</rdf:first>
                                                            <rdf:rest>
                                                               <rdf:Description rdf:type="http://www.w3.org/1999/02/22-rdf-syntax-ns#List">
                                                                  <rdf:first rdf:datatype="string">UNIFORM_EDGE_LENGTH</rdf:first>
                                                                  <rdf:rest>
                                                                     <rdf:Description rdf:type="http://www.w3.org/1999/02/22-rdf-syntax-ns#List">
                                                                        <rdf:first rdf:datatype="string">MAX_ANGULAR_RESOLUTION</rdf:first>
                                                                        <rdf:rest>
                                                                           <rdf:Description rdf:type="http://www.w3.org/1999/02/22-rdf-syntax-ns#List">
                                                                              <rdf:first rdf:datatype="string">MIN_ASPECT_RATIO</rdf:first>
                                                                              <rdf:rest>
                                                                                 <rdf:Description rdf:type="http://www.w3.org/1999/02/22-rdf-syntax-ns#List">
                                                                                    <rdf:first rdf:datatype="string">MAX_SYMMETRIES</rdf:first>
                                                                                    <rdf:rest rdf:resource="http://www.w3.org/1999/02/22-rdf-syntax-ns#nil"/>
                                                                                 </rdf:Description>
                                                                              </rdf:rest>
                                                                           </rdf:Description>
                                                                        </rdf:rest>
                                                                     </rdf:Description>
                                                                  </rdf:rest>
                                                               </rdf:Description>
                                                            </rdf:rest>
                                                         </rdf:Description>
                                                      </rdf:rest>
                                                   </rdf:Description>
                                                </rdf:rest>
                                             </rdf:Description>
                                          </rdf:rest>
                                       </rdf:Description>
                                    </rdf:rest>
                                 </rdf:Description>
                              </rdf:rest>
                           </rdf:Description>
                        </rdf:rest>
                     </rdf:Description>
                  </rdf:rest>
               </rdf:Description>
            </owl:oneOf>
         </rdfs:Datatype>
      </owl:equivalentClass>
   </rdfs:Datatype>
   <owl:DatatypeProperty rdf:about="http://www.opengis.net/gml#about">
      <rdfs:domain rdf:resource="http://www.opengis.net/gml#DefaultStylePropertyType"/>
      <rdfs:range rdf:resource="http://www.w3.org/2001/XMLSchema#anyURI"/>
   </owl:DatatypeProperty>
   <owl:DatatypeProperty rdf:about="http://www.opengis.net/gml#about">
      <rdfs:domain rdf:resource="http://www.opengis.net/gml#FeatureStylePropertyType"/>
      <rdfs:range rdf:resource="http://www.w3.org/2001/XMLSchema#anyURI"/>
   </owl:DatatypeProperty>
   <owl:DatatypeProperty rdf:about="http://www.opengis.net/gml#featureType">
      <rdfs:domain rdf:resource="http://www.opengis.net/gml#FeatureStyleType"/>
      <rdfs:range rdf:resource="http://www.w3.org/2001/XMLSchema#string"/>
   </owl:DatatypeProperty>
   <owl:DatatypeProperty rdf:about="http://www.opengis.net/gml#baseType">
      <rdfs:domain rdf:resource="http://www.opengis.net/gml#FeatureStyleType"/>
      <rdfs:range rdf:resource="http://www.w3.org/2001/XMLSchema#string"/>
   </owl:DatatypeProperty>
   <owl:DatatypeProperty rdf:about="http://www.opengis.net/gml#queryGrammar">
      <rdfs:domain rdf:resource="http://www.opengis.net/gml#FeatureStyleType"/>
      <rdfs:range rdf:resource="http://www.opengis.net/gml#QueryGrammarEnumeration"/>
   </owl:DatatypeProperty>
   <owl:DatatypeProperty rdf:about="http://www.opengis.net/gml#about">
      <rdfs:domain rdf:resource="http://www.opengis.net/gml#GeometryStylePropertyType"/>
      <rdfs:range rdf:resource="http://www.w3.org/2001/XMLSchema#anyURI"/>
   </owl:DatatypeProperty>
   <owl:DatatypeProperty rdf:about="http://www.opengis.net/gml#geometryProperty">
      <rdfs:domain rdf:resource="http://www.opengis.net/gml#GeometryStyleType"/>
      <rdfs:range rdf:resource="http://www.w3.org/2001/XMLSchema#string"/>
   </owl:DatatypeProperty>
   <owl:DatatypeProperty rdf:about="http://www.opengis.net/gml#geometryType">
      <rdfs:domain rdf:resource="http://www.opengis.net/gml#GeometryStyleType"/>
      <rdfs:range rdf:resource="http://www.w3.org/2001/XMLSchema#string"/>
   </owl:DatatypeProperty>
   <owl:DatatypeProperty rdf:about="http://www.opengis.net/gml#about">
      <rdfs:domain rdf:resource="http://www.opengis.net/gml#TopologyStylePropertyType"/>
      <rdfs:range rdf:resource="http://www.w3.org/2001/XMLSchema#anyURI"/>
   </owl:DatatypeProperty>
   <owl:DatatypeProperty rdf:about="http://www.opengis.net/gml#topologyProperty">
      <rdfs:domain rdf:resource="http://www.opengis.net/gml#TopologyStyleType"/>
      <rdfs:range rdf:resource="http://www.w3.org/2001/XMLSchema#string"/>
   </owl:DatatypeProperty>
   <owl:DatatypeProperty rdf:about="http://www.opengis.net/gml#topologyType">
      <rdfs:domain rdf:resource="http://www.opengis.net/gml#TopologyStyleType"/>
      <rdfs:range rdf:resource="http://www.w3.org/2001/XMLSchema#string"/>
   </owl:DatatypeProperty>
   <owl:DatatypeProperty rdf:about="http://www.opengis.net/gml#about">
      <rdfs:domain rdf:resource="http://www.opengis.net/gml#LabelStylePropertyType"/>
      <rdfs:range rdf:resource="http://www.w3.org/2001/XMLSchema#anyURI"/>
   </owl:DatatypeProperty>
   <owl:DatatypeProperty rdf:about="http://www.opengis.net/gml#about">
      <rdfs:domain rdf:resource="http://www.opengis.net/gml#GraphStylePropertyType"/>
      <rdfs:range rdf:resource="http://www.w3.org/2001/XMLSchema#anyURI"/>
   </owl:DatatypeProperty>
   <owl:DatatypeProperty rdf:about="http://www.opengis.net/gml#symbolType">
      <rdfs:domain rdf:resource="http://www.opengis.net/gml#SymbolType"/>
      <rdfs:range rdf:resource="http://www.opengis.net/gml#SymbolTypeEnumeration"/>
   </owl:DatatypeProperty>
   <owl:DatatypeProperty rdf:about="http://www.opengis.net/gml#hastransform">
      <rdfs:domain rdf:resource="http://www.opengis.net/gml#SymbolType"/>
      <rdfs:range rdf:resource="http://www.opengis.net/gml#transform"/>
   </owl:DatatypeProperty>
   <owl:DatatypeProperty rdf:about="http://www.opengis.net/gml#about">
      <rdfs:domain rdf:resource="http://www.opengis.net/gml#SymbolType"/>
      <rdfs:range rdf:resource="http://www.w3.org/2001/XMLSchema#anyURI"/>
   </owl:DatatypeProperty>
   <owl:DatatypeProperty rdf:about="http://www.opengis.net/gml#hastransform">
      <rdfs:domain rdf:resource="http://www.opengis.net/gml#LabelType"/>
      <rdfs:range rdf:resource="http://www.opengis.net/gml#transform"/>
   </owl:DatatypeProperty>
   <rdfs:Datatype rdf:about="http://www.opengis.net/gml#transform">
      <rdfs:comment>Defines the geometric transformation of entities. There is no particular grammar defined for this value.</rdfs:comment>
      <owl:equivalentClass rdf:resource="http://www.w3.org/2001/XMLSchema#string"/>
   </rdfs:Datatype>
   <owl:DatatypeProperty rdf:about="http://www.opengis.net/gml#styleProperty">
      <rdfs:domain rdf:resource="http://www.opengis.net/gml#StyleVariationType"/>
      <rdfs:range rdf:resource="http://www.w3.org/2001/XMLSchema#string"/>
   </owl:DatatypeProperty>
   <owl:DatatypeProperty rdf:about="http://www.opengis.net/gml#featurePropertyRange">
      <rdfs:domain rdf:resource="http://www.opengis.net/gml#StyleVariationType"/>
      <rdfs:range rdf:resource="http://www.w3.org/2001/XMLSchema#string"/>
   </owl:DatatypeProperty>
   <owl:Class rdf:about="http://www.opengis.net/gml#defaultStyle">
      <rdfs:subClassOf rdf:resource="http://www.opengis.net/gml#DefaultStylePropertyType"/>
      <rdfs:comment>Warning: This class type was declared outside of its original schema. This class may be declared incorrectly.</rdfs:comment>
   </owl:Class>
   <owl:Class rdf:about="http://www.opengis.net/gml#_Style">
      <rdfs:subClassOf rdf:resource="http://www.opengis.net/gml#_GML"/>
      <rdfs:subClassOf rdf:resource="http://www.opengis.net/gml#AbstractStyleType"/>
      <rdfs:comment>Warning: This class type was declared outside of its original schema. This class may be declared incorrectly.</rdfs:comment>
   </owl:Class>
   <owl:Class rdf:about="http://www.opengis.net/gml#Style">
      <rdfs:subClassOf rdf:resource="http://www.opengis.net/gml#_Style"/>
      <rdfs:subClassOf rdf:resource="http://www.opengis.net/gml#StyleType"/>
      <rdfs:comment>Warning: This class type was declared outside of its original schema. This class may be declared incorrectly.</rdfs:comment>
   </owl:Class>
   <owl:Class rdf:about="http://www.opengis.net/gml#featureStyle">
      <rdfs:subClassOf rdf:resource="http://www.opengis.net/gml#FeatureStylePropertyType"/>
      <rdfs:comment>Warning: This class type was declared outside of its original schema. This class may be declared incorrectly.</rdfs:comment>
   </owl:Class>
   <owl:Class rdf:about="http://www.opengis.net/gml#FeatureStyle">
      <rdfs:subClassOf rdf:resource="http://www.opengis.net/gml#_GML"/>
      <rdfs:subClassOf rdf:resource="http://www.opengis.net/gml#FeatureStyleType"/>
      <rdfs:comment>Warning: This class type was declared outside of its original schema. This class may be declared incorrectly.</rdfs:comment>
   </owl:Class>
   <owl:Class rdf:about="http://www.opengis.net/gml#geometryStyle">
      <rdfs:subClassOf rdf:resource="http://www.opengis.net/gml#GeometryStylePropertyType"/>
      <rdfs:comment>Warning: This class type was declared outside of its original schema. This class may be declared incorrectly.</rdfs:comment>
   </owl:Class>
   <owl:Class rdf:about="http://www.opengis.net/gml#GeometryStyle">
      <rdfs:subClassOf rdf:resource="http://www.opengis.net/gml#_GML"/>
      <rdfs:subClassOf rdf:resource="http://www.opengis.net/gml#GeometryStyleType"/>
      <rdfs:comment>Warning: This class type was declared outside of its original schema. This class may be declared incorrectly.</rdfs:comment>
   </owl:Class>
   <owl:Class rdf:about="http://www.opengis.net/gml#topologyStyle">
      <rdfs:subClassOf rdf:resource="http://www.opengis.net/gml#TopologyStylePropertyType"/>
      <rdfs:comment>Warning: This class type was declared outside of its original schema. This class may be declared incorrectly.</rdfs:comment>
   </owl:Class>
   <owl:Class rdf:about="http://www.opengis.net/gml#TopologyStyle">
      <rdfs:subClassOf rdf:resource="http://www.opengis.net/gml#_GML"/>
      <rdfs:subClassOf rdf:resource="http://www.opengis.net/gml#TopologyStyleType"/>
      <rdfs:comment>Warning: This class type was declared outside of its original schema. This class may be declared incorrectly.</rdfs:comment>
   </owl:Class>
   <owl:Class rdf:about="http://www.opengis.net/gml#labelStyle">
      <rdfs:subClassOf rdf:resource="http://www.opengis.net/gml#LabelStylePropertyType"/>
      <rdfs:comment>Warning: This class type was declared outside of its original schema. This class may be declared incorrectly.</rdfs:comment>
   </owl:Class>
   <owl:Class rdf:about="http://www.opengis.net/gml#LabelStyle">
      <rdfs:subClassOf rdf:resource="http://www.opengis.net/gml#_GML"/>
      <rdfs:subClassOf rdf:resource="http://www.opengis.net/gml#LabelStyleType"/>
      <rdfs:comment>Warning: This class type was declared outside of its original schema. This class may be declared incorrectly.</rdfs:comment>
   </owl:Class>
   <owl:Class rdf:about="http://www.opengis.net/gml#graphStyle">
      <rdfs:subClassOf rdf:resource="http://www.opengis.net/gml#GraphStylePropertyType"/>
      <rdfs:comment>Warning: This class type was declared outside of its original schema. This class may be declared incorrectly.</rdfs:comment>
   </owl:Class>
   <owl:Class rdf:about="http://www.opengis.net/gml#GraphStyle">
      <rdfs:subClassOf rdf:resource="http://www.opengis.net/gml#_GML"/>
      <rdfs:subClassOf rdf:resource="http://www.opengis.net/gml#GraphStyleType"/>
      <rdfs:comment>Warning: This class type was declared outside of its original schema. This class may be declared incorrectly.</rdfs:comment>
   </owl:Class>
   <owl:Class rdf:about="http://www.opengis.net/gml#symbol">
      <rdfs:subClassOf rdf:resource="http://www.opengis.net/gml#SymbolType"/>
      <rdfs:comment>Warning: This class type was declared outside of its original schema. This class may be declared incorrectly.</rdfs:comment>
   </owl:Class>
   <owl:ObjectProperty rdf:about="http://www.opengis.net/gml#has_Style">
      <rdfs:comment>Warning: This ObjectProperty reference was declared outside of its original schema. This ObjectProperty may be declared incorrectly.</rdfs:comment>
      <rdfs:domain rdf:resource="http://www.opengis.net/gml#DefaultStylePropertyType"/>
      <rdfs:range rdf:resource="http://www.opengis.net/gml#_Style"/>
   </owl:ObjectProperty>
   <owl:ObjectProperty rdf:about="http://www.opengis.net/gml#hasfeatureStyle">
      <rdfs:comment>Warning: This ObjectProperty reference was declared outside of its original schema. This ObjectProperty may be declared incorrectly.</rdfs:comment>
      <rdfs:domain rdf:resource="http://www.opengis.net/gml#StyleType"/>
      <rdfs:range rdf:resource="http://www.opengis.net/gml#featureStyle"/>
   </owl:ObjectProperty>
   <owl:ObjectProperty rdf:about="http://www.opengis.net/gml#hasgraphStyle">
      <rdfs:comment>Warning: This ObjectProperty reference was declared outside of its original schema. This ObjectProperty may be declared incorrectly.</rdfs:comment>
      <rdfs:domain rdf:resource="http://www.opengis.net/gml#StyleType"/>
      <rdfs:range rdf:resource="http://www.opengis.net/gml#graphStyle"/>
   </owl:ObjectProperty>
   <owl:ObjectProperty rdf:about="http://www.opengis.net/gml#hasFeatureStyle">
      <rdfs:comment>Warning: This ObjectProperty reference was declared outside of its original schema. This ObjectProperty may be declared incorrectly.</rdfs:comment>
      <rdfs:domain rdf:resource="http://www.opengis.net/gml#FeatureStylePropertyType"/>
      <rdfs:range rdf:resource="http://www.opengis.net/gml#FeatureStyle"/>
   </owl:ObjectProperty>
   <owl:DatatypeProperty rdf:about="http://www.opengis.net/gml#featureConstraint">
      <rdfs:domain rdf:resource="http://www.opengis.net/gml#FeatureStyleType"/>
      <rdfs:range rdf:resource="http://www.w3.org/2001/XMLSchema#string"/>
   </owl:DatatypeProperty>
   <owl:ObjectProperty rdf:about="http://www.opengis.net/gml#hasgeometryStyle">
      <rdfs:comment>Warning: This ObjectProperty reference was declared outside of its original schema. This ObjectProperty may be declared incorrectly.</rdfs:comment>
      <rdfs:domain rdf:resource="http://www.opengis.net/gml#FeatureStyleType"/>
      <rdfs:range rdf:resource="http://www.opengis.net/gml#geometryStyle"/>
   </owl:ObjectProperty>
   <owl:ObjectProperty rdf:about="http://www.opengis.net/gml#hastopologyStyle">
      <rdfs:comment>Warning: This ObjectProperty reference was declared outside of its original schema. This ObjectProperty may be declared incorrectly.</rdfs:comment>
      <rdfs:domain rdf:resource="http://www.opengis.net/gml#FeatureStyleType"/>
      <rdfs:range rdf:resource="http://www.opengis.net/gml#topologyStyle"/>
   </owl:ObjectProperty>
   <owl:ObjectProperty rdf:about="http://www.opengis.net/gml#haslabelStyle">
      <rdfs:comment>Warning: This ObjectProperty reference was declared outside of its original schema. This ObjectProperty may be declared incorrectly.</rdfs:comment>
      <rdfs:domain rdf:resource="http://www.opengis.net/gml#FeatureStyleType"/>
      <rdfs:range rdf:resource="http://www.opengis.net/gml#labelStyle"/>
   </owl:ObjectProperty>
   <owl:ObjectProperty rdf:about="http://www.opengis.net/gml#spatialResolution">
      <rdfs:comment>Warning: This ObjectProperty type was declared outside of its original schema. This ObjectProperty may be declared incorrectly.</rdfs:comment>
      <rdfs:domain rdf:resource="http://www.opengis.net/gml#BaseStyleDescriptorType"/>
      <rdfs:range rdf:resource="http://www.opengis.net/gml#ScaleType"/>
   </owl:ObjectProperty>
   <owl:ObjectProperty rdf:about="http://www.opengis.net/gml#styleVariation">
      <rdfs:comment>Warning: This ObjectProperty type was declared outside of its original schema. This ObjectProperty may be declared incorrectly.</rdfs:comment>
      <rdfs:domain rdf:resource="http://www.opengis.net/gml#BaseStyleDescriptorType"/>
      <rdfs:range rdf:resource="http://www.opengis.net/gml#StyleVariationType"/>
   </owl:ObjectProperty>
   <owl:ObjectProperty rdf:about="http://www.w3.org/2001/SMIL20/#hasanimate">
      <rdfs:comment>Warning: This ObjectProperty reference was declared outside of its original schema. This ObjectProperty may be declared incorrectly.</rdfs:comment>
      <rdfs:domain rdf:resource="http://www.opengis.net/gml#BaseStyleDescriptorType"/>
      <rdfs:range rdf:resource="http://www.w3.org/2001/SMIL20/#animate"/>
   </owl:ObjectProperty>
   <owl:ObjectProperty rdf:about="http://www.w3.org/2001/SMIL20/#hasanimateMotion">
      <rdfs:comment>Warning: This ObjectProperty reference was declared outside of its original schema. This ObjectProperty may be declared incorrectly.</rdfs:comment>
      <rdfs:domain rdf:resource="http://www.opengis.net/gml#BaseStyleDescriptorType"/>
      <rdfs:range rdf:resource="http://www.w3.org/2001/SMIL20/#animateMotion"/>
   </owl:ObjectProperty>
   <owl:ObjectProperty rdf:about="http://www.w3.org/2001/SMIL20/#hasanimateColor">
      <rdfs:comment>Warning: This ObjectProperty reference was declared outside of its original schema. This ObjectProperty may be declared incorrectly.</rdfs:comment>
      <rdfs:domain rdf:resource="http://www.opengis.net/gml#BaseStyleDescriptorType"/>
      <rdfs:range rdf:resource="http://www.w3.org/2001/SMIL20/#animateColor"/>
   </owl:ObjectProperty>
   <owl:ObjectProperty rdf:about="http://www.w3.org/2001/SMIL20/#hasset">
      <rdfs:comment>Warning: This ObjectProperty reference was declared outside of its original schema. This ObjectProperty may be declared incorrectly.</rdfs:comment>
      <rdfs:domain rdf:resource="http://www.opengis.net/gml#BaseStyleDescriptorType"/>
      <rdfs:range rdf:resource="http://www.w3.org/2001/SMIL20/#set"/>
   </owl:ObjectProperty>
   <owl:ObjectProperty rdf:about="http://www.opengis.net/gml#hasGeometryStyle">
      <rdfs:comment>Warning: This ObjectProperty reference was declared outside of its original schema. This ObjectProperty may be declared incorrectly.</rdfs:comment>
      <rdfs:domain rdf:resource="http://www.opengis.net/gml#GeometryStylePropertyType"/>
      <rdfs:range rdf:resource="http://www.opengis.net/gml#GeometryStyle"/>
   </owl:ObjectProperty>
   <owl:ObjectProperty rdf:about="http://www.opengis.net/gml#hassymbol">
      <rdfs:comment>Warning: This ObjectProperty reference was declared outside of its original schema. This ObjectProperty may be declared incorrectly.</rdfs:comment>
      <rdfs:domain rdf:resource="http://www.opengis.net/gml#GeometryStyleType"/>
      <rdfs:range rdf:resource="http://www.opengis.net/gml#symbol"/>
   </owl:ObjectProperty>
   <owl:DatatypeProperty rdf:about="http://www.opengis.net/gml#style">
      <rdfs:domain rdf:resource="http://www.opengis.net/gml#GeometryStyleType"/>
      <rdfs:range rdf:resource="http://www.w3.org/2001/XMLSchema#string"/>
   </owl:DatatypeProperty>
   <owl:ObjectProperty rdf:about="http://www.opengis.net/gml#haslabelStyle">
      <rdfs:comment>Warning: This ObjectProperty reference was declared outside of its original schema. This ObjectProperty may be declared incorrectly.</rdfs:comment>
      <rdfs:domain rdf:resource="http://www.opengis.net/gml#GeometryStyleType"/>
      <rdfs:range rdf:resource="http://www.opengis.net/gml#labelStyle"/>
   </owl:ObjectProperty>
   <owl:ObjectProperty rdf:about="http://www.opengis.net/gml#hasTopologyStyle">
      <rdfs:comment>Warning: This ObjectProperty reference was declared outside of its original schema. This ObjectProperty may be declared incorrectly.</rdfs:comment>
      <rdfs:domain rdf:resource="http://www.opengis.net/gml#TopologyStylePropertyType"/>
      <rdfs:range rdf:resource="http://www.opengis.net/gml#TopologyStyle"/>
   </owl:ObjectProperty>
   <owl:ObjectProperty rdf:about="http://www.opengis.net/gml#hassymbol">
      <rdfs:comment>Warning: This ObjectProperty reference was declared outside of its original schema. This ObjectProperty may be declared incorrectly.</rdfs:comment>
      <rdfs:domain rdf:resource="http://www.opengis.net/gml#TopologyStyleType"/>
      <rdfs:range rdf:resource="http://www.opengis.net/gml#symbol"/>
   </owl:ObjectProperty>
   <owl:DatatypeProperty rdf:about="http://www.opengis.net/gml#style">
      <rdfs:domain rdf:resource="http://www.opengis.net/gml#TopologyStyleType"/>
      <rdfs:range rdf:resource="http://www.w3.org/2001/XMLSchema#string"/>
   </owl:DatatypeProperty>
   <owl:ObjectProperty rdf:about="http://www.opengis.net/gml#haslabelStyle">
      <rdfs:comment>Warning: This ObjectProperty reference was declared outside of its original schema. This ObjectProperty may be declared incorrectly.</rdfs:comment>
      <rdfs:domain rdf:resource="http://www.opengis.net/gml#TopologyStyleType"/>
      <rdfs:range rdf:resource="http://www.opengis.net/gml#labelStyle"/>
   </owl:ObjectProperty>
   <owl:ObjectProperty rdf:about="http://www.opengis.net/gml#hasLabelStyle">
      <rdfs:comment>Warning: This ObjectProperty reference was declared outside of its original schema. This ObjectProperty may be declared incorrectly.</rdfs:comment>
      <rdfs:domain rdf:resource="http://www.opengis.net/gml#LabelStylePropertyType"/>
      <rdfs:range rdf:resource="http://www.opengis.net/gml#LabelStyle"/>
   </owl:ObjectProperty>
   <owl:DatatypeProperty rdf:about="http://www.opengis.net/gml#style">
      <rdfs:domain rdf:resource="http://www.opengis.net/gml#LabelStyleType"/>
      <rdfs:range rdf:resource="http://www.w3.org/2001/XMLSchema#string"/>
   </owl:DatatypeProperty>
   <owl:ObjectProperty rdf:about="http://www.opengis.net/gml#label">
      <rdfs:comment>Warning: This ObjectProperty type was declared outside of its original schema. This ObjectProperty may be declared incorrectly.</rdfs:comment>
      <rdfs:domain rdf:resource="http://www.opengis.net/gml#LabelStyleType"/>
      <rdfs:range rdf:resource="http://www.opengis.net/gml#LabelType"/>
   </owl:ObjectProperty>
   <owl:ObjectProperty rdf:about="http://www.opengis.net/gml#hasGraphStyle">
      <rdfs:comment>Warning: This ObjectProperty reference was declared outside of its original schema. This ObjectProperty may be declared incorrectly.</rdfs:comment>
      <rdfs:domain rdf:resource="http://www.opengis.net/gml#GraphStylePropertyType"/>
      <rdfs:range rdf:resource="http://www.opengis.net/gml#GraphStyle"/>
   </owl:ObjectProperty>
   <owl:DatatypeProperty rdf:about="http://www.opengis.net/gml#planar">
      <rdfs:domain rdf:resource="http://www.opengis.net/gml#GraphStyleType"/>
      <rdfs:range rdf:resource="http://www.w3.org/2001/XMLSchema#boolean"/>
   </owl:DatatypeProperty>
   <owl:DatatypeProperty rdf:about="http://www.opengis.net/gml#directed">
      <rdfs:domain rdf:resource="http://www.opengis.net/gml#GraphStyleType"/>
      <rdfs:range rdf:resource="http://www.w3.org/2001/XMLSchema#boolean"/>
   </owl:DatatypeProperty>
   <owl:DatatypeProperty rdf:about="http://www.opengis.net/gml#grid">
      <rdfs:domain rdf:resource="http://www.opengis.net/gml#GraphStyleType"/>
      <rdfs:range rdf:resource="http://www.w3.org/2001/XMLSchema#boolean"/>
   </owl:DatatypeProperty>
   <owl:DatatypeProperty rdf:about="http://www.opengis.net/gml#minDistance">
      <rdfs:domain rdf:resource="http://www.opengis.net/gml#GraphStyleType"/>
      <rdfs:range rdf:resource="http://www.w3.org/2001/XMLSchema#double"/>
   </owl:DatatypeProperty>
   <owl:DatatypeProperty rdf:about="http://www.opengis.net/gml#minAngle">
      <rdfs:domain rdf:resource="http://www.opengis.net/gml#GraphStyleType"/>
      <rdfs:range rdf:resource="http://www.w3.org/2001/XMLSchema#double"/>
   </owl:DatatypeProperty>
   <owl:ObjectProperty rdf:about="http://www.opengis.net/gml#graphType">
      <rdfs:comment>Warning: This ObjectProperty type was declared outside of its original schema. This ObjectProperty may be declared incorrectly.</rdfs:comment>
      <rdfs:domain rdf:resource="http://www.opengis.net/gml#GraphStyleType"/>
      <rdfs:range rdf:resource="http://www.opengis.net/gml#GraphTypeType"/>
   </owl:ObjectProperty>
   <owl:ObjectProperty rdf:about="http://www.opengis.net/gml#drawingType">
      <rdfs:comment>Warning: This ObjectProperty type was declared outside of its original schema. This ObjectProperty may be declared incorrectly.</rdfs:comment>
      <rdfs:domain rdf:resource="http://www.opengis.net/gml#GraphStyleType"/>
      <rdfs:range rdf:resource="http://www.opengis.net/gml#DrawingTypeType"/>
   </owl:ObjectProperty>
   <owl:ObjectProperty rdf:about="http://www.opengis.net/gml#lineType">
      <rdfs:comment>Warning: This ObjectProperty type was declared outside of its original schema. This ObjectProperty may be declared incorrectly.</rdfs:comment>
      <rdfs:domain rdf:resource="http://www.opengis.net/gml#GraphStyleType"/>
      <rdfs:range rdf:resource="http://www.opengis.net/gml#LineTypeType"/>
   </owl:ObjectProperty>
   <owl:ObjectProperty rdf:about="http://www.opengis.net/gml#aestheticCriteria">
      <rdfs:comment>Warning: This ObjectProperty type was declared outside of its original schema. This ObjectProperty may be declared incorrectly.</rdfs:comment>
      <rdfs:domain rdf:resource="http://www.opengis.net/gml#GraphStyleType"/>
      <rdfs:range rdf:resource="http://www.opengis.net/gml#AesheticCriteriaType"/>
   </owl:ObjectProperty>
   <owl:DatatypeProperty rdf:about="http://www.opengis.net/gml#LabelExpression">
      <rdfs:domain rdf:resource="http://www.opengis.net/gml#LabelType"/>
      <rdfs:range rdf:resource="http://www.w3.org/2001/XMLSchema#string"/>
   </owl:DatatypeProperty>
</rdf:RDF>
