<rdf:RDF xmlns:math="http://www.w3.org/2005/xpath-functions/math" xmlns:owl="http://www.w3.org/2002/07/owl#" xmlns:rdf="http://www.w3.org/1999/02/22-rdf-syntax-ns#" xmlns:rdfs="http://www.w3.org/2000/01/rdf-schema#" xmlns:xs="http://www.w3.org/2001/XMLSchema" xmlns:xsd="http://www.w3.org/2001/XMLSchema">
   <owl:Ontology rdf:about="http://liris.cnrs.fr/ontologies/dictionary">
      <rdfs:seeAlso>urn:opengis:specification:gml:schema-xsd:dictionary:3.1.1</rdfs:seeAlso>
      <rdfs:comment>
			Dictionary schema for GML 3.1.1 
			Components to support the lists of definitions.
			
			GML is an OGC Standard.
			Copyright (c) 2001,2005,2010 Open Geospatial Consortium.
			To obtain additional rights of use, visit http://www.opengeospatial.org/legal/ .
		</rdfs:comment>
   </owl:Ontology>
   <owl:Class rdf:about="http://www.opengis.net/gml#DefinitionType">
      <rdfs:comment>A definition, which can be included in or referenced by a dictionary. In this extended type, the inherited "description" optional element can hold the definition whenever only text is needed. The inherited "name" elements can provide one or more brief terms for which this is the definition. The inherited "metaDataProperty" elements can be used to reference or include more information about this definition.  
The gml:id attribute is required - it must be possible to reference this definition using this handle.  </rdfs:comment>
      <rdfs:subClassOf>
         <owl:Class>
            <owl:intersectionOf rdf:parseType="Collection">
               <owl:Restriction>
                  <owl:onProperty rdf:resource="http://www.opengis.net/gml#hasmetaDataProperty"/>
                  <owl:allValuesFrom rdf:resource="http://www.opengis.net/gml#metaDataProperty"/>
               </owl:Restriction>
               <owl:Restriction>
                  <owl:onProperty rdf:resource="http://www.opengis.net/gml#hasmetaDataProperty"/>
                  <owl:minCardinality rdf:datatype="http://www.w3.org/2001/XMLSchema#nonNegativeInteger">0</owl:minCardinality>
               </owl:Restriction>
               <owl:Restriction>
                  <owl:onProperty rdf:resource="http://www.opengis.net/gml#hasdescription"/>
                  <owl:allValuesFrom rdf:resource="http://www.opengis.net/gml#description"/>
               </owl:Restriction>
               <owl:Restriction>
                  <owl:onProperty rdf:resource="http://www.opengis.net/gml#hasdescription"/>
                  <owl:minCardinality rdf:datatype="http://www.w3.org/2001/XMLSchema#nonNegativeInteger">0</owl:minCardinality>
               </owl:Restriction>
               <owl:Restriction>
                  <owl:onProperty rdf:resource="http://www.opengis.net/gml#hasname"/>
                  <owl:allValuesFrom rdf:resource="http://www.opengis.net/gml#name"/>
               </owl:Restriction>
            </owl:intersectionOf>
         </owl:Class>
      </rdfs:subClassOf>
      <rdfs:subClassOf>
         <owl:Class>
            <owl:intersectionOf rdf:parseType="Collection">
               <owl:Restriction>
                  <owl:onProperty rdf:resource="http://www.opengis.net/gml#hasid"/>
                  <owl:allValuesFrom rdf:resource="http://www.opengis.net/gml#id"/>
               </owl:Restriction>
            </owl:intersectionOf>
         </owl:Class>
      </rdfs:subClassOf>
   </owl:Class>
   <owl:Class rdf:about="http://www.opengis.net/gml#DictionaryType">
      <rdfs:comment>A non-abstract bag that is specialized for use as a dictionary which contains a set of definitions. These definitions are referenced from other places, in the same and different XML documents. In this restricted type, the inherited optional "description" element can be used for a description of this dictionary. The inherited optional "name" element can be used for the name(s) of this dictionary. The inherited "metaDataProperty" elements can be used to reference or contain more information about this dictionary. The inherited required gml:id attribute allows the dictionary to be referenced using this handle. </rdfs:comment>
      <owl:disjointUnionOf rdf:parseType="Collection">
         <owl:Restriction>
            <owl:onProperty rdf:resource="http://www.opengis.net/gml#hasdictionaryEntry"/>
            <owl:someValuesFrom rdf:resource="http://www.opengis.net/gml#dictionaryEntry"/>
         </owl:Restriction>
         <owl:Restriction>
            <owl:onProperty rdf:resource="http://www.opengis.net/gml#hasindirectEntry"/>
            <owl:someValuesFrom rdf:resource="http://www.opengis.net/gml#indirectEntry"/>
         </owl:Restriction>
      </owl:disjointUnionOf>
      <rdfs:subClassOf rdf:resource="http://www.opengis.net/gml#DefinitionType"/>
   </owl:Class>
   <owl:Class rdf:about="http://www.opengis.net/gml#DictionaryEntryType">
      <rdfs:comment>An entry in a dictionary of definitions. An instance of this type contains or refers to a definition object.  

The number of definitions contained in this dictionaryEntry is restricted to one, but a DefinitionCollection or Dictionary that contains multiple definitions can be substituted if needed. Specialized descendents of this dictionaryEntry might be restricted in an application schema to allow only including specified types of definitions as valid entries in a dictionary. </rdfs:comment>
      <rdfs:subClassOf>
         <owl:Class>
            <owl:intersectionOf rdf:parseType="Collection">
               <owl:Restriction>
                  <owl:onProperty rdf:resource="http://www.opengis.net/gml#hasDefinition"/>
                  <owl:allValuesFrom rdf:resource="http://www.opengis.net/gml#Definition"/>
               </owl:Restriction>
            </owl:intersectionOf>
         </owl:Class>
      </rdfs:subClassOf>
   </owl:Class>
   <owl:Class rdf:about="http://www.opengis.net/gml#IndirectEntryType">
      <rdfs:comment>An entry in a dictionary of definitions that contains a GML object which references a remote definition object. This entry is expected to be convenient in allowing multiple elements in one XML document to contain short (abbreviated XPointer) references, which are resolved to an external definition provided in a Dictionary element in the same XML document. Specialized descendents of this dictionaryEntry might be restricted in an application schema to allow only including specified types of definitions as valid entries in a dictionary. </rdfs:comment>
      <rdfs:subClassOf>
         <owl:Class>
            <owl:intersectionOf rdf:parseType="Collection">
               <owl:Restriction>
                  <owl:onProperty rdf:resource="http://www.opengis.net/gml#hasDefinitionProxy"/>
                  <owl:allValuesFrom rdf:resource="http://www.opengis.net/gml#DefinitionProxy"/>
               </owl:Restriction>
            </owl:intersectionOf>
         </owl:Class>
      </rdfs:subClassOf>
   </owl:Class>
   <owl:Class rdf:about="http://www.opengis.net/gml#DefinitionProxyType">
      <rdfs:comment>A proxy entry in a dictionary of definitions. An element of this type contains a reference to a remote definition object. This entry is expected to be convenient in allowing multiple elements in one XML document to contain short (abbreviated XPointer) references, which are resolved to an external definition provided in a Dictionary element in the same XML document. </rdfs:comment>
      <rdfs:subClassOf>
         <owl:Class>
            <owl:intersectionOf rdf:parseType="Collection">
               <owl:Restriction>
                  <owl:onProperty rdf:resource="http://www.opengis.net/gml#hasdefinitionRef"/>
                  <owl:allValuesFrom rdf:resource="http://www.opengis.net/gml#definitionRef"/>
               </owl:Restriction>
            </owl:intersectionOf>
         </owl:Class>
      </rdfs:subClassOf>
      <rdfs:subClassOf rdf:resource="http://www.opengis.net/gml#DefinitionType"/>
   </owl:Class>
   <owl:Class rdf:about="http://www.opengis.net/gml#StandardDefinitionProperties">
      <rdfs:subClassOf>
         <owl:Class>
            <owl:intersectionOf rdf:parseType="Collection">
               <owl:Restriction>
                  <owl:onProperty rdf:resource="http://www.opengis.net/gml#hasmetaDataProperty"/>
                  <owl:allValuesFrom rdf:resource="http://www.opengis.net/gml#metaDataProperty"/>
               </owl:Restriction>
               <owl:Restriction>
                  <owl:onProperty rdf:resource="http://www.opengis.net/gml#hasmetaDataProperty"/>
                  <owl:minCardinality rdf:datatype="http://www.w3.org/2001/XMLSchema#nonNegativeInteger">0</owl:minCardinality>
               </owl:Restriction>
               <owl:Restriction>
                  <owl:onProperty rdf:resource="http://www.opengis.net/gml#hasdescription"/>
                  <owl:allValuesFrom rdf:resource="http://www.opengis.net/gml#description"/>
               </owl:Restriction>
               <owl:Restriction>
                  <owl:onProperty rdf:resource="http://www.opengis.net/gml#hasdescription"/>
                  <owl:minCardinality rdf:datatype="http://www.w3.org/2001/XMLSchema#nonNegativeInteger">0</owl:minCardinality>
               </owl:Restriction>
               <owl:Restriction>
                  <owl:onProperty rdf:resource="http://www.opengis.net/gml#hasname"/>
                  <owl:allValuesFrom rdf:resource="http://www.opengis.net/gml#name"/>
               </owl:Restriction>
            </owl:intersectionOf>
         </owl:Class>
      </rdfs:subClassOf>
      <rdfs:comment>This content model group makes it easier to construct types that 
      derive from DefinitionType and its descendents "by restriction".  
      A reference to the group saves having to enumerate the standard definition properties. 
      See definition of StandardObjectProperties for more documentation</rdfs:comment>
   </owl:Class>
   <owl:DatatypeProperty rdf:about="http://www.opengis.net/gml#hasid">
      <rdfs:domain rdf:resource="http://www.opengis.net/gml#DefinitionType"/>
      <rdfs:range rdf:resource="http://www.opengis.net/gml#id"/>
   </owl:DatatypeProperty>
   <owl:Class rdf:about="http://www.opengis.net/gml#Definition">
      <rdfs:subClassOf rdf:resource="http://www.opengis.net/gml#_GML"/>
      <rdfs:subClassOf rdf:resource="http://www.opengis.net/gml#DefinitionType"/>
   </owl:Class>
   <owl:Class rdf:about="http://www.opengis.net/gml#Dictionary">
      <rdfs:subClassOf rdf:resource="http://www.opengis.net/gml#Definition"/>
      <rdfs:subClassOf rdf:resource="http://www.opengis.net/gml#DictionaryType"/>
   </owl:Class>
   <owl:Class rdf:about="http://www.opengis.net/gml#DefinitionCollection">
      <rdfs:subClassOf rdf:resource="http://www.opengis.net/gml#Definition"/>
      <rdfs:subClassOf rdf:resource="http://www.opengis.net/gml#DictionaryType"/>
   </owl:Class>
   <owl:Class rdf:about="http://www.opengis.net/gml#dictionaryEntry">
      <rdfs:subClassOf rdf:resource="http://www.opengis.net/gml#DictionaryEntryType"/>
   </owl:Class>
   <owl:Class rdf:about="http://www.opengis.net/gml#definitionMember">
      <rdfs:subClassOf rdf:resource="http://www.opengis.net/gml#dictionaryEntry"/>
      <rdfs:subClassOf rdf:resource="http://www.opengis.net/gml#DictionaryEntryType"/>
   </owl:Class>
   <owl:Class rdf:about="http://www.opengis.net/gml#indirectEntry">
      <rdfs:subClassOf rdf:resource="http://www.opengis.net/gml#IndirectEntryType"/>
   </owl:Class>
   <owl:Class rdf:about="http://www.opengis.net/gml#DefinitionProxy">
      <rdfs:subClassOf rdf:resource="http://www.opengis.net/gml#Definition"/>
      <rdfs:subClassOf rdf:resource="http://www.opengis.net/gml#DefinitionProxyType"/>
   </owl:Class>
   <owl:Class rdf:about="http://www.opengis.net/gml#definitionRef">
      <rdfs:subClassOf rdf:resource="ReferenceType"/>
      <rdfs:comment>Warning: This class type was declared outside of its original schema. This class may be declared incorrectly.</rdfs:comment>
   </owl:Class>
   <owl:ObjectProperty rdf:about="http://www.opengis.net/gml#hasmetaDataProperty">
      <rdfs:comment>Warning: This ObjectProperty reference was declared outside of its original schema. This ObjectProperty may be declared incorrectly.</rdfs:comment>
      <rdfs:domain rdf:resource="http://www.opengis.net/gml#StandardDefinitionProperties"/>
      <rdfs:range rdf:resource="http://www.opengis.net/gml#metaDataProperty"/>
   </owl:ObjectProperty>
   <owl:ObjectProperty rdf:about="http://www.opengis.net/gml#hasdescription">
      <rdfs:comment>Warning: This ObjectProperty reference was declared outside of its original schema. This ObjectProperty may be declared incorrectly.</rdfs:comment>
      <rdfs:domain rdf:resource="http://www.opengis.net/gml#StandardDefinitionProperties"/>
      <rdfs:range rdf:resource="http://www.opengis.net/gml#description"/>
   </owl:ObjectProperty>
   <owl:ObjectProperty rdf:about="http://www.opengis.net/gml#hasname">
      <rdfs:comment>Warning: This ObjectProperty reference was declared outside of its original schema. This ObjectProperty may be declared incorrectly.</rdfs:comment>
      <rdfs:domain rdf:resource="http://www.opengis.net/gml#StandardDefinitionProperties"/>
      <rdfs:range rdf:resource="http://www.opengis.net/gml#name"/>
   </owl:ObjectProperty>
   <owl:ObjectProperty rdf:about="http://www.opengis.net/gml#hasmetaDataProperty">
      <rdfs:comment>Warning: This ObjectProperty reference was declared outside of its original schema. This ObjectProperty may be declared incorrectly.</rdfs:comment>
      <rdfs:domain rdf:resource="http://www.opengis.net/gml#DefinitionType"/>
      <rdfs:range rdf:resource="http://www.opengis.net/gml#metaDataProperty"/>
   </owl:ObjectProperty>
   <owl:ObjectProperty rdf:about="http://www.opengis.net/gml#hasdescription">
      <rdfs:comment>Warning: This ObjectProperty reference was declared outside of its original schema. This ObjectProperty may be declared incorrectly.</rdfs:comment>
      <rdfs:domain rdf:resource="http://www.opengis.net/gml#DefinitionType"/>
      <rdfs:range rdf:resource="http://www.opengis.net/gml#description"/>
   </owl:ObjectProperty>
   <owl:ObjectProperty rdf:about="http://www.opengis.net/gml#hasname">
      <rdfs:comment>Warning: This ObjectProperty reference was declared outside of its original schema. This ObjectProperty may be declared incorrectly.</rdfs:comment>
      <rdfs:domain rdf:resource="http://www.opengis.net/gml#DefinitionType"/>
      <rdfs:range rdf:resource="http://www.opengis.net/gml#name"/>
   </owl:ObjectProperty>
   <owl:ObjectProperty rdf:about="http://www.opengis.net/gml#hasdictionaryEntry">
      <rdfs:comment>Warning: This ObjectProperty reference was declared outside of its original schema. This ObjectProperty may be declared incorrectly.</rdfs:comment>
      <rdfs:domain rdf:resource="http://www.opengis.net/gml#DictionaryType"/>
      <rdfs:range rdf:resource="http://www.opengis.net/gml#dictionaryEntry"/>
   </owl:ObjectProperty>
   <owl:ObjectProperty rdf:about="http://www.opengis.net/gml#hasindirectEntry">
      <rdfs:comment>Warning: This ObjectProperty reference was declared outside of its original schema. This ObjectProperty may be declared incorrectly.</rdfs:comment>
      <rdfs:domain rdf:resource="http://www.opengis.net/gml#DictionaryType"/>
      <rdfs:range rdf:resource="http://www.opengis.net/gml#indirectEntry"/>
   </owl:ObjectProperty>
   <owl:ObjectProperty rdf:about="http://www.opengis.net/gml#hasDefinition">
      <rdfs:comment>Warning: This ObjectProperty reference was declared outside of its original schema. This ObjectProperty may be declared incorrectly.</rdfs:comment>
      <rdfs:domain rdf:resource="http://www.opengis.net/gml#DictionaryEntryType"/>
      <rdfs:range rdf:resource="http://www.opengis.net/gml#Definition"/>
   </owl:ObjectProperty>
   <owl:ObjectProperty rdf:about="http://www.opengis.net/gml#hasDefinitionProxy">
      <rdfs:comment>Warning: This ObjectProperty reference was declared outside of its original schema. This ObjectProperty may be declared incorrectly.</rdfs:comment>
      <rdfs:domain rdf:resource="http://www.opengis.net/gml#IndirectEntryType"/>
      <rdfs:range rdf:resource="http://www.opengis.net/gml#DefinitionProxy"/>
   </owl:ObjectProperty>
   <owl:ObjectProperty rdf:about="http://www.opengis.net/gml#hasdefinitionRef">
      <rdfs:comment>Warning: This ObjectProperty reference was declared outside of its original schema. This ObjectProperty may be declared incorrectly.</rdfs:comment>
      <rdfs:domain rdf:resource="http://www.opengis.net/gml#DefinitionProxyType"/>
      <rdfs:range rdf:resource="http://www.opengis.net/gml#definitionRef"/>
   </owl:ObjectProperty>
</rdf:RDF>
