<rdf:RDF xmlns:math="http://www.w3.org/2005/xpath-functions/math" xmlns:owl="http://www.w3.org/2002/07/owl#" xmlns:rdf="http://www.w3.org/1999/02/22-rdf-syntax-ns#" xmlns:rdfs="http://www.w3.org/2000/01/rdf-schema#" xmlns:xs="http://www.w3.org/2001/XMLSchema" xmlns:xsd="http://www.w3.org/2001/XMLSchema">
   <owl:Ontology rdf:about="http://liris.cnrs.fr/ontologies/direction">
      <owl:imports rdf:resource="http://liris.cnrs.fr/ontologies/gml"/>
      <owl:imports rdf:resource="http://liris.cnrs.fr/ontologies/geometryBasic0d1d"/>
      <rdfs:comment>direction.xsd</rdfs:comment>
      <rdfs:seeAlso>urn:opengis:specification:gml:schema-xsd:direction:3.1.1</rdfs:seeAlso>
      <rdfs:comment>This schema defines "direction" element and type.
			
			GML is an OGC Standard.
			Copyright (c) 2001,2005,2010 Open Geospatial Consortium.
			To obtain additional rights of use, visit http://www.opengeospatial.org/legal/ .
		</rdfs:comment>
   </owl:Ontology>
   <owl:Class rdf:about="http://www.opengis.net/gml#DirectionPropertyType">
      <owl:disjointUnionOf rdf:parseType="Collection">
         <owl:Restriction>
            <owl:onProperty rdf:resource="http://www.opengis.net/gml#hasDirectionVector"/>
            <owl:someValuesFrom rdf:resource="http://www.opengis.net/gml#DirectionVector"/>
         </owl:Restriction>
         <owl:Restriction>
            <owl:onProperty rdf:resource="http://www.opengis.net/gml#hasCompassPoint"/>
            <owl:someValuesFrom rdf:resource="http://www.opengis.net/gml#CompassPoint"/>
         </owl:Restriction>
         <owl:Restriction>
            <owl:onProperty rdf:resource="http://www.opengis.net/gml#DirectionKeyword"/>
            <owl:someValuesFrom rdf:resource="http://www.opengis.net/gml#CodeType"/>
         </owl:Restriction>
         <owl:Restriction>
            <owl:onProperty rdf:resource="http://www.opengis.net/gml#DirectionString"/>
            <owl:someValuesFrom rdf:resource="http://www.opengis.net/gml#StringOrRefType"/>
         </owl:Restriction>
      </owl:disjointUnionOf>
   </owl:Class>
   <owl:Class rdf:about="http://www.opengis.net/gml#DirectionVectorType">
      <rdfs:comment>Direction expressed as a vector, either using components, or using angles.</rdfs:comment>
      <owl:disjointUnionOf rdf:parseType="Collection">
         <owl:Restriction>
            <owl:onProperty rdf:resource="http://www.opengis.net/gml#hasvector"/>
            <owl:someValuesFrom rdf:resource="http://www.opengis.net/gml#vector"/>
         </owl:Restriction>
         <owl:Restriction>
            <owl:intersectionOf rdf:parseType="Collection">
               <owl:Restriction>
                  <owl:onProperty rdf:resource="http://www.opengis.net/gml#horizontalAngle"/>
                  <owl:allValuesFrom rdf:resource="http://www.opengis.net/gml#AngleType"/>
               </owl:Restriction>
               <owl:Restriction>
                  <owl:onProperty rdf:resource="http://www.opengis.net/gml#verticalAngle"/>
                  <owl:allValuesFrom rdf:resource="http://www.opengis.net/gml#AngleType"/>
               </owl:Restriction>
            </owl:intersectionOf>
         </owl:Restriction>
      </owl:disjointUnionOf>
   </owl:Class>
   <owl:ObjectProperty rdf:about="http://www.opengis.net/gml#hasAssociationAttributeGroup">
      <rdfs:domain rdf:resource="http://www.opengis.net/gml#DirectionPropertyType"/>
      <rdfs:range rdf:resource="http://www.opengis.net/gml#AssociationAttributeGroup"/>
   </owl:ObjectProperty>
   <rdfs:Datatype rdf:about="http://www.opengis.net/gml#CompassPointEnumeration">
      <owl:equivalentClass>
         <rdfs:Datatype>
            <owl:oneOf>
               <rdf:Description rdf:type="http://www.w3.org/1999/02/22-rdf-syntax-ns#List">
                  <rdf:first rdf:datatype="http://www.w3.org/2001/XMLSchema#string">N</rdf:first>
                  <rdf:rest>
                     <rdf:Description rdf:type="http://www.w3.org/1999/02/22-rdf-syntax-ns#List">
                        <rdf:first rdf:datatype="http://www.w3.org/2001/XMLSchema#string">NNE</rdf:first>
                        <rdf:rest>
                           <rdf:Description rdf:type="http://www.w3.org/1999/02/22-rdf-syntax-ns#List">
                              <rdf:first rdf:datatype="http://www.w3.org/2001/XMLSchema#string">NE</rdf:first>
                              <rdf:rest>
                                 <rdf:Description rdf:type="http://www.w3.org/1999/02/22-rdf-syntax-ns#List">
                                    <rdf:first rdf:datatype="http://www.w3.org/2001/XMLSchema#string">ENE</rdf:first>
                                    <rdf:rest>
                                       <rdf:Description rdf:type="http://www.w3.org/1999/02/22-rdf-syntax-ns#List">
                                          <rdf:first rdf:datatype="http://www.w3.org/2001/XMLSchema#string">E</rdf:first>
                                          <rdf:rest>
                                             <rdf:Description rdf:type="http://www.w3.org/1999/02/22-rdf-syntax-ns#List">
                                                <rdf:first rdf:datatype="http://www.w3.org/2001/XMLSchema#string">ESE</rdf:first>
                                                <rdf:rest>
                                                   <rdf:Description rdf:type="http://www.w3.org/1999/02/22-rdf-syntax-ns#List">
                                                      <rdf:first rdf:datatype="http://www.w3.org/2001/XMLSchema#string">SE</rdf:first>
                                                      <rdf:rest>
                                                         <rdf:Description rdf:type="http://www.w3.org/1999/02/22-rdf-syntax-ns#List">
                                                            <rdf:first rdf:datatype="http://www.w3.org/2001/XMLSchema#string">SSE</rdf:first>
                                                            <rdf:rest>
                                                               <rdf:Description rdf:type="http://www.w3.org/1999/02/22-rdf-syntax-ns#List">
                                                                  <rdf:first rdf:datatype="http://www.w3.org/2001/XMLSchema#string">S</rdf:first>
                                                                  <rdf:rest>
                                                                     <rdf:Description rdf:type="http://www.w3.org/1999/02/22-rdf-syntax-ns#List">
                                                                        <rdf:first rdf:datatype="http://www.w3.org/2001/XMLSchema#string">SSW</rdf:first>
                                                                        <rdf:rest>
                                                                           <rdf:Description rdf:type="http://www.w3.org/1999/02/22-rdf-syntax-ns#List">
                                                                              <rdf:first rdf:datatype="http://www.w3.org/2001/XMLSchema#string">SW</rdf:first>
                                                                              <rdf:rest>
                                                                                 <rdf:Description rdf:type="http://www.w3.org/1999/02/22-rdf-syntax-ns#List">
                                                                                    <rdf:first rdf:datatype="http://www.w3.org/2001/XMLSchema#string">WSW</rdf:first>
                                                                                    <rdf:rest>
                                                                                       <rdf:Description rdf:type="http://www.w3.org/1999/02/22-rdf-syntax-ns#List">
                                                                                          <rdf:first rdf:datatype="http://www.w3.org/2001/XMLSchema#string">W</rdf:first>
                                                                                          <rdf:rest>
                                                                                             <rdf:Description rdf:type="http://www.w3.org/1999/02/22-rdf-syntax-ns#List">
                                                                                                <rdf:first rdf:datatype="http://www.w3.org/2001/XMLSchema#string">WNW</rdf:first>
                                                                                                <rdf:rest>
                                                                                                   <rdf:Description rdf:type="http://www.w3.org/1999/02/22-rdf-syntax-ns#List">
                                                                                                      <rdf:first rdf:datatype="http://www.w3.org/2001/XMLSchema#string">NW</rdf:first>
                                                                                                      <rdf:rest>
                                                                                                         <rdf:Description rdf:type="http://www.w3.org/1999/02/22-rdf-syntax-ns#List">
                                                                                                            <rdf:first rdf:datatype="http://www.w3.org/2001/XMLSchema#string">NNW</rdf:first>
                                                                                                            <rdf:rest rdf:resource="http://www.w3.org/1999/02/22-rdf-syntax-ns#nil"/>
                                                                                                         </rdf:Description>
                                                                                                      </rdf:rest>
                                                                                                   </rdf:Description>
                                                                                                </rdf:rest>
                                                                                             </rdf:Description>
                                                                                          </rdf:rest>
                                                                                       </rdf:Description>
                                                                                    </rdf:rest>
                                                                                 </rdf:Description>
                                                                              </rdf:rest>
                                                                           </rdf:Description>
                                                                        </rdf:rest>
                                                                     </rdf:Description>
                                                                  </rdf:rest>
                                                               </rdf:Description>
                                                            </rdf:rest>
                                                         </rdf:Description>
                                                      </rdf:rest>
                                                   </rdf:Description>
                                                </rdf:rest>
                                             </rdf:Description>
                                          </rdf:rest>
                                       </rdf:Description>
                                    </rdf:rest>
                                 </rdf:Description>
                              </rdf:rest>
                           </rdf:Description>
                        </rdf:rest>
                     </rdf:Description>
                  </rdf:rest>
               </rdf:Description>
            </owl:oneOf>
         </rdfs:Datatype>
      </owl:equivalentClass>
   </rdfs:Datatype>
   <owl:Class rdf:about="http://www.opengis.net/gml#direction">
      <rdfs:subClassOf rdf:resource="http://www.opengis.net/gml#DirectionPropertyType"/>
      <rdfs:comment>Warning: This class type was declared outside of its original schema. This class may be declared incorrectly.</rdfs:comment>
   </owl:Class>
   <owl:Class rdf:about="http://www.opengis.net/gml#DirectionVector">
      <rdfs:subClassOf rdf:resource="http://www.opengis.net/gml#DirectionVectorType"/>
      <rdfs:comment>Warning: This class type was declared outside of its original schema. This class may be declared incorrectly.</rdfs:comment>
   </owl:Class>
   <owl:Class rdf:about="http://www.opengis.net/gml#CompassPoint">
      <rdfs:subClassOf rdf:resource="http://www.opengis.net/gml#CompassPointEnumeration"/>
      <rdfs:comment>Warning: This class type was declared outside of its original schema. This class may be declared incorrectly.</rdfs:comment>
   </owl:Class>
   <owl:ObjectProperty rdf:about="http://www.opengis.net/gml#hasDirectionVector">
      <rdfs:comment>Warning: This ObjectProperty reference was declared outside of its original schema. This ObjectProperty may be declared incorrectly.</rdfs:comment>
      <rdfs:domain rdf:resource="http://www.opengis.net/gml#DirectionPropertyType"/>
      <rdfs:range rdf:resource="http://www.opengis.net/gml#DirectionVector"/>
   </owl:ObjectProperty>
   <owl:ObjectProperty rdf:about="http://www.opengis.net/gml#hasCompassPoint">
      <rdfs:comment>Warning: This ObjectProperty reference was declared outside of its original schema. This ObjectProperty may be declared incorrectly.</rdfs:comment>
      <rdfs:domain rdf:resource="http://www.opengis.net/gml#DirectionPropertyType"/>
      <rdfs:range rdf:resource="http://www.opengis.net/gml#CompassPoint"/>
   </owl:ObjectProperty>
   <owl:ObjectProperty rdf:about="http://www.opengis.net/gml#DirectionKeyword">
      <rdfs:comment>Warning: This ObjectProperty type was declared outside of its original schema. This ObjectProperty may be declared incorrectly.</rdfs:comment>
      <rdfs:domain rdf:resource="http://www.opengis.net/gml#DirectionPropertyType"/>
      <rdfs:range rdf:resource="http://www.opengis.net/gml#CodeType"/>
   </owl:ObjectProperty>
   <owl:ObjectProperty rdf:about="http://www.opengis.net/gml#DirectionString">
      <rdfs:comment>Warning: This ObjectProperty type was declared outside of its original schema. This ObjectProperty may be declared incorrectly.</rdfs:comment>
      <rdfs:domain rdf:resource="http://www.opengis.net/gml#DirectionPropertyType"/>
      <rdfs:range rdf:resource="http://www.opengis.net/gml#StringOrRefType"/>
   </owl:ObjectProperty>
   <owl:ObjectProperty rdf:about="http://www.opengis.net/gml#hasvector">
      <rdfs:comment>Warning: This ObjectProperty reference was declared outside of its original schema. This ObjectProperty may be declared incorrectly.</rdfs:comment>
      <rdfs:domain rdf:resource="http://www.opengis.net/gml#DirectionVectorType"/>
      <rdfs:range rdf:resource="http://www.opengis.net/gml#vector"/>
   </owl:ObjectProperty>
   <owl:ObjectProperty rdf:about="http://www.opengis.net/gml#horizontalAngle">
      <rdfs:comment>Warning: This ObjectProperty type was declared outside of its original schema. This ObjectProperty may be declared incorrectly.</rdfs:comment>
      <rdfs:domain rdf:resource="http://www.opengis.net/gml#DirectionVectorType"/>
      <rdfs:range rdf:resource="http://www.opengis.net/gml#AngleType"/>
   </owl:ObjectProperty>
   <owl:ObjectProperty rdf:about="http://www.opengis.net/gml#verticalAngle">
      <rdfs:comment>Warning: This ObjectProperty type was declared outside of its original schema. This ObjectProperty may be declared incorrectly.</rdfs:comment>
      <rdfs:domain rdf:resource="http://www.opengis.net/gml#DirectionVectorType"/>
      <rdfs:range rdf:resource="http://www.opengis.net/gml#AngleType"/>
   </owl:ObjectProperty>
</rdf:RDF>
