<rdf:RDF xmlns:math="http://www.w3.org/2005/xpath-functions/math" xmlns:owl="http://www.w3.org/2002/07/owl#" xmlns:rdf="http://www.w3.org/1999/02/22-rdf-syntax-ns#" xmlns:rdfs="http://www.w3.org/2000/01/rdf-schema#" xmlns:xs="http://www.w3.org/2001/XMLSchema" xmlns:xsd="http://www.w3.org/2001/XMLSchema">
   <owl:Ontology rdf:about="http://liris.cnrs.fr/ontologies/dynamicFeature">
      <owl:imports rdf:resource="http://liris.cnrs.fr/ontologies/gml"/>
      <owl:imports rdf:resource="http://liris.cnrs.fr/ontologies/feature"/>
      <owl:imports rdf:resource="http://liris.cnrs.fr/ontologies/direction"/>
      <rdfs:seeAlso>urn:opengis:specification:gml:schema-xsd:dynamicFeature:3.1.1</rdfs:seeAlso>
      <rdfs:comment xml:lang="en">Basic support for tracking moving objects and objects with changing state.
			
			GML is an OGC Standard.
			Copyright (c) 2001,2005,2010 Open Geospatial Consortium.
			To obtain additional rights of use, visit http://www.opengeospatial.org/legal/ .
		</rdfs:comment>
   </owl:Ontology>
   <owl:Class rdf:about="http://www.opengis.net/gml#AbstractTimeSliceType">
      <rdfs:comment>This is an abstract class</rdfs:comment>
      <rdfs:comment xml:lang="en">A timeslice encapsulates the time-varying properties of a dynamic feature--it 
        must be extended to represent a timestamped projection of a feature. The dataSource 
        property describes how the temporal data was acquired.</rdfs:comment>
      <rdfs:subClassOf>
         <owl:Class>
            <owl:intersectionOf rdf:parseType="Collection">
               <owl:Restriction>
                  <owl:onProperty rdf:resource="http://www.opengis.net/gml#hasvalidTime"/>
                  <owl:allValuesFrom rdf:resource="http://www.opengis.net/gml#validTime"/>
               </owl:Restriction>
               <owl:Restriction>
                  <owl:onProperty rdf:resource="http://www.opengis.net/gml#hasdataSource"/>
                  <owl:allValuesFrom rdf:resource="http://www.opengis.net/gml#dataSource"/>
               </owl:Restriction>
               <owl:Restriction>
                  <owl:onProperty rdf:resource="http://www.opengis.net/gml#hasdataSource"/>
                  <owl:minCardinality rdf:datatype="http://www.w3.org/2001/XMLSchema#nonNegativeInteger">0</owl:minCardinality>
               </owl:Restriction>
            </owl:intersectionOf>
         </owl:Class>
      </rdfs:subClassOf>
      <rdfs:subClassOf rdf:resource="http://www.opengis.net/gml#AbstractGMLType"/>
      <rdfs:comment>Warning: The parent class 'gml:AbstractGMLType' is declared outside of this class' original schema. This class may be declared incorrectly.</rdfs:comment>
   </owl:Class>
   <owl:Class rdf:about="http://www.opengis.net/gml#MovingObjectStatusType">
      <rdfs:comment xml:lang="en">This type encapsulates various dynamic properties of moving objects        
             (points, lines, regions). It is useful for dealing with features whose        
             geometry or topology changes over time.</rdfs:comment>
      <rdfs:subClassOf>
         <owl:Class>
            <owl:intersectionOf rdf:parseType="Collection">
               <owl:Restriction>
                  <owl:onProperty rdf:resource="http://www.opengis.net/gml#haslocation"/>
                  <owl:allValuesFrom rdf:resource="http://www.opengis.net/gml#location"/>
               </owl:Restriction>
               <owl:Restriction>
                  <owl:onProperty rdf:resource="http://www.opengis.net/gml#speed"/>
                  <owl:allValuesFrom rdf:resource="http://www.opengis.net/gml#MeasureType"/>
               </owl:Restriction>
               <owl:Restriction>
                  <owl:onProperty rdf:resource="http://www.opengis.net/gml#speed"/>
                  <owl:minCardinality rdf:datatype="http://www.w3.org/2001/XMLSchema#nonNegativeInteger">0</owl:minCardinality>
               </owl:Restriction>
               <owl:Restriction>
                  <owl:onProperty rdf:resource="http://www.opengis.net/gml#bearing"/>
                  <owl:allValuesFrom rdf:resource="http://www.opengis.net/gml#DirectionPropertyType"/>
               </owl:Restriction>
               <owl:Restriction>
                  <owl:onProperty rdf:resource="http://www.opengis.net/gml#bearing"/>
                  <owl:minCardinality rdf:datatype="http://www.w3.org/2001/XMLSchema#nonNegativeInteger">0</owl:minCardinality>
               </owl:Restriction>
               <owl:Restriction>
                  <owl:onProperty rdf:resource="http://www.opengis.net/gml#acceleration"/>
                  <owl:allValuesFrom rdf:resource="http://www.opengis.net/gml#MeasureType"/>
               </owl:Restriction>
               <owl:Restriction>
                  <owl:onProperty rdf:resource="http://www.opengis.net/gml#acceleration"/>
                  <owl:minCardinality rdf:datatype="http://www.w3.org/2001/XMLSchema#nonNegativeInteger">0</owl:minCardinality>
               </owl:Restriction>
               <owl:Restriction>
                  <owl:onProperty rdf:resource="http://www.opengis.net/gml#elevation"/>
                  <owl:allValuesFrom rdf:resource="http://www.opengis.net/gml#MeasureType"/>
               </owl:Restriction>
               <owl:Restriction>
                  <owl:onProperty rdf:resource="http://www.opengis.net/gml#elevation"/>
                  <owl:minCardinality rdf:datatype="http://www.w3.org/2001/XMLSchema#nonNegativeInteger">0</owl:minCardinality>
               </owl:Restriction>
               <owl:Restriction>
                  <owl:onProperty rdf:resource="http://www.opengis.net/gml#hasstatus"/>
                  <owl:allValuesFrom rdf:resource="http://www.opengis.net/gml#status"/>
               </owl:Restriction>
               <owl:Restriction>
                  <owl:onProperty rdf:resource="http://www.opengis.net/gml#hasstatus"/>
                  <owl:minCardinality rdf:datatype="http://www.w3.org/2001/XMLSchema#nonNegativeInteger">0</owl:minCardinality>
               </owl:Restriction>
            </owl:intersectionOf>
         </owl:Class>
      </rdfs:subClassOf>
      <rdfs:subClassOf rdf:resource="http://www.opengis.net/gml#AbstractTimeSliceType"/>
      <rdfs:comment>Warning: The parent class 'gml:AbstractTimeSliceType' is declared outside of this class' original schema. This class may be declared incorrectly.</rdfs:comment>
   </owl:Class>
   <owl:Class rdf:about="http://www.opengis.net/gml#HistoryPropertyType">
      <rdfs:comment xml:lang="en">The history relationship associates a feature with a sequence of TimeSlice instances.</rdfs:comment>
      <rdfs:subClassOf>
         <owl:Class>
            <owl:intersectionOf rdf:parseType="Collection">
               <owl:Restriction>
                  <owl:onProperty rdf:resource="http://www.opengis.net/gml#has_TimeSlice"/>
                  <owl:allValuesFrom rdf:resource="http://www.opengis.net/gml#_TimeSlice"/>
               </owl:Restriction>
            </owl:intersectionOf>
         </owl:Class>
      </rdfs:subClassOf>
   </owl:Class>
   <owl:Class rdf:about="http://www.opengis.net/gml#TrackType">
      <rdfs:comment xml:lang="en">The track of a moving object is a sequence of specialized timeslices        that indicate the status of the object.</rdfs:comment>
      <rdfs:subClassOf>
         <owl:Class>
            <owl:intersectionOf rdf:parseType="Collection">
               <owl:Restriction>
                  <owl:onProperty rdf:resource="http://www.opengis.net/gml#hasMovingObjectStatus"/>
                  <owl:allValuesFrom rdf:resource="http://www.opengis.net/gml#MovingObjectStatus"/>
               </owl:Restriction>
            </owl:intersectionOf>
         </owl:Class>
      </rdfs:subClassOf>
      <rdfs:subClassOf rdf:resource="http://www.opengis.net/gml#HistoryPropertyType"/>
      <rdfs:comment>Warning: The parent class 'gml:HistoryPropertyType' is declared outside of this class' original schema. This class may be declared incorrectly.</rdfs:comment>
   </owl:Class>
   <owl:Class rdf:about="http://www.opengis.net/gml#DynamicFeatureType">
      <rdfs:comment>A dynamic feature may possess a history and/or a timestamp.</rdfs:comment>
      <rdfs:subClassOf rdf:resource="http://www.opengis.net/gml#AbstractFeatureType"/>
      <rdfs:comment>Warning: The parent class 'gml:AbstractFeatureType' is declared outside of this class' original schema. This class may be declared incorrectly.</rdfs:comment>
   </owl:Class>
   <owl:Class rdf:about="http://www.opengis.net/gml#DynamicFeatureCollectionType">
      <rdfs:comment>A dynamic feature collection may possess a history and/or a timestamp.</rdfs:comment>
      <rdfs:subClassOf rdf:resource="http://www.opengis.net/gml#FeatureCollectionType"/>
      <rdfs:comment>Warning: The parent class 'gml:FeatureCollectionType' is declared outside of this class' original schema. This class may be declared incorrectly.</rdfs:comment>
   </owl:Class>
   <owl:Class rdf:about="http://www.opengis.net/gml#dynamicProperties">
      <rdfs:subClassOf>
         <owl:Class>
            <owl:intersectionOf rdf:parseType="Collection"/>
         </owl:Class>
      </rdfs:subClassOf>
      <rdfs:subClassOf>
         <owl:Class>
            <owl:intersectionOf rdf:parseType="Collection">
               <owl:Restriction>
                  <owl:onProperty rdf:resource="http://www.opengis.net/gml#hasvalidTime"/>
                  <owl:allValuesFrom rdf:resource="http://www.opengis.net/gml#validTime"/>
               </owl:Restriction>
               <owl:Restriction>
                  <owl:onProperty rdf:resource="http://www.opengis.net/gml#hasvalidTime"/>
                  <owl:minCardinality rdf:datatype="http://www.w3.org/2001/XMLSchema#nonNegativeInteger">0</owl:minCardinality>
               </owl:Restriction>
               <owl:Restriction>
                  <owl:onProperty rdf:resource="http://www.opengis.net/gml#hashistory"/>
                  <owl:allValuesFrom rdf:resource="http://www.opengis.net/gml#history"/>
               </owl:Restriction>
               <owl:Restriction>
                  <owl:onProperty rdf:resource="http://www.opengis.net/gml#hashistory"/>
                  <owl:minCardinality rdf:datatype="http://www.w3.org/2001/XMLSchema#nonNegativeInteger">0</owl:minCardinality>
               </owl:Restriction>
               <owl:Restriction>
                  <owl:onProperty rdf:resource="http://www.opengis.net/gml#hasdataSource"/>
                  <owl:allValuesFrom rdf:resource="http://www.opengis.net/gml#dataSource"/>
               </owl:Restriction>
               <owl:Restriction>
                  <owl:onProperty rdf:resource="http://www.opengis.net/gml#hasdataSource"/>
                  <owl:minCardinality rdf:datatype="http://www.w3.org/2001/XMLSchema#nonNegativeInteger">0</owl:minCardinality>
               </owl:Restriction>
            </owl:intersectionOf>
         </owl:Class>
      </rdfs:subClassOf>
   </owl:Class>
   <owl:ObjectProperty rdf:about="http://www.opengis.net/gml#hasdynamicProperties">
      <rdfs:domain rdf:resource="http://www.opengis.net/gml#DynamicFeatureType"/>
      <rdfs:range rdf:resource="http://www.opengis.net/gml#dynamicProperties"/>
   </owl:ObjectProperty>
   <owl:ObjectProperty rdf:about="http://www.opengis.net/gml#hasdynamicProperties">
      <rdfs:domain rdf:resource="http://www.opengis.net/gml#DynamicFeatureCollectionType"/>
      <rdfs:range rdf:resource="http://www.opengis.net/gml#dynamicProperties"/>
   </owl:ObjectProperty>
   <owl:Class rdf:about="http://www.opengis.net/gml#dataSource">
      <rdfs:subClassOf rdf:resource="http://www.opengis.net/gml#StringOrRefType"/>
      <rdfs:comment>Warning: This class type was declared outside of its original schema. This class may be declared incorrectly.</rdfs:comment>
   </owl:Class>
   <owl:Class rdf:about="http://www.opengis.net/gml#status">
      <rdfs:subClassOf rdf:resource="http://www.opengis.net/gml#StringOrRefType"/>
      <rdfs:comment>Warning: This class type was declared outside of its original schema. This class may be declared incorrectly.</rdfs:comment>
   </owl:Class>
   <owl:Class rdf:about="http://www.opengis.net/gml#_TimeSlice">
      <rdfs:subClassOf rdf:resource="http://www.opengis.net/gml#_GML"/>
      <rdfs:subClassOf rdf:resource="http://www.opengis.net/gml#AbstractTimeSliceType"/>
      <rdfs:comment>Warning: This class type was declared outside of its original schema. This class may be declared incorrectly.</rdfs:comment>
   </owl:Class>
   <owl:Class rdf:about="http://www.opengis.net/gml#MovingObjectStatus">
      <rdfs:subClassOf rdf:resource="http://www.opengis.net/gml#_TimeSlice"/>
      <rdfs:subClassOf rdf:resource="http://www.opengis.net/gml#MovingObjectStatusType"/>
      <rdfs:comment>Warning: This class type was declared outside of its original schema. This class may be declared incorrectly.</rdfs:comment>
   </owl:Class>
   <owl:Class rdf:about="http://www.opengis.net/gml#history">
      <rdfs:subClassOf rdf:resource="http://www.opengis.net/gml#HistoryPropertyType"/>
      <rdfs:comment>Warning: This class type was declared outside of its original schema. This class may be declared incorrectly.</rdfs:comment>
   </owl:Class>
   <owl:Class rdf:about="http://www.opengis.net/gml#track">
      <rdfs:subClassOf rdf:resource="http://www.opengis.net/gml#history"/>
      <rdfs:subClassOf rdf:resource="http://www.opengis.net/gml#TrackType"/>
      <rdfs:comment>Warning: This class type was declared outside of its original schema. This class may be declared incorrectly.</rdfs:comment>
   </owl:Class>
   <owl:ObjectProperty rdf:about="http://www.opengis.net/gml#hasvalidTime">
      <rdfs:comment>Warning: This ObjectProperty reference was declared outside of its original schema. This ObjectProperty may be declared incorrectly.</rdfs:comment>
      <rdfs:domain rdf:resource="http://www.opengis.net/gml#AbstractTimeSliceType"/>
      <rdfs:range rdf:resource="http://www.opengis.net/gml#validTime"/>
   </owl:ObjectProperty>
   <owl:ObjectProperty rdf:about="http://www.opengis.net/gml#hasdataSource">
      <rdfs:comment>Warning: This ObjectProperty reference was declared outside of its original schema. This ObjectProperty may be declared incorrectly.</rdfs:comment>
      <rdfs:domain rdf:resource="http://www.opengis.net/gml#AbstractTimeSliceType"/>
      <rdfs:range rdf:resource="http://www.opengis.net/gml#dataSource"/>
   </owl:ObjectProperty>
   <owl:ObjectProperty rdf:about="http://www.opengis.net/gml#haslocation">
      <rdfs:comment>Warning: This ObjectProperty reference was declared outside of its original schema. This ObjectProperty may be declared incorrectly.</rdfs:comment>
      <rdfs:domain rdf:resource="http://www.opengis.net/gml#MovingObjectStatusType"/>
      <rdfs:range rdf:resource="http://www.opengis.net/gml#location"/>
   </owl:ObjectProperty>
   <owl:ObjectProperty rdf:about="http://www.opengis.net/gml#speed">
      <rdfs:comment>Warning: This ObjectProperty type was declared outside of its original schema. This ObjectProperty may be declared incorrectly.</rdfs:comment>
      <rdfs:domain rdf:resource="http://www.opengis.net/gml#MovingObjectStatusType"/>
      <rdfs:range rdf:resource="http://www.opengis.net/gml#MeasureType"/>
   </owl:ObjectProperty>
   <owl:ObjectProperty rdf:about="http://www.opengis.net/gml#bearing">
      <rdfs:comment>Warning: This ObjectProperty type was declared outside of its original schema. This ObjectProperty may be declared incorrectly.</rdfs:comment>
      <rdfs:domain rdf:resource="http://www.opengis.net/gml#MovingObjectStatusType"/>
      <rdfs:range rdf:resource="http://www.opengis.net/gml#DirectionPropertyType"/>
   </owl:ObjectProperty>
   <owl:ObjectProperty rdf:about="http://www.opengis.net/gml#acceleration">
      <rdfs:comment>Warning: This ObjectProperty type was declared outside of its original schema. This ObjectProperty may be declared incorrectly.</rdfs:comment>
      <rdfs:domain rdf:resource="http://www.opengis.net/gml#MovingObjectStatusType"/>
      <rdfs:range rdf:resource="http://www.opengis.net/gml#MeasureType"/>
   </owl:ObjectProperty>
   <owl:ObjectProperty rdf:about="http://www.opengis.net/gml#elevation">
      <rdfs:comment>Warning: This ObjectProperty type was declared outside of its original schema. This ObjectProperty may be declared incorrectly.</rdfs:comment>
      <rdfs:domain rdf:resource="http://www.opengis.net/gml#MovingObjectStatusType"/>
      <rdfs:range rdf:resource="http://www.opengis.net/gml#MeasureType"/>
   </owl:ObjectProperty>
   <owl:ObjectProperty rdf:about="http://www.opengis.net/gml#hasstatus">
      <rdfs:comment>Warning: This ObjectProperty reference was declared outside of its original schema. This ObjectProperty may be declared incorrectly.</rdfs:comment>
      <rdfs:domain rdf:resource="http://www.opengis.net/gml#MovingObjectStatusType"/>
      <rdfs:range rdf:resource="http://www.opengis.net/gml#status"/>
   </owl:ObjectProperty>
   <owl:ObjectProperty rdf:about="http://www.opengis.net/gml#has_TimeSlice">
      <rdfs:comment>Warning: This ObjectProperty reference was declared outside of its original schema. This ObjectProperty may be declared incorrectly.</rdfs:comment>
      <rdfs:domain rdf:resource="http://www.opengis.net/gml#HistoryPropertyType"/>
      <rdfs:range rdf:resource="http://www.opengis.net/gml#_TimeSlice"/>
   </owl:ObjectProperty>
   <owl:ObjectProperty rdf:about="http://www.opengis.net/gml#hasMovingObjectStatus">
      <rdfs:comment>Warning: This ObjectProperty reference was declared outside of its original schema. This ObjectProperty may be declared incorrectly.</rdfs:comment>
      <rdfs:domain rdf:resource="http://www.opengis.net/gml#TrackType"/>
      <rdfs:range rdf:resource="http://www.opengis.net/gml#MovingObjectStatus"/>
   </owl:ObjectProperty>
   <owl:ObjectProperty rdf:about="http://www.opengis.net/gml#hasvalidTime">
      <rdfs:comment>Warning: This ObjectProperty reference was declared outside of its original schema. This ObjectProperty may be declared incorrectly.</rdfs:comment>
      <rdfs:domain rdf:resource="http://www.opengis.net/gml#dynamicProperties"/>
      <rdfs:range rdf:resource="http://www.opengis.net/gml#validTime"/>
   </owl:ObjectProperty>
   <owl:ObjectProperty rdf:about="http://www.opengis.net/gml#hashistory">
      <rdfs:comment>Warning: This ObjectProperty reference was declared outside of its original schema. This ObjectProperty may be declared incorrectly.</rdfs:comment>
      <rdfs:domain rdf:resource="http://www.opengis.net/gml#dynamicProperties"/>
      <rdfs:range rdf:resource="http://www.opengis.net/gml#history"/>
   </owl:ObjectProperty>
   <owl:ObjectProperty rdf:about="http://www.opengis.net/gml#hasdataSource">
      <rdfs:comment>Warning: This ObjectProperty reference was declared outside of its original schema. This ObjectProperty may be declared incorrectly.</rdfs:comment>
      <rdfs:domain rdf:resource="http://www.opengis.net/gml#dynamicProperties"/>
      <rdfs:range rdf:resource="http://www.opengis.net/gml#dataSource"/>
   </owl:ObjectProperty>
</rdf:RDF>
