<?xml version="1.0"?>
<rdf:RDF xmlns="http://liris.cnrs.fr/ontologies/generics#"
     xml:base="http://liris.cnrs.fr/ontologies/generics"
     xmlns:owl="http://www.w3.org/2002/07/owl#"
     xmlns:rdf="http://www.w3.org/1999/02/22-rdf-syntax-ns#"
     xmlns:www="http://www.w3.org/2001/"
     xmlns:xml="http://www.w3.org/XML/1998/namespace"
     xmlns:xsd="http://www.w3.org/2001/XMLSchema#"
     xmlns:math="http://www.w3.org/2005/xpath-functions/math"
     xmlns:rdfs="http://www.w3.org/2000/01/rdf-schema#">
    <owl:Ontology rdf:about="http://liris.cnrs.fr/ontologies/generics">
        <owl:imports rdf:resource="http://liris.cnrs.fr/ontologies/cityGMLBase"/>
        <rdfs:comment>
	CityGML is an OGC Standard.
	Copyright (c) 2012 Open Geospatial Consortium.
	To obtain additional rights of use, visit http://www.opengeospatial.org/legal/ .
		</rdfs:comment>
        <rdfs:comment>Warning: The schema http://www.opengis.net/citygml/2.0 was not imported.</rdfs:comment>
        <rdfs:comment>Warning: The schema http://www.opengis.net/gml was not imported.</rdfs:comment>
    </owl:Ontology>
    


    <!-- 
    ///////////////////////////////////////////////////////////////////////////////////////
    //
    // Datatypes
    //
    ///////////////////////////////////////////////////////////////////////////////////////
     -->

    


    <!-- http://www.opengis.net/gml#MeasureType -->

    <rdfs:Datatype rdf:about="http://www.opengis.net/gml#MeasureType"/>
    


    <!-- 
    ///////////////////////////////////////////////////////////////////////////////////////
    //
    // Object Properties
    //
    ///////////////////////////////////////////////////////////////////////////////////////
     -->

    


    <!-- http://www.opengis.net/citygml/generics/2.0#class -->

    <owl:ObjectProperty rdf:about="http://www.opengis.net/citygml/generics/2.0#class">
        <rdfs:domain rdf:resource="http://www.opengis.net/citygml/generics/2.0#GenericCityObjectType"/>
        <rdfs:range rdf:resource="http://www.opengis.net/gml#CodeType"/>
        <rdfs:comment>Warning: This ObjectProperty type was declared outside of its original schema. This ObjectProperty may be declared incorrectly.</rdfs:comment>
    </owl:ObjectProperty>
    


    <!-- http://www.opengis.net/citygml/generics/2.0#function -->

    <owl:ObjectProperty rdf:about="http://www.opengis.net/citygml/generics/2.0#function">
        <rdfs:domain rdf:resource="http://www.opengis.net/citygml/generics/2.0#GenericCityObjectType"/>
        <rdfs:range rdf:resource="http://www.opengis.net/gml#CodeType"/>
        <rdfs:comment>Warning: This ObjectProperty type was declared outside of its original schema. This ObjectProperty may be declared incorrectly.</rdfs:comment>
    </owl:ObjectProperty>
    


    <!-- http://www.opengis.net/citygml/generics/2.0#has_genericAttribute -->

    <owl:ObjectProperty rdf:about="http://www.opengis.net/citygml/generics/2.0#has_genericAttribute">
        <rdfs:domain rdf:resource="http://www.opengis.net/citygml/generics/2.0#GenericAttributeSetType"/>
        <rdfs:range rdf:resource="http://www.opengis.net/citygml/generics/2.0#_genericAttribute"/>
    </owl:ObjectProperty>
    


    <!-- http://www.opengis.net/citygml/generics/2.0#lod0Geometry -->

    <owl:ObjectProperty rdf:about="http://www.opengis.net/citygml/generics/2.0#lod0Geometry">
        <rdfs:domain rdf:resource="http://www.opengis.net/citygml/generics/2.0#GenericCityObjectType"/>
        <rdfs:range rdf:resource="http://www.opengis.net/gml#GeometryPropertyType"/>
        <rdfs:comment>Warning: This ObjectProperty type was declared outside of its original schema. This ObjectProperty may be declared incorrectly.</rdfs:comment>
    </owl:ObjectProperty>
    


    <!-- http://www.opengis.net/citygml/generics/2.0#lod0ImplicitRepresentation -->

    <owl:ObjectProperty rdf:about="http://www.opengis.net/citygml/generics/2.0#lod0ImplicitRepresentation">
        <rdfs:domain rdf:resource="http://www.opengis.net/citygml/generics/2.0#GenericCityObjectType"/>
        <rdfs:range rdf:resource="http://www.opengis.net/citygml/2.0#ImplicitRepresentationPropertyType"/>
        <rdfs:comment>Warning: This ObjectProperty type was declared outside of its original schema. This ObjectProperty may be declared incorrectly.</rdfs:comment>
    </owl:ObjectProperty>
    


    <!-- http://www.opengis.net/citygml/generics/2.0#lod0TerrainIntersection -->

    <owl:ObjectProperty rdf:about="http://www.opengis.net/citygml/generics/2.0#lod0TerrainIntersection">
        <rdfs:domain rdf:resource="http://www.opengis.net/citygml/generics/2.0#GenericCityObjectType"/>
        <rdfs:range rdf:resource="http://www.opengis.net/gml#MultiCurvePropertyType"/>
        <rdfs:comment>Warning: This ObjectProperty type was declared outside of its original schema. This ObjectProperty may be declared incorrectly.</rdfs:comment>
    </owl:ObjectProperty>
    


    <!-- http://www.opengis.net/citygml/generics/2.0#lod1Geometry -->

    <owl:ObjectProperty rdf:about="http://www.opengis.net/citygml/generics/2.0#lod1Geometry">
        <rdfs:domain rdf:resource="http://www.opengis.net/citygml/generics/2.0#GenericCityObjectType"/>
        <rdfs:range rdf:resource="http://www.opengis.net/gml#GeometryPropertyType"/>
        <rdfs:comment>Warning: This ObjectProperty type was declared outside of its original schema. This ObjectProperty may be declared incorrectly.</rdfs:comment>
    </owl:ObjectProperty>
    


    <!-- http://www.opengis.net/citygml/generics/2.0#lod1ImplicitRepresentation -->

    <owl:ObjectProperty rdf:about="http://www.opengis.net/citygml/generics/2.0#lod1ImplicitRepresentation">
        <rdfs:domain rdf:resource="http://www.opengis.net/citygml/generics/2.0#GenericCityObjectType"/>
        <rdfs:range rdf:resource="http://www.opengis.net/citygml/2.0#ImplicitRepresentationPropertyType"/>
        <rdfs:comment>Warning: This ObjectProperty type was declared outside of its original schema. This ObjectProperty may be declared incorrectly.</rdfs:comment>
    </owl:ObjectProperty>
    


    <!-- http://www.opengis.net/citygml/generics/2.0#lod1TerrainIntersection -->

    <owl:ObjectProperty rdf:about="http://www.opengis.net/citygml/generics/2.0#lod1TerrainIntersection">
        <rdfs:domain rdf:resource="http://www.opengis.net/citygml/generics/2.0#GenericCityObjectType"/>
        <rdfs:range rdf:resource="http://www.opengis.net/gml#MultiCurvePropertyType"/>
        <rdfs:comment>Warning: This ObjectProperty type was declared outside of its original schema. This ObjectProperty may be declared incorrectly.</rdfs:comment>
    </owl:ObjectProperty>
    


    <!-- http://www.opengis.net/citygml/generics/2.0#lod2Geometry -->

    <owl:ObjectProperty rdf:about="http://www.opengis.net/citygml/generics/2.0#lod2Geometry">
        <rdfs:domain rdf:resource="http://www.opengis.net/citygml/generics/2.0#GenericCityObjectType"/>
        <rdfs:range rdf:resource="http://www.opengis.net/gml#GeometryPropertyType"/>
        <rdfs:comment>Warning: This ObjectProperty type was declared outside of its original schema. This ObjectProperty may be declared incorrectly.</rdfs:comment>
    </owl:ObjectProperty>
    


    <!-- http://www.opengis.net/citygml/generics/2.0#lod2ImplicitRepresentation -->

    <owl:ObjectProperty rdf:about="http://www.opengis.net/citygml/generics/2.0#lod2ImplicitRepresentation">
        <rdfs:domain rdf:resource="http://www.opengis.net/citygml/generics/2.0#GenericCityObjectType"/>
        <rdfs:range rdf:resource="http://www.opengis.net/citygml/2.0#ImplicitRepresentationPropertyType"/>
        <rdfs:comment>Warning: This ObjectProperty type was declared outside of its original schema. This ObjectProperty may be declared incorrectly.</rdfs:comment>
    </owl:ObjectProperty>
    


    <!-- http://www.opengis.net/citygml/generics/2.0#lod2TerrainIntersection -->

    <owl:ObjectProperty rdf:about="http://www.opengis.net/citygml/generics/2.0#lod2TerrainIntersection">
        <rdfs:domain rdf:resource="http://www.opengis.net/citygml/generics/2.0#GenericCityObjectType"/>
        <rdfs:range rdf:resource="http://www.opengis.net/gml#MultiCurvePropertyType"/>
        <rdfs:comment>Warning: This ObjectProperty type was declared outside of its original schema. This ObjectProperty may be declared incorrectly.</rdfs:comment>
    </owl:ObjectProperty>
    


    <!-- http://www.opengis.net/citygml/generics/2.0#lod3Geometry -->

    <owl:ObjectProperty rdf:about="http://www.opengis.net/citygml/generics/2.0#lod3Geometry">
        <rdfs:domain rdf:resource="http://www.opengis.net/citygml/generics/2.0#GenericCityObjectType"/>
        <rdfs:range rdf:resource="http://www.opengis.net/gml#GeometryPropertyType"/>
        <rdfs:comment>Warning: This ObjectProperty type was declared outside of its original schema. This ObjectProperty may be declared incorrectly.</rdfs:comment>
    </owl:ObjectProperty>
    


    <!-- http://www.opengis.net/citygml/generics/2.0#lod3ImplicitRepresentation -->

    <owl:ObjectProperty rdf:about="http://www.opengis.net/citygml/generics/2.0#lod3ImplicitRepresentation">
        <rdfs:domain rdf:resource="http://www.opengis.net/citygml/generics/2.0#GenericCityObjectType"/>
        <rdfs:range rdf:resource="http://www.opengis.net/citygml/2.0#ImplicitRepresentationPropertyType"/>
        <rdfs:comment>Warning: This ObjectProperty type was declared outside of its original schema. This ObjectProperty may be declared incorrectly.</rdfs:comment>
    </owl:ObjectProperty>
    


    <!-- http://www.opengis.net/citygml/generics/2.0#lod3TerrainIntersection -->

    <owl:ObjectProperty rdf:about="http://www.opengis.net/citygml/generics/2.0#lod3TerrainIntersection">
        <rdfs:domain rdf:resource="http://www.opengis.net/citygml/generics/2.0#GenericCityObjectType"/>
        <rdfs:range rdf:resource="http://www.opengis.net/gml#MultiCurvePropertyType"/>
        <rdfs:comment>Warning: This ObjectProperty type was declared outside of its original schema. This ObjectProperty may be declared incorrectly.</rdfs:comment>
    </owl:ObjectProperty>
    


    <!-- http://www.opengis.net/citygml/generics/2.0#lod4Geometry -->

    <owl:ObjectProperty rdf:about="http://www.opengis.net/citygml/generics/2.0#lod4Geometry">
        <rdfs:domain rdf:resource="http://www.opengis.net/citygml/generics/2.0#GenericCityObjectType"/>
        <rdfs:range rdf:resource="http://www.opengis.net/gml#GeometryPropertyType"/>
        <rdfs:comment>Warning: This ObjectProperty type was declared outside of its original schema. This ObjectProperty may be declared incorrectly.</rdfs:comment>
    </owl:ObjectProperty>
    


    <!-- http://www.opengis.net/citygml/generics/2.0#lod4ImplicitRepresentation -->

    <owl:ObjectProperty rdf:about="http://www.opengis.net/citygml/generics/2.0#lod4ImplicitRepresentation">
        <rdfs:domain rdf:resource="http://www.opengis.net/citygml/generics/2.0#GenericCityObjectType"/>
        <rdfs:range rdf:resource="http://www.opengis.net/citygml/2.0#ImplicitRepresentationPropertyType"/>
        <rdfs:comment>Warning: This ObjectProperty type was declared outside of its original schema. This ObjectProperty may be declared incorrectly.</rdfs:comment>
    </owl:ObjectProperty>
    


    <!-- http://www.opengis.net/citygml/generics/2.0#lod4TerrainIntersection -->

    <owl:ObjectProperty rdf:about="http://www.opengis.net/citygml/generics/2.0#lod4TerrainIntersection">
        <rdfs:domain rdf:resource="http://www.opengis.net/citygml/generics/2.0#GenericCityObjectType"/>
        <rdfs:range rdf:resource="http://www.opengis.net/gml#MultiCurvePropertyType"/>
        <rdfs:comment>Warning: This ObjectProperty type was declared outside of its original schema. This ObjectProperty may be declared incorrectly.</rdfs:comment>
    </owl:ObjectProperty>
    


    <!-- http://www.opengis.net/citygml/generics/2.0#usage -->

    <owl:ObjectProperty rdf:about="http://www.opengis.net/citygml/generics/2.0#usage">
        <rdfs:domain rdf:resource="http://www.opengis.net/citygml/generics/2.0#GenericCityObjectType"/>
        <rdfs:range rdf:resource="http://www.opengis.net/gml#CodeType"/>
        <rdfs:comment>Warning: This ObjectProperty type was declared outside of its original schema. This ObjectProperty may be declared incorrectly.</rdfs:comment>
    </owl:ObjectProperty>
    


    <!-- http://www.opengis.net/citygml/generics/2.0#value -->

    <owl:ObjectProperty rdf:about="http://www.opengis.net/citygml/generics/2.0#value">
        <rdfs:domain rdf:resource="http://www.opengis.net/citygml/generics/2.0#DateAttributeType"/>
        <rdfs:domain rdf:resource="http://www.opengis.net/citygml/generics/2.0#DoubleAttributeType"/>
        <rdfs:domain rdf:resource="http://www.opengis.net/citygml/generics/2.0#IntAttributeType"/>
        <rdfs:domain rdf:resource="http://www.opengis.net/citygml/generics/2.0#MeasureAttributeType"/>
        <rdfs:domain rdf:resource="http://www.opengis.net/citygml/generics/2.0#StringAttributeType"/>
        <rdfs:domain rdf:resource="http://www.opengis.net/citygml/generics/2.0#UriAttributeType"/>
    </owl:ObjectProperty>
    


    <!-- 
    ///////////////////////////////////////////////////////////////////////////////////////
    //
    // Data properties
    //
    ///////////////////////////////////////////////////////////////////////////////////////
     -->

    


    <!-- http://www.opengis.net/citygml/generics/2.0#codeSpace -->

    <owl:DatatypeProperty rdf:about="http://www.opengis.net/citygml/generics/2.0#codeSpace">
        <rdfs:domain rdf:resource="http://www.opengis.net/citygml/generics/2.0#GenericAttributeSetType"/>
        <rdfs:range rdf:resource="http://www.w3.org/2001/XMLSchema#anyURI"/>
    </owl:DatatypeProperty>
    


    <!-- http://www.opengis.net/citygml/generics/2.0#name -->

    <owl:DatatypeProperty rdf:about="http://www.opengis.net/citygml/generics/2.0#name">
        <rdfs:domain rdf:resource="http://www.opengis.net/citygml/generics/2.0#AbstractGenericAttributeType"/>
        <rdfs:range rdf:resource="http://www.w3.org/2001/XMLSchema#string"/>
    </owl:DatatypeProperty>
    


    <!-- http://www.opengis.net/citygml/generics/2.0#value -->

    <owl:DatatypeProperty rdf:about="http://www.opengis.net/citygml/generics/2.0#value">
        <rdfs:range rdf:resource="http://www.opengis.net/gml#MeasureType"/>
        <rdfs:range rdf:resource="http://www.w3.org/2001/XMLSchema#anyURI"/>
        <rdfs:range rdf:resource="http://www.w3.org/2001/XMLSchema#date"/>
        <rdfs:range rdf:resource="http://www.w3.org/2001/XMLSchema#double"/>
        <rdfs:range rdf:resource="http://www.w3.org/2001/XMLSchema#integer"/>
        <rdfs:range rdf:resource="http://www.w3.org/2001/XMLSchema#string"/>
    </owl:DatatypeProperty>
    


    <!-- 
    ///////////////////////////////////////////////////////////////////////////////////////
    //
    // Classes
    //
    ///////////////////////////////////////////////////////////////////////////////////////
     -->

    


    <!-- http://www.opengis.net/citygml/generics/2.0#AbstractGenericAttributeType -->

    <owl:Class rdf:about="http://www.opengis.net/citygml/generics/2.0#AbstractGenericAttributeType">
        <owl:equivalentClass>
            <owl:Class>
                <owl:intersectionOf rdf:resource="http://www.w3.org/1999/02/22-rdf-syntax-ns#nil"/>
            </owl:Class>
        </owl:equivalentClass>
        <owl:equivalentClass>
            <owl:Class>
                <owl:intersectionOf rdf:parseType="Collection">
                    <owl:Restriction>
                        <owl:onProperty rdf:resource="http://www.opengis.net/citygml/generics/2.0#name"/>
                        <owl:allValuesFrom rdf:resource="http://www.w3.org/2001/XMLSchema#string"/>
                    </owl:Restriction>
                </owl:intersectionOf>
            </owl:Class>
        </owl:equivalentClass>
        <rdfs:comment> Generic (user defined) attributes may be used to represent attributes which are not covered explicitly by
				the CityGML schema. Generic attributes must be used with care; they shall only be used if there is no appropiate attribute
				available in the overall CityGML schema. Oherwise, problems concerning semantic interoperability may arise. A generic
				attribute has a name and a value, which has further subclasses (IntAttrribute, StringAttribute, ...). </rdfs:comment>
        <rdfs:comment>This is an abstract class</rdfs:comment>
    </owl:Class>
    


    <!-- http://www.opengis.net/citygml/generics/2.0#DateAttributeType -->

    <owl:Class rdf:about="http://www.opengis.net/citygml/generics/2.0#DateAttributeType">
        <owl:equivalentClass>
            <owl:Class>
                <owl:intersectionOf rdf:parseType="Collection">
                    <owl:Restriction>
                        <owl:onProperty rdf:resource="http://www.opengis.net/citygml/generics/2.0#value"/>
                        <owl:allValuesFrom rdf:resource="http://www.w3.org/2001/XMLSchema#date"/>
                    </owl:Restriction>
                </owl:intersectionOf>
            </owl:Class>
        </owl:equivalentClass>
        <rdfs:comment></rdfs:comment>
    </owl:Class>
    


    <!-- http://www.opengis.net/citygml/generics/2.0#DoubleAttributeType -->

    <owl:Class rdf:about="http://www.opengis.net/citygml/generics/2.0#DoubleAttributeType">
        <owl:equivalentClass>
            <owl:Class>
                <owl:intersectionOf rdf:parseType="Collection">
                    <owl:Restriction>
                        <owl:onProperty rdf:resource="http://www.opengis.net/citygml/generics/2.0#value"/>
                        <owl:allValuesFrom rdf:resource="http://www.w3.org/2001/XMLSchema#double"/>
                    </owl:Restriction>
                </owl:intersectionOf>
            </owl:Class>
        </owl:equivalentClass>
        <rdfs:comment></rdfs:comment>
    </owl:Class>
    


    <!-- http://www.opengis.net/citygml/generics/2.0#GenericAttributeSetType -->

    <owl:Class rdf:about="http://www.opengis.net/citygml/generics/2.0#GenericAttributeSetType">
        <owl:equivalentClass>
            <owl:Class>
                <owl:intersectionOf rdf:parseType="Collection">
                    <owl:Restriction>
                        <owl:onProperty rdf:resource="http://www.opengis.net/citygml/generics/2.0#has_genericAttribute"/>
                        <owl:allValuesFrom rdf:resource="http://www.opengis.net/citygml/generics/2.0#_genericAttribute"/>
                    </owl:Restriction>
                    <owl:Restriction>
                        <owl:onProperty rdf:resource="http://www.opengis.net/citygml/generics/2.0#has_genericAttribute"/>
                        <owl:minCardinality rdf:datatype="http://www.w3.org/2001/XMLSchema#nonNegativeInteger">1</owl:minCardinality>
                    </owl:Restriction>
                </owl:intersectionOf>
            </owl:Class>
        </owl:equivalentClass>
        <owl:equivalentClass>
            <owl:Class>
                <owl:intersectionOf rdf:parseType="Collection">
                    <owl:Restriction>
                        <owl:onProperty rdf:resource="http://www.opengis.net/citygml/generics/2.0#codeSpace"/>
                        <owl:allValuesFrom rdf:resource="http://www.w3.org/2001/XMLSchema#anyURI"/>
                    </owl:Restriction>
                </owl:intersectionOf>
            </owl:Class>
        </owl:equivalentClass>
        <rdfs:comment>Set of generic attributes with an optional codeSpace. If the codeSpace attribute is present, then its
				value should identify an authority for the set, such as the organisation or community who defined its content. The generic
				attribute set may contain arbitrary generic attributes.</rdfs:comment>
    </owl:Class>
    


    <!-- http://www.opengis.net/citygml/generics/2.0#GenericCityObject -->

    <owl:Class rdf:about="http://www.opengis.net/citygml/generics/2.0#GenericCityObject">
        <rdfs:subClassOf rdf:resource="http://www.opengis.net/citygml/2.0#_CityObject"/>
        <rdfs:subClassOf rdf:resource="http://www.opengis.net/citygml/generics/2.0#GenericCityObjectType"/>
    </owl:Class>
    


    <!-- http://www.opengis.net/citygml/generics/2.0#GenericCityObjectType -->

    <owl:Class rdf:about="http://www.opengis.net/citygml/generics/2.0#GenericCityObjectType">
        <owl:equivalentClass>
            <owl:Class>
                <owl:intersectionOf rdf:parseType="Collection">
                    <owl:Restriction>
                        <owl:onProperty rdf:resource="http://www.opengis.net/citygml/generics/2.0#class"/>
                        <owl:allValuesFrom rdf:resource="http://www.opengis.net/gml#CodeType"/>
                    </owl:Restriction>
                    <owl:Restriction>
                        <owl:onProperty rdf:resource="http://www.opengis.net/citygml/generics/2.0#function"/>
                        <owl:allValuesFrom rdf:resource="http://www.opengis.net/gml#CodeType"/>
                    </owl:Restriction>
                    <owl:Restriction>
                        <owl:onProperty rdf:resource="http://www.opengis.net/citygml/generics/2.0#lod0Geometry"/>
                        <owl:allValuesFrom rdf:resource="http://www.opengis.net/gml#GeometryPropertyType"/>
                    </owl:Restriction>
                    <owl:Restriction>
                        <owl:onProperty rdf:resource="http://www.opengis.net/citygml/generics/2.0#lod0ImplicitRepresentation"/>
                        <owl:allValuesFrom rdf:resource="http://www.opengis.net/citygml/2.0#ImplicitRepresentationPropertyType"/>
                    </owl:Restriction>
                    <owl:Restriction>
                        <owl:onProperty rdf:resource="http://www.opengis.net/citygml/generics/2.0#lod0TerrainIntersection"/>
                        <owl:allValuesFrom rdf:resource="http://www.opengis.net/gml#MultiCurvePropertyType"/>
                    </owl:Restriction>
                    <owl:Restriction>
                        <owl:onProperty rdf:resource="http://www.opengis.net/citygml/generics/2.0#lod1Geometry"/>
                        <owl:allValuesFrom rdf:resource="http://www.opengis.net/gml#GeometryPropertyType"/>
                    </owl:Restriction>
                    <owl:Restriction>
                        <owl:onProperty rdf:resource="http://www.opengis.net/citygml/generics/2.0#lod1ImplicitRepresentation"/>
                        <owl:allValuesFrom rdf:resource="http://www.opengis.net/citygml/2.0#ImplicitRepresentationPropertyType"/>
                    </owl:Restriction>
                    <owl:Restriction>
                        <owl:onProperty rdf:resource="http://www.opengis.net/citygml/generics/2.0#lod1TerrainIntersection"/>
                        <owl:allValuesFrom rdf:resource="http://www.opengis.net/gml#MultiCurvePropertyType"/>
                    </owl:Restriction>
                    <owl:Restriction>
                        <owl:onProperty rdf:resource="http://www.opengis.net/citygml/generics/2.0#lod2Geometry"/>
                        <owl:allValuesFrom rdf:resource="http://www.opengis.net/gml#GeometryPropertyType"/>
                    </owl:Restriction>
                    <owl:Restriction>
                        <owl:onProperty rdf:resource="http://www.opengis.net/citygml/generics/2.0#lod2ImplicitRepresentation"/>
                        <owl:allValuesFrom rdf:resource="http://www.opengis.net/citygml/2.0#ImplicitRepresentationPropertyType"/>
                    </owl:Restriction>
                    <owl:Restriction>
                        <owl:onProperty rdf:resource="http://www.opengis.net/citygml/generics/2.0#lod2TerrainIntersection"/>
                        <owl:allValuesFrom rdf:resource="http://www.opengis.net/gml#MultiCurvePropertyType"/>
                    </owl:Restriction>
                    <owl:Restriction>
                        <owl:onProperty rdf:resource="http://www.opengis.net/citygml/generics/2.0#lod3Geometry"/>
                        <owl:allValuesFrom rdf:resource="http://www.opengis.net/gml#GeometryPropertyType"/>
                    </owl:Restriction>
                    <owl:Restriction>
                        <owl:onProperty rdf:resource="http://www.opengis.net/citygml/generics/2.0#lod3ImplicitRepresentation"/>
                        <owl:allValuesFrom rdf:resource="http://www.opengis.net/citygml/2.0#ImplicitRepresentationPropertyType"/>
                    </owl:Restriction>
                    <owl:Restriction>
                        <owl:onProperty rdf:resource="http://www.opengis.net/citygml/generics/2.0#lod3TerrainIntersection"/>
                        <owl:allValuesFrom rdf:resource="http://www.opengis.net/gml#MultiCurvePropertyType"/>
                    </owl:Restriction>
                    <owl:Restriction>
                        <owl:onProperty rdf:resource="http://www.opengis.net/citygml/generics/2.0#lod4Geometry"/>
                        <owl:allValuesFrom rdf:resource="http://www.opengis.net/gml#GeometryPropertyType"/>
                    </owl:Restriction>
                    <owl:Restriction>
                        <owl:onProperty rdf:resource="http://www.opengis.net/citygml/generics/2.0#lod4ImplicitRepresentation"/>
                        <owl:allValuesFrom rdf:resource="http://www.opengis.net/citygml/2.0#ImplicitRepresentationPropertyType"/>
                    </owl:Restriction>
                    <owl:Restriction>
                        <owl:onProperty rdf:resource="http://www.opengis.net/citygml/generics/2.0#lod4TerrainIntersection"/>
                        <owl:allValuesFrom rdf:resource="http://www.opengis.net/gml#MultiCurvePropertyType"/>
                    </owl:Restriction>
                    <owl:Restriction>
                        <owl:onProperty rdf:resource="http://www.opengis.net/citygml/generics/2.0#usage"/>
                        <owl:allValuesFrom rdf:resource="http://www.opengis.net/gml#CodeType"/>
                    </owl:Restriction>
                    <owl:Restriction>
                        <owl:onProperty rdf:resource="http://www.opengis.net/citygml/generics/2.0#class"/>
                        <owl:minCardinality rdf:datatype="http://www.w3.org/2001/XMLSchema#nonNegativeInteger">0</owl:minCardinality>
                    </owl:Restriction>
                    <owl:Restriction>
                        <owl:onProperty rdf:resource="http://www.opengis.net/citygml/generics/2.0#function"/>
                        <owl:minCardinality rdf:datatype="http://www.w3.org/2001/XMLSchema#nonNegativeInteger">0</owl:minCardinality>
                    </owl:Restriction>
                    <owl:Restriction>
                        <owl:onProperty rdf:resource="http://www.opengis.net/citygml/generics/2.0#lod0Geometry"/>
                        <owl:minCardinality rdf:datatype="http://www.w3.org/2001/XMLSchema#nonNegativeInteger">0</owl:minCardinality>
                    </owl:Restriction>
                    <owl:Restriction>
                        <owl:onProperty rdf:resource="http://www.opengis.net/citygml/generics/2.0#lod0ImplicitRepresentation"/>
                        <owl:minCardinality rdf:datatype="http://www.w3.org/2001/XMLSchema#nonNegativeInteger">0</owl:minCardinality>
                    </owl:Restriction>
                    <owl:Restriction>
                        <owl:onProperty rdf:resource="http://www.opengis.net/citygml/generics/2.0#lod0TerrainIntersection"/>
                        <owl:minCardinality rdf:datatype="http://www.w3.org/2001/XMLSchema#nonNegativeInteger">0</owl:minCardinality>
                    </owl:Restriction>
                    <owl:Restriction>
                        <owl:onProperty rdf:resource="http://www.opengis.net/citygml/generics/2.0#lod1Geometry"/>
                        <owl:minCardinality rdf:datatype="http://www.w3.org/2001/XMLSchema#nonNegativeInteger">0</owl:minCardinality>
                    </owl:Restriction>
                    <owl:Restriction>
                        <owl:onProperty rdf:resource="http://www.opengis.net/citygml/generics/2.0#lod1ImplicitRepresentation"/>
                        <owl:minCardinality rdf:datatype="http://www.w3.org/2001/XMLSchema#nonNegativeInteger">0</owl:minCardinality>
                    </owl:Restriction>
                    <owl:Restriction>
                        <owl:onProperty rdf:resource="http://www.opengis.net/citygml/generics/2.0#lod1TerrainIntersection"/>
                        <owl:minCardinality rdf:datatype="http://www.w3.org/2001/XMLSchema#nonNegativeInteger">0</owl:minCardinality>
                    </owl:Restriction>
                    <owl:Restriction>
                        <owl:onProperty rdf:resource="http://www.opengis.net/citygml/generics/2.0#lod2Geometry"/>
                        <owl:minCardinality rdf:datatype="http://www.w3.org/2001/XMLSchema#nonNegativeInteger">0</owl:minCardinality>
                    </owl:Restriction>
                    <owl:Restriction>
                        <owl:onProperty rdf:resource="http://www.opengis.net/citygml/generics/2.0#lod2ImplicitRepresentation"/>
                        <owl:minCardinality rdf:datatype="http://www.w3.org/2001/XMLSchema#nonNegativeInteger">0</owl:minCardinality>
                    </owl:Restriction>
                    <owl:Restriction>
                        <owl:onProperty rdf:resource="http://www.opengis.net/citygml/generics/2.0#lod2TerrainIntersection"/>
                        <owl:minCardinality rdf:datatype="http://www.w3.org/2001/XMLSchema#nonNegativeInteger">0</owl:minCardinality>
                    </owl:Restriction>
                    <owl:Restriction>
                        <owl:onProperty rdf:resource="http://www.opengis.net/citygml/generics/2.0#lod3Geometry"/>
                        <owl:minCardinality rdf:datatype="http://www.w3.org/2001/XMLSchema#nonNegativeInteger">0</owl:minCardinality>
                    </owl:Restriction>
                    <owl:Restriction>
                        <owl:onProperty rdf:resource="http://www.opengis.net/citygml/generics/2.0#lod3ImplicitRepresentation"/>
                        <owl:minCardinality rdf:datatype="http://www.w3.org/2001/XMLSchema#nonNegativeInteger">0</owl:minCardinality>
                    </owl:Restriction>
                    <owl:Restriction>
                        <owl:onProperty rdf:resource="http://www.opengis.net/citygml/generics/2.0#lod3TerrainIntersection"/>
                        <owl:minCardinality rdf:datatype="http://www.w3.org/2001/XMLSchema#nonNegativeInteger">0</owl:minCardinality>
                    </owl:Restriction>
                    <owl:Restriction>
                        <owl:onProperty rdf:resource="http://www.opengis.net/citygml/generics/2.0#lod4Geometry"/>
                        <owl:minCardinality rdf:datatype="http://www.w3.org/2001/XMLSchema#nonNegativeInteger">0</owl:minCardinality>
                    </owl:Restriction>
                    <owl:Restriction>
                        <owl:onProperty rdf:resource="http://www.opengis.net/citygml/generics/2.0#lod4ImplicitRepresentation"/>
                        <owl:minCardinality rdf:datatype="http://www.w3.org/2001/XMLSchema#nonNegativeInteger">0</owl:minCardinality>
                    </owl:Restriction>
                    <owl:Restriction>
                        <owl:onProperty rdf:resource="http://www.opengis.net/citygml/generics/2.0#lod4TerrainIntersection"/>
                        <owl:minCardinality rdf:datatype="http://www.w3.org/2001/XMLSchema#nonNegativeInteger">0</owl:minCardinality>
                    </owl:Restriction>
                    <owl:Restriction>
                        <owl:onProperty rdf:resource="http://www.opengis.net/citygml/generics/2.0#usage"/>
                        <owl:minCardinality rdf:datatype="http://www.w3.org/2001/XMLSchema#nonNegativeInteger">0</owl:minCardinality>
                    </owl:Restriction>
                </owl:intersectionOf>
            </owl:Class>
        </owl:equivalentClass>
        <rdfs:subClassOf rdf:resource="http://www.opengis.net/citygml/2.0#AbstractCityObjectType"/>
        <rdfs:comment>Generic (user defined) city objects may be used to model features which are not covered explicitly by the
				CityGML schema. Generic objects must be used with care; they shall only be used if there is no appropiate thematic class
				available in the overall CityGML schema. Oherwise, problems concerning semantic interoperability may arise. As subclass of
				_CityObject, a generic city object inherits all attributes and relations, in particular an id, names, external references,
				and generalization relations. </rdfs:comment>
        <rdfs:comment>Warning: The parent class &apos;core:AbstractCityObjectType&apos; is declared outside of this class&apos; original schema. This class may be declared incorrectly.</rdfs:comment>
    </owl:Class>
    


    <!-- http://www.opengis.net/citygml/generics/2.0#IntAttributeType -->

    <owl:Class rdf:about="http://www.opengis.net/citygml/generics/2.0#IntAttributeType">
        <owl:equivalentClass>
            <owl:Class>
                <owl:intersectionOf rdf:parseType="Collection">
                    <owl:Restriction>
                        <owl:onProperty rdf:resource="http://www.opengis.net/citygml/generics/2.0#value"/>
                        <owl:allValuesFrom rdf:resource="http://www.w3.org/2001/XMLSchema#integer"/>
                    </owl:Restriction>
                </owl:intersectionOf>
            </owl:Class>
        </owl:equivalentClass>
        <rdfs:comment></rdfs:comment>
    </owl:Class>
    


    <!-- http://www.opengis.net/citygml/generics/2.0#MeasureAttributeType -->

    <owl:Class rdf:about="http://www.opengis.net/citygml/generics/2.0#MeasureAttributeType">
        <owl:equivalentClass>
            <owl:Class>
                <owl:intersectionOf rdf:parseType="Collection">
                    <owl:Restriction>
                        <owl:onProperty rdf:resource="http://www.opengis.net/citygml/generics/2.0#value"/>
                        <owl:allValuesFrom rdf:resource="http://www.opengis.net/gml#MeasureType"/>
                    </owl:Restriction>
                </owl:intersectionOf>
            </owl:Class>
        </owl:equivalentClass>
        <rdfs:comment></rdfs:comment>
    </owl:Class>
    


    <!-- http://www.opengis.net/citygml/generics/2.0#StringAttributeType -->

    <owl:Class rdf:about="http://www.opengis.net/citygml/generics/2.0#StringAttributeType">
        <owl:equivalentClass>
            <owl:Class>
                <owl:intersectionOf rdf:parseType="Collection">
                    <owl:Restriction>
                        <owl:onProperty rdf:resource="http://www.opengis.net/citygml/generics/2.0#value"/>
                        <owl:allValuesFrom rdf:resource="http://www.w3.org/2001/XMLSchema#string"/>
                    </owl:Restriction>
                </owl:intersectionOf>
            </owl:Class>
        </owl:equivalentClass>
        <rdfs:comment></rdfs:comment>
    </owl:Class>
    


    <!-- http://www.opengis.net/citygml/generics/2.0#UriAttributeType -->

    <owl:Class rdf:about="http://www.opengis.net/citygml/generics/2.0#UriAttributeType">
        <owl:equivalentClass>
            <owl:Class>
                <owl:intersectionOf rdf:parseType="Collection">
                    <owl:Restriction>
                        <owl:onProperty rdf:resource="http://www.opengis.net/citygml/generics/2.0#value"/>
                        <owl:allValuesFrom rdf:resource="http://www.w3.org/2001/XMLSchema#anyURI"/>
                    </owl:Restriction>
                </owl:intersectionOf>
            </owl:Class>
        </owl:equivalentClass>
        <rdfs:comment></rdfs:comment>
    </owl:Class>
    


    <!-- http://www.opengis.net/citygml/generics/2.0#_genericAttribute -->

    <owl:Class rdf:about="http://www.opengis.net/citygml/generics/2.0#_genericAttribute">
        <rdfs:subClassOf rdf:resource="http://www.opengis.net/citygml/2.0#_GenericApplicationPropertyOfCityObject"/>
        <rdfs:subClassOf rdf:resource="http://www.opengis.net/citygml/generics/2.0#AbstractGenericAttributeType"/>
    </owl:Class>
    


    <!-- http://www.opengis.net/citygml/generics/2.0#dateAttribute -->

    <owl:Class rdf:about="http://www.opengis.net/citygml/generics/2.0#dateAttribute">
        <rdfs:subClassOf rdf:resource="http://www.opengis.net/citygml/generics/2.0#DateAttributeType"/>
        <rdfs:subClassOf rdf:resource="http://www.opengis.net/citygml/generics/2.0#_genericAttribute"/>
    </owl:Class>
    


    <!-- http://www.opengis.net/citygml/generics/2.0#doubleAttribute -->

    <owl:Class rdf:about="http://www.opengis.net/citygml/generics/2.0#doubleAttribute">
        <rdfs:subClassOf rdf:resource="http://www.opengis.net/citygml/generics/2.0#DoubleAttributeType"/>
        <rdfs:subClassOf rdf:resource="http://www.opengis.net/citygml/generics/2.0#_genericAttribute"/>
    </owl:Class>
    


    <!-- http://www.opengis.net/citygml/generics/2.0#genericAttributeSet -->

    <owl:Class rdf:about="http://www.opengis.net/citygml/generics/2.0#genericAttributeSet">
        <rdfs:subClassOf rdf:resource="http://www.opengis.net/citygml/generics/2.0#GenericAttributeSetType"/>
        <rdfs:subClassOf rdf:resource="http://www.opengis.net/citygml/generics/2.0#_genericAttribute"/>
    </owl:Class>
    


    <!-- http://www.opengis.net/citygml/generics/2.0#intAttribute -->

    <owl:Class rdf:about="http://www.opengis.net/citygml/generics/2.0#intAttribute">
        <rdfs:subClassOf rdf:resource="http://www.opengis.net/citygml/generics/2.0#IntAttributeType"/>
        <rdfs:subClassOf rdf:resource="http://www.opengis.net/citygml/generics/2.0#_genericAttribute"/>
    </owl:Class>
    


    <!-- http://www.opengis.net/citygml/generics/2.0#measureAttribute -->

    <owl:Class rdf:about="http://www.opengis.net/citygml/generics/2.0#measureAttribute">
        <rdfs:subClassOf rdf:resource="http://www.opengis.net/citygml/generics/2.0#MeasureAttributeType"/>
        <rdfs:subClassOf rdf:resource="http://www.opengis.net/citygml/generics/2.0#_genericAttribute"/>
    </owl:Class>
    


    <!-- http://www.opengis.net/citygml/generics/2.0#stringAttribute -->

    <owl:Class rdf:about="http://www.opengis.net/citygml/generics/2.0#stringAttribute">
        <rdfs:subClassOf rdf:resource="http://www.opengis.net/citygml/generics/2.0#StringAttributeType"/>
        <rdfs:subClassOf rdf:resource="http://www.opengis.net/citygml/generics/2.0#_genericAttribute"/>
    </owl:Class>
    


    <!-- http://www.opengis.net/citygml/generics/2.0#uriAttribute -->

    <owl:Class rdf:about="http://www.opengis.net/citygml/generics/2.0#uriAttribute">
        <rdfs:subClassOf rdf:resource="http://www.opengis.net/citygml/generics/2.0#UriAttributeType"/>
        <rdfs:subClassOf rdf:resource="http://www.opengis.net/citygml/generics/2.0#_genericAttribute"/>
    </owl:Class>
    


    <!-- http://www.opengis.net/gml#MultiCurvePropertyType -->

    <owl:Class rdf:about="http://www.opengis.net/gml#MultiCurvePropertyType"/>
    


    <!-- 
    ///////////////////////////////////////////////////////////////////////////////////////
    //
    // Annotations
    //
    ///////////////////////////////////////////////////////////////////////////////////////
     -->

    <rdf:Description rdf:about="http://www.opengis.net/citygml/generics/2.0#value">
        <rdfs:comment>Warning: This ObjectProperty type was declared outside of its original schema. This ObjectProperty may be declared incorrectly.</rdfs:comment>
    </rdf:Description>
</rdf:RDF>



<!-- Generated by the OWL API (version 4.5.9.2019-02-01T07:24:44Z) https://github.com/owlcs/owlapi -->

