<rdf:RDF xmlns:math="http://www.w3.org/2005/xpath-functions/math" xmlns:owl="http://www.w3.org/2002/07/owl#" xmlns:rdf="http://www.w3.org/1999/02/22-rdf-syntax-ns#" xmlns:rdfs="http://www.w3.org/2000/01/rdf-schema#" xmlns:xs="http://www.w3.org/2001/XMLSchema" xmlns:xsd="http://www.w3.org/2001/XMLSchema">
   <owl:Ontology rdf:about="http://liris.cnrs.fr/ontologies/geometryBasic0d1d">
      <owl:imports rdf:resource="http://liris.cnrs.fr/ontologies/gml"/>
      <owl:imports rdf:resource="http://liris.cnrs.fr/ontologies/measures"/>
      <rdfs:comment>geometryBasic0d1d.xsd</rdfs:comment>
      <rdfs:seeAlso>urn:opengis:specification:gml:schema-xsd:geometryBasic0d1d:v3.1.1</rdfs:seeAlso>
      <rdfs:seeAlso>urn:opengis:specification:gml:schema-xsd:geometryBasic0d1d:v3.1.1</rdfs:seeAlso>
      <rdfs:comment>
			GML is an OGC Standard.
			Copyright (c) 2001,2005,2010 Open Geospatial Consortium.
			To obtain additional rights of use, visit http://www.opengeospatial.org/legal/ .
		</rdfs:comment>
   </owl:Ontology>
   <owl:Class rdf:about="#GeometryPropertyType">
      <rdfs:comment>A geometric property can either be any geometry element encapsulated in an element of this type or an XLink reference 
			to a remote geometry element (where remote includes geometry elements located elsewhere in the same document). Note that either 
			the reference or the contained element must be given, but not both or none.</rdfs:comment>
      <rdfs:subClassOf>
         <owl:Class>
            <owl:intersectionOf rdf:parseType="Collection">
               <owl:Restriction>
                  <owl:onProperty rdf:resource="http://www.opengis.net/gml#has_Geometry"/>
                  <owl:allValuesFrom rdf:resource="http://www.opengis.net/gml#_Geometry"/>
               </owl:Restriction>
            </owl:intersectionOf>
         </owl:Class>
      </rdfs:subClassOf>
   </owl:Class>
   <owl:Class rdf:about="#GeometryArrayPropertyType">
      <rdfs:comment>A container for an array of geometry elements. The elements are always contained in the array property, 
			referencing geometry elements or arrays of geometry elements is not supported.</rdfs:comment>
      <rdfs:subClassOf>
         <owl:Class>
            <owl:intersectionOf rdf:parseType="Collection">
               <owl:Restriction>
                  <owl:onProperty rdf:resource="http://www.opengis.net/gml#has_Geometry"/>
                  <owl:allValuesFrom rdf:resource="http://www.opengis.net/gml#_Geometry"/>
               </owl:Restriction>
               <owl:Restriction>
                  <owl:onProperty rdf:resource="http://www.opengis.net/gml#has_Geometry"/>
                  <owl:minCardinality rdf:datatype="http://www.w3.org/2001/XMLSchema#nonNegativeInteger">0</owl:minCardinality>
               </owl:Restriction>
            </owl:intersectionOf>
         </owl:Class>
      </rdfs:subClassOf>
   </owl:Class>
   <owl:Class rdf:about="#AbstractGeometryType">
      <rdfs:comment>This is an abstract class</rdfs:comment>
      <rdfs:comment>All geometry elements are derived directly or indirectly from this abstract supertype. A geometry element may 
			have an identifying attribute ("gml:id"), a name (attribute "name") and a description (attribute "description"). It may be associated 
			with a spatial reference system (attribute "srsName"). The following rules shall be adhered: - Every geometry type shall derive 
			from this abstract type. - Every geometry element (i.e. an element of a geometry type) shall be directly or indirectly in the 
			substitution group of _Geometry.</rdfs:comment>
      <rdfs:subClassOf>
         <owl:Class>
            <owl:intersectionOf rdf:parseType="Collection">
               <owl:Restriction>
                  <owl:onProperty rdf:resource="#gid"/>
                  <owl:allValuesFrom rdf:resource="http://www.w3.org/2001/XMLSchema#string"/>
               </owl:Restriction>
            </owl:intersectionOf>
         </owl:Class>
      </rdfs:subClassOf>
      <rdfs:subClassOf rdf:resource="http://www.opengis.net/gml#AbstractGMLType"/>
      <rdfs:comment>Warning: The parent class 'gml:AbstractGMLType' is declared outside of this class' original schema. This class may be declared incorrectly.</rdfs:comment>
   </owl:Class>
   <owl:Class rdf:about="#AbstractGeometricPrimitiveType">
      <rdfs:comment>This is an abstract class</rdfs:comment>
      <rdfs:comment>This is the abstract root type of the geometric primitives. A geometric primitive is a geometric object that is not 
			decomposed further into other primitives in the system. All primitives are oriented in the direction implied by the sequence of their 
			coordinate tuples.</rdfs:comment>
      <rdfs:subClassOf rdf:resource="http://www.opengis.net/gml#AbstractGeometryType"/>
      <rdfs:comment>Warning: The parent class 'gml:AbstractGeometryType' is declared outside of this class' original schema. This class may be declared incorrectly.</rdfs:comment>
   </owl:Class>
   <owl:Class rdf:about="#GeometricPrimitivePropertyType">
      <rdfs:comment>A property that has a geometric primitive as its value domain can either be an appropriate geometry element 
			encapsulated in an element of this type or an XLink reference to a remote geometry element (where remote includes geometry 
			elements located elsewhere in the same document). Either the reference or the contained element must be given, but neither 
			both nor none.</rdfs:comment>
      <rdfs:subClassOf>
         <owl:Class>
            <owl:intersectionOf rdf:parseType="Collection">
               <owl:Restriction>
                  <owl:onProperty rdf:resource="http://www.opengis.net/gml#has_GeometricPrimitive"/>
                  <owl:allValuesFrom rdf:resource="http://www.opengis.net/gml#_GeometricPrimitive"/>
               </owl:Restriction>
            </owl:intersectionOf>
         </owl:Class>
      </rdfs:subClassOf>
   </owl:Class>
   <owl:Class rdf:about="#PointType">
      <rdfs:comment>A Point is defined by a single coordinate tuple.</rdfs:comment>
      <rdfs:subClassOf>
         <owl:Class>
            <owl:intersectionOf rdf:parseType="Collection"/>
         </owl:Class>
      </rdfs:subClassOf>
      <rdfs:subClassOf rdf:resource="http://www.opengis.net/gml#AbstractGeometricPrimitiveType"/>
      <rdfs:comment>Warning: The parent class 'gml:AbstractGeometricPrimitiveType' is declared outside of this class' original schema. This class may be declared incorrectly.</rdfs:comment>
   </owl:Class>
   <owl:Class rdf:about="#PointPropertyType">
      <rdfs:comment>A property that has a point as its value domain can either be an appropriate geometry element encapsulated in an 
			element of this type or an XLink reference to a remote geometry element (where remote includes geometry elements located 
			elsewhere in the same document). Either the reference or the contained element must be given, but neither both nor none.</rdfs:comment>
      <rdfs:subClassOf>
         <owl:Class>
            <owl:intersectionOf rdf:parseType="Collection">
               <owl:Restriction>
                  <owl:onProperty rdf:resource="http://www.opengis.net/gml#hasPoint"/>
                  <owl:allValuesFrom rdf:resource="http://www.opengis.net/gml#Point"/>
               </owl:Restriction>
            </owl:intersectionOf>
         </owl:Class>
      </rdfs:subClassOf>
   </owl:Class>
   <owl:Class rdf:about="#PointArrayPropertyType">
      <rdfs:comment>A container for an array of points. The elements are always contained in the array property, referencing geometry 
			elements or arrays of geometry elements is not supported.</rdfs:comment>
      <rdfs:subClassOf>
         <owl:Class>
            <owl:intersectionOf rdf:parseType="Collection">
               <owl:Restriction>
                  <owl:onProperty rdf:resource="http://www.opengis.net/gml#hasPoint"/>
                  <owl:allValuesFrom rdf:resource="http://www.opengis.net/gml#Point"/>
               </owl:Restriction>
               <owl:Restriction>
                  <owl:onProperty rdf:resource="http://www.opengis.net/gml#hasPoint"/>
                  <owl:minCardinality rdf:datatype="http://www.w3.org/2001/XMLSchema#nonNegativeInteger">0</owl:minCardinality>
               </owl:Restriction>
            </owl:intersectionOf>
         </owl:Class>
      </rdfs:subClassOf>
   </owl:Class>
   <owl:Class rdf:about="#AbstractCurveType">
      <rdfs:comment>This is an abstract class</rdfs:comment>
      <rdfs:comment>An abstraction of a curve to support the different levels of complexity. The curve can always be viewed as a geometric 
			primitive, i.e. is continuous.</rdfs:comment>
      <rdfs:subClassOf rdf:resource="http://www.opengis.net/gml#AbstractGeometricPrimitiveType"/>
      <rdfs:comment>Warning: The parent class 'gml:AbstractGeometricPrimitiveType' is declared outside of this class' original schema. This class may be declared incorrectly.</rdfs:comment>
   </owl:Class>
   <owl:Class rdf:about="#CurvePropertyType">
      <rdfs:comment>A property that has a curve as its value domain can either be an appropriate geometry element encapsulated in an 
			element of this type or an XLink reference to a remote geometry element (where remote includes geometry elements located elsewhere 
			in the same document). Either the reference or the contained element must be given, but neither both nor none.</rdfs:comment>
      <rdfs:subClassOf>
         <owl:Class>
            <owl:intersectionOf rdf:parseType="Collection">
               <owl:Restriction>
                  <owl:onProperty rdf:resource="http://www.opengis.net/gml#has_Curve"/>
                  <owl:allValuesFrom rdf:resource="http://www.opengis.net/gml#_Curve"/>
               </owl:Restriction>
            </owl:intersectionOf>
         </owl:Class>
      </rdfs:subClassOf>
   </owl:Class>
   <owl:Class rdf:about="#CurveArrayPropertyType">
      <rdfs:comment>A container for an array of curves. The elements are always contained in the array property, referencing geometry elements 
			or arrays of geometry elements is not supported.</rdfs:comment>
      <rdfs:subClassOf>
         <owl:Class>
            <owl:intersectionOf rdf:parseType="Collection">
               <owl:Restriction>
                  <owl:onProperty rdf:resource="http://www.opengis.net/gml#has_Curve"/>
                  <owl:allValuesFrom rdf:resource="http://www.opengis.net/gml#_Curve"/>
               </owl:Restriction>
               <owl:Restriction>
                  <owl:onProperty rdf:resource="http://www.opengis.net/gml#has_Curve"/>
                  <owl:minCardinality rdf:datatype="http://www.w3.org/2001/XMLSchema#nonNegativeInteger">0</owl:minCardinality>
               </owl:Restriction>
            </owl:intersectionOf>
         </owl:Class>
      </rdfs:subClassOf>
   </owl:Class>
   <owl:Class rdf:about="#LineStringType">
      <rdfs:comment>A LineString is a special curve that consists of a single segment with linear interpolation. It is defined by two or more coordinate 
			tuples, with linear interpolation between them. It is backwards compatible with the LineString of GML 2, GM_LineString of ISO 19107 is 
			implemented by LineStringSegment.</rdfs:comment>
      <rdfs:subClassOf>
         <owl:Class>
            <owl:intersectionOf rdf:parseType="Collection"/>
         </owl:Class>
      </rdfs:subClassOf>
      <rdfs:subClassOf rdf:resource="http://www.opengis.net/gml#AbstractCurveType"/>
      <rdfs:comment>Warning: The parent class 'gml:AbstractCurveType' is declared outside of this class' original schema. This class may be declared incorrectly.</rdfs:comment>
   </owl:Class>
   <owl:Class rdf:about="#DirectPositionType">
      <rdfs:comment>DirectPosition instances hold the coordinates for a position within some coordinate reference system (CRS). Since 
			DirectPositions, as data types, will often be included in larger objects (such as geometry elements) that have references to CRS, the 
			"srsName" attribute will in general be missing, if this particular DirectPosition is included in a larger element with such a reference to a 
			CRS. In this case, the CRS is implicitly assumed to take on the value of the containing object's CRS.</rdfs:comment>
      <rdfs:subClassOf rdf:resource="http://www.opengis.net/gml#doubleList"/>
      <rdfs:comment>Warning: The parent class 'gml:doubleList' is declared outside of this class' original schema. This class may be declared incorrectly.</rdfs:comment>
   </owl:Class>
   <owl:DatatypeProperty rdf:about="#hasDirectPositionType">
      <rdfs:domain rdf:resource="#DirectPositionType"/>
      <rdfs:range rdf:resource="http://www.opengis.net/gml#doubleList"/>
      <rdfs:subPropertyOf rdf:resource="http://www.opengis.net/gml#hasdoubleList"/>
      <rdfs:comment>Warning: The parent property 'gml:hasdoubleList' is declared outside of this property's original schema. This property may be declared incorrectly.</rdfs:comment>
   </owl:DatatypeProperty>
   <owl:Class rdf:about="#DirectPositionListType">
      <rdfs:comment>DirectPositionList instances hold the coordinates for a sequence of direct positions within the same coordinate 
			reference system (CRS).</rdfs:comment>
      <rdfs:subClassOf>
         <owl:Class>
            <owl:intersectionOf rdf:parseType="Collection">
               <owl:Restriction>
                  <owl:onProperty rdf:resource="#count"/>
                  <owl:allValuesFrom rdf:resource="http://www.w3.org/2001/XMLSchema#positiveInteger"/>
               </owl:Restriction>
            </owl:intersectionOf>
         </owl:Class>
      </rdfs:subClassOf>
      <rdfs:subClassOf rdf:resource="http://www.opengis.net/gml#doubleList"/>
      <rdfs:comment>Warning: The parent class 'gml:doubleList' is declared outside of this class' original schema. This class may be declared incorrectly.</rdfs:comment>
   </owl:Class>
   <owl:DatatypeProperty rdf:about="#hasDirectPositionListType">
      <rdfs:domain rdf:resource="#DirectPositionListType"/>
      <rdfs:range rdf:resource="http://www.opengis.net/gml#doubleList"/>
      <rdfs:subPropertyOf rdf:resource="http://www.opengis.net/gml#hasdoubleList"/>
      <rdfs:comment>Warning: The parent property 'gml:hasdoubleList' is declared outside of this property's original schema. This property may be declared incorrectly.</rdfs:comment>
   </owl:DatatypeProperty>
   <owl:Class rdf:about="#VectorType">
      <rdfs:comment>Vector instances hold the compoents for a (usually spatial) vector within some coordinate reference system (CRS). 
			Since Vectors will often be included in larger objects that have references to CRS, the "srsName" attribute may be missing. 
			In this case, the CRS is implicitly assumed to take on the value of the containing object's CRS.

			Note that this content model is the same as DirectPositionType, but is defined separately to reflect the distinct semantics, and to avoid validation problems. SJDC 2004-12-02</rdfs:comment>
      <rdfs:subClassOf rdf:resource="http://www.opengis.net/gml#doubleList"/>
      <rdfs:comment>Warning: The parent class 'gml:doubleList' is declared outside of this class' original schema. This class may be declared incorrectly.</rdfs:comment>
   </owl:Class>
   <owl:DatatypeProperty rdf:about="#hasVectorType">
      <rdfs:domain rdf:resource="#VectorType"/>
      <rdfs:range rdf:resource="http://www.opengis.net/gml#doubleList"/>
      <rdfs:subPropertyOf rdf:resource="http://www.opengis.net/gml#hasdoubleList"/>
      <rdfs:comment>Warning: The parent property 'gml:hasdoubleList' is declared outside of this property's original schema. This property may be declared incorrectly.</rdfs:comment>
   </owl:DatatypeProperty>
   <owl:Class rdf:about="#EnvelopeType">
      <rdfs:comment>Envelope defines an extent using a pair of positions defining opposite corners in arbitrary dimensions. The first direct 
			position is the "lower corner" (a coordinate position consisting of all the minimal ordinates for each dimension for all points within the envelope), 
			the second one the "upper corner" (a coordinate position consisting of all the maximal ordinates for each dimension for all points within the 
			envelope).</rdfs:comment>
      <owl:disjointUnionOf rdf:parseType="Collection">
         <owl:Restriction>
            <owl:onProperty rdf:resource="http://www.opengis.net/gml#hascoord"/>
            <owl:someValuesFrom rdf:resource="http://www.opengis.net/gml#coord"/>
         </owl:Restriction>
         <owl:Restriction>
            <owl:onProperty rdf:resource="http://www.opengis.net/gml#hascoord"/>
            <owl:cardinality rdf:datatype="http://www.w3.org/2001/XMLSchema#nonNegativeInteger">2</owl:cardinality>
         </owl:Restriction>
         <owl:Restriction>
            <owl:onProperty rdf:resource="http://www.opengis.net/gml#haspos"/>
            <owl:someValuesFrom rdf:resource="http://www.opengis.net/gml#pos"/>
         </owl:Restriction>
         <owl:Restriction>
            <owl:onProperty rdf:resource="http://www.opengis.net/gml#haspos"/>
            <owl:cardinality rdf:datatype="http://www.w3.org/2001/XMLSchema#nonNegativeInteger">2</owl:cardinality>
         </owl:Restriction>
         <owl:Restriction>
            <owl:onProperty rdf:resource="http://www.opengis.net/gml#hascoordinates"/>
            <owl:someValuesFrom rdf:resource="http://www.opengis.net/gml#coordinates"/>
         </owl:Restriction>
      </owl:disjointUnionOf>
   </owl:Class>
   <owl:Class rdf:about="#CoordType">
      <rdfs:comment>Represents a coordinate tuple in one, two, or three dimensions. Deprecated with GML 3.0 and replaced by 
			DirectPositionType.</rdfs:comment>
      <rdfs:subClassOf>
         <owl:Class>
            <owl:intersectionOf rdf:parseType="Collection">
               <owl:Restriction>
                  <owl:onProperty rdf:resource="#X"/>
                  <owl:allValuesFrom rdf:resource="http://www.w3.org/2001/XMLSchema#decimal"/>
               </owl:Restriction>
               <owl:Restriction>
                  <owl:onProperty rdf:resource="#Y"/>
                  <owl:allValuesFrom rdf:resource="http://www.w3.org/2001/XMLSchema#decimal"/>
               </owl:Restriction>
               <owl:Restriction>
                  <owl:onProperty rdf:resource="#Y"/>
                  <owl:minCardinality rdf:datatype="http://www.w3.org/2001/XMLSchema#nonNegativeInteger">0</owl:minCardinality>
               </owl:Restriction>
               <owl:Restriction>
                  <owl:onProperty rdf:resource="#Z"/>
                  <owl:allValuesFrom rdf:resource="http://www.w3.org/2001/XMLSchema#decimal"/>
               </owl:Restriction>
               <owl:Restriction>
                  <owl:onProperty rdf:resource="#Z"/>
                  <owl:minCardinality rdf:datatype="http://www.w3.org/2001/XMLSchema#nonNegativeInteger">0</owl:minCardinality>
               </owl:Restriction>
            </owl:intersectionOf>
         </owl:Class>
      </rdfs:subClassOf>
   </owl:Class>
   <owl:Class rdf:about="#LineStringPropertyType">
      <rdfs:comment>This type is deprecated with GML 3 and shall not be used. It is included for backwards compatibility with GML 2. Use 
			CurvePropertyType instead. A property that has a line string as its value domain can either be an appropriate geometry element encapsulated 
			in an element of this type or an XLink reference to a remote geometry element (where remote includes geometry elements located elsewhere 
			in the same document). Either the reference or the contained element must be given, but neither both nor none.</rdfs:comment>
      <rdfs:subClassOf>
         <owl:Class>
            <owl:intersectionOf rdf:parseType="Collection">
               <owl:Restriction>
                  <owl:onProperty rdf:resource="http://www.opengis.net/gml#hasLineString"/>
                  <owl:allValuesFrom rdf:resource="http://www.opengis.net/gml#LineString"/>
               </owl:Restriction>
            </owl:intersectionOf>
         </owl:Class>
      </rdfs:subClassOf>
   </owl:Class>
   <owl:Class rdf:about="#geometricPositionGroup">
      <rdfs:subClassOf>
         <owl:Class>
            <owl:intersectionOf rdf:parseType="Collection"/>
         </owl:Class>
      </rdfs:subClassOf>
      <owl:disjointUnionOf rdf:parseType="Collection">
         <owl:Restriction>
            <owl:onProperty rdf:resource="http://www.opengis.net/gml#haspos"/>
            <owl:someValuesFrom rdf:resource="http://www.opengis.net/gml#pos"/>
         </owl:Restriction>
         <owl:Restriction>
            <owl:onProperty rdf:resource="http://www.opengis.net/gml#haspointProperty"/>
            <owl:someValuesFrom rdf:resource="http://www.opengis.net/gml#pointProperty"/>
         </owl:Restriction>
      </owl:disjointUnionOf>
      <rdfs:comment>A geometric position represented either by a DirectPosition or a Point.</rdfs:comment>
   </owl:Class>
   <owl:Class rdf:about="#geometricPositionListGroup">
      <rdfs:subClassOf>
         <owl:Class>
            <owl:intersectionOf rdf:parseType="Collection"/>
         </owl:Class>
      </rdfs:subClassOf>
      <owl:disjointUnionOf rdf:parseType="Collection">
         <owl:Restriction>
            <owl:onProperty rdf:resource="http://www.opengis.net/gml#hasposList"/>
            <owl:someValuesFrom rdf:resource="http://www.opengis.net/gml#posList"/>
         </owl:Restriction>
      </owl:disjointUnionOf>
      <rdfs:comment>A list of geometric positions represented either by a DirectPosition or a Point.</rdfs:comment>
   </owl:Class>
   <owl:ObjectProperty rdf:about="http://www.opengis.net/gml#hasgeometricPositionGroup">
      <rdfs:domain rdf:resource="#geometricPositionListGroup"/>
      <rdfs:range rdf:resource="http://www.opengis.net/gml#geometricPositionGroup"/>
   </owl:ObjectProperty>
   <owl:ObjectProperty rdf:about="http://www.opengis.net/gml#hasAssociationAttributeGroup">
      <rdfs:domain rdf:resource="#GeometryPropertyType"/>
      <rdfs:range rdf:resource="http://www.opengis.net/gml#AssociationAttributeGroup"/>
   </owl:ObjectProperty>
   <owl:ObjectProperty rdf:about="http://www.opengis.net/gml#hasSRSReferenceGroup">
      <rdfs:domain rdf:resource="#AbstractGeometryType"/>
      <rdfs:range rdf:resource="http://www.opengis.net/gml#SRSReferenceGroup"/>
   </owl:ObjectProperty>
   <owl:Class rdf:about="#SRSReferenceGroup">
      <rdfs:subClassOf>
         <owl:Class>
            <owl:intersectionOf rdf:parseType="Collection">
               <owl:Restriction>
                  <owl:onProperty rdf:resource="#srsName"/>
                  <owl:allValuesFrom rdf:resource="http://www.w3.org/2001/XMLSchema#anyURI"/>
               </owl:Restriction>
               <owl:Restriction>
                  <owl:onProperty rdf:resource="#srsDimension"/>
                  <owl:allValuesFrom rdf:resource="http://www.w3.org/2001/XMLSchema#positiveInteger"/>
               </owl:Restriction>
            </owl:intersectionOf>
         </owl:Class>
      </rdfs:subClassOf>
      <rdfs:comment>Optional reference to the CRS used by this geometry, with optional additional information to simplify use when 
			a more complete definition of the CRS is not needed.</rdfs:comment>
   </owl:Class>
   <owl:ObjectProperty rdf:about="http://www.opengis.net/gml#hasSRSInformationGroup">
      <rdfs:domain rdf:resource="#SRSReferenceGroup"/>
      <rdfs:range rdf:resource="http://www.opengis.net/gml#SRSInformationGroup"/>
   </owl:ObjectProperty>
   <owl:Class rdf:about="#SRSInformationGroup">
      <rdfs:subClassOf>
         <owl:Class>
            <owl:intersectionOf rdf:parseType="Collection">
               <owl:Restriction>
                  <owl:onProperty rdf:resource="#axisLabels"/>
                  <owl:allValuesFrom rdf:resource="http://www.opengis.net/gml#NCNameList"/>
               </owl:Restriction>
               <owl:Restriction>
                  <owl:onProperty rdf:resource="#uomLabels"/>
                  <owl:allValuesFrom rdf:resource="http://www.opengis.net/gml#NCNameList"/>
               </owl:Restriction>
            </owl:intersectionOf>
         </owl:Class>
      </rdfs:subClassOf>
      <rdfs:comment>Optional additional and redundant information for a CRS to simplify use when a more complete definition of the 
			CRS is not needed. This information shall be the same as included in the more complete definition of the CRS, referenced by the 
			srsName attribute. When the srsName attribute is included, either both or neither of the axisLabels and uomLabels attributes 
			shall be included. When the srsName attribute is omitted, both of these attributes shall be omitted.</rdfs:comment>
   </owl:Class>
   <owl:ObjectProperty rdf:about="http://www.opengis.net/gml#hasAssociationAttributeGroup">
      <rdfs:domain rdf:resource="#GeometricPrimitivePropertyType"/>
      <rdfs:range rdf:resource="http://www.opengis.net/gml#AssociationAttributeGroup"/>
   </owl:ObjectProperty>
   <owl:ObjectProperty rdf:about="http://www.opengis.net/gml#hasAssociationAttributeGroup">
      <rdfs:domain rdf:resource="#PointPropertyType"/>
      <rdfs:range rdf:resource="http://www.opengis.net/gml#AssociationAttributeGroup"/>
   </owl:ObjectProperty>
   <owl:ObjectProperty rdf:about="http://www.opengis.net/gml#hasAssociationAttributeGroup">
      <rdfs:domain rdf:resource="#CurvePropertyType"/>
      <rdfs:range rdf:resource="http://www.opengis.net/gml#AssociationAttributeGroup"/>
   </owl:ObjectProperty>
   <owl:ObjectProperty rdf:about="http://www.opengis.net/gml#hasSRSReferenceGroup">
      <rdfs:domain rdf:resource="#DirectPositionType"/>
      <rdfs:range rdf:resource="http://www.opengis.net/gml#SRSReferenceGroup"/>
   </owl:ObjectProperty>
   <owl:ObjectProperty rdf:about="http://www.opengis.net/gml#hasSRSReferenceGroup">
      <rdfs:domain rdf:resource="#DirectPositionListType"/>
      <rdfs:range rdf:resource="http://www.opengis.net/gml#SRSReferenceGroup"/>
   </owl:ObjectProperty>
   <owl:ObjectProperty rdf:about="http://www.opengis.net/gml#hasSRSReferenceGroup">
      <rdfs:domain rdf:resource="#VectorType"/>
      <rdfs:range rdf:resource="http://www.opengis.net/gml#SRSReferenceGroup"/>
   </owl:ObjectProperty>
   <owl:ObjectProperty rdf:about="http://www.opengis.net/gml#hasSRSReferenceGroup">
      <rdfs:domain rdf:resource="#EnvelopeType"/>
      <rdfs:range rdf:resource="http://www.opengis.net/gml#SRSReferenceGroup"/>
   </owl:ObjectProperty>
   <owl:ObjectProperty rdf:about="http://www.opengis.net/gml#hasAssociationAttributeGroup">
      <rdfs:domain rdf:resource="#LineStringPropertyType"/>
      <rdfs:range rdf:resource="http://www.opengis.net/gml#AssociationAttributeGroup"/>
   </owl:ObjectProperty>
   <owl:DatatypeProperty rdf:about="#gid">
      <rdfs:domain rdf:resource="#AbstractGeometryType"/>
      <rdfs:range rdf:resource="#string"/>
   </owl:DatatypeProperty>
   <owl:DatatypeProperty rdf:about="#srsName">
      <rdfs:domain rdf:resource="#SRSReferenceGroup"/>
      <rdfs:range rdf:resource="#anyURI"/>
   </owl:DatatypeProperty>
   <owl:DatatypeProperty rdf:about="#srsDimension">
      <rdfs:domain rdf:resource="#SRSReferenceGroup"/>
      <rdfs:range rdf:resource="#positiveInteger"/>
   </owl:DatatypeProperty>
   <owl:DatatypeProperty rdf:about="#axisLabels">
      <rdfs:domain rdf:resource="#SRSInformationGroup"/>
      <rdfs:range rdf:resource="http://www.opengis.net/gml#NCNameList"/>
   </owl:DatatypeProperty>
   <owl:DatatypeProperty rdf:about="#uomLabels">
      <rdfs:domain rdf:resource="#SRSInformationGroup"/>
      <rdfs:range rdf:resource="http://www.opengis.net/gml#NCNameList"/>
   </owl:DatatypeProperty>
   <owl:DatatypeProperty rdf:about="#count">
      <rdfs:domain rdf:resource="#DirectPositionListType"/>
      <rdfs:range rdf:resource="#positiveInteger"/>
   </owl:DatatypeProperty>
   <owl:Class rdf:about="#_Geometry">
      <rdfs:subClassOf rdf:resource="http://www.opengis.net/gml#_GML"/>
      <rdfs:subClassOf rdf:resource="http://www.opengis.net/gml#AbstractGeometryType"/>
      <rdfs:comment>Warning: This class type was declared outside of its original schema. This class may be declared incorrectly.</rdfs:comment>
   </owl:Class>
   <owl:Class rdf:about="#_GeometricPrimitive">
      <rdfs:subClassOf rdf:resource="http://www.opengis.net/gml#_Geometry"/>
      <rdfs:subClassOf rdf:resource="http://www.opengis.net/gml#AbstractGeometricPrimitiveType"/>
      <rdfs:comment>Warning: This class type was declared outside of its original schema. This class may be declared incorrectly.</rdfs:comment>
   </owl:Class>
   <owl:Class rdf:about="#Point">
      <rdfs:subClassOf rdf:resource="http://www.opengis.net/gml#_GeometricPrimitive"/>
      <rdfs:subClassOf rdf:resource="http://www.opengis.net/gml#PointType"/>
      <rdfs:comment>Warning: This class type was declared outside of its original schema. This class may be declared incorrectly.</rdfs:comment>
   </owl:Class>
   <owl:Class rdf:about="#pointProperty">
      <rdfs:subClassOf rdf:resource="http://www.opengis.net/gml#PointPropertyType"/>
      <rdfs:comment>Warning: This class type was declared outside of its original schema. This class may be declared incorrectly.</rdfs:comment>
   </owl:Class>
   <owl:Class rdf:about="#pointRep">
      <rdfs:subClassOf rdf:resource="http://www.opengis.net/gml#PointPropertyType"/>
      <rdfs:comment>Warning: This class type was declared outside of its original schema. This class may be declared incorrectly.</rdfs:comment>
   </owl:Class>
   <owl:Class rdf:about="#pointArrayProperty">
      <rdfs:subClassOf rdf:resource="http://www.opengis.net/gml#PointArrayPropertyType"/>
      <rdfs:comment>Warning: This class type was declared outside of its original schema. This class may be declared incorrectly.</rdfs:comment>
   </owl:Class>
   <owl:Class rdf:about="#_Curve">
      <rdfs:subClassOf rdf:resource="http://www.opengis.net/gml#_GeometricPrimitive"/>
      <rdfs:subClassOf rdf:resource="http://www.opengis.net/gml#AbstractCurveType"/>
      <rdfs:comment>Warning: This class type was declared outside of its original schema. This class may be declared incorrectly.</rdfs:comment>
   </owl:Class>
   <owl:Class rdf:about="#curveProperty">
      <rdfs:subClassOf rdf:resource="http://www.opengis.net/gml#CurvePropertyType"/>
      <rdfs:comment>Warning: This class type was declared outside of its original schema. This class may be declared incorrectly.</rdfs:comment>
   </owl:Class>
   <owl:Class rdf:about="#curveArrayProperty">
      <rdfs:subClassOf rdf:resource="http://www.opengis.net/gml#CurveArrayPropertyType"/>
      <rdfs:comment>Warning: This class type was declared outside of its original schema. This class may be declared incorrectly.</rdfs:comment>
   </owl:Class>
   <owl:Class rdf:about="#LineString">
      <rdfs:subClassOf rdf:resource="http://www.opengis.net/gml#_Curve"/>
      <rdfs:subClassOf rdf:resource="http://www.opengis.net/gml#LineStringType"/>
      <rdfs:comment>Warning: This class type was declared outside of its original schema. This class may be declared incorrectly.</rdfs:comment>
   </owl:Class>
   <owl:Class rdf:about="#pos">
      <rdfs:subClassOf rdf:resource="http://www.opengis.net/gml#DirectPositionType"/>
      <rdfs:comment>Warning: This class type was declared outside of its original schema. This class may be declared incorrectly.</rdfs:comment>
   </owl:Class>
   <owl:Class rdf:about="#posList">
      <rdfs:subClassOf rdf:resource="http://www.opengis.net/gml#DirectPositionListType"/>
      <rdfs:comment>Warning: This class type was declared outside of its original schema. This class may be declared incorrectly.</rdfs:comment>
   </owl:Class>
   <owl:Class rdf:about="#vector">
      <rdfs:subClassOf rdf:resource="http://www.opengis.net/gml#VectorType"/>
      <rdfs:comment>Warning: This class type was declared outside of its original schema. This class may be declared incorrectly.</rdfs:comment>
   </owl:Class>
   <owl:Class rdf:about="#coordinates">
      <rdfs:subClassOf rdf:resource="http://www.opengis.net/gml#CoordinatesType"/>
      <rdfs:comment>Warning: This class type was declared outside of its original schema. This class may be declared incorrectly.</rdfs:comment>
   </owl:Class>
   <owl:Class rdf:about="#Envelope">
      <rdfs:subClassOf rdf:resource="http://www.opengis.net/gml#EnvelopeType"/>
      <rdfs:comment>Warning: This class type was declared outside of its original schema. This class may be declared incorrectly.</rdfs:comment>
   </owl:Class>
   <owl:Class rdf:about="#coord">
      <rdfs:subClassOf rdf:resource="http://www.opengis.net/gml#CoordType"/>
      <rdfs:comment>Warning: This class type was declared outside of its original schema. This class may be declared incorrectly.</rdfs:comment>
   </owl:Class>
   <owl:Class rdf:about="#lineStringProperty">
      <rdfs:subClassOf rdf:resource="http://www.opengis.net/gml#LineStringPropertyType"/>
      <rdfs:comment>Warning: This class type was declared outside of its original schema. This class may be declared incorrectly.</rdfs:comment>
   </owl:Class>
   <owl:ObjectProperty rdf:about="http://www.opengis.net/gml#has_Geometry">
      <rdfs:comment>Warning: This ObjectProperty reference was declared outside of its original schema. This ObjectProperty may be declared incorrectly.</rdfs:comment>
      <rdfs:domain rdf:resource="#GeometryPropertyType"/>
      <rdfs:range rdf:resource="http://www.opengis.net/gml#_Geometry"/>
   </owl:ObjectProperty>
   <owl:ObjectProperty rdf:about="http://www.opengis.net/gml#has_Geometry">
      <rdfs:comment>Warning: This ObjectProperty reference was declared outside of its original schema. This ObjectProperty may be declared incorrectly.</rdfs:comment>
      <rdfs:domain rdf:resource="#GeometryArrayPropertyType"/>
      <rdfs:range rdf:resource="http://www.opengis.net/gml#_Geometry"/>
   </owl:ObjectProperty>
   <owl:ObjectProperty rdf:about="http://www.opengis.net/gml#has_GeometricPrimitive">
      <rdfs:comment>Warning: This ObjectProperty reference was declared outside of its original schema. This ObjectProperty may be declared incorrectly.</rdfs:comment>
      <rdfs:domain rdf:resource="#GeometricPrimitivePropertyType"/>
      <rdfs:range rdf:resource="http://www.opengis.net/gml#_GeometricPrimitive"/>
   </owl:ObjectProperty>
   <owl:ObjectProperty rdf:about="http://www.opengis.net/gml#haspos">
      <rdfs:comment>Warning: This ObjectProperty reference was declared outside of its original schema. This ObjectProperty may be declared incorrectly.</rdfs:comment>
      <rdfs:domain rdf:resource="#PointType"/>
      <rdfs:range rdf:resource="http://www.opengis.net/gml#pos"/>
   </owl:ObjectProperty>
   <owl:ObjectProperty rdf:about="http://www.opengis.net/gml#hascoordinates">
      <rdfs:comment>Warning: This ObjectProperty reference was declared outside of its original schema. This ObjectProperty may be declared incorrectly.</rdfs:comment>
      <rdfs:domain rdf:resource="#PointType"/>
      <rdfs:range rdf:resource="http://www.opengis.net/gml#coordinates"/>
   </owl:ObjectProperty>
   <owl:ObjectProperty rdf:about="http://www.opengis.net/gml#hascoord">
      <rdfs:comment>Warning: This ObjectProperty reference was declared outside of its original schema. This ObjectProperty may be declared incorrectly.</rdfs:comment>
      <rdfs:domain rdf:resource="#PointType"/>
      <rdfs:range rdf:resource="http://www.opengis.net/gml#coord"/>
   </owl:ObjectProperty>
   <owl:ObjectProperty rdf:about="http://www.opengis.net/gml#hasPoint">
      <rdfs:comment>Warning: This ObjectProperty reference was declared outside of its original schema. This ObjectProperty may be declared incorrectly.</rdfs:comment>
      <rdfs:domain rdf:resource="#PointPropertyType"/>
      <rdfs:range rdf:resource="http://www.opengis.net/gml#Point"/>
   </owl:ObjectProperty>
   <owl:ObjectProperty rdf:about="http://www.opengis.net/gml#hasPoint">
      <rdfs:comment>Warning: This ObjectProperty reference was declared outside of its original schema. This ObjectProperty may be declared incorrectly.</rdfs:comment>
      <rdfs:domain rdf:resource="#PointArrayPropertyType"/>
      <rdfs:range rdf:resource="http://www.opengis.net/gml#Point"/>
   </owl:ObjectProperty>
   <owl:ObjectProperty rdf:about="http://www.opengis.net/gml#has_Curve">
      <rdfs:comment>Warning: This ObjectProperty reference was declared outside of its original schema. This ObjectProperty may be declared incorrectly.</rdfs:comment>
      <rdfs:domain rdf:resource="#CurvePropertyType"/>
      <rdfs:range rdf:resource="http://www.opengis.net/gml#_Curve"/>
   </owl:ObjectProperty>
   <owl:ObjectProperty rdf:about="http://www.opengis.net/gml#has_Curve">
      <rdfs:comment>Warning: This ObjectProperty reference was declared outside of its original schema. This ObjectProperty may be declared incorrectly.</rdfs:comment>
      <rdfs:domain rdf:resource="#CurveArrayPropertyType"/>
      <rdfs:range rdf:resource="http://www.opengis.net/gml#_Curve"/>
   </owl:ObjectProperty>
   <owl:ObjectProperty rdf:about="http://www.opengis.net/gml#haspos">
      <rdfs:comment>Warning: This ObjectProperty reference was declared outside of its original schema. This ObjectProperty may be declared incorrectly.</rdfs:comment>
      <rdfs:domain rdf:resource="#LineStringType"/>
      <rdfs:range rdf:resource="http://www.opengis.net/gml#pos"/>
   </owl:ObjectProperty>
   <owl:ObjectProperty rdf:about="http://www.opengis.net/gml#haspointProperty">
      <rdfs:comment>Warning: This ObjectProperty reference was declared outside of its original schema. This ObjectProperty may be declared incorrectly.</rdfs:comment>
      <rdfs:domain rdf:resource="#LineStringType"/>
      <rdfs:range rdf:resource="http://www.opengis.net/gml#pointProperty"/>
   </owl:ObjectProperty>
   <owl:ObjectProperty rdf:about="http://www.opengis.net/gml#haspointRep">
      <rdfs:comment>Warning: This ObjectProperty reference was declared outside of its original schema. This ObjectProperty may be declared incorrectly.</rdfs:comment>
      <rdfs:domain rdf:resource="#LineStringType"/>
      <rdfs:range rdf:resource="http://www.opengis.net/gml#pointRep"/>
   </owl:ObjectProperty>
   <owl:ObjectProperty rdf:about="http://www.opengis.net/gml#hascoord">
      <rdfs:comment>Warning: This ObjectProperty reference was declared outside of its original schema. This ObjectProperty may be declared incorrectly.</rdfs:comment>
      <rdfs:domain rdf:resource="#LineStringType"/>
      <rdfs:range rdf:resource="http://www.opengis.net/gml#coord"/>
   </owl:ObjectProperty>
   <owl:ObjectProperty rdf:about="http://www.opengis.net/gml#hasposList">
      <rdfs:comment>Warning: This ObjectProperty reference was declared outside of its original schema. This ObjectProperty may be declared incorrectly.</rdfs:comment>
      <rdfs:domain rdf:resource="#LineStringType"/>
      <rdfs:range rdf:resource="http://www.opengis.net/gml#posList"/>
   </owl:ObjectProperty>
   <owl:ObjectProperty rdf:about="http://www.opengis.net/gml#hascoordinates">
      <rdfs:comment>Warning: This ObjectProperty reference was declared outside of its original schema. This ObjectProperty may be declared incorrectly.</rdfs:comment>
      <rdfs:domain rdf:resource="#LineStringType"/>
      <rdfs:range rdf:resource="http://www.opengis.net/gml#coordinates"/>
   </owl:ObjectProperty>
   <owl:ObjectProperty rdf:about="http://www.opengis.net/gml#haspos">
      <rdfs:comment>Warning: This ObjectProperty reference was declared outside of its original schema. This ObjectProperty may be declared incorrectly.</rdfs:comment>
      <rdfs:domain rdf:resource="#geometricPositionGroup"/>
      <rdfs:range rdf:resource="http://www.opengis.net/gml#pos"/>
   </owl:ObjectProperty>
   <owl:ObjectProperty rdf:about="http://www.opengis.net/gml#haspointProperty">
      <rdfs:comment>Warning: This ObjectProperty reference was declared outside of its original schema. This ObjectProperty may be declared incorrectly.</rdfs:comment>
      <rdfs:domain rdf:resource="#geometricPositionGroup"/>
      <rdfs:range rdf:resource="http://www.opengis.net/gml#pointProperty"/>
   </owl:ObjectProperty>
   <owl:ObjectProperty rdf:about="http://www.opengis.net/gml#hasposList">
      <rdfs:comment>Warning: This ObjectProperty reference was declared outside of its original schema. This ObjectProperty may be declared incorrectly.</rdfs:comment>
      <rdfs:domain rdf:resource="#geometricPositionListGroup"/>
      <rdfs:range rdf:resource="http://www.opengis.net/gml#posList"/>
   </owl:ObjectProperty>
   <owl:ObjectProperty rdf:about="#lowerCorner">
      <rdfs:comment>Warning: This ObjectProperty type was declared outside of its original schema. This ObjectProperty may be declared incorrectly.</rdfs:comment>
      <rdfs:domain rdf:resource="#EnvelopeType"/>
      <rdfs:range rdf:resource="http://www.opengis.net/gml#DirectPositionType"/>
   </owl:ObjectProperty>
   <owl:ObjectProperty rdf:about="#upperCorner">
      <rdfs:comment>Warning: This ObjectProperty type was declared outside of its original schema. This ObjectProperty may be declared incorrectly.</rdfs:comment>
      <rdfs:domain rdf:resource="#EnvelopeType"/>
      <rdfs:range rdf:resource="http://www.opengis.net/gml#DirectPositionType"/>
   </owl:ObjectProperty>
   <owl:ObjectProperty rdf:about="http://www.opengis.net/gml#hascoord">
      <rdfs:comment>Warning: This ObjectProperty reference was declared outside of its original schema. This ObjectProperty may be declared incorrectly.</rdfs:comment>
      <rdfs:domain rdf:resource="#EnvelopeType"/>
      <rdfs:range rdf:resource="http://www.opengis.net/gml#coord"/>
   </owl:ObjectProperty>
   <owl:ObjectProperty rdf:about="http://www.opengis.net/gml#haspos">
      <rdfs:comment>Warning: This ObjectProperty reference was declared outside of its original schema. This ObjectProperty may be declared incorrectly.</rdfs:comment>
      <rdfs:domain rdf:resource="#EnvelopeType"/>
      <rdfs:range rdf:resource="http://www.opengis.net/gml#pos"/>
   </owl:ObjectProperty>
   <owl:ObjectProperty rdf:about="http://www.opengis.net/gml#hascoordinates">
      <rdfs:comment>Warning: This ObjectProperty reference was declared outside of its original schema. This ObjectProperty may be declared incorrectly.</rdfs:comment>
      <rdfs:domain rdf:resource="#EnvelopeType"/>
      <rdfs:range rdf:resource="http://www.opengis.net/gml#coordinates"/>
   </owl:ObjectProperty>
   <owl:DatatypeProperty rdf:about="#X">
      <rdfs:domain rdf:resource="#CoordType"/>
      <rdfs:range rdf:resource="http://www.w3.org/2001/XMLSchema#decimal"/>
   </owl:DatatypeProperty>
   <owl:DatatypeProperty rdf:about="#Y">
      <rdfs:domain rdf:resource="#CoordType"/>
      <rdfs:range rdf:resource="http://www.w3.org/2001/XMLSchema#decimal"/>
   </owl:DatatypeProperty>
   <owl:DatatypeProperty rdf:about="#Z">
      <rdfs:domain rdf:resource="#CoordType"/>
      <rdfs:range rdf:resource="http://www.w3.org/2001/XMLSchema#decimal"/>
   </owl:DatatypeProperty>
   <owl:ObjectProperty rdf:about="http://www.opengis.net/gml#hasLineString">
      <rdfs:comment>Warning: This ObjectProperty reference was declared outside of its original schema. This ObjectProperty may be declared incorrectly.</rdfs:comment>
      <rdfs:domain rdf:resource="#LineStringPropertyType"/>
      <rdfs:range rdf:resource="http://www.opengis.net/gml#LineString"/>
   </owl:ObjectProperty>
</rdf:RDF>
