<rdf:RDF xmlns:math="http://www.w3.org/2005/xpath-functions/math" xmlns:owl="http://www.w3.org/2002/07/owl#" xmlns:rdf="http://www.w3.org/1999/02/22-rdf-syntax-ns#" xmlns:rdfs="http://www.w3.org/2000/01/rdf-schema#" xmlns:xs="http://www.w3.org/2001/XMLSchema" xmlns:xsd="http://www.w3.org/2001/XMLSchema">
   <owl:Ontology rdf:about="http://liris.cnrs.fr/ontologies/geometryAggregates">
      <owl:imports rdf:resource="http://liris.cnrs.fr/ontologies/gml"/>
      <owl:imports rdf:resource="http://liris.cnrs.fr/ontologies/geometryPrimitives"/>
      <rdfs:comment>geometryAggregates.xsd</rdfs:comment>
      <rdfs:seeAlso>urn:opengis:specification:gml:schema-xsd:geometryAggregates:3.1.1</rdfs:seeAlso>
      <rdfs:comment>
			GML is an OGC Standard.
			Copyright (c) 2001,2005,2010 Open Geospatial Consortium.
			To obtain additional rights of use, visit http://www.opengeospatial.org/legal/ .
		</rdfs:comment>
   </owl:Ontology>
   <owl:Class rdf:about="http://www.opengis.net/gml#AbstractGeometricAggregateType">
      <rdfs:comment>This is an abstract class</rdfs:comment>
      <rdfs:comment>This is the abstract root type of the geometric aggregates.</rdfs:comment>
   </owl:Class>
   <owl:Class rdf:about="http://www.opengis.net/gml#MultiGeometryType">
      <rdfs:comment>A geometry collection must include one or more geometries, referenced through geometryMember elements.</rdfs:comment>
      <rdfs:subClassOf>
         <owl:Class>
            <owl:intersectionOf rdf:parseType="Collection">
               <owl:Restriction>
                  <owl:onProperty rdf:resource="http://www.opengis.net/gml#hasgeometryMember"/>
                  <owl:allValuesFrom rdf:resource="http://www.opengis.net/gml#geometryMember"/>
               </owl:Restriction>
               <owl:Restriction>
                  <owl:onProperty rdf:resource="http://www.opengis.net/gml#hasgeometryMember"/>
                  <owl:minCardinality rdf:datatype="http://www.w3.org/2001/XMLSchema#nonNegativeInteger">0</owl:minCardinality>
               </owl:Restriction>
               <owl:Restriction>
                  <owl:onProperty rdf:resource="http://www.opengis.net/gml#hasgeometryMembers"/>
                  <owl:allValuesFrom rdf:resource="http://www.opengis.net/gml#geometryMembers"/>
               </owl:Restriction>
               <owl:Restriction>
                  <owl:onProperty rdf:resource="http://www.opengis.net/gml#hasgeometryMembers"/>
                  <owl:minCardinality rdf:datatype="http://www.w3.org/2001/XMLSchema#nonNegativeInteger">0</owl:minCardinality>
               </owl:Restriction>
            </owl:intersectionOf>
         </owl:Class>
      </rdfs:subClassOf>
      <rdfs:subClassOf rdf:resource="http://www.opengis.net/gml#AbstractGeometricAggregateType"/>
   </owl:Class>
   <owl:Class rdf:about="http://www.opengis.net/gml#MultiGeometryPropertyType">
      <rdfs:comment>A property that has a geometric aggregate as its value domain can either be an appropriate geometry element encapsulated in an element of this type or an XLink reference to a remote geometry element (where remote includes geometry elements located elsewhere in the same document). Either the reference or the contained element must be given, but neither both nor none.</rdfs:comment>
      <rdfs:subClassOf>
         <owl:Class>
            <owl:intersectionOf rdf:parseType="Collection">
               <owl:Restriction>
                  <owl:onProperty rdf:resource="http://www.opengis.net/gml#has_GeometricAggregate"/>
                  <owl:allValuesFrom rdf:resource="http://www.opengis.net/gml#_GeometricAggregate"/>
               </owl:Restriction>
            </owl:intersectionOf>
         </owl:Class>
      </rdfs:subClassOf>
   </owl:Class>
   <owl:Class rdf:about="http://www.opengis.net/gml#MultiPointType">
      <rdfs:comment>A MultiPoint is defined by one or more Points, referenced through pointMember elements.</rdfs:comment>
      <rdfs:subClassOf>
         <owl:Class>
            <owl:intersectionOf rdf:parseType="Collection">
               <owl:Restriction>
                  <owl:onProperty rdf:resource="http://www.opengis.net/gml#haspointMember"/>
                  <owl:allValuesFrom rdf:resource="http://www.opengis.net/gml#pointMember"/>
               </owl:Restriction>
               <owl:Restriction>
                  <owl:onProperty rdf:resource="http://www.opengis.net/gml#haspointMember"/>
                  <owl:minCardinality rdf:datatype="http://www.w3.org/2001/XMLSchema#nonNegativeInteger">0</owl:minCardinality>
               </owl:Restriction>
               <owl:Restriction>
                  <owl:onProperty rdf:resource="http://www.opengis.net/gml#haspointMembers"/>
                  <owl:allValuesFrom rdf:resource="http://www.opengis.net/gml#pointMembers"/>
               </owl:Restriction>
               <owl:Restriction>
                  <owl:onProperty rdf:resource="http://www.opengis.net/gml#haspointMembers"/>
                  <owl:minCardinality rdf:datatype="http://www.w3.org/2001/XMLSchema#nonNegativeInteger">0</owl:minCardinality>
               </owl:Restriction>
            </owl:intersectionOf>
         </owl:Class>
      </rdfs:subClassOf>
      <rdfs:subClassOf rdf:resource="http://www.opengis.net/gml#AbstractGeometricAggregateType"/>
   </owl:Class>
   <owl:Class rdf:about="http://www.opengis.net/gml#MultiPointPropertyType">
      <rdfs:comment>A property that has a collection of points as its value domain can either be an appropriate geometry element encapsulated in an element of this type or an XLink reference to a remote geometry element (where remote includes geometry elements located elsewhere in the same document). Either the reference or the contained element must be given, but neither both nor none.</rdfs:comment>
      <rdfs:subClassOf>
         <owl:Class>
            <owl:intersectionOf rdf:parseType="Collection">
               <owl:Restriction>
                  <owl:onProperty rdf:resource="http://www.opengis.net/gml#hasMultiPoint"/>
                  <owl:allValuesFrom rdf:resource="http://www.opengis.net/gml#MultiPoint"/>
               </owl:Restriction>
            </owl:intersectionOf>
         </owl:Class>
      </rdfs:subClassOf>
   </owl:Class>
   <owl:Class rdf:about="http://www.opengis.net/gml#MultiCurveType">
      <rdfs:comment>A MultiCurve is defined by one or more Curves, referenced through curveMember elements.</rdfs:comment>
      <rdfs:subClassOf>
         <owl:Class>
            <owl:intersectionOf rdf:parseType="Collection">
               <owl:Restriction>
                  <owl:onProperty rdf:resource="http://www.opengis.net/gml#hascurveMember"/>
                  <owl:allValuesFrom rdf:resource="http://www.opengis.net/gml#curveMember"/>
               </owl:Restriction>
               <owl:Restriction>
                  <owl:onProperty rdf:resource="http://www.opengis.net/gml#hascurveMember"/>
                  <owl:minCardinality rdf:datatype="http://www.w3.org/2001/XMLSchema#nonNegativeInteger">0</owl:minCardinality>
               </owl:Restriction>
               <owl:Restriction>
                  <owl:onProperty rdf:resource="http://www.opengis.net/gml#hascurveMembers"/>
                  <owl:allValuesFrom rdf:resource="http://www.opengis.net/gml#curveMembers"/>
               </owl:Restriction>
               <owl:Restriction>
                  <owl:onProperty rdf:resource="http://www.opengis.net/gml#hascurveMembers"/>
                  <owl:minCardinality rdf:datatype="http://www.w3.org/2001/XMLSchema#nonNegativeInteger">0</owl:minCardinality>
               </owl:Restriction>
            </owl:intersectionOf>
         </owl:Class>
      </rdfs:subClassOf>
      <rdfs:subClassOf rdf:resource="http://www.opengis.net/gml#AbstractGeometricAggregateType"/>
   </owl:Class>
   <owl:Class rdf:about="http://www.opengis.net/gml#MultiCurvePropertyType">
      <rdfs:comment>A property that has a collection of curves as its value domain can either be an appropriate geometry element encapsulated in an element of this type or an XLink reference to a remote geometry element (where remote includes geometry elements located elsewhere in the same document). Either the reference or the contained element must be given, but neither both nor none.</rdfs:comment>
      <rdfs:subClassOf>
         <owl:Class>
            <owl:intersectionOf rdf:parseType="Collection">
               <owl:Restriction>
                  <owl:onProperty rdf:resource="http://www.opengis.net/gml#hasMultiCurve"/>
                  <owl:allValuesFrom rdf:resource="http://www.opengis.net/gml#MultiCurve"/>
               </owl:Restriction>
            </owl:intersectionOf>
         </owl:Class>
      </rdfs:subClassOf>
   </owl:Class>
   <owl:Class rdf:about="http://www.opengis.net/gml#MultiSurfaceType">
      <rdfs:comment>A MultiSurface is defined by one or more Surfaces, referenced through surfaceMember elements.</rdfs:comment>
      <rdfs:subClassOf>
         <owl:Class>
            <owl:intersectionOf rdf:parseType="Collection">
               <owl:Restriction>
                  <owl:onProperty rdf:resource="http://www.opengis.net/gml#hassurfaceMember"/>
                  <owl:allValuesFrom rdf:resource="http://www.opengis.net/gml#surfaceMember"/>
               </owl:Restriction>
               <owl:Restriction>
                  <owl:onProperty rdf:resource="http://www.opengis.net/gml#hassurfaceMember"/>
                  <owl:minCardinality rdf:datatype="http://www.w3.org/2001/XMLSchema#nonNegativeInteger">0</owl:minCardinality>
               </owl:Restriction>
               <owl:Restriction>
                  <owl:onProperty rdf:resource="http://www.opengis.net/gml#hassurfaceMembers"/>
                  <owl:allValuesFrom rdf:resource="http://www.opengis.net/gml#surfaceMembers"/>
               </owl:Restriction>
               <owl:Restriction>
                  <owl:onProperty rdf:resource="http://www.opengis.net/gml#hassurfaceMembers"/>
                  <owl:minCardinality rdf:datatype="http://www.w3.org/2001/XMLSchema#nonNegativeInteger">0</owl:minCardinality>
               </owl:Restriction>
            </owl:intersectionOf>
         </owl:Class>
      </rdfs:subClassOf>
      <rdfs:subClassOf rdf:resource="http://www.opengis.net/gml#AbstractGeometricAggregateType"/>
   </owl:Class>
   <owl:Class rdf:about="http://www.opengis.net/gml#MultiSurfacePropertyType">
      <rdfs:comment>A property that has a collection of surfaces as its value domain can either be an appropriate geometry element encapsulated in an element of this type or an XLink reference to a remote geometry element (where remote includes geometry elements located elsewhere in the same document). Either the reference or the contained element must be given, but neither both nor none.</rdfs:comment>
      <rdfs:subClassOf>
         <owl:Class>
            <owl:intersectionOf rdf:parseType="Collection">
               <owl:Restriction>
                  <owl:onProperty rdf:resource="http://www.opengis.net/gml#hasMultiSurface"/>
                  <owl:allValuesFrom rdf:resource="http://www.opengis.net/gml#MultiSurface"/>
               </owl:Restriction>
            </owl:intersectionOf>
         </owl:Class>
      </rdfs:subClassOf>
   </owl:Class>
   <owl:Class rdf:about="http://www.opengis.net/gml#MultiSolidType">
      <rdfs:comment>A MultiSolid is defined by one or more Solids, referenced through solidMember elements.</rdfs:comment>
      <rdfs:subClassOf>
         <owl:Class>
            <owl:intersectionOf rdf:parseType="Collection">
               <owl:Restriction>
                  <owl:onProperty rdf:resource="http://www.opengis.net/gml#hassolidMember"/>
                  <owl:allValuesFrom rdf:resource="http://www.opengis.net/gml#solidMember"/>
               </owl:Restriction>
               <owl:Restriction>
                  <owl:onProperty rdf:resource="http://www.opengis.net/gml#hassolidMember"/>
                  <owl:minCardinality rdf:datatype="http://www.w3.org/2001/XMLSchema#nonNegativeInteger">0</owl:minCardinality>
               </owl:Restriction>
               <owl:Restriction>
                  <owl:onProperty rdf:resource="http://www.opengis.net/gml#hassolidMembers"/>
                  <owl:allValuesFrom rdf:resource="http://www.opengis.net/gml#solidMembers"/>
               </owl:Restriction>
               <owl:Restriction>
                  <owl:onProperty rdf:resource="http://www.opengis.net/gml#hassolidMembers"/>
                  <owl:minCardinality rdf:datatype="http://www.w3.org/2001/XMLSchema#nonNegativeInteger">0</owl:minCardinality>
               </owl:Restriction>
            </owl:intersectionOf>
         </owl:Class>
      </rdfs:subClassOf>
      <rdfs:subClassOf rdf:resource="http://www.opengis.net/gml#AbstractGeometricAggregateType"/>
   </owl:Class>
   <owl:Class rdf:about="http://www.opengis.net/gml#MultiSolidPropertyType">
      <rdfs:comment>A property that has a collection of solids as its value domain can either be an appropriate geometry element encapsulated in an element of this type or an XLink reference to a remote geometry element (where remote includes geometry elements located elsewhere in the same document). Either the reference or the contained element must be given, but neither both nor none.</rdfs:comment>
      <rdfs:subClassOf>
         <owl:Class>
            <owl:intersectionOf rdf:parseType="Collection">
               <owl:Restriction>
                  <owl:onProperty rdf:resource="http://www.opengis.net/gml#hasMultiSolid"/>
                  <owl:allValuesFrom rdf:resource="http://www.opengis.net/gml#MultiSolid"/>
               </owl:Restriction>
            </owl:intersectionOf>
         </owl:Class>
      </rdfs:subClassOf>
   </owl:Class>
   <owl:Class rdf:about="http://www.opengis.net/gml#MultiLineStringType">
      <rdfs:comment>A MultiLineString is defined by one or more LineStrings, referenced through lineStringMember elements. Deprecated with GML version 3.0. Use MultiCurveType instead.</rdfs:comment>
      <rdfs:subClassOf>
         <owl:Class>
            <owl:intersectionOf rdf:parseType="Collection">
               <owl:Restriction>
                  <owl:onProperty rdf:resource="http://www.opengis.net/gml#haslineStringMember"/>
                  <owl:allValuesFrom rdf:resource="http://www.opengis.net/gml#lineStringMember"/>
               </owl:Restriction>
               <owl:Restriction>
                  <owl:onProperty rdf:resource="http://www.opengis.net/gml#haslineStringMember"/>
                  <owl:minCardinality rdf:datatype="http://www.w3.org/2001/XMLSchema#nonNegativeInteger">0</owl:minCardinality>
               </owl:Restriction>
            </owl:intersectionOf>
         </owl:Class>
      </rdfs:subClassOf>
      <rdfs:subClassOf rdf:resource="http://www.opengis.net/gml#AbstractGeometricAggregateType"/>
   </owl:Class>
   <owl:Class rdf:about="http://www.opengis.net/gml#MultiLineStringPropertyType">
      <rdfs:comment>This type is deprecated with GML 3 and shall not be used. It is included for backwards compatibility with GML 2. Use MultiCurvePropertyType instead.
A property that has a collection of line strings as its value domain can either be an appropriate geometry element encapsulated in an element of this type or an XLink reference to a remote geometry element (where remote includes geometry elements located elsewhere in the same document). Either the reference or the contained element must be given, but neither both nor none.</rdfs:comment>
      <rdfs:subClassOf>
         <owl:Class>
            <owl:intersectionOf rdf:parseType="Collection">
               <owl:Restriction>
                  <owl:onProperty rdf:resource="http://www.opengis.net/gml#hasMultiLineString"/>
                  <owl:allValuesFrom rdf:resource="http://www.opengis.net/gml#MultiLineString"/>
               </owl:Restriction>
            </owl:intersectionOf>
         </owl:Class>
      </rdfs:subClassOf>
   </owl:Class>
   <owl:Class rdf:about="http://www.opengis.net/gml#MultiPolygonType">
      <rdfs:comment>A MultiPolygon is defined by one or more Polygons, referenced through polygonMember elements. Deprecated with GML version 3.0. Use MultiSurfaceType instead.</rdfs:comment>
      <rdfs:subClassOf>
         <owl:Class>
            <owl:intersectionOf rdf:parseType="Collection">
               <owl:Restriction>
                  <owl:onProperty rdf:resource="http://www.opengis.net/gml#haspolygonMember"/>
                  <owl:allValuesFrom rdf:resource="http://www.opengis.net/gml#polygonMember"/>
               </owl:Restriction>
               <owl:Restriction>
                  <owl:onProperty rdf:resource="http://www.opengis.net/gml#haspolygonMember"/>
                  <owl:minCardinality rdf:datatype="http://www.w3.org/2001/XMLSchema#nonNegativeInteger">0</owl:minCardinality>
               </owl:Restriction>
            </owl:intersectionOf>
         </owl:Class>
      </rdfs:subClassOf>
      <rdfs:subClassOf rdf:resource="http://www.opengis.net/gml#AbstractGeometricAggregateType"/>
   </owl:Class>
   <owl:Class rdf:about="http://www.opengis.net/gml#MultiPolygonPropertyType">
      <rdfs:comment>This type is deprecated with GML 3 and shall not be used. It is included for backwards compatibility with GML 2. Use MultiSurfacePropertyType instead.

A property that has a collection of polygons as its value domain can either be an appropriate geometry element encapsulated in an element of this type or an XLink reference to a remote geometry element (where remote includes geometry elements located elsewhere in the same document). Either the reference or the contained element must be given, but neither both nor none.</rdfs:comment>
      <rdfs:subClassOf>
         <owl:Class>
            <owl:intersectionOf rdf:parseType="Collection">
               <owl:Restriction>
                  <owl:onProperty rdf:resource="http://www.opengis.net/gml#hasMultiPolygon"/>
                  <owl:allValuesFrom rdf:resource="http://www.opengis.net/gml#MultiPolygon"/>
               </owl:Restriction>
            </owl:intersectionOf>
         </owl:Class>
      </rdfs:subClassOf>
   </owl:Class>
   <owl:Class rdf:about="http://www.opengis.net/gml#_GeometricAggregate">
      <rdfs:subClassOf rdf:resource="http://www.opengis.net/gml#_Geometry"/>
      <rdfs:subClassOf rdf:resource="http://www.opengis.net/gml#AbstractGeometricAggregateType"/>
   </owl:Class>
   <owl:Class rdf:about="http://www.opengis.net/gml#MultiGeometry">
      <rdfs:subClassOf rdf:resource="http://www.opengis.net/gml#_GeometricAggregate"/>
      <rdfs:subClassOf rdf:resource="http://www.opengis.net/gml#MultiGeometryType"/>
   </owl:Class>
   <owl:Class rdf:about="http://www.opengis.net/gml#multiGeometryProperty">
      <rdfs:subClassOf rdf:resource="http://www.opengis.net/gml#MultiGeometryPropertyType"/>
   </owl:Class>
   <owl:Class rdf:about="http://www.opengis.net/gml#MultiPoint">
      <rdfs:subClassOf rdf:resource="http://www.opengis.net/gml#_GeometricAggregate"/>
      <rdfs:subClassOf rdf:resource="http://www.opengis.net/gml#MultiPointType"/>
   </owl:Class>
   <owl:Class rdf:about="http://www.opengis.net/gml#multiPointProperty">
      <rdfs:subClassOf rdf:resource="http://www.opengis.net/gml#MultiPointPropertyType"/>
   </owl:Class>
   <owl:Class rdf:about="http://www.opengis.net/gml#MultiCurve">
      <rdfs:subClassOf rdf:resource="http://www.opengis.net/gml#_GeometricAggregate"/>
      <rdfs:subClassOf rdf:resource="http://www.opengis.net/gml#MultiCurveType"/>
   </owl:Class>
   <owl:Class rdf:about="http://www.opengis.net/gml#multiCurveProperty">
      <rdfs:subClassOf rdf:resource="http://www.opengis.net/gml#MultiCurvePropertyType"/>
   </owl:Class>
   <owl:Class rdf:about="http://www.opengis.net/gml#MultiSurface">
      <rdfs:subClassOf rdf:resource="http://www.opengis.net/gml#_GeometricAggregate"/>
      <rdfs:subClassOf rdf:resource="http://www.opengis.net/gml#MultiSurfaceType"/>
   </owl:Class>
   <owl:Class rdf:about="http://www.opengis.net/gml#multiSurfaceProperty">
      <rdfs:subClassOf rdf:resource="http://www.opengis.net/gml#MultiSurfacePropertyType"/>
   </owl:Class>
   <owl:Class rdf:about="http://www.opengis.net/gml#MultiSolid">
      <rdfs:subClassOf rdf:resource="http://www.opengis.net/gml#_GeometricAggregate"/>
      <rdfs:subClassOf rdf:resource="http://www.opengis.net/gml#MultiSolidType"/>
   </owl:Class>
   <owl:Class rdf:about="http://www.opengis.net/gml#multiSolidProperty">
      <rdfs:subClassOf rdf:resource="http://www.opengis.net/gml#MultiSolidPropertyType"/>
   </owl:Class>
   <owl:Class rdf:about="http://www.opengis.net/gml#MultiPolygon">
      <rdfs:subClassOf rdf:resource="http://www.opengis.net/gml#_GeometricAggregate"/>
      <rdfs:subClassOf rdf:resource="http://www.opengis.net/gml#MultiPolygonType"/>
   </owl:Class>
   <owl:Class rdf:about="http://www.opengis.net/gml#MultiLineString">
      <rdfs:subClassOf rdf:resource="http://www.opengis.net/gml#_GeometricAggregate"/>
      <rdfs:subClassOf rdf:resource="http://www.opengis.net/gml#MultiLineStringType"/>
   </owl:Class>
   <owl:Class rdf:about="http://www.opengis.net/gml#geometryMember">
      <rdfs:subClassOf rdf:resource="GeometryPropertyType"/>
      <rdfs:comment>Warning: This class type was declared outside of its original schema. This class may be declared incorrectly.</rdfs:comment>
   </owl:Class>
   <owl:Class rdf:about="http://www.opengis.net/gml#geometryMembers">
      <rdfs:subClassOf rdf:resource="GeometryArrayPropertyType"/>
      <rdfs:comment>Warning: This class type was declared outside of its original schema. This class may be declared incorrectly.</rdfs:comment>
   </owl:Class>
   <owl:Class rdf:about="http://www.opengis.net/gml#pointMember">
      <rdfs:subClassOf rdf:resource="PointPropertyType"/>
      <rdfs:comment>Warning: This class type was declared outside of its original schema. This class may be declared incorrectly.</rdfs:comment>
   </owl:Class>
   <owl:Class rdf:about="http://www.opengis.net/gml#pointMembers">
      <rdfs:subClassOf rdf:resource="PointArrayPropertyType"/>
      <rdfs:comment>Warning: This class type was declared outside of its original schema. This class may be declared incorrectly.</rdfs:comment>
   </owl:Class>
   <owl:Class rdf:about="http://www.opengis.net/gml#curveMembers">
      <rdfs:subClassOf rdf:resource="CurveArrayPropertyType"/>
      <rdfs:comment>Warning: This class type was declared outside of its original schema. This class may be declared incorrectly.</rdfs:comment>
   </owl:Class>
   <owl:Class rdf:about="http://www.opengis.net/gml#surfaceMember">
      <rdfs:subClassOf rdf:resource="SurfacePropertyType"/>
      <rdfs:comment>Warning: This class type was declared outside of its original schema. This class may be declared incorrectly.</rdfs:comment>
   </owl:Class>
   <owl:Class rdf:about="http://www.opengis.net/gml#surfaceMembers">
      <rdfs:subClassOf rdf:resource="SurfaceArrayPropertyType"/>
      <rdfs:comment>Warning: This class type was declared outside of its original schema. This class may be declared incorrectly.</rdfs:comment>
   </owl:Class>
   <owl:Class rdf:about="http://www.opengis.net/gml#solidMember">
      <rdfs:subClassOf rdf:resource="SolidPropertyType"/>
      <rdfs:comment>Warning: This class type was declared outside of its original schema. This class may be declared incorrectly.</rdfs:comment>
   </owl:Class>
   <owl:Class rdf:about="http://www.opengis.net/gml#solidMembers">
      <rdfs:subClassOf rdf:resource="SolidArrayPropertyType"/>
      <rdfs:comment>Warning: This class type was declared outside of its original schema. This class may be declared incorrectly.</rdfs:comment>
   </owl:Class>
   <owl:Class rdf:about="http://www.opengis.net/gml#multiCenterOf">
      <rdfs:subClassOf rdf:resource="http://www.opengis.net/gml#MultiPointPropertyType"/>
   </owl:Class>
   <owl:Class rdf:about="http://www.opengis.net/gml#multiPosition">
      <rdfs:subClassOf rdf:resource="http://www.opengis.net/gml#MultiPointPropertyType"/>
   </owl:Class>
   <owl:Class rdf:about="http://www.opengis.net/gml#multiCenterLineOf">
      <rdfs:subClassOf rdf:resource="http://www.opengis.net/gml#MultiCurvePropertyType"/>
   </owl:Class>
   <owl:Class rdf:about="http://www.opengis.net/gml#multiEdgeOf">
      <rdfs:subClassOf rdf:resource="http://www.opengis.net/gml#MultiCurvePropertyType"/>
   </owl:Class>
   <owl:Class rdf:about="http://www.opengis.net/gml#multiCoverage">
      <rdfs:subClassOf rdf:resource="http://www.opengis.net/gml#MultiSurfacePropertyType"/>
   </owl:Class>
   <owl:Class rdf:about="http://www.opengis.net/gml#multiExtentOf">
      <rdfs:subClassOf rdf:resource="http://www.opengis.net/gml#MultiSurfacePropertyType"/>
   </owl:Class>
   <owl:Class rdf:about="http://www.opengis.net/gml#multiLocation">
      <rdfs:subClassOf rdf:resource="http://www.opengis.net/gml#MultiPointPropertyType"/>
   </owl:Class>
   <owl:Class rdf:about="http://www.opengis.net/gml#lineStringMember">
      <rdfs:subClassOf rdf:resource="LineStringPropertyType"/>
      <rdfs:comment>Warning: This class type was declared outside of its original schema. This class may be declared incorrectly.</rdfs:comment>
   </owl:Class>
   <owl:Class rdf:about="http://www.opengis.net/gml#polygonMember">
      <rdfs:subClassOf rdf:resource="PolygonPropertyType"/>
      <rdfs:comment>Warning: This class type was declared outside of its original schema. This class may be declared incorrectly.</rdfs:comment>
   </owl:Class>
   <owl:ObjectProperty rdf:about="http://www.opengis.net/gml#hasgeometryMember">
      <rdfs:comment>Warning: This ObjectProperty reference was declared outside of its original schema. This ObjectProperty may be declared incorrectly.</rdfs:comment>
      <rdfs:domain rdf:resource="http://www.opengis.net/gml#MultiGeometryType"/>
      <rdfs:range rdf:resource="http://www.opengis.net/gml#geometryMember"/>
   </owl:ObjectProperty>
   <owl:ObjectProperty rdf:about="http://www.opengis.net/gml#hasgeometryMembers">
      <rdfs:comment>Warning: This ObjectProperty reference was declared outside of its original schema. This ObjectProperty may be declared incorrectly.</rdfs:comment>
      <rdfs:domain rdf:resource="http://www.opengis.net/gml#MultiGeometryType"/>
      <rdfs:range rdf:resource="http://www.opengis.net/gml#geometryMembers"/>
   </owl:ObjectProperty>
   <owl:ObjectProperty rdf:about="http://www.opengis.net/gml#has_GeometricAggregate">
      <rdfs:comment>Warning: This ObjectProperty reference was declared outside of its original schema. This ObjectProperty may be declared incorrectly.</rdfs:comment>
      <rdfs:domain rdf:resource="http://www.opengis.net/gml#MultiGeometryPropertyType"/>
      <rdfs:range rdf:resource="http://www.opengis.net/gml#_GeometricAggregate"/>
   </owl:ObjectProperty>
   <owl:ObjectProperty rdf:about="http://www.opengis.net/gml#haspointMember">
      <rdfs:comment>Warning: This ObjectProperty reference was declared outside of its original schema. This ObjectProperty may be declared incorrectly.</rdfs:comment>
      <rdfs:domain rdf:resource="http://www.opengis.net/gml#MultiPointType"/>
      <rdfs:range rdf:resource="http://www.opengis.net/gml#pointMember"/>
   </owl:ObjectProperty>
   <owl:ObjectProperty rdf:about="http://www.opengis.net/gml#haspointMembers">
      <rdfs:comment>Warning: This ObjectProperty reference was declared outside of its original schema. This ObjectProperty may be declared incorrectly.</rdfs:comment>
      <rdfs:domain rdf:resource="http://www.opengis.net/gml#MultiPointType"/>
      <rdfs:range rdf:resource="http://www.opengis.net/gml#pointMembers"/>
   </owl:ObjectProperty>
   <owl:ObjectProperty rdf:about="http://www.opengis.net/gml#hasMultiPoint">
      <rdfs:comment>Warning: This ObjectProperty reference was declared outside of its original schema. This ObjectProperty may be declared incorrectly.</rdfs:comment>
      <rdfs:domain rdf:resource="http://www.opengis.net/gml#MultiPointPropertyType"/>
      <rdfs:range rdf:resource="http://www.opengis.net/gml#MultiPoint"/>
   </owl:ObjectProperty>
   <owl:ObjectProperty rdf:about="http://www.opengis.net/gml#hascurveMember">
      <rdfs:comment>Warning: This ObjectProperty reference was declared outside of its original schema. This ObjectProperty may be declared incorrectly.</rdfs:comment>
      <rdfs:domain rdf:resource="http://www.opengis.net/gml#MultiCurveType"/>
      <rdfs:range rdf:resource="http://www.opengis.net/gml#curveMember"/>
   </owl:ObjectProperty>
   <owl:ObjectProperty rdf:about="http://www.opengis.net/gml#hascurveMembers">
      <rdfs:comment>Warning: This ObjectProperty reference was declared outside of its original schema. This ObjectProperty may be declared incorrectly.</rdfs:comment>
      <rdfs:domain rdf:resource="http://www.opengis.net/gml#MultiCurveType"/>
      <rdfs:range rdf:resource="http://www.opengis.net/gml#curveMembers"/>
   </owl:ObjectProperty>
   <owl:ObjectProperty rdf:about="http://www.opengis.net/gml#hasMultiCurve">
      <rdfs:comment>Warning: This ObjectProperty reference was declared outside of its original schema. This ObjectProperty may be declared incorrectly.</rdfs:comment>
      <rdfs:domain rdf:resource="http://www.opengis.net/gml#MultiCurvePropertyType"/>
      <rdfs:range rdf:resource="http://www.opengis.net/gml#MultiCurve"/>
   </owl:ObjectProperty>
   <owl:ObjectProperty rdf:about="http://www.opengis.net/gml#hassurfaceMember">
      <rdfs:comment>Warning: This ObjectProperty reference was declared outside of its original schema. This ObjectProperty may be declared incorrectly.</rdfs:comment>
      <rdfs:domain rdf:resource="http://www.opengis.net/gml#MultiSurfaceType"/>
      <rdfs:range rdf:resource="http://www.opengis.net/gml#surfaceMember"/>
   </owl:ObjectProperty>
   <owl:ObjectProperty rdf:about="http://www.opengis.net/gml#hassurfaceMembers">
      <rdfs:comment>Warning: This ObjectProperty reference was declared outside of its original schema. This ObjectProperty may be declared incorrectly.</rdfs:comment>
      <rdfs:domain rdf:resource="http://www.opengis.net/gml#MultiSurfaceType"/>
      <rdfs:range rdf:resource="http://www.opengis.net/gml#surfaceMembers"/>
   </owl:ObjectProperty>
   <owl:ObjectProperty rdf:about="http://www.opengis.net/gml#hasMultiSurface">
      <rdfs:comment>Warning: This ObjectProperty reference was declared outside of its original schema. This ObjectProperty may be declared incorrectly.</rdfs:comment>
      <rdfs:domain rdf:resource="http://www.opengis.net/gml#MultiSurfacePropertyType"/>
      <rdfs:range rdf:resource="http://www.opengis.net/gml#MultiSurface"/>
   </owl:ObjectProperty>
   <owl:ObjectProperty rdf:about="http://www.opengis.net/gml#hassolidMember">
      <rdfs:comment>Warning: This ObjectProperty reference was declared outside of its original schema. This ObjectProperty may be declared incorrectly.</rdfs:comment>
      <rdfs:domain rdf:resource="http://www.opengis.net/gml#MultiSolidType"/>
      <rdfs:range rdf:resource="http://www.opengis.net/gml#solidMember"/>
   </owl:ObjectProperty>
   <owl:ObjectProperty rdf:about="http://www.opengis.net/gml#hassolidMembers">
      <rdfs:comment>Warning: This ObjectProperty reference was declared outside of its original schema. This ObjectProperty may be declared incorrectly.</rdfs:comment>
      <rdfs:domain rdf:resource="http://www.opengis.net/gml#MultiSolidType"/>
      <rdfs:range rdf:resource="http://www.opengis.net/gml#solidMembers"/>
   </owl:ObjectProperty>
   <owl:ObjectProperty rdf:about="http://www.opengis.net/gml#hasMultiSolid">
      <rdfs:comment>Warning: This ObjectProperty reference was declared outside of its original schema. This ObjectProperty may be declared incorrectly.</rdfs:comment>
      <rdfs:domain rdf:resource="http://www.opengis.net/gml#MultiSolidPropertyType"/>
      <rdfs:range rdf:resource="http://www.opengis.net/gml#MultiSolid"/>
   </owl:ObjectProperty>
   <owl:ObjectProperty rdf:about="http://www.opengis.net/gml#haslineStringMember">
      <rdfs:comment>Warning: This ObjectProperty reference was declared outside of its original schema. This ObjectProperty may be declared incorrectly.</rdfs:comment>
      <rdfs:domain rdf:resource="http://www.opengis.net/gml#MultiLineStringType"/>
      <rdfs:range rdf:resource="http://www.opengis.net/gml#lineStringMember"/>
   </owl:ObjectProperty>
   <owl:ObjectProperty rdf:about="http://www.opengis.net/gml#hasMultiLineString">
      <rdfs:comment>Warning: This ObjectProperty reference was declared outside of its original schema. This ObjectProperty may be declared incorrectly.</rdfs:comment>
      <rdfs:domain rdf:resource="http://www.opengis.net/gml#MultiLineStringPropertyType"/>
      <rdfs:range rdf:resource="http://www.opengis.net/gml#MultiLineString"/>
   </owl:ObjectProperty>
   <owl:ObjectProperty rdf:about="http://www.opengis.net/gml#haspolygonMember">
      <rdfs:comment>Warning: This ObjectProperty reference was declared outside of its original schema. This ObjectProperty may be declared incorrectly.</rdfs:comment>
      <rdfs:domain rdf:resource="http://www.opengis.net/gml#MultiPolygonType"/>
      <rdfs:range rdf:resource="http://www.opengis.net/gml#polygonMember"/>
   </owl:ObjectProperty>
   <owl:ObjectProperty rdf:about="http://www.opengis.net/gml#hasMultiPolygon">
      <rdfs:comment>Warning: This ObjectProperty reference was declared outside of its original schema. This ObjectProperty may be declared incorrectly.</rdfs:comment>
      <rdfs:domain rdf:resource="http://www.opengis.net/gml#MultiPolygonPropertyType"/>
      <rdfs:range rdf:resource="http://www.opengis.net/gml#MultiPolygon"/>
   </owl:ObjectProperty>
</rdf:RDF>
