<rdf:RDF xmlns:math="http://www.w3.org/2005/xpath-functions/math" xmlns:owl="http://www.w3.org/2002/07/owl#" xmlns:rdf="http://www.w3.org/1999/02/22-rdf-syntax-ns#" xmlns:rdfs="http://www.w3.org/2000/01/rdf-schema#" xmlns:xs="http://www.w3.org/2001/XMLSchema" xmlns:xsd="http://www.w3.org/2001/XMLSchema">
   <owl:Ontology rdf:about="http://liris.cnrs.fr/ontologies/geometryBasic2d">
      <owl:imports rdf:resource="http://liris.cnrs.fr/ontologies/gml"/>
      <owl:imports rdf:resource="http://liris.cnrs.fr/ontologies/geometryBasic0d1d"/>
      <rdfs:comment>geometryBasic2d.xsd</rdfs:comment>
      <rdfs:seeAlso>urn:opengis:specification:gml:schema-xsd:geometryBasic2d:3.1.1</rdfs:seeAlso>
      <rdfs:comment>
			GML is an OGC Standard.
			Copyright (c) 2001,2005,2010 Open Geospatial Consortium.
			To obtain additional rights of use, visit http://www.opengeospatial.org/legal/ .
		</rdfs:comment>
   </owl:Ontology>
   <owl:Class rdf:about="http://www.opengis.net/gml#AbstractSurfaceType">
      <rdfs:comment>An abstraction of a surface to support the different levels of complexity. A surface is always a continuous region of a plane.</rdfs:comment>
      <rdfs:subClassOf rdf:resource="http://www.opengis.net/gml#AbstractGeometricPrimitiveType"/>
      <rdfs:comment>Warning: The parent class 'gml:AbstractGeometricPrimitiveType' is declared outside of this class' original schema. This class may be declared incorrectly.</rdfs:comment>
   </owl:Class>
   <owl:Class rdf:about="http://www.opengis.net/gml#SurfacePropertyType">
      <rdfs:comment>A property that has a surface as its value domain can either be an appropriate geometry element encapsulated in an element of this type or an XLink reference to a remote geometry element (where remote includes geometry elements located elsewhere in the same document). Either the reference or the contained element must be given, but neither both nor none.</rdfs:comment>
      <rdfs:subClassOf>
         <owl:Class>
            <owl:intersectionOf rdf:parseType="Collection">
               <owl:Restriction>
                  <owl:onProperty rdf:resource="http://www.opengis.net/gml#has_Surface"/>
                  <owl:allValuesFrom rdf:resource="http://www.opengis.net/gml#_Surface"/>
               </owl:Restriction>
            </owl:intersectionOf>
         </owl:Class>
      </rdfs:subClassOf>
   </owl:Class>
   <owl:Class rdf:about="http://www.opengis.net/gml#SurfaceArrayPropertyType">
      <rdfs:comment>A container for an array of surfaces. The elements are always contained in the array property, referencing geometry elements or arrays of geometry elements is not supported.</rdfs:comment>
      <rdfs:subClassOf>
         <owl:Class>
            <owl:intersectionOf rdf:parseType="Collection">
               <owl:Restriction>
                  <owl:onProperty rdf:resource="http://www.opengis.net/gml#has_Surface"/>
                  <owl:allValuesFrom rdf:resource="http://www.opengis.net/gml#_Surface"/>
               </owl:Restriction>
               <owl:Restriction>
                  <owl:onProperty rdf:resource="http://www.opengis.net/gml#has_Surface"/>
                  <owl:minCardinality rdf:datatype="http://www.w3.org/2001/XMLSchema#nonNegativeInteger">0</owl:minCardinality>
               </owl:Restriction>
            </owl:intersectionOf>
         </owl:Class>
      </rdfs:subClassOf>
   </owl:Class>
   <owl:Class rdf:about="http://www.opengis.net/gml#PolygonType">
      <rdfs:comment>A Polygon is a special surface that is defined by a single surface patch. The boundary of this patch is coplanar and the polygon uses planar interpolation in its interior. It is backwards compatible with the Polygon of GML 2, GM_Polygon of ISO 19107 is implemented by PolygonPatch.</rdfs:comment>
      <rdfs:subClassOf>
         <owl:Class>
            <owl:intersectionOf rdf:parseType="Collection">
               <owl:Restriction>
                  <owl:onProperty rdf:resource="http://www.opengis.net/gml#hasexterior"/>
                  <owl:allValuesFrom rdf:resource="http://www.opengis.net/gml#exterior"/>
               </owl:Restriction>
               <owl:Restriction>
                  <owl:onProperty rdf:resource="http://www.opengis.net/gml#hasexterior"/>
                  <owl:minCardinality rdf:datatype="http://www.w3.org/2001/XMLSchema#nonNegativeInteger">0</owl:minCardinality>
               </owl:Restriction>
               <owl:Restriction>
                  <owl:onProperty rdf:resource="http://www.opengis.net/gml#hasinterior"/>
                  <owl:allValuesFrom rdf:resource="http://www.opengis.net/gml#interior"/>
               </owl:Restriction>
               <owl:Restriction>
                  <owl:onProperty rdf:resource="http://www.opengis.net/gml#hasinterior"/>
                  <owl:minCardinality rdf:datatype="http://www.w3.org/2001/XMLSchema#nonNegativeInteger">0</owl:minCardinality>
               </owl:Restriction>
            </owl:intersectionOf>
         </owl:Class>
      </rdfs:subClassOf>
      <rdfs:subClassOf rdf:resource="http://www.opengis.net/gml#AbstractSurfaceType"/>
      <rdfs:comment>Warning: The parent class 'gml:AbstractSurfaceType' is declared outside of this class' original schema. This class may be declared incorrectly.</rdfs:comment>
   </owl:Class>
   <owl:Class rdf:about="http://www.opengis.net/gml#AbstractRingType">
      <rdfs:comment>This is an abstract class</rdfs:comment>
      <rdfs:comment>An abstraction of a ring to support surface boundaries of different complexity.</rdfs:comment>
      <rdfs:subClassOf rdf:resource="http://www.opengis.net/gml#AbstractGeometryType"/>
      <rdfs:comment>Warning: The parent class 'gml:AbstractGeometryType' is declared outside of this class' original schema. This class may be declared incorrectly.</rdfs:comment>
   </owl:Class>
   <owl:Class rdf:about="http://www.opengis.net/gml#AbstractRingPropertyType">
      <rdfs:comment>Encapsulates a ring to represent the surface boundary property of a surface.</rdfs:comment>
      <rdfs:subClassOf>
         <owl:Class>
            <owl:intersectionOf rdf:parseType="Collection">
               <owl:Restriction>
                  <owl:onProperty rdf:resource="http://www.opengis.net/gml#has_Ring"/>
                  <owl:allValuesFrom rdf:resource="http://www.opengis.net/gml#_Ring"/>
               </owl:Restriction>
            </owl:intersectionOf>
         </owl:Class>
      </rdfs:subClassOf>
   </owl:Class>
   <owl:Class rdf:about="http://www.opengis.net/gml#LinearRingType">
      <rdfs:comment>A LinearRing is defined by four or more coordinate tuples, with linear interpolation between them; the first and last coordinates must be coincident.</rdfs:comment>
      <rdfs:subClassOf>
         <owl:Class>
            <owl:intersectionOf rdf:parseType="Collection"/>
         </owl:Class>
      </rdfs:subClassOf>
      <owl:disjointUnionOf rdf:parseType="Collection">
         <owl:Restriction>
            <owl:onProperty rdf:resource="http://www.opengis.net/gml#hasposList"/>
            <owl:allValuesFrom rdf:resource="http://www.opengis.net/gml#posList"/>
         </owl:Restriction>
         <owl:Restriction>
            <owl:onProperty rdf:resource="http://www.opengis.net/gml#hascoordinates"/>
            <owl:allValuesFrom rdf:resource="http://www.opengis.net/gml#coordinates"/>
         </owl:Restriction>
         <owl:Restriction>
            <owl:onProperty rdf:resource="http://www.opengis.net/gml#hascoord"/>
            <owl:allValuesFrom rdf:resource="http://www.opengis.net/gml#coord"/>
         </owl:Restriction>
         <owl:Restriction>
            <owl:onProperty rdf:resource="http://www.opengis.net/gml#hascoord"/>
            <owl:minCardinality rdf:datatype="http://www.w3.org/2001/XMLSchema#nonNegativeInteger">4</owl:minCardinality>
         </owl:Restriction>
      </owl:disjointUnionOf>
      <rdfs:subClassOf rdf:resource="http://www.opengis.net/gml#AbstractRingType"/>
      <rdfs:comment>Warning: The parent class 'gml:AbstractRingType' is declared outside of this class' original schema. This class may be declared incorrectly.</rdfs:comment>
   </owl:Class>
   <owl:Class rdf:about="http://www.opengis.net/gml#LinearRingPropertyType">
      <rdfs:comment>Encapsulates a ring to represent properties in features or geometry collections.</rdfs:comment>
      <owl:disjointUnionOf rdf:parseType="Collection">
         <owl:Restriction>
            <owl:onProperty rdf:resource="http://www.opengis.net/gml#hasLinearRing"/>
            <owl:allValuesFrom rdf:resource="http://www.opengis.net/gml#LinearRing"/>
         </owl:Restriction>
      </owl:disjointUnionOf>
   </owl:Class>
   <owl:Class rdf:about="http://www.opengis.net/gml#PolygonPropertyType">
      <rdfs:comment>This type is deprecated with GML 3 and shall not be used. It is included for backwards compatibility with GML 2. Use SurfacePropertyType instead.
A property that has a polygon as its value domain can either be an appropriate geometry element encapsulated in an element of this type or an XLink reference to a remote geometry element (where remote includes geometry elements located elsewhere in the same document). Either the reference or the contained element must be given, but neither both nor none.</rdfs:comment>
      <rdfs:subClassOf>
         <owl:Class>
            <owl:intersectionOf rdf:parseType="Collection">
               <owl:Restriction>
                  <owl:onProperty rdf:resource="http://www.opengis.net/gml#hasPolygon"/>
                  <owl:allValuesFrom rdf:resource="http://www.opengis.net/gml#Polygon"/>
               </owl:Restriction>
            </owl:intersectionOf>
         </owl:Class>
      </rdfs:subClassOf>
   </owl:Class>
   <owl:ObjectProperty rdf:about="http://www.opengis.net/gml#hasAssociationAttributeGroup">
      <rdfs:domain rdf:resource="http://www.opengis.net/gml#SurfacePropertyType"/>
      <rdfs:range rdf:resource="http://www.opengis.net/gml#AssociationAttributeGroup"/>
   </owl:ObjectProperty>
   <owl:ObjectProperty rdf:about="http://www.opengis.net/gml#hasAssociationAttributeGroup">
      <rdfs:domain rdf:resource="http://www.opengis.net/gml#PolygonPropertyType"/>
      <rdfs:range rdf:resource="http://www.opengis.net/gml#AssociationAttributeGroup"/>
   </owl:ObjectProperty>
   <owl:Class rdf:about="http://www.opengis.net/gml#_Surface">
      <rdfs:subClassOf rdf:resource="http://www.opengis.net/gml#_GeometricPrimitive"/>
      <rdfs:subClassOf rdf:resource="http://www.opengis.net/gml#AbstractSurfaceType"/>
      <rdfs:comment>Warning: This class type was declared outside of its original schema. This class may be declared incorrectly.</rdfs:comment>
   </owl:Class>
   <owl:Class rdf:about="http://www.opengis.net/gml#surfaceProperty">
      <rdfs:subClassOf rdf:resource="http://www.opengis.net/gml#SurfacePropertyType"/>
      <rdfs:comment>Warning: This class type was declared outside of its original schema. This class may be declared incorrectly.</rdfs:comment>
   </owl:Class>
   <owl:Class rdf:about="http://www.opengis.net/gml#surfaceArrayProperty">
      <rdfs:subClassOf rdf:resource="http://www.opengis.net/gml#SurfaceArrayPropertyType"/>
      <rdfs:comment>Warning: This class type was declared outside of its original schema. This class may be declared incorrectly.</rdfs:comment>
   </owl:Class>
   <owl:Class rdf:about="http://www.opengis.net/gml#Polygon">
      <rdfs:subClassOf rdf:resource="http://www.opengis.net/gml#_Surface"/>
      <rdfs:subClassOf rdf:resource="http://www.opengis.net/gml#PolygonType"/>
      <rdfs:comment>Warning: This class type was declared outside of its original schema. This class may be declared incorrectly.</rdfs:comment>
   </owl:Class>
   <owl:Class rdf:about="http://www.opengis.net/gml#_Ring">
      <rdfs:subClassOf rdf:resource="http://www.opengis.net/gml#_Geometry"/>
      <rdfs:subClassOf rdf:resource="http://www.opengis.net/gml#AbstractRingType"/>
      <rdfs:comment>Warning: This class type was declared outside of its original schema. This class may be declared incorrectly.</rdfs:comment>
   </owl:Class>
   <owl:Class rdf:about="http://www.opengis.net/gml#exterior">
      <rdfs:subClassOf rdf:resource="http://www.opengis.net/gml#AbstractRingPropertyType"/>
      <rdfs:comment>Warning: This class type was declared outside of its original schema. This class may be declared incorrectly.</rdfs:comment>
   </owl:Class>
   <owl:Class rdf:about="http://www.opengis.net/gml#interior">
      <rdfs:subClassOf rdf:resource="http://www.opengis.net/gml#AbstractRingPropertyType"/>
      <rdfs:comment>Warning: This class type was declared outside of its original schema. This class may be declared incorrectly.</rdfs:comment>
   </owl:Class>
   <owl:Class rdf:about="http://www.opengis.net/gml#outerBoundaryIs">
      <rdfs:subClassOf rdf:resource="http://www.opengis.net/gml#exterior"/>
      <rdfs:subClassOf rdf:resource="http://www.opengis.net/gml#AbstractRingPropertyType"/>
      <rdfs:comment>Warning: This class type was declared outside of its original schema. This class may be declared incorrectly.</rdfs:comment>
   </owl:Class>
   <owl:Class rdf:about="http://www.opengis.net/gml#innerBoundaryIs">
      <rdfs:subClassOf rdf:resource="http://www.opengis.net/gml#interior"/>
      <rdfs:subClassOf rdf:resource="http://www.opengis.net/gml#AbstractRingPropertyType"/>
      <rdfs:comment>Warning: This class type was declared outside of its original schema. This class may be declared incorrectly.</rdfs:comment>
   </owl:Class>
   <owl:Class rdf:about="http://www.opengis.net/gml#LinearRing">
      <rdfs:subClassOf rdf:resource="http://www.opengis.net/gml#_Ring"/>
      <rdfs:subClassOf rdf:resource="http://www.opengis.net/gml#LinearRingType"/>
      <rdfs:comment>Warning: This class type was declared outside of its original schema. This class may be declared incorrectly.</rdfs:comment>
   </owl:Class>
   <owl:Class rdf:about="http://www.opengis.net/gml#polygonProperty">
      <rdfs:subClassOf rdf:resource="http://www.opengis.net/gml#PolygonPropertyType"/>
      <rdfs:comment>Warning: This class type was declared outside of its original schema. This class may be declared incorrectly.</rdfs:comment>
   </owl:Class>
   <owl:ObjectProperty rdf:about="http://www.opengis.net/gml#has_Surface">
      <rdfs:comment>Warning: This ObjectProperty reference was declared outside of its original schema. This ObjectProperty may be declared incorrectly.</rdfs:comment>
      <rdfs:domain rdf:resource="http://www.opengis.net/gml#SurfacePropertyType"/>
      <rdfs:range rdf:resource="http://www.opengis.net/gml#_Surface"/>
   </owl:ObjectProperty>
   <owl:ObjectProperty rdf:about="http://www.opengis.net/gml#has_Surface">
      <rdfs:comment>Warning: This ObjectProperty reference was declared outside of its original schema. This ObjectProperty may be declared incorrectly.</rdfs:comment>
      <rdfs:domain rdf:resource="http://www.opengis.net/gml#SurfaceArrayPropertyType"/>
      <rdfs:range rdf:resource="http://www.opengis.net/gml#_Surface"/>
   </owl:ObjectProperty>
   <owl:ObjectProperty rdf:about="http://www.opengis.net/gml#hasexterior">
      <rdfs:comment>Warning: This ObjectProperty reference was declared outside of its original schema. This ObjectProperty may be declared incorrectly.</rdfs:comment>
      <rdfs:domain rdf:resource="http://www.opengis.net/gml#PolygonType"/>
      <rdfs:range rdf:resource="http://www.opengis.net/gml#exterior"/>
   </owl:ObjectProperty>
   <owl:ObjectProperty rdf:about="http://www.opengis.net/gml#hasinterior">
      <rdfs:comment>Warning: This ObjectProperty reference was declared outside of its original schema. This ObjectProperty may be declared incorrectly.</rdfs:comment>
      <rdfs:domain rdf:resource="http://www.opengis.net/gml#PolygonType"/>
      <rdfs:range rdf:resource="http://www.opengis.net/gml#interior"/>
   </owl:ObjectProperty>
   <owl:ObjectProperty rdf:about="http://www.opengis.net/gml#has_Ring">
      <rdfs:comment>Warning: This ObjectProperty reference was declared outside of its original schema. This ObjectProperty may be declared incorrectly.</rdfs:comment>
      <rdfs:domain rdf:resource="http://www.opengis.net/gml#AbstractRingPropertyType"/>
      <rdfs:range rdf:resource="http://www.opengis.net/gml#_Ring"/>
   </owl:ObjectProperty>
   <owl:ObjectProperty rdf:about="http://www.opengis.net/gml#haspos">
      <rdfs:comment>Warning: This ObjectProperty reference was declared outside of its original schema. This ObjectProperty may be declared incorrectly.</rdfs:comment>
      <rdfs:domain rdf:resource="http://www.opengis.net/gml#LinearRingType"/>
      <rdfs:range rdf:resource="http://www.opengis.net/gml#pos"/>
   </owl:ObjectProperty>
   <owl:ObjectProperty rdf:about="http://www.opengis.net/gml#haspointProperty">
      <rdfs:comment>Warning: This ObjectProperty reference was declared outside of its original schema. This ObjectProperty may be declared incorrectly.</rdfs:comment>
      <rdfs:domain rdf:resource="http://www.opengis.net/gml#LinearRingType"/>
      <rdfs:range rdf:resource="http://www.opengis.net/gml#pointProperty"/>
   </owl:ObjectProperty>
   <owl:ObjectProperty rdf:about="http://www.opengis.net/gml#haspointRep">
      <rdfs:comment>Warning: This ObjectProperty reference was declared outside of its original schema. This ObjectProperty may be declared incorrectly.</rdfs:comment>
      <rdfs:domain rdf:resource="http://www.opengis.net/gml#LinearRingType"/>
      <rdfs:range rdf:resource="http://www.opengis.net/gml#pointRep"/>
   </owl:ObjectProperty>
   <owl:ObjectProperty rdf:about="http://www.opengis.net/gml#hasposList">
      <rdfs:comment>Warning: This ObjectProperty reference was declared outside of its original schema. This ObjectProperty may be declared incorrectly.</rdfs:comment>
      <rdfs:domain rdf:resource="http://www.opengis.net/gml#LinearRingType"/>
      <rdfs:range rdf:resource="http://www.opengis.net/gml#posList"/>
   </owl:ObjectProperty>
   <owl:ObjectProperty rdf:about="http://www.opengis.net/gml#hascoordinates">
      <rdfs:comment>Warning: This ObjectProperty reference was declared outside of its original schema. This ObjectProperty may be declared incorrectly.</rdfs:comment>
      <rdfs:domain rdf:resource="http://www.opengis.net/gml#LinearRingType"/>
      <rdfs:range rdf:resource="http://www.opengis.net/gml#coordinates"/>
   </owl:ObjectProperty>
   <owl:ObjectProperty rdf:about="http://www.opengis.net/gml#hascoord">
      <rdfs:comment>Warning: This ObjectProperty reference was declared outside of its original schema. This ObjectProperty may be declared incorrectly.</rdfs:comment>
      <rdfs:domain rdf:resource="http://www.opengis.net/gml#LinearRingType"/>
      <rdfs:range rdf:resource="http://www.opengis.net/gml#coord"/>
   </owl:ObjectProperty>
   <owl:ObjectProperty rdf:about="http://www.opengis.net/gml#hasLinearRing">
      <rdfs:comment>Warning: This ObjectProperty reference was declared outside of its original schema. This ObjectProperty may be declared incorrectly.</rdfs:comment>
      <rdfs:domain rdf:resource="http://www.opengis.net/gml#LinearRingPropertyType"/>
      <rdfs:range rdf:resource="http://www.opengis.net/gml#LinearRing"/>
   </owl:ObjectProperty>
   <owl:ObjectProperty rdf:about="http://www.opengis.net/gml#hasPolygon">
      <rdfs:comment>Warning: This ObjectProperty reference was declared outside of its original schema. This ObjectProperty may be declared incorrectly.</rdfs:comment>
      <rdfs:domain rdf:resource="http://www.opengis.net/gml#PolygonPropertyType"/>
      <rdfs:range rdf:resource="http://www.opengis.net/gml#Polygon"/>
   </owl:ObjectProperty>
</rdf:RDF>
