<?xml version="1.0" encoding="UTF-8"?>
<rdf:RDF xmlns:math="http://www.w3.org/2005/xpath-functions/math"
         xmlns:owl="http://www.w3.org/2002/07/owl#"
         xmlns:rdf="http://www.w3.org/1999/02/22-rdf-syntax-ns#"
         xmlns:rdfs="http://www.w3.org/2000/01/rdf-schema#"
         xmlns:xs="http://www.w3.org/2001/XMLSchema"
         xmlns:xsd="http://www.w3.org/2001/XMLSchema">
   <owl:Ontology rdf:about="http://liris.cnrs.fr/ontologies/grids">
      <owl:imports rdf:resource="http://liris.cnrs.fr/ontologies/gml"/>
      <owl:imports rdf:resource="http://liris.cnrs.fr/ontologies/geometryBasic0d1d"/>
      <rdfs:comment>grids.xsd</rdfs:comment>
      <rdfs:seeAlso>urn:opengis:specification:gml:schema-xsd:grids:3.1.1</rdfs:seeAlso>
      <rdfs:comment xml:lang="en">Grid geometries
    A subset of implicit geometries
    Designed for use with GML Coverage schema, but maybe useful elsewhere as well.
    
    GML is an OGC Standard.
    Copyright (c) 2001,2005,2010 Open Geospatial Consortium.
    To obtain additional rights of use, visit http://www.opengeospatial.org/legal/ .
		</rdfs:comment>
   </owl:Ontology>
   <owl:Class rdf:about="http://www.opengis.net/gml#GridType">
      <rdfs:comment>An unrectified grid, which is a network composed of two or more sets of equally spaced parallel lines in which the members of each set intersect the members of the other sets at right angles.</rdfs:comment>
      <rdfs:subClassOf>
         <owl:Class>
            <owl:intersectionOf rdf:parseType="Collection">
               <owl:Restriction>
                  <owl:onProperty rdf:resource="http://www.opengis.net/gml#limits"/>
                  <owl:allValuesFrom rdf:resource="http://www.opengis.net/gml#GridLimitsType"/>
               </owl:Restriction>
               <owl:Restriction>
                  <owl:onProperty rdf:resource="http://www.opengis.net/gml#axisName"/>
                  <owl:allValuesFrom rdf:resource="http://www.opengis.net/gml#string"/>
               </owl:Restriction>
            </owl:intersectionOf>
         </owl:Class>
      </rdfs:subClassOf>
      <rdfs:subClassOf>
         <owl:Class>
            <owl:intersectionOf rdf:parseType="Collection">
               <owl:Restriction>
                  <owl:onProperty rdf:resource="http://www.opengis.net/gml#dimension"/>
                  <owl:allValuesFrom rdf:resource="http://www.opengis.net/gml#positiveInteger"/>
               </owl:Restriction>
            </owl:intersectionOf>
         </owl:Class>
      </rdfs:subClassOf>
      <rdfs:subClassOf rdf:resource="http://www.opengis.net/gml#AbstractGeometryType"/>
      <rdfs:comment>Warning: The parent class 'gml:AbstractGeometryType' is declared outside of this class' original schema. This class may be declared incorrectly.</rdfs:comment>
   </owl:Class>
   <owl:Class rdf:about="http://www.opengis.net/gml#GridLimitsType">
      <rdfs:subClassOf>
         <owl:Class>
            <owl:intersectionOf rdf:parseType="Collection">
               <owl:Restriction>
                  <owl:onProperty rdf:resource="http://www.opengis.net/gml#GridEnvelope"/>
                  <owl:allValuesFrom rdf:resource="http://www.opengis.net/gml#GridEnvelopeType"/>
               </owl:Restriction>
            </owl:intersectionOf>
         </owl:Class>
      </rdfs:subClassOf>
   </owl:Class>
   <owl:Class rdf:about="http://www.opengis.net/gml#GridEnvelopeType">
      <rdfs:comment>Provides grid coordinate values for the diametrically opposed corners of an envelope that bounds a section of grid. The value of a single coordinate is the number of offsets from the origin of the grid in the direction of a specific axis.</rdfs:comment>
      <rdfs:subClassOf>
         <owl:Class>
            <owl:intersectionOf rdf:parseType="Collection">
               <owl:Restriction>
                  <owl:onProperty rdf:resource="http://www.opengis.net/gml#low"/>
                  <owl:allValuesFrom rdf:resource="http://www.opengis.net/gml#integerList"/>
               </owl:Restriction>
               <owl:Restriction>
                  <owl:onProperty rdf:resource="http://www.opengis.net/gml#high"/>
                  <owl:allValuesFrom rdf:resource="http://www.opengis.net/gml#integerList"/>
               </owl:Restriction>
            </owl:intersectionOf>
         </owl:Class>
      </rdfs:subClassOf>
   </owl:Class>
   <owl:Class rdf:about="http://www.opengis.net/gml#RectifiedGridType">
      <rdfs:comment>A rectified grid has an origin and vectors that define its post locations.</rdfs:comment>
      <rdfs:subClassOf>
         <owl:Class>
            <owl:intersectionOf rdf:parseType="Collection">
               <owl:Restriction>
                  <owl:onProperty rdf:resource="http://www.opengis.net/gml#origin"/>
                  <owl:allValuesFrom rdf:resource="http://www.opengis.net/gml#PointPropertyType"/>
               </owl:Restriction>
               <owl:Restriction>
                  <owl:onProperty rdf:resource="http://www.opengis.net/gml#offsetVector"/>
                  <owl:allValuesFrom rdf:resource="http://www.opengis.net/gml#VectorType"/>
               </owl:Restriction>
            </owl:intersectionOf>
         </owl:Class>
      </rdfs:subClassOf>
      <rdfs:subClassOf rdf:resource="http://www.opengis.net/gml#GridType"/>
      <rdfs:comment>Warning: The parent class 'gml:GridType' is declared outside of this class' original schema. This class may be declared incorrectly.</rdfs:comment>
   </owl:Class>
   <owl:DatatypeProperty rdf:about="http://www.opengis.net/gml#dimension">
      <rdfs:domain rdf:resource="http://www.opengis.net/gml#GridType"/>
      <rdfs:range rdf:resource="http://www.opengis.net/gml#positiveInteger"/>
   </owl:DatatypeProperty>
   <owl:Class rdf:about="http://www.opengis.net/gml#_ImplicitGeometry">
      <rdfs:subClassOf rdf:resource="http://www.opengis.net/gml#_Geometry"/>
      <rdfs:subClassOf rdf:resource="http://www.opengis.net/gml#AbstractGeometryType"/>
      <rdfs:comment>Warning: This class type was declared outside of its original schema. This class may be declared incorrectly.</rdfs:comment>
   </owl:Class>
   <owl:Class rdf:about="http://www.opengis.net/gml#Grid">
      <rdfs:subClassOf rdf:resource="http://www.opengis.net/gml#_ImplicitGeometry"/>
      <rdfs:subClassOf rdf:resource="http://www.opengis.net/gml#GridType"/>
      <rdfs:comment>Warning: This class type was declared outside of its original schema. This class may be declared incorrectly.</rdfs:comment>
   </owl:Class>
   <owl:Class rdf:about="http://www.opengis.net/gml#RectifiedGrid">
      <rdfs:subClassOf rdf:resource="http://www.opengis.net/gml#_ImplicitGeometry"/>
      <rdfs:subClassOf rdf:resource="http://www.opengis.net/gml#RectifiedGridType"/>
      <rdfs:comment>Warning: This class type was declared outside of its original schema. This class may be declared incorrectly.</rdfs:comment>
   </owl:Class>
   <owl:ObjectProperty rdf:about="http://www.opengis.net/gml#limits">
      <rdfs:comment>Warning: This ObjectProperty type was declared outside of its original schema. This ObjectProperty may be declared incorrectly.</rdfs:comment>
      <rdfs:domain rdf:resource="http://www.opengis.net/gml#GridType"/>
      <rdfs:range rdf:resource="http://www.opengis.net/gml#GridLimitsType"/>
   </owl:ObjectProperty>
   <owl:DatatypeProperty rdf:about="http://www.opengis.net/gml#has">
      <rdfs:domain rdf:resource="http://www.opengis.net/gml#GridType"/>
      <rdfs:range rdf:resource="http://www.opengis.net/gml#"/>
   </owl:DatatypeProperty>
   <owl:ObjectProperty rdf:about="http://www.opengis.net/gml#GridEnvelope">
      <rdfs:comment>Warning: This ObjectProperty type was declared outside of its original schema. This ObjectProperty may be declared incorrectly.</rdfs:comment>
      <rdfs:domain rdf:resource="http://www.opengis.net/gml#GridLimitsType"/>
      <rdfs:range rdf:resource="http://www.opengis.net/gml#GridEnvelopeType"/>
   </owl:ObjectProperty>
   <owl:ObjectProperty rdf:about="http://www.opengis.net/gml#low">
      <rdfs:comment>Warning: This ObjectProperty type was declared outside of its original schema. This ObjectProperty may be declared incorrectly.</rdfs:comment>
      <rdfs:domain rdf:resource="http://www.opengis.net/gml#GridEnvelopeType"/>
      <rdfs:range rdf:resource="http://www.opengis.net/gml#integerList"/>
   </owl:ObjectProperty>
   <owl:ObjectProperty rdf:about="http://www.opengis.net/gml#high">
      <rdfs:comment>Warning: This ObjectProperty type was declared outside of its original schema. This ObjectProperty may be declared incorrectly.</rdfs:comment>
      <rdfs:domain rdf:resource="http://www.opengis.net/gml#GridEnvelopeType"/>
      <rdfs:range rdf:resource="http://www.opengis.net/gml#integerList"/>
   </owl:ObjectProperty>
   <owl:ObjectProperty rdf:about="http://www.opengis.net/gml#origin">
      <rdfs:comment>Warning: This ObjectProperty type was declared outside of its original schema. This ObjectProperty may be declared incorrectly.</rdfs:comment>
      <rdfs:domain rdf:resource="http://www.opengis.net/gml#RectifiedGridType"/>
      <rdfs:range rdf:resource="http://www.opengis.net/gml#PointPropertyType"/>
   </owl:ObjectProperty>
   <owl:ObjectProperty rdf:about="http://www.opengis.net/gml#offsetVector">
      <rdfs:comment>Warning: This ObjectProperty type was declared outside of its original schema. This ObjectProperty may be declared incorrectly.</rdfs:comment>
      <rdfs:domain rdf:resource="http://www.opengis.net/gml#RectifiedGridType"/>
      <rdfs:range rdf:resource="http://www.opengis.net/gml#VectorType"/>
   </owl:ObjectProperty>
</rdf:RDF>
