<rdf:RDF xmlns:math="http://www.w3.org/2005/xpath-functions/math" xmlns:owl="http://www.w3.org/2002/07/owl#" xmlns:rdf="http://www.w3.org/1999/02/22-rdf-syntax-ns#" xmlns:rdfs="http://www.w3.org/2000/01/rdf-schema#" xmlns:xs="http://www.w3.org/2001/XMLSchema" xmlns:xsd="http://www.w3.org/2001/XMLSchema">
   <owl:Ontology rdf:about="http://liris.cnrs.fr/ontologies/observation">
      <owl:imports rdf:resource="http://liris.cnrs.fr/ontologies/gml"/>
      <owl:imports rdf:resource="http://liris.cnrs.fr/ontologies/feature"/>
      <owl:imports rdf:resource="http://liris.cnrs.fr/ontologies/direction"/>
      <owl:imports rdf:resource="http://liris.cnrs.fr/ontologies/valueObjects"/>
      <rdfs:comment>observation.xsd</rdfs:comment>
      <rdfs:seeAlso>urn:opengis:specification:gml:schema-xsd:observation:3.1.1</rdfs:seeAlso>
      <rdfs:comment>Observation schema for GML 3.1
			
			GML is an OGC Standard.
			Copyright (c) 2001,2005,2010 Open Geospatial Consortium.
			To obtain additional rights of use, visit http://www.opengeospatial.org/legal/ .
		</rdfs:comment>
   </owl:Ontology>
   <owl:Class rdf:about="#TargetPropertyType">
      <rdfs:comment>Container for an object representing the target or subject of an observation.</rdfs:comment>
      <rdfs:subClassOf>
         <owl:Class>
            <owl:intersectionOf rdf:parseType="Collection"/>
         </owl:Class>
      </rdfs:subClassOf>
   </owl:Class>
   <owl:Class rdf:about="#ObservationType">
      <rdfs:subClassOf>
         <owl:Class>
            <owl:intersectionOf rdf:parseType="Collection">
               <owl:Restriction>
                  <owl:onProperty rdf:resource="gml:hasvalidTime"/>
                  <owl:allValuesFrom rdf:resource="gml:validTime"/>
               </owl:Restriction>
               <owl:Restriction>
                  <owl:onProperty rdf:resource="gml:hasusing"/>
                  <owl:allValuesFrom rdf:resource="gml:using"/>
               </owl:Restriction>
               <owl:Restriction>
                  <owl:onProperty rdf:resource="gml:hasusing"/>
                  <owl:minCardinality rdf:datatype="http://www.w3.org/2001/XMLSchema#nonNegativeInteger">0</owl:minCardinality>
               </owl:Restriction>
               <owl:Restriction>
                  <owl:onProperty rdf:resource="gml:hastarget"/>
                  <owl:allValuesFrom rdf:resource="gml:target"/>
               </owl:Restriction>
               <owl:Restriction>
                  <owl:onProperty rdf:resource="gml:hastarget"/>
                  <owl:minCardinality rdf:datatype="http://www.w3.org/2001/XMLSchema#nonNegativeInteger">0</owl:minCardinality>
               </owl:Restriction>
               <owl:Restriction>
                  <owl:onProperty rdf:resource="gml:hasresultOf"/>
                  <owl:allValuesFrom rdf:resource="gml:resultOf"/>
               </owl:Restriction>
            </owl:intersectionOf>
         </owl:Class>
      </rdfs:subClassOf>
      <rdfs:subClassOf rdf:resource="gml:AbstractFeatureType"/>
      <rdfs:comment>Warning: The parent class 'gml:AbstractFeatureType' is declared outside of this class' original schema. This class may be declared incorrectly.</rdfs:comment>
   </owl:Class>
   <owl:Class rdf:about="#DirectedObservationType">
      <rdfs:subClassOf>
         <owl:Class>
            <owl:intersectionOf rdf:parseType="Collection">
               <owl:Restriction>
                  <owl:onProperty rdf:resource="gml:hasdirection"/>
                  <owl:allValuesFrom rdf:resource="gml:direction"/>
               </owl:Restriction>
            </owl:intersectionOf>
         </owl:Class>
      </rdfs:subClassOf>
      <rdfs:subClassOf rdf:resource="gml:ObservationType"/>
      <rdfs:comment>Warning: The parent class 'gml:ObservationType' is declared outside of this class' original schema. This class may be declared incorrectly.</rdfs:comment>
   </owl:Class>
   <owl:Class rdf:about="#DirectedObservationAtDistanceType">
      <rdfs:subClassOf>
         <owl:Class>
            <owl:intersectionOf rdf:parseType="Collection">
               <owl:Restriction>
                  <owl:onProperty rdf:resource="#distance"/>
                  <owl:allValuesFrom rdf:resource="gml:MeasureType"/>
               </owl:Restriction>
            </owl:intersectionOf>
         </owl:Class>
      </rdfs:subClassOf>
      <rdfs:subClassOf rdf:resource="gml:DirectedObservationType"/>
      <rdfs:comment>Warning: The parent class 'gml:DirectedObservationType' is declared outside of this class' original schema. This class may be declared incorrectly.</rdfs:comment>
   </owl:Class>
   <owl:ObjectProperty rdf:about="gml:hasAssociationAttributeGroup">
      <rdfs:domain rdf:resource="#TargetPropertyType"/>
      <rdfs:range rdf:resource="gml:AssociationAttributeGroup"/>
   </owl:ObjectProperty>
   <owl:Class rdf:about="#using">
      <rdfs:subClassOf rdf:resource="gml:FeaturePropertyType"/>
      <rdfs:comment>Warning: This class type was declared outside of its original schema. This class may be declared incorrectly.</rdfs:comment>
   </owl:Class>
   <owl:Class rdf:about="#target">
      <rdfs:subClassOf rdf:resource="gml:TargetPropertyType"/>
      <rdfs:comment>Warning: This class type was declared outside of its original schema. This class may be declared incorrectly.</rdfs:comment>
   </owl:Class>
   <owl:Class rdf:about="#subject">
      <rdfs:subClassOf rdf:resource="gml:target"/>
      <rdfs:subClassOf rdf:resource="gml:TargetPropertyType"/>
      <rdfs:comment>Warning: This class type was declared outside of its original schema. This class may be declared incorrectly.</rdfs:comment>
   </owl:Class>
   <owl:Class rdf:about="#resultOf">
      <rdfs:subClassOf rdf:resource="gml:AssociationType"/>
      <rdfs:comment>Warning: This class type was declared outside of its original schema. This class may be declared incorrectly.</rdfs:comment>
   </owl:Class>
   <owl:Class rdf:about="#Observation">
      <rdfs:subClassOf rdf:resource="gml:_Feature"/>
      <rdfs:subClassOf rdf:resource="gml:ObservationType"/>
      <rdfs:comment>Warning: This class type was declared outside of its original schema. This class may be declared incorrectly.</rdfs:comment>
   </owl:Class>
   <owl:Class rdf:about="#DirectedObservation">
      <rdfs:subClassOf rdf:resource="gml:Observation"/>
      <rdfs:subClassOf rdf:resource="gml:DirectedObservationType"/>
      <rdfs:comment>Warning: This class type was declared outside of its original schema. This class may be declared incorrectly.</rdfs:comment>
   </owl:Class>
   <owl:Class rdf:about="#DirectedObservationAtDistance">
      <rdfs:subClassOf rdf:resource="gml:DirectedObservation"/>
      <rdfs:subClassOf rdf:resource="gml:DirectedObservationAtDistanceType"/>
      <rdfs:comment>Warning: This class type was declared outside of its original schema. This class may be declared incorrectly.</rdfs:comment>
   </owl:Class>
   <owl:ObjectProperty rdf:about="gml:has_Feature">
      <rdfs:comment>Warning: This ObjectProperty reference was declared outside of its original schema. This ObjectProperty may be declared incorrectly.</rdfs:comment>
      <rdfs:domain rdf:resource="#TargetPropertyType"/>
      <rdfs:range rdf:resource="gml:_Feature"/>
   </owl:ObjectProperty>
   <owl:ObjectProperty rdf:about="gml:has_Geometry">
      <rdfs:comment>Warning: This ObjectProperty reference was declared outside of its original schema. This ObjectProperty may be declared incorrectly.</rdfs:comment>
      <rdfs:domain rdf:resource="#TargetPropertyType"/>
      <rdfs:range rdf:resource="gml:_Geometry"/>
   </owl:ObjectProperty>
   <owl:ObjectProperty rdf:about="gml:hasvalidTime">
      <rdfs:comment>Warning: This ObjectProperty reference was declared outside of its original schema. This ObjectProperty may be declared incorrectly.</rdfs:comment>
      <rdfs:domain rdf:resource="#ObservationType"/>
      <rdfs:range rdf:resource="gml:validTime"/>
   </owl:ObjectProperty>
   <owl:ObjectProperty rdf:about="gml:hasusing">
      <rdfs:comment>Warning: This ObjectProperty reference was declared outside of its original schema. This ObjectProperty may be declared incorrectly.</rdfs:comment>
      <rdfs:domain rdf:resource="#ObservationType"/>
      <rdfs:range rdf:resource="gml:using"/>
   </owl:ObjectProperty>
   <owl:ObjectProperty rdf:about="gml:hastarget">
      <rdfs:comment>Warning: This ObjectProperty reference was declared outside of its original schema. This ObjectProperty may be declared incorrectly.</rdfs:comment>
      <rdfs:domain rdf:resource="#ObservationType"/>
      <rdfs:range rdf:resource="gml:target"/>
   </owl:ObjectProperty>
   <owl:ObjectProperty rdf:about="gml:hasresultOf">
      <rdfs:comment>Warning: This ObjectProperty reference was declared outside of its original schema. This ObjectProperty may be declared incorrectly.</rdfs:comment>
      <rdfs:domain rdf:resource="#ObservationType"/>
      <rdfs:range rdf:resource="gml:resultOf"/>
   </owl:ObjectProperty>
   <owl:ObjectProperty rdf:about="gml:hasdirection">
      <rdfs:comment>Warning: This ObjectProperty reference was declared outside of its original schema. This ObjectProperty may be declared incorrectly.</rdfs:comment>
      <rdfs:domain rdf:resource="#DirectedObservationType"/>
      <rdfs:range rdf:resource="gml:direction"/>
   </owl:ObjectProperty>
   <owl:ObjectProperty rdf:about="#distance">
      <rdfs:comment>Warning: This ObjectProperty type was declared outside of its original schema. This ObjectProperty may be declared incorrectly.</rdfs:comment>
      <rdfs:domain rdf:resource="#DirectedObservationAtDistanceType"/>
      <rdfs:range rdf:resource="gml:MeasureType"/>
   </owl:ObjectProperty>
</rdf:RDF>
