<?xml version="1.0" encoding="UTF-8"?>
<rdf:RDF xmlns:math="http://www.w3.org/2005/xpath-functions/math"
         xmlns:owl="http://www.w3.org/2002/07/owl#"
         xmlns:rdf="http://www.w3.org/1999/02/22-rdf-syntax-ns#"
         xmlns:rdfs="http://www.w3.org/2000/01/rdf-schema#"
         xmlns:xs="http://www.w3.org/2001/XMLSchema"
         xmlns:xsd="http://www.w3.org/2001/XMLSchema">
   <owl:Ontology rdf:about="http://liris.cnrs.fr/ontologies/relief">
      <rdfs:comment>Warning: The schema http://www.opengis.net/gml was not imported.</rdfs:comment>
      <rdfs:comment>Warning: The schema http://www.opengis.net/citygml/2.0 was not imported.</rdfs:comment>
      <rdfs:comment>
	CityGML is an OGC Standard.
	Copyright (c) 2012 Open Geospatial Consortium.
	To obtain additional rights of use, visit http://www.opengeospatial.org/legal/ .
		</rdfs:comment>
   </owl:Ontology>
   <owl:Class rdf:about="http://www.opengis.net/citygml/relief/2.0#ReliefFeatureType">
      <rdfs:comment>Type describing the features of the Digital Terrain Model. As subclass of _CityObject, a ReliefFeature
				inherits all attributes and relations, in particular an id, names, external references, and generalization relations.
			</rdfs:comment>
      <owl:equivalentClass>
         <owl:Class>
            <owl:intersectionOf rdf:parseType="Collection">
               <owl:Restriction>
                  <owl:onProperty rdf:resource="http://www.opengis.net/citygml/relief/2.0#lod"/>
                  <owl:allValuesFrom rdf:resource="http://www.opengis.net/citygml/2.0#integerBetween0and4"/>
               </owl:Restriction>
               <owl:Restriction>
                  <owl:onProperty rdf:resource="http://www.opengis.net/citygml/relief/2.0#reliefComponent"/>
                  <owl:allValuesFrom rdf:resource="http://www.opengis.net/citygml/relief/2.0#ReliefComponentPropertyType"/>
               </owl:Restriction>
               <owl:Restriction>
                  <owl:onProperty rdf:resource="http://www.opengis.net/citygml/relief/2.0#has_GenericApplicationPropertyOfReliefFeature"/>
                  <owl:allValuesFrom rdf:resource="http://www.opengis.net/citygml/relief/2.0#_GenericApplicationPropertyOfReliefFeature"/>
               </owl:Restriction>
               <owl:Restriction>
                  <owl:onProperty rdf:resource="http://www.opengis.net/citygml/relief/2.0#has_GenericApplicationPropertyOfReliefFeature"/>
                  <owl:minCardinality rdf:datatype="http://www.w3.org/2001/XMLSchema#nonNegativeInteger">0</owl:minCardinality>
               </owl:Restriction>
            </owl:intersectionOf>
         </owl:Class>
      </owl:equivalentClass>
      <rdfs:subClassOf rdf:resource="http://www.opengis.net/citygml/2.0#AbstractCityObjectType"/>
      <rdfs:comment>Warning: The parent class 'core:AbstractCityObjectType' is declared outside of this class' original schema. This class may be declared incorrectly.</rdfs:comment>
   </owl:Class>
   <owl:Class rdf:about="http://www.opengis.net/citygml/relief/2.0#AbstractReliefComponentType">
      <rdfs:comment>This is an abstract class</rdfs:comment>
      <rdfs:comment>Type describing the components of a relief feature - either a TIN, a Grid, mass points or break lines. As
				subclass of _CityObject, a ReliefComponent inherits all attributes and relations, in particular an id, names, external
				references, and generalization relations. </rdfs:comment>
      <owl:equivalentClass>
         <owl:Class>
            <owl:intersectionOf rdf:parseType="Collection">
               <owl:Restriction>
                  <owl:onProperty rdf:resource="http://www.opengis.net/citygml/relief/2.0#lod"/>
                  <owl:allValuesFrom rdf:resource="http://www.opengis.net/citygml/2.0#integerBetween0and4"/>
               </owl:Restriction>
               <owl:Restriction>
                  <owl:onProperty rdf:resource="http://www.opengis.net/citygml/relief/2.0#extent"/>
                  <owl:allValuesFrom rdf:resource="http://www.opengis.net/gml#PolygonPropertyType"/>
               </owl:Restriction>
               <owl:Restriction>
                  <owl:onProperty rdf:resource="http://www.opengis.net/citygml/relief/2.0#extent"/>
                  <owl:minCardinality rdf:datatype="http://www.w3.org/2001/XMLSchema#nonNegativeInteger">0</owl:minCardinality>
               </owl:Restriction>
               <owl:Restriction>
                  <owl:onProperty rdf:resource="http://www.opengis.net/citygml/relief/2.0#has_GenericApplicationPropertyOfReliefComponent"/>
                  <owl:allValuesFrom rdf:resource="http://www.opengis.net/citygml/relief/2.0#_GenericApplicationPropertyOfReliefComponent"/>
               </owl:Restriction>
               <owl:Restriction>
                  <owl:onProperty rdf:resource="http://www.opengis.net/citygml/relief/2.0#has_GenericApplicationPropertyOfReliefComponent"/>
                  <owl:minCardinality rdf:datatype="http://www.w3.org/2001/XMLSchema#nonNegativeInteger">0</owl:minCardinality>
               </owl:Restriction>
            </owl:intersectionOf>
         </owl:Class>
      </owl:equivalentClass>
      <rdfs:subClassOf rdf:resource="http://www.opengis.net/citygml/2.0#AbstractCityObjectType"/>
      <rdfs:comment>Warning: The parent class 'core:AbstractCityObjectType' is declared outside of this class' original schema. This class may be declared incorrectly.</rdfs:comment>
   </owl:Class>
   <owl:Class rdf:about="http://www.opengis.net/citygml/relief/2.0#ReliefComponentPropertyType">
      <rdfs:comment>Denotes the relation of a ReliefFeature to its components. The ReliefComponentPropertyType element must
				either carry a reference to a _ReliefComponent object or contain a _ReliefComponent object inline, but neither both nor
				none. </rdfs:comment>
      <owl:equivalentClass>
         <owl:Class>
            <owl:intersectionOf rdf:parseType="Collection">
               <owl:Restriction>
                  <owl:onProperty rdf:resource="http://www.opengis.net/citygml/relief/2.0#has_ReliefComponent"/>
                  <owl:allValuesFrom rdf:resource="http://www.opengis.net/citygml/relief/2.0#_ReliefComponent"/>
               </owl:Restriction>
            </owl:intersectionOf>
         </owl:Class>
      </owl:equivalentClass>
   </owl:Class>
   <owl:Class rdf:about="http://www.opengis.net/citygml/relief/2.0#TINReliefType">
      <rdfs:comment>Type describing the TIN component of a relief feature. As subclass of _CityObject, a TINRelief inherits
				all attributes and relations, in particular an id, names, external references, and generalization relations.
			</rdfs:comment>
      <owl:equivalentClass>
         <owl:Class>
            <owl:intersectionOf rdf:parseType="Collection">
               <owl:Restriction>
                  <owl:onProperty rdf:resource="http://www.opengis.net/citygml/relief/2.0#tin"/>
                  <owl:allValuesFrom rdf:resource="http://www.opengis.net/citygml/relief/2.0#tinPropertyType"/>
               </owl:Restriction>
               <owl:Restriction>
                  <owl:onProperty rdf:resource="http://www.opengis.net/citygml/relief/2.0#has_GenericApplicationPropertyOfTinRelief"/>
                  <owl:allValuesFrom rdf:resource="http://www.opengis.net/citygml/relief/2.0#_GenericApplicationPropertyOfTinRelief"/>
               </owl:Restriction>
               <owl:Restriction>
                  <owl:onProperty rdf:resource="http://www.opengis.net/citygml/relief/2.0#has_GenericApplicationPropertyOfTinRelief"/>
                  <owl:minCardinality rdf:datatype="http://www.w3.org/2001/XMLSchema#nonNegativeInteger">0</owl:minCardinality>
               </owl:Restriction>
            </owl:intersectionOf>
         </owl:Class>
      </owl:equivalentClass>
   </owl:Class>
   <owl:Class rdf:about="http://www.opengis.net/citygml/relief/2.0#RasterReliefType">
      <rdfs:comment>Type describing the raster component of a relief feature. As subclass of _CityObject, a RasterRelief
				inherits all attributes and relations, in particular an id, names, external references, and generalization relations.
			</rdfs:comment>
      <owl:equivalentClass>
         <owl:Class>
            <owl:intersectionOf rdf:parseType="Collection">
               <owl:Restriction>
                  <owl:onProperty rdf:resource="http://www.opengis.net/citygml/relief/2.0#grid"/>
                  <owl:allValuesFrom rdf:resource="http://www.opengis.net/citygml/relief/2.0#gridPropertyType"/>
               </owl:Restriction>
               <owl:Restriction>
                  <owl:onProperty rdf:resource="http://www.opengis.net/citygml/relief/2.0#has_GenericApplicationPropertyOfRasterRelief"/>
                  <owl:allValuesFrom rdf:resource="http://www.opengis.net/citygml/relief/2.0#_GenericApplicationPropertyOfRasterRelief"/>
               </owl:Restriction>
               <owl:Restriction>
                  <owl:onProperty rdf:resource="http://www.opengis.net/citygml/relief/2.0#has_GenericApplicationPropertyOfRasterRelief"/>
                  <owl:minCardinality rdf:datatype="http://www.w3.org/2001/XMLSchema#nonNegativeInteger">0</owl:minCardinality>
               </owl:Restriction>
            </owl:intersectionOf>
         </owl:Class>
      </owl:equivalentClass>
   </owl:Class>
   <owl:Class rdf:about="http://www.opengis.net/citygml/relief/2.0#MassPointReliefType">
      <rdfs:comment>Type describing the mass point component of a relief feature. As subclass of _CityObject, a MassPoint
				Relief inherits all attributes and relations, in particular an id, names, external references, and generalization
				relations. </rdfs:comment>
      <owl:equivalentClass>
         <owl:Class>
            <owl:intersectionOf rdf:parseType="Collection">
               <owl:Restriction>
                  <owl:onProperty rdf:resource="http://www.opengis.net/citygml/relief/2.0#reliefPoints"/>
                  <owl:allValuesFrom rdf:resource="http://www.opengis.net/gml#MultiPointPropertyType"/>
               </owl:Restriction>
               <owl:Restriction>
                  <owl:onProperty rdf:resource="http://www.opengis.net/citygml/relief/2.0#has_GenericApplicationPropertyOfMassPointRelief"/>
                  <owl:allValuesFrom rdf:resource="http://www.opengis.net/citygml/relief/2.0#_GenericApplicationPropertyOfMassPointRelief"/>
               </owl:Restriction>
               <owl:Restriction>
                  <owl:onProperty rdf:resource="http://www.opengis.net/citygml/relief/2.0#has_GenericApplicationPropertyOfMassPointRelief"/>
                  <owl:minCardinality rdf:datatype="http://www.w3.org/2001/XMLSchema#nonNegativeInteger">0</owl:minCardinality>
               </owl:Restriction>
            </owl:intersectionOf>
         </owl:Class>
      </owl:equivalentClass>
   </owl:Class>
   <owl:Class rdf:about="http://www.opengis.net/citygml/relief/2.0#BreaklineReliefType">
      <rdfs:comment>Type describing the break line Component of a relief feature. A break line relief consists of break lines
				or ridgeOrValleyLines. As subclass of _CityObject, a BreaklineRelief inherits all attributes and relations, in particular
				an id, names, external references, and generalization relations. </rdfs:comment>
      <owl:equivalentClass>
         <owl:Class>
            <owl:intersectionOf rdf:parseType="Collection">
               <owl:Restriction>
                  <owl:onProperty rdf:resource="http://www.opengis.net/citygml/relief/2.0#ridgeOrValleyLines"/>
                  <owl:allValuesFrom rdf:resource="http://www.opengis.net/gml#MultiCurvePropertyType"/>
               </owl:Restriction>
               <owl:Restriction>
                  <owl:onProperty rdf:resource="http://www.opengis.net/citygml/relief/2.0#ridgeOrValleyLines"/>
                  <owl:minCardinality rdf:datatype="http://www.w3.org/2001/XMLSchema#nonNegativeInteger">0</owl:minCardinality>
               </owl:Restriction>
               <owl:Restriction>
                  <owl:onProperty rdf:resource="http://www.opengis.net/citygml/relief/2.0#breaklines"/>
                  <owl:allValuesFrom rdf:resource="http://www.opengis.net/gml#MultiCurvePropertyType"/>
               </owl:Restriction>
               <owl:Restriction>
                  <owl:onProperty rdf:resource="http://www.opengis.net/citygml/relief/2.0#breaklines"/>
                  <owl:minCardinality rdf:datatype="http://www.w3.org/2001/XMLSchema#nonNegativeInteger">0</owl:minCardinality>
               </owl:Restriction>
               <owl:Restriction>
                  <owl:onProperty rdf:resource="http://www.opengis.net/citygml/relief/2.0#has_GenericApplicationPropertyOfBreaklineRelief"/>
                  <owl:allValuesFrom rdf:resource="http://www.opengis.net/citygml/relief/2.0#_GenericApplicationPropertyOfBreaklineRelief"/>
               </owl:Restriction>
               <owl:Restriction>
                  <owl:onProperty rdf:resource="http://www.opengis.net/citygml/relief/2.0#has_GenericApplicationPropertyOfBreaklineRelief"/>
                  <owl:minCardinality rdf:datatype="http://www.w3.org/2001/XMLSchema#nonNegativeInteger">0</owl:minCardinality>
               </owl:Restriction>
            </owl:intersectionOf>
         </owl:Class>
      </owl:equivalentClass>
   </owl:Class>
   <owl:Class rdf:about="http://www.opengis.net/citygml/relief/2.0#tinPropertyType">
      <rdfs:comment>Denotes the relation of a TINRelief to its components. The tinPropertyType element must either carry a
				reference to a gml:TriangulatedSurface object or contain a gml:TriangulatedSurface object inline, but neither both nor
				none. </rdfs:comment>
      <owl:equivalentClass>
         <owl:Class>
            <owl:intersectionOf rdf:parseType="Collection">
               <owl:Restriction>
                  <owl:onProperty rdf:resource="http://www.opengis.net/gml#hasTriangulatedSurface"/>
                  <owl:allValuesFrom rdf:resource="http://www.opengis.net/gml#TriangulatedSurface"/>
               </owl:Restriction>
            </owl:intersectionOf>
         </owl:Class>
      </owl:equivalentClass>
   </owl:Class>
   <owl:Class rdf:about="http://www.opengis.net/citygml/relief/2.0#gridPropertyType">
      <rdfs:comment>Denotes the relation of a RasterReliefType to its components. The gridPropertyType element must either
				carry a reference to a gml:RectifiedGridCoverage object or contain a gml:RectifiedGridCoverage object inline, but neither
				both nor none. </rdfs:comment>
      <owl:equivalentClass>
         <owl:Class>
            <owl:intersectionOf rdf:parseType="Collection">
               <owl:Restriction>
                  <owl:onProperty rdf:resource="http://www.opengis.net/gml#hasRectifiedGridCoverage"/>
                  <owl:allValuesFrom rdf:resource="http://www.opengis.net/gml#RectifiedGridCoverage"/>
               </owl:Restriction>
            </owl:intersectionOf>
         </owl:Class>
      </owl:equivalentClass>
   </owl:Class>
   <owl:Class rdf:about="http://www.opengis.net/citygml/relief/2.0#ReliefFeature">
      <rdfs:subClassOf rdf:resource="http://www.opengis.net/citygml/2.0#_CityObject"/>
      <rdfs:subClassOf rdf:resource="http://www.opengis.net/citygml/relief/2.0#ReliefFeatureType"/>
   </owl:Class>
   <owl:Class rdf:about="http://www.opengis.net/citygml/relief/2.0#_GenericApplicationPropertyOfReliefFeature">
      <rdfs:subClassOf rdf:resource="http://www.w3.org/2001/XMLSchema#anyType"/>
      <rdfs:comment>Warning: This class type was declared outside of its original schema. This class may be declared incorrectly.</rdfs:comment>
   </owl:Class>
   <owl:Class rdf:about="http://www.opengis.net/citygml/relief/2.0#_ReliefComponent">
      <rdfs:subClassOf rdf:resource="http://www.opengis.net/citygml/2.0#_CityObject"/>
      <rdfs:subClassOf rdf:resource="http://www.opengis.net/citygml/relief/2.0#AbstractReliefComponentType"/>
   </owl:Class>
   <owl:Class rdf:about="http://www.opengis.net/citygml/relief/2.0#_GenericApplicationPropertyOfReliefComponent">
      <rdfs:subClassOf rdf:resource="http://www.w3.org/2001/XMLSchema#anyType"/>
      <rdfs:comment>Warning: This class type was declared outside of its original schema. This class may be declared incorrectly.</rdfs:comment>
   </owl:Class>
   <owl:Class rdf:about="http://www.opengis.net/citygml/relief/2.0#TINRelief">
      <rdfs:subClassOf rdf:resource="http://www.opengis.net/citygml/relief/2.0#_ReliefComponent"/>
      <rdfs:subClassOf rdf:resource="http://www.opengis.net/citygml/relief/2.0#TINReliefType"/>
   </owl:Class>
   <owl:Class rdf:about="http://www.opengis.net/citygml/relief/2.0#_GenericApplicationPropertyOfTinRelief">
      <rdfs:subClassOf rdf:resource="http://www.w3.org/2001/XMLSchema#anyType"/>
      <rdfs:comment>Warning: This class type was declared outside of its original schema. This class may be declared incorrectly.</rdfs:comment>
   </owl:Class>
   <owl:Class rdf:about="http://www.opengis.net/citygml/relief/2.0#RasterRelief">
      <rdfs:subClassOf rdf:resource="http://www.opengis.net/citygml/relief/2.0#_ReliefComponent"/>
      <rdfs:subClassOf rdf:resource="http://www.opengis.net/citygml/relief/2.0#RasterReliefType"/>
   </owl:Class>
   <owl:Class rdf:about="http://www.opengis.net/citygml/relief/2.0#_GenericApplicationPropertyOfRasterRelief">
      <rdfs:subClassOf rdf:resource="http://www.w3.org/2001/XMLSchema#anyType"/>
      <rdfs:comment>Warning: This class type was declared outside of its original schema. This class may be declared incorrectly.</rdfs:comment>
   </owl:Class>
   <owl:Class rdf:about="http://www.opengis.net/citygml/relief/2.0#MassPointRelief">
      <rdfs:subClassOf rdf:resource="http://www.opengis.net/citygml/relief/2.0#_ReliefComponent"/>
      <rdfs:subClassOf rdf:resource="http://www.opengis.net/citygml/relief/2.0#MassPointReliefType"/>
   </owl:Class>
   <owl:Class rdf:about="http://www.opengis.net/citygml/relief/2.0#_GenericApplicationPropertyOfMassPointRelief">
      <rdfs:subClassOf rdf:resource="http://www.w3.org/2001/XMLSchema#anyType"/>
      <rdfs:comment>Warning: This class type was declared outside of its original schema. This class may be declared incorrectly.</rdfs:comment>
   </owl:Class>
   <owl:Class rdf:about="http://www.opengis.net/citygml/relief/2.0#BreaklineRelief">
      <rdfs:subClassOf rdf:resource="http://www.opengis.net/citygml/relief/2.0#_ReliefComponent"/>
      <rdfs:subClassOf rdf:resource="http://www.opengis.net/citygml/relief/2.0#BreaklineReliefType"/>
   </owl:Class>
   <owl:Class rdf:about="http://www.opengis.net/citygml/relief/2.0#_GenericApplicationPropertyOfBreaklineRelief">
      <rdfs:subClassOf rdf:resource="http://www.w3.org/2001/XMLSchema#anyType"/>
      <rdfs:comment>Warning: This class type was declared outside of its original schema. This class may be declared incorrectly.</rdfs:comment>
   </owl:Class>
   <owl:Class rdf:about="http://www.opengis.net/citygml/relief/2.0#Elevation">
      <rdfs:subClassOf rdf:resource="http://www.opengis.net/gml#_Object"/>
      <rdfs:subClassOf rdf:resource="http://www.opengis.net/gml#LengthType"/>
      <rdfs:comment>Warning: This class type was declared outside of its original schema. This class may be declared incorrectly.</rdfs:comment>
   </owl:Class>
   <owl:ObjectProperty rdf:about="http://www.opengis.net/citygml/relief/2.0#lod">
      <rdfs:comment>Warning: This ObjectProperty type was declared outside of its original schema. This ObjectProperty may be declared incorrectly.</rdfs:comment>
      <rdfs:domain rdf:resource="http://www.opengis.net/citygml/relief/2.0#ReliefFeatureType"/>
      <rdfs:range rdf:resource="http://www.opengis.net/citygml/2.0#integerBetween0and4"/>
   </owl:ObjectProperty>
   <owl:ObjectProperty rdf:about="http://www.opengis.net/citygml/relief/2.0#reliefComponent">
      <rdfs:domain rdf:resource="http://www.opengis.net/citygml/relief/2.0#ReliefFeatureType"/>
      <rdfs:range rdf:resource="http://www.opengis.net/citygml/relief/2.0#ReliefComponentPropertyType"/>
   </owl:ObjectProperty>
   <owl:ObjectProperty rdf:about="http://www.opengis.net/citygml/relief/2.0#has_GenericApplicationPropertyOfReliefFeature">
      <rdfs:domain rdf:resource="http://www.opengis.net/citygml/relief/2.0#ReliefFeatureType"/>
      <rdfs:range rdf:resource="http://www.opengis.net/citygml/relief/2.0#_GenericApplicationPropertyOfReliefFeature"/>
   </owl:ObjectProperty>
   <owl:ObjectProperty rdf:about="http://www.opengis.net/citygml/relief/2.0#lod">
      <rdfs:comment>Warning: This ObjectProperty type was declared outside of its original schema. This ObjectProperty may be declared incorrectly.</rdfs:comment>
      <rdfs:domain rdf:resource="http://www.opengis.net/citygml/relief/2.0#AbstractReliefComponentType"/>
      <rdfs:range rdf:resource="http://www.opengis.net/citygml/2.0#integerBetween0and4"/>
   </owl:ObjectProperty>
   <owl:ObjectProperty rdf:about="http://www.opengis.net/citygml/relief/2.0#extent">
      <rdfs:comment>Warning: This ObjectProperty type was declared outside of its original schema. This ObjectProperty may be declared incorrectly.</rdfs:comment>
      <rdfs:domain rdf:resource="http://www.opengis.net/citygml/relief/2.0#AbstractReliefComponentType"/>
      <rdfs:range rdf:resource="http://www.opengis.net/gml#PolygonPropertyType"/>
   </owl:ObjectProperty>
   <owl:ObjectProperty rdf:about="http://www.opengis.net/citygml/relief/2.0#has_GenericApplicationPropertyOfReliefComponent">
      <rdfs:domain rdf:resource="http://www.opengis.net/citygml/relief/2.0#AbstractReliefComponentType"/>
      <rdfs:range rdf:resource="http://www.opengis.net/citygml/relief/2.0#_GenericApplicationPropertyOfReliefComponent"/>
   </owl:ObjectProperty>
   <owl:ObjectProperty rdf:about="http://www.opengis.net/citygml/relief/2.0#has_ReliefComponent">
      <rdfs:domain rdf:resource="http://www.opengis.net/citygml/relief/2.0#ReliefComponentPropertyType"/>
      <rdfs:range rdf:resource="http://www.opengis.net/citygml/relief/2.0#_ReliefComponent"/>
   </owl:ObjectProperty>
   <owl:ObjectProperty rdf:about="http://www.opengis.net/citygml/relief/2.0#tin">
      <rdfs:domain rdf:resource="http://www.opengis.net/citygml/relief/2.0#TINReliefType"/>
      <rdfs:range rdf:resource="http://www.opengis.net/citygml/relief/2.0#tinPropertyType"/>
   </owl:ObjectProperty>
   <owl:ObjectProperty rdf:about="http://www.opengis.net/citygml/relief/2.0#has_GenericApplicationPropertyOfTinRelief">
      <rdfs:domain rdf:resource="http://www.opengis.net/citygml/relief/2.0#TINReliefType"/>
      <rdfs:range rdf:resource="http://www.opengis.net/citygml/relief/2.0#_GenericApplicationPropertyOfTinRelief"/>
   </owl:ObjectProperty>
   <owl:ObjectProperty rdf:about="http://www.opengis.net/citygml/relief/2.0#grid">
      <rdfs:domain rdf:resource="http://www.opengis.net/citygml/relief/2.0#RasterReliefType"/>
      <rdfs:range rdf:resource="http://www.opengis.net/citygml/relief/2.0#gridPropertyType"/>
   </owl:ObjectProperty>
   <owl:ObjectProperty rdf:about="http://www.opengis.net/citygml/relief/2.0#has_GenericApplicationPropertyOfRasterRelief">
      <rdfs:domain rdf:resource="http://www.opengis.net/citygml/relief/2.0#RasterReliefType"/>
      <rdfs:range rdf:resource="http://www.opengis.net/citygml/relief/2.0#_GenericApplicationPropertyOfRasterRelief"/>
   </owl:ObjectProperty>
   <owl:ObjectProperty rdf:about="http://www.opengis.net/citygml/relief/2.0#reliefPoints">
      <rdfs:comment>Warning: This ObjectProperty type was declared outside of its original schema. This ObjectProperty may be declared incorrectly.</rdfs:comment>
      <rdfs:domain rdf:resource="http://www.opengis.net/citygml/relief/2.0#MassPointReliefType"/>
      <rdfs:range rdf:resource="http://www.opengis.net/gml#MultiPointPropertyType"/>
   </owl:ObjectProperty>
   <owl:ObjectProperty rdf:about="http://www.opengis.net/citygml/relief/2.0#has_GenericApplicationPropertyOfMassPointRelief">
      <rdfs:domain rdf:resource="http://www.opengis.net/citygml/relief/2.0#MassPointReliefType"/>
      <rdfs:range rdf:resource="http://www.opengis.net/citygml/relief/2.0#_GenericApplicationPropertyOfMassPointRelief"/>
   </owl:ObjectProperty>
   <owl:ObjectProperty rdf:about="http://www.opengis.net/citygml/relief/2.0#ridgeOrValleyLines">
      <rdfs:comment>Warning: This ObjectProperty type was declared outside of its original schema. This ObjectProperty may be declared incorrectly.</rdfs:comment>
      <rdfs:domain rdf:resource="http://www.opengis.net/citygml/relief/2.0#BreaklineReliefType"/>
      <rdfs:range rdf:resource="http://www.opengis.net/gml#MultiCurvePropertyType"/>
   </owl:ObjectProperty>
   <owl:ObjectProperty rdf:about="http://www.opengis.net/citygml/relief/2.0#breaklines">
      <rdfs:comment>Warning: This ObjectProperty type was declared outside of its original schema. This ObjectProperty may be declared incorrectly.</rdfs:comment>
      <rdfs:domain rdf:resource="http://www.opengis.net/citygml/relief/2.0#BreaklineReliefType"/>
      <rdfs:range rdf:resource="http://www.opengis.net/gml#MultiCurvePropertyType"/>
   </owl:ObjectProperty>
   <owl:ObjectProperty rdf:about="http://www.opengis.net/citygml/relief/2.0#has_GenericApplicationPropertyOfBreaklineRelief">
      <rdfs:domain rdf:resource="http://www.opengis.net/citygml/relief/2.0#BreaklineReliefType"/>
      <rdfs:range rdf:resource="http://www.opengis.net/citygml/relief/2.0#_GenericApplicationPropertyOfBreaklineRelief"/>
   </owl:ObjectProperty>
   <owl:ObjectProperty rdf:about="http://www.opengis.net/gml#hasTriangulatedSurface">
      <rdfs:comment>Warning: This ObjectProperty reference was declared outside of its original schema. This ObjectProperty may be declared incorrectly.</rdfs:comment>
      <rdfs:domain rdf:resource="http://www.opengis.net/citygml/relief/2.0#tinPropertyType"/>
      <rdfs:range rdf:resource="http://www.opengis.net/gml#TriangulatedSurface"/>
   </owl:ObjectProperty>
   <owl:ObjectProperty rdf:about="http://www.opengis.net/gml#hasRectifiedGridCoverage">
      <rdfs:comment>Warning: This ObjectProperty reference was declared outside of its original schema. This ObjectProperty may be declared incorrectly.</rdfs:comment>
      <rdfs:domain rdf:resource="http://www.opengis.net/citygml/relief/2.0#gridPropertyType"/>
      <rdfs:range rdf:resource="http://www.opengis.net/gml#RectifiedGridCoverage"/>
   </owl:ObjectProperty>
</rdf:RDF>
