<rdf:RDF xmlns:math="http://www.w3.org/2005/xpath-functions/math" xmlns:owl="http://www.w3.org/2002/07/owl#" xmlns:rdf="http://www.w3.org/1999/02/22-rdf-syntax-ns#" xmlns:rdfs="http://www.w3.org/2000/01/rdf-schema#" xmlns:xs="http://www.w3.org/2001/XMLSchema" xmlns:xsd="http://www.w3.org/2001/XMLSchema">
   <owl:Ontology rdf:about="http://liris.cnrs.fr/ontologies/relief">
      <owl:imports rdf:resource="http://liris.cnrs.fr/ontologies/gml"/>
      <owl:imports rdf:resource="http://liris.cnrs.fr/ontologies/cityGMLBase"/>
      <rdfs:comment>
	CityGML is an OGC Standard.
	Copyright (c) 2012 Open Geospatial Consortium.
	To obtain additional rights of use, visit http://www.opengeospatial.org/legal/ .
		</rdfs:comment>
   </owl:Ontology>
   <owl:Class rdf:about="#ReliefFeatureType">
      <rdfs:comment>Type describing the features of the Digital Terrain Model. As subclass of _CityObject, a ReliefFeature
				inherits all attributes and relations, in particular an id, names, external references, and generalization relations.
			</rdfs:comment>
      <rdfs:subClassOf>
         <owl:Class>
            <owl:intersectionOf rdf:parseType="Collection">
               <owl:Restriction>
                  <owl:onProperty rdf:resource="#lod"/>
                  <owl:allValuesFrom rdf:resource="core:integerBetween0and4"/>
               </owl:Restriction>
               <owl:Restriction>
                  <owl:onProperty rdf:resource="#reliefComponent"/>
                  <owl:allValuesFrom rdf:resource="#ReliefComponentPropertyType"/>
               </owl:Restriction>
               <owl:Restriction>
                  <owl:onProperty rdf:resource="#has_GenericApplicationPropertyOfReliefFeature"/>
                  <owl:allValuesFrom rdf:resource="#_GenericApplicationPropertyOfReliefFeature"/>
               </owl:Restriction>
               <owl:Restriction>
                  <owl:onProperty rdf:resource="#has_GenericApplicationPropertyOfReliefFeature"/>
                  <owl:minCardinality rdf:datatype="http://www.w3.org/2001/XMLSchema#nonNegativeInteger">0</owl:minCardinality>
               </owl:Restriction>
            </owl:intersectionOf>
         </owl:Class>
      </rdfs:subClassOf>
      <rdfs:subClassOf rdf:resource="core:AbstractCityObjectType"/>
      <rdfs:comment>Warning: The parent class 'core:AbstractCityObjectType' is declared outside of this class' original schema. This class may be declared incorrectly.</rdfs:comment>
   </owl:Class>
   <owl:Class rdf:about="#AbstractReliefComponentType">
      <rdfs:comment>This is an abstract class</rdfs:comment>
      <rdfs:comment>Type describing the components of a relief feature - either a TIN, a Grid, mass points or break lines. As
				subclass of _CityObject, a ReliefComponent inherits all attributes and relations, in particular an id, names, external
				references, and generalization relations. </rdfs:comment>
      <rdfs:subClassOf>
         <owl:Class>
            <owl:intersectionOf rdf:parseType="Collection">
               <owl:Restriction>
                  <owl:onProperty rdf:resource="#lod"/>
                  <owl:allValuesFrom rdf:resource="core:integerBetween0and4"/>
               </owl:Restriction>
               <owl:Restriction>
                  <owl:onProperty rdf:resource="#extent"/>
                  <owl:allValuesFrom rdf:resource="gml:PolygonPropertyType"/>
               </owl:Restriction>
               <owl:Restriction>
                  <owl:onProperty rdf:resource="#extent"/>
                  <owl:minCardinality rdf:datatype="http://www.w3.org/2001/XMLSchema#nonNegativeInteger">0</owl:minCardinality>
               </owl:Restriction>
               <owl:Restriction>
                  <owl:onProperty rdf:resource="#has_GenericApplicationPropertyOfReliefComponent"/>
                  <owl:allValuesFrom rdf:resource="#_GenericApplicationPropertyOfReliefComponent"/>
               </owl:Restriction>
               <owl:Restriction>
                  <owl:onProperty rdf:resource="#has_GenericApplicationPropertyOfReliefComponent"/>
                  <owl:minCardinality rdf:datatype="http://www.w3.org/2001/XMLSchema#nonNegativeInteger">0</owl:minCardinality>
               </owl:Restriction>
            </owl:intersectionOf>
         </owl:Class>
      </rdfs:subClassOf>
      <rdfs:subClassOf rdf:resource="core:AbstractCityObjectType"/>
      <rdfs:comment>Warning: The parent class 'core:AbstractCityObjectType' is declared outside of this class' original schema. This class may be declared incorrectly.</rdfs:comment>
   </owl:Class>
   <owl:Class rdf:about="#ReliefComponentPropertyType">
      <rdfs:comment>Denotes the relation of a ReliefFeature to its components. The ReliefComponentPropertyType element must
				either carry a reference to a _ReliefComponent object or contain a _ReliefComponent object inline, but neither both nor
				none. </rdfs:comment>
      <rdfs:subClassOf>
         <owl:Class>
            <owl:intersectionOf rdf:parseType="Collection">
               <owl:Restriction>
                  <owl:onProperty rdf:resource="#has_ReliefComponent"/>
                  <owl:allValuesFrom rdf:resource="#_ReliefComponent"/>
               </owl:Restriction>
            </owl:intersectionOf>
         </owl:Class>
      </rdfs:subClassOf>
   </owl:Class>
   <owl:Class rdf:about="#TINReliefType">
      <rdfs:comment>Type describing the TIN component of a relief feature. As subclass of _CityObject, a TINRelief inherits
				all attributes and relations, in particular an id, names, external references, and generalization relations.
			</rdfs:comment>
      <rdfs:subClassOf>
         <owl:Class>
            <owl:intersectionOf rdf:parseType="Collection">
               <owl:Restriction>
                  <owl:onProperty rdf:resource="#tin"/>
                  <owl:allValuesFrom rdf:resource="#tinPropertyType"/>
               </owl:Restriction>
               <owl:Restriction>
                  <owl:onProperty rdf:resource="#has_GenericApplicationPropertyOfTinRelief"/>
                  <owl:allValuesFrom rdf:resource="#_GenericApplicationPropertyOfTinRelief"/>
               </owl:Restriction>
               <owl:Restriction>
                  <owl:onProperty rdf:resource="#has_GenericApplicationPropertyOfTinRelief"/>
                  <owl:minCardinality rdf:datatype="http://www.w3.org/2001/XMLSchema#nonNegativeInteger">0</owl:minCardinality>
               </owl:Restriction>
            </owl:intersectionOf>
         </owl:Class>
      </rdfs:subClassOf>
      <rdfs:subClassOf rdf:resource="#AbstractReliefComponentType"/>
   </owl:Class>
   <owl:Class rdf:about="#RasterReliefType">
      <rdfs:comment>Type describing the raster component of a relief feature. As subclass of _CityObject, a RasterRelief
				inherits all attributes and relations, in particular an id, names, external references, and generalization relations.
			</rdfs:comment>
      <rdfs:subClassOf>
         <owl:Class>
            <owl:intersectionOf rdf:parseType="Collection">
               <owl:Restriction>
                  <owl:onProperty rdf:resource="#grid"/>
                  <owl:allValuesFrom rdf:resource="#gridPropertyType"/>
               </owl:Restriction>
               <owl:Restriction>
                  <owl:onProperty rdf:resource="#has_GenericApplicationPropertyOfRasterRelief"/>
                  <owl:allValuesFrom rdf:resource="#_GenericApplicationPropertyOfRasterRelief"/>
               </owl:Restriction>
               <owl:Restriction>
                  <owl:onProperty rdf:resource="#has_GenericApplicationPropertyOfRasterRelief"/>
                  <owl:minCardinality rdf:datatype="http://www.w3.org/2001/XMLSchema#nonNegativeInteger">0</owl:minCardinality>
               </owl:Restriction>
            </owl:intersectionOf>
         </owl:Class>
      </rdfs:subClassOf>
      <rdfs:subClassOf rdf:resource="#AbstractReliefComponentType"/>
   </owl:Class>
   <owl:Class rdf:about="#MassPointReliefType">
      <rdfs:comment>Type describing the mass point component of a relief feature. As subclass of _CityObject, a MassPoint
				Relief inherits all attributes and relations, in particular an id, names, external references, and generalization
				relations. </rdfs:comment>
      <rdfs:subClassOf>
         <owl:Class>
            <owl:intersectionOf rdf:parseType="Collection">
               <owl:Restriction>
                  <owl:onProperty rdf:resource="#reliefPoints"/>
                  <owl:allValuesFrom rdf:resource="gml:MultiPointPropertyType"/>
               </owl:Restriction>
               <owl:Restriction>
                  <owl:onProperty rdf:resource="#has_GenericApplicationPropertyOfMassPointRelief"/>
                  <owl:allValuesFrom rdf:resource="#_GenericApplicationPropertyOfMassPointRelief"/>
               </owl:Restriction>
               <owl:Restriction>
                  <owl:onProperty rdf:resource="#has_GenericApplicationPropertyOfMassPointRelief"/>
                  <owl:minCardinality rdf:datatype="http://www.w3.org/2001/XMLSchema#nonNegativeInteger">0</owl:minCardinality>
               </owl:Restriction>
            </owl:intersectionOf>
         </owl:Class>
      </rdfs:subClassOf>
      <rdfs:subClassOf rdf:resource="#AbstractReliefComponentType"/>
   </owl:Class>
   <owl:Class rdf:about="#BreaklineReliefType">
      <rdfs:comment>Type describing the break line Component of a relief feature. A break line relief consists of break lines
				or ridgeOrValleyLines. As subclass of _CityObject, a BreaklineRelief inherits all attributes and relations, in particular
				an id, names, external references, and generalization relations. </rdfs:comment>
      <rdfs:subClassOf>
         <owl:Class>
            <owl:intersectionOf rdf:parseType="Collection">
               <owl:Restriction>
                  <owl:onProperty rdf:resource="#ridgeOrValleyLines"/>
                  <owl:allValuesFrom rdf:resource="gml:MultiCurvePropertyType"/>
               </owl:Restriction>
               <owl:Restriction>
                  <owl:onProperty rdf:resource="#ridgeOrValleyLines"/>
                  <owl:minCardinality rdf:datatype="http://www.w3.org/2001/XMLSchema#nonNegativeInteger">0</owl:minCardinality>
               </owl:Restriction>
               <owl:Restriction>
                  <owl:onProperty rdf:resource="#breaklines"/>
                  <owl:allValuesFrom rdf:resource="gml:MultiCurvePropertyType"/>
               </owl:Restriction>
               <owl:Restriction>
                  <owl:onProperty rdf:resource="#breaklines"/>
                  <owl:minCardinality rdf:datatype="http://www.w3.org/2001/XMLSchema#nonNegativeInteger">0</owl:minCardinality>
               </owl:Restriction>
               <owl:Restriction>
                  <owl:onProperty rdf:resource="#has_GenericApplicationPropertyOfBreaklineRelief"/>
                  <owl:allValuesFrom rdf:resource="#_GenericApplicationPropertyOfBreaklineRelief"/>
               </owl:Restriction>
               <owl:Restriction>
                  <owl:onProperty rdf:resource="#has_GenericApplicationPropertyOfBreaklineRelief"/>
                  <owl:minCardinality rdf:datatype="http://www.w3.org/2001/XMLSchema#nonNegativeInteger">0</owl:minCardinality>
               </owl:Restriction>
            </owl:intersectionOf>
         </owl:Class>
      </rdfs:subClassOf>
      <rdfs:subClassOf rdf:resource="#AbstractReliefComponentType"/>
   </owl:Class>
   <owl:Class rdf:about="#tinPropertyType">
      <rdfs:comment>Denotes the relation of a TINRelief to its components. The tinPropertyType element must either carry a
				reference to a gml:TriangulatedSurface object or contain a gml:TriangulatedSurface object inline, but neither both nor
				none. </rdfs:comment>
      <rdfs:subClassOf>
         <owl:Class>
            <owl:intersectionOf rdf:parseType="Collection">
               <owl:Restriction>
                  <owl:onProperty rdf:resource="gml:hasTriangulatedSurface"/>
                  <owl:allValuesFrom rdf:resource="gml:TriangulatedSurface"/>
               </owl:Restriction>
            </owl:intersectionOf>
         </owl:Class>
      </rdfs:subClassOf>
   </owl:Class>
   <owl:Class rdf:about="#gridPropertyType">
      <rdfs:comment>Denotes the relation of a RasterReliefType to its components. The gridPropertyType element must either
				carry a reference to a gml:RectifiedGridCoverage object or contain a gml:RectifiedGridCoverage object inline, but neither
				both nor none. </rdfs:comment>
      <rdfs:subClassOf>
         <owl:Class>
            <owl:intersectionOf rdf:parseType="Collection">
               <owl:Restriction>
                  <owl:onProperty rdf:resource="gml:hasRectifiedGridCoverage"/>
                  <owl:allValuesFrom rdf:resource="gml:RectifiedGridCoverage"/>
               </owl:Restriction>
            </owl:intersectionOf>
         </owl:Class>
      </rdfs:subClassOf>
   </owl:Class>
   <owl:ObjectProperty rdf:about="gml:hasAssociationAttributeGroup">
      <rdfs:domain rdf:resource="#ReliefComponentPropertyType"/>
      <rdfs:range rdf:resource="gml:AssociationAttributeGroup"/>
   </owl:ObjectProperty>
   <owl:ObjectProperty rdf:about="gml:hasAssociationAttributeGroup">
      <rdfs:domain rdf:resource="#tinPropertyType"/>
      <rdfs:range rdf:resource="gml:AssociationAttributeGroup"/>
   </owl:ObjectProperty>
   <owl:ObjectProperty rdf:about="gml:hasAssociationAttributeGroup">
      <rdfs:domain rdf:resource="#gridPropertyType"/>
      <rdfs:range rdf:resource="gml:AssociationAttributeGroup"/>
   </owl:ObjectProperty>
   <owl:Class rdf:about="#ReliefFeature">
      <rdfs:subClassOf rdf:resource="core:_CityObject"/>
      <rdfs:subClassOf rdf:resource="#ReliefFeatureType"/>
   </owl:Class>
   <owl:Class rdf:about="#_GenericApplicationPropertyOfReliefFeature">
      <rdfs:subClassOf rdf:resource="http://www.w3.org/2001/XMLSchema#anyType"/>
      <rdfs:comment>Warning: This class type was declared outside of its original schema. This class may be declared incorrectly.</rdfs:comment>
   </owl:Class>
   <owl:Class rdf:about="#_ReliefComponent">
      <rdfs:subClassOf rdf:resource="core:_CityObject"/>
      <rdfs:subClassOf rdf:resource="#AbstractReliefComponentType"/>
   </owl:Class>
   <owl:Class rdf:about="#_GenericApplicationPropertyOfReliefComponent">
      <rdfs:subClassOf rdf:resource="http://www.w3.org/2001/XMLSchema#anyType"/>
      <rdfs:comment>Warning: This class type was declared outside of its original schema. This class may be declared incorrectly.</rdfs:comment>
   </owl:Class>
   <owl:Class rdf:about="#TINRelief">
      <rdfs:subClassOf rdf:resource="#_ReliefComponent"/>
      <rdfs:subClassOf rdf:resource="#TINReliefType"/>
   </owl:Class>
   <owl:Class rdf:about="#_GenericApplicationPropertyOfTinRelief">
      <rdfs:subClassOf rdf:resource="http://www.w3.org/2001/XMLSchema#anyType"/>
      <rdfs:comment>Warning: This class type was declared outside of its original schema. This class may be declared incorrectly.</rdfs:comment>
   </owl:Class>
   <owl:Class rdf:about="#RasterRelief">
      <rdfs:subClassOf rdf:resource="#_ReliefComponent"/>
      <rdfs:subClassOf rdf:resource="#RasterReliefType"/>
   </owl:Class>
   <owl:Class rdf:about="#_GenericApplicationPropertyOfRasterRelief">
      <rdfs:subClassOf rdf:resource="http://www.w3.org/2001/XMLSchema#anyType"/>
      <rdfs:comment>Warning: This class type was declared outside of its original schema. This class may be declared incorrectly.</rdfs:comment>
   </owl:Class>
   <owl:Class rdf:about="#MassPointRelief">
      <rdfs:subClassOf rdf:resource="#_ReliefComponent"/>
      <rdfs:subClassOf rdf:resource="#MassPointReliefType"/>
   </owl:Class>
   <owl:Class rdf:about="#_GenericApplicationPropertyOfMassPointRelief">
      <rdfs:subClassOf rdf:resource="http://www.w3.org/2001/XMLSchema#anyType"/>
      <rdfs:comment>Warning: This class type was declared outside of its original schema. This class may be declared incorrectly.</rdfs:comment>
   </owl:Class>
   <owl:Class rdf:about="#BreaklineRelief">
      <rdfs:subClassOf rdf:resource="#_ReliefComponent"/>
      <rdfs:subClassOf rdf:resource="#BreaklineReliefType"/>
   </owl:Class>
   <owl:Class rdf:about="#_GenericApplicationPropertyOfBreaklineRelief">
      <rdfs:subClassOf rdf:resource="http://www.w3.org/2001/XMLSchema#anyType"/>
      <rdfs:comment>Warning: This class type was declared outside of its original schema. This class may be declared incorrectly.</rdfs:comment>
   </owl:Class>
   <owl:Class rdf:about="#Elevation">
      <rdfs:subClassOf rdf:resource="gml:_Object"/>
      <rdfs:subClassOf rdf:resource="gml:LengthType"/>
      <rdfs:comment>Warning: This class type was declared outside of its original schema. This class may be declared incorrectly.</rdfs:comment>
   </owl:Class>
   <owl:ObjectProperty rdf:about="#lod">
      <rdfs:comment>Warning: This ObjectProperty type was declared outside of its original schema. This ObjectProperty may be declared incorrectly.</rdfs:comment>
      <rdfs:domain rdf:resource="#ReliefFeatureType"/>
      <rdfs:range rdf:resource="core:integerBetween0and4"/>
   </owl:ObjectProperty>
   <owl:ObjectProperty rdf:about="#reliefComponent">
      <rdfs:domain rdf:resource="#ReliefFeatureType"/>
      <rdfs:range rdf:resource="#ReliefComponentPropertyType"/>
   </owl:ObjectProperty>
   <owl:ObjectProperty rdf:about="#has_GenericApplicationPropertyOfReliefFeature">
      <rdfs:domain rdf:resource="#ReliefFeatureType"/>
      <rdfs:range rdf:resource="#_GenericApplicationPropertyOfReliefFeature"/>
   </owl:ObjectProperty>
   <owl:ObjectProperty rdf:about="#lod">
      <rdfs:comment>Warning: This ObjectProperty type was declared outside of its original schema. This ObjectProperty may be declared incorrectly.</rdfs:comment>
      <rdfs:domain rdf:resource="#AbstractReliefComponentType"/>
      <rdfs:range rdf:resource="core:integerBetween0and4"/>
   </owl:ObjectProperty>
   <owl:ObjectProperty rdf:about="#extent">
      <rdfs:comment>Warning: This ObjectProperty type was declared outside of its original schema. This ObjectProperty may be declared incorrectly.</rdfs:comment>
      <rdfs:domain rdf:resource="#AbstractReliefComponentType"/>
      <rdfs:range rdf:resource="gml:PolygonPropertyType"/>
   </owl:ObjectProperty>
   <owl:ObjectProperty rdf:about="#has_GenericApplicationPropertyOfReliefComponent">
      <rdfs:domain rdf:resource="#AbstractReliefComponentType"/>
      <rdfs:range rdf:resource="#_GenericApplicationPropertyOfReliefComponent"/>
   </owl:ObjectProperty>
   <owl:ObjectProperty rdf:about="#has_ReliefComponent">
      <rdfs:domain rdf:resource="#ReliefComponentPropertyType"/>
      <rdfs:range rdf:resource="#_ReliefComponent"/>
   </owl:ObjectProperty>
   <owl:ObjectProperty rdf:about="#tin">
      <rdfs:domain rdf:resource="#TINReliefType"/>
      <rdfs:range rdf:resource="#tinPropertyType"/>
   </owl:ObjectProperty>
   <owl:ObjectProperty rdf:about="#has_GenericApplicationPropertyOfTinRelief">
      <rdfs:domain rdf:resource="#TINReliefType"/>
      <rdfs:range rdf:resource="#_GenericApplicationPropertyOfTinRelief"/>
   </owl:ObjectProperty>
   <owl:ObjectProperty rdf:about="#grid">
      <rdfs:domain rdf:resource="#RasterReliefType"/>
      <rdfs:range rdf:resource="#gridPropertyType"/>
   </owl:ObjectProperty>
   <owl:ObjectProperty rdf:about="#has_GenericApplicationPropertyOfRasterRelief">
      <rdfs:domain rdf:resource="#RasterReliefType"/>
      <rdfs:range rdf:resource="#_GenericApplicationPropertyOfRasterRelief"/>
   </owl:ObjectProperty>
   <owl:ObjectProperty rdf:about="#reliefPoints">
      <rdfs:comment>Warning: This ObjectProperty type was declared outside of its original schema. This ObjectProperty may be declared incorrectly.</rdfs:comment>
      <rdfs:domain rdf:resource="#MassPointReliefType"/>
      <rdfs:range rdf:resource="gml:MultiPointPropertyType"/>
   </owl:ObjectProperty>
   <owl:ObjectProperty rdf:about="#has_GenericApplicationPropertyOfMassPointRelief">
      <rdfs:domain rdf:resource="#MassPointReliefType"/>
      <rdfs:range rdf:resource="#_GenericApplicationPropertyOfMassPointRelief"/>
   </owl:ObjectProperty>
   <owl:ObjectProperty rdf:about="#ridgeOrValleyLines">
      <rdfs:comment>Warning: This ObjectProperty type was declared outside of its original schema. This ObjectProperty may be declared incorrectly.</rdfs:comment>
      <rdfs:domain rdf:resource="#BreaklineReliefType"/>
      <rdfs:range rdf:resource="gml:MultiCurvePropertyType"/>
   </owl:ObjectProperty>
   <owl:ObjectProperty rdf:about="#breaklines">
      <rdfs:comment>Warning: This ObjectProperty type was declared outside of its original schema. This ObjectProperty may be declared incorrectly.</rdfs:comment>
      <rdfs:domain rdf:resource="#BreaklineReliefType"/>
      <rdfs:range rdf:resource="gml:MultiCurvePropertyType"/>
   </owl:ObjectProperty>
   <owl:ObjectProperty rdf:about="#has_GenericApplicationPropertyOfBreaklineRelief">
      <rdfs:domain rdf:resource="#BreaklineReliefType"/>
      <rdfs:range rdf:resource="#_GenericApplicationPropertyOfBreaklineRelief"/>
   </owl:ObjectProperty>
   <owl:ObjectProperty rdf:about="gml:hasTriangulatedSurface">
      <rdfs:comment>Warning: This ObjectProperty reference was declared outside of its original schema. This ObjectProperty may be declared incorrectly.</rdfs:comment>
      <rdfs:domain rdf:resource="#tinPropertyType"/>
      <rdfs:range rdf:resource="gml:TriangulatedSurface"/>
   </owl:ObjectProperty>
   <owl:ObjectProperty rdf:about="gml:hasRectifiedGridCoverage">
      <rdfs:comment>Warning: This ObjectProperty reference was declared outside of its original schema. This ObjectProperty may be declared incorrectly.</rdfs:comment>
      <rdfs:domain rdf:resource="#gridPropertyType"/>
      <rdfs:range rdf:resource="gml:RectifiedGridCoverage"/>
   </owl:ObjectProperty>
</rdf:RDF>
