<rdf:RDF xmlns:math="http://www.w3.org/2005/xpath-functions/math" xmlns:owl="http://www.w3.org/2002/07/owl#" xmlns:rdf="http://www.w3.org/1999/02/22-rdf-syntax-ns#" xmlns:rdfs="http://www.w3.org/2000/01/rdf-schema#" xmlns:xs="http://www.w3.org/2001/XMLSchema" xmlns:xsd="http://www.w3.org/2001/XMLSchema">
   <owl:Ontology rdf:about="http://liris.cnrs.fr/ontologies/temporal">
      <owl:imports rdf:resource="http://liris.cnrs.fr/ontologies/gml"/>
      <owl:imports rdf:resource="http://liris.cnrs.fr/ontologies/gmlBase"/>
      <rdfs:seeAlso>urn:opengis:specification:gml:schema-xsd:temporal:3.1.1</rdfs:seeAlso>
      <rdfs:comment xml:lang="en">The temporal schema for GML 3.1 provides constructs for handling time-varying spatial data. 
    This schema reflects a partial implementation of the model described in ISO 19108:2002.
    
    GML is an OGC Standard.
    Copyright (c) 2001,2005,2010 Open Geospatial Consortium.
    To obtain additional rights of use, visit http://www.opengeospatial.org/legal/ .
		</rdfs:comment>
   </owl:Ontology>
   <owl:Class rdf:about="http://www.opengis.net/gml#AbstractTimeObjectType">
      <rdfs:comment>This is an abstract class</rdfs:comment>
      <rdfs:comment xml:lang="en">The abstract supertype for temporal objects.</rdfs:comment>
      <rdfs:subClassOf rdf:resource="http://www.opengis.net/gml#AbstractGMLType"/>
      <rdfs:comment>Warning: The parent class 'gml:AbstractGMLType' is declared outside of this class' original schema. This class may be declared incorrectly.</rdfs:comment>
   </owl:Class>
   <owl:Class rdf:about="http://www.opengis.net/gml#AbstractTimePrimitiveType">
      <rdfs:comment>This is an abstract class</rdfs:comment>
      <rdfs:comment xml:lang="en">The abstract supertype for temporal primitives.</rdfs:comment>
      <rdfs:subClassOf>
         <owl:Class>
            <owl:intersectionOf rdf:parseType="Collection">
               <owl:Restriction>
                  <owl:onProperty rdf:resource="http://www.opengis.net/gml#relatedTime"/>
                  <owl:allValuesFrom rdf:resource="http://www.opengis.net/gml#RelatedTimeType"/>
               </owl:Restriction>
               <owl:Restriction>
                  <owl:onProperty rdf:resource="http://www.opengis.net/gml#relatedTime"/>
                  <owl:minCardinality rdf:datatype="http://www.w3.org/2001/XMLSchema#nonNegativeInteger">0</owl:minCardinality>
               </owl:Restriction>
            </owl:intersectionOf>
         </owl:Class>
      </rdfs:subClassOf>
      <rdfs:subClassOf rdf:resource="http://www.opengis.net/gml#AbstractTimeObjectType"/>
      <rdfs:comment>Warning: The parent class 'gml:AbstractTimeObjectType' is declared outside of this class' original schema. This class may be declared incorrectly.</rdfs:comment>
   </owl:Class>
   <owl:Class rdf:about="http://www.opengis.net/gml#TimePrimitivePropertyType">
      <rdfs:subClassOf>
         <owl:Class>
            <owl:intersectionOf rdf:parseType="Collection">
               <owl:Restriction>
                  <owl:onProperty rdf:resource="http://www.opengis.net/gml#has_TimePrimitive"/>
                  <owl:allValuesFrom rdf:resource="http://www.opengis.net/gml#_TimePrimitive"/>
               </owl:Restriction>
            </owl:intersectionOf>
         </owl:Class>
      </rdfs:subClassOf>
   </owl:Class>
   <owl:Class rdf:about="http://www.opengis.net/gml#RelatedTimeType">
      <rdfs:subClassOf>
         <owl:Class>
            <owl:intersectionOf rdf:parseType="Collection">
               <owl:Restriction>
                  <owl:onProperty rdf:resource="http://www.opengis.net/gml#relativePosition"/>
                  <owl:allValuesFrom rdf:resource="http://www.w3.org/2001/XMLSchema#string"/>
               </owl:Restriction>
            </owl:intersectionOf>
         </owl:Class>
      </rdfs:subClassOf>
      <rdfs:subClassOf rdf:resource="http://www.opengis.net/gml#TimePrimitivePropertyType"/>
      <rdfs:comment>Warning: The parent class 'gml:TimePrimitivePropertyType' is declared outside of this class' original schema. This class may be declared incorrectly.</rdfs:comment>
   </owl:Class>
   <owl:Class rdf:about="http://www.opengis.net/gml#AbstractTimeComplexType">
      <rdfs:comment>This is an abstract class</rdfs:comment>
      <rdfs:comment xml:lang="en">The abstract supertype for temporal complexes.</rdfs:comment>
      <rdfs:subClassOf rdf:resource="http://www.opengis.net/gml#AbstractTimeObjectType"/>
      <rdfs:comment>Warning: The parent class 'gml:AbstractTimeObjectType' is declared outside of this class' original schema. This class may be declared incorrectly.</rdfs:comment>
   </owl:Class>
   <owl:Class rdf:about="http://www.opengis.net/gml#AbstractTimeGeometricPrimitiveType">
      <rdfs:comment>This is an abstract class</rdfs:comment>
      <rdfs:comment xml:lang="en">The abstract supertype for temporal geometric primitives.
       A temporal geometry must be associated with a temporal reference system via URI. 
       The Gregorian calendar with UTC is the default reference system, following ISO 
       8601. Other reference systems in common use include the GPS calendar and the 
       Julian calendar.</rdfs:comment>
      <rdfs:subClassOf>
         <owl:Class>
            <owl:intersectionOf rdf:parseType="Collection">
               <owl:Restriction>
                  <owl:onProperty rdf:resource="http://www.opengis.net/gml#frame"/>
                  <owl:allValuesFrom rdf:resource="http://www.w3.org/2001/XMLSchema#anyURI"/>
               </owl:Restriction>
            </owl:intersectionOf>
         </owl:Class>
      </rdfs:subClassOf>
      <rdfs:subClassOf rdf:resource="http://www.opengis.net/gml#AbstractTimePrimitiveType"/>
      <rdfs:comment>Warning: The parent class 'gml:AbstractTimePrimitiveType' is declared outside of this class' original schema. This class may be declared incorrectly.</rdfs:comment>
   </owl:Class>
   <owl:Class rdf:about="http://www.opengis.net/gml#TimeGeometricPrimitivePropertyType">
      <rdfs:subClassOf>
         <owl:Class>
            <owl:intersectionOf rdf:parseType="Collection">
               <owl:Restriction>
                  <owl:onProperty rdf:resource="http://www.opengis.net/gml#has_TimeGeometricPrimitive"/>
                  <owl:allValuesFrom rdf:resource="http://www.opengis.net/gml#_TimeGeometricPrimitive"/>
               </owl:Restriction>
            </owl:intersectionOf>
         </owl:Class>
      </rdfs:subClassOf>
   </owl:Class>
   <owl:Class rdf:about="http://www.opengis.net/gml#TimeInstantType">
      <rdfs:comment>Omit back-pointers begunBy, endedBy.</rdfs:comment>
      <rdfs:subClassOf>
         <owl:Class>
            <owl:intersectionOf rdf:parseType="Collection">
               <owl:Restriction>
                  <owl:onProperty rdf:resource="http://www.opengis.net/gml#hastimePosition"/>
                  <owl:allValuesFrom rdf:resource="http://www.opengis.net/gml#timePosition"/>
               </owl:Restriction>
            </owl:intersectionOf>
         </owl:Class>
      </rdfs:subClassOf>
      <rdfs:subClassOf rdf:resource="http://www.opengis.net/gml#AbstractTimeGeometricPrimitiveType"/>
      <rdfs:comment>Warning: The parent class 'gml:AbstractTimeGeometricPrimitiveType' is declared outside of this class' original schema. This class may be declared incorrectly.</rdfs:comment>
   </owl:Class>
   <owl:Class rdf:about="http://www.opengis.net/gml#TimeInstantPropertyType">
      <rdfs:subClassOf>
         <owl:Class>
            <owl:intersectionOf rdf:parseType="Collection">
               <owl:Restriction>
                  <owl:onProperty rdf:resource="http://www.opengis.net/gml#hasTimeInstant"/>
                  <owl:allValuesFrom rdf:resource="http://www.opengis.net/gml#TimeInstant"/>
               </owl:Restriction>
            </owl:intersectionOf>
         </owl:Class>
      </rdfs:subClassOf>
   </owl:Class>
   <owl:Class rdf:about="http://www.opengis.net/gml#TimePeriodType">
      <rdfs:subClassOf>
         <owl:Class>
            <owl:intersectionOf rdf:parseType="Collection"/>
         </owl:Class>
      </rdfs:subClassOf>
      <owl:disjointUnionOf rdf:parseType="Collection">
         <owl:Restriction>
            <owl:onProperty rdf:resource="http://www.opengis.net/gml#beginPosition"/>
            <owl:allValuesFrom rdf:resource="http://www.opengis.net/gml#TimePositionType"/>
         </owl:Restriction>
         <owl:Restriction>
            <owl:onProperty rdf:resource="http://www.opengis.net/gml#begin"/>
            <owl:allValuesFrom rdf:resource="http://www.opengis.net/gml#TimeInstantPropertyType"/>
         </owl:Restriction>
      </owl:disjointUnionOf>
      <owl:disjointUnionOf rdf:parseType="Collection">
         <owl:Restriction>
            <owl:onProperty rdf:resource="http://www.opengis.net/gml#endPosition"/>
            <owl:allValuesFrom rdf:resource="http://www.opengis.net/gml#TimePositionType"/>
         </owl:Restriction>
         <owl:Restriction>
            <owl:onProperty rdf:resource="http://www.opengis.net/gml#end"/>
            <owl:allValuesFrom rdf:resource="http://www.opengis.net/gml#TimeInstantPropertyType"/>
         </owl:Restriction>
      </owl:disjointUnionOf>
      <owl:ObjectProperty rdf:about="http://www.opengis.net/gml#hastimeLength">
         <rdfs:domain rdf:resource="http://www.opengis.net/gml#TimePeriodType"/>
         <rdfs:range rdf:resource="http://www.opengis.net/gml#timeLength"/>
      </owl:ObjectProperty>
      <rdfs:subClassOf rdf:resource="http://www.opengis.net/gml#AbstractTimeGeometricPrimitiveType"/>
      <rdfs:comment>Warning: The parent class 'gml:AbstractTimeGeometricPrimitiveType' is declared outside of this class' original schema. This class may be declared incorrectly.</rdfs:comment>
   </owl:Class>
   <owl:Class rdf:about="http://www.opengis.net/gml#TimePeriodPropertyType">
      <rdfs:subClassOf>
         <owl:Class>
            <owl:intersectionOf rdf:parseType="Collection">
               <owl:Restriction>
                  <owl:onProperty rdf:resource="http://www.opengis.net/gml#hasTimePeriod"/>
                  <owl:allValuesFrom rdf:resource="http://www.opengis.net/gml#TimePeriod"/>
               </owl:Restriction>
            </owl:intersectionOf>
         </owl:Class>
      </rdfs:subClassOf>
   </owl:Class>
   <owl:Class rdf:about="http://www.opengis.net/gml#TimeIntervalLengthType">
      <rdfs:comment xml:lang="en">This type extends the built-in xsd:decimal simple type to allow floating-point 
      values for temporal length. According to  the ISO 11404 model you have to use 
      positiveInteger together with appropriate values for radix and factor. The 
      resolution of the time interval is to one radix ^(-factor) of the specified 
      time unit (e.g. unit="second", radix="10", factor="3" specifies a resolution 
      of milliseconds). It is a subtype of TimeDurationType.</rdfs:comment>
      <rdfs:subClassOf>
         <owl:Class>
            <owl:intersectionOf rdf:parseType="Collection">
               <owl:Restriction>
                  <owl:onProperty rdf:resource="http://www.opengis.net/gml#unit"/>
                  <owl:allValuesFrom rdf:resource="http://www.opengis.net/gml#TimeUnitType"/>
               </owl:Restriction>
               <owl:Restriction>
                  <owl:onProperty rdf:resource="http://www.opengis.net/gml#radix"/>
                  <owl:allValuesFrom rdf:resource="http://www.w3.org/2001/XMLSchema#positiveInteger"/>
               </owl:Restriction>
               <owl:Restriction>
                  <owl:onProperty rdf:resource="http://www.opengis.net/gml#factor"/>
                  <owl:allValuesFrom rdf:resource="http://www.w3.org/2001/XMLSchema#integer"/>
               </owl:Restriction>
            </owl:intersectionOf>
         </owl:Class>
      </rdfs:subClassOf>
   </owl:Class>
   <owl:DatatypeProperty rdf:about="http://www.opengis.net/gml#hasTimeIntervalLengthType">
      <rdfs:domain rdf:resource="http://www.opengis.net/gml#TimeIntervalLengthType"/>
      <rdfs:range rdf:resource="http://www.opengis.net/gml#decimal"/>
      <rdfs:subPropertyOf rdf:resource="http://www.opengis.net/gml#hasdecimal"/>
   </owl:DatatypeProperty>
   <owl:Class rdf:about="http://www.opengis.net/gml#TimePositionType">
      <rdfs:comment xml:lang="en">Direct representation of a temporal position. 
      Indeterminate time values are also allowed, as described in ISO 19108. The indeterminatePosition 
      attribute can be used alone or it can qualify a specific value for temporal position (e.g. before 
      2002-12, after 1019624400). 
      For time values that identify position within a calendar, the calendarEraName attribute provides 
      the name of the calendar era to which the date is referenced (e.g. the Meiji era of the Japanese calendar).</rdfs:comment>
      <rdfs:subClassOf>
         <owl:Class>
            <owl:intersectionOf rdf:parseType="Collection">
               <owl:Restriction>
                  <owl:onProperty rdf:resource="http://www.opengis.net/gml#frame"/>
                  <owl:allValuesFrom rdf:resource="http://www.w3.org/2001/XMLSchema#anyURI"/>
               </owl:Restriction>
               <owl:Restriction>
                  <owl:onProperty rdf:resource="http://www.opengis.net/gml#calendarEraName"/>
                  <owl:allValuesFrom rdf:resource="http://www.w3.org/2001/XMLSchema#string"/>
               </owl:Restriction>
               <owl:Restriction>
                  <owl:onProperty rdf:resource="http://www.opengis.net/gml#indeterminatePosition"/>
                  <owl:allValuesFrom rdf:resource="http://www.opengis.net/gml#TimeIndeterminateValueType"/>
               </owl:Restriction>
            </owl:intersectionOf>
         </owl:Class>
      </rdfs:subClassOf>
      <rdfs:subClassOf rdf:resource="http://www.opengis.net/gml#TimePositionUnion"/>
      <rdfs:comment>Warning: The parent class 'gml:TimePositionUnion' is declared outside of this class' original schema. This class may be declared incorrectly.</rdfs:comment>
   </owl:Class>
   <owl:DatatypeProperty rdf:about="http://www.opengis.net/gml#hasTimePositionType">
      <rdfs:domain rdf:resource="http://www.opengis.net/gml#TimePositionType"/>
      <rdfs:range rdf:resource="http://www.opengis.net/gml#TimePositionUnion"/>
      <rdfs:subPropertyOf rdf:resource="http://www.opengis.net/gml#hasTimePositionUnion"/>
      <rdfs:comment>Warning: The parent property 'gml:hasTimePositionUnion' is declared outside of this property's original schema. This property may be declared incorrectly.</rdfs:comment>
   </owl:DatatypeProperty>
   <owl:ObjectProperty rdf:about="http://www.opengis.net/gml#hastimeLength">
      <rdfs:domain rdf:resource="http://www.opengis.net/gml#TimePeriodType"/>
      <rdfs:range rdf:resource="http://www.opengis.net/gml#timeLength"/>
   </owl:ObjectProperty>
   <owl:Class rdf:about="http://www.opengis.net/gml#timeLength">
      <rdfs:subClassOf>
         <owl:Class>
            <owl:intersectionOf rdf:parseType="Collection"/>
         </owl:Class>
      </rdfs:subClassOf>
      <owl:disjointUnionOf rdf:parseType="Collection">
         <owl:Restriction>
            <owl:onProperty rdf:resource="http://www.opengis.net/gml#hasduration"/>
            <owl:allValuesFrom rdf:resource="http://www.opengis.net/gml#duration"/>
         </owl:Restriction>
         <owl:Restriction>
            <owl:onProperty rdf:resource="http://www.opengis.net/gml#hastimeInterval"/>
            <owl:allValuesFrom rdf:resource="http://www.opengis.net/gml#timeInterval"/>
         </owl:Restriction>
      </owl:disjointUnionOf>
      <rdfs:comment>This model group is provided as an alternative to the abstract susbstitutionGroup head _timeLength.
		ISO 19136 comment 411</rdfs:comment>
   </owl:Class>
   <owl:ObjectProperty rdf:about="http://www.opengis.net/gml#hasAssociationAttributeGroup">
      <rdfs:domain rdf:resource="http://www.opengis.net/gml#TimePrimitivePropertyType"/>
      <rdfs:range rdf:resource="http://www.opengis.net/gml#AssociationAttributeGroup"/>
   </owl:ObjectProperty>
   <owl:ObjectProperty rdf:about="http://www.opengis.net/gml#hasAssociationAttributeGroup">
      <rdfs:domain rdf:resource="http://www.opengis.net/gml#TimeGeometricPrimitivePropertyType"/>
      <rdfs:range rdf:resource="http://www.opengis.net/gml#AssociationAttributeGroup"/>
   </owl:ObjectProperty>
   <owl:ObjectProperty rdf:about="http://www.opengis.net/gml#hasAssociationAttributeGroup">
      <rdfs:domain rdf:resource="http://www.opengis.net/gml#TimeInstantPropertyType"/>
      <rdfs:range rdf:resource="http://www.opengis.net/gml#AssociationAttributeGroup"/>
   </owl:ObjectProperty>
   <owl:ObjectProperty rdf:about="http://www.opengis.net/gml#hasAssociationAttributeGroup">
      <rdfs:domain rdf:resource="http://www.opengis.net/gml#TimePeriodPropertyType"/>
      <rdfs:range rdf:resource="http://www.opengis.net/gml#AssociationAttributeGroup"/>
   </owl:ObjectProperty>
   <rdfs:Datatype rdf:about="http://www.opengis.net/gml#relativePosition">
      <owl:equivalentClass>
         <rdfs:Datatype>
            <owl:oneOf>
               <rdf:Description rdf:type="http://www.w3.org/1999/02/22-rdf-syntax-ns#List">
                  <rdf:first rdf:datatype="string">Before</rdf:first>
                  <rdf:rest>
                     <rdf:Description rdf:type="http://www.w3.org/1999/02/22-rdf-syntax-ns#List">
                        <rdf:first rdf:datatype="string">After</rdf:first>
                        <rdf:rest>
                           <rdf:Description rdf:type="http://www.w3.org/1999/02/22-rdf-syntax-ns#List">
                              <rdf:first rdf:datatype="string">Begins</rdf:first>
                              <rdf:rest>
                                 <rdf:Description rdf:type="http://www.w3.org/1999/02/22-rdf-syntax-ns#List">
                                    <rdf:first rdf:datatype="string">Ends</rdf:first>
                                    <rdf:rest>
                                       <rdf:Description rdf:type="http://www.w3.org/1999/02/22-rdf-syntax-ns#List">
                                          <rdf:first rdf:datatype="string">During</rdf:first>
                                          <rdf:rest>
                                             <rdf:Description rdf:type="http://www.w3.org/1999/02/22-rdf-syntax-ns#List">
                                                <rdf:first rdf:datatype="string">Equals</rdf:first>
                                                <rdf:rest>
                                                   <rdf:Description rdf:type="http://www.w3.org/1999/02/22-rdf-syntax-ns#List">
                                                      <rdf:first rdf:datatype="string">Contains</rdf:first>
                                                      <rdf:rest>
                                                         <rdf:Description rdf:type="http://www.w3.org/1999/02/22-rdf-syntax-ns#List">
                                                            <rdf:first rdf:datatype="string">Overlaps</rdf:first>
                                                            <rdf:rest>
                                                               <rdf:Description rdf:type="http://www.w3.org/1999/02/22-rdf-syntax-ns#List">
                                                                  <rdf:first rdf:datatype="string">Meets</rdf:first>
                                                                  <rdf:rest>
                                                                     <rdf:Description rdf:type="http://www.w3.org/1999/02/22-rdf-syntax-ns#List">
                                                                        <rdf:first rdf:datatype="string">OverlappedBy</rdf:first>
                                                                        <rdf:rest>
                                                                           <rdf:Description rdf:type="http://www.w3.org/1999/02/22-rdf-syntax-ns#List">
                                                                              <rdf:first rdf:datatype="string">MetBy</rdf:first>
                                                                              <rdf:rest>
                                                                                 <rdf:Description rdf:type="http://www.w3.org/1999/02/22-rdf-syntax-ns#List">
                                                                                    <rdf:first rdf:datatype="string">BegunBy</rdf:first>
                                                                                    <rdf:rest>
                                                                                       <rdf:Description rdf:type="http://www.w3.org/1999/02/22-rdf-syntax-ns#List">
                                                                                          <rdf:first rdf:datatype="string">EndedBy</rdf:first>
                                                                                          <rdf:rest rdf:resource="http://www.w3.org/1999/02/22-rdf-syntax-ns#nil"/>
                                                                                       </rdf:Description>
                                                                                    </rdf:rest>
                                                                                 </rdf:Description>
                                                                              </rdf:rest>
                                                                           </rdf:Description>
                                                                        </rdf:rest>
                                                                     </rdf:Description>
                                                                  </rdf:rest>
                                                               </rdf:Description>
                                                            </rdf:rest>
                                                         </rdf:Description>
                                                      </rdf:rest>
                                                   </rdf:Description>
                                                </rdf:rest>
                                             </rdf:Description>
                                          </rdf:rest>
                                       </rdf:Description>
                                    </rdf:rest>
                                 </rdf:Description>
                              </rdf:rest>
                           </rdf:Description>
                        </rdf:rest>
                     </rdf:Description>
                  </rdf:rest>
               </rdf:Description>
            </owl:oneOf>
         </rdfs:Datatype>
      </owl:equivalentClass>
   </rdfs:Datatype>
   <owl:DatatypeProperty rdf:about="http://www.opengis.net/gml#hasrelativePosition">
      <rdfs:range rdf:resource="http://www.opengis.net/gml#relativePosition"/>
   </owl:DatatypeProperty>
   <rdfs:Datatype rdf:about="http://www.opengis.net/gml#TimeUnitType">
      <rdfs:comment xml:lang="en">Standard units for measuring time intervals (see ISO 31-1).</rdfs:comment>
      <owl:equivalentClass>
         <rdfs:Datatype>
            <owl:oneOf>
               <rdf:Description rdf:type="http://www.w3.org/1999/02/22-rdf-syntax-ns#List">
                  <rdf:first rdf:datatype="string">year</rdf:first>
                  <rdf:rest>
                     <rdf:Description rdf:type="http://www.w3.org/1999/02/22-rdf-syntax-ns#List">
                        <rdf:first rdf:datatype="string">day</rdf:first>
                        <rdf:rest>
                           <rdf:Description rdf:type="http://www.w3.org/1999/02/22-rdf-syntax-ns#List">
                              <rdf:first rdf:datatype="string">hour</rdf:first>
                              <rdf:rest>
                                 <rdf:Description rdf:type="http://www.w3.org/1999/02/22-rdf-syntax-ns#List">
                                    <rdf:first rdf:datatype="string">minute</rdf:first>
                                    <rdf:rest>
                                       <rdf:Description rdf:type="http://www.w3.org/1999/02/22-rdf-syntax-ns#List">
                                          <rdf:first rdf:datatype="string">second</rdf:first>
                                          <rdf:rest rdf:resource="http://www.w3.org/1999/02/22-rdf-syntax-ns#nil"/>
                                       </rdf:Description>
                                    </rdf:rest>
                                 </rdf:Description>
                              </rdf:rest>
                           </rdf:Description>
                        </rdf:rest>
                     </rdf:Description>
                  </rdf:rest>
               </rdf:Description>
            </owl:oneOf>
         </rdfs:Datatype>
      </owl:equivalentClass>
   </rdfs:Datatype>
   <rdfs:Datatype rdf:about="http://www.opengis.net/gml#TimePositionUnion">
      <rdfs:comment xml:lang="en">The ISO 19108:2002 hierarchy of subtypes for temporal position are collapsed 
      by defining a union of XML Schema simple types for indicating temporal position relative 
      to a specific reference system. 
      
      Dates and dateTime may be indicated with varying degrees of precision.  
      dateTime by itself does not allow right-truncation, except for fractions of seconds. 
      When used with non-Gregorian calendars based on years, months, days, 
      the same lexical representation should still be used, with leading zeros added if the 
      year value would otherwise have fewer than four digits.  
      
      An ordinal position may be referenced via URI identifying the definition of an ordinal era.  
      
      A time coordinate value is indicated as a decimal (e.g. UNIX time, GPS calendar).</rdfs:comment>
      <owl:equivalentClass rdf:resource="http://www.opengis.net/gml#CalDate"/>
      <owl:equivalentClass rdf:resource="http://www.opengis.net/gml#time"/>
      <owl:equivalentClass rdf:resource="http://www.opengis.net/gml#dateTime"/>
      <owl:equivalentClass rdf:resource="http://www.opengis.net/gml#anyURI"/>
      <owl:equivalentClass rdf:resource="http://www.opengis.net/gml#decimal"/>
   </rdfs:Datatype>
   <rdfs:Datatype rdf:about="http://www.opengis.net/gml#CalDate">
      <rdfs:comment xml:lang="en">Calendar dates may be indicated with varying degrees of precision, 
      using year, year-month, date. 
      When used with non-Gregorian calendars based on years, months, days, 
      the same lexical representation should still be used, with leading zeros added if the 
      year value would otherwise have fewer than four digits.  
      time is used for a position that recurs daily (see clause 5.4.4.2 of ISO 19108:2002).</rdfs:comment>
      <owl:equivalentClass rdf:resource="http://www.opengis.net/gml#date"/>
      <owl:equivalentClass rdf:resource="http://www.opengis.net/gml#gYearMonth"/>
      <owl:equivalentClass rdf:resource="http://www.opengis.net/gml#gYear"/>
   </rdfs:Datatype>
   <rdfs:Datatype rdf:about="http://www.opengis.net/gml#TimeIndeterminateValueType">
      <rdfs:comment xml:lang="en">This enumerated data type specifies values for indeterminate positions.</rdfs:comment>
      <owl:equivalentClass>
         <rdfs:Datatype>
            <owl:oneOf>
               <rdf:Description rdf:type="http://www.w3.org/1999/02/22-rdf-syntax-ns#List">
                  <rdf:first rdf:datatype="string">after</rdf:first>
                  <rdf:rest>
                     <rdf:Description rdf:type="http://www.w3.org/1999/02/22-rdf-syntax-ns#List">
                        <rdf:first rdf:datatype="string">before</rdf:first>
                        <rdf:rest>
                           <rdf:Description rdf:type="http://www.w3.org/1999/02/22-rdf-syntax-ns#List">
                              <rdf:first rdf:datatype="string">now</rdf:first>
                              <rdf:rest>
                                 <rdf:Description rdf:type="http://www.w3.org/1999/02/22-rdf-syntax-ns#List">
                                    <rdf:first rdf:datatype="string">unknown</rdf:first>
                                    <rdf:rest rdf:resource="http://www.w3.org/1999/02/22-rdf-syntax-ns#nil"/>
                                 </rdf:Description>
                              </rdf:rest>
                           </rdf:Description>
                        </rdf:rest>
                     </rdf:Description>
                  </rdf:rest>
               </rdf:Description>
            </owl:oneOf>
         </rdfs:Datatype>
      </owl:equivalentClass>
   </rdfs:Datatype>
   <owl:DatatypeProperty rdf:about="http://www.opengis.net/gml#relativePosition">
      <rdfs:domain rdf:resource="http://www.opengis.net/gml#RelatedTimeType"/>
      <rdfs:range rdf:resource="http://www.w3.org/2001/XMLSchema#string"/>
   </owl:DatatypeProperty>
   <owl:DatatypeProperty rdf:about="http://www.opengis.net/gml#frame">
      <rdfs:domain rdf:resource="http://www.opengis.net/gml#AbstractTimeGeometricPrimitiveType"/>
      <rdfs:range rdf:resource="http://www.w3.org/2001/XMLSchema#anyURI"/>
   </owl:DatatypeProperty>
   <owl:DatatypeProperty rdf:about="http://www.opengis.net/gml#unit">
      <rdfs:domain rdf:resource="http://www.opengis.net/gml#TimeIntervalLengthType"/>
      <rdfs:range rdf:resource="http://www.opengis.net/gml#TimeUnitType"/>
   </owl:DatatypeProperty>
   <owl:DatatypeProperty rdf:about="http://www.opengis.net/gml#radix">
      <rdfs:domain rdf:resource="http://www.opengis.net/gml#TimeIntervalLengthType"/>
      <rdfs:range rdf:resource="http://www.w3.org/2001/XMLSchema#positiveInteger"/>
   </owl:DatatypeProperty>
   <owl:DatatypeProperty rdf:about="http://www.opengis.net/gml#factor">
      <rdfs:domain rdf:resource="http://www.opengis.net/gml#TimeIntervalLengthType"/>
      <rdfs:range rdf:resource="http://www.w3.org/2001/XMLSchema#integer"/>
   </owl:DatatypeProperty>
   <owl:DatatypeProperty rdf:about="http://www.opengis.net/gml#frame">
      <rdfs:domain rdf:resource="http://www.opengis.net/gml#TimePositionType"/>
      <rdfs:range rdf:resource="http://www.w3.org/2001/XMLSchema#anyURI"/>
   </owl:DatatypeProperty>
   <owl:DatatypeProperty rdf:about="http://www.opengis.net/gml#calendarEraName">
      <rdfs:domain rdf:resource="http://www.opengis.net/gml#TimePositionType"/>
      <rdfs:range rdf:resource="http://www.w3.org/2001/XMLSchema#string"/>
   </owl:DatatypeProperty>
   <owl:DatatypeProperty rdf:about="http://www.opengis.net/gml#indeterminatePosition">
      <rdfs:domain rdf:resource="http://www.opengis.net/gml#TimePositionType"/>
      <rdfs:range rdf:resource="http://www.opengis.net/gml#TimeIndeterminateValueType"/>
   </owl:DatatypeProperty>
   <owl:Class rdf:about="http://www.opengis.net/gml#_TimeObject">
      <rdfs:subClassOf rdf:resource="http://www.opengis.net/gml#_GML"/>
      <rdfs:subClassOf rdf:resource="http://www.opengis.net/gml#AbstractTimeObjectType"/>
      <rdfs:comment>Warning: This class type was declared outside of its original schema. This class may be declared incorrectly.</rdfs:comment>
   </owl:Class>
   <owl:Class rdf:about="http://www.opengis.net/gml#_TimePrimitive">
      <rdfs:subClassOf rdf:resource="http://www.opengis.net/gml#_TimeObject"/>
      <rdfs:subClassOf rdf:resource="http://www.opengis.net/gml#AbstractTimePrimitiveType"/>
      <rdfs:comment>Warning: This class type was declared outside of its original schema. This class may be declared incorrectly.</rdfs:comment>
   </owl:Class>
   <owl:Class rdf:about="http://www.opengis.net/gml#_TimeComplex">
      <rdfs:subClassOf rdf:resource="http://www.opengis.net/gml#_TimeObject"/>
      <rdfs:subClassOf rdf:resource="http://www.opengis.net/gml#AbstractTimeComplexType"/>
      <rdfs:comment>Warning: This class type was declared outside of its original schema. This class may be declared incorrectly.</rdfs:comment>
   </owl:Class>
   <owl:Class rdf:about="http://www.opengis.net/gml#_TimeGeometricPrimitive">
      <rdfs:subClassOf rdf:resource="http://www.opengis.net/gml#_TimePrimitive"/>
      <rdfs:subClassOf rdf:resource="http://www.opengis.net/gml#AbstractTimeGeometricPrimitiveType"/>
      <rdfs:comment>Warning: This class type was declared outside of its original schema. This class may be declared incorrectly.</rdfs:comment>
   </owl:Class>
   <owl:Class rdf:about="http://www.opengis.net/gml#TimeInstant">
      <rdfs:subClassOf rdf:resource="http://www.opengis.net/gml#_TimeGeometricPrimitive"/>
      <rdfs:subClassOf rdf:resource="http://www.opengis.net/gml#TimeInstantType"/>
      <rdfs:comment>Warning: This class type was declared outside of its original schema. This class may be declared incorrectly.</rdfs:comment>
   </owl:Class>
   <owl:Class rdf:about="http://www.opengis.net/gml#TimePeriod">
      <rdfs:subClassOf rdf:resource="http://www.opengis.net/gml#_TimeGeometricPrimitive"/>
      <rdfs:subClassOf rdf:resource="http://www.opengis.net/gml#TimePeriodType"/>
      <rdfs:comment>Warning: This class type was declared outside of its original schema. This class may be declared incorrectly.</rdfs:comment>
   </owl:Class>
   <rdfs:Datatype rdf:about="concat( $namespace, '#', @name )">
      <owl:equivalentClass rdf:resource="http://www.w3.org/2001/XMLSchema#duration"/>
   </rdfs:Datatype>
   <owl:Class rdf:about="http://www.opengis.net/gml#timeInterval">
      <rdfs:subClassOf rdf:resource="http://www.opengis.net/gml#TimeIntervalLengthType"/>
      <rdfs:comment>Warning: This class type was declared outside of its original schema. This class may be declared incorrectly.</rdfs:comment>
   </owl:Class>
   <owl:Class rdf:about="http://www.opengis.net/gml#timePosition">
      <rdfs:subClassOf rdf:resource="http://www.opengis.net/gml#TimePositionType"/>
      <rdfs:comment>Warning: This class type was declared outside of its original schema. This class may be declared incorrectly.</rdfs:comment>
   </owl:Class>
   <owl:Class rdf:about="http://www.opengis.net/gml#validTime">
      <rdfs:subClassOf rdf:resource="http://www.opengis.net/gml#TimePrimitivePropertyType"/>
      <rdfs:comment>Warning: This class type was declared outside of its original schema. This class may be declared incorrectly.</rdfs:comment>
   </owl:Class>
   <owl:ObjectProperty rdf:about="http://www.opengis.net/gml#relatedTime">
      <rdfs:comment>Warning: This ObjectProperty type was declared outside of its original schema. This ObjectProperty may be declared incorrectly.</rdfs:comment>
      <rdfs:domain rdf:resource="http://www.opengis.net/gml#AbstractTimePrimitiveType"/>
      <rdfs:range rdf:resource="http://www.opengis.net/gml#RelatedTimeType"/>
   </owl:ObjectProperty>
   <owl:ObjectProperty rdf:about="http://www.opengis.net/gml#has_TimePrimitive">
      <rdfs:comment>Warning: This ObjectProperty reference was declared outside of its original schema. This ObjectProperty may be declared incorrectly.</rdfs:comment>
      <rdfs:domain rdf:resource="http://www.opengis.net/gml#TimePrimitivePropertyType"/>
      <rdfs:range rdf:resource="http://www.opengis.net/gml#_TimePrimitive"/>
   </owl:ObjectProperty>
   <owl:ObjectProperty rdf:about="http://www.opengis.net/gml#has_TimeGeometricPrimitive">
      <rdfs:comment>Warning: This ObjectProperty reference was declared outside of its original schema. This ObjectProperty may be declared incorrectly.</rdfs:comment>
      <rdfs:domain rdf:resource="http://www.opengis.net/gml#TimeGeometricPrimitivePropertyType"/>
      <rdfs:range rdf:resource="http://www.opengis.net/gml#_TimeGeometricPrimitive"/>
   </owl:ObjectProperty>
   <owl:ObjectProperty rdf:about="http://www.opengis.net/gml#hastimePosition">
      <rdfs:comment>Warning: This ObjectProperty reference was declared outside of its original schema. This ObjectProperty may be declared incorrectly.</rdfs:comment>
      <rdfs:domain rdf:resource="http://www.opengis.net/gml#TimeInstantType"/>
      <rdfs:range rdf:resource="http://www.opengis.net/gml#timePosition"/>
   </owl:ObjectProperty>
   <owl:ObjectProperty rdf:about="http://www.opengis.net/gml#hasTimeInstant">
      <rdfs:comment>Warning: This ObjectProperty reference was declared outside of its original schema. This ObjectProperty may be declared incorrectly.</rdfs:comment>
      <rdfs:domain rdf:resource="http://www.opengis.net/gml#TimeInstantPropertyType"/>
      <rdfs:range rdf:resource="http://www.opengis.net/gml#TimeInstant"/>
   </owl:ObjectProperty>
   <owl:ObjectProperty rdf:about="http://www.opengis.net/gml#beginPosition">
      <rdfs:comment>Warning: This ObjectProperty type was declared outside of its original schema. This ObjectProperty may be declared incorrectly.</rdfs:comment>
      <rdfs:domain rdf:resource="http://www.opengis.net/gml#TimePeriodType"/>
      <rdfs:range rdf:resource="http://www.opengis.net/gml#TimePositionType"/>
   </owl:ObjectProperty>
   <owl:ObjectProperty rdf:about="http://www.opengis.net/gml#begin">
      <rdfs:comment>Warning: This ObjectProperty type was declared outside of its original schema. This ObjectProperty may be declared incorrectly.</rdfs:comment>
      <rdfs:domain rdf:resource="http://www.opengis.net/gml#TimePeriodType"/>
      <rdfs:range rdf:resource="http://www.opengis.net/gml#TimeInstantPropertyType"/>
   </owl:ObjectProperty>
   <owl:ObjectProperty rdf:about="http://www.opengis.net/gml#endPosition">
      <rdfs:comment>Warning: This ObjectProperty type was declared outside of its original schema. This ObjectProperty may be declared incorrectly.</rdfs:comment>
      <rdfs:domain rdf:resource="http://www.opengis.net/gml#TimePeriodType"/>
      <rdfs:range rdf:resource="http://www.opengis.net/gml#TimePositionType"/>
   </owl:ObjectProperty>
   <owl:ObjectProperty rdf:about="http://www.opengis.net/gml#end">
      <rdfs:comment>Warning: This ObjectProperty type was declared outside of its original schema. This ObjectProperty may be declared incorrectly.</rdfs:comment>
      <rdfs:domain rdf:resource="http://www.opengis.net/gml#TimePeriodType"/>
      <rdfs:range rdf:resource="http://www.opengis.net/gml#TimeInstantPropertyType"/>
   </owl:ObjectProperty>
   <owl:ObjectProperty rdf:about="http://www.opengis.net/gml#hasTimePeriod">
      <rdfs:comment>Warning: This ObjectProperty reference was declared outside of its original schema. This ObjectProperty may be declared incorrectly.</rdfs:comment>
      <rdfs:domain rdf:resource="http://www.opengis.net/gml#TimePeriodPropertyType"/>
      <rdfs:range rdf:resource="http://www.opengis.net/gml#TimePeriod"/>
   </owl:ObjectProperty>
   <owl:ObjectProperty rdf:about="http://www.opengis.net/gml#hasduration">
      <rdfs:comment>Warning: This ObjectProperty reference was declared outside of its original schema. This ObjectProperty may be declared incorrectly.</rdfs:comment>
      <rdfs:domain rdf:resource="http://www.opengis.net/gml#timeLength"/>
      <rdfs:range rdf:resource="http://www.opengis.net/gml#duration"/>
   </owl:ObjectProperty>
   <owl:ObjectProperty rdf:about="http://www.opengis.net/gml#hastimeInterval">
      <rdfs:comment>Warning: This ObjectProperty reference was declared outside of its original schema. This ObjectProperty may be declared incorrectly.</rdfs:comment>
      <rdfs:domain rdf:resource="http://www.opengis.net/gml#timeLength"/>
      <rdfs:range rdf:resource="http://www.opengis.net/gml#timeInterval"/>
   </owl:ObjectProperty>
</rdf:RDF>
