<rdf:RDF xmlns:math="http://www.w3.org/2005/xpath-functions/math" xmlns:owl="http://www.w3.org/2002/07/owl#" xmlns:rdf="http://www.w3.org/1999/02/22-rdf-syntax-ns#" xmlns:rdfs="http://www.w3.org/2000/01/rdf-schema#" xmlns:xs="http://www.w3.org/2001/XMLSchema" xmlns:xsd="http://www.w3.org/2001/XMLSchema">
   <owl:Ontology rdf:about="http://liris.cnrs.fr/ontologies/temporalTopology">
      <owl:imports rdf:resource="http://liris.cnrs.fr/ontologies/gml"/>
      <owl:imports rdf:resource="http://liris.cnrs.fr/ontologies/temporal"/>
      <rdfs:seeAlso>urn:opengis:specification:gml:schema-xsd:temporalTopology:3.1.1</rdfs:seeAlso>
      <rdfs:comment xml:lang="en">The temporal topology schema for ISO19136 provides constructs for handling topological complexes and 
		temporal feature relationships. 
		Temporal geometric characteristics of features are represented as instants and periods. 
		While, temporal context of features that does not relate to the position of time is described as connectivity relationships 
		among instants and periods. These relationships are called temporal topology as they do not change in time, 
		as long as the direction of time does not change. 
		It is used effectively in the case of describing a family tree expressing evolution of species, an ecological cycle, 
		a lineage of lands or buildings, or a history of separation and merger of administrative boundaries.
		This schema reflects a partial yet consistent implementation of the model described in ISO 19108:2002.
		
		GML is an OGC Standard.
		Copyright (c) 2001,2005,2010 Open Geospatial Consortium.
		To obtain additional rights of use, visit http://www.opengeospatial.org/legal/ .
		</rdfs:comment>
   </owl:Ontology>
   <owl:Class rdf:about="#TimeTopologyComplexType">
      <rdfs:comment xml:lang="en">A temporal topology complex.</rdfs:comment>
      <rdfs:subClassOf>
         <owl:Class>
            <owl:intersectionOf rdf:parseType="Collection">
               <owl:Restriction>
                  <owl:onProperty rdf:resource="#primitive"/>
                  <owl:allValuesFrom rdf:resource="http://www.opengis.net/gml#TimeTopologyPrimitivePropertyType"/>
               </owl:Restriction>
            </owl:intersectionOf>
         </owl:Class>
      </rdfs:subClassOf>
      <rdfs:subClassOf rdf:resource="http://www.opengis.net/gml#AbstractTimeComplexType"/>
      <rdfs:comment>Warning: The parent class 'gml:AbstractTimeComplexType' is declared outside of this class' original schema. This class may be declared incorrectly.</rdfs:comment>
   </owl:Class>
   <owl:Class rdf:about="#TimeTopologyComplexPropertyType">
      <rdfs:comment>A time topology complex property can either be any time topology complex element
			 encapsulated in an element of this type or an XLink reference to a remote time topology complex element 
			 (where remote includes elements located elsewhere in the same document). 
			 Note that either the reference or the contained element must be given, but not both or none.</rdfs:comment>
      <rdfs:subClassOf>
         <owl:Class>
            <owl:intersectionOf rdf:parseType="Collection">
               <owl:Restriction>
                  <owl:onProperty rdf:resource="http://www.opengis.net/gml#hasTimeTopologyComplex"/>
                  <owl:allValuesFrom rdf:resource="http://www.opengis.net/gml#TimeTopologyComplex"/>
               </owl:Restriction>
            </owl:intersectionOf>
         </owl:Class>
      </rdfs:subClassOf>
   </owl:Class>
   <owl:Class rdf:about="#AbstractTimeTopologyPrimitiveType">
      <rdfs:comment>This is an abstract class</rdfs:comment>
      <rdfs:comment xml:lang="en">The element "complex" carries a reference to the complex containing this primitive.</rdfs:comment>
      <rdfs:subClassOf>
         <owl:Class>
            <owl:intersectionOf rdf:parseType="Collection">
               <owl:Restriction>
                  <owl:onProperty rdf:resource="#complex"/>
                  <owl:allValuesFrom rdf:resource="http://www.opengis.net/gml#ReferenceType"/>
               </owl:Restriction>
               <owl:Restriction>
                  <owl:onProperty rdf:resource="#complex"/>
                  <owl:minCardinality rdf:datatype="http://www.w3.org/2001/XMLSchema#nonNegativeInteger">0</owl:minCardinality>
               </owl:Restriction>
            </owl:intersectionOf>
         </owl:Class>
      </rdfs:subClassOf>
      <rdfs:subClassOf rdf:resource="http://www.opengis.net/gml#AbstractTimePrimitiveType"/>
      <rdfs:comment>Warning: The parent class 'gml:AbstractTimePrimitiveType' is declared outside of this class' original schema. This class may be declared incorrectly.</rdfs:comment>
   </owl:Class>
   <owl:Class rdf:about="#TimeTopologyPrimitivePropertyType">
      <rdfs:comment>A time topology primitive property can either hold any time topology complex element
			 eor carry an XLink reference to a remote time topology complex element 
			 (where remote includes elements located elsewhere in the same document). 
			 Note that either the reference or the contained element must be given, but not both or none.</rdfs:comment>
      <rdfs:subClassOf>
         <owl:Class>
            <owl:intersectionOf rdf:parseType="Collection">
               <owl:Restriction>
                  <owl:onProperty rdf:resource="http://www.opengis.net/gml#has_TimeTopologyPrimitive"/>
                  <owl:allValuesFrom rdf:resource="http://www.opengis.net/gml#_TimeTopologyPrimitive"/>
               </owl:Restriction>
            </owl:intersectionOf>
         </owl:Class>
      </rdfs:subClassOf>
   </owl:Class>
   <owl:Class rdf:about="#TimeNodeType">
      <rdfs:comment xml:lang="en">Type declaration of the element "TimeNode".</rdfs:comment>
      <rdfs:subClassOf>
         <owl:Class>
            <owl:intersectionOf rdf:parseType="Collection">
               <owl:Restriction>
                  <owl:onProperty rdf:resource="#previousEdge"/>
                  <owl:allValuesFrom rdf:resource="http://www.opengis.net/gml#TimeEdgePropertyType"/>
               </owl:Restriction>
               <owl:Restriction>
                  <owl:onProperty rdf:resource="#previousEdge"/>
                  <owl:minCardinality rdf:datatype="http://www.w3.org/2001/XMLSchema#nonNegativeInteger">0</owl:minCardinality>
               </owl:Restriction>
               <owl:Restriction>
                  <owl:onProperty rdf:resource="#nextEdge"/>
                  <owl:allValuesFrom rdf:resource="http://www.opengis.net/gml#TimeEdgePropertyType"/>
               </owl:Restriction>
               <owl:Restriction>
                  <owl:onProperty rdf:resource="#nextEdge"/>
                  <owl:minCardinality rdf:datatype="http://www.w3.org/2001/XMLSchema#nonNegativeInteger">0</owl:minCardinality>
               </owl:Restriction>
               <owl:Restriction>
                  <owl:onProperty rdf:resource="#position"/>
                  <owl:allValuesFrom rdf:resource="http://www.opengis.net/gml#TimeInstantPropertyType"/>
               </owl:Restriction>
               <owl:Restriction>
                  <owl:onProperty rdf:resource="#position"/>
                  <owl:minCardinality rdf:datatype="http://www.w3.org/2001/XMLSchema#nonNegativeInteger">0</owl:minCardinality>
               </owl:Restriction>
            </owl:intersectionOf>
         </owl:Class>
      </rdfs:subClassOf>
      <rdfs:subClassOf rdf:resource="http://www.opengis.net/gml#AbstractTimeTopologyPrimitiveType"/>
      <rdfs:comment>Warning: The parent class 'gml:AbstractTimeTopologyPrimitiveType' is declared outside of this class' original schema. This class may be declared incorrectly.</rdfs:comment>
   </owl:Class>
   <owl:Class rdf:about="#TimeNodePropertyType">
      <rdfs:comment>A time node property can either be any time node element encapsulated in an element of this type 
			or an XLink reference to a remote time node element (where remote includes elements located elsewhere in the same document). 
			Note that either the reference or the contained element must be given, but not both or none.</rdfs:comment>
      <rdfs:subClassOf>
         <owl:Class>
            <owl:intersectionOf rdf:parseType="Collection">
               <owl:Restriction>
                  <owl:onProperty rdf:resource="http://www.opengis.net/gml#hasTimeNode"/>
                  <owl:allValuesFrom rdf:resource="http://www.opengis.net/gml#TimeNode"/>
               </owl:Restriction>
            </owl:intersectionOf>
         </owl:Class>
      </rdfs:subClassOf>
   </owl:Class>
   <owl:Class rdf:about="#TimeEdgeType">
      <rdfs:comment xml:lang="en">Type declaration of the element "TimeEdge".</rdfs:comment>
      <rdfs:subClassOf>
         <owl:Class>
            <owl:intersectionOf rdf:parseType="Collection">
               <owl:Restriction>
                  <owl:onProperty rdf:resource="#start"/>
                  <owl:allValuesFrom rdf:resource="http://www.opengis.net/gml#TimeNodePropertyType"/>
               </owl:Restriction>
               <owl:Restriction>
                  <owl:onProperty rdf:resource="#end"/>
                  <owl:allValuesFrom rdf:resource="http://www.opengis.net/gml#TimeNodePropertyType"/>
               </owl:Restriction>
               <owl:Restriction>
                  <owl:onProperty rdf:resource="#extent"/>
                  <owl:allValuesFrom rdf:resource="http://www.opengis.net/gml#TimePeriodPropertyType"/>
               </owl:Restriction>
               <owl:Restriction>
                  <owl:onProperty rdf:resource="#extent"/>
                  <owl:minCardinality rdf:datatype="http://www.w3.org/2001/XMLSchema#nonNegativeInteger">0</owl:minCardinality>
               </owl:Restriction>
            </owl:intersectionOf>
         </owl:Class>
      </rdfs:subClassOf>
      <rdfs:subClassOf rdf:resource="http://www.opengis.net/gml#AbstractTimeTopologyPrimitiveType"/>
      <rdfs:comment>Warning: The parent class 'gml:AbstractTimeTopologyPrimitiveType' is declared outside of this class' original schema. This class may be declared incorrectly.</rdfs:comment>
   </owl:Class>
   <owl:Class rdf:about="#TimeEdgePropertyType">
      <rdfs:comment>A time edge property can either be any time edge element encapsulated in an element of this type 
			or an XLink reference to a remote time edge element (where remote includes elements located elsewhere in the same document). 
			Note that either the reference or the contained element must be given, but not both or none.</rdfs:comment>
      <rdfs:subClassOf>
         <owl:Class>
            <owl:intersectionOf rdf:parseType="Collection">
               <owl:Restriction>
                  <owl:onProperty rdf:resource="http://www.opengis.net/gml#hasTimeEdge"/>
                  <owl:allValuesFrom rdf:resource="http://www.opengis.net/gml#TimeEdge"/>
               </owl:Restriction>
            </owl:intersectionOf>
         </owl:Class>
      </rdfs:subClassOf>
   </owl:Class>
   <owl:ObjectProperty rdf:about="http://www.opengis.net/gml#hasAssociationAttributeGroup">
      <rdfs:domain rdf:resource="#TimeTopologyComplexPropertyType"/>
      <rdfs:range rdf:resource="http://www.opengis.net/gml#AssociationAttributeGroup"/>
   </owl:ObjectProperty>
   <owl:ObjectProperty rdf:about="http://www.opengis.net/gml#hasAssociationAttributeGroup">
      <rdfs:domain rdf:resource="#TimeTopologyPrimitivePropertyType"/>
      <rdfs:range rdf:resource="http://www.opengis.net/gml#AssociationAttributeGroup"/>
   </owl:ObjectProperty>
   <owl:ObjectProperty rdf:about="http://www.opengis.net/gml#hasAssociationAttributeGroup">
      <rdfs:domain rdf:resource="#TimeNodePropertyType"/>
      <rdfs:range rdf:resource="http://www.opengis.net/gml#AssociationAttributeGroup"/>
   </owl:ObjectProperty>
   <owl:ObjectProperty rdf:about="http://www.opengis.net/gml#hasAssociationAttributeGroup">
      <rdfs:domain rdf:resource="#TimeEdgePropertyType"/>
      <rdfs:range rdf:resource="http://www.opengis.net/gml#AssociationAttributeGroup"/>
   </owl:ObjectProperty>
   <rdfs:Datatype rdf:about="#SuccessionType">
      <rdfs:comment>Feature succession is a semantic relationship derived from evaluation of observer, and 
			Feature Substitution, Feature Division and Feature Fusion are defined as associations between 
			previous features and next features in the temporal context. 
			Successions shall be represented in either following two ways. 
			* define a temporal topological complex element as a feature element 
			* define an association same as temporal topological complex between features.</rdfs:comment>
      <owl:equivalentClass>
         <rdfs:Datatype>
            <owl:oneOf>
               <rdf:Description rdf:type="http://www.w3.org/1999/02/22-rdf-syntax-ns#List">
                  <rdf:first rdf:datatype="string">substitution</rdf:first>
                  <rdf:rest>
                     <rdf:Description rdf:type="http://www.w3.org/1999/02/22-rdf-syntax-ns#List">
                        <rdf:first rdf:datatype="string">division</rdf:first>
                        <rdf:rest>
                           <rdf:Description rdf:type="http://www.w3.org/1999/02/22-rdf-syntax-ns#List">
                              <rdf:first rdf:datatype="string">fusion</rdf:first>
                              <rdf:rest>
                                 <rdf:Description rdf:type="http://www.w3.org/1999/02/22-rdf-syntax-ns#List">
                                    <rdf:first rdf:datatype="string">initiation</rdf:first>
                                    <rdf:rest rdf:resource="http://www.w3.org/1999/02/22-rdf-syntax-ns#nil"/>
                                 </rdf:Description>
                              </rdf:rest>
                           </rdf:Description>
                        </rdf:rest>
                     </rdf:Description>
                  </rdf:rest>
               </rdf:Description>
            </owl:oneOf>
         </rdfs:Datatype>
      </owl:equivalentClass>
   </rdfs:Datatype>
   <owl:Class rdf:about="#TimeTopologyComplex">
      <rdfs:subClassOf rdf:resource="http://www.opengis.net/gml#_TimeComplex"/>
      <rdfs:subClassOf rdf:resource="http://www.opengis.net/gml#TimeTopologyComplexType"/>
      <rdfs:comment>Warning: This class type was declared outside of its original schema. This class may be declared incorrectly.</rdfs:comment>
   </owl:Class>
   <owl:Class rdf:about="#_TimeTopologyPrimitive">
      <rdfs:subClassOf rdf:resource="http://www.opengis.net/gml#_TimePrimitive"/>
      <rdfs:subClassOf rdf:resource="http://www.opengis.net/gml#AbstractTimeTopologyPrimitiveType"/>
      <rdfs:comment>Warning: This class type was declared outside of its original schema. This class may be declared incorrectly.</rdfs:comment>
   </owl:Class>
   <owl:Class rdf:about="#TimeNode">
      <rdfs:subClassOf rdf:resource="http://www.opengis.net/gml#_TimeTopologyPrimitive"/>
      <rdfs:subClassOf rdf:resource="http://www.opengis.net/gml#TimeNodeType"/>
      <rdfs:comment>Warning: This class type was declared outside of its original schema. This class may be declared incorrectly.</rdfs:comment>
   </owl:Class>
   <owl:Class rdf:about="#TimeEdge">
      <rdfs:subClassOf rdf:resource="http://www.opengis.net/gml#_TimeTopologyPrimitive"/>
      <rdfs:subClassOf rdf:resource="http://www.opengis.net/gml#TimeEdgeType"/>
      <rdfs:comment>Warning: This class type was declared outside of its original schema. This class may be declared incorrectly.</rdfs:comment>
   </owl:Class>
   <owl:ObjectProperty rdf:about="#primitive">
      <rdfs:comment>Warning: This ObjectProperty type was declared outside of its original schema. This ObjectProperty may be declared incorrectly.</rdfs:comment>
      <rdfs:domain rdf:resource="#TimeTopologyComplexType"/>
      <rdfs:range rdf:resource="http://www.opengis.net/gml#TimeTopologyPrimitivePropertyType"/>
   </owl:ObjectProperty>
   <owl:ObjectProperty rdf:about="http://www.opengis.net/gml#hasTimeTopologyComplex">
      <rdfs:comment>Warning: This ObjectProperty reference was declared outside of its original schema. This ObjectProperty may be declared incorrectly.</rdfs:comment>
      <rdfs:domain rdf:resource="#TimeTopologyComplexPropertyType"/>
      <rdfs:range rdf:resource="http://www.opengis.net/gml#TimeTopologyComplex"/>
   </owl:ObjectProperty>
   <owl:ObjectProperty rdf:about="#complex">
      <rdfs:comment>Warning: This ObjectProperty type was declared outside of its original schema. This ObjectProperty may be declared incorrectly.</rdfs:comment>
      <rdfs:domain rdf:resource="#AbstractTimeTopologyPrimitiveType"/>
      <rdfs:range rdf:resource="http://www.opengis.net/gml#ReferenceType"/>
   </owl:ObjectProperty>
   <owl:ObjectProperty rdf:about="http://www.opengis.net/gml#has_TimeTopologyPrimitive">
      <rdfs:comment>Warning: This ObjectProperty reference was declared outside of its original schema. This ObjectProperty may be declared incorrectly.</rdfs:comment>
      <rdfs:domain rdf:resource="#TimeTopologyPrimitivePropertyType"/>
      <rdfs:range rdf:resource="http://www.opengis.net/gml#_TimeTopologyPrimitive"/>
   </owl:ObjectProperty>
   <owl:ObjectProperty rdf:about="#previousEdge">
      <rdfs:comment>Warning: This ObjectProperty type was declared outside of its original schema. This ObjectProperty may be declared incorrectly.</rdfs:comment>
      <rdfs:domain rdf:resource="#TimeNodeType"/>
      <rdfs:range rdf:resource="http://www.opengis.net/gml#TimeEdgePropertyType"/>
   </owl:ObjectProperty>
   <owl:ObjectProperty rdf:about="#nextEdge">
      <rdfs:comment>Warning: This ObjectProperty type was declared outside of its original schema. This ObjectProperty may be declared incorrectly.</rdfs:comment>
      <rdfs:domain rdf:resource="#TimeNodeType"/>
      <rdfs:range rdf:resource="http://www.opengis.net/gml#TimeEdgePropertyType"/>
   </owl:ObjectProperty>
   <owl:ObjectProperty rdf:about="#position">
      <rdfs:comment>Warning: This ObjectProperty type was declared outside of its original schema. This ObjectProperty may be declared incorrectly.</rdfs:comment>
      <rdfs:domain rdf:resource="#TimeNodeType"/>
      <rdfs:range rdf:resource="http://www.opengis.net/gml#TimeInstantPropertyType"/>
   </owl:ObjectProperty>
   <owl:ObjectProperty rdf:about="http://www.opengis.net/gml#hasTimeNode">
      <rdfs:comment>Warning: This ObjectProperty reference was declared outside of its original schema. This ObjectProperty may be declared incorrectly.</rdfs:comment>
      <rdfs:domain rdf:resource="#TimeNodePropertyType"/>
      <rdfs:range rdf:resource="http://www.opengis.net/gml#TimeNode"/>
   </owl:ObjectProperty>
   <owl:ObjectProperty rdf:about="#start">
      <rdfs:comment>Warning: This ObjectProperty type was declared outside of its original schema. This ObjectProperty may be declared incorrectly.</rdfs:comment>
      <rdfs:domain rdf:resource="#TimeEdgeType"/>
      <rdfs:range rdf:resource="http://www.opengis.net/gml#TimeNodePropertyType"/>
   </owl:ObjectProperty>
   <owl:ObjectProperty rdf:about="#end">
      <rdfs:comment>Warning: This ObjectProperty type was declared outside of its original schema. This ObjectProperty may be declared incorrectly.</rdfs:comment>
      <rdfs:domain rdf:resource="#TimeEdgeType"/>
      <rdfs:range rdf:resource="http://www.opengis.net/gml#TimeNodePropertyType"/>
   </owl:ObjectProperty>
   <owl:ObjectProperty rdf:about="#extent">
      <rdfs:comment>Warning: This ObjectProperty type was declared outside of its original schema. This ObjectProperty may be declared incorrectly.</rdfs:comment>
      <rdfs:domain rdf:resource="#TimeEdgeType"/>
      <rdfs:range rdf:resource="http://www.opengis.net/gml#TimePeriodPropertyType"/>
   </owl:ObjectProperty>
   <owl:ObjectProperty rdf:about="http://www.opengis.net/gml#hasTimeEdge">
      <rdfs:comment>Warning: This ObjectProperty reference was declared outside of its original schema. This ObjectProperty may be declared incorrectly.</rdfs:comment>
      <rdfs:domain rdf:resource="#TimeEdgePropertyType"/>
      <rdfs:range rdf:resource="http://www.opengis.net/gml#TimeEdge"/>
   </owl:ObjectProperty>
</rdf:RDF>
