<rdf:RDF xmlns:math="http://www.w3.org/2005/xpath-functions/math" xmlns:owl="http://www.w3.org/2002/07/owl#" xmlns:rdf="http://www.w3.org/1999/02/22-rdf-syntax-ns#" xmlns:rdfs="http://www.w3.org/2000/01/rdf-schema#" xmlns:xs="http://www.w3.org/2001/XMLSchema" xmlns:xsd="http://www.w3.org/2001/XMLSchema">
   <owl:Ontology rdf:about="http://liris.cnrs.fr/ontologies/temporalReferenceSystems">
      <owl:imports rdf:resource="http://liris.cnrs.fr/ontologies/gml"/>
      <owl:imports rdf:resource="http://liris.cnrs.fr/ontologies/temporalTopology"/>
      <owl:imports rdf:resource="http://liris.cnrs.fr/ontologies/dictionary"/>
      <rdfs:seeAlso>urn:opengis:specification:gml:schema-xsd:temporalReferenceSystems:3.1.1</rdfs:seeAlso>
      <rdfs:comment xml:lang="en">The Temporal Reference Systems schema for GML 3.1 provides constructs for handling various styles of temporal reference system. 
    This schema reflects a partial implementation of the model described in ISO 19108:2002.
    
    GML is an OGC Standard.
    Copyright (c) 2001,2005,2010 Open Geospatial Consortium.
    To obtain additional rights of use, visit http://www.opengeospatial.org/legal/ .
		</rdfs:comment>
   </owl:Ontology>
   <owl:Class rdf:about="http://www.opengis.net/gml#AbstractTimeReferenceSystemType">
      <rdfs:comment>This is an abstract class</rdfs:comment>
      <rdfs:comment xml:lang="en">A value in the time domain is measured relative to a temporal reference system. Common 
        types of reference systems include calendars, ordinal temporal reference systems, and 
        temporal coordinate systems (time elapsed since some epoch, e.g. UNIX time).</rdfs:comment>
      <rdfs:subClassOf>
         <owl:Class>
            <owl:intersectionOf rdf:parseType="Collection">
               <owl:Restriction>
                  <owl:onProperty rdf:resource="http://www.opengis.net/gml#domainOfValidity"/>
                  <owl:allValuesFrom rdf:resource="http://www.w3.org/2001/XMLSchema#string"/>
               </owl:Restriction>
               <owl:Restriction>
                  <owl:onProperty rdf:resource="http://www.opengis.net/gml#domainOfValidity"/>
                  <owl:minCardinality rdf:datatype="http://www.w3.org/2001/XMLSchema#nonNegativeInteger">0</owl:minCardinality>
               </owl:Restriction>
            </owl:intersectionOf>
         </owl:Class>
      </rdfs:subClassOf>
      <rdfs:subClassOf rdf:resource="http://www.opengis.net/gml#DefinitionType"/>
      <rdfs:comment>Warning: The parent class 'gml:DefinitionType' is declared outside of this class' original schema. This class may be declared incorrectly.</rdfs:comment>
   </owl:Class>
   <owl:Class rdf:about="http://www.opengis.net/gml#TimeCoordinateSystemType">
      <rdfs:comment xml:lang="en">A temporal coordinate system is based on a continuous interval scale defined in terms of a single time interval.</rdfs:comment>
      <rdfs:subClassOf>
         <owl:Class>
            <owl:intersectionOf rdf:parseType="Collection">
               <owl:Restriction>
                  <owl:onProperty rdf:resource="http://www.opengis.net/gml#interval"/>
                  <owl:allValuesFrom rdf:resource="http://www.opengis.net/gml#TimeIntervalLengthType"/>
               </owl:Restriction>
            </owl:intersectionOf>
         </owl:Class>
      </rdfs:subClassOf>
      <owl:disjointUnionOf rdf:parseType="Collection">
         <owl:Restriction>
            <owl:onProperty rdf:resource="http://www.opengis.net/gml#originPosition"/>
            <owl:someValuesFrom rdf:resource="http://www.opengis.net/gml#TimePositionType"/>
         </owl:Restriction>
         <owl:Restriction>
            <owl:onProperty rdf:resource="http://www.opengis.net/gml#origin"/>
            <owl:someValuesFrom rdf:resource="http://www.opengis.net/gml#TimeInstantPropertyType"/>
         </owl:Restriction>
      </owl:disjointUnionOf>
      <rdfs:subClassOf rdf:resource="http://www.opengis.net/gml#AbstractTimeReferenceSystemType"/>
      <rdfs:comment>Warning: The parent class 'gml:AbstractTimeReferenceSystemType' is declared outside of this class' original schema. This class may be declared incorrectly.</rdfs:comment>
   </owl:Class>
   <owl:Class rdf:about="http://www.opengis.net/gml#TimeOrdinalReferenceSystemType">
      <rdfs:comment xml:lang="en">In an ordinal reference system the order of events in time can be well 
      established, but the magnitude of the intervals between them can not be 
      accurately determined (e.g. a stratigraphic sequence).</rdfs:comment>
      <rdfs:subClassOf>
         <owl:Class>
            <owl:intersectionOf rdf:parseType="Collection">
               <owl:Restriction>
                  <owl:onProperty rdf:resource="http://www.opengis.net/gml#component"/>
                  <owl:allValuesFrom rdf:resource="http://www.opengis.net/gml#TimeOrdinalEraPropertyType"/>
               </owl:Restriction>
            </owl:intersectionOf>
         </owl:Class>
      </rdfs:subClassOf>
      <rdfs:subClassOf rdf:resource="http://www.opengis.net/gml#AbstractTimeReferenceSystemType"/>
      <rdfs:comment>Warning: The parent class 'gml:AbstractTimeReferenceSystemType' is declared outside of this class' original schema. This class may be declared incorrectly.</rdfs:comment>
   </owl:Class>
   <owl:Class rdf:about="http://www.opengis.net/gml#TimeOrdinalEraType">
      <rdfs:comment xml:lang="en">Ordinal temporal reference systems are often hierarchically structured 
      such that an ordinal era at a given level of the hierarchy includes a 
      sequence of shorter, coterminous ordinal eras. This captured using the member/group properties.  
      
      Note that in this schema, TIme Ordinal Era is patterned on TimeEdge, which is a variation from ISO 19108.  
      This is in order to fulfill the requirements of ordinal reference systems based on eras delimited by 
      named points or nodes, which are common in geology, archeology, etc.  
      
      This change is subject of a change proposal to ISO</rdfs:comment>
      <rdfs:subClassOf>
         <owl:Class>
            <owl:intersectionOf rdf:parseType="Collection">
               <owl:Restriction>
                  <owl:onProperty rdf:resource="http://www.opengis.net/gml#relatedTime"/>
                  <owl:allValuesFrom rdf:resource="http://www.opengis.net/gml#RelatedTimeType"/>
               </owl:Restriction>
               <owl:Restriction>
                  <owl:onProperty rdf:resource="http://www.opengis.net/gml#relatedTime"/>
                  <owl:minCardinality rdf:datatype="http://www.w3.org/2001/XMLSchema#nonNegativeInteger">0</owl:minCardinality>
               </owl:Restriction>
               <owl:Restriction>
                  <owl:onProperty rdf:resource="http://www.opengis.net/gml#start"/>
                  <owl:allValuesFrom rdf:resource="http://www.opengis.net/gml#TimeNodePropertyType"/>
               </owl:Restriction>
               <owl:Restriction>
                  <owl:onProperty rdf:resource="http://www.opengis.net/gml#end"/>
                  <owl:allValuesFrom rdf:resource="http://www.opengis.net/gml#TimeNodePropertyType"/>
               </owl:Restriction>
               <owl:Restriction>
                  <owl:onProperty rdf:resource="http://www.opengis.net/gml#extent"/>
                  <owl:allValuesFrom rdf:resource="http://www.opengis.net/gml#TimePeriodPropertyType"/>
               </owl:Restriction>
               <owl:Restriction>
                  <owl:onProperty rdf:resource="http://www.opengis.net/gml#extent"/>
                  <owl:minCardinality rdf:datatype="http://www.w3.org/2001/XMLSchema#nonNegativeInteger">0</owl:minCardinality>
               </owl:Restriction>
               <owl:Restriction>
                  <owl:onProperty rdf:resource="http://www.opengis.net/gml#member"/>
                  <owl:allValuesFrom rdf:resource="http://www.opengis.net/gml#TimeOrdinalEraPropertyType"/>
               </owl:Restriction>
               <owl:Restriction>
                  <owl:onProperty rdf:resource="http://www.opengis.net/gml#member"/>
                  <owl:minCardinality rdf:datatype="http://www.w3.org/2001/XMLSchema#nonNegativeInteger">0</owl:minCardinality>
               </owl:Restriction>
               <owl:Restriction>
                  <owl:onProperty rdf:resource="http://www.opengis.net/gml#group"/>
                  <owl:allValuesFrom rdf:resource="http://www.opengis.net/gml#ReferenceType"/>
               </owl:Restriction>
               <owl:Restriction>
                  <owl:onProperty rdf:resource="http://www.opengis.net/gml#group"/>
                  <owl:minCardinality rdf:datatype="http://www.w3.org/2001/XMLSchema#nonNegativeInteger">0</owl:minCardinality>
               </owl:Restriction>
            </owl:intersectionOf>
         </owl:Class>
      </rdfs:subClassOf>
      <rdfs:subClassOf rdf:resource="http://www.opengis.net/gml#DefinitionType"/>
      <rdfs:comment>Warning: The parent class 'gml:DefinitionType' is declared outside of this class' original schema. This class may be declared incorrectly.</rdfs:comment>
   </owl:Class>
   <owl:Class rdf:about="http://www.opengis.net/gml#TimeOrdinalEraPropertyType">
      <rdfs:subClassOf>
         <owl:Class>
            <owl:intersectionOf rdf:parseType="Collection">
               <owl:Restriction>
                  <owl:onProperty rdf:resource="http://www.opengis.net/gml#hasTimeOrdinalEra"/>
                  <owl:allValuesFrom rdf:resource="http://www.opengis.net/gml#TimeOrdinalEra"/>
               </owl:Restriction>
            </owl:intersectionOf>
         </owl:Class>
      </rdfs:subClassOf>
   </owl:Class>
   <owl:Class rdf:about="http://www.opengis.net/gml#TimeCalendarType">
      <rdfs:comment xml:lang="en">A calendar is a discrete temporal reference system 
      that provides a basis for defining temporal position to a resolution of one day. 
      A single calendar may reference more than one calendar era.</rdfs:comment>
      <rdfs:subClassOf>
         <owl:Class>
            <owl:intersectionOf rdf:parseType="Collection">
               <owl:Restriction>
                  <owl:onProperty rdf:resource="http://www.opengis.net/gml#referenceFrame"/>
                  <owl:allValuesFrom rdf:resource="http://www.opengis.net/gml#TimeCalendarEraPropertyType"/>
               </owl:Restriction>
            </owl:intersectionOf>
         </owl:Class>
      </rdfs:subClassOf>
      <rdfs:subClassOf rdf:resource="http://www.opengis.net/gml#AbstractTimeReferenceSystemType"/>
      <rdfs:comment>Warning: The parent class 'gml:AbstractTimeReferenceSystemType' is declared outside of this class' original schema. This class may be declared incorrectly.</rdfs:comment>
   </owl:Class>
   <owl:Class rdf:about="http://www.opengis.net/gml#TimeCalendarPropertyType">
      <rdfs:subClassOf>
         <owl:Class>
            <owl:intersectionOf rdf:parseType="Collection">
               <owl:Restriction>
                  <owl:onProperty rdf:resource="http://www.opengis.net/gml#hasTimeCalendar"/>
                  <owl:allValuesFrom rdf:resource="http://www.opengis.net/gml#TimeCalendar"/>
               </owl:Restriction>
            </owl:intersectionOf>
         </owl:Class>
      </rdfs:subClassOf>
   </owl:Class>
   <owl:Class rdf:about="http://www.opengis.net/gml#TimeCalendarEraType">
      <rdfs:comment xml:lang="en">In every calendar, years are numbered relative to the date of a 
      reference event that defines a calendar era. 
      In this implementation, we omit the back-pointer "datingSystem".</rdfs:comment>
      <rdfs:subClassOf>
         <owl:Class>
            <owl:intersectionOf rdf:parseType="Collection">
               <owl:Restriction>
                  <owl:onProperty rdf:resource="http://www.opengis.net/gml#referenceEvent"/>
                  <owl:allValuesFrom rdf:resource="http://www.opengis.net/gml#StringOrRefType"/>
               </owl:Restriction>
               <owl:Restriction>
                  <owl:onProperty rdf:resource="http://www.opengis.net/gml#referenceDate"/>
                  <owl:allValuesFrom rdf:resource="http://www.w3.org/2001/XMLSchema#date"/>
               </owl:Restriction>
               <owl:Restriction>
                  <owl:onProperty rdf:resource="http://www.opengis.net/gml#referenceDate"/>
                  <owl:minCardinality rdf:datatype="http://www.w3.org/2001/XMLSchema#nonNegativeInteger">0</owl:minCardinality>
               </owl:Restriction>
               <owl:Restriction>
                  <owl:onProperty rdf:resource="http://www.opengis.net/gml#julianReference"/>
                  <owl:allValuesFrom rdf:resource="http://www.w3.org/2001/XMLSchema#decimal"/>
               </owl:Restriction>
               <owl:Restriction>
                  <owl:onProperty rdf:resource="http://www.opengis.net/gml#epochOfUse"/>
                  <owl:allValuesFrom rdf:resource="http://www.opengis.net/gml#TimePeriodPropertyType"/>
               </owl:Restriction>
            </owl:intersectionOf>
         </owl:Class>
      </rdfs:subClassOf>
      <rdfs:subClassOf rdf:resource="http://www.opengis.net/gml#DefinitionType"/>
      <rdfs:comment>Warning: The parent class 'gml:DefinitionType' is declared outside of this class' original schema. This class may be declared incorrectly.</rdfs:comment>
   </owl:Class>
   <owl:Class rdf:about="http://www.opengis.net/gml#TimeCalendarEraPropertyType">
      <rdfs:subClassOf>
         <owl:Class>
            <owl:intersectionOf rdf:parseType="Collection">
               <owl:Restriction>
                  <owl:onProperty rdf:resource="http://www.opengis.net/gml#hasTimeCalendarEra"/>
                  <owl:allValuesFrom rdf:resource="http://www.opengis.net/gml#TimeCalendarEra"/>
               </owl:Restriction>
            </owl:intersectionOf>
         </owl:Class>
      </rdfs:subClassOf>
   </owl:Class>
   <owl:Class rdf:about="http://www.opengis.net/gml#TimeClockType">
      <rdfs:comment xml:lang="en">A clock provides a basis for defining temporal position within a day. 
      A clock must be used with a calendar in order to provide a complete description of a temporal position 
      within a specific day.</rdfs:comment>
      <rdfs:subClassOf>
         <owl:Class>
            <owl:intersectionOf rdf:parseType="Collection">
               <owl:Restriction>
                  <owl:onProperty rdf:resource="http://www.opengis.net/gml#referenceEvent"/>
                  <owl:allValuesFrom rdf:resource="http://www.opengis.net/gml#StringOrRefType"/>
               </owl:Restriction>
               <owl:Restriction>
                  <owl:onProperty rdf:resource="http://www.opengis.net/gml#referenceTime"/>
                  <owl:allValuesFrom rdf:resource="http://www.w3.org/2001/XMLSchema#time"/>
               </owl:Restriction>
               <owl:Restriction>
                  <owl:onProperty rdf:resource="http://www.opengis.net/gml#utcReference"/>
                  <owl:allValuesFrom rdf:resource="http://www.w3.org/2001/XMLSchema#time"/>
               </owl:Restriction>
               <owl:Restriction>
                  <owl:onProperty rdf:resource="http://www.opengis.net/gml#dateBasis"/>
                  <owl:allValuesFrom rdf:resource="http://www.opengis.net/gml#TimeCalendarPropertyType"/>
               </owl:Restriction>
               <owl:Restriction>
                  <owl:onProperty rdf:resource="http://www.opengis.net/gml#dateBasis"/>
                  <owl:minCardinality rdf:datatype="http://www.w3.org/2001/XMLSchema#nonNegativeInteger">0</owl:minCardinality>
               </owl:Restriction>
            </owl:intersectionOf>
         </owl:Class>
      </rdfs:subClassOf>
      <rdfs:subClassOf rdf:resource="http://www.opengis.net/gml#AbstractTimeReferenceSystemType"/>
      <rdfs:comment>Warning: The parent class 'gml:AbstractTimeReferenceSystemType' is declared outside of this class' original schema. This class may be declared incorrectly.</rdfs:comment>
   </owl:Class>
   <owl:Class rdf:about="http://www.opengis.net/gml#TimeClockPropertyType">
      <rdfs:subClassOf>
         <owl:Class>
            <owl:intersectionOf rdf:parseType="Collection">
               <owl:Restriction>
                  <owl:onProperty rdf:resource="http://www.opengis.net/gml#hasTimeClock"/>
                  <owl:allValuesFrom rdf:resource="http://www.opengis.net/gml#TimeClock"/>
               </owl:Restriction>
            </owl:intersectionOf>
         </owl:Class>
      </rdfs:subClassOf>
   </owl:Class>
   <owl:Class rdf:about="http://www.opengis.net/gml#_TimeReferenceSystem">
      <rdfs:subClassOf rdf:resource="http://www.opengis.net/gml#Definition"/>
      <rdfs:subClassOf rdf:resource="http://www.opengis.net/gml#AbstractTimeReferenceSystemType"/>
      <rdfs:comment>Warning: This class type was declared outside of its original schema. This class may be declared incorrectly.</rdfs:comment>
   </owl:Class>
   <owl:Class rdf:about="http://www.opengis.net/gml#TimeCoordinateSystem">
      <rdfs:subClassOf rdf:resource="http://www.opengis.net/gml#_TimeReferenceSystem"/>
      <rdfs:subClassOf rdf:resource="http://www.opengis.net/gml#TimeCoordinateSystemType"/>
      <rdfs:comment>Warning: This class type was declared outside of its original schema. This class may be declared incorrectly.</rdfs:comment>
   </owl:Class>
   <owl:Class rdf:about="http://www.opengis.net/gml#TimeOrdinalReferenceSystem">
      <rdfs:subClassOf rdf:resource="http://www.opengis.net/gml#_TimeReferenceSystem"/>
      <rdfs:subClassOf rdf:resource="http://www.opengis.net/gml#TimeOrdinalReferenceSystemType"/>
      <rdfs:comment>Warning: This class type was declared outside of its original schema. This class may be declared incorrectly.</rdfs:comment>
   </owl:Class>
   <owl:Class rdf:about="http://www.opengis.net/gml#TimeOrdinalEra">
      <rdfs:subClassOf rdf:resource="http://www.opengis.net/gml#TimeOrdinalEraType"/>
      <rdfs:comment>Warning: This class type was declared outside of its original schema. This class may be declared incorrectly.</rdfs:comment>
   </owl:Class>
   <owl:Class rdf:about="http://www.opengis.net/gml#TimeCalendar">
      <rdfs:subClassOf rdf:resource="http://www.opengis.net/gml#_TimeReferenceSystem"/>
      <rdfs:subClassOf rdf:resource="http://www.opengis.net/gml#TimeCalendarType"/>
      <rdfs:comment>Warning: This class type was declared outside of its original schema. This class may be declared incorrectly.</rdfs:comment>
   </owl:Class>
   <owl:Class rdf:about="http://www.opengis.net/gml#TimeCalendarEra">
      <rdfs:subClassOf rdf:resource="http://www.opengis.net/gml#Definition"/>
      <rdfs:subClassOf rdf:resource="http://www.opengis.net/gml#TimeCalendarEraType"/>
      <rdfs:comment>Warning: This class type was declared outside of its original schema. This class may be declared incorrectly.</rdfs:comment>
   </owl:Class>
   <owl:Class rdf:about="http://www.opengis.net/gml#TimeClock">
      <rdfs:subClassOf rdf:resource="http://www.opengis.net/gml#_TimeReferenceSystem"/>
      <rdfs:subClassOf rdf:resource="http://www.opengis.net/gml#TimeClockType"/>
      <rdfs:comment>Warning: This class type was declared outside of its original schema. This class may be declared incorrectly.</rdfs:comment>
   </owl:Class>
   <owl:DatatypeProperty rdf:about="http://www.opengis.net/gml#domainOfValidity">
      <rdfs:domain rdf:resource="http://www.opengis.net/gml#AbstractTimeReferenceSystemType"/>
      <rdfs:range rdf:resource="http://www.w3.org/2001/XMLSchema#string"/>
   </owl:DatatypeProperty>
   <owl:ObjectProperty rdf:about="http://www.opengis.net/gml#originPosition">
      <rdfs:comment>Warning: This ObjectProperty type was declared outside of its original schema. This ObjectProperty may be declared incorrectly.</rdfs:comment>
      <rdfs:domain rdf:resource="http://www.opengis.net/gml#TimeCoordinateSystemType"/>
      <rdfs:range rdf:resource="http://www.opengis.net/gml#TimePositionType"/>
   </owl:ObjectProperty>
   <owl:ObjectProperty rdf:about="http://www.opengis.net/gml#origin">
      <rdfs:comment>Warning: This ObjectProperty type was declared outside of its original schema. This ObjectProperty may be declared incorrectly.</rdfs:comment>
      <rdfs:domain rdf:resource="http://www.opengis.net/gml#TimeCoordinateSystemType"/>
      <rdfs:range rdf:resource="http://www.opengis.net/gml#TimeInstantPropertyType"/>
   </owl:ObjectProperty>
   <owl:ObjectProperty rdf:about="http://www.opengis.net/gml#interval">
      <rdfs:comment>Warning: This ObjectProperty type was declared outside of its original schema. This ObjectProperty may be declared incorrectly.</rdfs:comment>
      <rdfs:domain rdf:resource="http://www.opengis.net/gml#TimeCoordinateSystemType"/>
      <rdfs:range rdf:resource="http://www.opengis.net/gml#TimeIntervalLengthType"/>
   </owl:ObjectProperty>
   <owl:ObjectProperty rdf:about="http://www.opengis.net/gml#component">
      <rdfs:comment>Warning: This ObjectProperty type was declared outside of its original schema. This ObjectProperty may be declared incorrectly.</rdfs:comment>
      <rdfs:domain rdf:resource="http://www.opengis.net/gml#TimeOrdinalReferenceSystemType"/>
      <rdfs:range rdf:resource="http://www.opengis.net/gml#TimeOrdinalEraPropertyType"/>
   </owl:ObjectProperty>
   <owl:ObjectProperty rdf:about="http://www.opengis.net/gml#relatedTime">
      <rdfs:comment>Warning: This ObjectProperty type was declared outside of its original schema. This ObjectProperty may be declared incorrectly.</rdfs:comment>
      <rdfs:domain rdf:resource="http://www.opengis.net/gml#TimeOrdinalEraType"/>
      <rdfs:range rdf:resource="http://www.opengis.net/gml#RelatedTimeType"/>
   </owl:ObjectProperty>
   <owl:ObjectProperty rdf:about="http://www.opengis.net/gml#start">
      <rdfs:comment>Warning: This ObjectProperty type was declared outside of its original schema. This ObjectProperty may be declared incorrectly.</rdfs:comment>
      <rdfs:domain rdf:resource="http://www.opengis.net/gml#TimeOrdinalEraType"/>
      <rdfs:range rdf:resource="http://www.opengis.net/gml#TimeNodePropertyType"/>
   </owl:ObjectProperty>
   <owl:ObjectProperty rdf:about="http://www.opengis.net/gml#end">
      <rdfs:comment>Warning: This ObjectProperty type was declared outside of its original schema. This ObjectProperty may be declared incorrectly.</rdfs:comment>
      <rdfs:domain rdf:resource="http://www.opengis.net/gml#TimeOrdinalEraType"/>
      <rdfs:range rdf:resource="http://www.opengis.net/gml#TimeNodePropertyType"/>
   </owl:ObjectProperty>
   <owl:ObjectProperty rdf:about="http://www.opengis.net/gml#extent">
      <rdfs:comment>Warning: This ObjectProperty type was declared outside of its original schema. This ObjectProperty may be declared incorrectly.</rdfs:comment>
      <rdfs:domain rdf:resource="http://www.opengis.net/gml#TimeOrdinalEraType"/>
      <rdfs:range rdf:resource="http://www.opengis.net/gml#TimePeriodPropertyType"/>
   </owl:ObjectProperty>
   <owl:ObjectProperty rdf:about="http://www.opengis.net/gml#member">
      <rdfs:comment>Warning: This ObjectProperty type was declared outside of its original schema. This ObjectProperty may be declared incorrectly.</rdfs:comment>
      <rdfs:domain rdf:resource="http://www.opengis.net/gml#TimeOrdinalEraType"/>
      <rdfs:range rdf:resource="http://www.opengis.net/gml#TimeOrdinalEraPropertyType"/>
   </owl:ObjectProperty>
   <owl:ObjectProperty rdf:about="http://www.opengis.net/gml#group">
      <rdfs:comment>Warning: This ObjectProperty type was declared outside of its original schema. This ObjectProperty may be declared incorrectly.</rdfs:comment>
      <rdfs:domain rdf:resource="http://www.opengis.net/gml#TimeOrdinalEraType"/>
      <rdfs:range rdf:resource="http://www.opengis.net/gml#ReferenceType"/>
   </owl:ObjectProperty>
   <owl:ObjectProperty rdf:about="http://www.opengis.net/gml#hasTimeOrdinalEra">
      <rdfs:comment>Warning: This ObjectProperty reference was declared outside of its original schema. This ObjectProperty may be declared incorrectly.</rdfs:comment>
      <rdfs:domain rdf:resource="http://www.opengis.net/gml#TimeOrdinalEraPropertyType"/>
      <rdfs:range rdf:resource="http://www.opengis.net/gml#TimeOrdinalEra"/>
   </owl:ObjectProperty>
   <owl:ObjectProperty rdf:about="http://www.opengis.net/gml#referenceFrame">
      <rdfs:comment>Warning: This ObjectProperty type was declared outside of its original schema. This ObjectProperty may be declared incorrectly.</rdfs:comment>
      <rdfs:domain rdf:resource="http://www.opengis.net/gml#TimeCalendarType"/>
      <rdfs:range rdf:resource="http://www.opengis.net/gml#TimeCalendarEraPropertyType"/>
   </owl:ObjectProperty>
   <owl:ObjectProperty rdf:about="http://www.opengis.net/gml#hasTimeCalendar">
      <rdfs:comment>Warning: This ObjectProperty reference was declared outside of its original schema. This ObjectProperty may be declared incorrectly.</rdfs:comment>
      <rdfs:domain rdf:resource="http://www.opengis.net/gml#TimeCalendarPropertyType"/>
      <rdfs:range rdf:resource="http://www.opengis.net/gml#TimeCalendar"/>
   </owl:ObjectProperty>
   <owl:ObjectProperty rdf:about="http://www.opengis.net/gml#referenceEvent">
      <rdfs:comment>Warning: This ObjectProperty type was declared outside of its original schema. This ObjectProperty may be declared incorrectly.</rdfs:comment>
      <rdfs:domain rdf:resource="http://www.opengis.net/gml#TimeCalendarEraType"/>
      <rdfs:range rdf:resource="http://www.opengis.net/gml#StringOrRefType"/>
   </owl:ObjectProperty>
   <owl:DatatypeProperty rdf:about="http://www.opengis.net/gml#referenceDate">
      <rdfs:domain rdf:resource="http://www.opengis.net/gml#TimeCalendarEraType"/>
      <rdfs:range rdf:resource="http://www.w3.org/2001/XMLSchema#date"/>
   </owl:DatatypeProperty>
   <owl:DatatypeProperty rdf:about="http://www.opengis.net/gml#julianReference">
      <rdfs:domain rdf:resource="http://www.opengis.net/gml#TimeCalendarEraType"/>
      <rdfs:range rdf:resource="http://www.w3.org/2001/XMLSchema#decimal"/>
   </owl:DatatypeProperty>
   <owl:ObjectProperty rdf:about="http://www.opengis.net/gml#epochOfUse">
      <rdfs:comment>Warning: This ObjectProperty type was declared outside of its original schema. This ObjectProperty may be declared incorrectly.</rdfs:comment>
      <rdfs:domain rdf:resource="http://www.opengis.net/gml#TimeCalendarEraType"/>
      <rdfs:range rdf:resource="http://www.opengis.net/gml#TimePeriodPropertyType"/>
   </owl:ObjectProperty>
   <owl:ObjectProperty rdf:about="http://www.opengis.net/gml#hasTimeCalendarEra">
      <rdfs:comment>Warning: This ObjectProperty reference was declared outside of its original schema. This ObjectProperty may be declared incorrectly.</rdfs:comment>
      <rdfs:domain rdf:resource="http://www.opengis.net/gml#TimeCalendarEraPropertyType"/>
      <rdfs:range rdf:resource="http://www.opengis.net/gml#TimeCalendarEra"/>
   </owl:ObjectProperty>
   <owl:ObjectProperty rdf:about="http://www.opengis.net/gml#referenceEvent">
      <rdfs:comment>Warning: This ObjectProperty type was declared outside of its original schema. This ObjectProperty may be declared incorrectly.</rdfs:comment>
      <rdfs:domain rdf:resource="http://www.opengis.net/gml#TimeClockType"/>
      <rdfs:range rdf:resource="http://www.opengis.net/gml#StringOrRefType"/>
   </owl:ObjectProperty>
   <owl:DatatypeProperty rdf:about="http://www.opengis.net/gml#referenceTime">
      <rdfs:domain rdf:resource="http://www.opengis.net/gml#TimeClockType"/>
      <rdfs:range rdf:resource="http://www.w3.org/2001/XMLSchema#time"/>
   </owl:DatatypeProperty>
   <owl:DatatypeProperty rdf:about="http://www.opengis.net/gml#utcReference">
      <rdfs:domain rdf:resource="http://www.opengis.net/gml#TimeClockType"/>
      <rdfs:range rdf:resource="http://www.w3.org/2001/XMLSchema#time"/>
   </owl:DatatypeProperty>
   <owl:ObjectProperty rdf:about="http://www.opengis.net/gml#dateBasis">
      <rdfs:comment>Warning: This ObjectProperty type was declared outside of its original schema. This ObjectProperty may be declared incorrectly.</rdfs:comment>
      <rdfs:domain rdf:resource="http://www.opengis.net/gml#TimeClockType"/>
      <rdfs:range rdf:resource="http://www.opengis.net/gml#TimeCalendarPropertyType"/>
   </owl:ObjectProperty>
   <owl:ObjectProperty rdf:about="http://www.opengis.net/gml#hasTimeClock">
      <rdfs:comment>Warning: This ObjectProperty reference was declared outside of its original schema. This ObjectProperty may be declared incorrectly.</rdfs:comment>
      <rdfs:domain rdf:resource="http://www.opengis.net/gml#TimeClockPropertyType"/>
      <rdfs:range rdf:resource="http://www.opengis.net/gml#TimeClock"/>
   </owl:ObjectProperty>
</rdf:RDF>
