<rdf:RDF xmlns:math="http://www.w3.org/2005/xpath-functions/math" xmlns:owl="http://www.w3.org/2002/07/owl#" xmlns:rdf="http://www.w3.org/1999/02/22-rdf-syntax-ns#" xmlns:rdfs="http://www.w3.org/2000/01/rdf-schema#" xmlns:xs="http://www.w3.org/2001/XMLSchema" xmlns:xsd="http://www.w3.org/2001/XMLSchema">
   <owl:Ontology rdf:about="http://liris.cnrs.fr/ontologies/topology">
      <rdfs:comment>topology.xsd</rdfs:comment>
      <rdfs:seeAlso>urn:opengis:specification:gml:schema-xsd:topology:3.1.1</rdfs:seeAlso>
      <rdfs:comment>
			GML is an OGC Standard.
			Copyright (c) 2001,2005,2010 Open Geospatial Consortium.
			To obtain additional rights of use, visit http://www.opengeospatial.org/legal/ .
		</rdfs:comment>
   </owl:Ontology>
   <owl:Class rdf:about="http://www.opengis.net/gml#AbstractTopologyType">
      <rdfs:comment>This is an abstract class</rdfs:comment>
   </owl:Class>
   <owl:Class rdf:about="http://www.opengis.net/gml#AbstractTopoPrimitiveType">
      <rdfs:comment>This is an abstract class</rdfs:comment>
      <rdfs:subClassOf>
         <owl:Class>
            <owl:intersectionOf rdf:parseType="Collection">
               <owl:Restriction>
                  <owl:onProperty rdf:resource="http://www.opengis.net/gml#hasisolated"/>
                  <owl:allValuesFrom rdf:resource="http://www.opengis.net/gml#isolated"/>
               </owl:Restriction>
               <owl:Restriction>
                  <owl:onProperty rdf:resource="http://www.opengis.net/gml#hasisolated"/>
                  <owl:minCardinality rdf:datatype="http://www.w3.org/2001/XMLSchema#nonNegativeInteger">0</owl:minCardinality>
               </owl:Restriction>
               <owl:Restriction>
                  <owl:onProperty rdf:resource="http://www.opengis.net/gml#hascontainer"/>
                  <owl:allValuesFrom rdf:resource="http://www.opengis.net/gml#container"/>
               </owl:Restriction>
               <owl:Restriction>
                  <owl:onProperty rdf:resource="http://www.opengis.net/gml#hascontainer"/>
                  <owl:minCardinality rdf:datatype="http://www.w3.org/2001/XMLSchema#nonNegativeInteger">0</owl:minCardinality>
               </owl:Restriction>
            </owl:intersectionOf>
         </owl:Class>
      </rdfs:subClassOf>
      <rdfs:subClassOf rdf:resource="http://www.opengis.net/gml#AbstractTopologyType"/>
   </owl:Class>
   <owl:Class rdf:about="http://www.opengis.net/gml#IsolatedPropertyType">
      <owl:disjointUnionOf rdf:parseType="Collection">
         <owl:Restriction>
            <owl:onProperty rdf:resource="http://www.opengis.net/gml#hasNode"/>
            <owl:someValuesFrom rdf:resource="http://www.opengis.net/gml#Node"/>
         </owl:Restriction>
         <owl:Restriction>
            <owl:onProperty rdf:resource="http://www.opengis.net/gml#hasEdge"/>
            <owl:someValuesFrom rdf:resource="http://www.opengis.net/gml#Edge"/>
         </owl:Restriction>
      </owl:disjointUnionOf>
   </owl:Class>
   <owl:Class rdf:about="http://www.opengis.net/gml#ContainerPropertyType">
      <owl:disjointUnionOf rdf:parseType="Collection">
         <owl:Restriction>
            <owl:onProperty rdf:resource="http://www.opengis.net/gml#hasFace"/>
            <owl:someValuesFrom rdf:resource="http://www.opengis.net/gml#Face"/>
         </owl:Restriction>
         <owl:Restriction>
            <owl:onProperty rdf:resource="http://www.opengis.net/gml#hasTopoSolid"/>
            <owl:someValuesFrom rdf:resource="http://www.opengis.net/gml#TopoSolid"/>
         </owl:Restriction>
      </owl:disjointUnionOf>
   </owl:Class>
   <owl:Class rdf:about="http://www.opengis.net/gml#NodeType">
      <rdfs:comment>Its optional co-boundary is a set of connected directedEdges.  The orientation of one of these dirEdges is "+" if the Node is the "to" node of the Edge, and "-" if it is the "from" node.</rdfs:comment>
      <rdfs:subClassOf>
         <owl:Class>
            <owl:intersectionOf rdf:parseType="Collection">
               <owl:Restriction>
                  <owl:onProperty rdf:resource="http://www.opengis.net/gml#hasdirectedEdge"/>
                  <owl:allValuesFrom rdf:resource="http://www.opengis.net/gml#directedEdge"/>
               </owl:Restriction>
               <owl:Restriction>
                  <owl:onProperty rdf:resource="http://www.opengis.net/gml#hasdirectedEdge"/>
                  <owl:minCardinality rdf:datatype="http://www.w3.org/2001/XMLSchema#nonNegativeInteger">0</owl:minCardinality>
               </owl:Restriction>
               <owl:Restriction>
                  <owl:onProperty rdf:resource="http://www.opengis.net/gml#haspointProperty"/>
                  <owl:allValuesFrom rdf:resource="http://www.opengis.net/gml#pointProperty"/>
               </owl:Restriction>
               <owl:Restriction>
                  <owl:onProperty rdf:resource="http://www.opengis.net/gml#haspointProperty"/>
                  <owl:minCardinality rdf:datatype="http://www.w3.org/2001/XMLSchema#nonNegativeInteger">0</owl:minCardinality>
               </owl:Restriction>
            </owl:intersectionOf>
         </owl:Class>
      </rdfs:subClassOf>
      <rdfs:subClassOf rdf:resource="http://www.opengis.net/gml#AbstractTopoPrimitiveType"/>
   </owl:Class>
   <owl:Class rdf:about="http://www.opengis.net/gml#DirectedNodePropertyType">
      <rdfs:subClassOf>
         <owl:Class>
            <owl:intersectionOf rdf:parseType="Collection">
               <owl:Restriction>
                  <owl:onProperty rdf:resource="http://www.opengis.net/gml#hasNode"/>
                  <owl:allValuesFrom rdf:resource="http://www.opengis.net/gml#Node"/>
               </owl:Restriction>
            </owl:intersectionOf>
         </owl:Class>
      </rdfs:subClassOf>
      <rdfs:subClassOf>
         <owl:Class>
            <owl:intersectionOf rdf:parseType="Collection">
               <owl:Restriction>
                  <owl:onProperty rdf:resource="http://www.opengis.net/gml#orientation"/>
                  <owl:allValuesFrom rdf:resource="http://www.opengis.net/gml#SignType"/>
               </owl:Restriction>
            </owl:intersectionOf>
         </owl:Class>
      </rdfs:subClassOf>
   </owl:Class>
   <owl:Class rdf:about="http://www.opengis.net/gml#EdgeType">
      <rdfs:comment>There is precisely one positively directed and one negatively directed node in the boundary of every edge. The negatively and positively directed nodes correspond to the start and end nodes respectively. The optional coboundary of an edge is a circular sequence of directed faces which are incident on this edge in document order. Faces which use a particular boundary edge in its positive orientation appear with positive orientation on the coboundary of the same edge. In the 2D case, the orientation of the face on the left of the edge is "+"; the orientation of the face on the right on its right is "-". An edge may optionally be realised by a 1-dimensional (curve) geometric primitive.</rdfs:comment>
      <rdfs:subClassOf>
         <owl:Class>
            <owl:intersectionOf rdf:parseType="Collection">
               <owl:Restriction>
                  <owl:onProperty rdf:resource="http://www.opengis.net/gml#hasdirectedNode"/>
                  <owl:allValuesFrom rdf:resource="http://www.opengis.net/gml#directedNode"/>
               </owl:Restriction>
               <owl:Restriction>
                  <owl:onProperty rdf:resource="http://www.opengis.net/gml#hasdirectedNode"/>
                  <owl:cardinality rdf:datatype="http://www.w3.org/2001/XMLSchema#nonNegativeInteger">2</owl:cardinality>
               </owl:Restriction>
               <owl:Restriction>
                  <owl:onProperty rdf:resource="http://www.opengis.net/gml#hasdirectedFace"/>
                  <owl:allValuesFrom rdf:resource="http://www.opengis.net/gml#directedFace"/>
               </owl:Restriction>
               <owl:Restriction>
                  <owl:onProperty rdf:resource="http://www.opengis.net/gml#hasdirectedFace"/>
                  <owl:minCardinality rdf:datatype="http://www.w3.org/2001/XMLSchema#nonNegativeInteger">0</owl:minCardinality>
               </owl:Restriction>
               <owl:Restriction>
                  <owl:onProperty rdf:resource="http://www.opengis.net/gml#hascurveProperty"/>
                  <owl:allValuesFrom rdf:resource="http://www.opengis.net/gml#curveProperty"/>
               </owl:Restriction>
               <owl:Restriction>
                  <owl:onProperty rdf:resource="http://www.opengis.net/gml#hascurveProperty"/>
                  <owl:minCardinality rdf:datatype="http://www.w3.org/2001/XMLSchema#nonNegativeInteger">0</owl:minCardinality>
               </owl:Restriction>
            </owl:intersectionOf>
         </owl:Class>
      </rdfs:subClassOf>
      <rdfs:subClassOf rdf:resource="http://www.opengis.net/gml#AbstractTopoPrimitiveType"/>
   </owl:Class>
   <owl:Class rdf:about="http://www.opengis.net/gml#DirectedEdgePropertyType">
      <rdfs:subClassOf>
         <owl:Class>
            <owl:intersectionOf rdf:parseType="Collection">
               <owl:Restriction>
                  <owl:onProperty rdf:resource="http://www.opengis.net/gml#hasEdge"/>
                  <owl:allValuesFrom rdf:resource="http://www.opengis.net/gml#Edge"/>
               </owl:Restriction>
            </owl:intersectionOf>
         </owl:Class>
      </rdfs:subClassOf>
      <rdfs:subClassOf>
         <owl:Class>
            <owl:intersectionOf rdf:parseType="Collection">
               <owl:Restriction>
                  <owl:onProperty rdf:resource="http://www.opengis.net/gml#orientation"/>
                  <owl:allValuesFrom rdf:resource="http://www.opengis.net/gml#SignType"/>
               </owl:Restriction>
            </owl:intersectionOf>
         </owl:Class>
      </rdfs:subClassOf>
   </owl:Class>
   <owl:Class rdf:about="http://www.opengis.net/gml#FaceType">
      <rdfs:comment>. The topological boundary of a face consists of a set of directed edges. Note that all edges associated with a Face, including dangling and interior edges, appear in the boundary.  Dangling and interior edges are each referenced by pairs of directedEdges with opposing orientations.  The optional coboundary of a face is a pair of directed solids which are bounded by this face. If present, there is precisely one positively directed and one negatively directed solid in the coboundary of every face. The positively directed solid corresponds to the solid which lies in the direction of the positively directed normal to the face in any geometric realisation.  A face may optionally be realised by a 2-dimensional (surface) geometric primitive.</rdfs:comment>
      <rdfs:subClassOf>
         <owl:Class>
            <owl:intersectionOf rdf:parseType="Collection">
               <owl:Restriction>
                  <owl:onProperty rdf:resource="http://www.opengis.net/gml#hasdirectedEdge"/>
                  <owl:allValuesFrom rdf:resource="http://www.opengis.net/gml#directedEdge"/>
               </owl:Restriction>
               <owl:Restriction>
                  <owl:onProperty rdf:resource="http://www.opengis.net/gml#hasdirectedTopoSolid"/>
                  <owl:allValuesFrom rdf:resource="http://www.opengis.net/gml#directedTopoSolid"/>
               </owl:Restriction>
               <owl:Restriction>
                  <owl:onProperty rdf:resource="http://www.opengis.net/gml#hasdirectedTopoSolid"/>
                  <owl:minCardinality rdf:datatype="http://www.w3.org/2001/XMLSchema#nonNegativeInteger">0</owl:minCardinality>
                  <owl:onProperty rdf:resource="http://www.opengis.net/gml#hasdirectedTopoSolid"/>
                  <owl:minCardinality rdf:datatype="http://www.w3.org/2001/XMLSchema#nonNegativeInteger">2</owl:minCardinality>
               </owl:Restriction>
               <owl:Restriction>
                  <owl:onProperty rdf:resource="http://www.opengis.net/gml#hassurfaceProperty"/>
                  <owl:allValuesFrom rdf:resource="http://www.opengis.net/gml#surfaceProperty"/>
               </owl:Restriction>
               <owl:Restriction>
                  <owl:onProperty rdf:resource="http://www.opengis.net/gml#hassurfaceProperty"/>
                  <owl:minCardinality rdf:datatype="http://www.w3.org/2001/XMLSchema#nonNegativeInteger">0</owl:minCardinality>
               </owl:Restriction>
            </owl:intersectionOf>
         </owl:Class>
      </rdfs:subClassOf>
      <rdfs:subClassOf rdf:resource="http://www.opengis.net/gml#AbstractTopoPrimitiveType"/>
   </owl:Class>
   <owl:Class rdf:about="http://www.opengis.net/gml#DirectedFacePropertyType">
      <rdfs:subClassOf>
         <owl:Class>
            <owl:intersectionOf rdf:parseType="Collection">
               <owl:Restriction>
                  <owl:onProperty rdf:resource="http://www.opengis.net/gml#hasFace"/>
                  <owl:allValuesFrom rdf:resource="http://www.opengis.net/gml#Face"/>
               </owl:Restriction>
            </owl:intersectionOf>
         </owl:Class>
      </rdfs:subClassOf>
      <rdfs:subClassOf>
         <owl:Class>
            <owl:intersectionOf rdf:parseType="Collection">
               <owl:Restriction>
                  <owl:onProperty rdf:resource="http://www.opengis.net/gml#orientation"/>
                  <owl:allValuesFrom rdf:resource="http://www.opengis.net/gml#SignType"/>
               </owl:Restriction>
            </owl:intersectionOf>
         </owl:Class>
      </rdfs:subClassOf>
   </owl:Class>
   <owl:Class rdf:about="http://www.opengis.net/gml#TopoSolidType">
      <rdfs:comment>The topological boundary of a TopoSolid consists of a set of directed faces. Note that all faces associated with the TopoSolid, including dangling faces, appear in the boundary. The coboundary of a TopoSolid is empty and hence requires no representation.</rdfs:comment>
      <rdfs:subClassOf>
         <owl:Class>
            <owl:intersectionOf rdf:parseType="Collection">
               <owl:Restriction>
                  <owl:onProperty rdf:resource="http://www.opengis.net/gml#hasdirectedFace"/>
                  <owl:allValuesFrom rdf:resource="http://www.opengis.net/gml#directedFace"/>
               </owl:Restriction>
            </owl:intersectionOf>
         </owl:Class>
      </rdfs:subClassOf>
      <rdfs:subClassOf rdf:resource="http://www.opengis.net/gml#AbstractTopoPrimitiveType"/>
   </owl:Class>
   <owl:Class rdf:about="http://www.opengis.net/gml#DirectedTopoSolidPropertyType">
      <rdfs:subClassOf>
         <owl:Class>
            <owl:intersectionOf rdf:parseType="Collection">
               <owl:Restriction>
                  <owl:onProperty rdf:resource="http://www.opengis.net/gml#hasTopoSolid"/>
                  <owl:allValuesFrom rdf:resource="http://www.opengis.net/gml#TopoSolid"/>
               </owl:Restriction>
            </owl:intersectionOf>
         </owl:Class>
      </rdfs:subClassOf>
      <rdfs:subClassOf>
         <owl:Class>
            <owl:intersectionOf rdf:parseType="Collection">
               <owl:Restriction>
                  <owl:onProperty rdf:resource="http://www.opengis.net/gml#orientation"/>
                  <owl:allValuesFrom rdf:resource="http://www.opengis.net/gml#SignType"/>
               </owl:Restriction>
            </owl:intersectionOf>
         </owl:Class>
      </rdfs:subClassOf>
   </owl:Class>
   <owl:Class rdf:about="http://www.opengis.net/gml#TopoPointType">
      <rdfs:comment>The intended use of TopoPoint is to appear within a point feature to express the structural and possibly geometric relationships of this point to other features via shared node definitions. Note the orientation assigned to the directedNode has no meaning in this context. It is preserved for symmetry with the types and elements which follow.</rdfs:comment>
      <rdfs:subClassOf>
         <owl:Class>
            <owl:intersectionOf rdf:parseType="Collection">
               <owl:Restriction>
                  <owl:onProperty rdf:resource="http://www.opengis.net/gml#hasdirectedNode"/>
                  <owl:allValuesFrom rdf:resource="http://www.opengis.net/gml#directedNode"/>
               </owl:Restriction>
            </owl:intersectionOf>
         </owl:Class>
      </rdfs:subClassOf>
      <rdfs:subClassOf rdf:resource="http://www.opengis.net/gml#AbstractTopologyType"/>
   </owl:Class>
   <owl:Class rdf:about="http://www.opengis.net/gml#TopoPointPropertyType">
      <rdfs:subClassOf>
         <owl:Class>
            <owl:intersectionOf rdf:parseType="Collection">
               <owl:Restriction>
                  <owl:onProperty rdf:resource="http://www.opengis.net/gml#hasTopoPoint"/>
                  <owl:allValuesFrom rdf:resource="http://www.opengis.net/gml#TopoPoint"/>
               </owl:Restriction>
            </owl:intersectionOf>
         </owl:Class>
      </rdfs:subClassOf>
   </owl:Class>
   <owl:Class rdf:about="http://www.opengis.net/gml#TopoCurveType">
      <rdfs:comment>The end Node of each directedEdge of a TopoCurveType
is the start Node of the next directedEdge of the TopoCurveType in document order.  The TopoCurve type and element represent a homogeneous topological expression, a list of directed edges, which if realised are isomorphic to a geometric curve primitive. The intended use of TopoCurve is to appear within a line feature instance to express the structural and geometric relationships of this line to other features via the shared edge definitions.</rdfs:comment>
      <rdfs:subClassOf>
         <owl:Class>
            <owl:intersectionOf rdf:parseType="Collection">
               <owl:Restriction>
                  <owl:onProperty rdf:resource="http://www.opengis.net/gml#hasdirectedEdge"/>
                  <owl:allValuesFrom rdf:resource="http://www.opengis.net/gml#directedEdge"/>
               </owl:Restriction>
            </owl:intersectionOf>
         </owl:Class>
      </rdfs:subClassOf>
      <rdfs:subClassOf rdf:resource="http://www.opengis.net/gml#AbstractTopologyType"/>
   </owl:Class>
   <owl:Class rdf:about="http://www.opengis.net/gml#TopoCurvePropertyType">
      <rdfs:subClassOf>
         <owl:Class>
            <owl:intersectionOf rdf:parseType="Collection">
               <owl:Restriction>
                  <owl:onProperty rdf:resource="http://www.opengis.net/gml#hasTopoCurve"/>
                  <owl:allValuesFrom rdf:resource="http://www.opengis.net/gml#TopoCurve"/>
               </owl:Restriction>
            </owl:intersectionOf>
         </owl:Class>
      </rdfs:subClassOf>
   </owl:Class>
   <owl:Class rdf:about="http://www.opengis.net/gml#TopoSurfaceType">
      <rdfs:comment>The TopoSurface type and element represent a homogeneous topological expression, a set of directed faces, which if realised are isomorphic to a geometric surface primitive. The intended use of TopoSurface is to appear within a surface feature instance to express the structural and possibly geometric relationships of this surface to other features via the shared face definitions.</rdfs:comment>
      <rdfs:subClassOf>
         <owl:Class>
            <owl:intersectionOf rdf:parseType="Collection">
               <owl:Restriction>
                  <owl:onProperty rdf:resource="http://www.opengis.net/gml#hasdirectedFace"/>
                  <owl:allValuesFrom rdf:resource="http://www.opengis.net/gml#directedFace"/>
               </owl:Restriction>
            </owl:intersectionOf>
         </owl:Class>
      </rdfs:subClassOf>
      <rdfs:subClassOf rdf:resource="http://www.opengis.net/gml#AbstractTopologyType"/>
   </owl:Class>
   <owl:Class rdf:about="http://www.opengis.net/gml#TopoSurfacePropertyType">
      <rdfs:subClassOf>
         <owl:Class>
            <owl:intersectionOf rdf:parseType="Collection">
               <owl:Restriction>
                  <owl:onProperty rdf:resource="http://www.opengis.net/gml#hasTopoSurface"/>
                  <owl:allValuesFrom rdf:resource="http://www.opengis.net/gml#TopoSurface"/>
               </owl:Restriction>
            </owl:intersectionOf>
         </owl:Class>
      </rdfs:subClassOf>
   </owl:Class>
   <owl:Class rdf:about="http://www.opengis.net/gml#TopoVolumeType">
      <rdfs:comment>The TopoVolume type and element represent a homogeneous topological expression, a set of directed TopoSolids, which if realised are isomorphic to a geometric solid primitive. The intended use of TopoVolume is to appear within a 3D solid feature instance to express the structural and geometric relationships of this solid to other features via the shared TopoSolid definitions.  . Note the orientation assigned to the directedSolid has no meaning in three dimensions. It is preserved for symmetry with the preceding types and elements.</rdfs:comment>
      <rdfs:subClassOf>
         <owl:Class>
            <owl:intersectionOf rdf:parseType="Collection">
               <owl:Restriction>
                  <owl:onProperty rdf:resource="http://www.opengis.net/gml#hasdirectedTopoSolid"/>
                  <owl:allValuesFrom rdf:resource="http://www.opengis.net/gml#directedTopoSolid"/>
               </owl:Restriction>
            </owl:intersectionOf>
         </owl:Class>
      </rdfs:subClassOf>
      <rdfs:subClassOf rdf:resource="http://www.opengis.net/gml#AbstractTopologyType"/>
   </owl:Class>
   <owl:Class rdf:about="http://www.opengis.net/gml#TopoVolumePropertyType">
      <rdfs:subClassOf>
         <owl:Class>
            <owl:intersectionOf rdf:parseType="Collection">
               <owl:Restriction>
                  <owl:onProperty rdf:resource="http://www.opengis.net/gml#hasTopoVolume"/>
                  <owl:allValuesFrom rdf:resource="http://www.opengis.net/gml#TopoVolume"/>
               </owl:Restriction>
            </owl:intersectionOf>
         </owl:Class>
      </rdfs:subClassOf>
   </owl:Class>
   <owl:Class rdf:about="http://www.opengis.net/gml#TopoComplexType">
      <rdfs:comment>This type represents a TP_Complex capable of holding topological primitives.</rdfs:comment>
      <rdfs:subClassOf>
         <owl:Class>
            <owl:intersectionOf rdf:parseType="Collection">
               <owl:Restriction>
                  <owl:onProperty rdf:resource="http://www.opengis.net/gml#hasmaximalComplex"/>
                  <owl:allValuesFrom rdf:resource="http://www.opengis.net/gml#maximalComplex"/>
               </owl:Restriction>
               <owl:Restriction>
                  <owl:onProperty rdf:resource="http://www.opengis.net/gml#hassuperComplex"/>
                  <owl:allValuesFrom rdf:resource="http://www.opengis.net/gml#superComplex"/>
               </owl:Restriction>
               <owl:Restriction>
                  <owl:onProperty rdf:resource="http://www.opengis.net/gml#hassuperComplex"/>
                  <owl:minCardinality rdf:datatype="http://www.w3.org/2001/XMLSchema#nonNegativeInteger">0</owl:minCardinality>
               </owl:Restriction>
               <owl:Restriction>
                  <owl:onProperty rdf:resource="http://www.opengis.net/gml#hassubComplex"/>
                  <owl:allValuesFrom rdf:resource="http://www.opengis.net/gml#subComplex"/>
               </owl:Restriction>
               <owl:Restriction>
                  <owl:onProperty rdf:resource="http://www.opengis.net/gml#hassubComplex"/>
                  <owl:minCardinality rdf:datatype="http://www.w3.org/2001/XMLSchema#nonNegativeInteger">0</owl:minCardinality>
               </owl:Restriction>
               <owl:Restriction>
                  <owl:onProperty rdf:resource="http://www.opengis.net/gml#hastopoPrimitiveMember"/>
                  <owl:allValuesFrom rdf:resource="http://www.opengis.net/gml#topoPrimitiveMember"/>
               </owl:Restriction>
               <owl:Restriction>
                  <owl:onProperty rdf:resource="http://www.opengis.net/gml#hastopoPrimitiveMember"/>
                  <owl:minCardinality rdf:datatype="http://www.w3.org/2001/XMLSchema#nonNegativeInteger">0</owl:minCardinality>
               </owl:Restriction>
               <owl:Restriction>
                  <owl:onProperty rdf:resource="http://www.opengis.net/gml#hastopoPrimitiveMembers"/>
                  <owl:allValuesFrom rdf:resource="http://www.opengis.net/gml#topoPrimitiveMembers"/>
               </owl:Restriction>
               <owl:Restriction>
                  <owl:onProperty rdf:resource="http://www.opengis.net/gml#hastopoPrimitiveMembers"/>
                  <owl:minCardinality rdf:datatype="http://www.w3.org/2001/XMLSchema#nonNegativeInteger">0</owl:minCardinality>
               </owl:Restriction>
            </owl:intersectionOf>
         </owl:Class>
      </rdfs:subClassOf>
      <rdfs:subClassOf>
         <owl:Class>
            <owl:intersectionOf rdf:parseType="Collection">
               <owl:Restriction>
                  <owl:onProperty rdf:resource="http://www.opengis.net/gml#isMaximal"/>
                  <owl:allValuesFrom rdf:resource="http://www.w3.org/2001/XMLSchema#boolean"/>
               </owl:Restriction>
            </owl:intersectionOf>
         </owl:Class>
      </rdfs:subClassOf>
      <rdfs:subClassOf rdf:resource="http://www.opengis.net/gml#AbstractTopologyType"/>
   </owl:Class>
   <owl:Class rdf:about="http://www.opengis.net/gml#TopoComplexMemberType">
      <rdfs:comment>This Property can be used to embed a TopoComplex in a feature collection.</rdfs:comment>
      <rdfs:subClassOf>
         <owl:Class>
            <owl:intersectionOf rdf:parseType="Collection">
               <owl:Restriction>
                  <owl:onProperty rdf:resource="http://www.opengis.net/gml#hasTopoComplex"/>
                  <owl:allValuesFrom rdf:resource="http://www.opengis.net/gml#TopoComplex"/>
               </owl:Restriction>
               <owl:Restriction>
                  <owl:onProperty rdf:resource="http://www.opengis.net/gml#hasTopoComplex"/>
                  <owl:minCardinality rdf:datatype="http://www.w3.org/2001/XMLSchema#nonNegativeInteger">0</owl:minCardinality>
               </owl:Restriction>
            </owl:intersectionOf>
         </owl:Class>
      </rdfs:subClassOf>
   </owl:Class>
   <owl:Class rdf:about="http://www.opengis.net/gml#TopoPrimitiveMemberType">
      <rdfs:comment>This type supports embedding topological primitives in a TopoComplex.</rdfs:comment>
      <rdfs:subClassOf>
         <owl:Class>
            <owl:intersectionOf rdf:parseType="Collection">
               <owl:Restriction>
                  <owl:onProperty rdf:resource="http://www.opengis.net/gml#has_TopoPrimitive"/>
                  <owl:allValuesFrom rdf:resource="http://www.opengis.net/gml#_TopoPrimitive"/>
               </owl:Restriction>
               <owl:Restriction>
                  <owl:onProperty rdf:resource="http://www.opengis.net/gml#has_TopoPrimitive"/>
                  <owl:minCardinality rdf:datatype="http://www.w3.org/2001/XMLSchema#nonNegativeInteger">0</owl:minCardinality>
               </owl:Restriction>
            </owl:intersectionOf>
         </owl:Class>
      </rdfs:subClassOf>
   </owl:Class>
   <owl:Class rdf:about="http://www.opengis.net/gml#TopoPrimitiveArrayAssociationType">
      <rdfs:comment>This type supports embedding an array of topological primitives in a TopoComplex</rdfs:comment>
      <owl:disjointUnionOf rdf:parseType="Collection">
         <owl:Restriction>
            <owl:onProperty rdf:resource="http://www.opengis.net/gml#has_TopoPrimitive"/>
            <owl:someValuesFrom rdf:resource="http://www.opengis.net/gml#_TopoPrimitive"/>
         </owl:Restriction>
      </owl:disjointUnionOf>
   </owl:Class>
   <owl:DatatypeProperty rdf:about="http://www.opengis.net/gml#orientation">
      <rdfs:domain rdf:resource="http://www.opengis.net/gml#DirectedNodePropertyType"/>
      <rdfs:range rdf:resource="http://www.opengis.net/gml#SignType"/>
   </owl:DatatypeProperty>
   <owl:DatatypeProperty rdf:about="http://www.opengis.net/gml#orientation">
      <rdfs:domain rdf:resource="http://www.opengis.net/gml#DirectedEdgePropertyType"/>
      <rdfs:range rdf:resource="http://www.opengis.net/gml#SignType"/>
   </owl:DatatypeProperty>
   <owl:DatatypeProperty rdf:about="http://www.opengis.net/gml#orientation">
      <rdfs:domain rdf:resource="http://www.opengis.net/gml#DirectedFacePropertyType"/>
      <rdfs:range rdf:resource="http://www.opengis.net/gml#SignType"/>
   </owl:DatatypeProperty>
   <owl:DatatypeProperty rdf:about="http://www.opengis.net/gml#orientation">
      <rdfs:domain rdf:resource="http://www.opengis.net/gml#DirectedTopoSolidPropertyType"/>
      <rdfs:range rdf:resource="http://www.opengis.net/gml#SignType"/>
   </owl:DatatypeProperty>
   <owl:DatatypeProperty rdf:about="http://www.opengis.net/gml#isMaximal">
      <rdfs:domain rdf:resource="http://www.opengis.net/gml#TopoComplexType"/>
      <rdfs:range rdf:resource="http://www.w3.org/2001/XMLSchema#boolean"/>
   </owl:DatatypeProperty>
   <owl:Class rdf:about="http://www.opengis.net/gml#_Topology">
      <rdfs:subClassOf rdf:resource="http://www.opengis.net/gml#_GML"/>
      <rdfs:subClassOf rdf:resource="http://www.opengis.net/gml#AbstractTopologyType"/>
   </owl:Class>
   <owl:Class rdf:about="http://www.opengis.net/gml#_TopoPrimitive">
      <rdfs:subClassOf rdf:resource="http://www.opengis.net/gml#_Topology"/>
      <rdfs:subClassOf rdf:resource="http://www.opengis.net/gml#AbstractTopoPrimitiveType"/>
   </owl:Class>
   <owl:Class rdf:about="http://www.opengis.net/gml#isolated">
      <rdfs:subClassOf rdf:resource="http://www.opengis.net/gml#IsolatedPropertyType"/>
   </owl:Class>
   <owl:Class rdf:about="http://www.opengis.net/gml#container">
      <rdfs:subClassOf rdf:resource="http://www.opengis.net/gml#ContainerPropertyType"/>
   </owl:Class>
   <owl:Class rdf:about="http://www.opengis.net/gml#Node">
      <rdfs:subClassOf rdf:resource="http://www.opengis.net/gml#_TopoPrimitive"/>
      <rdfs:subClassOf rdf:resource="http://www.opengis.net/gml#NodeType"/>
   </owl:Class>
   <owl:Class rdf:about="http://www.opengis.net/gml#directedNode">
      <rdfs:subClassOf rdf:resource="http://www.opengis.net/gml#DirectedNodePropertyType"/>
   </owl:Class>
   <owl:Class rdf:about="http://www.opengis.net/gml#Edge">
      <rdfs:subClassOf rdf:resource="http://www.opengis.net/gml#_TopoPrimitive"/>
      <rdfs:subClassOf rdf:resource="http://www.opengis.net/gml#EdgeType"/>
   </owl:Class>
   <owl:Class rdf:about="http://www.opengis.net/gml#directedEdge">
      <rdfs:subClassOf rdf:resource="http://www.opengis.net/gml#DirectedEdgePropertyType"/>
   </owl:Class>
   <owl:Class rdf:about="http://www.opengis.net/gml#Face">
      <rdfs:subClassOf rdf:resource="http://www.opengis.net/gml#_TopoPrimitive"/>
      <rdfs:subClassOf rdf:resource="http://www.opengis.net/gml#FaceType"/>
   </owl:Class>
   <owl:Class rdf:about="http://www.opengis.net/gml#directedFace">
      <rdfs:subClassOf rdf:resource="http://www.opengis.net/gml#DirectedFacePropertyType"/>
   </owl:Class>
   <owl:Class rdf:about="http://www.opengis.net/gml#TopoSolid">
      <rdfs:subClassOf rdf:resource="http://www.opengis.net/gml#_TopoPrimitive"/>
      <rdfs:subClassOf rdf:resource="http://www.opengis.net/gml#TopoSolidType"/>
   </owl:Class>
   <owl:Class rdf:about="http://www.opengis.net/gml#directedTopoSolid">
      <rdfs:subClassOf rdf:resource="http://www.opengis.net/gml#DirectedTopoSolidPropertyType"/>
   </owl:Class>
   <owl:Class rdf:about="http://www.opengis.net/gml#TopoPoint">
      <rdfs:subClassOf rdf:resource="http://www.opengis.net/gml#TopoPointType"/>
   </owl:Class>
   <owl:Class rdf:about="http://www.opengis.net/gml#topoPointProperty">
      <rdfs:subClassOf rdf:resource="http://www.opengis.net/gml#TopoPointPropertyType"/>
   </owl:Class>
   <owl:Class rdf:about="http://www.opengis.net/gml#TopoCurve">
      <rdfs:subClassOf rdf:resource="http://www.opengis.net/gml#TopoCurveType"/>
   </owl:Class>
   <owl:Class rdf:about="http://www.opengis.net/gml#topoCurveProperty">
      <rdfs:subClassOf rdf:resource="http://www.opengis.net/gml#TopoCurvePropertyType"/>
   </owl:Class>
   <owl:Class rdf:about="http://www.opengis.net/gml#TopoSurface">
      <rdfs:subClassOf rdf:resource="http://www.opengis.net/gml#TopoSurfaceType"/>
   </owl:Class>
   <owl:Class rdf:about="http://www.opengis.net/gml#topoSurfaceProperty">
      <rdfs:subClassOf rdf:resource="http://www.opengis.net/gml#TopoSurfacePropertyType"/>
   </owl:Class>
   <owl:Class rdf:about="http://www.opengis.net/gml#TopoVolume">
      <rdfs:subClassOf rdf:resource="http://www.opengis.net/gml#TopoVolumeType"/>
   </owl:Class>
   <owl:Class rdf:about="http://www.opengis.net/gml#topoVolumeProperty">
      <rdfs:subClassOf rdf:resource="http://www.opengis.net/gml#TopoVolumePropertyType"/>
   </owl:Class>
   <owl:Class rdf:about="http://www.opengis.net/gml#TopoComplex">
      <rdfs:subClassOf rdf:resource="http://www.opengis.net/gml#_Topology"/>
      <rdfs:subClassOf rdf:resource="http://www.opengis.net/gml#TopoComplexType"/>
   </owl:Class>
   <owl:Class rdf:about="http://www.opengis.net/gml#topoComplexProperty">
      <rdfs:subClassOf rdf:resource="http://www.opengis.net/gml#TopoComplexMemberType"/>
   </owl:Class>
   <owl:Class rdf:about="http://www.opengis.net/gml#subComplex">
      <rdfs:subClassOf rdf:resource="http://www.opengis.net/gml#TopoComplexMemberType"/>
   </owl:Class>
   <owl:Class rdf:about="http://www.opengis.net/gml#superComplex">
      <rdfs:subClassOf rdf:resource="http://www.opengis.net/gml#TopoComplexMemberType"/>
   </owl:Class>
   <owl:Class rdf:about="http://www.opengis.net/gml#maximalComplex">
      <rdfs:subClassOf rdf:resource="http://www.opengis.net/gml#TopoComplexMemberType"/>
   </owl:Class>
   <owl:Class rdf:about="http://www.opengis.net/gml#topoPrimitiveMember">
      <rdfs:subClassOf rdf:resource="http://www.opengis.net/gml#TopoPrimitiveMemberType"/>
   </owl:Class>
   <owl:Class rdf:about="http://www.opengis.net/gml#topoPrimitiveMembers">
      <rdfs:subClassOf rdf:resource="http://www.opengis.net/gml#TopoPrimitiveArrayAssociationType"/>
   </owl:Class>
   <owl:ObjectProperty rdf:about="http://www.opengis.net/gml#hasisolated">
      <rdfs:comment>Warning: This ObjectProperty reference was declared outside of its original schema. This ObjectProperty may be declared incorrectly.</rdfs:comment>
      <rdfs:domain rdf:resource="http://www.opengis.net/gml#AbstractTopoPrimitiveType"/>
      <rdfs:range rdf:resource="http://www.opengis.net/gml#isolated"/>
   </owl:ObjectProperty>
   <owl:ObjectProperty rdf:about="http://www.opengis.net/gml#hascontainer">
      <rdfs:comment>Warning: This ObjectProperty reference was declared outside of its original schema. This ObjectProperty may be declared incorrectly.</rdfs:comment>
      <rdfs:domain rdf:resource="http://www.opengis.net/gml#AbstractTopoPrimitiveType"/>
      <rdfs:range rdf:resource="http://www.opengis.net/gml#container"/>
   </owl:ObjectProperty>
   <owl:ObjectProperty rdf:about="http://www.opengis.net/gml#hasNode">
      <rdfs:comment>Warning: This ObjectProperty reference was declared outside of its original schema. This ObjectProperty may be declared incorrectly.</rdfs:comment>
      <rdfs:domain rdf:resource="http://www.opengis.net/gml#IsolatedPropertyType"/>
      <rdfs:range rdf:resource="http://www.opengis.net/gml#Node"/>
   </owl:ObjectProperty>
   <owl:ObjectProperty rdf:about="http://www.opengis.net/gml#hasEdge">
      <rdfs:comment>Warning: This ObjectProperty reference was declared outside of its original schema. This ObjectProperty may be declared incorrectly.</rdfs:comment>
      <rdfs:domain rdf:resource="http://www.opengis.net/gml#IsolatedPropertyType"/>
      <rdfs:range rdf:resource="http://www.opengis.net/gml#Edge"/>
   </owl:ObjectProperty>
   <owl:ObjectProperty rdf:about="http://www.opengis.net/gml#hasFace">
      <rdfs:comment>Warning: This ObjectProperty reference was declared outside of its original schema. This ObjectProperty may be declared incorrectly.</rdfs:comment>
      <rdfs:domain rdf:resource="http://www.opengis.net/gml#ContainerPropertyType"/>
      <rdfs:range rdf:resource="http://www.opengis.net/gml#Face"/>
   </owl:ObjectProperty>
   <owl:ObjectProperty rdf:about="http://www.opengis.net/gml#hasTopoSolid">
      <rdfs:comment>Warning: This ObjectProperty reference was declared outside of its original schema. This ObjectProperty may be declared incorrectly.</rdfs:comment>
      <rdfs:domain rdf:resource="http://www.opengis.net/gml#ContainerPropertyType"/>
      <rdfs:range rdf:resource="http://www.opengis.net/gml#TopoSolid"/>
   </owl:ObjectProperty>
   <owl:ObjectProperty rdf:about="http://www.opengis.net/gml#hasdirectedEdge">
      <rdfs:comment>Warning: This ObjectProperty reference was declared outside of its original schema. This ObjectProperty may be declared incorrectly.</rdfs:comment>
      <rdfs:domain rdf:resource="http://www.opengis.net/gml#NodeType"/>
      <rdfs:range rdf:resource="http://www.opengis.net/gml#directedEdge"/>
   </owl:ObjectProperty>
   <owl:ObjectProperty rdf:about="http://www.opengis.net/gml#haspointProperty">
      <rdfs:comment>Warning: This ObjectProperty reference was declared outside of its original schema. This ObjectProperty may be declared incorrectly.</rdfs:comment>
      <rdfs:domain rdf:resource="http://www.opengis.net/gml#NodeType"/>
      <rdfs:range rdf:resource="http://www.opengis.net/gml#pointProperty"/>
   </owl:ObjectProperty>
   <owl:ObjectProperty rdf:about="http://www.opengis.net/gml#hasNode">
      <rdfs:comment>Warning: This ObjectProperty reference was declared outside of its original schema. This ObjectProperty may be declared incorrectly.</rdfs:comment>
      <rdfs:domain rdf:resource="http://www.opengis.net/gml#DirectedNodePropertyType"/>
      <rdfs:range rdf:resource="http://www.opengis.net/gml#Node"/>
   </owl:ObjectProperty>
   <owl:ObjectProperty rdf:about="http://www.opengis.net/gml#hasdirectedNode">
      <rdfs:comment>Warning: This ObjectProperty reference was declared outside of its original schema. This ObjectProperty may be declared incorrectly.</rdfs:comment>
      <rdfs:domain rdf:resource="http://www.opengis.net/gml#EdgeType"/>
      <rdfs:range rdf:resource="http://www.opengis.net/gml#directedNode"/>
   </owl:ObjectProperty>
   <owl:ObjectProperty rdf:about="http://www.opengis.net/gml#hasdirectedFace">
      <rdfs:comment>Warning: This ObjectProperty reference was declared outside of its original schema. This ObjectProperty may be declared incorrectly.</rdfs:comment>
      <rdfs:domain rdf:resource="http://www.opengis.net/gml#EdgeType"/>
      <rdfs:range rdf:resource="http://www.opengis.net/gml#directedFace"/>
   </owl:ObjectProperty>
   <owl:ObjectProperty rdf:about="http://www.opengis.net/gml#hascurveProperty">
      <rdfs:comment>Warning: This ObjectProperty reference was declared outside of its original schema. This ObjectProperty may be declared incorrectly.</rdfs:comment>
      <rdfs:domain rdf:resource="http://www.opengis.net/gml#EdgeType"/>
      <rdfs:range rdf:resource="http://www.opengis.net/gml#curveProperty"/>
   </owl:ObjectProperty>
   <owl:ObjectProperty rdf:about="http://www.opengis.net/gml#hasEdge">
      <rdfs:comment>Warning: This ObjectProperty reference was declared outside of its original schema. This ObjectProperty may be declared incorrectly.</rdfs:comment>
      <rdfs:domain rdf:resource="http://www.opengis.net/gml#DirectedEdgePropertyType"/>
      <rdfs:range rdf:resource="http://www.opengis.net/gml#Edge"/>
   </owl:ObjectProperty>
   <owl:ObjectProperty rdf:about="http://www.opengis.net/gml#hasdirectedEdge">
      <rdfs:comment>Warning: This ObjectProperty reference was declared outside of its original schema. This ObjectProperty may be declared incorrectly.</rdfs:comment>
      <rdfs:domain rdf:resource="http://www.opengis.net/gml#FaceType"/>
      <rdfs:range rdf:resource="http://www.opengis.net/gml#directedEdge"/>
   </owl:ObjectProperty>
   <owl:ObjectProperty rdf:about="http://www.opengis.net/gml#hasdirectedTopoSolid">
      <rdfs:comment>Warning: This ObjectProperty reference was declared outside of its original schema. This ObjectProperty may be declared incorrectly.</rdfs:comment>
      <rdfs:domain rdf:resource="http://www.opengis.net/gml#FaceType"/>
      <rdfs:range rdf:resource="http://www.opengis.net/gml#directedTopoSolid"/>
   </owl:ObjectProperty>
   <owl:ObjectProperty rdf:about="http://www.opengis.net/gml#hassurfaceProperty">
      <rdfs:comment>Warning: This ObjectProperty reference was declared outside of its original schema. This ObjectProperty may be declared incorrectly.</rdfs:comment>
      <rdfs:domain rdf:resource="http://www.opengis.net/gml#FaceType"/>
      <rdfs:range rdf:resource="http://www.opengis.net/gml#surfaceProperty"/>
   </owl:ObjectProperty>
   <owl:ObjectProperty rdf:about="http://www.opengis.net/gml#hasFace">
      <rdfs:comment>Warning: This ObjectProperty reference was declared outside of its original schema. This ObjectProperty may be declared incorrectly.</rdfs:comment>
      <rdfs:domain rdf:resource="http://www.opengis.net/gml#DirectedFacePropertyType"/>
      <rdfs:range rdf:resource="http://www.opengis.net/gml#Face"/>
   </owl:ObjectProperty>
   <owl:ObjectProperty rdf:about="http://www.opengis.net/gml#hasdirectedFace">
      <rdfs:comment>Warning: This ObjectProperty reference was declared outside of its original schema. This ObjectProperty may be declared incorrectly.</rdfs:comment>
      <rdfs:domain rdf:resource="http://www.opengis.net/gml#TopoSolidType"/>
      <rdfs:range rdf:resource="http://www.opengis.net/gml#directedFace"/>
   </owl:ObjectProperty>
   <owl:ObjectProperty rdf:about="http://www.opengis.net/gml#hasTopoSolid">
      <rdfs:comment>Warning: This ObjectProperty reference was declared outside of its original schema. This ObjectProperty may be declared incorrectly.</rdfs:comment>
      <rdfs:domain rdf:resource="http://www.opengis.net/gml#DirectedTopoSolidPropertyType"/>
      <rdfs:range rdf:resource="http://www.opengis.net/gml#TopoSolid"/>
   </owl:ObjectProperty>
   <owl:ObjectProperty rdf:about="http://www.opengis.net/gml#hasdirectedNode">
      <rdfs:comment>Warning: This ObjectProperty reference was declared outside of its original schema. This ObjectProperty may be declared incorrectly.</rdfs:comment>
      <rdfs:domain rdf:resource="http://www.opengis.net/gml#TopoPointType"/>
      <rdfs:range rdf:resource="http://www.opengis.net/gml#directedNode"/>
   </owl:ObjectProperty>
   <owl:ObjectProperty rdf:about="http://www.opengis.net/gml#hasTopoPoint">
      <rdfs:comment>Warning: This ObjectProperty reference was declared outside of its original schema. This ObjectProperty may be declared incorrectly.</rdfs:comment>
      <rdfs:domain rdf:resource="http://www.opengis.net/gml#TopoPointPropertyType"/>
      <rdfs:range rdf:resource="http://www.opengis.net/gml#TopoPoint"/>
   </owl:ObjectProperty>
   <owl:ObjectProperty rdf:about="http://www.opengis.net/gml#hasdirectedEdge">
      <rdfs:comment>Warning: This ObjectProperty reference was declared outside of its original schema. This ObjectProperty may be declared incorrectly.</rdfs:comment>
      <rdfs:domain rdf:resource="http://www.opengis.net/gml#TopoCurveType"/>
      <rdfs:range rdf:resource="http://www.opengis.net/gml#directedEdge"/>
   </owl:ObjectProperty>
   <owl:ObjectProperty rdf:about="http://www.opengis.net/gml#hasTopoCurve">
      <rdfs:comment>Warning: This ObjectProperty reference was declared outside of its original schema. This ObjectProperty may be declared incorrectly.</rdfs:comment>
      <rdfs:domain rdf:resource="http://www.opengis.net/gml#TopoCurvePropertyType"/>
      <rdfs:range rdf:resource="http://www.opengis.net/gml#TopoCurve"/>
   </owl:ObjectProperty>
   <owl:ObjectProperty rdf:about="http://www.opengis.net/gml#hasdirectedFace">
      <rdfs:comment>Warning: This ObjectProperty reference was declared outside of its original schema. This ObjectProperty may be declared incorrectly.</rdfs:comment>
      <rdfs:domain rdf:resource="http://www.opengis.net/gml#TopoSurfaceType"/>
      <rdfs:range rdf:resource="http://www.opengis.net/gml#directedFace"/>
   </owl:ObjectProperty>
   <owl:ObjectProperty rdf:about="http://www.opengis.net/gml#hasTopoSurface">
      <rdfs:comment>Warning: This ObjectProperty reference was declared outside of its original schema. This ObjectProperty may be declared incorrectly.</rdfs:comment>
      <rdfs:domain rdf:resource="http://www.opengis.net/gml#TopoSurfacePropertyType"/>
      <rdfs:range rdf:resource="http://www.opengis.net/gml#TopoSurface"/>
   </owl:ObjectProperty>
   <owl:ObjectProperty rdf:about="http://www.opengis.net/gml#hasdirectedTopoSolid">
      <rdfs:comment>Warning: This ObjectProperty reference was declared outside of its original schema. This ObjectProperty may be declared incorrectly.</rdfs:comment>
      <rdfs:domain rdf:resource="http://www.opengis.net/gml#TopoVolumeType"/>
      <rdfs:range rdf:resource="http://www.opengis.net/gml#directedTopoSolid"/>
   </owl:ObjectProperty>
   <owl:ObjectProperty rdf:about="http://www.opengis.net/gml#hasTopoVolume">
      <rdfs:comment>Warning: This ObjectProperty reference was declared outside of its original schema. This ObjectProperty may be declared incorrectly.</rdfs:comment>
      <rdfs:domain rdf:resource="http://www.opengis.net/gml#TopoVolumePropertyType"/>
      <rdfs:range rdf:resource="http://www.opengis.net/gml#TopoVolume"/>
   </owl:ObjectProperty>
   <owl:ObjectProperty rdf:about="http://www.opengis.net/gml#hasmaximalComplex">
      <rdfs:comment>Warning: This ObjectProperty reference was declared outside of its original schema. This ObjectProperty may be declared incorrectly.</rdfs:comment>
      <rdfs:domain rdf:resource="http://www.opengis.net/gml#TopoComplexType"/>
      <rdfs:range rdf:resource="http://www.opengis.net/gml#maximalComplex"/>
   </owl:ObjectProperty>
   <owl:ObjectProperty rdf:about="http://www.opengis.net/gml#hassuperComplex">
      <rdfs:comment>Warning: This ObjectProperty reference was declared outside of its original schema. This ObjectProperty may be declared incorrectly.</rdfs:comment>
      <rdfs:domain rdf:resource="http://www.opengis.net/gml#TopoComplexType"/>
      <rdfs:range rdf:resource="http://www.opengis.net/gml#superComplex"/>
   </owl:ObjectProperty>
   <owl:ObjectProperty rdf:about="http://www.opengis.net/gml#hassubComplex">
      <rdfs:comment>Warning: This ObjectProperty reference was declared outside of its original schema. This ObjectProperty may be declared incorrectly.</rdfs:comment>
      <rdfs:domain rdf:resource="http://www.opengis.net/gml#TopoComplexType"/>
      <rdfs:range rdf:resource="http://www.opengis.net/gml#subComplex"/>
   </owl:ObjectProperty>
   <owl:ObjectProperty rdf:about="http://www.opengis.net/gml#hastopoPrimitiveMember">
      <rdfs:comment>Warning: This ObjectProperty reference was declared outside of its original schema. This ObjectProperty may be declared incorrectly.</rdfs:comment>
      <rdfs:domain rdf:resource="http://www.opengis.net/gml#TopoComplexType"/>
      <rdfs:range rdf:resource="http://www.opengis.net/gml#topoPrimitiveMember"/>
   </owl:ObjectProperty>
   <owl:ObjectProperty rdf:about="http://www.opengis.net/gml#hastopoPrimitiveMembers">
      <rdfs:comment>Warning: This ObjectProperty reference was declared outside of its original schema. This ObjectProperty may be declared incorrectly.</rdfs:comment>
      <rdfs:domain rdf:resource="http://www.opengis.net/gml#TopoComplexType"/>
      <rdfs:range rdf:resource="http://www.opengis.net/gml#topoPrimitiveMembers"/>
   </owl:ObjectProperty>
   <owl:ObjectProperty rdf:about="http://www.opengis.net/gml#hasTopoComplex">
      <rdfs:comment>Warning: This ObjectProperty reference was declared outside of its original schema. This ObjectProperty may be declared incorrectly.</rdfs:comment>
      <rdfs:domain rdf:resource="http://www.opengis.net/gml#TopoComplexMemberType"/>
      <rdfs:range rdf:resource="http://www.opengis.net/gml#TopoComplex"/>
   </owl:ObjectProperty>
   <owl:ObjectProperty rdf:about="http://www.opengis.net/gml#has_TopoPrimitive">
      <rdfs:comment>Warning: This ObjectProperty reference was declared outside of its original schema. This ObjectProperty may be declared incorrectly.</rdfs:comment>
      <rdfs:domain rdf:resource="http://www.opengis.net/gml#TopoPrimitiveMemberType"/>
      <rdfs:range rdf:resource="http://www.opengis.net/gml#_TopoPrimitive"/>
   </owl:ObjectProperty>
   <owl:ObjectProperty rdf:about="http://www.opengis.net/gml#has_TopoPrimitive">
      <rdfs:comment>Warning: This ObjectProperty reference was declared outside of its original schema. This ObjectProperty may be declared incorrectly.</rdfs:comment>
      <rdfs:domain rdf:resource="http://www.opengis.net/gml#TopoPrimitiveArrayAssociationType"/>
      <rdfs:range rdf:resource="http://www.opengis.net/gml#_TopoPrimitive"/>
   </owl:ObjectProperty>
</rdf:RDF>
