<rdf:RDF xmlns:math="http://www.w3.org/2005/xpath-functions/math" xmlns:owl="http://www.w3.org/2002/07/owl#" xmlns:rdf="http://www.w3.org/1999/02/22-rdf-syntax-ns#" xmlns:rdfs="http://www.w3.org/2000/01/rdf-schema#" xmlns:xs="http://www.w3.org/2001/XMLSchema" xmlns:xsd="http://www.w3.org/2001/XMLSchema">
   <owl:Ontology rdf:about="http://liris.cnrs.fr/ontologies/transportation">
      <owl:imports rdf:resource="http://liris.cnrs.fr/ontologies/gml"/>
      <owl:imports rdf:resource="http://liris.cnrs.fr/ontologies/cityGMLBase"/>
      <rdfs:comment>
	CityGML is an OGC Standard.
	Copyright (c) 2012 Open Geospatial Consortium.
	To obtain additional rights of use, visit http://www.opengeospatial.org/legal/ .
		</rdfs:comment>
   </owl:Ontology>
   <owl:Class rdf:about="#AbstractTransportationObjectType">
      <rdfs:comment>This is an abstract class</rdfs:comment>
      <rdfs:comment>Type describing the abstract superclass for transportation objects. </rdfs:comment>
      <rdfs:subClassOf>
         <owl:Class>
            <owl:intersectionOf rdf:parseType="Collection">
               <owl:Restriction>
                  <owl:onProperty rdf:resource="#has_GenericApplicationPropertyOfTransportationObject"/>
                  <owl:allValuesFrom rdf:resource="#_GenericApplicationPropertyOfTransportationObject"/>
               </owl:Restriction>
               <owl:Restriction>
                  <owl:onProperty rdf:resource="#has_GenericApplicationPropertyOfTransportationObject"/>
                  <owl:minCardinality rdf:datatype="http://www.w3.org/2001/XMLSchema#nonNegativeInteger">0</owl:minCardinality>
               </owl:Restriction>
            </owl:intersectionOf>
         </owl:Class>
      </rdfs:subClassOf>
      <rdfs:subClassOf rdf:resource="http://www.opengis.net/citygml/2.0#AbstractCityObjectType"/>
      <rdfs:comment>Warning: The parent class 'core:AbstractCityObjectType' is declared outside of this class' original schema. This class may be declared incorrectly.</rdfs:comment>
   </owl:Class>
   <owl:Class rdf:about="#TransportationComplexType">
      <rdfs:comment>Type describing transportation complexes, which are aggregated features, e.g. roads, which consist of
				parts (traffic areas, e.g. pedestrian path, and auxiliary traffic areas). As subclass of _CityObject, a
				TransportationComplex inherits all attributes and relations, in particular an id, names, external references, and
				generalization relations. </rdfs:comment>
      <rdfs:subClassOf>
         <owl:Class>
            <owl:intersectionOf rdf:parseType="Collection">
               <owl:Restriction>
                  <owl:onProperty rdf:resource="#class"/>
                  <owl:allValuesFrom rdf:resource="http://www.opengis.net/gml#CodeType"/>
               </owl:Restriction>
               <owl:Restriction>
                  <owl:onProperty rdf:resource="#class"/>
                  <owl:minCardinality rdf:datatype="http://www.w3.org/2001/XMLSchema#nonNegativeInteger">0</owl:minCardinality>
               </owl:Restriction>
               <owl:Restriction>
                  <owl:onProperty rdf:resource="#function"/>
                  <owl:allValuesFrom rdf:resource="http://www.opengis.net/gml#CodeType"/>
               </owl:Restriction>
               <owl:Restriction>
                  <owl:onProperty rdf:resource="#function"/>
                  <owl:minCardinality rdf:datatype="http://www.w3.org/2001/XMLSchema#nonNegativeInteger">0</owl:minCardinality>
               </owl:Restriction>
               <owl:Restriction>
                  <owl:onProperty rdf:resource="#usage"/>
                  <owl:allValuesFrom rdf:resource="http://www.opengis.net/gml#CodeType"/>
               </owl:Restriction>
               <owl:Restriction>
                  <owl:onProperty rdf:resource="#usage"/>
                  <owl:minCardinality rdf:datatype="http://www.w3.org/2001/XMLSchema#nonNegativeInteger">0</owl:minCardinality>
               </owl:Restriction>
               <owl:Restriction>
                  <owl:onProperty rdf:resource="#trafficArea"/>
                  <owl:allValuesFrom rdf:resource="#TrafficAreaPropertyType"/>
               </owl:Restriction>
               <owl:Restriction>
                  <owl:onProperty rdf:resource="#trafficArea"/>
                  <owl:minCardinality rdf:datatype="http://www.w3.org/2001/XMLSchema#nonNegativeInteger">0</owl:minCardinality>
               </owl:Restriction>
               <owl:Restriction>
                  <owl:onProperty rdf:resource="#auxiliaryTrafficArea"/>
                  <owl:allValuesFrom rdf:resource="#AuxiliaryTrafficAreaPropertyType"/>
               </owl:Restriction>
               <owl:Restriction>
                  <owl:onProperty rdf:resource="#auxiliaryTrafficArea"/>
                  <owl:minCardinality rdf:datatype="http://www.w3.org/2001/XMLSchema#nonNegativeInteger">0</owl:minCardinality>
               </owl:Restriction>
               <owl:Restriction>
                  <owl:onProperty rdf:resource="#lod0Network"/>
                  <owl:allValuesFrom rdf:resource="http://www.opengis.net/gml#GeometricComplexPropertyType"/>
               </owl:Restriction>
               <owl:Restriction>
                  <owl:onProperty rdf:resource="#lod0Network"/>
                  <owl:minCardinality rdf:datatype="http://www.w3.org/2001/XMLSchema#nonNegativeInteger">0</owl:minCardinality>
               </owl:Restriction>
               <owl:Restriction>
                  <owl:onProperty rdf:resource="#lod1MultiSurface"/>
                  <owl:allValuesFrom rdf:resource="http://www.opengis.net/gml#MultiSurfacePropertyType"/>
               </owl:Restriction>
               <owl:Restriction>
                  <owl:onProperty rdf:resource="#lod1MultiSurface"/>
                  <owl:minCardinality rdf:datatype="http://www.w3.org/2001/XMLSchema#nonNegativeInteger">0</owl:minCardinality>
               </owl:Restriction>
               <owl:Restriction>
                  <owl:onProperty rdf:resource="#lod2MultiSurface"/>
                  <owl:allValuesFrom rdf:resource="http://www.opengis.net/gml#MultiSurfacePropertyType"/>
               </owl:Restriction>
               <owl:Restriction>
                  <owl:onProperty rdf:resource="#lod2MultiSurface"/>
                  <owl:minCardinality rdf:datatype="http://www.w3.org/2001/XMLSchema#nonNegativeInteger">0</owl:minCardinality>
               </owl:Restriction>
               <owl:Restriction>
                  <owl:onProperty rdf:resource="#lod3MultiSurface"/>
                  <owl:allValuesFrom rdf:resource="http://www.opengis.net/gml#MultiSurfacePropertyType"/>
               </owl:Restriction>
               <owl:Restriction>
                  <owl:onProperty rdf:resource="#lod3MultiSurface"/>
                  <owl:minCardinality rdf:datatype="http://www.w3.org/2001/XMLSchema#nonNegativeInteger">0</owl:minCardinality>
               </owl:Restriction>
               <owl:Restriction>
                  <owl:onProperty rdf:resource="#lod4MultiSurface"/>
                  <owl:allValuesFrom rdf:resource="http://www.opengis.net/gml#MultiSurfacePropertyType"/>
               </owl:Restriction>
               <owl:Restriction>
                  <owl:onProperty rdf:resource="#lod4MultiSurface"/>
                  <owl:minCardinality rdf:datatype="http://www.w3.org/2001/XMLSchema#nonNegativeInteger">0</owl:minCardinality>
               </owl:Restriction>
               <owl:Restriction>
                  <owl:onProperty rdf:resource="#has_GenericApplicationPropertyOfTransportationComplex"/>
                  <owl:allValuesFrom rdf:resource="#_GenericApplicationPropertyOfTransportationComplex"/>
               </owl:Restriction>
               <owl:Restriction>
                  <owl:onProperty rdf:resource="#has_GenericApplicationPropertyOfTransportationComplex"/>
                  <owl:minCardinality rdf:datatype="http://www.w3.org/2001/XMLSchema#nonNegativeInteger">0</owl:minCardinality>
               </owl:Restriction>
            </owl:intersectionOf>
         </owl:Class>
      </rdfs:subClassOf>
      <rdfs:subClassOf rdf:resource="#AbstractTransportationObjectType"/>
   </owl:Class>
   <owl:Class rdf:about="#TrafficAreaType">
      <rdfs:comment>Type describing the class for traffic Areas. Traffic areas are the surfaces where traffic actually takes
				place. As subclass of _CityObject, a TrafficArea inherits all attributes and relations, in particular an id, names,
				external references, and generalization relations. </rdfs:comment>
      <rdfs:subClassOf>
         <owl:Class>
            <owl:intersectionOf rdf:parseType="Collection">
               <owl:Restriction>
                  <owl:onProperty rdf:resource="#class"/>
                  <owl:allValuesFrom rdf:resource="http://www.opengis.net/gml#CodeType"/>
               </owl:Restriction>
               <owl:Restriction>
                  <owl:onProperty rdf:resource="#class"/>
                  <owl:minCardinality rdf:datatype="http://www.w3.org/2001/XMLSchema#nonNegativeInteger">0</owl:minCardinality>
               </owl:Restriction>
               <owl:Restriction>
                  <owl:onProperty rdf:resource="#function"/>
                  <owl:allValuesFrom rdf:resource="http://www.opengis.net/gml#CodeType"/>
               </owl:Restriction>
               <owl:Restriction>
                  <owl:onProperty rdf:resource="#function"/>
                  <owl:minCardinality rdf:datatype="http://www.w3.org/2001/XMLSchema#nonNegativeInteger">0</owl:minCardinality>
               </owl:Restriction>
               <owl:Restriction>
                  <owl:onProperty rdf:resource="#usage"/>
                  <owl:allValuesFrom rdf:resource="http://www.opengis.net/gml#CodeType"/>
               </owl:Restriction>
               <owl:Restriction>
                  <owl:onProperty rdf:resource="#usage"/>
                  <owl:minCardinality rdf:datatype="http://www.w3.org/2001/XMLSchema#nonNegativeInteger">0</owl:minCardinality>
               </owl:Restriction>
               <owl:Restriction>
                  <owl:onProperty rdf:resource="#surfaceMaterial"/>
                  <owl:allValuesFrom rdf:resource="http://www.opengis.net/gml#CodeType"/>
               </owl:Restriction>
               <owl:Restriction>
                  <owl:onProperty rdf:resource="#surfaceMaterial"/>
                  <owl:minCardinality rdf:datatype="http://www.w3.org/2001/XMLSchema#nonNegativeInteger">0</owl:minCardinality>
               </owl:Restriction>
               <owl:Restriction>
                  <owl:onProperty rdf:resource="#lod2MultiSurface"/>
                  <owl:allValuesFrom rdf:resource="http://www.opengis.net/gml#MultiSurfacePropertyType"/>
               </owl:Restriction>
               <owl:Restriction>
                  <owl:onProperty rdf:resource="#lod2MultiSurface"/>
                  <owl:minCardinality rdf:datatype="http://www.w3.org/2001/XMLSchema#nonNegativeInteger">0</owl:minCardinality>
               </owl:Restriction>
               <owl:Restriction>
                  <owl:onProperty rdf:resource="#lod3MultiSurface"/>
                  <owl:allValuesFrom rdf:resource="http://www.opengis.net/gml#MultiSurfacePropertyType"/>
               </owl:Restriction>
               <owl:Restriction>
                  <owl:onProperty rdf:resource="#lod3MultiSurface"/>
                  <owl:minCardinality rdf:datatype="http://www.w3.org/2001/XMLSchema#nonNegativeInteger">0</owl:minCardinality>
               </owl:Restriction>
               <owl:Restriction>
                  <owl:onProperty rdf:resource="#lod4MultiSurface"/>
                  <owl:allValuesFrom rdf:resource="http://www.opengis.net/gml#MultiSurfacePropertyType"/>
               </owl:Restriction>
               <owl:Restriction>
                  <owl:onProperty rdf:resource="#lod4MultiSurface"/>
                  <owl:minCardinality rdf:datatype="http://www.w3.org/2001/XMLSchema#nonNegativeInteger">0</owl:minCardinality>
               </owl:Restriction>
               <owl:Restriction>
                  <owl:onProperty rdf:resource="#has_GenericApplicationPropertyOfTrafficArea"/>
                  <owl:allValuesFrom rdf:resource="#_GenericApplicationPropertyOfTrafficArea"/>
               </owl:Restriction>
               <owl:Restriction>
                  <owl:onProperty rdf:resource="#has_GenericApplicationPropertyOfTrafficArea"/>
                  <owl:minCardinality rdf:datatype="http://www.w3.org/2001/XMLSchema#nonNegativeInteger">0</owl:minCardinality>
               </owl:Restriction>
            </owl:intersectionOf>
         </owl:Class>
      </rdfs:subClassOf>
      <rdfs:subClassOf rdf:resource="#AbstractTransportationObjectType"/>
   </owl:Class>
   <owl:Class rdf:about="#AuxiliaryTrafficAreaType">
      <rdfs:comment>Type describing the class for auxiliary traffic Areas. These are the surfaces where no traffic actually
				takes place, but which belong to a transportation object. Examples are kerbstones, road markings and grass stripes. As
				subclass of _CityObject, an AuxiliaryTrafficArea inherits all attributes and relations, in particular an id, names,
				external references, and generalization relations. </rdfs:comment>
      <rdfs:subClassOf>
         <owl:Class>
            <owl:intersectionOf rdf:parseType="Collection">
               <owl:Restriction>
                  <owl:onProperty rdf:resource="#class"/>
                  <owl:allValuesFrom rdf:resource="http://www.opengis.net/gml#CodeType"/>
               </owl:Restriction>
               <owl:Restriction>
                  <owl:onProperty rdf:resource="#class"/>
                  <owl:minCardinality rdf:datatype="http://www.w3.org/2001/XMLSchema#nonNegativeInteger">0</owl:minCardinality>
               </owl:Restriction>
               <owl:Restriction>
                  <owl:onProperty rdf:resource="#function"/>
                  <owl:allValuesFrom rdf:resource="http://www.opengis.net/gml#CodeType"/>
               </owl:Restriction>
               <owl:Restriction>
                  <owl:onProperty rdf:resource="#function"/>
                  <owl:minCardinality rdf:datatype="http://www.w3.org/2001/XMLSchema#nonNegativeInteger">0</owl:minCardinality>
               </owl:Restriction>
               <owl:Restriction>
                  <owl:onProperty rdf:resource="#usage"/>
                  <owl:allValuesFrom rdf:resource="http://www.opengis.net/gml#CodeType"/>
               </owl:Restriction>
               <owl:Restriction>
                  <owl:onProperty rdf:resource="#usage"/>
                  <owl:minCardinality rdf:datatype="http://www.w3.org/2001/XMLSchema#nonNegativeInteger">0</owl:minCardinality>
               </owl:Restriction>
               <owl:Restriction>
                  <owl:onProperty rdf:resource="#surfaceMaterial"/>
                  <owl:allValuesFrom rdf:resource="http://www.opengis.net/gml#CodeType"/>
               </owl:Restriction>
               <owl:Restriction>
                  <owl:onProperty rdf:resource="#surfaceMaterial"/>
                  <owl:minCardinality rdf:datatype="http://www.w3.org/2001/XMLSchema#nonNegativeInteger">0</owl:minCardinality>
               </owl:Restriction>
               <owl:Restriction>
                  <owl:onProperty rdf:resource="#lod2MultiSurface"/>
                  <owl:allValuesFrom rdf:resource="http://www.opengis.net/gml#MultiSurfacePropertyType"/>
               </owl:Restriction>
               <owl:Restriction>
                  <owl:onProperty rdf:resource="#lod2MultiSurface"/>
                  <owl:minCardinality rdf:datatype="http://www.w3.org/2001/XMLSchema#nonNegativeInteger">0</owl:minCardinality>
               </owl:Restriction>
               <owl:Restriction>
                  <owl:onProperty rdf:resource="#lod3MultiSurface"/>
                  <owl:allValuesFrom rdf:resource="http://www.opengis.net/gml#MultiSurfacePropertyType"/>
               </owl:Restriction>
               <owl:Restriction>
                  <owl:onProperty rdf:resource="#lod3MultiSurface"/>
                  <owl:minCardinality rdf:datatype="http://www.w3.org/2001/XMLSchema#nonNegativeInteger">0</owl:minCardinality>
               </owl:Restriction>
               <owl:Restriction>
                  <owl:onProperty rdf:resource="#lod4MultiSurface"/>
                  <owl:allValuesFrom rdf:resource="http://www.opengis.net/gml#MultiSurfacePropertyType"/>
               </owl:Restriction>
               <owl:Restriction>
                  <owl:onProperty rdf:resource="#lod4MultiSurface"/>
                  <owl:minCardinality rdf:datatype="http://www.w3.org/2001/XMLSchema#nonNegativeInteger">0</owl:minCardinality>
               </owl:Restriction>
               <owl:Restriction>
                  <owl:onProperty rdf:resource="#has_GenericApplicationPropertyOfAuxiliaryTrafficArea"/>
                  <owl:allValuesFrom rdf:resource="#_GenericApplicationPropertyOfAuxiliaryTrafficArea"/>
               </owl:Restriction>
               <owl:Restriction>
                  <owl:onProperty rdf:resource="#has_GenericApplicationPropertyOfAuxiliaryTrafficArea"/>
                  <owl:minCardinality rdf:datatype="http://www.w3.org/2001/XMLSchema#nonNegativeInteger">0</owl:minCardinality>
               </owl:Restriction>
            </owl:intersectionOf>
         </owl:Class>
      </rdfs:subClassOf>
      <rdfs:subClassOf rdf:resource="#AbstractTransportationObjectType"/>
   </owl:Class>
   <owl:Class rdf:about="#TrafficAreaPropertyType">
      <rdfs:comment>Denotes the relation of TransportationComplex to its parts, which are traffic areas. The
				TrafficAreaPropertyType element must either carry a reference to a TrafficArea object or contain a TrafficArea object
				inline, but neither both nor none. </rdfs:comment>
      <rdfs:subClassOf>
         <owl:Class>
            <owl:intersectionOf rdf:parseType="Collection">
               <owl:Restriction>
                  <owl:onProperty rdf:resource="#hasTrafficArea"/>
                  <owl:allValuesFrom rdf:resource="#TrafficArea"/>
               </owl:Restriction>
            </owl:intersectionOf>
         </owl:Class>
      </rdfs:subClassOf>
   </owl:Class>
   <owl:Class rdf:about="#AuxiliaryTrafficAreaPropertyType">
      <rdfs:comment>Denotes the relation of TransportationComplex to its parts, which are auxiliary traffic areas. The
				TrafficAreaPropertyType element must either carry a reference to a TrafficArea object or contain a TrafficArea object
				inline, but neither both nor none. </rdfs:comment>
      <rdfs:subClassOf>
         <owl:Class>
            <owl:intersectionOf rdf:parseType="Collection">
               <owl:Restriction>
                  <owl:onProperty rdf:resource="#hasAuxiliaryTrafficArea"/>
                  <owl:allValuesFrom rdf:resource="#AuxiliaryTrafficArea"/>
               </owl:Restriction>
            </owl:intersectionOf>
         </owl:Class>
      </rdfs:subClassOf>
   </owl:Class>
   <owl:Class rdf:about="#TrackType">
      <rdfs:comment>Type describing the class for tracks. A track is a small path mainly used by pedestrians. As subclass of
				_CityObject, a Track inherits all attributes and relations, in particular an id, names, external references, and
				generalization relations. </rdfs:comment>
      <rdfs:subClassOf>
         <owl:Class>
            <owl:intersectionOf rdf:parseType="Collection">
               <owl:Restriction>
                  <owl:onProperty rdf:resource="#has_GenericApplicationPropertyOfTrack"/>
                  <owl:allValuesFrom rdf:resource="#_GenericApplicationPropertyOfTrack"/>
               </owl:Restriction>
               <owl:Restriction>
                  <owl:onProperty rdf:resource="#has_GenericApplicationPropertyOfTrack"/>
                  <owl:minCardinality rdf:datatype="http://www.w3.org/2001/XMLSchema#nonNegativeInteger">0</owl:minCardinality>
               </owl:Restriction>
            </owl:intersectionOf>
         </owl:Class>
      </rdfs:subClassOf>
      <rdfs:subClassOf rdf:resource="#TransportationComplexType"/>
   </owl:Class>
   <owl:Class rdf:about="#RoadType">
      <rdfs:comment>Type describing the class for roads. As subclass of _CityObject, a Road inherits all attributes and
				relations, in particular an id, names, external references, and generalization relations. </rdfs:comment>
      <rdfs:subClassOf>
         <owl:Class>
            <owl:intersectionOf rdf:parseType="Collection">
               <owl:Restriction>
                  <owl:onProperty rdf:resource="#has_GenericApplicationPropertyOfRoad"/>
                  <owl:allValuesFrom rdf:resource="#_GenericApplicationPropertyOfRoad"/>
               </owl:Restriction>
               <owl:Restriction>
                  <owl:onProperty rdf:resource="#has_GenericApplicationPropertyOfRoad"/>
                  <owl:minCardinality rdf:datatype="http://www.w3.org/2001/XMLSchema#nonNegativeInteger">0</owl:minCardinality>
               </owl:Restriction>
            </owl:intersectionOf>
         </owl:Class>
      </rdfs:subClassOf>
      <rdfs:subClassOf rdf:resource="#TransportationComplexType"/>
   </owl:Class>
   <owl:Class rdf:about="#RailwayType">
      <rdfs:comment>Type describing the class for railways. As subclass of _CityObject, a Railway inherits all attributes and
				relations, in particular an id, names, external references, and generalization relations. </rdfs:comment>
      <rdfs:subClassOf>
         <owl:Class>
            <owl:intersectionOf rdf:parseType="Collection">
               <owl:Restriction>
                  <owl:onProperty rdf:resource="#has_GenericApplicationPropertyOfRailway"/>
                  <owl:allValuesFrom rdf:resource="#_GenericApplicationPropertyOfRailway"/>
               </owl:Restriction>
               <owl:Restriction>
                  <owl:onProperty rdf:resource="#has_GenericApplicationPropertyOfRailway"/>
                  <owl:minCardinality rdf:datatype="http://www.w3.org/2001/XMLSchema#nonNegativeInteger">0</owl:minCardinality>
               </owl:Restriction>
            </owl:intersectionOf>
         </owl:Class>
      </rdfs:subClassOf>
      <rdfs:subClassOf rdf:resource="#TransportationComplexType"/>
   </owl:Class>
   <owl:Class rdf:about="#SquareType">
      <rdfs:comment>Type describing the class for squares. A square is an open area commonly found in cities (like a plaza).
				As subclass of _CityObject, a Square inherits all attributes and relations, in particular an id, names, external
				references, and generalization relations. </rdfs:comment>
      <rdfs:subClassOf>
         <owl:Class>
            <owl:intersectionOf rdf:parseType="Collection">
               <owl:Restriction>
                  <owl:onProperty rdf:resource="#has_GenericApplicationPropertyOfSquare"/>
                  <owl:allValuesFrom rdf:resource="#_GenericApplicationPropertyOfSquare"/>
               </owl:Restriction>
               <owl:Restriction>
                  <owl:onProperty rdf:resource="#has_GenericApplicationPropertyOfSquare"/>
                  <owl:minCardinality rdf:datatype="http://www.w3.org/2001/XMLSchema#nonNegativeInteger">0</owl:minCardinality>
               </owl:Restriction>
            </owl:intersectionOf>
         </owl:Class>
      </rdfs:subClassOf>
      <rdfs:subClassOf rdf:resource="#TransportationComplexType"/>
   </owl:Class>
   <owl:ObjectProperty rdf:about="http://www.opengis.net/gml#hasAssociationAttributeGroup">
      <rdfs:domain rdf:resource="#TrafficAreaPropertyType"/>
      <rdfs:range rdf:resource="http://www.opengis.net/gml#AssociationAttributeGroup"/>
   </owl:ObjectProperty>
   <owl:ObjectProperty rdf:about="http://www.opengis.net/gml#hasAssociationAttributeGroup">
      <rdfs:domain rdf:resource="#AuxiliaryTrafficAreaPropertyType"/>
      <rdfs:range rdf:resource="http://www.opengis.net/gml#AssociationAttributeGroup"/>
   </owl:ObjectProperty>
   <owl:Class rdf:about="#_TransportationObject">
      <rdfs:subClassOf rdf:resource="http://www.opengis.net/citygml/2.0#_CityObject"/>
      <rdfs:subClassOf rdf:resource="#AbstractTransportationObjectType"/>
   </owl:Class>
   <owl:Class rdf:about="#_GenericApplicationPropertyOfTransportationObject">
      <rdfs:subClassOf rdf:resource="http://www.w3.org/2001/XMLSchema#anyType"/>
      <rdfs:comment>Warning: This class type was declared outside of its original schema. This class may be declared incorrectly.</rdfs:comment>
   </owl:Class>
   <owl:Class rdf:about="#TransportationComplex">
      <rdfs:subClassOf rdf:resource="#_TransportationObject"/>
      <rdfs:subClassOf rdf:resource="#TransportationComplexType"/>
   </owl:Class>
   <owl:Class rdf:about="#_GenericApplicationPropertyOfTransportationComplex">
      <rdfs:subClassOf rdf:resource="http://www.w3.org/2001/XMLSchema#anyType"/>
      <rdfs:comment>Warning: This class type was declared outside of its original schema. This class may be declared incorrectly.</rdfs:comment>
   </owl:Class>
   <owl:Class rdf:about="#TrafficArea">
      <rdfs:subClassOf rdf:resource="#_TransportationObject"/>
      <rdfs:subClassOf rdf:resource="#TrafficAreaType"/>
   </owl:Class>
   <owl:Class rdf:about="#_GenericApplicationPropertyOfTrafficArea">
      <rdfs:subClassOf rdf:resource="http://www.w3.org/2001/XMLSchema#anyType"/>
      <rdfs:comment>Warning: This class type was declared outside of its original schema. This class may be declared incorrectly.</rdfs:comment>
   </owl:Class>
   <owl:Class rdf:about="#AuxiliaryTrafficArea">
      <rdfs:subClassOf rdf:resource="#_TransportationObject"/>
      <rdfs:subClassOf rdf:resource="#AuxiliaryTrafficAreaType"/>
   </owl:Class>
   <owl:Class rdf:about="#_GenericApplicationPropertyOfAuxiliaryTrafficArea">
      <rdfs:subClassOf rdf:resource="http://www.w3.org/2001/XMLSchema#anyType"/>
      <rdfs:comment>Warning: This class type was declared outside of its original schema. This class may be declared incorrectly.</rdfs:comment>
   </owl:Class>
   <owl:Class rdf:about="#Track">
      <rdfs:subClassOf rdf:resource="#TransportationComplex"/>
      <rdfs:subClassOf rdf:resource="#TrackType"/>
   </owl:Class>
   <owl:Class rdf:about="#_GenericApplicationPropertyOfTrack">
      <rdfs:subClassOf rdf:resource="http://www.w3.org/2001/XMLSchema#anyType"/>
      <rdfs:comment>Warning: This class type was declared outside of its original schema. This class may be declared incorrectly.</rdfs:comment>
   </owl:Class>
   <owl:Class rdf:about="#Road">
      <rdfs:subClassOf rdf:resource="#TransportationComplex"/>
      <rdfs:subClassOf rdf:resource="#RoadType"/>
   </owl:Class>
   <owl:Class rdf:about="#_GenericApplicationPropertyOfRoad">
      <rdfs:subClassOf rdf:resource="http://www.w3.org/2001/XMLSchema#anyType"/>
      <rdfs:comment>Warning: This class type was declared outside of its original schema. This class may be declared incorrectly.</rdfs:comment>
   </owl:Class>
   <owl:Class rdf:about="#Railway">
      <rdfs:subClassOf rdf:resource="#TransportationComplex"/>
      <rdfs:subClassOf rdf:resource="#RailwayType"/>
   </owl:Class>
   <owl:Class rdf:about="#_GenericApplicationPropertyOfRailway">
      <rdfs:subClassOf rdf:resource="http://www.w3.org/2001/XMLSchema#anyType"/>
      <rdfs:comment>Warning: This class type was declared outside of its original schema. This class may be declared incorrectly.</rdfs:comment>
   </owl:Class>
   <owl:Class rdf:about="#Square">
      <rdfs:subClassOf rdf:resource="#TransportationComplex"/>
      <rdfs:subClassOf rdf:resource="#SquareType"/>
   </owl:Class>
   <owl:Class rdf:about="#_GenericApplicationPropertyOfSquare">
      <rdfs:subClassOf rdf:resource="http://www.w3.org/2001/XMLSchema#anyType"/>
      <rdfs:comment>Warning: This class type was declared outside of its original schema. This class may be declared incorrectly.</rdfs:comment>
   </owl:Class>
   <owl:ObjectProperty rdf:about="#has_GenericApplicationPropertyOfTransportationObject">
      <rdfs:domain rdf:resource="#AbstractTransportationObjectType"/>
      <rdfs:range rdf:resource="#_GenericApplicationPropertyOfTransportationObject"/>
   </owl:ObjectProperty>
   <owl:ObjectProperty rdf:about="#class">
      <rdfs:comment>Warning: This ObjectProperty type was declared outside of its original schema. This ObjectProperty may be declared incorrectly.</rdfs:comment>
      <rdfs:domain rdf:resource="#TransportationComplexType"/>
      <rdfs:range rdf:resource="http://www.opengis.net/gml#CodeType"/>
   </owl:ObjectProperty>
   <owl:ObjectProperty rdf:about="#function">
      <rdfs:comment>Warning: This ObjectProperty type was declared outside of its original schema. This ObjectProperty may be declared incorrectly.</rdfs:comment>
      <rdfs:domain rdf:resource="#TransportationComplexType"/>
      <rdfs:range rdf:resource="http://www.opengis.net/gml#CodeType"/>
   </owl:ObjectProperty>
   <owl:ObjectProperty rdf:about="#usage">
      <rdfs:comment>Warning: This ObjectProperty type was declared outside of its original schema. This ObjectProperty may be declared incorrectly.</rdfs:comment>
      <rdfs:domain rdf:resource="#TransportationComplexType"/>
      <rdfs:range rdf:resource="http://www.opengis.net/gml#CodeType"/>
   </owl:ObjectProperty>
   <owl:ObjectProperty rdf:about="#trafficArea">
      <rdfs:domain rdf:resource="#TransportationComplexType"/>
      <rdfs:range rdf:resource="#TrafficAreaPropertyType"/>
   </owl:ObjectProperty>
   <owl:ObjectProperty rdf:about="#auxiliaryTrafficArea">
      <rdfs:domain rdf:resource="#TransportationComplexType"/>
      <rdfs:range rdf:resource="#AuxiliaryTrafficAreaPropertyType"/>
   </owl:ObjectProperty>
   <owl:ObjectProperty rdf:about="#lod0Network">
      <rdfs:comment>Warning: This ObjectProperty type was declared outside of its original schema. This ObjectProperty may be declared incorrectly.</rdfs:comment>
      <rdfs:domain rdf:resource="#TransportationComplexType"/>
      <rdfs:range rdf:resource="http://www.opengis.net/gml#GeometricComplexPropertyType"/>
   </owl:ObjectProperty>
   <owl:ObjectProperty rdf:about="#lod1MultiSurface">
      <rdfs:comment>Warning: This ObjectProperty type was declared outside of its original schema. This ObjectProperty may be declared incorrectly.</rdfs:comment>
      <rdfs:domain rdf:resource="#TransportationComplexType"/>
      <rdfs:range rdf:resource="http://www.opengis.net/gml#MultiSurfacePropertyType"/>
   </owl:ObjectProperty>
   <owl:ObjectProperty rdf:about="#lod2MultiSurface">
      <rdfs:comment>Warning: This ObjectProperty type was declared outside of its original schema. This ObjectProperty may be declared incorrectly.</rdfs:comment>
      <rdfs:domain rdf:resource="#TransportationComplexType"/>
      <rdfs:range rdf:resource="http://www.opengis.net/gml#MultiSurfacePropertyType"/>
   </owl:ObjectProperty>
   <owl:ObjectProperty rdf:about="#lod3MultiSurface">
      <rdfs:comment>Warning: This ObjectProperty type was declared outside of its original schema. This ObjectProperty may be declared incorrectly.</rdfs:comment>
      <rdfs:domain rdf:resource="#TransportationComplexType"/>
      <rdfs:range rdf:resource="http://www.opengis.net/gml#MultiSurfacePropertyType"/>
   </owl:ObjectProperty>
   <owl:ObjectProperty rdf:about="#lod4MultiSurface">
      <rdfs:comment>Warning: This ObjectProperty type was declared outside of its original schema. This ObjectProperty may be declared incorrectly.</rdfs:comment>
      <rdfs:domain rdf:resource="#TransportationComplexType"/>
      <rdfs:range rdf:resource="http://www.opengis.net/gml#MultiSurfacePropertyType"/>
   </owl:ObjectProperty>
   <owl:ObjectProperty rdf:about="#has_GenericApplicationPropertyOfTransportationComplex">
      <rdfs:domain rdf:resource="#TransportationComplexType"/>
      <rdfs:range rdf:resource="#_GenericApplicationPropertyOfTransportationComplex"/>
   </owl:ObjectProperty>
   <owl:ObjectProperty rdf:about="#class">
      <rdfs:comment>Warning: This ObjectProperty type was declared outside of its original schema. This ObjectProperty may be declared incorrectly.</rdfs:comment>
      <rdfs:domain rdf:resource="#TrafficAreaType"/>
      <rdfs:range rdf:resource="http://www.opengis.net/gml#CodeType"/>
   </owl:ObjectProperty>
   <owl:ObjectProperty rdf:about="#function">
      <rdfs:comment>Warning: This ObjectProperty type was declared outside of its original schema. This ObjectProperty may be declared incorrectly.</rdfs:comment>
      <rdfs:domain rdf:resource="#TrafficAreaType"/>
      <rdfs:range rdf:resource="http://www.opengis.net/gml#CodeType"/>
   </owl:ObjectProperty>
   <owl:ObjectProperty rdf:about="#usage">
      <rdfs:comment>Warning: This ObjectProperty type was declared outside of its original schema. This ObjectProperty may be declared incorrectly.</rdfs:comment>
      <rdfs:domain rdf:resource="#TrafficAreaType"/>
      <rdfs:range rdf:resource="http://www.opengis.net/gml#CodeType"/>
   </owl:ObjectProperty>
   <owl:ObjectProperty rdf:about="#surfaceMaterial">
      <rdfs:comment>Warning: This ObjectProperty type was declared outside of its original schema. This ObjectProperty may be declared incorrectly.</rdfs:comment>
      <rdfs:domain rdf:resource="#TrafficAreaType"/>
      <rdfs:range rdf:resource="http://www.opengis.net/gml#CodeType"/>
   </owl:ObjectProperty>
   <owl:ObjectProperty rdf:about="#lod2MultiSurface">
      <rdfs:comment>Warning: This ObjectProperty type was declared outside of its original schema. This ObjectProperty may be declared incorrectly.</rdfs:comment>
      <rdfs:domain rdf:resource="#TrafficAreaType"/>
      <rdfs:range rdf:resource="http://www.opengis.net/gml#MultiSurfacePropertyType"/>
   </owl:ObjectProperty>
   <owl:ObjectProperty rdf:about="#lod3MultiSurface">
      <rdfs:comment>Warning: This ObjectProperty type was declared outside of its original schema. This ObjectProperty may be declared incorrectly.</rdfs:comment>
      <rdfs:domain rdf:resource="#TrafficAreaType"/>
      <rdfs:range rdf:resource="http://www.opengis.net/gml#MultiSurfacePropertyType"/>
   </owl:ObjectProperty>
   <owl:ObjectProperty rdf:about="#lod4MultiSurface">
      <rdfs:comment>Warning: This ObjectProperty type was declared outside of its original schema. This ObjectProperty may be declared incorrectly.</rdfs:comment>
      <rdfs:domain rdf:resource="#TrafficAreaType"/>
      <rdfs:range rdf:resource="http://www.opengis.net/gml#MultiSurfacePropertyType"/>
   </owl:ObjectProperty>
   <owl:ObjectProperty rdf:about="#has_GenericApplicationPropertyOfTrafficArea">
      <rdfs:domain rdf:resource="#TrafficAreaType"/>
      <rdfs:range rdf:resource="#_GenericApplicationPropertyOfTrafficArea"/>
   </owl:ObjectProperty>
   <owl:ObjectProperty rdf:about="#class">
      <rdfs:comment>Warning: This ObjectProperty type was declared outside of its original schema. This ObjectProperty may be declared incorrectly.</rdfs:comment>
      <rdfs:domain rdf:resource="#AuxiliaryTrafficAreaType"/>
      <rdfs:range rdf:resource="http://www.opengis.net/gml#CodeType"/>
   </owl:ObjectProperty>
   <owl:ObjectProperty rdf:about="#function">
      <rdfs:comment>Warning: This ObjectProperty type was declared outside of its original schema. This ObjectProperty may be declared incorrectly.</rdfs:comment>
      <rdfs:domain rdf:resource="#AuxiliaryTrafficAreaType"/>
      <rdfs:range rdf:resource="http://www.opengis.net/gml#CodeType"/>
   </owl:ObjectProperty>
   <owl:ObjectProperty rdf:about="#usage">
      <rdfs:comment>Warning: This ObjectProperty type was declared outside of its original schema. This ObjectProperty may be declared incorrectly.</rdfs:comment>
      <rdfs:domain rdf:resource="#AuxiliaryTrafficAreaType"/>
      <rdfs:range rdf:resource="http://www.opengis.net/gml#CodeType"/>
   </owl:ObjectProperty>
   <owl:ObjectProperty rdf:about="#surfaceMaterial">
      <rdfs:comment>Warning: This ObjectProperty type was declared outside of its original schema. This ObjectProperty may be declared incorrectly.</rdfs:comment>
      <rdfs:domain rdf:resource="#AuxiliaryTrafficAreaType"/>
      <rdfs:range rdf:resource="http://www.opengis.net/gml#CodeType"/>
   </owl:ObjectProperty>
   <owl:ObjectProperty rdf:about="#lod2MultiSurface">
      <rdfs:comment>Warning: This ObjectProperty type was declared outside of its original schema. This ObjectProperty may be declared incorrectly.</rdfs:comment>
      <rdfs:domain rdf:resource="#AuxiliaryTrafficAreaType"/>
      <rdfs:range rdf:resource="http://www.opengis.net/gml#MultiSurfacePropertyType"/>
   </owl:ObjectProperty>
   <owl:ObjectProperty rdf:about="#lod3MultiSurface">
      <rdfs:comment>Warning: This ObjectProperty type was declared outside of its original schema. This ObjectProperty may be declared incorrectly.</rdfs:comment>
      <rdfs:domain rdf:resource="#AuxiliaryTrafficAreaType"/>
      <rdfs:range rdf:resource="http://www.opengis.net/gml#MultiSurfacePropertyType"/>
   </owl:ObjectProperty>
   <owl:ObjectProperty rdf:about="#lod4MultiSurface">
      <rdfs:comment>Warning: This ObjectProperty type was declared outside of its original schema. This ObjectProperty may be declared incorrectly.</rdfs:comment>
      <rdfs:domain rdf:resource="#AuxiliaryTrafficAreaType"/>
      <rdfs:range rdf:resource="http://www.opengis.net/gml#MultiSurfacePropertyType"/>
   </owl:ObjectProperty>
   <owl:ObjectProperty rdf:about="#has_GenericApplicationPropertyOfAuxiliaryTrafficArea">
      <rdfs:domain rdf:resource="#AuxiliaryTrafficAreaType"/>
      <rdfs:range rdf:resource="#_GenericApplicationPropertyOfAuxiliaryTrafficArea"/>
   </owl:ObjectProperty>
   <owl:ObjectProperty rdf:about="#hasTrafficArea">
      <rdfs:domain rdf:resource="#TrafficAreaPropertyType"/>
      <rdfs:range rdf:resource="#TrafficArea"/>
   </owl:ObjectProperty>
   <owl:ObjectProperty rdf:about="#hasAuxiliaryTrafficArea">
      <rdfs:domain rdf:resource="#AuxiliaryTrafficAreaPropertyType"/>
      <rdfs:range rdf:resource="#AuxiliaryTrafficArea"/>
   </owl:ObjectProperty>
   <owl:ObjectProperty rdf:about="#has_GenericApplicationPropertyOfTrack">
      <rdfs:domain rdf:resource="#TrackType"/>
      <rdfs:range rdf:resource="#_GenericApplicationPropertyOfTrack"/>
   </owl:ObjectProperty>
   <owl:ObjectProperty rdf:about="#has_GenericApplicationPropertyOfRoad">
      <rdfs:domain rdf:resource="#RoadType"/>
      <rdfs:range rdf:resource="#_GenericApplicationPropertyOfRoad"/>
   </owl:ObjectProperty>
   <owl:ObjectProperty rdf:about="#has_GenericApplicationPropertyOfRailway">
      <rdfs:domain rdf:resource="#RailwayType"/>
      <rdfs:range rdf:resource="#_GenericApplicationPropertyOfRailway"/>
   </owl:ObjectProperty>
   <owl:ObjectProperty rdf:about="#has_GenericApplicationPropertyOfSquare">
      <rdfs:domain rdf:resource="#SquareType"/>
      <rdfs:range rdf:resource="#_GenericApplicationPropertyOfSquare"/>
   </owl:ObjectProperty>
</rdf:RDF>
