<?xml version="1.0" encoding="UTF-8"?>
<rdf:RDF xmlns:math="http://www.w3.org/2005/xpath-functions/math"
         xmlns:owl="http://www.w3.org/2002/07/owl#"
         xmlns:rdf="http://www.w3.org/1999/02/22-rdf-syntax-ns#"
         xmlns:rdfs="http://www.w3.org/2000/01/rdf-schema#"
         xmlns:xs="http://www.w3.org/2001/XMLSchema"
         xmlns:xsd="http://www.w3.org/2001/XMLSchema">
   <owl:Ontology rdf:about="http://liris.cnrs.fr/ontologies/transportation">
      <owl:imports rdf:resource="http://liris.cnrs.fr/ontologies/gml"/>
      <owl:imports rdf:resource="http://liris.cnrs.fr/ontologies/cityGMLBase"/>
      <rdfs:comment>
	CityGML is an OGC Standard.
	Copyright (c) 2012 Open Geospatial Consortium.
	To obtain additional rights of use, visit http://www.opengeospatial.org/legal/ .
		</rdfs:comment>
   </owl:Ontology>
   <owl:Class rdf:about="http://www.opengis.net/citygml/transportation/2.0#AbstractTransportationObjectType">
      <rdfs:comment>This is an abstract class</rdfs:comment>
      <rdfs:comment>Type describing the abstract superclass for transportation objects. </rdfs:comment>
      <owl:equivalentClass>
         <owl:Class>
            <owl:intersectionOf rdf:parseType="Collection">
               <owl:Restriction>
                  <owl:onProperty rdf:resource="http://www.opengis.net/citygml/transportation/2.0#has_GenericApplicationPropertyOfTransportationObject"/>
                  <owl:allValuesFrom rdf:resource="http://www.opengis.net/citygml/transportation/2.0#_GenericApplicationPropertyOfTransportationObject"/>
               </owl:Restriction>
               <owl:Restriction>
                  <owl:onProperty rdf:resource="http://www.opengis.net/citygml/transportation/2.0#has_GenericApplicationPropertyOfTransportationObject"/>
                  <owl:minCardinality rdf:datatype="http://www.w3.org/2001/XMLSchema#nonNegativeInteger">0</owl:minCardinality>
               </owl:Restriction>
            </owl:intersectionOf>
         </owl:Class>
      </owl:equivalentClass>
      <rdfs:subClassOf rdf:resource="http://www.opengis.net/citygml/2.0#AbstractCityObjectType"/>
      <rdfs:comment>Warning: The parent class 'core:AbstractCityObjectType' is declared outside of this class' original schema. This class may be declared incorrectly.</rdfs:comment>
   </owl:Class>
   <owl:Class rdf:about="http://www.opengis.net/citygml/transportation/2.0#TransportationComplexType">
      <rdfs:comment>Type describing transportation complexes, which are aggregated features, e.g. roads, which consist of
				parts (traffic areas, e.g. pedestrian path, and auxiliary traffic areas). As subclass of _CityObject, a
				TransportationComplex inherits all attributes and relations, in particular an id, names, external references, and
				generalization relations. </rdfs:comment>
      <owl:equivalentClass>
         <owl:Class>
            <owl:intersectionOf rdf:parseType="Collection">
               <owl:Restriction>
                  <owl:onProperty rdf:resource="http://www.opengis.net/citygml/transportation/2.0#class"/>
                  <owl:allValuesFrom rdf:resource="http://www.opengis.net/gml#CodeType"/>
               </owl:Restriction>
               <owl:Restriction>
                  <owl:onProperty rdf:resource="http://www.opengis.net/citygml/transportation/2.0#class"/>
                  <owl:minCardinality rdf:datatype="http://www.w3.org/2001/XMLSchema#nonNegativeInteger">0</owl:minCardinality>
               </owl:Restriction>
               <owl:Restriction>
                  <owl:onProperty rdf:resource="http://www.opengis.net/citygml/transportation/2.0#function"/>
                  <owl:allValuesFrom rdf:resource="http://www.opengis.net/gml#CodeType"/>
               </owl:Restriction>
               <owl:Restriction>
                  <owl:onProperty rdf:resource="http://www.opengis.net/citygml/transportation/2.0#function"/>
                  <owl:minCardinality rdf:datatype="http://www.w3.org/2001/XMLSchema#nonNegativeInteger">0</owl:minCardinality>
               </owl:Restriction>
               <owl:Restriction>
                  <owl:onProperty rdf:resource="http://www.opengis.net/citygml/transportation/2.0#usage"/>
                  <owl:allValuesFrom rdf:resource="http://www.opengis.net/gml#CodeType"/>
               </owl:Restriction>
               <owl:Restriction>
                  <owl:onProperty rdf:resource="http://www.opengis.net/citygml/transportation/2.0#usage"/>
                  <owl:minCardinality rdf:datatype="http://www.w3.org/2001/XMLSchema#nonNegativeInteger">0</owl:minCardinality>
               </owl:Restriction>
               <owl:Restriction>
                  <owl:onProperty rdf:resource="http://www.opengis.net/citygml/transportation/2.0#trafficArea"/>
                  <owl:allValuesFrom rdf:resource="http://www.opengis.net/citygml/transportation/2.0#TrafficAreaPropertyType"/>
               </owl:Restriction>
               <owl:Restriction>
                  <owl:onProperty rdf:resource="http://www.opengis.net/citygml/transportation/2.0#trafficArea"/>
                  <owl:minCardinality rdf:datatype="http://www.w3.org/2001/XMLSchema#nonNegativeInteger">0</owl:minCardinality>
               </owl:Restriction>
               <owl:Restriction>
                  <owl:onProperty rdf:resource="http://www.opengis.net/citygml/transportation/2.0#auxiliaryTrafficArea"/>
                  <owl:allValuesFrom rdf:resource="http://www.opengis.net/citygml/transportation/2.0#AuxiliaryTrafficAreaPropertyType"/>
               </owl:Restriction>
               <owl:Restriction>
                  <owl:onProperty rdf:resource="http://www.opengis.net/citygml/transportation/2.0#auxiliaryTrafficArea"/>
                  <owl:minCardinality rdf:datatype="http://www.w3.org/2001/XMLSchema#nonNegativeInteger">0</owl:minCardinality>
               </owl:Restriction>
               <owl:Restriction>
                  <owl:onProperty rdf:resource="http://www.opengis.net/citygml/transportation/2.0#lod0Network"/>
                  <owl:allValuesFrom rdf:resource="http://www.opengis.net/gml#GeometricComplexPropertyType"/>
               </owl:Restriction>
               <owl:Restriction>
                  <owl:onProperty rdf:resource="http://www.opengis.net/citygml/transportation/2.0#lod0Network"/>
                  <owl:minCardinality rdf:datatype="http://www.w3.org/2001/XMLSchema#nonNegativeInteger">0</owl:minCardinality>
               </owl:Restriction>
               <owl:Restriction>
                  <owl:onProperty rdf:resource="http://www.opengis.net/citygml/transportation/2.0#lod1MultiSurface"/>
                  <owl:allValuesFrom rdf:resource="http://www.opengis.net/gml#MultiSurfacePropertyType"/>
               </owl:Restriction>
               <owl:Restriction>
                  <owl:onProperty rdf:resource="http://www.opengis.net/citygml/transportation/2.0#lod1MultiSurface"/>
                  <owl:minCardinality rdf:datatype="http://www.w3.org/2001/XMLSchema#nonNegativeInteger">0</owl:minCardinality>
               </owl:Restriction>
               <owl:Restriction>
                  <owl:onProperty rdf:resource="http://www.opengis.net/citygml/transportation/2.0#lod2MultiSurface"/>
                  <owl:allValuesFrom rdf:resource="http://www.opengis.net/gml#MultiSurfacePropertyType"/>
               </owl:Restriction>
               <owl:Restriction>
                  <owl:onProperty rdf:resource="http://www.opengis.net/citygml/transportation/2.0#lod2MultiSurface"/>
                  <owl:minCardinality rdf:datatype="http://www.w3.org/2001/XMLSchema#nonNegativeInteger">0</owl:minCardinality>
               </owl:Restriction>
               <owl:Restriction>
                  <owl:onProperty rdf:resource="http://www.opengis.net/citygml/transportation/2.0#lod3MultiSurface"/>
                  <owl:allValuesFrom rdf:resource="http://www.opengis.net/gml#MultiSurfacePropertyType"/>
               </owl:Restriction>
               <owl:Restriction>
                  <owl:onProperty rdf:resource="http://www.opengis.net/citygml/transportation/2.0#lod3MultiSurface"/>
                  <owl:minCardinality rdf:datatype="http://www.w3.org/2001/XMLSchema#nonNegativeInteger">0</owl:minCardinality>
               </owl:Restriction>
               <owl:Restriction>
                  <owl:onProperty rdf:resource="http://www.opengis.net/citygml/transportation/2.0#lod4MultiSurface"/>
                  <owl:allValuesFrom rdf:resource="http://www.opengis.net/gml#MultiSurfacePropertyType"/>
               </owl:Restriction>
               <owl:Restriction>
                  <owl:onProperty rdf:resource="http://www.opengis.net/citygml/transportation/2.0#lod4MultiSurface"/>
                  <owl:minCardinality rdf:datatype="http://www.w3.org/2001/XMLSchema#nonNegativeInteger">0</owl:minCardinality>
               </owl:Restriction>
               <owl:Restriction>
                  <owl:onProperty rdf:resource="http://www.opengis.net/citygml/transportation/2.0#has_GenericApplicationPropertyOfTransportationComplex"/>
                  <owl:allValuesFrom rdf:resource="http://www.opengis.net/citygml/transportation/2.0#_GenericApplicationPropertyOfTransportationComplex"/>
               </owl:Restriction>
               <owl:Restriction>
                  <owl:onProperty rdf:resource="http://www.opengis.net/citygml/transportation/2.0#has_GenericApplicationPropertyOfTransportationComplex"/>
                  <owl:minCardinality rdf:datatype="http://www.w3.org/2001/XMLSchema#nonNegativeInteger">0</owl:minCardinality>
               </owl:Restriction>
            </owl:intersectionOf>
         </owl:Class>
      </owl:equivalentClass>
   </owl:Class>
   <owl:Class rdf:about="http://www.opengis.net/citygml/transportation/2.0#TrafficAreaType">
      <rdfs:comment>Type describing the class for traffic Areas. Traffic areas are the surfaces where traffic actually takes
				place. As subclass of _CityObject, a TrafficArea inherits all attributes and relations, in particular an id, names,
				external references, and generalization relations. </rdfs:comment>
      <owl:equivalentClass>
         <owl:Class>
            <owl:intersectionOf rdf:parseType="Collection">
               <owl:Restriction>
                  <owl:onProperty rdf:resource="http://www.opengis.net/citygml/transportation/2.0#class"/>
                  <owl:allValuesFrom rdf:resource="http://www.opengis.net/gml#CodeType"/>
               </owl:Restriction>
               <owl:Restriction>
                  <owl:onProperty rdf:resource="http://www.opengis.net/citygml/transportation/2.0#class"/>
                  <owl:minCardinality rdf:datatype="http://www.w3.org/2001/XMLSchema#nonNegativeInteger">0</owl:minCardinality>
               </owl:Restriction>
               <owl:Restriction>
                  <owl:onProperty rdf:resource="http://www.opengis.net/citygml/transportation/2.0#function"/>
                  <owl:allValuesFrom rdf:resource="http://www.opengis.net/gml#CodeType"/>
               </owl:Restriction>
               <owl:Restriction>
                  <owl:onProperty rdf:resource="http://www.opengis.net/citygml/transportation/2.0#function"/>
                  <owl:minCardinality rdf:datatype="http://www.w3.org/2001/XMLSchema#nonNegativeInteger">0</owl:minCardinality>
               </owl:Restriction>
               <owl:Restriction>
                  <owl:onProperty rdf:resource="http://www.opengis.net/citygml/transportation/2.0#usage"/>
                  <owl:allValuesFrom rdf:resource="http://www.opengis.net/gml#CodeType"/>
               </owl:Restriction>
               <owl:Restriction>
                  <owl:onProperty rdf:resource="http://www.opengis.net/citygml/transportation/2.0#usage"/>
                  <owl:minCardinality rdf:datatype="http://www.w3.org/2001/XMLSchema#nonNegativeInteger">0</owl:minCardinality>
               </owl:Restriction>
               <owl:Restriction>
                  <owl:onProperty rdf:resource="http://www.opengis.net/citygml/transportation/2.0#surfaceMaterial"/>
                  <owl:allValuesFrom rdf:resource="http://www.opengis.net/gml#CodeType"/>
               </owl:Restriction>
               <owl:Restriction>
                  <owl:onProperty rdf:resource="http://www.opengis.net/citygml/transportation/2.0#surfaceMaterial"/>
                  <owl:minCardinality rdf:datatype="http://www.w3.org/2001/XMLSchema#nonNegativeInteger">0</owl:minCardinality>
               </owl:Restriction>
               <owl:Restriction>
                  <owl:onProperty rdf:resource="http://www.opengis.net/citygml/transportation/2.0#lod2MultiSurface"/>
                  <owl:allValuesFrom rdf:resource="http://www.opengis.net/gml#MultiSurfacePropertyType"/>
               </owl:Restriction>
               <owl:Restriction>
                  <owl:onProperty rdf:resource="http://www.opengis.net/citygml/transportation/2.0#lod2MultiSurface"/>
                  <owl:minCardinality rdf:datatype="http://www.w3.org/2001/XMLSchema#nonNegativeInteger">0</owl:minCardinality>
               </owl:Restriction>
               <owl:Restriction>
                  <owl:onProperty rdf:resource="http://www.opengis.net/citygml/transportation/2.0#lod3MultiSurface"/>
                  <owl:allValuesFrom rdf:resource="http://www.opengis.net/gml#MultiSurfacePropertyType"/>
               </owl:Restriction>
               <owl:Restriction>
                  <owl:onProperty rdf:resource="http://www.opengis.net/citygml/transportation/2.0#lod3MultiSurface"/>
                  <owl:minCardinality rdf:datatype="http://www.w3.org/2001/XMLSchema#nonNegativeInteger">0</owl:minCardinality>
               </owl:Restriction>
               <owl:Restriction>
                  <owl:onProperty rdf:resource="http://www.opengis.net/citygml/transportation/2.0#lod4MultiSurface"/>
                  <owl:allValuesFrom rdf:resource="http://www.opengis.net/gml#MultiSurfacePropertyType"/>
               </owl:Restriction>
               <owl:Restriction>
                  <owl:onProperty rdf:resource="http://www.opengis.net/citygml/transportation/2.0#lod4MultiSurface"/>
                  <owl:minCardinality rdf:datatype="http://www.w3.org/2001/XMLSchema#nonNegativeInteger">0</owl:minCardinality>
               </owl:Restriction>
               <owl:Restriction>
                  <owl:onProperty rdf:resource="http://www.opengis.net/citygml/transportation/2.0#has_GenericApplicationPropertyOfTrafficArea"/>
                  <owl:allValuesFrom rdf:resource="http://www.opengis.net/citygml/transportation/2.0#_GenericApplicationPropertyOfTrafficArea"/>
               </owl:Restriction>
               <owl:Restriction>
                  <owl:onProperty rdf:resource="http://www.opengis.net/citygml/transportation/2.0#has_GenericApplicationPropertyOfTrafficArea"/>
                  <owl:minCardinality rdf:datatype="http://www.w3.org/2001/XMLSchema#nonNegativeInteger">0</owl:minCardinality>
               </owl:Restriction>
            </owl:intersectionOf>
         </owl:Class>
      </owl:equivalentClass>
   </owl:Class>
   <owl:Class rdf:about="http://www.opengis.net/citygml/transportation/2.0#AuxiliaryTrafficAreaType">
      <rdfs:comment>Type describing the class for auxiliary traffic Areas. These are the surfaces where no traffic actually
				takes place, but which belong to a transportation object. Examples are kerbstones, road markings and grass stripes. As
				subclass of _CityObject, an AuxiliaryTrafficArea inherits all attributes and relations, in particular an id, names,
				external references, and generalization relations. </rdfs:comment>
      <owl:equivalentClass>
         <owl:Class>
            <owl:intersectionOf rdf:parseType="Collection">
               <owl:Restriction>
                  <owl:onProperty rdf:resource="http://www.opengis.net/citygml/transportation/2.0#class"/>
                  <owl:allValuesFrom rdf:resource="http://www.opengis.net/gml#CodeType"/>
               </owl:Restriction>
               <owl:Restriction>
                  <owl:onProperty rdf:resource="http://www.opengis.net/citygml/transportation/2.0#class"/>
                  <owl:minCardinality rdf:datatype="http://www.w3.org/2001/XMLSchema#nonNegativeInteger">0</owl:minCardinality>
               </owl:Restriction>
               <owl:Restriction>
                  <owl:onProperty rdf:resource="http://www.opengis.net/citygml/transportation/2.0#function"/>
                  <owl:allValuesFrom rdf:resource="http://www.opengis.net/gml#CodeType"/>
               </owl:Restriction>
               <owl:Restriction>
                  <owl:onProperty rdf:resource="http://www.opengis.net/citygml/transportation/2.0#function"/>
                  <owl:minCardinality rdf:datatype="http://www.w3.org/2001/XMLSchema#nonNegativeInteger">0</owl:minCardinality>
               </owl:Restriction>
               <owl:Restriction>
                  <owl:onProperty rdf:resource="http://www.opengis.net/citygml/transportation/2.0#usage"/>
                  <owl:allValuesFrom rdf:resource="http://www.opengis.net/gml#CodeType"/>
               </owl:Restriction>
               <owl:Restriction>
                  <owl:onProperty rdf:resource="http://www.opengis.net/citygml/transportation/2.0#usage"/>
                  <owl:minCardinality rdf:datatype="http://www.w3.org/2001/XMLSchema#nonNegativeInteger">0</owl:minCardinality>
               </owl:Restriction>
               <owl:Restriction>
                  <owl:onProperty rdf:resource="http://www.opengis.net/citygml/transportation/2.0#surfaceMaterial"/>
                  <owl:allValuesFrom rdf:resource="http://www.opengis.net/gml#CodeType"/>
               </owl:Restriction>
               <owl:Restriction>
                  <owl:onProperty rdf:resource="http://www.opengis.net/citygml/transportation/2.0#surfaceMaterial"/>
                  <owl:minCardinality rdf:datatype="http://www.w3.org/2001/XMLSchema#nonNegativeInteger">0</owl:minCardinality>
               </owl:Restriction>
               <owl:Restriction>
                  <owl:onProperty rdf:resource="http://www.opengis.net/citygml/transportation/2.0#lod2MultiSurface"/>
                  <owl:allValuesFrom rdf:resource="http://www.opengis.net/gml#MultiSurfacePropertyType"/>
               </owl:Restriction>
               <owl:Restriction>
                  <owl:onProperty rdf:resource="http://www.opengis.net/citygml/transportation/2.0#lod2MultiSurface"/>
                  <owl:minCardinality rdf:datatype="http://www.w3.org/2001/XMLSchema#nonNegativeInteger">0</owl:minCardinality>
               </owl:Restriction>
               <owl:Restriction>
                  <owl:onProperty rdf:resource="http://www.opengis.net/citygml/transportation/2.0#lod3MultiSurface"/>
                  <owl:allValuesFrom rdf:resource="http://www.opengis.net/gml#MultiSurfacePropertyType"/>
               </owl:Restriction>
               <owl:Restriction>
                  <owl:onProperty rdf:resource="http://www.opengis.net/citygml/transportation/2.0#lod3MultiSurface"/>
                  <owl:minCardinality rdf:datatype="http://www.w3.org/2001/XMLSchema#nonNegativeInteger">0</owl:minCardinality>
               </owl:Restriction>
               <owl:Restriction>
                  <owl:onProperty rdf:resource="http://www.opengis.net/citygml/transportation/2.0#lod4MultiSurface"/>
                  <owl:allValuesFrom rdf:resource="http://www.opengis.net/gml#MultiSurfacePropertyType"/>
               </owl:Restriction>
               <owl:Restriction>
                  <owl:onProperty rdf:resource="http://www.opengis.net/citygml/transportation/2.0#lod4MultiSurface"/>
                  <owl:minCardinality rdf:datatype="http://www.w3.org/2001/XMLSchema#nonNegativeInteger">0</owl:minCardinality>
               </owl:Restriction>
               <owl:Restriction>
                  <owl:onProperty rdf:resource="http://www.opengis.net/citygml/transportation/2.0#has_GenericApplicationPropertyOfAuxiliaryTrafficArea"/>
                  <owl:allValuesFrom rdf:resource="http://www.opengis.net/citygml/transportation/2.0#_GenericApplicationPropertyOfAuxiliaryTrafficArea"/>
               </owl:Restriction>
               <owl:Restriction>
                  <owl:onProperty rdf:resource="http://www.opengis.net/citygml/transportation/2.0#has_GenericApplicationPropertyOfAuxiliaryTrafficArea"/>
                  <owl:minCardinality rdf:datatype="http://www.w3.org/2001/XMLSchema#nonNegativeInteger">0</owl:minCardinality>
               </owl:Restriction>
            </owl:intersectionOf>
         </owl:Class>
      </owl:equivalentClass>
   </owl:Class>
   <owl:Class rdf:about="http://www.opengis.net/citygml/transportation/2.0#TrafficAreaPropertyType">
      <rdfs:comment>Denotes the relation of TransportationComplex to its parts, which are traffic areas. The
				TrafficAreaPropertyType element must either carry a reference to a TrafficArea object or contain a TrafficArea object
				inline, but neither both nor none. </rdfs:comment>
      <owl:equivalentClass>
         <owl:Class>
            <owl:intersectionOf rdf:parseType="Collection">
               <owl:Restriction>
                  <owl:onProperty rdf:resource="http://www.opengis.net/citygml/transportation/2.0#hasTrafficArea"/>
                  <owl:allValuesFrom rdf:resource="http://www.opengis.net/citygml/transportation/2.0#TrafficArea"/>
               </owl:Restriction>
            </owl:intersectionOf>
         </owl:Class>
      </owl:equivalentClass>
   </owl:Class>
   <owl:Class rdf:about="http://www.opengis.net/citygml/transportation/2.0#AuxiliaryTrafficAreaPropertyType">
      <rdfs:comment>Denotes the relation of TransportationComplex to its parts, which are auxiliary traffic areas. The
				TrafficAreaPropertyType element must either carry a reference to a TrafficArea object or contain a TrafficArea object
				inline, but neither both nor none. </rdfs:comment>
      <owl:equivalentClass>
         <owl:Class>
            <owl:intersectionOf rdf:parseType="Collection">
               <owl:Restriction>
                  <owl:onProperty rdf:resource="http://www.opengis.net/citygml/transportation/2.0#hasAuxiliaryTrafficArea"/>
                  <owl:allValuesFrom rdf:resource="http://www.opengis.net/citygml/transportation/2.0#AuxiliaryTrafficArea"/>
               </owl:Restriction>
            </owl:intersectionOf>
         </owl:Class>
      </owl:equivalentClass>
   </owl:Class>
   <owl:Class rdf:about="http://www.opengis.net/citygml/transportation/2.0#TrackType">
      <rdfs:comment>Type describing the class for tracks. A track is a small path mainly used by pedestrians. As subclass of
				_CityObject, a Track inherits all attributes and relations, in particular an id, names, external references, and
				generalization relations. </rdfs:comment>
      <owl:equivalentClass>
         <owl:Class>
            <owl:intersectionOf rdf:parseType="Collection">
               <owl:Restriction>
                  <owl:onProperty rdf:resource="http://www.opengis.net/citygml/transportation/2.0#has_GenericApplicationPropertyOfTrack"/>
                  <owl:allValuesFrom rdf:resource="http://www.opengis.net/citygml/transportation/2.0#_GenericApplicationPropertyOfTrack"/>
               </owl:Restriction>
               <owl:Restriction>
                  <owl:onProperty rdf:resource="http://www.opengis.net/citygml/transportation/2.0#has_GenericApplicationPropertyOfTrack"/>
                  <owl:minCardinality rdf:datatype="http://www.w3.org/2001/XMLSchema#nonNegativeInteger">0</owl:minCardinality>
               </owl:Restriction>
            </owl:intersectionOf>
         </owl:Class>
      </owl:equivalentClass>
   </owl:Class>
   <owl:Class rdf:about="http://www.opengis.net/citygml/transportation/2.0#RoadType">
      <rdfs:comment>Type describing the class for roads. As subclass of _CityObject, a Road inherits all attributes and
				relations, in particular an id, names, external references, and generalization relations. </rdfs:comment>
      <owl:equivalentClass>
         <owl:Class>
            <owl:intersectionOf rdf:parseType="Collection">
               <owl:Restriction>
                  <owl:onProperty rdf:resource="http://www.opengis.net/citygml/transportation/2.0#has_GenericApplicationPropertyOfRoad"/>
                  <owl:allValuesFrom rdf:resource="http://www.opengis.net/citygml/transportation/2.0#_GenericApplicationPropertyOfRoad"/>
               </owl:Restriction>
               <owl:Restriction>
                  <owl:onProperty rdf:resource="http://www.opengis.net/citygml/transportation/2.0#has_GenericApplicationPropertyOfRoad"/>
                  <owl:minCardinality rdf:datatype="http://www.w3.org/2001/XMLSchema#nonNegativeInteger">0</owl:minCardinality>
               </owl:Restriction>
            </owl:intersectionOf>
         </owl:Class>
      </owl:equivalentClass>
   </owl:Class>
   <owl:Class rdf:about="http://www.opengis.net/citygml/transportation/2.0#RailwayType">
      <rdfs:comment>Type describing the class for railways. As subclass of _CityObject, a Railway inherits all attributes and
				relations, in particular an id, names, external references, and generalization relations. </rdfs:comment>
      <owl:equivalentClass>
         <owl:Class>
            <owl:intersectionOf rdf:parseType="Collection">
               <owl:Restriction>
                  <owl:onProperty rdf:resource="http://www.opengis.net/citygml/transportation/2.0#has_GenericApplicationPropertyOfRailway"/>
                  <owl:allValuesFrom rdf:resource="http://www.opengis.net/citygml/transportation/2.0#_GenericApplicationPropertyOfRailway"/>
               </owl:Restriction>
               <owl:Restriction>
                  <owl:onProperty rdf:resource="http://www.opengis.net/citygml/transportation/2.0#has_GenericApplicationPropertyOfRailway"/>
                  <owl:minCardinality rdf:datatype="http://www.w3.org/2001/XMLSchema#nonNegativeInteger">0</owl:minCardinality>
               </owl:Restriction>
            </owl:intersectionOf>
         </owl:Class>
      </owl:equivalentClass>
   </owl:Class>
   <owl:Class rdf:about="http://www.opengis.net/citygml/transportation/2.0#SquareType">
      <rdfs:comment>Type describing the class for squares. A square is an open area commonly found in cities (like a plaza).
				As subclass of _CityObject, a Square inherits all attributes and relations, in particular an id, names, external
				references, and generalization relations. </rdfs:comment>
      <owl:equivalentClass>
         <owl:Class>
            <owl:intersectionOf rdf:parseType="Collection">
               <owl:Restriction>
                  <owl:onProperty rdf:resource="http://www.opengis.net/citygml/transportation/2.0#has_GenericApplicationPropertyOfSquare"/>
                  <owl:allValuesFrom rdf:resource="http://www.opengis.net/citygml/transportation/2.0#_GenericApplicationPropertyOfSquare"/>
               </owl:Restriction>
               <owl:Restriction>
                  <owl:onProperty rdf:resource="http://www.opengis.net/citygml/transportation/2.0#has_GenericApplicationPropertyOfSquare"/>
                  <owl:minCardinality rdf:datatype="http://www.w3.org/2001/XMLSchema#nonNegativeInteger">0</owl:minCardinality>
               </owl:Restriction>
            </owl:intersectionOf>
         </owl:Class>
      </owl:equivalentClass>
   </owl:Class>
   <owl:ObjectProperty rdf:about="http://www.opengis.net/gml#hasAssociationAttributeGroup">
      <rdfs:domain rdf:resource="http://www.opengis.net/citygml/transportation/2.0#TrafficAreaPropertyType"/>
      <rdfs:range rdf:resource="http://www.opengis.net/gml#AssociationAttributeGroup"/>
   </owl:ObjectProperty>
   <owl:ObjectProperty rdf:about="http://www.opengis.net/gml#hasAssociationAttributeGroup">
      <rdfs:domain rdf:resource="http://www.opengis.net/citygml/transportation/2.0#AuxiliaryTrafficAreaPropertyType"/>
      <rdfs:range rdf:resource="http://www.opengis.net/gml#AssociationAttributeGroup"/>
   </owl:ObjectProperty>
   <owl:Class rdf:about="http://www.opengis.net/citygml/transportation/2.0#_TransportationObject">
      <rdfs:subClassOf rdf:resource="http://www.opengis.net/citygml/2.0#_CityObject"/>
      <rdfs:subClassOf rdf:resource="http://www.opengis.net/citygml/transportation/2.0#AbstractTransportationObjectType"/>
   </owl:Class>
   <owl:Class rdf:about="http://www.opengis.net/citygml/transportation/2.0#_GenericApplicationPropertyOfTransportationObject">
      <rdfs:subClassOf rdf:resource="http://www.w3.org/2001/XMLSchema#anyType"/>
      <rdfs:comment>Warning: This class type was declared outside of its original schema. This class may be declared incorrectly.</rdfs:comment>
   </owl:Class>
   <owl:Class rdf:about="http://www.opengis.net/citygml/transportation/2.0#TransportationComplex">
      <rdfs:subClassOf rdf:resource="http://www.opengis.net/citygml/transportation/2.0#_TransportationObject"/>
      <rdfs:subClassOf rdf:resource="http://www.opengis.net/citygml/transportation/2.0#TransportationComplexType"/>
   </owl:Class>
   <owl:Class rdf:about="http://www.opengis.net/citygml/transportation/2.0#_GenericApplicationPropertyOfTransportationComplex">
      <rdfs:subClassOf rdf:resource="http://www.w3.org/2001/XMLSchema#anyType"/>
      <rdfs:comment>Warning: This class type was declared outside of its original schema. This class may be declared incorrectly.</rdfs:comment>
   </owl:Class>
   <owl:Class rdf:about="http://www.opengis.net/citygml/transportation/2.0#TrafficArea">
      <rdfs:subClassOf rdf:resource="http://www.opengis.net/citygml/transportation/2.0#_TransportationObject"/>
      <rdfs:subClassOf rdf:resource="http://www.opengis.net/citygml/transportation/2.0#TrafficAreaType"/>
   </owl:Class>
   <owl:Class rdf:about="http://www.opengis.net/citygml/transportation/2.0#_GenericApplicationPropertyOfTrafficArea">
      <rdfs:subClassOf rdf:resource="http://www.w3.org/2001/XMLSchema#anyType"/>
      <rdfs:comment>Warning: This class type was declared outside of its original schema. This class may be declared incorrectly.</rdfs:comment>
   </owl:Class>
   <owl:Class rdf:about="http://www.opengis.net/citygml/transportation/2.0#AuxiliaryTrafficArea">
      <rdfs:subClassOf rdf:resource="http://www.opengis.net/citygml/transportation/2.0#_TransportationObject"/>
      <rdfs:subClassOf rdf:resource="http://www.opengis.net/citygml/transportation/2.0#AuxiliaryTrafficAreaType"/>
   </owl:Class>
   <owl:Class rdf:about="http://www.opengis.net/citygml/transportation/2.0#_GenericApplicationPropertyOfAuxiliaryTrafficArea">
      <rdfs:subClassOf rdf:resource="http://www.w3.org/2001/XMLSchema#anyType"/>
      <rdfs:comment>Warning: This class type was declared outside of its original schema. This class may be declared incorrectly.</rdfs:comment>
   </owl:Class>
   <owl:Class rdf:about="http://www.opengis.net/citygml/transportation/2.0#Track">
      <rdfs:subClassOf rdf:resource="http://www.opengis.net/citygml/transportation/2.0#TransportationComplex"/>
      <rdfs:subClassOf rdf:resource="http://www.opengis.net/citygml/transportation/2.0#TrackType"/>
   </owl:Class>
   <owl:Class rdf:about="http://www.opengis.net/citygml/transportation/2.0#_GenericApplicationPropertyOfTrack">
      <rdfs:subClassOf rdf:resource="http://www.w3.org/2001/XMLSchema#anyType"/>
      <rdfs:comment>Warning: This class type was declared outside of its original schema. This class may be declared incorrectly.</rdfs:comment>
   </owl:Class>
   <owl:Class rdf:about="http://www.opengis.net/citygml/transportation/2.0#Road">
      <rdfs:subClassOf rdf:resource="http://www.opengis.net/citygml/transportation/2.0#TransportationComplex"/>
      <rdfs:subClassOf rdf:resource="http://www.opengis.net/citygml/transportation/2.0#RoadType"/>
   </owl:Class>
   <owl:Class rdf:about="http://www.opengis.net/citygml/transportation/2.0#_GenericApplicationPropertyOfRoad">
      <rdfs:subClassOf rdf:resource="http://www.w3.org/2001/XMLSchema#anyType"/>
      <rdfs:comment>Warning: This class type was declared outside of its original schema. This class may be declared incorrectly.</rdfs:comment>
   </owl:Class>
   <owl:Class rdf:about="http://www.opengis.net/citygml/transportation/2.0#Railway">
      <rdfs:subClassOf rdf:resource="http://www.opengis.net/citygml/transportation/2.0#TransportationComplex"/>
      <rdfs:subClassOf rdf:resource="http://www.opengis.net/citygml/transportation/2.0#RailwayType"/>
   </owl:Class>
   <owl:Class rdf:about="http://www.opengis.net/citygml/transportation/2.0#_GenericApplicationPropertyOfRailway">
      <rdfs:subClassOf rdf:resource="http://www.w3.org/2001/XMLSchema#anyType"/>
      <rdfs:comment>Warning: This class type was declared outside of its original schema. This class may be declared incorrectly.</rdfs:comment>
   </owl:Class>
   <owl:Class rdf:about="http://www.opengis.net/citygml/transportation/2.0#Square">
      <rdfs:subClassOf rdf:resource="http://www.opengis.net/citygml/transportation/2.0#TransportationComplex"/>
      <rdfs:subClassOf rdf:resource="http://www.opengis.net/citygml/transportation/2.0#SquareType"/>
   </owl:Class>
   <owl:Class rdf:about="http://www.opengis.net/citygml/transportation/2.0#_GenericApplicationPropertyOfSquare">
      <rdfs:subClassOf rdf:resource="http://www.w3.org/2001/XMLSchema#anyType"/>
      <rdfs:comment>Warning: This class type was declared outside of its original schema. This class may be declared incorrectly.</rdfs:comment>
   </owl:Class>
   <owl:ObjectProperty rdf:about="http://www.opengis.net/citygml/transportation/2.0#has_GenericApplicationPropertyOfTransportationObject">
      <rdfs:domain rdf:resource="http://www.opengis.net/citygml/transportation/2.0#AbstractTransportationObjectType"/>
      <rdfs:range rdf:resource="http://www.opengis.net/citygml/transportation/2.0#_GenericApplicationPropertyOfTransportationObject"/>
   </owl:ObjectProperty>
   <owl:ObjectProperty rdf:about="http://www.opengis.net/citygml/transportation/2.0#class">
      <rdfs:comment>Warning: This ObjectProperty type was declared outside of its original schema. This ObjectProperty may be declared incorrectly.</rdfs:comment>
      <rdfs:domain rdf:resource="http://www.opengis.net/citygml/transportation/2.0#TransportationComplexType"/>
      <rdfs:range rdf:resource="http://www.opengis.net/gml#CodeType"/>
   </owl:ObjectProperty>
   <owl:ObjectProperty rdf:about="http://www.opengis.net/citygml/transportation/2.0#function">
      <rdfs:comment>Warning: This ObjectProperty type was declared outside of its original schema. This ObjectProperty may be declared incorrectly.</rdfs:comment>
      <rdfs:domain rdf:resource="http://www.opengis.net/citygml/transportation/2.0#TransportationComplexType"/>
      <rdfs:range rdf:resource="http://www.opengis.net/gml#CodeType"/>
   </owl:ObjectProperty>
   <owl:ObjectProperty rdf:about="http://www.opengis.net/citygml/transportation/2.0#usage">
      <rdfs:comment>Warning: This ObjectProperty type was declared outside of its original schema. This ObjectProperty may be declared incorrectly.</rdfs:comment>
      <rdfs:domain rdf:resource="http://www.opengis.net/citygml/transportation/2.0#TransportationComplexType"/>
      <rdfs:range rdf:resource="http://www.opengis.net/gml#CodeType"/>
   </owl:ObjectProperty>
   <owl:ObjectProperty rdf:about="http://www.opengis.net/citygml/transportation/2.0#trafficArea">
      <rdfs:domain rdf:resource="http://www.opengis.net/citygml/transportation/2.0#TransportationComplexType"/>
      <rdfs:range rdf:resource="http://www.opengis.net/citygml/transportation/2.0#TrafficAreaPropertyType"/>
   </owl:ObjectProperty>
   <owl:ObjectProperty rdf:about="http://www.opengis.net/citygml/transportation/2.0#auxiliaryTrafficArea">
      <rdfs:domain rdf:resource="http://www.opengis.net/citygml/transportation/2.0#TransportationComplexType"/>
      <rdfs:range rdf:resource="http://www.opengis.net/citygml/transportation/2.0#AuxiliaryTrafficAreaPropertyType"/>
   </owl:ObjectProperty>
   <owl:ObjectProperty rdf:about="http://www.opengis.net/citygml/transportation/2.0#lod0Network">
      <rdfs:comment>Warning: This ObjectProperty type was declared outside of its original schema. This ObjectProperty may be declared incorrectly.</rdfs:comment>
      <rdfs:domain rdf:resource="http://www.opengis.net/citygml/transportation/2.0#TransportationComplexType"/>
      <rdfs:range rdf:resource="http://www.opengis.net/gml#GeometricComplexPropertyType"/>
   </owl:ObjectProperty>
   <owl:ObjectProperty rdf:about="http://www.opengis.net/citygml/transportation/2.0#lod1MultiSurface">
      <rdfs:comment>Warning: This ObjectProperty type was declared outside of its original schema. This ObjectProperty may be declared incorrectly.</rdfs:comment>
      <rdfs:domain rdf:resource="http://www.opengis.net/citygml/transportation/2.0#TransportationComplexType"/>
      <rdfs:range rdf:resource="http://www.opengis.net/gml#MultiSurfacePropertyType"/>
   </owl:ObjectProperty>
   <owl:ObjectProperty rdf:about="http://www.opengis.net/citygml/transportation/2.0#lod2MultiSurface">
      <rdfs:comment>Warning: This ObjectProperty type was declared outside of its original schema. This ObjectProperty may be declared incorrectly.</rdfs:comment>
      <rdfs:domain rdf:resource="http://www.opengis.net/citygml/transportation/2.0#TransportationComplexType"/>
      <rdfs:range rdf:resource="http://www.opengis.net/gml#MultiSurfacePropertyType"/>
   </owl:ObjectProperty>
   <owl:ObjectProperty rdf:about="http://www.opengis.net/citygml/transportation/2.0#lod3MultiSurface">
      <rdfs:comment>Warning: This ObjectProperty type was declared outside of its original schema. This ObjectProperty may be declared incorrectly.</rdfs:comment>
      <rdfs:domain rdf:resource="http://www.opengis.net/citygml/transportation/2.0#TransportationComplexType"/>
      <rdfs:range rdf:resource="http://www.opengis.net/gml#MultiSurfacePropertyType"/>
   </owl:ObjectProperty>
   <owl:ObjectProperty rdf:about="http://www.opengis.net/citygml/transportation/2.0#lod4MultiSurface">
      <rdfs:comment>Warning: This ObjectProperty type was declared outside of its original schema. This ObjectProperty may be declared incorrectly.</rdfs:comment>
      <rdfs:domain rdf:resource="http://www.opengis.net/citygml/transportation/2.0#TransportationComplexType"/>
      <rdfs:range rdf:resource="http://www.opengis.net/gml#MultiSurfacePropertyType"/>
   </owl:ObjectProperty>
   <owl:ObjectProperty rdf:about="http://www.opengis.net/citygml/transportation/2.0#has_GenericApplicationPropertyOfTransportationComplex">
      <rdfs:domain rdf:resource="http://www.opengis.net/citygml/transportation/2.0#TransportationComplexType"/>
      <rdfs:range rdf:resource="http://www.opengis.net/citygml/transportation/2.0#_GenericApplicationPropertyOfTransportationComplex"/>
   </owl:ObjectProperty>
   <owl:ObjectProperty rdf:about="http://www.opengis.net/citygml/transportation/2.0#class">
      <rdfs:comment>Warning: This ObjectProperty type was declared outside of its original schema. This ObjectProperty may be declared incorrectly.</rdfs:comment>
      <rdfs:domain rdf:resource="http://www.opengis.net/citygml/transportation/2.0#TrafficAreaType"/>
      <rdfs:range rdf:resource="http://www.opengis.net/gml#CodeType"/>
   </owl:ObjectProperty>
   <owl:ObjectProperty rdf:about="http://www.opengis.net/citygml/transportation/2.0#function">
      <rdfs:comment>Warning: This ObjectProperty type was declared outside of its original schema. This ObjectProperty may be declared incorrectly.</rdfs:comment>
      <rdfs:domain rdf:resource="http://www.opengis.net/citygml/transportation/2.0#TrafficAreaType"/>
      <rdfs:range rdf:resource="http://www.opengis.net/gml#CodeType"/>
   </owl:ObjectProperty>
   <owl:ObjectProperty rdf:about="http://www.opengis.net/citygml/transportation/2.0#usage">
      <rdfs:comment>Warning: This ObjectProperty type was declared outside of its original schema. This ObjectProperty may be declared incorrectly.</rdfs:comment>
      <rdfs:domain rdf:resource="http://www.opengis.net/citygml/transportation/2.0#TrafficAreaType"/>
      <rdfs:range rdf:resource="http://www.opengis.net/gml#CodeType"/>
   </owl:ObjectProperty>
   <owl:ObjectProperty rdf:about="http://www.opengis.net/citygml/transportation/2.0#surfaceMaterial">
      <rdfs:comment>Warning: This ObjectProperty type was declared outside of its original schema. This ObjectProperty may be declared incorrectly.</rdfs:comment>
      <rdfs:domain rdf:resource="http://www.opengis.net/citygml/transportation/2.0#TrafficAreaType"/>
      <rdfs:range rdf:resource="http://www.opengis.net/gml#CodeType"/>
   </owl:ObjectProperty>
   <owl:ObjectProperty rdf:about="http://www.opengis.net/citygml/transportation/2.0#lod2MultiSurface">
      <rdfs:comment>Warning: This ObjectProperty type was declared outside of its original schema. This ObjectProperty may be declared incorrectly.</rdfs:comment>
      <rdfs:domain rdf:resource="http://www.opengis.net/citygml/transportation/2.0#TrafficAreaType"/>
      <rdfs:range rdf:resource="http://www.opengis.net/gml#MultiSurfacePropertyType"/>
   </owl:ObjectProperty>
   <owl:ObjectProperty rdf:about="http://www.opengis.net/citygml/transportation/2.0#lod3MultiSurface">
      <rdfs:comment>Warning: This ObjectProperty type was declared outside of its original schema. This ObjectProperty may be declared incorrectly.</rdfs:comment>
      <rdfs:domain rdf:resource="http://www.opengis.net/citygml/transportation/2.0#TrafficAreaType"/>
      <rdfs:range rdf:resource="http://www.opengis.net/gml#MultiSurfacePropertyType"/>
   </owl:ObjectProperty>
   <owl:ObjectProperty rdf:about="http://www.opengis.net/citygml/transportation/2.0#lod4MultiSurface">
      <rdfs:comment>Warning: This ObjectProperty type was declared outside of its original schema. This ObjectProperty may be declared incorrectly.</rdfs:comment>
      <rdfs:domain rdf:resource="http://www.opengis.net/citygml/transportation/2.0#TrafficAreaType"/>
      <rdfs:range rdf:resource="http://www.opengis.net/gml#MultiSurfacePropertyType"/>
   </owl:ObjectProperty>
   <owl:ObjectProperty rdf:about="http://www.opengis.net/citygml/transportation/2.0#has_GenericApplicationPropertyOfTrafficArea">
      <rdfs:domain rdf:resource="http://www.opengis.net/citygml/transportation/2.0#TrafficAreaType"/>
      <rdfs:range rdf:resource="http://www.opengis.net/citygml/transportation/2.0#_GenericApplicationPropertyOfTrafficArea"/>
   </owl:ObjectProperty>
   <owl:ObjectProperty rdf:about="http://www.opengis.net/citygml/transportation/2.0#class">
      <rdfs:comment>Warning: This ObjectProperty type was declared outside of its original schema. This ObjectProperty may be declared incorrectly.</rdfs:comment>
      <rdfs:domain rdf:resource="http://www.opengis.net/citygml/transportation/2.0#AuxiliaryTrafficAreaType"/>
      <rdfs:range rdf:resource="http://www.opengis.net/gml#CodeType"/>
   </owl:ObjectProperty>
   <owl:ObjectProperty rdf:about="http://www.opengis.net/citygml/transportation/2.0#function">
      <rdfs:comment>Warning: This ObjectProperty type was declared outside of its original schema. This ObjectProperty may be declared incorrectly.</rdfs:comment>
      <rdfs:domain rdf:resource="http://www.opengis.net/citygml/transportation/2.0#AuxiliaryTrafficAreaType"/>
      <rdfs:range rdf:resource="http://www.opengis.net/gml#CodeType"/>
   </owl:ObjectProperty>
   <owl:ObjectProperty rdf:about="http://www.opengis.net/citygml/transportation/2.0#usage">
      <rdfs:comment>Warning: This ObjectProperty type was declared outside of its original schema. This ObjectProperty may be declared incorrectly.</rdfs:comment>
      <rdfs:domain rdf:resource="http://www.opengis.net/citygml/transportation/2.0#AuxiliaryTrafficAreaType"/>
      <rdfs:range rdf:resource="http://www.opengis.net/gml#CodeType"/>
   </owl:ObjectProperty>
   <owl:ObjectProperty rdf:about="http://www.opengis.net/citygml/transportation/2.0#surfaceMaterial">
      <rdfs:comment>Warning: This ObjectProperty type was declared outside of its original schema. This ObjectProperty may be declared incorrectly.</rdfs:comment>
      <rdfs:domain rdf:resource="http://www.opengis.net/citygml/transportation/2.0#AuxiliaryTrafficAreaType"/>
      <rdfs:range rdf:resource="http://www.opengis.net/gml#CodeType"/>
   </owl:ObjectProperty>
   <owl:ObjectProperty rdf:about="http://www.opengis.net/citygml/transportation/2.0#lod2MultiSurface">
      <rdfs:comment>Warning: This ObjectProperty type was declared outside of its original schema. This ObjectProperty may be declared incorrectly.</rdfs:comment>
      <rdfs:domain rdf:resource="http://www.opengis.net/citygml/transportation/2.0#AuxiliaryTrafficAreaType"/>
      <rdfs:range rdf:resource="http://www.opengis.net/gml#MultiSurfacePropertyType"/>
   </owl:ObjectProperty>
   <owl:ObjectProperty rdf:about="http://www.opengis.net/citygml/transportation/2.0#lod3MultiSurface">
      <rdfs:comment>Warning: This ObjectProperty type was declared outside of its original schema. This ObjectProperty may be declared incorrectly.</rdfs:comment>
      <rdfs:domain rdf:resource="http://www.opengis.net/citygml/transportation/2.0#AuxiliaryTrafficAreaType"/>
      <rdfs:range rdf:resource="http://www.opengis.net/gml#MultiSurfacePropertyType"/>
   </owl:ObjectProperty>
   <owl:ObjectProperty rdf:about="http://www.opengis.net/citygml/transportation/2.0#lod4MultiSurface">
      <rdfs:comment>Warning: This ObjectProperty type was declared outside of its original schema. This ObjectProperty may be declared incorrectly.</rdfs:comment>
      <rdfs:domain rdf:resource="http://www.opengis.net/citygml/transportation/2.0#AuxiliaryTrafficAreaType"/>
      <rdfs:range rdf:resource="http://www.opengis.net/gml#MultiSurfacePropertyType"/>
   </owl:ObjectProperty>
   <owl:ObjectProperty rdf:about="http://www.opengis.net/citygml/transportation/2.0#has_GenericApplicationPropertyOfAuxiliaryTrafficArea">
      <rdfs:domain rdf:resource="http://www.opengis.net/citygml/transportation/2.0#AuxiliaryTrafficAreaType"/>
      <rdfs:range rdf:resource="http://www.opengis.net/citygml/transportation/2.0#_GenericApplicationPropertyOfAuxiliaryTrafficArea"/>
   </owl:ObjectProperty>
   <owl:ObjectProperty rdf:about="http://www.opengis.net/citygml/transportation/2.0#hasTrafficArea">
      <rdfs:domain rdf:resource="http://www.opengis.net/citygml/transportation/2.0#TrafficAreaPropertyType"/>
      <rdfs:range rdf:resource="http://www.opengis.net/citygml/transportation/2.0#TrafficArea"/>
   </owl:ObjectProperty>
   <owl:ObjectProperty rdf:about="http://www.opengis.net/citygml/transportation/2.0#hasAuxiliaryTrafficArea">
      <rdfs:domain rdf:resource="http://www.opengis.net/citygml/transportation/2.0#AuxiliaryTrafficAreaPropertyType"/>
      <rdfs:range rdf:resource="http://www.opengis.net/citygml/transportation/2.0#AuxiliaryTrafficArea"/>
   </owl:ObjectProperty>
   <owl:ObjectProperty rdf:about="http://www.opengis.net/citygml/transportation/2.0#has_GenericApplicationPropertyOfTrack">
      <rdfs:domain rdf:resource="http://www.opengis.net/citygml/transportation/2.0#TrackType"/>
      <rdfs:range rdf:resource="http://www.opengis.net/citygml/transportation/2.0#_GenericApplicationPropertyOfTrack"/>
   </owl:ObjectProperty>
   <owl:ObjectProperty rdf:about="http://www.opengis.net/citygml/transportation/2.0#has_GenericApplicationPropertyOfRoad">
      <rdfs:domain rdf:resource="http://www.opengis.net/citygml/transportation/2.0#RoadType"/>
      <rdfs:range rdf:resource="http://www.opengis.net/citygml/transportation/2.0#_GenericApplicationPropertyOfRoad"/>
   </owl:ObjectProperty>
   <owl:ObjectProperty rdf:about="http://www.opengis.net/citygml/transportation/2.0#has_GenericApplicationPropertyOfRailway">
      <rdfs:domain rdf:resource="http://www.opengis.net/citygml/transportation/2.0#RailwayType"/>
      <rdfs:range rdf:resource="http://www.opengis.net/citygml/transportation/2.0#_GenericApplicationPropertyOfRailway"/>
   </owl:ObjectProperty>
   <owl:ObjectProperty rdf:about="http://www.opengis.net/citygml/transportation/2.0#has_GenericApplicationPropertyOfSquare">
      <rdfs:domain rdf:resource="http://www.opengis.net/citygml/transportation/2.0#SquareType"/>
      <rdfs:range rdf:resource="http://www.opengis.net/citygml/transportation/2.0#_GenericApplicationPropertyOfSquare"/>
   </owl:ObjectProperty>
</rdf:RDF>
