<?xml version="1.0" encoding="UTF-8"?>
<rdf:RDF xmlns:math="http://www.w3.org/2005/xpath-functions/math"
         xmlns:owl="http://www.w3.org/2002/07/owl#"
         xmlns:rdf="http://www.w3.org/1999/02/22-rdf-syntax-ns#"
         xmlns:rdfs="http://www.w3.org/2000/01/rdf-schema#"
         xmlns:xs="http://www.w3.org/2001/XMLSchema"
         xmlns:xsd="http://www.w3.org/2001/XMLSchema">
   <owl:Ontology rdf:about="http://liris.cnrs.fr/ontologies/tunnel">
      <owl:imports rdf:resource="http://liris.cnrs.fr/ontologies/gml"/>
      <owl:imports rdf:resource="http://liris.cnrs.fr/ontologies/cityGMLBase"/>
      <rdfs:comment>
	CityGML is an OGC Standard.
	Copyright (c) 2012 Open Geospatial Consortium.
	To obtain additional rights of use, visit http://www.opengeospatial.org/legal/ .
		</rdfs:comment>
   </owl:Ontology>
   <owl:Class rdf:about="http://www.opengis.net/citygml/tunnel/2.0#AbstractTunnelType">
      <rdfs:comment>Abstract super class of the features Tunnel and TunnelPart</rdfs:comment>
      <owl:equivalentClass>
         <owl:Class>
            <owl:intersectionOf rdf:parseType="Collection">
               <owl:Restriction>
                  <owl:onProperty rdf:resource="http://www.opengis.net/citygml/tunnel/2.0#class"/>
                  <owl:allValuesFrom rdf:resource="http://www.opengis.net/gml#CodeType"/>
               </owl:Restriction>
               <owl:Restriction>
                  <owl:onProperty rdf:resource="http://www.opengis.net/citygml/tunnel/2.0#class"/>
                  <owl:minCardinality rdf:datatype="http://www.w3.org/2001/XMLSchema#nonNegativeInteger">0</owl:minCardinality>
               </owl:Restriction>
               <owl:Restriction>
                  <owl:onProperty rdf:resource="http://www.opengis.net/citygml/tunnel/2.0#function"/>
                  <owl:allValuesFrom rdf:resource="http://www.opengis.net/gml#CodeType"/>
               </owl:Restriction>
               <owl:Restriction>
                  <owl:onProperty rdf:resource="http://www.opengis.net/citygml/tunnel/2.0#function"/>
                  <owl:minCardinality rdf:datatype="http://www.w3.org/2001/XMLSchema#nonNegativeInteger">0</owl:minCardinality>
               </owl:Restriction>
               <owl:Restriction>
                  <owl:onProperty rdf:resource="http://www.opengis.net/citygml/tunnel/2.0#usage"/>
                  <owl:allValuesFrom rdf:resource="http://www.opengis.net/gml#CodeType"/>
               </owl:Restriction>
               <owl:Restriction>
                  <owl:onProperty rdf:resource="http://www.opengis.net/citygml/tunnel/2.0#usage"/>
                  <owl:minCardinality rdf:datatype="http://www.w3.org/2001/XMLSchema#nonNegativeInteger">0</owl:minCardinality>
               </owl:Restriction>
               <owl:Restriction>
                  <owl:onProperty rdf:resource="http://www.opengis.net/citygml/tunnel/2.0#yearOfConstruction"/>
                  <owl:allValuesFrom rdf:resource="http://www.w3.org/2001/XMLSchema#gYear"/>
               </owl:Restriction>
               <owl:Restriction>
                  <owl:onProperty rdf:resource="http://www.opengis.net/citygml/tunnel/2.0#yearOfConstruction"/>
                  <owl:minCardinality rdf:datatype="http://www.w3.org/2001/XMLSchema#nonNegativeInteger">0</owl:minCardinality>
               </owl:Restriction>
               <owl:Restriction>
                  <owl:onProperty rdf:resource="http://www.opengis.net/citygml/tunnel/2.0#yearOfDemolition"/>
                  <owl:allValuesFrom rdf:resource="http://www.w3.org/2001/XMLSchema#gYear"/>
               </owl:Restriction>
               <owl:Restriction>
                  <owl:onProperty rdf:resource="http://www.opengis.net/citygml/tunnel/2.0#yearOfDemolition"/>
                  <owl:minCardinality rdf:datatype="http://www.w3.org/2001/XMLSchema#nonNegativeInteger">0</owl:minCardinality>
               </owl:Restriction>
               <owl:Restriction>
                  <owl:onProperty rdf:resource="http://www.opengis.net/citygml/tunnel/2.0#lod1Solid"/>
                  <owl:allValuesFrom rdf:resource="http://www.opengis.net/gml#SolidPropertyType"/>
               </owl:Restriction>
               <owl:Restriction>
                  <owl:onProperty rdf:resource="http://www.opengis.net/citygml/tunnel/2.0#lod1Solid"/>
                  <owl:minCardinality rdf:datatype="http://www.w3.org/2001/XMLSchema#nonNegativeInteger">0</owl:minCardinality>
               </owl:Restriction>
               <owl:Restriction>
                  <owl:onProperty rdf:resource="http://www.opengis.net/citygml/tunnel/2.0#lod1MultiSurface"/>
                  <owl:allValuesFrom rdf:resource="http://www.opengis.net/gml#MultiSurfacePropertyType"/>
               </owl:Restriction>
               <owl:Restriction>
                  <owl:onProperty rdf:resource="http://www.opengis.net/citygml/tunnel/2.0#lod1MultiSurface"/>
                  <owl:minCardinality rdf:datatype="http://www.w3.org/2001/XMLSchema#nonNegativeInteger">0</owl:minCardinality>
               </owl:Restriction>
               <owl:Restriction>
                  <owl:onProperty rdf:resource="http://www.opengis.net/citygml/tunnel/2.0#lod1TerrainIntersection"/>
                  <owl:allValuesFrom rdf:resource="http://www.opengis.net/gml#MultiCurvePropertyType"/>
               </owl:Restriction>
               <owl:Restriction>
                  <owl:onProperty rdf:resource="http://www.opengis.net/citygml/tunnel/2.0#lod1TerrainIntersection"/>
                  <owl:minCardinality rdf:datatype="http://www.w3.org/2001/XMLSchema#nonNegativeInteger">0</owl:minCardinality>
               </owl:Restriction>
               <owl:Restriction>
                  <owl:onProperty rdf:resource="http://www.opengis.net/citygml/tunnel/2.0#lod2Solid"/>
                  <owl:allValuesFrom rdf:resource="http://www.opengis.net/gml#SolidPropertyType"/>
               </owl:Restriction>
               <owl:Restriction>
                  <owl:onProperty rdf:resource="http://www.opengis.net/citygml/tunnel/2.0#lod2Solid"/>
                  <owl:minCardinality rdf:datatype="http://www.w3.org/2001/XMLSchema#nonNegativeInteger">0</owl:minCardinality>
               </owl:Restriction>
               <owl:Restriction>
                  <owl:onProperty rdf:resource="http://www.opengis.net/citygml/tunnel/2.0#lod2MultiSurface"/>
                  <owl:allValuesFrom rdf:resource="http://www.opengis.net/gml#MultiSurfacePropertyType"/>
               </owl:Restriction>
               <owl:Restriction>
                  <owl:onProperty rdf:resource="http://www.opengis.net/citygml/tunnel/2.0#lod2MultiSurface"/>
                  <owl:minCardinality rdf:datatype="http://www.w3.org/2001/XMLSchema#nonNegativeInteger">0</owl:minCardinality>
               </owl:Restriction>
               <owl:Restriction>
                  <owl:onProperty rdf:resource="http://www.opengis.net/citygml/tunnel/2.0#lod2MultiCurve"/>
                  <owl:allValuesFrom rdf:resource="http://www.opengis.net/gml#MultiCurvePropertyType"/>
               </owl:Restriction>
               <owl:Restriction>
                  <owl:onProperty rdf:resource="http://www.opengis.net/citygml/tunnel/2.0#lod2MultiCurve"/>
                  <owl:minCardinality rdf:datatype="http://www.w3.org/2001/XMLSchema#nonNegativeInteger">0</owl:minCardinality>
               </owl:Restriction>
               <owl:Restriction>
                  <owl:onProperty rdf:resource="http://www.opengis.net/citygml/tunnel/2.0#lod2TerrainIntersection"/>
                  <owl:allValuesFrom rdf:resource="http://www.opengis.net/gml#MultiCurvePropertyType"/>
               </owl:Restriction>
               <owl:Restriction>
                  <owl:onProperty rdf:resource="http://www.opengis.net/citygml/tunnel/2.0#lod2TerrainIntersection"/>
                  <owl:minCardinality rdf:datatype="http://www.w3.org/2001/XMLSchema#nonNegativeInteger">0</owl:minCardinality>
               </owl:Restriction>
               <owl:Restriction>
                  <owl:onProperty rdf:resource="http://www.opengis.net/citygml/tunnel/2.0#outerTunnelInstallation"/>
                  <owl:allValuesFrom rdf:resource="http://www.opengis.net/citygml/tunnel/2.0#TunnelInstallationPropertyType"/>
               </owl:Restriction>
               <owl:Restriction>
                  <owl:onProperty rdf:resource="http://www.opengis.net/citygml/tunnel/2.0#outerTunnelInstallation"/>
                  <owl:minCardinality rdf:datatype="http://www.w3.org/2001/XMLSchema#nonNegativeInteger">0</owl:minCardinality>
               </owl:Restriction>
               <owl:Restriction>
                  <owl:onProperty rdf:resource="http://www.opengis.net/citygml/tunnel/2.0#interiorTunnelInstallation"/>
                  <owl:allValuesFrom rdf:resource="http://www.opengis.net/citygml/tunnel/2.0#IntTunnelInstallationPropertyType"/>
               </owl:Restriction>
               <owl:Restriction>
                  <owl:onProperty rdf:resource="http://www.opengis.net/citygml/tunnel/2.0#interiorTunnelInstallation"/>
                  <owl:minCardinality rdf:datatype="http://www.w3.org/2001/XMLSchema#nonNegativeInteger">0</owl:minCardinality>
               </owl:Restriction>
               <owl:Restriction>
                  <owl:onProperty rdf:resource="http://www.opengis.net/citygml/tunnel/2.0#boundedBy"/>
                  <owl:allValuesFrom rdf:resource="http://www.opengis.net/citygml/tunnel/2.0#BoundarySurfacePropertyType"/>
               </owl:Restriction>
               <owl:Restriction>
                  <owl:onProperty rdf:resource="http://www.opengis.net/citygml/tunnel/2.0#boundedBy"/>
                  <owl:minCardinality rdf:datatype="http://www.w3.org/2001/XMLSchema#nonNegativeInteger">0</owl:minCardinality>
               </owl:Restriction>
               <owl:Restriction>
                  <owl:onProperty rdf:resource="http://www.opengis.net/citygml/tunnel/2.0#lod3Solid"/>
                  <owl:allValuesFrom rdf:resource="http://www.opengis.net/gml#SolidPropertyType"/>
               </owl:Restriction>
               <owl:Restriction>
                  <owl:onProperty rdf:resource="http://www.opengis.net/citygml/tunnel/2.0#lod3Solid"/>
                  <owl:minCardinality rdf:datatype="http://www.w3.org/2001/XMLSchema#nonNegativeInteger">0</owl:minCardinality>
               </owl:Restriction>
               <owl:Restriction>
                  <owl:onProperty rdf:resource="http://www.opengis.net/citygml/tunnel/2.0#lod3MultiSurface"/>
                  <owl:allValuesFrom rdf:resource="http://www.opengis.net/gml#MultiSurfacePropertyType"/>
               </owl:Restriction>
               <owl:Restriction>
                  <owl:onProperty rdf:resource="http://www.opengis.net/citygml/tunnel/2.0#lod3MultiSurface"/>
                  <owl:minCardinality rdf:datatype="http://www.w3.org/2001/XMLSchema#nonNegativeInteger">0</owl:minCardinality>
               </owl:Restriction>
               <owl:Restriction>
                  <owl:onProperty rdf:resource="http://www.opengis.net/citygml/tunnel/2.0#lod3MultiCurve"/>
                  <owl:allValuesFrom rdf:resource="http://www.opengis.net/gml#MultiCurvePropertyType"/>
               </owl:Restriction>
               <owl:Restriction>
                  <owl:onProperty rdf:resource="http://www.opengis.net/citygml/tunnel/2.0#lod3MultiCurve"/>
                  <owl:minCardinality rdf:datatype="http://www.w3.org/2001/XMLSchema#nonNegativeInteger">0</owl:minCardinality>
               </owl:Restriction>
               <owl:Restriction>
                  <owl:onProperty rdf:resource="http://www.opengis.net/citygml/tunnel/2.0#lod3TerrainIntersection"/>
                  <owl:allValuesFrom rdf:resource="http://www.opengis.net/gml#MultiCurvePropertyType"/>
               </owl:Restriction>
               <owl:Restriction>
                  <owl:onProperty rdf:resource="http://www.opengis.net/citygml/tunnel/2.0#lod3TerrainIntersection"/>
                  <owl:minCardinality rdf:datatype="http://www.w3.org/2001/XMLSchema#nonNegativeInteger">0</owl:minCardinality>
               </owl:Restriction>
               <owl:Restriction>
                  <owl:onProperty rdf:resource="http://www.opengis.net/citygml/tunnel/2.0#lod4Solid"/>
                  <owl:allValuesFrom rdf:resource="http://www.opengis.net/gml#SolidPropertyType"/>
               </owl:Restriction>
               <owl:Restriction>
                  <owl:onProperty rdf:resource="http://www.opengis.net/citygml/tunnel/2.0#lod4Solid"/>
                  <owl:minCardinality rdf:datatype="http://www.w3.org/2001/XMLSchema#nonNegativeInteger">0</owl:minCardinality>
               </owl:Restriction>
               <owl:Restriction>
                  <owl:onProperty rdf:resource="http://www.opengis.net/citygml/tunnel/2.0#lod4MultiSurface"/>
                  <owl:allValuesFrom rdf:resource="http://www.opengis.net/gml#MultiSurfacePropertyType"/>
               </owl:Restriction>
               <owl:Restriction>
                  <owl:onProperty rdf:resource="http://www.opengis.net/citygml/tunnel/2.0#lod4MultiSurface"/>
                  <owl:minCardinality rdf:datatype="http://www.w3.org/2001/XMLSchema#nonNegativeInteger">0</owl:minCardinality>
               </owl:Restriction>
               <owl:Restriction>
                  <owl:onProperty rdf:resource="http://www.opengis.net/citygml/tunnel/2.0#lod4MultiCurve"/>
                  <owl:allValuesFrom rdf:resource="http://www.opengis.net/gml#MultiCurvePropertyType"/>
               </owl:Restriction>
               <owl:Restriction>
                  <owl:onProperty rdf:resource="http://www.opengis.net/citygml/tunnel/2.0#lod4MultiCurve"/>
                  <owl:minCardinality rdf:datatype="http://www.w3.org/2001/XMLSchema#nonNegativeInteger">0</owl:minCardinality>
               </owl:Restriction>
               <owl:Restriction>
                  <owl:onProperty rdf:resource="http://www.opengis.net/citygml/tunnel/2.0#lod4TerrainIntersection"/>
                  <owl:allValuesFrom rdf:resource="http://www.opengis.net/gml#MultiCurvePropertyType"/>
               </owl:Restriction>
               <owl:Restriction>
                  <owl:onProperty rdf:resource="http://www.opengis.net/citygml/tunnel/2.0#lod4TerrainIntersection"/>
                  <owl:minCardinality rdf:datatype="http://www.w3.org/2001/XMLSchema#nonNegativeInteger">0</owl:minCardinality>
               </owl:Restriction>
               <owl:Restriction>
                  <owl:onProperty rdf:resource="http://www.opengis.net/citygml/tunnel/2.0#interiorHollowSpace"/>
                  <owl:allValuesFrom rdf:resource="http://www.opengis.net/citygml/tunnel/2.0#InteriorHollowSpacePropertyType"/>
               </owl:Restriction>
               <owl:Restriction>
                  <owl:onProperty rdf:resource="http://www.opengis.net/citygml/tunnel/2.0#interiorHollowSpace"/>
                  <owl:minCardinality rdf:datatype="http://www.w3.org/2001/XMLSchema#nonNegativeInteger">0</owl:minCardinality>
               </owl:Restriction>
               <owl:Restriction>
                  <owl:onProperty rdf:resource="http://www.opengis.net/citygml/tunnel/2.0#consistsOfTunnelPart"/>
                  <owl:allValuesFrom rdf:resource="http://www.opengis.net/citygml/tunnel/2.0#TunnelPartPropertyType"/>
               </owl:Restriction>
               <owl:Restriction>
                  <owl:onProperty rdf:resource="http://www.opengis.net/citygml/tunnel/2.0#consistsOfTunnelPart"/>
                  <owl:minCardinality rdf:datatype="http://www.w3.org/2001/XMLSchema#nonNegativeInteger">0</owl:minCardinality>
               </owl:Restriction>
               <owl:Restriction>
                  <owl:onProperty rdf:resource="http://www.opengis.net/citygml/tunnel/2.0#has_GenericApplicationPropertyOfAbstractTunnel"/>
                  <owl:allValuesFrom rdf:resource="http://www.opengis.net/citygml/tunnel/2.0#_GenericApplicationPropertyOfAbstractTunnel"/>
               </owl:Restriction>
               <owl:Restriction>
                  <owl:onProperty rdf:resource="http://www.opengis.net/citygml/tunnel/2.0#has_GenericApplicationPropertyOfAbstractTunnel"/>
                  <owl:minCardinality rdf:datatype="http://www.w3.org/2001/XMLSchema#nonNegativeInteger">0</owl:minCardinality>
               </owl:Restriction>
            </owl:intersectionOf>
         </owl:Class>
      </owl:equivalentClass>
      <rdfs:subClassOf rdf:resource="http://www.opengis.net/citygml/2.0#AbstractSiteType"/>
      <rdfs:comment>Warning: The parent class 'core:AbstractSiteType' is declared outside of this class' original schema. This class may be declared incorrectly.</rdfs:comment>
   </owl:Class>
   <owl:Class rdf:about="http://www.opengis.net/citygml/tunnel/2.0#TunnelType">
      <rdfs:comment>Horizontal or sloping underground or partly underground, enclosed way of some length (ISO
				6707-1)</rdfs:comment>
      <owl:equivalentClass>
         <owl:Class>
            <owl:intersectionOf rdf:parseType="Collection">
               <owl:Restriction>
                  <owl:onProperty rdf:resource="http://www.opengis.net/citygml/tunnel/2.0#has_GenericApplicationPropertyOfTunnel"/>
                  <owl:allValuesFrom rdf:resource="http://www.opengis.net/citygml/tunnel/2.0#_GenericApplicationPropertyOfTunnel"/>
               </owl:Restriction>
               <owl:Restriction>
                  <owl:onProperty rdf:resource="http://www.opengis.net/citygml/tunnel/2.0#has_GenericApplicationPropertyOfTunnel"/>
                  <owl:minCardinality rdf:datatype="http://www.w3.org/2001/XMLSchema#nonNegativeInteger">0</owl:minCardinality>
               </owl:Restriction>
            </owl:intersectionOf>
         </owl:Class>
      </owl:equivalentClass>
   </owl:Class>
   <owl:Class rdf:about="http://www.opengis.net/citygml/tunnel/2.0#TunnelPartType">
      <rdfs:comment>A Tunnel composed of structural segments differing in important geometrical or semantical properties can
				be separated into one Tunnel and additional TunnelParts. </rdfs:comment>
      <owl:equivalentClass>
         <owl:Class>
            <owl:intersectionOf rdf:parseType="Collection">
               <owl:Restriction>
                  <owl:onProperty rdf:resource="http://www.opengis.net/citygml/tunnel/2.0#has_GenericApplicationPropertyOfTunnelPart"/>
                  <owl:allValuesFrom rdf:resource="http://www.opengis.net/citygml/tunnel/2.0#_GenericApplicationPropertyOfTunnelPart"/>
               </owl:Restriction>
               <owl:Restriction>
                  <owl:onProperty rdf:resource="http://www.opengis.net/citygml/tunnel/2.0#has_GenericApplicationPropertyOfTunnelPart"/>
                  <owl:minCardinality rdf:datatype="http://www.w3.org/2001/XMLSchema#nonNegativeInteger">0</owl:minCardinality>
               </owl:Restriction>
            </owl:intersectionOf>
         </owl:Class>
      </owl:equivalentClass>
   </owl:Class>
   <owl:Class rdf:about="http://www.opengis.net/citygml/tunnel/2.0#TunnelPartPropertyType">
      <rdfs:comment>Denotes the relation of an _AbstractTunnel to its parts. The TunnelPartPropertyType element must either
				carry a reference to a TunnelPart object or contain a TunnelPart object inline, but neither both nor
				none.</rdfs:comment>
      <owl:equivalentClass>
         <owl:Class>
            <owl:intersectionOf rdf:parseType="Collection">
               <owl:Restriction>
                  <owl:onProperty rdf:resource="http://www.opengis.net/citygml/tunnel/2.0#hasTunnelPart"/>
                  <owl:allValuesFrom rdf:resource="http://www.opengis.net/citygml/tunnel/2.0#TunnelPart"/>
               </owl:Restriction>
            </owl:intersectionOf>
         </owl:Class>
      </owl:equivalentClass>
   </owl:Class>
   <owl:Class rdf:about="http://www.opengis.net/citygml/tunnel/2.0#TunnelInstallationType">
      <rdfs:comment>Immovable structural component of a Tunnel which has not the significance of a TunnelPart. As subclass of
				_CityObject, a TunnelInstallation inherits all attributes and relations, in particular an id, names, external references,
				generic attributes and generalization relations. </rdfs:comment>
      <owl:equivalentClass>
         <owl:Class>
            <owl:intersectionOf rdf:parseType="Collection">
               <owl:Restriction>
                  <owl:onProperty rdf:resource="http://www.opengis.net/citygml/tunnel/2.0#class"/>
                  <owl:allValuesFrom rdf:resource="http://www.opengis.net/gml#CodeType"/>
               </owl:Restriction>
               <owl:Restriction>
                  <owl:onProperty rdf:resource="http://www.opengis.net/citygml/tunnel/2.0#class"/>
                  <owl:minCardinality rdf:datatype="http://www.w3.org/2001/XMLSchema#nonNegativeInteger">0</owl:minCardinality>
               </owl:Restriction>
               <owl:Restriction>
                  <owl:onProperty rdf:resource="http://www.opengis.net/citygml/tunnel/2.0#function"/>
                  <owl:allValuesFrom rdf:resource="http://www.opengis.net/gml#CodeType"/>
               </owl:Restriction>
               <owl:Restriction>
                  <owl:onProperty rdf:resource="http://www.opengis.net/citygml/tunnel/2.0#function"/>
                  <owl:minCardinality rdf:datatype="http://www.w3.org/2001/XMLSchema#nonNegativeInteger">0</owl:minCardinality>
               </owl:Restriction>
               <owl:Restriction>
                  <owl:onProperty rdf:resource="http://www.opengis.net/citygml/tunnel/2.0#usage"/>
                  <owl:allValuesFrom rdf:resource="http://www.opengis.net/gml#CodeType"/>
               </owl:Restriction>
               <owl:Restriction>
                  <owl:onProperty rdf:resource="http://www.opengis.net/citygml/tunnel/2.0#usage"/>
                  <owl:minCardinality rdf:datatype="http://www.w3.org/2001/XMLSchema#nonNegativeInteger">0</owl:minCardinality>
               </owl:Restriction>
               <owl:Restriction>
                  <owl:onProperty rdf:resource="http://www.opengis.net/citygml/tunnel/2.0#lod2Geometry"/>
                  <owl:allValuesFrom rdf:resource="http://www.opengis.net/gml#GeometryPropertyType"/>
               </owl:Restriction>
               <owl:Restriction>
                  <owl:onProperty rdf:resource="http://www.opengis.net/citygml/tunnel/2.0#lod2Geometry"/>
                  <owl:minCardinality rdf:datatype="http://www.w3.org/2001/XMLSchema#nonNegativeInteger">0</owl:minCardinality>
               </owl:Restriction>
               <owl:Restriction>
                  <owl:onProperty rdf:resource="http://www.opengis.net/citygml/tunnel/2.0#lod3Geometry"/>
                  <owl:allValuesFrom rdf:resource="http://www.opengis.net/gml#GeometryPropertyType"/>
               </owl:Restriction>
               <owl:Restriction>
                  <owl:onProperty rdf:resource="http://www.opengis.net/citygml/tunnel/2.0#lod3Geometry"/>
                  <owl:minCardinality rdf:datatype="http://www.w3.org/2001/XMLSchema#nonNegativeInteger">0</owl:minCardinality>
               </owl:Restriction>
               <owl:Restriction>
                  <owl:onProperty rdf:resource="http://www.opengis.net/citygml/tunnel/2.0#lod4Geometry"/>
                  <owl:allValuesFrom rdf:resource="http://www.opengis.net/gml#GeometryPropertyType"/>
               </owl:Restriction>
               <owl:Restriction>
                  <owl:onProperty rdf:resource="http://www.opengis.net/citygml/tunnel/2.0#lod4Geometry"/>
                  <owl:minCardinality rdf:datatype="http://www.w3.org/2001/XMLSchema#nonNegativeInteger">0</owl:minCardinality>
               </owl:Restriction>
               <owl:Restriction>
                  <owl:onProperty rdf:resource="http://www.opengis.net/citygml/tunnel/2.0#lod2ImplicitRepresentation"/>
                  <owl:allValuesFrom rdf:resource="http://www.opengis.net/citygml/2.0#ImplicitRepresentationPropertyType"/>
               </owl:Restriction>
               <owl:Restriction>
                  <owl:onProperty rdf:resource="http://www.opengis.net/citygml/tunnel/2.0#lod2ImplicitRepresentation"/>
                  <owl:minCardinality rdf:datatype="http://www.w3.org/2001/XMLSchema#nonNegativeInteger">0</owl:minCardinality>
               </owl:Restriction>
               <owl:Restriction>
                  <owl:onProperty rdf:resource="http://www.opengis.net/citygml/tunnel/2.0#lod3ImplicitRepresentation"/>
                  <owl:allValuesFrom rdf:resource="http://www.opengis.net/citygml/2.0#ImplicitRepresentationPropertyType"/>
               </owl:Restriction>
               <owl:Restriction>
                  <owl:onProperty rdf:resource="http://www.opengis.net/citygml/tunnel/2.0#lod3ImplicitRepresentation"/>
                  <owl:minCardinality rdf:datatype="http://www.w3.org/2001/XMLSchema#nonNegativeInteger">0</owl:minCardinality>
               </owl:Restriction>
               <owl:Restriction>
                  <owl:onProperty rdf:resource="http://www.opengis.net/citygml/tunnel/2.0#lod4ImplicitRepresentation"/>
                  <owl:allValuesFrom rdf:resource="http://www.opengis.net/citygml/2.0#ImplicitRepresentationPropertyType"/>
               </owl:Restriction>
               <owl:Restriction>
                  <owl:onProperty rdf:resource="http://www.opengis.net/citygml/tunnel/2.0#lod4ImplicitRepresentation"/>
                  <owl:minCardinality rdf:datatype="http://www.w3.org/2001/XMLSchema#nonNegativeInteger">0</owl:minCardinality>
               </owl:Restriction>
               <owl:Restriction>
                  <owl:onProperty rdf:resource="http://www.opengis.net/citygml/tunnel/2.0#boundedBy"/>
                  <owl:allValuesFrom rdf:resource="http://www.opengis.net/citygml/tunnel/2.0#BoundarySurfacePropertyType"/>
               </owl:Restriction>
               <owl:Restriction>
                  <owl:onProperty rdf:resource="http://www.opengis.net/citygml/tunnel/2.0#boundedBy"/>
                  <owl:minCardinality rdf:datatype="http://www.w3.org/2001/XMLSchema#nonNegativeInteger">0</owl:minCardinality>
               </owl:Restriction>
               <owl:Restriction>
                  <owl:onProperty rdf:resource="http://www.opengis.net/citygml/tunnel/2.0#has_GenericApplicationPropertyOfTunnelInstallation"/>
                  <owl:allValuesFrom rdf:resource="http://www.opengis.net/citygml/tunnel/2.0#_GenericApplicationPropertyOfTunnelInstallation"/>
               </owl:Restriction>
               <owl:Restriction>
                  <owl:onProperty rdf:resource="http://www.opengis.net/citygml/tunnel/2.0#has_GenericApplicationPropertyOfTunnelInstallation"/>
                  <owl:minCardinality rdf:datatype="http://www.w3.org/2001/XMLSchema#nonNegativeInteger">0</owl:minCardinality>
               </owl:Restriction>
            </owl:intersectionOf>
         </owl:Class>
      </owl:equivalentClass>
      <rdfs:subClassOf rdf:resource="http://www.opengis.net/citygml/2.0#AbstractCityObjectType"/>
      <rdfs:comment>Warning: The parent class 'core:AbstractCityObjectType' is declared outside of this class' original schema. This class may be declared incorrectly.</rdfs:comment>
   </owl:Class>
   <owl:Class rdf:about="http://www.opengis.net/citygml/tunnel/2.0#TunnelInstallationPropertyType">
      <rdfs:comment>Denotes the relation of a Tunnel to its external installations. The TunnelInstallationPropertyType element
				must either carry a reference to a TunnelInstallation object or contain a TunnelInstallation object inline, but neither
				both nor none. </rdfs:comment>
      <owl:equivalentClass>
         <owl:Class>
            <owl:intersectionOf rdf:parseType="Collection">
               <owl:Restriction>
                  <owl:onProperty rdf:resource="http://www.opengis.net/citygml/tunnel/2.0#hasTunnelInstallation"/>
                  <owl:allValuesFrom rdf:resource="http://www.opengis.net/citygml/tunnel/2.0#TunnelInstallation"/>
               </owl:Restriction>
            </owl:intersectionOf>
         </owl:Class>
      </owl:equivalentClass>
   </owl:Class>
   <owl:Class rdf:about="http://www.opengis.net/citygml/tunnel/2.0#IntTunnelInstallationType">
      <rdfs:comment>Immovable interior structural component of a Tunnel or a HollowSpace. Examples are interior stairs,
				railings, radiators or pipes. As subclass of _CityObject, an IntTunnelInstallation inherits all attributes and relations,
				in particular an id, names, external references, and generalization relations. </rdfs:comment>
      <owl:equivalentClass>
         <owl:Class>
            <owl:intersectionOf rdf:parseType="Collection">
               <owl:Restriction>
                  <owl:onProperty rdf:resource="http://www.opengis.net/citygml/tunnel/2.0#class"/>
                  <owl:allValuesFrom rdf:resource="http://www.opengis.net/gml#CodeType"/>
               </owl:Restriction>
               <owl:Restriction>
                  <owl:onProperty rdf:resource="http://www.opengis.net/citygml/tunnel/2.0#class"/>
                  <owl:minCardinality rdf:datatype="http://www.w3.org/2001/XMLSchema#nonNegativeInteger">0</owl:minCardinality>
               </owl:Restriction>
               <owl:Restriction>
                  <owl:onProperty rdf:resource="http://www.opengis.net/citygml/tunnel/2.0#function"/>
                  <owl:allValuesFrom rdf:resource="http://www.opengis.net/gml#CodeType"/>
               </owl:Restriction>
               <owl:Restriction>
                  <owl:onProperty rdf:resource="http://www.opengis.net/citygml/tunnel/2.0#function"/>
                  <owl:minCardinality rdf:datatype="http://www.w3.org/2001/XMLSchema#nonNegativeInteger">0</owl:minCardinality>
               </owl:Restriction>
               <owl:Restriction>
                  <owl:onProperty rdf:resource="http://www.opengis.net/citygml/tunnel/2.0#usage"/>
                  <owl:allValuesFrom rdf:resource="http://www.opengis.net/gml#CodeType"/>
               </owl:Restriction>
               <owl:Restriction>
                  <owl:onProperty rdf:resource="http://www.opengis.net/citygml/tunnel/2.0#usage"/>
                  <owl:minCardinality rdf:datatype="http://www.w3.org/2001/XMLSchema#nonNegativeInteger">0</owl:minCardinality>
               </owl:Restriction>
               <owl:Restriction>
                  <owl:onProperty rdf:resource="http://www.opengis.net/citygml/tunnel/2.0#lod4Geometry"/>
                  <owl:allValuesFrom rdf:resource="http://www.opengis.net/gml#GeometryPropertyType"/>
               </owl:Restriction>
               <owl:Restriction>
                  <owl:onProperty rdf:resource="http://www.opengis.net/citygml/tunnel/2.0#lod4Geometry"/>
                  <owl:minCardinality rdf:datatype="http://www.w3.org/2001/XMLSchema#nonNegativeInteger">0</owl:minCardinality>
               </owl:Restriction>
               <owl:Restriction>
                  <owl:onProperty rdf:resource="http://www.opengis.net/citygml/tunnel/2.0#lod4ImplicitRepresentation"/>
                  <owl:allValuesFrom rdf:resource="http://www.opengis.net/citygml/2.0#ImplicitRepresentationPropertyType"/>
               </owl:Restriction>
               <owl:Restriction>
                  <owl:onProperty rdf:resource="http://www.opengis.net/citygml/tunnel/2.0#lod4ImplicitRepresentation"/>
                  <owl:minCardinality rdf:datatype="http://www.w3.org/2001/XMLSchema#nonNegativeInteger">0</owl:minCardinality>
               </owl:Restriction>
               <owl:Restriction>
                  <owl:onProperty rdf:resource="http://www.opengis.net/citygml/tunnel/2.0#boundedBy"/>
                  <owl:allValuesFrom rdf:resource="http://www.opengis.net/citygml/tunnel/2.0#BoundarySurfacePropertyType"/>
               </owl:Restriction>
               <owl:Restriction>
                  <owl:onProperty rdf:resource="http://www.opengis.net/citygml/tunnel/2.0#boundedBy"/>
                  <owl:minCardinality rdf:datatype="http://www.w3.org/2001/XMLSchema#nonNegativeInteger">0</owl:minCardinality>
               </owl:Restriction>
               <owl:Restriction>
                  <owl:onProperty rdf:resource="http://www.opengis.net/citygml/tunnel/2.0#has_GenericApplicationPropertyOfIntTunnelInstallation"/>
                  <owl:allValuesFrom rdf:resource="http://www.opengis.net/citygml/tunnel/2.0#_GenericApplicationPropertyOfIntTunnelInstallation"/>
               </owl:Restriction>
               <owl:Restriction>
                  <owl:onProperty rdf:resource="http://www.opengis.net/citygml/tunnel/2.0#has_GenericApplicationPropertyOfIntTunnelInstallation"/>
                  <owl:minCardinality rdf:datatype="http://www.w3.org/2001/XMLSchema#nonNegativeInteger">0</owl:minCardinality>
               </owl:Restriction>
            </owl:intersectionOf>
         </owl:Class>
      </owl:equivalentClass>
      <rdfs:subClassOf rdf:resource="http://www.opengis.net/citygml/2.0#AbstractCityObjectType"/>
      <rdfs:comment>Warning: The parent class 'core:AbstractCityObjectType' is declared outside of this class' original schema. This class may be declared incorrectly.</rdfs:comment>
   </owl:Class>
   <owl:Class rdf:about="http://www.opengis.net/citygml/tunnel/2.0#IntTunnelInstallationPropertyType">
      <rdfs:comment>Denotes the relation of a Tunnel to its internal installations. The InteriorTunnelInstallationPropertyType
				element must either carry a reference to a IntTunnelInstallation object or contain a IntTunnelInstallation object inline,
				but neither both nor none. </rdfs:comment>
      <owl:equivalentClass>
         <owl:Class>
            <owl:intersectionOf rdf:parseType="Collection">
               <owl:Restriction>
                  <owl:onProperty rdf:resource="http://www.opengis.net/citygml/tunnel/2.0#hasIntTunnelInstallation"/>
                  <owl:allValuesFrom rdf:resource="http://www.opengis.net/citygml/tunnel/2.0#IntTunnelInstallation"/>
               </owl:Restriction>
            </owl:intersectionOf>
         </owl:Class>
      </owl:equivalentClass>
   </owl:Class>
   <owl:Class rdf:about="http://www.opengis.net/citygml/tunnel/2.0#BoundarySurfacePropertyType">
      <rdfs:comment>Denotes the relation of an tunnel or hollow space to its bounding thematic surfaces (walls, roofs, ..).
				There is no differentiation between interior surfaces bounding hollow spaces and outer ones bounding tunnels (one reason
				is, that ClosureSurface belongs to both types). It has to be made sure by additional integrity constraints that, e.g. a
				tunnel is not related to CeilingSurfaces or a room not to RoofSurfaces. </rdfs:comment>
      <owl:equivalentClass>
         <owl:Class>
            <owl:intersectionOf rdf:parseType="Collection">
               <owl:Restriction>
                  <owl:onProperty rdf:resource="http://www.opengis.net/citygml/tunnel/2.0#has_BoundarySurface"/>
                  <owl:allValuesFrom rdf:resource="http://www.opengis.net/citygml/tunnel/2.0#_BoundarySurface"/>
               </owl:Restriction>
            </owl:intersectionOf>
         </owl:Class>
      </owl:equivalentClass>
   </owl:Class>
   <owl:Class rdf:about="http://www.opengis.net/citygml/tunnel/2.0#AbstractBoundarySurfaceType">
      <rdfs:comment>This is an abstract class</rdfs:comment>
      <rdfs:comment>Abstract super class of the features RoofSurface, WallSurface, GroundSurface, ClosureSurface,
				FloorSurface, OuterFloorSurface, CeilingSurface and OuterCeilingSurface</rdfs:comment>
      <owl:equivalentClass>
         <owl:Class>
            <owl:intersectionOf rdf:parseType="Collection">
               <owl:Restriction>
                  <owl:onProperty rdf:resource="http://www.opengis.net/citygml/tunnel/2.0#lod2MultiSurface"/>
                  <owl:allValuesFrom rdf:resource="http://www.opengis.net/gml#MultiSurfacePropertyType"/>
               </owl:Restriction>
               <owl:Restriction>
                  <owl:onProperty rdf:resource="http://www.opengis.net/citygml/tunnel/2.0#lod2MultiSurface"/>
                  <owl:minCardinality rdf:datatype="http://www.w3.org/2001/XMLSchema#nonNegativeInteger">0</owl:minCardinality>
               </owl:Restriction>
               <owl:Restriction>
                  <owl:onProperty rdf:resource="http://www.opengis.net/citygml/tunnel/2.0#lod3MultiSurface"/>
                  <owl:allValuesFrom rdf:resource="http://www.opengis.net/gml#MultiSurfacePropertyType"/>
               </owl:Restriction>
               <owl:Restriction>
                  <owl:onProperty rdf:resource="http://www.opengis.net/citygml/tunnel/2.0#lod3MultiSurface"/>
                  <owl:minCardinality rdf:datatype="http://www.w3.org/2001/XMLSchema#nonNegativeInteger">0</owl:minCardinality>
               </owl:Restriction>
               <owl:Restriction>
                  <owl:onProperty rdf:resource="http://www.opengis.net/citygml/tunnel/2.0#lod4MultiSurface"/>
                  <owl:allValuesFrom rdf:resource="http://www.opengis.net/gml#MultiSurfacePropertyType"/>
               </owl:Restriction>
               <owl:Restriction>
                  <owl:onProperty rdf:resource="http://www.opengis.net/citygml/tunnel/2.0#lod4MultiSurface"/>
                  <owl:minCardinality rdf:datatype="http://www.w3.org/2001/XMLSchema#nonNegativeInteger">0</owl:minCardinality>
               </owl:Restriction>
               <owl:Restriction>
                  <owl:onProperty rdf:resource="http://www.opengis.net/citygml/tunnel/2.0#opening"/>
                  <owl:allValuesFrom rdf:resource="http://www.opengis.net/citygml/tunnel/2.0#OpeningPropertyType"/>
               </owl:Restriction>
               <owl:Restriction>
                  <owl:onProperty rdf:resource="http://www.opengis.net/citygml/tunnel/2.0#opening"/>
                  <owl:minCardinality rdf:datatype="http://www.w3.org/2001/XMLSchema#nonNegativeInteger">0</owl:minCardinality>
               </owl:Restriction>
               <owl:Restriction>
                  <owl:onProperty rdf:resource="http://www.opengis.net/citygml/tunnel/2.0#has_GenericApplicationPropertyOfBoundarySurface"/>
                  <owl:allValuesFrom rdf:resource="http://www.opengis.net/citygml/tunnel/2.0#_GenericApplicationPropertyOfBoundarySurface"/>
               </owl:Restriction>
               <owl:Restriction>
                  <owl:onProperty rdf:resource="http://www.opengis.net/citygml/tunnel/2.0#has_GenericApplicationPropertyOfBoundarySurface"/>
                  <owl:minCardinality rdf:datatype="http://www.w3.org/2001/XMLSchema#nonNegativeInteger">0</owl:minCardinality>
               </owl:Restriction>
            </owl:intersectionOf>
         </owl:Class>
      </owl:equivalentClass>
      <rdfs:subClassOf rdf:resource="http://www.opengis.net/citygml/2.0#AbstractCityObjectType"/>
      <rdfs:comment>Warning: The parent class 'core:AbstractCityObjectType' is declared outside of this class' original schema. This class may be declared incorrectly.</rdfs:comment>
   </owl:Class>
   <owl:Class rdf:about="http://www.opengis.net/citygml/tunnel/2.0#RoofSurfaceType">
      <rdfs:comment>Construction that separates the interior part of the Tunnel from the ambient medium ( water, air, ..) from
				above.</rdfs:comment>
      <owl:equivalentClass>
         <owl:Class>
            <owl:intersectionOf rdf:parseType="Collection">
               <owl:Restriction>
                  <owl:onProperty rdf:resource="http://www.opengis.net/citygml/tunnel/2.0#has_GenericApplicationPropertyOfRoofSurface"/>
                  <owl:allValuesFrom rdf:resource="http://www.opengis.net/citygml/tunnel/2.0#_GenericApplicationPropertyOfRoofSurface"/>
               </owl:Restriction>
               <owl:Restriction>
                  <owl:onProperty rdf:resource="http://www.opengis.net/citygml/tunnel/2.0#has_GenericApplicationPropertyOfRoofSurface"/>
                  <owl:minCardinality rdf:datatype="http://www.w3.org/2001/XMLSchema#nonNegativeInteger">0</owl:minCardinality>
               </owl:Restriction>
            </owl:intersectionOf>
         </owl:Class>
      </owl:equivalentClass>
   </owl:Class>
   <owl:Class rdf:about="http://www.opengis.net/citygml/tunnel/2.0#WallSurfaceType">
      <rdfs:comment>Mainly vertical construction that separates the interior part of the Tunnel from the ambient medium (rock,
				earth, water, air, ..)</rdfs:comment>
      <owl:equivalentClass>
         <owl:Class>
            <owl:intersectionOf rdf:parseType="Collection">
               <owl:Restriction>
                  <owl:onProperty rdf:resource="http://www.opengis.net/citygml/tunnel/2.0#has_GenericApplicationPropertyOfWallSurface"/>
                  <owl:allValuesFrom rdf:resource="http://www.opengis.net/citygml/tunnel/2.0#_GenericApplicationPropertyOfWallSurface"/>
               </owl:Restriction>
               <owl:Restriction>
                  <owl:onProperty rdf:resource="http://www.opengis.net/citygml/tunnel/2.0#has_GenericApplicationPropertyOfWallSurface"/>
                  <owl:minCardinality rdf:datatype="http://www.w3.org/2001/XMLSchema#nonNegativeInteger">0</owl:minCardinality>
               </owl:Restriction>
            </owl:intersectionOf>
         </owl:Class>
      </owl:equivalentClass>
   </owl:Class>
   <owl:Class rdf:about="http://www.opengis.net/citygml/tunnel/2.0#GroundSurfaceType">
      <rdfs:comment>Horizontal construction that separates the interior part of the Tunnel from the ambient medium (rock,
				earth, water, air, ..) from below on the lowest level. </rdfs:comment>
      <owl:equivalentClass>
         <owl:Class>
            <owl:intersectionOf rdf:parseType="Collection">
               <owl:Restriction>
                  <owl:onProperty rdf:resource="http://www.opengis.net/citygml/tunnel/2.0#has_GenericApplicationPropertyOfGroundSurface"/>
                  <owl:allValuesFrom rdf:resource="http://www.opengis.net/citygml/tunnel/2.0#_GenericApplicationPropertyOfGroundSurface"/>
               </owl:Restriction>
               <owl:Restriction>
                  <owl:onProperty rdf:resource="http://www.opengis.net/citygml/tunnel/2.0#has_GenericApplicationPropertyOfGroundSurface"/>
                  <owl:minCardinality rdf:datatype="http://www.w3.org/2001/XMLSchema#nonNegativeInteger">0</owl:minCardinality>
               </owl:Restriction>
            </owl:intersectionOf>
         </owl:Class>
      </owl:equivalentClass>
   </owl:Class>
   <owl:Class rdf:about="http://www.opengis.net/citygml/tunnel/2.0#ClosureSurfaceType">
      <rdfs:comment>Virtual surface which can be used to define the volume of geometric objects being not totally bounded by
				real surfaces (e. g. the entrance of an open Tunnel).</rdfs:comment>
      <owl:equivalentClass>
         <owl:Class>
            <owl:intersectionOf rdf:parseType="Collection">
               <owl:Restriction>
                  <owl:onProperty rdf:resource="http://www.opengis.net/citygml/tunnel/2.0#has_GenericApplicationPropertyOfClosureSurface"/>
                  <owl:allValuesFrom rdf:resource="http://www.opengis.net/citygml/tunnel/2.0#_GenericApplicationPropertyOfClosureSurface"/>
               </owl:Restriction>
               <owl:Restriction>
                  <owl:onProperty rdf:resource="http://www.opengis.net/citygml/tunnel/2.0#has_GenericApplicationPropertyOfClosureSurface"/>
                  <owl:minCardinality rdf:datatype="http://www.w3.org/2001/XMLSchema#nonNegativeInteger">0</owl:minCardinality>
               </owl:Restriction>
            </owl:intersectionOf>
         </owl:Class>
      </owl:equivalentClass>
   </owl:Class>
   <owl:Class rdf:about="http://www.opengis.net/citygml/tunnel/2.0#FloorSurfaceType">
      <rdfs:comment>Mostly horizontal construction that bounds a HollowSpace from below. </rdfs:comment>
      <owl:equivalentClass>
         <owl:Class>
            <owl:intersectionOf rdf:parseType="Collection">
               <owl:Restriction>
                  <owl:onProperty rdf:resource="http://www.opengis.net/citygml/tunnel/2.0#has_GenericApplicationPropertyOfFloorSurface"/>
                  <owl:allValuesFrom rdf:resource="http://www.opengis.net/citygml/tunnel/2.0#_GenericApplicationPropertyOfFloorSurface"/>
               </owl:Restriction>
               <owl:Restriction>
                  <owl:onProperty rdf:resource="http://www.opengis.net/citygml/tunnel/2.0#has_GenericApplicationPropertyOfFloorSurface"/>
                  <owl:minCardinality rdf:datatype="http://www.w3.org/2001/XMLSchema#nonNegativeInteger">0</owl:minCardinality>
               </owl:Restriction>
            </owl:intersectionOf>
         </owl:Class>
      </owl:equivalentClass>
   </owl:Class>
   <owl:Class rdf:about="http://www.opengis.net/citygml/tunnel/2.0#OuterFloorSurfaceType">
      <rdfs:comment>Horizontal construction that separates the interior part of the Tunnel from the ambient medium (rock,
				earth, water, air, ..) from below.</rdfs:comment>
      <owl:equivalentClass>
         <owl:Class>
            <owl:intersectionOf rdf:parseType="Collection">
               <owl:Restriction>
                  <owl:onProperty rdf:resource="http://www.opengis.net/citygml/tunnel/2.0#has_GenericApplicationPropertyOfOuterFloorSurface"/>
                  <owl:allValuesFrom rdf:resource="http://www.opengis.net/citygml/tunnel/2.0#_GenericApplicationPropertyOfOuterFloorSurface"/>
               </owl:Restriction>
               <owl:Restriction>
                  <owl:onProperty rdf:resource="http://www.opengis.net/citygml/tunnel/2.0#has_GenericApplicationPropertyOfOuterFloorSurface"/>
                  <owl:minCardinality rdf:datatype="http://www.w3.org/2001/XMLSchema#nonNegativeInteger">0</owl:minCardinality>
               </owl:Restriction>
            </owl:intersectionOf>
         </owl:Class>
      </owl:equivalentClass>
   </owl:Class>
   <owl:Class rdf:about="http://www.opengis.net/citygml/tunnel/2.0#InteriorWallSurfaceType">
      <rdfs:comment>Mostly vertical construction that bounds a HollowSpace.</rdfs:comment>
      <owl:equivalentClass>
         <owl:Class>
            <owl:intersectionOf rdf:parseType="Collection">
               <owl:Restriction>
                  <owl:onProperty rdf:resource="http://www.opengis.net/citygml/tunnel/2.0#has_GenericApplicationPropertyOfInteriorWallSurface"/>
                  <owl:allValuesFrom rdf:resource="http://www.opengis.net/citygml/tunnel/2.0#_GenericApplicationPropertyOfInteriorWallSurface"/>
               </owl:Restriction>
               <owl:Restriction>
                  <owl:onProperty rdf:resource="http://www.opengis.net/citygml/tunnel/2.0#has_GenericApplicationPropertyOfInteriorWallSurface"/>
                  <owl:minCardinality rdf:datatype="http://www.w3.org/2001/XMLSchema#nonNegativeInteger">0</owl:minCardinality>
               </owl:Restriction>
            </owl:intersectionOf>
         </owl:Class>
      </owl:equivalentClass>
   </owl:Class>
   <owl:Class rdf:about="http://www.opengis.net/citygml/tunnel/2.0#CeilingSurfaceType">
      <rdfs:comment>Mostly horizontal construction that bounds a HollowSpace from above.</rdfs:comment>
      <owl:equivalentClass>
         <owl:Class>
            <owl:intersectionOf rdf:parseType="Collection">
               <owl:Restriction>
                  <owl:onProperty rdf:resource="http://www.opengis.net/citygml/tunnel/2.0#has_GenericApplicationPropertyOfCeilingSurface"/>
                  <owl:allValuesFrom rdf:resource="http://www.opengis.net/citygml/tunnel/2.0#_GenericApplicationPropertyOfCeilingSurface"/>
               </owl:Restriction>
               <owl:Restriction>
                  <owl:onProperty rdf:resource="http://www.opengis.net/citygml/tunnel/2.0#has_GenericApplicationPropertyOfCeilingSurface"/>
                  <owl:minCardinality rdf:datatype="http://www.w3.org/2001/XMLSchema#nonNegativeInteger">0</owl:minCardinality>
               </owl:Restriction>
            </owl:intersectionOf>
         </owl:Class>
      </owl:equivalentClass>
   </owl:Class>
   <owl:Class rdf:about="http://www.opengis.net/citygml/tunnel/2.0#OuterCeilingSurfaceType">
      <rdfs:comment>Mainly horizontal construction that separates the interior part of the Tunnel from the ambient medium
				(rock, earth, ..) from above.</rdfs:comment>
      <owl:equivalentClass>
         <owl:Class>
            <owl:intersectionOf rdf:parseType="Collection">
               <owl:Restriction>
                  <owl:onProperty rdf:resource="http://www.opengis.net/citygml/tunnel/2.0#has_GenericApplicationPropertyOfOuterCeilingSurface"/>
                  <owl:allValuesFrom rdf:resource="http://www.opengis.net/citygml/tunnel/2.0#_GenericApplicationPropertyOfOuterCeilingSurface"/>
               </owl:Restriction>
               <owl:Restriction>
                  <owl:onProperty rdf:resource="http://www.opengis.net/citygml/tunnel/2.0#has_GenericApplicationPropertyOfOuterCeilingSurface"/>
                  <owl:minCardinality rdf:datatype="http://www.w3.org/2001/XMLSchema#nonNegativeInteger">0</owl:minCardinality>
               </owl:Restriction>
            </owl:intersectionOf>
         </owl:Class>
      </owl:equivalentClass>
   </owl:Class>
   <owl:Class rdf:about="http://www.opengis.net/citygml/tunnel/2.0#HollowSpaceType">
      <rdfs:comment>Area or volume within a Tunnel bounded actually or theoretically </rdfs:comment>
      <owl:equivalentClass>
         <owl:Class>
            <owl:intersectionOf rdf:parseType="Collection">
               <owl:Restriction>
                  <owl:onProperty rdf:resource="http://www.opengis.net/citygml/tunnel/2.0#class"/>
                  <owl:allValuesFrom rdf:resource="http://www.opengis.net/gml#CodeType"/>
               </owl:Restriction>
               <owl:Restriction>
                  <owl:onProperty rdf:resource="http://www.opengis.net/citygml/tunnel/2.0#class"/>
                  <owl:minCardinality rdf:datatype="http://www.w3.org/2001/XMLSchema#nonNegativeInteger">0</owl:minCardinality>
               </owl:Restriction>
               <owl:Restriction>
                  <owl:onProperty rdf:resource="http://www.opengis.net/citygml/tunnel/2.0#function"/>
                  <owl:allValuesFrom rdf:resource="http://www.opengis.net/gml#CodeType"/>
               </owl:Restriction>
               <owl:Restriction>
                  <owl:onProperty rdf:resource="http://www.opengis.net/citygml/tunnel/2.0#function"/>
                  <owl:minCardinality rdf:datatype="http://www.w3.org/2001/XMLSchema#nonNegativeInteger">0</owl:minCardinality>
               </owl:Restriction>
               <owl:Restriction>
                  <owl:onProperty rdf:resource="http://www.opengis.net/citygml/tunnel/2.0#usage"/>
                  <owl:allValuesFrom rdf:resource="http://www.opengis.net/gml#CodeType"/>
               </owl:Restriction>
               <owl:Restriction>
                  <owl:onProperty rdf:resource="http://www.opengis.net/citygml/tunnel/2.0#usage"/>
                  <owl:minCardinality rdf:datatype="http://www.w3.org/2001/XMLSchema#nonNegativeInteger">0</owl:minCardinality>
               </owl:Restriction>
               <owl:Restriction>
                  <owl:onProperty rdf:resource="http://www.opengis.net/citygml/tunnel/2.0#lod4Solid"/>
                  <owl:allValuesFrom rdf:resource="http://www.opengis.net/gml#SolidPropertyType"/>
               </owl:Restriction>
               <owl:Restriction>
                  <owl:onProperty rdf:resource="http://www.opengis.net/citygml/tunnel/2.0#lod4Solid"/>
                  <owl:minCardinality rdf:datatype="http://www.w3.org/2001/XMLSchema#nonNegativeInteger">0</owl:minCardinality>
               </owl:Restriction>
               <owl:Restriction>
                  <owl:onProperty rdf:resource="http://www.opengis.net/citygml/tunnel/2.0#lod4MultiSurface"/>
                  <owl:allValuesFrom rdf:resource="http://www.opengis.net/gml#MultiSurfacePropertyType"/>
               </owl:Restriction>
               <owl:Restriction>
                  <owl:onProperty rdf:resource="http://www.opengis.net/citygml/tunnel/2.0#lod4MultiSurface"/>
                  <owl:minCardinality rdf:datatype="http://www.w3.org/2001/XMLSchema#nonNegativeInteger">0</owl:minCardinality>
               </owl:Restriction>
               <owl:Restriction>
                  <owl:onProperty rdf:resource="http://www.opengis.net/citygml/tunnel/2.0#boundedBy"/>
                  <owl:allValuesFrom rdf:resource="http://www.opengis.net/citygml/tunnel/2.0#BoundarySurfacePropertyType"/>
               </owl:Restriction>
               <owl:Restriction>
                  <owl:onProperty rdf:resource="http://www.opengis.net/citygml/tunnel/2.0#boundedBy"/>
                  <owl:minCardinality rdf:datatype="http://www.w3.org/2001/XMLSchema#nonNegativeInteger">0</owl:minCardinality>
               </owl:Restriction>
               <owl:Restriction>
                  <owl:onProperty rdf:resource="http://www.opengis.net/citygml/tunnel/2.0#interiorFurniture"/>
                  <owl:allValuesFrom rdf:resource="http://www.opengis.net/citygml/tunnel/2.0#InteriorFurniturePropertyType"/>
               </owl:Restriction>
               <owl:Restriction>
                  <owl:onProperty rdf:resource="http://www.opengis.net/citygml/tunnel/2.0#interiorFurniture"/>
                  <owl:minCardinality rdf:datatype="http://www.w3.org/2001/XMLSchema#nonNegativeInteger">0</owl:minCardinality>
               </owl:Restriction>
               <owl:Restriction>
                  <owl:onProperty rdf:resource="http://www.opengis.net/citygml/tunnel/2.0#hollowSpaceInstallation"/>
                  <owl:allValuesFrom rdf:resource="http://www.opengis.net/citygml/tunnel/2.0#IntTunnelInstallationPropertyType"/>
               </owl:Restriction>
               <owl:Restriction>
                  <owl:onProperty rdf:resource="http://www.opengis.net/citygml/tunnel/2.0#hollowSpaceInstallation"/>
                  <owl:minCardinality rdf:datatype="http://www.w3.org/2001/XMLSchema#nonNegativeInteger">0</owl:minCardinality>
               </owl:Restriction>
               <owl:Restriction>
                  <owl:onProperty rdf:resource="http://www.opengis.net/citygml/tunnel/2.0#has_GenericApplicationPropertyOfHollowSpace"/>
                  <owl:allValuesFrom rdf:resource="http://www.opengis.net/citygml/tunnel/2.0#_GenericApplicationPropertyOfHollowSpace"/>
               </owl:Restriction>
               <owl:Restriction>
                  <owl:onProperty rdf:resource="http://www.opengis.net/citygml/tunnel/2.0#has_GenericApplicationPropertyOfHollowSpace"/>
                  <owl:minCardinality rdf:datatype="http://www.w3.org/2001/XMLSchema#nonNegativeInteger">0</owl:minCardinality>
               </owl:Restriction>
            </owl:intersectionOf>
         </owl:Class>
      </owl:equivalentClass>
      <rdfs:subClassOf rdf:resource="http://www.opengis.net/citygml/2.0#AbstractCityObjectType"/>
      <rdfs:comment>Warning: The parent class 'core:AbstractCityObjectType' is declared outside of this class' original schema. This class may be declared incorrectly.</rdfs:comment>
   </owl:Class>
   <owl:Class rdf:about="http://www.opengis.net/citygml/tunnel/2.0#InteriorHollowSpacePropertyType">
      <rdfs:comment>Denotes the relation of a Tunnel to its internal holllow spaces. The InteriorHollowSpacePropertyType
				element must either carry a reference to a HollowSpace object or contain a HollowSpace object inline, but neither both nor
				none. </rdfs:comment>
      <owl:equivalentClass>
         <owl:Class>
            <owl:intersectionOf rdf:parseType="Collection">
               <owl:Restriction>
                  <owl:onProperty rdf:resource="http://www.opengis.net/citygml/tunnel/2.0#hasHollowSpace"/>
                  <owl:allValuesFrom rdf:resource="http://www.opengis.net/citygml/tunnel/2.0#HollowSpace"/>
               </owl:Restriction>
            </owl:intersectionOf>
         </owl:Class>
      </owl:equivalentClass>
   </owl:Class>
   <owl:Class rdf:about="http://www.opengis.net/citygml/tunnel/2.0#TunnelFurnitureType">
      <rdfs:comment>Movable, functional objects, whether useful or ornamental, usually found in a
				HollowSpace</rdfs:comment>
      <owl:equivalentClass>
         <owl:Class>
            <owl:intersectionOf rdf:parseType="Collection">
               <owl:Restriction>
                  <owl:onProperty rdf:resource="http://www.opengis.net/citygml/tunnel/2.0#class"/>
                  <owl:allValuesFrom rdf:resource="http://www.opengis.net/gml#CodeType"/>
               </owl:Restriction>
               <owl:Restriction>
                  <owl:onProperty rdf:resource="http://www.opengis.net/citygml/tunnel/2.0#class"/>
                  <owl:minCardinality rdf:datatype="http://www.w3.org/2001/XMLSchema#nonNegativeInteger">0</owl:minCardinality>
               </owl:Restriction>
               <owl:Restriction>
                  <owl:onProperty rdf:resource="http://www.opengis.net/citygml/tunnel/2.0#function"/>
                  <owl:allValuesFrom rdf:resource="http://www.opengis.net/gml#CodeType"/>
               </owl:Restriction>
               <owl:Restriction>
                  <owl:onProperty rdf:resource="http://www.opengis.net/citygml/tunnel/2.0#function"/>
                  <owl:minCardinality rdf:datatype="http://www.w3.org/2001/XMLSchema#nonNegativeInteger">0</owl:minCardinality>
               </owl:Restriction>
               <owl:Restriction>
                  <owl:onProperty rdf:resource="http://www.opengis.net/citygml/tunnel/2.0#usage"/>
                  <owl:allValuesFrom rdf:resource="http://www.opengis.net/gml#CodeType"/>
               </owl:Restriction>
               <owl:Restriction>
                  <owl:onProperty rdf:resource="http://www.opengis.net/citygml/tunnel/2.0#usage"/>
                  <owl:minCardinality rdf:datatype="http://www.w3.org/2001/XMLSchema#nonNegativeInteger">0</owl:minCardinality>
               </owl:Restriction>
               <owl:Restriction>
                  <owl:onProperty rdf:resource="http://www.opengis.net/citygml/tunnel/2.0#lod4Geometry"/>
                  <owl:allValuesFrom rdf:resource="http://www.opengis.net/gml#GeometryPropertyType"/>
               </owl:Restriction>
               <owl:Restriction>
                  <owl:onProperty rdf:resource="http://www.opengis.net/citygml/tunnel/2.0#lod4Geometry"/>
                  <owl:minCardinality rdf:datatype="http://www.w3.org/2001/XMLSchema#nonNegativeInteger">0</owl:minCardinality>
               </owl:Restriction>
               <owl:Restriction>
                  <owl:onProperty rdf:resource="http://www.opengis.net/citygml/tunnel/2.0#lod4ImplicitRepresentation"/>
                  <owl:allValuesFrom rdf:resource="http://www.opengis.net/citygml/2.0#ImplicitRepresentationPropertyType"/>
               </owl:Restriction>
               <owl:Restriction>
                  <owl:onProperty rdf:resource="http://www.opengis.net/citygml/tunnel/2.0#lod4ImplicitRepresentation"/>
                  <owl:minCardinality rdf:datatype="http://www.w3.org/2001/XMLSchema#nonNegativeInteger">0</owl:minCardinality>
               </owl:Restriction>
               <owl:Restriction>
                  <owl:onProperty rdf:resource="http://www.opengis.net/citygml/tunnel/2.0#has_GenericApplicationPropertyOfTunnelFurniture"/>
                  <owl:allValuesFrom rdf:resource="http://www.opengis.net/citygml/tunnel/2.0#_GenericApplicationPropertyOfTunnelFurniture"/>
               </owl:Restriction>
               <owl:Restriction>
                  <owl:onProperty rdf:resource="http://www.opengis.net/citygml/tunnel/2.0#has_GenericApplicationPropertyOfTunnelFurniture"/>
                  <owl:minCardinality rdf:datatype="http://www.w3.org/2001/XMLSchema#nonNegativeInteger">0</owl:minCardinality>
               </owl:Restriction>
            </owl:intersectionOf>
         </owl:Class>
      </owl:equivalentClass>
      <rdfs:subClassOf rdf:resource="http://www.opengis.net/citygml/2.0#AbstractCityObjectType"/>
      <rdfs:comment>Warning: The parent class 'core:AbstractCityObjectType' is declared outside of this class' original schema. This class may be declared incorrectly.</rdfs:comment>
   </owl:Class>
   <owl:Class rdf:about="http://www.opengis.net/citygml/tunnel/2.0#InteriorFurniturePropertyType">
      <rdfs:comment>Denotes the relation of a hollow space to the furnitures it contains. </rdfs:comment>
      <owl:equivalentClass>
         <owl:Class>
            <owl:intersectionOf rdf:parseType="Collection">
               <owl:Restriction>
                  <owl:onProperty rdf:resource="http://www.opengis.net/citygml/tunnel/2.0#hasTunnelFurniture"/>
                  <owl:allValuesFrom rdf:resource="http://www.opengis.net/citygml/tunnel/2.0#TunnelFurniture"/>
               </owl:Restriction>
            </owl:intersectionOf>
         </owl:Class>
      </owl:equivalentClass>
   </owl:Class>
   <owl:Class rdf:about="http://www.opengis.net/citygml/tunnel/2.0#AbstractOpeningType">
      <rdfs:comment>This is an abstract class</rdfs:comment>
      <rdfs:comment> Type for openings (doors, windows) in boundary surfaces. Used in LOD3 and LOD4 only. As subclass of
				_CityObject, an _Opening inherits all attributes and relations, in particular an id, names, external references, and
				generalization relations. </rdfs:comment>
      <owl:equivalentClass>
         <owl:Class>
            <owl:intersectionOf rdf:parseType="Collection">
               <owl:Restriction>
                  <owl:onProperty rdf:resource="http://www.opengis.net/citygml/tunnel/2.0#lod3MultiSurface"/>
                  <owl:allValuesFrom rdf:resource="http://www.opengis.net/gml#MultiSurfacePropertyType"/>
               </owl:Restriction>
               <owl:Restriction>
                  <owl:onProperty rdf:resource="http://www.opengis.net/citygml/tunnel/2.0#lod3MultiSurface"/>
                  <owl:minCardinality rdf:datatype="http://www.w3.org/2001/XMLSchema#nonNegativeInteger">0</owl:minCardinality>
               </owl:Restriction>
               <owl:Restriction>
                  <owl:onProperty rdf:resource="http://www.opengis.net/citygml/tunnel/2.0#lod4MultiSurface"/>
                  <owl:allValuesFrom rdf:resource="http://www.opengis.net/gml#MultiSurfacePropertyType"/>
               </owl:Restriction>
               <owl:Restriction>
                  <owl:onProperty rdf:resource="http://www.opengis.net/citygml/tunnel/2.0#lod4MultiSurface"/>
                  <owl:minCardinality rdf:datatype="http://www.w3.org/2001/XMLSchema#nonNegativeInteger">0</owl:minCardinality>
               </owl:Restriction>
               <owl:Restriction>
                  <owl:onProperty rdf:resource="http://www.opengis.net/citygml/tunnel/2.0#lod3ImplicitRepresentation"/>
                  <owl:allValuesFrom rdf:resource="http://www.opengis.net/citygml/2.0#ImplicitRepresentationPropertyType"/>
               </owl:Restriction>
               <owl:Restriction>
                  <owl:onProperty rdf:resource="http://www.opengis.net/citygml/tunnel/2.0#lod3ImplicitRepresentation"/>
                  <owl:minCardinality rdf:datatype="http://www.w3.org/2001/XMLSchema#nonNegativeInteger">0</owl:minCardinality>
               </owl:Restriction>
               <owl:Restriction>
                  <owl:onProperty rdf:resource="http://www.opengis.net/citygml/tunnel/2.0#lod4ImplicitRepresentation"/>
                  <owl:allValuesFrom rdf:resource="http://www.opengis.net/citygml/2.0#ImplicitRepresentationPropertyType"/>
               </owl:Restriction>
               <owl:Restriction>
                  <owl:onProperty rdf:resource="http://www.opengis.net/citygml/tunnel/2.0#lod4ImplicitRepresentation"/>
                  <owl:minCardinality rdf:datatype="http://www.w3.org/2001/XMLSchema#nonNegativeInteger">0</owl:minCardinality>
               </owl:Restriction>
               <owl:Restriction>
                  <owl:onProperty rdf:resource="http://www.opengis.net/citygml/tunnel/2.0#has_GenericApplicationPropertyOfOpening"/>
                  <owl:allValuesFrom rdf:resource="http://www.opengis.net/citygml/tunnel/2.0#_GenericApplicationPropertyOfOpening"/>
               </owl:Restriction>
               <owl:Restriction>
                  <owl:onProperty rdf:resource="http://www.opengis.net/citygml/tunnel/2.0#has_GenericApplicationPropertyOfOpening"/>
                  <owl:minCardinality rdf:datatype="http://www.w3.org/2001/XMLSchema#nonNegativeInteger">0</owl:minCardinality>
               </owl:Restriction>
            </owl:intersectionOf>
         </owl:Class>
      </owl:equivalentClass>
      <rdfs:subClassOf rdf:resource="http://www.opengis.net/citygml/2.0#AbstractCityObjectType"/>
      <rdfs:comment>Warning: The parent class 'core:AbstractCityObjectType' is declared outside of this class' original schema. This class may be declared incorrectly.</rdfs:comment>
   </owl:Class>
   <owl:Class rdf:about="http://www.opengis.net/citygml/tunnel/2.0#OpeningPropertyType">
      <rdfs:comment>Denotes the relation of an _BondarySurface to its openings (doors, windows). The OpeningPropertyType
				element must either carry a reference to an _Opening object or contain an _Opening object inline, but neither both nor
				none. </rdfs:comment>
      <owl:equivalentClass>
         <owl:Class>
            <owl:intersectionOf rdf:parseType="Collection">
               <owl:Restriction>
                  <owl:onProperty rdf:resource="http://www.opengis.net/citygml/tunnel/2.0#has_Opening"/>
                  <owl:allValuesFrom rdf:resource="http://www.opengis.net/citygml/tunnel/2.0#_Opening"/>
               </owl:Restriction>
            </owl:intersectionOf>
         </owl:Class>
      </owl:equivalentClass>
   </owl:Class>
   <owl:Class rdf:about="http://www.opengis.net/citygml/tunnel/2.0#WindowType">
      <rdfs:comment>Construction for closing an _Opening not intended for access or regress.</rdfs:comment>
      <owl:equivalentClass>
         <owl:Class>
            <owl:intersectionOf rdf:parseType="Collection">
               <owl:Restriction>
                  <owl:onProperty rdf:resource="http://www.opengis.net/citygml/tunnel/2.0#has_GenericApplicationPropertyOfWindow"/>
                  <owl:allValuesFrom rdf:resource="http://www.opengis.net/citygml/tunnel/2.0#_GenericApplicationPropertyOfWindow"/>
               </owl:Restriction>
               <owl:Restriction>
                  <owl:onProperty rdf:resource="http://www.opengis.net/citygml/tunnel/2.0#has_GenericApplicationPropertyOfWindow"/>
                  <owl:minCardinality rdf:datatype="http://www.w3.org/2001/XMLSchema#nonNegativeInteger">0</owl:minCardinality>
               </owl:Restriction>
            </owl:intersectionOf>
         </owl:Class>
      </owl:equivalentClass>
   </owl:Class>
   <owl:Class rdf:about="http://www.opengis.net/citygml/tunnel/2.0#DoorType">
      <rdfs:comment>Construction for closing an _Opening intended primarily for access or regress or both. </rdfs:comment>
      <owl:equivalentClass>
         <owl:Class>
            <owl:intersectionOf rdf:parseType="Collection">
               <owl:Restriction>
                  <owl:onProperty rdf:resource="http://www.opengis.net/citygml/tunnel/2.0#has_GenericApplicationPropertyOfDoor"/>
                  <owl:allValuesFrom rdf:resource="http://www.opengis.net/citygml/tunnel/2.0#_GenericApplicationPropertyOfDoor"/>
               </owl:Restriction>
               <owl:Restriction>
                  <owl:onProperty rdf:resource="http://www.opengis.net/citygml/tunnel/2.0#has_GenericApplicationPropertyOfDoor"/>
                  <owl:minCardinality rdf:datatype="http://www.w3.org/2001/XMLSchema#nonNegativeInteger">0</owl:minCardinality>
               </owl:Restriction>
            </owl:intersectionOf>
         </owl:Class>
      </owl:equivalentClass>
   </owl:Class>
   <owl:ObjectProperty rdf:about="http://www.opengis.net/gml#hasAssociationAttributeGroup">
      <rdfs:domain rdf:resource="http://www.opengis.net/citygml/tunnel/2.0#TunnelPartPropertyType"/>
      <rdfs:range rdf:resource="http://www.opengis.net/gml#AssociationAttributeGroup"/>
   </owl:ObjectProperty>
   <owl:ObjectProperty rdf:about="http://www.opengis.net/gml#hasAssociationAttributeGroup">
      <rdfs:domain rdf:resource="http://www.opengis.net/citygml/tunnel/2.0#TunnelInstallationPropertyType"/>
      <rdfs:range rdf:resource="http://www.opengis.net/gml#AssociationAttributeGroup"/>
   </owl:ObjectProperty>
   <owl:ObjectProperty rdf:about="http://www.opengis.net/gml#hasAssociationAttributeGroup">
      <rdfs:domain rdf:resource="http://www.opengis.net/citygml/tunnel/2.0#IntTunnelInstallationPropertyType"/>
      <rdfs:range rdf:resource="http://www.opengis.net/gml#AssociationAttributeGroup"/>
   </owl:ObjectProperty>
   <owl:ObjectProperty rdf:about="http://www.opengis.net/gml#hasAssociationAttributeGroup">
      <rdfs:domain rdf:resource="http://www.opengis.net/citygml/tunnel/2.0#BoundarySurfacePropertyType"/>
      <rdfs:range rdf:resource="http://www.opengis.net/gml#AssociationAttributeGroup"/>
   </owl:ObjectProperty>
   <owl:ObjectProperty rdf:about="http://www.opengis.net/gml#hasAssociationAttributeGroup">
      <rdfs:domain rdf:resource="http://www.opengis.net/citygml/tunnel/2.0#InteriorHollowSpacePropertyType"/>
      <rdfs:range rdf:resource="http://www.opengis.net/gml#AssociationAttributeGroup"/>
   </owl:ObjectProperty>
   <owl:ObjectProperty rdf:about="http://www.opengis.net/gml#hasAssociationAttributeGroup">
      <rdfs:domain rdf:resource="http://www.opengis.net/citygml/tunnel/2.0#InteriorFurniturePropertyType"/>
      <rdfs:range rdf:resource="http://www.opengis.net/gml#AssociationAttributeGroup"/>
   </owl:ObjectProperty>
   <owl:ObjectProperty rdf:about="http://www.opengis.net/gml#hasAssociationAttributeGroup">
      <rdfs:domain rdf:resource="http://www.opengis.net/citygml/tunnel/2.0#OpeningPropertyType"/>
      <rdfs:range rdf:resource="http://www.opengis.net/gml#AssociationAttributeGroup"/>
   </owl:ObjectProperty>
   <owl:Class rdf:about="http://www.opengis.net/citygml/tunnel/2.0#_AbstractTunnel">
      <rdfs:subClassOf rdf:resource="http://www.opengis.net/citygml/2.0#_Site"/>
      <rdfs:subClassOf rdf:resource="http://www.opengis.net/citygml/tunnel/2.0#AbstractTunnelType"/>
   </owl:Class>
   <owl:Class rdf:about="http://www.opengis.net/citygml/tunnel/2.0#_GenericApplicationPropertyOfAbstractTunnel">
      <rdfs:subClassOf rdf:resource="http://www.w3.org/2001/XMLSchema#anyType"/>
      <rdfs:comment>Warning: This class type was declared outside of its original schema. This class may be declared incorrectly.</rdfs:comment>
   </owl:Class>
   <owl:Class rdf:about="http://www.opengis.net/citygml/tunnel/2.0#Tunnel">
      <rdfs:subClassOf rdf:resource="http://www.opengis.net/citygml/tunnel/2.0#_AbstractTunnel"/>
      <rdfs:subClassOf rdf:resource="http://www.opengis.net/citygml/tunnel/2.0#TunnelType"/>
   </owl:Class>
   <owl:Class rdf:about="http://www.opengis.net/citygml/tunnel/2.0#_GenericApplicationPropertyOfTunnel">
      <rdfs:subClassOf rdf:resource="http://www.w3.org/2001/XMLSchema#anyType"/>
      <rdfs:comment>Warning: This class type was declared outside of its original schema. This class may be declared incorrectly.</rdfs:comment>
   </owl:Class>
   <owl:Class rdf:about="http://www.opengis.net/citygml/tunnel/2.0#TunnelPart">
      <rdfs:subClassOf rdf:resource="http://www.opengis.net/citygml/tunnel/2.0#_AbstractTunnel"/>
      <rdfs:subClassOf rdf:resource="http://www.opengis.net/citygml/tunnel/2.0#TunnelPartType"/>
   </owl:Class>
   <owl:Class rdf:about="http://www.opengis.net/citygml/tunnel/2.0#_GenericApplicationPropertyOfTunnelPart">
      <rdfs:subClassOf rdf:resource="http://www.w3.org/2001/XMLSchema#anyType"/>
      <rdfs:comment>Warning: This class type was declared outside of its original schema. This class may be declared incorrectly.</rdfs:comment>
   </owl:Class>
   <owl:Class rdf:about="http://www.opengis.net/citygml/tunnel/2.0#TunnelInstallation">
      <rdfs:subClassOf rdf:resource="http://www.opengis.net/citygml/2.0#_CityObject"/>
      <rdfs:subClassOf rdf:resource="http://www.opengis.net/citygml/tunnel/2.0#TunnelInstallationType"/>
   </owl:Class>
   <owl:Class rdf:about="http://www.opengis.net/citygml/tunnel/2.0#_GenericApplicationPropertyOfTunnelInstallation">
      <rdfs:subClassOf rdf:resource="http://www.w3.org/2001/XMLSchema#anyType"/>
      <rdfs:comment>Warning: This class type was declared outside of its original schema. This class may be declared incorrectly.</rdfs:comment>
   </owl:Class>
   <owl:Class rdf:about="http://www.opengis.net/citygml/tunnel/2.0#IntTunnelInstallation">
      <rdfs:subClassOf rdf:resource="http://www.opengis.net/citygml/2.0#_CityObject"/>
      <rdfs:subClassOf rdf:resource="http://www.opengis.net/citygml/tunnel/2.0#IntTunnelInstallationType"/>
   </owl:Class>
   <owl:Class rdf:about="http://www.opengis.net/citygml/tunnel/2.0#_GenericApplicationPropertyOfIntTunnelInstallation">
      <rdfs:subClassOf rdf:resource="http://www.w3.org/2001/XMLSchema#anyType"/>
      <rdfs:comment>Warning: This class type was declared outside of its original schema. This class may be declared incorrectly.</rdfs:comment>
   </owl:Class>
   <owl:Class rdf:about="http://www.opengis.net/citygml/tunnel/2.0#_BoundarySurface">
      <rdfs:subClassOf rdf:resource="http://www.opengis.net/citygml/2.0#_CityObject"/>
      <rdfs:subClassOf rdf:resource="http://www.opengis.net/citygml/tunnel/2.0#AbstractBoundarySurfaceType"/>
   </owl:Class>
   <owl:Class rdf:about="http://www.opengis.net/citygml/tunnel/2.0#_GenericApplicationPropertyOfBoundarySurface">
      <rdfs:subClassOf rdf:resource="http://www.w3.org/2001/XMLSchema#anyType"/>
      <rdfs:comment>Warning: This class type was declared outside of its original schema. This class may be declared incorrectly.</rdfs:comment>
   </owl:Class>
   <owl:Class rdf:about="http://www.opengis.net/citygml/tunnel/2.0#RoofSurface">
      <rdfs:subClassOf rdf:resource="http://www.opengis.net/citygml/tunnel/2.0#_BoundarySurface"/>
      <rdfs:subClassOf rdf:resource="http://www.opengis.net/citygml/tunnel/2.0#RoofSurfaceType"/>
   </owl:Class>
   <owl:Class rdf:about="http://www.opengis.net/citygml/tunnel/2.0#_GenericApplicationPropertyOfRoofSurface">
      <rdfs:subClassOf rdf:resource="http://www.w3.org/2001/XMLSchema#anyType"/>
      <rdfs:comment>Warning: This class type was declared outside of its original schema. This class may be declared incorrectly.</rdfs:comment>
   </owl:Class>
   <owl:Class rdf:about="http://www.opengis.net/citygml/tunnel/2.0#WallSurface">
      <rdfs:subClassOf rdf:resource="http://www.opengis.net/citygml/tunnel/2.0#_BoundarySurface"/>
      <rdfs:subClassOf rdf:resource="http://www.opengis.net/citygml/tunnel/2.0#WallSurfaceType"/>
   </owl:Class>
   <owl:Class rdf:about="http://www.opengis.net/citygml/tunnel/2.0#_GenericApplicationPropertyOfWallSurface">
      <rdfs:subClassOf rdf:resource="http://www.w3.org/2001/XMLSchema#anyType"/>
      <rdfs:comment>Warning: This class type was declared outside of its original schema. This class may be declared incorrectly.</rdfs:comment>
   </owl:Class>
   <owl:Class rdf:about="http://www.opengis.net/citygml/tunnel/2.0#GroundSurface">
      <rdfs:subClassOf rdf:resource="http://www.opengis.net/citygml/tunnel/2.0#_BoundarySurface"/>
      <rdfs:subClassOf rdf:resource="http://www.opengis.net/citygml/tunnel/2.0#GroundSurfaceType"/>
   </owl:Class>
   <owl:Class rdf:about="http://www.opengis.net/citygml/tunnel/2.0#_GenericApplicationPropertyOfGroundSurface">
      <rdfs:subClassOf rdf:resource="http://www.w3.org/2001/XMLSchema#anyType"/>
      <rdfs:comment>Warning: This class type was declared outside of its original schema. This class may be declared incorrectly.</rdfs:comment>
   </owl:Class>
   <owl:Class rdf:about="http://www.opengis.net/citygml/tunnel/2.0#ClosureSurface">
      <rdfs:subClassOf rdf:resource="http://www.opengis.net/citygml/tunnel/2.0#_BoundarySurface"/>
      <rdfs:subClassOf rdf:resource="http://www.opengis.net/citygml/tunnel/2.0#ClosureSurfaceType"/>
   </owl:Class>
   <owl:Class rdf:about="http://www.opengis.net/citygml/tunnel/2.0#_GenericApplicationPropertyOfClosureSurface">
      <rdfs:subClassOf rdf:resource="http://www.w3.org/2001/XMLSchema#anyType"/>
      <rdfs:comment>Warning: This class type was declared outside of its original schema. This class may be declared incorrectly.</rdfs:comment>
   </owl:Class>
   <owl:Class rdf:about="http://www.opengis.net/citygml/tunnel/2.0#FloorSurface">
      <rdfs:subClassOf rdf:resource="http://www.opengis.net/citygml/tunnel/2.0#_BoundarySurface"/>
      <rdfs:subClassOf rdf:resource="http://www.opengis.net/citygml/tunnel/2.0#FloorSurfaceType"/>
   </owl:Class>
   <owl:Class rdf:about="http://www.opengis.net/citygml/tunnel/2.0#_GenericApplicationPropertyOfFloorSurface">
      <rdfs:subClassOf rdf:resource="http://www.w3.org/2001/XMLSchema#anyType"/>
      <rdfs:comment>Warning: This class type was declared outside of its original schema. This class may be declared incorrectly.</rdfs:comment>
   </owl:Class>
   <owl:Class rdf:about="http://www.opengis.net/citygml/tunnel/2.0#OuterFloorSurface">
      <rdfs:subClassOf rdf:resource="http://www.opengis.net/citygml/tunnel/2.0#_BoundarySurface"/>
      <rdfs:subClassOf rdf:resource="http://www.opengis.net/citygml/tunnel/2.0#OuterFloorSurfaceType"/>
   </owl:Class>
   <owl:Class rdf:about="http://www.opengis.net/citygml/tunnel/2.0#_GenericApplicationPropertyOfOuterFloorSurface">
      <rdfs:subClassOf rdf:resource="http://www.w3.org/2001/XMLSchema#anyType"/>
      <rdfs:comment>Warning: This class type was declared outside of its original schema. This class may be declared incorrectly.</rdfs:comment>
   </owl:Class>
   <owl:Class rdf:about="http://www.opengis.net/citygml/tunnel/2.0#InteriorWallSurface">
      <rdfs:subClassOf rdf:resource="http://www.opengis.net/citygml/tunnel/2.0#_BoundarySurface"/>
      <rdfs:subClassOf rdf:resource="http://www.opengis.net/citygml/tunnel/2.0#InteriorWallSurfaceType"/>
   </owl:Class>
   <owl:Class rdf:about="http://www.opengis.net/citygml/tunnel/2.0#_GenericApplicationPropertyOfInteriorWallSurface">
      <rdfs:subClassOf rdf:resource="http://www.w3.org/2001/XMLSchema#anyType"/>
      <rdfs:comment>Warning: This class type was declared outside of its original schema. This class may be declared incorrectly.</rdfs:comment>
   </owl:Class>
   <owl:Class rdf:about="http://www.opengis.net/citygml/tunnel/2.0#CeilingSurface">
      <rdfs:subClassOf rdf:resource="http://www.opengis.net/citygml/tunnel/2.0#_BoundarySurface"/>
      <rdfs:subClassOf rdf:resource="http://www.opengis.net/citygml/tunnel/2.0#CeilingSurfaceType"/>
   </owl:Class>
   <owl:Class rdf:about="http://www.opengis.net/citygml/tunnel/2.0#_GenericApplicationPropertyOfCeilingSurface">
      <rdfs:subClassOf rdf:resource="http://www.w3.org/2001/XMLSchema#anyType"/>
      <rdfs:comment>Warning: This class type was declared outside of its original schema. This class may be declared incorrectly.</rdfs:comment>
   </owl:Class>
   <owl:Class rdf:about="http://www.opengis.net/citygml/tunnel/2.0#OuterCeilingSurface">
      <rdfs:subClassOf rdf:resource="http://www.opengis.net/citygml/tunnel/2.0#_BoundarySurface"/>
      <rdfs:subClassOf rdf:resource="http://www.opengis.net/citygml/tunnel/2.0#OuterCeilingSurfaceType"/>
   </owl:Class>
   <owl:Class rdf:about="http://www.opengis.net/citygml/tunnel/2.0#_GenericApplicationPropertyOfOuterCeilingSurface">
      <rdfs:subClassOf rdf:resource="http://www.w3.org/2001/XMLSchema#anyType"/>
      <rdfs:comment>Warning: This class type was declared outside of its original schema. This class may be declared incorrectly.</rdfs:comment>
   </owl:Class>
   <owl:Class rdf:about="http://www.opengis.net/citygml/tunnel/2.0#HollowSpace">
      <rdfs:subClassOf rdf:resource="http://www.opengis.net/citygml/2.0#_CityObject"/>
      <rdfs:subClassOf rdf:resource="http://www.opengis.net/citygml/tunnel/2.0#HollowSpaceType"/>
   </owl:Class>
   <owl:Class rdf:about="http://www.opengis.net/citygml/tunnel/2.0#_GenericApplicationPropertyOfHollowSpace">
      <rdfs:subClassOf rdf:resource="http://www.w3.org/2001/XMLSchema#anyType"/>
      <rdfs:comment>Warning: This class type was declared outside of its original schema. This class may be declared incorrectly.</rdfs:comment>
   </owl:Class>
   <owl:Class rdf:about="http://www.opengis.net/citygml/tunnel/2.0#TunnelFurniture">
      <rdfs:subClassOf rdf:resource="http://www.opengis.net/citygml/2.0#_CityObject"/>
      <rdfs:subClassOf rdf:resource="http://www.opengis.net/citygml/tunnel/2.0#TunnelFurnitureType"/>
   </owl:Class>
   <owl:Class rdf:about="http://www.opengis.net/citygml/tunnel/2.0#_GenericApplicationPropertyOfTunnelFurniture">
      <rdfs:subClassOf rdf:resource="http://www.w3.org/2001/XMLSchema#anyType"/>
      <rdfs:comment>Warning: This class type was declared outside of its original schema. This class may be declared incorrectly.</rdfs:comment>
   </owl:Class>
   <owl:Class rdf:about="http://www.opengis.net/citygml/tunnel/2.0#_Opening">
      <rdfs:subClassOf rdf:resource="http://www.opengis.net/citygml/2.0#_CityObject"/>
      <rdfs:subClassOf rdf:resource="http://www.opengis.net/citygml/tunnel/2.0#AbstractOpeningType"/>
   </owl:Class>
   <owl:Class rdf:about="http://www.opengis.net/citygml/tunnel/2.0#_GenericApplicationPropertyOfOpening">
      <rdfs:subClassOf rdf:resource="http://www.w3.org/2001/XMLSchema#anyType"/>
      <rdfs:comment>Warning: This class type was declared outside of its original schema. This class may be declared incorrectly.</rdfs:comment>
   </owl:Class>
   <owl:Class rdf:about="http://www.opengis.net/citygml/tunnel/2.0#Window">
      <rdfs:subClassOf rdf:resource="http://www.opengis.net/citygml/tunnel/2.0#_Opening"/>
      <rdfs:subClassOf rdf:resource="http://www.opengis.net/citygml/tunnel/2.0#WindowType"/>
   </owl:Class>
   <owl:Class rdf:about="http://www.opengis.net/citygml/tunnel/2.0#_GenericApplicationPropertyOfWindow">
      <rdfs:subClassOf rdf:resource="http://www.w3.org/2001/XMLSchema#anyType"/>
      <rdfs:comment>Warning: This class type was declared outside of its original schema. This class may be declared incorrectly.</rdfs:comment>
   </owl:Class>
   <owl:Class rdf:about="http://www.opengis.net/citygml/tunnel/2.0#Door">
      <rdfs:subClassOf rdf:resource="http://www.opengis.net/citygml/tunnel/2.0#_Opening"/>
      <rdfs:subClassOf rdf:resource="http://www.opengis.net/citygml/tunnel/2.0#DoorType"/>
   </owl:Class>
   <owl:Class rdf:about="http://www.opengis.net/citygml/tunnel/2.0#_GenericApplicationPropertyOfDoor">
      <rdfs:subClassOf rdf:resource="http://www.w3.org/2001/XMLSchema#anyType"/>
      <rdfs:comment>Warning: This class type was declared outside of its original schema. This class may be declared incorrectly.</rdfs:comment>
   </owl:Class>
   <owl:ObjectProperty rdf:about="http://www.opengis.net/citygml/tunnel/2.0#class">
      <rdfs:comment>Warning: This ObjectProperty type was declared outside of its original schema. This ObjectProperty may be declared incorrectly.</rdfs:comment>
      <rdfs:domain rdf:resource="http://www.opengis.net/citygml/tunnel/2.0#AbstractTunnelType"/>
      <rdfs:range rdf:resource="http://www.opengis.net/gml#CodeType"/>
   </owl:ObjectProperty>
   <owl:ObjectProperty rdf:about="http://www.opengis.net/citygml/tunnel/2.0#function">
      <rdfs:comment>Warning: This ObjectProperty type was declared outside of its original schema. This ObjectProperty may be declared incorrectly.</rdfs:comment>
      <rdfs:domain rdf:resource="http://www.opengis.net/citygml/tunnel/2.0#AbstractTunnelType"/>
      <rdfs:range rdf:resource="http://www.opengis.net/gml#CodeType"/>
   </owl:ObjectProperty>
   <owl:ObjectProperty rdf:about="http://www.opengis.net/citygml/tunnel/2.0#usage">
      <rdfs:comment>Warning: This ObjectProperty type was declared outside of its original schema. This ObjectProperty may be declared incorrectly.</rdfs:comment>
      <rdfs:domain rdf:resource="http://www.opengis.net/citygml/tunnel/2.0#AbstractTunnelType"/>
      <rdfs:range rdf:resource="http://www.opengis.net/gml#CodeType"/>
   </owl:ObjectProperty>
   <owl:DatatypeProperty rdf:about="http://www.opengis.net/citygml/tunnel/2.0#yearOfConstruction">
      <rdfs:domain rdf:resource="http://www.opengis.net/citygml/tunnel/2.0#AbstractTunnelType"/>
      <rdfs:range rdf:resource="http://www.w3.org/2001/XMLSchema#gYear"/>
   </owl:DatatypeProperty>
   <owl:DatatypeProperty rdf:about="http://www.opengis.net/citygml/tunnel/2.0#yearOfDemolition">
      <rdfs:domain rdf:resource="http://www.opengis.net/citygml/tunnel/2.0#AbstractTunnelType"/>
      <rdfs:range rdf:resource="http://www.w3.org/2001/XMLSchema#gYear"/>
   </owl:DatatypeProperty>
   <owl:ObjectProperty rdf:about="http://www.opengis.net/citygml/tunnel/2.0#lod1Solid">
      <rdfs:comment>Warning: This ObjectProperty type was declared outside of its original schema. This ObjectProperty may be declared incorrectly.</rdfs:comment>
      <rdfs:domain rdf:resource="http://www.opengis.net/citygml/tunnel/2.0#AbstractTunnelType"/>
      <rdfs:range rdf:resource="http://www.opengis.net/gml#SolidPropertyType"/>
   </owl:ObjectProperty>
   <owl:ObjectProperty rdf:about="http://www.opengis.net/citygml/tunnel/2.0#lod1MultiSurface">
      <rdfs:comment>Warning: This ObjectProperty type was declared outside of its original schema. This ObjectProperty may be declared incorrectly.</rdfs:comment>
      <rdfs:domain rdf:resource="http://www.opengis.net/citygml/tunnel/2.0#AbstractTunnelType"/>
      <rdfs:range rdf:resource="http://www.opengis.net/gml#MultiSurfacePropertyType"/>
   </owl:ObjectProperty>
   <owl:ObjectProperty rdf:about="http://www.opengis.net/citygml/tunnel/2.0#lod1TerrainIntersection">
      <rdfs:comment>Warning: This ObjectProperty type was declared outside of its original schema. This ObjectProperty may be declared incorrectly.</rdfs:comment>
      <rdfs:domain rdf:resource="http://www.opengis.net/citygml/tunnel/2.0#AbstractTunnelType"/>
      <rdfs:range rdf:resource="http://www.opengis.net/gml#MultiCurvePropertyType"/>
   </owl:ObjectProperty>
   <owl:ObjectProperty rdf:about="http://www.opengis.net/citygml/tunnel/2.0#lod2Solid">
      <rdfs:comment>Warning: This ObjectProperty type was declared outside of its original schema. This ObjectProperty may be declared incorrectly.</rdfs:comment>
      <rdfs:domain rdf:resource="http://www.opengis.net/citygml/tunnel/2.0#AbstractTunnelType"/>
      <rdfs:range rdf:resource="http://www.opengis.net/gml#SolidPropertyType"/>
   </owl:ObjectProperty>
   <owl:ObjectProperty rdf:about="http://www.opengis.net/citygml/tunnel/2.0#lod2MultiSurface">
      <rdfs:comment>Warning: This ObjectProperty type was declared outside of its original schema. This ObjectProperty may be declared incorrectly.</rdfs:comment>
      <rdfs:domain rdf:resource="http://www.opengis.net/citygml/tunnel/2.0#AbstractTunnelType"/>
      <rdfs:range rdf:resource="http://www.opengis.net/gml#MultiSurfacePropertyType"/>
   </owl:ObjectProperty>
   <owl:ObjectProperty rdf:about="http://www.opengis.net/citygml/tunnel/2.0#lod2MultiCurve">
      <rdfs:comment>Warning: This ObjectProperty type was declared outside of its original schema. This ObjectProperty may be declared incorrectly.</rdfs:comment>
      <rdfs:domain rdf:resource="http://www.opengis.net/citygml/tunnel/2.0#AbstractTunnelType"/>
      <rdfs:range rdf:resource="http://www.opengis.net/gml#MultiCurvePropertyType"/>
   </owl:ObjectProperty>
   <owl:ObjectProperty rdf:about="http://www.opengis.net/citygml/tunnel/2.0#lod2TerrainIntersection">
      <rdfs:comment>Warning: This ObjectProperty type was declared outside of its original schema. This ObjectProperty may be declared incorrectly.</rdfs:comment>
      <rdfs:domain rdf:resource="http://www.opengis.net/citygml/tunnel/2.0#AbstractTunnelType"/>
      <rdfs:range rdf:resource="http://www.opengis.net/gml#MultiCurvePropertyType"/>
   </owl:ObjectProperty>
   <owl:ObjectProperty rdf:about="http://www.opengis.net/citygml/tunnel/2.0#outerTunnelInstallation">
      <rdfs:domain rdf:resource="http://www.opengis.net/citygml/tunnel/2.0#AbstractTunnelType"/>
      <rdfs:range rdf:resource="http://www.opengis.net/citygml/tunnel/2.0#TunnelInstallationPropertyType"/>
   </owl:ObjectProperty>
   <owl:ObjectProperty rdf:about="http://www.opengis.net/citygml/tunnel/2.0#interiorTunnelInstallation">
      <rdfs:domain rdf:resource="http://www.opengis.net/citygml/tunnel/2.0#AbstractTunnelType"/>
      <rdfs:range rdf:resource="http://www.opengis.net/citygml/tunnel/2.0#IntTunnelInstallationPropertyType"/>
   </owl:ObjectProperty>
   <owl:ObjectProperty rdf:about="http://www.opengis.net/citygml/tunnel/2.0#boundedBy">
      <rdfs:domain rdf:resource="http://www.opengis.net/citygml/tunnel/2.0#AbstractTunnelType"/>
      <rdfs:range rdf:resource="http://www.opengis.net/citygml/tunnel/2.0#BoundarySurfacePropertyType"/>
   </owl:ObjectProperty>
   <owl:ObjectProperty rdf:about="http://www.opengis.net/citygml/tunnel/2.0#lod3Solid">
      <rdfs:comment>Warning: This ObjectProperty type was declared outside of its original schema. This ObjectProperty may be declared incorrectly.</rdfs:comment>
      <rdfs:domain rdf:resource="http://www.opengis.net/citygml/tunnel/2.0#AbstractTunnelType"/>
      <rdfs:range rdf:resource="http://www.opengis.net/gml#SolidPropertyType"/>
   </owl:ObjectProperty>
   <owl:ObjectProperty rdf:about="http://www.opengis.net/citygml/tunnel/2.0#lod3MultiSurface">
      <rdfs:comment>Warning: This ObjectProperty type was declared outside of its original schema. This ObjectProperty may be declared incorrectly.</rdfs:comment>
      <rdfs:domain rdf:resource="http://www.opengis.net/citygml/tunnel/2.0#AbstractTunnelType"/>
      <rdfs:range rdf:resource="http://www.opengis.net/gml#MultiSurfacePropertyType"/>
   </owl:ObjectProperty>
   <owl:ObjectProperty rdf:about="http://www.opengis.net/citygml/tunnel/2.0#lod3MultiCurve">
      <rdfs:comment>Warning: This ObjectProperty type was declared outside of its original schema. This ObjectProperty may be declared incorrectly.</rdfs:comment>
      <rdfs:domain rdf:resource="http://www.opengis.net/citygml/tunnel/2.0#AbstractTunnelType"/>
      <rdfs:range rdf:resource="http://www.opengis.net/gml#MultiCurvePropertyType"/>
   </owl:ObjectProperty>
   <owl:ObjectProperty rdf:about="http://www.opengis.net/citygml/tunnel/2.0#lod3TerrainIntersection">
      <rdfs:comment>Warning: This ObjectProperty type was declared outside of its original schema. This ObjectProperty may be declared incorrectly.</rdfs:comment>
      <rdfs:domain rdf:resource="http://www.opengis.net/citygml/tunnel/2.0#AbstractTunnelType"/>
      <rdfs:range rdf:resource="http://www.opengis.net/gml#MultiCurvePropertyType"/>
   </owl:ObjectProperty>
   <owl:ObjectProperty rdf:about="http://www.opengis.net/citygml/tunnel/2.0#lod4Solid">
      <rdfs:comment>Warning: This ObjectProperty type was declared outside of its original schema. This ObjectProperty may be declared incorrectly.</rdfs:comment>
      <rdfs:domain rdf:resource="http://www.opengis.net/citygml/tunnel/2.0#AbstractTunnelType"/>
      <rdfs:range rdf:resource="http://www.opengis.net/gml#SolidPropertyType"/>
   </owl:ObjectProperty>
   <owl:ObjectProperty rdf:about="http://www.opengis.net/citygml/tunnel/2.0#lod4MultiSurface">
      <rdfs:comment>Warning: This ObjectProperty type was declared outside of its original schema. This ObjectProperty may be declared incorrectly.</rdfs:comment>
      <rdfs:domain rdf:resource="http://www.opengis.net/citygml/tunnel/2.0#AbstractTunnelType"/>
      <rdfs:range rdf:resource="http://www.opengis.net/gml#MultiSurfacePropertyType"/>
   </owl:ObjectProperty>
   <owl:ObjectProperty rdf:about="http://www.opengis.net/citygml/tunnel/2.0#lod4MultiCurve">
      <rdfs:comment>Warning: This ObjectProperty type was declared outside of its original schema. This ObjectProperty may be declared incorrectly.</rdfs:comment>
      <rdfs:domain rdf:resource="http://www.opengis.net/citygml/tunnel/2.0#AbstractTunnelType"/>
      <rdfs:range rdf:resource="http://www.opengis.net/gml#MultiCurvePropertyType"/>
   </owl:ObjectProperty>
   <owl:ObjectProperty rdf:about="http://www.opengis.net/citygml/tunnel/2.0#lod4TerrainIntersection">
      <rdfs:comment>Warning: This ObjectProperty type was declared outside of its original schema. This ObjectProperty may be declared incorrectly.</rdfs:comment>
      <rdfs:domain rdf:resource="http://www.opengis.net/citygml/tunnel/2.0#AbstractTunnelType"/>
      <rdfs:range rdf:resource="http://www.opengis.net/gml#MultiCurvePropertyType"/>
   </owl:ObjectProperty>
   <owl:ObjectProperty rdf:about="http://www.opengis.net/citygml/tunnel/2.0#interiorHollowSpace">
      <rdfs:domain rdf:resource="http://www.opengis.net/citygml/tunnel/2.0#AbstractTunnelType"/>
      <rdfs:range rdf:resource="http://www.opengis.net/citygml/tunnel/2.0#InteriorHollowSpacePropertyType"/>
   </owl:ObjectProperty>
   <owl:ObjectProperty rdf:about="http://www.opengis.net/citygml/tunnel/2.0#consistsOfTunnelPart">
      <rdfs:domain rdf:resource="http://www.opengis.net/citygml/tunnel/2.0#AbstractTunnelType"/>
      <rdfs:range rdf:resource="http://www.opengis.net/citygml/tunnel/2.0#TunnelPartPropertyType"/>
   </owl:ObjectProperty>
   <owl:ObjectProperty rdf:about="http://www.opengis.net/citygml/tunnel/2.0#has_GenericApplicationPropertyOfAbstractTunnel">
      <rdfs:domain rdf:resource="http://www.opengis.net/citygml/tunnel/2.0#AbstractTunnelType"/>
      <rdfs:range rdf:resource="http://www.opengis.net/citygml/tunnel/2.0#_GenericApplicationPropertyOfAbstractTunnel"/>
   </owl:ObjectProperty>
   <owl:ObjectProperty rdf:about="http://www.opengis.net/citygml/tunnel/2.0#has_GenericApplicationPropertyOfTunnel">
      <rdfs:domain rdf:resource="http://www.opengis.net/citygml/tunnel/2.0#TunnelType"/>
      <rdfs:range rdf:resource="http://www.opengis.net/citygml/tunnel/2.0#_GenericApplicationPropertyOfTunnel"/>
   </owl:ObjectProperty>
   <owl:ObjectProperty rdf:about="http://www.opengis.net/citygml/tunnel/2.0#has_GenericApplicationPropertyOfTunnelPart">
      <rdfs:domain rdf:resource="http://www.opengis.net/citygml/tunnel/2.0#TunnelPartType"/>
      <rdfs:range rdf:resource="http://www.opengis.net/citygml/tunnel/2.0#_GenericApplicationPropertyOfTunnelPart"/>
   </owl:ObjectProperty>
   <owl:ObjectProperty rdf:about="http://www.opengis.net/citygml/tunnel/2.0#hasTunnelPart">
      <rdfs:domain rdf:resource="http://www.opengis.net/citygml/tunnel/2.0#TunnelPartPropertyType"/>
      <rdfs:range rdf:resource="http://www.opengis.net/citygml/tunnel/2.0#TunnelPart"/>
   </owl:ObjectProperty>
   <owl:ObjectProperty rdf:about="http://www.opengis.net/citygml/tunnel/2.0#class">
      <rdfs:comment>Warning: This ObjectProperty type was declared outside of its original schema. This ObjectProperty may be declared incorrectly.</rdfs:comment>
      <rdfs:domain rdf:resource="http://www.opengis.net/citygml/tunnel/2.0#TunnelInstallationType"/>
      <rdfs:range rdf:resource="http://www.opengis.net/gml#CodeType"/>
   </owl:ObjectProperty>
   <owl:ObjectProperty rdf:about="http://www.opengis.net/citygml/tunnel/2.0#function">
      <rdfs:comment>Warning: This ObjectProperty type was declared outside of its original schema. This ObjectProperty may be declared incorrectly.</rdfs:comment>
      <rdfs:domain rdf:resource="http://www.opengis.net/citygml/tunnel/2.0#TunnelInstallationType"/>
      <rdfs:range rdf:resource="http://www.opengis.net/gml#CodeType"/>
   </owl:ObjectProperty>
   <owl:ObjectProperty rdf:about="http://www.opengis.net/citygml/tunnel/2.0#usage">
      <rdfs:comment>Warning: This ObjectProperty type was declared outside of its original schema. This ObjectProperty may be declared incorrectly.</rdfs:comment>
      <rdfs:domain rdf:resource="http://www.opengis.net/citygml/tunnel/2.0#TunnelInstallationType"/>
      <rdfs:range rdf:resource="http://www.opengis.net/gml#CodeType"/>
   </owl:ObjectProperty>
   <owl:ObjectProperty rdf:about="http://www.opengis.net/citygml/tunnel/2.0#lod2Geometry">
      <rdfs:comment>Warning: This ObjectProperty type was declared outside of its original schema. This ObjectProperty may be declared incorrectly.</rdfs:comment>
      <rdfs:domain rdf:resource="http://www.opengis.net/citygml/tunnel/2.0#TunnelInstallationType"/>
      <rdfs:range rdf:resource="http://www.opengis.net/gml#GeometryPropertyType"/>
   </owl:ObjectProperty>
   <owl:ObjectProperty rdf:about="http://www.opengis.net/citygml/tunnel/2.0#lod3Geometry">
      <rdfs:comment>Warning: This ObjectProperty type was declared outside of its original schema. This ObjectProperty may be declared incorrectly.</rdfs:comment>
      <rdfs:domain rdf:resource="http://www.opengis.net/citygml/tunnel/2.0#TunnelInstallationType"/>
      <rdfs:range rdf:resource="http://www.opengis.net/gml#GeometryPropertyType"/>
   </owl:ObjectProperty>
   <owl:ObjectProperty rdf:about="http://www.opengis.net/citygml/tunnel/2.0#lod4Geometry">
      <rdfs:comment>Warning: This ObjectProperty type was declared outside of its original schema. This ObjectProperty may be declared incorrectly.</rdfs:comment>
      <rdfs:domain rdf:resource="http://www.opengis.net/citygml/tunnel/2.0#TunnelInstallationType"/>
      <rdfs:range rdf:resource="http://www.opengis.net/gml#GeometryPropertyType"/>
   </owl:ObjectProperty>
   <owl:ObjectProperty rdf:about="http://www.opengis.net/citygml/tunnel/2.0#lod2ImplicitRepresentation">
      <rdfs:comment>Warning: This ObjectProperty type was declared outside of its original schema. This ObjectProperty may be declared incorrectly.</rdfs:comment>
      <rdfs:domain rdf:resource="http://www.opengis.net/citygml/tunnel/2.0#TunnelInstallationType"/>
      <rdfs:range rdf:resource="http://www.opengis.net/citygml/2.0#ImplicitRepresentationPropertyType"/>
   </owl:ObjectProperty>
   <owl:ObjectProperty rdf:about="http://www.opengis.net/citygml/tunnel/2.0#lod3ImplicitRepresentation">
      <rdfs:comment>Warning: This ObjectProperty type was declared outside of its original schema. This ObjectProperty may be declared incorrectly.</rdfs:comment>
      <rdfs:domain rdf:resource="http://www.opengis.net/citygml/tunnel/2.0#TunnelInstallationType"/>
      <rdfs:range rdf:resource="http://www.opengis.net/citygml/2.0#ImplicitRepresentationPropertyType"/>
   </owl:ObjectProperty>
   <owl:ObjectProperty rdf:about="http://www.opengis.net/citygml/tunnel/2.0#lod4ImplicitRepresentation">
      <rdfs:comment>Warning: This ObjectProperty type was declared outside of its original schema. This ObjectProperty may be declared incorrectly.</rdfs:comment>
      <rdfs:domain rdf:resource="http://www.opengis.net/citygml/tunnel/2.0#TunnelInstallationType"/>
      <rdfs:range rdf:resource="http://www.opengis.net/citygml/2.0#ImplicitRepresentationPropertyType"/>
   </owl:ObjectProperty>
   <owl:ObjectProperty rdf:about="http://www.opengis.net/citygml/tunnel/2.0#boundedBy">
      <rdfs:domain rdf:resource="http://www.opengis.net/citygml/tunnel/2.0#TunnelInstallationType"/>
      <rdfs:range rdf:resource="http://www.opengis.net/citygml/tunnel/2.0#BoundarySurfacePropertyType"/>
   </owl:ObjectProperty>
   <owl:ObjectProperty rdf:about="http://www.opengis.net/citygml/tunnel/2.0#has_GenericApplicationPropertyOfTunnelInstallation">
      <rdfs:domain rdf:resource="http://www.opengis.net/citygml/tunnel/2.0#TunnelInstallationType"/>
      <rdfs:range rdf:resource="http://www.opengis.net/citygml/tunnel/2.0#_GenericApplicationPropertyOfTunnelInstallation"/>
   </owl:ObjectProperty>
   <owl:ObjectProperty rdf:about="http://www.opengis.net/citygml/tunnel/2.0#hasTunnelInstallation">
      <rdfs:domain rdf:resource="http://www.opengis.net/citygml/tunnel/2.0#TunnelInstallationPropertyType"/>
      <rdfs:range rdf:resource="http://www.opengis.net/citygml/tunnel/2.0#TunnelInstallation"/>
   </owl:ObjectProperty>
   <owl:ObjectProperty rdf:about="http://www.opengis.net/citygml/tunnel/2.0#class">
      <rdfs:comment>Warning: This ObjectProperty type was declared outside of its original schema. This ObjectProperty may be declared incorrectly.</rdfs:comment>
      <rdfs:domain rdf:resource="http://www.opengis.net/citygml/tunnel/2.0#IntTunnelInstallationType"/>
      <rdfs:range rdf:resource="http://www.opengis.net/gml#CodeType"/>
   </owl:ObjectProperty>
   <owl:ObjectProperty rdf:about="http://www.opengis.net/citygml/tunnel/2.0#function">
      <rdfs:comment>Warning: This ObjectProperty type was declared outside of its original schema. This ObjectProperty may be declared incorrectly.</rdfs:comment>
      <rdfs:domain rdf:resource="http://www.opengis.net/citygml/tunnel/2.0#IntTunnelInstallationType"/>
      <rdfs:range rdf:resource="http://www.opengis.net/gml#CodeType"/>
   </owl:ObjectProperty>
   <owl:ObjectProperty rdf:about="http://www.opengis.net/citygml/tunnel/2.0#usage">
      <rdfs:comment>Warning: This ObjectProperty type was declared outside of its original schema. This ObjectProperty may be declared incorrectly.</rdfs:comment>
      <rdfs:domain rdf:resource="http://www.opengis.net/citygml/tunnel/2.0#IntTunnelInstallationType"/>
      <rdfs:range rdf:resource="http://www.opengis.net/gml#CodeType"/>
   </owl:ObjectProperty>
   <owl:ObjectProperty rdf:about="http://www.opengis.net/citygml/tunnel/2.0#lod4Geometry">
      <rdfs:comment>Warning: This ObjectProperty type was declared outside of its original schema. This ObjectProperty may be declared incorrectly.</rdfs:comment>
      <rdfs:domain rdf:resource="http://www.opengis.net/citygml/tunnel/2.0#IntTunnelInstallationType"/>
      <rdfs:range rdf:resource="http://www.opengis.net/gml#GeometryPropertyType"/>
   </owl:ObjectProperty>
   <owl:ObjectProperty rdf:about="http://www.opengis.net/citygml/tunnel/2.0#lod4ImplicitRepresentation">
      <rdfs:comment>Warning: This ObjectProperty type was declared outside of its original schema. This ObjectProperty may be declared incorrectly.</rdfs:comment>
      <rdfs:domain rdf:resource="http://www.opengis.net/citygml/tunnel/2.0#IntTunnelInstallationType"/>
      <rdfs:range rdf:resource="http://www.opengis.net/citygml/2.0#ImplicitRepresentationPropertyType"/>
   </owl:ObjectProperty>
   <owl:ObjectProperty rdf:about="http://www.opengis.net/citygml/tunnel/2.0#boundedBy">
      <rdfs:domain rdf:resource="http://www.opengis.net/citygml/tunnel/2.0#IntTunnelInstallationType"/>
      <rdfs:range rdf:resource="http://www.opengis.net/citygml/tunnel/2.0#BoundarySurfacePropertyType"/>
   </owl:ObjectProperty>
   <owl:ObjectProperty rdf:about="http://www.opengis.net/citygml/tunnel/2.0#has_GenericApplicationPropertyOfIntTunnelInstallation">
      <rdfs:domain rdf:resource="http://www.opengis.net/citygml/tunnel/2.0#IntTunnelInstallationType"/>
      <rdfs:range rdf:resource="http://www.opengis.net/citygml/tunnel/2.0#_GenericApplicationPropertyOfIntTunnelInstallation"/>
   </owl:ObjectProperty>
   <owl:ObjectProperty rdf:about="http://www.opengis.net/citygml/tunnel/2.0#hasIntTunnelInstallation">
      <rdfs:domain rdf:resource="http://www.opengis.net/citygml/tunnel/2.0#IntTunnelInstallationPropertyType"/>
      <rdfs:range rdf:resource="http://www.opengis.net/citygml/tunnel/2.0#IntTunnelInstallation"/>
   </owl:ObjectProperty>
   <owl:ObjectProperty rdf:about="http://www.opengis.net/citygml/tunnel/2.0#has_BoundarySurface">
      <rdfs:domain rdf:resource="http://www.opengis.net/citygml/tunnel/2.0#BoundarySurfacePropertyType"/>
      <rdfs:range rdf:resource="http://www.opengis.net/citygml/tunnel/2.0#_BoundarySurface"/>
   </owl:ObjectProperty>
   <owl:ObjectProperty rdf:about="http://www.opengis.net/citygml/tunnel/2.0#lod2MultiSurface">
      <rdfs:comment>Warning: This ObjectProperty type was declared outside of its original schema. This ObjectProperty may be declared incorrectly.</rdfs:comment>
      <rdfs:domain rdf:resource="http://www.opengis.net/citygml/tunnel/2.0#AbstractBoundarySurfaceType"/>
      <rdfs:range rdf:resource="http://www.opengis.net/gml#MultiSurfacePropertyType"/>
   </owl:ObjectProperty>
   <owl:ObjectProperty rdf:about="http://www.opengis.net/citygml/tunnel/2.0#lod3MultiSurface">
      <rdfs:comment>Warning: This ObjectProperty type was declared outside of its original schema. This ObjectProperty may be declared incorrectly.</rdfs:comment>
      <rdfs:domain rdf:resource="http://www.opengis.net/citygml/tunnel/2.0#AbstractBoundarySurfaceType"/>
      <rdfs:range rdf:resource="http://www.opengis.net/gml#MultiSurfacePropertyType"/>
   </owl:ObjectProperty>
   <owl:ObjectProperty rdf:about="http://www.opengis.net/citygml/tunnel/2.0#lod4MultiSurface">
      <rdfs:comment>Warning: This ObjectProperty type was declared outside of its original schema. This ObjectProperty may be declared incorrectly.</rdfs:comment>
      <rdfs:domain rdf:resource="http://www.opengis.net/citygml/tunnel/2.0#AbstractBoundarySurfaceType"/>
      <rdfs:range rdf:resource="http://www.opengis.net/gml#MultiSurfacePropertyType"/>
   </owl:ObjectProperty>
   <owl:ObjectProperty rdf:about="http://www.opengis.net/citygml/tunnel/2.0#opening">
      <rdfs:domain rdf:resource="http://www.opengis.net/citygml/tunnel/2.0#AbstractBoundarySurfaceType"/>
      <rdfs:range rdf:resource="http://www.opengis.net/citygml/tunnel/2.0#OpeningPropertyType"/>
   </owl:ObjectProperty>
   <owl:ObjectProperty rdf:about="http://www.opengis.net/citygml/tunnel/2.0#has_GenericApplicationPropertyOfBoundarySurface">
      <rdfs:domain rdf:resource="http://www.opengis.net/citygml/tunnel/2.0#AbstractBoundarySurfaceType"/>
      <rdfs:range rdf:resource="http://www.opengis.net/citygml/tunnel/2.0#_GenericApplicationPropertyOfBoundarySurface"/>
   </owl:ObjectProperty>
   <owl:ObjectProperty rdf:about="http://www.opengis.net/citygml/tunnel/2.0#has_GenericApplicationPropertyOfRoofSurface">
      <rdfs:domain rdf:resource="http://www.opengis.net/citygml/tunnel/2.0#RoofSurfaceType"/>
      <rdfs:range rdf:resource="http://www.opengis.net/citygml/tunnel/2.0#_GenericApplicationPropertyOfRoofSurface"/>
   </owl:ObjectProperty>
   <owl:ObjectProperty rdf:about="http://www.opengis.net/citygml/tunnel/2.0#has_GenericApplicationPropertyOfWallSurface">
      <rdfs:domain rdf:resource="http://www.opengis.net/citygml/tunnel/2.0#WallSurfaceType"/>
      <rdfs:range rdf:resource="http://www.opengis.net/citygml/tunnel/2.0#_GenericApplicationPropertyOfWallSurface"/>
   </owl:ObjectProperty>
   <owl:ObjectProperty rdf:about="http://www.opengis.net/citygml/tunnel/2.0#has_GenericApplicationPropertyOfGroundSurface">
      <rdfs:domain rdf:resource="http://www.opengis.net/citygml/tunnel/2.0#GroundSurfaceType"/>
      <rdfs:range rdf:resource="http://www.opengis.net/citygml/tunnel/2.0#_GenericApplicationPropertyOfGroundSurface"/>
   </owl:ObjectProperty>
   <owl:ObjectProperty rdf:about="http://www.opengis.net/citygml/tunnel/2.0#has_GenericApplicationPropertyOfClosureSurface">
      <rdfs:domain rdf:resource="http://www.opengis.net/citygml/tunnel/2.0#ClosureSurfaceType"/>
      <rdfs:range rdf:resource="http://www.opengis.net/citygml/tunnel/2.0#_GenericApplicationPropertyOfClosureSurface"/>
   </owl:ObjectProperty>
   <owl:ObjectProperty rdf:about="http://www.opengis.net/citygml/tunnel/2.0#has_GenericApplicationPropertyOfFloorSurface">
      <rdfs:domain rdf:resource="http://www.opengis.net/citygml/tunnel/2.0#FloorSurfaceType"/>
      <rdfs:range rdf:resource="http://www.opengis.net/citygml/tunnel/2.0#_GenericApplicationPropertyOfFloorSurface"/>
   </owl:ObjectProperty>
   <owl:ObjectProperty rdf:about="http://www.opengis.net/citygml/tunnel/2.0#has_GenericApplicationPropertyOfOuterFloorSurface">
      <rdfs:domain rdf:resource="http://www.opengis.net/citygml/tunnel/2.0#OuterFloorSurfaceType"/>
      <rdfs:range rdf:resource="http://www.opengis.net/citygml/tunnel/2.0#_GenericApplicationPropertyOfOuterFloorSurface"/>
   </owl:ObjectProperty>
   <owl:ObjectProperty rdf:about="http://www.opengis.net/citygml/tunnel/2.0#has_GenericApplicationPropertyOfInteriorWallSurface">
      <rdfs:domain rdf:resource="http://www.opengis.net/citygml/tunnel/2.0#InteriorWallSurfaceType"/>
      <rdfs:range rdf:resource="http://www.opengis.net/citygml/tunnel/2.0#_GenericApplicationPropertyOfInteriorWallSurface"/>
   </owl:ObjectProperty>
   <owl:ObjectProperty rdf:about="http://www.opengis.net/citygml/tunnel/2.0#has_GenericApplicationPropertyOfCeilingSurface">
      <rdfs:domain rdf:resource="http://www.opengis.net/citygml/tunnel/2.0#CeilingSurfaceType"/>
      <rdfs:range rdf:resource="http://www.opengis.net/citygml/tunnel/2.0#_GenericApplicationPropertyOfCeilingSurface"/>
   </owl:ObjectProperty>
   <owl:ObjectProperty rdf:about="http://www.opengis.net/citygml/tunnel/2.0#has_GenericApplicationPropertyOfOuterCeilingSurface">
      <rdfs:domain rdf:resource="http://www.opengis.net/citygml/tunnel/2.0#OuterCeilingSurfaceType"/>
      <rdfs:range rdf:resource="http://www.opengis.net/citygml/tunnel/2.0#_GenericApplicationPropertyOfOuterCeilingSurface"/>
   </owl:ObjectProperty>
   <owl:ObjectProperty rdf:about="http://www.opengis.net/citygml/tunnel/2.0#class">
      <rdfs:comment>Warning: This ObjectProperty type was declared outside of its original schema. This ObjectProperty may be declared incorrectly.</rdfs:comment>
      <rdfs:domain rdf:resource="http://www.opengis.net/citygml/tunnel/2.0#HollowSpaceType"/>
      <rdfs:range rdf:resource="http://www.opengis.net/gml#CodeType"/>
   </owl:ObjectProperty>
   <owl:ObjectProperty rdf:about="http://www.opengis.net/citygml/tunnel/2.0#function">
      <rdfs:comment>Warning: This ObjectProperty type was declared outside of its original schema. This ObjectProperty may be declared incorrectly.</rdfs:comment>
      <rdfs:domain rdf:resource="http://www.opengis.net/citygml/tunnel/2.0#HollowSpaceType"/>
      <rdfs:range rdf:resource="http://www.opengis.net/gml#CodeType"/>
   </owl:ObjectProperty>
   <owl:ObjectProperty rdf:about="http://www.opengis.net/citygml/tunnel/2.0#usage">
      <rdfs:comment>Warning: This ObjectProperty type was declared outside of its original schema. This ObjectProperty may be declared incorrectly.</rdfs:comment>
      <rdfs:domain rdf:resource="http://www.opengis.net/citygml/tunnel/2.0#HollowSpaceType"/>
      <rdfs:range rdf:resource="http://www.opengis.net/gml#CodeType"/>
   </owl:ObjectProperty>
   <owl:ObjectProperty rdf:about="http://www.opengis.net/citygml/tunnel/2.0#lod4Solid">
      <rdfs:comment>Warning: This ObjectProperty type was declared outside of its original schema. This ObjectProperty may be declared incorrectly.</rdfs:comment>
      <rdfs:domain rdf:resource="http://www.opengis.net/citygml/tunnel/2.0#HollowSpaceType"/>
      <rdfs:range rdf:resource="http://www.opengis.net/gml#SolidPropertyType"/>
   </owl:ObjectProperty>
   <owl:ObjectProperty rdf:about="http://www.opengis.net/citygml/tunnel/2.0#lod4MultiSurface">
      <rdfs:comment>Warning: This ObjectProperty type was declared outside of its original schema. This ObjectProperty may be declared incorrectly.</rdfs:comment>
      <rdfs:domain rdf:resource="http://www.opengis.net/citygml/tunnel/2.0#HollowSpaceType"/>
      <rdfs:range rdf:resource="http://www.opengis.net/gml#MultiSurfacePropertyType"/>
   </owl:ObjectProperty>
   <owl:ObjectProperty rdf:about="http://www.opengis.net/citygml/tunnel/2.0#boundedBy">
      <rdfs:domain rdf:resource="http://www.opengis.net/citygml/tunnel/2.0#HollowSpaceType"/>
      <rdfs:range rdf:resource="http://www.opengis.net/citygml/tunnel/2.0#BoundarySurfacePropertyType"/>
   </owl:ObjectProperty>
   <owl:ObjectProperty rdf:about="http://www.opengis.net/citygml/tunnel/2.0#interiorFurniture">
      <rdfs:domain rdf:resource="http://www.opengis.net/citygml/tunnel/2.0#HollowSpaceType"/>
      <rdfs:range rdf:resource="http://www.opengis.net/citygml/tunnel/2.0#InteriorFurniturePropertyType"/>
   </owl:ObjectProperty>
   <owl:ObjectProperty rdf:about="http://www.opengis.net/citygml/tunnel/2.0#hollowSpaceInstallation">
      <rdfs:domain rdf:resource="http://www.opengis.net/citygml/tunnel/2.0#HollowSpaceType"/>
      <rdfs:range rdf:resource="http://www.opengis.net/citygml/tunnel/2.0#IntTunnelInstallationPropertyType"/>
   </owl:ObjectProperty>
   <owl:ObjectProperty rdf:about="http://www.opengis.net/citygml/tunnel/2.0#has_GenericApplicationPropertyOfHollowSpace">
      <rdfs:domain rdf:resource="http://www.opengis.net/citygml/tunnel/2.0#HollowSpaceType"/>
      <rdfs:range rdf:resource="http://www.opengis.net/citygml/tunnel/2.0#_GenericApplicationPropertyOfHollowSpace"/>
   </owl:ObjectProperty>
   <owl:ObjectProperty rdf:about="http://www.opengis.net/citygml/tunnel/2.0#hasHollowSpace">
      <rdfs:domain rdf:resource="http://www.opengis.net/citygml/tunnel/2.0#InteriorHollowSpacePropertyType"/>
      <rdfs:range rdf:resource="http://www.opengis.net/citygml/tunnel/2.0#HollowSpace"/>
   </owl:ObjectProperty>
   <owl:ObjectProperty rdf:about="http://www.opengis.net/citygml/tunnel/2.0#class">
      <rdfs:comment>Warning: This ObjectProperty type was declared outside of its original schema. This ObjectProperty may be declared incorrectly.</rdfs:comment>
      <rdfs:domain rdf:resource="http://www.opengis.net/citygml/tunnel/2.0#TunnelFurnitureType"/>
      <rdfs:range rdf:resource="http://www.opengis.net/gml#CodeType"/>
   </owl:ObjectProperty>
   <owl:ObjectProperty rdf:about="http://www.opengis.net/citygml/tunnel/2.0#function">
      <rdfs:comment>Warning: This ObjectProperty type was declared outside of its original schema. This ObjectProperty may be declared incorrectly.</rdfs:comment>
      <rdfs:domain rdf:resource="http://www.opengis.net/citygml/tunnel/2.0#TunnelFurnitureType"/>
      <rdfs:range rdf:resource="http://www.opengis.net/gml#CodeType"/>
   </owl:ObjectProperty>
   <owl:ObjectProperty rdf:about="http://www.opengis.net/citygml/tunnel/2.0#usage">
      <rdfs:comment>Warning: This ObjectProperty type was declared outside of its original schema. This ObjectProperty may be declared incorrectly.</rdfs:comment>
      <rdfs:domain rdf:resource="http://www.opengis.net/citygml/tunnel/2.0#TunnelFurnitureType"/>
      <rdfs:range rdf:resource="http://www.opengis.net/gml#CodeType"/>
   </owl:ObjectProperty>
   <owl:ObjectProperty rdf:about="http://www.opengis.net/citygml/tunnel/2.0#lod4Geometry">
      <rdfs:comment>Warning: This ObjectProperty type was declared outside of its original schema. This ObjectProperty may be declared incorrectly.</rdfs:comment>
      <rdfs:domain rdf:resource="http://www.opengis.net/citygml/tunnel/2.0#TunnelFurnitureType"/>
      <rdfs:range rdf:resource="http://www.opengis.net/gml#GeometryPropertyType"/>
   </owl:ObjectProperty>
   <owl:ObjectProperty rdf:about="http://www.opengis.net/citygml/tunnel/2.0#lod4ImplicitRepresentation">
      <rdfs:comment>Warning: This ObjectProperty type was declared outside of its original schema. This ObjectProperty may be declared incorrectly.</rdfs:comment>
      <rdfs:domain rdf:resource="http://www.opengis.net/citygml/tunnel/2.0#TunnelFurnitureType"/>
      <rdfs:range rdf:resource="http://www.opengis.net/citygml/2.0#ImplicitRepresentationPropertyType"/>
   </owl:ObjectProperty>
   <owl:ObjectProperty rdf:about="http://www.opengis.net/citygml/tunnel/2.0#has_GenericApplicationPropertyOfTunnelFurniture">
      <rdfs:domain rdf:resource="http://www.opengis.net/citygml/tunnel/2.0#TunnelFurnitureType"/>
      <rdfs:range rdf:resource="http://www.opengis.net/citygml/tunnel/2.0#_GenericApplicationPropertyOfTunnelFurniture"/>
   </owl:ObjectProperty>
   <owl:ObjectProperty rdf:about="http://www.opengis.net/citygml/tunnel/2.0#hasTunnelFurniture">
      <rdfs:domain rdf:resource="http://www.opengis.net/citygml/tunnel/2.0#InteriorFurniturePropertyType"/>
      <rdfs:range rdf:resource="http://www.opengis.net/citygml/tunnel/2.0#TunnelFurniture"/>
   </owl:ObjectProperty>
   <owl:ObjectProperty rdf:about="http://www.opengis.net/citygml/tunnel/2.0#lod3MultiSurface">
      <rdfs:comment>Warning: This ObjectProperty type was declared outside of its original schema. This ObjectProperty may be declared incorrectly.</rdfs:comment>
      <rdfs:domain rdf:resource="http://www.opengis.net/citygml/tunnel/2.0#AbstractOpeningType"/>
      <rdfs:range rdf:resource="http://www.opengis.net/gml#MultiSurfacePropertyType"/>
   </owl:ObjectProperty>
   <owl:ObjectProperty rdf:about="http://www.opengis.net/citygml/tunnel/2.0#lod4MultiSurface">
      <rdfs:comment>Warning: This ObjectProperty type was declared outside of its original schema. This ObjectProperty may be declared incorrectly.</rdfs:comment>
      <rdfs:domain rdf:resource="http://www.opengis.net/citygml/tunnel/2.0#AbstractOpeningType"/>
      <rdfs:range rdf:resource="http://www.opengis.net/gml#MultiSurfacePropertyType"/>
   </owl:ObjectProperty>
   <owl:ObjectProperty rdf:about="http://www.opengis.net/citygml/tunnel/2.0#lod3ImplicitRepresentation">
      <rdfs:comment>Warning: This ObjectProperty type was declared outside of its original schema. This ObjectProperty may be declared incorrectly.</rdfs:comment>
      <rdfs:domain rdf:resource="http://www.opengis.net/citygml/tunnel/2.0#AbstractOpeningType"/>
      <rdfs:range rdf:resource="http://www.opengis.net/citygml/2.0#ImplicitRepresentationPropertyType"/>
   </owl:ObjectProperty>
   <owl:ObjectProperty rdf:about="http://www.opengis.net/citygml/tunnel/2.0#lod4ImplicitRepresentation">
      <rdfs:comment>Warning: This ObjectProperty type was declared outside of its original schema. This ObjectProperty may be declared incorrectly.</rdfs:comment>
      <rdfs:domain rdf:resource="http://www.opengis.net/citygml/tunnel/2.0#AbstractOpeningType"/>
      <rdfs:range rdf:resource="http://www.opengis.net/citygml/2.0#ImplicitRepresentationPropertyType"/>
   </owl:ObjectProperty>
   <owl:ObjectProperty rdf:about="http://www.opengis.net/citygml/tunnel/2.0#has_GenericApplicationPropertyOfOpening">
      <rdfs:domain rdf:resource="http://www.opengis.net/citygml/tunnel/2.0#AbstractOpeningType"/>
      <rdfs:range rdf:resource="http://www.opengis.net/citygml/tunnel/2.0#_GenericApplicationPropertyOfOpening"/>
   </owl:ObjectProperty>
   <owl:ObjectProperty rdf:about="http://www.opengis.net/citygml/tunnel/2.0#has_Opening">
      <rdfs:domain rdf:resource="http://www.opengis.net/citygml/tunnel/2.0#OpeningPropertyType"/>
      <rdfs:range rdf:resource="http://www.opengis.net/citygml/tunnel/2.0#_Opening"/>
   </owl:ObjectProperty>
   <owl:ObjectProperty rdf:about="http://www.opengis.net/citygml/tunnel/2.0#has_GenericApplicationPropertyOfWindow">
      <rdfs:domain rdf:resource="http://www.opengis.net/citygml/tunnel/2.0#WindowType"/>
      <rdfs:range rdf:resource="http://www.opengis.net/citygml/tunnel/2.0#_GenericApplicationPropertyOfWindow"/>
   </owl:ObjectProperty>
   <owl:ObjectProperty rdf:about="http://www.opengis.net/citygml/tunnel/2.0#has_GenericApplicationPropertyOfDoor">
      <rdfs:domain rdf:resource="http://www.opengis.net/citygml/tunnel/2.0#DoorType"/>
      <rdfs:range rdf:resource="http://www.opengis.net/citygml/tunnel/2.0#_GenericApplicationPropertyOfDoor"/>
   </owl:ObjectProperty>
</rdf:RDF>
