<rdf:RDF xmlns:math="http://www.w3.org/2005/xpath-functions/math" xmlns:owl="http://www.w3.org/2002/07/owl#" xmlns:rdf="http://www.w3.org/1999/02/22-rdf-syntax-ns#" xmlns:rdfs="http://www.w3.org/2000/01/rdf-schema#" xmlns:xs="http://www.w3.org/2001/XMLSchema" xmlns:xsd="http://www.w3.org/2001/XMLSchema">
   <owl:Ontology rdf:about="http://liris.cnrs.fr/ontologies/units">
      <owl:imports rdf:resource="http://liris.cnrs.fr/ontologies/gml"/>
      <owl:imports rdf:resource="http://liris.cnrs.fr/ontologies/dictionary"/>
      <rdfs:comment/>
      <rdfs:seeAlso>urn:opengis:specification:gml:schema-units:3.1.1</rdfs:seeAlso>
      <rdfs:comment>Builds on gmlBase.xsd to encode units of measure (or uom), including definitions of units of measure and dictionaries of such definitions. GML 3.0 candidate schema, primary editor: Arliss Whiteside.			
	Parts of this schema are based on Subclause 6.5.7 of ISO/CD 19103 Geographic information - Conceptual schema language, on Subclause A.5.2.2.3 of ISO/CD 19118 Geographic information - Encoding, and on most of OpenGIS Recommendation Paper OGC 02-007r4 Units of Measure Use and Definition Recommendations.
		
		GML is an OGC Standard.
		Copyright (c) 2001,2005,2010 Open Geospatial Consortium.
		To obtain additional rights of use, visit http://www.opengeospatial.org/legal/ .
		</rdfs:comment>
   </owl:Ontology>
   <owl:Class rdf:about="#UnitOfMeasureType">
      <rdfs:comment>Reference to a unit of measure definition that applies to all the numerical values described by the element containing this element. Notice that a complexType which needs to include the uom attribute can do so by extending this complexType. Alternately, this complexType can be used as a pattern for a new complexType.</rdfs:comment>
      <rdfs:subClassOf>
         <owl:Class>
            <owl:intersectionOf rdf:parseType="Collection">
               <owl:Restriction>
                  <owl:onProperty rdf:resource="#uom"/>
                  <owl:allValuesFrom rdf:resource="#anyURI"/>
               </owl:Restriction>
            </owl:intersectionOf>
         </owl:Class>
      </rdfs:subClassOf>
   </owl:Class>
   <owl:Class rdf:about="#UnitDefinitionType">
      <rdfs:comment>Definition of a unit of measure (or uom). The definition includes a quantityType property, which indicates the phenomenon to which the units apply, and a catalogSymbol, which gives the short symbol used for this unit. This element is used when the relationship of this unit to other units or units systems is unknown.</rdfs:comment>
      <rdfs:subClassOf>
         <owl:Class>
            <owl:intersectionOf rdf:parseType="Collection">
               <owl:Restriction>
                  <owl:onProperty rdf:resource="gml:hasquantityType"/>
                  <owl:allValuesFrom rdf:resource="gml:quantityType"/>
               </owl:Restriction>
               <owl:Restriction>
                  <owl:onProperty rdf:resource="gml:hascatalogSymbol"/>
                  <owl:allValuesFrom rdf:resource="gml:catalogSymbol"/>
               </owl:Restriction>
               <owl:Restriction>
                  <owl:onProperty rdf:resource="gml:hascatalogSymbol"/>
                  <owl:minCardinality rdf:datatype="http://www.w3.org/2001/XMLSchema#nonNegativeInteger">0</owl:minCardinality>
               </owl:Restriction>
            </owl:intersectionOf>
         </owl:Class>
      </rdfs:subClassOf>
      <rdfs:subClassOf rdf:resource="gml:DefinitionType"/>
      <rdfs:comment>Warning: The parent class 'gml:DefinitionType' is declared outside of this class' original schema. This class may be declared incorrectly.</rdfs:comment>
   </owl:Class>
   <owl:Class rdf:about="#BaseUnitType">
      <rdfs:comment>Definition of a unit of measure which is a base unit from the system of units.  A base unit cannot be derived by combination of other base units within this system.  Sometimes known as "fundamental unit".</rdfs:comment>
      <rdfs:subClassOf>
         <owl:Class>
            <owl:intersectionOf rdf:parseType="Collection">
               <owl:Restriction>
                  <owl:onProperty rdf:resource="#unitsSystem"/>
                  <owl:allValuesFrom rdf:resource="gml:ReferenceType"/>
               </owl:Restriction>
            </owl:intersectionOf>
         </owl:Class>
      </rdfs:subClassOf>
      <rdfs:subClassOf rdf:resource="gml:UnitDefinitionType"/>
      <rdfs:comment>Warning: The parent class 'gml:UnitDefinitionType' is declared outside of this class' original schema. This class may be declared incorrectly.</rdfs:comment>
   </owl:Class>
   <owl:Class rdf:about="#DerivedUnitType">
      <rdfs:comment>Definition of a unit of measure which is defined through algebraic combination of more primitive units, which are usually base units from a particular system of units. Derived units based directly on base units are usually preferred for quantities other than the base units or fundamental quantities within a system.  If a derived unit is not the preferred unit, the ConventionalUnit element should be used instead.</rdfs:comment>
      <rdfs:subClassOf>
         <owl:Class>
            <owl:intersectionOf rdf:parseType="Collection">
               <owl:Restriction>
                  <owl:onProperty rdf:resource="gml:hasderivationUnitTerm"/>
                  <owl:allValuesFrom rdf:resource="gml:derivationUnitTerm"/>
               </owl:Restriction>
            </owl:intersectionOf>
         </owl:Class>
      </rdfs:subClassOf>
      <rdfs:subClassOf rdf:resource="gml:UnitDefinitionType"/>
      <rdfs:comment>Warning: The parent class 'gml:UnitDefinitionType' is declared outside of this class' original schema. This class may be declared incorrectly.</rdfs:comment>
   </owl:Class>
   <owl:Class rdf:about="#ConventionalUnitType">
      <rdfs:comment>Definition of a unit of measure which is related to a preferred unit for this quantity type through a conversion formula.  A method for deriving this unit by algebraic combination of more primitive units, may also be provided.</rdfs:comment>
      <rdfs:subClassOf>
         <owl:Class>
            <owl:intersectionOf rdf:parseType="Collection">
               <owl:Restriction>
                  <owl:onProperty rdf:resource="gml:hasderivationUnitTerm"/>
                  <owl:allValuesFrom rdf:resource="gml:derivationUnitTerm"/>
               </owl:Restriction>
               <owl:Restriction>
                  <owl:onProperty rdf:resource="gml:hasderivationUnitTerm"/>
                  <owl:minCardinality rdf:datatype="http://www.w3.org/2001/XMLSchema#nonNegativeInteger">0</owl:minCardinality>
               </owl:Restriction>
            </owl:intersectionOf>
         </owl:Class>
      </rdfs:subClassOf>
      <rdfs:subClassOf rdf:resource="gml:UnitDefinitionType"/>
      <rdfs:comment>Warning: The parent class 'gml:UnitDefinitionType' is declared outside of this class' original schema. This class may be declared incorrectly.</rdfs:comment>
   </owl:Class>
   <owl:Class rdf:about="#DerivationUnitTermType">
      <rdfs:comment>Definition of one unit term for a derived unit of measure. This unit term references another unit of measure (uom) and provides an integer exponent applied to that unit in defining the compound unit. The exponent can be positive or negative, but not zero.</rdfs:comment>
      <rdfs:subClassOf>
         <owl:Class>
            <owl:intersectionOf rdf:parseType="Collection">
               <owl:Restriction>
                  <owl:onProperty rdf:resource="#exponent"/>
                  <owl:allValuesFrom rdf:resource="#integer"/>
               </owl:Restriction>
            </owl:intersectionOf>
         </owl:Class>
      </rdfs:subClassOf>
      <rdfs:subClassOf rdf:resource="gml:UnitOfMeasureType"/>
      <rdfs:comment>Warning: The parent class 'gml:UnitOfMeasureType' is declared outside of this class' original schema. This class may be declared incorrectly.</rdfs:comment>
   </owl:Class>
   <owl:Class rdf:about="#ConversionToPreferredUnitType">
      <rdfs:comment>Relation of a unit to the preferred unit for this quantity type, specified by an arithmetic conversion (scaling and/or offset). A preferred unit is either a base unit or a derived unit selected for all units of one quantity type. The mandatory attribute "uom" shall reference the preferred unit that this conversion applies to. The conversion is specified by one of two alternative elements: "factor" or "formula".</rdfs:comment>
      <owl:disjointUnionOf rdf:parseType="Collection">
         <owl:Restriction>
            <owl:onProperty rdf:resource="#factor"/>
            <owl:someValuesFrom rdf:resource="#double"/>
         </owl:Restriction>
         <owl:Restriction>
            <owl:onProperty rdf:resource="#formula"/>
            <owl:someValuesFrom rdf:resource="gml:FormulaType"/>
         </owl:Restriction>
      </owl:disjointUnionOf>
      <rdfs:subClassOf rdf:resource="gml:UnitOfMeasureType"/>
      <rdfs:comment>Warning: The parent class 'gml:UnitOfMeasureType' is declared outside of this class' original schema. This class may be declared incorrectly.</rdfs:comment>
   </owl:Class>
   <owl:Class rdf:about="#FormulaType">
      <rdfs:comment>Paremeters of a simple formula by which a value using this unit of measure can be converted to the corresponding value using the preferred unit of measure. The formula element contains elements a, b, c and d, whose values use the XML Schema type "double". These values are used in the formula y = (a + bx) / (c + dx), where x is a value using this unit, and y is the corresponding value using the preferred unit. The elements a and d are optional, and if values are not provided, those parameters are considered to be zero. If values are not provided for both a and d, the formula is equivalent to a fraction with numerator and denominator parameters.</rdfs:comment>
      <rdfs:subClassOf>
         <owl:Class>
            <owl:intersectionOf rdf:parseType="Collection">
               <owl:Restriction>
                  <owl:onProperty rdf:resource="#a"/>
                  <owl:allValuesFrom rdf:resource="#double"/>
               </owl:Restriction>
               <owl:Restriction>
                  <owl:onProperty rdf:resource="#a"/>
                  <owl:minCardinality rdf:datatype="http://www.w3.org/2001/XMLSchema#nonNegativeInteger">0</owl:minCardinality>
               </owl:Restriction>
               <owl:Restriction>
                  <owl:onProperty rdf:resource="#b"/>
                  <owl:allValuesFrom rdf:resource="#double"/>
               </owl:Restriction>
               <owl:Restriction>
                  <owl:onProperty rdf:resource="#c"/>
                  <owl:allValuesFrom rdf:resource="#double"/>
               </owl:Restriction>
               <owl:Restriction>
                  <owl:onProperty rdf:resource="#d"/>
                  <owl:allValuesFrom rdf:resource="#double"/>
               </owl:Restriction>
               <owl:Restriction>
                  <owl:onProperty rdf:resource="#d"/>
                  <owl:minCardinality rdf:datatype="http://www.w3.org/2001/XMLSchema#nonNegativeInteger">0</owl:minCardinality>
               </owl:Restriction>
            </owl:intersectionOf>
         </owl:Class>
      </rdfs:subClassOf>
   </owl:Class>
   <owl:DatatypeProperty rdf:about="#uom">
      <rdfs:domain rdf:resource="#UnitOfMeasureType"/>
      <rdfs:range rdf:resource="#anyURI"/>
   </owl:DatatypeProperty>
   <owl:DatatypeProperty rdf:about="#exponent">
      <rdfs:domain rdf:resource="#DerivationUnitTermType"/>
      <rdfs:range rdf:resource="#integer"/>
   </owl:DatatypeProperty>
   <owl:Class rdf:about="#unitOfMeasure">
      <rdfs:subClassOf rdf:resource="gml:UnitOfMeasureType"/>
      <rdfs:comment>Warning: This class type was declared outside of its original schema. This class may be declared incorrectly.</rdfs:comment>
   </owl:Class>
   <owl:Class rdf:about="#UnitDefinition">
      <rdfs:subClassOf rdf:resource="gml:Definition"/>
      <rdfs:subClassOf rdf:resource="gml:UnitDefinitionType"/>
      <rdfs:comment>Warning: This class type was declared outside of its original schema. This class may be declared incorrectly.</rdfs:comment>
   </owl:Class>
   <owl:Class rdf:about="#BaseUnit">
      <rdfs:subClassOf rdf:resource="gml:UnitDefinition"/>
      <rdfs:subClassOf rdf:resource="gml:BaseUnitType"/>
      <rdfs:comment>Warning: This class type was declared outside of its original schema. This class may be declared incorrectly.</rdfs:comment>
   </owl:Class>
   <owl:Class rdf:about="#DerivedUnit">
      <rdfs:subClassOf rdf:resource="gml:UnitDefinition"/>
      <rdfs:subClassOf rdf:resource="gml:DerivedUnitType"/>
      <rdfs:comment>Warning: This class type was declared outside of its original schema. This class may be declared incorrectly.</rdfs:comment>
   </owl:Class>
   <owl:Class rdf:about="#ConventionalUnit">
      <rdfs:subClassOf rdf:resource="gml:UnitDefinition"/>
      <rdfs:subClassOf rdf:resource="gml:ConventionalUnitType"/>
      <rdfs:comment>Warning: This class type was declared outside of its original schema. This class may be declared incorrectly.</rdfs:comment>
   </owl:Class>
   <owl:Class rdf:about="#quantityType">
      <rdfs:subClassOf rdf:resource="gml:StringOrRefType"/>
      <rdfs:comment>Warning: This class type was declared outside of its original schema. This class may be declared incorrectly.</rdfs:comment>
   </owl:Class>
   <owl:Class rdf:about="#catalogSymbol">
      <rdfs:subClassOf rdf:resource="gml:CodeType"/>
      <rdfs:comment>Warning: This class type was declared outside of its original schema. This class may be declared incorrectly.</rdfs:comment>
   </owl:Class>
   <owl:Class rdf:about="#derivationUnitTerm">
      <rdfs:subClassOf rdf:resource="gml:DerivationUnitTermType"/>
      <rdfs:comment>Warning: This class type was declared outside of its original schema. This class may be declared incorrectly.</rdfs:comment>
   </owl:Class>
   <owl:Class rdf:about="#conversionToPreferredUnit">
      <rdfs:subClassOf rdf:resource="gml:ConversionToPreferredUnitType"/>
      <rdfs:comment>Warning: This class type was declared outside of its original schema. This class may be declared incorrectly.</rdfs:comment>
   </owl:Class>
   <owl:Class rdf:about="#roughConversionToPreferredUnit">
      <rdfs:subClassOf rdf:resource="gml:ConversionToPreferredUnitType"/>
      <rdfs:comment>Warning: This class type was declared outside of its original schema. This class may be declared incorrectly.</rdfs:comment>
   </owl:Class>
   <owl:ObjectProperty rdf:about="gml:hasquantityType">
      <rdfs:comment>Warning: This ObjectProperty reference was declared outside of its original schema. This ObjectProperty may be declared incorrectly.</rdfs:comment>
      <rdfs:domain rdf:resource="#UnitDefinitionType"/>
      <rdfs:range rdf:resource="gml:quantityType"/>
   </owl:ObjectProperty>
   <owl:ObjectProperty rdf:about="gml:hascatalogSymbol">
      <rdfs:comment>Warning: This ObjectProperty reference was declared outside of its original schema. This ObjectProperty may be declared incorrectly.</rdfs:comment>
      <rdfs:domain rdf:resource="#UnitDefinitionType"/>
      <rdfs:range rdf:resource="gml:catalogSymbol"/>
   </owl:ObjectProperty>
   <owl:ObjectProperty rdf:about="#unitsSystem">
      <rdfs:comment>Warning: This ObjectProperty type was declared outside of its original schema. This ObjectProperty may be declared incorrectly.</rdfs:comment>
      <rdfs:domain rdf:resource="#BaseUnitType"/>
      <rdfs:range rdf:resource="gml:ReferenceType"/>
   </owl:ObjectProperty>
   <owl:ObjectProperty rdf:about="gml:hasderivationUnitTerm">
      <rdfs:comment>Warning: This ObjectProperty reference was declared outside of its original schema. This ObjectProperty may be declared incorrectly.</rdfs:comment>
      <rdfs:domain rdf:resource="#DerivedUnitType"/>
      <rdfs:range rdf:resource="gml:derivationUnitTerm"/>
   </owl:ObjectProperty>
   <owl:ObjectProperty rdf:about="gml:hasconversionToPreferredUnit">
      <rdfs:comment>Warning: This ObjectProperty reference was declared outside of its original schema. This ObjectProperty may be declared incorrectly.</rdfs:comment>
      <rdfs:domain rdf:resource="#ConventionalUnitType"/>
      <rdfs:range rdf:resource="gml:conversionToPreferredUnit"/>
   </owl:ObjectProperty>
   <owl:ObjectProperty rdf:about="gml:hasroughConversionToPreferredUnit">
      <rdfs:comment>Warning: This ObjectProperty reference was declared outside of its original schema. This ObjectProperty may be declared incorrectly.</rdfs:comment>
      <rdfs:domain rdf:resource="#ConventionalUnitType"/>
      <rdfs:range rdf:resource="gml:roughConversionToPreferredUnit"/>
   </owl:ObjectProperty>
   <owl:ObjectProperty rdf:about="gml:hasderivationUnitTerm">
      <rdfs:comment>Warning: This ObjectProperty reference was declared outside of its original schema. This ObjectProperty may be declared incorrectly.</rdfs:comment>
      <rdfs:domain rdf:resource="#ConventionalUnitType"/>
      <rdfs:range rdf:resource="gml:derivationUnitTerm"/>
   </owl:ObjectProperty>
   <owl:DatatypeProperty rdf:about="#has">
      <rdfs:domain rdf:resource="#ConversionToPreferredUnitType"/>
      <rdfs:range rdf:resource="#"/>
   </owl:DatatypeProperty>
   <owl:ObjectProperty rdf:about="#formula">
      <rdfs:comment>Warning: This ObjectProperty type was declared outside of its original schema. This ObjectProperty may be declared incorrectly.</rdfs:comment>
      <rdfs:domain rdf:resource="#ConversionToPreferredUnitType"/>
      <rdfs:range rdf:resource="gml:FormulaType"/>
   </owl:ObjectProperty>
   <owl:DatatypeProperty rdf:about="#has">
      <rdfs:domain rdf:resource="#FormulaType"/>
      <rdfs:range rdf:resource="#"/>
   </owl:DatatypeProperty>
   <owl:DatatypeProperty rdf:about="#has">
      <rdfs:domain rdf:resource="#FormulaType"/>
      <rdfs:range rdf:resource="#"/>
   </owl:DatatypeProperty>
   <owl:DatatypeProperty rdf:about="#has">
      <rdfs:domain rdf:resource="#FormulaType"/>
      <rdfs:range rdf:resource="#"/>
   </owl:DatatypeProperty>
   <owl:DatatypeProperty rdf:about="#has">
      <rdfs:domain rdf:resource="#FormulaType"/>
      <rdfs:range rdf:resource="#"/>
   </owl:DatatypeProperty>
</rdf:RDF>
