<rdf:RDF xmlns:math="http://www.w3.org/2005/xpath-functions/math" xmlns:owl="http://www.w3.org/2002/07/owl#" xmlns:rdf="http://www.w3.org/1999/02/22-rdf-syntax-ns#" xmlns:rdfs="http://www.w3.org/2000/01/rdf-schema#" xmlns:xs="http://www.w3.org/2001/XMLSchema" xmlns:xsd="http://www.w3.org/2001/XMLSchema">
   <owl:Ontology rdf:about="http://liris.cnrs.fr/ontologies/waterBody">
      <owl:imports rdf:resource="http://liris.cnrs.fr/ontologies/gml"/>
      <owl:imports rdf:resource="http://liris.cnrs.fr/ontologies/cityGMLBase"/>
      <rdfs:comment>
	CityGML is an OGC Standard.
	Copyright (c) 2012 Open Geospatial Consortium.
	To obtain additional rights of use, visit http://www.opengeospatial.org/legal/ .
		</rdfs:comment>
   </owl:Ontology>
   <owl:Class rdf:about="#AbstractWaterObjectType">
      <rdfs:comment>This is an abstract class</rdfs:comment>
      <rdfs:comment>Type describing the abstract superclass for water objects. As subclass of _CityObject, a _WaterObject
				inherits all attributes and relations, in particular an id, names, external references, and generalization relations.
			</rdfs:comment>
      <rdfs:subClassOf>
         <owl:Class>
            <owl:intersectionOf rdf:parseType="Collection">
               <owl:Restriction>
                  <owl:onProperty rdf:resource="#has_GenericApplicationPropertyOfWaterObject"/>
                  <owl:allValuesFrom rdf:resource="#_GenericApplicationPropertyOfWaterObject"/>
               </owl:Restriction>
               <owl:Restriction>
                  <owl:onProperty rdf:resource="#has_GenericApplicationPropertyOfWaterObject"/>
                  <owl:minCardinality rdf:datatype="http://www.w3.org/2001/XMLSchema#nonNegativeInteger">0</owl:minCardinality>
               </owl:Restriction>
            </owl:intersectionOf>
         </owl:Class>
      </rdfs:subClassOf>
      <rdfs:subClassOf rdf:resource="core:AbstractCityObjectType"/>
      <rdfs:comment>Warning: The parent class 'core:AbstractCityObjectType' is declared outside of this class' original schema. This class may be declared incorrectly.</rdfs:comment>
   </owl:Class>
   <owl:Class rdf:about="#WaterBodyType">
      <rdfs:comment>Type describing Water Bodies, e.g., lakes, rivers. As subclass of _CityObject, a WaterBody inherits all
				attributes and relations, in particular an id, names, external references, and generalization relations.
			</rdfs:comment>
      <rdfs:subClassOf>
         <owl:Class>
            <owl:intersectionOf rdf:parseType="Collection">
               <owl:Restriction>
                  <owl:onProperty rdf:resource="#class"/>
                  <owl:allValuesFrom rdf:resource="gml:CodeType"/>
               </owl:Restriction>
               <owl:Restriction>
                  <owl:onProperty rdf:resource="#class"/>
                  <owl:minCardinality rdf:datatype="http://www.w3.org/2001/XMLSchema#nonNegativeInteger">0</owl:minCardinality>
               </owl:Restriction>
               <owl:Restriction>
                  <owl:onProperty rdf:resource="#function"/>
                  <owl:allValuesFrom rdf:resource="gml:CodeType"/>
               </owl:Restriction>
               <owl:Restriction>
                  <owl:onProperty rdf:resource="#function"/>
                  <owl:minCardinality rdf:datatype="http://www.w3.org/2001/XMLSchema#nonNegativeInteger">0</owl:minCardinality>
               </owl:Restriction>
               <owl:Restriction>
                  <owl:onProperty rdf:resource="#usage"/>
                  <owl:allValuesFrom rdf:resource="gml:CodeType"/>
               </owl:Restriction>
               <owl:Restriction>
                  <owl:onProperty rdf:resource="#usage"/>
                  <owl:minCardinality rdf:datatype="http://www.w3.org/2001/XMLSchema#nonNegativeInteger">0</owl:minCardinality>
               </owl:Restriction>
               <owl:Restriction>
                  <owl:onProperty rdf:resource="#lod0MultiCurve"/>
                  <owl:allValuesFrom rdf:resource="gml:MultiCurvePropertyType"/>
               </owl:Restriction>
               <owl:Restriction>
                  <owl:onProperty rdf:resource="#lod0MultiCurve"/>
                  <owl:minCardinality rdf:datatype="http://www.w3.org/2001/XMLSchema#nonNegativeInteger">0</owl:minCardinality>
               </owl:Restriction>
               <owl:Restriction>
                  <owl:onProperty rdf:resource="#lod0MultiSurface"/>
                  <owl:allValuesFrom rdf:resource="gml:MultiSurfacePropertyType"/>
               </owl:Restriction>
               <owl:Restriction>
                  <owl:onProperty rdf:resource="#lod0MultiSurface"/>
                  <owl:minCardinality rdf:datatype="http://www.w3.org/2001/XMLSchema#nonNegativeInteger">0</owl:minCardinality>
               </owl:Restriction>
               <owl:Restriction>
                  <owl:onProperty rdf:resource="#lod1MultiCurve"/>
                  <owl:allValuesFrom rdf:resource="gml:MultiCurvePropertyType"/>
               </owl:Restriction>
               <owl:Restriction>
                  <owl:onProperty rdf:resource="#lod1MultiCurve"/>
                  <owl:minCardinality rdf:datatype="http://www.w3.org/2001/XMLSchema#nonNegativeInteger">0</owl:minCardinality>
               </owl:Restriction>
               <owl:Restriction>
                  <owl:onProperty rdf:resource="#lod1MultiSurface"/>
                  <owl:allValuesFrom rdf:resource="gml:MultiSurfacePropertyType"/>
               </owl:Restriction>
               <owl:Restriction>
                  <owl:onProperty rdf:resource="#lod1MultiSurface"/>
                  <owl:minCardinality rdf:datatype="http://www.w3.org/2001/XMLSchema#nonNegativeInteger">0</owl:minCardinality>
               </owl:Restriction>
               <owl:Restriction>
                  <owl:onProperty rdf:resource="#lod1Solid"/>
                  <owl:allValuesFrom rdf:resource="gml:SolidPropertyType"/>
               </owl:Restriction>
               <owl:Restriction>
                  <owl:onProperty rdf:resource="#lod1Solid"/>
                  <owl:minCardinality rdf:datatype="http://www.w3.org/2001/XMLSchema#nonNegativeInteger">0</owl:minCardinality>
               </owl:Restriction>
               <owl:Restriction>
                  <owl:onProperty rdf:resource="#lod2Solid"/>
                  <owl:allValuesFrom rdf:resource="gml:SolidPropertyType"/>
               </owl:Restriction>
               <owl:Restriction>
                  <owl:onProperty rdf:resource="#lod2Solid"/>
                  <owl:minCardinality rdf:datatype="http://www.w3.org/2001/XMLSchema#nonNegativeInteger">0</owl:minCardinality>
               </owl:Restriction>
               <owl:Restriction>
                  <owl:onProperty rdf:resource="#lod3Solid"/>
                  <owl:allValuesFrom rdf:resource="gml:SolidPropertyType"/>
               </owl:Restriction>
               <owl:Restriction>
                  <owl:onProperty rdf:resource="#lod3Solid"/>
                  <owl:minCardinality rdf:datatype="http://www.w3.org/2001/XMLSchema#nonNegativeInteger">0</owl:minCardinality>
               </owl:Restriction>
               <owl:Restriction>
                  <owl:onProperty rdf:resource="#lod4Solid"/>
                  <owl:allValuesFrom rdf:resource="gml:SolidPropertyType"/>
               </owl:Restriction>
               <owl:Restriction>
                  <owl:onProperty rdf:resource="#lod4Solid"/>
                  <owl:minCardinality rdf:datatype="http://www.w3.org/2001/XMLSchema#nonNegativeInteger">0</owl:minCardinality>
               </owl:Restriction>
               <owl:Restriction>
                  <owl:onProperty rdf:resource="#boundedBy"/>
                  <owl:allValuesFrom rdf:resource="#BoundedByWaterSurfacePropertyType"/>
               </owl:Restriction>
               <owl:Restriction>
                  <owl:onProperty rdf:resource="#boundedBy"/>
                  <owl:minCardinality rdf:datatype="http://www.w3.org/2001/XMLSchema#nonNegativeInteger">0</owl:minCardinality>
               </owl:Restriction>
               <owl:Restriction>
                  <owl:onProperty rdf:resource="#has_GenericApplicationPropertyOfWaterBody"/>
                  <owl:allValuesFrom rdf:resource="#_GenericApplicationPropertyOfWaterBody"/>
               </owl:Restriction>
               <owl:Restriction>
                  <owl:onProperty rdf:resource="#has_GenericApplicationPropertyOfWaterBody"/>
                  <owl:minCardinality rdf:datatype="http://www.w3.org/2001/XMLSchema#nonNegativeInteger">0</owl:minCardinality>
               </owl:Restriction>
            </owl:intersectionOf>
         </owl:Class>
      </rdfs:subClassOf>
      <rdfs:subClassOf rdf:resource="#AbstractWaterObjectType"/>
   </owl:Class>
   <owl:Class rdf:about="#BoundedByWaterSurfacePropertyType">
      <rdfs:comment>Denotes the relation of a WaterBody to its boundary surfaces, which are of type _WaterBoundarySurface. The
				BoundedByWaterSurfacePropertyType element must either carry a reference to a _WaterBoundarySurface object or contain a
				_WaterBoundarySurface object inline, but neither both nor none. </rdfs:comment>
      <rdfs:subClassOf>
         <owl:Class>
            <owl:intersectionOf rdf:parseType="Collection">
               <owl:Restriction>
                  <owl:onProperty rdf:resource="#has_WaterBoundarySurface"/>
                  <owl:allValuesFrom rdf:resource="#_WaterBoundarySurface"/>
               </owl:Restriction>
            </owl:intersectionOf>
         </owl:Class>
      </rdfs:subClassOf>
   </owl:Class>
   <owl:Class rdf:about="#AbstractWaterBoundarySurfaceType">
      <rdfs:comment>This is an abstract class</rdfs:comment>
      <rdfs:comment>A WaterBoundarySurface is a thematic object which classifies surfaces bounding a water body.
			</rdfs:comment>
      <rdfs:subClassOf>
         <owl:Class>
            <owl:intersectionOf rdf:parseType="Collection">
               <owl:Restriction>
                  <owl:onProperty rdf:resource="#lod2Surface"/>
                  <owl:allValuesFrom rdf:resource="gml:SurfacePropertyType"/>
               </owl:Restriction>
               <owl:Restriction>
                  <owl:onProperty rdf:resource="#lod2Surface"/>
                  <owl:minCardinality rdf:datatype="http://www.w3.org/2001/XMLSchema#nonNegativeInteger">0</owl:minCardinality>
               </owl:Restriction>
               <owl:Restriction>
                  <owl:onProperty rdf:resource="#lod3Surface"/>
                  <owl:allValuesFrom rdf:resource="gml:SurfacePropertyType"/>
               </owl:Restriction>
               <owl:Restriction>
                  <owl:onProperty rdf:resource="#lod3Surface"/>
                  <owl:minCardinality rdf:datatype="http://www.w3.org/2001/XMLSchema#nonNegativeInteger">0</owl:minCardinality>
               </owl:Restriction>
               <owl:Restriction>
                  <owl:onProperty rdf:resource="#lod4Surface"/>
                  <owl:allValuesFrom rdf:resource="gml:SurfacePropertyType"/>
               </owl:Restriction>
               <owl:Restriction>
                  <owl:onProperty rdf:resource="#lod4Surface"/>
                  <owl:minCardinality rdf:datatype="http://www.w3.org/2001/XMLSchema#nonNegativeInteger">0</owl:minCardinality>
               </owl:Restriction>
               <owl:Restriction>
                  <owl:onProperty rdf:resource="#has_GenericApplicationPropertyOfWaterBoundarySurface"/>
                  <owl:allValuesFrom rdf:resource="#_GenericApplicationPropertyOfWaterBoundarySurface"/>
               </owl:Restriction>
               <owl:Restriction>
                  <owl:onProperty rdf:resource="#has_GenericApplicationPropertyOfWaterBoundarySurface"/>
                  <owl:minCardinality rdf:datatype="http://www.w3.org/2001/XMLSchema#nonNegativeInteger">0</owl:minCardinality>
               </owl:Restriction>
            </owl:intersectionOf>
         </owl:Class>
      </rdfs:subClassOf>
      <rdfs:subClassOf rdf:resource="core:AbstractCityObjectType"/>
      <rdfs:comment>Warning: The parent class 'core:AbstractCityObjectType' is declared outside of this class' original schema. This class may be declared incorrectly.</rdfs:comment>
   </owl:Class>
   <owl:Class rdf:about="#WaterSurfaceType">
      <rdfs:comment>Type describing the surface of a water body, which separates the water from the air. As subclass of
				_CityObject, a WaterSurface inherits all attributes and relations, in particular an id, names, external references, and
				generalization relations. </rdfs:comment>
      <rdfs:subClassOf>
         <owl:Class>
            <owl:intersectionOf rdf:parseType="Collection">
               <owl:Restriction>
                  <owl:onProperty rdf:resource="#waterLevel"/>
                  <owl:allValuesFrom rdf:resource="gml:CodeType"/>
               </owl:Restriction>
               <owl:Restriction>
                  <owl:onProperty rdf:resource="#waterLevel"/>
                  <owl:minCardinality rdf:datatype="http://www.w3.org/2001/XMLSchema#nonNegativeInteger">0</owl:minCardinality>
               </owl:Restriction>
               <owl:Restriction>
                  <owl:onProperty rdf:resource="#has_GenericApplicationPropertyOfWaterSurface"/>
                  <owl:allValuesFrom rdf:resource="#_GenericApplicationPropertyOfWaterSurface"/>
               </owl:Restriction>
               <owl:Restriction>
                  <owl:onProperty rdf:resource="#has_GenericApplicationPropertyOfWaterSurface"/>
                  <owl:minCardinality rdf:datatype="http://www.w3.org/2001/XMLSchema#nonNegativeInteger">0</owl:minCardinality>
               </owl:Restriction>
            </owl:intersectionOf>
         </owl:Class>
      </rdfs:subClassOf>
      <rdfs:subClassOf rdf:resource="#AbstractWaterBoundarySurfaceType"/>
   </owl:Class>
   <owl:Class rdf:about="#WaterGroundSurfaceType">
      <rdfs:comment>Type describing the ground surface of a water body, i.e. the boundary to the digital terrain model. As
				subclass of _CityObject, a WaterGroundSurface inherits all attributes and relations, in particular an id, names, external
				references, and generalization relations. </rdfs:comment>
      <rdfs:subClassOf>
         <owl:Class>
            <owl:intersectionOf rdf:parseType="Collection">
               <owl:Restriction>
                  <owl:onProperty rdf:resource="#has_GenericApplicationPropertyOfWaterGroundSurface"/>
                  <owl:allValuesFrom rdf:resource="#_GenericApplicationPropertyOfWaterGroundSurface"/>
               </owl:Restriction>
               <owl:Restriction>
                  <owl:onProperty rdf:resource="#has_GenericApplicationPropertyOfWaterGroundSurface"/>
                  <owl:minCardinality rdf:datatype="http://www.w3.org/2001/XMLSchema#nonNegativeInteger">0</owl:minCardinality>
               </owl:Restriction>
            </owl:intersectionOf>
         </owl:Class>
      </rdfs:subClassOf>
      <rdfs:subClassOf rdf:resource="#AbstractWaterBoundarySurfaceType"/>
   </owl:Class>
   <owl:Class rdf:about="#WaterClosureSurfaceType">
      <rdfs:comment>Type describing the closure surface between water bodys. As subclass of _CityObject, a WaterClosureSurface
				inherits all attributes and relations, in particular an id, names, external references, and generalization relations.
			</rdfs:comment>
      <rdfs:subClassOf>
         <owl:Class>
            <owl:intersectionOf rdf:parseType="Collection">
               <owl:Restriction>
                  <owl:onProperty rdf:resource="#has_GenericApplicationPropertyOfWaterClosureSurface"/>
                  <owl:allValuesFrom rdf:resource="#_GenericApplicationPropertyOfWaterClosureSurface"/>
               </owl:Restriction>
               <owl:Restriction>
                  <owl:onProperty rdf:resource="#has_GenericApplicationPropertyOfWaterClosureSurface"/>
                  <owl:minCardinality rdf:datatype="http://www.w3.org/2001/XMLSchema#nonNegativeInteger">0</owl:minCardinality>
               </owl:Restriction>
            </owl:intersectionOf>
         </owl:Class>
      </rdfs:subClassOf>
      <rdfs:subClassOf rdf:resource="#AbstractWaterBoundarySurfaceType"/>
   </owl:Class>
   <owl:ObjectProperty rdf:about="gml:hasAssociationAttributeGroup">
      <rdfs:domain rdf:resource="#BoundedByWaterSurfacePropertyType"/>
      <rdfs:range rdf:resource="gml:AssociationAttributeGroup"/>
   </owl:ObjectProperty>
   <owl:Class rdf:about="#_WaterObject">
      <rdfs:subClassOf rdf:resource="core:_CityObject"/>
      <rdfs:subClassOf rdf:resource="#AbstractWaterObjectType"/>
   </owl:Class>
   <owl:Class rdf:about="#_GenericApplicationPropertyOfWaterObject">
      <rdfs:subClassOf rdf:resource="http://www.w3.org/2001/XMLSchema#anyType"/>
      <rdfs:comment>Warning: This class type was declared outside of its original schema. This class may be declared incorrectly.</rdfs:comment>
   </owl:Class>
   <owl:Class rdf:about="#WaterBody">
      <rdfs:subClassOf rdf:resource="#_WaterObject"/>
      <rdfs:subClassOf rdf:resource="#WaterBodyType"/>
   </owl:Class>
   <owl:Class rdf:about="#_GenericApplicationPropertyOfWaterBody">
      <rdfs:subClassOf rdf:resource="http://www.w3.org/2001/XMLSchema#anyType"/>
      <rdfs:comment>Warning: This class type was declared outside of its original schema. This class may be declared incorrectly.</rdfs:comment>
   </owl:Class>
   <owl:Class rdf:about="#_WaterBoundarySurface">
      <rdfs:subClassOf rdf:resource="core:_CityObject"/>
      <rdfs:subClassOf rdf:resource="#AbstractWaterBoundarySurfaceType"/>
   </owl:Class>
   <owl:Class rdf:about="#_GenericApplicationPropertyOfWaterBoundarySurface">
      <rdfs:subClassOf rdf:resource="http://www.w3.org/2001/XMLSchema#anyType"/>
      <rdfs:comment>Warning: This class type was declared outside of its original schema. This class may be declared incorrectly.</rdfs:comment>
   </owl:Class>
   <owl:Class rdf:about="#WaterSurface">
      <rdfs:subClassOf rdf:resource="#_WaterBoundarySurface"/>
      <rdfs:subClassOf rdf:resource="#WaterSurfaceType"/>
   </owl:Class>
   <owl:Class rdf:about="#_GenericApplicationPropertyOfWaterSurface">
      <rdfs:subClassOf rdf:resource="http://www.w3.org/2001/XMLSchema#anyType"/>
      <rdfs:comment>Warning: This class type was declared outside of its original schema. This class may be declared incorrectly.</rdfs:comment>
   </owl:Class>
   <owl:Class rdf:about="#WaterGroundSurface">
      <rdfs:subClassOf rdf:resource="#_WaterBoundarySurface"/>
      <rdfs:subClassOf rdf:resource="#WaterGroundSurfaceType"/>
   </owl:Class>
   <owl:Class rdf:about="#_GenericApplicationPropertyOfWaterGroundSurface">
      <rdfs:subClassOf rdf:resource="http://www.w3.org/2001/XMLSchema#anyType"/>
      <rdfs:comment>Warning: This class type was declared outside of its original schema. This class may be declared incorrectly.</rdfs:comment>
   </owl:Class>
   <owl:Class rdf:about="#WaterClosureSurface">
      <rdfs:subClassOf rdf:resource="#_WaterBoundarySurface"/>
      <rdfs:subClassOf rdf:resource="#WaterClosureSurfaceType"/>
   </owl:Class>
   <owl:Class rdf:about="#_GenericApplicationPropertyOfWaterClosureSurface">
      <rdfs:subClassOf rdf:resource="http://www.w3.org/2001/XMLSchema#anyType"/>
      <rdfs:comment>Warning: This class type was declared outside of its original schema. This class may be declared incorrectly.</rdfs:comment>
   </owl:Class>
   <owl:ObjectProperty rdf:about="#has_GenericApplicationPropertyOfWaterObject">
      <rdfs:domain rdf:resource="#AbstractWaterObjectType"/>
      <rdfs:range rdf:resource="#_GenericApplicationPropertyOfWaterObject"/>
   </owl:ObjectProperty>
   <owl:ObjectProperty rdf:about="#class">
      <rdfs:comment>Warning: This ObjectProperty type was declared outside of its original schema. This ObjectProperty may be declared incorrectly.</rdfs:comment>
      <rdfs:domain rdf:resource="#WaterBodyType"/>
      <rdfs:range rdf:resource="gml:CodeType"/>
   </owl:ObjectProperty>
   <owl:ObjectProperty rdf:about="#function">
      <rdfs:comment>Warning: This ObjectProperty type was declared outside of its original schema. This ObjectProperty may be declared incorrectly.</rdfs:comment>
      <rdfs:domain rdf:resource="#WaterBodyType"/>
      <rdfs:range rdf:resource="gml:CodeType"/>
   </owl:ObjectProperty>
   <owl:ObjectProperty rdf:about="#usage">
      <rdfs:comment>Warning: This ObjectProperty type was declared outside of its original schema. This ObjectProperty may be declared incorrectly.</rdfs:comment>
      <rdfs:domain rdf:resource="#WaterBodyType"/>
      <rdfs:range rdf:resource="gml:CodeType"/>
   </owl:ObjectProperty>
   <owl:ObjectProperty rdf:about="#lod0MultiCurve">
      <rdfs:comment>Warning: This ObjectProperty type was declared outside of its original schema. This ObjectProperty may be declared incorrectly.</rdfs:comment>
      <rdfs:domain rdf:resource="#WaterBodyType"/>
      <rdfs:range rdf:resource="gml:MultiCurvePropertyType"/>
   </owl:ObjectProperty>
   <owl:ObjectProperty rdf:about="#lod0MultiSurface">
      <rdfs:comment>Warning: This ObjectProperty type was declared outside of its original schema. This ObjectProperty may be declared incorrectly.</rdfs:comment>
      <rdfs:domain rdf:resource="#WaterBodyType"/>
      <rdfs:range rdf:resource="gml:MultiSurfacePropertyType"/>
   </owl:ObjectProperty>
   <owl:ObjectProperty rdf:about="#lod1MultiCurve">
      <rdfs:comment>Warning: This ObjectProperty type was declared outside of its original schema. This ObjectProperty may be declared incorrectly.</rdfs:comment>
      <rdfs:domain rdf:resource="#WaterBodyType"/>
      <rdfs:range rdf:resource="gml:MultiCurvePropertyType"/>
   </owl:ObjectProperty>
   <owl:ObjectProperty rdf:about="#lod1MultiSurface">
      <rdfs:comment>Warning: This ObjectProperty type was declared outside of its original schema. This ObjectProperty may be declared incorrectly.</rdfs:comment>
      <rdfs:domain rdf:resource="#WaterBodyType"/>
      <rdfs:range rdf:resource="gml:MultiSurfacePropertyType"/>
   </owl:ObjectProperty>
   <owl:ObjectProperty rdf:about="#lod1Solid">
      <rdfs:comment>Warning: This ObjectProperty type was declared outside of its original schema. This ObjectProperty may be declared incorrectly.</rdfs:comment>
      <rdfs:domain rdf:resource="#WaterBodyType"/>
      <rdfs:range rdf:resource="gml:SolidPropertyType"/>
   </owl:ObjectProperty>
   <owl:ObjectProperty rdf:about="#lod2Solid">
      <rdfs:comment>Warning: This ObjectProperty type was declared outside of its original schema. This ObjectProperty may be declared incorrectly.</rdfs:comment>
      <rdfs:domain rdf:resource="#WaterBodyType"/>
      <rdfs:range rdf:resource="gml:SolidPropertyType"/>
   </owl:ObjectProperty>
   <owl:ObjectProperty rdf:about="#lod3Solid">
      <rdfs:comment>Warning: This ObjectProperty type was declared outside of its original schema. This ObjectProperty may be declared incorrectly.</rdfs:comment>
      <rdfs:domain rdf:resource="#WaterBodyType"/>
      <rdfs:range rdf:resource="gml:SolidPropertyType"/>
   </owl:ObjectProperty>
   <owl:ObjectProperty rdf:about="#lod4Solid">
      <rdfs:comment>Warning: This ObjectProperty type was declared outside of its original schema. This ObjectProperty may be declared incorrectly.</rdfs:comment>
      <rdfs:domain rdf:resource="#WaterBodyType"/>
      <rdfs:range rdf:resource="gml:SolidPropertyType"/>
   </owl:ObjectProperty>
   <owl:ObjectProperty rdf:about="#boundedBy">
      <rdfs:domain rdf:resource="#WaterBodyType"/>
      <rdfs:range rdf:resource="#BoundedByWaterSurfacePropertyType"/>
   </owl:ObjectProperty>
   <owl:ObjectProperty rdf:about="#has_GenericApplicationPropertyOfWaterBody">
      <rdfs:domain rdf:resource="#WaterBodyType"/>
      <rdfs:range rdf:resource="#_GenericApplicationPropertyOfWaterBody"/>
   </owl:ObjectProperty>
   <owl:ObjectProperty rdf:about="#has_WaterBoundarySurface">
      <rdfs:domain rdf:resource="#BoundedByWaterSurfacePropertyType"/>
      <rdfs:range rdf:resource="#_WaterBoundarySurface"/>
   </owl:ObjectProperty>
   <owl:ObjectProperty rdf:about="#lod2Surface">
      <rdfs:comment>Warning: This ObjectProperty type was declared outside of its original schema. This ObjectProperty may be declared incorrectly.</rdfs:comment>
      <rdfs:domain rdf:resource="#AbstractWaterBoundarySurfaceType"/>
      <rdfs:range rdf:resource="gml:SurfacePropertyType"/>
   </owl:ObjectProperty>
   <owl:ObjectProperty rdf:about="#lod3Surface">
      <rdfs:comment>Warning: This ObjectProperty type was declared outside of its original schema. This ObjectProperty may be declared incorrectly.</rdfs:comment>
      <rdfs:domain rdf:resource="#AbstractWaterBoundarySurfaceType"/>
      <rdfs:range rdf:resource="gml:SurfacePropertyType"/>
   </owl:ObjectProperty>
   <owl:ObjectProperty rdf:about="#lod4Surface">
      <rdfs:comment>Warning: This ObjectProperty type was declared outside of its original schema. This ObjectProperty may be declared incorrectly.</rdfs:comment>
      <rdfs:domain rdf:resource="#AbstractWaterBoundarySurfaceType"/>
      <rdfs:range rdf:resource="gml:SurfacePropertyType"/>
   </owl:ObjectProperty>
   <owl:ObjectProperty rdf:about="#has_GenericApplicationPropertyOfWaterBoundarySurface">
      <rdfs:domain rdf:resource="#AbstractWaterBoundarySurfaceType"/>
      <rdfs:range rdf:resource="#_GenericApplicationPropertyOfWaterBoundarySurface"/>
   </owl:ObjectProperty>
   <owl:ObjectProperty rdf:about="#waterLevel">
      <rdfs:comment>Warning: This ObjectProperty type was declared outside of its original schema. This ObjectProperty may be declared incorrectly.</rdfs:comment>
      <rdfs:domain rdf:resource="#WaterSurfaceType"/>
      <rdfs:range rdf:resource="gml:CodeType"/>
   </owl:ObjectProperty>
   <owl:ObjectProperty rdf:about="#has_GenericApplicationPropertyOfWaterSurface">
      <rdfs:domain rdf:resource="#WaterSurfaceType"/>
      <rdfs:range rdf:resource="#_GenericApplicationPropertyOfWaterSurface"/>
   </owl:ObjectProperty>
   <owl:ObjectProperty rdf:about="#has_GenericApplicationPropertyOfWaterGroundSurface">
      <rdfs:domain rdf:resource="#WaterGroundSurfaceType"/>
      <rdfs:range rdf:resource="#_GenericApplicationPropertyOfWaterGroundSurface"/>
   </owl:ObjectProperty>
   <owl:ObjectProperty rdf:about="#has_GenericApplicationPropertyOfWaterClosureSurface">
      <rdfs:domain rdf:resource="#WaterClosureSurfaceType"/>
      <rdfs:range rdf:resource="#_GenericApplicationPropertyOfWaterClosureSurface"/>
   </owl:ObjectProperty>
</rdf:RDF>
