<?xml version="1.0" encoding="UTF-8"?>
<rdf:RDF xmlns:math="http://www.w3.org/2005/xpath-functions/math"
         xmlns:owl="http://www.w3.org/2002/07/owl#"
         xmlns:rdf="http://www.w3.org/1999/02/22-rdf-syntax-ns#"
         xmlns:rdfs="http://www.w3.org/2000/01/rdf-schema#"
         xmlns:xs="http://www.w3.org/2001/XMLSchema"
         xmlns:xsd="http://www.w3.org/2001/XMLSchema">
   <owl:Ontology rdf:about="http://liris.cnrs.fr/ontologies/waterBody">
      <owl:imports rdf:resource="http://liris.cnrs.fr/ontologies/gml"/>
      <owl:imports rdf:resource="http://liris.cnrs.fr/ontologies/cityGMLBase"/>
      <rdfs:comment>
	CityGML is an OGC Standard.
	Copyright (c) 2012 Open Geospatial Consortium.
	To obtain additional rights of use, visit http://www.opengeospatial.org/legal/ .
		</rdfs:comment>
   </owl:Ontology>
   <owl:Class rdf:about="http://www.opengis.net/citygml/waterbody/2.0#AbstractWaterObjectType">
      <rdfs:comment>This is an abstract class</rdfs:comment>
      <rdfs:comment>Type describing the abstract superclass for water objects. As subclass of _CityObject, a _WaterObject
				inherits all attributes and relations, in particular an id, names, external references, and generalization relations.
			</rdfs:comment>
      <rdfs:subClassOf>
         <owl:Class>
            <owl:intersectionOf rdf:parseType="Collection">
               <owl:Restriction>
                  <owl:onProperty rdf:resource="http://www.opengis.net/citygml/waterbody/2.0#has_GenericApplicationPropertyOfWaterObject"/>
                  <owl:allValuesFrom rdf:resource="http://www.opengis.net/citygml/waterbody/2.0#_GenericApplicationPropertyOfWaterObject"/>
               </owl:Restriction>
               <owl:Restriction>
                  <owl:onProperty rdf:resource="http://www.opengis.net/citygml/waterbody/2.0#has_GenericApplicationPropertyOfWaterObject"/>
                  <owl:minCardinality rdf:datatype="http://www.w3.org/2001/XMLSchema#nonNegativeInteger">0</owl:minCardinality>
               </owl:Restriction>
            </owl:intersectionOf>
         </owl:Class>
      </rdfs:subClassOf>
      <rdfs:subClassOf rdf:resource="http://www.opengis.net/citygml/2.0#AbstractCityObjectType"/>
      <rdfs:comment>Warning: The parent class 'core:AbstractCityObjectType' is declared outside of this class' original schema. This class may be declared incorrectly.</rdfs:comment>
   </owl:Class>
   <owl:Class rdf:about="http://www.opengis.net/citygml/waterbody/2.0#WaterBodyType">
      <rdfs:comment>Type describing Water Bodies, e.g., lakes, rivers. As subclass of _CityObject, a WaterBody inherits all
				attributes and relations, in particular an id, names, external references, and generalization relations.
			</rdfs:comment>
      <rdfs:subClassOf>
         <owl:Class>
            <owl:intersectionOf rdf:parseType="Collection">
               <owl:Restriction>
                  <owl:onProperty rdf:resource="http://www.opengis.net/citygml/waterbody/2.0#class"/>
                  <owl:allValuesFrom rdf:resource="http://www.opengis.net/gml#CodeType"/>
               </owl:Restriction>
               <owl:Restriction>
                  <owl:onProperty rdf:resource="http://www.opengis.net/citygml/waterbody/2.0#class"/>
                  <owl:minCardinality rdf:datatype="http://www.w3.org/2001/XMLSchema#nonNegativeInteger">0</owl:minCardinality>
               </owl:Restriction>
               <owl:Restriction>
                  <owl:onProperty rdf:resource="http://www.opengis.net/citygml/waterbody/2.0#function"/>
                  <owl:allValuesFrom rdf:resource="http://www.opengis.net/gml#CodeType"/>
               </owl:Restriction>
               <owl:Restriction>
                  <owl:onProperty rdf:resource="http://www.opengis.net/citygml/waterbody/2.0#function"/>
                  <owl:minCardinality rdf:datatype="http://www.w3.org/2001/XMLSchema#nonNegativeInteger">0</owl:minCardinality>
               </owl:Restriction>
               <owl:Restriction>
                  <owl:onProperty rdf:resource="http://www.opengis.net/citygml/waterbody/2.0#usage"/>
                  <owl:allValuesFrom rdf:resource="http://www.opengis.net/gml#CodeType"/>
               </owl:Restriction>
               <owl:Restriction>
                  <owl:onProperty rdf:resource="http://www.opengis.net/citygml/waterbody/2.0#usage"/>
                  <owl:minCardinality rdf:datatype="http://www.w3.org/2001/XMLSchema#nonNegativeInteger">0</owl:minCardinality>
               </owl:Restriction>
               <owl:Restriction>
                  <owl:onProperty rdf:resource="http://www.opengis.net/citygml/waterbody/2.0#lod0MultiCurve"/>
                  <owl:allValuesFrom rdf:resource="http://www.opengis.net/gml#MultiCurvePropertyType"/>
               </owl:Restriction>
               <owl:Restriction>
                  <owl:onProperty rdf:resource="http://www.opengis.net/citygml/waterbody/2.0#lod0MultiCurve"/>
                  <owl:minCardinality rdf:datatype="http://www.w3.org/2001/XMLSchema#nonNegativeInteger">0</owl:minCardinality>
               </owl:Restriction>
               <owl:Restriction>
                  <owl:onProperty rdf:resource="http://www.opengis.net/citygml/waterbody/2.0#lod0MultiSurface"/>
                  <owl:allValuesFrom rdf:resource="http://www.opengis.net/gml#MultiSurfacePropertyType"/>
               </owl:Restriction>
               <owl:Restriction>
                  <owl:onProperty rdf:resource="http://www.opengis.net/citygml/waterbody/2.0#lod0MultiSurface"/>
                  <owl:minCardinality rdf:datatype="http://www.w3.org/2001/XMLSchema#nonNegativeInteger">0</owl:minCardinality>
               </owl:Restriction>
               <owl:Restriction>
                  <owl:onProperty rdf:resource="http://www.opengis.net/citygml/waterbody/2.0#lod1MultiCurve"/>
                  <owl:allValuesFrom rdf:resource="http://www.opengis.net/gml#MultiCurvePropertyType"/>
               </owl:Restriction>
               <owl:Restriction>
                  <owl:onProperty rdf:resource="http://www.opengis.net/citygml/waterbody/2.0#lod1MultiCurve"/>
                  <owl:minCardinality rdf:datatype="http://www.w3.org/2001/XMLSchema#nonNegativeInteger">0</owl:minCardinality>
               </owl:Restriction>
               <owl:Restriction>
                  <owl:onProperty rdf:resource="http://www.opengis.net/citygml/waterbody/2.0#lod1MultiSurface"/>
                  <owl:allValuesFrom rdf:resource="http://www.opengis.net/gml#MultiSurfacePropertyType"/>
               </owl:Restriction>
               <owl:Restriction>
                  <owl:onProperty rdf:resource="http://www.opengis.net/citygml/waterbody/2.0#lod1MultiSurface"/>
                  <owl:minCardinality rdf:datatype="http://www.w3.org/2001/XMLSchema#nonNegativeInteger">0</owl:minCardinality>
               </owl:Restriction>
               <owl:Restriction>
                  <owl:onProperty rdf:resource="http://www.opengis.net/citygml/waterbody/2.0#lod1Solid"/>
                  <owl:allValuesFrom rdf:resource="http://www.opengis.net/gml#SolidPropertyType"/>
               </owl:Restriction>
               <owl:Restriction>
                  <owl:onProperty rdf:resource="http://www.opengis.net/citygml/waterbody/2.0#lod1Solid"/>
                  <owl:minCardinality rdf:datatype="http://www.w3.org/2001/XMLSchema#nonNegativeInteger">0</owl:minCardinality>
               </owl:Restriction>
               <owl:Restriction>
                  <owl:onProperty rdf:resource="http://www.opengis.net/citygml/waterbody/2.0#lod2Solid"/>
                  <owl:allValuesFrom rdf:resource="http://www.opengis.net/gml#SolidPropertyType"/>
               </owl:Restriction>
               <owl:Restriction>
                  <owl:onProperty rdf:resource="http://www.opengis.net/citygml/waterbody/2.0#lod2Solid"/>
                  <owl:minCardinality rdf:datatype="http://www.w3.org/2001/XMLSchema#nonNegativeInteger">0</owl:minCardinality>
               </owl:Restriction>
               <owl:Restriction>
                  <owl:onProperty rdf:resource="http://www.opengis.net/citygml/waterbody/2.0#lod3Solid"/>
                  <owl:allValuesFrom rdf:resource="http://www.opengis.net/gml#SolidPropertyType"/>
               </owl:Restriction>
               <owl:Restriction>
                  <owl:onProperty rdf:resource="http://www.opengis.net/citygml/waterbody/2.0#lod3Solid"/>
                  <owl:minCardinality rdf:datatype="http://www.w3.org/2001/XMLSchema#nonNegativeInteger">0</owl:minCardinality>
               </owl:Restriction>
               <owl:Restriction>
                  <owl:onProperty rdf:resource="http://www.opengis.net/citygml/waterbody/2.0#lod4Solid"/>
                  <owl:allValuesFrom rdf:resource="http://www.opengis.net/gml#SolidPropertyType"/>
               </owl:Restriction>
               <owl:Restriction>
                  <owl:onProperty rdf:resource="http://www.opengis.net/citygml/waterbody/2.0#lod4Solid"/>
                  <owl:minCardinality rdf:datatype="http://www.w3.org/2001/XMLSchema#nonNegativeInteger">0</owl:minCardinality>
               </owl:Restriction>
               <owl:Restriction>
                  <owl:onProperty rdf:resource="http://www.opengis.net/citygml/waterbody/2.0#boundedBy"/>
                  <owl:allValuesFrom rdf:resource="http://www.opengis.net/citygml/waterbody/2.0#BoundedByWaterSurfacePropertyType"/>
               </owl:Restriction>
               <owl:Restriction>
                  <owl:onProperty rdf:resource="http://www.opengis.net/citygml/waterbody/2.0#boundedBy"/>
                  <owl:minCardinality rdf:datatype="http://www.w3.org/2001/XMLSchema#nonNegativeInteger">0</owl:minCardinality>
               </owl:Restriction>
               <owl:Restriction>
                  <owl:onProperty rdf:resource="http://www.opengis.net/citygml/waterbody/2.0#has_GenericApplicationPropertyOfWaterBody"/>
                  <owl:allValuesFrom rdf:resource="http://www.opengis.net/citygml/waterbody/2.0#_GenericApplicationPropertyOfWaterBody"/>
               </owl:Restriction>
               <owl:Restriction>
                  <owl:onProperty rdf:resource="http://www.opengis.net/citygml/waterbody/2.0#has_GenericApplicationPropertyOfWaterBody"/>
                  <owl:minCardinality rdf:datatype="http://www.w3.org/2001/XMLSchema#nonNegativeInteger">0</owl:minCardinality>
               </owl:Restriction>
            </owl:intersectionOf>
         </owl:Class>
      </rdfs:subClassOf>
      <rdfs:subClassOf rdf:resource="http://www.opengis.net/citygml/waterbody/2.0#AbstractWaterObjectType"/>
   </owl:Class>
   <owl:Class rdf:about="http://www.opengis.net/citygml/waterbody/2.0#BoundedByWaterSurfacePropertyType">
      <rdfs:comment>Denotes the relation of a WaterBody to its boundary surfaces, which are of type _WaterBoundarySurface. The
				BoundedByWaterSurfacePropertyType element must either carry a reference to a _WaterBoundarySurface object or contain a
				_WaterBoundarySurface object inline, but neither both nor none. </rdfs:comment>
      <rdfs:subClassOf>
         <owl:Class>
            <owl:intersectionOf rdf:parseType="Collection">
               <owl:Restriction>
                  <owl:onProperty rdf:resource="http://www.opengis.net/citygml/waterbody/2.0#has_WaterBoundarySurface"/>
                  <owl:allValuesFrom rdf:resource="http://www.opengis.net/citygml/waterbody/2.0#_WaterBoundarySurface"/>
               </owl:Restriction>
            </owl:intersectionOf>
         </owl:Class>
      </rdfs:subClassOf>
   </owl:Class>
   <owl:Class rdf:about="http://www.opengis.net/citygml/waterbody/2.0#AbstractWaterBoundarySurfaceType">
      <rdfs:comment>This is an abstract class</rdfs:comment>
      <rdfs:comment>A WaterBoundarySurface is a thematic object which classifies surfaces bounding a water body.
			</rdfs:comment>
      <rdfs:subClassOf>
         <owl:Class>
            <owl:intersectionOf rdf:parseType="Collection">
               <owl:Restriction>
                  <owl:onProperty rdf:resource="http://www.opengis.net/citygml/waterbody/2.0#lod2Surface"/>
                  <owl:allValuesFrom rdf:resource="http://www.opengis.net/gml#SurfacePropertyType"/>
               </owl:Restriction>
               <owl:Restriction>
                  <owl:onProperty rdf:resource="http://www.opengis.net/citygml/waterbody/2.0#lod2Surface"/>
                  <owl:minCardinality rdf:datatype="http://www.w3.org/2001/XMLSchema#nonNegativeInteger">0</owl:minCardinality>
               </owl:Restriction>
               <owl:Restriction>
                  <owl:onProperty rdf:resource="http://www.opengis.net/citygml/waterbody/2.0#lod3Surface"/>
                  <owl:allValuesFrom rdf:resource="http://www.opengis.net/gml#SurfacePropertyType"/>
               </owl:Restriction>
               <owl:Restriction>
                  <owl:onProperty rdf:resource="http://www.opengis.net/citygml/waterbody/2.0#lod3Surface"/>
                  <owl:minCardinality rdf:datatype="http://www.w3.org/2001/XMLSchema#nonNegativeInteger">0</owl:minCardinality>
               </owl:Restriction>
               <owl:Restriction>
                  <owl:onProperty rdf:resource="http://www.opengis.net/citygml/waterbody/2.0#lod4Surface"/>
                  <owl:allValuesFrom rdf:resource="http://www.opengis.net/gml#SurfacePropertyType"/>
               </owl:Restriction>
               <owl:Restriction>
                  <owl:onProperty rdf:resource="http://www.opengis.net/citygml/waterbody/2.0#lod4Surface"/>
                  <owl:minCardinality rdf:datatype="http://www.w3.org/2001/XMLSchema#nonNegativeInteger">0</owl:minCardinality>
               </owl:Restriction>
               <owl:Restriction>
                  <owl:onProperty rdf:resource="http://www.opengis.net/citygml/waterbody/2.0#has_GenericApplicationPropertyOfWaterBoundarySurface"/>
                  <owl:allValuesFrom rdf:resource="http://www.opengis.net/citygml/waterbody/2.0#_GenericApplicationPropertyOfWaterBoundarySurface"/>
               </owl:Restriction>
               <owl:Restriction>
                  <owl:onProperty rdf:resource="http://www.opengis.net/citygml/waterbody/2.0#has_GenericApplicationPropertyOfWaterBoundarySurface"/>
                  <owl:minCardinality rdf:datatype="http://www.w3.org/2001/XMLSchema#nonNegativeInteger">0</owl:minCardinality>
               </owl:Restriction>
            </owl:intersectionOf>
         </owl:Class>
      </rdfs:subClassOf>
      <rdfs:subClassOf rdf:resource="http://www.opengis.net/citygml/2.0#AbstractCityObjectType"/>
      <rdfs:comment>Warning: The parent class 'core:AbstractCityObjectType' is declared outside of this class' original schema. This class may be declared incorrectly.</rdfs:comment>
   </owl:Class>
   <owl:Class rdf:about="http://www.opengis.net/citygml/waterbody/2.0#WaterSurfaceType">
      <rdfs:comment>Type describing the surface of a water body, which separates the water from the air. As subclass of
				_CityObject, a WaterSurface inherits all attributes and relations, in particular an id, names, external references, and
				generalization relations. </rdfs:comment>
      <rdfs:subClassOf>
         <owl:Class>
            <owl:intersectionOf rdf:parseType="Collection">
               <owl:Restriction>
                  <owl:onProperty rdf:resource="http://www.opengis.net/citygml/waterbody/2.0#waterLevel"/>
                  <owl:allValuesFrom rdf:resource="http://www.opengis.net/gml#CodeType"/>
               </owl:Restriction>
               <owl:Restriction>
                  <owl:onProperty rdf:resource="http://www.opengis.net/citygml/waterbody/2.0#waterLevel"/>
                  <owl:minCardinality rdf:datatype="http://www.w3.org/2001/XMLSchema#nonNegativeInteger">0</owl:minCardinality>
               </owl:Restriction>
               <owl:Restriction>
                  <owl:onProperty rdf:resource="http://www.opengis.net/citygml/waterbody/2.0#has_GenericApplicationPropertyOfWaterSurface"/>
                  <owl:allValuesFrom rdf:resource="http://www.opengis.net/citygml/waterbody/2.0#_GenericApplicationPropertyOfWaterSurface"/>
               </owl:Restriction>
               <owl:Restriction>
                  <owl:onProperty rdf:resource="http://www.opengis.net/citygml/waterbody/2.0#has_GenericApplicationPropertyOfWaterSurface"/>
                  <owl:minCardinality rdf:datatype="http://www.w3.org/2001/XMLSchema#nonNegativeInteger">0</owl:minCardinality>
               </owl:Restriction>
            </owl:intersectionOf>
         </owl:Class>
      </rdfs:subClassOf>
      <rdfs:subClassOf rdf:resource="http://www.opengis.net/citygml/waterbody/2.0#AbstractWaterBoundarySurfaceType"/>
   </owl:Class>
   <owl:Class rdf:about="http://www.opengis.net/citygml/waterbody/2.0#WaterGroundSurfaceType">
      <rdfs:comment>Type describing the ground surface of a water body, i.e. the boundary to the digital terrain model. As
				subclass of _CityObject, a WaterGroundSurface inherits all attributes and relations, in particular an id, names, external
				references, and generalization relations. </rdfs:comment>
      <rdfs:subClassOf>
         <owl:Class>
            <owl:intersectionOf rdf:parseType="Collection">
               <owl:Restriction>
                  <owl:onProperty rdf:resource="http://www.opengis.net/citygml/waterbody/2.0#has_GenericApplicationPropertyOfWaterGroundSurface"/>
                  <owl:allValuesFrom rdf:resource="http://www.opengis.net/citygml/waterbody/2.0#_GenericApplicationPropertyOfWaterGroundSurface"/>
               </owl:Restriction>
               <owl:Restriction>
                  <owl:onProperty rdf:resource="http://www.opengis.net/citygml/waterbody/2.0#has_GenericApplicationPropertyOfWaterGroundSurface"/>
                  <owl:minCardinality rdf:datatype="http://www.w3.org/2001/XMLSchema#nonNegativeInteger">0</owl:minCardinality>
               </owl:Restriction>
            </owl:intersectionOf>
         </owl:Class>
      </rdfs:subClassOf>
      <rdfs:subClassOf rdf:resource="http://www.opengis.net/citygml/waterbody/2.0#AbstractWaterBoundarySurfaceType"/>
   </owl:Class>
   <owl:Class rdf:about="http://www.opengis.net/citygml/waterbody/2.0#WaterClosureSurfaceType">
      <rdfs:comment>Type describing the closure surface between water bodys. As subclass of _CityObject, a WaterClosureSurface
				inherits all attributes and relations, in particular an id, names, external references, and generalization relations.
			</rdfs:comment>
      <rdfs:subClassOf>
         <owl:Class>
            <owl:intersectionOf rdf:parseType="Collection">
               <owl:Restriction>
                  <owl:onProperty rdf:resource="http://www.opengis.net/citygml/waterbody/2.0#has_GenericApplicationPropertyOfWaterClosureSurface"/>
                  <owl:allValuesFrom rdf:resource="http://www.opengis.net/citygml/waterbody/2.0#_GenericApplicationPropertyOfWaterClosureSurface"/>
               </owl:Restriction>
               <owl:Restriction>
                  <owl:onProperty rdf:resource="http://www.opengis.net/citygml/waterbody/2.0#has_GenericApplicationPropertyOfWaterClosureSurface"/>
                  <owl:minCardinality rdf:datatype="http://www.w3.org/2001/XMLSchema#nonNegativeInteger">0</owl:minCardinality>
               </owl:Restriction>
            </owl:intersectionOf>
         </owl:Class>
      </rdfs:subClassOf>
      <rdfs:subClassOf rdf:resource="http://www.opengis.net/citygml/waterbody/2.0#AbstractWaterBoundarySurfaceType"/>
   </owl:Class>
   <owl:ObjectProperty rdf:about="http://www.opengis.net/gml#hasAssociationAttributeGroup">
      <rdfs:domain rdf:resource="http://www.opengis.net/citygml/waterbody/2.0#BoundedByWaterSurfacePropertyType"/>
      <rdfs:range rdf:resource="http://www.opengis.net/gml#AssociationAttributeGroup"/>
   </owl:ObjectProperty>
   <owl:Class rdf:about="http://www.opengis.net/citygml/waterbody/2.0#_WaterObject">
      <rdfs:subClassOf rdf:resource="http://www.opengis.net/citygml/2.0#_CityObject"/>
      <rdfs:subClassOf rdf:resource="http://www.opengis.net/citygml/waterbody/2.0#AbstractWaterObjectType"/>
   </owl:Class>
   <owl:Class rdf:about="http://www.opengis.net/citygml/waterbody/2.0#_GenericApplicationPropertyOfWaterObject">
      <rdfs:subClassOf rdf:resource="http://www.w3.org/2001/XMLSchema#anyType"/>
      <rdfs:comment>Warning: This class type was declared outside of its original schema. This class may be declared incorrectly.</rdfs:comment>
   </owl:Class>
   <owl:Class rdf:about="http://www.opengis.net/citygml/waterbody/2.0#WaterBody">
      <rdfs:subClassOf rdf:resource="http://www.opengis.net/citygml/waterbody/2.0#_WaterObject"/>
      <rdfs:subClassOf rdf:resource="http://www.opengis.net/citygml/waterbody/2.0#WaterBodyType"/>
   </owl:Class>
   <owl:Class rdf:about="http://www.opengis.net/citygml/waterbody/2.0#_GenericApplicationPropertyOfWaterBody">
      <rdfs:subClassOf rdf:resource="http://www.w3.org/2001/XMLSchema#anyType"/>
      <rdfs:comment>Warning: This class type was declared outside of its original schema. This class may be declared incorrectly.</rdfs:comment>
   </owl:Class>
   <owl:Class rdf:about="http://www.opengis.net/citygml/waterbody/2.0#_WaterBoundarySurface">
      <rdfs:subClassOf rdf:resource="http://www.opengis.net/citygml/2.0#_CityObject"/>
      <rdfs:subClassOf rdf:resource="http://www.opengis.net/citygml/waterbody/2.0#AbstractWaterBoundarySurfaceType"/>
   </owl:Class>
   <owl:Class rdf:about="http://www.opengis.net/citygml/waterbody/2.0#_GenericApplicationPropertyOfWaterBoundarySurface">
      <rdfs:subClassOf rdf:resource="http://www.w3.org/2001/XMLSchema#anyType"/>
      <rdfs:comment>Warning: This class type was declared outside of its original schema. This class may be declared incorrectly.</rdfs:comment>
   </owl:Class>
   <owl:Class rdf:about="http://www.opengis.net/citygml/waterbody/2.0#WaterSurface">
      <rdfs:subClassOf rdf:resource="http://www.opengis.net/citygml/waterbody/2.0#_WaterBoundarySurface"/>
      <rdfs:subClassOf rdf:resource="http://www.opengis.net/citygml/waterbody/2.0#WaterSurfaceType"/>
   </owl:Class>
   <owl:Class rdf:about="http://www.opengis.net/citygml/waterbody/2.0#_GenericApplicationPropertyOfWaterSurface">
      <rdfs:subClassOf rdf:resource="http://www.w3.org/2001/XMLSchema#anyType"/>
      <rdfs:comment>Warning: This class type was declared outside of its original schema. This class may be declared incorrectly.</rdfs:comment>
   </owl:Class>
   <owl:Class rdf:about="http://www.opengis.net/citygml/waterbody/2.0#WaterGroundSurface">
      <rdfs:subClassOf rdf:resource="http://www.opengis.net/citygml/waterbody/2.0#_WaterBoundarySurface"/>
      <rdfs:subClassOf rdf:resource="http://www.opengis.net/citygml/waterbody/2.0#WaterGroundSurfaceType"/>
   </owl:Class>
   <owl:Class rdf:about="http://www.opengis.net/citygml/waterbody/2.0#_GenericApplicationPropertyOfWaterGroundSurface">
      <rdfs:subClassOf rdf:resource="http://www.w3.org/2001/XMLSchema#anyType"/>
      <rdfs:comment>Warning: This class type was declared outside of its original schema. This class may be declared incorrectly.</rdfs:comment>
   </owl:Class>
   <owl:Class rdf:about="http://www.opengis.net/citygml/waterbody/2.0#WaterClosureSurface">
      <rdfs:subClassOf rdf:resource="http://www.opengis.net/citygml/waterbody/2.0#_WaterBoundarySurface"/>
      <rdfs:subClassOf rdf:resource="http://www.opengis.net/citygml/waterbody/2.0#WaterClosureSurfaceType"/>
   </owl:Class>
   <owl:Class rdf:about="http://www.opengis.net/citygml/waterbody/2.0#_GenericApplicationPropertyOfWaterClosureSurface">
      <rdfs:subClassOf rdf:resource="http://www.w3.org/2001/XMLSchema#anyType"/>
      <rdfs:comment>Warning: This class type was declared outside of its original schema. This class may be declared incorrectly.</rdfs:comment>
   </owl:Class>
   <owl:ObjectProperty rdf:about="http://www.opengis.net/citygml/waterbody/2.0#has_GenericApplicationPropertyOfWaterObject">
      <rdfs:domain rdf:resource="http://www.opengis.net/citygml/waterbody/2.0#AbstractWaterObjectType"/>
      <rdfs:range rdf:resource="http://www.opengis.net/citygml/waterbody/2.0#_GenericApplicationPropertyOfWaterObject"/>
   </owl:ObjectProperty>
   <owl:ObjectProperty rdf:about="http://www.opengis.net/citygml/waterbody/2.0#class">
      <rdfs:comment>Warning: This ObjectProperty type was declared outside of its original schema. This ObjectProperty may be declared incorrectly.</rdfs:comment>
      <rdfs:domain rdf:resource="http://www.opengis.net/citygml/waterbody/2.0#WaterBodyType"/>
      <rdfs:range rdf:resource="http://www.opengis.net/gml#CodeType"/>
   </owl:ObjectProperty>
   <owl:ObjectProperty rdf:about="http://www.opengis.net/citygml/waterbody/2.0#function">
      <rdfs:comment>Warning: This ObjectProperty type was declared outside of its original schema. This ObjectProperty may be declared incorrectly.</rdfs:comment>
      <rdfs:domain rdf:resource="http://www.opengis.net/citygml/waterbody/2.0#WaterBodyType"/>
      <rdfs:range rdf:resource="http://www.opengis.net/gml#CodeType"/>
   </owl:ObjectProperty>
   <owl:ObjectProperty rdf:about="http://www.opengis.net/citygml/waterbody/2.0#usage">
      <rdfs:comment>Warning: This ObjectProperty type was declared outside of its original schema. This ObjectProperty may be declared incorrectly.</rdfs:comment>
      <rdfs:domain rdf:resource="http://www.opengis.net/citygml/waterbody/2.0#WaterBodyType"/>
      <rdfs:range rdf:resource="http://www.opengis.net/gml#CodeType"/>
   </owl:ObjectProperty>
   <owl:ObjectProperty rdf:about="http://www.opengis.net/citygml/waterbody/2.0#lod0MultiCurve">
      <rdfs:comment>Warning: This ObjectProperty type was declared outside of its original schema. This ObjectProperty may be declared incorrectly.</rdfs:comment>
      <rdfs:domain rdf:resource="http://www.opengis.net/citygml/waterbody/2.0#WaterBodyType"/>
      <rdfs:range rdf:resource="http://www.opengis.net/gml#MultiCurvePropertyType"/>
   </owl:ObjectProperty>
   <owl:ObjectProperty rdf:about="http://www.opengis.net/citygml/waterbody/2.0#lod0MultiSurface">
      <rdfs:comment>Warning: This ObjectProperty type was declared outside of its original schema. This ObjectProperty may be declared incorrectly.</rdfs:comment>
      <rdfs:domain rdf:resource="http://www.opengis.net/citygml/waterbody/2.0#WaterBodyType"/>
      <rdfs:range rdf:resource="http://www.opengis.net/gml#MultiSurfacePropertyType"/>
   </owl:ObjectProperty>
   <owl:ObjectProperty rdf:about="http://www.opengis.net/citygml/waterbody/2.0#lod1MultiCurve">
      <rdfs:comment>Warning: This ObjectProperty type was declared outside of its original schema. This ObjectProperty may be declared incorrectly.</rdfs:comment>
      <rdfs:domain rdf:resource="http://www.opengis.net/citygml/waterbody/2.0#WaterBodyType"/>
      <rdfs:range rdf:resource="http://www.opengis.net/gml#MultiCurvePropertyType"/>
   </owl:ObjectProperty>
   <owl:ObjectProperty rdf:about="http://www.opengis.net/citygml/waterbody/2.0#lod1MultiSurface">
      <rdfs:comment>Warning: This ObjectProperty type was declared outside of its original schema. This ObjectProperty may be declared incorrectly.</rdfs:comment>
      <rdfs:domain rdf:resource="http://www.opengis.net/citygml/waterbody/2.0#WaterBodyType"/>
      <rdfs:range rdf:resource="http://www.opengis.net/gml#MultiSurfacePropertyType"/>
   </owl:ObjectProperty>
   <owl:ObjectProperty rdf:about="http://www.opengis.net/citygml/waterbody/2.0#lod1Solid">
      <rdfs:comment>Warning: This ObjectProperty type was declared outside of its original schema. This ObjectProperty may be declared incorrectly.</rdfs:comment>
      <rdfs:domain rdf:resource="http://www.opengis.net/citygml/waterbody/2.0#WaterBodyType"/>
      <rdfs:range rdf:resource="http://www.opengis.net/gml#SolidPropertyType"/>
   </owl:ObjectProperty>
   <owl:ObjectProperty rdf:about="http://www.opengis.net/citygml/waterbody/2.0#lod2Solid">
      <rdfs:comment>Warning: This ObjectProperty type was declared outside of its original schema. This ObjectProperty may be declared incorrectly.</rdfs:comment>
      <rdfs:domain rdf:resource="http://www.opengis.net/citygml/waterbody/2.0#WaterBodyType"/>
      <rdfs:range rdf:resource="http://www.opengis.net/gml#SolidPropertyType"/>
   </owl:ObjectProperty>
   <owl:ObjectProperty rdf:about="http://www.opengis.net/citygml/waterbody/2.0#lod3Solid">
      <rdfs:comment>Warning: This ObjectProperty type was declared outside of its original schema. This ObjectProperty may be declared incorrectly.</rdfs:comment>
      <rdfs:domain rdf:resource="http://www.opengis.net/citygml/waterbody/2.0#WaterBodyType"/>
      <rdfs:range rdf:resource="http://www.opengis.net/gml#SolidPropertyType"/>
   </owl:ObjectProperty>
   <owl:ObjectProperty rdf:about="http://www.opengis.net/citygml/waterbody/2.0#lod4Solid">
      <rdfs:comment>Warning: This ObjectProperty type was declared outside of its original schema. This ObjectProperty may be declared incorrectly.</rdfs:comment>
      <rdfs:domain rdf:resource="http://www.opengis.net/citygml/waterbody/2.0#WaterBodyType"/>
      <rdfs:range rdf:resource="http://www.opengis.net/gml#SolidPropertyType"/>
   </owl:ObjectProperty>
   <owl:ObjectProperty rdf:about="http://www.opengis.net/citygml/waterbody/2.0#boundedBy">
      <rdfs:domain rdf:resource="http://www.opengis.net/citygml/waterbody/2.0#WaterBodyType"/>
      <rdfs:range rdf:resource="http://www.opengis.net/citygml/waterbody/2.0#BoundedByWaterSurfacePropertyType"/>
   </owl:ObjectProperty>
   <owl:ObjectProperty rdf:about="http://www.opengis.net/citygml/waterbody/2.0#has_GenericApplicationPropertyOfWaterBody">
      <rdfs:domain rdf:resource="http://www.opengis.net/citygml/waterbody/2.0#WaterBodyType"/>
      <rdfs:range rdf:resource="http://www.opengis.net/citygml/waterbody/2.0#_GenericApplicationPropertyOfWaterBody"/>
   </owl:ObjectProperty>
   <owl:ObjectProperty rdf:about="http://www.opengis.net/citygml/waterbody/2.0#has_WaterBoundarySurface">
      <rdfs:domain rdf:resource="http://www.opengis.net/citygml/waterbody/2.0#BoundedByWaterSurfacePropertyType"/>
      <rdfs:range rdf:resource="http://www.opengis.net/citygml/waterbody/2.0#_WaterBoundarySurface"/>
   </owl:ObjectProperty>
   <owl:ObjectProperty rdf:about="http://www.opengis.net/citygml/waterbody/2.0#lod2Surface">
      <rdfs:comment>Warning: This ObjectProperty type was declared outside of its original schema. This ObjectProperty may be declared incorrectly.</rdfs:comment>
      <rdfs:domain rdf:resource="http://www.opengis.net/citygml/waterbody/2.0#AbstractWaterBoundarySurfaceType"/>
      <rdfs:range rdf:resource="http://www.opengis.net/gml#SurfacePropertyType"/>
   </owl:ObjectProperty>
   <owl:ObjectProperty rdf:about="http://www.opengis.net/citygml/waterbody/2.0#lod3Surface">
      <rdfs:comment>Warning: This ObjectProperty type was declared outside of its original schema. This ObjectProperty may be declared incorrectly.</rdfs:comment>
      <rdfs:domain rdf:resource="http://www.opengis.net/citygml/waterbody/2.0#AbstractWaterBoundarySurfaceType"/>
      <rdfs:range rdf:resource="http://www.opengis.net/gml#SurfacePropertyType"/>
   </owl:ObjectProperty>
   <owl:ObjectProperty rdf:about="http://www.opengis.net/citygml/waterbody/2.0#lod4Surface">
      <rdfs:comment>Warning: This ObjectProperty type was declared outside of its original schema. This ObjectProperty may be declared incorrectly.</rdfs:comment>
      <rdfs:domain rdf:resource="http://www.opengis.net/citygml/waterbody/2.0#AbstractWaterBoundarySurfaceType"/>
      <rdfs:range rdf:resource="http://www.opengis.net/gml#SurfacePropertyType"/>
   </owl:ObjectProperty>
   <owl:ObjectProperty rdf:about="http://www.opengis.net/citygml/waterbody/2.0#has_GenericApplicationPropertyOfWaterBoundarySurface">
      <rdfs:domain rdf:resource="http://www.opengis.net/citygml/waterbody/2.0#AbstractWaterBoundarySurfaceType"/>
      <rdfs:range rdf:resource="http://www.opengis.net/citygml/waterbody/2.0#_GenericApplicationPropertyOfWaterBoundarySurface"/>
   </owl:ObjectProperty>
   <owl:ObjectProperty rdf:about="http://www.opengis.net/citygml/waterbody/2.0#waterLevel">
      <rdfs:comment>Warning: This ObjectProperty type was declared outside of its original schema. This ObjectProperty may be declared incorrectly.</rdfs:comment>
      <rdfs:domain rdf:resource="http://www.opengis.net/citygml/waterbody/2.0#WaterSurfaceType"/>
      <rdfs:range rdf:resource="http://www.opengis.net/gml#CodeType"/>
   </owl:ObjectProperty>
   <owl:ObjectProperty rdf:about="http://www.opengis.net/citygml/waterbody/2.0#has_GenericApplicationPropertyOfWaterSurface">
      <rdfs:domain rdf:resource="http://www.opengis.net/citygml/waterbody/2.0#WaterSurfaceType"/>
      <rdfs:range rdf:resource="http://www.opengis.net/citygml/waterbody/2.0#_GenericApplicationPropertyOfWaterSurface"/>
   </owl:ObjectProperty>
   <owl:ObjectProperty rdf:about="http://www.opengis.net/citygml/waterbody/2.0#has_GenericApplicationPropertyOfWaterGroundSurface">
      <rdfs:domain rdf:resource="http://www.opengis.net/citygml/waterbody/2.0#WaterGroundSurfaceType"/>
      <rdfs:range rdf:resource="http://www.opengis.net/citygml/waterbody/2.0#_GenericApplicationPropertyOfWaterGroundSurface"/>
   </owl:ObjectProperty>
   <owl:ObjectProperty rdf:about="http://www.opengis.net/citygml/waterbody/2.0#has_GenericApplicationPropertyOfWaterClosureSurface">
      <rdfs:domain rdf:resource="http://www.opengis.net/citygml/waterbody/2.0#WaterClosureSurfaceType"/>
      <rdfs:range rdf:resource="http://www.opengis.net/citygml/waterbody/2.0#_GenericApplicationPropertyOfWaterClosureSurface"/>
   </owl:ObjectProperty>
</rdf:RDF>
