@prefix sc:    <http://shapechange.net/resources/ont/base#> .
@prefix core:  <https://github.com/VCityTeam/UD-Graph/Ontologies/core#> .
@prefix iso19150-2: <http://def.isotc211.org/iso19150/-2/2012/base#> .
@prefix rdf:   <http://www.w3.org/1999/02/22-rdf-syntax-ns#> .
@prefix owl:   <http://www.w3.org/2002/07/owl#> .
@prefix xsd:   <http://www.w3.org/2001/XMLSchema#> .
@prefix skos:  <http://www.w3.org/2004/02/skos/core#> .
@prefix veg:   <https://github.com/VCityTeam/UD-Graph/Ontologies/vegetation#> .
@prefix rdfs:  <http://www.w3.org/2000/01/rdf-schema#> .

veg:PlantCoverFunctionValue
        a                owl:Class ;
        rdfs:subClassOf  skos:Concept ;
        skos:definition  "PlantCoverFunctionValue is a code list that enumerates the different purposes of a PlantCover."@en ;
        skos:prefLabel   "PlantCoverFunctionValue"@en .

veg:SolitaryVegetationObjectClassValue
        a                owl:Class ;
        rdfs:subClassOf  skos:Concept ;
        skos:definition  "SolitaryVegetationObjectClassValue is a code list used to further classify a SolitaryVegetationObject."@en ;
        skos:prefLabel   "SolitaryVegetationObjectClassValue"@en .

veg:SolitaryVegetationObject.usage
        a                owl:ObjectProperty ;
        rdfs:domain      veg:SolitaryVegetationObject ;
        rdfs:range       veg:SolitaryVegetationObjectUsageValue ;
        skos:definition  "Specifies the actual uses of the SolitaryVegetationObject."@en ;
        skos:prefLabel   "usage"@en .

veg:PlantCover.function
        a                owl:ObjectProperty ;
        rdfs:domain      veg:PlantCover ;
        rdfs:range       veg:PlantCoverFunctionValue ;
        skos:definition  "Specifies the intended purposes of the PlantCover."@en ;
        skos:prefLabel   "function"@en .

veg:SolitaryVegetationObject.class
        a                owl:ObjectProperty ;
        rdfs:domain      veg:SolitaryVegetationObject ;
        rdfs:range       veg:SolitaryVegetationObjectClassValue ;
        skos:definition  "Indicates the specific type of the SolitaryVegetationObject."@en ;
        skos:prefLabel   "class"@en .

veg:ADEOfPlantCover  a         owl:Class ;
        iso19150-2:isAbstract  true ;
        skos:definition        "ADEOfPlantCover acts as a hook to define properties within an ADE that are to be added to a PlantCover."@en ;
        skos:prefLabel         "ADEOfPlantCover"@en .

veg:SolitaryVegetationObject.species
        a                owl:ObjectProperty ;
        rdfs:domain      veg:SolitaryVegetationObject ;
        rdfs:range       veg:SpeciesValue ;
        skos:definition  "Indicates the botanical name of the SolitaryVegetationObject."@en ;
        skos:prefLabel   "species"@en .

veg:SolitaryVegetationObject.crownDiameter
        a                owl:DatatypeProperty ;
        rdfs:domain      veg:SolitaryVegetationObject ;
        rdfs:range       sc:Measure ;
        skos:definition  "Specifies the diameter of the SolitaryCityObject's crown."@en ;
        skos:prefLabel   "crownDiameter"@en .

veg:PlantCover.averageHeight
        a                owl:DatatypeProperty ;
        rdfs:domain      veg:PlantCover ;
        rdfs:range       sc:Measure ;
        skos:definition  "Specifies the average height of the PlantCover."@en ;
        skos:prefLabel   "averageHeight"@en .

veg:PlantCover.maxHeight
        a                owl:DatatypeProperty ;
        rdfs:domain      veg:PlantCover ;
        rdfs:range       sc:Measure ;
        skos:definition  "Specifies the maximum height of the PlantCover."@en ;
        skos:prefLabel   "maxHeight"@en .

veg:AbstractVegetationObject
        a                      owl:Class ;
        rdfs:subClassOf        core:AbstractOccupiedSpace ;
        iso19150-2:isAbstract  true ;
        skos:definition        "AbstractVegetationObject is the abstract superclass for all kinds of vegetation objects."@en ;
        skos:prefLabel         "AbstractVegetationObject"@en .

veg:PlantCoverUsageValue
        a                owl:Class ;
        rdfs:subClassOf  skos:Concept ;
        skos:definition  "PlantCoverUsageValue is a code list that enumerates the different uses of a PlantCover."@en ;
        skos:prefLabel   "PlantCoverUsageValue"@en .

veg:ADEOfAbstractVegetationObject
        a                      owl:Class ;
        iso19150-2:isAbstract  true ;
        skos:definition        "ADEOfAbstractVegetationObject acts as a hook to define properties within an ADE that are to be added to AbstractVegetationObject."@en ;
        skos:prefLabel         "ADEOfAbstractVegetationObject"@en .

veg:PlantCover.class  a  owl:ObjectProperty ;
        rdfs:domain      veg:PlantCover ;
        rdfs:range       veg:PlantCoverClassValue ;
        skos:definition  "Indicates the specific type of the PlantCover."@en ;
        skos:prefLabel   "class"@en .

veg:SolitaryVegetationObjectFunctionValue
        a                owl:Class ;
        rdfs:subClassOf  skos:Concept ;
        skos:definition  "SolitaryVegetationObjectFunctionValue is a code list that enumerates the different purposes of a SolitaryVegetationObject."@en ;
        skos:prefLabel   "SolitaryVegetationObjectFunctionValue"@en .

<https://github.com/VCityTeam/UD-Graph/Ontologies/vegetation>
        a                owl:Ontology ;
        owl:imports      <https://github.com/VCityTeam/UD-Graph/Ontologies/core> , <http://shapechange.net/resources/ont/base> , <http://def.isotc211.org/iso19150/-2/2012/base> ;
        owl:versionIRI   "https://github.com/VCityTeam/UD-Graph/Ontologies/vegetation/3.0.0" ;
        owl:versionInfo  "3.0.0" ;
        skos:definition  "The Vegetation module supports representation of vegetation objects with vegetation-specific thematic classes. CityGMLâ€™s vegetation model distinguishes between solitary vegetation objects like trees, and vegetation areas which represent biotopes like forests or other plant communities."@en ;
        skos:prefLabel   "Vegetation"@en .

veg:PlantCover.usage  a  owl:ObjectProperty ;
        rdfs:domain      veg:PlantCover ;
        rdfs:range       veg:PlantCoverUsageValue ;
        skos:definition  "Specifies the actual uses of the PlantCover."@en ;
        skos:prefLabel   "usage"@en .

veg:SolitaryVegetationObject.adeOfSolitaryVegetationObject
        a                owl:ObjectProperty ;
        rdfs:domain      veg:SolitaryVegetationObject ;
        rdfs:range       veg:ADEOfSolitaryVegetationObject ;
        skos:definition  "Augments the SolitaryVegetationObject with properties defined in an ADE."@en ;
        skos:prefLabel   "adeOfSolitaryVegetationObject"@en .

veg:AbstractVegetationObject.adeOfAbstractVegetationObject
        a                owl:ObjectProperty ;
        rdfs:domain      veg:AbstractVegetationObject ;
        rdfs:range       veg:ADEOfAbstractVegetationObject ;
        skos:definition  "Augments AbstractVegetationObject with properties defined in an ADE."@en ;
        skos:prefLabel   "adeOfAbstractVegetationObject"@en .

veg:SolitaryVegetationObject.height
        a                owl:DatatypeProperty ;
        rdfs:domain      veg:SolitaryVegetationObject ;
        rdfs:range       sc:Measure ;
        skos:definition  "Distance between the highest point of the vegetation object and the lowest point of the terrain at the bottom of the object."@en ;
        skos:prefLabel   "height"@en .

veg:SolitaryVegetationObjectUsageValue
        a                owl:Class ;
        rdfs:subClassOf  skos:Concept ;
        skos:definition  "SolitaryVegetationObjectUsageValue is a code list that enumerates the different uses of a SolitaryVegetationObject."@en ;
        skos:prefLabel   "SolitaryVegetationObjectUsageValue"@en .

veg:PlantCover  a        owl:Class ;
        rdfs:subClassOf  veg:AbstractVegetationObject ;
        skos:definition  "A PlantCover represents a space covered by vegetation."@en ;
        skos:prefLabel   "PlantCover"@en .

veg:PlantCoverClassValue
        a                owl:Class ;
        rdfs:subClassOf  skos:Concept ;
        skos:definition  "PlantCoverClassValue is a code list used to further classify a PlantCover."@en ;
        skos:prefLabel   "PlantCoverClassValue"@en .

veg:PlantCover.adeOfPlantCover
        a                owl:ObjectProperty ;
        rdfs:domain      veg:PlantCover ;
        rdfs:range       veg:ADEOfPlantCover ;
        skos:definition  "Augments the PlantCover with properties defined in an ADE."@en ;
        skos:prefLabel   "adeOfPlantCover"@en .

veg:SpeciesValue  a      owl:Class ;
        rdfs:subClassOf  skos:Concept ;
        skos:definition  "A SpeciesValue is a code list that enumerates the species of a SolitaryVegetationObject."@en ;
        skos:prefLabel   "SpeciesValue"@en .

veg:SolitaryVegetationObject
        a                owl:Class ;
        rdfs:subClassOf  veg:AbstractVegetationObject ;
        skos:definition  "A SolitaryVegetationObject represents individual vegetation objects, e.g. trees or bushes."@en ;
        skos:prefLabel   "SolitaryVegetationObject"@en .

veg:SolitaryVegetationObject.rootBallDiameter
        a                owl:DatatypeProperty ;
        rdfs:domain      veg:SolitaryVegetationObject ;
        rdfs:range       sc:Measure ;
        skos:definition  "Specifies the diameter of the SolitaryCityObject's root ball."@en ;
        skos:prefLabel   "rootBallDiameter"@en .

veg:ADEOfSolitaryVegetationObject
        a                      owl:Class ;
        iso19150-2:isAbstract  true ;
        skos:definition        "ADEOfSolitaryVegetationObject acts as a hook to define properties within an ADE that are to be added to a SolitaryVegetationObject."@en ;
        skos:prefLabel         "ADEOfSolitaryVegetationObject"@en .

veg:SolitaryVegetationObject.maxRootBallDepth
        a                owl:DatatypeProperty ;
        rdfs:domain      veg:SolitaryVegetationObject ;
        rdfs:range       sc:Measure ;
        skos:definition  "Specifies the vertical distance between the lowest point of the SolitaryVegetationObject's root ball and the terrain surface."@en ;
        skos:prefLabel   "maxRootBallDepth"@en .

veg:PlantCover.minHeight
        a                owl:DatatypeProperty ;
        rdfs:domain      veg:PlantCover ;
        rdfs:range       sc:Measure ;
        skos:definition  "Specifies the minimum height of the PlantCover."@en ;
        skos:prefLabel   "minHeight"@en .

veg:SolitaryVegetationObject.function
        a                owl:ObjectProperty ;
        rdfs:domain      veg:SolitaryVegetationObject ;
        rdfs:range       veg:SolitaryVegetationObjectFunctionValue ;
        skos:definition  "Specifies the intended purposes of the SolitaryVegetationObject."@en ;
        skos:prefLabel   "function"@en .

veg:SolitaryVegetationObject.trunkDiameter
        a                owl:DatatypeProperty ;
        rdfs:domain      veg:SolitaryVegetationObject ;
        rdfs:range       sc:Measure ;
        skos:definition  "Specifies the diameter of the SolitaryCityObject's trunk."@en ;
        skos:prefLabel   "trunkDiameter"@en .
