@prefix sc:    <http://shapechange.net/resources/ont/base#> .
@prefix core:  <https://github.com/VCityTeam/UD-Graph/Ontologies/core#> .
@prefix con:   <https://github.com/VCityTeam/UD-Graph/Ontologies/construction#> .
@prefix bldg:  <https://github.com/VCityTeam/UD-Graph/Ontologies/building#> .
@prefix iso19150-2: <http://def.isotc211.org/iso19150/-2/2012/base#> .
@prefix rdf:   <http://www.w3.org/1999/02/22-rdf-syntax-ns#> .
@prefix owl:   <http://www.w3.org/2002/07/owl#> .
@prefix iso19136: <http://def.isotc211.org/iso19136/2007/GML> .
@prefix xsd:   <http://www.w3.org/2001/XMLSchema#> .
@prefix skos:  <http://www.w3.org/2004/02/skos/core#> .
@prefix rdfs:  <http://www.w3.org/2000/01/rdf-schema#> .

bldg:BuildingRoom.adeOfBuildingRoom
        a                owl:ObjectProperty ;
        rdfs:domain      bldg:BuildingRoom ;
        rdfs:range       bldg:ADEOfBuildingRoom ;
        skos:definition  "Augments the BuildingRoom with properties defined in an ADE."@en ;
        skos:prefLabel   "adeOfBuildingRoom"@en .

bldg:Building.buildingPart
        a                owl:ObjectProperty ;
        rdfs:domain      bldg:Building ;
        rdfs:range       bldg:BuildingPart ;
        skos:definition  "Relates the building parts to the Building."@en ;
        skos:prefLabel   "buildingPart"@en .

bldg:ADEOfBuildingPart
        a                      owl:Class ;
        iso19150-2:isAbstract  true ;
        skos:definition        "ADEOfBuildingPart acts as a hook to define properties within an ADE that are to be added to a BuildingPart."@en ;
        skos:prefLabel         "ADEOfBuildingPart"@en .

bldg:ADEOfAbstractBuildingSubdivision
        a                      owl:Class ;
        iso19150-2:isAbstract  true ;
        skos:definition        "ADEOfAbstractBuildingSubdivision acts as a hook to define properties within an ADE that are to be added to AbstractBuildingSubdivision."@en ;
        skos:prefLabel         "ADEOfAbstractBuildingSubdivision"@en .

bldg:AbstractBuildingSubdivision.sortKey
        a                owl:DatatypeProperty ;
        rdfs:domain      bldg:AbstractBuildingSubdivision ;
        rdfs:range       xsd:double ;
        skos:definition  "Defines an order among the objects that belong to the building subdivision. An example is the sorting of storeys."@en ;
        skos:prefLabel   "sortKey"@en .

bldg:AbstractBuildingSubdivision.adeOfAbstractBuildingSubdivision
        a                owl:ObjectProperty ;
        rdfs:domain      bldg:AbstractBuildingSubdivision ;
        rdfs:range       bldg:ADEOfAbstractBuildingSubdivision ;
        skos:definition  "Augments AbstractBuildingSubdivision with properties defined in an ADE."@en ;
        skos:prefLabel   "adeOfAbstractBuildingSubdivision"@en .

bldg:ADEOfBuildingUnit
        a                      owl:Class ;
        iso19150-2:isAbstract  true ;
        skos:definition        "ADEOfBuildingUnit acts as a hook to define properties within an ADE that are to be added to a BuildingUnit."@en ;
        skos:prefLabel         "ADEOfBuildingUnit"@en .

bldg:AbstractBuildingSubdivision.function
        a                owl:ObjectProperty ;
        rdfs:domain      bldg:AbstractBuildingSubdivision ;
        rdfs:range       bldg:BuildingSubdivisionFunctionValue ;
        skos:definition  "Specifies the intended purposes of the building subdivision."@en ;
        skos:prefLabel   "function"@en .

bldg:BuildingConstructiveElement.function
        a                owl:ObjectProperty ;
        rdfs:domain      bldg:BuildingConstructiveElement ;
        rdfs:range       bldg:BuildingConstructiveElementFunctionValue ;
        skos:definition  "Specifies the intended purposes of the BuildingConstructiveElement."@en ;
        skos:prefLabel   "function"@en .

bldg:RoomElevationReferenceValue
        a                owl:Class ;
        rdfs:subClassOf  skos:Concept ;
        skos:definition  "RoomElevationReferenceValue is a code list that enumerates the different elevation reference levels used to measure room heights."@en ;
        skos:prefLabel   "RoomElevationReferenceValue"@en .

bldg:BuildingConstructiveElementUsageValue
        a                owl:Class ;
        rdfs:subClassOf  skos:Concept ;
        skos:definition  "BuildingConstructiveElementUsageValue is a code list that enumerates the different uses of a BuildingConstructiveElement."@en ;
        skos:prefLabel   "BuildingConstructiveElementUsageValue"@en .

bldg:AbstractBuilding.function
        a                owl:ObjectProperty ;
        rdfs:domain      bldg:AbstractBuilding ;
        rdfs:range       bldg:BuildingFunctionValue ;
        skos:definition  "Specifies the intended purposes of the Building or BuildingPart."@en ;
        skos:prefLabel   "function"@en .

bldg:BuildingRoom.usage
        a                owl:ObjectProperty ;
        rdfs:domain      bldg:BuildingRoom ;
        rdfs:range       bldg:BuildingRoomUsageValue ;
        skos:definition  "Specifies the actual uses of the BuildingRoom."@en ;
        skos:prefLabel   "usage"@en .

bldg:BuildingConstructiveElement.usage
        a                owl:ObjectProperty ;
        rdfs:domain      bldg:BuildingConstructiveElement ;
        rdfs:range       bldg:BuildingConstructiveElementUsageValue ;
        skos:definition  "Specifies the actual uses of the BuildingConstructiveElement."@en ;
        skos:prefLabel   "usage"@en .

bldg:Storey.boundary  a  owl:ObjectProperty ;
        rdfs:domain     bldg:Storey ;
        rdfs:range      core:AbstractThematicSurface ;
        skos:prefLabel  "boundary"@en .

bldg:AbstractBuilding.adeOfAbstractBuilding
        a                owl:ObjectProperty ;
        rdfs:domain      bldg:AbstractBuilding ;
        rdfs:range       bldg:ADEOfAbstractBuilding ;
        skos:definition  "Augments AbstractBuilding with properties defined in an ADE."@en ;
        skos:prefLabel   "adeOfAbstractBuilding"@en .

bldg:BuildingInstallationUsageValue
        a                owl:Class ;
        rdfs:subClassOf  skos:Concept ;
        skos:definition  "BuildingInstallationUsageValue is a code list that enumerates the different uses of a BuildingInstallation."@en ;
        skos:prefLabel   "BuildingInstallationUsageValue"@en .

bldg:Storey.buildingUnit
        a                owl:ObjectProperty ;
        rdfs:domain      bldg:Storey ;
        rdfs:range       bldg:BuildingUnit ;
        skos:definition  "Relates to the building units that belong to the Storey."@en ;
        skos:prefLabel   "buildingUnit"@en .

bldg:BuildingInstallation
        a                owl:Class ;
        rdfs:subClassOf  con:AbstractInstallation ;
        skos:definition  "A BuildingInstallation is a permanent part of a Building (inside and/or outside) which has not the significance of a BuildingPart. Examples are stairs, antennas, balconies or small roofs."@en ;
        skos:prefLabel   "BuildingInstallation"@en .

bldg:BuildingUsageValue
        a                owl:Class ;
        rdfs:subClassOf  skos:Concept ;
        skos:definition  "BuildingUsageValue is a code list that enumerates the different uses of a Building."@en ;
        skos:prefLabel   "BuildingUsageValue"@en .

bldg:BuildingSubdivisionClassValue
        a                owl:Class ;
        rdfs:subClassOf  skos:Concept ;
        skos:definition  "BuildingSubdivisionClassValue is a code list used to further classify a BuildingSubdivision."@en ;
        skos:prefLabel   "BuildingSubdivisionClassValue"@en .

bldg:AbstractBuildingSubdivision.buildingFurniture
        a                owl:ObjectProperty ;
        rdfs:domain      bldg:AbstractBuildingSubdivision ;
        rdfs:range       bldg:BuildingFurniture ;
        skos:definition  "Relates the furniture objects to the building subdivision."@en ;
        skos:prefLabel   "buildingFurniture"@en .

bldg:RoomHeight.status
        a                owl:ObjectProperty ;
        rdfs:domain      bldg:RoomHeight ;
        rdfs:range       con:HeightStatusValue ;
        skos:definition  "Indicates the way the room height has been captured."@en ;
        skos:prefLabel   "status"@en .

bldg:BuildingRoomFunctionValue
        a                owl:Class ;
        rdfs:subClassOf  skos:Concept ;
        skos:definition  "BuildingRoomFunctionValue is a code list that enumerates the different purposes of a BuildingRoom."@en ;
        skos:prefLabel   "BuildingRoomFunctionValue"@en .

bldg:AbstractBuilding.usage
        a                owl:ObjectProperty ;
        rdfs:domain      bldg:AbstractBuilding ;
        rdfs:range       bldg:BuildingUsageValue ;
        skos:definition  "Specifies the actual uses of the Building or BuildingPart."@en ;
        skos:prefLabel   "usage"@en .

bldg:AbstractBuilding
        a                      owl:Class ;
        rdfs:subClassOf        con:AbstractConstruction ;
        iso19150-2:isAbstract  true ;
        skos:definition        "AbstractBuilding is an abstract superclass representing the common attributes and associations of the classes Building and BuildingPart."@en ;
        skos:prefLabel         "AbstractBuilding"@en .

bldg:ADEOfBuilding  a          owl:Class ;
        iso19150-2:isAbstract  true ;
        skos:definition        "ADEOfBuilding acts as a hook to define properties within an ADE that are to be added to a Building."@en ;
        skos:prefLabel         "ADEOfBuilding"@en .

bldg:AbstractBuilding.buildingSubdivision
        a                owl:ObjectProperty ;
        rdfs:domain      bldg:AbstractBuilding ;
        rdfs:range       bldg:AbstractBuildingSubdivision ;
        skos:definition  "Relates the logical subdivisions to the Building or BuildingPart."@en ;
        skos:prefLabel   "buildingSubdivision"@en .

bldg:Storey  a           owl:Class ;
        rdfs:subClassOf  bldg:AbstractBuildingSubdivision ;
        skos:definition  "A Storey is a horizontal section of a Building."@en ;
        skos:prefLabel   "Storey"@en .

bldg:AbstractBuilding.buildingRoom
        a                owl:ObjectProperty ;
        rdfs:domain      bldg:AbstractBuilding ;
        rdfs:range       bldg:BuildingRoom ;
        skos:definition  "Relates the rooms to the Building or BuildingPart."@en ;
        skos:prefLabel   "buildingRoom"@en .

bldg:BuildingFurniture.function
        a                owl:ObjectProperty ;
        rdfs:domain      bldg:BuildingFurniture ;
        rdfs:range       bldg:BuildingFurnitureFunctionValue ;
        skos:definition  "Specifies the intended purposes of the BuildingFurniture."@en ;
        skos:prefLabel   "function"@en .

bldg:BuildingRoom.buildingInstallation
        a                owl:ObjectProperty ;
        rdfs:domain      bldg:BuildingRoom ;
        rdfs:range       bldg:BuildingInstallation ;
        skos:definition  "Relates the installation objects to the BuildingRoom."@en ;
        skos:prefLabel   "buildingInstallation"@en .

bldg:ADEOfStorey  a            owl:Class ;
        iso19150-2:isAbstract  true ;
        skos:definition        "ADEOfStorey acts as a hook to define properties within an ADE that are to be added to a Storey."@en ;
        skos:prefLabel         "ADEOfStorey"@en .

bldg:BuildingUnit.storey
        a                owl:ObjectProperty ;
        rdfs:domain      bldg:BuildingUnit ;
        rdfs:range       bldg:Storey ;
        skos:definition  "Relates to the storeys on which the BuildingUnit is located."@en ;
        skos:prefLabel   "storey"@en .

<https://github.com/VCityTeam/UD-Graph/Ontologies/building>
        a                owl:Ontology ;
        owl:imports      <http://shapechange.net/resources/ont/base> , <https://github.com/VCityTeam/UD-Graph/Ontologies/construction> , <https://github.com/VCityTeam/UD-Graph/Ontologies/core> , <http://def.isotc211.org/iso19150/-2/2012/base> ;
        owl:versionIRI   "https://github.com/VCityTeam/UD-Graph/Ontologies/building/3.0.0" ;
        owl:versionInfo  "3.0.0" ;
        skos:definition  "The Building module supports representation of thematic and spatial aspects of buildings, building parts, building installations, building subdivisions, and interior building structures."@en ;
        skos:prefLabel   "Building"@en .

bldg:BuildingUnit.adeOfBuildingUnit
        a                owl:ObjectProperty ;
        rdfs:domain      bldg:BuildingUnit ;
        rdfs:range       bldg:ADEOfBuildingUnit ;
        skos:definition  "Augments the BuildingUnit with properties defined in an ADE."@en ;
        skos:prefLabel   "adeOfBuildingUnit"@en .

bldg:ADEOfAbstractBuilding
        a                      owl:Class ;
        iso19150-2:isAbstract  true ;
        skos:definition        "ADEOfAbstractBuilding acts as a hook to define properties within an ADE that are to be added to AbstractBuilding."@en ;
        skos:prefLabel         "ADEOfAbstractBuilding"@en .

bldg:BuildingSubdivisionUsageValue
        a                owl:Class ;
        rdfs:subClassOf  skos:Concept ;
        skos:definition  "BuildingSubdivisionUsageValue is a code list that enumerates the different uses of a BuildingSubdivision."@en ;
        skos:prefLabel   "BuildingSubdivisionUsageValue"@en .

bldg:AbstractBuildingSubdivision.elevation
        a                owl:ObjectProperty ;
        rdfs:domain      bldg:AbstractBuildingSubdivision ;
        rdfs:range       con:Elevation ;
        skos:definition  "Specifies qualified elevations of the building subdivision in relation to a well-defined surface which is commonly taken as origin (e.g. geoid or water level). [cf. INSPIRE]"@en ;
        skos:prefLabel   "elevation"@en .

bldg:AbstractBuildingSubdivision.buildingInstallation
        a                owl:ObjectProperty ;
        rdfs:domain      bldg:AbstractBuildingSubdivision ;
        rdfs:range       bldg:BuildingInstallation ;
        skos:definition  "Relates the installation objects to the building subdivision."@en ;
        skos:prefLabel   "buildingInstallation"@en .

bldg:BuildingFurnitureClassValue
        a                owl:Class ;
        rdfs:subClassOf  skos:Concept ;
        skos:definition  "BuildingFurnitureClassValue is a code list used to further classify a BuildingFurniture."@en ;
        skos:prefLabel   "BuildingFurnitureClassValue"@en .

bldg:BuildingFurniture.class
        a                owl:ObjectProperty ;
        rdfs:domain      bldg:BuildingFurniture ;
        rdfs:range       bldg:BuildingFurnitureClassValue ;
        skos:definition  "Indicates the specific type of the BuildingFurniture."@en ;
        skos:prefLabel   "class"@en .

bldg:BuildingInstallationFunctionValue
        a                owl:Class ;
        rdfs:subClassOf  skos:Concept ;
        skos:definition  "BuildingInstallationFunctionValue is a code list that enumerates the different purposes of a BuildingInstallation."@en ;
        skos:prefLabel   "BuildingInstallationFunctionValue"@en .

bldg:BuildingRoomClassValue
        a                owl:Class ;
        rdfs:subClassOf  skos:Concept ;
        skos:definition  "BuildingRoomClassValue is a code list used to further classify a BuildingRoom."@en ;
        skos:prefLabel   "BuildingRoomClassValue"@en .

bldg:AbstractBuildingSubdivision.buildingRoom
        a                owl:ObjectProperty ;
        rdfs:domain      bldg:AbstractBuildingSubdivision ;
        rdfs:range       bldg:BuildingRoom ;
        skos:definition  "Relates the rooms to the building subdivision."@en ;
        skos:prefLabel   "buildingRoom"@en .

bldg:BuildingConstructiveElement
        a                owl:Class ;
        rdfs:subClassOf  con:AbstractConstructiveElement ;
        skos:definition  "A BuildingConstructiveElement is an element of a Building which is essential from a structural point of view. Examples are walls, slabs, staircases, beams."@en ;
        skos:prefLabel   "BuildingConstructiveElement"@en .

bldg:RoomHeight.lowReference
        a                owl:ObjectProperty ;
        rdfs:domain      bldg:RoomHeight ;
        rdfs:range       bldg:RoomElevationReferenceValue ;
        skos:definition  "Indicates the low point used to calculate the value of the room height."@en ;
        skos:prefLabel   "lowReference"@en .

bldg:BuildingRoom.boundary
        a               owl:ObjectProperty ;
        rdfs:domain     bldg:BuildingRoom ;
        rdfs:range      core:AbstractThematicSurface ;
        skos:prefLabel  "boundary"@en .

bldg:BuildingUnit.address
        a                owl:ObjectProperty ;
        rdfs:domain      bldg:BuildingUnit ;
        rdfs:range       core:Address ;
        skos:definition  "Relates to the addresses that are assigned to the BuildingUnit."@en ;
        skos:prefLabel   "address"@en .

bldg:AbstractBuildingSubdivision.class
        a                owl:ObjectProperty ;
        rdfs:domain      bldg:AbstractBuildingSubdivision ;
        rdfs:range       bldg:BuildingSubdivisionClassValue ;
        skos:definition  "Indicates the specific type of the building subdivision."@en ;
        skos:prefLabel   "class"@en .

bldg:BuildingRoom.buildingFurniture
        a                owl:ObjectProperty ;
        rdfs:domain      bldg:BuildingRoom ;
        rdfs:range       bldg:BuildingFurniture ;
        skos:definition  "Relates the furniture objects to the BuildingRoom."@en ;
        skos:prefLabel   "buildingFurniture"@en .

bldg:Storey.adeOfStorey
        a                owl:ObjectProperty ;
        rdfs:domain      bldg:Storey ;
        rdfs:range       bldg:ADEOfStorey ;
        skos:definition  "Augments the Storey with properties defined in an ADE."@en ;
        skos:prefLabel   "adeOfStorey"@en .

bldg:BuildingPart.adeOfBuildingPart
        a                owl:ObjectProperty ;
        rdfs:domain      bldg:BuildingPart ;
        rdfs:range       bldg:ADEOfBuildingPart ;
        skos:definition  "Augments the BuildingPart with properties defined in an ADE."@en ;
        skos:prefLabel   "adeOfBuildingPart"@en .

bldg:BuildingFunctionValue
        a                owl:Class ;
        rdfs:subClassOf  skos:Concept ;
        skos:definition  "BuildingFunctionValue is a code list that enumerates the different purposes of a Building."@en ;
        skos:prefLabel   "BuildingFunctionValue"@en .

bldg:BuildingFurniture
        a                owl:Class ;
        rdfs:subClassOf  con:AbstractFurniture ;
        skos:definition  "A BuildingFurniture is an equipment for occupant use, usually not fixed to the building. [cf. ISO 6707-1]"@en ;
        skos:prefLabel   "BuildingFurniture"@en .

bldg:Building.adeOfBuilding
        a                owl:ObjectProperty ;
        rdfs:domain      bldg:Building ;
        rdfs:range       bldg:ADEOfBuilding ;
        skos:definition  "Augments the Building with properties defined in an ADE."@en ;
        skos:prefLabel   "adeOfBuilding"@en .

bldg:BuildingInstallation.class
        a                owl:ObjectProperty ;
        rdfs:domain      bldg:BuildingInstallation ;
        rdfs:range       bldg:BuildingInstallationClassValue ;
        skos:definition  "Indicates the specific type of the BuildingInstallation."@en ;
        skos:prefLabel   "class"@en .

bldg:BuildingFurnitureUsageValue
        a                owl:Class ;
        rdfs:subClassOf  skos:Concept ;
        skos:definition  "BuildingFurnitureUsageValue is a code list that enumerates the different uses of a BuildingFurniture."@en ;
        skos:prefLabel   "BuildingFurnitureUsageValue"@en .

bldg:BuildingConstructiveElementFunctionValue
        a                owl:Class ;
        rdfs:subClassOf  skos:Concept ;
        skos:definition  "BuildingConstructiveElementFunctionValue is a code list that enumerates the different purposes of a BuildingConstructiveElement."@en ;
        skos:prefLabel   "BuildingConstructiveElementFunctionValue"@en .

bldg:AbstractBuilding.roofType
        a                owl:ObjectProperty ;
        rdfs:domain      bldg:AbstractBuilding ;
        rdfs:range       bldg:RoofTypeValue ;
        skos:definition  "Indicates the shape of the roof of the Building or BuildingPart."@en ;
        skos:prefLabel   "roofType"@en .

bldg:BuildingRoom.function
        a                owl:ObjectProperty ;
        rdfs:domain      bldg:BuildingRoom ;
        rdfs:range       bldg:BuildingRoomFunctionValue ;
        skos:definition  "Specifies the intended purposes of the BuildingRoom."@en ;
        skos:prefLabel   "function"@en .

bldg:BuildingRoomUsageValue
        a                owl:Class ;
        rdfs:subClassOf  skos:Concept ;
        skos:definition  "BuildingRoomUsageValue is a code list that enumerates the different uses of a BuildingRoom."@en ;
        skos:prefLabel   "BuildingRoomUsageValue"@en .

bldg:AbstractBuildingSubdivision.buildingConstructiveElement
        a                owl:ObjectProperty ;
        rdfs:domain      bldg:AbstractBuildingSubdivision ;
        rdfs:range       bldg:BuildingConstructiveElement ;
        skos:definition  "Relates the constructive elements to the building subdivision."@en ;
        skos:prefLabel   "buildingConstructiveElement"@en .

bldg:BuildingInstallation.function
        a                owl:ObjectProperty ;
        rdfs:domain      bldg:BuildingInstallation ;
        rdfs:range       bldg:BuildingInstallationFunctionValue ;
        skos:definition  "Specifies the intended purposes of the BuildingInstallation."@en ;
        skos:prefLabel   "function"@en .

bldg:AbstractBuilding.buildingFurniture
        a                owl:ObjectProperty ;
        rdfs:domain      bldg:AbstractBuilding ;
        rdfs:range       bldg:BuildingFurniture ;
        skos:definition  "Relates the furniture objects to the Building or BuildingPart."@en ;
        skos:prefLabel   "buildingFurniture"@en .

bldg:AbstractBuilding.buildingConstructiveElement
        a                owl:ObjectProperty ;
        rdfs:domain      bldg:AbstractBuilding ;
        rdfs:range       bldg:BuildingConstructiveElement ;
        skos:definition  "Relates the constructive elements to the Building or BuildingPart."@en ;
        skos:prefLabel   "buildingConstructiveElement"@en .

bldg:BuildingSubdivisionFunctionValue
        a                owl:Class ;
        rdfs:subClassOf  skos:Concept ;
        skos:definition  "BuildingSubdivisionFunctionValue is a code list that enumerates the different purposes of a BuildingSubdivision."@en ;
        skos:prefLabel   "BuildingSubdivisionFunctionValue"@en .

bldg:BuildingFurniture.usage
        a                owl:ObjectProperty ;
        rdfs:domain      bldg:BuildingFurniture ;
        rdfs:range       bldg:BuildingFurnitureUsageValue ;
        skos:definition  "Specifies the actual uses of the BuildingFurniture."@en ;
        skos:prefLabel   "usage"@en .

bldg:ADEOfBuildingInstallation
        a                      owl:Class ;
        iso19150-2:isAbstract  true ;
        skos:definition        "ADEOfBuildingInstallation acts as a hook to define properties within an ADE that are to be added to a BuildingInstallation."@en ;
        skos:prefLabel         "ADEOfBuildingInstallation"@en .

bldg:RoofTypeValue  a    owl:Class ;
        rdfs:subClassOf  skos:Concept ;
        skos:definition  "RoofTypeValue is a code list that enumerates different roof types."@en ;
        skos:prefLabel   "RoofTypeValue"@en .

bldg:BuildingRoom  a     owl:Class ;
        rdfs:subClassOf  core:AbstractUnoccupiedSpace ;
        skos:definition  "A BuildingRoom is a space within a Building or BuildingPart intended for human occupancy (e.g. a place of work or recreation) and/or containment of animals or things. A BuildingRoom is bounded physically and/or virtually (e.g. by ClosureSurfaces or GenericSurfaces)."@en ;
        skos:prefLabel   "BuildingRoom"@en .

bldg:AbstractBuilding.storeysBelowGround
        a                owl:DatatypeProperty ;
        rdfs:domain      bldg:AbstractBuilding ;
        rdfs:range       xsd:integer ;
        skos:definition  "Indicates the number of storeys positioned below ground level."@en ;
        skos:prefLabel   "storeysBelowGround"@en .

bldg:AbstractBuilding.storeysAboveGround
        a                owl:DatatypeProperty ;
        rdfs:domain      bldg:AbstractBuilding ;
        rdfs:range       xsd:integer ;
        skos:definition  "Indicates the number of storeys positioned above ground level."@en ;
        skos:prefLabel   "storeysAboveGround"@en .

bldg:RoomHeight.value
        a                owl:DatatypeProperty ;
        rdfs:domain      bldg:RoomHeight ;
        rdfs:range       sc:Measure ;
        skos:definition  "Specifies the value of the room height."@en ;
        skos:prefLabel   "value"@en .

bldg:BuildingRoom.class
        a                owl:ObjectProperty ;
        rdfs:domain      bldg:BuildingRoom ;
        rdfs:range       bldg:BuildingRoomClassValue ;
        skos:definition  "Indicates the specific type of the BuildingRoom."@en ;
        skos:prefLabel   "class"@en .

bldg:BuildingConstructiveElement.adeOfBuildingConstructiveElement
        a                owl:ObjectProperty ;
        rdfs:domain      bldg:BuildingConstructiveElement ;
        rdfs:range       bldg:ADEOfBuildingConstructiveElement ;
        skos:definition  "Augments the BuildingConstructiveElement with properties defined in an ADE."@en ;
        skos:prefLabel   "adeOfBuildingConstructiveElement"@en .

bldg:Building  a         owl:Class ;
        rdfs:subClassOf  bldg:AbstractBuilding ;
        skos:definition  "A Building is a free-standing, self-supporting construction that is roofed, usually walled, and can be entered by humans and is normally designed to stand permanently in one place. It is intended for human occupancy (e.g. a place of work or recreation), habitation and/or shelter of humans, animals or things."@en ;
        skos:prefLabel   "Building"@en .

bldg:AbstractBuildingSubdivision
        a                      owl:Class ;
        rdfs:subClassOf        core:AbstractLogicalSpace ;
        iso19150-2:isAbstract  true ;
        skos:definition        "AbstractBuildingSubdivision is the abstract superclass for different kinds of logical building subdivisions."@en ;
        skos:prefLabel         "AbstractBuildingSubdivision"@en .

bldg:AbstractBuilding.buildingInstallation
        a                owl:ObjectProperty ;
        rdfs:domain      bldg:AbstractBuilding ;
        rdfs:range       bldg:BuildingInstallation ;
        skos:definition  "Relates the installation objects to the Building or BuildingPart."@en ;
        skos:prefLabel   "buildingInstallation"@en .

bldg:BuildingConstructiveElement.class
        a                owl:ObjectProperty ;
        rdfs:domain      bldg:BuildingConstructiveElement ;
        rdfs:range       bldg:BuildingConstructiveElementClassValue ;
        skos:definition  "Indicates the specific type of the BuildingConstructiveElement."@en ;
        skos:prefLabel   "class"@en .

bldg:AbstractBuildingSubdivision.usage
        a                owl:ObjectProperty ;
        rdfs:domain      bldg:AbstractBuildingSubdivision ;
        rdfs:range       bldg:BuildingSubdivisionUsageValue ;
        skos:definition  "Specifies the actual uses of the building subdivision."@en ;
        skos:prefLabel   "usage"@en .

bldg:ADEOfBuildingFurniture
        a                      owl:Class ;
        iso19150-2:isAbstract  true ;
        skos:definition        "ADEOfBuildingFurniture acts as a hook to define properties within an ADE that are to be added to a BuildingFurniture."@en ;
        skos:prefLabel         "ADEOfBuildingFurniture"@en .

bldg:ADEOfBuildingRoom
        a                      owl:Class ;
        iso19150-2:isAbstract  true ;
        skos:definition        "ADEOfBuildingRoom acts as a hook to define properties within an ADE that are to be added to a BuildingRoom."@en ;
        skos:prefLabel         "ADEOfBuildingRoom"@en .

bldg:BuildingConstructiveElementClassValue
        a                owl:Class ;
        rdfs:subClassOf  skos:Concept ;
        skos:definition  "BuildingConstructiveElementClassValue is a code list used to further classify a BuildingConstructiveElement."@en ;
        skos:prefLabel   "BuildingConstructiveElementClassValue"@en .

bldg:BuildingFurniture.adeOfBuildingFurniture
        a                owl:ObjectProperty ;
        rdfs:domain      bldg:BuildingFurniture ;
        rdfs:range       bldg:ADEOfBuildingFurniture ;
        skos:definition  "Augments the BuildingFurniture with properties defined in an ADE."@en ;
        skos:prefLabel   "adeOfBuildingFurniture"@en .

bldg:AbstractBuilding.storeyHeightsBelowGround
        a                owl:ObjectProperty ;
        rdfs:domain      bldg:AbstractBuilding ;
        rdfs:range       iso19136:MeasureOrNilReasonList ;
        skos:definition  "Lists the height of each storey below ground. The first value in the list denotes the height of the storey closest to the ground level, the last value denotes the height furthest away."@en ;
        skos:prefLabel   "storeyHeightsBelowGround"@en .

bldg:RoomHeight.highReference
        a                owl:ObjectProperty ;
        rdfs:domain      bldg:RoomHeight ;
        rdfs:range       bldg:RoomElevationReferenceValue ;
        skos:definition  "Indicates the high point used to calculate the value of the room height."@en ;
        skos:prefLabel   "highReference"@en .

bldg:BuildingFurnitureFunctionValue
        a                owl:Class ;
        rdfs:subClassOf  skos:Concept ;
        skos:definition  "BuildingFurnitureFunctionValue is a code list that enumerates the different purposes of a BuildingFurniture."@en ;
        skos:prefLabel   "BuildingFurnitureFunctionValue"@en .

bldg:BuildingPart  a     owl:Class ;
        rdfs:subClassOf  bldg:AbstractBuilding ;
        skos:definition  "A BuildingPart is a physical or functional subdivision of a Building. It would be considered a Building, if it were not part of a collection of other BuildingParts."@en ;
        skos:prefLabel   "BuildingPart"@en .

bldg:AbstractBuilding.address
        a                owl:ObjectProperty ;
        rdfs:domain      bldg:AbstractBuilding ;
        rdfs:range       core:Address ;
        skos:definition  "Relates the addresses to the Building or BuildingPart."@en ;
        skos:prefLabel   "address"@en .

bldg:AbstractBuilding.storeyHeightsAboveGround
        a                owl:ObjectProperty ;
        rdfs:domain      bldg:AbstractBuilding ;
        rdfs:range       iso19136:MeasureOrNilReasonList ;
        skos:definition  "Lists the heights of each storey above ground. The first value in the list denotes the height of the storey closest to the ground level, the last value denotes the height furthest away."@en ;
        skos:prefLabel   "storeyHeightsAboveGround"@en .

bldg:BuildingInstallationClassValue
        a                owl:Class ;
        rdfs:subClassOf  skos:Concept ;
        skos:definition  "BuildingInstallationClassValue is a code list used to further classify a BuildingInstallation."@en ;
        skos:prefLabel   "BuildingInstallationClassValue"@en .

bldg:BuildingRoom.roomHeight
        a                owl:ObjectProperty ;
        rdfs:domain      bldg:BuildingRoom ;
        rdfs:range       bldg:RoomHeight ;
        skos:definition  "Specifies qualified heights of the BuildingRoom."@en ;
        skos:prefLabel   "roomHeight"@en .

bldg:BuildingInstallation.usage
        a                owl:ObjectProperty ;
        rdfs:domain      bldg:BuildingInstallation ;
        rdfs:range       bldg:BuildingInstallationUsageValue ;
        skos:definition  "Specifies the actual uses of the BuildingInstallation."@en ;
        skos:prefLabel   "usage"@en .

bldg:RoomHeight  a       owl:Class ;
        skos:definition  "The RoomHeight represents a vertical distance (measured or estimated) between a low reference and a high reference. [cf. INSPIRE]"@en ;
        skos:prefLabel   "RoomHeight"@en .

bldg:BuildingUnit  a     owl:Class ;
        rdfs:subClassOf  bldg:AbstractBuildingSubdivision ;
        skos:definition  "A BuildingUnit is a logical subdivision of a Building. BuildingUnits are formed according to some homogeneous property like function, ownership, management, or accessability. They may be separately sold, rented out, inherited, managed, etc."@en ;
        skos:prefLabel   "BuildingUnit"@en .

bldg:BuildingClassValue
        a                owl:Class ;
        rdfs:subClassOf  skos:Concept ;
        skos:definition  "BuildingClassValue is a code list used to further classify a Building."@en ;
        skos:prefLabel   "BuildingClassValue"@en .

bldg:ADEOfBuildingConstructiveElement
        a                      owl:Class ;
        iso19150-2:isAbstract  true ;
        skos:definition        "ADEOfBuildingConstructiveElement acts as a hook to define properties within an ADE that are to be added to a BuildingConstructiveElement."@en ;
        skos:prefLabel         "ADEOfBuildingConstructiveElement"@en .

bldg:AbstractBuilding.class
        a                owl:ObjectProperty ;
        rdfs:domain      bldg:AbstractBuilding ;
        rdfs:range       bldg:BuildingClassValue ;
        skos:definition  "Indicates the specific type of the Building or BuildingPart."@en ;
        skos:prefLabel   "class"@en .

bldg:BuildingInstallation.adeOfBuildingInstallation
        a                owl:ObjectProperty ;
        rdfs:domain      bldg:BuildingInstallation ;
        rdfs:range       bldg:ADEOfBuildingInstallation ;
        skos:definition  "Augments the BuildingInstallation with properties defined in an ADE."@en ;
        skos:prefLabel   "adeOfBuildingInstallation"@en .
