@prefix core:  <https://github.com/VCityTeam/UD-Graph/core#> .
@prefix gen:   <https://github.com/VCityTeam/UD-Graph/generics#> .
@prefix iso19150-2: <http://def.isotc211.org/iso19150/-2/2012/base#> .
@prefix owl:   <http://www.w3.org/2002/07/owl#> .
@prefix rdf:   <http://www.w3.org/1999/02/22-rdf-syntax-ns#> .
@prefix gsp:   <http://www.opengis.net/ont/geosparql#> .
@prefix xsd:   <http://www.w3.org/2001/XMLSchema#> .
@prefix iso19136: <http://def.isotc211.org/iso19136/2007/GML> .
@prefix skos:  <http://www.w3.org/2004/02/skos/core#> .
@prefix rdfs:  <http://www.w3.org/2000/01/rdf-schema#> .

core:XALAddressDetails
        a               owl:Class ;
        skos:prefLabel  "XALAddressDetails"@en .

core:CityModel  a        owl:Class ;
        skos:definition  "SIG3D: Collection of CityObjects with optional metadata."@en ;
        skos:prefLabel   "CityModel"@en .

core:ExternalObjectReference
        a                owl:Class ;
        rdfs:subClassOf  [ a            owl:Class ;
                           owl:unionOf  ( [ a                   owl:Class ;
                                            owl:intersectionOf  ( [ a                   owl:Restriction ;
                                                                    owl:minCardinality  "0"^^xsd:nonNegativeInteger ;
                                                                    owl:onProperty      core:ExternalObjectReference.name
                                                                  ]
                                                                  [ a                owl:Restriction ;
                                                                    owl:cardinality  "0"^^xsd:nonNegativeInteger ;
                                                                    owl:onProperty   core:ExternalObjectReference.uri
                                                                  ]
                                                                )
                                          ]
                                          [ a                   owl:Class ;
                                            owl:intersectionOf  ( [ a                owl:Restriction ;
                                                                    owl:cardinality  "0"^^xsd:nonNegativeInteger ;
                                                                    owl:onProperty   core:ExternalObjectReference.name
                                                                  ]
                                                                  [ a                   owl:Restriction ;
                                                                    owl:minCardinality  "0"^^xsd:nonNegativeInteger ;
                                                                    owl:onProperty      core:ExternalObjectReference.uri
                                                                  ]
                                                                )
                                          ]
                                        )
                         ] ;
        skos:definition  "SIG3D: Object in  an external information system or data set."@en ;
        skos:prefLabel   "ExternalObjectReference"@en .

core:AbstractCityObject.terminationDate
        a                owl:DatatypeProperty ;
        rdfs:domain      core:AbstractCityObject ;
        rdfs:range       xsd:date ;
        skos:definition  "SIG3D:  Date the AbstractCityObject was removed"@en ;
        skos:prefLabel   "terminationDate"@en .

core:AbstractCityObject.relativeToTerrain
        a                owl:ObjectProperty ;
        rdfs:domain      core:AbstractCityObject ;
        rdfs:range       core:RelativeToTerrain ;
        skos:definition  "SIG3D: Vertical position of the \r\nAbstractCityObject relative to the surrounding terrain."@en ;
        skos:prefLabel   "relativeToTerrain"@en .

core:AbstractCityObject.creationDate
        a                owl:DatatypeProperty ;
        rdfs:domain      core:AbstractCityObject ;
        rdfs:range       xsd:date ;
        skos:definition  "SIG3D: Date the AbstractCityObject was generated."@en ;
        skos:prefLabel   "creationDate"@en .

core:ExternalObjectReference.uri
        a                owl:DatatypeProperty ;
        rdfs:domain      core:ExternalObjectReference ;
        rdfs:range       xsd:anyURI ;
        skos:definition  "SIG3D: URL or URN of the object."@en ;
        skos:prefLabel   "uri"@en .

core:ExternalReference.externalObject
        a                owl:ObjectProperty ;
        rdfs:domain      core:ExternalReference ;
        rdfs:range       core:ExternalObjectReference ;
        skos:definition  "SIG3D: Referenced object in the external information system or data set."@en ;
        skos:prefLabel   "externalObject"@en .

core:AbstractAppearance
        a                      owl:Class ;
        iso19150-2:isAbstract  true ;
        skos:prefLabel         "AbstractAppearance"@en .

core:AbstractCityObject.externalReference
        a                owl:ObjectProperty ;
        rdfs:domain      core:AbstractCityObject ;
        rdfs:range       core:ExternalReference ;
        skos:definition  "SIG3D: Relation to an ExternalReference"@en ;
        skos:prefLabel   "externalReference"@en .

core:ExternalObjectReference.name
        a                owl:DatatypeProperty ;
        rdfs:domain      core:ExternalObjectReference ;
        rdfs:range       xsd:string ;
        skos:definition  "SIG3D: Name of the object"@en ;
        skos:prefLabel   "name"@en .

core:TransformationMatrix3x4.list
        a               owl:ObjectProperty ;
        rdfs:domain     core:TransformationMatrix3x4 ;
        rdfs:range      iso19136:doubleList ;
        skos:prefLabel  "list"@en .

core:TransformationMatrix2x2
        a                owl:Class ;
        skos:definition  "SIG3D: 2x2 Transformation matrix (z-rotation and scaling)"@en ;
        skos:prefLabel   "TransformationMatrix2x2"@en .

core:CityModel.appearanceMember
        a               owl:ObjectProperty ;
        rdfs:domain     core:CityModel ;
        rdfs:range      core:AbstractAppearance ;
        skos:prefLabel  "appearanceMember"@en .

core:ImplicitGeometry
        a                owl:Class ;
        skos:definition  "SIG3D: A  geometric representation where the shape is stored only once as a prototypical geometry, for example a tree or other vegetation object, a traffic light or a traffic sign. This prototypic geometry object can be re-used or referenced many times, wherever the corresponding feature occurs in the 3D city model."@en ;
        skos:prefLabel   "ImplicitGeometry"@en .

core:IntegerBetween0and4
        a               owl:Class ;
        skos:prefLabel  "IntegerBetween0and4"@en .

core:AbstractCityObject.abstractGenericAttribute
        a               owl:ObjectProperty ;
        rdfs:domain     core:AbstractCityObject ;
        rdfs:range      gen:AbstractGenericAttribute ;
        skos:prefLabel  "abstractGenericAttribute"@en .

<https://github.com/VCityTeam/UD-Graph/core>
        a                owl:Ontology ;
        owl:imports      <https://github.com/VCityTeam/UD-Graph/generics> , <http://www.opengis.net/ont/geosparql> , <http://def.isotc211.org/iso19150/-2/2012/base> ;
        owl:versionIRI   "https://github.com/VCityTeam/UD-Graph/core/1.0" ;
        owl:versionInfo  "1.0" ;
        skos:prefLabel   "Core"@en .

core:TransformationMatrix4x4.list
        a                owl:ObjectProperty ;
        rdfs:domain      core:TransformationMatrix4x4 ;
        rdfs:range       iso19136:doubleList ;
        skos:definition  "SIG3D: Elements of the transformation matrix in row major order."@en ;
        skos:prefLabel   "list"@en .

core:CityModel.cityObjectMember
        a                owl:ObjectProperty ;
        rdfs:domain      core:CityModel ;
        rdfs:range       core:AbstractCityObject ;
        skos:definition  "SIG3D: Relation of CityModel to AbstractCityObject."@en ;
        skos:prefLabel   "cityObjectMember"@en .

core:ImplicitGeometry.relativeGMLGeometry
        a               owl:ObjectProperty ;
        rdfs:domain     core:ImplicitGeometry ;
        rdfs:range      gsp:Geometry ;
        skos:prefLabel  "relativeGMLGeometry"@en .

core:ImplicitGeometry.mimeType
        a                owl:ObjectProperty ;
        rdfs:domain      core:ImplicitGeometry ;
        rdfs:range       iso19136:Code ;
        skos:definition  "SIG3D: Mime type of the referenced external geometric object (attribute libraryObject)."@en ;
        skos:prefLabel   "mimeType"@en .

core:Address  a          owl:Class ;
        skos:definition  "SIG3D: Proxy for the OASIS address schema"@en ;
        skos:prefLabel   "Address"@en .

core:Address.xalAddress
        a               owl:ObjectProperty ;
        rdfs:domain     core:Address ;
        rdfs:range      core:XALAddressDetails ;
        skos:prefLabel  "xalAddress"@en .

core:DoubleBetween0and1List
        a               owl:Class ;
        skos:prefLabel  "DoubleBetween0and1List"@en .

core:ImplicitGeometry.referencePoint
        a               owl:ObjectProperty ;
        rdfs:domain     core:ImplicitGeometry ;
        rdfs:range      gsp:Geometry ;
        skos:prefLabel  "referencePoint"@en .

core:RelativeToTerrain
        a               rdfs:Datatype ;
        owl:oneOf       ( "entirelyAboveTerrain" "substantiallyAboveTerrain" "substantiallyAboveAndBelowTerrain" "substantiallyBelowTerrain" "entirelyBelowTerrain" ) ;
        skos:prefLabel  "RelativeToTerrain"@en .

core:AbstractSite  a           owl:Class ;
        rdfs:subClassOf        core:AbstractCityObject ;
        iso19150-2:isAbstract  true ;
        skos:definition        "SIG3D: Abstract superclass of buildings,tunnels, bridges and other constructions."@en ;
        skos:prefLabel         "AbstractSite"@en .

core:AbstractCityObject.relativeToWater
        a                owl:ObjectProperty ;
        rdfs:domain      core:AbstractCityObject ;
        rdfs:range       core:RelativeToWater ;
        skos:definition  "SIG3D: Vertical position of the AbstractCityObject relative to a surrounding water surface."@en ;
        skos:prefLabel   "relativeToWater"@en .

core:AbstractCityObject
        a                      owl:Class ;
        iso19150-2:isAbstract  true ;
        skos:definition        "SIG3D: Abstract super class of all thematic classes within CityGML data model."@en ;
        skos:prefLabel         "AbstractCityObject"@en .

core:ExternalReference
        a                owl:Class ;
        skos:definition  "SIG3D: Reference to a corresponding object in another information system, for example in the German cadastre (ALKIS), the German topographic information system (ATKIS), or the OS UK MasterMap?."@en ;
        skos:prefLabel   "ExternalReference"@en .

core:Address.multiPoint
        a               owl:ObjectProperty ;
        rdfs:domain     core:Address ;
        rdfs:range      gsp:Geometry ;
        skos:prefLabel  "multiPoint"@en .

core:TransformationMatrix4x4
        a                owl:Class ;
        skos:definition  "SIG3D: Transformation matrix with 4 rows and columns, used for simultaneously specifying translation, rotation and scaling."@en ;
        skos:prefLabel   "TransformationMatrix4x4"@en .

core:ImplicitGeometry.libraryObject
        a                owl:DatatypeProperty ;
        rdfs:domain      core:ImplicitGeometry ;
        rdfs:range       xsd:anyURI ;
        skos:definition  "SIG3D: External link to a prototype geometry."@en ;
        skos:prefLabel   "libraryObject"@en .

core:DoubleBetween0and1
        a               owl:Class ;
        skos:prefLabel  "DoubleBetween0and1"@en .

core:TransformationMatrix3x4
        a                owl:Class ;
        skos:definition  "SIG3D: 3x4 transformation matrix, (arbitrary rotation and scaling and translation)."@en ;
        skos:prefLabel   "TransformationMatrix3x4"@en .

core:RelativeToWater  a  rdfs:Datatype ;
        owl:oneOf       ( "entirelyAboveWaterSurface" "substantiallyAboveWaterSurface" "substantiallyAboveAndBelowWaterSurface" "substantiallyBelowWaterSurface" "entirelyBelowWaterSurface" "temporarilyAboveAndBelowWaterSurface" ) ;
        skos:prefLabel  "RelativeToWater"@en .

core:ExternalReference.informationSystem
        a                owl:DatatypeProperty ;
        rdfs:domain      core:ExternalReference ;
        rdfs:range       xsd:anyURI ;
        skos:definition  "SIG3D: URL or URN of the information system or data set."@en ;
        skos:prefLabel   "informationSystem"@en .

core:TransformationMatrix2x2.list
        a                owl:ObjectProperty ;
        rdfs:domain      core:TransformationMatrix2x2 ;
        rdfs:range       iso19136:doubleList ;
        skos:definition  "SIG3D: Elements of the matrix in row major order."@en ;
        skos:prefLabel   "list"@en .

core:AbstractCityObject.generalizesTo
        a               owl:ObjectProperty ;
        rdfs:domain     core:AbstractCityObject ;
        rdfs:range      core:AbstractCityObject ;
        skos:prefLabel  "generalizesTo"@en .

core:ImplicitGeometry.transformationMatrix
        a                owl:ObjectProperty ;
        rdfs:domain      core:ImplicitGeometry ;
        rdfs:range       core:TransformationMatrix4x4 ;
        skos:definition  "SIG3D: Mathematical transformation (translation, rotation and scaling) between the prototype geometry and the actual spatial position of the object."@en ;
        skos:prefLabel   "transformationMatrix"@en .

core:DoubleBetween0and1List.list
        a               owl:ObjectProperty ;
        rdfs:domain     core:DoubleBetween0and1List ;
        rdfs:range      iso19136:doubleList ;
        skos:prefLabel  "list"@en .

core:AbstractCityObject.appearance
        a               owl:ObjectProperty ;
        rdfs:domain     core:AbstractCityObject ;
        rdfs:range      core:AbstractAppearance ;
        skos:prefLabel  "appearance"@en .
