@prefix core:  <https://github.com/VCityTeam/UD-Graph/Ontologies/core#> .
@prefix con:   <https://github.com/VCityTeam/UD-Graph/Ontologies/construction#> .
@prefix iso19150-2: <http://def.isotc211.org/iso19150/-2/2012/base#> .
@prefix owl:   <http://www.w3.org/2002/07/owl#> .
@prefix rdf:   <http://www.w3.org/1999/02/22-rdf-syntax-ns#> .
@prefix xsd:   <http://www.w3.org/2001/XMLSchema#> .
@prefix skos:  <http://www.w3.org/2004/02/skos/core#> .
@prefix rdfs:  <http://www.w3.org/2000/01/rdf-schema#> .
@prefix tun:   <https://github.com/VCityTeam/UD-Graph/Ontologies/tunnel#> .

tun:TunnelConstructiveElement
        a                owl:Class ;
        rdfs:subClassOf  con:AbstractConstructiveElement ;
        skos:definition  "A TunnelConstructiveElement is an element of a Tunnel which is essential from a structural point of view. Examples are walls, slabs, beams."@en ;
        skos:prefLabel   "TunnelConstructiveElement"@en .

tun:ADEOfTunnel  a             owl:Class ;
        iso19150-2:isAbstract  true ;
        skos:definition        "ADEOfTunnel acts as a hook to define properties within an ADE that are to be added to a Tunnel."@en ;
        skos:prefLabel         "ADEOfTunnel"@en .

tun:TunnelClassValue  a  owl:Class ;
        rdfs:subClassOf  skos:Concept ;
        skos:definition  "TunnelClassValue is a code list used to further classify a Tunnel."@en ;
        skos:prefLabel   "TunnelClassValue"@en .

tun:HollowSpace.function
        a                owl:ObjectProperty ;
        rdfs:domain      tun:HollowSpace ;
        rdfs:range       tun:HollowSpaceFunctionValue ;
        skos:definition  "Specifies the intended purposes of the HollowSpace."@en ;
        skos:prefLabel   "function"@en .

tun:TunnelConstructiveElement.function
        a                owl:ObjectProperty ;
        rdfs:domain      tun:TunnelConstructiveElement ;
        rdfs:range       tun:TunnelConstructiveElementFunctionValue ;
        skos:definition  "Specifies the intended purposes of the TunnelConstructiveElement."@en ;
        skos:prefLabel   "function"@en .

tun:TunnelConstructiveElement.class
        a                owl:ObjectProperty ;
        rdfs:domain      tun:TunnelConstructiveElement ;
        rdfs:range       tun:TunnelConstructiveElementClassValue ;
        skos:definition  "Indicates the specific type of the TunnelConstructiveElement."@en ;
        skos:prefLabel   "class"@en .

tun:ADEOfTunnelConstructiveElement
        a                      owl:Class ;
        iso19150-2:isAbstract  true ;
        skos:definition        "ADEOfTunnelConstructiveElement acts as a hook to define properties within an ADE that are to be added to a TunnelConstructiveElement."@en ;
        skos:prefLabel         "ADEOfTunnelConstructiveElement"@en .

tun:TunnelFurniture.adeOfTunnelFurniture
        a                owl:ObjectProperty ;
        rdfs:domain      tun:TunnelFurniture ;
        rdfs:range       tun:ADEOfTunnelFurniture ;
        skos:definition  "Augments the TunnelFurniture with properties defined in an ADE."@en ;
        skos:prefLabel   "adeOfTunnelFurniture"@en .

tun:TunnelFurnitureUsageValue
        a                owl:Class ;
        rdfs:subClassOf  skos:Concept ;
        skos:definition  "TunnelFurnitureUsageValue is a code list that enumerates the different uses of a TunnelFurniture."@en ;
        skos:prefLabel   "TunnelFurnitureUsageValue"@en .

tun:TunnelInstallation.usage
        a                owl:ObjectProperty ;
        rdfs:domain      tun:TunnelInstallation ;
        rdfs:range       tun:TunnelInstallationUsageValue ;
        skos:definition  "Specifies the actual uses of the TunnelInstallation."@en ;
        skos:prefLabel   "usage"@en .

tun:AbstractTunnel.tunnelFurniture
        a                owl:ObjectProperty ;
        rdfs:domain      tun:AbstractTunnel ;
        rdfs:range       tun:TunnelFurniture ;
        skos:definition  "Relates the furniture objects to the Tunnel or TunnelPart."@en ;
        skos:prefLabel   "tunnelFurniture"@en .

tun:TunnelInstallation
        a                owl:Class ;
        rdfs:subClassOf  con:AbstractInstallation ;
        skos:definition  "A TunnelInstallation is a permanent part of a Tunnel (inside and/or outside) which does not have the significance of a TunnelPart. In contrast to TunnelConstructiveElement, a TunnelInstallation is not essential from a structural point of view. Examples are stairs, antennas or railings."@en ;
        skos:prefLabel   "TunnelInstallation"@en .

tun:AbstractTunnel.tunnelInstallation
        a                owl:ObjectProperty ;
        rdfs:domain      tun:AbstractTunnel ;
        rdfs:range       tun:TunnelInstallation ;
        skos:definition  "Relates the installation objects to the Tunnel or TunnelPart."@en ;
        skos:prefLabel   "tunnelInstallation"@en .

tun:TunnelUsageValue  a  owl:Class ;
        rdfs:subClassOf  skos:Concept ;
        skos:definition  "TunnelUsageValue is a code list that enumerates the different uses of a Tunnel."@en ;
        skos:prefLabel   "TunnelUsageValue"@en .

tun:AbstractTunnel.class
        a                owl:ObjectProperty ;
        rdfs:domain      tun:AbstractTunnel ;
        rdfs:range       tun:TunnelClassValue ;
        skos:definition  "Indicates the specific type of the Tunnel or TunnelPart."@en ;
        skos:prefLabel   "class"@en .

tun:Tunnel.adeOfTunnel
        a                owl:ObjectProperty ;
        rdfs:domain      tun:Tunnel ;
        rdfs:range       tun:ADEOfTunnel ;
        skos:definition  "Augments the Tunnel with properties defined in an ADE."@en ;
        skos:prefLabel   "adeOfTunnel"@en .

tun:TunnelFurniture  a   owl:Class ;
        rdfs:subClassOf  con:AbstractFurniture ;
        skos:definition  "A TunnelFurniture is an equipment for occupant use, usually not fixed to the tunnel. [cf. ISO 6707-1]"@en ;
        skos:prefLabel   "TunnelFurniture"@en .

tun:TunnelFurnitureFunctionValue
        a                owl:Class ;
        rdfs:subClassOf  skos:Concept ;
        skos:definition  "TunnelFurnitureFunctionValue is a code list that enumerates the different purposes of a TunnelFurniture."@en ;
        skos:prefLabel   "TunnelFurnitureFunctionValue"@en .

tun:ADEOfTunnelInstallation
        a                      owl:Class ;
        iso19150-2:isAbstract  true ;
        skos:definition        "ADEOfTunnelInstallation acts as a hook to define properties within an ADE that are to be added to a TunnelInstallation."@en ;
        skos:prefLabel         "ADEOfTunnelInstallation"@en .

tun:TunnelInstallation.adeOfTunnelInstallation
        a                owl:ObjectProperty ;
        rdfs:domain      tun:TunnelInstallation ;
        rdfs:range       tun:ADEOfTunnelInstallation ;
        skos:definition  "Augments the TunnelInstallation with properties defined in an ADE."@en ;
        skos:prefLabel   "adeOfTunnelInstallation"@en .

tun:AbstractTunnel  a          owl:Class ;
        rdfs:subClassOf        con:AbstractConstruction ;
        iso19150-2:isAbstract  true ;
        skos:definition        "AbstractTunnel is an abstract superclass representing the common attributes and associations of the classes Tunnel and TunnelPart."@en ;
        skos:prefLabel         "AbstractTunnel"@en .

tun:TunnelInstallationClassValue
        a                owl:Class ;
        rdfs:subClassOf  skos:Concept ;
        skos:definition  "TunnelInstallationClassValue is a code list used to further classify a TunnelInstallation."@en ;
        skos:prefLabel   "TunnelInstallationClassValue"@en .

tun:HollowSpace.class
        a                owl:ObjectProperty ;
        rdfs:domain      tun:HollowSpace ;
        rdfs:range       tun:HollowSpaceClassValue ;
        skos:definition  "Indicates the specific type of the HollowSpace."@en ;
        skos:prefLabel   "class"@en .

tun:HollowSpaceClassValue
        a                owl:Class ;
        rdfs:subClassOf  skos:Concept ;
        skos:definition  "HollowSpaceClassValue is a code list used to further classify a HollowSpace."@en ;
        skos:prefLabel   "HollowSpaceClassValue"@en .

tun:ADEOfAbstractTunnel
        a                      owl:Class ;
        iso19150-2:isAbstract  true ;
        skos:definition        "ADEOfAbstractTunnel acts as a hook to define properties within an ADE that are to be added to AbstractTunnel."@en ;
        skos:prefLabel         "ADEOfAbstractTunnel"@en .

tun:TunnelConstructiveElementFunctionValue
        a                owl:Class ;
        rdfs:subClassOf  skos:Concept ;
        skos:definition  "TunnelConstructiveElementFunctionValue is a code list that enumerates the different purposes of a TunnelConstructiveElement."@en ;
        skos:prefLabel   "TunnelConstructiveElementFunctionValue"@en .

tun:TunnelPart.adeOfTunnelPart
        a                owl:ObjectProperty ;
        rdfs:domain      tun:TunnelPart ;
        rdfs:range       tun:ADEOfTunnelPart ;
        skos:definition  "Augments the TunnelPart with properties defined in an ADE."@en ;
        skos:prefLabel   "adeOfTunnelPart"@en .

tun:TunnelConstructiveElementClassValue
        a                owl:Class ;
        rdfs:subClassOf  skos:Concept ;
        skos:definition  "TunnelConstructiveElementClassValue is a code list used to further classify a TunnelConstructiveElement."@en ;
        skos:prefLabel   "TunnelConstructiveElementClassValue"@en .

tun:TunnelConstructiveElement.usage
        a                owl:ObjectProperty ;
        rdfs:domain      tun:TunnelConstructiveElement ;
        rdfs:range       tun:TunnelConstructiveElementUsageValue ;
        skos:definition  "Specifies the actual uses of the TunnelConstructiveElement."@en ;
        skos:prefLabel   "usage"@en .

tun:HollowSpace.adeOfHollowSpace
        a                owl:ObjectProperty ;
        rdfs:domain      tun:HollowSpace ;
        rdfs:range       tun:ADEOfHollowSpace ;
        skos:definition  "Augments the HollowSpace with properties defined in an ADE."@en ;
        skos:prefLabel   "adeOfHollowSpace"@en .

tun:ADEOfTunnelPart  a         owl:Class ;
        iso19150-2:isAbstract  true ;
        skos:definition        "ADEOfTunnelPart acts as a hook to define properties within an ADE that are to be added to a TunnelPart."@en ;
        skos:prefLabel         "ADEOfTunnelPart"@en .

tun:HollowSpace.tunnelInstallation
        a                owl:ObjectProperty ;
        rdfs:domain      tun:HollowSpace ;
        rdfs:range       tun:TunnelInstallation ;
        skos:definition  "Relates the installation objects to the HollowSpace."@en ;
        skos:prefLabel   "tunnelInstallation"@en .

tun:TunnelInstallationUsageValue
        a                owl:Class ;
        rdfs:subClassOf  skos:Concept ;
        skos:definition  "TunnelInstallationUsageValue is a code list that enumerates the different uses of a TunnelInstallation."@en ;
        skos:prefLabel   "TunnelInstallationUsageValue"@en .

tun:TunnelFunctionValue
        a                owl:Class ;
        rdfs:subClassOf  skos:Concept ;
        skos:definition  "TunnelFunctionValue is a code list that enumerates the different purposes of a Tunnel."@en ;
        skos:prefLabel   "TunnelFunctionValue"@en .

tun:AbstractTunnel.usage
        a                owl:ObjectProperty ;
        rdfs:domain      tun:AbstractTunnel ;
        rdfs:range       tun:TunnelUsageValue ;
        skos:definition  "Specifies the actual uses of the Tunnel or TunnelPart."@en ;
        skos:prefLabel   "usage"@en .

<https://github.com/VCityTeam/UD-Graph/Ontologies/tunnel>
        a                owl:Ontology ;
        owl:imports      <https://github.com/VCityTeam/UD-Graph/Ontologies/construction> , <https://github.com/VCityTeam/UD-Graph/Ontologies/core> , <http://def.isotc211.org/iso19150/-2/2012/base> ;
        owl:versionIRI   "https://github.com/VCityTeam/UD-Graph/Ontologies/tunnel/3.0.0" ;
        owl:versionInfo  "3.0.0" ;
        skos:definition  "The Tunnel module supports representation of thematic and spatial aspects of tunnels, tunnel parts, tunnel installations, and interior tunnel structures."@en ;
        skos:prefLabel   "Tunnel"@en .

tun:HollowSpaceUsageValue
        a                owl:Class ;
        rdfs:subClassOf  skos:Concept ;
        skos:definition  "HollowSpaceUsageValue is a code list that enumerates the different uses of a HollowSpace."@en ;
        skos:prefLabel   "HollowSpaceUsageValue"@en .

tun:TunnelFurniture.function
        a                owl:ObjectProperty ;
        rdfs:domain      tun:TunnelFurniture ;
        rdfs:range       tun:TunnelFurnitureFunctionValue ;
        skos:definition  "Specifies the intended purposes of the TunnelFurniture."@en ;
        skos:prefLabel   "function"@en .

tun:Tunnel  a            owl:Class ;
        rdfs:subClassOf  tun:AbstractTunnel ;
        skos:definition  "A Tunnel represents a horizontal or sloping enclosed passage way of a certain length, mainly underground or underwater. [cf. ISO 6707-1]"@en ;
        skos:prefLabel   "Tunnel"@en .

tun:Tunnel.tunnelPart
        a                owl:ObjectProperty ;
        rdfs:domain      tun:Tunnel ;
        rdfs:range       tun:TunnelPart ;
        skos:definition  "Relates the tunnel parts to the Tunnel."@en ;
        skos:prefLabel   "tunnelPart"@en .

tun:TunnelFurniture.class
        a                owl:ObjectProperty ;
        rdfs:domain      tun:TunnelFurniture ;
        rdfs:range       tun:TunnelFurnitureClassValue ;
        skos:definition  "Indicates the specific type of the TunnelFurniture."@en ;
        skos:prefLabel   "class"@en .

tun:ADEOfTunnelFurniture
        a                      owl:Class ;
        iso19150-2:isAbstract  true ;
        skos:definition        "ADEOfTunnelFurniture acts as a hook to define properties within an ADE that are to be added to a TunnelFurniture."@en ;
        skos:prefLabel         "ADEOfTunnelFurniture"@en .

tun:TunnelConstructiveElementUsageValue
        a                owl:Class ;
        rdfs:subClassOf  skos:Concept ;
        skos:definition  "TunnelConstructiveElementUsageValue is a code list that enumerates the different uses of a TunnelConstructiveElement."@en ;
        skos:prefLabel   "TunnelConstructiveElementUsageValue"@en .

tun:TunnelInstallation.function
        a                owl:ObjectProperty ;
        rdfs:domain      tun:TunnelInstallation ;
        rdfs:range       tun:TunnelInstallationFunctionValue ;
        skos:definition  "Specifies the intended purposes of the TunnelInstallation."@en ;
        skos:prefLabel   "function"@en .

tun:HollowSpace.usage
        a                owl:ObjectProperty ;
        rdfs:domain      tun:HollowSpace ;
        rdfs:range       tun:HollowSpaceUsageValue ;
        skos:definition  "Specifies the actual uses of the HollowSpace."@en ;
        skos:prefLabel   "usage"@en .

tun:TunnelPart  a        owl:Class ;
        rdfs:subClassOf  tun:AbstractTunnel ;
        skos:definition  "A TunnelPart is a physical or functional subdivision of a Tunnel. It would be considered a Tunnel, if it were not part of a collection of other TunnelParts."@en ;
        skos:prefLabel   "TunnelPart"@en .

tun:AbstractTunnel.hollowSpace
        a                owl:ObjectProperty ;
        rdfs:domain      tun:AbstractTunnel ;
        rdfs:range       tun:HollowSpace ;
        skos:definition  "Relates the hollow spaces to the Tunnel or TunnelPart."@en ;
        skos:prefLabel   "hollowSpace"@en .

tun:TunnelInstallationFunctionValue
        a                owl:Class ;
        rdfs:subClassOf  skos:Concept ;
        skos:definition  "TunnelInstallationFunctionValue is a code list that enumerates the different purposes of a TunnelInstallation."@en ;
        skos:prefLabel   "TunnelInstallationFunctionValue"@en .

tun:AbstractTunnel.tunnelConstructiveElement
        a                owl:ObjectProperty ;
        rdfs:domain      tun:AbstractTunnel ;
        rdfs:range       tun:TunnelConstructiveElement ;
        skos:definition  "Relates the constructive elements to the Tunnel or TunnelPart."@en ;
        skos:prefLabel   "tunnelConstructiveElement"@en .

tun:HollowSpace.tunnelFurniture
        a                owl:ObjectProperty ;
        rdfs:domain      tun:HollowSpace ;
        rdfs:range       tun:TunnelFurniture ;
        skos:definition  "Relates the furniture objects to the HollowSpace."@en ;
        skos:prefLabel   "tunnelFurniture"@en .

tun:AbstractTunnel.function
        a                owl:ObjectProperty ;
        rdfs:domain      tun:AbstractTunnel ;
        rdfs:range       tun:TunnelFunctionValue ;
        skos:definition  "Specifies the intended purposes of the Tunnel or TunnelPart."@en ;
        skos:prefLabel   "function"@en .

tun:TunnelInstallation.class
        a                owl:ObjectProperty ;
        rdfs:domain      tun:TunnelInstallation ;
        rdfs:range       tun:TunnelInstallationClassValue ;
        skos:definition  "Indicates the specific type of the TunnelInstallation."@en ;
        skos:prefLabel   "class"@en .

tun:HollowSpaceFunctionValue
        a                owl:Class ;
        rdfs:subClassOf  skos:Concept ;
        skos:definition  "HollowSpaceFunctionValue is a code list that enumerates the different purposes of a HollowSpace."@en ;
        skos:prefLabel   "HollowSpaceFunctionValue"@en .

tun:HollowSpace.boundary
        a               owl:ObjectProperty ;
        rdfs:domain     tun:HollowSpace ;
        rdfs:range      core:AbstractThematicSurface ;
        skos:prefLabel  "boundary"@en .

tun:ADEOfHollowSpace  a        owl:Class ;
        iso19150-2:isAbstract  true ;
        skos:definition        "ADEOfHollowSpace acts as a hook to define properties within an ADE that are to be added to a HollowSpace."@en ;
        skos:prefLabel         "ADEOfHollowSpace"@en .

tun:TunnelConstructiveElement.adeOfTunnelConstructiveElement
        a                owl:ObjectProperty ;
        rdfs:domain      tun:TunnelConstructiveElement ;
        rdfs:range       tun:ADEOfTunnelConstructiveElement ;
        skos:definition  "Augments the TunnelConstructiveElement with properties defined in an ADE."@en ;
        skos:prefLabel   "adeOfTunnelConstructiveElement"@en .

tun:HollowSpace  a       owl:Class ;
        rdfs:subClassOf  core:AbstractUnoccupiedSpace ;
        skos:definition  "A HollowSpace is a space within a Tunnel or TunnelPart intended for certain functions (e.g. transport or passage ways, service rooms, emergency shelters). A HollowSpace is bounded physically and/or virtually (e.g. by ClosureSurfaces or GenericSurfaces)."@en ;
        skos:prefLabel   "HollowSpace"@en .

tun:TunnelFurniture.usage
        a                owl:ObjectProperty ;
        rdfs:domain      tun:TunnelFurniture ;
        rdfs:range       tun:TunnelFurnitureUsageValue ;
        skos:definition  "Specifies the actual uses of the TunnelFurniture."@en ;
        skos:prefLabel   "usage"@en .

tun:TunnelFurnitureClassValue
        a                owl:Class ;
        rdfs:subClassOf  skos:Concept ;
        skos:definition  "TunnelFurnitureClassValue is a code list used to further classify a TunnelFurniture."@en ;
        skos:prefLabel   "TunnelFurnitureClassValue"@en .

tun:AbstractTunnel.adeOfAbstractTunnel
        a                owl:ObjectProperty ;
        rdfs:domain      tun:AbstractTunnel ;
        rdfs:range       tun:ADEOfAbstractTunnel ;
        skos:definition  "Augments AbstractTunnel with properties defined in an ADE."@en ;
        skos:prefLabel   "adeOfAbstractTunnel"@en .
