@prefix core:  <https://github.com/VCityTeam/UD-Graph/Ontologies/core#> .
@prefix iso19108: <http://def.isotc211.org/iso19108/2006/TemporalSchema#> .
@prefix iso19150-2: <http://def.isotc211.org/iso19150/-2/2012/base#> .
@prefix owl:   <http://www.w3.org/2002/07/owl#> .
@prefix rdf:   <http://www.w3.org/1999/02/22-rdf-syntax-ns#> .
@prefix gsp:   <http://www.opengis.net/ont/geosparql#> .
@prefix xsd:   <http://www.w3.org/2001/XMLSchema#> .
@prefix dyn:   <https://github.com/VCityTeam/UD-Graph/Ontologies/dynamizer#> .
@prefix skos:  <http://www.w3.org/2004/02/skos/core#> .
@prefix rdfs:  <http://www.w3.org/2000/01/rdf-schema#> .

dyn:TabulatedFileTypeValue
        a                owl:Class ;
        rdfs:subClassOf  skos:Concept ;
        skos:definition  "TabulatedFileTypeValue is a code list used to specify the data format of the referenced external tabulated data file."@en ;
        skos:prefLabel   "TabulatedFileTypeValue"@en .

dyn:GenericTimeseries.adeOfGenericTimeseries
        a                owl:ObjectProperty ;
        rdfs:domain      dyn:GenericTimeseries ;
        rdfs:range       dyn:ADEOfGenericTimeseries ;
        skos:definition  "Augments the GenericTimeseries with properties defined in an ADE."@en ;
        skos:prefLabel   "adeOfGenericTimeseries"@en .

dyn:SensorConnection.sensorLocation
        a                owl:ObjectProperty ;
        rdfs:domain      dyn:SensorConnection ;
        rdfs:range       core:AbstractCityObject ;
        skos:definition  "Relates the sensor to the city object where it is located."@en ;
        skos:prefLabel   "sensorLocation"@en .

dyn:TabulatedFileTimeseries.fieldSeparator
        a                owl:DatatypeProperty ;
        rdfs:domain      dyn:TabulatedFileTimeseries ;
        rdfs:range       xsd:string ;
        skos:definition  "Indicates which symbol is used to separate the individual values in the tabulated file."@en ;
        skos:prefLabel   "fieldSeparator"@en .

dyn:SensorConnection.datastreamID
        a                owl:DatatypeProperty ;
        rdfs:domain      dyn:SensorConnection ;
        rdfs:range       xsd:string ;
        skos:definition  "Specifies the datastream that is retrieved by the SensorConnection."@en ;
        skos:prefLabel   "datastreamID"@en .

dyn:TabulatedFileTimeseries.valueColumnName
        a                owl:DatatypeProperty ;
        rdfs:domain      dyn:TabulatedFileTimeseries ;
        rdfs:range       xsd:string ;
        skos:definition  "Specifies the name of the column that stores the value of the time-value-pair."@en ;
        skos:prefLabel   "valueColumnName"@en .

dyn:GenericTimeseries.valueType
        a                owl:ObjectProperty ;
        rdfs:domain      dyn:GenericTimeseries ;
        rdfs:range       dyn:TimeseriesTypeValue ;
        skos:definition  "Indicates the specific type of all time-value-pairs that are part of the GenericTimeseries."@en ;
        skos:prefLabel   "valueType"@en .

dyn:TimeValuePair.appearanceValue
        a                owl:ObjectProperty ;
        rdfs:domain      dyn:TimeValuePair ;
        rdfs:range       core:AbstractAppearance ;
        skos:definition  "Specifies the \"Appearance\" value of the TimeValuePair."@en ;
        skos:prefLabel   "appearanceValue"@en .

dyn:ADEOfTabulatedFileTimeseries
        a                      owl:Class ;
        iso19150-2:isAbstract  true ;
        skos:definition        "ADEOfTabulatedFileTimeseries acts as a hook to define properties within an ADE that are to be added to a TabulatedFileTimeseries."@en ;
        skos:prefLabel         "ADEOfTabulatedFileTimeseries"@en .

dyn:ADEOfGenericTimeseries
        a                      owl:Class ;
        iso19150-2:isAbstract  true ;
        skos:definition        "ADEOfGenericTimeseries acts as a hook to define properties within an ADE that are to be added to a GenericTimeseries."@en ;
        skos:prefLabel         "ADEOfGenericTimeseries"@en .

dyn:TabulatedFileTimeseries.valueType
        a                owl:ObjectProperty ;
        rdfs:domain      dyn:TabulatedFileTimeseries ;
        rdfs:range       dyn:TimeseriesTypeValue ;
        skos:definition  "Indicates the specific type of the timeseries data."@en ;
        skos:prefLabel   "valueType"@en .

dyn:SensorConnection.connectionType
        a                owl:ObjectProperty ;
        rdfs:domain      dyn:SensorConnection ;
        rdfs:range       dyn:SensorConnectionTypeValue ;
        skos:definition  "Indicates the type of Sensor API to which the SensorConnection refers."@en ;
        skos:prefLabel   "connectionType"@en .

dyn:TimeValuePair.implicitGeometryValue
        a                owl:ObjectProperty ;
        rdfs:domain      dyn:TimeValuePair ;
        rdfs:range       core:ImplicitGeometry ;
        skos:definition  "Specifies the \"ImplicitGeometry\" value of the TimeValuePair."@en ;
        skos:prefLabel   "implicitGeometryValue"@en .

dyn:TabulatedFileTimeseries.numberOfHeaderLines
        a                owl:DatatypeProperty ;
        rdfs:domain      dyn:TabulatedFileTimeseries ;
        rdfs:range       xsd:integer ;
        skos:definition  "Indicates the number of lines at the beginning of the tabulated file that represent headers."@en ;
        skos:prefLabel   "numberOfHeaderLines"@en .

dyn:SensorConnection.mqttTopic
        a                owl:DatatypeProperty ;
        rdfs:domain      dyn:SensorConnection ;
        rdfs:range       xsd:string ;
        skos:definition  "Names the specific datastream that is retrieved by the SensorConnection."@en ;
        skos:prefLabel   "mqttTopic"@en .

dyn:TimeseriesComponent
        a                owl:Class ;
        skos:definition  "TimeseriesComponent represents an element of a CompositeTimeseries."@en ;
        skos:prefLabel   "TimeseriesComponent"@en .

dyn:ADEOfStandardFileTimeseries
        a                      owl:Class ;
        iso19150-2:isAbstract  true ;
        skos:definition        "ADEOfStandardFileTimeseries acts as a hook to define properties within an ADE that are to be added to a StandardFileTimeseries."@en ;
        skos:prefLabel         "ADEOfStandardFileTimeseries"@en .

dyn:TabulatedFileTimeseries.mimeType
        a                owl:ObjectProperty ;
        rdfs:domain      dyn:TabulatedFileTimeseries ;
        rdfs:range       core:MimeTypeValue ;
        skos:definition  "Specifies the MIME type of the external timeseries file."@en ;
        skos:prefLabel   "mimeType"@en .

dyn:TabulatedFileTimeseries.timeColumnNo
        a                owl:DatatypeProperty ;
        rdfs:domain      dyn:TabulatedFileTimeseries ;
        rdfs:range       xsd:integer ;
        skos:definition  "Specifies the number of the column that stores the timestamp of the time-value-pair."@en ;
        skos:prefLabel   "timeColumnNo"@en .

dyn:SensorConnection.uom
        a                owl:DatatypeProperty ;
        rdfs:domain      dyn:SensorConnection ;
        rdfs:range       xsd:string ;
        skos:definition  "Specifies the unit of measurement of the observations."@en ;
        skos:prefLabel   "uom"@en .

dyn:ADEOfDynamizer  a          owl:Class ;
        iso19150-2:isAbstract  true ;
        skos:definition        "ADEOfDynamizer acts as a hook to define properties within an ADE that are to be added to a Dynamizer."@en ;
        skos:prefLabel         "ADEOfDynamizer"@en .

dyn:TimeseriesComponent.repetitions
        a                owl:DatatypeProperty ;
        rdfs:domain      dyn:TimeseriesComponent ;
        rdfs:range       xsd:integer ;
        skos:definition  "Specifies how often the timeseries that is referenced by the TimeseriesComponent should be iterated."@en ;
        skos:prefLabel   "repetitions"@en .

dyn:SensorConnection.linkToObservation
        a                owl:DatatypeProperty ;
        rdfs:domain      dyn:SensorConnection ;
        rdfs:range       xsd:string ;
        skos:definition  "Specifies the complete URL to the observation request."@en ;
        skos:prefLabel   "linkToObservation"@en .

dyn:AbstractTimeseries.firstTimestamp
        a                owl:ObjectProperty ;
        rdfs:domain      dyn:AbstractTimeseries ;
        rdfs:range       iso19108:TM_Position ;
        skos:definition  "Specifies the beginning of the timeseries."@en ;
        skos:prefLabel   "firstTimestamp"@en .

dyn:SensorConnection.baseURL
        a                owl:DatatypeProperty ;
        rdfs:domain      dyn:SensorConnection ;
        rdfs:range       xsd:anyURI ;
        skos:definition  "Specifies the base URL of the Sensor API request."@en ;
        skos:prefLabel   "baseURL"@en .

dyn:StandardFileTimeseries
        a                owl:Class ;
        rdfs:subClassOf  dyn:AbstractAtomicTimeseries ;
        skos:definition  "A StandardFileTimeseries represents time-varying data for a single contiguous time interval. The data is provided in an external file referenced in the StandardFileTimeseries. The data within the external file shall be encoded according to a dedicated format for the representation of timeseries data, for example, the OGC TimeseriesML or OGC Observations & Measurements standard. The data type of the data has to be specified within the external file."@en ;
        skos:prefLabel   "StandardFileTimeseries"@en .

dyn:TabulatedFileTimeseries.decimalSymbol
        a                owl:DatatypeProperty ;
        rdfs:domain      dyn:TabulatedFileTimeseries ;
        rdfs:range       xsd:string ;
        skos:definition  "Indicates which symbol is used to separate the integer part from the fractional part of a decimal number."@en ;
        skos:prefLabel   "decimalSymbol"@en .

dyn:TimeseriesTypeValue
        a                rdfs:Datatype ;
        owl:oneOf        ( "integer" "double" "string" "geometry" "uri" "bool" "implicitGeometry" "appearance" ) ;
        skos:definition  "TimeseriesTypeValue enumerates the possible value types for GenericTimeseries and TimeValuePair."@en ;
        skos:prefLabel   "TimeseriesTypeValue"@en .

dyn:CompositeTimeseries
        a                owl:Class ;
        rdfs:subClassOf  dyn:AbstractTimeseries ;
        skos:definition  "A CompositeTimeseries is a (possibly recursive) aggregation of atomic and composite timeseries. The components of a composite timeseries must have non-overlapping time intervals."@en ;
        skos:prefLabel   "CompositeTimeseries"@en .

dyn:ADEOfCompositeTimeseries
        a                      owl:Class ;
        iso19150-2:isAbstract  true ;
        skos:definition        "ADEOfCompositeTimeseries acts as a hook to define properties within an ADE that are to be added to a CompositeTimeseries."@en ;
        skos:prefLabel         "ADEOfCompositeTimeseries"@en .

dyn:TabulatedFileTimeseries.idValue
        a                owl:DatatypeProperty ;
        rdfs:domain      dyn:TabulatedFileTimeseries ;
        rdfs:range       xsd:string ;
        skos:definition  "Specifies the value of the identifier for which the time-value-pairs are to be selected."@en ;
        skos:prefLabel   "idValue"@en .

dyn:TimeValuePair  a     owl:Class ;
        skos:definition  "A TimeValuePair represents a value that is valid for a given timepoint. For each TimeValuePair only one of the value properties can be used mutually exclusive. Which value property has to be provided depends on the selected value type in the GenericTimeSeries feature, in which the TimeValuePair is included."@en ;
        skos:prefLabel   "TimeValuePair"@en .

dyn:SensorConnection  a  owl:Class ;
        skos:definition  "A SensorConnection provides all details that are required to retrieve a specific datastream from an external sensor web service. It comprises the service type (e.g. OGC SensorThings API, OGC Sensor Observation Services, MQTT, proprietary platforms), the URL of the sensor service, the identifier for the sensor or thing and its observed property as well as information about the required authentication method."@en ;
        skos:prefLabel   "SensorConnection"@en .

dyn:ADEOfAbstractTimeseries
        a                      owl:Class ;
        iso19150-2:isAbstract  true ;
        skos:definition        "ADEOfAbstractTimeseries acts as a hook to define properties within an ADE that are to be added to AbstractTimeseries."@en ;
        skos:prefLabel         "ADEOfAbstractTimeseries"@en .

dyn:TabulatedFileTimeseries.valueColumnNo
        a                owl:DatatypeProperty ;
        rdfs:domain      dyn:TabulatedFileTimeseries ;
        rdfs:range       xsd:integer ;
        skos:definition  "Specifies the number of the column that stores the value of the time-value-pair."@en ;
        skos:prefLabel   "valueColumnNo"@en .

dyn:StandardFileTimeseries.mimeType
        a                owl:ObjectProperty ;
        rdfs:domain      dyn:StandardFileTimeseries ;
        rdfs:range       core:MimeTypeValue ;
        skos:definition  "Specifies the MIME type of the external timeseries file."@en ;
        skos:prefLabel   "mimeType"@en .

dyn:CompositeTimeseries.adeOfCompositeTimeseries
        a                owl:ObjectProperty ;
        rdfs:domain      dyn:CompositeTimeseries ;
        rdfs:range       dyn:ADEOfCompositeTimeseries ;
        skos:definition  "Augments the CompositeTimeseries with properties defined in an ADE."@en ;
        skos:prefLabel   "adeOfCompositeTimeseries"@en .

dyn:TimeValuePair.doubleValue
        a                owl:DatatypeProperty ;
        rdfs:domain      dyn:TimeValuePair ;
        rdfs:range       xsd:double ;
        skos:definition  "Specifies the \"Double\" value of the TimeValuePair."@en ;
        skos:prefLabel   "doubleValue"@en .

dyn:TabulatedFileTimeseries.timeColumnName
        a                owl:DatatypeProperty ;
        rdfs:domain      dyn:TabulatedFileTimeseries ;
        rdfs:range       xsd:string ;
        skos:definition  "Specifies the name of the column that stores the timestamp of the time-value-pair."@en ;
        skos:prefLabel   "timeColumnName"@en .

dyn:Dynamizer.dynamicData
        a                owl:ObjectProperty ;
        rdfs:domain      dyn:Dynamizer ;
        rdfs:range       dyn:AbstractTimeseries ;
        skos:definition  "Relates to the timeseries data that is given either inline within a CityGML dataset or by a link to an external file containing timeseries data."@en ;
        skos:prefLabel   "dynamicData"@en .

dyn:SensorConnectionTypeValue
        a                owl:Class ;
        rdfs:subClassOf  skos:Concept ;
        skos:definition  "SensorConnectionTypeValue is a code list used to specify the type of the referenced sensor service. Each value shall provide enough information such that a software application would be able to identify the API type and version."@en ;
        skos:prefLabel   "SensorConnectionTypeValue"@en .

dyn:AbstractTimeseries
        a                      owl:Class ;
        rdfs:subClassOf        core:AbstractFeature ;
        iso19150-2:isAbstract  true ;
        skos:definition        "AbstractTimeseries is the abstract superclass representing any type of timeseries data."@en ;
        skos:prefLabel         "AbstractTimeseries"@en .

dyn:TimeValuePair.intValue
        a                owl:DatatypeProperty ;
        rdfs:domain      dyn:TimeValuePair ;
        rdfs:range       xsd:integer ;
        skos:definition  "Specifies the \"Integer\" value of the TimeValuePair."@en ;
        skos:prefLabel   "intValue"@en .

dyn:TabulatedFileTimeseries.fileType
        a                owl:ObjectProperty ;
        rdfs:domain      dyn:TabulatedFileTimeseries ;
        rdfs:range       dyn:TabulatedFileTypeValue ;
        skos:definition  "Specifies the format used to represent the timeseries data."@en ;
        skos:prefLabel   "fileType"@en .

dyn:AbstractAtomicTimeseries.uom
        a                owl:DatatypeProperty ;
        rdfs:domain      dyn:AbstractAtomicTimeseries ;
        rdfs:range       xsd:string ;
        skos:definition  "Specifies the unit of measurement of the observation values."@en ;
        skos:prefLabel   "uom"@en .

dyn:StandardFileTimeseries.fileLocation
        a                owl:DatatypeProperty ;
        rdfs:domain      dyn:StandardFileTimeseries ;
        rdfs:range       xsd:anyURI ;
        skos:definition  "Specifies the URI that points to the external timeseries file."@en ;
        skos:prefLabel   "fileLocation"@en .

dyn:TabulatedFileTimeseries.fileLocation
        a                owl:DatatypeProperty ;
        rdfs:domain      dyn:TabulatedFileTimeseries ;
        rdfs:range       xsd:anyURI ;
        skos:definition  "Specifies the URI that points to the external timeseries file."@en ;
        skos:prefLabel   "fileLocation"@en .

dyn:Dynamizer  a         owl:Class ;
        rdfs:subClassOf  core:AbstractDynamizer ;
        skos:definition  "A Dynamizer is an object that injects timeseries data for an individual attribute of the city object in which it is included. The timeseries data overrides the static value of the referenced city object attribute in order to represent dynamic, i.e. time-dependent, variations of its value."@en ;
        skos:prefLabel   "Dynamizer"@en .

dyn:TabulatedFileTimeseries.idColumnName
        a                owl:DatatypeProperty ;
        rdfs:domain      dyn:TabulatedFileTimeseries ;
        rdfs:range       xsd:string ;
        skos:definition  "Specifies the name of the column that stores the identifier of the time-value-pair."@en ;
        skos:prefLabel   "idColumnName"@en .

dyn:TimeseriesComponent.timeseries
        a                owl:ObjectProperty ;
        rdfs:domain      dyn:TimeseriesComponent ;
        rdfs:range       dyn:AbstractTimeseries ;
        skos:definition  "Relates a timeseries to the TimeseriesComponent."@en ;
        skos:prefLabel   "timeseries"@en .

dyn:AuthenticationTypeValue
        a                owl:Class ;
        rdfs:subClassOf  skos:Concept ;
        skos:definition  "AuthenticationTypeValue is a code list used to specify the authentication method to be used to access the referenced sensor service. Each value shall provide enough information such that a software application could determine the required access credentials."@en ;
        skos:prefLabel   "AuthenticationTypeValue"@en .

dyn:AbstractAtomicTimeseries.observationProperty
        a                owl:DatatypeProperty ;
        rdfs:domain      dyn:AbstractAtomicTimeseries ;
        rdfs:range       xsd:string ;
        skos:definition  "Specifies the phenomenon for which the atomic timeseries provides observation values."@en ;
        skos:prefLabel   "observationProperty"@en .

dyn:ADEOfAbstractAtomicTimeseries
        a                      owl:Class ;
        iso19150-2:isAbstract  true ;
        skos:definition        "ADEOfAbstractAtomicTimeseries acts as a hook to define properties within an ADE that are to be added to AbstractAtomicTimeseries."@en ;
        skos:prefLabel         "ADEOfAbstractAtomicTimeseries"@en .

dyn:TimeValuePair.stringValue
        a                owl:DatatypeProperty ;
        rdfs:domain      dyn:TimeValuePair ;
        rdfs:range       xsd:string ;
        skos:definition  "Specifies the \"String\" value of the TimeValuePair."@en ;
        skos:prefLabel   "stringValue"@en .

dyn:StandardFileTimeseries.fileType
        a                owl:ObjectProperty ;
        rdfs:domain      dyn:StandardFileTimeseries ;
        rdfs:range       dyn:StandardFileTypeValue ;
        skos:definition  "Specifies the format used to represent the timeseries data."@en ;
        skos:prefLabel   "fileType"@en .

dyn:SensorConnection.sensorName
        a                owl:DatatypeProperty ;
        rdfs:domain      dyn:SensorConnection ;
        rdfs:range       xsd:string ;
        skos:definition  "Specifies the name of the sensor from which the SensorConnection retrieves observations."@en ;
        skos:prefLabel   "sensorName"@en .

dyn:SensorConnection.authType
        a                owl:ObjectProperty ;
        rdfs:domain      dyn:SensorConnection ;
        rdfs:range       dyn:AuthenticationTypeValue ;
        skos:definition  "Specifies the type of authentication required to be able to access the Sensor API."@en ;
        skos:prefLabel   "authType"@en .

dyn:Dynamizer.adeOfDynamizer
        a                owl:ObjectProperty ;
        rdfs:domain      dyn:Dynamizer ;
        rdfs:range       dyn:ADEOfDynamizer ;
        skos:definition  "Augments the Dynamizer with properties defined in an ADE."@en ;
        skos:prefLabel   "adeOfDynamizer"@en .

dyn:AbstractTimeseries.adeOfAbstractTimeseries
        a                owl:ObjectProperty ;
        rdfs:domain      dyn:AbstractTimeseries ;
        rdfs:range       dyn:ADEOfAbstractTimeseries ;
        skos:definition  "Augments AbstractTimeseries with properties defined in an ADE."@en ;
        skos:prefLabel   "adeOfAbstractTimeseries"@en .

dyn:Dynamizer.sensorConnection
        a                owl:ObjectProperty ;
        rdfs:domain      dyn:Dynamizer ;
        rdfs:range       dyn:SensorConnection ;
        skos:definition  "Relates to the sensor API that delivers timeseries data."@en ;
        skos:prefLabel   "sensorConnection"@en .

dyn:AbstractAtomicTimeseries
        a                      owl:Class ;
        rdfs:subClassOf        dyn:AbstractTimeseries ;
        iso19150-2:isAbstract  true ;
        skos:definition        "AbstractAtomicTimeseries represents the attributes and relationships that are common to all kinds of atomic timeseries (GenericTimeseries, TabulatedFileTimeseries, StandardFileTimeseries). An atomic timeseries represents time-varying data of a specific data type for a single contiguous time interval."@en ;
        skos:prefLabel         "AbstractAtomicTimeseries"@en .

dyn:SensorConnection.observationID
        a                owl:DatatypeProperty ;
        rdfs:domain      dyn:SensorConnection ;
        rdfs:range       xsd:string ;
        skos:definition  "Specifies the unique identifier of the observation that is retrieved by the SensorConnection."@en ;
        skos:prefLabel   "observationID"@en .

dyn:Dynamizer.attributeRef
        a                owl:DatatypeProperty ;
        rdfs:domain      dyn:Dynamizer ;
        rdfs:range       xsd:string ;
        skos:definition  "Specifies the attribute of a CityGML feature whose value is overridden or replaced by the (dynamic) values specified by the Dynamizer."@en ;
        skos:prefLabel   "attributeRef"@en .

dyn:TimeValuePair.geometryValue
        a                owl:ObjectProperty ;
        rdfs:domain      dyn:TimeValuePair ;
        rdfs:range       gsp:Geometry ;
        skos:definition  "Specifies the geometry value of the TimeValuePair."@en ;
        skos:prefLabel   "geometryValue"@en .

dyn:TimeValuePair.boolValue
        a                owl:DatatypeProperty ;
        rdfs:domain      dyn:TimeValuePair ;
        rdfs:range       xsd:boolean ;
        skos:definition  "Specifies the \"Boolean\" value of the TimeValuePair."@en ;
        skos:prefLabel   "boolValue"@en .

dyn:Dynamizer.startTime
        a                owl:ObjectProperty ;
        rdfs:domain      dyn:Dynamizer ;
        rdfs:range       iso19108:TM_Position ;
        skos:definition  "Specifies the beginning of the time span for which the Dynamizer provides dynamic values."@en ;
        skos:prefLabel   "startTime"@en .

dyn:TabulatedFileTimeseries
        a                owl:Class ;
        rdfs:subClassOf  dyn:AbstractAtomicTimeseries ;
        skos:definition  "A TabulatedFileTimeseries represents time-varying data of a specific data type for a single contiguous time interval. The data is provided in an external file referenced in the TabulatedFileTimeseries. The file shall contain table structured data using an appropriate file format like comma separated values (CSV), Microsoft Excel (XLSX) or Google Spreadsheet. The timestamps and the values are given in specific columns of the table. Each row represents a single time-value-pair. A subset of rows can be selected using the idColumn and idValue attributes."@en ;
        skos:prefLabel   "TabulatedFileTimeseries"@en .

dyn:StandardFileTypeValue
        a                owl:Class ;
        rdfs:subClassOf  skos:Concept ;
        skos:definition  "StandardFileTypeValue is a code list used to specify the type of the referenced external timeseries data file. Each value shall provide information about the standard and version."@en ;
        skos:prefLabel   "StandardFileTypeValue"@en .

dyn:SensorConnection.linkToSensorDescription
        a                owl:DatatypeProperty ;
        rdfs:domain      dyn:SensorConnection ;
        rdfs:range       xsd:string ;
        skos:definition  "Specifies the complete URL to the sensor description request."@en ;
        skos:prefLabel   "linkToSensorDescription"@en .

dyn:StandardFileTimeseries.adeOfStandardFileTimeseries
        a                owl:ObjectProperty ;
        rdfs:domain      dyn:StandardFileTimeseries ;
        rdfs:range       dyn:ADEOfStandardFileTimeseries ;
        skos:definition  "Augments the StandardFileTimeseries with properties defined in an ADE."@en ;
        skos:prefLabel   "adeOfStandardFileTimeseries"@en .

dyn:TabulatedFileTimeseries.idColumnNo
        a                owl:DatatypeProperty ;
        rdfs:domain      dyn:TabulatedFileTimeseries ;
        rdfs:range       xsd:integer ;
        skos:definition  "Specifies the number of the column that stores the identifier of the time-value-pair."@en ;
        skos:prefLabel   "idColumnNo"@en .

dyn:TimeValuePair.timestamp
        a                owl:ObjectProperty ;
        rdfs:domain      dyn:TimeValuePair ;
        rdfs:range       iso19108:TM_Position ;
        skos:definition  "Specifies the timepoint at which the value of the TimeValuePair is valid."@en ;
        skos:prefLabel   "timestamp"@en .

dyn:TimeseriesComponent.additionalGap
        a                owl:ObjectProperty ;
        rdfs:domain      dyn:TimeseriesComponent ;
        rdfs:range       iso19108:TM_Duration ;
        skos:definition  "Specifies how much extra time is added after all repetitions as an additional gap."@en ;
        skos:prefLabel   "additionalGap"@en .

dyn:SensorConnection.mqttServer
        a                owl:DatatypeProperty ;
        rdfs:domain      dyn:SensorConnection ;
        rdfs:range       xsd:string ;
        skos:definition  "Specifies the name of the MQTT Server. This attribute is relevant when the MQTT Protocol is used to connect to a Sensor API."@en ;
        skos:prefLabel   "mqttServer"@en .

dyn:GenericTimeseries.timeValuePair
        a                owl:ObjectProperty ;
        rdfs:domain      dyn:GenericTimeseries ;
        rdfs:range       dyn:TimeValuePair ;
        skos:definition  "Relates to the time-value-pairs that are part of the GenericTimeseries."@en ;
        skos:prefLabel   "timeValuePair"@en .

dyn:SensorConnection.sensorID
        a                owl:DatatypeProperty ;
        rdfs:domain      dyn:SensorConnection ;
        rdfs:range       xsd:string ;
        skos:definition  "Specifies the unique identifier of the sensor from which the SensorConnection retrieves observations."@en ;
        skos:prefLabel   "sensorID"@en .

dyn:SensorConnection.observationProperty
        a                owl:DatatypeProperty ;
        rdfs:domain      dyn:SensorConnection ;
        rdfs:range       xsd:string ;
        skos:definition  "Specifies the phenomenon for which the SensorConnection provides observations."@en ;
        skos:prefLabel   "observationProperty"@en .

dyn:AbstractTimeseries.lastTimestamp
        a                owl:ObjectProperty ;
        rdfs:domain      dyn:AbstractTimeseries ;
        rdfs:range       iso19108:TM_Position ;
        skos:definition  "Specifies the end of the timeseries."@en ;
        skos:prefLabel   "lastTimestamp"@en .

dyn:CompositeTimeseries.component
        a                owl:ObjectProperty ;
        rdfs:domain      dyn:CompositeTimeseries ;
        rdfs:range       dyn:TimeseriesComponent ;
        skos:definition  "Relates to the atomic and composite timeseries that are part of the CompositeTimeseries. The referenced timeseries are sequentially ordered."@en ;
        skos:prefLabel   "component"@en .

<https://github.com/VCityTeam/UD-Graph/Ontologies/dynamizer>
        a                owl:Ontology ;
        owl:imports      <http://www.opengis.net/ont/geosparql> , <https://github.com/VCityTeam/UD-Graph/Ontologies/core> , <http://def.isotc211.org/iso19150/-2/2012/base> ;
        owl:versionIRI   "https://github.com/VCityTeam/UD-Graph/Ontologies/dynamizer/3.0.0" ;
        owl:versionInfo  "3.0.0" ;
        skos:definition  "The Dynamizer module supports the injection of timeseries data for individual attributes of CityGML features. Timeseries data can either be retrieved from external Sensor APIs (e.g. OGC SensorThings API, OGC Sensor Observation Services, MQTT, proprietary platforms), external standardized timeseries files (e.g. OGC TimeseriesML or OGC Observations & Measurements), external tabulated files (e.g CSV) or can be represented inline as basic time-value pairs."@en ;
        skos:prefLabel   "Dynamizer"@en .

dyn:GenericTimeseries
        a                owl:Class ;
        rdfs:subClassOf  dyn:AbstractAtomicTimeseries ;
        skos:definition  "A GenericTimeseries represents time-varying data in the form of embedded time-value-pairs of a specific data type for a single contiguous time interval."@en ;
        skos:prefLabel   "GenericTimeseries"@en .

dyn:TabulatedFileTimeseries.adeOfTabulatedFileTimeseries
        a                owl:ObjectProperty ;
        rdfs:domain      dyn:TabulatedFileTimeseries ;
        rdfs:range       dyn:ADEOfTabulatedFileTimeseries ;
        skos:definition  "Augments the TabulatedFileTimeseries with properties defined in an ADE."@en ;
        skos:prefLabel   "adeOfTabulatedFileTimeseries"@en .

dyn:TimeValuePair.uriValue
        a                owl:DatatypeProperty ;
        rdfs:domain      dyn:TimeValuePair ;
        rdfs:range       xsd:anyURI ;
        skos:definition  "Specifies the \"URI\" value of the TimeValuePair."@en ;
        skos:prefLabel   "uriValue"@en .

dyn:AbstractAtomicTimeseries.adeOfAbstractAtomicTimeseries
        a                owl:ObjectProperty ;
        rdfs:domain      dyn:AbstractAtomicTimeseries ;
        rdfs:range       dyn:ADEOfAbstractAtomicTimeseries ;
        skos:definition  "Augments AbstractAtomicTimeseries with properties defined in an ADE."@en ;
        skos:prefLabel   "adeOfAbstractAtomicTimeseries"@en .

dyn:Dynamizer.endTime
        a                owl:ObjectProperty ;
        rdfs:domain      dyn:Dynamizer ;
        rdfs:range       iso19108:TM_Position ;
        skos:definition  "Specifies the end of the time span for which the Dynamizer provides dynamic values."@en ;
        skos:prefLabel   "endTime"@en .
