@prefix core:  <https://github.com/VCityTeam/UD-Graph/Ontologies/core#> .
@prefix grp:   <https://github.com/VCityTeam/UD-Graph/Ontologies/cityobjectgroup#> .
@prefix iso19150-2: <http://def.isotc211.org/iso19150/-2/2012/base#> .
@prefix owl:   <http://www.w3.org/2002/07/owl#> .
@prefix rdf:   <http://www.w3.org/1999/02/22-rdf-syntax-ns#> .
@prefix gsp:   <http://www.opengis.net/ont/geosparql#> .
@prefix xsd:   <http://www.w3.org/2001/XMLSchema#> .
@prefix iso19136: <http://def.isotc211.org/iso19136/2007/GML> .
@prefix skos:  <http://www.w3.org/2004/02/skos/core#> .
@prefix rdfs:  <http://www.w3.org/2000/01/rdf-schema#> .

grp:CityObjectGroup.usage
        a                owl:ObjectProperty ;
        rdfs:domain      grp:CityObjectGroup ;
        rdfs:range       iso19136:Code ;
        skos:definition  "SIG3D: Usage of the aggregation as given by the relevant national regulations, information communities, or specific applications."@en ;
        skos:prefLabel   "usage"@en .

grp:Role.groupMember  a  owl:ObjectProperty ;
        rdfs:domain      grp:Role ;
        rdfs:range       core:AbstractCityObject ;
        skos:definition  "SIG3D: Reference to a city object."@en ;
        skos:prefLabel   "groupMember"@en .

grp:CityObjectGroup.groupMember
        a               owl:ObjectProperty ;
        rdfs:domain     grp:CityObjectGroup ;
        rdfs:range      grp:Role ;
        skos:prefLabel  "groupMember"@en .

grp:CityObjectGroup.function
        a                owl:ObjectProperty ;
        rdfs:domain      grp:CityObjectGroup ;
        rdfs:range       iso19136:Code ;
        skos:definition  "SIG3D: Specific semantic meaning of the aggregation. Function of the aggregation as given by the relevant national regulations, information communities, or specific applications."@en ;
        skos:prefLabel   "function"@en .

grp:Role.role  a         owl:DatatypeProperty ;
        rdfs:domain      grp:Role ;
        rdfs:range       xsd:string ;
        skos:definition  "SIG3D: Description of the role."@en ;
        skos:prefLabel   "role"@en .

grp:CityObjectGroup.class
        a                owl:ObjectProperty ;
        rdfs:domain      grp:CityObjectGroup ;
        rdfs:range       iso19136:Code ;
        skos:definition  "SIG3D: General semantical meaning of the aggregation. Classification of the aggregation as given by the relevant national regulations, information communities, or specific applications."@en ;
        skos:prefLabel   "class"@en .

grp:Role  a              owl:Class ;
        skos:definition  "SIG3D: Specification of a CityObject and its specific role in a CityObjectGroup."@en ;
        skos:prefLabel   "Role"@en .

grp:CityObjectGroup.geometry
        a                owl:ObjectProperty ;
        rdfs:domain      grp:CityObjectGroup ;
        rdfs:range       gsp:Geometry ;
        skos:definition  "SIG3D: Specific geometry assigned to the aggregation (e. g. the floor surface of a building storey represented by an aggregation of rooms)."@en ;
        skos:prefLabel   "geometry"@en .

<https://github.com/VCityTeam/UD-Graph/Ontologies/cityobjectgroup>
        a                owl:Ontology ;
        owl:imports      <http://www.opengis.net/ont/geosparql> , <https://github.com/VCityTeam/UD-Graph/Ontologies/core> , <http://def.isotc211.org/iso19150/-2/2012/base> ;
        owl:versionIRI   "https://github.com/VCityTeam/UD-Graph/Ontologies/cityobjectgroup/1.0" ;
        owl:versionInfo  "1.0" ;
        skos:prefLabel   "CityObjectGroup"@en .

grp:CityObjectGroup.parent
        a                owl:ObjectProperty ;
        rdfs:domain      grp:CityObjectGroup ;
        rdfs:range       core:AbstractCityObject ;
        skos:definition  "SIG3D: Reference to an AbstractCityObject related to the aggregation as a whole (e.g. the corresponding building object for the aggregation of rooms to a storey)."@en ;
        skos:prefLabel   "parent"@en .

grp:CityObjectGroup  a   owl:Class ;
        rdfs:subClassOf  core:AbstractCityObject ;
        skos:definition  "SIG3D: Aggregation of city objects according to user defined criteria (e.g. grouping of rooms belonging to a certain storey)."@en ;
        skos:prefLabel   "CityObjectGroup"@en .
