<rdf:RDF xmlns:math="http://www.w3.org/2005/xpath-functions/math" xmlns:owl="http://www.w3.org/2002/07/owl#" xmlns:rdf="http://www.w3.org/1999/02/22-rdf-syntax-ns#" xmlns:rdfs="http://www.w3.org/2000/01/rdf-schema#" xmlns:xs="http://www.w3.org/2001/XMLSchema" xmlns:xsd="http://www.w3.org/2001/XMLSchema">
   <owl:Ontology rdf:about="http://liris.cnrs.fr/ontologies/cityGMLBase">
      <owl:imports rdf:resource="http://liris.cnrs.fr/ontologies/gml"/>
      <owl:imports rdf:resource="http://liris.cnrs.fr/ontologies/xAL"/>
      <rdfs:comment>
    CityGML is an OGC Standard.
    Copyright (c) 2012 Open Geospatial Consortium.
    To obtain additional rights of use, visit http://www.opengeospatial.org/legal/ .
		</rdfs:comment>
   </owl:Ontology>
   <owl:Class rdf:about="http://www.opengis.net/citygml/2.0#CityModelType">
      <rdfs:comment>Type describing the "root" element of any city model file. It is a collection whose members are restricted
				to be features of a city model. All features are included as cityObjectMember. </rdfs:comment>
      <rdfs:subClassOf>
         <owl:Class>
            <owl:intersectionOf rdf:parseType="Collection">
               <owl:Restriction>
                  <owl:onProperty rdf:resource="http://www.opengis.net/citygml/2.0#has_GenericApplicationPropertyOfCityModel"/>
                  <owl:allValuesFrom rdf:resource="http://www.opengis.net/citygml/2.0#_GenericApplicationPropertyOfCityModel"/>
               </owl:Restriction>
               <owl:Restriction>
                  <owl:onProperty rdf:resource="http://www.opengis.net/citygml/2.0#has_GenericApplicationPropertyOfCityModel"/>
                  <owl:minCardinality rdf:datatype="http://www.w3.org/2001/XMLSchema#nonNegativeInteger">0</owl:minCardinality>
               </owl:Restriction>
            </owl:intersectionOf>
         </owl:Class>
      </rdfs:subClassOf>
      <rdfs:subClassOf rdf:resource="http://www.opengis.net/gml#AbstractFeatureCollectionType"/>
      <rdfs:comment>Warning: The parent class 'gml:AbstractFeatureCollectionType' is declared outside of this class' original schema. This class may be declared incorrectly.</rdfs:comment>
   </owl:Class>
   <owl:Class rdf:about="http://www.opengis.net/citygml/2.0#AbstractCityObjectType">
      <rdfs:comment>This is an abstract class</rdfs:comment>
      <rdfs:comment>Type describing the abstract superclass of most CityGML features. Its purpose is to provide a creation and
				a termination date as well as a reference to corresponding objects in other information systems. A generalization relation
				may be used to relate features, which represent the same real-world object in different Levels-of-Detail, i.e. a feature
				and its generalized counterpart(s). The direction of this relation is from the feature to the corresponding generalized
				feature.</rdfs:comment>
      <rdfs:subClassOf>
         <owl:Class>
            <owl:intersectionOf rdf:parseType="Collection">
               <owl:Restriction>
                  <owl:onProperty rdf:resource="http://www.opengis.net/citygml/2.0#creationDate"/>
                  <owl:allValuesFrom rdf:resource="http://www.w3.org/2001/XMLSchema#date"/>
               </owl:Restriction>
               <owl:Restriction>
                  <owl:onProperty rdf:resource="http://www.opengis.net/citygml/2.0#creationDate"/>
                  <owl:minCardinality rdf:datatype="http://www.w3.org/2001/XMLSchema#nonNegativeInteger">0</owl:minCardinality>
               </owl:Restriction>
               <owl:Restriction>
                  <owl:onProperty rdf:resource="http://www.opengis.net/citygml/2.0#terminationDate"/>
                  <owl:allValuesFrom rdf:resource="http://www.w3.org/2001/XMLSchema#date"/>
               </owl:Restriction>
               <owl:Restriction>
                  <owl:onProperty rdf:resource="http://www.opengis.net/citygml/2.0#terminationDate"/>
                  <owl:minCardinality rdf:datatype="http://www.w3.org/2001/XMLSchema#nonNegativeInteger">0</owl:minCardinality>
               </owl:Restriction>
               <owl:Restriction>
                  <owl:onProperty rdf:resource="http://www.opengis.net/citygml/2.0#externalReference"/>
                  <owl:allValuesFrom rdf:resource="http://www.opengis.net/citygml/2.0#ExternalReferenceType"/>
               </owl:Restriction>
               <owl:Restriction>
                  <owl:onProperty rdf:resource="http://www.opengis.net/citygml/2.0#externalReference"/>
                  <owl:minCardinality rdf:datatype="http://www.w3.org/2001/XMLSchema#nonNegativeInteger">0</owl:minCardinality>
               </owl:Restriction>
               <owl:Restriction>
                  <owl:onProperty rdf:resource="http://www.opengis.net/citygml/2.0#generalizesTo"/>
                  <owl:allValuesFrom rdf:resource="http://www.opengis.net/citygml/2.0#GeneralizationRelationType"/>
               </owl:Restriction>
               <owl:Restriction>
                  <owl:onProperty rdf:resource="http://www.opengis.net/citygml/2.0#generalizesTo"/>
                  <owl:minCardinality rdf:datatype="http://www.w3.org/2001/XMLSchema#nonNegativeInteger">0</owl:minCardinality>
               </owl:Restriction>
               <owl:Restriction>
                  <owl:onProperty rdf:resource="http://www.opengis.net/citygml/2.0#relativeToTerrain"/>
                  <owl:allValuesFrom rdf:resource="http://www.opengis.net/citygml/2.0#RelativeToTerrainType"/>
               </owl:Restriction>
               <owl:Restriction>
                  <owl:onProperty rdf:resource="http://www.opengis.net/citygml/2.0#relativeToTerrain"/>
                  <owl:minCardinality rdf:datatype="http://www.w3.org/2001/XMLSchema#nonNegativeInteger">0</owl:minCardinality>
               </owl:Restriction>
               <owl:Restriction>
                  <owl:onProperty rdf:resource="http://www.opengis.net/citygml/2.0#relativeToWater"/>
                  <owl:allValuesFrom rdf:resource="http://www.opengis.net/citygml/2.0#RelativeToWaterType"/>
               </owl:Restriction>
               <owl:Restriction>
                  <owl:onProperty rdf:resource="http://www.opengis.net/citygml/2.0#relativeToWater"/>
                  <owl:minCardinality rdf:datatype="http://www.w3.org/2001/XMLSchema#nonNegativeInteger">0</owl:minCardinality>
               </owl:Restriction>
               <owl:Restriction>
                  <owl:onProperty rdf:resource="http://www.opengis.net/citygml/2.0#has_GenericApplicationPropertyOfCityObject"/>
                  <owl:allValuesFrom rdf:resource="http://www.opengis.net/citygml/2.0#_GenericApplicationPropertyOfCityObject"/>
               </owl:Restriction>
               <owl:Restriction>
                  <owl:onProperty rdf:resource="http://www.opengis.net/citygml/2.0#has_GenericApplicationPropertyOfCityObject"/>
                  <owl:minCardinality rdf:datatype="http://www.w3.org/2001/XMLSchema#nonNegativeInteger">0</owl:minCardinality>
               </owl:Restriction>
            </owl:intersectionOf>
         </owl:Class>
      </rdfs:subClassOf>
      <rdfs:subClassOf rdf:resource="http://www.opengis.net/gml#AbstractFeatureType"/>
      <rdfs:comment>Warning: The parent class 'gml:AbstractFeatureType' is declared outside of this class' original schema. This class may be declared incorrectly.</rdfs:comment>
   </owl:Class>
   <owl:Class rdf:about="http://www.opengis.net/citygml/2.0#AbstractSiteType">
      <rdfs:comment>This is an abstract class</rdfs:comment>
      <rdfs:comment>Type describing the abstract superclass for buildings, facilities, etc. Future extensions of CityGML like
				bridges and tunnels would be modelled as subclasses of _Site. As subclass of _CityObject, a _Site inherits all attributes
				and relations, in particular an id, names, external references, and generalization relations. </rdfs:comment>
      <rdfs:subClassOf>
         <owl:Class>
            <owl:intersectionOf rdf:parseType="Collection">
               <owl:Restriction>
                  <owl:onProperty rdf:resource="http://www.opengis.net/citygml/2.0#has_GenericApplicationPropertyOfSite"/>
                  <owl:allValuesFrom rdf:resource="http://www.opengis.net/citygml/2.0#_GenericApplicationPropertyOfSite"/>
               </owl:Restriction>
               <owl:Restriction>
                  <owl:onProperty rdf:resource="http://www.opengis.net/citygml/2.0#has_GenericApplicationPropertyOfSite"/>
                  <owl:minCardinality rdf:datatype="http://www.w3.org/2001/XMLSchema#nonNegativeInteger">0</owl:minCardinality>
               </owl:Restriction>
            </owl:intersectionOf>
         </owl:Class>
      </rdfs:subClassOf>
      <rdfs:subClassOf rdf:resource="http://www.opengis.net/citygml/2.0#AbstractCityObjectType"/>
   </owl:Class>
   <owl:Class rdf:about="http://www.opengis.net/citygml/2.0#GeneralizationRelationType">
      <rdfs:comment>Denotes the relation of a _CityObject to its corresponding _CityObject in higher LOD, i.e. to the
				_CityObjects representing the same real world object in higher LOD. The GeneralizationRelationType element must either
				carry a reference to a _CityObject object or contain a _CityObject object inline, but neither both nor none.
			</rdfs:comment>
      <rdfs:subClassOf>
         <owl:Class>
            <owl:intersectionOf rdf:parseType="Collection">
               <owl:Restriction>
                  <owl:onProperty rdf:resource="http://www.opengis.net/citygml/2.0#has_CityObject"/>
                  <owl:allValuesFrom rdf:resource="http://www.opengis.net/citygml/2.0#_CityObject"/>
               </owl:Restriction>
            </owl:intersectionOf>
         </owl:Class>
      </rdfs:subClassOf>
   </owl:Class>
   <owl:Class rdf:about="http://www.opengis.net/citygml/2.0#ExternalReferenceType">
      <rdfs:comment>Type describing the reference to an corresponding object in an other information system, for example in
				the german cadastre ALKIS, the german topographic information system or ATKIS, or the OS MasterMap. The reference consists
				of the name of the external information system, represented by an URI, and the reference of the external object, given
				either by a string or by an URI. If the informationSystem element is missing in the ExternalReference, the
				ExternalObjectReference must be an URI, which contains an indication of the informationSystem.</rdfs:comment>
      <rdfs:subClassOf>
         <owl:Class>
            <owl:intersectionOf rdf:parseType="Collection">
               <owl:Restriction>
                  <owl:onProperty rdf:resource="http://www.opengis.net/citygml/2.0#informationSystem"/>
                  <owl:allValuesFrom rdf:resource="http://www.w3.org/2001/XMLSchema#anyURI"/>
               </owl:Restriction>
               <owl:Restriction>
                  <owl:onProperty rdf:resource="http://www.opengis.net/citygml/2.0#informationSystem"/>
                  <owl:minCardinality rdf:datatype="http://www.w3.org/2001/XMLSchema#nonNegativeInteger">0</owl:minCardinality>
               </owl:Restriction>
               <owl:Restriction>
                  <owl:onProperty rdf:resource="http://www.opengis.net/citygml/2.0#externalObject"/>
                  <owl:allValuesFrom rdf:resource="http://www.opengis.net/citygml/2.0#ExternalObjectReferenceType"/>
               </owl:Restriction>
            </owl:intersectionOf>
         </owl:Class>
      </rdfs:subClassOf>
   </owl:Class>
   <owl:Class rdf:about="http://www.opengis.net/citygml/2.0#ExternalObjectReferenceType">
      <owl:disjointUnionOf rdf:parseType="Collection">
         <owl:Restriction>
            <owl:onProperty rdf:resource="http://www.opengis.net/citygml/2.0#name"/>
            <owl:someValuesFrom rdf:resource="http://www.w3.org/2001/XMLSchema#string"/>
         </owl:Restriction>
         <owl:Restriction>
            <owl:onProperty rdf:resource="http://www.opengis.net/citygml/2.0#uri"/>
            <owl:someValuesFrom rdf:resource="http://www.w3.org/2001/XMLSchema#anyURI"/>
         </owl:Restriction>
      </owl:disjointUnionOf>
   </owl:Class>
   <owl:Class rdf:about="http://www.opengis.net/citygml/2.0#AddressPropertyType">
      <rdfs:comment>Denotes the relation of an _CityObject to its addresses. The AddressPropertyType element must either carry
				a reference to an Address object or contain an Address object inline, but neither both nor none. </rdfs:comment>
      <rdfs:subClassOf>
         <owl:Class>
            <owl:intersectionOf rdf:parseType="Collection">
               <owl:Restriction>
                  <owl:onProperty rdf:resource="http://www.opengis.net/citygml/2.0#hasAddress"/>
                  <owl:allValuesFrom rdf:resource="http://www.opengis.net/citygml/2.0#Address"/>
               </owl:Restriction>
            </owl:intersectionOf>
         </owl:Class>
      </rdfs:subClassOf>
   </owl:Class>
   <owl:Class rdf:about="http://www.opengis.net/citygml/2.0#AddressType">
      <rdfs:comment>Type for addresses. It references the xAL address standard issued by the OASIS consortium. Please note,
				that addresses are modelled as GML features. Every address can be assigned zero or more 2D or 3D point geometries (one
				gml:MultiPoint geometry) locating the entrance(s). </rdfs:comment>
      <rdfs:subClassOf>
         <owl:Class>
            <owl:intersectionOf rdf:parseType="Collection">
               <owl:Restriction>
                  <owl:onProperty rdf:resource="http://www.opengis.net/citygml/2.0#xalAddress"/>
                  <owl:allValuesFrom rdf:resource="http://www.opengis.net/citygml/2.0#xalAddressPropertyType"/>
               </owl:Restriction>
               <owl:Restriction>
                  <owl:onProperty rdf:resource="http://www.opengis.net/citygml/2.0#multiPoint"/>
                  <owl:allValuesFrom rdf:resource="http://www.opengis.net/gml#MultiPointPropertyType"/>
               </owl:Restriction>
               <owl:Restriction>
                  <owl:onProperty rdf:resource="http://www.opengis.net/citygml/2.0#multiPoint"/>
                  <owl:minCardinality rdf:datatype="http://www.w3.org/2001/XMLSchema#nonNegativeInteger">0</owl:minCardinality>
               </owl:Restriction>
               <owl:Restriction>
                  <owl:onProperty rdf:resource="http://www.opengis.net/citygml/2.0#has_GenericApplicationPropertyOfAddress"/>
                  <owl:allValuesFrom rdf:resource="http://www.opengis.net/citygml/2.0#_GenericApplicationPropertyOfAddress"/>
               </owl:Restriction>
               <owl:Restriction>
                  <owl:onProperty rdf:resource="http://www.opengis.net/citygml/2.0#has_GenericApplicationPropertyOfAddress"/>
                  <owl:minCardinality rdf:datatype="http://www.w3.org/2001/XMLSchema#nonNegativeInteger">0</owl:minCardinality>
               </owl:Restriction>
            </owl:intersectionOf>
         </owl:Class>
      </rdfs:subClassOf>
      <rdfs:subClassOf rdf:resource="http://www.opengis.net/gml#AbstractFeatureType"/>
      <rdfs:comment>Warning: The parent class 'gml:AbstractFeatureType' is declared outside of this class' original schema. This class may be declared incorrectly.</rdfs:comment>
   </owl:Class>
   <owl:Class rdf:about="http://www.opengis.net/citygml/2.0#xalAddressPropertyType">
      <rdfs:comment>Denotes the relation of an Address feature to the xAL address element.</rdfs:comment>
      <rdfs:subClassOf>
         <owl:Class>
            <owl:intersectionOf rdf:parseType="Collection">
               <owl:Restriction>
                  <owl:onProperty rdf:resource="urn:oasis:names:tc:ciq:xsdschema:xAL:2.0#hasAddressDetails"/>
                  <owl:allValuesFrom rdf:resource="urn:oasis:names:tc:ciq:xsdschema:xAL:2.0#AddressDetails"/>
               </owl:Restriction>
            </owl:intersectionOf>
         </owl:Class>
      </rdfs:subClassOf>
   </owl:Class>
   <owl:Class rdf:about="http://www.opengis.net/citygml/2.0#ImplicitGeometryType">
      <rdfs:comment> Type for the implicit representation of a geometry. An implicit geometry is a geometric object, where the
				shape is stored only once as a prototypical geometry, e.g. a tree or other vegetation object, a traffic light or a traffic
				sign. This prototypic geometry object is re-used or referenced many times, wherever the corresponding feature occurs in
				the 3D city model. Each occurrence is represented by a link to the prototypic shape geometry (in a local cartesian
				coordinate system), by a transforma-tion matrix that is multiplied with each 3D coordinate tuple of the prototype, and by
				an anchor point denoting the base point of the object in the world coordinate reference system. In order to determine the
				absolute coordinates of an implicit geometry, the anchor point coordinates have to be added to the matrix multiplication
				results. The transformation matrix accounts for the intended rotation, scaling, and local translation of the prototype. It
				is a 4x4 matrix that is multiplied with the prototype coordinates using homogeneous coordinates, i.e. (x,y,z,1). This way
				even a projection might be modelled by the transformation matrix. The concept of implicit geometries is an enhancement of
				the geometry model of GML3. </rdfs:comment>
      <rdfs:subClassOf>
         <owl:Class>
            <owl:intersectionOf rdf:parseType="Collection">
               <owl:Restriction>
                  <owl:onProperty rdf:resource="http://www.opengis.net/citygml/2.0#mimeType"/>
                  <owl:allValuesFrom rdf:resource="http://www.opengis.net/gml#CodeType"/>
               </owl:Restriction>
               <owl:Restriction>
                  <owl:onProperty rdf:resource="http://www.opengis.net/citygml/2.0#mimeType"/>
                  <owl:minCardinality rdf:datatype="http://www.w3.org/2001/XMLSchema#nonNegativeInteger">0</owl:minCardinality>
               </owl:Restriction>
               <owl:Restriction>
                  <owl:onProperty rdf:resource="http://www.opengis.net/citygml/2.0#transformationMatrix"/>
                  <owl:allValuesFrom rdf:resource="http://www.opengis.net/citygml/2.0#TransformationMatrix4x4Type"/>
               </owl:Restriction>
               <owl:Restriction>
                  <owl:onProperty rdf:resource="http://www.opengis.net/citygml/2.0#transformationMatrix"/>
                  <owl:minCardinality rdf:datatype="http://www.w3.org/2001/XMLSchema#nonNegativeInteger">0</owl:minCardinality>
               </owl:Restriction>
               <owl:Restriction>
                  <owl:onProperty rdf:resource="http://www.opengis.net/citygml/2.0#libraryObject"/>
                  <owl:allValuesFrom rdf:resource="http://www.w3.org/2001/XMLSchema#anyURI"/>
               </owl:Restriction>
               <owl:Restriction>
                  <owl:onProperty rdf:resource="http://www.opengis.net/citygml/2.0#libraryObject"/>
                  <owl:minCardinality rdf:datatype="http://www.w3.org/2001/XMLSchema#nonNegativeInteger">0</owl:minCardinality>
               </owl:Restriction>
               <owl:Restriction>
                  <owl:onProperty rdf:resource="http://www.opengis.net/citygml/2.0#relativeGMLGeometry"/>
                  <owl:allValuesFrom rdf:resource="http://www.opengis.net/gml#GeometryPropertyType"/>
               </owl:Restriction>
               <owl:Restriction>
                  <owl:onProperty rdf:resource="http://www.opengis.net/citygml/2.0#relativeGMLGeometry"/>
                  <owl:minCardinality rdf:datatype="http://www.w3.org/2001/XMLSchema#nonNegativeInteger">0</owl:minCardinality>
               </owl:Restriction>
               <owl:Restriction>
                  <owl:onProperty rdf:resource="http://www.opengis.net/citygml/2.0#referencePoint"/>
                  <owl:allValuesFrom rdf:resource="http://www.opengis.net/gml#PointPropertyType"/>
               </owl:Restriction>
            </owl:intersectionOf>
         </owl:Class>
      </rdfs:subClassOf>
      <rdfs:subClassOf rdf:resource="http://www.opengis.net/gml#AbstractGMLType"/>
      <rdfs:comment>Warning: The parent class 'gml:AbstractGMLType' is declared outside of this class' original schema. This class may be declared incorrectly.</rdfs:comment>
   </owl:Class>
   <owl:Class rdf:about="http://www.opengis.net/citygml/2.0#ImplicitRepresentationPropertyType">
      <rdfs:comment>Denotes the relation of a _CityObject to its implicit geometry representation, which is a representation
				of a geometry by referencing a prototype and transforming it to its real position in space. The
				ImplicitRepresentationPropertyType element must either carry a reference to a ImplicitGeometry object or contain a
				ImplicitGeometry object inline, but neither both nor none. </rdfs:comment>
      <rdfs:subClassOf>
         <owl:Class>
            <owl:intersectionOf rdf:parseType="Collection">
               <owl:Restriction>
                  <owl:onProperty rdf:resource="http://www.opengis.net/citygml/2.0#hasImplicitGeometry"/>
                  <owl:allValuesFrom rdf:resource="http://www.opengis.net/citygml/2.0#ImplicitGeometry"/>
               </owl:Restriction>
            </owl:intersectionOf>
         </owl:Class>
      </rdfs:subClassOf>
   </owl:Class>
   <rdfs:Datatype rdf:about="http://www.opengis.net/citygml/2.0#RelativeToTerrainType">
      <rdfs:comment>Specifies the spatial relation of a CityObject realativ to terrain in a qualitative way. The values of
				this type are defined in the XML file RelativeToTerrainType.xml, according to the dictionary concept of
				GML3.</rdfs:comment>
      <owl:equivalentClass>
         <rdfs:Datatype>
            <owl:oneOf>
               <rdf:Description rdf:type="http://www.w3.org/1999/02/22-rdf-syntax-ns#List">
                  <rdf:first rdf:datatype="http://www.w3.org/2001/XMLSchema#string">entirelyAboveTerrain</rdf:first>
                  <rdf:rest>
                     <rdf:Description rdf:type="http://www.w3.org/1999/02/22-rdf-syntax-ns#List">
                        <rdf:first rdf:datatype="http://www.w3.org/2001/XMLSchema#string">substantiallyAboveTerrain</rdf:first>
                        <rdf:rest>
                           <rdf:Description rdf:type="http://www.w3.org/1999/02/22-rdf-syntax-ns#List">
                              <rdf:first rdf:datatype="http://www.w3.org/2001/XMLSchema#string">substantiallyAboveAndBelowTerrain</rdf:first>
                              <rdf:rest>
                                 <rdf:Description rdf:type="http://www.w3.org/1999/02/22-rdf-syntax-ns#List">
                                    <rdf:first rdf:datatype="http://www.w3.org/2001/XMLSchema#string">substantiallyBelowTerrain</rdf:first>
                                    <rdf:rest>
                                       <rdf:Description rdf:type="http://www.w3.org/1999/02/22-rdf-syntax-ns#List">
                                          <rdf:first rdf:datatype="http://www.w3.org/2001/XMLSchema#string">entirelyBelowTerrain</rdf:first>
                                          <rdf:rest rdf:resource="http://www.w3.org/1999/02/22-rdf-syntax-ns#nil"/>
                                       </rdf:Description>
                                    </rdf:rest>
                                 </rdf:Description>
                              </rdf:rest>
                           </rdf:Description>
                        </rdf:rest>
                     </rdf:Description>
                  </rdf:rest>
               </rdf:Description>
            </owl:oneOf>
         </rdfs:Datatype>
      </owl:equivalentClass>
   </rdfs:Datatype>
   <rdfs:Datatype rdf:about="http://www.opengis.net/citygml/2.0#RelativeToWaterType">
      <rdfs:comment>Specifies the spatial relation of a CityObject realativ to the water surface in a qualitative way. The
				values of this type are defined in the XML file RelativeToTerrainType.xml, according to the dictionary concept of
				GML3.</rdfs:comment>
      <owl:equivalentClass>
         <rdfs:Datatype>
            <owl:oneOf>
               <rdf:Description rdf:type="http://www.w3.org/1999/02/22-rdf-syntax-ns#List">
                  <rdf:first rdf:datatype="http://www.w3.org/2001/XMLSchema#string">entirelyAboveWaterSurface</rdf:first>
                  <rdf:rest>
                     <rdf:Description rdf:type="http://www.w3.org/1999/02/22-rdf-syntax-ns#List">
                        <rdf:first rdf:datatype="http://www.w3.org/2001/XMLSchema#string">substantiallyAboveWaterSurface</rdf:first>
                        <rdf:rest>
                           <rdf:Description rdf:type="http://www.w3.org/1999/02/22-rdf-syntax-ns#List">
                              <rdf:first rdf:datatype="http://www.w3.org/2001/XMLSchema#string">substantiallyAboveAndBelowWaterSurface</rdf:first>
                              <rdf:rest>
                                 <rdf:Description rdf:type="http://www.w3.org/1999/02/22-rdf-syntax-ns#List">
                                    <rdf:first rdf:datatype="http://www.w3.org/2001/XMLSchema#string">substantiallyBelowWaterSurface</rdf:first>
                                    <rdf:rest>
                                       <rdf:Description rdf:type="http://www.w3.org/1999/02/22-rdf-syntax-ns#List">
                                          <rdf:first rdf:datatype="http://www.w3.org/2001/XMLSchema#string">entirelyBelowWaterSurface</rdf:first>
                                          <rdf:rest>
                                             <rdf:Description rdf:type="http://www.w3.org/1999/02/22-rdf-syntax-ns#List">
                                                <rdf:first rdf:datatype="http://www.w3.org/2001/XMLSchema#string">temporarilyAboveAndBelowWaterSurface</rdf:first>
                                                <rdf:rest rdf:resource="http://www.w3.org/1999/02/22-rdf-syntax-ns#nil"/>
                                             </rdf:Description>
                                          </rdf:rest>
                                       </rdf:Description>
                                    </rdf:rest>
                                 </rdf:Description>
                              </rdf:rest>
                           </rdf:Description>
                        </rdf:rest>
                     </rdf:Description>
                  </rdf:rest>
               </rdf:Description>
            </owl:oneOf>
         </rdfs:Datatype>
      </owl:equivalentClass>
   </rdfs:Datatype>
   <rdfs:Datatype rdf:about="http://www.opengis.net/citygml/2.0#doubleBetween0and1">
      <rdfs:comment>Type for values, which are greater or equal than 0 and less or equal than 1. Used for color encoding, for
				example. </rdfs:comment>
      <owl:equivalentClass>
         <rdfs:Datatype>
            <owl:onDatatype rdf:resource="http://www.w3.org/2001/XMLSchema#double"/>
            <owl:withRestrictions rdf:parseType="Collection">
               <rdf:Description>
                  <xs:minInclusive rdf:datatype="http://www.w3.org/2001/XMLSchema#double">0</xs:minInclusive>
               </rdf:Description>
               <rdf:Description>
                  <xs:maxInclusive rdf:datatype="http://www.w3.org/2001/XMLSchema#double">1</xs:maxInclusive>
               </rdf:Description>
            </owl:withRestrictions>
         </rdfs:Datatype>
      </owl:equivalentClass>
   </rdfs:Datatype>
   <rdfs:Datatype rdf:about="http://www.opengis.net/citygml/2.0#doubleBetween0and1List">
      <rdfs:comment>List for double values, which are greater or equal than 0 and less or equal than 1. Used for color
				encoding, for example. </rdfs:comment>
      <owl:equivalentClass rdf:resource="http://www.w3.org/2001/XMLSchema#string"/>
   </rdfs:Datatype>
   <rdfs:Datatype rdf:about="http://www.opengis.net/citygml/2.0#TransformationMatrix4x4Type">
      <rdfs:comment>Used for implicit geometries. The Transformation matrix is a 4 by 4 matrix, thus it must be a list with 16
				items. The order the matrix element are represented is row-major, i. e. the first 4 elements represent the first row, the
				fifth to the eight element the second row,... </rdfs:comment>
   </rdfs:Datatype>
   <rdfs:Datatype rdf:about="http://www.opengis.net/citygml/2.0#TransformationMatrix2x2Type">
      <rdfs:comment>Used for georeferencing. The Transformation matrix is a 2 by 2 matrix, thus it must be a list with 4
				items. The order the matrix element are represented is row-major, i. e. the first 2 elements represent the first row, the
				fifth to the eight element the second row,... </rdfs:comment>
   </rdfs:Datatype>
   <rdfs:Datatype rdf:about="http://www.opengis.net/citygml/2.0#TransformationMatrix3x4Type">
      <rdfs:comment>Used for texture parameterization. The Transformation matrix is a 3 by 4 matrix, thus it must be a list
				with 12 items. The order the matrix element are represented is row-major, i. e. the first 4 elements represent the first
				row, the fifth to the eight element the second row,... </rdfs:comment>
   </rdfs:Datatype>
   <rdfs:Datatype rdf:about="http://www.opengis.net/citygml/2.0#integerBetween0and4">
      <rdfs:comment>Type for integer values, which are greater or equal than 0 and less or equal than 4. Used for encoding of
				the LOD number. </rdfs:comment>
      <owl:equivalentClass>
         <rdfs:Datatype>
            <owl:onDatatype rdf:resource="http://www.w3.org/2001/XMLSchema#integer"/>
            <owl:withRestrictions rdf:parseType="Collection">
               <rdf:Description>
                  <xs:minInclusive rdf:datatype="http://www.w3.org/2001/XMLSchema#integer">0</xs:minInclusive>
               </rdf:Description>
               <rdf:Description>
                  <xs:maxInclusive rdf:datatype="http://www.w3.org/2001/XMLSchema#integer">4</xs:maxInclusive>
               </rdf:Description>
            </owl:withRestrictions>
         </rdfs:Datatype>
      </owl:equivalentClass>
   </rdfs:Datatype>
   <owl:Class rdf:about="http://www.opengis.net/citygml/2.0#CityModel">
      <rdfs:subClassOf rdf:resource="http://www.opengis.net/gml#_FeatureCollection"/>
      <rdfs:subClassOf rdf:resource="http://www.opengis.net/citygml/2.0#CityModelType"/>
   </owl:Class>
   <owl:Class rdf:about="http://www.opengis.net/citygml/2.0#_GenericApplicationPropertyOfCityModel">
      <rdfs:subClassOf rdf:resource="http://www.w3.org/2001/XMLSchema#anyType"/>
      <rdfs:comment>Warning: This class type was declared outside of its original schema. This class may be declared incorrectly.</rdfs:comment>
   </owl:Class>
   <owl:Class rdf:about="http://www.opengis.net/citygml/2.0#cityObjectMember">
      <rdfs:subClassOf rdf:resource="http://www.opengis.net/gml#featureMember"/>
      <rdfs:subClassOf rdf:resource="http://www.opengis.net/gml#FeaturePropertyType"/>
      <rdfs:comment>Warning: This class type was declared outside of its original schema. This class may be declared incorrectly.</rdfs:comment>
   </owl:Class>
   <owl:Class rdf:about="http://www.opengis.net/citygml/2.0#_CityObject">
      <rdfs:subClassOf rdf:resource="http://www.opengis.net/gml#_Feature"/>
      <rdfs:subClassOf rdf:resource="http://www.opengis.net/citygml/2.0#AbstractCityObjectType"/>
   </owl:Class>
   <owl:Class rdf:about="http://www.opengis.net/citygml/2.0#_GenericApplicationPropertyOfCityObject">
      <rdfs:subClassOf rdf:resource="http://www.w3.org/2001/XMLSchema#anyType"/>
      <rdfs:comment>Warning: This class type was declared outside of its original schema. This class may be declared incorrectly.</rdfs:comment>
   </owl:Class>
   <owl:Class rdf:about="http://www.opengis.net/citygml/2.0#_Site">
      <rdfs:subClassOf rdf:resource="http://www.opengis.net/citygml/2.0#_CityObject"/>
      <rdfs:subClassOf rdf:resource="http://www.opengis.net/citygml/2.0#AbstractSiteType"/>
   </owl:Class>
   <owl:Class rdf:about="http://www.opengis.net/citygml/2.0#_GenericApplicationPropertyOfSite">
      <rdfs:subClassOf rdf:resource="http://www.w3.org/2001/XMLSchema#anyType"/>
      <rdfs:comment>Warning: This class type was declared outside of its original schema. This class may be declared incorrectly.</rdfs:comment>
   </owl:Class>
   <owl:Class rdf:about="http://www.opengis.net/citygml/2.0#Address">
      <rdfs:subClassOf rdf:resource="http://www.opengis.net/gml#_Feature"/>
      <rdfs:subClassOf rdf:resource="http://www.opengis.net/citygml/2.0#AddressType"/>
   </owl:Class>
   <owl:Class rdf:about="http://www.opengis.net/citygml/2.0#_GenericApplicationPropertyOfAddress">
      <rdfs:subClassOf rdf:resource="http://www.w3.org/2001/XMLSchema#anyType"/>
      <rdfs:comment>Warning: This class type was declared outside of its original schema. This class may be declared incorrectly.</rdfs:comment>
   </owl:Class>
   <owl:Class rdf:about="http://www.opengis.net/citygml/2.0#ImplicitGeometry">
      <rdfs:subClassOf rdf:resource="http://www.opengis.net/gml#_GML"/>
      <rdfs:subClassOf rdf:resource="http://www.opengis.net/citygml/2.0#ImplicitGeometryType"/>
   </owl:Class>
   <owl:ObjectProperty rdf:about="http://www.opengis.net/citygml/2.0#has_GenericApplicationPropertyOfCityModel">
      <rdfs:domain rdf:resource="http://www.opengis.net/citygml/2.0#CityModelType"/>
      <rdfs:range rdf:resource="http://www.opengis.net/citygml/2.0#_GenericApplicationPropertyOfCityModel"/>
   </owl:ObjectProperty>
   <owl:DatatypeProperty rdf:about="http://www.opengis.net/citygml/2.0#creationDate">
      <rdfs:domain rdf:resource="http://www.opengis.net/citygml/2.0#AbstractCityObjectType"/>
      <rdfs:range rdf:resource="http://www.w3.org/2001/XMLSchema#date"/>
   </owl:DatatypeProperty>
   <owl:DatatypeProperty rdf:about="http://www.opengis.net/citygml/2.0#terminationDate">
      <rdfs:domain rdf:resource="http://www.opengis.net/citygml/2.0#AbstractCityObjectType"/>
      <rdfs:range rdf:resource="http://www.w3.org/2001/XMLSchema#date"/>
   </owl:DatatypeProperty>
   <owl:ObjectProperty rdf:about="http://www.opengis.net/citygml/2.0#externalReference">
      <rdfs:domain rdf:resource="http://www.opengis.net/citygml/2.0#AbstractCityObjectType"/>
      <rdfs:range rdf:resource="http://www.opengis.net/citygml/2.0#ExternalReferenceType"/>
   </owl:ObjectProperty>
   <owl:ObjectProperty rdf:about="http://www.opengis.net/citygml/2.0#generalizesTo">
      <rdfs:domain rdf:resource="http://www.opengis.net/citygml/2.0#AbstractCityObjectType"/>
      <rdfs:range rdf:resource="http://www.opengis.net/citygml/2.0#GeneralizationRelationType"/>
   </owl:ObjectProperty>
   <owl:DatatypeProperty rdf:about="http://www.opengis.net/citygml/2.0#relativeToTerrain">
      <rdfs:domain rdf:resource="http://www.opengis.net/citygml/2.0#AbstractCityObjectType"/>
      <rdfs:range rdf:resource="http://www.opengis.net/citygml/2.0#RelativeToTerrainType"/>
   </owl:DatatypeProperty>
   <owl:DatatypeProperty rdf:about="http://www.opengis.net/citygml/2.0#relativeToWater">
      <rdfs:domain rdf:resource="http://www.opengis.net/citygml/2.0#AbstractCityObjectType"/>
      <rdfs:range rdf:resource="http://www.opengis.net/citygml/2.0#RelativeToWaterType"/>
   </owl:DatatypeProperty>
   <owl:ObjectProperty rdf:about="http://www.opengis.net/citygml/2.0#has_GenericApplicationPropertyOfCityObject">
      <rdfs:domain rdf:resource="http://www.opengis.net/citygml/2.0#AbstractCityObjectType"/>
      <rdfs:range rdf:resource="http://www.opengis.net/citygml/2.0#_GenericApplicationPropertyOfCityObject"/>
   </owl:ObjectProperty>
   <owl:ObjectProperty rdf:about="http://www.opengis.net/citygml/2.0#has_GenericApplicationPropertyOfSite">
      <rdfs:domain rdf:resource="http://www.opengis.net/citygml/2.0#AbstractSiteType"/>
      <rdfs:range rdf:resource="http://www.opengis.net/citygml/2.0#_GenericApplicationPropertyOfSite"/>
   </owl:ObjectProperty>
   <owl:ObjectProperty rdf:about="http://www.opengis.net/citygml/2.0#has_CityObject">
      <rdfs:domain rdf:resource="http://www.opengis.net/citygml/2.0#GeneralizationRelationType"/>
      <rdfs:range rdf:resource="http://www.opengis.net/citygml/2.0#_CityObject"/>
   </owl:ObjectProperty>
   <owl:DatatypeProperty rdf:about="http://www.opengis.net/citygml/2.0#informationSystem">
      <rdfs:domain rdf:resource="http://www.opengis.net/citygml/2.0#ExternalReferenceType"/>
      <rdfs:range rdf:resource="http://www.w3.org/2001/XMLSchema#anyURI"/>
   </owl:DatatypeProperty>
   <owl:ObjectProperty rdf:about="http://www.opengis.net/citygml/2.0#externalObject">
      <rdfs:domain rdf:resource="http://www.opengis.net/citygml/2.0#ExternalReferenceType"/>
      <rdfs:range rdf:resource="http://www.opengis.net/citygml/2.0#ExternalObjectReferenceType"/>
   </owl:ObjectProperty>
   <owl:DatatypeProperty rdf:about="http://www.opengis.net/citygml/2.0#name">
      <rdfs:domain rdf:resource="http://www.opengis.net/citygml/2.0#ExternalObjectReferenceType"/>
      <rdfs:range rdf:resource="http://www.w3.org/2001/XMLSchema#string"/>
   </owl:DatatypeProperty>
   <owl:DatatypeProperty rdf:about="http://www.opengis.net/citygml/2.0#uri">
      <rdfs:domain rdf:resource="http://www.opengis.net/citygml/2.0#ExternalObjectReferenceType"/>
      <rdfs:range rdf:resource="http://www.w3.org/2001/XMLSchema#anyURI"/>
   </owl:DatatypeProperty>
   <owl:ObjectProperty rdf:about="http://www.opengis.net/citygml/2.0#hasAddress">
      <rdfs:domain rdf:resource="http://www.opengis.net/citygml/2.0#AddressPropertyType"/>
      <rdfs:range rdf:resource="http://www.opengis.net/citygml/2.0#Address"/>
   </owl:ObjectProperty>
   <owl:ObjectProperty rdf:about="http://www.opengis.net/citygml/2.0#xalAddress">
      <rdfs:domain rdf:resource="http://www.opengis.net/citygml/2.0#AddressType"/>
      <rdfs:range rdf:resource="http://www.opengis.net/citygml/2.0#xalAddressPropertyType"/>
   </owl:ObjectProperty>
   <owl:ObjectProperty rdf:about="http://www.opengis.net/citygml/2.0#multiPoint">
      <rdfs:comment>Warning: This ObjectProperty type was declared outside of its original schema. This ObjectProperty may be declared incorrectly.</rdfs:comment>
      <rdfs:domain rdf:resource="http://www.opengis.net/citygml/2.0#AddressType"/>
      <rdfs:range rdf:resource="http://www.opengis.net/gml#MultiPointPropertyType"/>
   </owl:ObjectProperty>
   <owl:ObjectProperty rdf:about="http://www.opengis.net/citygml/2.0#has_GenericApplicationPropertyOfAddress">
      <rdfs:domain rdf:resource="http://www.opengis.net/citygml/2.0#AddressType"/>
      <rdfs:range rdf:resource="http://www.opengis.net/citygml/2.0#_GenericApplicationPropertyOfAddress"/>
   </owl:ObjectProperty>
   <owl:ObjectProperty rdf:about="urn:oasis:names:tc:ciq:xsdschema:xAL:2.0#hasAddressDetails">
      <rdfs:comment>Warning: This ObjectProperty reference was declared outside of its original schema. This ObjectProperty may be declared incorrectly.</rdfs:comment>
      <rdfs:domain rdf:resource="http://www.opengis.net/citygml/2.0#xalAddressPropertyType"/>
      <rdfs:range rdf:resource="urn:oasis:names:tc:ciq:xsdschema:xAL:2.0#AddressDetails"/>
   </owl:ObjectProperty>
   <owl:ObjectProperty rdf:about="http://www.opengis.net/citygml/2.0#mimeType">
      <rdfs:comment>Warning: This ObjectProperty type was declared outside of its original schema. This ObjectProperty may be declared incorrectly.</rdfs:comment>
      <rdfs:domain rdf:resource="http://www.opengis.net/citygml/2.0#ImplicitGeometryType"/>
      <rdfs:range rdf:resource="http://www.opengis.net/gml#CodeType"/>
   </owl:ObjectProperty>
   <owl:DatatypeProperty rdf:about="http://www.opengis.net/citygml/2.0#transformationMatrix">
      <rdfs:domain rdf:resource="http://www.opengis.net/citygml/2.0#ImplicitGeometryType"/>
      <rdfs:range rdf:resource="http://www.opengis.net/citygml/2.0#TransformationMatrix4x4Type"/>
   </owl:DatatypeProperty>
   <owl:DatatypeProperty rdf:about="http://www.opengis.net/citygml/2.0#libraryObject">
      <rdfs:domain rdf:resource="http://www.opengis.net/citygml/2.0#ImplicitGeometryType"/>
      <rdfs:range rdf:resource="http://www.w3.org/2001/XMLSchema#anyURI"/>
   </owl:DatatypeProperty>
   <owl:ObjectProperty rdf:about="http://www.opengis.net/citygml/2.0#relativeGMLGeometry">
      <rdfs:comment>Warning: This ObjectProperty type was declared outside of its original schema. This ObjectProperty may be declared incorrectly.</rdfs:comment>
      <rdfs:domain rdf:resource="http://www.opengis.net/citygml/2.0#ImplicitGeometryType"/>
      <rdfs:range rdf:resource="http://www.opengis.net/gml#GeometryPropertyType"/>
   </owl:ObjectProperty>
   <owl:ObjectProperty rdf:about="http://www.opengis.net/citygml/2.0#referencePoint">
      <rdfs:comment>Warning: This ObjectProperty type was declared outside of its original schema. This ObjectProperty may be declared incorrectly.</rdfs:comment>
      <rdfs:domain rdf:resource="http://www.opengis.net/citygml/2.0#ImplicitGeometryType"/>
      <rdfs:range rdf:resource="http://www.opengis.net/gml#PointPropertyType"/>
   </owl:ObjectProperty>
   <owl:ObjectProperty rdf:about="http://www.opengis.net/citygml/2.0#hasImplicitGeometry">
      <rdfs:domain rdf:resource="http://www.opengis.net/citygml/2.0#ImplicitRepresentationPropertyType"/>
      <rdfs:range rdf:resource="http://www.opengis.net/citygml/2.0#ImplicitGeometry"/>
   </owl:ObjectProperty>
</rdf:RDF>
