<rdf:RDF xmlns:math="http://www.w3.org/2005/xpath-functions/math" xmlns:owl="http://www.w3.org/2002/07/owl#" xmlns:rdf="http://www.w3.org/1999/02/22-rdf-syntax-ns#" xmlns:rdfs="http://www.w3.org/2000/01/rdf-schema#" xmlns:xs="http://www.w3.org/2001/XMLSchema" xmlns:xsd="http://www.w3.org/2001/XMLSchema">
   <owl:Ontology rdf:about="http://liris.cnrs.fr/ontologies/compositegml">
      <owl:imports rdf:resource="http://liris.cnrs.fr/ontologies/xlink"/>
      <owl:imports rdf:resource="http://liris.cnrs.fr/ontologies/smil20"/>
      <rdfs:comment>gml.xsd</rdfs:comment>
      <rdfs:seeAlso>urn:opengis:specification:gml:schema-xsd:gml:3.1.1</rdfs:seeAlso>
      <rdfs:comment>Top level GML schema
      
      GML is an OGC Standard.
      Copyright (c) 2001,2005,2010 Open Geospatial Consortium.
      To obtain additional rights of use, visit http://www.opengeospatial.org/legal/ .
    </rdfs:comment>
      <rdfs:seeAlso>urn:opengis:specification:gml:schema-xsd:dynamicFeature:3.1.1</rdfs:seeAlso>
      <rdfs:comment xml:lang="en">Basic support for tracking moving objects and objects with changing state.
      
      GML is an OGC Standard.
      Copyright (c) 2001,2005,2010 Open Geospatial Consortium.
      To obtain additional rights of use, visit http://www.opengeospatial.org/legal/ .
    </rdfs:comment>
      <rdfs:seeAlso>urn:opengis:specification:gml:schema-xsd:feature:v3.1.1</rdfs:seeAlso>
      <rdfs:comment>GML Feature schema.
      
      GML is an OGC Standard.
      Copyright (c) 2001,2005,2010 Open Geospatial Consortium.
      To obtain additional rights of use, visit http://www.opengeospatial.org/legal/ .
    </rdfs:comment>
      <rdfs:comment>geometryBasic2d.xsd</rdfs:comment>
      <rdfs:seeAlso>urn:opengis:specification:gml:schema-xsd:geometryBasic2d:3.1.1</rdfs:seeAlso>
      <rdfs:comment>
      GML is an OGC Standard.
      Copyright (c) 2001,2005,2010 Open Geospatial Consortium.
      To obtain additional rights of use, visit http://www.opengeospatial.org/legal/ .
    </rdfs:comment>
      <rdfs:comment>geometryBasic0d1d.xsd</rdfs:comment>
      <rdfs:seeAlso>urn:opengis:specification:gml:schema-xsd:geometryBasic0d1d:v3.1.1</rdfs:seeAlso>
      <rdfs:seeAlso>urn:opengis:specification:gml:schema-xsd:geometryBasic0d1d:v3.1.1</rdfs:seeAlso>
      <rdfs:comment>
      GML is an OGC Standard.
      Copyright (c) 2001,2005,2010 Open Geospatial Consortium.
      To obtain additional rights of use, visit http://www.opengeospatial.org/legal/ .
    </rdfs:comment>
      <rdfs:seeAlso>urn:opengis:specification:gml:schema-measures:3.1.1</rdfs:seeAlso>
      <rdfs:comment>Extends the units.xsd and basicTypes.xsd schemas with types for recording measures using specific types of units, especially the measures and units needed for coordinate reference systems and coordinate operations. The specific unit types encoded are length, angle, scale factor, time, area, volume, speed, and grid length. This schema allows angle values to be recorded as single numbers or in degree-minute-second format. 
    Parts of this schema are based on Subclause 6.5.7 of ISO/CD 19103 Geographic information - Conceptual schema language, on Subclause A.5.2.2.3 of ISO/CD 19118 Geographic information - Encoding, and on Subclause 4.7 of OpenGIS Recommendation Paper OGC 02-007r4 Units of Measure Use and Definition Recommendations.
    
    GML is an OGC Standard.
    Copyright (c) 2001,2005,2010 Open Geospatial Consortium.
    To obtain additional rights of use, visit http://www.opengeospatial.org/legal/ .
    </rdfs:comment>
      <rdfs:seeAlso>urn:opengis:specification:gml:schema-units:3.1.1</rdfs:seeAlso>
      <rdfs:comment>Builds on gmlBase.xsd to encode units of measure (or uom), including definitions of units of measure and dictionaries of such definitions. GML 3.0 candidate schema, primary editor: Arliss Whiteside.      
  Parts of this schema are based on Subclause 6.5.7 of ISO/CD 19103 Geographic information - Conceptual schema language, on Subclause A.5.2.2.3 of ISO/CD 19118 Geographic information - Encoding, and on most of OpenGIS Recommendation Paper OGC 02-007r4 Units of Measure Use and Definition Recommendations.
    
    GML is an OGC Standard.
    Copyright (c) 2001,2005,2010 Open Geospatial Consortium.
    To obtain additional rights of use, visit http://www.opengeospatial.org/legal/ .
    </rdfs:comment>
      <rdfs:seeAlso>urn:opengis:specification:gml:schema-xsd:dictionary:3.1.1</rdfs:seeAlso>
      <rdfs:comment>
      Dictionary schema for GML 3.1.1 
      Components to support the lists of definitions.
      
      GML is an OGC Standard.
      Copyright (c) 2001,2005,2010 Open Geospatial Consortium.
      To obtain additional rights of use, visit http://www.opengeospatial.org/legal/ .
    </rdfs:comment>
      <rdfs:seeAlso>urn:opengis:specification:gml:schema-xsd:gmlBase:3.1.1</rdfs:seeAlso>
      <rdfs:comment>GML base schema for GML 3
      Components to support the GML encoding model.
      The abstract Schematron rules can be used by any schema that includes gmlBase.
      
      GML is an OGC Standard.
      Copyright (c) 2001,2005,2010 Open Geospatial Consortium.
      To obtain additional rights of use, visit http://www.opengeospatial.org/legal/ .
    </rdfs:comment>
      <rdfs:comment>basicTypes.xsd</rdfs:comment>
      <rdfs:seeAlso>urn:opengis:specification:gml:schema-xsd:basicTypes:3.1.1</rdfs:seeAlso>
      <rdfs:comment>
    Generic simpleContent components for use in GML
    
    GML is an OGC Standard.
    Copyright (c) 2001,2005,2010 Open Geospatial Consortium.
    To obtain additional rights of use, visit http://www.opengeospatial.org/legal/ .
    </rdfs:comment>
      <rdfs:seeAlso>urn:opengis:specification:gml:schema-xsd:temporal:3.1.1</rdfs:seeAlso>
      <rdfs:comment xml:lang="en">The temporal schema for GML 3.1 provides constructs for handling time-varying spatial data. 
    This schema reflects a partial implementation of the model described in ISO 19108:2002.
    
    GML is an OGC Standard.
    Copyright (c) 2001,2005,2010 Open Geospatial Consortium.
    To obtain additional rights of use, visit http://www.opengeospatial.org/legal/ .
    </rdfs:comment>
      <rdfs:comment>direction.xsd</rdfs:comment>
      <rdfs:seeAlso>urn:opengis:specification:gml:schema-xsd:direction:3.1.1</rdfs:seeAlso>
      <rdfs:comment>This schema defines "direction" element and type.
      
      GML is an OGC Standard.
      Copyright (c) 2001,2005,2010 Open Geospatial Consortium.
      To obtain additional rights of use, visit http://www.opengeospatial.org/legal/ .
    </rdfs:comment>
      <rdfs:comment>topology.xsd</rdfs:comment>
      <rdfs:seeAlso>urn:opengis:specification:gml:schema-xsd:topology:3.1.1</rdfs:seeAlso>
      <rdfs:comment>
      GML is an OGC Standard.
      Copyright (c) 2001,2005,2010 Open Geospatial Consortium.
      To obtain additional rights of use, visit http://www.opengeospatial.org/legal/ .
    </rdfs:comment>
      <rdfs:comment>geometryComplexes.xsd</rdfs:comment>
      <rdfs:seeAlso>urn:opengis:specification:gml:schema-xsd:geometryComplexes:v3.1.1</rdfs:seeAlso>
      <rdfs:comment>
      GML is an OGC Standard.
      Copyright (c) 2001,2005,2010 Open Geospatial Consortium.
      To obtain additional rights of use, visit http://www.opengeospatial.org/legal/ .
    </rdfs:comment>
      <rdfs:comment>geometryAggregates.xsd</rdfs:comment>
      <rdfs:seeAlso>urn:opengis:specification:gml:schema-xsd:geometryAggregates:3.1.1</rdfs:seeAlso>
      <rdfs:comment>
      GML is an OGC Standard.
      Copyright (c) 2001,2005,2010 Open Geospatial Consortium.
      To obtain additional rights of use, visit http://www.opengeospatial.org/legal/ .
    </rdfs:comment>
      <rdfs:comment>geometryPrimitives.xsd</rdfs:comment>
      <rdfs:seeAlso>urn:opengis:specification:gml:schema-xsd:geometryPrimitives:3.1.1</rdfs:seeAlso>
      <rdfs:comment>
      GML is an OGC Standard.
      Copyright (c) 2001,2005,2010 Open Geospatial Consortium.
      To obtain additional rights of use, visit http://www.opengeospatial.org/legal/ .
    </rdfs:comment>
      <rdfs:comment>coverage.xsd</rdfs:comment>
      <rdfs:seeAlso>urn:opengis:specification:gml:schema-xsd:coverage:3.1.1</rdfs:seeAlso>
      <rdfs:comment xml:lang="en">GML Coverage schema.
      
      GML is an OGC Standard.
      Copyright (c) 2001,2005,2010 Open Geospatial Consortium.
      To obtain additional rights of use, visit http://www.opengeospatial.org/legal/ .
    </rdfs:comment>
      <rdfs:comment>valueObjects.xsd</rdfs:comment>
      <rdfs:seeAlso>urn:opengis:specification:gml:schema-xsd:valueObjects:3.1.1</rdfs:seeAlso>
      <rdfs:comment>GML conformant schema for Values in which the  
        * scalar Value types and lists have their values recorded in simpleContent elements 
        * complex Value types are built recursively
        
        GML is an OGC Standard.
        Copyright (c) 2001,2005,2010 Open Geospatial Consortium.
        To obtain additional rights of use, visit http://www.opengeospatial.org/legal/ .
    </rdfs:comment>
      <rdfs:comment>grids.xsd</rdfs:comment>
      <rdfs:seeAlso>urn:opengis:specification:gml:schema-xsd:grids:3.1.1</rdfs:seeAlso>
      <rdfs:comment xml:lang="en">Grid geometries
    A subset of implicit geometries
    Designed for use with GML Coverage schema, but maybe useful elsewhere as well.
    
    GML is an OGC Standard.
    Copyright (c) 2001,2005,2010 Open Geospatial Consortium.
    To obtain additional rights of use, visit http://www.opengeospatial.org/legal/ .
    </rdfs:comment>
      <rdfs:seeAlso>urn:opengis:specification:gml:schema-xsd:coordinateReferenceSystems:3.1.1</rdfs:seeAlso>
      <rdfs:comment>How to encode coordinate reference system definitions. Builds on referenceSystems.xsd to encode the data needed to define coordinate reference systems, including the specific subtypes of coordinate reference systems. 
    This schema encodes the Coordinate Reference System (SC_) package of the extended UML Model for OGC Abstract Specification Topic 2: Spatial Referencing by Coordinates, with the exception of the abstract "SC_CRS" class. The "SC_CRS" class is encoded in referenceSystems.xsd, to eliminate the (circular) references from coordinateOperations.xsd to coordinateReferenceSystems.xsd. That UML model is adapted from ISO 19111 - Spatial referencing by coordinates, as described in Annex C of Topic 2. 
    Caution: The CRS package in GML 3.1 and GML 3.1.1 is preliminary, and is expected to undergo some modifications that are not backward compatible during the development of GML 3.2 (ISO 19136). The GML 3.2 package will implement the model described in the revised version of ISO 19111. 
    
    GML is an OGC Standard.
    Copyright (c) 2001,2005,2010 Open Geospatial Consortium.
    To obtain additional rights of use, visit http://www.opengeospatial.org/legal/ .
    </rdfs:comment>
      <rdfs:seeAlso>urn:opengis:specification:gml:schema-xsd:coordinateSystems:3.1.1</rdfs:seeAlso>
      <rdfs:comment>How to encode coordinate system definitions. Builds on referenceSystems.xsd to encode the data needed to define coordinate systems, including the specific subtypes of coordinate systems. 
    This schema encodes the Coordinate System (CS_) package of the extended UML Model for OGC Abstract Specification Topic 2: Spatial Referencing by Coordinates. That UML model is adapted from ISO 19111 - Spatial referencing by coordinates, as described in Annex C of Topic 2. 
    Caution: The CRS package in GML 3.1 and GML 3.1.1 is preliminary, and is expected to undergo some modifications that are not backward compatible during the development of GML 3.2 (ISO 19136). The GML 3.2 package will implement the model described in the revised version of ISO 19111.
    
    GML is an OGC Standard.
    Copyright (c) 2001,2005,2010 Open Geospatial Consortium.
    To obtain additional rights of use, visit http://www.opengeospatial.org/legal/ .
    </rdfs:comment>
      <rdfs:seeAlso>urn:opengis:specification:gml:schema-xsd:referenceSystems:3.1.1</rdfs:seeAlso>
      <rdfs:comment>How to encode reference system definitions. Builds on several other parts of GML 3 to encode the data needed to define reference systems.
    This schema encodes the Reference System (RS_) package of the extended UML Model for OGC Abstract Specification Topic 2: Spatial Referencing by Coordinates. That UML model is adapted from ISO 19111 - Spatial referencing by coordinates, as described in Annex C of Topic 2. The SC_CRS class is also encoded here, to eliminate the (circular) references from coordinateOperations.xsd to coordinateReferenceSystems.xsd. The RS_SpatialReferenceSystemUsingGeographicIdentifier class is not encoded, since it is not applicable to coordinate positions. The CI_Citation class is not directly encoded, since such information can be included as metaDataProperty elements which are optionally allowed. A modified version of the EX_Extent (DataType) class from ISO 19115 is currently encoded here, using GML 3 schema types. (A more extensive version of the EX_Extent package might be XML encoded in the future, probably in a separate extent.xsd schema.)
    Caution: The CRS package in GML 3.1 and GML 3.1.1 is preliminary, and is expected to undergo some modifications that are not backward compatible during the development of GML 3.2 (ISO 19136). The GML 3.2 package will implement the model described in the revised version of ISO 19111.
    
    GML is an OGC Standard.
    Copyright (c) 2001,2005,2010 Open Geospatial Consortium.
    To obtain additional rights of use, visit http://www.opengeospatial.org/legal/ .
    </rdfs:comment>
      <rdfs:seeAlso>urn:opengis:specification:gml:schema-xsd:datums:3.1.1</rdfs:seeAlso>
      <rdfs:comment>How to encode datum definitions. Builds on referenceSystems.xsd to encode the data needed to define datums, including the specific subtypes of datums. 
    This schema encodes the Datum (CD_) package of the extended UML Model for OGC Abstract Specification Topic 2: Spatial Referencing by Coordinates. That UML model is adapted from ISO 19111 - Spatial referencing by coordinates, as described in Annex C of Topic 2. 
    Caution: The CRS package in GML 3.1 and GML 3.1.1 is preliminary, and is expected to undergo some modifications that are not backward compatible during the development of GML 3.2 (ISO 19136). The GML 3.2 package will implement the model described in the revised version of ISO 19111.
    
    GML is an OGC Standard.
    Copyright (c) 2001,2005,2010 Open Geospatial Consortium.
    To obtain additional rights of use, visit http://www.opengeospatial.org/legal/ .
    </rdfs:comment>
      <rdfs:seeAlso>urn:opengis:specification:gml:schema-xsd:coordinateOperations:3.1.1</rdfs:seeAlso>
      <rdfs:comment>How to encode coordinate operation definitions. Builds on referenceSystems.xsd to encode the data needed to define coordinate operations, including Transformations, Conversions, and other specific subtypes of operations. 
    
    This schema encodes the Coordinate Operation (CC_) package of the extended UML Model for OGC Abstract Specification Topic 2: Spatial Referencing by Coordinates. That UML model is adapted from ISO 19111 - Spatial referencing by coordinates, as described in Annex C of Topic 2. 
    Caution: The CRS package in GML 3.1 and GML 3.1.1 is preliminary, and is expected to undergo some modifications that are not backward compatible during the development of GML 3.2 (ISO 19136). The GML 3.2 package will implement the model described in the revised version of ISO 19111.
    
    GML is an OGC Standard.
    Copyright (c) 2001,2005,2010 Open Geospatial Consortium.
    To obtain additional rights of use, visit http://www.opengeospatial.org/legal/ .
    </rdfs:comment>
      <rdfs:seeAlso>urn:opengis:specification:gml:schema-xsd:dataQuality:3.1.1</rdfs:seeAlso>
      <rdfs:comment>How to encode positional data quality information. Builds on units.xsd to encode the data needed to describe the positional accuracy of coordinate operations. 
    This schema encodes the Data Quality (DQ) package of the extended UML Model for OGC Abstract Specification Topic 2: Spatial Referencing by Coordinates. That UML model is adapted from ISO 19111 - Spatial referencing by coordinates, as described in Annex C of Topic 2. 
    Caution: The CRS package in GML 3.1 and GML 3.1.1 is preliminary, and is expected to undergo some modifications that are not backward compatible during the development of GML 3.2 (ISO 19136). The GML 3.2 package will implement the model described in the revised version of ISO 19111. 
    
    GML is an OGC Standard.
    Copyright (c) 2001,2005,2010 Open Geospatial Consortium.
    To obtain additional rights of use, visit http://www.opengeospatial.org/legal/ .
    </rdfs:comment>
      <rdfs:comment>observation.xsd</rdfs:comment>
      <rdfs:seeAlso>urn:opengis:specification:gml:schema-xsd:observation:3.1.1</rdfs:seeAlso>
      <rdfs:comment>Observation schema for GML 3.1
      
      GML is an OGC Standard.
      Copyright (c) 2001,2005,2010 Open Geospatial Consortium.
      To obtain additional rights of use, visit http://www.opengeospatial.org/legal/ .
    </rdfs:comment>
      <rdfs:comment>defaultStyle.xsd</rdfs:comment>
      <rdfs:seeAlso>urn:opengis:specification:gml:schema-defaultStyle:v3.1.0</rdfs:seeAlso>
      <rdfs:comment>
      Default Style schema for GML 3.1.1
      
      GML is an OGC Standard.
      Copyright (c) 2001,2005,2010 Open Geospatial Consortium.
      To obtain additional rights of use, visit http://www.opengeospatial.org/legal/ .
    </rdfs:comment>
      <rdfs:seeAlso>urn:opengis:specification:gml:schema-xsd:temporalReferenceSystems:3.1.1</rdfs:seeAlso>
      <rdfs:comment xml:lang="en">The Temporal Reference Systems schema for GML 3.1 provides constructs for handling various styles of temporal reference system. 
    This schema reflects a partial implementation of the model described in ISO 19108:2002.
    
    GML is an OGC Standard.
    Copyright (c) 2001,2005,2010 Open Geospatial Consortium.
    To obtain additional rights of use, visit http://www.opengeospatial.org/legal/ .
    </rdfs:comment>
      <rdfs:seeAlso>urn:opengis:specification:gml:schema-xsd:temporalTopology:3.1.1</rdfs:seeAlso>
      <rdfs:comment xml:lang="en">The temporal topology schema for ISO19136 provides constructs for handling topological complexes and 
    temporal feature relationships. 
    Temporal geometric characteristics of features are represented as instants and periods. 
    While, temporal context of features that does not relate to the position of time is described as connectivity relationships 
    among instants and periods. These relationships are called temporal topology as they do not change in time, 
    as long as the direction of time does not change. 
    It is used effectively in the case of describing a family tree expressing evolution of species, an ecological cycle, 
    a lineage of lands or buildings, or a history of separation and merger of administrative boundaries.
    This schema reflects a partial yet consistent implementation of the model described in ISO 19108:2002.
    
    GML is an OGC Standard.
    Copyright (c) 2001,2005,2010 Open Geospatial Consortium.
    To obtain additional rights of use, visit http://www.opengeospatial.org/legal/ .
    </rdfs:comment>
   </owl:Ontology>
   <owl:Class rdf:about="http://www.opengis.net/gml#AbstractTimeSliceType">
      <rdfs:comment>This is an abstract class</rdfs:comment>
      <rdfs:comment xml:lang="en">A timeslice encapsulates the time-varying properties of a dynamic feature--it 
        must be extended to represent a timestamped projection of a feature. The dataSource 
        property describes how the temporal data was acquired.</rdfs:comment>
      <rdfs:subClassOf>
         <owl:Class>
            <owl:intersectionOf rdf:parseType="Collection">
               <owl:Restriction>
                  <owl:onProperty rdf:resource="http://www.opengis.net/gml#hasvalidTime"/>
                  <owl:allValuesFrom rdf:resource="http://www.opengis.net/gml#validTime"/>
               </owl:Restriction>
               <owl:Restriction>
                  <owl:onProperty rdf:resource="http://www.opengis.net/gml#hasdataSource"/>
                  <owl:allValuesFrom rdf:resource="http://www.opengis.net/gml#dataSource"/>
               </owl:Restriction>
               <owl:Restriction>
                  <owl:onProperty rdf:resource="http://www.opengis.net/gml#hasdataSource"/>
                  <owl:minCardinality rdf:datatype="http://www.w3.org/2001/XMLSchema#nonNegativeInteger">0</owl:minCardinality>
               </owl:Restriction>
            </owl:intersectionOf>
         </owl:Class>
      </rdfs:subClassOf>
      <rdfs:subClassOf rdf:resource="http://www.opengis.net/gml#AbstractGMLType"/>
   </owl:Class>
   <owl:Class rdf:about="http://www.opengis.net/gml#MovingObjectStatusType">
      <rdfs:comment xml:lang="en">This type encapsulates various dynamic properties of moving objects        
             (points, lines, regions). It is useful for dealing with features whose        
             geometry or topology changes over time.</rdfs:comment>
      <rdfs:subClassOf>
         <owl:Class>
            <owl:intersectionOf rdf:parseType="Collection">
               <owl:Restriction>
                  <owl:onProperty rdf:resource="http://www.opengis.net/gml#haslocation"/>
                  <owl:allValuesFrom rdf:resource="http://www.opengis.net/gml#location"/>
               </owl:Restriction>
               <owl:Restriction>
                  <owl:onProperty rdf:resource="http://www.opengis.net/gml#speed"/>
                  <owl:allValuesFrom rdf:resource="http://www.opengis.net/gml#MeasureType"/>
               </owl:Restriction>
               <owl:Restriction>
                  <owl:onProperty rdf:resource="http://www.opengis.net/gml#speed"/>
                  <owl:minCardinality rdf:datatype="http://www.w3.org/2001/XMLSchema#nonNegativeInteger">0</owl:minCardinality>
               </owl:Restriction>
               <owl:Restriction>
                  <owl:onProperty rdf:resource="http://www.opengis.net/gml#bearing"/>
                  <owl:allValuesFrom rdf:resource="http://www.opengis.net/gml#DirectionPropertyType"/>
               </owl:Restriction>
               <owl:Restriction>
                  <owl:onProperty rdf:resource="http://www.opengis.net/gml#bearing"/>
                  <owl:minCardinality rdf:datatype="http://www.w3.org/2001/XMLSchema#nonNegativeInteger">0</owl:minCardinality>
               </owl:Restriction>
               <owl:Restriction>
                  <owl:onProperty rdf:resource="http://www.opengis.net/gml#acceleration"/>
                  <owl:allValuesFrom rdf:resource="http://www.opengis.net/gml#MeasureType"/>
               </owl:Restriction>
               <owl:Restriction>
                  <owl:onProperty rdf:resource="http://www.opengis.net/gml#acceleration"/>
                  <owl:minCardinality rdf:datatype="http://www.w3.org/2001/XMLSchema#nonNegativeInteger">0</owl:minCardinality>
               </owl:Restriction>
               <owl:Restriction>
                  <owl:onProperty rdf:resource="http://www.opengis.net/gml#elevation"/>
                  <owl:allValuesFrom rdf:resource="http://www.opengis.net/gml#MeasureType"/>
               </owl:Restriction>
               <owl:Restriction>
                  <owl:onProperty rdf:resource="http://www.opengis.net/gml#elevation"/>
                  <owl:minCardinality rdf:datatype="http://www.w3.org/2001/XMLSchema#nonNegativeInteger">0</owl:minCardinality>
               </owl:Restriction>
               <owl:Restriction>
                  <owl:onProperty rdf:resource="http://www.opengis.net/gml#hasstatus"/>
                  <owl:allValuesFrom rdf:resource="http://www.opengis.net/gml#status"/>
               </owl:Restriction>
               <owl:Restriction>
                  <owl:onProperty rdf:resource="http://www.opengis.net/gml#hasstatus"/>
                  <owl:minCardinality rdf:datatype="http://www.w3.org/2001/XMLSchema#nonNegativeInteger">0</owl:minCardinality>
               </owl:Restriction>
            </owl:intersectionOf>
         </owl:Class>
      </rdfs:subClassOf>
      <rdfs:subClassOf rdf:resource="http://www.opengis.net/gml#AbstractTimeSliceType"/>
   </owl:Class>
   <owl:Class rdf:about="http://www.opengis.net/gml#HistoryPropertyType">
      <rdfs:comment xml:lang="en">The history relationship associates a feature with a sequence of TimeSlice instances.</rdfs:comment>
      <rdfs:subClassOf>
         <owl:Class>
            <owl:intersectionOf rdf:parseType="Collection">
               <owl:Restriction>
                  <owl:onProperty rdf:resource="http://www.opengis.net/gml#has_TimeSlice"/>
                  <owl:allValuesFrom rdf:resource="http://www.opengis.net/gml#_TimeSlice"/>
               </owl:Restriction>
            </owl:intersectionOf>
         </owl:Class>
      </rdfs:subClassOf>
   </owl:Class>
   <owl:Class rdf:about="http://www.opengis.net/gml#TrackType">
      <rdfs:comment xml:lang="en">The track of a moving object is a sequence of specialized timeslices        that indicate the status of the object.</rdfs:comment>
      <rdfs:subClassOf>
         <owl:Class>
            <owl:intersectionOf rdf:parseType="Collection">
               <owl:Restriction>
                  <owl:onProperty rdf:resource="http://www.opengis.net/gml#hasMovingObjectStatus"/>
                  <owl:allValuesFrom rdf:resource="http://www.opengis.net/gml#MovingObjectStatus"/>
               </owl:Restriction>
            </owl:intersectionOf>
         </owl:Class>
      </rdfs:subClassOf>
      <rdfs:subClassOf rdf:resource="http://www.opengis.net/gml#HistoryPropertyType"/>
   </owl:Class>
   <owl:Class rdf:about="http://www.opengis.net/gml#DynamicFeatureType">
      <rdfs:comment>A dynamic feature may possess a history and/or a timestamp.</rdfs:comment>
      <rdfs:subClassOf rdf:resource="http://www.opengis.net/gml#AbstractFeatureType"/>
   </owl:Class>
   <owl:Class rdf:about="http://www.opengis.net/gml#DynamicFeatureCollectionType">
      <rdfs:comment>A dynamic feature collection may possess a history and/or a timestamp.</rdfs:comment>
      <rdfs:subClassOf rdf:resource="http://www.opengis.net/gml#FeatureCollectionType"/>
   </owl:Class>
   <owl:Class rdf:about="http://www.opengis.net/gml#AbstractFeatureType">
      <rdfs:comment>This is an abstract class</rdfs:comment>
      <rdfs:comment>An abstract feature provides a set of common properties, including id, metaDataProperty, name and description inherited from AbstractGMLType, plus boundedBy.    A concrete feature type must derive from this type and specify additional  properties in an application schema. A feature must possess an identifying attribute ('id' - 'fid' has been deprecated).</rdfs:comment>
      <rdfs:subClassOf>
         <owl:Class>
            <owl:intersectionOf rdf:parseType="Collection">
               <owl:Restriction>
                  <owl:onProperty rdf:resource="http://www.opengis.net/gml#hasboundedBy"/>
                  <owl:allValuesFrom rdf:resource="http://www.opengis.net/gml#boundedBy"/>
               </owl:Restriction>
               <owl:Restriction>
                  <owl:onProperty rdf:resource="http://www.opengis.net/gml#hasboundedBy"/>
                  <owl:minCardinality rdf:datatype="http://www.w3.org/2001/XMLSchema#nonNegativeInteger">0</owl:minCardinality>
               </owl:Restriction>
               <owl:Restriction>
                  <owl:onProperty rdf:resource="http://www.opengis.net/gml#haslocation"/>
                  <owl:allValuesFrom rdf:resource="http://www.opengis.net/gml#location"/>
               </owl:Restriction>
               <owl:Restriction>
                  <owl:onProperty rdf:resource="http://www.opengis.net/gml#haslocation"/>
                  <owl:minCardinality rdf:datatype="http://www.w3.org/2001/XMLSchema#nonNegativeInteger">0</owl:minCardinality>
               </owl:Restriction>
            </owl:intersectionOf>
         </owl:Class>
      </rdfs:subClassOf>
      <rdfs:subClassOf rdf:resource="http://www.opengis.net/gml#AbstractGMLType"/>
   </owl:Class>
   <owl:Class rdf:about="http://www.opengis.net/gml#BoundingShapeType">
      <rdfs:comment>Bounding shape.</rdfs:comment>
      <owl:disjointUnionOf rdf:parseType="Collection">
         <owl:Restriction>
            <owl:onProperty rdf:resource="http://www.opengis.net/gml#hasEnvelope"/>
            <owl:someValuesFrom rdf:resource="http://www.opengis.net/gml#Envelope"/>
         </owl:Restriction>
         <owl:Restriction>
            <owl:onProperty rdf:resource="http://www.opengis.net/gml#hasNull"/>
            <owl:someValuesFrom rdf:resource="http://www.opengis.net/gml#Null"/>
         </owl:Restriction>
      </owl:disjointUnionOf>
   </owl:Class>
   <owl:Class rdf:about="http://www.opengis.net/gml#EnvelopeWithTimePeriodType">
      <rdfs:comment>Envelope that includes also a temporal extent.</rdfs:comment>
      <rdfs:subClassOf>
         <owl:Class>
            <owl:intersectionOf rdf:parseType="Collection">
               <owl:Restriction>
                  <owl:onProperty rdf:resource="http://www.opengis.net/gml#hastimePosition"/>
                  <owl:allValuesFrom rdf:resource="http://www.opengis.net/gml#timePosition"/>
               </owl:Restriction>
               <owl:Restriction>
                  <owl:onProperty rdf:resource="http://www.opengis.net/gml#hastimePosition"/>
                  <owl:cardinality rdf:datatype="http://www.w3.org/2001/XMLSchema#nonNegativeInteger">2</owl:cardinality>
               </owl:Restriction>
            </owl:intersectionOf>
         </owl:Class>
      </rdfs:subClassOf>
      <rdfs:subClassOf>
         <owl:Class>
            <owl:intersectionOf rdf:parseType="Collection">
               <owl:Restriction>
                  <owl:onProperty rdf:resource="http://www.opengis.net/gml#frame"/>
                  <owl:allValuesFrom rdf:resource="http://www.w3.org/2001/XMLSchema#anyURI"/>
               </owl:Restriction>
            </owl:intersectionOf>
         </owl:Class>
      </rdfs:subClassOf>
      <rdfs:subClassOf rdf:resource="http://www.opengis.net/gml#EnvelopeType"/>
   </owl:Class>
   <owl:Class rdf:about="http://www.opengis.net/gml#FeaturePropertyType">
      <rdfs:comment>Container for a feature - follow gml:AssociationType pattern.</rdfs:comment>
      <rdfs:subClassOf>
         <owl:Class>
            <owl:intersectionOf rdf:parseType="Collection">
               <owl:Restriction>
                  <owl:onProperty rdf:resource="http://www.opengis.net/gml#has_Feature"/>
                  <owl:allValuesFrom rdf:resource="http://www.opengis.net/gml#_Feature"/>
               </owl:Restriction>
            </owl:intersectionOf>
         </owl:Class>
      </rdfs:subClassOf>
   </owl:Class>
   <owl:Class rdf:about="http://www.opengis.net/gml#FeatureArrayPropertyType">
      <rdfs:comment>Container for features - follow gml:ArrayAssociationType pattern.</rdfs:comment>
      <rdfs:subClassOf>
         <owl:Class>
            <owl:intersectionOf rdf:parseType="Collection">
               <owl:Restriction>
                  <owl:onProperty rdf:resource="http://www.opengis.net/gml#has_Feature"/>
                  <owl:allValuesFrom rdf:resource="http://www.opengis.net/gml#_Feature"/>
               </owl:Restriction>
               <owl:Restriction>
                  <owl:onProperty rdf:resource="http://www.opengis.net/gml#has_Feature"/>
                  <owl:minCardinality rdf:datatype="http://www.w3.org/2001/XMLSchema#nonNegativeInteger">0</owl:minCardinality>
               </owl:Restriction>
            </owl:intersectionOf>
         </owl:Class>
      </rdfs:subClassOf>
   </owl:Class>
   <owl:Class rdf:about="http://www.opengis.net/gml#AbstractFeatureCollectionType">
      <rdfs:comment>This is an abstract class</rdfs:comment>
      <rdfs:comment>A feature collection contains zero or more features.</rdfs:comment>
      <rdfs:subClassOf>
         <owl:Class>
            <owl:intersectionOf rdf:parseType="Collection">
               <owl:Restriction>
                  <owl:onProperty rdf:resource="http://www.opengis.net/gml#hasfeatureMember"/>
                  <owl:allValuesFrom rdf:resource="http://www.opengis.net/gml#featureMember"/>
               </owl:Restriction>
               <owl:Restriction>
                  <owl:onProperty rdf:resource="http://www.opengis.net/gml#hasfeatureMember"/>
                  <owl:minCardinality rdf:datatype="http://www.w3.org/2001/XMLSchema#nonNegativeInteger">0</owl:minCardinality>
               </owl:Restriction>
               <owl:Restriction>
                  <owl:onProperty rdf:resource="http://www.opengis.net/gml#hasfeatureMembers"/>
                  <owl:allValuesFrom rdf:resource="http://www.opengis.net/gml#featureMembers"/>
               </owl:Restriction>
               <owl:Restriction>
                  <owl:onProperty rdf:resource="http://www.opengis.net/gml#hasfeatureMembers"/>
                  <owl:minCardinality rdf:datatype="http://www.w3.org/2001/XMLSchema#nonNegativeInteger">0</owl:minCardinality>
               </owl:Restriction>
            </owl:intersectionOf>
         </owl:Class>
      </rdfs:subClassOf>
      <rdfs:subClassOf rdf:resource="http://www.opengis.net/gml#AbstractFeatureType"/>
   </owl:Class>
   <owl:Class rdf:about="http://www.opengis.net/gml#FeatureCollectionType">
      <rdfs:comment>Concrete generic feature collection.</rdfs:comment>
      <rdfs:subClassOf rdf:resource="http://www.opengis.net/gml#AbstractFeatureCollectionType"/>
   </owl:Class>
   <owl:Class rdf:about="http://www.opengis.net/gml#BoundedFeatureType">
      <rdfs:comment>This is an abstract class</rdfs:comment>
      <rdfs:comment>Makes boundedBy mandatory</rdfs:comment>
      <rdfs:subClassOf>
         <owl:Class>
            <owl:intersectionOf rdf:parseType="Collection">
               <owl:Restriction>
                  <owl:onProperty rdf:resource="http://www.opengis.net/gml#hasboundedBy"/>
                  <owl:allValuesFrom rdf:resource="http://www.opengis.net/gml#boundedBy"/>
               </owl:Restriction>
               <owl:Restriction>
                  <owl:onProperty rdf:resource="http://www.opengis.net/gml#haslocation"/>
                  <owl:allValuesFrom rdf:resource="http://www.opengis.net/gml#location"/>
               </owl:Restriction>
               <owl:Restriction>
                  <owl:onProperty rdf:resource="http://www.opengis.net/gml#haslocation"/>
                  <owl:minCardinality rdf:datatype="http://www.w3.org/2001/XMLSchema#nonNegativeInteger">0</owl:minCardinality>
               </owl:Restriction>
            </owl:intersectionOf>
         </owl:Class>
      </rdfs:subClassOf>
      <rdfs:subClassOf rdf:resource="http://www.opengis.net/gml#StandardObjectProperties"/>
      <rdfs:subClassOf rdf:resource="http://www.opengis.net/gml#AbstractFeatureType"/>
   </owl:Class>
   <owl:Class rdf:about="http://www.opengis.net/gml#LocationPropertyType">
      <rdfs:comment>Convenience property for generalised location.  
      A representative location for plotting or analysis.  
      Often augmented by one or more additional geometry properties with more specific semantics.</rdfs:comment>
      <rdfs:comment>Deprecated in GML 3.1.0</rdfs:comment>
      <owl:disjointUnionOf rdf:parseType="Collection">
         <owl:Restriction>
            <owl:onProperty rdf:resource="http://www.opengis.net/gml#has_Geometry"/>
            <owl:someValuesFrom rdf:resource="http://www.opengis.net/gml#_Geometry"/>
         </owl:Restriction>
         <owl:Restriction>
            <owl:onProperty rdf:resource="http://www.opengis.net/gml#hasLocationKeyWord"/>
            <owl:someValuesFrom rdf:resource="http://www.opengis.net/gml#LocationKeyWord"/>
         </owl:Restriction>
         <owl:Restriction>
            <owl:onProperty rdf:resource="http://www.opengis.net/gml#hasLocationString"/>
            <owl:someValuesFrom rdf:resource="http://www.opengis.net/gml#LocationString"/>
         </owl:Restriction>
         <owl:Restriction>
            <owl:onProperty rdf:resource="http://www.opengis.net/gml#hasNull"/>
            <owl:someValuesFrom rdf:resource="http://www.opengis.net/gml#Null"/>
         </owl:Restriction>
      </owl:disjointUnionOf>
   </owl:Class>
   <owl:Class rdf:about="http://www.opengis.net/gml#PriorityLocationPropertyType">
      <rdfs:comment>G-XML component</rdfs:comment>
      <rdfs:comment>Deprecated in GML 3.1.0</rdfs:comment>
      <rdfs:subClassOf>
         <owl:Class>
            <owl:intersectionOf rdf:parseType="Collection">
               <owl:Restriction>
                  <owl:onProperty rdf:resource="http://www.opengis.net/gml#priority"/>
                  <owl:allValuesFrom rdf:resource="http://www.w3.org/2001/XMLSchema#string"/>
               </owl:Restriction>
            </owl:intersectionOf>
         </owl:Class>
      </rdfs:subClassOf>
      <rdfs:subClassOf rdf:resource="http://www.opengis.net/gml#LocationPropertyType"/>
   </owl:Class>
   <owl:Class rdf:about="http://www.opengis.net/gml#AbstractSurfaceType">
      <rdfs:comment>An abstraction of a surface to support the different levels of complexity. A surface is always a continuous region of a plane.</rdfs:comment>
      <rdfs:subClassOf rdf:resource="http://www.opengis.net/gml#AbstractGeometricPrimitiveType"/>
   </owl:Class>
   <owl:Class rdf:about="http://www.opengis.net/gml#SurfacePropertyType">
      <rdfs:comment>A property that has a surface as its value domain can either be an appropriate geometry element encapsulated in an element of this type or an XLink reference to a remote geometry element (where remote includes geometry elements located elsewhere in the same document). Either the reference or the contained element must be given, but neither both nor none.</rdfs:comment>
      <rdfs:subClassOf>
         <owl:Class>
            <owl:intersectionOf rdf:parseType="Collection">
               <owl:Restriction>
                  <owl:onProperty rdf:resource="http://www.opengis.net/gml#has_Surface"/>
                  <owl:allValuesFrom rdf:resource="http://www.opengis.net/gml#_Surface"/>
               </owl:Restriction>
            </owl:intersectionOf>
         </owl:Class>
      </rdfs:subClassOf>
   </owl:Class>
   <owl:Class rdf:about="http://www.opengis.net/gml#SurfaceArrayPropertyType">
      <rdfs:comment>A container for an array of surfaces. The elements are always contained in the array property, referencing geometry elements or arrays of geometry elements is not supported.</rdfs:comment>
      <rdfs:subClassOf>
         <owl:Class>
            <owl:intersectionOf rdf:parseType="Collection">
               <owl:Restriction>
                  <owl:onProperty rdf:resource="http://www.opengis.net/gml#has_Surface"/>
                  <owl:allValuesFrom rdf:resource="http://www.opengis.net/gml#_Surface"/>
               </owl:Restriction>
               <owl:Restriction>
                  <owl:onProperty rdf:resource="http://www.opengis.net/gml#has_Surface"/>
                  <owl:minCardinality rdf:datatype="http://www.w3.org/2001/XMLSchema#nonNegativeInteger">0</owl:minCardinality>
               </owl:Restriction>
            </owl:intersectionOf>
         </owl:Class>
      </rdfs:subClassOf>
   </owl:Class>
   <owl:Class rdf:about="http://www.opengis.net/gml#PolygonType">
      <rdfs:comment>A Polygon is a special surface that is defined by a single surface patch. The boundary of this patch is coplanar and the polygon uses planar interpolation in its interior. It is backwards compatible with the Polygon of GML 2, GM_Polygon of ISO 19107 is implemented by PolygonPatch.</rdfs:comment>
      <rdfs:subClassOf>
         <owl:Class>
            <owl:intersectionOf rdf:parseType="Collection">
               <owl:Restriction>
                  <owl:onProperty rdf:resource="http://www.opengis.net/gml#hasexterior"/>
                  <owl:allValuesFrom rdf:resource="http://www.opengis.net/gml#exterior"/>
               </owl:Restriction>
               <owl:Restriction>
                  <owl:onProperty rdf:resource="http://www.opengis.net/gml#hasexterior"/>
                  <owl:minCardinality rdf:datatype="http://www.w3.org/2001/XMLSchema#nonNegativeInteger">0</owl:minCardinality>
               </owl:Restriction>
               <owl:Restriction>
                  <owl:onProperty rdf:resource="http://www.opengis.net/gml#hasinterior"/>
                  <owl:allValuesFrom rdf:resource="http://www.opengis.net/gml#interior"/>
               </owl:Restriction>
               <owl:Restriction>
                  <owl:onProperty rdf:resource="http://www.opengis.net/gml#hasinterior"/>
                  <owl:minCardinality rdf:datatype="http://www.w3.org/2001/XMLSchema#nonNegativeInteger">0</owl:minCardinality>
               </owl:Restriction>
            </owl:intersectionOf>
         </owl:Class>
      </rdfs:subClassOf>
      <rdfs:subClassOf rdf:resource="http://www.opengis.net/gml#AbstractSurfaceType"/>
   </owl:Class>
   <owl:Class rdf:about="http://www.opengis.net/gml#AbstractRingType">
      <rdfs:comment>This is an abstract class</rdfs:comment>
      <rdfs:comment>An abstraction of a ring to support surface boundaries of different complexity.</rdfs:comment>
      <rdfs:subClassOf rdf:resource="http://www.opengis.net/gml#AbstractGeometryType"/>
   </owl:Class>
   <owl:Class rdf:about="http://www.opengis.net/gml#AbstractRingPropertyType">
      <rdfs:comment>Encapsulates a ring to represent the surface boundary property of a surface.</rdfs:comment>
      <rdfs:subClassOf>
         <owl:Class>
            <owl:intersectionOf rdf:parseType="Collection">
               <owl:Restriction>
                  <owl:onProperty rdf:resource="http://www.opengis.net/gml#has_Ring"/>
                  <owl:allValuesFrom rdf:resource="http://www.opengis.net/gml#_Ring"/>
               </owl:Restriction>
            </owl:intersectionOf>
         </owl:Class>
      </rdfs:subClassOf>
   </owl:Class>
   <owl:Class rdf:about="http://www.opengis.net/gml#LinearRingType">
      <rdfs:comment>A LinearRing is defined by four or more coordinate tuples, with linear interpolation between them; the first and last coordinates must be coincident.</rdfs:comment>
      <owl:disjointUnionOf rdf:parseType="Collection">
         <owl:Restriction>
            <owl:onProperty rdf:resource="http://www.opengis.net/gml#hasposList"/>
            <owl:someValuesFrom rdf:resource="http://www.opengis.net/gml#posList"/>
         </owl:Restriction>
         <owl:Restriction>
            <owl:onProperty rdf:resource="http://www.opengis.net/gml#hascoordinates"/>
            <owl:someValuesFrom rdf:resource="http://www.opengis.net/gml#coordinates"/>
         </owl:Restriction>
         <owl:Restriction>
            <owl:onProperty rdf:resource="http://www.opengis.net/gml#hascoord"/>
            <owl:someValuesFrom rdf:resource="http://www.opengis.net/gml#coord"/>
         </owl:Restriction>
         <owl:Restriction>
            <owl:onProperty rdf:resource="http://www.opengis.net/gml#hascoord"/>
            <owl:minCardinality rdf:datatype="http://www.w3.org/2001/XMLSchema#nonNegativeInteger">4</owl:minCardinality>
         </owl:Restriction>
         <owl:Restriction>
            <owl:onProperty rdf:resource="http://www.opengis.net/gml#haspos"/>
            <owl:someValuesFrom rdf:resource="http://www.opengis.net/gml#pos"/>
         </owl:Restriction>
         <owl:Restriction>
            <owl:onProperty rdf:resource="http://www.opengis.net/gml#haspointProperty"/>
            <owl:someValuesFrom rdf:resource="http://www.opengis.net/gml#pointProperty"/>
         </owl:Restriction>
         <owl:Restriction>
            <owl:onProperty rdf:resource="http://www.opengis.net/gml#haspointRep"/>
            <owl:someValuesFrom rdf:resource="http://www.opengis.net/gml#pointRep"/>
         </owl:Restriction>
      </owl:disjointUnionOf>
      <rdfs:subClassOf rdf:resource="http://www.opengis.net/gml#AbstractRingType"/>
   </owl:Class>
   <owl:Class rdf:about="http://www.opengis.net/gml#LinearRingPropertyType">
      <rdfs:comment>Encapsulates a ring to represent properties in features or geometry collections.</rdfs:comment>
      <owl:disjointUnionOf rdf:parseType="Collection">
         <owl:Restriction>
            <owl:onProperty rdf:resource="http://www.opengis.net/gml#hasLinearRing"/>
            <owl:someValuesFrom rdf:resource="http://www.opengis.net/gml#LinearRing"/>
         </owl:Restriction>
      </owl:disjointUnionOf>
   </owl:Class>
   <owl:Class rdf:about="http://www.opengis.net/gml#PolygonPropertyType">
      <rdfs:comment>This type is deprecated with GML 3 and shall not be used. It is included for backwards compatibility with GML 2. Use SurfacePropertyType instead.
A property that has a polygon as its value domain can either be an appropriate geometry element encapsulated in an element of this type or an XLink reference to a remote geometry element (where remote includes geometry elements located elsewhere in the same document). Either the reference or the contained element must be given, but neither both nor none.</rdfs:comment>
      <rdfs:subClassOf>
         <owl:Class>
            <owl:intersectionOf rdf:parseType="Collection">
               <owl:Restriction>
                  <owl:onProperty rdf:resource="http://www.opengis.net/gml#hasPolygon"/>
                  <owl:allValuesFrom rdf:resource="http://www.opengis.net/gml#Polygon"/>
               </owl:Restriction>
            </owl:intersectionOf>
         </owl:Class>
      </rdfs:subClassOf>
   </owl:Class>
   <owl:Class rdf:about="http://www.opengis.net/gml#GeometryPropertyType">
      <rdfs:comment>A geometric property can either be any geometry element encapsulated in an element of this type or an XLink reference 
      to a remote geometry element (where remote includes geometry elements located elsewhere in the same document). Note that either 
      the reference or the contained element must be given, but not both or none.</rdfs:comment>
      <rdfs:subClassOf>
         <owl:Class>
            <owl:intersectionOf rdf:parseType="Collection">
               <owl:Restriction>
                  <owl:onProperty rdf:resource="http://www.opengis.net/gml#has_Geometry"/>
                  <owl:allValuesFrom rdf:resource="http://www.opengis.net/gml#_Geometry"/>
               </owl:Restriction>
            </owl:intersectionOf>
         </owl:Class>
      </rdfs:subClassOf>
   </owl:Class>
   <owl:Class rdf:about="http://www.opengis.net/gml#GeometryArrayPropertyType">
      <rdfs:comment>A container for an array of geometry elements. The elements are always contained in the array property, 
      referencing geometry elements or arrays of geometry elements is not supported.</rdfs:comment>
      <rdfs:subClassOf>
         <owl:Class>
            <owl:intersectionOf rdf:parseType="Collection">
               <owl:Restriction>
                  <owl:onProperty rdf:resource="http://www.opengis.net/gml#has_Geometry"/>
                  <owl:allValuesFrom rdf:resource="http://www.opengis.net/gml#_Geometry"/>
               </owl:Restriction>
               <owl:Restriction>
                  <owl:onProperty rdf:resource="http://www.opengis.net/gml#has_Geometry"/>
                  <owl:minCardinality rdf:datatype="http://www.w3.org/2001/XMLSchema#nonNegativeInteger">0</owl:minCardinality>
               </owl:Restriction>
            </owl:intersectionOf>
         </owl:Class>
      </rdfs:subClassOf>
   </owl:Class>
   <owl:Class rdf:about="http://www.opengis.net/gml#AbstractGeometryType">
      <rdfs:comment>This is an abstract class</rdfs:comment>
      <rdfs:comment>All geometry elements are derived directly or indirectly from this abstract supertype. A geometry element may 
      have an identifying attribute ("gml:id"), a name (attribute "name") and a description (attribute "description"). It may be associated 
      with a spatial reference system (attribute "srsName"). The following rules shall be adhered: - Every geometry type shall derive 
      from this abstract type. - Every geometry element (i.e. an element of a geometry type) shall be directly or indirectly in the 
      substitution group of _Geometry.</rdfs:comment>
      <rdfs:subClassOf>
         <owl:Class>
            <owl:intersectionOf rdf:parseType="Collection">
               <owl:Restriction>
                  <owl:onProperty rdf:resource="http://www.opengis.net/gml#gid"/>
                  <owl:allValuesFrom rdf:resource="http://www.w3.org/2001/XMLSchema#string"/>
               </owl:Restriction>
            </owl:intersectionOf>
         </owl:Class>
      </rdfs:subClassOf>
      <rdfs:subClassOf rdf:resource="http://www.opengis.net/gml#AbstractGMLType"/>
   </owl:Class>
   <owl:Class rdf:about="http://www.opengis.net/gml#AbstractGeometricPrimitiveType">
      <rdfs:comment>This is an abstract class</rdfs:comment>
      <rdfs:comment>This is the abstract root type of the geometric primitives. A geometric primitive is a geometric object that is not 
      decomposed further into other primitives in the system. All primitives are oriented in the direction implied by the sequence of their 
      coordinate tuples.</rdfs:comment>
      <rdfs:subClassOf rdf:resource="http://www.opengis.net/gml#AbstractGeometryType"/>
   </owl:Class>
   <owl:Class rdf:about="http://www.opengis.net/gml#GeometricPrimitivePropertyType">
      <rdfs:comment>A property that has a geometric primitive as its value domain can either be an appropriate geometry element 
      encapsulated in an element of this type or an XLink reference to a remote geometry element (where remote includes geometry 
      elements located elsewhere in the same document). Either the reference or the contained element must be given, but neither 
      both nor none.</rdfs:comment>
      <rdfs:subClassOf>
         <owl:Class>
            <owl:intersectionOf rdf:parseType="Collection">
               <owl:Restriction>
                  <owl:onProperty rdf:resource="http://www.opengis.net/gml#has_GeometricPrimitive"/>
                  <owl:allValuesFrom rdf:resource="http://www.opengis.net/gml#_GeometricPrimitive"/>
               </owl:Restriction>
            </owl:intersectionOf>
         </owl:Class>
      </rdfs:subClassOf>
   </owl:Class>
   <owl:Class rdf:about="http://www.opengis.net/gml#PointType">
      <rdfs:comment>A Point is defined by a single coordinate tuple.</rdfs:comment>
      <owl:disjointUnionOf rdf:parseType="Collection">
         <owl:Restriction>
            <owl:onProperty rdf:resource="http://www.opengis.net/gml#haspos"/>
            <owl:someValuesFrom rdf:resource="http://www.opengis.net/gml#pos"/>
         </owl:Restriction>
         <owl:Restriction>
            <owl:onProperty rdf:resource="http://www.opengis.net/gml#hascoordinates"/>
            <owl:someValuesFrom rdf:resource="http://www.opengis.net/gml#coordinates"/>
         </owl:Restriction>
         <owl:Restriction>
            <owl:onProperty rdf:resource="http://www.opengis.net/gml#hascoord"/>
            <owl:someValuesFrom rdf:resource="http://www.opengis.net/gml#coord"/>
         </owl:Restriction>
      </owl:disjointUnionOf>
      <rdfs:subClassOf rdf:resource="http://www.opengis.net/gml#AbstractGeometricPrimitiveType"/>
   </owl:Class>
   <owl:Class rdf:about="http://www.opengis.net/gml#PointPropertyType">
      <rdfs:comment>A property that has a point as its value domain can either be an appropriate geometry element encapsulated in an 
      element of this type or an XLink reference to a remote geometry element (where remote includes geometry elements located 
      elsewhere in the same document). Either the reference or the contained element must be given, but neither both nor none.</rdfs:comment>
      <rdfs:subClassOf>
         <owl:Class>
            <owl:intersectionOf rdf:parseType="Collection">
               <owl:Restriction>
                  <owl:onProperty rdf:resource="http://www.opengis.net/gml#hasPoint"/>
                  <owl:allValuesFrom rdf:resource="http://www.opengis.net/gml#Point"/>
               </owl:Restriction>
            </owl:intersectionOf>
         </owl:Class>
      </rdfs:subClassOf>
   </owl:Class>
   <owl:Class rdf:about="http://www.opengis.net/gml#PointArrayPropertyType">
      <rdfs:comment>A container for an array of points. The elements are always contained in the array property, referencing geometry 
      elements or arrays of geometry elements is not supported.</rdfs:comment>
      <rdfs:subClassOf>
         <owl:Class>
            <owl:intersectionOf rdf:parseType="Collection">
               <owl:Restriction>
                  <owl:onProperty rdf:resource="http://www.opengis.net/gml#hasPoint"/>
                  <owl:allValuesFrom rdf:resource="http://www.opengis.net/gml#Point"/>
               </owl:Restriction>
               <owl:Restriction>
                  <owl:onProperty rdf:resource="http://www.opengis.net/gml#hasPoint"/>
                  <owl:minCardinality rdf:datatype="http://www.w3.org/2001/XMLSchema#nonNegativeInteger">0</owl:minCardinality>
               </owl:Restriction>
            </owl:intersectionOf>
         </owl:Class>
      </rdfs:subClassOf>
   </owl:Class>
   <owl:Class rdf:about="http://www.opengis.net/gml#AbstractCurveType">
      <rdfs:comment>This is an abstract class</rdfs:comment>
      <rdfs:comment>An abstraction of a curve to support the different levels of complexity. The curve can always be viewed as a geometric 
      primitive, i.e. is continuous.</rdfs:comment>
      <rdfs:subClassOf rdf:resource="http://www.opengis.net/gml#AbstractGeometricPrimitiveType"/>
   </owl:Class>
   <owl:Class rdf:about="http://www.opengis.net/gml#CurvePropertyType">
      <rdfs:comment>A property that has a curve as its value domain can either be an appropriate geometry element encapsulated in an 
      element of this type or an XLink reference to a remote geometry element (where remote includes geometry elements located elsewhere 
      in the same document). Either the reference or the contained element must be given, but neither both nor none.</rdfs:comment>
      <rdfs:subClassOf>
         <owl:Class>
            <owl:intersectionOf rdf:parseType="Collection">
               <owl:Restriction>
                  <owl:onProperty rdf:resource="http://www.opengis.net/gml#has_Curve"/>
                  <owl:allValuesFrom rdf:resource="http://www.opengis.net/gml#_Curve"/>
               </owl:Restriction>
            </owl:intersectionOf>
         </owl:Class>
      </rdfs:subClassOf>
   </owl:Class>
   <owl:Class rdf:about="http://www.opengis.net/gml#CurveArrayPropertyType">
      <rdfs:comment>A container for an array of curves. The elements are always contained in the array property, referencing geometry elements 
      or arrays of geometry elements is not supported.</rdfs:comment>
      <rdfs:subClassOf>
         <owl:Class>
            <owl:intersectionOf rdf:parseType="Collection">
               <owl:Restriction>
                  <owl:onProperty rdf:resource="http://www.opengis.net/gml#has_Curve"/>
                  <owl:allValuesFrom rdf:resource="http://www.opengis.net/gml#_Curve"/>
               </owl:Restriction>
               <owl:Restriction>
                  <owl:onProperty rdf:resource="http://www.opengis.net/gml#has_Curve"/>
                  <owl:minCardinality rdf:datatype="http://www.w3.org/2001/XMLSchema#nonNegativeInteger">0</owl:minCardinality>
               </owl:Restriction>
            </owl:intersectionOf>
         </owl:Class>
      </rdfs:subClassOf>
   </owl:Class>
   <owl:Class rdf:about="http://www.opengis.net/gml#LineStringType">
      <rdfs:comment>A LineString is a special curve that consists of a single segment with linear interpolation. It is defined by two or more coordinate 
      tuples, with linear interpolation between them. It is backwards compatible with the LineString of GML 2, GM_LineString of ISO 19107 is 
      implemented by LineStringSegment.</rdfs:comment>
      <owl:disjointUnionOf rdf:parseType="Collection">
         <owl:Restriction>
            <owl:onProperty rdf:resource="http://www.opengis.net/gml#hasposList"/>
            <owl:someValuesFrom rdf:resource="http://www.opengis.net/gml#posList"/>
         </owl:Restriction>
         <owl:Restriction>
            <owl:onProperty rdf:resource="http://www.opengis.net/gml#hascoordinates"/>
            <owl:someValuesFrom rdf:resource="http://www.opengis.net/gml#coordinates"/>
         </owl:Restriction>
         <owl:Restriction>
            <owl:onProperty rdf:resource="http://www.opengis.net/gml#haspos"/>
            <owl:someValuesFrom rdf:resource="http://www.opengis.net/gml#pos"/>
         </owl:Restriction>
         <owl:Restriction>
            <owl:onProperty rdf:resource="http://www.opengis.net/gml#haspointProperty"/>
            <owl:someValuesFrom rdf:resource="http://www.opengis.net/gml#pointProperty"/>
         </owl:Restriction>
         <owl:Restriction>
            <owl:onProperty rdf:resource="http://www.opengis.net/gml#haspointRep"/>
            <owl:someValuesFrom rdf:resource="http://www.opengis.net/gml#pointRep"/>
         </owl:Restriction>
         <owl:Restriction>
            <owl:onProperty rdf:resource="http://www.opengis.net/gml#hascoord"/>
            <owl:someValuesFrom rdf:resource="http://www.opengis.net/gml#coord"/>
         </owl:Restriction>
      </owl:disjointUnionOf>
      <rdfs:subClassOf rdf:resource="http://www.opengis.net/gml#AbstractCurveType"/>
   </owl:Class>
   <owl:Class rdf:about="http://www.opengis.net/gml#DirectPositionType">
      <rdfs:comment>DirectPosition instances hold the coordinates for a position within some coordinate reference system (CRS). Since 
      DirectPositions, as data types, will often be included in larger objects (such as geometry elements) that have references to CRS, the 
      "srsName" attribute will in general be missing, if this particular DirectPosition is included in a larger element with such a reference to a 
      CRS. In this case, the CRS is implicitly assumed to take on the value of the containing object's CRS.</rdfs:comment>
      <rdfs:subClassOf>
         <owl:Restriction>
            <owl:onProperty rdf:resource="http://www.opengis.net/gml#hasdoubleList"/>
            <owl:someValuesFrom rdf:resource="doubleList"/>
         </owl:Restriction>
      </rdfs:subClassOf>
   </owl:Class>
   <owl:DatatypeProperty rdf:about="http://www.opengis.net/gml#hasdoubleList">
      <rdfs:domain rdf:resource="http://www.opengis.net/gml#DirectPositionType"/>
      <rdfs:range rdf:resource="http://www.opengis.net/gml#doubleList"/>
   </owl:DatatypeProperty>
   <owl:Class rdf:about="http://www.opengis.net/gml#DirectPositionListType">
      <rdfs:comment>DirectPositionList instances hold the coordinates for a sequence of direct positions within the same coordinate 
      reference system (CRS).</rdfs:comment>
      <rdfs:subClassOf>
         <owl:Class>
            <owl:intersectionOf rdf:parseType="Collection">
               <owl:Restriction>
                  <owl:onProperty rdf:resource="http://www.opengis.net/gml#count"/>
                  <owl:allValuesFrom rdf:resource="http://www.w3.org/2001/XMLSchema#positiveInteger"/>
               </owl:Restriction>
            </owl:intersectionOf>
         </owl:Class>
      </rdfs:subClassOf>
      <rdfs:subClassOf>
         <owl:Restriction>
            <owl:onProperty rdf:resource="http://www.opengis.net/gml#hasdoubleList"/>
            <owl:someValuesFrom rdf:resource="doubleList"/>
         </owl:Restriction>
      </rdfs:subClassOf>
   </owl:Class>
   <owl:DatatypeProperty rdf:about="http://www.opengis.net/gml#hasdoubleList">
      <rdfs:domain rdf:resource="http://www.opengis.net/gml#DirectPositionListType"/>
      <rdfs:range rdf:resource="http://www.opengis.net/gml#doubleList"/>
   </owl:DatatypeProperty>
   <owl:Class rdf:about="http://www.opengis.net/gml#VectorType">
      <rdfs:comment>Vector instances hold the compoents for a (usually spatial) vector within some coordinate reference system (CRS). 
      Since Vectors will often be included in larger objects that have references to CRS, the "srsName" attribute may be missing. 
      In this case, the CRS is implicitly assumed to take on the value of the containing object's CRS.

      Note that this content model is the same as DirectPositionType, but is defined separately to reflect the distinct semantics, and to avoid validation problems. SJDC 2004-12-02</rdfs:comment>
      <rdfs:subClassOf>
         <owl:Restriction>
            <owl:onProperty rdf:resource="http://www.opengis.net/gml#hasdoubleList"/>
            <owl:someValuesFrom rdf:resource="doubleList"/>
         </owl:Restriction>
      </rdfs:subClassOf>
   </owl:Class>
   <owl:DatatypeProperty rdf:about="http://www.opengis.net/gml#hasdoubleList">
      <rdfs:domain rdf:resource="http://www.opengis.net/gml#VectorType"/>
      <rdfs:range rdf:resource="http://www.opengis.net/gml#doubleList"/>
   </owl:DatatypeProperty>
   <owl:Class rdf:about="http://www.opengis.net/gml#EnvelopeType">
      <rdfs:comment>Envelope defines an extent using a pair of positions defining opposite corners in arbitrary dimensions. The first direct 
      position is the "lower corner" (a coordinate position consisting of all the minimal ordinates for each dimension for all points within the envelope), 
      the second one the "upper corner" (a coordinate position consisting of all the maximal ordinates for each dimension for all points within the 
      envelope).</rdfs:comment>
      <owl:disjointUnionOf rdf:parseType="Collection">
         <owl:Restriction>
            <owl:onProperty rdf:resource="http://www.opengis.net/gml#hascoord"/>
            <owl:someValuesFrom rdf:resource="http://www.opengis.net/gml#coord"/>
         </owl:Restriction>
         <owl:Restriction>
            <owl:onProperty rdf:resource="http://www.opengis.net/gml#hascoord"/>
            <owl:cardinality rdf:datatype="http://www.w3.org/2001/XMLSchema#nonNegativeInteger">2</owl:cardinality>
         </owl:Restriction>
         <owl:Restriction>
            <owl:onProperty rdf:resource="http://www.opengis.net/gml#haspos"/>
            <owl:someValuesFrom rdf:resource="http://www.opengis.net/gml#pos"/>
         </owl:Restriction>
         <owl:Restriction>
            <owl:onProperty rdf:resource="http://www.opengis.net/gml#haspos"/>
            <owl:cardinality rdf:datatype="http://www.w3.org/2001/XMLSchema#nonNegativeInteger">2</owl:cardinality>
         </owl:Restriction>
         <owl:Restriction>
            <owl:onProperty rdf:resource="http://www.opengis.net/gml#hascoordinates"/>
            <owl:someValuesFrom rdf:resource="http://www.opengis.net/gml#coordinates"/>
         </owl:Restriction>
         <owl:Restriction>
            <owl:intersectionOf rdf:parseType="Collection">
               <owl:Restriction>
                  <owl:onProperty rdf:resource="http://www.opengis.net/gml#lowerCorner"/>
                  <owl:allValuesFrom rdf:resource="http://www.opengis.net/gml#DirectPositionType"/>
               </owl:Restriction>
               <owl:Restriction>
                  <owl:onProperty rdf:resource="http://www.opengis.net/gml#upperCorner"/>
                  <owl:allValuesFrom rdf:resource="http://www.opengis.net/gml#DirectPositionType"/>
               </owl:Restriction>
            </owl:intersectionOf>
         </owl:Restriction>
      </owl:disjointUnionOf>
   </owl:Class>
   <owl:Class rdf:about="http://www.opengis.net/gml#CoordType">
      <rdfs:comment>Represents a coordinate tuple in one, two, or three dimensions. Deprecated with GML 3.0 and replaced by 
      DirectPositionType.</rdfs:comment>
      <rdfs:subClassOf>
         <owl:Class>
            <owl:intersectionOf rdf:parseType="Collection">
               <owl:Restriction>
                  <owl:onProperty rdf:resource="http://www.opengis.net/gml#X"/>
                  <owl:allValuesFrom rdf:resource="http://www.w3.org/2001/XMLSchema#decimal"/>
               </owl:Restriction>
               <owl:Restriction>
                  <owl:onProperty rdf:resource="http://www.opengis.net/gml#Y"/>
                  <owl:allValuesFrom rdf:resource="http://www.w3.org/2001/XMLSchema#decimal"/>
               </owl:Restriction>
               <owl:Restriction>
                  <owl:onProperty rdf:resource="http://www.opengis.net/gml#Y"/>
                  <owl:minCardinality rdf:datatype="http://www.w3.org/2001/XMLSchema#nonNegativeInteger">0</owl:minCardinality>
               </owl:Restriction>
               <owl:Restriction>
                  <owl:onProperty rdf:resource="http://www.opengis.net/gml#Z"/>
                  <owl:allValuesFrom rdf:resource="http://www.w3.org/2001/XMLSchema#decimal"/>
               </owl:Restriction>
               <owl:Restriction>
                  <owl:onProperty rdf:resource="http://www.opengis.net/gml#Z"/>
                  <owl:minCardinality rdf:datatype="http://www.w3.org/2001/XMLSchema#nonNegativeInteger">0</owl:minCardinality>
               </owl:Restriction>
            </owl:intersectionOf>
         </owl:Class>
      </rdfs:subClassOf>
   </owl:Class>
   <owl:Class rdf:about="http://www.opengis.net/gml#LineStringPropertyType">
      <rdfs:comment>This type is deprecated with GML 3 and shall not be used. It is included for backwards compatibility with GML 2. Use 
      CurvePropertyType instead. A property that has a line string as its value domain can either be an appropriate geometry element encapsulated 
      in an element of this type or an XLink reference to a remote geometry element (where remote includes geometry elements located elsewhere 
      in the same document). Either the reference or the contained element must be given, but neither both nor none.</rdfs:comment>
      <rdfs:subClassOf>
         <owl:Class>
            <owl:intersectionOf rdf:parseType="Collection">
               <owl:Restriction>
                  <owl:onProperty rdf:resource="http://www.opengis.net/gml#hasLineString"/>
                  <owl:allValuesFrom rdf:resource="http://www.opengis.net/gml#LineString"/>
               </owl:Restriction>
            </owl:intersectionOf>
         </owl:Class>
      </rdfs:subClassOf>
   </owl:Class>
   <owl:Class rdf:about="http://www.opengis.net/gml#LengthType">
      <rdfs:comment>Value of a length (or distance) quantity, with its units. Uses the MeasureType with the restriction that the unit of measure referenced by uom must be suitable for a length, such as metres or feet.</rdfs:comment>
      <rdfs:subClassOf>
         <owl:Restriction>
            <owl:onProperty rdf:resource="http://www.opengis.net/gml#hasLengthTypeDatatype"/>
            <owl:someValuesFrom rdf:resource="http://www.opengis.net/gml#LengthTypeDatatype"/>
         </owl:Restriction>
      </rdfs:subClassOf>
      <rdfs:subClassOf rdf:resource="http://www.opengis.net/gml#MeasureType"/>
   </owl:Class>
   <rdfs:Datatype rdf:about="http://www.opengis.net/gml#LengthTypeDatatype">
      <owl:equivalentClass rdf:resource="http://www.opengis.net/gml#MeasureType"/>
   </rdfs:Datatype>
   <owl:DatatypeProperty rdf:about="http://www.opengis.net/gml#hasLengthTypeDatatype">
      <rdfs:domain rdf:resource="http://www.opengis.net/gml#LengthType"/>
      <rdfs:range rdf:resource="http://www.opengis.net/gml#LengthTypeDatatype"/>
   </owl:DatatypeProperty>
   <owl:Class rdf:about="http://www.opengis.net/gml#ScaleType">
      <rdfs:comment>Value of a scale factor (or ratio) that has no physical unit. Uses the MeasureType with the restriction that the unit of measure referenced by uom must be suitable for a scale factor, such as percent, permil, or parts-per-million.</rdfs:comment>
      <rdfs:subClassOf>
         <owl:Restriction>
            <owl:onProperty rdf:resource="http://www.opengis.net/gml#hasScaleTypeDatatype"/>
            <owl:someValuesFrom rdf:resource="http://www.opengis.net/gml#ScaleTypeDatatype"/>
         </owl:Restriction>
      </rdfs:subClassOf>
      <rdfs:subClassOf rdf:resource="http://www.opengis.net/gml#MeasureType"/>
   </owl:Class>
   <rdfs:Datatype rdf:about="http://www.opengis.net/gml#ScaleTypeDatatype">
      <owl:equivalentClass rdf:resource="http://www.opengis.net/gml#MeasureType"/>
   </rdfs:Datatype>
   <owl:DatatypeProperty rdf:about="http://www.opengis.net/gml#hasScaleTypeDatatype">
      <rdfs:domain rdf:resource="http://www.opengis.net/gml#ScaleType"/>
      <rdfs:range rdf:resource="http://www.opengis.net/gml#ScaleTypeDatatype"/>
   </owl:DatatypeProperty>
   <owl:Class rdf:about="http://www.opengis.net/gml#TimeType">
      <rdfs:comment>Value of a time or temporal quantity, with its units. Uses the MeasureType with the restriction that the unit of measure referenced by uom must be suitable for a time value, such as seconds or weeks.</rdfs:comment>
      <rdfs:subClassOf>
         <owl:Restriction>
            <owl:onProperty rdf:resource="http://www.opengis.net/gml#hasTimeTypeDatatype"/>
            <owl:someValuesFrom rdf:resource="http://www.opengis.net/gml#TimeTypeDatatype"/>
         </owl:Restriction>
      </rdfs:subClassOf>
      <rdfs:subClassOf rdf:resource="http://www.opengis.net/gml#MeasureType"/>
   </owl:Class>
   <rdfs:Datatype rdf:about="http://www.opengis.net/gml#TimeTypeDatatype">
      <owl:equivalentClass rdf:resource="http://www.opengis.net/gml#MeasureType"/>
   </rdfs:Datatype>
   <owl:DatatypeProperty rdf:about="http://www.opengis.net/gml#hasTimeTypeDatatype">
      <rdfs:domain rdf:resource="http://www.opengis.net/gml#TimeType"/>
      <rdfs:range rdf:resource="http://www.opengis.net/gml#TimeTypeDatatype"/>
   </owl:DatatypeProperty>
   <owl:Class rdf:about="http://www.opengis.net/gml#GridLengthType">
      <rdfs:comment>Value of a length (or distance) quantity in a grid, where the grid spacing does not have any associated physical units, or does not have a constant physical spacing. This grid length will often be used in a digital image grid, where the base units are likely to be pixel spacings. Uses the MeasureType with the restriction that the unit of measure referenced by uom must be suitable for length along the axes of a grid, such as pixel spacings or grid spacings.</rdfs:comment>
      <rdfs:subClassOf>
         <owl:Restriction>
            <owl:onProperty rdf:resource="http://www.opengis.net/gml#hasGridLengthTypeDatatype"/>
            <owl:someValuesFrom rdf:resource="http://www.opengis.net/gml#GridLengthTypeDatatype"/>
         </owl:Restriction>
      </rdfs:subClassOf>
      <rdfs:subClassOf rdf:resource="http://www.opengis.net/gml#MeasureType"/>
   </owl:Class>
   <rdfs:Datatype rdf:about="http://www.opengis.net/gml#GridLengthTypeDatatype">
      <owl:equivalentClass rdf:resource="http://www.opengis.net/gml#MeasureType"/>
   </rdfs:Datatype>
   <owl:DatatypeProperty rdf:about="http://www.opengis.net/gml#hasGridLengthTypeDatatype">
      <rdfs:domain rdf:resource="http://www.opengis.net/gml#GridLengthType"/>
      <rdfs:range rdf:resource="http://www.opengis.net/gml#GridLengthTypeDatatype"/>
   </owl:DatatypeProperty>
   <owl:Class rdf:about="http://www.opengis.net/gml#AreaType">
      <rdfs:comment>Value of a spatial area quantity, with its units. Uses the MeasureType with the restriction that the unit of measure referenced by uom must be suitable for an area, such as square metres or square miles.</rdfs:comment>
      <rdfs:subClassOf>
         <owl:Restriction>
            <owl:onProperty rdf:resource="http://www.opengis.net/gml#hasAreaTypeDatatype"/>
            <owl:someValuesFrom rdf:resource="http://www.opengis.net/gml#AreaTypeDatatype"/>
         </owl:Restriction>
      </rdfs:subClassOf>
      <rdfs:subClassOf rdf:resource="http://www.opengis.net/gml#MeasureType"/>
   </owl:Class>
   <rdfs:Datatype rdf:about="http://www.opengis.net/gml#AreaTypeDatatype">
      <owl:equivalentClass rdf:resource="http://www.opengis.net/gml#MeasureType"/>
   </rdfs:Datatype>
   <owl:DatatypeProperty rdf:about="http://www.opengis.net/gml#hasAreaTypeDatatype">
      <rdfs:domain rdf:resource="http://www.opengis.net/gml#AreaType"/>
      <rdfs:range rdf:resource="http://www.opengis.net/gml#AreaTypeDatatype"/>
   </owl:DatatypeProperty>
   <owl:Class rdf:about="http://www.opengis.net/gml#VolumeType">
      <rdfs:comment>Value of a spatial volume quantity, with its units. Uses the MeasureType with the restriction that the unit of measure referenced by uom must be suitable for a volume, such as cubic metres or cubic feet.</rdfs:comment>
      <rdfs:subClassOf>
         <owl:Restriction>
            <owl:onProperty rdf:resource="http://www.opengis.net/gml#hasVolumeTypeDatatype"/>
            <owl:someValuesFrom rdf:resource="http://www.opengis.net/gml#VolumeTypeDatatype"/>
         </owl:Restriction>
      </rdfs:subClassOf>
      <rdfs:subClassOf rdf:resource="http://www.opengis.net/gml#MeasureType"/>
   </owl:Class>
   <rdfs:Datatype rdf:about="http://www.opengis.net/gml#VolumeTypeDatatype">
      <owl:equivalentClass rdf:resource="http://www.opengis.net/gml#MeasureType"/>
   </rdfs:Datatype>
   <owl:DatatypeProperty rdf:about="http://www.opengis.net/gml#hasVolumeTypeDatatype">
      <rdfs:domain rdf:resource="http://www.opengis.net/gml#VolumeType"/>
      <rdfs:range rdf:resource="http://www.opengis.net/gml#VolumeTypeDatatype"/>
   </owl:DatatypeProperty>
   <owl:Class rdf:about="http://www.opengis.net/gml#SpeedType">
      <rdfs:comment>Value of a speed, with its units. Uses the MeasureType with the restriction that the unit of measure referenced by uom must be suitable for a velocity, such as metres per second or miles per hour.</rdfs:comment>
      <rdfs:subClassOf>
         <owl:Restriction>
            <owl:onProperty rdf:resource="http://www.opengis.net/gml#hasSpeedTypeDatatype"/>
            <owl:someValuesFrom rdf:resource="http://www.opengis.net/gml#SpeedTypeDatatype"/>
         </owl:Restriction>
      </rdfs:subClassOf>
      <rdfs:subClassOf rdf:resource="http://www.opengis.net/gml#MeasureType"/>
   </owl:Class>
   <rdfs:Datatype rdf:about="http://www.opengis.net/gml#SpeedTypeDatatype">
      <owl:equivalentClass rdf:resource="http://www.opengis.net/gml#MeasureType"/>
   </rdfs:Datatype>
   <owl:DatatypeProperty rdf:about="http://www.opengis.net/gml#hasSpeedTypeDatatype">
      <rdfs:domain rdf:resource="http://www.opengis.net/gml#SpeedType"/>
      <rdfs:range rdf:resource="http://www.opengis.net/gml#SpeedTypeDatatype"/>
   </owl:DatatypeProperty>
   <owl:Class rdf:about="http://www.opengis.net/gml#AngleChoiceType">
      <rdfs:comment>Value of an angle quantity provided in either degree-minute-second format or single value format.</rdfs:comment>
      <owl:disjointUnionOf rdf:parseType="Collection">
         <owl:Restriction>
            <owl:onProperty rdf:resource="http://www.opengis.net/gml#hasangle"/>
            <owl:someValuesFrom rdf:resource="http://www.opengis.net/gml#angle"/>
         </owl:Restriction>
         <owl:Restriction>
            <owl:onProperty rdf:resource="http://www.opengis.net/gml#hasdmsAngle"/>
            <owl:someValuesFrom rdf:resource="http://www.opengis.net/gml#dmsAngle"/>
         </owl:Restriction>
      </owl:disjointUnionOf>
   </owl:Class>
   <owl:Class rdf:about="http://www.opengis.net/gml#AngleType">
      <rdfs:comment>Value of an angle quantity recorded as a single number, with its units. Uses the MeasureType with the restriction that the unit of measure referenced by uom must be suitable for an angle, such as degrees or radians.</rdfs:comment>
      <rdfs:subClassOf>
         <owl:Restriction>
            <owl:onProperty rdf:resource="http://www.opengis.net/gml#hasAngleTypeDatatype"/>
            <owl:someValuesFrom rdf:resource="http://www.opengis.net/gml#AngleTypeDatatype"/>
         </owl:Restriction>
      </rdfs:subClassOf>
      <rdfs:subClassOf rdf:resource="http://www.opengis.net/gml#MeasureType"/>
   </owl:Class>
   <rdfs:Datatype rdf:about="http://www.opengis.net/gml#AngleTypeDatatype">
      <owl:equivalentClass rdf:resource="http://www.opengis.net/gml#MeasureType"/>
   </rdfs:Datatype>
   <owl:DatatypeProperty rdf:about="http://www.opengis.net/gml#hasAngleTypeDatatype">
      <rdfs:domain rdf:resource="http://www.opengis.net/gml#AngleType"/>
      <rdfs:range rdf:resource="http://www.opengis.net/gml#AngleTypeDatatype"/>
   </owl:DatatypeProperty>
   <owl:Class rdf:about="http://www.opengis.net/gml#DMSAngleType">
      <rdfs:comment>Angle value provided in degree-minute-second or degree-minute format.</rdfs:comment>
      <rdfs:subClassOf>
         <owl:Class>
            <owl:intersectionOf rdf:parseType="Collection">
               <owl:Restriction>
                  <owl:onProperty rdf:resource="http://www.opengis.net/gml#hasdegrees"/>
                  <owl:allValuesFrom rdf:resource="http://www.opengis.net/gml#degrees"/>
               </owl:Restriction>
            </owl:intersectionOf>
         </owl:Class>
      </rdfs:subClassOf>
      <owl:disjointUnionOf rdf:parseType="Collection">
         <owl:Restriction>
            <owl:onProperty rdf:resource="http://www.opengis.net/gml#hasdecimalMinutes"/>
            <owl:someValuesFrom rdf:resource="http://www.opengis.net/gml#decimalMinutes"/>
         </owl:Restriction>
         <owl:Restriction>
            <owl:intersectionOf rdf:parseType="Collection">
               <owl:Restriction>
                  <owl:onProperty rdf:resource="http://www.opengis.net/gml#hasminutes"/>
                  <owl:allValuesFrom rdf:resource="http://www.opengis.net/gml#minutes"/>
               </owl:Restriction>
               <owl:Restriction>
                  <owl:onProperty rdf:resource="http://www.opengis.net/gml#hasseconds"/>
                  <owl:allValuesFrom rdf:resource="http://www.opengis.net/gml#seconds"/>
               </owl:Restriction>
               <owl:Restriction>
                  <owl:onProperty rdf:resource="http://www.opengis.net/gml#hasseconds"/>
                  <owl:minCardinality rdf:datatype="http://www.w3.org/2001/XMLSchema#nonNegativeInteger">0</owl:minCardinality>
               </owl:Restriction>
            </owl:intersectionOf>
         </owl:Restriction>
      </owl:disjointUnionOf>
   </owl:Class>
   <owl:Class rdf:about="http://www.opengis.net/gml#DegreesType">
      <rdfs:comment>Integer number of degrees, plus the angle direction. This element can be used for geographic Latitude and Longitude. For Latitude, the XML attribute direction can take the values "N" or "S", meaning North or South of the equator. For Longitude, direction can take the values "E" or "W", meaning East or West of the prime meridian. This element can also be used for other angles. In that case, the direction can take the values "+" or "-" (of SignType), in the specified rotational direction from a specified reference direction.</rdfs:comment>
      <rdfs:subClassOf>
         <owl:Class>
            <owl:intersectionOf rdf:parseType="Collection">
               <owl:Restriction>
                  <owl:onProperty rdf:resource="http://www.opengis.net/gml#direction"/>
                  <owl:allValuesFrom rdf:resource="http://www.w3.org/2001/XMLSchema#string"/>
               </owl:Restriction>
            </owl:intersectionOf>
         </owl:Class>
      </rdfs:subClassOf>
      <rdfs:subClassOf>
         <owl:Restriction>
            <owl:onProperty rdf:resource="http://www.opengis.net/gml#hasDegreeValueType"/>
            <owl:someValuesFrom rdf:resource="DegreeValueType"/>
         </owl:Restriction>
      </rdfs:subClassOf>
   </owl:Class>
   <owl:DatatypeProperty rdf:about="http://www.opengis.net/gml#hasDegreeValueType">
      <rdfs:domain rdf:resource="http://www.opengis.net/gml#DegreesType"/>
      <rdfs:range rdf:resource="http://www.opengis.net/gml#DegreeValueType"/>
   </owl:DatatypeProperty>
   <owl:Class rdf:about="http://www.opengis.net/gml#UnitOfMeasureType">
      <rdfs:comment>Reference to a unit of measure definition that applies to all the numerical values described by the element containing this element. Notice that a complexType which needs to include the uom attribute can do so by extending this complexType. Alternately, this complexType can be used as a pattern for a new complexType.</rdfs:comment>
      <rdfs:subClassOf>
         <owl:Class>
            <owl:intersectionOf rdf:parseType="Collection">
               <owl:Restriction>
                  <owl:onProperty rdf:resource="http://www.opengis.net/gml#uom"/>
                  <owl:allValuesFrom rdf:resource="http://www.w3.org/2001/XMLSchema#anyURI"/>
               </owl:Restriction>
            </owl:intersectionOf>
         </owl:Class>
      </rdfs:subClassOf>
   </owl:Class>
   <owl:Class rdf:about="http://www.opengis.net/gml#UnitDefinitionType">
      <rdfs:comment>Definition of a unit of measure (or uom). The definition includes a quantityType property, which indicates the phenomenon to which the units apply, and a catalogSymbol, which gives the short symbol used for this unit. This element is used when the relationship of this unit to other units or units systems is unknown.</rdfs:comment>
      <rdfs:subClassOf>
         <owl:Class>
            <owl:intersectionOf rdf:parseType="Collection">
               <owl:Restriction>
                  <owl:onProperty rdf:resource="http://www.opengis.net/gml#hasquantityType"/>
                  <owl:allValuesFrom rdf:resource="http://www.opengis.net/gml#quantityType"/>
               </owl:Restriction>
               <owl:Restriction>
                  <owl:onProperty rdf:resource="http://www.opengis.net/gml#hascatalogSymbol"/>
                  <owl:allValuesFrom rdf:resource="http://www.opengis.net/gml#catalogSymbol"/>
               </owl:Restriction>
               <owl:Restriction>
                  <owl:onProperty rdf:resource="http://www.opengis.net/gml#hascatalogSymbol"/>
                  <owl:minCardinality rdf:datatype="http://www.w3.org/2001/XMLSchema#nonNegativeInteger">0</owl:minCardinality>
               </owl:Restriction>
            </owl:intersectionOf>
         </owl:Class>
      </rdfs:subClassOf>
      <rdfs:subClassOf rdf:resource="http://www.opengis.net/gml#DefinitionType"/>
   </owl:Class>
   <owl:Class rdf:about="http://www.opengis.net/gml#BaseUnitType">
      <rdfs:comment>Definition of a unit of measure which is a base unit from the system of units.  A base unit cannot be derived by combination of other base units within this system.  Sometimes known as "fundamental unit".</rdfs:comment>
      <rdfs:subClassOf>
         <owl:Class>
            <owl:intersectionOf rdf:parseType="Collection">
               <owl:Restriction>
                  <owl:onProperty rdf:resource="http://www.opengis.net/gml#unitsSystem"/>
                  <owl:allValuesFrom rdf:resource="http://www.opengis.net/gml#ReferenceType"/>
               </owl:Restriction>
            </owl:intersectionOf>
         </owl:Class>
      </rdfs:subClassOf>
      <rdfs:subClassOf rdf:resource="http://www.opengis.net/gml#UnitDefinitionType"/>
   </owl:Class>
   <owl:Class rdf:about="http://www.opengis.net/gml#DerivedUnitType">
      <rdfs:comment>Definition of a unit of measure which is defined through algebraic combination of more primitive units, which are usually base units from a particular system of units. Derived units based directly on base units are usually preferred for quantities other than the base units or fundamental quantities within a system.  If a derived unit is not the preferred unit, the ConventionalUnit element should be used instead.</rdfs:comment>
      <rdfs:subClassOf>
         <owl:Class>
            <owl:intersectionOf rdf:parseType="Collection">
               <owl:Restriction>
                  <owl:onProperty rdf:resource="http://www.opengis.net/gml#hasderivationUnitTerm"/>
                  <owl:allValuesFrom rdf:resource="http://www.opengis.net/gml#derivationUnitTerm"/>
               </owl:Restriction>
            </owl:intersectionOf>
         </owl:Class>
      </rdfs:subClassOf>
      <rdfs:subClassOf rdf:resource="http://www.opengis.net/gml#UnitDefinitionType"/>
   </owl:Class>
   <owl:Class rdf:about="http://www.opengis.net/gml#ConventionalUnitType">
      <rdfs:comment>Definition of a unit of measure which is related to a preferred unit for this quantity type through a conversion formula.  A method for deriving this unit by algebraic combination of more primitive units, may also be provided.</rdfs:comment>
      <rdfs:subClassOf>
         <owl:Class>
            <owl:intersectionOf rdf:parseType="Collection">
               <owl:Restriction>
                  <owl:onProperty rdf:resource="http://www.opengis.net/gml#hasderivationUnitTerm"/>
                  <owl:allValuesFrom rdf:resource="http://www.opengis.net/gml#derivationUnitTerm"/>
               </owl:Restriction>
               <owl:Restriction>
                  <owl:onProperty rdf:resource="http://www.opengis.net/gml#hasderivationUnitTerm"/>
                  <owl:minCardinality rdf:datatype="http://www.w3.org/2001/XMLSchema#nonNegativeInteger">0</owl:minCardinality>
               </owl:Restriction>
            </owl:intersectionOf>
         </owl:Class>
      </rdfs:subClassOf>
      <owl:disjointUnionOf rdf:parseType="Collection">
         <owl:Restriction>
            <owl:onProperty rdf:resource="http://www.opengis.net/gml#hasconversionToPreferredUnit"/>
            <owl:someValuesFrom rdf:resource="http://www.opengis.net/gml#conversionToPreferredUnit"/>
         </owl:Restriction>
         <owl:Restriction>
            <owl:onProperty rdf:resource="http://www.opengis.net/gml#hasroughConversionToPreferredUnit"/>
            <owl:someValuesFrom rdf:resource="http://www.opengis.net/gml#roughConversionToPreferredUnit"/>
         </owl:Restriction>
      </owl:disjointUnionOf>
      <rdfs:subClassOf rdf:resource="http://www.opengis.net/gml#UnitDefinitionType"/>
   </owl:Class>
   <owl:Class rdf:about="http://www.opengis.net/gml#DerivationUnitTermType">
      <rdfs:comment>Definition of one unit term for a derived unit of measure. This unit term references another unit of measure (uom) and provides an integer exponent applied to that unit in defining the compound unit. The exponent can be positive or negative, but not zero.</rdfs:comment>
      <rdfs:subClassOf>
         <owl:Class>
            <owl:intersectionOf rdf:parseType="Collection">
               <owl:Restriction>
                  <owl:onProperty rdf:resource="http://www.opengis.net/gml#exponent"/>
                  <owl:allValuesFrom rdf:resource="http://www.w3.org/2001/XMLSchema#integer"/>
               </owl:Restriction>
            </owl:intersectionOf>
         </owl:Class>
      </rdfs:subClassOf>
      <rdfs:subClassOf rdf:resource="http://www.opengis.net/gml#UnitOfMeasureType"/>
   </owl:Class>
   <owl:Class rdf:about="http://www.opengis.net/gml#ConversionToPreferredUnitType">
      <rdfs:comment>Relation of a unit to the preferred unit for this quantity type, specified by an arithmetic conversion (scaling and/or offset). A preferred unit is either a base unit or a derived unit selected for all units of one quantity type. The mandatory attribute "uom" shall reference the preferred unit that this conversion applies to. The conversion is specified by one of two alternative elements: "factor" or "formula".</rdfs:comment>
      <owl:disjointUnionOf rdf:parseType="Collection">
         <owl:Restriction>
            <owl:onProperty rdf:resource="http://www.opengis.net/gml#factor"/>
            <owl:someValuesFrom rdf:resource="http://www.w3.org/2001/XMLSchema#double"/>
         </owl:Restriction>
         <owl:Restriction>
            <owl:onProperty rdf:resource="http://www.opengis.net/gml#formula"/>
            <owl:someValuesFrom rdf:resource="http://www.opengis.net/gml#FormulaType"/>
         </owl:Restriction>
      </owl:disjointUnionOf>
      <rdfs:subClassOf rdf:resource="http://www.opengis.net/gml#UnitOfMeasureType"/>
   </owl:Class>
   <owl:Class rdf:about="http://www.opengis.net/gml#FormulaType">
      <rdfs:comment>Paremeters of a simple formula by which a value using this unit of measure can be converted to the corresponding value using the preferred unit of measure. The formula element contains elements a, b, c and d, whose values use the XML Schema type "double". These values are used in the formula y = (a + bx) / (c + dx), where x is a value using this unit, and y is the corresponding value using the preferred unit. The elements a and d are optional, and if values are not provided, those parameters are considered to be zero. If values are not provided for both a and d, the formula is equivalent to a fraction with numerator and denominator parameters.</rdfs:comment>
      <rdfs:subClassOf>
         <owl:Class>
            <owl:intersectionOf rdf:parseType="Collection">
               <owl:Restriction>
                  <owl:onProperty rdf:resource="http://www.opengis.net/gml#a"/>
                  <owl:allValuesFrom rdf:resource="http://www.w3.org/2001/XMLSchema#double"/>
               </owl:Restriction>
               <owl:Restriction>
                  <owl:onProperty rdf:resource="http://www.opengis.net/gml#a"/>
                  <owl:minCardinality rdf:datatype="http://www.w3.org/2001/XMLSchema#nonNegativeInteger">0</owl:minCardinality>
               </owl:Restriction>
               <owl:Restriction>
                  <owl:onProperty rdf:resource="http://www.opengis.net/gml#b"/>
                  <owl:allValuesFrom rdf:resource="http://www.w3.org/2001/XMLSchema#double"/>
               </owl:Restriction>
               <owl:Restriction>
                  <owl:onProperty rdf:resource="http://www.opengis.net/gml#c"/>
                  <owl:allValuesFrom rdf:resource="http://www.w3.org/2001/XMLSchema#double"/>
               </owl:Restriction>
               <owl:Restriction>
                  <owl:onProperty rdf:resource="http://www.opengis.net/gml#d"/>
                  <owl:allValuesFrom rdf:resource="http://www.w3.org/2001/XMLSchema#double"/>
               </owl:Restriction>
               <owl:Restriction>
                  <owl:onProperty rdf:resource="http://www.opengis.net/gml#d"/>
                  <owl:minCardinality rdf:datatype="http://www.w3.org/2001/XMLSchema#nonNegativeInteger">0</owl:minCardinality>
               </owl:Restriction>
            </owl:intersectionOf>
         </owl:Class>
      </rdfs:subClassOf>
   </owl:Class>
   <owl:Class rdf:about="http://www.opengis.net/gml#DefinitionType">
      <rdfs:comment>A definition, which can be included in or referenced by a dictionary. In this extended type, the inherited "description" optional element can hold the definition whenever only text is needed. The inherited "name" elements can provide one or more brief terms for which this is the definition. The inherited "metaDataProperty" elements can be used to reference or include more information about this definition.  
The gml:id attribute is required - it must be possible to reference this definition using this handle.  </rdfs:comment>
      <rdfs:subClassOf>
         <owl:Class>
            <owl:intersectionOf rdf:parseType="Collection">
               <owl:Restriction>
                  <owl:onProperty rdf:resource="http://www.opengis.net/gml#hasmetaDataProperty"/>
                  <owl:allValuesFrom rdf:resource="http://www.opengis.net/gml#metaDataProperty"/>
               </owl:Restriction>
               <owl:Restriction>
                  <owl:onProperty rdf:resource="http://www.opengis.net/gml#hasmetaDataProperty"/>
                  <owl:minCardinality rdf:datatype="http://www.w3.org/2001/XMLSchema#nonNegativeInteger">0</owl:minCardinality>
               </owl:Restriction>
               <owl:Restriction>
                  <owl:onProperty rdf:resource="http://www.opengis.net/gml#hasdescription"/>
                  <owl:allValuesFrom rdf:resource="http://www.opengis.net/gml#description"/>
               </owl:Restriction>
               <owl:Restriction>
                  <owl:onProperty rdf:resource="http://www.opengis.net/gml#hasdescription"/>
                  <owl:minCardinality rdf:datatype="http://www.w3.org/2001/XMLSchema#nonNegativeInteger">0</owl:minCardinality>
               </owl:Restriction>
               <owl:Restriction>
                  <owl:onProperty rdf:resource="http://www.opengis.net/gml#hasname"/>
                  <owl:allValuesFrom rdf:resource="http://www.opengis.net/gml#name"/>
               </owl:Restriction>
            </owl:intersectionOf>
         </owl:Class>
      </rdfs:subClassOf>
      <rdfs:subClassOf>
         <owl:Class>
            <owl:intersectionOf rdf:parseType="Collection">
               <owl:Restriction>
                  <owl:onProperty rdf:resource="http://www.opengis.net/gml#hasid"/>
                  <owl:allValuesFrom rdf:resource="http://www.opengis.net/gml#id"/>
               </owl:Restriction>
            </owl:intersectionOf>
         </owl:Class>
      </rdfs:subClassOf>
      <rdfs:subClassOf rdf:resource="http://www.opengis.net/gml#AbstractGMLType"/>
   </owl:Class>
   <owl:Class rdf:about="http://www.opengis.net/gml#DictionaryType">
      <rdfs:comment>A non-abstract bag that is specialized for use as a dictionary which contains a set of definitions. These definitions are referenced from other places, in the same and different XML documents. In this restricted type, the inherited optional "description" element can be used for a description of this dictionary. The inherited optional "name" element can be used for the name(s) of this dictionary. The inherited "metaDataProperty" elements can be used to reference or contain more information about this dictionary. The inherited required gml:id attribute allows the dictionary to be referenced using this handle. </rdfs:comment>
      <owl:disjointUnionOf rdf:parseType="Collection">
         <owl:Restriction>
            <owl:onProperty rdf:resource="http://www.opengis.net/gml#hasdictionaryEntry"/>
            <owl:someValuesFrom rdf:resource="http://www.opengis.net/gml#dictionaryEntry"/>
         </owl:Restriction>
         <owl:Restriction>
            <owl:onProperty rdf:resource="http://www.opengis.net/gml#hasindirectEntry"/>
            <owl:someValuesFrom rdf:resource="http://www.opengis.net/gml#indirectEntry"/>
         </owl:Restriction>
      </owl:disjointUnionOf>
      <rdfs:subClassOf rdf:resource="http://www.opengis.net/gml#DefinitionType"/>
   </owl:Class>
   <owl:Class rdf:about="http://www.opengis.net/gml#DictionaryEntryType">
      <rdfs:comment>An entry in a dictionary of definitions. An instance of this type contains or refers to a definition object.  

The number of definitions contained in this dictionaryEntry is restricted to one, but a DefinitionCollection or Dictionary that contains multiple definitions can be substituted if needed. Specialized descendents of this dictionaryEntry might be restricted in an application schema to allow only including specified types of definitions as valid entries in a dictionary. </rdfs:comment>
      <rdfs:subClassOf>
         <owl:Class>
            <owl:intersectionOf rdf:parseType="Collection">
               <owl:Restriction>
                  <owl:onProperty rdf:resource="http://www.opengis.net/gml#hasDefinition"/>
                  <owl:allValuesFrom rdf:resource="http://www.opengis.net/gml#Definition"/>
               </owl:Restriction>
            </owl:intersectionOf>
         </owl:Class>
      </rdfs:subClassOf>
   </owl:Class>
   <owl:Class rdf:about="http://www.opengis.net/gml#IndirectEntryType">
      <rdfs:comment>An entry in a dictionary of definitions that contains a GML object which references a remote definition object. This entry is expected to be convenient in allowing multiple elements in one XML document to contain short (abbreviated XPointer) references, which are resolved to an external definition provided in a Dictionary element in the same XML document. Specialized descendents of this dictionaryEntry might be restricted in an application schema to allow only including specified types of definitions as valid entries in a dictionary. </rdfs:comment>
      <rdfs:subClassOf>
         <owl:Class>
            <owl:intersectionOf rdf:parseType="Collection">
               <owl:Restriction>
                  <owl:onProperty rdf:resource="http://www.opengis.net/gml#hasDefinitionProxy"/>
                  <owl:allValuesFrom rdf:resource="http://www.opengis.net/gml#DefinitionProxy"/>
               </owl:Restriction>
            </owl:intersectionOf>
         </owl:Class>
      </rdfs:subClassOf>
   </owl:Class>
   <owl:Class rdf:about="http://www.opengis.net/gml#DefinitionProxyType">
      <rdfs:comment>A proxy entry in a dictionary of definitions. An element of this type contains a reference to a remote definition object. This entry is expected to be convenient in allowing multiple elements in one XML document to contain short (abbreviated XPointer) references, which are resolved to an external definition provided in a Dictionary element in the same XML document. </rdfs:comment>
      <rdfs:subClassOf>
         <owl:Class>
            <owl:intersectionOf rdf:parseType="Collection">
               <owl:Restriction>
                  <owl:onProperty rdf:resource="http://www.opengis.net/gml#hasdefinitionRef"/>
                  <owl:allValuesFrom rdf:resource="http://www.opengis.net/gml#definitionRef"/>
               </owl:Restriction>
            </owl:intersectionOf>
         </owl:Class>
      </rdfs:subClassOf>
      <rdfs:subClassOf rdf:resource="http://www.opengis.net/gml#DefinitionType"/>
   </owl:Class>
   <owl:Class rdf:about="http://www.opengis.net/gml#AbstractGMLType">
      <rdfs:comment>This is an abstract class</rdfs:comment>
      <rdfs:comment>All complexContent GML elements are directly or indirectly derived from this abstract supertype 
  to establish a hierarchy of GML types that may be distinguished from other XML types by their ancestry. 
  Elements in this hierarchy may have an ID and are thus referenceable.</rdfs:comment>
      <rdfs:subClassOf rdf:resource="http://www.opengis.net/gml#StandardObjectProperties"/>
      <rdfs:subClassOf>
         <owl:Class>
            <owl:intersectionOf rdf:parseType="Collection">
               <owl:Restriction>
                  <owl:onProperty rdf:resource="http://www.opengis.net/gml#hasid"/>
                  <owl:allValuesFrom rdf:resource="http://www.opengis.net/gml#id"/>
               </owl:Restriction>
            </owl:intersectionOf>
         </owl:Class>
      </rdfs:subClassOf>
   </owl:Class>
   <owl:Class rdf:about="http://www.opengis.net/gml#BagType">
      <rdfs:comment>A non-abstract generic collection type that can be used as a document element for a collection of any GML types - Geometries, Topologies, Features ...

FeatureCollections may only contain Features.  GeometryCollections may only contain Geometrys.  Bags are less constrained  they must contain objects that are substitutable for gml:_Object.  This may mix several levels, including Features, Definitions, Dictionaries, Geometries etc.  

The content model would ideally be 
   member 0..*
   members 0..1
   member 0..*
for maximum flexibility in building a collection from both homogeneous and distinct components: 
included "member" elements each contain a single Object
an included "members" element contains a set of Objects 

However, this is non-deterministic, thus prohibited by XSD.</rdfs:comment>
      <rdfs:subClassOf>
         <owl:Class>
            <owl:intersectionOf rdf:parseType="Collection">
               <owl:Restriction>
                  <owl:onProperty rdf:resource="http://www.opengis.net/gml#hasmember"/>
                  <owl:allValuesFrom rdf:resource="http://www.opengis.net/gml#member"/>
               </owl:Restriction>
               <owl:Restriction>
                  <owl:onProperty rdf:resource="http://www.opengis.net/gml#hasmember"/>
                  <owl:minCardinality rdf:datatype="http://www.w3.org/2001/XMLSchema#nonNegativeInteger">0</owl:minCardinality>
               </owl:Restriction>
               <owl:Restriction>
                  <owl:onProperty rdf:resource="http://www.opengis.net/gml#hasmembers"/>
                  <owl:allValuesFrom rdf:resource="http://www.opengis.net/gml#members"/>
               </owl:Restriction>
               <owl:Restriction>
                  <owl:onProperty rdf:resource="http://www.opengis.net/gml#hasmembers"/>
                  <owl:minCardinality rdf:datatype="http://www.w3.org/2001/XMLSchema#nonNegativeInteger">0</owl:minCardinality>
               </owl:Restriction>
            </owl:intersectionOf>
         </owl:Class>
      </rdfs:subClassOf>
      <rdfs:subClassOf rdf:resource="http://www.opengis.net/gml#AbstractGMLType"/>
   </owl:Class>
   <owl:Class rdf:about="http://www.opengis.net/gml#ArrayType">
      <rdfs:comment>A non-abstract generic collection type that can be used as a document element for a homogeneous collection of any GML types - Geometries, Topologies, Features ...</rdfs:comment>
      <rdfs:subClassOf>
         <owl:Class>
            <owl:intersectionOf rdf:parseType="Collection">
               <owl:Restriction>
                  <owl:onProperty rdf:resource="http://www.opengis.net/gml#hasmembers"/>
                  <owl:allValuesFrom rdf:resource="http://www.opengis.net/gml#members"/>
               </owl:Restriction>
               <owl:Restriction>
                  <owl:onProperty rdf:resource="http://www.opengis.net/gml#hasmembers"/>
                  <owl:minCardinality rdf:datatype="http://www.w3.org/2001/XMLSchema#nonNegativeInteger">0</owl:minCardinality>
               </owl:Restriction>
            </owl:intersectionOf>
         </owl:Class>
      </rdfs:subClassOf>
      <rdfs:subClassOf rdf:resource="http://www.opengis.net/gml#AbstractGMLType"/>
   </owl:Class>
   <owl:Class rdf:about="http://www.opengis.net/gml#AbstractMetaDataType">
      <rdfs:comment>This is an abstract class</rdfs:comment>
      <rdfs:comment>An abstract base type for complex metadata types.</rdfs:comment>
      <rdfs:subClassOf>
         <owl:Class>
            <owl:intersectionOf rdf:parseType="Collection">
               <owl:Restriction>
                  <owl:onProperty rdf:resource="http://www.opengis.net/gml#hasid"/>
                  <owl:allValuesFrom rdf:resource="http://www.opengis.net/gml#id"/>
               </owl:Restriction>
            </owl:intersectionOf>
         </owl:Class>
      </rdfs:subClassOf>
   </owl:Class>
   <owl:Class rdf:about="http://www.opengis.net/gml#GenericMetaDataType">
      <rdfs:comment>Deprecated with GML version 3.1.0.</rdfs:comment>
      <rdfs:subClassOf rdf:resource="http://www.opengis.net/gml#AbstractMetaDataType"/>
   </owl:Class>
   <owl:Class rdf:about="http://www.opengis.net/gml#AssociationType">
      <rdfs:comment>A pattern or base for derived types used to specify complex types corresponding to an  unspecified UML association - either composition or aggregation.  Restricts the cardinality of Objects contained in the association to a maximum of one.  An instance of this type can contain an element representing an Object, or serve as a pointer to a remote Object.  

Descendents of this type can be restricted in an application schema to 
* allow only specified classes as valid participants in the aggregation
* allow only association by reference (i.e. empty the content model) or by value (i.e. remove the xlinks).    

When used for association by reference, the value of the gml:remoteSchema attribute can be used to locate a schema fragment that constrains the target instance.   

In many cases it is desirable to impose the constraint prohibiting the occurence of both reference and value in the same instance, as that would be ambiguous.  This is accomplished by adding a directive in the annotation element of the element declaration.  This directive can be in the form of normative prose, or can use a Schematron pattern to automatically constrain co-occurrence - see the declaration for _strictAssociation below.   

If co-occurence is not prohibited, then both a link and content may be present.  If this occurs in an instance, then the rule for interpretation is that the instance found by traversing the href provides the normative value of the property, and should be used when possible.  The value(s) included as content may be used if the remote instance cannot be resolved.  This may be considered to be a "cached" version of the value(s).</rdfs:comment>
      <rdfs:subClassOf>
         <owl:Class>
            <owl:intersectionOf rdf:parseType="Collection">
               <owl:Restriction>
                  <owl:onProperty rdf:resource="http://www.opengis.net/gml#has_Object"/>
                  <owl:allValuesFrom rdf:resource="http://www.opengis.net/gml#_Object"/>
               </owl:Restriction>
            </owl:intersectionOf>
         </owl:Class>
      </rdfs:subClassOf>
   </owl:Class>
   <owl:Class rdf:about="http://www.opengis.net/gml#ReferenceType">
      <rdfs:comment>A pattern or base for derived types used to specify complex types corresponding to a UML aggregation association.  An instance of this type serves as a pointer to a remote Object.</rdfs:comment>
   </owl:Class>
   <owl:Class rdf:about="http://www.opengis.net/gml#ArrayAssociationType">
      <rdfs:comment>A base for derived types used to specify complex types containing an array of objects, by unspecified UML association - either composition or aggregation.  An instance of this type contains elements representing Objects.

Ideally this type would be derived by extension of AssociationType.  
However, this leads to a non-deterministic content model, since both the base and the extension have minOccurs="0", and is thus prohibited in XML Schema.</rdfs:comment>
      <rdfs:subClassOf>
         <owl:Class>
            <owl:intersectionOf rdf:parseType="Collection">
               <owl:Restriction>
                  <owl:onProperty rdf:resource="http://www.opengis.net/gml#has_Object"/>
                  <owl:allValuesFrom rdf:resource="http://www.opengis.net/gml#_Object"/>
               </owl:Restriction>
               <owl:Restriction>
                  <owl:onProperty rdf:resource="http://www.opengis.net/gml#has_Object"/>
                  <owl:minCardinality rdf:datatype="http://www.w3.org/2001/XMLSchema#nonNegativeInteger">0</owl:minCardinality>
               </owl:Restriction>
            </owl:intersectionOf>
         </owl:Class>
      </rdfs:subClassOf>
   </owl:Class>
   <owl:Class rdf:about="http://www.opengis.net/gml#MetaDataPropertyType">
      <rdfs:comment>Base type for complex metadata property types.</rdfs:comment>
      <rdfs:subClassOf>
         <owl:Class>
            <owl:intersectionOf rdf:parseType="Collection">
               <owl:Restriction>
                  <owl:onProperty rdf:resource="http://www.opengis.net/gml#about"/>
                  <owl:allValuesFrom rdf:resource="http://www.w3.org/2001/XMLSchema#anyURI"/>
               </owl:Restriction>
            </owl:intersectionOf>
         </owl:Class>
      </rdfs:subClassOf>
   </owl:Class>
   <owl:Class rdf:about="http://www.opengis.net/gml#StringOrRefType">
      <rdfs:comment>This type is available wherever there is a need for a "text" type property. It is of string type, so the text can be included inline, but the value can also be referenced remotely via xlinks from the AssociationAttributeGroup. If the remote reference is present, then the value obtained by traversing the link should be used, and the string content of the element can be used for an annotation.</rdfs:comment>
      <rdfs:subClassOf>
         <owl:Restriction>
            <owl:onProperty rdf:resource="http://www.opengis.net/gml#hasstring"/>
            <owl:someValuesFrom rdf:resource="http://www.w3.org/2001/XMLSchema#string"/>
         </owl:Restriction>
      </rdfs:subClassOf>
   </owl:Class>
   <owl:DatatypeProperty rdf:about="http://www.opengis.net/gml#hasstring">
      <rdfs:domain rdf:resource="http://www.opengis.net/gml#StringOrRefType"/>
      <rdfs:range rdf:resource="http://www.w3.org/2001/XMLSchema#string"/>
   </owl:DatatypeProperty>
   <owl:Class rdf:about="http://www.opengis.net/gml#CodeType">
      <rdfs:comment>Name or code with an (optional) authority.  Text token.  
      If the codeSpace attribute is present, then its value should identify a dictionary, thesaurus 
      or authority for the term, such as the organisation who assigned the value, 
      or the dictionary from which it is taken.  
      A text string with an optional codeSpace attribute. </rdfs:comment>
      <rdfs:subClassOf>
         <owl:Class>
            <owl:intersectionOf rdf:parseType="Collection">
               <owl:Restriction>
                  <owl:onProperty rdf:resource="http://www.opengis.net/gml#codeSpace"/>
                  <owl:allValuesFrom rdf:resource="http://www.w3.org/2001/XMLSchema#anyURI"/>
               </owl:Restriction>
            </owl:intersectionOf>
         </owl:Class>
      </rdfs:subClassOf>
      <rdfs:subClassOf>
         <owl:Restriction>
            <owl:onProperty rdf:resource="http://www.opengis.net/gml#hasstring"/>
            <owl:someValuesFrom rdf:resource="http://www.w3.org/2001/XMLSchema#string"/>
         </owl:Restriction>
      </rdfs:subClassOf>
   </owl:Class>
   <owl:DatatypeProperty rdf:about="http://www.opengis.net/gml#hasstring">
      <rdfs:domain rdf:resource="http://www.opengis.net/gml#CodeType"/>
      <rdfs:range rdf:resource="http://www.w3.org/2001/XMLSchema#string"/>
   </owl:DatatypeProperty>
   <owl:Class rdf:about="http://www.opengis.net/gml#CodeListType">
      <rdfs:comment>List of values on a uniform nominal scale.  List of text tokens.   
      In a list context a token should not include any spaces, so xsd:Name is used instead of xsd:string.   
      If a codeSpace attribute is present, then its value is a reference to 
      a Reference System for the value, a dictionary or code list.</rdfs:comment>
      <rdfs:subClassOf>
         <owl:Class>
            <owl:intersectionOf rdf:parseType="Collection">
               <owl:Restriction>
                  <owl:onProperty rdf:resource="http://www.opengis.net/gml#codeSpace"/>
                  <owl:allValuesFrom rdf:resource="http://www.w3.org/2001/XMLSchema#anyURI"/>
               </owl:Restriction>
            </owl:intersectionOf>
         </owl:Class>
      </rdfs:subClassOf>
      <rdfs:subClassOf>
         <owl:Restriction>
            <owl:onProperty rdf:resource="http://www.opengis.net/gml#hasNameList"/>
            <owl:someValuesFrom rdf:resource="NameList"/>
         </owl:Restriction>
      </rdfs:subClassOf>
   </owl:Class>
   <owl:DatatypeProperty rdf:about="http://www.opengis.net/gml#hasNameList">
      <rdfs:domain rdf:resource="http://www.opengis.net/gml#CodeListType"/>
      <rdfs:range rdf:resource="http://www.opengis.net/gml#NameList"/>
   </owl:DatatypeProperty>
   <owl:Class rdf:about="http://www.opengis.net/gml#CodeOrNullListType">
      <rdfs:comment>List of values on a uniform nominal scale.  List of text tokens.   
      In a list context a token should not include any spaces, so xsd:Name is used instead of xsd:string.  
      A member of the list may be a typed null.  
      If a codeSpace attribute is present, then its value is a reference to 
      a Reference System for the value, a dictionary or code list.</rdfs:comment>
      <rdfs:subClassOf>
         <owl:Class>
            <owl:intersectionOf rdf:parseType="Collection">
               <owl:Restriction>
                  <owl:onProperty rdf:resource="http://www.opengis.net/gml#codeSpace"/>
                  <owl:allValuesFrom rdf:resource="http://www.w3.org/2001/XMLSchema#anyURI"/>
               </owl:Restriction>
            </owl:intersectionOf>
         </owl:Class>
      </rdfs:subClassOf>
      <rdfs:subClassOf>
         <owl:Restriction>
            <owl:onProperty rdf:resource="http://www.opengis.net/gml#hasNameOrNullList"/>
            <owl:someValuesFrom rdf:resource="NameOrNullList"/>
         </owl:Restriction>
      </rdfs:subClassOf>
   </owl:Class>
   <owl:DatatypeProperty rdf:about="http://www.opengis.net/gml#hasNameOrNullList">
      <rdfs:domain rdf:resource="http://www.opengis.net/gml#CodeOrNullListType"/>
      <rdfs:range rdf:resource="http://www.opengis.net/gml#NameOrNullList"/>
   </owl:DatatypeProperty>
   <owl:Class rdf:about="http://www.opengis.net/gml#MeasureType">
      <rdfs:comment>Number with a scale.  
      The value of uom (Units Of Measure) attribute is a reference to a Reference System for the amount, either a ratio or position scale. </rdfs:comment>
      <rdfs:subClassOf>
         <owl:Class>
            <owl:intersectionOf rdf:parseType="Collection">
               <owl:Restriction>
                  <owl:onProperty rdf:resource="http://www.opengis.net/gml#uom"/>
                  <owl:allValuesFrom rdf:resource="http://www.w3.org/2001/XMLSchema#anyURI"/>
               </owl:Restriction>
            </owl:intersectionOf>
         </owl:Class>
      </rdfs:subClassOf>
      <rdfs:subClassOf>
         <owl:Restriction>
            <owl:onProperty rdf:resource="http://www.opengis.net/gml#hasdouble"/>
            <owl:someValuesFrom rdf:resource="http://www.w3.org/2001/XMLSchema#double"/>
         </owl:Restriction>
      </rdfs:subClassOf>
   </owl:Class>
   <owl:DatatypeProperty rdf:about="http://www.opengis.net/gml#hasdouble">
      <rdfs:domain rdf:resource="http://www.opengis.net/gml#MeasureType"/>
      <rdfs:range rdf:resource="http://www.w3.org/2001/XMLSchema#double"/>
   </owl:DatatypeProperty>
   <owl:Class rdf:about="http://www.opengis.net/gml#MeasureListType">
      <rdfs:comment>List of numbers with a uniform scale.  
      The value of uom (Units Of Measure) attribute is a reference to 
      a Reference System for the amount, either a ratio or position scale. </rdfs:comment>
      <rdfs:subClassOf>
         <owl:Class>
            <owl:intersectionOf rdf:parseType="Collection">
               <owl:Restriction>
                  <owl:onProperty rdf:resource="http://www.opengis.net/gml#uom"/>
                  <owl:allValuesFrom rdf:resource="http://www.w3.org/2001/XMLSchema#anyURI"/>
               </owl:Restriction>
            </owl:intersectionOf>
         </owl:Class>
      </rdfs:subClassOf>
      <rdfs:subClassOf>
         <owl:Restriction>
            <owl:onProperty rdf:resource="http://www.opengis.net/gml#hasdoubleList"/>
            <owl:someValuesFrom rdf:resource="doubleList"/>
         </owl:Restriction>
      </rdfs:subClassOf>
   </owl:Class>
   <owl:DatatypeProperty rdf:about="http://www.opengis.net/gml#hasdoubleList">
      <rdfs:domain rdf:resource="http://www.opengis.net/gml#MeasureListType"/>
      <rdfs:range rdf:resource="http://www.opengis.net/gml#doubleList"/>
   </owl:DatatypeProperty>
   <owl:Class rdf:about="http://www.opengis.net/gml#MeasureOrNullListType">
      <rdfs:comment>List of numbers with a uniform scale.  
      A member of the list may be a typed null. 
      The value of uom (Units Of Measure) attribute is a reference to 
      a Reference System for the amount, either a ratio or position scale. </rdfs:comment>
      <rdfs:subClassOf>
         <owl:Class>
            <owl:intersectionOf rdf:parseType="Collection">
               <owl:Restriction>
                  <owl:onProperty rdf:resource="http://www.opengis.net/gml#uom"/>
                  <owl:allValuesFrom rdf:resource="http://www.w3.org/2001/XMLSchema#anyURI"/>
               </owl:Restriction>
            </owl:intersectionOf>
         </owl:Class>
      </rdfs:subClassOf>
      <rdfs:subClassOf>
         <owl:Restriction>
            <owl:onProperty rdf:resource="http://www.opengis.net/gml#hasdoubleOrNullList"/>
            <owl:someValuesFrom rdf:resource="doubleOrNullList"/>
         </owl:Restriction>
      </rdfs:subClassOf>
   </owl:Class>
   <owl:DatatypeProperty rdf:about="http://www.opengis.net/gml#hasdoubleOrNullList">
      <rdfs:domain rdf:resource="http://www.opengis.net/gml#MeasureOrNullListType"/>
      <rdfs:range rdf:resource="http://www.opengis.net/gml#doubleOrNullList"/>
   </owl:DatatypeProperty>
   <owl:Class rdf:about="http://www.opengis.net/gml#CoordinatesType">
      <rdfs:comment>Tables or arrays of tuples.  
        May be used for text-encoding of values from a table.  
        Actually just a string, but allows the user to indicate which characters are used as separators.  
        The value of the 'cs' attribute is the separator for coordinate values, 
        and the value of the 'ts' attribute gives the tuple separator (a single space by default); 
        the default values may be changed to reflect local usage.
        Defaults to CSV within a tuple, space between tuples.  
        However, any string content will be schema-valid.  </rdfs:comment>
      <rdfs:subClassOf>
         <owl:Class>
            <owl:intersectionOf rdf:parseType="Collection">
               <owl:Restriction>
                  <owl:onProperty rdf:resource="http://www.opengis.net/gml#decimal"/>
                  <owl:allValuesFrom rdf:resource="http://www.w3.org/2001/XMLSchema#string"/>
               </owl:Restriction>
               <owl:Restriction>
                  <owl:onProperty rdf:resource="http://www.opengis.net/gml#cs"/>
                  <owl:allValuesFrom rdf:resource="http://www.w3.org/2001/XMLSchema#string"/>
               </owl:Restriction>
               <owl:Restriction>
                  <owl:onProperty rdf:resource="http://www.opengis.net/gml#ts"/>
                  <owl:allValuesFrom rdf:resource="http://www.w3.org/2001/XMLSchema#string"/>
               </owl:Restriction>
            </owl:intersectionOf>
         </owl:Class>
      </rdfs:subClassOf>
      <rdfs:subClassOf>
         <owl:Restriction>
            <owl:onProperty rdf:resource="http://www.opengis.net/gml#hasstring"/>
            <owl:someValuesFrom rdf:resource="http://www.w3.org/2001/XMLSchema#string"/>
         </owl:Restriction>
      </rdfs:subClassOf>
   </owl:Class>
   <owl:DatatypeProperty rdf:about="http://www.opengis.net/gml#hasstring">
      <rdfs:domain rdf:resource="http://www.opengis.net/gml#CoordinatesType"/>
      <rdfs:range rdf:resource="http://www.w3.org/2001/XMLSchema#string"/>
   </owl:DatatypeProperty>
   <owl:Class rdf:about="http://www.opengis.net/gml#AbstractTimeObjectType">
      <rdfs:comment>This is an abstract class</rdfs:comment>
      <rdfs:comment xml:lang="en">The abstract supertype for temporal objects.</rdfs:comment>
      <rdfs:subClassOf rdf:resource="http://www.opengis.net/gml#AbstractGMLType"/>
   </owl:Class>
   <owl:Class rdf:about="http://www.opengis.net/gml#AbstractTimePrimitiveType">
      <rdfs:comment>This is an abstract class</rdfs:comment>
      <rdfs:comment xml:lang="en">The abstract supertype for temporal primitives.</rdfs:comment>
      <rdfs:subClassOf>
         <owl:Class>
            <owl:intersectionOf rdf:parseType="Collection">
               <owl:Restriction>
                  <owl:onProperty rdf:resource="http://www.opengis.net/gml#relatedTime"/>
                  <owl:allValuesFrom rdf:resource="http://www.opengis.net/gml#RelatedTimeType"/>
               </owl:Restriction>
               <owl:Restriction>
                  <owl:onProperty rdf:resource="http://www.opengis.net/gml#relatedTime"/>
                  <owl:minCardinality rdf:datatype="http://www.w3.org/2001/XMLSchema#nonNegativeInteger">0</owl:minCardinality>
               </owl:Restriction>
            </owl:intersectionOf>
         </owl:Class>
      </rdfs:subClassOf>
      <rdfs:subClassOf rdf:resource="http://www.opengis.net/gml#AbstractTimeObjectType"/>
   </owl:Class>
   <owl:Class rdf:about="http://www.opengis.net/gml#TimePrimitivePropertyType">
      <rdfs:subClassOf>
         <owl:Class>
            <owl:intersectionOf rdf:parseType="Collection">
               <owl:Restriction>
                  <owl:onProperty rdf:resource="http://www.opengis.net/gml#has_TimePrimitive"/>
                  <owl:allValuesFrom rdf:resource="http://www.opengis.net/gml#_TimePrimitive"/>
               </owl:Restriction>
            </owl:intersectionOf>
         </owl:Class>
      </rdfs:subClassOf>
   </owl:Class>
   <owl:Class rdf:about="http://www.opengis.net/gml#RelatedTimeType">
      <rdfs:subClassOf>
         <owl:Class>
            <owl:intersectionOf rdf:parseType="Collection">
               <owl:Restriction>
                  <owl:onProperty rdf:resource="http://www.opengis.net/gml#relativePosition"/>
                  <owl:allValuesFrom rdf:resource="http://www.w3.org/2001/XMLSchema#string"/>
               </owl:Restriction>
            </owl:intersectionOf>
         </owl:Class>
      </rdfs:subClassOf>
      <rdfs:subClassOf rdf:resource="http://www.opengis.net/gml#TimePrimitivePropertyType"/>
   </owl:Class>
   <owl:Class rdf:about="http://www.opengis.net/gml#AbstractTimeComplexType">
      <rdfs:comment>This is an abstract class</rdfs:comment>
      <rdfs:comment xml:lang="en">The abstract supertype for temporal complexes.</rdfs:comment>
      <rdfs:subClassOf rdf:resource="http://www.opengis.net/gml#AbstractTimeObjectType"/>
   </owl:Class>
   <owl:Class rdf:about="http://www.opengis.net/gml#AbstractTimeGeometricPrimitiveType">
      <rdfs:comment>This is an abstract class</rdfs:comment>
      <rdfs:comment xml:lang="en">The abstract supertype for temporal geometric primitives.
       A temporal geometry must be associated with a temporal reference system via URI. 
       The Gregorian calendar with UTC is the default reference system, following ISO 
       8601. Other reference systems in common use include the GPS calendar and the 
       Julian calendar.</rdfs:comment>
      <rdfs:subClassOf>
         <owl:Class>
            <owl:intersectionOf rdf:parseType="Collection">
               <owl:Restriction>
                  <owl:onProperty rdf:resource="http://www.opengis.net/gml#frame"/>
                  <owl:allValuesFrom rdf:resource="http://www.w3.org/2001/XMLSchema#anyURI"/>
               </owl:Restriction>
            </owl:intersectionOf>
         </owl:Class>
      </rdfs:subClassOf>
      <rdfs:subClassOf rdf:resource="http://www.opengis.net/gml#AbstractTimePrimitiveType"/>
   </owl:Class>
   <owl:Class rdf:about="http://www.opengis.net/gml#TimeGeometricPrimitivePropertyType">
      <rdfs:subClassOf>
         <owl:Class>
            <owl:intersectionOf rdf:parseType="Collection">
               <owl:Restriction>
                  <owl:onProperty rdf:resource="http://www.opengis.net/gml#has_TimeGeometricPrimitive"/>
                  <owl:allValuesFrom rdf:resource="http://www.opengis.net/gml#_TimeGeometricPrimitive"/>
               </owl:Restriction>
            </owl:intersectionOf>
         </owl:Class>
      </rdfs:subClassOf>
   </owl:Class>
   <owl:Class rdf:about="http://www.opengis.net/gml#TimeInstantType">
      <rdfs:comment>Omit back-pointers begunBy, endedBy.</rdfs:comment>
      <rdfs:subClassOf>
         <owl:Class>
            <owl:intersectionOf rdf:parseType="Collection">
               <owl:Restriction>
                  <owl:onProperty rdf:resource="http://www.opengis.net/gml#hastimePosition"/>
                  <owl:allValuesFrom rdf:resource="http://www.opengis.net/gml#timePosition"/>
               </owl:Restriction>
            </owl:intersectionOf>
         </owl:Class>
      </rdfs:subClassOf>
      <rdfs:subClassOf rdf:resource="http://www.opengis.net/gml#AbstractTimeGeometricPrimitiveType"/>
   </owl:Class>
   <owl:Class rdf:about="http://www.opengis.net/gml#TimeInstantPropertyType">
      <rdfs:subClassOf>
         <owl:Class>
            <owl:intersectionOf rdf:parseType="Collection">
               <owl:Restriction>
                  <owl:onProperty rdf:resource="http://www.opengis.net/gml#hasTimeInstant"/>
                  <owl:allValuesFrom rdf:resource="http://www.opengis.net/gml#TimeInstant"/>
               </owl:Restriction>
            </owl:intersectionOf>
         </owl:Class>
      </rdfs:subClassOf>
   </owl:Class>
   <owl:Class rdf:about="http://www.opengis.net/gml#TimePeriodType">
      <owl:disjointUnionOf rdf:parseType="Collection">
         <owl:Restriction>
            <owl:onProperty rdf:resource="http://www.opengis.net/gml#beginPosition"/>
            <owl:someValuesFrom rdf:resource="http://www.opengis.net/gml#TimePositionType"/>
         </owl:Restriction>
         <owl:Restriction>
            <owl:onProperty rdf:resource="http://www.opengis.net/gml#begin"/>
            <owl:someValuesFrom rdf:resource="http://www.opengis.net/gml#TimeInstantPropertyType"/>
         </owl:Restriction>
      </owl:disjointUnionOf>
      <owl:disjointUnionOf rdf:parseType="Collection">
         <owl:Restriction>
            <owl:onProperty rdf:resource="http://www.opengis.net/gml#endPosition"/>
            <owl:someValuesFrom rdf:resource="http://www.opengis.net/gml#TimePositionType"/>
         </owl:Restriction>
         <owl:Restriction>
            <owl:onProperty rdf:resource="http://www.opengis.net/gml#end"/>
            <owl:someValuesFrom rdf:resource="http://www.opengis.net/gml#TimeInstantPropertyType"/>
         </owl:Restriction>
      </owl:disjointUnionOf>
      <rdfs:subClassOf rdf:resource="http://www.opengis.net/gml#timeLength"/>
      <rdfs:subClassOf rdf:resource="http://www.opengis.net/gml#AbstractTimeGeometricPrimitiveType"/>
   </owl:Class>
   <owl:Class rdf:about="http://www.opengis.net/gml#TimePeriodPropertyType">
      <rdfs:subClassOf>
         <owl:Class>
            <owl:intersectionOf rdf:parseType="Collection">
               <owl:Restriction>
                  <owl:onProperty rdf:resource="http://www.opengis.net/gml#hasTimePeriod"/>
                  <owl:allValuesFrom rdf:resource="http://www.opengis.net/gml#TimePeriod"/>
               </owl:Restriction>
            </owl:intersectionOf>
         </owl:Class>
      </rdfs:subClassOf>
   </owl:Class>
   <owl:Class rdf:about="http://www.opengis.net/gml#TimeIntervalLengthType">
      <rdfs:comment xml:lang="en">This type extends the built-in xsd:decimal simple type to allow floating-point 
      values for temporal length. According to  the ISO 11404 model you have to use 
      positiveInteger together with appropriate values for radix and factor. The 
      resolution of the time interval is to one radix ^(-factor) of the specified 
      time unit (e.g. unit="second", radix="10", factor="3" specifies a resolution 
      of milliseconds). It is a subtype of TimeDurationType.</rdfs:comment>
      <rdfs:subClassOf>
         <owl:Class>
            <owl:intersectionOf rdf:parseType="Collection">
               <owl:Restriction>
                  <owl:onProperty rdf:resource="http://www.opengis.net/gml#unit"/>
                  <owl:allValuesFrom rdf:resource="http://www.opengis.net/gml#TimeUnitType"/>
               </owl:Restriction>
               <owl:Restriction>
                  <owl:onProperty rdf:resource="http://www.opengis.net/gml#radix"/>
                  <owl:allValuesFrom rdf:resource="http://www.w3.org/2001/XMLSchema#positiveInteger"/>
               </owl:Restriction>
               <owl:Restriction>
                  <owl:onProperty rdf:resource="http://www.opengis.net/gml#factor"/>
                  <owl:allValuesFrom rdf:resource="http://www.w3.org/2001/XMLSchema#integer"/>
               </owl:Restriction>
            </owl:intersectionOf>
         </owl:Class>
      </rdfs:subClassOf>
      <rdfs:subClassOf>
         <owl:Restriction>
            <owl:onProperty rdf:resource="http://www.opengis.net/gml#hasdecimal"/>
            <owl:someValuesFrom rdf:resource="http://www.w3.org/2001/XMLSchema#decimal"/>
         </owl:Restriction>
      </rdfs:subClassOf>
   </owl:Class>
   <owl:DatatypeProperty rdf:about="http://www.opengis.net/gml#hasdecimal">
      <rdfs:domain rdf:resource="http://www.opengis.net/gml#TimeIntervalLengthType"/>
      <rdfs:range rdf:resource="http://www.w3.org/2001/XMLSchema#decimal"/>
   </owl:DatatypeProperty>
   <owl:Class rdf:about="http://www.opengis.net/gml#TimePositionType">
      <rdfs:comment xml:lang="en">Direct representation of a temporal position. 
      Indeterminate time values are also allowed, as described in ISO 19108. The indeterminatePosition 
      attribute can be used alone or it can qualify a specific value for temporal position (e.g. before 
      2002-12, after 1019624400). 
      For time values that identify position within a calendar, the calendarEraName attribute provides 
      the name of the calendar era to which the date is referenced (e.g. the Meiji era of the Japanese calendar).</rdfs:comment>
      <rdfs:subClassOf>
         <owl:Class>
            <owl:intersectionOf rdf:parseType="Collection">
               <owl:Restriction>
                  <owl:onProperty rdf:resource="http://www.opengis.net/gml#frame"/>
                  <owl:allValuesFrom rdf:resource="http://www.w3.org/2001/XMLSchema#anyURI"/>
               </owl:Restriction>
               <owl:Restriction>
                  <owl:onProperty rdf:resource="http://www.opengis.net/gml#calendarEraName"/>
                  <owl:allValuesFrom rdf:resource="http://www.w3.org/2001/XMLSchema#string"/>
               </owl:Restriction>
               <owl:Restriction>
                  <owl:onProperty rdf:resource="http://www.opengis.net/gml#indeterminatePosition"/>
                  <owl:allValuesFrom rdf:resource="http://www.opengis.net/gml#TimeIndeterminateValueType"/>
               </owl:Restriction>
            </owl:intersectionOf>
         </owl:Class>
      </rdfs:subClassOf>
      <rdfs:subClassOf>
         <owl:Restriction>
            <owl:onProperty rdf:resource="http://www.opengis.net/gml#hasTimePositionUnion"/>
            <owl:someValuesFrom rdf:resource="TimePositionUnion"/>
         </owl:Restriction>
      </rdfs:subClassOf>
   </owl:Class>
   <owl:DatatypeProperty rdf:about="http://www.opengis.net/gml#hasTimePositionUnion">
      <rdfs:domain rdf:resource="http://www.opengis.net/gml#TimePositionType"/>
      <rdfs:range rdf:resource="http://www.opengis.net/gml#TimePositionUnion"/>
   </owl:DatatypeProperty>
   <owl:Class rdf:about="http://www.opengis.net/gml#DirectionPropertyType">
      <owl:disjointUnionOf rdf:parseType="Collection">
         <owl:Restriction>
            <owl:onProperty rdf:resource="http://www.opengis.net/gml#hasDirectionVector"/>
            <owl:someValuesFrom rdf:resource="http://www.opengis.net/gml#DirectionVector"/>
         </owl:Restriction>
         <owl:Restriction>
            <owl:onProperty rdf:resource="http://www.opengis.net/gml#hasCompassPoint"/>
            <owl:someValuesFrom rdf:resource="http://www.opengis.net/gml#CompassPoint"/>
         </owl:Restriction>
         <owl:Restriction>
            <owl:onProperty rdf:resource="http://www.opengis.net/gml#DirectionKeyword"/>
            <owl:someValuesFrom rdf:resource="http://www.opengis.net/gml#CodeType"/>
         </owl:Restriction>
         <owl:Restriction>
            <owl:onProperty rdf:resource="http://www.opengis.net/gml#DirectionString"/>
            <owl:someValuesFrom rdf:resource="http://www.opengis.net/gml#StringOrRefType"/>
         </owl:Restriction>
      </owl:disjointUnionOf>
   </owl:Class>
   <owl:Class rdf:about="http://www.opengis.net/gml#DirectionVectorType">
      <rdfs:comment>Direction expressed as a vector, either using components, or using angles.</rdfs:comment>
      <owl:disjointUnionOf rdf:parseType="Collection">
         <owl:Restriction>
            <owl:onProperty rdf:resource="http://www.opengis.net/gml#hasvector"/>
            <owl:someValuesFrom rdf:resource="http://www.opengis.net/gml#vector"/>
         </owl:Restriction>
         <owl:Restriction>
            <owl:intersectionOf rdf:parseType="Collection">
               <owl:Restriction>
                  <owl:onProperty rdf:resource="http://www.opengis.net/gml#horizontalAngle"/>
                  <owl:allValuesFrom rdf:resource="http://www.opengis.net/gml#AngleType"/>
               </owl:Restriction>
               <owl:Restriction>
                  <owl:onProperty rdf:resource="http://www.opengis.net/gml#verticalAngle"/>
                  <owl:allValuesFrom rdf:resource="http://www.opengis.net/gml#AngleType"/>
               </owl:Restriction>
            </owl:intersectionOf>
         </owl:Restriction>
      </owl:disjointUnionOf>
   </owl:Class>
   <owl:Class rdf:about="http://www.opengis.net/gml#AbstractTopologyType">
      <rdfs:comment>This is an abstract class</rdfs:comment>
      <rdfs:subClassOf rdf:resource="http://www.opengis.net/gml#AbstractGMLType"/>
   </owl:Class>
   <owl:Class rdf:about="http://www.opengis.net/gml#AbstractTopoPrimitiveType">
      <rdfs:comment>This is an abstract class</rdfs:comment>
      <rdfs:subClassOf>
         <owl:Class>
            <owl:intersectionOf rdf:parseType="Collection">
               <owl:Restriction>
                  <owl:onProperty rdf:resource="http://www.opengis.net/gml#hasisolated"/>
                  <owl:allValuesFrom rdf:resource="http://www.opengis.net/gml#isolated"/>
               </owl:Restriction>
               <owl:Restriction>
                  <owl:onProperty rdf:resource="http://www.opengis.net/gml#hasisolated"/>
                  <owl:minCardinality rdf:datatype="http://www.w3.org/2001/XMLSchema#nonNegativeInteger">0</owl:minCardinality>
               </owl:Restriction>
               <owl:Restriction>
                  <owl:onProperty rdf:resource="http://www.opengis.net/gml#hascontainer"/>
                  <owl:allValuesFrom rdf:resource="http://www.opengis.net/gml#container"/>
               </owl:Restriction>
               <owl:Restriction>
                  <owl:onProperty rdf:resource="http://www.opengis.net/gml#hascontainer"/>
                  <owl:minCardinality rdf:datatype="http://www.w3.org/2001/XMLSchema#nonNegativeInteger">0</owl:minCardinality>
               </owl:Restriction>
            </owl:intersectionOf>
         </owl:Class>
      </rdfs:subClassOf>
      <rdfs:subClassOf rdf:resource="http://www.opengis.net/gml#AbstractTopologyType"/>
   </owl:Class>
   <owl:Class rdf:about="http://www.opengis.net/gml#IsolatedPropertyType">
      <owl:disjointUnionOf rdf:parseType="Collection">
         <owl:Restriction>
            <owl:onProperty rdf:resource="http://www.opengis.net/gml#hasNode"/>
            <owl:someValuesFrom rdf:resource="http://www.opengis.net/gml#Node"/>
         </owl:Restriction>
         <owl:Restriction>
            <owl:onProperty rdf:resource="http://www.opengis.net/gml#hasEdge"/>
            <owl:someValuesFrom rdf:resource="http://www.opengis.net/gml#Edge"/>
         </owl:Restriction>
      </owl:disjointUnionOf>
   </owl:Class>
   <owl:Class rdf:about="http://www.opengis.net/gml#ContainerPropertyType">
      <owl:disjointUnionOf rdf:parseType="Collection">
         <owl:Restriction>
            <owl:onProperty rdf:resource="http://www.opengis.net/gml#hasFace"/>
            <owl:someValuesFrom rdf:resource="http://www.opengis.net/gml#Face"/>
         </owl:Restriction>
         <owl:Restriction>
            <owl:onProperty rdf:resource="http://www.opengis.net/gml#hasTopoSolid"/>
            <owl:someValuesFrom rdf:resource="http://www.opengis.net/gml#TopoSolid"/>
         </owl:Restriction>
      </owl:disjointUnionOf>
   </owl:Class>
   <owl:Class rdf:about="http://www.opengis.net/gml#NodeType">
      <rdfs:comment>Its optional co-boundary is a set of connected directedEdges.  The orientation of one of these dirEdges is "+" if the Node is the "to" node of the Edge, and "-" if it is the "from" node.</rdfs:comment>
      <rdfs:subClassOf>
         <owl:Class>
            <owl:intersectionOf rdf:parseType="Collection">
               <owl:Restriction>
                  <owl:onProperty rdf:resource="http://www.opengis.net/gml#hasdirectedEdge"/>
                  <owl:allValuesFrom rdf:resource="http://www.opengis.net/gml#directedEdge"/>
               </owl:Restriction>
               <owl:Restriction>
                  <owl:onProperty rdf:resource="http://www.opengis.net/gml#hasdirectedEdge"/>
                  <owl:minCardinality rdf:datatype="http://www.w3.org/2001/XMLSchema#nonNegativeInteger">0</owl:minCardinality>
               </owl:Restriction>
               <owl:Restriction>
                  <owl:onProperty rdf:resource="http://www.opengis.net/gml#haspointProperty"/>
                  <owl:allValuesFrom rdf:resource="http://www.opengis.net/gml#pointProperty"/>
               </owl:Restriction>
               <owl:Restriction>
                  <owl:onProperty rdf:resource="http://www.opengis.net/gml#haspointProperty"/>
                  <owl:minCardinality rdf:datatype="http://www.w3.org/2001/XMLSchema#nonNegativeInteger">0</owl:minCardinality>
               </owl:Restriction>
            </owl:intersectionOf>
         </owl:Class>
      </rdfs:subClassOf>
      <rdfs:subClassOf rdf:resource="http://www.opengis.net/gml#AbstractTopoPrimitiveType"/>
   </owl:Class>
   <owl:Class rdf:about="http://www.opengis.net/gml#DirectedNodePropertyType">
      <rdfs:subClassOf>
         <owl:Class>
            <owl:intersectionOf rdf:parseType="Collection">
               <owl:Restriction>
                  <owl:onProperty rdf:resource="http://www.opengis.net/gml#hasNode"/>
                  <owl:allValuesFrom rdf:resource="http://www.opengis.net/gml#Node"/>
               </owl:Restriction>
            </owl:intersectionOf>
         </owl:Class>
      </rdfs:subClassOf>
      <rdfs:subClassOf>
         <owl:Class>
            <owl:intersectionOf rdf:parseType="Collection">
               <owl:Restriction>
                  <owl:onProperty rdf:resource="http://www.opengis.net/gml#orientation"/>
                  <owl:allValuesFrom rdf:resource="http://www.opengis.net/gml#SignType"/>
               </owl:Restriction>
            </owl:intersectionOf>
         </owl:Class>
      </rdfs:subClassOf>
   </owl:Class>
   <owl:Class rdf:about="http://www.opengis.net/gml#EdgeType">
      <rdfs:comment>There is precisely one positively directed and one negatively directed node in the boundary of every edge. The negatively and positively directed nodes correspond to the start and end nodes respectively. The optional coboundary of an edge is a circular sequence of directed faces which are incident on this edge in document order. Faces which use a particular boundary edge in its positive orientation appear with positive orientation on the coboundary of the same edge. In the 2D case, the orientation of the face on the left of the edge is "+"; the orientation of the face on the right on its right is "-". An edge may optionally be realised by a 1-dimensional (curve) geometric primitive.</rdfs:comment>
      <rdfs:subClassOf>
         <owl:Class>
            <owl:intersectionOf rdf:parseType="Collection">
               <owl:Restriction>
                  <owl:onProperty rdf:resource="http://www.opengis.net/gml#hasdirectedNode"/>
                  <owl:allValuesFrom rdf:resource="http://www.opengis.net/gml#directedNode"/>
               </owl:Restriction>
               <owl:Restriction>
                  <owl:onProperty rdf:resource="http://www.opengis.net/gml#hasdirectedNode"/>
                  <owl:cardinality rdf:datatype="http://www.w3.org/2001/XMLSchema#nonNegativeInteger">2</owl:cardinality>
               </owl:Restriction>
               <owl:Restriction>
                  <owl:onProperty rdf:resource="http://www.opengis.net/gml#hasdirectedFace"/>
                  <owl:allValuesFrom rdf:resource="http://www.opengis.net/gml#directedFace"/>
               </owl:Restriction>
               <owl:Restriction>
                  <owl:onProperty rdf:resource="http://www.opengis.net/gml#hasdirectedFace"/>
                  <owl:minCardinality rdf:datatype="http://www.w3.org/2001/XMLSchema#nonNegativeInteger">0</owl:minCardinality>
               </owl:Restriction>
               <owl:Restriction>
                  <owl:onProperty rdf:resource="http://www.opengis.net/gml#hascurveProperty"/>
                  <owl:allValuesFrom rdf:resource="http://www.opengis.net/gml#curveProperty"/>
               </owl:Restriction>
               <owl:Restriction>
                  <owl:onProperty rdf:resource="http://www.opengis.net/gml#hascurveProperty"/>
                  <owl:minCardinality rdf:datatype="http://www.w3.org/2001/XMLSchema#nonNegativeInteger">0</owl:minCardinality>
               </owl:Restriction>
            </owl:intersectionOf>
         </owl:Class>
      </rdfs:subClassOf>
      <rdfs:subClassOf rdf:resource="http://www.opengis.net/gml#AbstractTopoPrimitiveType"/>
   </owl:Class>
   <owl:Class rdf:about="http://www.opengis.net/gml#DirectedEdgePropertyType">
      <rdfs:subClassOf>
         <owl:Class>
            <owl:intersectionOf rdf:parseType="Collection">
               <owl:Restriction>
                  <owl:onProperty rdf:resource="http://www.opengis.net/gml#hasEdge"/>
                  <owl:allValuesFrom rdf:resource="http://www.opengis.net/gml#Edge"/>
               </owl:Restriction>
            </owl:intersectionOf>
         </owl:Class>
      </rdfs:subClassOf>
      <rdfs:subClassOf>
         <owl:Class>
            <owl:intersectionOf rdf:parseType="Collection">
               <owl:Restriction>
                  <owl:onProperty rdf:resource="http://www.opengis.net/gml#orientation"/>
                  <owl:allValuesFrom rdf:resource="http://www.opengis.net/gml#SignType"/>
               </owl:Restriction>
            </owl:intersectionOf>
         </owl:Class>
      </rdfs:subClassOf>
   </owl:Class>
   <owl:Class rdf:about="http://www.opengis.net/gml#FaceType">
      <rdfs:comment>. The topological boundary of a face consists of a set of directed edges. Note that all edges associated with a Face, including dangling and interior edges, appear in the boundary.  Dangling and interior edges are each referenced by pairs of directedEdges with opposing orientations.  The optional coboundary of a face is a pair of directed solids which are bounded by this face. If present, there is precisely one positively directed and one negatively directed solid in the coboundary of every face. The positively directed solid corresponds to the solid which lies in the direction of the positively directed normal to the face in any geometric realisation.  A face may optionally be realised by a 2-dimensional (surface) geometric primitive.</rdfs:comment>
      <rdfs:subClassOf>
         <owl:Class>
            <owl:intersectionOf rdf:parseType="Collection">
               <owl:Restriction>
                  <owl:onProperty rdf:resource="http://www.opengis.net/gml#hasdirectedEdge"/>
                  <owl:allValuesFrom rdf:resource="http://www.opengis.net/gml#directedEdge"/>
               </owl:Restriction>
               <owl:Restriction>
                  <owl:onProperty rdf:resource="http://www.opengis.net/gml#hasdirectedTopoSolid"/>
                  <owl:allValuesFrom rdf:resource="http://www.opengis.net/gml#directedTopoSolid"/>
               </owl:Restriction>
               <owl:Restriction>
                  <owl:onProperty rdf:resource="http://www.opengis.net/gml#hasdirectedTopoSolid"/>
                  <owl:minCardinality rdf:datatype="http://www.w3.org/2001/XMLSchema#nonNegativeInteger">0</owl:minCardinality>
                  <owl:onProperty rdf:resource="http://www.opengis.net/gml#hasdirectedTopoSolid"/>
                  <owl:minCardinality rdf:datatype="http://www.w3.org/2001/XMLSchema#nonNegativeInteger">2</owl:minCardinality>
               </owl:Restriction>
               <owl:Restriction>
                  <owl:onProperty rdf:resource="http://www.opengis.net/gml#hassurfaceProperty"/>
                  <owl:allValuesFrom rdf:resource="http://www.opengis.net/gml#surfaceProperty"/>
               </owl:Restriction>
               <owl:Restriction>
                  <owl:onProperty rdf:resource="http://www.opengis.net/gml#hassurfaceProperty"/>
                  <owl:minCardinality rdf:datatype="http://www.w3.org/2001/XMLSchema#nonNegativeInteger">0</owl:minCardinality>
               </owl:Restriction>
            </owl:intersectionOf>
         </owl:Class>
      </rdfs:subClassOf>
      <rdfs:subClassOf rdf:resource="http://www.opengis.net/gml#AbstractTopoPrimitiveType"/>
   </owl:Class>
   <owl:Class rdf:about="http://www.opengis.net/gml#DirectedFacePropertyType">
      <rdfs:subClassOf>
         <owl:Class>
            <owl:intersectionOf rdf:parseType="Collection">
               <owl:Restriction>
                  <owl:onProperty rdf:resource="http://www.opengis.net/gml#hasFace"/>
                  <owl:allValuesFrom rdf:resource="http://www.opengis.net/gml#Face"/>
               </owl:Restriction>
            </owl:intersectionOf>
         </owl:Class>
      </rdfs:subClassOf>
      <rdfs:subClassOf>
         <owl:Class>
            <owl:intersectionOf rdf:parseType="Collection">
               <owl:Restriction>
                  <owl:onProperty rdf:resource="http://www.opengis.net/gml#orientation"/>
                  <owl:allValuesFrom rdf:resource="http://www.opengis.net/gml#SignType"/>
               </owl:Restriction>
            </owl:intersectionOf>
         </owl:Class>
      </rdfs:subClassOf>
   </owl:Class>
   <owl:Class rdf:about="http://www.opengis.net/gml#TopoSolidType">
      <rdfs:comment>The topological boundary of a TopoSolid consists of a set of directed faces. Note that all faces associated with the TopoSolid, including dangling faces, appear in the boundary. The coboundary of a TopoSolid is empty and hence requires no representation.</rdfs:comment>
      <rdfs:subClassOf>
         <owl:Class>
            <owl:intersectionOf rdf:parseType="Collection">
               <owl:Restriction>
                  <owl:onProperty rdf:resource="http://www.opengis.net/gml#hasdirectedFace"/>
                  <owl:allValuesFrom rdf:resource="http://www.opengis.net/gml#directedFace"/>
               </owl:Restriction>
            </owl:intersectionOf>
         </owl:Class>
      </rdfs:subClassOf>
      <rdfs:subClassOf rdf:resource="http://www.opengis.net/gml#AbstractTopoPrimitiveType"/>
   </owl:Class>
   <owl:Class rdf:about="http://www.opengis.net/gml#DirectedTopoSolidPropertyType">
      <rdfs:subClassOf>
         <owl:Class>
            <owl:intersectionOf rdf:parseType="Collection">
               <owl:Restriction>
                  <owl:onProperty rdf:resource="http://www.opengis.net/gml#hasTopoSolid"/>
                  <owl:allValuesFrom rdf:resource="http://www.opengis.net/gml#TopoSolid"/>
               </owl:Restriction>
            </owl:intersectionOf>
         </owl:Class>
      </rdfs:subClassOf>
      <rdfs:subClassOf>
         <owl:Class>
            <owl:intersectionOf rdf:parseType="Collection">
               <owl:Restriction>
                  <owl:onProperty rdf:resource="http://www.opengis.net/gml#orientation"/>
                  <owl:allValuesFrom rdf:resource="http://www.opengis.net/gml#SignType"/>
               </owl:Restriction>
            </owl:intersectionOf>
         </owl:Class>
      </rdfs:subClassOf>
   </owl:Class>
   <owl:Class rdf:about="http://www.opengis.net/gml#TopoPointType">
      <rdfs:comment>The intended use of TopoPoint is to appear within a point feature to express the structural and possibly geometric relationships of this point to other features via shared node definitions. Note the orientation assigned to the directedNode has no meaning in this context. It is preserved for symmetry with the types and elements which follow.</rdfs:comment>
      <rdfs:subClassOf>
         <owl:Class>
            <owl:intersectionOf rdf:parseType="Collection">
               <owl:Restriction>
                  <owl:onProperty rdf:resource="http://www.opengis.net/gml#hasdirectedNode"/>
                  <owl:allValuesFrom rdf:resource="http://www.opengis.net/gml#directedNode"/>
               </owl:Restriction>
            </owl:intersectionOf>
         </owl:Class>
      </rdfs:subClassOf>
      <rdfs:subClassOf rdf:resource="http://www.opengis.net/gml#AbstractTopologyType"/>
   </owl:Class>
   <owl:Class rdf:about="http://www.opengis.net/gml#TopoPointPropertyType">
      <rdfs:subClassOf>
         <owl:Class>
            <owl:intersectionOf rdf:parseType="Collection">
               <owl:Restriction>
                  <owl:onProperty rdf:resource="http://www.opengis.net/gml#hasTopoPoint"/>
                  <owl:allValuesFrom rdf:resource="http://www.opengis.net/gml#TopoPoint"/>
               </owl:Restriction>
            </owl:intersectionOf>
         </owl:Class>
      </rdfs:subClassOf>
   </owl:Class>
   <owl:Class rdf:about="http://www.opengis.net/gml#TopoCurveType">
      <rdfs:comment>The end Node of each directedEdge of a TopoCurveType
is the start Node of the next directedEdge of the TopoCurveType in document order.  The TopoCurve type and element represent a homogeneous topological expression, a list of directed edges, which if realised are isomorphic to a geometric curve primitive. The intended use of TopoCurve is to appear within a line feature instance to express the structural and geometric relationships of this line to other features via the shared edge definitions.</rdfs:comment>
      <rdfs:subClassOf>
         <owl:Class>
            <owl:intersectionOf rdf:parseType="Collection">
               <owl:Restriction>
                  <owl:onProperty rdf:resource="http://www.opengis.net/gml#hasdirectedEdge"/>
                  <owl:allValuesFrom rdf:resource="http://www.opengis.net/gml#directedEdge"/>
               </owl:Restriction>
            </owl:intersectionOf>
         </owl:Class>
      </rdfs:subClassOf>
      <rdfs:subClassOf rdf:resource="http://www.opengis.net/gml#AbstractTopologyType"/>
   </owl:Class>
   <owl:Class rdf:about="http://www.opengis.net/gml#TopoCurvePropertyType">
      <rdfs:subClassOf>
         <owl:Class>
            <owl:intersectionOf rdf:parseType="Collection">
               <owl:Restriction>
                  <owl:onProperty rdf:resource="http://www.opengis.net/gml#hasTopoCurve"/>
                  <owl:allValuesFrom rdf:resource="http://www.opengis.net/gml#TopoCurve"/>
               </owl:Restriction>
            </owl:intersectionOf>
         </owl:Class>
      </rdfs:subClassOf>
   </owl:Class>
   <owl:Class rdf:about="http://www.opengis.net/gml#TopoSurfaceType">
      <rdfs:comment>The TopoSurface type and element represent a homogeneous topological expression, a set of directed faces, which if realised are isomorphic to a geometric surface primitive. The intended use of TopoSurface is to appear within a surface feature instance to express the structural and possibly geometric relationships of this surface to other features via the shared face definitions.</rdfs:comment>
      <rdfs:subClassOf>
         <owl:Class>
            <owl:intersectionOf rdf:parseType="Collection">
               <owl:Restriction>
                  <owl:onProperty rdf:resource="http://www.opengis.net/gml#hasdirectedFace"/>
                  <owl:allValuesFrom rdf:resource="http://www.opengis.net/gml#directedFace"/>
               </owl:Restriction>
            </owl:intersectionOf>
         </owl:Class>
      </rdfs:subClassOf>
      <rdfs:subClassOf rdf:resource="http://www.opengis.net/gml#AbstractTopologyType"/>
   </owl:Class>
   <owl:Class rdf:about="http://www.opengis.net/gml#TopoSurfacePropertyType">
      <rdfs:subClassOf>
         <owl:Class>
            <owl:intersectionOf rdf:parseType="Collection">
               <owl:Restriction>
                  <owl:onProperty rdf:resource="http://www.opengis.net/gml#hasTopoSurface"/>
                  <owl:allValuesFrom rdf:resource="http://www.opengis.net/gml#TopoSurface"/>
               </owl:Restriction>
            </owl:intersectionOf>
         </owl:Class>
      </rdfs:subClassOf>
   </owl:Class>
   <owl:Class rdf:about="http://www.opengis.net/gml#TopoVolumeType">
      <rdfs:comment>The TopoVolume type and element represent a homogeneous topological expression, a set of directed TopoSolids, which if realised are isomorphic to a geometric solid primitive. The intended use of TopoVolume is to appear within a 3D solid feature instance to express the structural and geometric relationships of this solid to other features via the shared TopoSolid definitions.  . Note the orientation assigned to the directedSolid has no meaning in three dimensions. It is preserved for symmetry with the preceding types and elements.</rdfs:comment>
      <rdfs:subClassOf>
         <owl:Class>
            <owl:intersectionOf rdf:parseType="Collection">
               <owl:Restriction>
                  <owl:onProperty rdf:resource="http://www.opengis.net/gml#hasdirectedTopoSolid"/>
                  <owl:allValuesFrom rdf:resource="http://www.opengis.net/gml#directedTopoSolid"/>
               </owl:Restriction>
            </owl:intersectionOf>
         </owl:Class>
      </rdfs:subClassOf>
      <rdfs:subClassOf rdf:resource="http://www.opengis.net/gml#AbstractTopologyType"/>
   </owl:Class>
   <owl:Class rdf:about="http://www.opengis.net/gml#TopoVolumePropertyType">
      <rdfs:subClassOf>
         <owl:Class>
            <owl:intersectionOf rdf:parseType="Collection">
               <owl:Restriction>
                  <owl:onProperty rdf:resource="http://www.opengis.net/gml#hasTopoVolume"/>
                  <owl:allValuesFrom rdf:resource="http://www.opengis.net/gml#TopoVolume"/>
               </owl:Restriction>
            </owl:intersectionOf>
         </owl:Class>
      </rdfs:subClassOf>
   </owl:Class>
   <owl:Class rdf:about="http://www.opengis.net/gml#TopoComplexType">
      <rdfs:comment>This type represents a TP_Complex capable of holding topological primitives.</rdfs:comment>
      <rdfs:subClassOf>
         <owl:Class>
            <owl:intersectionOf rdf:parseType="Collection">
               <owl:Restriction>
                  <owl:onProperty rdf:resource="http://www.opengis.net/gml#hasmaximalComplex"/>
                  <owl:allValuesFrom rdf:resource="http://www.opengis.net/gml#maximalComplex"/>
               </owl:Restriction>
               <owl:Restriction>
                  <owl:onProperty rdf:resource="http://www.opengis.net/gml#hassuperComplex"/>
                  <owl:allValuesFrom rdf:resource="http://www.opengis.net/gml#superComplex"/>
               </owl:Restriction>
               <owl:Restriction>
                  <owl:onProperty rdf:resource="http://www.opengis.net/gml#hassuperComplex"/>
                  <owl:minCardinality rdf:datatype="http://www.w3.org/2001/XMLSchema#nonNegativeInteger">0</owl:minCardinality>
               </owl:Restriction>
               <owl:Restriction>
                  <owl:onProperty rdf:resource="http://www.opengis.net/gml#hassubComplex"/>
                  <owl:allValuesFrom rdf:resource="http://www.opengis.net/gml#subComplex"/>
               </owl:Restriction>
               <owl:Restriction>
                  <owl:onProperty rdf:resource="http://www.opengis.net/gml#hassubComplex"/>
                  <owl:minCardinality rdf:datatype="http://www.w3.org/2001/XMLSchema#nonNegativeInteger">0</owl:minCardinality>
               </owl:Restriction>
               <owl:Restriction>
                  <owl:onProperty rdf:resource="http://www.opengis.net/gml#hastopoPrimitiveMember"/>
                  <owl:allValuesFrom rdf:resource="http://www.opengis.net/gml#topoPrimitiveMember"/>
               </owl:Restriction>
               <owl:Restriction>
                  <owl:onProperty rdf:resource="http://www.opengis.net/gml#hastopoPrimitiveMember"/>
                  <owl:minCardinality rdf:datatype="http://www.w3.org/2001/XMLSchema#nonNegativeInteger">0</owl:minCardinality>
               </owl:Restriction>
               <owl:Restriction>
                  <owl:onProperty rdf:resource="http://www.opengis.net/gml#hastopoPrimitiveMembers"/>
                  <owl:allValuesFrom rdf:resource="http://www.opengis.net/gml#topoPrimitiveMembers"/>
               </owl:Restriction>
               <owl:Restriction>
                  <owl:onProperty rdf:resource="http://www.opengis.net/gml#hastopoPrimitiveMembers"/>
                  <owl:minCardinality rdf:datatype="http://www.w3.org/2001/XMLSchema#nonNegativeInteger">0</owl:minCardinality>
               </owl:Restriction>
            </owl:intersectionOf>
         </owl:Class>
      </rdfs:subClassOf>
      <rdfs:subClassOf>
         <owl:Class>
            <owl:intersectionOf rdf:parseType="Collection">
               <owl:Restriction>
                  <owl:onProperty rdf:resource="http://www.opengis.net/gml#isMaximal"/>
                  <owl:allValuesFrom rdf:resource="http://www.w3.org/2001/XMLSchema#boolean"/>
               </owl:Restriction>
            </owl:intersectionOf>
         </owl:Class>
      </rdfs:subClassOf>
      <rdfs:subClassOf rdf:resource="http://www.opengis.net/gml#AbstractTopologyType"/>
   </owl:Class>
   <owl:Class rdf:about="http://www.opengis.net/gml#TopoComplexMemberType">
      <rdfs:comment>This Property can be used to embed a TopoComplex in a feature collection.</rdfs:comment>
      <rdfs:subClassOf>
         <owl:Class>
            <owl:intersectionOf rdf:parseType="Collection">
               <owl:Restriction>
                  <owl:onProperty rdf:resource="http://www.opengis.net/gml#hasTopoComplex"/>
                  <owl:allValuesFrom rdf:resource="http://www.opengis.net/gml#TopoComplex"/>
               </owl:Restriction>
               <owl:Restriction>
                  <owl:onProperty rdf:resource="http://www.opengis.net/gml#hasTopoComplex"/>
                  <owl:minCardinality rdf:datatype="http://www.w3.org/2001/XMLSchema#nonNegativeInteger">0</owl:minCardinality>
               </owl:Restriction>
            </owl:intersectionOf>
         </owl:Class>
      </rdfs:subClassOf>
   </owl:Class>
   <owl:Class rdf:about="http://www.opengis.net/gml#TopoPrimitiveMemberType">
      <rdfs:comment>This type supports embedding topological primitives in a TopoComplex.</rdfs:comment>
      <rdfs:subClassOf>
         <owl:Class>
            <owl:intersectionOf rdf:parseType="Collection">
               <owl:Restriction>
                  <owl:onProperty rdf:resource="http://www.opengis.net/gml#has_TopoPrimitive"/>
                  <owl:allValuesFrom rdf:resource="http://www.opengis.net/gml#_TopoPrimitive"/>
               </owl:Restriction>
               <owl:Restriction>
                  <owl:onProperty rdf:resource="http://www.opengis.net/gml#has_TopoPrimitive"/>
                  <owl:minCardinality rdf:datatype="http://www.w3.org/2001/XMLSchema#nonNegativeInteger">0</owl:minCardinality>
               </owl:Restriction>
            </owl:intersectionOf>
         </owl:Class>
      </rdfs:subClassOf>
   </owl:Class>
   <owl:Class rdf:about="http://www.opengis.net/gml#TopoPrimitiveArrayAssociationType">
      <rdfs:comment>This type supports embedding an array of topological primitives in a TopoComplex</rdfs:comment>
      <owl:disjointUnionOf rdf:parseType="Collection">
         <owl:Restriction>
            <owl:onProperty rdf:resource="http://www.opengis.net/gml#has_TopoPrimitive"/>
            <owl:someValuesFrom rdf:resource="http://www.opengis.net/gml#_TopoPrimitive"/>
         </owl:Restriction>
      </owl:disjointUnionOf>
   </owl:Class>
   <owl:Class rdf:about="http://www.opengis.net/gml#CompositeCurveType">
      <rdfs:comment>A CompositeCurve is defined by a sequence of (orientable) curves such that the each curve in the sequence terminates at the start point of the subsequent curve in the list.</rdfs:comment>
      <rdfs:subClassOf>
         <owl:Class>
            <owl:intersectionOf rdf:parseType="Collection">
               <owl:Restriction>
                  <owl:onProperty rdf:resource="http://www.opengis.net/gml#hascurveMember"/>
                  <owl:allValuesFrom rdf:resource="http://www.opengis.net/gml#curveMember"/>
               </owl:Restriction>
            </owl:intersectionOf>
         </owl:Class>
      </rdfs:subClassOf>
      <rdfs:subClassOf rdf:resource="http://www.opengis.net/gml#AbstractCurveType"/>
   </owl:Class>
   <owl:Class rdf:about="http://www.opengis.net/gml#CompositeCurvePropertyType">
      <rdfs:subClassOf>
         <owl:Class>
            <owl:intersectionOf rdf:parseType="Collection">
               <owl:Restriction>
                  <owl:onProperty rdf:resource="http://www.opengis.net/gml#hasCompositeCurve"/>
                  <owl:allValuesFrom rdf:resource="http://www.opengis.net/gml#CompositeCurve"/>
               </owl:Restriction>
            </owl:intersectionOf>
         </owl:Class>
      </rdfs:subClassOf>
   </owl:Class>
   <owl:Class rdf:about="http://www.opengis.net/gml#CompositeSurfaceType">
      <rdfs:comment>A CompositeSurface is defined by a set of orientable surfaces. A composite surface is geometry type with all the geometric properties of a (primitive) surface. Essentially, a composite surface is a collection of surfaces that join in pairs on common boundary curves and which, when considered as a whole, form a single surface.</rdfs:comment>
      <rdfs:subClassOf>
         <owl:Class>
            <owl:intersectionOf rdf:parseType="Collection">
               <owl:Restriction>
                  <owl:onProperty rdf:resource="http://www.opengis.net/gml#hassurfaceMember"/>
                  <owl:allValuesFrom rdf:resource="http://www.opengis.net/gml#surfaceMember"/>
               </owl:Restriction>
            </owl:intersectionOf>
         </owl:Class>
      </rdfs:subClassOf>
      <rdfs:subClassOf rdf:resource="http://www.opengis.net/gml#AbstractSurfaceType"/>
   </owl:Class>
   <owl:Class rdf:about="http://www.opengis.net/gml#CompositeSurfacePropertyType">
      <rdfs:subClassOf>
         <owl:Class>
            <owl:intersectionOf rdf:parseType="Collection">
               <owl:Restriction>
                  <owl:onProperty rdf:resource="http://www.opengis.net/gml#hasCompositeSurface"/>
                  <owl:allValuesFrom rdf:resource="http://www.opengis.net/gml#CompositeSurface"/>
               </owl:Restriction>
            </owl:intersectionOf>
         </owl:Class>
      </rdfs:subClassOf>
   </owl:Class>
   <owl:Class rdf:about="http://www.opengis.net/gml#CompositeSolidType">
      <rdfs:comment>A composite solid is a geometry type with all the geometric properties of a (primitive) solid. 
        Essentially, a composite solid is a collection of solids that join in pairs on common boundary surfaces and which, when considered as a whole, form a single solid.</rdfs:comment>
      <rdfs:subClassOf>
         <owl:Class>
            <owl:intersectionOf rdf:parseType="Collection">
               <owl:Restriction>
                  <owl:onProperty rdf:resource="http://www.opengis.net/gml#hassolidMember"/>
                  <owl:allValuesFrom rdf:resource="http://www.opengis.net/gml#solidMember"/>
               </owl:Restriction>
            </owl:intersectionOf>
         </owl:Class>
      </rdfs:subClassOf>
      <rdfs:subClassOf rdf:resource="http://www.opengis.net/gml#AbstractSolidType"/>
   </owl:Class>
   <owl:Class rdf:about="http://www.opengis.net/gml#CompositeSolidPropertyType">
      <rdfs:subClassOf>
         <owl:Class>
            <owl:intersectionOf rdf:parseType="Collection">
               <owl:Restriction>
                  <owl:onProperty rdf:resource="http://www.opengis.net/gml#hasCompositeSolid"/>
                  <owl:allValuesFrom rdf:resource="http://www.opengis.net/gml#CompositeSolid"/>
               </owl:Restriction>
            </owl:intersectionOf>
         </owl:Class>
      </rdfs:subClassOf>
   </owl:Class>
   <owl:Class rdf:about="http://www.opengis.net/gml#GeometricComplexType">
      <rdfs:comment>A geometric complex.</rdfs:comment>
      <rdfs:subClassOf>
         <owl:Class>
            <owl:intersectionOf rdf:parseType="Collection">
               <owl:Restriction>
                  <owl:onProperty rdf:resource="http://www.opengis.net/gml#element"/>
                  <owl:allValuesFrom rdf:resource="http://www.opengis.net/gml#GeometricPrimitivePropertyType"/>
               </owl:Restriction>
            </owl:intersectionOf>
         </owl:Class>
      </rdfs:subClassOf>
      <rdfs:subClassOf rdf:resource="http://www.opengis.net/gml#AbstractGeometryType"/>
   </owl:Class>
   <owl:Class rdf:about="http://www.opengis.net/gml#GeometricComplexPropertyType">
      <rdfs:comment>A property that has a geometric complex as its value domain can either be an appropriate geometry element encapsulated in an element of this type or an XLink reference to a remote geometry element (where remote includes geometry elements located elsewhere in the same document). Either the reference or the contained element must be given, but neither both nor none.
NOTE: The allowed geometry elements contained in such a property (or referenced by it) have to be modelled by an XML Schema choice element since the composites inherit both from geometric complex *and* geometric primitive and are already part of the _GeometricPrimitive substitution group.</rdfs:comment>
      <owl:disjointUnionOf rdf:parseType="Collection">
         <owl:Restriction>
            <owl:onProperty rdf:resource="http://www.opengis.net/gml#hasGeometricComplex"/>
            <owl:someValuesFrom rdf:resource="http://www.opengis.net/gml#GeometricComplex"/>
         </owl:Restriction>
         <owl:Restriction>
            <owl:onProperty rdf:resource="http://www.opengis.net/gml#hasCompositeCurve"/>
            <owl:someValuesFrom rdf:resource="http://www.opengis.net/gml#CompositeCurve"/>
         </owl:Restriction>
         <owl:Restriction>
            <owl:onProperty rdf:resource="http://www.opengis.net/gml#hasCompositeSurface"/>
            <owl:someValuesFrom rdf:resource="http://www.opengis.net/gml#CompositeSurface"/>
         </owl:Restriction>
         <owl:Restriction>
            <owl:onProperty rdf:resource="http://www.opengis.net/gml#hasCompositeSolid"/>
            <owl:someValuesFrom rdf:resource="http://www.opengis.net/gml#CompositeSolid"/>
         </owl:Restriction>
      </owl:disjointUnionOf>
   </owl:Class>
   <owl:Class rdf:about="http://www.opengis.net/gml#AbstractGeometricAggregateType">
      <rdfs:comment>This is an abstract class</rdfs:comment>
      <rdfs:comment>This is the abstract root type of the geometric aggregates.</rdfs:comment>
      <rdfs:subClassOf rdf:resource="http://www.opengis.net/gml#AbstractGeometryType"/>
   </owl:Class>
   <owl:Class rdf:about="http://www.opengis.net/gml#MultiGeometryType">
      <rdfs:comment>A geometry collection must include one or more geometries, referenced through geometryMember elements.</rdfs:comment>
      <rdfs:subClassOf>
         <owl:Class>
            <owl:intersectionOf rdf:parseType="Collection">
               <owl:Restriction>
                  <owl:onProperty rdf:resource="http://www.opengis.net/gml#hasgeometryMember"/>
                  <owl:allValuesFrom rdf:resource="http://www.opengis.net/gml#geometryMember"/>
               </owl:Restriction>
               <owl:Restriction>
                  <owl:onProperty rdf:resource="http://www.opengis.net/gml#hasgeometryMember"/>
                  <owl:minCardinality rdf:datatype="http://www.w3.org/2001/XMLSchema#nonNegativeInteger">0</owl:minCardinality>
               </owl:Restriction>
               <owl:Restriction>
                  <owl:onProperty rdf:resource="http://www.opengis.net/gml#hasgeometryMembers"/>
                  <owl:allValuesFrom rdf:resource="http://www.opengis.net/gml#geometryMembers"/>
               </owl:Restriction>
               <owl:Restriction>
                  <owl:onProperty rdf:resource="http://www.opengis.net/gml#hasgeometryMembers"/>
                  <owl:minCardinality rdf:datatype="http://www.w3.org/2001/XMLSchema#nonNegativeInteger">0</owl:minCardinality>
               </owl:Restriction>
            </owl:intersectionOf>
         </owl:Class>
      </rdfs:subClassOf>
      <rdfs:subClassOf rdf:resource="http://www.opengis.net/gml#AbstractGeometricAggregateType"/>
   </owl:Class>
   <owl:Class rdf:about="http://www.opengis.net/gml#MultiGeometryPropertyType">
      <rdfs:comment>A property that has a geometric aggregate as its value domain can either be an appropriate geometry element encapsulated in an element of this type or an XLink reference to a remote geometry element (where remote includes geometry elements located elsewhere in the same document). Either the reference or the contained element must be given, but neither both nor none.</rdfs:comment>
      <rdfs:subClassOf>
         <owl:Class>
            <owl:intersectionOf rdf:parseType="Collection">
               <owl:Restriction>
                  <owl:onProperty rdf:resource="http://www.opengis.net/gml#has_GeometricAggregate"/>
                  <owl:allValuesFrom rdf:resource="http://www.opengis.net/gml#_GeometricAggregate"/>
               </owl:Restriction>
            </owl:intersectionOf>
         </owl:Class>
      </rdfs:subClassOf>
   </owl:Class>
   <owl:Class rdf:about="http://www.opengis.net/gml#MultiPointType">
      <rdfs:comment>A MultiPoint is defined by one or more Points, referenced through pointMember elements.</rdfs:comment>
      <rdfs:subClassOf>
         <owl:Class>
            <owl:intersectionOf rdf:parseType="Collection">
               <owl:Restriction>
                  <owl:onProperty rdf:resource="http://www.opengis.net/gml#haspointMember"/>
                  <owl:allValuesFrom rdf:resource="http://www.opengis.net/gml#pointMember"/>
               </owl:Restriction>
               <owl:Restriction>
                  <owl:onProperty rdf:resource="http://www.opengis.net/gml#haspointMember"/>
                  <owl:minCardinality rdf:datatype="http://www.w3.org/2001/XMLSchema#nonNegativeInteger">0</owl:minCardinality>
               </owl:Restriction>
               <owl:Restriction>
                  <owl:onProperty rdf:resource="http://www.opengis.net/gml#haspointMembers"/>
                  <owl:allValuesFrom rdf:resource="http://www.opengis.net/gml#pointMembers"/>
               </owl:Restriction>
               <owl:Restriction>
                  <owl:onProperty rdf:resource="http://www.opengis.net/gml#haspointMembers"/>
                  <owl:minCardinality rdf:datatype="http://www.w3.org/2001/XMLSchema#nonNegativeInteger">0</owl:minCardinality>
               </owl:Restriction>
            </owl:intersectionOf>
         </owl:Class>
      </rdfs:subClassOf>
      <rdfs:subClassOf rdf:resource="http://www.opengis.net/gml#AbstractGeometricAggregateType"/>
   </owl:Class>
   <owl:Class rdf:about="http://www.opengis.net/gml#MultiPointPropertyType">
      <rdfs:comment>A property that has a collection of points as its value domain can either be an appropriate geometry element encapsulated in an element of this type or an XLink reference to a remote geometry element (where remote includes geometry elements located elsewhere in the same document). Either the reference or the contained element must be given, but neither both nor none.</rdfs:comment>
      <rdfs:subClassOf>
         <owl:Class>
            <owl:intersectionOf rdf:parseType="Collection">
               <owl:Restriction>
                  <owl:onProperty rdf:resource="http://www.opengis.net/gml#hasMultiPoint"/>
                  <owl:allValuesFrom rdf:resource="http://www.opengis.net/gml#MultiPoint"/>
               </owl:Restriction>
            </owl:intersectionOf>
         </owl:Class>
      </rdfs:subClassOf>
   </owl:Class>
   <owl:Class rdf:about="http://www.opengis.net/gml#MultiCurveType">
      <rdfs:comment>A MultiCurve is defined by one or more Curves, referenced through curveMember elements.</rdfs:comment>
      <rdfs:subClassOf>
         <owl:Class>
            <owl:intersectionOf rdf:parseType="Collection">
               <owl:Restriction>
                  <owl:onProperty rdf:resource="http://www.opengis.net/gml#hascurveMember"/>
                  <owl:allValuesFrom rdf:resource="http://www.opengis.net/gml#curveMember"/>
               </owl:Restriction>
               <owl:Restriction>
                  <owl:onProperty rdf:resource="http://www.opengis.net/gml#hascurveMember"/>
                  <owl:minCardinality rdf:datatype="http://www.w3.org/2001/XMLSchema#nonNegativeInteger">0</owl:minCardinality>
               </owl:Restriction>
               <owl:Restriction>
                  <owl:onProperty rdf:resource="http://www.opengis.net/gml#hascurveMembers"/>
                  <owl:allValuesFrom rdf:resource="http://www.opengis.net/gml#curveMembers"/>
               </owl:Restriction>
               <owl:Restriction>
                  <owl:onProperty rdf:resource="http://www.opengis.net/gml#hascurveMembers"/>
                  <owl:minCardinality rdf:datatype="http://www.w3.org/2001/XMLSchema#nonNegativeInteger">0</owl:minCardinality>
               </owl:Restriction>
            </owl:intersectionOf>
         </owl:Class>
      </rdfs:subClassOf>
      <rdfs:subClassOf rdf:resource="http://www.opengis.net/gml#AbstractGeometricAggregateType"/>
   </owl:Class>
   <owl:Class rdf:about="http://www.opengis.net/gml#MultiCurvePropertyType">
      <rdfs:comment>A property that has a collection of curves as its value domain can either be an appropriate geometry element encapsulated in an element of this type or an XLink reference to a remote geometry element (where remote includes geometry elements located elsewhere in the same document). Either the reference or the contained element must be given, but neither both nor none.</rdfs:comment>
      <rdfs:subClassOf>
         <owl:Class>
            <owl:intersectionOf rdf:parseType="Collection">
               <owl:Restriction>
                  <owl:onProperty rdf:resource="http://www.opengis.net/gml#hasMultiCurve"/>
                  <owl:allValuesFrom rdf:resource="http://www.opengis.net/gml#MultiCurve"/>
               </owl:Restriction>
            </owl:intersectionOf>
         </owl:Class>
      </rdfs:subClassOf>
   </owl:Class>
   <owl:Class rdf:about="http://www.opengis.net/gml#MultiSurfaceType">
      <rdfs:comment>A MultiSurface is defined by one or more Surfaces, referenced through surfaceMember elements.</rdfs:comment>
      <rdfs:subClassOf>
         <owl:Class>
            <owl:intersectionOf rdf:parseType="Collection">
               <owl:Restriction>
                  <owl:onProperty rdf:resource="http://www.opengis.net/gml#hassurfaceMember"/>
                  <owl:allValuesFrom rdf:resource="http://www.opengis.net/gml#surfaceMember"/>
               </owl:Restriction>
               <owl:Restriction>
                  <owl:onProperty rdf:resource="http://www.opengis.net/gml#hassurfaceMember"/>
                  <owl:minCardinality rdf:datatype="http://www.w3.org/2001/XMLSchema#nonNegativeInteger">0</owl:minCardinality>
               </owl:Restriction>
               <owl:Restriction>
                  <owl:onProperty rdf:resource="http://www.opengis.net/gml#hassurfaceMembers"/>
                  <owl:allValuesFrom rdf:resource="http://www.opengis.net/gml#surfaceMembers"/>
               </owl:Restriction>
               <owl:Restriction>
                  <owl:onProperty rdf:resource="http://www.opengis.net/gml#hassurfaceMembers"/>
                  <owl:minCardinality rdf:datatype="http://www.w3.org/2001/XMLSchema#nonNegativeInteger">0</owl:minCardinality>
               </owl:Restriction>
            </owl:intersectionOf>
         </owl:Class>
      </rdfs:subClassOf>
      <rdfs:subClassOf rdf:resource="http://www.opengis.net/gml#AbstractGeometricAggregateType"/>
   </owl:Class>
   <owl:Class rdf:about="http://www.opengis.net/gml#MultiSurfacePropertyType">
      <rdfs:comment>A property that has a collection of surfaces as its value domain can either be an appropriate geometry element encapsulated in an element of this type or an XLink reference to a remote geometry element (where remote includes geometry elements located elsewhere in the same document). Either the reference or the contained element must be given, but neither both nor none.</rdfs:comment>
      <rdfs:subClassOf>
         <owl:Class>
            <owl:intersectionOf rdf:parseType="Collection">
               <owl:Restriction>
                  <owl:onProperty rdf:resource="http://www.opengis.net/gml#hasMultiSurface"/>
                  <owl:allValuesFrom rdf:resource="http://www.opengis.net/gml#MultiSurface"/>
               </owl:Restriction>
            </owl:intersectionOf>
         </owl:Class>
      </rdfs:subClassOf>
   </owl:Class>
   <owl:Class rdf:about="http://www.opengis.net/gml#MultiSolidType">
      <rdfs:comment>A MultiSolid is defined by one or more Solids, referenced through solidMember elements.</rdfs:comment>
      <rdfs:subClassOf>
         <owl:Class>
            <owl:intersectionOf rdf:parseType="Collection">
               <owl:Restriction>
                  <owl:onProperty rdf:resource="http://www.opengis.net/gml#hassolidMember"/>
                  <owl:allValuesFrom rdf:resource="http://www.opengis.net/gml#solidMember"/>
               </owl:Restriction>
               <owl:Restriction>
                  <owl:onProperty rdf:resource="http://www.opengis.net/gml#hassolidMember"/>
                  <owl:minCardinality rdf:datatype="http://www.w3.org/2001/XMLSchema#nonNegativeInteger">0</owl:minCardinality>
               </owl:Restriction>
               <owl:Restriction>
                  <owl:onProperty rdf:resource="http://www.opengis.net/gml#hassolidMembers"/>
                  <owl:allValuesFrom rdf:resource="http://www.opengis.net/gml#solidMembers"/>
               </owl:Restriction>
               <owl:Restriction>
                  <owl:onProperty rdf:resource="http://www.opengis.net/gml#hassolidMembers"/>
                  <owl:minCardinality rdf:datatype="http://www.w3.org/2001/XMLSchema#nonNegativeInteger">0</owl:minCardinality>
               </owl:Restriction>
            </owl:intersectionOf>
         </owl:Class>
      </rdfs:subClassOf>
      <rdfs:subClassOf rdf:resource="http://www.opengis.net/gml#AbstractGeometricAggregateType"/>
   </owl:Class>
   <owl:Class rdf:about="http://www.opengis.net/gml#MultiSolidPropertyType">
      <rdfs:comment>A property that has a collection of solids as its value domain can either be an appropriate geometry element encapsulated in an element of this type or an XLink reference to a remote geometry element (where remote includes geometry elements located elsewhere in the same document). Either the reference or the contained element must be given, but neither both nor none.</rdfs:comment>
      <rdfs:subClassOf>
         <owl:Class>
            <owl:intersectionOf rdf:parseType="Collection">
               <owl:Restriction>
                  <owl:onProperty rdf:resource="http://www.opengis.net/gml#hasMultiSolid"/>
                  <owl:allValuesFrom rdf:resource="http://www.opengis.net/gml#MultiSolid"/>
               </owl:Restriction>
            </owl:intersectionOf>
         </owl:Class>
      </rdfs:subClassOf>
   </owl:Class>
   <owl:Class rdf:about="http://www.opengis.net/gml#MultiLineStringType">
      <rdfs:comment>A MultiLineString is defined by one or more LineStrings, referenced through lineStringMember elements. Deprecated with GML version 3.0. Use MultiCurveType instead.</rdfs:comment>
      <rdfs:subClassOf>
         <owl:Class>
            <owl:intersectionOf rdf:parseType="Collection">
               <owl:Restriction>
                  <owl:onProperty rdf:resource="http://www.opengis.net/gml#haslineStringMember"/>
                  <owl:allValuesFrom rdf:resource="http://www.opengis.net/gml#lineStringMember"/>
               </owl:Restriction>
               <owl:Restriction>
                  <owl:onProperty rdf:resource="http://www.opengis.net/gml#haslineStringMember"/>
                  <owl:minCardinality rdf:datatype="http://www.w3.org/2001/XMLSchema#nonNegativeInteger">0</owl:minCardinality>
               </owl:Restriction>
            </owl:intersectionOf>
         </owl:Class>
      </rdfs:subClassOf>
      <rdfs:subClassOf rdf:resource="http://www.opengis.net/gml#AbstractGeometricAggregateType"/>
   </owl:Class>
   <owl:Class rdf:about="http://www.opengis.net/gml#MultiLineStringPropertyType">
      <rdfs:comment>This type is deprecated with GML 3 and shall not be used. It is included for backwards compatibility with GML 2. Use MultiCurvePropertyType instead.
A property that has a collection of line strings as its value domain can either be an appropriate geometry element encapsulated in an element of this type or an XLink reference to a remote geometry element (where remote includes geometry elements located elsewhere in the same document). Either the reference or the contained element must be given, but neither both nor none.</rdfs:comment>
      <rdfs:subClassOf>
         <owl:Class>
            <owl:intersectionOf rdf:parseType="Collection">
               <owl:Restriction>
                  <owl:onProperty rdf:resource="http://www.opengis.net/gml#hasMultiLineString"/>
                  <owl:allValuesFrom rdf:resource="http://www.opengis.net/gml#MultiLineString"/>
               </owl:Restriction>
            </owl:intersectionOf>
         </owl:Class>
      </rdfs:subClassOf>
   </owl:Class>
   <owl:Class rdf:about="http://www.opengis.net/gml#MultiPolygonType">
      <rdfs:comment>A MultiPolygon is defined by one or more Polygons, referenced through polygonMember elements. Deprecated with GML version 3.0. Use MultiSurfaceType instead.</rdfs:comment>
      <rdfs:subClassOf>
         <owl:Class>
            <owl:intersectionOf rdf:parseType="Collection">
               <owl:Restriction>
                  <owl:onProperty rdf:resource="http://www.opengis.net/gml#haspolygonMember"/>
                  <owl:allValuesFrom rdf:resource="http://www.opengis.net/gml#polygonMember"/>
               </owl:Restriction>
               <owl:Restriction>
                  <owl:onProperty rdf:resource="http://www.opengis.net/gml#haspolygonMember"/>
                  <owl:minCardinality rdf:datatype="http://www.w3.org/2001/XMLSchema#nonNegativeInteger">0</owl:minCardinality>
               </owl:Restriction>
            </owl:intersectionOf>
         </owl:Class>
      </rdfs:subClassOf>
      <rdfs:subClassOf rdf:resource="http://www.opengis.net/gml#AbstractGeometricAggregateType"/>
   </owl:Class>
   <owl:Class rdf:about="http://www.opengis.net/gml#MultiPolygonPropertyType">
      <rdfs:comment>This type is deprecated with GML 3 and shall not be used. It is included for backwards compatibility with GML 2. Use MultiSurfacePropertyType instead.

A property that has a collection of polygons as its value domain can either be an appropriate geometry element encapsulated in an element of this type or an XLink reference to a remote geometry element (where remote includes geometry elements located elsewhere in the same document). Either the reference or the contained element must be given, but neither both nor none.</rdfs:comment>
      <rdfs:subClassOf>
         <owl:Class>
            <owl:intersectionOf rdf:parseType="Collection">
               <owl:Restriction>
                  <owl:onProperty rdf:resource="http://www.opengis.net/gml#hasMultiPolygon"/>
                  <owl:allValuesFrom rdf:resource="http://www.opengis.net/gml#MultiPolygon"/>
               </owl:Restriction>
            </owl:intersectionOf>
         </owl:Class>
      </rdfs:subClassOf>
   </owl:Class>
   <owl:Class rdf:about="http://www.opengis.net/gml#CurveType">
      <rdfs:comment>Curve is a 1-dimensional primitive. Curves are continuous, connected, and have a measurable length in terms of the coordinate system. 
        A curve is composed of one or more curve segments. Each curve segment within a curve may be defined using a different interpolation method. The curve segments are connected to one another, with the end point of each segment except the last being the start point of the next segment in the segment list.
        The orientation of the curve is positive.</rdfs:comment>
      <rdfs:subClassOf>
         <owl:Class>
            <owl:intersectionOf rdf:parseType="Collection">
               <owl:Restriction>
                  <owl:onProperty rdf:resource="http://www.opengis.net/gml#hassegments"/>
                  <owl:allValuesFrom rdf:resource="http://www.opengis.net/gml#segments"/>
               </owl:Restriction>
            </owl:intersectionOf>
         </owl:Class>
      </rdfs:subClassOf>
      <rdfs:subClassOf rdf:resource="http://www.opengis.net/gml#AbstractCurveType"/>
   </owl:Class>
   <owl:Class rdf:about="http://www.opengis.net/gml#OrientableCurveType">
      <rdfs:comment>OrientableCurve consists of a curve and an orientation. If the orientation is "+", then the OrientableCurve is identical to the baseCurve. If the orientation is "-", then the OrientableCurve is related to another _Curve with a parameterization that reverses the sense of the curve traversal.</rdfs:comment>
      <rdfs:subClassOf>
         <owl:Class>
            <owl:intersectionOf rdf:parseType="Collection">
               <owl:Restriction>
                  <owl:onProperty rdf:resource="http://www.opengis.net/gml#hasbaseCurve"/>
                  <owl:allValuesFrom rdf:resource="http://www.opengis.net/gml#baseCurve"/>
               </owl:Restriction>
            </owl:intersectionOf>
         </owl:Class>
      </rdfs:subClassOf>
      <rdfs:subClassOf>
         <owl:Class>
            <owl:intersectionOf rdf:parseType="Collection">
               <owl:Restriction>
                  <owl:onProperty rdf:resource="http://www.opengis.net/gml#orientation"/>
                  <owl:allValuesFrom rdf:resource="http://www.opengis.net/gml#SignType"/>
               </owl:Restriction>
            </owl:intersectionOf>
         </owl:Class>
      </rdfs:subClassOf>
      <rdfs:subClassOf rdf:resource="http://www.opengis.net/gml#AbstractCurveType"/>
   </owl:Class>
   <owl:Class rdf:about="http://www.opengis.net/gml#AbstractCurveSegmentType">
      <rdfs:comment>This is an abstract class</rdfs:comment>
      <rdfs:comment>Curve segment defines a homogeneous segment of a curve.</rdfs:comment>
      <rdfs:subClassOf>
         <owl:Class>
            <owl:intersectionOf rdf:parseType="Collection">
               <owl:Restriction>
                  <owl:onProperty rdf:resource="http://www.opengis.net/gml#numDerivativesAtStart"/>
                  <owl:allValuesFrom rdf:resource="http://www.w3.org/2001/XMLSchema#integer"/>
               </owl:Restriction>
               <owl:Restriction>
                  <owl:onProperty rdf:resource="http://www.opengis.net/gml#numDerivativesAtEnd"/>
                  <owl:allValuesFrom rdf:resource="http://www.w3.org/2001/XMLSchema#integer"/>
               </owl:Restriction>
               <owl:Restriction>
                  <owl:onProperty rdf:resource="http://www.opengis.net/gml#numDerivativeInterior"/>
                  <owl:allValuesFrom rdf:resource="http://www.w3.org/2001/XMLSchema#integer"/>
               </owl:Restriction>
            </owl:intersectionOf>
         </owl:Class>
      </rdfs:subClassOf>
   </owl:Class>
   <owl:Class rdf:about="http://www.opengis.net/gml#CurveSegmentArrayPropertyType">
      <rdfs:comment>A container for an array of curve segments.</rdfs:comment>
      <rdfs:subClassOf>
         <owl:Class>
            <owl:intersectionOf rdf:parseType="Collection">
               <owl:Restriction>
                  <owl:onProperty rdf:resource="http://www.opengis.net/gml#has_CurveSegment"/>
                  <owl:allValuesFrom rdf:resource="http://www.opengis.net/gml#_CurveSegment"/>
               </owl:Restriction>
               <owl:Restriction>
                  <owl:onProperty rdf:resource="http://www.opengis.net/gml#has_CurveSegment"/>
                  <owl:minCardinality rdf:datatype="http://www.w3.org/2001/XMLSchema#nonNegativeInteger">0</owl:minCardinality>
               </owl:Restriction>
            </owl:intersectionOf>
         </owl:Class>
      </rdfs:subClassOf>
   </owl:Class>
   <owl:Class rdf:about="http://www.opengis.net/gml#LineStringSegmentType">
      <rdfs:comment>A LineStringSegment is a curve segment that is defined by two or more coordinate tuples, with linear interpolation between them.
        Note: LineStringSegment implements GM_LineString of ISO 19107.</rdfs:comment>
      <owl:disjointUnionOf rdf:parseType="Collection">
         <owl:Restriction>
            <owl:onProperty rdf:resource="http://www.opengis.net/gml#hasposList"/>
            <owl:someValuesFrom rdf:resource="http://www.opengis.net/gml#posList"/>
         </owl:Restriction>
         <owl:Restriction>
            <owl:onProperty rdf:resource="http://www.opengis.net/gml#hascoordinates"/>
            <owl:someValuesFrom rdf:resource="http://www.opengis.net/gml#coordinates"/>
         </owl:Restriction>
         <owl:Restriction>
            <owl:onProperty rdf:resource="http://www.opengis.net/gml#haspos"/>
            <owl:someValuesFrom rdf:resource="http://www.opengis.net/gml#pos"/>
         </owl:Restriction>
         <owl:Restriction>
            <owl:onProperty rdf:resource="http://www.opengis.net/gml#haspointProperty"/>
            <owl:someValuesFrom rdf:resource="http://www.opengis.net/gml#pointProperty"/>
         </owl:Restriction>
         <owl:Restriction>
            <owl:onProperty rdf:resource="http://www.opengis.net/gml#haspointRep"/>
            <owl:someValuesFrom rdf:resource="http://www.opengis.net/gml#pointRep"/>
         </owl:Restriction>
      </owl:disjointUnionOf>
      <rdfs:subClassOf>
         <owl:Class>
            <owl:intersectionOf rdf:parseType="Collection">
               <owl:Restriction>
                  <owl:onProperty rdf:resource="http://www.opengis.net/gml#interpolation"/>
                  <owl:allValuesFrom rdf:resource="http://www.opengis.net/gml#CurveInterpolationType"/>
               </owl:Restriction>
            </owl:intersectionOf>
         </owl:Class>
      </rdfs:subClassOf>
      <rdfs:subClassOf rdf:resource="http://www.opengis.net/gml#AbstractCurveSegmentType"/>
   </owl:Class>
   <owl:Class rdf:about="http://www.opengis.net/gml#ArcStringType">
      <rdfs:comment>An ArcString is a curve segment that uses three-point circular arc interpolation.</rdfs:comment>
      <owl:disjointUnionOf rdf:parseType="Collection">
         <owl:Restriction>
            <owl:onProperty rdf:resource="http://www.opengis.net/gml#hasposList"/>
            <owl:someValuesFrom rdf:resource="http://www.opengis.net/gml#posList"/>
         </owl:Restriction>
         <owl:Restriction>
            <owl:onProperty rdf:resource="http://www.opengis.net/gml#hascoordinates"/>
            <owl:someValuesFrom rdf:resource="http://www.opengis.net/gml#coordinates"/>
         </owl:Restriction>
         <owl:Restriction>
            <owl:onProperty rdf:resource="http://www.opengis.net/gml#haspos"/>
            <owl:someValuesFrom rdf:resource="http://www.opengis.net/gml#pos"/>
         </owl:Restriction>
         <owl:Restriction>
            <owl:onProperty rdf:resource="http://www.opengis.net/gml#haspointProperty"/>
            <owl:someValuesFrom rdf:resource="http://www.opengis.net/gml#pointProperty"/>
         </owl:Restriction>
         <owl:Restriction>
            <owl:onProperty rdf:resource="http://www.opengis.net/gml#haspointRep"/>
            <owl:someValuesFrom rdf:resource="http://www.opengis.net/gml#pointRep"/>
         </owl:Restriction>
      </owl:disjointUnionOf>
      <rdfs:subClassOf>
         <owl:Class>
            <owl:intersectionOf rdf:parseType="Collection">
               <owl:Restriction>
                  <owl:onProperty rdf:resource="http://www.opengis.net/gml#interpolation"/>
                  <owl:allValuesFrom rdf:resource="http://www.opengis.net/gml#CurveInterpolationType"/>
               </owl:Restriction>
               <owl:Restriction>
                  <owl:onProperty rdf:resource="http://www.opengis.net/gml#numArc"/>
                  <owl:allValuesFrom rdf:resource="http://www.w3.org/2001/XMLSchema#integer"/>
               </owl:Restriction>
            </owl:intersectionOf>
         </owl:Class>
      </rdfs:subClassOf>
      <rdfs:subClassOf rdf:resource="http://www.opengis.net/gml#AbstractCurveSegmentType"/>
   </owl:Class>
   <owl:Class rdf:about="http://www.opengis.net/gml#ArcType">
      <rdfs:comment>An Arc is an arc string with only one arc unit, i.e. three control points.</rdfs:comment>
      <owl:disjointUnionOf rdf:parseType="Collection">
         <owl:Restriction>
            <owl:onProperty rdf:resource="http://www.opengis.net/gml#hasposList"/>
            <owl:someValuesFrom rdf:resource="http://www.opengis.net/gml#posList"/>
         </owl:Restriction>
         <owl:Restriction>
            <owl:onProperty rdf:resource="http://www.opengis.net/gml#hascoordinates"/>
            <owl:someValuesFrom rdf:resource="http://www.opengis.net/gml#coordinates"/>
         </owl:Restriction>
         <owl:Restriction>
            <owl:onProperty rdf:resource="http://www.opengis.net/gml#haspos"/>
            <owl:someValuesFrom rdf:resource="http://www.opengis.net/gml#pos"/>
         </owl:Restriction>
         <owl:Restriction>
            <owl:onProperty rdf:resource="http://www.opengis.net/gml#haspointProperty"/>
            <owl:someValuesFrom rdf:resource="http://www.opengis.net/gml#pointProperty"/>
         </owl:Restriction>
         <owl:Restriction>
            <owl:onProperty rdf:resource="http://www.opengis.net/gml#haspointRep"/>
            <owl:someValuesFrom rdf:resource="http://www.opengis.net/gml#pointRep"/>
         </owl:Restriction>
      </owl:disjointUnionOf>
      <rdfs:subClassOf>
         <owl:Class>
            <owl:intersectionOf rdf:parseType="Collection">
               <owl:Restriction>
                  <owl:onProperty rdf:resource="http://www.opengis.net/gml#numArc"/>
                  <owl:allValuesFrom rdf:resource="http://www.w3.org/2001/XMLSchema#integer"/>
               </owl:Restriction>
            </owl:intersectionOf>
         </owl:Class>
      </rdfs:subClassOf>
      <rdfs:subClassOf rdf:resource="http://www.opengis.net/gml#ArcStringType"/>
   </owl:Class>
   <owl:Class rdf:about="http://www.opengis.net/gml#CircleType">
      <rdfs:comment>A Circle is an arc whose ends coincide to form a simple closed loop. The "start" and "end" bearing are equal and shall be the bearing for the first controlPoint listed. The three control points must be distinct non-co-linear points for the Circle to be unambiguously defined. The arc is simply extended past the third control point until the first control point is encountered.</rdfs:comment>
      <rdfs:subClassOf rdf:resource="http://www.opengis.net/gml#ArcType"/>
   </owl:Class>
   <owl:Class rdf:about="http://www.opengis.net/gml#ArcStringByBulgeType">
      <rdfs:comment>This variant of the arc computes the mid points of the arcs instead of storing the coordinates directly. The control point sequence consists of the start and end points of each arc plus the bulge.</rdfs:comment>
      <rdfs:subClassOf>
         <owl:Class>
            <owl:intersectionOf rdf:parseType="Collection">
               <owl:Restriction>
                  <owl:onProperty rdf:resource="http://www.opengis.net/gml#bulge"/>
                  <owl:allValuesFrom rdf:resource="http://www.w3.org/2001/XMLSchema#double"/>
               </owl:Restriction>
               <owl:Restriction>
                  <owl:onProperty rdf:resource="http://www.opengis.net/gml#normal"/>
                  <owl:allValuesFrom rdf:resource="http://www.opengis.net/gml#VectorType"/>
               </owl:Restriction>
            </owl:intersectionOf>
         </owl:Class>
      </rdfs:subClassOf>
      <owl:disjointUnionOf rdf:parseType="Collection">
         <owl:Restriction>
            <owl:onProperty rdf:resource="http://www.opengis.net/gml#hasposList"/>
            <owl:someValuesFrom rdf:resource="http://www.opengis.net/gml#posList"/>
         </owl:Restriction>
         <owl:Restriction>
            <owl:onProperty rdf:resource="http://www.opengis.net/gml#hascoordinates"/>
            <owl:someValuesFrom rdf:resource="http://www.opengis.net/gml#coordinates"/>
         </owl:Restriction>
         <owl:Restriction>
            <owl:onProperty rdf:resource="http://www.opengis.net/gml#haspos"/>
            <owl:someValuesFrom rdf:resource="http://www.opengis.net/gml#pos"/>
         </owl:Restriction>
         <owl:Restriction>
            <owl:onProperty rdf:resource="http://www.opengis.net/gml#haspointProperty"/>
            <owl:someValuesFrom rdf:resource="http://www.opengis.net/gml#pointProperty"/>
         </owl:Restriction>
         <owl:Restriction>
            <owl:onProperty rdf:resource="http://www.opengis.net/gml#haspointRep"/>
            <owl:someValuesFrom rdf:resource="http://www.opengis.net/gml#pointRep"/>
         </owl:Restriction>
      </owl:disjointUnionOf>
      <rdfs:subClassOf>
         <owl:Class>
            <owl:intersectionOf rdf:parseType="Collection">
               <owl:Restriction>
                  <owl:onProperty rdf:resource="http://www.opengis.net/gml#interpolation"/>
                  <owl:allValuesFrom rdf:resource="http://www.opengis.net/gml#CurveInterpolationType"/>
               </owl:Restriction>
               <owl:Restriction>
                  <owl:onProperty rdf:resource="http://www.opengis.net/gml#numArc"/>
                  <owl:allValuesFrom rdf:resource="http://www.w3.org/2001/XMLSchema#integer"/>
               </owl:Restriction>
            </owl:intersectionOf>
         </owl:Class>
      </rdfs:subClassOf>
      <rdfs:subClassOf rdf:resource="http://www.opengis.net/gml#AbstractCurveSegmentType"/>
   </owl:Class>
   <owl:Class rdf:about="http://www.opengis.net/gml#ArcByBulgeType">
      <rdfs:comment>An ArcByBulge is an arc string with only one arc unit, i.e. two control points and one bulge.</rdfs:comment>
      <rdfs:subClassOf>
         <owl:Class>
            <owl:intersectionOf rdf:parseType="Collection">
               <owl:Restriction>
                  <owl:onProperty rdf:resource="http://www.opengis.net/gml#bulge"/>
                  <owl:allValuesFrom rdf:resource="http://www.w3.org/2001/XMLSchema#double"/>
               </owl:Restriction>
               <owl:Restriction>
                  <owl:onProperty rdf:resource="http://www.opengis.net/gml#normal"/>
                  <owl:allValuesFrom rdf:resource="http://www.opengis.net/gml#VectorType"/>
               </owl:Restriction>
            </owl:intersectionOf>
         </owl:Class>
      </rdfs:subClassOf>
      <owl:disjointUnionOf rdf:parseType="Collection">
         <owl:Restriction>
            <owl:onProperty rdf:resource="http://www.opengis.net/gml#hasposList"/>
            <owl:someValuesFrom rdf:resource="http://www.opengis.net/gml#posList"/>
         </owl:Restriction>
         <owl:Restriction>
            <owl:onProperty rdf:resource="http://www.opengis.net/gml#hascoordinates"/>
            <owl:someValuesFrom rdf:resource="http://www.opengis.net/gml#coordinates"/>
         </owl:Restriction>
         <owl:Restriction>
            <owl:onProperty rdf:resource="http://www.opengis.net/gml#haspos"/>
            <owl:someValuesFrom rdf:resource="http://www.opengis.net/gml#pos"/>
         </owl:Restriction>
         <owl:Restriction>
            <owl:onProperty rdf:resource="http://www.opengis.net/gml#haspointProperty"/>
            <owl:someValuesFrom rdf:resource="http://www.opengis.net/gml#pointProperty"/>
         </owl:Restriction>
         <owl:Restriction>
            <owl:onProperty rdf:resource="http://www.opengis.net/gml#haspointRep"/>
            <owl:someValuesFrom rdf:resource="http://www.opengis.net/gml#pointRep"/>
         </owl:Restriction>
      </owl:disjointUnionOf>
      <rdfs:subClassOf>
         <owl:Class>
            <owl:intersectionOf rdf:parseType="Collection">
               <owl:Restriction>
                  <owl:onProperty rdf:resource="http://www.opengis.net/gml#numArc"/>
                  <owl:allValuesFrom rdf:resource="http://www.w3.org/2001/XMLSchema#integer"/>
               </owl:Restriction>
            </owl:intersectionOf>
         </owl:Class>
      </rdfs:subClassOf>
      <rdfs:subClassOf rdf:resource="http://www.opengis.net/gml#ArcStringByBulgeType"/>
   </owl:Class>
   <owl:Class rdf:about="http://www.opengis.net/gml#ArcByCenterPointType">
      <rdfs:comment>This variant of the arc requires that the points on the arc have to be computed instead of storing the coordinates directly. The control point is the center point of the arc plus the radius and the bearing at start and end. This represenation can be used only in 2D.</rdfs:comment>
      <rdfs:subClassOf>
         <owl:Class>
            <owl:intersectionOf rdf:parseType="Collection">
               <owl:Restriction>
                  <owl:onProperty rdf:resource="http://www.opengis.net/gml#radius"/>
                  <owl:allValuesFrom rdf:resource="http://www.opengis.net/gml#LengthType"/>
               </owl:Restriction>
               <owl:Restriction>
                  <owl:onProperty rdf:resource="http://www.opengis.net/gml#startAngle"/>
                  <owl:allValuesFrom rdf:resource="http://www.opengis.net/gml#AngleType"/>
               </owl:Restriction>
               <owl:Restriction>
                  <owl:onProperty rdf:resource="http://www.opengis.net/gml#startAngle"/>
                  <owl:minCardinality rdf:datatype="http://www.w3.org/2001/XMLSchema#nonNegativeInteger">0</owl:minCardinality>
               </owl:Restriction>
               <owl:Restriction>
                  <owl:onProperty rdf:resource="http://www.opengis.net/gml#endAngle"/>
                  <owl:allValuesFrom rdf:resource="http://www.opengis.net/gml#AngleType"/>
               </owl:Restriction>
               <owl:Restriction>
                  <owl:onProperty rdf:resource="http://www.opengis.net/gml#endAngle"/>
                  <owl:minCardinality rdf:datatype="http://www.w3.org/2001/XMLSchema#nonNegativeInteger">0</owl:minCardinality>
               </owl:Restriction>
            </owl:intersectionOf>
         </owl:Class>
      </rdfs:subClassOf>
      <owl:disjointUnionOf rdf:parseType="Collection">
         <owl:Restriction>
            <owl:onProperty rdf:resource="http://www.opengis.net/gml#hasposList"/>
            <owl:someValuesFrom rdf:resource="http://www.opengis.net/gml#posList"/>
         </owl:Restriction>
         <owl:Restriction>
            <owl:onProperty rdf:resource="http://www.opengis.net/gml#hascoordinates"/>
            <owl:someValuesFrom rdf:resource="http://www.opengis.net/gml#coordinates"/>
         </owl:Restriction>
         <owl:Restriction>
            <owl:onProperty rdf:resource="http://www.opengis.net/gml#haspos"/>
            <owl:someValuesFrom rdf:resource="http://www.opengis.net/gml#pos"/>
         </owl:Restriction>
         <owl:Restriction>
            <owl:onProperty rdf:resource="http://www.opengis.net/gml#haspointProperty"/>
            <owl:someValuesFrom rdf:resource="http://www.opengis.net/gml#pointProperty"/>
         </owl:Restriction>
         <owl:Restriction>
            <owl:onProperty rdf:resource="http://www.opengis.net/gml#haspointRep"/>
            <owl:someValuesFrom rdf:resource="http://www.opengis.net/gml#pointRep"/>
         </owl:Restriction>
      </owl:disjointUnionOf>
      <rdfs:subClassOf>
         <owl:Class>
            <owl:intersectionOf rdf:parseType="Collection">
               <owl:Restriction>
                  <owl:onProperty rdf:resource="http://www.opengis.net/gml#interpolation"/>
                  <owl:allValuesFrom rdf:resource="http://www.opengis.net/gml#CurveInterpolationType"/>
               </owl:Restriction>
               <owl:Restriction>
                  <owl:onProperty rdf:resource="http://www.opengis.net/gml#numArc"/>
                  <owl:allValuesFrom rdf:resource="http://www.w3.org/2001/XMLSchema#integer"/>
               </owl:Restriction>
            </owl:intersectionOf>
         </owl:Class>
      </rdfs:subClassOf>
      <rdfs:subClassOf rdf:resource="http://www.opengis.net/gml#AbstractCurveSegmentType"/>
   </owl:Class>
   <owl:Class rdf:about="http://www.opengis.net/gml#CircleByCenterPointType">
      <rdfs:comment>A CircleByCenterPoint is an ArcByCenterPoint with identical start and end angle to form a full circle. Again, this represenation can be used only in 2D.</rdfs:comment>
      <rdfs:subClassOf rdf:resource="http://www.opengis.net/gml#ArcByCenterPointType"/>
   </owl:Class>
   <owl:Class rdf:about="http://www.opengis.net/gml#OffsetCurveType">
      <rdfs:comment>An offset curve is a curve at a constant
     distance from the basis curve. They can be useful as a cheap
     and simple alternative to constructing curves that are offsets 
     by definition.</rdfs:comment>
      <rdfs:subClassOf>
         <owl:Class>
            <owl:intersectionOf rdf:parseType="Collection">
               <owl:Restriction>
                  <owl:onProperty rdf:resource="http://www.opengis.net/gml#offsetBase"/>
                  <owl:allValuesFrom rdf:resource="http://www.opengis.net/gml#CurvePropertyType"/>
               </owl:Restriction>
               <owl:Restriction>
                  <owl:onProperty rdf:resource="http://www.opengis.net/gml#distance"/>
                  <owl:allValuesFrom rdf:resource="http://www.opengis.net/gml#LengthType"/>
               </owl:Restriction>
               <owl:Restriction>
                  <owl:onProperty rdf:resource="http://www.opengis.net/gml#refDirection"/>
                  <owl:allValuesFrom rdf:resource="http://www.opengis.net/gml#VectorType"/>
               </owl:Restriction>
               <owl:Restriction>
                  <owl:onProperty rdf:resource="http://www.opengis.net/gml#refDirection"/>
                  <owl:minCardinality rdf:datatype="http://www.w3.org/2001/XMLSchema#nonNegativeInteger">0</owl:minCardinality>
               </owl:Restriction>
            </owl:intersectionOf>
         </owl:Class>
      </rdfs:subClassOf>
      <rdfs:subClassOf rdf:resource="http://www.opengis.net/gml#AbstractCurveSegmentType"/>
   </owl:Class>
   <owl:Class rdf:about="http://www.opengis.net/gml#AffinePlacementType">
      <rdfs:comment>A placement takes a standard geometric
   construction and places it in geographic space. It defines a
   transformation from a constructive parameter space to the 
   co-ordinate space of the co-ordinate reference system being used.  
   Parameter spaces in formulae in this International Standard are 
   given as (u, v) in 2D and(u, v, w) in 3D. Co-ordinate reference 
   systems positions are given in formulae, in this International 
   Standard, by either (x, y) in 2D, or (x, y, z) in 3D.

   Affine placements are defined by linear transformations from 
   parameter space to the target co-ordiante space. 2-dimensional 
   Cartesian parameter space,(u,v) transforms into 3-dimensional co-
   ordinate reference systems,(x,y,z) by using an affine 
   transformation,(u,v)-&gt;(x,y,z) which is defined :

  x ux vx   x0
       u    
  y = uy vy   + y0
       v    
  x uz vz z0
  
   Then, given this equation, the location element of the 
   AffinePlacement is the direct position (x0, y0, z0), which is the
   target position of the origin in (u, v). The two reference
   directions (ux, uy, uz) and (vx, vy, vz) are the target     
   directions of the unit vectors at the origin in (u, v).</rdfs:comment>
      <rdfs:subClassOf>
         <owl:Class>
            <owl:intersectionOf rdf:parseType="Collection">
               <owl:Restriction>
                  <owl:onProperty rdf:resource="http://www.opengis.net/gml#location"/>
                  <owl:allValuesFrom rdf:resource="http://www.opengis.net/gml#DirectPositionType"/>
               </owl:Restriction>
               <owl:Restriction>
                  <owl:onProperty rdf:resource="http://www.opengis.net/gml#refDirection"/>
                  <owl:allValuesFrom rdf:resource="http://www.opengis.net/gml#VectorType"/>
               </owl:Restriction>
               <owl:Restriction>
                  <owl:onProperty rdf:resource="http://www.opengis.net/gml#inDimension"/>
                  <owl:allValuesFrom rdf:resource="http://www.w3.org/2001/XMLSchema#positiveInteger"/>
               </owl:Restriction>
               <owl:Restriction>
                  <owl:onProperty rdf:resource="http://www.opengis.net/gml#outDimension"/>
                  <owl:allValuesFrom rdf:resource="http://www.w3.org/2001/XMLSchema#positiveInteger"/>
               </owl:Restriction>
            </owl:intersectionOf>
         </owl:Class>
      </rdfs:subClassOf>
   </owl:Class>
   <owl:Class rdf:about="http://www.opengis.net/gml#ClothoidType">
      <rdfs:comment>A clothoid, or Cornu's spiral, is plane
   curve whose curvature is a fixed function of its length.
   In suitably chosen co-ordinates it is given by Fresnel's
   integrals.

    x(t) = 0-integral-t cos(AT*T/2)dT    
    
    y(t) = 0-integral-t sin(AT*T/2)dT
   
   This geometry is mainly used as a transition curve between
   curves of type straight line to circular arc or circular arc
   to circular arc. With this curve type it is possible to 
   achieve a C2-continous transition between the above mentioned
   curve types. One formula for the Clothoid is A*A = R*t where
   A is constant, R is the varying radius of curvature along the
   the curve and t is the length along and given in the Fresnel 
   integrals.</rdfs:comment>
      <rdfs:subClassOf>
         <owl:Class>
            <owl:intersectionOf rdf:parseType="Collection">
               <owl:Restriction>
                  <owl:onProperty rdf:resource="http://www.opengis.net/gml#hasrefLocation"/>
                  <owl:allValuesFrom rdf:resource="http://www.opengis.net/gml#refLocation"/>
               </owl:Restriction>
               <owl:Restriction>
                  <owl:onProperty rdf:resource="http://www.opengis.net/gml#scaleFactor"/>
                  <owl:allValuesFrom rdf:resource="http://www.w3.org/2001/XMLSchema#decimal"/>
               </owl:Restriction>
               <owl:Restriction>
                  <owl:onProperty rdf:resource="http://www.opengis.net/gml#startParameter"/>
                  <owl:allValuesFrom rdf:resource="http://www.w3.org/2001/XMLSchema#double"/>
               </owl:Restriction>
               <owl:Restriction>
                  <owl:onProperty rdf:resource="http://www.opengis.net/gml#endParameter"/>
                  <owl:allValuesFrom rdf:resource="http://www.w3.org/2001/XMLSchema#double"/>
               </owl:Restriction>
            </owl:intersectionOf>
         </owl:Class>
      </rdfs:subClassOf>
      <rdfs:subClassOf rdf:resource="http://www.opengis.net/gml#AbstractCurveSegmentType"/>
   </owl:Class>
   <owl:Class rdf:about="http://www.opengis.net/gml#refLocation">
      <rdfs:subClassOf>
         <owl:Class>
            <owl:intersectionOf rdf:parseType="Collection">
               <owl:Restriction>
                  <owl:onProperty rdf:resource="http://www.opengis.net/gml#hasAffinePlacement"/>
                  <owl:allValuesFrom rdf:resource="http://www.opengis.net/gml#AffinePlacement"/>
               </owl:Restriction>
            </owl:intersectionOf>
         </owl:Class>
      </rdfs:subClassOf>
   </owl:Class>
   <owl:Class rdf:about="http://www.opengis.net/gml#GeodesicStringType">
      <rdfs:comment>A GeodesicString consists of sequence of
   geodesic segments. The type essentially combines a sequence of
   Geodesic into a single object.
   The GeodesicString is computed from two or more positions and an
   interpolation using geodesics defined from the geoid (or 
   ellipsoid) of the co-ordinate reference system being used.</rdfs:comment>
      <owl:disjointUnionOf rdf:parseType="Collection">
         <owl:Restriction>
            <owl:onProperty rdf:resource="http://www.opengis.net/gml#hasposList"/>
            <owl:someValuesFrom rdf:resource="http://www.opengis.net/gml#posList"/>
         </owl:Restriction>
         <owl:Restriction>
            <owl:onProperty rdf:resource="http://www.opengis.net/gml#hasgeometricPositionGroup"/>
            <owl:allValuesFrom rdf:resource="http://www.opengis.net/gml#geometricPositionGroup"/>
         </owl:Restriction>
      </owl:disjointUnionOf>
      <rdfs:subClassOf>
         <owl:Class>
            <owl:intersectionOf rdf:parseType="Collection">
               <owl:Restriction>
                  <owl:onProperty rdf:resource="http://www.opengis.net/gml#interpolation"/>
                  <owl:allValuesFrom rdf:resource="http://www.opengis.net/gml#CurveInterpolationType"/>
               </owl:Restriction>
            </owl:intersectionOf>
         </owl:Class>
      </rdfs:subClassOf>
      <rdfs:subClassOf rdf:resource="http://www.opengis.net/gml#AbstractCurveSegmentType"/>
   </owl:Class>
   <owl:Class rdf:about="http://www.opengis.net/gml#GeodesicType">
      <rdfs:comment>A Geodesic consists of two distinct
   positions joined by a geodesic curve. The control points of
   a Geodesic shall lie on the geodesic between its start
   point and end points. Between these two points, a geodesic
   curve defined from ellipsoid or geoid model used by the
   co-ordinate reference systems may be used to interpolate
   other positions. Any other point in the controlPoint array
   must fall on this geodesic.</rdfs:comment>
      <rdfs:subClassOf rdf:resource="http://www.opengis.net/gml#GeodesicStringType"/>
   </owl:Class>
   <owl:Class rdf:about="http://www.opengis.net/gml#CubicSplineType">
      <rdfs:comment>Cubic splines are similar to line strings in that they are a sequence of segments each with its own defining function. A cubic spline uses the control points and a set of derivative parameters to define a piecewise 3rd degree polynomial interpolation. Unlike line-strings, the parameterization by arc length is not necessarily still a polynomial. 
        The function describing the curve must be C2, that is, have a continuous 1st and 2nd derivative at all points, and pass through the controlPoints in the order given. Between the control points, the curve segment is defined by a cubic polynomial. At each control point, the polynomial changes in such a manner that the 1st and 2nd derivative vectors are the same from either side. The control parameters record must contain vectorAtStart, and vectorAtEnd which are the unit tangent vectors at controlPoint[1] and controlPoint[n] where n = controlPoint.count. 
        Note: only the direction of the vectors is relevant, not their length.</rdfs:comment>
      <rdfs:subClassOf>
         <owl:Class>
            <owl:intersectionOf rdf:parseType="Collection">
               <owl:Restriction>
                  <owl:onProperty rdf:resource="http://www.opengis.net/gml#vectorAtStart"/>
                  <owl:allValuesFrom rdf:resource="http://www.opengis.net/gml#VectorType"/>
               </owl:Restriction>
               <owl:Restriction>
                  <owl:onProperty rdf:resource="http://www.opengis.net/gml#vectorAtEnd"/>
                  <owl:allValuesFrom rdf:resource="http://www.opengis.net/gml#VectorType"/>
               </owl:Restriction>
            </owl:intersectionOf>
         </owl:Class>
      </rdfs:subClassOf>
      <owl:disjointUnionOf rdf:parseType="Collection">
         <owl:Restriction>
            <owl:onProperty rdf:resource="http://www.opengis.net/gml#hasposList"/>
            <owl:someValuesFrom rdf:resource="http://www.opengis.net/gml#posList"/>
         </owl:Restriction>
         <owl:Restriction>
            <owl:onProperty rdf:resource="http://www.opengis.net/gml#hascoordinates"/>
            <owl:someValuesFrom rdf:resource="http://www.opengis.net/gml#coordinates"/>
         </owl:Restriction>
         <owl:Restriction>
            <owl:onProperty rdf:resource="http://www.opengis.net/gml#haspos"/>
            <owl:someValuesFrom rdf:resource="http://www.opengis.net/gml#pos"/>
         </owl:Restriction>
         <owl:Restriction>
            <owl:onProperty rdf:resource="http://www.opengis.net/gml#haspointProperty"/>
            <owl:someValuesFrom rdf:resource="http://www.opengis.net/gml#pointProperty"/>
         </owl:Restriction>
         <owl:Restriction>
            <owl:onProperty rdf:resource="http://www.opengis.net/gml#haspointRep"/>
            <owl:someValuesFrom rdf:resource="http://www.opengis.net/gml#pointRep"/>
         </owl:Restriction>
      </owl:disjointUnionOf>
      <rdfs:subClassOf>
         <owl:Class>
            <owl:intersectionOf rdf:parseType="Collection">
               <owl:Restriction>
                  <owl:onProperty rdf:resource="http://www.opengis.net/gml#interpolation"/>
                  <owl:allValuesFrom rdf:resource="http://www.opengis.net/gml#CurveInterpolationType"/>
               </owl:Restriction>
               <owl:Restriction>
                  <owl:onProperty rdf:resource="http://www.opengis.net/gml#degree"/>
                  <owl:allValuesFrom rdf:resource="http://www.w3.org/2001/XMLSchema#integer"/>
               </owl:Restriction>
            </owl:intersectionOf>
         </owl:Class>
      </rdfs:subClassOf>
      <rdfs:subClassOf rdf:resource="http://www.opengis.net/gml#AbstractCurveSegmentType"/>
   </owl:Class>
   <owl:Class rdf:about="http://www.opengis.net/gml#KnotType">
      <rdfs:comment>A knot is a breakpoint on a piecewise spline curve.</rdfs:comment>
      <rdfs:subClassOf>
         <owl:Class>
            <owl:intersectionOf rdf:parseType="Collection">
               <owl:Restriction>
                  <owl:onProperty rdf:resource="http://www.opengis.net/gml#value"/>
                  <owl:allValuesFrom rdf:resource="http://www.w3.org/2001/XMLSchema#double"/>
               </owl:Restriction>
               <owl:Restriction>
                  <owl:onProperty rdf:resource="http://www.opengis.net/gml#multiplicity"/>
                  <owl:allValuesFrom rdf:resource="http://www.w3.org/2001/XMLSchema#nonNegativeInteger"/>
               </owl:Restriction>
               <owl:Restriction>
                  <owl:onProperty rdf:resource="http://www.opengis.net/gml#weight"/>
                  <owl:allValuesFrom rdf:resource="http://www.w3.org/2001/XMLSchema#double"/>
               </owl:Restriction>
            </owl:intersectionOf>
         </owl:Class>
      </rdfs:subClassOf>
   </owl:Class>
   <owl:Class rdf:about="http://www.opengis.net/gml#KnotPropertyType">
      <rdfs:comment>Encapsulates a knot to use it in a geometric type.</rdfs:comment>
      <rdfs:subClassOf>
         <owl:Class>
            <owl:intersectionOf rdf:parseType="Collection">
               <owl:Restriction>
                  <owl:onProperty rdf:resource="http://www.opengis.net/gml#Knot"/>
                  <owl:allValuesFrom rdf:resource="http://www.opengis.net/gml#KnotType"/>
               </owl:Restriction>
            </owl:intersectionOf>
         </owl:Class>
      </rdfs:subClassOf>
   </owl:Class>
   <owl:Class rdf:about="http://www.opengis.net/gml#BSplineType">
      <rdfs:comment>A B-Spline is a piecewise parametric polynomial or rational curve described in terms of control points and basis functions. Knots are breakpoints on the curve that connect its pieces. They are given as a non-decreasing sequence of real numbers. If the weights in the knots are equal then it is a polynomial spline. The degree is the algebraic degree of the basis functions.</rdfs:comment>
      <rdfs:subClassOf>
         <owl:Class>
            <owl:intersectionOf rdf:parseType="Collection">
               <owl:Restriction>
                  <owl:onProperty rdf:resource="http://www.opengis.net/gml#degree"/>
                  <owl:allValuesFrom rdf:resource="http://www.w3.org/2001/XMLSchema#nonNegativeInteger"/>
               </owl:Restriction>
               <owl:Restriction>
                  <owl:onProperty rdf:resource="http://www.opengis.net/gml#knot"/>
                  <owl:allValuesFrom rdf:resource="http://www.opengis.net/gml#KnotPropertyType"/>
               </owl:Restriction>
               <owl:Restriction>
                  <owl:onProperty rdf:resource="http://www.opengis.net/gml#knot"/>
                  <owl:minCardinality rdf:datatype="http://www.w3.org/2001/XMLSchema#nonNegativeInteger">2</owl:minCardinality>
               </owl:Restriction>
            </owl:intersectionOf>
         </owl:Class>
      </rdfs:subClassOf>
      <owl:disjointUnionOf rdf:parseType="Collection">
         <owl:Restriction>
            <owl:onProperty rdf:resource="http://www.opengis.net/gml#hasposList"/>
            <owl:someValuesFrom rdf:resource="http://www.opengis.net/gml#posList"/>
         </owl:Restriction>
         <owl:Restriction>
            <owl:onProperty rdf:resource="http://www.opengis.net/gml#hascoordinates"/>
            <owl:someValuesFrom rdf:resource="http://www.opengis.net/gml#coordinates"/>
         </owl:Restriction>
         <owl:Restriction>
            <owl:onProperty rdf:resource="http://www.opengis.net/gml#haspos"/>
            <owl:someValuesFrom rdf:resource="http://www.opengis.net/gml#pos"/>
         </owl:Restriction>
         <owl:Restriction>
            <owl:onProperty rdf:resource="http://www.opengis.net/gml#haspointProperty"/>
            <owl:someValuesFrom rdf:resource="http://www.opengis.net/gml#pointProperty"/>
         </owl:Restriction>
         <owl:Restriction>
            <owl:onProperty rdf:resource="http://www.opengis.net/gml#haspointRep"/>
            <owl:someValuesFrom rdf:resource="http://www.opengis.net/gml#pointRep"/>
         </owl:Restriction>
      </owl:disjointUnionOf>
      <rdfs:subClassOf>
         <owl:Class>
            <owl:intersectionOf rdf:parseType="Collection">
               <owl:Restriction>
                  <owl:onProperty rdf:resource="http://www.opengis.net/gml#interpolation"/>
                  <owl:allValuesFrom rdf:resource="http://www.opengis.net/gml#CurveInterpolationType"/>
               </owl:Restriction>
               <owl:Restriction>
                  <owl:onProperty rdf:resource="http://www.opengis.net/gml#isPolynomial"/>
                  <owl:allValuesFrom rdf:resource="http://www.w3.org/2001/XMLSchema#boolean"/>
               </owl:Restriction>
               <owl:Restriction>
                  <owl:onProperty rdf:resource="http://www.opengis.net/gml#knotType"/>
                  <owl:allValuesFrom rdf:resource="http://www.opengis.net/gml#KnotTypesType"/>
               </owl:Restriction>
            </owl:intersectionOf>
         </owl:Class>
      </rdfs:subClassOf>
      <rdfs:subClassOf rdf:resource="http://www.opengis.net/gml#AbstractCurveSegmentType"/>
   </owl:Class>
   <owl:Class rdf:about="http://www.opengis.net/gml#BezierType">
      <rdfs:comment>Bezier curves are polynomial splines that use Bezier or Bernstein polynomials for interpolation purposes. It is a special case of the B-Spline curve with two knots.</rdfs:comment>
      <rdfs:subClassOf>
         <owl:Class>
            <owl:intersectionOf rdf:parseType="Collection">
               <owl:Restriction>
                  <owl:onProperty rdf:resource="http://www.opengis.net/gml#degree"/>
                  <owl:allValuesFrom rdf:resource="http://www.w3.org/2001/XMLSchema#nonNegativeInteger"/>
               </owl:Restriction>
               <owl:Restriction>
                  <owl:onProperty rdf:resource="http://www.opengis.net/gml#knot"/>
                  <owl:allValuesFrom rdf:resource="http://www.opengis.net/gml#KnotPropertyType"/>
               </owl:Restriction>
               <owl:Restriction>
                  <owl:onProperty rdf:resource="http://www.opengis.net/gml#knot"/>
                  <owl:cardinality rdf:datatype="http://www.w3.org/2001/XMLSchema#nonNegativeInteger">2</owl:cardinality>
               </owl:Restriction>
            </owl:intersectionOf>
         </owl:Class>
      </rdfs:subClassOf>
      <owl:disjointUnionOf rdf:parseType="Collection">
         <owl:Restriction>
            <owl:onProperty rdf:resource="http://www.opengis.net/gml#hasposList"/>
            <owl:someValuesFrom rdf:resource="http://www.opengis.net/gml#posList"/>
         </owl:Restriction>
         <owl:Restriction>
            <owl:onProperty rdf:resource="http://www.opengis.net/gml#hascoordinates"/>
            <owl:someValuesFrom rdf:resource="http://www.opengis.net/gml#coordinates"/>
         </owl:Restriction>
         <owl:Restriction>
            <owl:onProperty rdf:resource="http://www.opengis.net/gml#haspos"/>
            <owl:someValuesFrom rdf:resource="http://www.opengis.net/gml#pos"/>
         </owl:Restriction>
         <owl:Restriction>
            <owl:onProperty rdf:resource="http://www.opengis.net/gml#haspointProperty"/>
            <owl:someValuesFrom rdf:resource="http://www.opengis.net/gml#pointProperty"/>
         </owl:Restriction>
         <owl:Restriction>
            <owl:onProperty rdf:resource="http://www.opengis.net/gml#haspointRep"/>
            <owl:someValuesFrom rdf:resource="http://www.opengis.net/gml#pointRep"/>
         </owl:Restriction>
      </owl:disjointUnionOf>
      <rdfs:subClassOf>
         <owl:Class>
            <owl:intersectionOf rdf:parseType="Collection">
               <owl:Restriction>
                  <owl:onProperty rdf:resource="http://www.opengis.net/gml#interpolation"/>
                  <owl:allValuesFrom rdf:resource="http://www.opengis.net/gml#CurveInterpolationType"/>
               </owl:Restriction>
               <owl:Restriction>
                  <owl:onProperty rdf:resource="http://www.opengis.net/gml#isPolynomial"/>
                  <owl:allValuesFrom rdf:resource="http://www.w3.org/2001/XMLSchema#boolean"/>
               </owl:Restriction>
               <owl:Restriction>
                  <owl:onProperty rdf:resource="http://www.opengis.net/gml#knotType"/>
                  <owl:allValuesFrom rdf:resource="http://www.opengis.net/gml#KnotTypesType"/>
               </owl:Restriction>
            </owl:intersectionOf>
         </owl:Class>
      </rdfs:subClassOf>
      <rdfs:subClassOf rdf:resource="http://www.opengis.net/gml#BSplineType"/>
   </owl:Class>
   <owl:Class rdf:about="http://www.opengis.net/gml#SurfaceType">
      <rdfs:comment>A Surface is a 2-dimensional primitive and is composed of one or more surface patches. The surface patches are connected to one another.
        The orientation of the surface is positive ("up"). The orientation of a surface chooses an "up" direction through the choice of the upward normal, which, if the surface is not a cycle, is the side of the surface from which the exterior boundary appears counterclockwise. Reversal of the surface orientation reverses the curve orientation of each boundary component, and interchanges the conceptual "up" and "down" direction of the surface. If the surface is the boundary of a solid, the "up" direction is usually outward. For closed surfaces, which have no boundary, the up direction is that of the surface patches, which must be consistent with one another. Its included surface patches describe the interior structure of the Surface.</rdfs:comment>
      <rdfs:subClassOf>
         <owl:Class>
            <owl:intersectionOf rdf:parseType="Collection">
               <owl:Restriction>
                  <owl:onProperty rdf:resource="http://www.opengis.net/gml#haspatches"/>
                  <owl:allValuesFrom rdf:resource="http://www.opengis.net/gml#patches"/>
               </owl:Restriction>
            </owl:intersectionOf>
         </owl:Class>
      </rdfs:subClassOf>
      <rdfs:subClassOf rdf:resource="http://www.opengis.net/gml#AbstractSurfaceType"/>
   </owl:Class>
   <owl:Class rdf:about="http://www.opengis.net/gml#OrientableSurfaceType">
      <rdfs:comment>OrientableSurface consists of a surface and an orientation. If the orientation is "+", then the OrientableSurface is identical to the baseSurface. If the orientation is "-", then the OrientableSurface is a reference to a Surface with an up-normal that reverses the direction for this OrientableSurface, the sense of "the top of the surface".</rdfs:comment>
      <rdfs:subClassOf>
         <owl:Class>
            <owl:intersectionOf rdf:parseType="Collection">
               <owl:Restriction>
                  <owl:onProperty rdf:resource="http://www.opengis.net/gml#hasbaseSurface"/>
                  <owl:allValuesFrom rdf:resource="http://www.opengis.net/gml#baseSurface"/>
               </owl:Restriction>
            </owl:intersectionOf>
         </owl:Class>
      </rdfs:subClassOf>
      <rdfs:subClassOf>
         <owl:Class>
            <owl:intersectionOf rdf:parseType="Collection">
               <owl:Restriction>
                  <owl:onProperty rdf:resource="http://www.opengis.net/gml#orientation"/>
                  <owl:allValuesFrom rdf:resource="http://www.opengis.net/gml#SignType"/>
               </owl:Restriction>
            </owl:intersectionOf>
         </owl:Class>
      </rdfs:subClassOf>
      <rdfs:subClassOf rdf:resource="http://www.opengis.net/gml#AbstractSurfaceType"/>
   </owl:Class>
   <owl:Class rdf:about="http://www.opengis.net/gml#AbstractSurfacePatchType">
      <rdfs:comment>This is an abstract class</rdfs:comment>
      <rdfs:comment>A surface patch defines a homogenuous portion of a surface.</rdfs:comment>
   </owl:Class>
   <owl:Class rdf:about="http://www.opengis.net/gml#SurfacePatchArrayPropertyType">
      <rdfs:comment>A container for an array of surface patches.</rdfs:comment>
      <rdfs:subClassOf>
         <owl:Class>
            <owl:intersectionOf rdf:parseType="Collection">
               <owl:Restriction>
                  <owl:onProperty rdf:resource="http://www.opengis.net/gml#has_SurfacePatch"/>
                  <owl:allValuesFrom rdf:resource="http://www.opengis.net/gml#_SurfacePatch"/>
               </owl:Restriction>
            </owl:intersectionOf>
         </owl:Class>
      </rdfs:subClassOf>
   </owl:Class>
   <owl:Class rdf:about="http://www.opengis.net/gml#PolygonPatchType">
      <rdfs:comment>A PolygonPatch is a surface patch that is defined by a set of boundary curves and an underlying surface to which these curves adhere. The curves are coplanar and the polygon uses planar interpolation in its interior. Implements GM_Polygon of ISO 19107.</rdfs:comment>
      <rdfs:subClassOf>
         <owl:Class>
            <owl:intersectionOf rdf:parseType="Collection">
               <owl:Restriction>
                  <owl:onProperty rdf:resource="http://www.opengis.net/gml#hasexterior"/>
                  <owl:allValuesFrom rdf:resource="http://www.opengis.net/gml#exterior"/>
               </owl:Restriction>
               <owl:Restriction>
                  <owl:onProperty rdf:resource="http://www.opengis.net/gml#hasexterior"/>
                  <owl:minCardinality rdf:datatype="http://www.w3.org/2001/XMLSchema#nonNegativeInteger">0</owl:minCardinality>
               </owl:Restriction>
               <owl:Restriction>
                  <owl:onProperty rdf:resource="http://www.opengis.net/gml#hasinterior"/>
                  <owl:allValuesFrom rdf:resource="http://www.opengis.net/gml#interior"/>
               </owl:Restriction>
               <owl:Restriction>
                  <owl:onProperty rdf:resource="http://www.opengis.net/gml#hasinterior"/>
                  <owl:minCardinality rdf:datatype="http://www.w3.org/2001/XMLSchema#nonNegativeInteger">0</owl:minCardinality>
               </owl:Restriction>
            </owl:intersectionOf>
         </owl:Class>
      </rdfs:subClassOf>
      <rdfs:subClassOf>
         <owl:Class>
            <owl:intersectionOf rdf:parseType="Collection">
               <owl:Restriction>
                  <owl:onProperty rdf:resource="http://www.opengis.net/gml#interpolation"/>
                  <owl:allValuesFrom rdf:resource="http://www.opengis.net/gml#SurfaceInterpolationType"/>
               </owl:Restriction>
            </owl:intersectionOf>
         </owl:Class>
      </rdfs:subClassOf>
      <rdfs:subClassOf rdf:resource="http://www.opengis.net/gml#AbstractSurfacePatchType"/>
   </owl:Class>
   <owl:Class rdf:about="http://www.opengis.net/gml#TriangleType">
      <rdfs:comment>Represents a triangle as a surface with an outer boundary consisting of a linear ring. Note that this is a polygon (subtype) with no inner boundaries. The number of points in the linear ring must be four.</rdfs:comment>
      <rdfs:subClassOf>
         <owl:Class>
            <owl:intersectionOf rdf:parseType="Collection">
               <owl:Restriction>
                  <owl:onProperty rdf:resource="http://www.opengis.net/gml#hasexterior"/>
                  <owl:allValuesFrom rdf:resource="http://www.opengis.net/gml#exterior"/>
               </owl:Restriction>
            </owl:intersectionOf>
         </owl:Class>
      </rdfs:subClassOf>
      <rdfs:subClassOf>
         <owl:Class>
            <owl:intersectionOf rdf:parseType="Collection">
               <owl:Restriction>
                  <owl:onProperty rdf:resource="http://www.opengis.net/gml#interpolation"/>
                  <owl:allValuesFrom rdf:resource="http://www.opengis.net/gml#SurfaceInterpolationType"/>
               </owl:Restriction>
            </owl:intersectionOf>
         </owl:Class>
      </rdfs:subClassOf>
      <rdfs:subClassOf rdf:resource="http://www.opengis.net/gml#AbstractSurfacePatchType"/>
   </owl:Class>
   <owl:Class rdf:about="http://www.opengis.net/gml#RectangleType">
      <rdfs:comment>Represents a rectangle as a surface with an outer boundary consisting of a linear ring. Note that this is a polygon (subtype) with no inner boundaries. The number of points in the linear ring must be five.</rdfs:comment>
      <rdfs:subClassOf>
         <owl:Class>
            <owl:intersectionOf rdf:parseType="Collection">
               <owl:Restriction>
                  <owl:onProperty rdf:resource="http://www.opengis.net/gml#hasexterior"/>
                  <owl:allValuesFrom rdf:resource="http://www.opengis.net/gml#exterior"/>
               </owl:Restriction>
            </owl:intersectionOf>
         </owl:Class>
      </rdfs:subClassOf>
      <rdfs:subClassOf>
         <owl:Class>
            <owl:intersectionOf rdf:parseType="Collection">
               <owl:Restriction>
                  <owl:onProperty rdf:resource="http://www.opengis.net/gml#interpolation"/>
                  <owl:allValuesFrom rdf:resource="http://www.opengis.net/gml#SurfaceInterpolationType"/>
               </owl:Restriction>
            </owl:intersectionOf>
         </owl:Class>
      </rdfs:subClassOf>
      <rdfs:subClassOf rdf:resource="http://www.opengis.net/gml#AbstractSurfacePatchType"/>
   </owl:Class>
   <owl:Class rdf:about="http://www.opengis.net/gml#RingType">
      <rdfs:comment>A Ring is used to represent a single connected component of a surface boundary. It consists of a sequence of curves connected in a cycle (an object whose boundary is empty).
A Ring is structurally similar to a composite curve in that the endPoint of each curve in the sequence is the startPoint of the next curve in the Sequence. Since the sequence is circular, there is no exception to this rule. Each ring, like all boundaries, is a cycle and each ring is simple.
NOTE: Even though each Ring is simple, the boundary need not be simple. The easiest case of this is where one of the interior rings of a surface is tangent to its exterior ring.</rdfs:comment>
      <rdfs:subClassOf>
         <owl:Class>
            <owl:intersectionOf rdf:parseType="Collection">
               <owl:Restriction>
                  <owl:onProperty rdf:resource="http://www.opengis.net/gml#hascurveMember"/>
                  <owl:allValuesFrom rdf:resource="http://www.opengis.net/gml#curveMember"/>
               </owl:Restriction>
            </owl:intersectionOf>
         </owl:Class>
      </rdfs:subClassOf>
      <rdfs:subClassOf rdf:resource="http://www.opengis.net/gml#AbstractRingType"/>
   </owl:Class>
   <owl:Class rdf:about="http://www.opengis.net/gml#RingPropertyType">
      <rdfs:comment>Encapsulates a ring to represent properties in features or geometry collections.</rdfs:comment>
      <rdfs:subClassOf>
         <owl:Class>
            <owl:intersectionOf rdf:parseType="Collection">
               <owl:Restriction>
                  <owl:onProperty rdf:resource="http://www.opengis.net/gml#hasRing"/>
                  <owl:allValuesFrom rdf:resource="http://www.opengis.net/gml#Ring"/>
               </owl:Restriction>
            </owl:intersectionOf>
         </owl:Class>
      </rdfs:subClassOf>
   </owl:Class>
   <owl:Class rdf:about="http://www.opengis.net/gml#row">
      <rdfs:subClassOf rdf:resource="http://www.opengis.net/gml#geometricPositionListGroup"/>
   </owl:Class>
   <owl:Class rdf:about="http://www.opengis.net/gml#AbstractParametricCurveSurfaceType">
      <rdfs:subClassOf rdf:resource="http://www.opengis.net/gml#AbstractSurfacePatchType"/>
   </owl:Class>
   <owl:Class rdf:about="http://www.opengis.net/gml#AbstractGriddedSurfaceType">
      <rdfs:comment>A gridded surface is a parametric curve
   surface derived from a rectangular grid in the parameter
   space. The rows from this grid are control points for
   horizontal surface curves; the columns are control points
   for vertical surface curves. The working assumption is that
   for a pair of parametric co-ordinates (s, t) that the
   horizontal curves for each integer offset are calculated
   and evaluated at "s". The defines a sequence of control
   points:
   
   cn(s) : s  1 .....columns 

   From this sequence a vertical curve is calculated for "s",
   and evaluated at "t". In most cases, the order of
   calculation (horizontal-vertical vs. vertical-horizontal)
   does not make a difference. Where it does, the horizontal-   
   vertical order shall be the one used.

   Logically, any pair of curve interpolation types can lead
   to a subtype of GriddedSurface. The following clauses
   define some most commonly encountered surfaces that can
   be represented in this manner.</rdfs:comment>
      <rdfs:subClassOf>
         <owl:Class>
            <owl:intersectionOf rdf:parseType="Collection">
               <owl:Restriction>
                  <owl:onProperty rdf:resource="http://www.opengis.net/gml#rows"/>
                  <owl:allValuesFrom rdf:resource="http://www.w3.org/2001/XMLSchema#integer"/>
               </owl:Restriction>
               <owl:Restriction>
                  <owl:onProperty rdf:resource="http://www.opengis.net/gml#rows"/>
                  <owl:minCardinality rdf:datatype="http://www.w3.org/2001/XMLSchema#nonNegativeInteger">0</owl:minCardinality>
               </owl:Restriction>
               <owl:Restriction>
                  <owl:onProperty rdf:resource="http://www.opengis.net/gml#columns"/>
                  <owl:allValuesFrom rdf:resource="http://www.w3.org/2001/XMLSchema#integer"/>
               </owl:Restriction>
               <owl:Restriction>
                  <owl:onProperty rdf:resource="http://www.opengis.net/gml#columns"/>
                  <owl:minCardinality rdf:datatype="http://www.w3.org/2001/XMLSchema#nonNegativeInteger">0</owl:minCardinality>
               </owl:Restriction>
            </owl:intersectionOf>
         </owl:Class>
      </rdfs:subClassOf>
      <rdfs:subClassOf rdf:resource="http://www.opengis.net/gml#PointGrid"/>
      <rdfs:subClassOf rdf:resource="http://www.opengis.net/gml#AbstractParametricCurveSurfaceType"/>
   </owl:Class>
   <owl:Class rdf:about="http://www.opengis.net/gml#ConeType">
      <rdfs:comment>A cone is a gridded surface given as a
   family of conic sections whose control points vary linearly.
   NOTE! A 5-point ellipse with all defining positions identical
   is a point. Thus, a truncated elliptical cone can be given as a
   2x5 set of control points
   ((P1, P1, P1, P1, P1), (P2, P3, P4, P5, P6)). P1 is the apex 
   of the cone. P2, P3,P4, P5 and P6 are any five distinct points
   around the base ellipse of the cone. If the horizontal curves
   are circles as opposed to ellipses, the a circular cone can
   be constructed using ((P1, P1, P1),(P2, P3, P4)). The apex most     
   not coinside with the other plane.</rdfs:comment>
      <rdfs:subClassOf>
         <owl:Class>
            <owl:intersectionOf rdf:parseType="Collection">
               <owl:Restriction>
                  <owl:onProperty rdf:resource="http://www.opengis.net/gml#horizontalCurveType"/>
                  <owl:allValuesFrom rdf:resource="http://www.opengis.net/gml#CurveInterpolationType"/>
               </owl:Restriction>
               <owl:Restriction>
                  <owl:onProperty rdf:resource="http://www.opengis.net/gml#verticalCurveType"/>
                  <owl:allValuesFrom rdf:resource="http://www.opengis.net/gml#CurveInterpolationType"/>
               </owl:Restriction>
            </owl:intersectionOf>
         </owl:Class>
      </rdfs:subClassOf>
      <rdfs:subClassOf rdf:resource="http://www.opengis.net/gml#AbstractGriddedSurfaceType"/>
   </owl:Class>
   <owl:Class rdf:about="http://www.opengis.net/gml#CylinderType">
      <rdfs:comment>A cylinder is a gridded surface given as a
   family of circles whose positions vary along a set of parallel
   lines, keeping the cross sectional horizontal curves of a
   constant shape.
   NOTE! Given the same working assumptions as in the previous
   note, a Cylinder can be given by two circles, giving us the
   control points of the form ((P1, P2, P3),(P4, P5, P6)).</rdfs:comment>
      <rdfs:subClassOf>
         <owl:Class>
            <owl:intersectionOf rdf:parseType="Collection">
               <owl:Restriction>
                  <owl:onProperty rdf:resource="http://www.opengis.net/gml#horizontalCurveType"/>
                  <owl:allValuesFrom rdf:resource="http://www.opengis.net/gml#CurveInterpolationType"/>
               </owl:Restriction>
               <owl:Restriction>
                  <owl:onProperty rdf:resource="http://www.opengis.net/gml#verticalCurveType"/>
                  <owl:allValuesFrom rdf:resource="http://www.opengis.net/gml#CurveInterpolationType"/>
               </owl:Restriction>
            </owl:intersectionOf>
         </owl:Class>
      </rdfs:subClassOf>
      <rdfs:subClassOf rdf:resource="http://www.opengis.net/gml#AbstractGriddedSurfaceType"/>
   </owl:Class>
   <owl:Class rdf:about="http://www.opengis.net/gml#SphereType">
      <rdfs:comment>A sphere is a gridded surface given as a
   family of circles whose positions vary linearly along the
   axis of the sphere, and whise radius varies in proportions to
   the cosine function of the central angle. The horizontal 
   circles resemble lines of constant latitude, and the vertical
   arcs resemble lines of constant longitude. 
   NOTE! If the control points are sorted in terms of increasing
   longitude, and increasing latitude, the upNormal of a sphere
   is the outward normal.
   EXAMPLE If we take a gridded set of latitudes and longitudes
   in degrees,(u,v) such as

  (-90,-180)  (-90,-90)  (-90,0)  (-90,  90) (-90, 180) 
  (-45,-180)  (-45,-90)  (-45,0)  (-45,  90) (-45, 180) 
  (  0,-180)  (  0,-90)  (  0,0)  (  0,  90) (  0, 180)
  ( 45,-180)  ( 45,-90)  ( 45,0)  ( 45, -90) ( 45, 180)
  ( 90,-180)  ( 90,-90)  ( 90,0)  ( 90, -90) ( 90, 180)
   
   And map these points to 3D using the usual equations (where R
   is the radius of the required sphere).

    z = R sin u
    x = (R cos u)(sin v)
    y = (R cos u)(cos v)

   We have a sphere of Radius R, centred at (0,0), as a gridded
   surface. Notice that the entire first row and the entire last
   row of the control points map to a single point in each 3D
   Euclidean space, North and South poles respectively, and that
   each horizontal curve closes back on itself forming a 
   geometric cycle. This gives us a metrically bounded (of finite
   size), topologically unbounded (not having a boundary, a
   cycle) surface.</rdfs:comment>
      <rdfs:subClassOf>
         <owl:Class>
            <owl:intersectionOf rdf:parseType="Collection">
               <owl:Restriction>
                  <owl:onProperty rdf:resource="http://www.opengis.net/gml#horizontalCurveType"/>
                  <owl:allValuesFrom rdf:resource="http://www.opengis.net/gml#CurveInterpolationType"/>
               </owl:Restriction>
               <owl:Restriction>
                  <owl:onProperty rdf:resource="http://www.opengis.net/gml#verticalCurveType"/>
                  <owl:allValuesFrom rdf:resource="http://www.opengis.net/gml#CurveInterpolationType"/>
               </owl:Restriction>
            </owl:intersectionOf>
         </owl:Class>
      </rdfs:subClassOf>
      <rdfs:subClassOf rdf:resource="http://www.opengis.net/gml#AbstractGriddedSurfaceType"/>
   </owl:Class>
   <owl:Class rdf:about="http://www.opengis.net/gml#PolyhedralSurfaceType">
      <rdfs:comment>A polyhedral surface is a surface composed
   of polygon surfaces connected along their common boundary 
   curves. This differs from the surface type only in the
   restriction on the types of surface patches acceptable.</rdfs:comment>
      <rdfs:subClassOf>
         <owl:Class>
            <owl:intersectionOf rdf:parseType="Collection">
               <owl:Restriction>
                  <owl:onProperty rdf:resource="http://www.opengis.net/gml#haspolygonPatches"/>
                  <owl:allValuesFrom rdf:resource="http://www.opengis.net/gml#polygonPatches"/>
               </owl:Restriction>
            </owl:intersectionOf>
         </owl:Class>
      </rdfs:subClassOf>
      <rdfs:subClassOf rdf:resource="http://www.opengis.net/gml#StandardObjectProperties"/>
      <rdfs:subClassOf rdf:resource="http://www.opengis.net/gml#SurfaceType"/>
   </owl:Class>
   <owl:Class rdf:about="http://www.opengis.net/gml#PolygonPatchArrayPropertyType">
      <rdfs:comment>This type defines a container for an array of 
   polygon patches.</rdfs:comment>
      <rdfs:subClassOf>
         <owl:Class>
            <owl:intersectionOf rdf:parseType="Collection">
               <owl:Restriction>
                  <owl:onProperty rdf:resource="http://www.opengis.net/gml#hasPolygonPatch"/>
                  <owl:allValuesFrom rdf:resource="http://www.opengis.net/gml#PolygonPatch"/>
               </owl:Restriction>
            </owl:intersectionOf>
         </owl:Class>
      </rdfs:subClassOf>
      <rdfs:subClassOf rdf:resource="http://www.opengis.net/gml#SurfacePatchArrayPropertyType"/>
   </owl:Class>
   <owl:Class rdf:about="http://www.opengis.net/gml#TrianglePatchArrayPropertyType">
      <rdfs:comment>This type defines a container for an array of 
     triangle patches.</rdfs:comment>
      <rdfs:subClassOf>
         <owl:Class>
            <owl:intersectionOf rdf:parseType="Collection">
               <owl:Restriction>
                  <owl:onProperty rdf:resource="http://www.opengis.net/gml#hasTriangle"/>
                  <owl:allValuesFrom rdf:resource="http://www.opengis.net/gml#Triangle"/>
               </owl:Restriction>
            </owl:intersectionOf>
         </owl:Class>
      </rdfs:subClassOf>
      <rdfs:subClassOf rdf:resource="http://www.opengis.net/gml#SurfacePatchArrayPropertyType"/>
   </owl:Class>
   <owl:Class rdf:about="http://www.opengis.net/gml#TriangulatedSurfaceType">
      <rdfs:comment>A triangulated surface is a polyhedral 
   surface that is composed only of triangles. There is no
   restriction on how the triangulation is derived.</rdfs:comment>
      <rdfs:subClassOf>
         <owl:Class>
            <owl:intersectionOf rdf:parseType="Collection">
               <owl:Restriction>
                  <owl:onProperty rdf:resource="http://www.opengis.net/gml#hastrianglePatches"/>
                  <owl:allValuesFrom rdf:resource="http://www.opengis.net/gml#trianglePatches"/>
               </owl:Restriction>
            </owl:intersectionOf>
         </owl:Class>
      </rdfs:subClassOf>
      <rdfs:subClassOf rdf:resource="http://www.opengis.net/gml#StandardObjectProperties"/>
      <rdfs:subClassOf rdf:resource="http://www.opengis.net/gml#SurfaceType"/>
   </owl:Class>
   <owl:Class rdf:about="http://www.opengis.net/gml#TinType">
      <rdfs:comment>A tin is a triangulated surface that uses
   the Delauny algorithm or a similar algorithm complemented with
   consideration of breaklines, stoplines, and maximum length of 
   triangle sides. These networks satisfy the Delauny's criterion
   away from the modifications: Fore each triangle in the 
   network, the circle passing through its vertices does not
   contain, in its interior, the vertex of any other triangle.</rdfs:comment>
      <rdfs:subClassOf>
         <owl:Class>
            <owl:intersectionOf rdf:parseType="Collection">
               <owl:Restriction>
                  <owl:onProperty rdf:resource="http://www.opengis.net/gml#stopLines"/>
                  <owl:allValuesFrom rdf:resource="http://www.opengis.net/gml#LineStringSegmentArrayPropertyType"/>
               </owl:Restriction>
               <owl:Restriction>
                  <owl:onProperty rdf:resource="http://www.opengis.net/gml#stopLines"/>
                  <owl:minCardinality rdf:datatype="http://www.w3.org/2001/XMLSchema#nonNegativeInteger">0</owl:minCardinality>
               </owl:Restriction>
               <owl:Restriction>
                  <owl:onProperty rdf:resource="http://www.opengis.net/gml#breakLines"/>
                  <owl:allValuesFrom rdf:resource="http://www.opengis.net/gml#LineStringSegmentArrayPropertyType"/>
               </owl:Restriction>
               <owl:Restriction>
                  <owl:onProperty rdf:resource="http://www.opengis.net/gml#breakLines"/>
                  <owl:minCardinality rdf:datatype="http://www.w3.org/2001/XMLSchema#nonNegativeInteger">0</owl:minCardinality>
               </owl:Restriction>
               <owl:Restriction>
                  <owl:onProperty rdf:resource="http://www.opengis.net/gml#maxLength"/>
                  <owl:allValuesFrom rdf:resource="http://www.opengis.net/gml#LengthType"/>
               </owl:Restriction>
               <owl:Restriction>
                  <owl:onProperty rdf:resource="http://www.opengis.net/gml#hascontrolPoint"/>
                  <owl:allValuesFrom rdf:resource="http://www.opengis.net/gml#controlPoint"/>
               </owl:Restriction>
            </owl:intersectionOf>
         </owl:Class>
      </rdfs:subClassOf>
      <rdfs:subClassOf rdf:resource="http://www.opengis.net/gml#TriangulatedSurfaceType"/>
   </owl:Class>
   <owl:Class rdf:about="http://www.opengis.net/gml#controlPoint">
      <rdfs:comment>The corners of the triangles in the TIN 
  are often referred to as pots. ControlPoint shall contain a 
  set of the GM_Position used as posts for this TIN. Since each  
  TIN contains triangles, there must be at least 3 posts. The 
       order in which these points are given does not affect the 
       surface that is represented. Application schemas may add 
       information based on ordering of control points to facilitate 
       the reconstruction of the TIN from the control points.</rdfs:comment>
      <owl:disjointUnionOf rdf:parseType="Collection">
         <owl:Restriction>
            <owl:onProperty rdf:resource="http://www.opengis.net/gml#hasposList"/>
            <owl:someValuesFrom rdf:resource="http://www.opengis.net/gml#posList"/>
         </owl:Restriction>
         <owl:Restriction>
            <owl:onProperty rdf:resource="http://www.opengis.net/gml#hasgeometricPositionGroup"/>
            <owl:allValuesFrom rdf:resource="http://www.opengis.net/gml#geometricPositionGroup"/>
         </owl:Restriction>
      </owl:disjointUnionOf>
   </owl:Class>
   <owl:Class rdf:about="http://www.opengis.net/gml#LineStringSegmentArrayPropertyType">
      <rdfs:subClassOf>
         <owl:Class>
            <owl:intersectionOf rdf:parseType="Collection">
               <owl:Restriction>
                  <owl:onProperty rdf:resource="http://www.opengis.net/gml#hasLineStringSegment"/>
                  <owl:allValuesFrom rdf:resource="http://www.opengis.net/gml#LineStringSegment"/>
               </owl:Restriction>
               <owl:Restriction>
                  <owl:onProperty rdf:resource="http://www.opengis.net/gml#hasLineStringSegment"/>
                  <owl:minCardinality rdf:datatype="http://www.w3.org/2001/XMLSchema#nonNegativeInteger">0</owl:minCardinality>
               </owl:Restriction>
            </owl:intersectionOf>
         </owl:Class>
      </rdfs:subClassOf>
   </owl:Class>
   <owl:Class rdf:about="http://www.opengis.net/gml#AbstractSolidType">
      <rdfs:comment>An abstraction of a solid to support the different levels of complexity. A solid is always contiguous.</rdfs:comment>
      <rdfs:subClassOf rdf:resource="http://www.opengis.net/gml#AbstractGeometricPrimitiveType"/>
   </owl:Class>
   <owl:Class rdf:about="http://www.opengis.net/gml#SolidPropertyType">
      <rdfs:comment>A property that has a solid as its value domain can either be an appropriate geometry element encapsulated in an element of this type or an XLink reference to a remote geometry element (where remote includes geometry elements located elsewhere in the same document). Either the reference or the contained element must be given, but neither both nor none.</rdfs:comment>
      <rdfs:subClassOf>
         <owl:Class>
            <owl:intersectionOf rdf:parseType="Collection">
               <owl:Restriction>
                  <owl:onProperty rdf:resource="http://www.opengis.net/gml#has_Solid"/>
                  <owl:allValuesFrom rdf:resource="http://www.opengis.net/gml#_Solid"/>
               </owl:Restriction>
            </owl:intersectionOf>
         </owl:Class>
      </rdfs:subClassOf>
   </owl:Class>
   <owl:Class rdf:about="http://www.opengis.net/gml#SolidArrayPropertyType">
      <rdfs:comment>A container for an array of solids. The elements are always contained in the array property, referencing geometry elements or arrays of geometry elements is not supported.</rdfs:comment>
      <rdfs:subClassOf>
         <owl:Class>
            <owl:intersectionOf rdf:parseType="Collection">
               <owl:Restriction>
                  <owl:onProperty rdf:resource="http://www.opengis.net/gml#has_Solid"/>
                  <owl:allValuesFrom rdf:resource="http://www.opengis.net/gml#_Solid"/>
               </owl:Restriction>
            </owl:intersectionOf>
         </owl:Class>
      </rdfs:subClassOf>
   </owl:Class>
   <owl:Class rdf:about="http://www.opengis.net/gml#SolidType">
      <rdfs:comment>A solid is the basis for 3-dimensional geometry. The extent of a solid is defined by the boundary surfaces (shells). A shell is represented by a composite surface, where every  shell is used to represent a single connected component of the boundary of a solid. It consists of a composite surface (a list of orientable surfaces) connected in a topological cycle (an object whose boundary is empty). Unlike a Ring, a Shell's elements have no natural sort order. Like Rings, Shells are simple.</rdfs:comment>
      <rdfs:subClassOf>
         <owl:Class>
            <owl:intersectionOf rdf:parseType="Collection">
               <owl:Restriction>
                  <owl:onProperty rdf:resource="http://www.opengis.net/gml#exterior"/>
                  <owl:allValuesFrom rdf:resource="http://www.opengis.net/gml#SurfacePropertyType"/>
               </owl:Restriction>
               <owl:Restriction>
                  <owl:onProperty rdf:resource="http://www.opengis.net/gml#exterior"/>
                  <owl:minCardinality rdf:datatype="http://www.w3.org/2001/XMLSchema#nonNegativeInteger">0</owl:minCardinality>
               </owl:Restriction>
               <owl:Restriction>
                  <owl:onProperty rdf:resource="http://www.opengis.net/gml#interior"/>
                  <owl:allValuesFrom rdf:resource="http://www.opengis.net/gml#SurfacePropertyType"/>
               </owl:Restriction>
               <owl:Restriction>
                  <owl:onProperty rdf:resource="http://www.opengis.net/gml#interior"/>
                  <owl:minCardinality rdf:datatype="http://www.w3.org/2001/XMLSchema#nonNegativeInteger">0</owl:minCardinality>
               </owl:Restriction>
            </owl:intersectionOf>
         </owl:Class>
      </rdfs:subClassOf>
      <rdfs:subClassOf rdf:resource="http://www.opengis.net/gml#AbstractSolidType"/>
   </owl:Class>
   <owl:Class rdf:about="http://www.opengis.net/gml#AbstractCoverageType">
      <rdfs:comment>This is an abstract class</rdfs:comment>
      <rdfs:comment>Abstract element which acts as the head of a substitution group for coverages. Note that a coverage is a GML feature.</rdfs:comment>
      <rdfs:subClassOf>
         <owl:Class>
            <owl:intersectionOf rdf:parseType="Collection">
               <owl:Restriction>
                  <owl:onProperty rdf:resource="http://www.opengis.net/gml#hasdomainSet"/>
                  <owl:allValuesFrom rdf:resource="http://www.opengis.net/gml#domainSet"/>
               </owl:Restriction>
               <owl:Restriction>
                  <owl:onProperty rdf:resource="http://www.opengis.net/gml#hasrangeSet"/>
                  <owl:allValuesFrom rdf:resource="http://www.opengis.net/gml#rangeSet"/>
               </owl:Restriction>
            </owl:intersectionOf>
         </owl:Class>
      </rdfs:subClassOf>
      <rdfs:subClassOf>
         <owl:Class>
            <owl:intersectionOf rdf:parseType="Collection">
               <owl:Restriction>
                  <owl:onProperty rdf:resource="http://www.opengis.net/gml#dimension"/>
                  <owl:allValuesFrom rdf:resource="http://www.w3.org/2001/XMLSchema#positiveInteger"/>
               </owl:Restriction>
            </owl:intersectionOf>
         </owl:Class>
      </rdfs:subClassOf>
      <rdfs:subClassOf rdf:resource="http://www.opengis.net/gml#AbstractFeatureType"/>
   </owl:Class>
   <owl:Class rdf:about="http://www.opengis.net/gml#AbstractContinuousCoverageType">
      <rdfs:comment>This is an abstract class</rdfs:comment>
      <rdfs:comment>A continuous coverage as defined in ISO 19123 is a coverage that can return different values for the same feature attribute at different direct positions within a single spatiotemporal object in its spatiotemporal domain</rdfs:comment>
      <rdfs:subClassOf>
         <owl:Class>
            <owl:intersectionOf rdf:parseType="Collection">
               <owl:Restriction>
                  <owl:onProperty rdf:resource="http://www.opengis.net/gml#hascoverageFunction"/>
                  <owl:allValuesFrom rdf:resource="http://www.opengis.net/gml#coverageFunction"/>
               </owl:Restriction>
               <owl:Restriction>
                  <owl:onProperty rdf:resource="http://www.opengis.net/gml#hascoverageFunction"/>
                  <owl:minCardinality rdf:datatype="http://www.w3.org/2001/XMLSchema#nonNegativeInteger">0</owl:minCardinality>
               </owl:Restriction>
            </owl:intersectionOf>
         </owl:Class>
      </rdfs:subClassOf>
      <rdfs:subClassOf rdf:resource="http://www.opengis.net/gml#AbstractCoverageType"/>
   </owl:Class>
   <owl:Class rdf:about="http://www.opengis.net/gml#AbstractDiscreteCoverageType">
      <rdfs:comment>This is an abstract class</rdfs:comment>
      <rdfs:comment>A discrete coverage consists of a domain set, range set and optionally a coverage function. The domain set consists of either geometry or temporal objects, finite in number. The range set is comprised of a finite number of attribute values each of which is associated to every direct position within any single spatiotemporal object in the domain. In other words, the range values are constant on each spatiotemporal object in the domain. This coverage function maps each element from the coverage domain to an element in its range. This definition conforms to ISO 19123.</rdfs:comment>
      <rdfs:subClassOf>
         <owl:Class>
            <owl:intersectionOf rdf:parseType="Collection">
               <owl:Restriction>
                  <owl:onProperty rdf:resource="http://www.opengis.net/gml#hascoverageFunction"/>
                  <owl:allValuesFrom rdf:resource="http://www.opengis.net/gml#coverageFunction"/>
               </owl:Restriction>
               <owl:Restriction>
                  <owl:onProperty rdf:resource="http://www.opengis.net/gml#hascoverageFunction"/>
                  <owl:minCardinality rdf:datatype="http://www.w3.org/2001/XMLSchema#nonNegativeInteger">0</owl:minCardinality>
               </owl:Restriction>
            </owl:intersectionOf>
         </owl:Class>
      </rdfs:subClassOf>
      <rdfs:subClassOf rdf:resource="http://www.opengis.net/gml#AbstractCoverageType"/>
   </owl:Class>
   <owl:Class rdf:about="http://www.opengis.net/gml#DomainSetType">
      <rdfs:comment>The spatiotemporal domain of a coverage.  
  Typically 
  * a geometry collection, 
  * an implicit geometry (e.g. a grid), 
  * an explicit or implicit collection of time instances or periods, or

N.B. Temporal geometric complexes and temporal grids are not yet implemented in GML.</rdfs:comment>
      <owl:disjointUnionOf rdf:parseType="Collection">
         <owl:Restriction>
            <owl:onProperty rdf:resource="http://www.opengis.net/gml#has_Geometry"/>
            <owl:someValuesFrom rdf:resource="http://www.opengis.net/gml#_Geometry"/>
         </owl:Restriction>
         <owl:Restriction>
            <owl:onProperty rdf:resource="http://www.opengis.net/gml#has_TimeObject"/>
            <owl:someValuesFrom rdf:resource="http://www.opengis.net/gml#_TimeObject"/>
         </owl:Restriction>
      </owl:disjointUnionOf>
   </owl:Class>
   <owl:Class rdf:about="http://www.opengis.net/gml#RangeSetType">
      <owl:disjointUnionOf rdf:parseType="Collection">
         <owl:Restriction>
            <owl:onProperty rdf:resource="http://www.opengis.net/gml#hasValueArray"/>
            <owl:someValuesFrom rdf:resource="http://www.opengis.net/gml#ValueArray"/>
         </owl:Restriction>
         <owl:Restriction>
            <owl:onProperty rdf:resource="http://www.opengis.net/gml#hasDataBlock"/>
            <owl:someValuesFrom rdf:resource="http://www.opengis.net/gml#DataBlock"/>
         </owl:Restriction>
         <owl:Restriction>
            <owl:onProperty rdf:resource="http://www.opengis.net/gml#hasFile"/>
            <owl:someValuesFrom rdf:resource="http://www.opengis.net/gml#File"/>
         </owl:Restriction>
         <owl:Restriction>
            <owl:onProperty rdf:resource="http://www.opengis.net/gml#hasScalarValueList"/>
            <owl:allValuesFrom rdf:resource="http://www.opengis.net/gml#ScalarValueList"/>
         </owl:Restriction>
      </owl:disjointUnionOf>
   </owl:Class>
   <owl:Class rdf:about="http://www.opengis.net/gml#CoverageFunctionType">
      <rdfs:comment>The function or rule which defines the map from members of the domainSet to the range.  
      More functions will be added to this list</rdfs:comment>
      <owl:disjointUnionOf rdf:parseType="Collection">
         <owl:Restriction>
            <owl:onProperty rdf:resource="http://www.opengis.net/gml#hasMappingRule"/>
            <owl:someValuesFrom rdf:resource="http://www.opengis.net/gml#MappingRule"/>
         </owl:Restriction>
         <owl:Restriction>
            <owl:onProperty rdf:resource="http://www.opengis.net/gml#hasGridFunction"/>
            <owl:someValuesFrom rdf:resource="http://www.opengis.net/gml#GridFunction"/>
         </owl:Restriction>
      </owl:disjointUnionOf>
   </owl:Class>
   <owl:Class rdf:about="http://www.opengis.net/gml#DataBlockType">
      <rdfs:subClassOf>
         <owl:Class>
            <owl:intersectionOf rdf:parseType="Collection">
               <owl:Restriction>
                  <owl:onProperty rdf:resource="http://www.opengis.net/gml#hasrangeParameters"/>
                  <owl:allValuesFrom rdf:resource="http://www.opengis.net/gml#rangeParameters"/>
               </owl:Restriction>
            </owl:intersectionOf>
         </owl:Class>
      </rdfs:subClassOf>
      <owl:disjointUnionOf rdf:parseType="Collection">
         <owl:Restriction>
            <owl:onProperty rdf:resource="http://www.opengis.net/gml#hastupleList"/>
            <owl:someValuesFrom rdf:resource="http://www.opengis.net/gml#tupleList"/>
         </owl:Restriction>
         <owl:Restriction>
            <owl:onProperty rdf:resource="http://www.opengis.net/gml#hasdoubleOrNullTupleList"/>
            <owl:someValuesFrom rdf:resource="http://www.opengis.net/gml#doubleOrNullTupleList"/>
         </owl:Restriction>
      </owl:disjointUnionOf>
   </owl:Class>
   <owl:Class rdf:about="http://www.opengis.net/gml#FileType">
      <rdfs:subClassOf>
         <owl:Class>
            <owl:intersectionOf rdf:parseType="Collection">
               <owl:Restriction>
                  <owl:onProperty rdf:resource="http://www.opengis.net/gml#hasrangeParameters"/>
                  <owl:allValuesFrom rdf:resource="http://www.opengis.net/gml#rangeParameters"/>
               </owl:Restriction>
               <owl:Restriction>
                  <owl:onProperty rdf:resource="http://www.opengis.net/gml#fileName"/>
                  <owl:allValuesFrom rdf:resource="http://www.w3.org/2001/XMLSchema#anyURI"/>
               </owl:Restriction>
               <owl:Restriction>
                  <owl:onProperty rdf:resource="http://www.opengis.net/gml#fileStructure"/>
                  <owl:allValuesFrom rdf:resource="http://www.opengis.net/gml#FileValueModelType"/>
               </owl:Restriction>
               <owl:Restriction>
                  <owl:onProperty rdf:resource="http://www.opengis.net/gml#mimeType"/>
                  <owl:allValuesFrom rdf:resource="http://www.w3.org/2001/XMLSchema#anyURI"/>
               </owl:Restriction>
               <owl:Restriction>
                  <owl:onProperty rdf:resource="http://www.opengis.net/gml#mimeType"/>
                  <owl:minCardinality rdf:datatype="http://www.w3.org/2001/XMLSchema#nonNegativeInteger">0</owl:minCardinality>
               </owl:Restriction>
               <owl:Restriction>
                  <owl:onProperty rdf:resource="http://www.opengis.net/gml#compression"/>
                  <owl:allValuesFrom rdf:resource="http://www.w3.org/2001/XMLSchema#anyURI"/>
               </owl:Restriction>
               <owl:Restriction>
                  <owl:onProperty rdf:resource="http://www.opengis.net/gml#compression"/>
                  <owl:minCardinality rdf:datatype="http://www.w3.org/2001/XMLSchema#nonNegativeInteger">0</owl:minCardinality>
               </owl:Restriction>
            </owl:intersectionOf>
         </owl:Class>
      </rdfs:subClassOf>
   </owl:Class>
   <owl:Class rdf:about="http://www.opengis.net/gml#RangeParametersType">
      <rdfs:comment>Metadata about the rangeSet.  Definition of record structure.   
      This is required if the rangeSet is encoded in a DataBlock.  
      We use a gml:_Value with empty values as a map of the composite value structure.</rdfs:comment>
      <rdfs:subClassOf rdf:resource="http://www.opengis.net/gml#ValueObject"/>
   </owl:Class>
   <owl:Class rdf:about="http://www.opengis.net/gml#GridFunctionType">
      <rdfs:comment>Defines how values in the domain are mapped to the range set. The start point and the sequencing rule are specified here.</rdfs:comment>
      <rdfs:subClassOf>
         <owl:Class>
            <owl:intersectionOf rdf:parseType="Collection">
               <owl:Restriction>
                  <owl:onProperty rdf:resource="http://www.opengis.net/gml#sequenceRule"/>
                  <owl:allValuesFrom rdf:resource="http://www.opengis.net/gml#SequenceRuleType"/>
               </owl:Restriction>
               <owl:Restriction>
                  <owl:onProperty rdf:resource="http://www.opengis.net/gml#sequenceRule"/>
                  <owl:minCardinality rdf:datatype="http://www.w3.org/2001/XMLSchema#nonNegativeInteger">0</owl:minCardinality>
               </owl:Restriction>
               <owl:Restriction>
                  <owl:onProperty rdf:resource="http://www.opengis.net/gml#startPoint"/>
                  <owl:allValuesFrom rdf:resource="http://www.opengis.net/gml#integerList"/>
               </owl:Restriction>
               <owl:Restriction>
                  <owl:onProperty rdf:resource="http://www.opengis.net/gml#startPoint"/>
                  <owl:minCardinality rdf:datatype="http://www.w3.org/2001/XMLSchema#nonNegativeInteger">0</owl:minCardinality>
               </owl:Restriction>
            </owl:intersectionOf>
         </owl:Class>
      </rdfs:subClassOf>
   </owl:Class>
   <owl:Class rdf:about="http://www.opengis.net/gml#IndexMapType">
      <rdfs:comment>Exends GridFunctionType with a lookUpTable.  This contains a list of indexes of members within the rangeSet corresponding with the members of the domainSet.  The domainSet is traversed in list order if it is enumerated explicitly, or in the order specified by a SequenceRule if the domain is an implicit set.    The length of the lookUpTable corresponds with the length of the subset of the domainSet for which the coverage is defined.</rdfs:comment>
      <rdfs:subClassOf>
         <owl:Class>
            <owl:intersectionOf rdf:parseType="Collection">
               <owl:Restriction>
                  <owl:onProperty rdf:resource="http://www.opengis.net/gml#lookUpTable"/>
                  <owl:allValuesFrom rdf:resource="http://www.opengis.net/gml#integerList"/>
               </owl:Restriction>
            </owl:intersectionOf>
         </owl:Class>
      </rdfs:subClassOf>
      <rdfs:subClassOf rdf:resource="http://www.opengis.net/gml#GridFunctionType"/>
   </owl:Class>
   <owl:Class rdf:about="http://www.opengis.net/gml#SequenceRuleType">
      <rdfs:subClassOf>
         <owl:Class>
            <owl:intersectionOf rdf:parseType="Collection">
               <owl:Restriction>
                  <owl:onProperty rdf:resource="http://www.opengis.net/gml#order"/>
                  <owl:allValuesFrom rdf:resource="http://www.opengis.net/gml#IncrementOrder"/>
               </owl:Restriction>
            </owl:intersectionOf>
         </owl:Class>
      </rdfs:subClassOf>
      <rdfs:subClassOf>
         <owl:Restriction>
            <owl:onProperty rdf:resource="http://www.opengis.net/gml#hasSequenceRuleNames"/>
            <owl:someValuesFrom rdf:resource="SequenceRuleNames"/>
         </owl:Restriction>
      </rdfs:subClassOf>
   </owl:Class>
   <owl:DatatypeProperty rdf:about="http://www.opengis.net/gml#hasSequenceRuleNames">
      <rdfs:domain rdf:resource="http://www.opengis.net/gml#SequenceRuleType"/>
      <rdfs:range rdf:resource="http://www.opengis.net/gml#SequenceRuleNames"/>
   </owl:DatatypeProperty>
   <owl:Class rdf:about="http://www.opengis.net/gml#MultiPointCoverageType">
      <rdfs:comment>A discrete coverage type whose domain is defined by a collection of point</rdfs:comment>
      <rdfs:subClassOf>
         <owl:Class>
            <owl:intersectionOf rdf:parseType="Collection">
               <owl:Restriction>
                  <owl:onProperty rdf:resource="http://www.opengis.net/gml#hasboundedBy"/>
                  <owl:allValuesFrom rdf:resource="http://www.opengis.net/gml#boundedBy"/>
               </owl:Restriction>
               <owl:Restriction>
                  <owl:onProperty rdf:resource="http://www.opengis.net/gml#hasboundedBy"/>
                  <owl:minCardinality rdf:datatype="http://www.w3.org/2001/XMLSchema#nonNegativeInteger">0</owl:minCardinality>
               </owl:Restriction>
               <owl:Restriction>
                  <owl:onProperty rdf:resource="http://www.opengis.net/gml#hasmultiPointDomain"/>
                  <owl:allValuesFrom rdf:resource="http://www.opengis.net/gml#multiPointDomain"/>
               </owl:Restriction>
               <owl:Restriction>
                  <owl:onProperty rdf:resource="http://www.opengis.net/gml#hasrangeSet"/>
                  <owl:allValuesFrom rdf:resource="http://www.opengis.net/gml#rangeSet"/>
               </owl:Restriction>
               <owl:Restriction>
                  <owl:onProperty rdf:resource="http://www.opengis.net/gml#hascoverageFunction"/>
                  <owl:allValuesFrom rdf:resource="http://www.opengis.net/gml#coverageFunction"/>
               </owl:Restriction>
               <owl:Restriction>
                  <owl:onProperty rdf:resource="http://www.opengis.net/gml#hascoverageFunction"/>
                  <owl:minCardinality rdf:datatype="http://www.w3.org/2001/XMLSchema#nonNegativeInteger">0</owl:minCardinality>
               </owl:Restriction>
            </owl:intersectionOf>
         </owl:Class>
      </rdfs:subClassOf>
      <rdfs:subClassOf rdf:resource="http://www.opengis.net/gml#StandardObjectProperties"/>
      <rdfs:subClassOf rdf:resource="http://www.opengis.net/gml#AbstractDiscreteCoverageType"/>
   </owl:Class>
   <owl:Class rdf:about="http://www.opengis.net/gml#MultiPointDomainType">
      <rdfs:subClassOf>
         <owl:Class>
            <owl:intersectionOf rdf:parseType="Collection">
               <owl:Restriction>
                  <owl:onProperty rdf:resource="http://www.opengis.net/gml#hasMultiPoint"/>
                  <owl:allValuesFrom rdf:resource="http://www.opengis.net/gml#MultiPoint"/>
               </owl:Restriction>
            </owl:intersectionOf>
         </owl:Class>
      </rdfs:subClassOf>
      <rdfs:subClassOf rdf:resource="http://www.opengis.net/gml#DomainSetType"/>
   </owl:Class>
   <owl:Class rdf:about="http://www.opengis.net/gml#MultiCurveCoverageType">
      <rdfs:comment>A discrete coverage type whose domain is defined by a collection of curves.</rdfs:comment>
      <rdfs:subClassOf>
         <owl:Class>
            <owl:intersectionOf rdf:parseType="Collection">
               <owl:Restriction>
                  <owl:onProperty rdf:resource="http://www.opengis.net/gml#hasboundedBy"/>
                  <owl:allValuesFrom rdf:resource="http://www.opengis.net/gml#boundedBy"/>
               </owl:Restriction>
               <owl:Restriction>
                  <owl:onProperty rdf:resource="http://www.opengis.net/gml#hasboundedBy"/>
                  <owl:minCardinality rdf:datatype="http://www.w3.org/2001/XMLSchema#nonNegativeInteger">0</owl:minCardinality>
               </owl:Restriction>
               <owl:Restriction>
                  <owl:onProperty rdf:resource="http://www.opengis.net/gml#hasmultiCurveDomain"/>
                  <owl:allValuesFrom rdf:resource="http://www.opengis.net/gml#multiCurveDomain"/>
               </owl:Restriction>
               <owl:Restriction>
                  <owl:onProperty rdf:resource="http://www.opengis.net/gml#hasrangeSet"/>
                  <owl:allValuesFrom rdf:resource="http://www.opengis.net/gml#rangeSet"/>
               </owl:Restriction>
               <owl:Restriction>
                  <owl:onProperty rdf:resource="http://www.opengis.net/gml#hascoverageFunction"/>
                  <owl:allValuesFrom rdf:resource="http://www.opengis.net/gml#coverageFunction"/>
               </owl:Restriction>
               <owl:Restriction>
                  <owl:onProperty rdf:resource="http://www.opengis.net/gml#hascoverageFunction"/>
                  <owl:minCardinality rdf:datatype="http://www.w3.org/2001/XMLSchema#nonNegativeInteger">0</owl:minCardinality>
               </owl:Restriction>
            </owl:intersectionOf>
         </owl:Class>
      </rdfs:subClassOf>
      <rdfs:subClassOf rdf:resource="http://www.opengis.net/gml#StandardObjectProperties"/>
      <rdfs:subClassOf rdf:resource="http://www.opengis.net/gml#AbstractDiscreteCoverageType"/>
   </owl:Class>
   <owl:Class rdf:about="http://www.opengis.net/gml#MultiCurveDomainType">
      <rdfs:subClassOf>
         <owl:Class>
            <owl:intersectionOf rdf:parseType="Collection">
               <owl:Restriction>
                  <owl:onProperty rdf:resource="http://www.opengis.net/gml#hasMultiCurve"/>
                  <owl:allValuesFrom rdf:resource="http://www.opengis.net/gml#MultiCurve"/>
               </owl:Restriction>
            </owl:intersectionOf>
         </owl:Class>
      </rdfs:subClassOf>
      <rdfs:subClassOf rdf:resource="http://www.opengis.net/gml#DomainSetType"/>
   </owl:Class>
   <owl:Class rdf:about="http://www.opengis.net/gml#MultiSurfaceCoverageType">
      <rdfs:comment>A discrete coverage type whose domain is defined by a collection of surface patches (includes polygons, triangles, rectangles, etc).</rdfs:comment>
      <rdfs:subClassOf>
         <owl:Class>
            <owl:intersectionOf rdf:parseType="Collection">
               <owl:Restriction>
                  <owl:onProperty rdf:resource="http://www.opengis.net/gml#hasboundedBy"/>
                  <owl:allValuesFrom rdf:resource="http://www.opengis.net/gml#boundedBy"/>
               </owl:Restriction>
               <owl:Restriction>
                  <owl:onProperty rdf:resource="http://www.opengis.net/gml#hasboundedBy"/>
                  <owl:minCardinality rdf:datatype="http://www.w3.org/2001/XMLSchema#nonNegativeInteger">0</owl:minCardinality>
               </owl:Restriction>
               <owl:Restriction>
                  <owl:onProperty rdf:resource="http://www.opengis.net/gml#hasmultiSurfaceDomain"/>
                  <owl:allValuesFrom rdf:resource="http://www.opengis.net/gml#multiSurfaceDomain"/>
               </owl:Restriction>
               <owl:Restriction>
                  <owl:onProperty rdf:resource="http://www.opengis.net/gml#hasrangeSet"/>
                  <owl:allValuesFrom rdf:resource="http://www.opengis.net/gml#rangeSet"/>
               </owl:Restriction>
               <owl:Restriction>
                  <owl:onProperty rdf:resource="http://www.opengis.net/gml#hascoverageFunction"/>
                  <owl:allValuesFrom rdf:resource="http://www.opengis.net/gml#coverageFunction"/>
               </owl:Restriction>
               <owl:Restriction>
                  <owl:onProperty rdf:resource="http://www.opengis.net/gml#hascoverageFunction"/>
                  <owl:minCardinality rdf:datatype="http://www.w3.org/2001/XMLSchema#nonNegativeInteger">0</owl:minCardinality>
               </owl:Restriction>
            </owl:intersectionOf>
         </owl:Class>
      </rdfs:subClassOf>
      <rdfs:subClassOf rdf:resource="http://www.opengis.net/gml#StandardObjectProperties"/>
      <rdfs:subClassOf rdf:resource="http://www.opengis.net/gml#AbstractDiscreteCoverageType"/>
   </owl:Class>
   <owl:Class rdf:about="http://www.opengis.net/gml#MultiSurfaceDomainType">
      <rdfs:subClassOf>
         <owl:Class>
            <owl:intersectionOf rdf:parseType="Collection">
               <owl:Restriction>
                  <owl:onProperty rdf:resource="http://www.opengis.net/gml#hasMultiSurface"/>
                  <owl:allValuesFrom rdf:resource="http://www.opengis.net/gml#MultiSurface"/>
               </owl:Restriction>
            </owl:intersectionOf>
         </owl:Class>
      </rdfs:subClassOf>
      <rdfs:subClassOf rdf:resource="http://www.opengis.net/gml#DomainSetType"/>
   </owl:Class>
   <owl:Class rdf:about="http://www.opengis.net/gml#MultiSolidCoverageType">
      <rdfs:comment>A discrete coverage type whose domain is defined by a collection of Solids.</rdfs:comment>
      <rdfs:subClassOf>
         <owl:Class>
            <owl:intersectionOf rdf:parseType="Collection">
               <owl:Restriction>
                  <owl:onProperty rdf:resource="http://www.opengis.net/gml#hasboundedBy"/>
                  <owl:allValuesFrom rdf:resource="http://www.opengis.net/gml#boundedBy"/>
               </owl:Restriction>
               <owl:Restriction>
                  <owl:onProperty rdf:resource="http://www.opengis.net/gml#hasboundedBy"/>
                  <owl:minCardinality rdf:datatype="http://www.w3.org/2001/XMLSchema#nonNegativeInteger">0</owl:minCardinality>
               </owl:Restriction>
               <owl:Restriction>
                  <owl:onProperty rdf:resource="http://www.opengis.net/gml#hasmultiSolidDomain"/>
                  <owl:allValuesFrom rdf:resource="http://www.opengis.net/gml#multiSolidDomain"/>
               </owl:Restriction>
               <owl:Restriction>
                  <owl:onProperty rdf:resource="http://www.opengis.net/gml#hasrangeSet"/>
                  <owl:allValuesFrom rdf:resource="http://www.opengis.net/gml#rangeSet"/>
               </owl:Restriction>
               <owl:Restriction>
                  <owl:onProperty rdf:resource="http://www.opengis.net/gml#hascoverageFunction"/>
                  <owl:allValuesFrom rdf:resource="http://www.opengis.net/gml#coverageFunction"/>
               </owl:Restriction>
               <owl:Restriction>
                  <owl:onProperty rdf:resource="http://www.opengis.net/gml#hascoverageFunction"/>
                  <owl:minCardinality rdf:datatype="http://www.w3.org/2001/XMLSchema#nonNegativeInteger">0</owl:minCardinality>
               </owl:Restriction>
            </owl:intersectionOf>
         </owl:Class>
      </rdfs:subClassOf>
      <rdfs:subClassOf rdf:resource="http://www.opengis.net/gml#StandardObjectProperties"/>
      <rdfs:subClassOf rdf:resource="http://www.opengis.net/gml#AbstractDiscreteCoverageType"/>
   </owl:Class>
   <owl:Class rdf:about="http://www.opengis.net/gml#MultiSolidDomainType">
      <rdfs:subClassOf>
         <owl:Class>
            <owl:intersectionOf rdf:parseType="Collection">
               <owl:Restriction>
                  <owl:onProperty rdf:resource="http://www.opengis.net/gml#hasMultiSolid"/>
                  <owl:allValuesFrom rdf:resource="http://www.opengis.net/gml#MultiSolid"/>
               </owl:Restriction>
            </owl:intersectionOf>
         </owl:Class>
      </rdfs:subClassOf>
      <rdfs:subClassOf rdf:resource="http://www.opengis.net/gml#DomainSetType"/>
   </owl:Class>
   <owl:Class rdf:about="http://www.opengis.net/gml#GridCoverageType">
      <rdfs:subClassOf>
         <owl:Class>
            <owl:intersectionOf rdf:parseType="Collection">
               <owl:Restriction>
                  <owl:onProperty rdf:resource="http://www.opengis.net/gml#hasboundedBy"/>
                  <owl:allValuesFrom rdf:resource="http://www.opengis.net/gml#boundedBy"/>
               </owl:Restriction>
               <owl:Restriction>
                  <owl:onProperty rdf:resource="http://www.opengis.net/gml#hasboundedBy"/>
                  <owl:minCardinality rdf:datatype="http://www.w3.org/2001/XMLSchema#nonNegativeInteger">0</owl:minCardinality>
               </owl:Restriction>
               <owl:Restriction>
                  <owl:onProperty rdf:resource="http://www.opengis.net/gml#hasgridDomain"/>
                  <owl:allValuesFrom rdf:resource="http://www.opengis.net/gml#gridDomain"/>
               </owl:Restriction>
               <owl:Restriction>
                  <owl:onProperty rdf:resource="http://www.opengis.net/gml#hasrangeSet"/>
                  <owl:allValuesFrom rdf:resource="http://www.opengis.net/gml#rangeSet"/>
               </owl:Restriction>
               <owl:Restriction>
                  <owl:onProperty rdf:resource="http://www.opengis.net/gml#hascoverageFunction"/>
                  <owl:allValuesFrom rdf:resource="http://www.opengis.net/gml#coverageFunction"/>
               </owl:Restriction>
               <owl:Restriction>
                  <owl:onProperty rdf:resource="http://www.opengis.net/gml#hascoverageFunction"/>
                  <owl:minCardinality rdf:datatype="http://www.w3.org/2001/XMLSchema#nonNegativeInteger">0</owl:minCardinality>
               </owl:Restriction>
            </owl:intersectionOf>
         </owl:Class>
      </rdfs:subClassOf>
      <rdfs:subClassOf rdf:resource="http://www.opengis.net/gml#StandardObjectProperties"/>
      <rdfs:subClassOf rdf:resource="http://www.opengis.net/gml#AbstractDiscreteCoverageType"/>
   </owl:Class>
   <owl:Class rdf:about="http://www.opengis.net/gml#GridDomainType">
      <rdfs:subClassOf>
         <owl:Class>
            <owl:intersectionOf rdf:parseType="Collection">
               <owl:Restriction>
                  <owl:onProperty rdf:resource="http://www.opengis.net/gml#hasGrid"/>
                  <owl:allValuesFrom rdf:resource="http://www.opengis.net/gml#Grid"/>
               </owl:Restriction>
            </owl:intersectionOf>
         </owl:Class>
      </rdfs:subClassOf>
      <rdfs:subClassOf rdf:resource="http://www.opengis.net/gml#DomainSetType"/>
   </owl:Class>
   <owl:Class rdf:about="http://www.opengis.net/gml#RectifiedGridCoverageType">
      <rdfs:subClassOf>
         <owl:Class>
            <owl:intersectionOf rdf:parseType="Collection">
               <owl:Restriction>
                  <owl:onProperty rdf:resource="http://www.opengis.net/gml#hasboundedBy"/>
                  <owl:allValuesFrom rdf:resource="http://www.opengis.net/gml#boundedBy"/>
               </owl:Restriction>
               <owl:Restriction>
                  <owl:onProperty rdf:resource="http://www.opengis.net/gml#hasboundedBy"/>
                  <owl:minCardinality rdf:datatype="http://www.w3.org/2001/XMLSchema#nonNegativeInteger">0</owl:minCardinality>
               </owl:Restriction>
               <owl:Restriction>
                  <owl:onProperty rdf:resource="http://www.opengis.net/gml#hasrectifiedGridDomain"/>
                  <owl:allValuesFrom rdf:resource="http://www.opengis.net/gml#rectifiedGridDomain"/>
               </owl:Restriction>
               <owl:Restriction>
                  <owl:onProperty rdf:resource="http://www.opengis.net/gml#hasrangeSet"/>
                  <owl:allValuesFrom rdf:resource="http://www.opengis.net/gml#rangeSet"/>
               </owl:Restriction>
               <owl:Restriction>
                  <owl:onProperty rdf:resource="http://www.opengis.net/gml#hascoverageFunction"/>
                  <owl:allValuesFrom rdf:resource="http://www.opengis.net/gml#coverageFunction"/>
               </owl:Restriction>
               <owl:Restriction>
                  <owl:onProperty rdf:resource="http://www.opengis.net/gml#hascoverageFunction"/>
                  <owl:minCardinality rdf:datatype="http://www.w3.org/2001/XMLSchema#nonNegativeInteger">0</owl:minCardinality>
               </owl:Restriction>
            </owl:intersectionOf>
         </owl:Class>
      </rdfs:subClassOf>
      <rdfs:subClassOf rdf:resource="http://www.opengis.net/gml#StandardObjectProperties"/>
      <rdfs:subClassOf rdf:resource="http://www.opengis.net/gml#AbstractDiscreteCoverageType"/>
   </owl:Class>
   <owl:Class rdf:about="http://www.opengis.net/gml#RectifiedGridDomainType">
      <rdfs:subClassOf>
         <owl:Class>
            <owl:intersectionOf rdf:parseType="Collection">
               <owl:Restriction>
                  <owl:onProperty rdf:resource="http://www.opengis.net/gml#hasRectifiedGrid"/>
                  <owl:allValuesFrom rdf:resource="http://www.opengis.net/gml#RectifiedGrid"/>
               </owl:Restriction>
            </owl:intersectionOf>
         </owl:Class>
      </rdfs:subClassOf>
      <rdfs:subClassOf rdf:resource="http://www.opengis.net/gml#DomainSetType"/>
   </owl:Class>
   <owl:Class rdf:about="http://www.opengis.net/gml#CompositeValueType">
      <rdfs:comment>Aggregate value built from other Values using the Composite pattern. It contains zero or an arbitrary number of valueComponent elements, and zero or one valueComponents elements.  It may be used for strongly coupled aggregates (vectors, tensors) or for arbitrary collections of values.</rdfs:comment>
      <rdfs:subClassOf>
         <owl:Class>
            <owl:intersectionOf rdf:parseType="Collection">
               <owl:Restriction>
                  <owl:onProperty rdf:resource="http://www.opengis.net/gml#hasvalueComponent"/>
                  <owl:allValuesFrom rdf:resource="http://www.opengis.net/gml#valueComponent"/>
               </owl:Restriction>
               <owl:Restriction>
                  <owl:onProperty rdf:resource="http://www.opengis.net/gml#hasvalueComponent"/>
                  <owl:minCardinality rdf:datatype="http://www.w3.org/2001/XMLSchema#nonNegativeInteger">0</owl:minCardinality>
               </owl:Restriction>
               <owl:Restriction>
                  <owl:onProperty rdf:resource="http://www.opengis.net/gml#hasvalueComponents"/>
                  <owl:allValuesFrom rdf:resource="http://www.opengis.net/gml#valueComponents"/>
               </owl:Restriction>
               <owl:Restriction>
                  <owl:onProperty rdf:resource="http://www.opengis.net/gml#hasvalueComponents"/>
                  <owl:minCardinality rdf:datatype="http://www.w3.org/2001/XMLSchema#nonNegativeInteger">0</owl:minCardinality>
               </owl:Restriction>
            </owl:intersectionOf>
         </owl:Class>
      </rdfs:subClassOf>
      <rdfs:subClassOf rdf:resource="http://www.opengis.net/gml#AbstractGMLType"/>
   </owl:Class>
   <owl:Class rdf:about="http://www.opengis.net/gml#ValueArrayType">
      <rdfs:comment>A Value Array is used for homogeneous arrays of primitive and aggregate values.  The member values may be scalars, composites, arrays or lists.  ValueArray has the same content model as CompositeValue, but the member values must be homogeneous.  The element declaration contains a Schematron constraint which expresses this restriction precisely.            Since the members are homogeneous, the referenceSystem (uom, codeSpace) may be specified on the ValueArray itself and implicitly inherited by all the members if desired.    Note that a_ScalarValueList is preferred for arrays of Scalar Values since this is a more efficient encoding.</rdfs:comment>
      <rdfs:subClassOf rdf:resource="http://www.opengis.net/gml#CompositeValueType"/>
   </owl:Class>
   <owl:Class rdf:about="http://www.opengis.net/gml#QuantityExtentType">
      <rdfs:comment>Restriction of list type to store a 2-point range of numeric values. If one member is a null, then this is a single ended interval.</rdfs:comment>
      <rdfs:subClassOf>
         <owl:Restriction>
            <owl:onProperty rdf:resource="http://www.opengis.net/gml#hasQuantityExtentTypeDatatype"/>
            <owl:someValuesFrom rdf:resource="http://www.opengis.net/gml#QuantityExtentTypeDatatype"/>
         </owl:Restriction>
      </rdfs:subClassOf>
      <rdfs:subClassOf rdf:resource="http://www.opengis.net/gml#MeasureOrNullListType"/>
   </owl:Class>
   <rdfs:Datatype rdf:about="http://www.opengis.net/gml#QuantityExtentTypeDatatype">
      <owl:equivalentClass rdf:resource="http://www.opengis.net/gml#MeasureOrNullListType"/>
   </rdfs:Datatype>
   <owl:DatatypeProperty rdf:about="http://www.opengis.net/gml#hasQuantityExtentTypeDatatype">
      <rdfs:domain rdf:resource="http://www.opengis.net/gml#QuantityExtentType"/>
      <rdfs:range rdf:resource="http://www.opengis.net/gml#QuantityExtentTypeDatatype"/>
   </owl:DatatypeProperty>
   <owl:Class rdf:about="http://www.opengis.net/gml#CategoryExtentType">
      <rdfs:comment>Restriction of list type to store a 2-point range of ordinal values. If one member is a null, then this is a single ended interval.</rdfs:comment>
      <rdfs:subClassOf>
         <owl:Restriction>
            <owl:onProperty rdf:resource="http://www.opengis.net/gml#hasCategoryExtentTypeDatatype"/>
            <owl:someValuesFrom rdf:resource="http://www.opengis.net/gml#CategoryExtentTypeDatatype"/>
         </owl:Restriction>
      </rdfs:subClassOf>
      <rdfs:subClassOf rdf:resource="http://www.opengis.net/gml#CodeOrNullListType"/>
   </owl:Class>
   <rdfs:Datatype rdf:about="http://www.opengis.net/gml#CategoryExtentTypeDatatype">
      <owl:equivalentClass rdf:resource="http://www.opengis.net/gml#CodeOrNullListType"/>
   </rdfs:Datatype>
   <owl:DatatypeProperty rdf:about="http://www.opengis.net/gml#hasCategoryExtentTypeDatatype">
      <rdfs:domain rdf:resource="http://www.opengis.net/gml#CategoryExtentType"/>
      <rdfs:range rdf:resource="http://www.opengis.net/gml#CategoryExtentTypeDatatype"/>
   </owl:DatatypeProperty>
   <owl:Class rdf:about="http://www.opengis.net/gml#ValuePropertyType">
      <rdfs:comment>GML property which refers to, or contains, a Value</rdfs:comment>
      <rdfs:subClassOf rdf:resource="http://www.opengis.net/gml#Value"/>
   </owl:Class>
   <owl:Class rdf:about="http://www.opengis.net/gml#ValueArrayPropertyType">
      <rdfs:comment>GML property which refers to, or contains, a set of homogeneously typed Values.</rdfs:comment>
      <rdfs:subClassOf rdf:resource="http://www.opengis.net/gml#Value"/>
   </owl:Class>
   <owl:Class rdf:about="http://www.opengis.net/gml#ScalarValuePropertyType">
      <rdfs:comment>Property whose content is a scalar value.</rdfs:comment>
      <rdfs:subClassOf rdf:resource="http://www.opengis.net/gml#ScalarValue"/>
      <rdfs:subClassOf rdf:resource="http://www.opengis.net/gml#ValuePropertyType"/>
   </owl:Class>
   <owl:Class rdf:about="http://www.opengis.net/gml#BooleanPropertyType">
      <rdfs:comment>Property whose content is a Boolean value.</rdfs:comment>
      <rdfs:subClassOf>
         <owl:Class>
            <owl:intersectionOf rdf:parseType="Collection">
               <owl:Restriction>
                  <owl:onProperty rdf:resource="http://www.opengis.net/gml#hasBoolean"/>
                  <owl:allValuesFrom rdf:resource="http://www.opengis.net/gml#Boolean"/>
               </owl:Restriction>
            </owl:intersectionOf>
         </owl:Class>
      </rdfs:subClassOf>
      <rdfs:subClassOf rdf:resource="http://www.opengis.net/gml#ValuePropertyType"/>
   </owl:Class>
   <owl:Class rdf:about="http://www.opengis.net/gml#CategoryPropertyType">
      <rdfs:comment>Property whose content is a Category.</rdfs:comment>
      <rdfs:subClassOf>
         <owl:Class>
            <owl:intersectionOf rdf:parseType="Collection">
               <owl:Restriction>
                  <owl:onProperty rdf:resource="http://www.opengis.net/gml#hasCategory"/>
                  <owl:allValuesFrom rdf:resource="http://www.opengis.net/gml#Category"/>
               </owl:Restriction>
            </owl:intersectionOf>
         </owl:Class>
      </rdfs:subClassOf>
      <rdfs:subClassOf rdf:resource="http://www.opengis.net/gml#ValuePropertyType"/>
   </owl:Class>
   <owl:Class rdf:about="http://www.opengis.net/gml#QuantityPropertyType">
      <rdfs:comment>Property whose content is a Quantity.</rdfs:comment>
      <rdfs:subClassOf>
         <owl:Class>
            <owl:intersectionOf rdf:parseType="Collection">
               <owl:Restriction>
                  <owl:onProperty rdf:resource="http://www.opengis.net/gml#hasQuantity"/>
                  <owl:allValuesFrom rdf:resource="http://www.opengis.net/gml#Quantity"/>
               </owl:Restriction>
            </owl:intersectionOf>
         </owl:Class>
      </rdfs:subClassOf>
      <rdfs:subClassOf rdf:resource="http://www.opengis.net/gml#ValuePropertyType"/>
   </owl:Class>
   <owl:Class rdf:about="http://www.opengis.net/gml#CountPropertyType">
      <rdfs:comment>Property whose content is a Count.</rdfs:comment>
      <rdfs:subClassOf>
         <owl:Class>
            <owl:intersectionOf rdf:parseType="Collection">
               <owl:Restriction>
                  <owl:onProperty rdf:resource="http://www.opengis.net/gml#hasCount"/>
                  <owl:allValuesFrom rdf:resource="http://www.opengis.net/gml#Count"/>
               </owl:Restriction>
            </owl:intersectionOf>
         </owl:Class>
      </rdfs:subClassOf>
      <rdfs:subClassOf rdf:resource="http://www.opengis.net/gml#ValuePropertyType"/>
   </owl:Class>
   <owl:Class rdf:about="http://www.opengis.net/gml#GridType">
      <rdfs:comment>An unrectified grid, which is a network composed of two or more sets of equally spaced parallel lines in which the members of each set intersect the members of the other sets at right angles.</rdfs:comment>
      <rdfs:subClassOf>
         <owl:Class>
            <owl:intersectionOf rdf:parseType="Collection">
               <owl:Restriction>
                  <owl:onProperty rdf:resource="http://www.opengis.net/gml#limits"/>
                  <owl:allValuesFrom rdf:resource="http://www.opengis.net/gml#GridLimitsType"/>
               </owl:Restriction>
               <owl:Restriction>
                  <owl:onProperty rdf:resource="http://www.opengis.net/gml#axisName"/>
                  <owl:allValuesFrom rdf:resource="http://www.w3.org/2001/XMLSchema#string"/>
               </owl:Restriction>
            </owl:intersectionOf>
         </owl:Class>
      </rdfs:subClassOf>
      <rdfs:subClassOf>
         <owl:Class>
            <owl:intersectionOf rdf:parseType="Collection">
               <owl:Restriction>
                  <owl:onProperty rdf:resource="http://www.opengis.net/gml#dimension"/>
                  <owl:allValuesFrom rdf:resource="http://www.w3.org/2001/XMLSchema#positiveInteger"/>
               </owl:Restriction>
            </owl:intersectionOf>
         </owl:Class>
      </rdfs:subClassOf>
      <rdfs:subClassOf rdf:resource="http://www.opengis.net/gml#AbstractGeometryType"/>
   </owl:Class>
   <owl:Class rdf:about="http://www.opengis.net/gml#GridLimitsType">
      <rdfs:subClassOf>
         <owl:Class>
            <owl:intersectionOf rdf:parseType="Collection">
               <owl:Restriction>
                  <owl:onProperty rdf:resource="http://www.opengis.net/gml#GridEnvelope"/>
                  <owl:allValuesFrom rdf:resource="http://www.opengis.net/gml#GridEnvelopeType"/>
               </owl:Restriction>
            </owl:intersectionOf>
         </owl:Class>
      </rdfs:subClassOf>
   </owl:Class>
   <owl:Class rdf:about="http://www.opengis.net/gml#GridEnvelopeType">
      <rdfs:comment>Provides grid coordinate values for the diametrically opposed corners of an envelope that bounds a section of grid. The value of a single coordinate is the number of offsets from the origin of the grid in the direction of a specific axis.</rdfs:comment>
      <rdfs:subClassOf>
         <owl:Class>
            <owl:intersectionOf rdf:parseType="Collection">
               <owl:Restriction>
                  <owl:onProperty rdf:resource="http://www.opengis.net/gml#low"/>
                  <owl:allValuesFrom rdf:resource="http://www.opengis.net/gml#integerList"/>
               </owl:Restriction>
               <owl:Restriction>
                  <owl:onProperty rdf:resource="http://www.opengis.net/gml#high"/>
                  <owl:allValuesFrom rdf:resource="http://www.opengis.net/gml#integerList"/>
               </owl:Restriction>
            </owl:intersectionOf>
         </owl:Class>
      </rdfs:subClassOf>
   </owl:Class>
   <owl:Class rdf:about="http://www.opengis.net/gml#RectifiedGridType">
      <rdfs:comment>A rectified grid has an origin and vectors that define its post locations.</rdfs:comment>
      <rdfs:subClassOf>
         <owl:Class>
            <owl:intersectionOf rdf:parseType="Collection">
               <owl:Restriction>
                  <owl:onProperty rdf:resource="http://www.opengis.net/gml#origin"/>
                  <owl:allValuesFrom rdf:resource="http://www.opengis.net/gml#PointPropertyType"/>
               </owl:Restriction>
               <owl:Restriction>
                  <owl:onProperty rdf:resource="http://www.opengis.net/gml#offsetVector"/>
                  <owl:allValuesFrom rdf:resource="http://www.opengis.net/gml#VectorType"/>
               </owl:Restriction>
            </owl:intersectionOf>
         </owl:Class>
      </rdfs:subClassOf>
      <rdfs:subClassOf rdf:resource="http://www.opengis.net/gml#GridType"/>
   </owl:Class>
   <owl:Class rdf:about="http://www.opengis.net/gml#CoordinateReferenceSystemRefType">
      <rdfs:comment>Association to a coordinate reference system, either referencing or containing the definition of that reference system. </rdfs:comment>
      <rdfs:subClassOf>
         <owl:Class>
            <owl:intersectionOf rdf:parseType="Collection">
               <owl:Restriction>
                  <owl:onProperty rdf:resource="http://www.opengis.net/gml#has_CoordinateReferenceSystem"/>
                  <owl:allValuesFrom rdf:resource="http://www.opengis.net/gml#_CoordinateReferenceSystem"/>
               </owl:Restriction>
            </owl:intersectionOf>
         </owl:Class>
      </rdfs:subClassOf>
   </owl:Class>
   <owl:Class rdf:about="http://www.opengis.net/gml#CompoundCRSType">
      <rdfs:comment>A coordinate reference system describing the position of points through two or more independent coordinate reference systems. </rdfs:comment>
      <rdfs:subClassOf>
         <owl:Class>
            <owl:intersectionOf rdf:parseType="Collection">
               <owl:Restriction>
                  <owl:onProperty rdf:resource="http://www.opengis.net/gml#hasincludesCRS"/>
                  <owl:allValuesFrom rdf:resource="http://www.opengis.net/gml#includesCRS"/>
               </owl:Restriction>
               <owl:Restriction>
                  <owl:onProperty rdf:resource="http://www.opengis.net/gml#hasincludesCRS"/>
                  <owl:minCardinality rdf:datatype="http://www.w3.org/2001/XMLSchema#nonNegativeInteger">2</owl:minCardinality>
               </owl:Restriction>
            </owl:intersectionOf>
         </owl:Class>
      </rdfs:subClassOf>
      <rdfs:subClassOf rdf:resource="http://www.opengis.net/gml#AbstractReferenceSystemType"/>
   </owl:Class>
   <owl:Class rdf:about="http://www.opengis.net/gml#CompoundCRSRefType">
      <rdfs:comment>Association to a compound coordinate reference system, either referencing or containing the definition of that reference system. </rdfs:comment>
      <rdfs:subClassOf>
         <owl:Class>
            <owl:intersectionOf rdf:parseType="Collection">
               <owl:Restriction>
                  <owl:onProperty rdf:resource="http://www.opengis.net/gml#hasCompoundCRS"/>
                  <owl:allValuesFrom rdf:resource="http://www.opengis.net/gml#CompoundCRS"/>
               </owl:Restriction>
            </owl:intersectionOf>
         </owl:Class>
      </rdfs:subClassOf>
   </owl:Class>
   <owl:Class rdf:about="http://www.opengis.net/gml#GeographicCRSType">
      <rdfs:comment>A coordinate reference system based on an ellipsoidal approximation of the geoid; this provides an accurate representation of the geometry of geographic features for a large portion of the earth's surface.</rdfs:comment>
      <rdfs:subClassOf>
         <owl:Class>
            <owl:intersectionOf rdf:parseType="Collection">
               <owl:Restriction>
                  <owl:onProperty rdf:resource="http://www.opengis.net/gml#hasusesEllipsoidalCS"/>
                  <owl:allValuesFrom rdf:resource="http://www.opengis.net/gml#usesEllipsoidalCS"/>
               </owl:Restriction>
               <owl:Restriction>
                  <owl:onProperty rdf:resource="http://www.opengis.net/gml#hasusesGeodeticDatum"/>
                  <owl:allValuesFrom rdf:resource="http://www.opengis.net/gml#usesGeodeticDatum"/>
               </owl:Restriction>
            </owl:intersectionOf>
         </owl:Class>
      </rdfs:subClassOf>
      <rdfs:subClassOf rdf:resource="http://www.opengis.net/gml#AbstractReferenceSystemType"/>
   </owl:Class>
   <owl:Class rdf:about="http://www.opengis.net/gml#GeographicCRSRefType">
      <rdfs:comment>Association to a geographic coordinate reference system, either referencing or containing the definition of that reference system. </rdfs:comment>
      <rdfs:subClassOf>
         <owl:Class>
            <owl:intersectionOf rdf:parseType="Collection">
               <owl:Restriction>
                  <owl:onProperty rdf:resource="http://www.opengis.net/gml#hasGeographicCRS"/>
                  <owl:allValuesFrom rdf:resource="http://www.opengis.net/gml#GeographicCRS"/>
               </owl:Restriction>
            </owl:intersectionOf>
         </owl:Class>
      </rdfs:subClassOf>
   </owl:Class>
   <owl:Class rdf:about="http://www.opengis.net/gml#VerticalCRSType">
      <rdfs:comment>A 1D coordinate reference system used for recording heights or depths. Vertical CRSs make use of the direction of gravity to define the concept of height or depth, but the relationship with gravity may not be straightforward. By implication, ellipsoidal heights (h) cannot be captured in a vertical coordinate reference system. Ellipsoidal heights cannot exist independently, but only as an inseparable part of a 3D coordinate tuple defined in a geographic 3D coordinate reference system. </rdfs:comment>
      <rdfs:subClassOf>
         <owl:Class>
            <owl:intersectionOf rdf:parseType="Collection">
               <owl:Restriction>
                  <owl:onProperty rdf:resource="http://www.opengis.net/gml#hasusesVerticalCS"/>
                  <owl:allValuesFrom rdf:resource="http://www.opengis.net/gml#usesVerticalCS"/>
               </owl:Restriction>
               <owl:Restriction>
                  <owl:onProperty rdf:resource="http://www.opengis.net/gml#hasusesVerticalDatum"/>
                  <owl:allValuesFrom rdf:resource="http://www.opengis.net/gml#usesVerticalDatum"/>
               </owl:Restriction>
            </owl:intersectionOf>
         </owl:Class>
      </rdfs:subClassOf>
      <rdfs:subClassOf rdf:resource="http://www.opengis.net/gml#AbstractReferenceSystemType"/>
   </owl:Class>
   <owl:Class rdf:about="http://www.opengis.net/gml#VerticalCRSRefType">
      <rdfs:comment>Association to a vertical coordinate reference system, either referencing or containing the definition of that reference system. </rdfs:comment>
      <rdfs:subClassOf>
         <owl:Class>
            <owl:intersectionOf rdf:parseType="Collection">
               <owl:Restriction>
                  <owl:onProperty rdf:resource="http://www.opengis.net/gml#hasVerticalCRS"/>
                  <owl:allValuesFrom rdf:resource="http://www.opengis.net/gml#VerticalCRS"/>
               </owl:Restriction>
            </owl:intersectionOf>
         </owl:Class>
      </rdfs:subClassOf>
   </owl:Class>
   <owl:Class rdf:about="http://www.opengis.net/gml#GeocentricCRSType">
      <rdfs:comment>A 3D coordinate reference system with the origin at the approximate centre of mass of the earth. A geocentric CRS deals with the earth's curvature by taking a 3D spatial view, which obviates the need to model the earth's curvature. </rdfs:comment>
      <rdfs:subClassOf>
         <owl:Class>
            <owl:intersectionOf rdf:parseType="Collection">
               <owl:Restriction>
                  <owl:onProperty rdf:resource="http://www.opengis.net/gml#hasusesGeodeticDatum"/>
                  <owl:allValuesFrom rdf:resource="http://www.opengis.net/gml#usesGeodeticDatum"/>
               </owl:Restriction>
            </owl:intersectionOf>
         </owl:Class>
      </rdfs:subClassOf>
      <owl:disjointUnionOf rdf:parseType="Collection">
         <owl:Restriction>
            <owl:onProperty rdf:resource="http://www.opengis.net/gml#hasusesCartesianCS"/>
            <owl:someValuesFrom rdf:resource="http://www.opengis.net/gml#usesCartesianCS"/>
         </owl:Restriction>
         <owl:Restriction>
            <owl:onProperty rdf:resource="http://www.opengis.net/gml#hasusesSphericalCS"/>
            <owl:someValuesFrom rdf:resource="http://www.opengis.net/gml#usesSphericalCS"/>
         </owl:Restriction>
      </owl:disjointUnionOf>
      <rdfs:subClassOf rdf:resource="http://www.opengis.net/gml#AbstractReferenceSystemType"/>
   </owl:Class>
   <owl:Class rdf:about="http://www.opengis.net/gml#GeocentricCRSRefType">
      <rdfs:comment>Association to a geocentric coordinate reference system, either referencing or containing the definition of that reference system. </rdfs:comment>
      <rdfs:subClassOf>
         <owl:Class>
            <owl:intersectionOf rdf:parseType="Collection">
               <owl:Restriction>
                  <owl:onProperty rdf:resource="http://www.opengis.net/gml#hasGeocentricCRS"/>
                  <owl:allValuesFrom rdf:resource="http://www.opengis.net/gml#GeocentricCRS"/>
               </owl:Restriction>
            </owl:intersectionOf>
         </owl:Class>
      </rdfs:subClassOf>
   </owl:Class>
   <owl:Class rdf:about="http://www.opengis.net/gml#AbstractGeneralDerivedCRSType">
      <rdfs:comment>This is an abstract class</rdfs:comment>
      <rdfs:comment>A coordinate reference system that is defined by its coordinate conversion from another coordinate reference system (not by a datum). This abstract complexType shall not be used, extended, or restricted, in an Application Schema, to define a concrete subtype with a meaning equivalent to a concrete subtype specified in this document. </rdfs:comment>
      <rdfs:subClassOf>
         <owl:Class>
            <owl:intersectionOf rdf:parseType="Collection">
               <owl:Restriction>
                  <owl:onProperty rdf:resource="http://www.opengis.net/gml#hasbaseCRS"/>
                  <owl:allValuesFrom rdf:resource="http://www.opengis.net/gml#baseCRS"/>
               </owl:Restriction>
               <owl:Restriction>
                  <owl:onProperty rdf:resource="http://www.opengis.net/gml#hasdefinedByConversion"/>
                  <owl:allValuesFrom rdf:resource="http://www.opengis.net/gml#definedByConversion"/>
               </owl:Restriction>
            </owl:intersectionOf>
         </owl:Class>
      </rdfs:subClassOf>
      <rdfs:subClassOf rdf:resource="http://www.opengis.net/gml#AbstractReferenceSystemType"/>
   </owl:Class>
   <owl:Class rdf:about="http://www.opengis.net/gml#ProjectedCRSType">
      <rdfs:comment>A 2D coordinate reference system used to approximate the shape of the earth on a planar surface, but in such a way that the distortion that is inherent to the approximation is carefully controlled and known. Distortion correction is commonly applied to calculated bearings and distances to produce values that are a close match to actual field values. </rdfs:comment>
      <rdfs:subClassOf>
         <owl:Class>
            <owl:intersectionOf rdf:parseType="Collection">
               <owl:Restriction>
                  <owl:onProperty rdf:resource="http://www.opengis.net/gml#hasusesCartesianCS"/>
                  <owl:allValuesFrom rdf:resource="http://www.opengis.net/gml#usesCartesianCS"/>
               </owl:Restriction>
            </owl:intersectionOf>
         </owl:Class>
      </rdfs:subClassOf>
      <rdfs:subClassOf rdf:resource="http://www.opengis.net/gml#AbstractGeneralDerivedCRSType"/>
   </owl:Class>
   <owl:Class rdf:about="http://www.opengis.net/gml#ProjectedCRSRefType">
      <rdfs:comment>Association to a projected coordinate reference system, either referencing or containing the definition of that reference system. </rdfs:comment>
      <rdfs:subClassOf>
         <owl:Class>
            <owl:intersectionOf rdf:parseType="Collection">
               <owl:Restriction>
                  <owl:onProperty rdf:resource="http://www.opengis.net/gml#hasProjectedCRS"/>
                  <owl:allValuesFrom rdf:resource="http://www.opengis.net/gml#ProjectedCRS"/>
               </owl:Restriction>
            </owl:intersectionOf>
         </owl:Class>
      </rdfs:subClassOf>
   </owl:Class>
   <owl:Class rdf:about="http://www.opengis.net/gml#DerivedCRSType">
      <rdfs:comment>A coordinate reference system that is defined by its coordinate conversion from another coordinate reference system but is not a projected coordinate reference system. This category includes coordinate reference systems derived from a projected coordinate reference system. </rdfs:comment>
      <rdfs:subClassOf>
         <owl:Class>
            <owl:intersectionOf rdf:parseType="Collection">
               <owl:Restriction>
                  <owl:onProperty rdf:resource="http://www.opengis.net/gml#hasderivedCRSType"/>
                  <owl:allValuesFrom rdf:resource="http://www.opengis.net/gml#derivedCRSType"/>
               </owl:Restriction>
               <owl:Restriction>
                  <owl:onProperty rdf:resource="http://www.opengis.net/gml#hasusesCS"/>
                  <owl:allValuesFrom rdf:resource="http://www.opengis.net/gml#usesCS"/>
               </owl:Restriction>
            </owl:intersectionOf>
         </owl:Class>
      </rdfs:subClassOf>
      <rdfs:subClassOf rdf:resource="http://www.opengis.net/gml#AbstractGeneralDerivedCRSType"/>
   </owl:Class>
   <owl:Class rdf:about="http://www.opengis.net/gml#DerivedCRSTypeType">
      <rdfs:comment>Type of a derived coordinate reference system. </rdfs:comment>
      <rdfs:subClassOf>
         <owl:Restriction>
            <owl:onProperty rdf:resource="http://www.opengis.net/gml#hasDerivedCRSTypeTypeDatatype"/>
            <owl:someValuesFrom rdf:resource="http://www.opengis.net/gml#DerivedCRSTypeTypeDatatype"/>
         </owl:Restriction>
      </rdfs:subClassOf>
      <rdfs:subClassOf rdf:resource="http://www.opengis.net/gml#CodeType"/>
   </owl:Class>
   <rdfs:Datatype rdf:about="http://www.opengis.net/gml#DerivedCRSTypeTypeDatatype">
      <owl:equivalentClass rdf:resource="http://www.opengis.net/gml#CodeType"/>
   </rdfs:Datatype>
   <owl:DatatypeProperty rdf:about="http://www.opengis.net/gml#hasDerivedCRSTypeTypeDatatype">
      <rdfs:domain rdf:resource="http://www.opengis.net/gml#DerivedCRSTypeType"/>
      <rdfs:range rdf:resource="http://www.opengis.net/gml#DerivedCRSTypeTypeDatatype"/>
   </owl:DatatypeProperty>
   <owl:Class rdf:about="http://www.opengis.net/gml#DerivedCRSRefType">
      <rdfs:comment>Association to a non-projected derived coordinate reference system, either referencing or containing the definition of that reference system. </rdfs:comment>
      <rdfs:subClassOf>
         <owl:Class>
            <owl:intersectionOf rdf:parseType="Collection">
               <owl:Restriction>
                  <owl:onProperty rdf:resource="http://www.opengis.net/gml#hasDerivedCRS"/>
                  <owl:allValuesFrom rdf:resource="http://www.opengis.net/gml#DerivedCRS"/>
               </owl:Restriction>
            </owl:intersectionOf>
         </owl:Class>
      </rdfs:subClassOf>
   </owl:Class>
   <owl:Class rdf:about="http://www.opengis.net/gml#EngineeringCRSType">
      <rdfs:comment>A contextually local coordinate reference system; which can be divided into two broad categories:
- earth-fixed systems applied to engineering activities on or near the surface of the earth;
- CRSs on moving platforms such as road vehicles, vessels, aircraft, or spacecraft.
For further information, see OGC Abstract Specification Topic 2. </rdfs:comment>
      <rdfs:subClassOf>
         <owl:Class>
            <owl:intersectionOf rdf:parseType="Collection">
               <owl:Restriction>
                  <owl:onProperty rdf:resource="http://www.opengis.net/gml#hasusesCS"/>
                  <owl:allValuesFrom rdf:resource="http://www.opengis.net/gml#usesCS"/>
               </owl:Restriction>
               <owl:Restriction>
                  <owl:onProperty rdf:resource="http://www.opengis.net/gml#hasusesEngineeringDatum"/>
                  <owl:allValuesFrom rdf:resource="http://www.opengis.net/gml#usesEngineeringDatum"/>
               </owl:Restriction>
            </owl:intersectionOf>
         </owl:Class>
      </rdfs:subClassOf>
      <rdfs:subClassOf rdf:resource="http://www.opengis.net/gml#AbstractReferenceSystemType"/>
   </owl:Class>
   <owl:Class rdf:about="http://www.opengis.net/gml#EngineeringCRSRefType">
      <rdfs:comment>Association to an engineering coordinate reference system, either referencing or containing the definition of that reference system. </rdfs:comment>
      <rdfs:subClassOf>
         <owl:Class>
            <owl:intersectionOf rdf:parseType="Collection">
               <owl:Restriction>
                  <owl:onProperty rdf:resource="http://www.opengis.net/gml#hasEngineeringCRS"/>
                  <owl:allValuesFrom rdf:resource="http://www.opengis.net/gml#EngineeringCRS"/>
               </owl:Restriction>
            </owl:intersectionOf>
         </owl:Class>
      </rdfs:subClassOf>
   </owl:Class>
   <owl:Class rdf:about="http://www.opengis.net/gml#ImageCRSType">
      <rdfs:comment>An engineering coordinate reference system applied to locations in images. Image coordinate reference systems are treated as a separate sub-type because a separate user community exists for images with its own terms of reference. </rdfs:comment>
      <rdfs:subClassOf>
         <owl:Class>
            <owl:intersectionOf rdf:parseType="Collection">
               <owl:Restriction>
                  <owl:onProperty rdf:resource="http://www.opengis.net/gml#hasusesImageDatum"/>
                  <owl:allValuesFrom rdf:resource="http://www.opengis.net/gml#usesImageDatum"/>
               </owl:Restriction>
            </owl:intersectionOf>
         </owl:Class>
      </rdfs:subClassOf>
      <owl:disjointUnionOf rdf:parseType="Collection">
         <owl:Restriction>
            <owl:onProperty rdf:resource="http://www.opengis.net/gml#hasusesCartesianCS"/>
            <owl:someValuesFrom rdf:resource="http://www.opengis.net/gml#usesCartesianCS"/>
         </owl:Restriction>
         <owl:Restriction>
            <owl:onProperty rdf:resource="http://www.opengis.net/gml#hasusesObliqueCartesianCS"/>
            <owl:someValuesFrom rdf:resource="http://www.opengis.net/gml#usesObliqueCartesianCS"/>
         </owl:Restriction>
      </owl:disjointUnionOf>
      <rdfs:subClassOf rdf:resource="http://www.opengis.net/gml#AbstractReferenceSystemType"/>
   </owl:Class>
   <owl:Class rdf:about="http://www.opengis.net/gml#ImageCRSRefType">
      <rdfs:comment>Association to an image coordinate reference system, either referencing or containing the definition of that reference system. </rdfs:comment>
      <rdfs:subClassOf>
         <owl:Class>
            <owl:intersectionOf rdf:parseType="Collection">
               <owl:Restriction>
                  <owl:onProperty rdf:resource="http://www.opengis.net/gml#hasImageCRS"/>
                  <owl:allValuesFrom rdf:resource="http://www.opengis.net/gml#ImageCRS"/>
               </owl:Restriction>
            </owl:intersectionOf>
         </owl:Class>
      </rdfs:subClassOf>
   </owl:Class>
   <owl:Class rdf:about="http://www.opengis.net/gml#TemporalCRSType">
      <rdfs:comment>A 1D coordinate reference system used for the recording of time. </rdfs:comment>
      <rdfs:subClassOf>
         <owl:Class>
            <owl:intersectionOf rdf:parseType="Collection">
               <owl:Restriction>
                  <owl:onProperty rdf:resource="http://www.opengis.net/gml#hasusesTemporalCS"/>
                  <owl:allValuesFrom rdf:resource="http://www.opengis.net/gml#usesTemporalCS"/>
               </owl:Restriction>
               <owl:Restriction>
                  <owl:onProperty rdf:resource="http://www.opengis.net/gml#hasusesTemporalDatum"/>
                  <owl:allValuesFrom rdf:resource="http://www.opengis.net/gml#usesTemporalDatum"/>
               </owl:Restriction>
            </owl:intersectionOf>
         </owl:Class>
      </rdfs:subClassOf>
      <rdfs:subClassOf rdf:resource="http://www.opengis.net/gml#AbstractReferenceSystemType"/>
   </owl:Class>
   <owl:Class rdf:about="http://www.opengis.net/gml#TemporalCRSRefType">
      <rdfs:comment>Association to a temporal coordinate reference system, either referencing or containing the definition of that reference system. </rdfs:comment>
      <rdfs:subClassOf>
         <owl:Class>
            <owl:intersectionOf rdf:parseType="Collection">
               <owl:Restriction>
                  <owl:onProperty rdf:resource="http://www.opengis.net/gml#hasTemporalCRS"/>
                  <owl:allValuesFrom rdf:resource="http://www.opengis.net/gml#TemporalCRS"/>
               </owl:Restriction>
            </owl:intersectionOf>
         </owl:Class>
      </rdfs:subClassOf>
   </owl:Class>
   <owl:Class rdf:about="http://www.opengis.net/gml#CoordinateSystemAxisBaseType">
      <rdfs:comment>This is an abstract class</rdfs:comment>
      <rdfs:comment>Basic encoding for coordinate system axis objects, simplifying and restricting the DefinitionType as needed. </rdfs:comment>
      <rdfs:subClassOf>
         <owl:Class>
            <owl:intersectionOf rdf:parseType="Collection">
               <owl:Restriction>
                  <owl:onProperty rdf:resource="http://www.opengis.net/gml#hasmetaDataProperty"/>
                  <owl:allValuesFrom rdf:resource="http://www.opengis.net/gml#metaDataProperty"/>
               </owl:Restriction>
               <owl:Restriction>
                  <owl:onProperty rdf:resource="http://www.opengis.net/gml#hasmetaDataProperty"/>
                  <owl:minCardinality rdf:datatype="http://www.w3.org/2001/XMLSchema#nonNegativeInteger">0</owl:minCardinality>
               </owl:Restriction>
               <owl:Restriction>
                  <owl:onProperty rdf:resource="http://www.opengis.net/gml#hasname"/>
                  <owl:allValuesFrom rdf:resource="http://www.opengis.net/gml#name"/>
               </owl:Restriction>
            </owl:intersectionOf>
         </owl:Class>
      </rdfs:subClassOf>
      <rdfs:subClassOf>
         <owl:Class>
            <owl:intersectionOf rdf:parseType="Collection">
               <owl:Restriction>
                  <owl:onProperty rdf:resource="http://www.opengis.net/gml#hasid"/>
                  <owl:allValuesFrom rdf:resource="http://www.opengis.net/gml#id"/>
               </owl:Restriction>
            </owl:intersectionOf>
         </owl:Class>
      </rdfs:subClassOf>
      <rdfs:subClassOf rdf:resource="http://www.opengis.net/gml#DefinitionType"/>
   </owl:Class>
   <owl:Class rdf:about="http://www.opengis.net/gml#CoordinateSystemAxisType">
      <rdfs:comment>Definition of a coordinate system axis. </rdfs:comment>
      <rdfs:subClassOf>
         <owl:Class>
            <owl:intersectionOf rdf:parseType="Collection">
               <owl:Restriction>
                  <owl:onProperty rdf:resource="http://www.opengis.net/gml#hasaxisID"/>
                  <owl:allValuesFrom rdf:resource="http://www.opengis.net/gml#axisID"/>
               </owl:Restriction>
               <owl:Restriction>
                  <owl:onProperty rdf:resource="http://www.opengis.net/gml#hasaxisID"/>
                  <owl:minCardinality rdf:datatype="http://www.w3.org/2001/XMLSchema#nonNegativeInteger">0</owl:minCardinality>
               </owl:Restriction>
               <owl:Restriction>
                  <owl:onProperty rdf:resource="http://www.opengis.net/gml#hasremarks"/>
                  <owl:allValuesFrom rdf:resource="http://www.opengis.net/gml#remarks"/>
               </owl:Restriction>
               <owl:Restriction>
                  <owl:onProperty rdf:resource="http://www.opengis.net/gml#hasremarks"/>
                  <owl:minCardinality rdf:datatype="http://www.w3.org/2001/XMLSchema#nonNegativeInteger">0</owl:minCardinality>
               </owl:Restriction>
               <owl:Restriction>
                  <owl:onProperty rdf:resource="http://www.opengis.net/gml#hasaxisAbbrev"/>
                  <owl:allValuesFrom rdf:resource="http://www.opengis.net/gml#axisAbbrev"/>
               </owl:Restriction>
               <owl:Restriction>
                  <owl:onProperty rdf:resource="http://www.opengis.net/gml#hasaxisDirection"/>
                  <owl:allValuesFrom rdf:resource="http://www.opengis.net/gml#axisDirection"/>
               </owl:Restriction>
            </owl:intersectionOf>
         </owl:Class>
      </rdfs:subClassOf>
      <rdfs:subClassOf>
         <owl:Class>
            <owl:intersectionOf rdf:parseType="Collection">
               <owl:Restriction>
                  <owl:onProperty rdf:resource="http://www.opengis.net/gml#hasuom"/>
                  <owl:allValuesFrom rdf:resource="http://www.opengis.net/gml#uom"/>
               </owl:Restriction>
            </owl:intersectionOf>
         </owl:Class>
      </rdfs:subClassOf>
      <rdfs:subClassOf rdf:resource="http://www.opengis.net/gml#CoordinateSystemAxisBaseType"/>
   </owl:Class>
   <owl:Class rdf:about="http://www.opengis.net/gml#CoordinateSystemAxisRefType">
      <rdfs:comment>Association to a coordinate system axis, either referencing or containing the definition of that axis. </rdfs:comment>
      <rdfs:subClassOf>
         <owl:Class>
            <owl:intersectionOf rdf:parseType="Collection">
               <owl:Restriction>
                  <owl:onProperty rdf:resource="http://www.opengis.net/gml#hasCoordinateSystemAxis"/>
                  <owl:allValuesFrom rdf:resource="http://www.opengis.net/gml#CoordinateSystemAxis"/>
               </owl:Restriction>
            </owl:intersectionOf>
         </owl:Class>
      </rdfs:subClassOf>
   </owl:Class>
   <owl:Class rdf:about="http://www.opengis.net/gml#AbstractCoordinateSystemBaseType">
      <rdfs:comment>This is an abstract class</rdfs:comment>
      <rdfs:comment>Basic encoding for coordinate system objects, simplifying and restricting the DefinitionType as needed. </rdfs:comment>
      <rdfs:subClassOf>
         <owl:Class>
            <owl:intersectionOf rdf:parseType="Collection">
               <owl:Restriction>
                  <owl:onProperty rdf:resource="http://www.opengis.net/gml#hasmetaDataProperty"/>
                  <owl:allValuesFrom rdf:resource="http://www.opengis.net/gml#metaDataProperty"/>
               </owl:Restriction>
               <owl:Restriction>
                  <owl:onProperty rdf:resource="http://www.opengis.net/gml#hasmetaDataProperty"/>
                  <owl:minCardinality rdf:datatype="http://www.w3.org/2001/XMLSchema#nonNegativeInteger">0</owl:minCardinality>
               </owl:Restriction>
               <owl:Restriction>
                  <owl:onProperty rdf:resource="http://www.opengis.net/gml#hascsName"/>
                  <owl:allValuesFrom rdf:resource="http://www.opengis.net/gml#csName"/>
               </owl:Restriction>
            </owl:intersectionOf>
         </owl:Class>
      </rdfs:subClassOf>
      <rdfs:subClassOf>
         <owl:Class>
            <owl:intersectionOf rdf:parseType="Collection">
               <owl:Restriction>
                  <owl:onProperty rdf:resource="http://www.opengis.net/gml#hasid"/>
                  <owl:allValuesFrom rdf:resource="http://www.opengis.net/gml#id"/>
               </owl:Restriction>
            </owl:intersectionOf>
         </owl:Class>
      </rdfs:subClassOf>
      <rdfs:subClassOf rdf:resource="http://www.opengis.net/gml#DefinitionType"/>
   </owl:Class>
   <owl:Class rdf:about="http://www.opengis.net/gml#AbstractCoordinateSystemType">
      <rdfs:comment>This is an abstract class</rdfs:comment>
      <rdfs:comment>A coordinate system (CS) is the set of coordinate system axes that spans a given coordinate space. A CS is derived from a set of (mathematical) rules for specifying how coordinates in a given space are to be assigned to points. The coordinate values in a coordinate tuple shall be recorded in the order in which the coordinate system axes associations are recorded, whenever those coordinates use a coordinate reference system that uses this coordinate system. This abstract complexType shall not be used, extended, or restricted, in an Application Schema, to define a concrete subtype with a meaning equivalent to a concrete subtype specified in this document. </rdfs:comment>
      <rdfs:subClassOf>
         <owl:Class>
            <owl:intersectionOf rdf:parseType="Collection">
               <owl:Restriction>
                  <owl:onProperty rdf:resource="http://www.opengis.net/gml#hascsID"/>
                  <owl:allValuesFrom rdf:resource="http://www.opengis.net/gml#csID"/>
               </owl:Restriction>
               <owl:Restriction>
                  <owl:onProperty rdf:resource="http://www.opengis.net/gml#hascsID"/>
                  <owl:minCardinality rdf:datatype="http://www.w3.org/2001/XMLSchema#nonNegativeInteger">0</owl:minCardinality>
               </owl:Restriction>
               <owl:Restriction>
                  <owl:onProperty rdf:resource="http://www.opengis.net/gml#hasremarks"/>
                  <owl:allValuesFrom rdf:resource="http://www.opengis.net/gml#remarks"/>
               </owl:Restriction>
               <owl:Restriction>
                  <owl:onProperty rdf:resource="http://www.opengis.net/gml#hasremarks"/>
                  <owl:minCardinality rdf:datatype="http://www.w3.org/2001/XMLSchema#nonNegativeInteger">0</owl:minCardinality>
               </owl:Restriction>
               <owl:Restriction>
                  <owl:onProperty rdf:resource="http://www.opengis.net/gml#hasusesAxis"/>
                  <owl:allValuesFrom rdf:resource="http://www.opengis.net/gml#usesAxis"/>
               </owl:Restriction>
            </owl:intersectionOf>
         </owl:Class>
      </rdfs:subClassOf>
      <rdfs:subClassOf rdf:resource="http://www.opengis.net/gml#AbstractCoordinateSystemBaseType"/>
   </owl:Class>
   <owl:Class rdf:about="http://www.opengis.net/gml#CoordinateSystemRefType">
      <rdfs:comment>Association to a coordinate system, either referencing or containing the definition of that coordinate system. </rdfs:comment>
      <rdfs:subClassOf>
         <owl:Class>
            <owl:intersectionOf rdf:parseType="Collection">
               <owl:Restriction>
                  <owl:onProperty rdf:resource="http://www.opengis.net/gml#has_CoordinateSystem"/>
                  <owl:allValuesFrom rdf:resource="http://www.opengis.net/gml#_CoordinateSystem"/>
               </owl:Restriction>
            </owl:intersectionOf>
         </owl:Class>
      </rdfs:subClassOf>
   </owl:Class>
   <owl:Class rdf:about="http://www.opengis.net/gml#EllipsoidalCSType">
      <rdfs:comment>A two- or three-dimensional coordinate system in which position is specified by geodetic latitude, geodetic longitude, and (in the three-dimensional case) ellipsoidal height. An EllipsoidalCS shall have two or three usesAxis associations. </rdfs:comment>
      <rdfs:subClassOf rdf:resource="http://www.opengis.net/gml#AbstractCoordinateSystemType"/>
   </owl:Class>
   <owl:Class rdf:about="http://www.opengis.net/gml#EllipsoidalCSRefType">
      <rdfs:comment>Association to an ellipsoidal coordinate system, either referencing or containing the definition of that coordinate system. </rdfs:comment>
      <rdfs:subClassOf>
         <owl:Class>
            <owl:intersectionOf rdf:parseType="Collection">
               <owl:Restriction>
                  <owl:onProperty rdf:resource="http://www.opengis.net/gml#hasEllipsoidalCS"/>
                  <owl:allValuesFrom rdf:resource="http://www.opengis.net/gml#EllipsoidalCS"/>
               </owl:Restriction>
            </owl:intersectionOf>
         </owl:Class>
      </rdfs:subClassOf>
   </owl:Class>
   <owl:Class rdf:about="http://www.opengis.net/gml#CartesianCSType">
      <rdfs:comment>A 1-, 2-, or 3-dimensional coordinate system. Gives the position of points relative to orthogonal straight axes in the 2- and 3-dimensional cases. In the 1-dimensional case, it contains a single straight coordinate axis. In the multi-dimensional case, all axes shall have the same length unit of measure. A CartesianCS shall have one, two, or three usesAxis associations. </rdfs:comment>
      <rdfs:subClassOf rdf:resource="http://www.opengis.net/gml#AbstractCoordinateSystemType"/>
   </owl:Class>
   <owl:Class rdf:about="http://www.opengis.net/gml#CartesianCSRefType">
      <rdfs:comment>Association to a Cartesian coordinate system, either referencing or containing the definition of that coordinate system. </rdfs:comment>
      <rdfs:subClassOf>
         <owl:Class>
            <owl:intersectionOf rdf:parseType="Collection">
               <owl:Restriction>
                  <owl:onProperty rdf:resource="http://www.opengis.net/gml#hasCartesianCS"/>
                  <owl:allValuesFrom rdf:resource="http://www.opengis.net/gml#CartesianCS"/>
               </owl:Restriction>
            </owl:intersectionOf>
         </owl:Class>
      </rdfs:subClassOf>
   </owl:Class>
   <owl:Class rdf:about="http://www.opengis.net/gml#VerticalCSType">
      <rdfs:comment>A one-dimensional coordinate system used to record the heights (or depths) of points. Such a coordinate system is usually dependent on the Earth's gravity field, perhaps loosely as when atmospheric pressure is the basis for the vertical coordinate system axis. A VerticalCS shall have one usesAxis association. </rdfs:comment>
      <rdfs:subClassOf rdf:resource="http://www.opengis.net/gml#AbstractCoordinateSystemType"/>
   </owl:Class>
   <owl:Class rdf:about="http://www.opengis.net/gml#VerticalCSRefType">
      <rdfs:comment>Association to a vertical coordinate system, either referencing or containing the definition of that coordinate system. </rdfs:comment>
      <rdfs:subClassOf>
         <owl:Class>
            <owl:intersectionOf rdf:parseType="Collection">
               <owl:Restriction>
                  <owl:onProperty rdf:resource="http://www.opengis.net/gml#hasVerticalCS"/>
                  <owl:allValuesFrom rdf:resource="http://www.opengis.net/gml#VerticalCS"/>
               </owl:Restriction>
            </owl:intersectionOf>
         </owl:Class>
      </rdfs:subClassOf>
   </owl:Class>
   <owl:Class rdf:about="http://www.opengis.net/gml#TemporalCSType">
      <rdfs:comment>A one-dimensional coordinate system containing a single time axis, used to describe the temporal position of a point in the specified time units from a specified time origin. A TemporalCS shall have one usesAxis association. </rdfs:comment>
      <rdfs:subClassOf rdf:resource="http://www.opengis.net/gml#AbstractCoordinateSystemType"/>
   </owl:Class>
   <owl:Class rdf:about="http://www.opengis.net/gml#TemporalCSRefType">
      <rdfs:comment>Association to a temporal coordinate system, either referencing or containing the definition of that coordinate system. </rdfs:comment>
      <rdfs:subClassOf>
         <owl:Class>
            <owl:intersectionOf rdf:parseType="Collection">
               <owl:Restriction>
                  <owl:onProperty rdf:resource="http://www.opengis.net/gml#hasTemporalCS"/>
                  <owl:allValuesFrom rdf:resource="http://www.opengis.net/gml#TemporalCS"/>
               </owl:Restriction>
            </owl:intersectionOf>
         </owl:Class>
      </rdfs:subClassOf>
   </owl:Class>
   <owl:Class rdf:about="http://www.opengis.net/gml#LinearCSType">
      <rdfs:comment>A one-dimensional coordinate system that consists of the points that lie on the single axis described. The associated ordinate is the distance from the specified origin to the point along the axis. Example: usage of the line feature representing a road to describe points on or along that road. A LinearCS shall have one usesAxis association. </rdfs:comment>
      <rdfs:subClassOf rdf:resource="http://www.opengis.net/gml#AbstractCoordinateSystemType"/>
   </owl:Class>
   <owl:Class rdf:about="http://www.opengis.net/gml#LinearCSRefType">
      <rdfs:comment>Association to a linear coordinate system, either referencing or containing the definition of that coordinate system. </rdfs:comment>
      <rdfs:subClassOf>
         <owl:Class>
            <owl:intersectionOf rdf:parseType="Collection">
               <owl:Restriction>
                  <owl:onProperty rdf:resource="http://www.opengis.net/gml#hasLinearCS"/>
                  <owl:allValuesFrom rdf:resource="http://www.opengis.net/gml#LinearCS"/>
               </owl:Restriction>
            </owl:intersectionOf>
         </owl:Class>
      </rdfs:subClassOf>
   </owl:Class>
   <owl:Class rdf:about="http://www.opengis.net/gml#UserDefinedCSType">
      <rdfs:comment>A two- or three-dimensional coordinate system that consists of any combination of coordinate axes not covered by any other coordinate system type. An example is a multilinear coordinate system which contains one coordinate axis that may have any 1-D shape which has no intersections with itself. This non-straight axis is supplemented by one or two straight axes to complete a 2 or 3 dimensional coordinate system. The non-straight axis is typically incrementally straight or curved. A UserDefinedCS shall have two or three usesAxis associations. </rdfs:comment>
      <rdfs:subClassOf rdf:resource="http://www.opengis.net/gml#AbstractCoordinateSystemType"/>
   </owl:Class>
   <owl:Class rdf:about="http://www.opengis.net/gml#UserDefinedCSRefType">
      <rdfs:comment>Association to a user-defined coordinate system, either referencing or containing the definition of that coordinate system. </rdfs:comment>
      <rdfs:subClassOf>
         <owl:Class>
            <owl:intersectionOf rdf:parseType="Collection">
               <owl:Restriction>
                  <owl:onProperty rdf:resource="http://www.opengis.net/gml#hasUserDefinedCS"/>
                  <owl:allValuesFrom rdf:resource="http://www.opengis.net/gml#UserDefinedCS"/>
               </owl:Restriction>
            </owl:intersectionOf>
         </owl:Class>
      </rdfs:subClassOf>
   </owl:Class>
   <owl:Class rdf:about="http://www.opengis.net/gml#SphericalCSType">
      <rdfs:comment>A three-dimensional coordinate system with one distance measured from the origin and two angular coordinates. Not to be confused with an ellipsoidal coordinate system based on an ellipsoid "degenerated" into a sphere. A SphericalCS shall have three usesAxis associations. </rdfs:comment>
      <rdfs:subClassOf rdf:resource="http://www.opengis.net/gml#AbstractCoordinateSystemType"/>
   </owl:Class>
   <owl:Class rdf:about="http://www.opengis.net/gml#SphericalCSRefType">
      <rdfs:comment>Association to a spherical coordinate system, either referencing or containing the definition of that coordinate system. </rdfs:comment>
      <rdfs:subClassOf>
         <owl:Class>
            <owl:intersectionOf rdf:parseType="Collection">
               <owl:Restriction>
                  <owl:onProperty rdf:resource="http://www.opengis.net/gml#hasSphericalCS"/>
                  <owl:allValuesFrom rdf:resource="http://www.opengis.net/gml#SphericalCS"/>
               </owl:Restriction>
            </owl:intersectionOf>
         </owl:Class>
      </rdfs:subClassOf>
   </owl:Class>
   <owl:Class rdf:about="http://www.opengis.net/gml#PolarCSType">
      <rdfs:comment>A two-dimensional coordinate system in which position is specified by the distance from the origin and the angle between the line from the origin to a point and a reference direction. A PolarCS shall have two usesAxis associations. </rdfs:comment>
      <rdfs:subClassOf rdf:resource="http://www.opengis.net/gml#AbstractCoordinateSystemType"/>
   </owl:Class>
   <owl:Class rdf:about="http://www.opengis.net/gml#PolarCSRefType">
      <rdfs:comment>Association to a polar coordinate system, either referencing or containing the definition of that coordinate system. </rdfs:comment>
      <rdfs:subClassOf>
         <owl:Class>
            <owl:intersectionOf rdf:parseType="Collection">
               <owl:Restriction>
                  <owl:onProperty rdf:resource="http://www.opengis.net/gml#hasPolarCS"/>
                  <owl:allValuesFrom rdf:resource="http://www.opengis.net/gml#PolarCS"/>
               </owl:Restriction>
            </owl:intersectionOf>
         </owl:Class>
      </rdfs:subClassOf>
   </owl:Class>
   <owl:Class rdf:about="http://www.opengis.net/gml#CylindricalCSType">
      <rdfs:comment>A three-dimensional coordinate system consisting of a polar coordinate system extended by a straight coordinate axis perpendicular to the plane spanned by the polar coordinate system. A CylindricalCS shall have three usesAxis associations. </rdfs:comment>
      <rdfs:subClassOf rdf:resource="http://www.opengis.net/gml#AbstractCoordinateSystemType"/>
   </owl:Class>
   <owl:Class rdf:about="http://www.opengis.net/gml#CylindricalCSRefType">
      <rdfs:comment>Association to a cylindrical coordinate system, either referencing or containing the definition of that coordinate system. </rdfs:comment>
      <rdfs:subClassOf>
         <owl:Class>
            <owl:intersectionOf rdf:parseType="Collection">
               <owl:Restriction>
                  <owl:onProperty rdf:resource="http://www.opengis.net/gml#hasCylindricalCS"/>
                  <owl:allValuesFrom rdf:resource="http://www.opengis.net/gml#CylindricalCS"/>
               </owl:Restriction>
            </owl:intersectionOf>
         </owl:Class>
      </rdfs:subClassOf>
   </owl:Class>
   <owl:Class rdf:about="http://www.opengis.net/gml#ObliqueCartesianCSType">
      <rdfs:comment>A two- or three-dimensional coordinate system with straight axes that are not necessarily orthogonal. An ObliqueCartesianCS shall have two or three usesAxis associations. </rdfs:comment>
      <rdfs:subClassOf rdf:resource="http://www.opengis.net/gml#AbstractCoordinateSystemType"/>
   </owl:Class>
   <owl:Class rdf:about="http://www.opengis.net/gml#ObliqueCartesianCSRefType">
      <rdfs:comment>Association to an oblique-Cartesian coordinate system, either referencing or containing the definition of that coordinate system. </rdfs:comment>
      <rdfs:subClassOf>
         <owl:Class>
            <owl:intersectionOf rdf:parseType="Collection">
               <owl:Restriction>
                  <owl:onProperty rdf:resource="http://www.opengis.net/gml#hasObliqueCartesianCS"/>
                  <owl:allValuesFrom rdf:resource="http://www.opengis.net/gml#ObliqueCartesianCS"/>
               </owl:Restriction>
            </owl:intersectionOf>
         </owl:Class>
      </rdfs:subClassOf>
   </owl:Class>
   <owl:Class rdf:about="http://www.opengis.net/gml#AbstractReferenceSystemBaseType">
      <rdfs:comment>This is an abstract class</rdfs:comment>
      <rdfs:comment>Basic encoding for reference system objects, simplifying and restricting the DefinitionType as needed.</rdfs:comment>
      <rdfs:subClassOf>
         <owl:Class>
            <owl:intersectionOf rdf:parseType="Collection">
               <owl:Restriction>
                  <owl:onProperty rdf:resource="http://www.opengis.net/gml#hasmetaDataProperty"/>
                  <owl:allValuesFrom rdf:resource="http://www.opengis.net/gml#metaDataProperty"/>
               </owl:Restriction>
               <owl:Restriction>
                  <owl:onProperty rdf:resource="http://www.opengis.net/gml#hasmetaDataProperty"/>
                  <owl:minCardinality rdf:datatype="http://www.w3.org/2001/XMLSchema#nonNegativeInteger">0</owl:minCardinality>
               </owl:Restriction>
               <owl:Restriction>
                  <owl:onProperty rdf:resource="http://www.opengis.net/gml#hassrsName"/>
                  <owl:allValuesFrom rdf:resource="http://www.opengis.net/gml#srsName"/>
               </owl:Restriction>
            </owl:intersectionOf>
         </owl:Class>
      </rdfs:subClassOf>
      <rdfs:subClassOf>
         <owl:Class>
            <owl:intersectionOf rdf:parseType="Collection">
               <owl:Restriction>
                  <owl:onProperty rdf:resource="http://www.opengis.net/gml#hasid"/>
                  <owl:allValuesFrom rdf:resource="http://www.opengis.net/gml#id"/>
               </owl:Restriction>
            </owl:intersectionOf>
         </owl:Class>
      </rdfs:subClassOf>
      <rdfs:subClassOf rdf:resource="http://www.opengis.net/gml#DefinitionType"/>
   </owl:Class>
   <owl:Class rdf:about="http://www.opengis.net/gml#AbstractReferenceSystemType">
      <rdfs:comment>This is an abstract class</rdfs:comment>
      <rdfs:comment>Description of a spatial and/or temporal reference system used by a dataset.</rdfs:comment>
      <rdfs:subClassOf>
         <owl:Class>
            <owl:intersectionOf rdf:parseType="Collection">
               <owl:Restriction>
                  <owl:onProperty rdf:resource="http://www.opengis.net/gml#hassrsID"/>
                  <owl:allValuesFrom rdf:resource="http://www.opengis.net/gml#srsID"/>
               </owl:Restriction>
               <owl:Restriction>
                  <owl:onProperty rdf:resource="http://www.opengis.net/gml#hassrsID"/>
                  <owl:minCardinality rdf:datatype="http://www.w3.org/2001/XMLSchema#nonNegativeInteger">0</owl:minCardinality>
               </owl:Restriction>
               <owl:Restriction>
                  <owl:onProperty rdf:resource="http://www.opengis.net/gml#hasremarks"/>
                  <owl:allValuesFrom rdf:resource="http://www.opengis.net/gml#remarks"/>
               </owl:Restriction>
               <owl:Restriction>
                  <owl:onProperty rdf:resource="http://www.opengis.net/gml#hasremarks"/>
                  <owl:minCardinality rdf:datatype="http://www.w3.org/2001/XMLSchema#nonNegativeInteger">0</owl:minCardinality>
               </owl:Restriction>
               <owl:Restriction>
                  <owl:onProperty rdf:resource="http://www.opengis.net/gml#hasvalidArea"/>
                  <owl:allValuesFrom rdf:resource="http://www.opengis.net/gml#validArea"/>
               </owl:Restriction>
               <owl:Restriction>
                  <owl:onProperty rdf:resource="http://www.opengis.net/gml#hasvalidArea"/>
                  <owl:minCardinality rdf:datatype="http://www.w3.org/2001/XMLSchema#nonNegativeInteger">0</owl:minCardinality>
               </owl:Restriction>
               <owl:Restriction>
                  <owl:onProperty rdf:resource="http://www.opengis.net/gml#hasscope"/>
                  <owl:allValuesFrom rdf:resource="http://www.opengis.net/gml#scope"/>
               </owl:Restriction>
               <owl:Restriction>
                  <owl:onProperty rdf:resource="http://www.opengis.net/gml#hasscope"/>
                  <owl:minCardinality rdf:datatype="http://www.w3.org/2001/XMLSchema#nonNegativeInteger">0</owl:minCardinality>
               </owl:Restriction>
            </owl:intersectionOf>
         </owl:Class>
      </rdfs:subClassOf>
      <rdfs:subClassOf rdf:resource="http://www.opengis.net/gml#AbstractReferenceSystemBaseType"/>
   </owl:Class>
   <owl:Class rdf:about="http://www.opengis.net/gml#ReferenceSystemRefType">
      <rdfs:comment>Association to a reference system, either referencing or containing the definition of that reference system.</rdfs:comment>
      <rdfs:subClassOf>
         <owl:Class>
            <owl:intersectionOf rdf:parseType="Collection">
               <owl:Restriction>
                  <owl:onProperty rdf:resource="http://www.opengis.net/gml#has_ReferenceSystem"/>
                  <owl:allValuesFrom rdf:resource="http://www.opengis.net/gml#_ReferenceSystem"/>
               </owl:Restriction>
            </owl:intersectionOf>
         </owl:Class>
      </rdfs:subClassOf>
   </owl:Class>
   <owl:Class rdf:about="http://www.opengis.net/gml#CRSRefType">
      <rdfs:comment>Association to a CRS abstract coordinate reference system, either referencing or containing the definition of that CRS.</rdfs:comment>
      <rdfs:subClassOf>
         <owl:Class>
            <owl:intersectionOf rdf:parseType="Collection">
               <owl:Restriction>
                  <owl:onProperty rdf:resource="http://www.opengis.net/gml#has_CRS"/>
                  <owl:allValuesFrom rdf:resource="http://www.opengis.net/gml#_CRS"/>
               </owl:Restriction>
            </owl:intersectionOf>
         </owl:Class>
      </rdfs:subClassOf>
   </owl:Class>
   <owl:Class rdf:about="http://www.opengis.net/gml#IdentifierType">
      <rdfs:comment>An identification of a CRS object. The first use of the IdentifierType for an object, if any, is normally the primary identification code, and any others are aliases.</rdfs:comment>
      <rdfs:subClassOf>
         <owl:Class>
            <owl:intersectionOf rdf:parseType="Collection">
               <owl:Restriction>
                  <owl:onProperty rdf:resource="http://www.opengis.net/gml#hasname"/>
                  <owl:allValuesFrom rdf:resource="http://www.opengis.net/gml#name"/>
               </owl:Restriction>
               <owl:Restriction>
                  <owl:onProperty rdf:resource="http://www.opengis.net/gml#hasversion"/>
                  <owl:allValuesFrom rdf:resource="http://www.opengis.net/gml#version"/>
               </owl:Restriction>
               <owl:Restriction>
                  <owl:onProperty rdf:resource="http://www.opengis.net/gml#hasversion"/>
                  <owl:minCardinality rdf:datatype="http://www.w3.org/2001/XMLSchema#nonNegativeInteger">0</owl:minCardinality>
               </owl:Restriction>
               <owl:Restriction>
                  <owl:onProperty rdf:resource="http://www.opengis.net/gml#hasremarks"/>
                  <owl:allValuesFrom rdf:resource="http://www.opengis.net/gml#remarks"/>
               </owl:Restriction>
               <owl:Restriction>
                  <owl:onProperty rdf:resource="http://www.opengis.net/gml#hasremarks"/>
                  <owl:minCardinality rdf:datatype="http://www.w3.org/2001/XMLSchema#nonNegativeInteger">0</owl:minCardinality>
               </owl:Restriction>
            </owl:intersectionOf>
         </owl:Class>
      </rdfs:subClassOf>
   </owl:Class>
   <owl:Class rdf:about="http://www.opengis.net/gml#ExtentType">
      <rdfs:comment>Information about the spatial, vertical, and/or temporal extent of a reference system object. Constraints: At least one of the elements "description", "boundingBox", "boundingPolygon", "verticalExtent", and temporalExtent" must be included, but more that one can be included when appropriate. Furthermore, more than one "boundingBox", "boundingPolygon", "verticalExtent", and/or temporalExtent" element can be included, with more than one meaning the union of the individual domains.</rdfs:comment>
      <rdfs:subClassOf>
         <owl:Class>
            <owl:intersectionOf rdf:parseType="Collection">
               <owl:Restriction>
                  <owl:onProperty rdf:resource="http://www.opengis.net/gml#hasdescription"/>
                  <owl:allValuesFrom rdf:resource="http://www.opengis.net/gml#description"/>
               </owl:Restriction>
               <owl:Restriction>
                  <owl:onProperty rdf:resource="http://www.opengis.net/gml#hasdescription"/>
                  <owl:minCardinality rdf:datatype="http://www.w3.org/2001/XMLSchema#nonNegativeInteger">0</owl:minCardinality>
               </owl:Restriction>
               <owl:Restriction>
                  <owl:onProperty rdf:resource="http://www.opengis.net/gml#hasverticalExtent"/>
                  <owl:allValuesFrom rdf:resource="http://www.opengis.net/gml#verticalExtent"/>
               </owl:Restriction>
               <owl:Restriction>
                  <owl:onProperty rdf:resource="http://www.opengis.net/gml#hasverticalExtent"/>
                  <owl:minCardinality rdf:datatype="http://www.w3.org/2001/XMLSchema#nonNegativeInteger">0</owl:minCardinality>
               </owl:Restriction>
               <owl:Restriction>
                  <owl:onProperty rdf:resource="http://www.opengis.net/gml#hastemporalExtent"/>
                  <owl:allValuesFrom rdf:resource="http://www.opengis.net/gml#temporalExtent"/>
               </owl:Restriction>
               <owl:Restriction>
                  <owl:onProperty rdf:resource="http://www.opengis.net/gml#hastemporalExtent"/>
                  <owl:minCardinality rdf:datatype="http://www.w3.org/2001/XMLSchema#nonNegativeInteger">0</owl:minCardinality>
               </owl:Restriction>
            </owl:intersectionOf>
         </owl:Class>
      </rdfs:subClassOf>
      <owl:disjointUnionOf rdf:parseType="Collection">
         <owl:Restriction>
            <owl:onProperty rdf:resource="http://www.opengis.net/gml#hasboundingBox"/>
            <owl:someValuesFrom rdf:resource="http://www.opengis.net/gml#boundingBox"/>
         </owl:Restriction>
         <owl:Restriction>
            <owl:onProperty rdf:resource="http://www.opengis.net/gml#hasboundingBox"/>
            <owl:minCardinality rdf:datatype="http://www.w3.org/2001/XMLSchema#nonNegativeInteger">0</owl:minCardinality>
         </owl:Restriction>
         <owl:Restriction>
            <owl:onProperty rdf:resource="http://www.opengis.net/gml#hasboundingPolygon"/>
            <owl:someValuesFrom rdf:resource="http://www.opengis.net/gml#boundingPolygon"/>
         </owl:Restriction>
         <owl:Restriction>
            <owl:onProperty rdf:resource="http://www.opengis.net/gml#hasboundingPolygon"/>
            <owl:minCardinality rdf:datatype="http://www.w3.org/2001/XMLSchema#nonNegativeInteger">0</owl:minCardinality>
         </owl:Restriction>
      </owl:disjointUnionOf>
   </owl:Class>
   <owl:Class rdf:about="http://www.opengis.net/gml#AbstractDatumBaseType">
      <rdfs:comment>This is an abstract class</rdfs:comment>
      <rdfs:comment>Basic encoding for datum objects, simplifying and restricting the DefinitionType as needed. </rdfs:comment>
      <rdfs:subClassOf>
         <owl:Class>
            <owl:intersectionOf rdf:parseType="Collection">
               <owl:Restriction>
                  <owl:onProperty rdf:resource="http://www.opengis.net/gml#hasmetaDataProperty"/>
                  <owl:allValuesFrom rdf:resource="http://www.opengis.net/gml#metaDataProperty"/>
               </owl:Restriction>
               <owl:Restriction>
                  <owl:onProperty rdf:resource="http://www.opengis.net/gml#hasmetaDataProperty"/>
                  <owl:minCardinality rdf:datatype="http://www.w3.org/2001/XMLSchema#nonNegativeInteger">0</owl:minCardinality>
               </owl:Restriction>
               <owl:Restriction>
                  <owl:onProperty rdf:resource="http://www.opengis.net/gml#hasdatumName"/>
                  <owl:allValuesFrom rdf:resource="http://www.opengis.net/gml#datumName"/>
               </owl:Restriction>
            </owl:intersectionOf>
         </owl:Class>
      </rdfs:subClassOf>
      <rdfs:subClassOf>
         <owl:Class>
            <owl:intersectionOf rdf:parseType="Collection">
               <owl:Restriction>
                  <owl:onProperty rdf:resource="http://www.opengis.net/gml#hasid"/>
                  <owl:allValuesFrom rdf:resource="http://www.opengis.net/gml#id"/>
               </owl:Restriction>
            </owl:intersectionOf>
         </owl:Class>
      </rdfs:subClassOf>
      <rdfs:subClassOf rdf:resource="http://www.opengis.net/gml#DefinitionType"/>
   </owl:Class>
   <owl:Class rdf:about="http://www.opengis.net/gml#AbstractDatumType">
      <rdfs:comment>This is an abstract class</rdfs:comment>
      <rdfs:comment>A datum specifies the relationship of a coordinate system to the earth, thus creating a coordinate reference system. A datum uses a parameter or set of parameters that determine the location of the origin of the coordinate reference system. Each datum subtype can be associated with only specific types of coordinate systems. This abstract complexType shall not be used, extended, or restricted, in an Application Schema, to define a concrete subtype with a meaning equivalent to a concrete subtype specified in this document. </rdfs:comment>
      <rdfs:subClassOf>
         <owl:Class>
            <owl:intersectionOf rdf:parseType="Collection">
               <owl:Restriction>
                  <owl:onProperty rdf:resource="http://www.opengis.net/gml#hasdatumID"/>
                  <owl:allValuesFrom rdf:resource="http://www.opengis.net/gml#datumID"/>
               </owl:Restriction>
               <owl:Restriction>
                  <owl:onProperty rdf:resource="http://www.opengis.net/gml#hasdatumID"/>
                  <owl:minCardinality rdf:datatype="http://www.w3.org/2001/XMLSchema#nonNegativeInteger">0</owl:minCardinality>
               </owl:Restriction>
               <owl:Restriction>
                  <owl:onProperty rdf:resource="http://www.opengis.net/gml#hasremarks"/>
                  <owl:allValuesFrom rdf:resource="http://www.opengis.net/gml#remarks"/>
               </owl:Restriction>
               <owl:Restriction>
                  <owl:onProperty rdf:resource="http://www.opengis.net/gml#hasremarks"/>
                  <owl:minCardinality rdf:datatype="http://www.w3.org/2001/XMLSchema#nonNegativeInteger">0</owl:minCardinality>
               </owl:Restriction>
               <owl:Restriction>
                  <owl:onProperty rdf:resource="http://www.opengis.net/gml#hasanchorPoint"/>
                  <owl:allValuesFrom rdf:resource="http://www.opengis.net/gml#anchorPoint"/>
               </owl:Restriction>
               <owl:Restriction>
                  <owl:onProperty rdf:resource="http://www.opengis.net/gml#hasanchorPoint"/>
                  <owl:minCardinality rdf:datatype="http://www.w3.org/2001/XMLSchema#nonNegativeInteger">0</owl:minCardinality>
               </owl:Restriction>
               <owl:Restriction>
                  <owl:onProperty rdf:resource="http://www.opengis.net/gml#hasrealizationEpoch"/>
                  <owl:allValuesFrom rdf:resource="http://www.opengis.net/gml#realizationEpoch"/>
               </owl:Restriction>
               <owl:Restriction>
                  <owl:onProperty rdf:resource="http://www.opengis.net/gml#hasrealizationEpoch"/>
                  <owl:minCardinality rdf:datatype="http://www.w3.org/2001/XMLSchema#nonNegativeInteger">0</owl:minCardinality>
               </owl:Restriction>
               <owl:Restriction>
                  <owl:onProperty rdf:resource="http://www.opengis.net/gml#hasvalidArea"/>
                  <owl:allValuesFrom rdf:resource="http://www.opengis.net/gml#validArea"/>
               </owl:Restriction>
               <owl:Restriction>
                  <owl:onProperty rdf:resource="http://www.opengis.net/gml#hasvalidArea"/>
                  <owl:minCardinality rdf:datatype="http://www.w3.org/2001/XMLSchema#nonNegativeInteger">0</owl:minCardinality>
               </owl:Restriction>
               <owl:Restriction>
                  <owl:onProperty rdf:resource="http://www.opengis.net/gml#hasscope"/>
                  <owl:allValuesFrom rdf:resource="http://www.opengis.net/gml#scope"/>
               </owl:Restriction>
               <owl:Restriction>
                  <owl:onProperty rdf:resource="http://www.opengis.net/gml#hasscope"/>
                  <owl:minCardinality rdf:datatype="http://www.w3.org/2001/XMLSchema#nonNegativeInteger">0</owl:minCardinality>
               </owl:Restriction>
            </owl:intersectionOf>
         </owl:Class>
      </rdfs:subClassOf>
      <rdfs:subClassOf rdf:resource="http://www.opengis.net/gml#AbstractDatumBaseType"/>
   </owl:Class>
   <owl:Class rdf:about="http://www.opengis.net/gml#DatumRefType">
      <rdfs:comment>Association to a datum, either referencing or containing the definition of that datum. </rdfs:comment>
      <rdfs:subClassOf>
         <owl:Class>
            <owl:intersectionOf rdf:parseType="Collection">
               <owl:Restriction>
                  <owl:onProperty rdf:resource="http://www.opengis.net/gml#has_Datum"/>
                  <owl:allValuesFrom rdf:resource="http://www.opengis.net/gml#_Datum"/>
               </owl:Restriction>
            </owl:intersectionOf>
         </owl:Class>
      </rdfs:subClassOf>
   </owl:Class>
   <owl:Class rdf:about="http://www.opengis.net/gml#EngineeringDatumType">
      <rdfs:comment>An engineering datum defines the origin of an engineering coordinate reference system, and is used in a region around that origin. This origin can be fixed with respect to the earth (such as a defined point at a construction site), or be a defined point on a moving vehicle (such as on a ship or satellite). </rdfs:comment>
      <rdfs:subClassOf rdf:resource="http://www.opengis.net/gml#AbstractDatumType"/>
   </owl:Class>
   <owl:Class rdf:about="http://www.opengis.net/gml#EngineeringDatumRefType">
      <rdfs:comment>Association to an engineering datum, either referencing or containing the definition of that datum. </rdfs:comment>
      <rdfs:subClassOf>
         <owl:Class>
            <owl:intersectionOf rdf:parseType="Collection">
               <owl:Restriction>
                  <owl:onProperty rdf:resource="http://www.opengis.net/gml#hasEngineeringDatum"/>
                  <owl:allValuesFrom rdf:resource="http://www.opengis.net/gml#EngineeringDatum"/>
               </owl:Restriction>
            </owl:intersectionOf>
         </owl:Class>
      </rdfs:subClassOf>
   </owl:Class>
   <owl:Class rdf:about="http://www.opengis.net/gml#ImageDatumType">
      <rdfs:comment>An image datum defines the origin of an image coordinate reference system, and is used in a local context only. For more information, see OGC Abstract Specification Topic 2. </rdfs:comment>
      <rdfs:subClassOf>
         <owl:Class>
            <owl:intersectionOf rdf:parseType="Collection">
               <owl:Restriction>
                  <owl:onProperty rdf:resource="http://www.opengis.net/gml#haspixelInCell"/>
                  <owl:allValuesFrom rdf:resource="http://www.opengis.net/gml#pixelInCell"/>
               </owl:Restriction>
            </owl:intersectionOf>
         </owl:Class>
      </rdfs:subClassOf>
      <rdfs:subClassOf rdf:resource="http://www.opengis.net/gml#AbstractDatumType"/>
   </owl:Class>
   <owl:Class rdf:about="http://www.opengis.net/gml#PixelInCellType">
      <rdfs:comment>Specification of the way an image grid is associated with the image data attributes. </rdfs:comment>
      <rdfs:subClassOf>
         <owl:Restriction>
            <owl:onProperty rdf:resource="http://www.opengis.net/gml#hasPixelInCellTypeDatatype"/>
            <owl:someValuesFrom rdf:resource="http://www.opengis.net/gml#PixelInCellTypeDatatype"/>
         </owl:Restriction>
      </rdfs:subClassOf>
      <rdfs:subClassOf rdf:resource="http://www.opengis.net/gml#CodeType"/>
   </owl:Class>
   <rdfs:Datatype rdf:about="http://www.opengis.net/gml#PixelInCellTypeDatatype">
      <owl:equivalentClass rdf:resource="http://www.opengis.net/gml#CodeType"/>
   </rdfs:Datatype>
   <owl:DatatypeProperty rdf:about="http://www.opengis.net/gml#hasPixelInCellTypeDatatype">
      <rdfs:domain rdf:resource="http://www.opengis.net/gml#PixelInCellType"/>
      <rdfs:range rdf:resource="http://www.opengis.net/gml#PixelInCellTypeDatatype"/>
   </owl:DatatypeProperty>
   <owl:Class rdf:about="http://www.opengis.net/gml#ImageDatumRefType">
      <rdfs:comment>Association to an image datum, either referencing or containing the definition of that datum. </rdfs:comment>
      <rdfs:subClassOf>
         <owl:Class>
            <owl:intersectionOf rdf:parseType="Collection">
               <owl:Restriction>
                  <owl:onProperty rdf:resource="http://www.opengis.net/gml#hasImageDatum"/>
                  <owl:allValuesFrom rdf:resource="http://www.opengis.net/gml#ImageDatum"/>
               </owl:Restriction>
            </owl:intersectionOf>
         </owl:Class>
      </rdfs:subClassOf>
   </owl:Class>
   <owl:Class rdf:about="http://www.opengis.net/gml#VerticalDatumType">
      <rdfs:comment>A textual description and/or a set of parameters identifying a particular reference level surface used as a zero-height surface, including its position with respect to the Earth for any of the height types recognized by this standard. There are several types of Vertical Datums, and each may place constraints on the Coordinate Axis with which it is combined to create a Vertical CRS. </rdfs:comment>
      <rdfs:subClassOf>
         <owl:Class>
            <owl:intersectionOf rdf:parseType="Collection">
               <owl:Restriction>
                  <owl:onProperty rdf:resource="http://www.opengis.net/gml#hasverticalDatumType"/>
                  <owl:allValuesFrom rdf:resource="http://www.opengis.net/gml#verticalDatumType"/>
               </owl:Restriction>
               <owl:Restriction>
                  <owl:onProperty rdf:resource="http://www.opengis.net/gml#hasverticalDatumType"/>
                  <owl:minCardinality rdf:datatype="http://www.w3.org/2001/XMLSchema#nonNegativeInteger">0</owl:minCardinality>
               </owl:Restriction>
            </owl:intersectionOf>
         </owl:Class>
      </rdfs:subClassOf>
      <rdfs:subClassOf rdf:resource="http://www.opengis.net/gml#AbstractDatumType"/>
   </owl:Class>
   <owl:Class rdf:about="http://www.opengis.net/gml#VerticalDatumTypeType">
      <rdfs:comment>Type of a vertical datum. </rdfs:comment>
      <rdfs:subClassOf>
         <owl:Restriction>
            <owl:onProperty rdf:resource="http://www.opengis.net/gml#hasVerticalDatumTypeTypeDatatype"/>
            <owl:someValuesFrom rdf:resource="http://www.opengis.net/gml#VerticalDatumTypeTypeDatatype"/>
         </owl:Restriction>
      </rdfs:subClassOf>
      <rdfs:subClassOf rdf:resource="http://www.opengis.net/gml#CodeType"/>
   </owl:Class>
   <rdfs:Datatype rdf:about="http://www.opengis.net/gml#VerticalDatumTypeTypeDatatype">
      <owl:equivalentClass rdf:resource="http://www.opengis.net/gml#CodeType"/>
   </rdfs:Datatype>
   <owl:DatatypeProperty rdf:about="http://www.opengis.net/gml#hasVerticalDatumTypeTypeDatatype">
      <rdfs:domain rdf:resource="http://www.opengis.net/gml#VerticalDatumTypeType"/>
      <rdfs:range rdf:resource="http://www.opengis.net/gml#VerticalDatumTypeTypeDatatype"/>
   </owl:DatatypeProperty>
   <owl:Class rdf:about="http://www.opengis.net/gml#VerticalDatumRefType">
      <rdfs:comment>Association to a vertical datum, either referencing or containing the definition of that datum. </rdfs:comment>
      <rdfs:subClassOf>
         <owl:Class>
            <owl:intersectionOf rdf:parseType="Collection">
               <owl:Restriction>
                  <owl:onProperty rdf:resource="http://www.opengis.net/gml#hasVerticalDatum"/>
                  <owl:allValuesFrom rdf:resource="http://www.opengis.net/gml#VerticalDatum"/>
               </owl:Restriction>
            </owl:intersectionOf>
         </owl:Class>
      </rdfs:subClassOf>
   </owl:Class>
   <owl:Class rdf:about="http://www.opengis.net/gml#TemporalDatumBaseType">
      <rdfs:comment>This is an abstract class</rdfs:comment>
      <rdfs:comment>Partially defines the origin of a temporal coordinate reference system. This type restricts the AbstractDatumType to remove the "anchorPoint" and "realizationEpoch" elements. </rdfs:comment>
      <rdfs:subClassOf>
         <owl:Class>
            <owl:intersectionOf rdf:parseType="Collection">
               <owl:Restriction>
                  <owl:onProperty rdf:resource="http://www.opengis.net/gml#hasmetaDataProperty"/>
                  <owl:allValuesFrom rdf:resource="http://www.opengis.net/gml#metaDataProperty"/>
               </owl:Restriction>
               <owl:Restriction>
                  <owl:onProperty rdf:resource="http://www.opengis.net/gml#hasmetaDataProperty"/>
                  <owl:minCardinality rdf:datatype="http://www.w3.org/2001/XMLSchema#nonNegativeInteger">0</owl:minCardinality>
               </owl:Restriction>
               <owl:Restriction>
                  <owl:onProperty rdf:resource="http://www.opengis.net/gml#hasdatumName"/>
                  <owl:allValuesFrom rdf:resource="http://www.opengis.net/gml#datumName"/>
               </owl:Restriction>
               <owl:Restriction>
                  <owl:onProperty rdf:resource="http://www.opengis.net/gml#hasdatumID"/>
                  <owl:allValuesFrom rdf:resource="http://www.opengis.net/gml#datumID"/>
               </owl:Restriction>
               <owl:Restriction>
                  <owl:onProperty rdf:resource="http://www.opengis.net/gml#hasdatumID"/>
                  <owl:minCardinality rdf:datatype="http://www.w3.org/2001/XMLSchema#nonNegativeInteger">0</owl:minCardinality>
               </owl:Restriction>
               <owl:Restriction>
                  <owl:onProperty rdf:resource="http://www.opengis.net/gml#hasvalidArea"/>
                  <owl:allValuesFrom rdf:resource="http://www.opengis.net/gml#validArea"/>
               </owl:Restriction>
               <owl:Restriction>
                  <owl:onProperty rdf:resource="http://www.opengis.net/gml#hasvalidArea"/>
                  <owl:minCardinality rdf:datatype="http://www.w3.org/2001/XMLSchema#nonNegativeInteger">0</owl:minCardinality>
               </owl:Restriction>
               <owl:Restriction>
                  <owl:onProperty rdf:resource="http://www.opengis.net/gml#hasscope"/>
                  <owl:allValuesFrom rdf:resource="http://www.opengis.net/gml#scope"/>
               </owl:Restriction>
               <owl:Restriction>
                  <owl:onProperty rdf:resource="http://www.opengis.net/gml#hasscope"/>
                  <owl:minCardinality rdf:datatype="http://www.w3.org/2001/XMLSchema#nonNegativeInteger">0</owl:minCardinality>
               </owl:Restriction>
            </owl:intersectionOf>
         </owl:Class>
      </rdfs:subClassOf>
      <rdfs:subClassOf>
         <owl:Class>
            <owl:intersectionOf rdf:parseType="Collection">
               <owl:Restriction>
                  <owl:onProperty rdf:resource="http://www.opengis.net/gml#hasid"/>
                  <owl:allValuesFrom rdf:resource="http://www.opengis.net/gml#id"/>
               </owl:Restriction>
            </owl:intersectionOf>
         </owl:Class>
      </rdfs:subClassOf>
      <rdfs:subClassOf rdf:resource="http://www.opengis.net/gml#AbstractDatumType"/>
   </owl:Class>
   <owl:Class rdf:about="http://www.opengis.net/gml#TemporalDatumType">
      <rdfs:comment>Defines the origin of a temporal coordinate reference system. This type extends the TemporalDatumRestrictionType to add the "origin" element with the dateTime type. </rdfs:comment>
      <rdfs:subClassOf>
         <owl:Class>
            <owl:intersectionOf rdf:parseType="Collection">
               <owl:Restriction>
                  <owl:onProperty rdf:resource="http://www.opengis.net/gml#hasorigin"/>
                  <owl:allValuesFrom rdf:resource="http://www.opengis.net/gml#origin"/>
               </owl:Restriction>
            </owl:intersectionOf>
         </owl:Class>
      </rdfs:subClassOf>
      <rdfs:subClassOf rdf:resource="http://www.opengis.net/gml#TemporalDatumBaseType"/>
   </owl:Class>
   <owl:Class rdf:about="http://www.opengis.net/gml#TemporalDatumRefType">
      <rdfs:comment>Association to a temporal datum, either referencing or containing the definition of that datum. </rdfs:comment>
      <rdfs:subClassOf>
         <owl:Class>
            <owl:intersectionOf rdf:parseType="Collection">
               <owl:Restriction>
                  <owl:onProperty rdf:resource="http://www.opengis.net/gml#hasTemporalDatum"/>
                  <owl:allValuesFrom rdf:resource="http://www.opengis.net/gml#TemporalDatum"/>
               </owl:Restriction>
            </owl:intersectionOf>
         </owl:Class>
      </rdfs:subClassOf>
   </owl:Class>
   <owl:Class rdf:about="http://www.opengis.net/gml#GeodeticDatumType">
      <rdfs:comment>A geodetic datum defines the precise location and orientation in 3-dimensional space of a defined ellipsoid (or sphere) that approximates the shape of the earth, or of a Cartesian coordinate system centered in this ellipsoid (or sphere). </rdfs:comment>
      <rdfs:subClassOf>
         <owl:Class>
            <owl:intersectionOf rdf:parseType="Collection">
               <owl:Restriction>
                  <owl:onProperty rdf:resource="http://www.opengis.net/gml#hasusesPrimeMeridian"/>
                  <owl:allValuesFrom rdf:resource="http://www.opengis.net/gml#usesPrimeMeridian"/>
               </owl:Restriction>
               <owl:Restriction>
                  <owl:onProperty rdf:resource="http://www.opengis.net/gml#hasusesEllipsoid"/>
                  <owl:allValuesFrom rdf:resource="http://www.opengis.net/gml#usesEllipsoid"/>
               </owl:Restriction>
            </owl:intersectionOf>
         </owl:Class>
      </rdfs:subClassOf>
      <rdfs:subClassOf rdf:resource="http://www.opengis.net/gml#AbstractDatumType"/>
   </owl:Class>
   <owl:Class rdf:about="http://www.opengis.net/gml#GeodeticDatumRefType">
      <rdfs:comment>Association to a geodetic datum, either referencing or containing the definition of that datum. </rdfs:comment>
      <rdfs:subClassOf>
         <owl:Class>
            <owl:intersectionOf rdf:parseType="Collection">
               <owl:Restriction>
                  <owl:onProperty rdf:resource="http://www.opengis.net/gml#hasGeodeticDatum"/>
                  <owl:allValuesFrom rdf:resource="http://www.opengis.net/gml#GeodeticDatum"/>
               </owl:Restriction>
            </owl:intersectionOf>
         </owl:Class>
      </rdfs:subClassOf>
   </owl:Class>
   <owl:Class rdf:about="http://www.opengis.net/gml#PrimeMeridianBaseType">
      <rdfs:comment>This is an abstract class</rdfs:comment>
      <rdfs:comment>Basic encoding for prime meridian objects, simplifying and restricting the DefinitionType as needed. </rdfs:comment>
      <rdfs:subClassOf>
         <owl:Class>
            <owl:intersectionOf rdf:parseType="Collection">
               <owl:Restriction>
                  <owl:onProperty rdf:resource="http://www.opengis.net/gml#hasmetaDataProperty"/>
                  <owl:allValuesFrom rdf:resource="http://www.opengis.net/gml#metaDataProperty"/>
               </owl:Restriction>
               <owl:Restriction>
                  <owl:onProperty rdf:resource="http://www.opengis.net/gml#hasmetaDataProperty"/>
                  <owl:minCardinality rdf:datatype="http://www.w3.org/2001/XMLSchema#nonNegativeInteger">0</owl:minCardinality>
               </owl:Restriction>
               <owl:Restriction>
                  <owl:onProperty rdf:resource="http://www.opengis.net/gml#hasmeridianName"/>
                  <owl:allValuesFrom rdf:resource="http://www.opengis.net/gml#meridianName"/>
               </owl:Restriction>
            </owl:intersectionOf>
         </owl:Class>
      </rdfs:subClassOf>
      <rdfs:subClassOf>
         <owl:Class>
            <owl:intersectionOf rdf:parseType="Collection">
               <owl:Restriction>
                  <owl:onProperty rdf:resource="http://www.opengis.net/gml#hasid"/>
                  <owl:allValuesFrom rdf:resource="http://www.opengis.net/gml#id"/>
               </owl:Restriction>
            </owl:intersectionOf>
         </owl:Class>
      </rdfs:subClassOf>
      <rdfs:subClassOf rdf:resource="http://www.opengis.net/gml#DefinitionType"/>
   </owl:Class>
   <owl:Class rdf:about="http://www.opengis.net/gml#PrimeMeridianType">
      <rdfs:comment>A prime meridian defines the origin from which longitude values are determined.</rdfs:comment>
      <rdfs:subClassOf>
         <owl:Class>
            <owl:intersectionOf rdf:parseType="Collection">
               <owl:Restriction>
                  <owl:onProperty rdf:resource="http://www.opengis.net/gml#hasmeridianID"/>
                  <owl:allValuesFrom rdf:resource="http://www.opengis.net/gml#meridianID"/>
               </owl:Restriction>
               <owl:Restriction>
                  <owl:onProperty rdf:resource="http://www.opengis.net/gml#hasmeridianID"/>
                  <owl:minCardinality rdf:datatype="http://www.w3.org/2001/XMLSchema#nonNegativeInteger">0</owl:minCardinality>
               </owl:Restriction>
               <owl:Restriction>
                  <owl:onProperty rdf:resource="http://www.opengis.net/gml#hasremarks"/>
                  <owl:allValuesFrom rdf:resource="http://www.opengis.net/gml#remarks"/>
               </owl:Restriction>
               <owl:Restriction>
                  <owl:onProperty rdf:resource="http://www.opengis.net/gml#hasremarks"/>
                  <owl:minCardinality rdf:datatype="http://www.w3.org/2001/XMLSchema#nonNegativeInteger">0</owl:minCardinality>
               </owl:Restriction>
               <owl:Restriction>
                  <owl:onProperty rdf:resource="http://www.opengis.net/gml#hasgreenwichLongitude"/>
                  <owl:allValuesFrom rdf:resource="http://www.opengis.net/gml#greenwichLongitude"/>
               </owl:Restriction>
            </owl:intersectionOf>
         </owl:Class>
      </rdfs:subClassOf>
      <rdfs:subClassOf rdf:resource="http://www.opengis.net/gml#PrimeMeridianBaseType"/>
   </owl:Class>
   <owl:Class rdf:about="http://www.opengis.net/gml#PrimeMeridianRefType">
      <rdfs:comment>Association to a prime meridian, either referencing or containing the definition of that meridian. </rdfs:comment>
      <rdfs:subClassOf>
         <owl:Class>
            <owl:intersectionOf rdf:parseType="Collection">
               <owl:Restriction>
                  <owl:onProperty rdf:resource="http://www.opengis.net/gml#hasPrimeMeridian"/>
                  <owl:allValuesFrom rdf:resource="http://www.opengis.net/gml#PrimeMeridian"/>
               </owl:Restriction>
            </owl:intersectionOf>
         </owl:Class>
      </rdfs:subClassOf>
   </owl:Class>
   <owl:Class rdf:about="http://www.opengis.net/gml#EllipsoidBaseType">
      <rdfs:comment>This is an abstract class</rdfs:comment>
      <rdfs:comment>Basic encoding for ellipsoid objects, simplifying and restricting the DefinitionType as needed. </rdfs:comment>
      <rdfs:subClassOf>
         <owl:Class>
            <owl:intersectionOf rdf:parseType="Collection">
               <owl:Restriction>
                  <owl:onProperty rdf:resource="http://www.opengis.net/gml#hasmetaDataProperty"/>
                  <owl:allValuesFrom rdf:resource="http://www.opengis.net/gml#metaDataProperty"/>
               </owl:Restriction>
               <owl:Restriction>
                  <owl:onProperty rdf:resource="http://www.opengis.net/gml#hasmetaDataProperty"/>
                  <owl:minCardinality rdf:datatype="http://www.w3.org/2001/XMLSchema#nonNegativeInteger">0</owl:minCardinality>
               </owl:Restriction>
               <owl:Restriction>
                  <owl:onProperty rdf:resource="http://www.opengis.net/gml#hasellipsoidName"/>
                  <owl:allValuesFrom rdf:resource="http://www.opengis.net/gml#ellipsoidName"/>
               </owl:Restriction>
            </owl:intersectionOf>
         </owl:Class>
      </rdfs:subClassOf>
      <rdfs:subClassOf>
         <owl:Class>
            <owl:intersectionOf rdf:parseType="Collection">
               <owl:Restriction>
                  <owl:onProperty rdf:resource="http://www.opengis.net/gml#hasid"/>
                  <owl:allValuesFrom rdf:resource="http://www.opengis.net/gml#id"/>
               </owl:Restriction>
            </owl:intersectionOf>
         </owl:Class>
      </rdfs:subClassOf>
      <rdfs:subClassOf rdf:resource="http://www.opengis.net/gml#DefinitionType"/>
   </owl:Class>
   <owl:Class rdf:about="http://www.opengis.net/gml#EllipsoidType">
      <rdfs:comment>An ellipsoid is a geometric figure that can be used to describe the approximate shape of the earth. In mathematical terms, it is a surface formed by the rotation of an ellipse about its minor axis.</rdfs:comment>
      <rdfs:subClassOf>
         <owl:Class>
            <owl:intersectionOf rdf:parseType="Collection">
               <owl:Restriction>
                  <owl:onProperty rdf:resource="http://www.opengis.net/gml#hasellipsoidID"/>
                  <owl:allValuesFrom rdf:resource="http://www.opengis.net/gml#ellipsoidID"/>
               </owl:Restriction>
               <owl:Restriction>
                  <owl:onProperty rdf:resource="http://www.opengis.net/gml#hasellipsoidID"/>
                  <owl:minCardinality rdf:datatype="http://www.w3.org/2001/XMLSchema#nonNegativeInteger">0</owl:minCardinality>
               </owl:Restriction>
               <owl:Restriction>
                  <owl:onProperty rdf:resource="http://www.opengis.net/gml#hasremarks"/>
                  <owl:allValuesFrom rdf:resource="http://www.opengis.net/gml#remarks"/>
               </owl:Restriction>
               <owl:Restriction>
                  <owl:onProperty rdf:resource="http://www.opengis.net/gml#hasremarks"/>
                  <owl:minCardinality rdf:datatype="http://www.w3.org/2001/XMLSchema#nonNegativeInteger">0</owl:minCardinality>
               </owl:Restriction>
               <owl:Restriction>
                  <owl:onProperty rdf:resource="http://www.opengis.net/gml#hassemiMajorAxis"/>
                  <owl:allValuesFrom rdf:resource="http://www.opengis.net/gml#semiMajorAxis"/>
               </owl:Restriction>
               <owl:Restriction>
                  <owl:onProperty rdf:resource="http://www.opengis.net/gml#hassecondDefiningParameter"/>
                  <owl:allValuesFrom rdf:resource="http://www.opengis.net/gml#secondDefiningParameter"/>
               </owl:Restriction>
            </owl:intersectionOf>
         </owl:Class>
      </rdfs:subClassOf>
      <rdfs:subClassOf rdf:resource="http://www.opengis.net/gml#EllipsoidBaseType"/>
   </owl:Class>
   <owl:Class rdf:about="http://www.opengis.net/gml#EllipsoidRefType">
      <rdfs:comment>Association to an ellipsoid, either referencing or containing the definition of that ellipsoid. </rdfs:comment>
      <rdfs:subClassOf>
         <owl:Class>
            <owl:intersectionOf rdf:parseType="Collection">
               <owl:Restriction>
                  <owl:onProperty rdf:resource="http://www.opengis.net/gml#hasEllipsoid"/>
                  <owl:allValuesFrom rdf:resource="http://www.opengis.net/gml#Ellipsoid"/>
               </owl:Restriction>
            </owl:intersectionOf>
         </owl:Class>
      </rdfs:subClassOf>
   </owl:Class>
   <owl:Class rdf:about="http://www.opengis.net/gml#SecondDefiningParameterType">
      <rdfs:comment>Definition of the second parameter that defines the shape of an ellipsoid. An ellipsoid requires two defining parameters: semi-major axis and inverse flattening or semi-major axis and semi-minor axis. When the reference body is a sphere rather than an ellipsoid, only a single defining parameter is required, namely the radius of the sphere; in that case, the semi-major axis "degenerates" into the radius of the sphere.</rdfs:comment>
      <owl:disjointUnionOf rdf:parseType="Collection">
         <owl:Restriction>
            <owl:onProperty rdf:resource="http://www.opengis.net/gml#hasinverseFlattening"/>
            <owl:someValuesFrom rdf:resource="http://www.opengis.net/gml#inverseFlattening"/>
         </owl:Restriction>
         <owl:Restriction>
            <owl:onProperty rdf:resource="http://www.opengis.net/gml#hassemiMinorAxis"/>
            <owl:someValuesFrom rdf:resource="http://www.opengis.net/gml#semiMinorAxis"/>
         </owl:Restriction>
         <owl:Restriction>
            <owl:onProperty rdf:resource="http://www.opengis.net/gml#hasisSphere"/>
            <owl:someValuesFrom rdf:resource="http://www.opengis.net/gml#isSphere"/>
         </owl:Restriction>
      </owl:disjointUnionOf>
   </owl:Class>
   <owl:Class rdf:about="http://www.opengis.net/gml#AbstractCoordinateOperationBaseType">
      <rdfs:comment>This is an abstract class</rdfs:comment>
      <rdfs:comment>Basic encoding for coordinate operation objects, simplifying and restricting the DefinitionType as needed. </rdfs:comment>
      <rdfs:subClassOf>
         <owl:Class>
            <owl:intersectionOf rdf:parseType="Collection">
               <owl:Restriction>
                  <owl:onProperty rdf:resource="http://www.opengis.net/gml#hasmetaDataProperty"/>
                  <owl:allValuesFrom rdf:resource="http://www.opengis.net/gml#metaDataProperty"/>
               </owl:Restriction>
               <owl:Restriction>
                  <owl:onProperty rdf:resource="http://www.opengis.net/gml#hasmetaDataProperty"/>
                  <owl:minCardinality rdf:datatype="http://www.w3.org/2001/XMLSchema#nonNegativeInteger">0</owl:minCardinality>
               </owl:Restriction>
               <owl:Restriction>
                  <owl:onProperty rdf:resource="http://www.opengis.net/gml#hascoordinateOperationName"/>
                  <owl:allValuesFrom rdf:resource="http://www.opengis.net/gml#coordinateOperationName"/>
               </owl:Restriction>
            </owl:intersectionOf>
         </owl:Class>
      </rdfs:subClassOf>
      <rdfs:subClassOf>
         <owl:Class>
            <owl:intersectionOf rdf:parseType="Collection">
               <owl:Restriction>
                  <owl:onProperty rdf:resource="http://www.opengis.net/gml#hasid"/>
                  <owl:allValuesFrom rdf:resource="http://www.opengis.net/gml#id"/>
               </owl:Restriction>
            </owl:intersectionOf>
         </owl:Class>
      </rdfs:subClassOf>
      <rdfs:subClassOf rdf:resource="http://www.opengis.net/gml#DefinitionType"/>
   </owl:Class>
   <owl:Class rdf:about="http://www.opengis.net/gml#AbstractCoordinateOperationType">
      <rdfs:comment>This is an abstract class</rdfs:comment>
      <rdfs:comment>A mathematical operation on coordinates that transforms or converts coordinates to another coordinate reference system. Many but not all coordinate operations (from CRS A to CRS B) also uniquely define the inverse operation (from CRS B to CRS A). In some cases, the operation method algorithm for the inverse operation is the same as for the forward algorithm, but the signs of some operation parameter values must be reversed. In other cases, different algorithms are required for the forward and inverse operations, but the same operation parameter values are used. If (some) entirely different parameter values are needed, a different coordinate operation shall be defined.</rdfs:comment>
      <rdfs:subClassOf>
         <owl:Class>
            <owl:intersectionOf rdf:parseType="Collection">
               <owl:Restriction>
                  <owl:onProperty rdf:resource="http://www.opengis.net/gml#hascoordinateOperationID"/>
                  <owl:allValuesFrom rdf:resource="http://www.opengis.net/gml#coordinateOperationID"/>
               </owl:Restriction>
               <owl:Restriction>
                  <owl:onProperty rdf:resource="http://www.opengis.net/gml#hascoordinateOperationID"/>
                  <owl:minCardinality rdf:datatype="http://www.w3.org/2001/XMLSchema#nonNegativeInteger">0</owl:minCardinality>
               </owl:Restriction>
               <owl:Restriction>
                  <owl:onProperty rdf:resource="http://www.opengis.net/gml#hasremarks"/>
                  <owl:allValuesFrom rdf:resource="http://www.opengis.net/gml#remarks"/>
               </owl:Restriction>
               <owl:Restriction>
                  <owl:onProperty rdf:resource="http://www.opengis.net/gml#hasremarks"/>
                  <owl:minCardinality rdf:datatype="http://www.w3.org/2001/XMLSchema#nonNegativeInteger">0</owl:minCardinality>
               </owl:Restriction>
               <owl:Restriction>
                  <owl:onProperty rdf:resource="http://www.opengis.net/gml#hasoperationVersion"/>
                  <owl:allValuesFrom rdf:resource="http://www.opengis.net/gml#operationVersion"/>
               </owl:Restriction>
               <owl:Restriction>
                  <owl:onProperty rdf:resource="http://www.opengis.net/gml#hasoperationVersion"/>
                  <owl:minCardinality rdf:datatype="http://www.w3.org/2001/XMLSchema#nonNegativeInteger">0</owl:minCardinality>
               </owl:Restriction>
               <owl:Restriction>
                  <owl:onProperty rdf:resource="http://www.opengis.net/gml#hasvalidArea"/>
                  <owl:allValuesFrom rdf:resource="http://www.opengis.net/gml#validArea"/>
               </owl:Restriction>
               <owl:Restriction>
                  <owl:onProperty rdf:resource="http://www.opengis.net/gml#hasvalidArea"/>
                  <owl:minCardinality rdf:datatype="http://www.w3.org/2001/XMLSchema#nonNegativeInteger">0</owl:minCardinality>
               </owl:Restriction>
               <owl:Restriction>
                  <owl:onProperty rdf:resource="http://www.opengis.net/gml#hasscope"/>
                  <owl:allValuesFrom rdf:resource="http://www.opengis.net/gml#scope"/>
               </owl:Restriction>
               <owl:Restriction>
                  <owl:onProperty rdf:resource="http://www.opengis.net/gml#hasscope"/>
                  <owl:minCardinality rdf:datatype="http://www.w3.org/2001/XMLSchema#nonNegativeInteger">0</owl:minCardinality>
               </owl:Restriction>
               <owl:Restriction>
                  <owl:onProperty rdf:resource="http://www.opengis.net/gml#has_positionalAccuracy"/>
                  <owl:allValuesFrom rdf:resource="http://www.opengis.net/gml#_positionalAccuracy"/>
               </owl:Restriction>
               <owl:Restriction>
                  <owl:onProperty rdf:resource="http://www.opengis.net/gml#has_positionalAccuracy"/>
                  <owl:minCardinality rdf:datatype="http://www.w3.org/2001/XMLSchema#nonNegativeInteger">0</owl:minCardinality>
               </owl:Restriction>
               <owl:Restriction>
                  <owl:onProperty rdf:resource="http://www.opengis.net/gml#hassourceCRS"/>
                  <owl:allValuesFrom rdf:resource="http://www.opengis.net/gml#sourceCRS"/>
               </owl:Restriction>
               <owl:Restriction>
                  <owl:onProperty rdf:resource="http://www.opengis.net/gml#hassourceCRS"/>
                  <owl:minCardinality rdf:datatype="http://www.w3.org/2001/XMLSchema#nonNegativeInteger">0</owl:minCardinality>
               </owl:Restriction>
               <owl:Restriction>
                  <owl:onProperty rdf:resource="http://www.opengis.net/gml#hastargetCRS"/>
                  <owl:allValuesFrom rdf:resource="http://www.opengis.net/gml#targetCRS"/>
               </owl:Restriction>
               <owl:Restriction>
                  <owl:onProperty rdf:resource="http://www.opengis.net/gml#hastargetCRS"/>
                  <owl:minCardinality rdf:datatype="http://www.w3.org/2001/XMLSchema#nonNegativeInteger">0</owl:minCardinality>
               </owl:Restriction>
            </owl:intersectionOf>
         </owl:Class>
      </rdfs:subClassOf>
      <rdfs:subClassOf rdf:resource="http://www.opengis.net/gml#AbstractCoordinateOperationBaseType"/>
   </owl:Class>
   <owl:Class rdf:about="http://www.opengis.net/gml#CoordinateOperationRefType">
      <rdfs:comment>Association to a coordinate operation, either referencing or containing the definition of that coordinate operation. </rdfs:comment>
      <rdfs:subClassOf>
         <owl:Class>
            <owl:intersectionOf rdf:parseType="Collection">
               <owl:Restriction>
                  <owl:onProperty rdf:resource="http://www.opengis.net/gml#has_CoordinateOperation"/>
                  <owl:allValuesFrom rdf:resource="http://www.opengis.net/gml#_CoordinateOperation"/>
               </owl:Restriction>
            </owl:intersectionOf>
         </owl:Class>
      </rdfs:subClassOf>
   </owl:Class>
   <owl:Class rdf:about="http://www.opengis.net/gml#ConcatenatedOperationType">
      <rdfs:comment>An ordered sequence of two or more single coordinate operations. The sequence of operations is constrained by the requirement that the source coordinate reference system of step (n+1) must be the same as the target coordinate reference system of step (n). The source coordinate reference system of the first step and the target coordinate reference system of the last step are the source and target coordinate reference system associated with the concatenated operation. Instead of a forward operation, an inverse operation may be used for one or more of the operation steps mentioned above, if the inverse operation is uniquely defined by the forward operation.</rdfs:comment>
      <rdfs:subClassOf>
         <owl:Class>
            <owl:intersectionOf rdf:parseType="Collection">
               <owl:Restriction>
                  <owl:onProperty rdf:resource="http://www.opengis.net/gml#hasusesSingleOperation"/>
                  <owl:allValuesFrom rdf:resource="http://www.opengis.net/gml#usesSingleOperation"/>
               </owl:Restriction>
               <owl:Restriction>
                  <owl:onProperty rdf:resource="http://www.opengis.net/gml#hasusesSingleOperation"/>
                  <owl:minCardinality rdf:datatype="http://www.w3.org/2001/XMLSchema#nonNegativeInteger">2</owl:minCardinality>
               </owl:Restriction>
            </owl:intersectionOf>
         </owl:Class>
      </rdfs:subClassOf>
      <rdfs:subClassOf rdf:resource="http://www.opengis.net/gml#AbstractCoordinateOperationType"/>
   </owl:Class>
   <owl:Class rdf:about="http://www.opengis.net/gml#ConcatenatedOperationRefType">
      <rdfs:comment>Association to a concatenated operation, either referencing or containing the definition of that concatenated operation. </rdfs:comment>
      <rdfs:subClassOf>
         <owl:Class>
            <owl:intersectionOf rdf:parseType="Collection">
               <owl:Restriction>
                  <owl:onProperty rdf:resource="http://www.opengis.net/gml#hasConcatenatedOperation"/>
                  <owl:allValuesFrom rdf:resource="http://www.opengis.net/gml#ConcatenatedOperation"/>
               </owl:Restriction>
            </owl:intersectionOf>
         </owl:Class>
      </rdfs:subClassOf>
   </owl:Class>
   <owl:Class rdf:about="http://www.opengis.net/gml#SingleOperationRefType">
      <rdfs:comment>Association to a single operation, either referencing or containing the definition of that single operation. </rdfs:comment>
      <rdfs:subClassOf>
         <owl:Class>
            <owl:intersectionOf rdf:parseType="Collection">
               <owl:Restriction>
                  <owl:onProperty rdf:resource="http://www.opengis.net/gml#has_SingleOperation"/>
                  <owl:allValuesFrom rdf:resource="http://www.opengis.net/gml#_SingleOperation"/>
               </owl:Restriction>
            </owl:intersectionOf>
         </owl:Class>
      </rdfs:subClassOf>
   </owl:Class>
   <owl:Class rdf:about="http://www.opengis.net/gml#PassThroughOperationType">
      <rdfs:comment>A pass-through operation specifies that a subset of a coordinate tuple is subject to a specific coordinate operation. </rdfs:comment>
      <rdfs:subClassOf>
         <owl:Class>
            <owl:intersectionOf rdf:parseType="Collection">
               <owl:Restriction>
                  <owl:onProperty rdf:resource="http://www.opengis.net/gml#hasmodifiedCoordinate"/>
                  <owl:allValuesFrom rdf:resource="http://www.opengis.net/gml#modifiedCoordinate"/>
               </owl:Restriction>
               <owl:Restriction>
                  <owl:onProperty rdf:resource="http://www.opengis.net/gml#hasusesOperation"/>
                  <owl:allValuesFrom rdf:resource="http://www.opengis.net/gml#usesOperation"/>
               </owl:Restriction>
            </owl:intersectionOf>
         </owl:Class>
      </rdfs:subClassOf>
      <rdfs:subClassOf rdf:resource="http://www.opengis.net/gml#AbstractCoordinateOperationType"/>
   </owl:Class>
   <owl:Class rdf:about="http://www.opengis.net/gml#PassThroughOperationRefType">
      <rdfs:comment>Association to a pass through operation, either referencing or containing the definition of that pass through operation. </rdfs:comment>
      <rdfs:subClassOf>
         <owl:Class>
            <owl:intersectionOf rdf:parseType="Collection">
               <owl:Restriction>
                  <owl:onProperty rdf:resource="http://www.opengis.net/gml#hasPassThroughOperation"/>
                  <owl:allValuesFrom rdf:resource="http://www.opengis.net/gml#PassThroughOperation"/>
               </owl:Restriction>
            </owl:intersectionOf>
         </owl:Class>
      </rdfs:subClassOf>
   </owl:Class>
   <owl:Class rdf:about="http://www.opengis.net/gml#OperationRefType">
      <rdfs:comment>Association to an abstract operation, either referencing or containing the definition of that operation. </rdfs:comment>
      <rdfs:subClassOf>
         <owl:Class>
            <owl:intersectionOf rdf:parseType="Collection">
               <owl:Restriction>
                  <owl:onProperty rdf:resource="http://www.opengis.net/gml#has_Operation"/>
                  <owl:allValuesFrom rdf:resource="http://www.opengis.net/gml#_Operation"/>
               </owl:Restriction>
            </owl:intersectionOf>
         </owl:Class>
      </rdfs:subClassOf>
   </owl:Class>
   <owl:Class rdf:about="http://www.opengis.net/gml#AbstractGeneralConversionType">
      <rdfs:comment>This is an abstract class</rdfs:comment>
      <rdfs:comment>An abstract operation on coordinates that does not include any change of datum. The best-known example of a coordinate conversion is a map projection. The parameters describing coordinate conversions are defined rather than empirically derived. Note that some conversions have no parameters.

This abstract complexType is expected to be extended for well-known operation methods with many Conversion instances, in Application Schemas that define operation-method-specialized element names and contents. This conversion uses an operation method, usually with associated parameter values. However, operation methods and parameter values are directly associated with concrete subtypes, not with this abstract type. All concrete types derived from this type shall extend this type to include a "usesMethod" element that references the "OperationMethod" element. Similarly, all concrete types derived from this type shall extend this type to include zero or more elements each named "uses...Value" that each use the type of an element substitutable for the "_generalParameterValue" element. </rdfs:comment>
      <rdfs:subClassOf>
         <owl:Class>
            <owl:intersectionOf rdf:parseType="Collection">
               <owl:Restriction>
                  <owl:onProperty rdf:resource="http://www.opengis.net/gml#hasmetaDataProperty"/>
                  <owl:allValuesFrom rdf:resource="http://www.opengis.net/gml#metaDataProperty"/>
               </owl:Restriction>
               <owl:Restriction>
                  <owl:onProperty rdf:resource="http://www.opengis.net/gml#hasmetaDataProperty"/>
                  <owl:minCardinality rdf:datatype="http://www.w3.org/2001/XMLSchema#nonNegativeInteger">0</owl:minCardinality>
               </owl:Restriction>
               <owl:Restriction>
                  <owl:onProperty rdf:resource="http://www.opengis.net/gml#hascoordinateOperationName"/>
                  <owl:allValuesFrom rdf:resource="http://www.opengis.net/gml#coordinateOperationName"/>
               </owl:Restriction>
               <owl:Restriction>
                  <owl:onProperty rdf:resource="http://www.opengis.net/gml#hascoordinateOperationID"/>
                  <owl:allValuesFrom rdf:resource="http://www.opengis.net/gml#coordinateOperationID"/>
               </owl:Restriction>
               <owl:Restriction>
                  <owl:onProperty rdf:resource="http://www.opengis.net/gml#hascoordinateOperationID"/>
                  <owl:minCardinality rdf:datatype="http://www.w3.org/2001/XMLSchema#nonNegativeInteger">0</owl:minCardinality>
               </owl:Restriction>
               <owl:Restriction>
                  <owl:onProperty rdf:resource="http://www.opengis.net/gml#hasremarks"/>
                  <owl:allValuesFrom rdf:resource="http://www.opengis.net/gml#remarks"/>
               </owl:Restriction>
               <owl:Restriction>
                  <owl:onProperty rdf:resource="http://www.opengis.net/gml#hasremarks"/>
                  <owl:minCardinality rdf:datatype="http://www.w3.org/2001/XMLSchema#nonNegativeInteger">0</owl:minCardinality>
               </owl:Restriction>
               <owl:Restriction>
                  <owl:onProperty rdf:resource="http://www.opengis.net/gml#hasvalidArea"/>
                  <owl:allValuesFrom rdf:resource="http://www.opengis.net/gml#validArea"/>
               </owl:Restriction>
               <owl:Restriction>
                  <owl:onProperty rdf:resource="http://www.opengis.net/gml#hasvalidArea"/>
                  <owl:minCardinality rdf:datatype="http://www.w3.org/2001/XMLSchema#nonNegativeInteger">0</owl:minCardinality>
               </owl:Restriction>
               <owl:Restriction>
                  <owl:onProperty rdf:resource="http://www.opengis.net/gml#hasscope"/>
                  <owl:allValuesFrom rdf:resource="http://www.opengis.net/gml#scope"/>
               </owl:Restriction>
               <owl:Restriction>
                  <owl:onProperty rdf:resource="http://www.opengis.net/gml#hasscope"/>
                  <owl:minCardinality rdf:datatype="http://www.w3.org/2001/XMLSchema#nonNegativeInteger">0</owl:minCardinality>
               </owl:Restriction>
               <owl:Restriction>
                  <owl:onProperty rdf:resource="http://www.opengis.net/gml#has_positionalAccuracy"/>
                  <owl:allValuesFrom rdf:resource="http://www.opengis.net/gml#_positionalAccuracy"/>
               </owl:Restriction>
               <owl:Restriction>
                  <owl:onProperty rdf:resource="http://www.opengis.net/gml#has_positionalAccuracy"/>
                  <owl:minCardinality rdf:datatype="http://www.w3.org/2001/XMLSchema#nonNegativeInteger">0</owl:minCardinality>
               </owl:Restriction>
            </owl:intersectionOf>
         </owl:Class>
      </rdfs:subClassOf>
      <rdfs:subClassOf>
         <owl:Class>
            <owl:intersectionOf rdf:parseType="Collection">
               <owl:Restriction>
                  <owl:onProperty rdf:resource="http://www.opengis.net/gml#hasid"/>
                  <owl:allValuesFrom rdf:resource="http://www.opengis.net/gml#id"/>
               </owl:Restriction>
            </owl:intersectionOf>
         </owl:Class>
      </rdfs:subClassOf>
      <rdfs:subClassOf rdf:resource="http://www.opengis.net/gml#AbstractCoordinateOperationType"/>
   </owl:Class>
   <owl:Class rdf:about="http://www.opengis.net/gml#GeneralConversionRefType">
      <rdfs:comment>Association to a general conversion, either referencing or containing the definition of that conversion. </rdfs:comment>
      <rdfs:subClassOf>
         <owl:Class>
            <owl:intersectionOf rdf:parseType="Collection">
               <owl:Restriction>
                  <owl:onProperty rdf:resource="http://www.opengis.net/gml#has_GeneralConversion"/>
                  <owl:allValuesFrom rdf:resource="http://www.opengis.net/gml#_GeneralConversion"/>
               </owl:Restriction>
            </owl:intersectionOf>
         </owl:Class>
      </rdfs:subClassOf>
   </owl:Class>
   <owl:Class rdf:about="http://www.opengis.net/gml#ConversionType">
      <rdfs:comment>A concrete operation on coordinates that does not include any change of Datum. The best-known example of a coordinate conversion is a map projection. The parameters describing coordinate conversions are defined rather than empirically derived. Note that some conversions have no parameters.

This concrete complexType can be used with all operation methods, without using an Application Schema that defines operation-method-specialized element names and contents, especially for methods with only one Conversion instance. </rdfs:comment>
      <rdfs:subClassOf>
         <owl:Class>
            <owl:intersectionOf rdf:parseType="Collection">
               <owl:Restriction>
                  <owl:onProperty rdf:resource="http://www.opengis.net/gml#hasusesMethod"/>
                  <owl:allValuesFrom rdf:resource="http://www.opengis.net/gml#usesMethod"/>
               </owl:Restriction>
               <owl:Restriction>
                  <owl:onProperty rdf:resource="http://www.opengis.net/gml#hasusesValue"/>
                  <owl:allValuesFrom rdf:resource="http://www.opengis.net/gml#usesValue"/>
               </owl:Restriction>
               <owl:Restriction>
                  <owl:onProperty rdf:resource="http://www.opengis.net/gml#hasusesValue"/>
                  <owl:minCardinality rdf:datatype="http://www.w3.org/2001/XMLSchema#nonNegativeInteger">0</owl:minCardinality>
               </owl:Restriction>
            </owl:intersectionOf>
         </owl:Class>
      </rdfs:subClassOf>
      <rdfs:subClassOf rdf:resource="http://www.opengis.net/gml#AbstractGeneralConversionType"/>
   </owl:Class>
   <owl:Class rdf:about="http://www.opengis.net/gml#ConversionRefType">
      <rdfs:comment>Association to a concrete general-purpose conversion, either referencing or containing the definition of that conversion. </rdfs:comment>
      <rdfs:subClassOf>
         <owl:Class>
            <owl:intersectionOf rdf:parseType="Collection">
               <owl:Restriction>
                  <owl:onProperty rdf:resource="http://www.opengis.net/gml#hasConversion"/>
                  <owl:allValuesFrom rdf:resource="http://www.opengis.net/gml#Conversion"/>
               </owl:Restriction>
            </owl:intersectionOf>
         </owl:Class>
      </rdfs:subClassOf>
   </owl:Class>
   <owl:Class rdf:about="http://www.opengis.net/gml#AbstractGeneralTransformationType">
      <rdfs:comment>This is an abstract class</rdfs:comment>
      <rdfs:comment>An abstract operation on coordinates that usually includes a change of Datum. The parameters of a coordinate transformation are empirically derived from data containing the coordinates of a series of points in both coordinate reference systems. This computational process is usually "over-determined", allowing derivation of error (or accuracy) estimates for the transformation. Also, the stochastic nature of the parameters may result in multiple (different) versions of the same coordinate transformation.

This abstract complexType is expected to be extended for well-known operation methods with many Transformation instances, in Application Schemas that define operation-method-specialized value element names and contents. This transformation uses an operation method with associated parameter values. However, operation methods and parameter values are directly associated with concrete subtypes, not with this abstract type. All concrete types derived from this type shall extend this type to include a "usesMethod" element that references one "OperationMethod" element. Similarly, all concrete types derived from this type shall extend this type to include one or more elements each named "uses...Value" that each use the type of an element substitutable for the "_generalParameterValue" element. </rdfs:comment>
      <rdfs:subClassOf>
         <owl:Class>
            <owl:intersectionOf rdf:parseType="Collection">
               <owl:Restriction>
                  <owl:onProperty rdf:resource="http://www.opengis.net/gml#hasmetaDataProperty"/>
                  <owl:allValuesFrom rdf:resource="http://www.opengis.net/gml#metaDataProperty"/>
               </owl:Restriction>
               <owl:Restriction>
                  <owl:onProperty rdf:resource="http://www.opengis.net/gml#hasmetaDataProperty"/>
                  <owl:minCardinality rdf:datatype="http://www.w3.org/2001/XMLSchema#nonNegativeInteger">0</owl:minCardinality>
               </owl:Restriction>
               <owl:Restriction>
                  <owl:onProperty rdf:resource="http://www.opengis.net/gml#hascoordinateOperationName"/>
                  <owl:allValuesFrom rdf:resource="http://www.opengis.net/gml#coordinateOperationName"/>
               </owl:Restriction>
               <owl:Restriction>
                  <owl:onProperty rdf:resource="http://www.opengis.net/gml#hascoordinateOperationID"/>
                  <owl:allValuesFrom rdf:resource="http://www.opengis.net/gml#coordinateOperationID"/>
               </owl:Restriction>
               <owl:Restriction>
                  <owl:onProperty rdf:resource="http://www.opengis.net/gml#hascoordinateOperationID"/>
                  <owl:minCardinality rdf:datatype="http://www.w3.org/2001/XMLSchema#nonNegativeInteger">0</owl:minCardinality>
               </owl:Restriction>
               <owl:Restriction>
                  <owl:onProperty rdf:resource="http://www.opengis.net/gml#hasremarks"/>
                  <owl:allValuesFrom rdf:resource="http://www.opengis.net/gml#remarks"/>
               </owl:Restriction>
               <owl:Restriction>
                  <owl:onProperty rdf:resource="http://www.opengis.net/gml#hasremarks"/>
                  <owl:minCardinality rdf:datatype="http://www.w3.org/2001/XMLSchema#nonNegativeInteger">0</owl:minCardinality>
               </owl:Restriction>
               <owl:Restriction>
                  <owl:onProperty rdf:resource="http://www.opengis.net/gml#hasoperationVersion"/>
                  <owl:allValuesFrom rdf:resource="http://www.opengis.net/gml#operationVersion"/>
               </owl:Restriction>
               <owl:Restriction>
                  <owl:onProperty rdf:resource="http://www.opengis.net/gml#hasvalidArea"/>
                  <owl:allValuesFrom rdf:resource="http://www.opengis.net/gml#validArea"/>
               </owl:Restriction>
               <owl:Restriction>
                  <owl:onProperty rdf:resource="http://www.opengis.net/gml#hasvalidArea"/>
                  <owl:minCardinality rdf:datatype="http://www.w3.org/2001/XMLSchema#nonNegativeInteger">0</owl:minCardinality>
               </owl:Restriction>
               <owl:Restriction>
                  <owl:onProperty rdf:resource="http://www.opengis.net/gml#hasscope"/>
                  <owl:allValuesFrom rdf:resource="http://www.opengis.net/gml#scope"/>
               </owl:Restriction>
               <owl:Restriction>
                  <owl:onProperty rdf:resource="http://www.opengis.net/gml#hasscope"/>
                  <owl:minCardinality rdf:datatype="http://www.w3.org/2001/XMLSchema#nonNegativeInteger">0</owl:minCardinality>
               </owl:Restriction>
               <owl:Restriction>
                  <owl:onProperty rdf:resource="http://www.opengis.net/gml#has_positionalAccuracy"/>
                  <owl:allValuesFrom rdf:resource="http://www.opengis.net/gml#_positionalAccuracy"/>
               </owl:Restriction>
               <owl:Restriction>
                  <owl:onProperty rdf:resource="http://www.opengis.net/gml#has_positionalAccuracy"/>
                  <owl:minCardinality rdf:datatype="http://www.w3.org/2001/XMLSchema#nonNegativeInteger">0</owl:minCardinality>
               </owl:Restriction>
               <owl:Restriction>
                  <owl:onProperty rdf:resource="http://www.opengis.net/gml#hassourceCRS"/>
                  <owl:allValuesFrom rdf:resource="http://www.opengis.net/gml#sourceCRS"/>
               </owl:Restriction>
               <owl:Restriction>
                  <owl:onProperty rdf:resource="http://www.opengis.net/gml#hastargetCRS"/>
                  <owl:allValuesFrom rdf:resource="http://www.opengis.net/gml#targetCRS"/>
               </owl:Restriction>
            </owl:intersectionOf>
         </owl:Class>
      </rdfs:subClassOf>
      <rdfs:subClassOf>
         <owl:Class>
            <owl:intersectionOf rdf:parseType="Collection">
               <owl:Restriction>
                  <owl:onProperty rdf:resource="http://www.opengis.net/gml#hasid"/>
                  <owl:allValuesFrom rdf:resource="http://www.opengis.net/gml#id"/>
               </owl:Restriction>
            </owl:intersectionOf>
         </owl:Class>
      </rdfs:subClassOf>
      <rdfs:subClassOf rdf:resource="http://www.opengis.net/gml#AbstractCoordinateOperationType"/>
   </owl:Class>
   <owl:Class rdf:about="http://www.opengis.net/gml#GeneralTransformationRefType">
      <rdfs:comment>Association to a general transformation, either referencing or containing the definition of that transformation. </rdfs:comment>
      <rdfs:subClassOf>
         <owl:Class>
            <owl:intersectionOf rdf:parseType="Collection">
               <owl:Restriction>
                  <owl:onProperty rdf:resource="http://www.opengis.net/gml#has_GeneralTransformation"/>
                  <owl:allValuesFrom rdf:resource="http://www.opengis.net/gml#_GeneralTransformation"/>
               </owl:Restriction>
            </owl:intersectionOf>
         </owl:Class>
      </rdfs:subClassOf>
   </owl:Class>
   <owl:Class rdf:about="http://www.opengis.net/gml#TransformationType">
      <rdfs:comment>A concrete operation on coordinates that usually includes a change of datum. The parameters of a coordinate transformation are empirically derived from data containing the coordinates of a series of points in both coordinate reference systems. This computational process is usually "over-determined", allowing derivation of error (or accuracy) estimates for the transformation. Also, the stochastic nature of the parameters may result in multiple (different) versions of the same coordinate transformation.

This concrete complexType can be used for all operation methods, without using an Application Schema that defines operation-method-specialized element names and contents, especially for methods with only one Transformation instance. </rdfs:comment>
      <rdfs:subClassOf>
         <owl:Class>
            <owl:intersectionOf rdf:parseType="Collection">
               <owl:Restriction>
                  <owl:onProperty rdf:resource="http://www.opengis.net/gml#hasusesMethod"/>
                  <owl:allValuesFrom rdf:resource="http://www.opengis.net/gml#usesMethod"/>
               </owl:Restriction>
               <owl:Restriction>
                  <owl:onProperty rdf:resource="http://www.opengis.net/gml#hasusesValue"/>
                  <owl:allValuesFrom rdf:resource="http://www.opengis.net/gml#usesValue"/>
               </owl:Restriction>
               <owl:Restriction>
                  <owl:onProperty rdf:resource="http://www.opengis.net/gml#hasusesValue"/>
                  <owl:minCardinality rdf:datatype="http://www.w3.org/2001/XMLSchema#nonNegativeInteger">0</owl:minCardinality>
               </owl:Restriction>
            </owl:intersectionOf>
         </owl:Class>
      </rdfs:subClassOf>
      <rdfs:subClassOf rdf:resource="http://www.opengis.net/gml#AbstractGeneralTransformationType"/>
   </owl:Class>
   <owl:Class rdf:about="http://www.opengis.net/gml#TransformationRefType">
      <rdfs:comment>Association to a transformation, either referencing or containing the definition of that transformation. </rdfs:comment>
      <rdfs:subClassOf>
         <owl:Class>
            <owl:intersectionOf rdf:parseType="Collection">
               <owl:Restriction>
                  <owl:onProperty rdf:resource="http://www.opengis.net/gml#hasTransformation"/>
                  <owl:allValuesFrom rdf:resource="http://www.opengis.net/gml#Transformation"/>
               </owl:Restriction>
            </owl:intersectionOf>
         </owl:Class>
      </rdfs:subClassOf>
   </owl:Class>
   <owl:Class rdf:about="http://www.opengis.net/gml#AbstractGeneralParameterValueType">
      <rdfs:comment>This is an abstract class</rdfs:comment>
      <rdfs:comment>Abstract parameter value or group of parameter values.
      
This abstract complexType is expected to be extended and restricted for well-known operation methods with many instances, in Application Schemas that define operation-method-specialized element names and contents. Specific parameter value elements are directly contained in concrete subtypes, not in this abstract type. All concrete types derived from this type shall extend this type to include one "...Value" element with an appropriate type, which should be one of the element types allowed in the ParameterValueType. In addition, all derived concrete types shall extend this type to include a "valueOfParameter" element that references one element substitutable for the "OperationParameter" element. </rdfs:comment>
   </owl:Class>
   <owl:Class rdf:about="http://www.opengis.net/gml#ParameterValueType">
      <rdfs:comment>A parameter value, ordered sequence of values, or reference to a file of parameter values. This concrete complexType can be used for operation methods without using an Application Schema that defines operation-method-specialized element names and contents, especially for methods with only one instance. This complexType can be used, extended, or restricted for well-known operation methods, especially for methods with many instances. </rdfs:comment>
      <rdfs:subClassOf>
         <owl:Class>
            <owl:intersectionOf rdf:parseType="Collection">
               <owl:Restriction>
                  <owl:onProperty rdf:resource="http://www.opengis.net/gml#hasvalueOfParameter"/>
                  <owl:allValuesFrom rdf:resource="http://www.opengis.net/gml#valueOfParameter"/>
               </owl:Restriction>
            </owl:intersectionOf>
         </owl:Class>
      </rdfs:subClassOf>
      <owl:disjointUnionOf rdf:parseType="Collection">
         <owl:Restriction>
            <owl:onProperty rdf:resource="http://www.opengis.net/gml#hasvalue"/>
            <owl:someValuesFrom rdf:resource="http://www.opengis.net/gml#value"/>
         </owl:Restriction>
         <owl:Restriction>
            <owl:onProperty rdf:resource="http://www.opengis.net/gml#hasdmsAngleValue"/>
            <owl:someValuesFrom rdf:resource="http://www.opengis.net/gml#dmsAngleValue"/>
         </owl:Restriction>
         <owl:Restriction>
            <owl:onProperty rdf:resource="http://www.opengis.net/gml#hasstringValue"/>
            <owl:someValuesFrom rdf:resource="http://www.opengis.net/gml#stringValue"/>
         </owl:Restriction>
         <owl:Restriction>
            <owl:onProperty rdf:resource="http://www.opengis.net/gml#hasintegerValue"/>
            <owl:someValuesFrom rdf:resource="http://www.opengis.net/gml#integerValue"/>
         </owl:Restriction>
         <owl:Restriction>
            <owl:onProperty rdf:resource="http://www.opengis.net/gml#hasbooleanValue"/>
            <owl:someValuesFrom rdf:resource="http://www.opengis.net/gml#booleanValue"/>
         </owl:Restriction>
         <owl:Restriction>
            <owl:onProperty rdf:resource="http://www.opengis.net/gml#hasvalueList"/>
            <owl:someValuesFrom rdf:resource="http://www.opengis.net/gml#valueList"/>
         </owl:Restriction>
         <owl:Restriction>
            <owl:onProperty rdf:resource="http://www.opengis.net/gml#hasintegerValueList"/>
            <owl:someValuesFrom rdf:resource="http://www.opengis.net/gml#integerValueList"/>
         </owl:Restriction>
         <owl:Restriction>
            <owl:onProperty rdf:resource="http://www.opengis.net/gml#hasvalueFile"/>
            <owl:someValuesFrom rdf:resource="http://www.opengis.net/gml#valueFile"/>
         </owl:Restriction>
      </owl:disjointUnionOf>
      <rdfs:subClassOf rdf:resource="http://www.opengis.net/gml#AbstractGeneralParameterValueType"/>
   </owl:Class>
   <owl:Class rdf:about="http://www.opengis.net/gml#ParameterValueGroupType">
      <rdfs:comment>A group of related parameter values. The same group can be repeated more than once in a Conversion, Transformation, or higher level parameterValueGroup, if those instances contain different values of one or more parameterValues which suitably distinquish among those groups. This concrete complexType can be used for operation methods without using an Application Schema that defines operation-method-specialized element names and contents, especially for methods with only one instance. This complexType can be used, extended, or restricted for well-known operation methods, especially for methods with many instances. </rdfs:comment>
      <rdfs:subClassOf>
         <owl:Class>
            <owl:intersectionOf rdf:parseType="Collection">
               <owl:Restriction>
                  <owl:onProperty rdf:resource="http://www.opengis.net/gml#hasincludesValue"/>
                  <owl:allValuesFrom rdf:resource="http://www.opengis.net/gml#includesValue"/>
               </owl:Restriction>
               <owl:Restriction>
                  <owl:onProperty rdf:resource="http://www.opengis.net/gml#hasincludesValue"/>
                  <owl:minCardinality rdf:datatype="http://www.w3.org/2001/XMLSchema#nonNegativeInteger">2</owl:minCardinality>
               </owl:Restriction>
               <owl:Restriction>
                  <owl:onProperty rdf:resource="http://www.opengis.net/gml#hasvaluesOfGroup"/>
                  <owl:allValuesFrom rdf:resource="http://www.opengis.net/gml#valuesOfGroup"/>
               </owl:Restriction>
            </owl:intersectionOf>
         </owl:Class>
      </rdfs:subClassOf>
      <rdfs:subClassOf rdf:resource="http://www.opengis.net/gml#AbstractGeneralParameterValueType"/>
   </owl:Class>
   <owl:Class rdf:about="http://www.opengis.net/gml#OperationMethodBaseType">
      <rdfs:comment>This is an abstract class</rdfs:comment>
      <rdfs:comment>Basic encoding for operation method objects, simplifying and restricting the DefinitionType as needed. </rdfs:comment>
      <rdfs:subClassOf>
         <owl:Class>
            <owl:intersectionOf rdf:parseType="Collection">
               <owl:Restriction>
                  <owl:onProperty rdf:resource="http://www.opengis.net/gml#hasmetaDataProperty"/>
                  <owl:allValuesFrom rdf:resource="http://www.opengis.net/gml#metaDataProperty"/>
               </owl:Restriction>
               <owl:Restriction>
                  <owl:onProperty rdf:resource="http://www.opengis.net/gml#hasmetaDataProperty"/>
                  <owl:minCardinality rdf:datatype="http://www.w3.org/2001/XMLSchema#nonNegativeInteger">0</owl:minCardinality>
               </owl:Restriction>
               <owl:Restriction>
                  <owl:onProperty rdf:resource="http://www.opengis.net/gml#hasmethodName"/>
                  <owl:allValuesFrom rdf:resource="http://www.opengis.net/gml#methodName"/>
               </owl:Restriction>
            </owl:intersectionOf>
         </owl:Class>
      </rdfs:subClassOf>
      <rdfs:subClassOf>
         <owl:Class>
            <owl:intersectionOf rdf:parseType="Collection">
               <owl:Restriction>
                  <owl:onProperty rdf:resource="http://www.opengis.net/gml#hasid"/>
                  <owl:allValuesFrom rdf:resource="http://www.opengis.net/gml#id"/>
               </owl:Restriction>
            </owl:intersectionOf>
         </owl:Class>
      </rdfs:subClassOf>
      <rdfs:subClassOf rdf:resource="http://www.opengis.net/gml#DefinitionType"/>
   </owl:Class>
   <owl:Class rdf:about="http://www.opengis.net/gml#OperationMethodType">
      <rdfs:comment>Definition of an algorithm used to perform a coordinate operation. Most operation methods use a number of operation parameters, although some coordinate conversions use none. Each coordinate operation using the method assigns values to these parameters. </rdfs:comment>
      <rdfs:subClassOf>
         <owl:Class>
            <owl:intersectionOf rdf:parseType="Collection">
               <owl:Restriction>
                  <owl:onProperty rdf:resource="http://www.opengis.net/gml#hasmethodID"/>
                  <owl:allValuesFrom rdf:resource="http://www.opengis.net/gml#methodID"/>
               </owl:Restriction>
               <owl:Restriction>
                  <owl:onProperty rdf:resource="http://www.opengis.net/gml#hasmethodID"/>
                  <owl:minCardinality rdf:datatype="http://www.w3.org/2001/XMLSchema#nonNegativeInteger">0</owl:minCardinality>
               </owl:Restriction>
               <owl:Restriction>
                  <owl:onProperty rdf:resource="http://www.opengis.net/gml#hasremarks"/>
                  <owl:allValuesFrom rdf:resource="http://www.opengis.net/gml#remarks"/>
               </owl:Restriction>
               <owl:Restriction>
                  <owl:onProperty rdf:resource="http://www.opengis.net/gml#hasremarks"/>
                  <owl:minCardinality rdf:datatype="http://www.w3.org/2001/XMLSchema#nonNegativeInteger">0</owl:minCardinality>
               </owl:Restriction>
               <owl:Restriction>
                  <owl:onProperty rdf:resource="http://www.opengis.net/gml#hasmethodFormula"/>
                  <owl:allValuesFrom rdf:resource="http://www.opengis.net/gml#methodFormula"/>
               </owl:Restriction>
               <owl:Restriction>
                  <owl:onProperty rdf:resource="http://www.opengis.net/gml#hassourceDimensions"/>
                  <owl:allValuesFrom rdf:resource="http://www.opengis.net/gml#sourceDimensions"/>
               </owl:Restriction>
               <owl:Restriction>
                  <owl:onProperty rdf:resource="http://www.opengis.net/gml#hastargetDimensions"/>
                  <owl:allValuesFrom rdf:resource="http://www.opengis.net/gml#targetDimensions"/>
               </owl:Restriction>
               <owl:Restriction>
                  <owl:onProperty rdf:resource="http://www.opengis.net/gml#hasusesParameter"/>
                  <owl:allValuesFrom rdf:resource="http://www.opengis.net/gml#usesParameter"/>
               </owl:Restriction>
               <owl:Restriction>
                  <owl:onProperty rdf:resource="http://www.opengis.net/gml#hasusesParameter"/>
                  <owl:minCardinality rdf:datatype="http://www.w3.org/2001/XMLSchema#nonNegativeInteger">0</owl:minCardinality>
               </owl:Restriction>
            </owl:intersectionOf>
         </owl:Class>
      </rdfs:subClassOf>
      <rdfs:subClassOf rdf:resource="http://www.opengis.net/gml#OperationMethodBaseType"/>
   </owl:Class>
   <owl:Class rdf:about="http://www.opengis.net/gml#OperationMethodRefType">
      <rdfs:comment>Association to a concrete general-purpose operation method, either referencing or containing the definition of that method. </rdfs:comment>
      <rdfs:subClassOf>
         <owl:Class>
            <owl:intersectionOf rdf:parseType="Collection">
               <owl:Restriction>
                  <owl:onProperty rdf:resource="http://www.opengis.net/gml#hasOperationMethod"/>
                  <owl:allValuesFrom rdf:resource="http://www.opengis.net/gml#OperationMethod"/>
               </owl:Restriction>
            </owl:intersectionOf>
         </owl:Class>
      </rdfs:subClassOf>
   </owl:Class>
   <owl:Class rdf:about="http://www.opengis.net/gml#AbstractGeneralOperationParameterType">
      <rdfs:comment>This is an abstract class</rdfs:comment>
      <rdfs:comment>Abstract definition of a parameter or group of parameters used by an operation method. </rdfs:comment>
      <rdfs:subClassOf>
         <owl:Class>
            <owl:intersectionOf rdf:parseType="Collection">
               <owl:Restriction>
                  <owl:onProperty rdf:resource="http://www.opengis.net/gml#hasminimumOccurs"/>
                  <owl:allValuesFrom rdf:resource="http://www.opengis.net/gml#minimumOccurs"/>
               </owl:Restriction>
               <owl:Restriction>
                  <owl:onProperty rdf:resource="http://www.opengis.net/gml#hasminimumOccurs"/>
                  <owl:minCardinality rdf:datatype="http://www.w3.org/2001/XMLSchema#nonNegativeInteger">0</owl:minCardinality>
               </owl:Restriction>
            </owl:intersectionOf>
         </owl:Class>
      </rdfs:subClassOf>
      <rdfs:subClassOf rdf:resource="http://www.opengis.net/gml#DefinitionType"/>
   </owl:Class>
   <owl:Class rdf:about="http://www.opengis.net/gml#AbstractGeneralOperationParameterRefType">
      <rdfs:comment>Association to an operation parameter or group, either referencing or containing the definition of that parameter or group. </rdfs:comment>
      <rdfs:subClassOf>
         <owl:Class>
            <owl:intersectionOf rdf:parseType="Collection">
               <owl:Restriction>
                  <owl:onProperty rdf:resource="http://www.opengis.net/gml#has_GeneralOperationParameter"/>
                  <owl:allValuesFrom rdf:resource="http://www.opengis.net/gml#_GeneralOperationParameter"/>
               </owl:Restriction>
            </owl:intersectionOf>
         </owl:Class>
      </rdfs:subClassOf>
   </owl:Class>
   <owl:Class rdf:about="http://www.opengis.net/gml#OperationParameterBaseType">
      <rdfs:comment>This is an abstract class</rdfs:comment>
      <rdfs:comment>Basic encoding for operation parameter objects, simplifying and restricting the DefinitionType as needed. </rdfs:comment>
      <rdfs:subClassOf>
         <owl:Class>
            <owl:intersectionOf rdf:parseType="Collection">
               <owl:Restriction>
                  <owl:onProperty rdf:resource="http://www.opengis.net/gml#hasmetaDataProperty"/>
                  <owl:allValuesFrom rdf:resource="http://www.opengis.net/gml#metaDataProperty"/>
               </owl:Restriction>
               <owl:Restriction>
                  <owl:onProperty rdf:resource="http://www.opengis.net/gml#hasmetaDataProperty"/>
                  <owl:minCardinality rdf:datatype="http://www.w3.org/2001/XMLSchema#nonNegativeInteger">0</owl:minCardinality>
               </owl:Restriction>
               <owl:Restriction>
                  <owl:onProperty rdf:resource="http://www.opengis.net/gml#hasparameterName"/>
                  <owl:allValuesFrom rdf:resource="http://www.opengis.net/gml#parameterName"/>
               </owl:Restriction>
               <owl:Restriction>
                  <owl:onProperty rdf:resource="http://www.opengis.net/gml#hasminimumOccurs"/>
                  <owl:allValuesFrom rdf:resource="http://www.opengis.net/gml#minimumOccurs"/>
               </owl:Restriction>
               <owl:Restriction>
                  <owl:onProperty rdf:resource="http://www.opengis.net/gml#hasminimumOccurs"/>
                  <owl:minCardinality rdf:datatype="http://www.w3.org/2001/XMLSchema#nonNegativeInteger">0</owl:minCardinality>
               </owl:Restriction>
            </owl:intersectionOf>
         </owl:Class>
      </rdfs:subClassOf>
      <rdfs:subClassOf>
         <owl:Class>
            <owl:intersectionOf rdf:parseType="Collection">
               <owl:Restriction>
                  <owl:onProperty rdf:resource="http://www.opengis.net/gml#hasid"/>
                  <owl:allValuesFrom rdf:resource="http://www.opengis.net/gml#id"/>
               </owl:Restriction>
            </owl:intersectionOf>
         </owl:Class>
      </rdfs:subClassOf>
      <rdfs:subClassOf rdf:resource="http://www.opengis.net/gml#AbstractGeneralOperationParameterType"/>
   </owl:Class>
   <owl:Class rdf:about="http://www.opengis.net/gml#OperationParameterType">
      <rdfs:comment>The definition of a parameter used by an operation method. Most parameter values are numeric, but other types of parameter values are possible. This complexType is expected to be used or extended for all operation methods, without defining operation-method-specialized element names.  </rdfs:comment>
      <rdfs:subClassOf>
         <owl:Class>
            <owl:intersectionOf rdf:parseType="Collection">
               <owl:Restriction>
                  <owl:onProperty rdf:resource="http://www.opengis.net/gml#hasparameterID"/>
                  <owl:allValuesFrom rdf:resource="http://www.opengis.net/gml#parameterID"/>
               </owl:Restriction>
               <owl:Restriction>
                  <owl:onProperty rdf:resource="http://www.opengis.net/gml#hasparameterID"/>
                  <owl:minCardinality rdf:datatype="http://www.w3.org/2001/XMLSchema#nonNegativeInteger">0</owl:minCardinality>
               </owl:Restriction>
               <owl:Restriction>
                  <owl:onProperty rdf:resource="http://www.opengis.net/gml#hasremarks"/>
                  <owl:allValuesFrom rdf:resource="http://www.opengis.net/gml#remarks"/>
               </owl:Restriction>
               <owl:Restriction>
                  <owl:onProperty rdf:resource="http://www.opengis.net/gml#hasremarks"/>
                  <owl:minCardinality rdf:datatype="http://www.w3.org/2001/XMLSchema#nonNegativeInteger">0</owl:minCardinality>
               </owl:Restriction>
            </owl:intersectionOf>
         </owl:Class>
      </rdfs:subClassOf>
      <rdfs:subClassOf rdf:resource="http://www.opengis.net/gml#OperationParameterBaseType"/>
   </owl:Class>
   <owl:Class rdf:about="http://www.opengis.net/gml#OperationParameterRefType">
      <rdfs:comment>Association to an operation parameter, either referencing or containing the definition of that parameter. </rdfs:comment>
      <rdfs:subClassOf>
         <owl:Class>
            <owl:intersectionOf rdf:parseType="Collection">
               <owl:Restriction>
                  <owl:onProperty rdf:resource="http://www.opengis.net/gml#hasOperationParameter"/>
                  <owl:allValuesFrom rdf:resource="http://www.opengis.net/gml#OperationParameter"/>
               </owl:Restriction>
            </owl:intersectionOf>
         </owl:Class>
      </rdfs:subClassOf>
   </owl:Class>
   <owl:Class rdf:about="http://www.opengis.net/gml#OperationParameterGroupBaseType">
      <rdfs:comment>This is an abstract class</rdfs:comment>
      <rdfs:comment>Basic encoding for operation parameter group objects, simplifying and restricting the DefinitionType as needed. </rdfs:comment>
      <rdfs:subClassOf>
         <owl:Class>
            <owl:intersectionOf rdf:parseType="Collection">
               <owl:Restriction>
                  <owl:onProperty rdf:resource="http://www.opengis.net/gml#hasmetaDataProperty"/>
                  <owl:allValuesFrom rdf:resource="http://www.opengis.net/gml#metaDataProperty"/>
               </owl:Restriction>
               <owl:Restriction>
                  <owl:onProperty rdf:resource="http://www.opengis.net/gml#hasmetaDataProperty"/>
                  <owl:minCardinality rdf:datatype="http://www.w3.org/2001/XMLSchema#nonNegativeInteger">0</owl:minCardinality>
               </owl:Restriction>
               <owl:Restriction>
                  <owl:onProperty rdf:resource="http://www.opengis.net/gml#hasgroupName"/>
                  <owl:allValuesFrom rdf:resource="http://www.opengis.net/gml#groupName"/>
               </owl:Restriction>
               <owl:Restriction>
                  <owl:onProperty rdf:resource="http://www.opengis.net/gml#hasminimumOccurs"/>
                  <owl:allValuesFrom rdf:resource="http://www.opengis.net/gml#minimumOccurs"/>
               </owl:Restriction>
               <owl:Restriction>
                  <owl:onProperty rdf:resource="http://www.opengis.net/gml#hasminimumOccurs"/>
                  <owl:minCardinality rdf:datatype="http://www.w3.org/2001/XMLSchema#nonNegativeInteger">0</owl:minCardinality>
               </owl:Restriction>
            </owl:intersectionOf>
         </owl:Class>
      </rdfs:subClassOf>
      <rdfs:subClassOf>
         <owl:Class>
            <owl:intersectionOf rdf:parseType="Collection">
               <owl:Restriction>
                  <owl:onProperty rdf:resource="http://www.opengis.net/gml#hasid"/>
                  <owl:allValuesFrom rdf:resource="http://www.opengis.net/gml#id"/>
               </owl:Restriction>
            </owl:intersectionOf>
         </owl:Class>
      </rdfs:subClassOf>
      <rdfs:subClassOf rdf:resource="http://www.opengis.net/gml#AbstractGeneralOperationParameterType"/>
   </owl:Class>
   <owl:Class rdf:about="http://www.opengis.net/gml#OperationParameterGroupType">
      <rdfs:comment>The definition of a group of parameters used by an operation method. This complexType is expected to be used or extended for all applicable operation methods, without defining operation-method-specialized element names.  </rdfs:comment>
      <rdfs:subClassOf>
         <owl:Class>
            <owl:intersectionOf rdf:parseType="Collection">
               <owl:Restriction>
                  <owl:onProperty rdf:resource="http://www.opengis.net/gml#hasgroupID"/>
                  <owl:allValuesFrom rdf:resource="http://www.opengis.net/gml#groupID"/>
               </owl:Restriction>
               <owl:Restriction>
                  <owl:onProperty rdf:resource="http://www.opengis.net/gml#hasgroupID"/>
                  <owl:minCardinality rdf:datatype="http://www.w3.org/2001/XMLSchema#nonNegativeInteger">0</owl:minCardinality>
               </owl:Restriction>
               <owl:Restriction>
                  <owl:onProperty rdf:resource="http://www.opengis.net/gml#hasremarks"/>
                  <owl:allValuesFrom rdf:resource="http://www.opengis.net/gml#remarks"/>
               </owl:Restriction>
               <owl:Restriction>
                  <owl:onProperty rdf:resource="http://www.opengis.net/gml#hasremarks"/>
                  <owl:minCardinality rdf:datatype="http://www.w3.org/2001/XMLSchema#nonNegativeInteger">0</owl:minCardinality>
               </owl:Restriction>
               <owl:Restriction>
                  <owl:onProperty rdf:resource="http://www.opengis.net/gml#hasmaximumOccurs"/>
                  <owl:allValuesFrom rdf:resource="http://www.opengis.net/gml#maximumOccurs"/>
               </owl:Restriction>
               <owl:Restriction>
                  <owl:onProperty rdf:resource="http://www.opengis.net/gml#hasmaximumOccurs"/>
                  <owl:minCardinality rdf:datatype="http://www.w3.org/2001/XMLSchema#nonNegativeInteger">0</owl:minCardinality>
               </owl:Restriction>
               <owl:Restriction>
                  <owl:onProperty rdf:resource="http://www.opengis.net/gml#hasincludesParameter"/>
                  <owl:allValuesFrom rdf:resource="http://www.opengis.net/gml#includesParameter"/>
               </owl:Restriction>
               <owl:Restriction>
                  <owl:onProperty rdf:resource="http://www.opengis.net/gml#hasincludesParameter"/>
                  <owl:minCardinality rdf:datatype="http://www.w3.org/2001/XMLSchema#nonNegativeInteger">2</owl:minCardinality>
               </owl:Restriction>
            </owl:intersectionOf>
         </owl:Class>
      </rdfs:subClassOf>
      <rdfs:subClassOf rdf:resource="http://www.opengis.net/gml#OperationParameterGroupBaseType"/>
   </owl:Class>
   <owl:Class rdf:about="http://www.opengis.net/gml#OperationParameterGroupRefType">
      <rdfs:comment>Association to an operation parameter, either referencing or containing the definition of that parameter. </rdfs:comment>
      <rdfs:subClassOf>
         <owl:Class>
            <owl:intersectionOf rdf:parseType="Collection">
               <owl:Restriction>
                  <owl:onProperty rdf:resource="http://www.opengis.net/gml#hasOperationParameterGroup"/>
                  <owl:allValuesFrom rdf:resource="http://www.opengis.net/gml#OperationParameterGroup"/>
               </owl:Restriction>
            </owl:intersectionOf>
         </owl:Class>
      </rdfs:subClassOf>
   </owl:Class>
   <owl:Class rdf:about="http://www.opengis.net/gml#AbstractPositionalAccuracyType">
      <rdfs:comment>This is an abstract class</rdfs:comment>
      <rdfs:comment>Position error estimate (or accuracy) data. </rdfs:comment>
      <rdfs:subClassOf>
         <owl:Class>
            <owl:intersectionOf rdf:parseType="Collection">
               <owl:Restriction>
                  <owl:onProperty rdf:resource="http://www.opengis.net/gml#hasmeasureDescription"/>
                  <owl:allValuesFrom rdf:resource="http://www.opengis.net/gml#measureDescription"/>
               </owl:Restriction>
               <owl:Restriction>
                  <owl:onProperty rdf:resource="http://www.opengis.net/gml#hasmeasureDescription"/>
                  <owl:minCardinality rdf:datatype="http://www.w3.org/2001/XMLSchema#nonNegativeInteger">0</owl:minCardinality>
               </owl:Restriction>
            </owl:intersectionOf>
         </owl:Class>
      </rdfs:subClassOf>
   </owl:Class>
   <owl:Class rdf:about="http://www.opengis.net/gml#AbsoluteExternalPositionalAccuracyType">
      <rdfs:comment>Closeness of reported coordinate values to values accepted as or being true. </rdfs:comment>
      <rdfs:subClassOf>
         <owl:Class>
            <owl:intersectionOf rdf:parseType="Collection">
               <owl:Restriction>
                  <owl:onProperty rdf:resource="http://www.opengis.net/gml#hasresult"/>
                  <owl:allValuesFrom rdf:resource="http://www.opengis.net/gml#result"/>
               </owl:Restriction>
            </owl:intersectionOf>
         </owl:Class>
      </rdfs:subClassOf>
      <rdfs:subClassOf rdf:resource="http://www.opengis.net/gml#AbstractPositionalAccuracyType"/>
   </owl:Class>
   <owl:Class rdf:about="http://www.opengis.net/gml#RelativeInternalPositionalAccuracyType">
      <rdfs:comment>Closeness of the relative positions of two or more positions to their respective relative positions accepted as or being true. </rdfs:comment>
      <rdfs:subClassOf>
         <owl:Class>
            <owl:intersectionOf rdf:parseType="Collection">
               <owl:Restriction>
                  <owl:onProperty rdf:resource="http://www.opengis.net/gml#hasresult"/>
                  <owl:allValuesFrom rdf:resource="http://www.opengis.net/gml#result"/>
               </owl:Restriction>
            </owl:intersectionOf>
         </owl:Class>
      </rdfs:subClassOf>
      <rdfs:subClassOf rdf:resource="http://www.opengis.net/gml#AbstractPositionalAccuracyType"/>
   </owl:Class>
   <owl:Class rdf:about="http://www.opengis.net/gml#CovarianceMatrixType">
      <rdfs:comment>Error estimate covariance matrix. </rdfs:comment>
      <rdfs:subClassOf>
         <owl:Class>
            <owl:intersectionOf rdf:parseType="Collection">
               <owl:Restriction>
                  <owl:onProperty rdf:resource="http://www.opengis.net/gml#hasunitOfMeasure"/>
                  <owl:allValuesFrom rdf:resource="http://www.opengis.net/gml#unitOfMeasure"/>
               </owl:Restriction>
               <owl:Restriction>
                  <owl:onProperty rdf:resource="http://www.opengis.net/gml#hasincludesElement"/>
                  <owl:allValuesFrom rdf:resource="http://www.opengis.net/gml#includesElement"/>
               </owl:Restriction>
            </owl:intersectionOf>
         </owl:Class>
      </rdfs:subClassOf>
      <rdfs:subClassOf rdf:resource="http://www.opengis.net/gml#AbstractPositionalAccuracyType"/>
   </owl:Class>
   <owl:Class rdf:about="http://www.opengis.net/gml#CovarianceElementType">
      <rdfs:comment>An element of a covariance matrix.</rdfs:comment>
      <rdfs:subClassOf>
         <owl:Class>
            <owl:intersectionOf rdf:parseType="Collection">
               <owl:Restriction>
                  <owl:onProperty rdf:resource="http://www.opengis.net/gml#hasrowIndex"/>
                  <owl:allValuesFrom rdf:resource="http://www.opengis.net/gml#rowIndex"/>
               </owl:Restriction>
               <owl:Restriction>
                  <owl:onProperty rdf:resource="http://www.opengis.net/gml#hascolumnIndex"/>
                  <owl:allValuesFrom rdf:resource="http://www.opengis.net/gml#columnIndex"/>
               </owl:Restriction>
               <owl:Restriction>
                  <owl:onProperty rdf:resource="http://www.opengis.net/gml#hascovariance"/>
                  <owl:allValuesFrom rdf:resource="http://www.opengis.net/gml#covariance"/>
               </owl:Restriction>
            </owl:intersectionOf>
         </owl:Class>
      </rdfs:subClassOf>
   </owl:Class>
   <owl:Class rdf:about="http://www.opengis.net/gml#TargetPropertyType">
      <rdfs:comment>Container for an object representing the target or subject of an observation.</rdfs:comment>
      <owl:disjointUnionOf rdf:parseType="Collection">
         <owl:Restriction>
            <owl:onProperty rdf:resource="http://www.opengis.net/gml#has_Feature"/>
            <owl:someValuesFrom rdf:resource="http://www.opengis.net/gml#_Feature"/>
         </owl:Restriction>
         <owl:Restriction>
            <owl:onProperty rdf:resource="http://www.opengis.net/gml#has_Geometry"/>
            <owl:someValuesFrom rdf:resource="http://www.opengis.net/gml#_Geometry"/>
         </owl:Restriction>
      </owl:disjointUnionOf>
   </owl:Class>
   <owl:Class rdf:about="http://www.opengis.net/gml#ObservationType">
      <rdfs:subClassOf>
         <owl:Class>
            <owl:intersectionOf rdf:parseType="Collection">
               <owl:Restriction>
                  <owl:onProperty rdf:resource="http://www.opengis.net/gml#hasvalidTime"/>
                  <owl:allValuesFrom rdf:resource="http://www.opengis.net/gml#validTime"/>
               </owl:Restriction>
               <owl:Restriction>
                  <owl:onProperty rdf:resource="http://www.opengis.net/gml#hasusing"/>
                  <owl:allValuesFrom rdf:resource="http://www.opengis.net/gml#using"/>
               </owl:Restriction>
               <owl:Restriction>
                  <owl:onProperty rdf:resource="http://www.opengis.net/gml#hasusing"/>
                  <owl:minCardinality rdf:datatype="http://www.w3.org/2001/XMLSchema#nonNegativeInteger">0</owl:minCardinality>
               </owl:Restriction>
               <owl:Restriction>
                  <owl:onProperty rdf:resource="http://www.opengis.net/gml#hastarget"/>
                  <owl:allValuesFrom rdf:resource="http://www.opengis.net/gml#target"/>
               </owl:Restriction>
               <owl:Restriction>
                  <owl:onProperty rdf:resource="http://www.opengis.net/gml#hastarget"/>
                  <owl:minCardinality rdf:datatype="http://www.w3.org/2001/XMLSchema#nonNegativeInteger">0</owl:minCardinality>
               </owl:Restriction>
               <owl:Restriction>
                  <owl:onProperty rdf:resource="http://www.opengis.net/gml#hasresultOf"/>
                  <owl:allValuesFrom rdf:resource="http://www.opengis.net/gml#resultOf"/>
               </owl:Restriction>
            </owl:intersectionOf>
         </owl:Class>
      </rdfs:subClassOf>
      <rdfs:subClassOf rdf:resource="http://www.opengis.net/gml#AbstractFeatureType"/>
   </owl:Class>
   <owl:Class rdf:about="http://www.opengis.net/gml#DirectedObservationType">
      <rdfs:subClassOf>
         <owl:Class>
            <owl:intersectionOf rdf:parseType="Collection">
               <owl:Restriction>
                  <owl:onProperty rdf:resource="http://www.opengis.net/gml#hasdirection"/>
                  <owl:allValuesFrom rdf:resource="http://www.opengis.net/gml#direction"/>
               </owl:Restriction>
            </owl:intersectionOf>
         </owl:Class>
      </rdfs:subClassOf>
      <rdfs:subClassOf rdf:resource="http://www.opengis.net/gml#ObservationType"/>
   </owl:Class>
   <owl:Class rdf:about="http://www.opengis.net/gml#DirectedObservationAtDistanceType">
      <rdfs:subClassOf>
         <owl:Class>
            <owl:intersectionOf rdf:parseType="Collection">
               <owl:Restriction>
                  <owl:onProperty rdf:resource="http://www.opengis.net/gml#distance"/>
                  <owl:allValuesFrom rdf:resource="http://www.opengis.net/gml#MeasureType"/>
               </owl:Restriction>
            </owl:intersectionOf>
         </owl:Class>
      </rdfs:subClassOf>
      <rdfs:subClassOf rdf:resource="http://www.opengis.net/gml#DirectedObservationType"/>
   </owl:Class>
   <owl:Class rdf:about="http://www.opengis.net/gml#DefaultStylePropertyType">
      <rdfs:comment>[complexType of] Top-level property. Used in application schemas to "attach" the styling information to GML data. The link between the data and the style should be established through this property only.</rdfs:comment>
      <rdfs:subClassOf>
         <owl:Class>
            <owl:intersectionOf rdf:parseType="Collection">
               <owl:Restriction>
                  <owl:onProperty rdf:resource="http://www.opengis.net/gml#has_Style"/>
                  <owl:allValuesFrom rdf:resource="http://www.opengis.net/gml#_Style"/>
               </owl:Restriction>
               <owl:Restriction>
                  <owl:onProperty rdf:resource="http://www.opengis.net/gml#has_Style"/>
                  <owl:minCardinality rdf:datatype="http://www.w3.org/2001/XMLSchema#nonNegativeInteger">0</owl:minCardinality>
               </owl:Restriction>
            </owl:intersectionOf>
         </owl:Class>
      </rdfs:subClassOf>
      <rdfs:subClassOf>
         <owl:Class>
            <owl:intersectionOf rdf:parseType="Collection">
               <owl:Restriction>
                  <owl:onProperty rdf:resource="http://www.opengis.net/gml#about"/>
                  <owl:allValuesFrom rdf:resource="http://www.w3.org/2001/XMLSchema#anyURI"/>
               </owl:Restriction>
            </owl:intersectionOf>
         </owl:Class>
      </rdfs:subClassOf>
   </owl:Class>
   <owl:Class rdf:about="http://www.opengis.net/gml#AbstractStyleType">
      <rdfs:comment>This is an abstract class</rdfs:comment>
      <rdfs:comment>[complexType of] The value of the top-level property. It is an abstract element. Used as the head element of the substitution group for extensibility purposes.</rdfs:comment>
      <rdfs:subClassOf rdf:resource="http://www.opengis.net/gml#AbstractGMLType"/>
   </owl:Class>
   <owl:Class rdf:about="http://www.opengis.net/gml#StyleType">
      <rdfs:comment>[complexType of] Predefined concrete value of the top-level property. Encapsulates all other styling information.</rdfs:comment>
      <rdfs:subClassOf>
         <owl:Class>
            <owl:intersectionOf rdf:parseType="Collection">
               <owl:Restriction>
                  <owl:onProperty rdf:resource="http://www.opengis.net/gml#hasfeatureStyle"/>
                  <owl:allValuesFrom rdf:resource="http://www.opengis.net/gml#featureStyle"/>
               </owl:Restriction>
               <owl:Restriction>
                  <owl:onProperty rdf:resource="http://www.opengis.net/gml#hasgraphStyle"/>
                  <owl:allValuesFrom rdf:resource="http://www.opengis.net/gml#graphStyle"/>
               </owl:Restriction>
               <owl:Restriction>
                  <owl:onProperty rdf:resource="http://www.opengis.net/gml#hasgraphStyle"/>
                  <owl:minCardinality rdf:datatype="http://www.w3.org/2001/XMLSchema#nonNegativeInteger">0</owl:minCardinality>
               </owl:Restriction>
            </owl:intersectionOf>
         </owl:Class>
      </rdfs:subClassOf>
      <rdfs:subClassOf rdf:resource="http://www.opengis.net/gml#AbstractStyleType"/>
   </owl:Class>
   <owl:Class rdf:about="http://www.opengis.net/gml#FeatureStylePropertyType">
      <rdfs:subClassOf>
         <owl:Class>
            <owl:intersectionOf rdf:parseType="Collection">
               <owl:Restriction>
                  <owl:onProperty rdf:resource="http://www.opengis.net/gml#hasFeatureStyle"/>
                  <owl:allValuesFrom rdf:resource="http://www.opengis.net/gml#FeatureStyle"/>
               </owl:Restriction>
               <owl:Restriction>
                  <owl:onProperty rdf:resource="http://www.opengis.net/gml#hasFeatureStyle"/>
                  <owl:minCardinality rdf:datatype="http://www.w3.org/2001/XMLSchema#nonNegativeInteger">0</owl:minCardinality>
               </owl:Restriction>
            </owl:intersectionOf>
         </owl:Class>
      </rdfs:subClassOf>
      <rdfs:subClassOf>
         <owl:Class>
            <owl:intersectionOf rdf:parseType="Collection">
               <owl:Restriction>
                  <owl:onProperty rdf:resource="http://www.opengis.net/gml#about"/>
                  <owl:allValuesFrom rdf:resource="http://www.w3.org/2001/XMLSchema#anyURI"/>
               </owl:Restriction>
            </owl:intersectionOf>
         </owl:Class>
      </rdfs:subClassOf>
   </owl:Class>
   <owl:Class rdf:about="http://www.opengis.net/gml#FeatureStyleType">
      <rdfs:comment>[complexType of] The style descriptor for features.</rdfs:comment>
      <rdfs:subClassOf>
         <owl:Class>
            <owl:intersectionOf rdf:parseType="Collection">
               <owl:Restriction>
                  <owl:onProperty rdf:resource="http://www.opengis.net/gml#featureConstraint"/>
                  <owl:allValuesFrom rdf:resource="http://www.w3.org/2001/XMLSchema#string"/>
               </owl:Restriction>
               <owl:Restriction>
                  <owl:onProperty rdf:resource="http://www.opengis.net/gml#featureConstraint"/>
                  <owl:minCardinality rdf:datatype="http://www.w3.org/2001/XMLSchema#nonNegativeInteger">0</owl:minCardinality>
               </owl:Restriction>
               <owl:Restriction>
                  <owl:onProperty rdf:resource="http://www.opengis.net/gml#hasgeometryStyle"/>
                  <owl:allValuesFrom rdf:resource="http://www.opengis.net/gml#geometryStyle"/>
               </owl:Restriction>
               <owl:Restriction>
                  <owl:onProperty rdf:resource="http://www.opengis.net/gml#hasgeometryStyle"/>
                  <owl:minCardinality rdf:datatype="http://www.w3.org/2001/XMLSchema#nonNegativeInteger">0</owl:minCardinality>
               </owl:Restriction>
               <owl:Restriction>
                  <owl:onProperty rdf:resource="http://www.opengis.net/gml#hastopologyStyle"/>
                  <owl:allValuesFrom rdf:resource="http://www.opengis.net/gml#topologyStyle"/>
               </owl:Restriction>
               <owl:Restriction>
                  <owl:onProperty rdf:resource="http://www.opengis.net/gml#hastopologyStyle"/>
                  <owl:minCardinality rdf:datatype="http://www.w3.org/2001/XMLSchema#nonNegativeInteger">0</owl:minCardinality>
               </owl:Restriction>
               <owl:Restriction>
                  <owl:onProperty rdf:resource="http://www.opengis.net/gml#haslabelStyle"/>
                  <owl:allValuesFrom rdf:resource="http://www.opengis.net/gml#labelStyle"/>
               </owl:Restriction>
               <owl:Restriction>
                  <owl:onProperty rdf:resource="http://www.opengis.net/gml#haslabelStyle"/>
                  <owl:minCardinality rdf:datatype="http://www.w3.org/2001/XMLSchema#nonNegativeInteger">0</owl:minCardinality>
               </owl:Restriction>
            </owl:intersectionOf>
         </owl:Class>
      </rdfs:subClassOf>
      <rdfs:subClassOf>
         <owl:Class>
            <owl:intersectionOf rdf:parseType="Collection">
               <owl:Restriction>
                  <owl:onProperty rdf:resource="http://www.opengis.net/gml#featureType"/>
                  <owl:allValuesFrom rdf:resource="http://www.w3.org/2001/XMLSchema#string"/>
               </owl:Restriction>
               <owl:Restriction>
                  <owl:onProperty rdf:resource="http://www.opengis.net/gml#baseType"/>
                  <owl:allValuesFrom rdf:resource="http://www.w3.org/2001/XMLSchema#string"/>
               </owl:Restriction>
               <owl:Restriction>
                  <owl:onProperty rdf:resource="http://www.opengis.net/gml#queryGrammar"/>
                  <owl:allValuesFrom rdf:resource="http://www.opengis.net/gml#QueryGrammarEnumeration"/>
               </owl:Restriction>
            </owl:intersectionOf>
         </owl:Class>
      </rdfs:subClassOf>
      <rdfs:subClassOf rdf:resource="http://www.opengis.net/gml#AbstractGMLType"/>
   </owl:Class>
   <owl:Class rdf:about="http://www.opengis.net/gml#BaseStyleDescriptorType">
      <rdfs:comment>Base complex type for geometry, topology, label and graph styles.</rdfs:comment>
      <rdfs:subClassOf>
         <owl:Class>
            <owl:intersectionOf rdf:parseType="Collection">
               <owl:Restriction>
                  <owl:onProperty rdf:resource="http://www.opengis.net/gml#spatialResolution"/>
                  <owl:allValuesFrom rdf:resource="http://www.opengis.net/gml#ScaleType"/>
               </owl:Restriction>
               <owl:Restriction>
                  <owl:onProperty rdf:resource="http://www.opengis.net/gml#spatialResolution"/>
                  <owl:minCardinality rdf:datatype="http://www.w3.org/2001/XMLSchema#nonNegativeInteger">0</owl:minCardinality>
               </owl:Restriction>
               <owl:Restriction>
                  <owl:onProperty rdf:resource="http://www.opengis.net/gml#styleVariation"/>
                  <owl:allValuesFrom rdf:resource="http://www.opengis.net/gml#StyleVariationType"/>
               </owl:Restriction>
               <owl:Restriction>
                  <owl:onProperty rdf:resource="http://www.opengis.net/gml#styleVariation"/>
                  <owl:minCardinality rdf:datatype="http://www.w3.org/2001/XMLSchema#nonNegativeInteger">0</owl:minCardinality>
               </owl:Restriction>
               <owl:Restriction>
                  <owl:onProperty rdf:resource="smil20:hasanimate"/>
                  <owl:allValuesFrom rdf:resource="smil20:animate"/>
               </owl:Restriction>
               <owl:Restriction>
                  <owl:onProperty rdf:resource="smil20:hasanimate"/>
                  <owl:minCardinality rdf:datatype="http://www.w3.org/2001/XMLSchema#nonNegativeInteger">0</owl:minCardinality>
               </owl:Restriction>
               <owl:Restriction>
                  <owl:onProperty rdf:resource="smil20:hasanimateMotion"/>
                  <owl:allValuesFrom rdf:resource="smil20:animateMotion"/>
               </owl:Restriction>
               <owl:Restriction>
                  <owl:onProperty rdf:resource="smil20:hasanimateMotion"/>
                  <owl:minCardinality rdf:datatype="http://www.w3.org/2001/XMLSchema#nonNegativeInteger">0</owl:minCardinality>
               </owl:Restriction>
               <owl:Restriction>
                  <owl:onProperty rdf:resource="smil20:hasanimateColor"/>
                  <owl:allValuesFrom rdf:resource="smil20:animateColor"/>
               </owl:Restriction>
               <owl:Restriction>
                  <owl:onProperty rdf:resource="smil20:hasanimateColor"/>
                  <owl:minCardinality rdf:datatype="http://www.w3.org/2001/XMLSchema#nonNegativeInteger">0</owl:minCardinality>
               </owl:Restriction>
               <owl:Restriction>
                  <owl:onProperty rdf:resource="smil20:hasset"/>
                  <owl:allValuesFrom rdf:resource="smil20:set"/>
               </owl:Restriction>
               <owl:Restriction>
                  <owl:onProperty rdf:resource="smil20:hasset"/>
                  <owl:minCardinality rdf:datatype="http://www.w3.org/2001/XMLSchema#nonNegativeInteger">0</owl:minCardinality>
               </owl:Restriction>
            </owl:intersectionOf>
         </owl:Class>
      </rdfs:subClassOf>
      <rdfs:subClassOf rdf:resource="http://www.opengis.net/gml#AbstractGMLType"/>
   </owl:Class>
   <owl:Class rdf:about="http://www.opengis.net/gml#GeometryStylePropertyType">
      <rdfs:subClassOf>
         <owl:Class>
            <owl:intersectionOf rdf:parseType="Collection">
               <owl:Restriction>
                  <owl:onProperty rdf:resource="http://www.opengis.net/gml#hasGeometryStyle"/>
                  <owl:allValuesFrom rdf:resource="http://www.opengis.net/gml#GeometryStyle"/>
               </owl:Restriction>
               <owl:Restriction>
                  <owl:onProperty rdf:resource="http://www.opengis.net/gml#hasGeometryStyle"/>
                  <owl:minCardinality rdf:datatype="http://www.w3.org/2001/XMLSchema#nonNegativeInteger">0</owl:minCardinality>
               </owl:Restriction>
            </owl:intersectionOf>
         </owl:Class>
      </rdfs:subClassOf>
      <rdfs:subClassOf>
         <owl:Class>
            <owl:intersectionOf rdf:parseType="Collection">
               <owl:Restriction>
                  <owl:onProperty rdf:resource="http://www.opengis.net/gml#about"/>
                  <owl:allValuesFrom rdf:resource="http://www.w3.org/2001/XMLSchema#anyURI"/>
               </owl:Restriction>
            </owl:intersectionOf>
         </owl:Class>
      </rdfs:subClassOf>
   </owl:Class>
   <owl:Class rdf:about="http://www.opengis.net/gml#GeometryStyleType">
      <rdfs:comment>[complexType of] The style descriptor for geometries of a feature.</rdfs:comment>
      <rdfs:subClassOf>
         <owl:Class>
            <owl:intersectionOf rdf:parseType="Collection">
               <owl:Restriction>
                  <owl:onProperty rdf:resource="http://www.opengis.net/gml#haslabelStyle"/>
                  <owl:allValuesFrom rdf:resource="http://www.opengis.net/gml#labelStyle"/>
               </owl:Restriction>
               <owl:Restriction>
                  <owl:onProperty rdf:resource="http://www.opengis.net/gml#haslabelStyle"/>
                  <owl:minCardinality rdf:datatype="http://www.w3.org/2001/XMLSchema#nonNegativeInteger">0</owl:minCardinality>
               </owl:Restriction>
            </owl:intersectionOf>
         </owl:Class>
      </rdfs:subClassOf>
      <owl:disjointUnionOf rdf:parseType="Collection">
         <owl:Restriction>
            <owl:onProperty rdf:resource="http://www.opengis.net/gml#hassymbol"/>
            <owl:someValuesFrom rdf:resource="http://www.opengis.net/gml#symbol"/>
         </owl:Restriction>
         <owl:Restriction>
            <owl:onProperty rdf:resource="http://www.opengis.net/gml#style"/>
            <owl:someValuesFrom rdf:resource="http://www.w3.org/2001/XMLSchema#string"/>
         </owl:Restriction>
      </owl:disjointUnionOf>
      <rdfs:subClassOf>
         <owl:Class>
            <owl:intersectionOf rdf:parseType="Collection">
               <owl:Restriction>
                  <owl:onProperty rdf:resource="http://www.opengis.net/gml#geometryProperty"/>
                  <owl:allValuesFrom rdf:resource="http://www.w3.org/2001/XMLSchema#string"/>
               </owl:Restriction>
               <owl:Restriction>
                  <owl:onProperty rdf:resource="http://www.opengis.net/gml#geometryType"/>
                  <owl:allValuesFrom rdf:resource="http://www.w3.org/2001/XMLSchema#string"/>
               </owl:Restriction>
            </owl:intersectionOf>
         </owl:Class>
      </rdfs:subClassOf>
      <rdfs:subClassOf rdf:resource="http://www.opengis.net/gml#BaseStyleDescriptorType"/>
   </owl:Class>
   <owl:Class rdf:about="http://www.opengis.net/gml#TopologyStylePropertyType">
      <rdfs:subClassOf>
         <owl:Class>
            <owl:intersectionOf rdf:parseType="Collection">
               <owl:Restriction>
                  <owl:onProperty rdf:resource="http://www.opengis.net/gml#hasTopologyStyle"/>
                  <owl:allValuesFrom rdf:resource="http://www.opengis.net/gml#TopologyStyle"/>
               </owl:Restriction>
               <owl:Restriction>
                  <owl:onProperty rdf:resource="http://www.opengis.net/gml#hasTopologyStyle"/>
                  <owl:minCardinality rdf:datatype="http://www.w3.org/2001/XMLSchema#nonNegativeInteger">0</owl:minCardinality>
               </owl:Restriction>
            </owl:intersectionOf>
         </owl:Class>
      </rdfs:subClassOf>
      <rdfs:subClassOf>
         <owl:Class>
            <owl:intersectionOf rdf:parseType="Collection">
               <owl:Restriction>
                  <owl:onProperty rdf:resource="http://www.opengis.net/gml#about"/>
                  <owl:allValuesFrom rdf:resource="http://www.w3.org/2001/XMLSchema#anyURI"/>
               </owl:Restriction>
            </owl:intersectionOf>
         </owl:Class>
      </rdfs:subClassOf>
   </owl:Class>
   <owl:Class rdf:about="http://www.opengis.net/gml#TopologyStyleType">
      <rdfs:comment>[complexType of] The style descriptor for topologies of a feature. Describes individual topology elements styles.</rdfs:comment>
      <rdfs:subClassOf>
         <owl:Class>
            <owl:intersectionOf rdf:parseType="Collection">
               <owl:Restriction>
                  <owl:onProperty rdf:resource="http://www.opengis.net/gml#haslabelStyle"/>
                  <owl:allValuesFrom rdf:resource="http://www.opengis.net/gml#labelStyle"/>
               </owl:Restriction>
               <owl:Restriction>
                  <owl:onProperty rdf:resource="http://www.opengis.net/gml#haslabelStyle"/>
                  <owl:minCardinality rdf:datatype="http://www.w3.org/2001/XMLSchema#nonNegativeInteger">0</owl:minCardinality>
               </owl:Restriction>
            </owl:intersectionOf>
         </owl:Class>
      </rdfs:subClassOf>
      <owl:disjointUnionOf rdf:parseType="Collection">
         <owl:Restriction>
            <owl:onProperty rdf:resource="http://www.opengis.net/gml#hassymbol"/>
            <owl:someValuesFrom rdf:resource="http://www.opengis.net/gml#symbol"/>
         </owl:Restriction>
         <owl:Restriction>
            <owl:onProperty rdf:resource="http://www.opengis.net/gml#style"/>
            <owl:someValuesFrom rdf:resource="http://www.w3.org/2001/XMLSchema#string"/>
         </owl:Restriction>
      </owl:disjointUnionOf>
      <rdfs:subClassOf>
         <owl:Class>
            <owl:intersectionOf rdf:parseType="Collection">
               <owl:Restriction>
                  <owl:onProperty rdf:resource="http://www.opengis.net/gml#topologyProperty"/>
                  <owl:allValuesFrom rdf:resource="http://www.w3.org/2001/XMLSchema#string"/>
               </owl:Restriction>
               <owl:Restriction>
                  <owl:onProperty rdf:resource="http://www.opengis.net/gml#topologyType"/>
                  <owl:allValuesFrom rdf:resource="http://www.w3.org/2001/XMLSchema#string"/>
               </owl:Restriction>
            </owl:intersectionOf>
         </owl:Class>
      </rdfs:subClassOf>
      <rdfs:subClassOf rdf:resource="http://www.opengis.net/gml#BaseStyleDescriptorType"/>
   </owl:Class>
   <owl:Class rdf:about="http://www.opengis.net/gml#LabelStylePropertyType">
      <rdfs:subClassOf>
         <owl:Class>
            <owl:intersectionOf rdf:parseType="Collection">
               <owl:Restriction>
                  <owl:onProperty rdf:resource="http://www.opengis.net/gml#hasLabelStyle"/>
                  <owl:allValuesFrom rdf:resource="http://www.opengis.net/gml#LabelStyle"/>
               </owl:Restriction>
               <owl:Restriction>
                  <owl:onProperty rdf:resource="http://www.opengis.net/gml#hasLabelStyle"/>
                  <owl:minCardinality rdf:datatype="http://www.w3.org/2001/XMLSchema#nonNegativeInteger">0</owl:minCardinality>
               </owl:Restriction>
            </owl:intersectionOf>
         </owl:Class>
      </rdfs:subClassOf>
      <rdfs:subClassOf>
         <owl:Class>
            <owl:intersectionOf rdf:parseType="Collection">
               <owl:Restriction>
                  <owl:onProperty rdf:resource="http://www.opengis.net/gml#about"/>
                  <owl:allValuesFrom rdf:resource="http://www.w3.org/2001/XMLSchema#anyURI"/>
               </owl:Restriction>
            </owl:intersectionOf>
         </owl:Class>
      </rdfs:subClassOf>
   </owl:Class>
   <owl:Class rdf:about="http://www.opengis.net/gml#LabelStyleType">
      <rdfs:comment>[complexType of] The style descriptor for labels of a feature, geometry or topology.</rdfs:comment>
      <rdfs:subClassOf>
         <owl:Class>
            <owl:intersectionOf rdf:parseType="Collection">
               <owl:Restriction>
                  <owl:onProperty rdf:resource="http://www.opengis.net/gml#style"/>
                  <owl:allValuesFrom rdf:resource="http://www.w3.org/2001/XMLSchema#string"/>
               </owl:Restriction>
               <owl:Restriction>
                  <owl:onProperty rdf:resource="http://www.opengis.net/gml#label"/>
                  <owl:allValuesFrom rdf:resource="http://www.opengis.net/gml#LabelType"/>
               </owl:Restriction>
            </owl:intersectionOf>
         </owl:Class>
      </rdfs:subClassOf>
      <rdfs:subClassOf rdf:resource="http://www.opengis.net/gml#BaseStyleDescriptorType"/>
   </owl:Class>
   <owl:Class rdf:about="http://www.opengis.net/gml#GraphStylePropertyType">
      <rdfs:subClassOf>
         <owl:Class>
            <owl:intersectionOf rdf:parseType="Collection">
               <owl:Restriction>
                  <owl:onProperty rdf:resource="http://www.opengis.net/gml#hasGraphStyle"/>
                  <owl:allValuesFrom rdf:resource="http://www.opengis.net/gml#GraphStyle"/>
               </owl:Restriction>
               <owl:Restriction>
                  <owl:onProperty rdf:resource="http://www.opengis.net/gml#hasGraphStyle"/>
                  <owl:minCardinality rdf:datatype="http://www.w3.org/2001/XMLSchema#nonNegativeInteger">0</owl:minCardinality>
               </owl:Restriction>
            </owl:intersectionOf>
         </owl:Class>
      </rdfs:subClassOf>
      <rdfs:subClassOf>
         <owl:Class>
            <owl:intersectionOf rdf:parseType="Collection">
               <owl:Restriction>
                  <owl:onProperty rdf:resource="http://www.opengis.net/gml#about"/>
                  <owl:allValuesFrom rdf:resource="http://www.w3.org/2001/XMLSchema#anyURI"/>
               </owl:Restriction>
            </owl:intersectionOf>
         </owl:Class>
      </rdfs:subClassOf>
   </owl:Class>
   <owl:Class rdf:about="http://www.opengis.net/gml#GraphStyleType">
      <rdfs:comment>[complexType of] The style descriptor for a graph consisting of a number of features. Describes graph-specific style attributes.</rdfs:comment>
      <rdfs:subClassOf>
         <owl:Class>
            <owl:intersectionOf rdf:parseType="Collection">
               <owl:Restriction>
                  <owl:onProperty rdf:resource="http://www.opengis.net/gml#planar"/>
                  <owl:allValuesFrom rdf:resource="http://www.w3.org/2001/XMLSchema#boolean"/>
               </owl:Restriction>
               <owl:Restriction>
                  <owl:onProperty rdf:resource="http://www.opengis.net/gml#planar"/>
                  <owl:minCardinality rdf:datatype="http://www.w3.org/2001/XMLSchema#nonNegativeInteger">0</owl:minCardinality>
               </owl:Restriction>
               <owl:Restriction>
                  <owl:onProperty rdf:resource="http://www.opengis.net/gml#directed"/>
                  <owl:allValuesFrom rdf:resource="http://www.w3.org/2001/XMLSchema#boolean"/>
               </owl:Restriction>
               <owl:Restriction>
                  <owl:onProperty rdf:resource="http://www.opengis.net/gml#directed"/>
                  <owl:minCardinality rdf:datatype="http://www.w3.org/2001/XMLSchema#nonNegativeInteger">0</owl:minCardinality>
               </owl:Restriction>
               <owl:Restriction>
                  <owl:onProperty rdf:resource="http://www.opengis.net/gml#grid"/>
                  <owl:allValuesFrom rdf:resource="http://www.w3.org/2001/XMLSchema#boolean"/>
               </owl:Restriction>
               <owl:Restriction>
                  <owl:onProperty rdf:resource="http://www.opengis.net/gml#grid"/>
                  <owl:minCardinality rdf:datatype="http://www.w3.org/2001/XMLSchema#nonNegativeInteger">0</owl:minCardinality>
               </owl:Restriction>
               <owl:Restriction>
                  <owl:onProperty rdf:resource="http://www.opengis.net/gml#minDistance"/>
                  <owl:allValuesFrom rdf:resource="http://www.w3.org/2001/XMLSchema#double"/>
               </owl:Restriction>
               <owl:Restriction>
                  <owl:onProperty rdf:resource="http://www.opengis.net/gml#minDistance"/>
                  <owl:minCardinality rdf:datatype="http://www.w3.org/2001/XMLSchema#nonNegativeInteger">0</owl:minCardinality>
               </owl:Restriction>
               <owl:Restriction>
                  <owl:onProperty rdf:resource="http://www.opengis.net/gml#minAngle"/>
                  <owl:allValuesFrom rdf:resource="http://www.w3.org/2001/XMLSchema#double"/>
               </owl:Restriction>
               <owl:Restriction>
                  <owl:onProperty rdf:resource="http://www.opengis.net/gml#minAngle"/>
                  <owl:minCardinality rdf:datatype="http://www.w3.org/2001/XMLSchema#nonNegativeInteger">0</owl:minCardinality>
               </owl:Restriction>
               <owl:Restriction>
                  <owl:onProperty rdf:resource="http://www.opengis.net/gml#graphType"/>
                  <owl:allValuesFrom rdf:resource="http://www.opengis.net/gml#GraphTypeType"/>
               </owl:Restriction>
               <owl:Restriction>
                  <owl:onProperty rdf:resource="http://www.opengis.net/gml#graphType"/>
                  <owl:minCardinality rdf:datatype="http://www.w3.org/2001/XMLSchema#nonNegativeInteger">0</owl:minCardinality>
               </owl:Restriction>
               <owl:Restriction>
                  <owl:onProperty rdf:resource="http://www.opengis.net/gml#drawingType"/>
                  <owl:allValuesFrom rdf:resource="http://www.opengis.net/gml#DrawingTypeType"/>
               </owl:Restriction>
               <owl:Restriction>
                  <owl:onProperty rdf:resource="http://www.opengis.net/gml#drawingType"/>
                  <owl:minCardinality rdf:datatype="http://www.w3.org/2001/XMLSchema#nonNegativeInteger">0</owl:minCardinality>
               </owl:Restriction>
               <owl:Restriction>
                  <owl:onProperty rdf:resource="http://www.opengis.net/gml#lineType"/>
                  <owl:allValuesFrom rdf:resource="http://www.opengis.net/gml#LineTypeType"/>
               </owl:Restriction>
               <owl:Restriction>
                  <owl:onProperty rdf:resource="http://www.opengis.net/gml#lineType"/>
                  <owl:minCardinality rdf:datatype="http://www.w3.org/2001/XMLSchema#nonNegativeInteger">0</owl:minCardinality>
               </owl:Restriction>
               <owl:Restriction>
                  <owl:onProperty rdf:resource="http://www.opengis.net/gml#aestheticCriteria"/>
                  <owl:allValuesFrom rdf:resource="http://www.opengis.net/gml#AesheticCriteriaType"/>
               </owl:Restriction>
               <owl:Restriction>
                  <owl:onProperty rdf:resource="http://www.opengis.net/gml#aestheticCriteria"/>
                  <owl:minCardinality rdf:datatype="http://www.w3.org/2001/XMLSchema#nonNegativeInteger">0</owl:minCardinality>
               </owl:Restriction>
            </owl:intersectionOf>
         </owl:Class>
      </rdfs:subClassOf>
      <rdfs:subClassOf rdf:resource="http://www.opengis.net/gml#BaseStyleDescriptorType"/>
   </owl:Class>
   <owl:Class rdf:about="http://www.opengis.net/gml#SymbolType">
      <rdfs:comment>[complexType of] The symbol property. Allows for remote referencing of symbols.</rdfs:comment>
      <rdfs:subClassOf>
         <owl:Class>
            <owl:intersectionOf rdf:parseType="Collection">
               <owl:Restriction>
                  <owl:onProperty rdf:resource="http://www.opengis.net/gml#symbolType"/>
                  <owl:allValuesFrom rdf:resource="http://www.opengis.net/gml#SymbolTypeEnumeration"/>
               </owl:Restriction>
               <owl:Restriction>
                  <owl:onProperty rdf:resource="http://www.opengis.net/gml#hastransform"/>
                  <owl:allValuesFrom rdf:resource="http://www.opengis.net/gml#transform"/>
               </owl:Restriction>
               <owl:Restriction>
                  <owl:onProperty rdf:resource="http://www.opengis.net/gml#about"/>
                  <owl:allValuesFrom rdf:resource="http://www.w3.org/2001/XMLSchema#anyURI"/>
               </owl:Restriction>
            </owl:intersectionOf>
         </owl:Class>
      </rdfs:subClassOf>
   </owl:Class>
   <owl:Class rdf:about="http://www.opengis.net/gml#LabelType">
      <rdfs:comment>Label is mixed -- composed of text and XPath expressions used to extract the useful information from the feature.</rdfs:comment>
      <rdfs:subClassOf>
         <owl:Class>
            <owl:intersectionOf rdf:parseType="Collection">
               <owl:Restriction>
                  <owl:onProperty rdf:resource="http://www.opengis.net/gml#LabelExpression"/>
                  <owl:allValuesFrom rdf:resource="http://www.w3.org/2001/XMLSchema#string"/>
               </owl:Restriction>
               <owl:Restriction>
                  <owl:onProperty rdf:resource="http://www.opengis.net/gml#LabelExpression"/>
                  <owl:minCardinality rdf:datatype="http://www.w3.org/2001/XMLSchema#nonNegativeInteger">0</owl:minCardinality>
               </owl:Restriction>
            </owl:intersectionOf>
         </owl:Class>
      </rdfs:subClassOf>
      <rdfs:subClassOf>
         <owl:Class>
            <owl:intersectionOf rdf:parseType="Collection">
               <owl:Restriction>
                  <owl:onProperty rdf:resource="http://www.opengis.net/gml#hastransform"/>
                  <owl:allValuesFrom rdf:resource="http://www.opengis.net/gml#transform"/>
               </owl:Restriction>
            </owl:intersectionOf>
         </owl:Class>
      </rdfs:subClassOf>
   </owl:Class>
   <owl:Class rdf:about="http://www.opengis.net/gml#StyleVariationType">
      <rdfs:comment>Used to vary individual graphic parameters and attributes of the style, symbol or text.</rdfs:comment>
      <rdfs:subClassOf>
         <owl:Class>
            <owl:intersectionOf rdf:parseType="Collection">
               <owl:Restriction>
                  <owl:onProperty rdf:resource="http://www.opengis.net/gml#styleProperty"/>
                  <owl:allValuesFrom rdf:resource="http://www.w3.org/2001/XMLSchema#string"/>
               </owl:Restriction>
               <owl:Restriction>
                  <owl:onProperty rdf:resource="http://www.opengis.net/gml#featurePropertyRange"/>
                  <owl:allValuesFrom rdf:resource="http://www.w3.org/2001/XMLSchema#string"/>
               </owl:Restriction>
            </owl:intersectionOf>
         </owl:Class>
      </rdfs:subClassOf>
      <rdfs:subClassOf>
         <owl:Restriction>
            <owl:onProperty rdf:resource="http://www.opengis.net/gml#hasstring"/>
            <owl:someValuesFrom rdf:resource="http://www.w3.org/2001/XMLSchema#string"/>
         </owl:Restriction>
      </rdfs:subClassOf>
   </owl:Class>
   <owl:DatatypeProperty rdf:about="http://www.opengis.net/gml#hasstring">
      <rdfs:domain rdf:resource="http://www.opengis.net/gml#StyleVariationType"/>
      <rdfs:range rdf:resource="http://www.w3.org/2001/XMLSchema#string"/>
   </owl:DatatypeProperty>
   <owl:Class rdf:about="http://www.opengis.net/gml#AbstractTimeReferenceSystemType">
      <rdfs:comment>This is an abstract class</rdfs:comment>
      <rdfs:comment xml:lang="en">A value in the time domain is measured relative to a temporal reference system. Common 
        types of reference systems include calendars, ordinal temporal reference systems, and 
        temporal coordinate systems (time elapsed since some epoch, e.g. UNIX time).</rdfs:comment>
      <rdfs:subClassOf>
         <owl:Class>
            <owl:intersectionOf rdf:parseType="Collection">
               <owl:Restriction>
                  <owl:onProperty rdf:resource="http://www.opengis.net/gml#domainOfValidity"/>
                  <owl:allValuesFrom rdf:resource="http://www.w3.org/2001/XMLSchema#string"/>
               </owl:Restriction>
               <owl:Restriction>
                  <owl:onProperty rdf:resource="http://www.opengis.net/gml#domainOfValidity"/>
                  <owl:minCardinality rdf:datatype="http://www.w3.org/2001/XMLSchema#nonNegativeInteger">0</owl:minCardinality>
               </owl:Restriction>
            </owl:intersectionOf>
         </owl:Class>
      </rdfs:subClassOf>
      <rdfs:subClassOf rdf:resource="http://www.opengis.net/gml#DefinitionType"/>
   </owl:Class>
   <owl:Class rdf:about="http://www.opengis.net/gml#TimeCoordinateSystemType">
      <rdfs:comment xml:lang="en">A temporal coordinate system is based on a continuous interval scale defined in terms of a single time interval.</rdfs:comment>
      <rdfs:subClassOf>
         <owl:Class>
            <owl:intersectionOf rdf:parseType="Collection">
               <owl:Restriction>
                  <owl:onProperty rdf:resource="http://www.opengis.net/gml#interval"/>
                  <owl:allValuesFrom rdf:resource="http://www.opengis.net/gml#TimeIntervalLengthType"/>
               </owl:Restriction>
            </owl:intersectionOf>
         </owl:Class>
      </rdfs:subClassOf>
      <owl:disjointUnionOf rdf:parseType="Collection">
         <owl:Restriction>
            <owl:onProperty rdf:resource="http://www.opengis.net/gml#originPosition"/>
            <owl:someValuesFrom rdf:resource="http://www.opengis.net/gml#TimePositionType"/>
         </owl:Restriction>
         <owl:Restriction>
            <owl:onProperty rdf:resource="http://www.opengis.net/gml#origin"/>
            <owl:someValuesFrom rdf:resource="http://www.opengis.net/gml#TimeInstantPropertyType"/>
         </owl:Restriction>
      </owl:disjointUnionOf>
      <rdfs:subClassOf rdf:resource="http://www.opengis.net/gml#AbstractTimeReferenceSystemType"/>
   </owl:Class>
   <owl:Class rdf:about="http://www.opengis.net/gml#TimeOrdinalReferenceSystemType">
      <rdfs:comment xml:lang="en">In an ordinal reference system the order of events in time can be well 
      established, but the magnitude of the intervals between them can not be 
      accurately determined (e.g. a stratigraphic sequence).</rdfs:comment>
      <rdfs:subClassOf>
         <owl:Class>
            <owl:intersectionOf rdf:parseType="Collection">
               <owl:Restriction>
                  <owl:onProperty rdf:resource="http://www.opengis.net/gml#component"/>
                  <owl:allValuesFrom rdf:resource="http://www.opengis.net/gml#TimeOrdinalEraPropertyType"/>
               </owl:Restriction>
            </owl:intersectionOf>
         </owl:Class>
      </rdfs:subClassOf>
      <rdfs:subClassOf rdf:resource="http://www.opengis.net/gml#AbstractTimeReferenceSystemType"/>
   </owl:Class>
   <owl:Class rdf:about="http://www.opengis.net/gml#TimeOrdinalEraType">
      <rdfs:comment xml:lang="en">Ordinal temporal reference systems are often hierarchically structured 
      such that an ordinal era at a given level of the hierarchy includes a 
      sequence of shorter, coterminous ordinal eras. This captured using the member/group properties.  
      
      Note that in this schema, TIme Ordinal Era is patterned on TimeEdge, which is a variation from ISO 19108.  
      This is in order to fulfill the requirements of ordinal reference systems based on eras delimited by 
      named points or nodes, which are common in geology, archeology, etc.  
      
      This change is subject of a change proposal to ISO</rdfs:comment>
      <rdfs:subClassOf>
         <owl:Class>
            <owl:intersectionOf rdf:parseType="Collection">
               <owl:Restriction>
                  <owl:onProperty rdf:resource="http://www.opengis.net/gml#relatedTime"/>
                  <owl:allValuesFrom rdf:resource="http://www.opengis.net/gml#RelatedTimeType"/>
               </owl:Restriction>
               <owl:Restriction>
                  <owl:onProperty rdf:resource="http://www.opengis.net/gml#relatedTime"/>
                  <owl:minCardinality rdf:datatype="http://www.w3.org/2001/XMLSchema#nonNegativeInteger">0</owl:minCardinality>
               </owl:Restriction>
               <owl:Restriction>
                  <owl:onProperty rdf:resource="http://www.opengis.net/gml#start"/>
                  <owl:allValuesFrom rdf:resource="http://www.opengis.net/gml#TimeNodePropertyType"/>
               </owl:Restriction>
               <owl:Restriction>
                  <owl:onProperty rdf:resource="http://www.opengis.net/gml#end"/>
                  <owl:allValuesFrom rdf:resource="http://www.opengis.net/gml#TimeNodePropertyType"/>
               </owl:Restriction>
               <owl:Restriction>
                  <owl:onProperty rdf:resource="http://www.opengis.net/gml#extent"/>
                  <owl:allValuesFrom rdf:resource="http://www.opengis.net/gml#TimePeriodPropertyType"/>
               </owl:Restriction>
               <owl:Restriction>
                  <owl:onProperty rdf:resource="http://www.opengis.net/gml#extent"/>
                  <owl:minCardinality rdf:datatype="http://www.w3.org/2001/XMLSchema#nonNegativeInteger">0</owl:minCardinality>
               </owl:Restriction>
               <owl:Restriction>
                  <owl:onProperty rdf:resource="http://www.opengis.net/gml#member"/>
                  <owl:allValuesFrom rdf:resource="http://www.opengis.net/gml#TimeOrdinalEraPropertyType"/>
               </owl:Restriction>
               <owl:Restriction>
                  <owl:onProperty rdf:resource="http://www.opengis.net/gml#member"/>
                  <owl:minCardinality rdf:datatype="http://www.w3.org/2001/XMLSchema#nonNegativeInteger">0</owl:minCardinality>
               </owl:Restriction>
               <owl:Restriction>
                  <owl:onProperty rdf:resource="http://www.opengis.net/gml#group"/>
                  <owl:allValuesFrom rdf:resource="http://www.opengis.net/gml#ReferenceType"/>
               </owl:Restriction>
               <owl:Restriction>
                  <owl:onProperty rdf:resource="http://www.opengis.net/gml#group"/>
                  <owl:minCardinality rdf:datatype="http://www.w3.org/2001/XMLSchema#nonNegativeInteger">0</owl:minCardinality>
               </owl:Restriction>
            </owl:intersectionOf>
         </owl:Class>
      </rdfs:subClassOf>
      <rdfs:subClassOf rdf:resource="http://www.opengis.net/gml#DefinitionType"/>
   </owl:Class>
   <owl:Class rdf:about="http://www.opengis.net/gml#TimeOrdinalEraPropertyType">
      <rdfs:subClassOf>
         <owl:Class>
            <owl:intersectionOf rdf:parseType="Collection">
               <owl:Restriction>
                  <owl:onProperty rdf:resource="http://www.opengis.net/gml#hasTimeOrdinalEra"/>
                  <owl:allValuesFrom rdf:resource="http://www.opengis.net/gml#TimeOrdinalEra"/>
               </owl:Restriction>
            </owl:intersectionOf>
         </owl:Class>
      </rdfs:subClassOf>
   </owl:Class>
   <owl:Class rdf:about="http://www.opengis.net/gml#TimeCalendarType">
      <rdfs:comment xml:lang="en">A calendar is a discrete temporal reference system 
      that provides a basis for defining temporal position to a resolution of one day. 
      A single calendar may reference more than one calendar era.</rdfs:comment>
      <rdfs:subClassOf>
         <owl:Class>
            <owl:intersectionOf rdf:parseType="Collection">
               <owl:Restriction>
                  <owl:onProperty rdf:resource="http://www.opengis.net/gml#referenceFrame"/>
                  <owl:allValuesFrom rdf:resource="http://www.opengis.net/gml#TimeCalendarEraPropertyType"/>
               </owl:Restriction>
            </owl:intersectionOf>
         </owl:Class>
      </rdfs:subClassOf>
      <rdfs:subClassOf rdf:resource="http://www.opengis.net/gml#AbstractTimeReferenceSystemType"/>
   </owl:Class>
   <owl:Class rdf:about="http://www.opengis.net/gml#TimeCalendarPropertyType">
      <rdfs:subClassOf>
         <owl:Class>
            <owl:intersectionOf rdf:parseType="Collection">
               <owl:Restriction>
                  <owl:onProperty rdf:resource="http://www.opengis.net/gml#hasTimeCalendar"/>
                  <owl:allValuesFrom rdf:resource="http://www.opengis.net/gml#TimeCalendar"/>
               </owl:Restriction>
            </owl:intersectionOf>
         </owl:Class>
      </rdfs:subClassOf>
   </owl:Class>
   <owl:Class rdf:about="http://www.opengis.net/gml#TimeCalendarEraType">
      <rdfs:comment xml:lang="en">In every calendar, years are numbered relative to the date of a 
      reference event that defines a calendar era. 
      In this implementation, we omit the back-pointer "datingSystem".</rdfs:comment>
      <rdfs:subClassOf>
         <owl:Class>
            <owl:intersectionOf rdf:parseType="Collection">
               <owl:Restriction>
                  <owl:onProperty rdf:resource="http://www.opengis.net/gml#referenceEvent"/>
                  <owl:allValuesFrom rdf:resource="http://www.opengis.net/gml#StringOrRefType"/>
               </owl:Restriction>
               <owl:Restriction>
                  <owl:onProperty rdf:resource="http://www.opengis.net/gml#referenceDate"/>
                  <owl:allValuesFrom rdf:resource="http://www.w3.org/2001/XMLSchema#date"/>
               </owl:Restriction>
               <owl:Restriction>
                  <owl:onProperty rdf:resource="http://www.opengis.net/gml#referenceDate"/>
                  <owl:minCardinality rdf:datatype="http://www.w3.org/2001/XMLSchema#nonNegativeInteger">0</owl:minCardinality>
               </owl:Restriction>
               <owl:Restriction>
                  <owl:onProperty rdf:resource="http://www.opengis.net/gml#julianReference"/>
                  <owl:allValuesFrom rdf:resource="http://www.w3.org/2001/XMLSchema#decimal"/>
               </owl:Restriction>
               <owl:Restriction>
                  <owl:onProperty rdf:resource="http://www.opengis.net/gml#epochOfUse"/>
                  <owl:allValuesFrom rdf:resource="http://www.opengis.net/gml#TimePeriodPropertyType"/>
               </owl:Restriction>
            </owl:intersectionOf>
         </owl:Class>
      </rdfs:subClassOf>
      <rdfs:subClassOf rdf:resource="http://www.opengis.net/gml#DefinitionType"/>
   </owl:Class>
   <owl:Class rdf:about="http://www.opengis.net/gml#TimeCalendarEraPropertyType">
      <rdfs:subClassOf>
         <owl:Class>
            <owl:intersectionOf rdf:parseType="Collection">
               <owl:Restriction>
                  <owl:onProperty rdf:resource="http://www.opengis.net/gml#hasTimeCalendarEra"/>
                  <owl:allValuesFrom rdf:resource="http://www.opengis.net/gml#TimeCalendarEra"/>
               </owl:Restriction>
            </owl:intersectionOf>
         </owl:Class>
      </rdfs:subClassOf>
   </owl:Class>
   <owl:Class rdf:about="http://www.opengis.net/gml#TimeClockType">
      <rdfs:comment xml:lang="en">A clock provides a basis for defining temporal position within a day. 
      A clock must be used with a calendar in order to provide a complete description of a temporal position 
      within a specific day.</rdfs:comment>
      <rdfs:subClassOf>
         <owl:Class>
            <owl:intersectionOf rdf:parseType="Collection">
               <owl:Restriction>
                  <owl:onProperty rdf:resource="http://www.opengis.net/gml#referenceEvent"/>
                  <owl:allValuesFrom rdf:resource="http://www.opengis.net/gml#StringOrRefType"/>
               </owl:Restriction>
               <owl:Restriction>
                  <owl:onProperty rdf:resource="http://www.opengis.net/gml#referenceTime"/>
                  <owl:allValuesFrom rdf:resource="http://www.w3.org/2001/XMLSchema#time"/>
               </owl:Restriction>
               <owl:Restriction>
                  <owl:onProperty rdf:resource="http://www.opengis.net/gml#utcReference"/>
                  <owl:allValuesFrom rdf:resource="http://www.w3.org/2001/XMLSchema#time"/>
               </owl:Restriction>
               <owl:Restriction>
                  <owl:onProperty rdf:resource="http://www.opengis.net/gml#dateBasis"/>
                  <owl:allValuesFrom rdf:resource="http://www.opengis.net/gml#TimeCalendarPropertyType"/>
               </owl:Restriction>
               <owl:Restriction>
                  <owl:onProperty rdf:resource="http://www.opengis.net/gml#dateBasis"/>
                  <owl:minCardinality rdf:datatype="http://www.w3.org/2001/XMLSchema#nonNegativeInteger">0</owl:minCardinality>
               </owl:Restriction>
            </owl:intersectionOf>
         </owl:Class>
      </rdfs:subClassOf>
      <rdfs:subClassOf rdf:resource="http://www.opengis.net/gml#AbstractTimeReferenceSystemType"/>
   </owl:Class>
   <owl:Class rdf:about="http://www.opengis.net/gml#TimeClockPropertyType">
      <rdfs:subClassOf>
         <owl:Class>
            <owl:intersectionOf rdf:parseType="Collection">
               <owl:Restriction>
                  <owl:onProperty rdf:resource="http://www.opengis.net/gml#hasTimeClock"/>
                  <owl:allValuesFrom rdf:resource="http://www.opengis.net/gml#TimeClock"/>
               </owl:Restriction>
            </owl:intersectionOf>
         </owl:Class>
      </rdfs:subClassOf>
   </owl:Class>
   <owl:Class rdf:about="http://www.opengis.net/gml#TimeTopologyComplexType">
      <rdfs:comment xml:lang="en">A temporal topology complex.</rdfs:comment>
      <rdfs:subClassOf>
         <owl:Class>
            <owl:intersectionOf rdf:parseType="Collection">
               <owl:Restriction>
                  <owl:onProperty rdf:resource="http://www.opengis.net/gml#primitive"/>
                  <owl:allValuesFrom rdf:resource="http://www.opengis.net/gml#TimeTopologyPrimitivePropertyType"/>
               </owl:Restriction>
            </owl:intersectionOf>
         </owl:Class>
      </rdfs:subClassOf>
      <rdfs:subClassOf rdf:resource="http://www.opengis.net/gml#AbstractTimeComplexType"/>
   </owl:Class>
   <owl:Class rdf:about="http://www.opengis.net/gml#TimeTopologyComplexPropertyType">
      <rdfs:comment>A time topology complex property can either be any time topology complex element
       encapsulated in an element of this type or an XLink reference to a remote time topology complex element 
       (where remote includes elements located elsewhere in the same document). 
       Note that either the reference or the contained element must be given, but not both or none.</rdfs:comment>
      <rdfs:subClassOf>
         <owl:Class>
            <owl:intersectionOf rdf:parseType="Collection">
               <owl:Restriction>
                  <owl:onProperty rdf:resource="http://www.opengis.net/gml#hasTimeTopologyComplex"/>
                  <owl:allValuesFrom rdf:resource="http://www.opengis.net/gml#TimeTopologyComplex"/>
               </owl:Restriction>
            </owl:intersectionOf>
         </owl:Class>
      </rdfs:subClassOf>
   </owl:Class>
   <owl:Class rdf:about="http://www.opengis.net/gml#AbstractTimeTopologyPrimitiveType">
      <rdfs:comment>This is an abstract class</rdfs:comment>
      <rdfs:comment xml:lang="en">The element "complex" carries a reference to the complex containing this primitive.</rdfs:comment>
      <rdfs:subClassOf>
         <owl:Class>
            <owl:intersectionOf rdf:parseType="Collection">
               <owl:Restriction>
                  <owl:onProperty rdf:resource="http://www.opengis.net/gml#complex"/>
                  <owl:allValuesFrom rdf:resource="http://www.opengis.net/gml#ReferenceType"/>
               </owl:Restriction>
               <owl:Restriction>
                  <owl:onProperty rdf:resource="http://www.opengis.net/gml#complex"/>
                  <owl:minCardinality rdf:datatype="http://www.w3.org/2001/XMLSchema#nonNegativeInteger">0</owl:minCardinality>
               </owl:Restriction>
            </owl:intersectionOf>
         </owl:Class>
      </rdfs:subClassOf>
      <rdfs:subClassOf rdf:resource="http://www.opengis.net/gml#AbstractTimePrimitiveType"/>
   </owl:Class>
   <owl:Class rdf:about="http://www.opengis.net/gml#TimeTopologyPrimitivePropertyType">
      <rdfs:comment>A time topology primitive property can either hold any time topology complex element
       eor carry an XLink reference to a remote time topology complex element 
       (where remote includes elements located elsewhere in the same document). 
       Note that either the reference or the contained element must be given, but not both or none.</rdfs:comment>
      <rdfs:subClassOf>
         <owl:Class>
            <owl:intersectionOf rdf:parseType="Collection">
               <owl:Restriction>
                  <owl:onProperty rdf:resource="http://www.opengis.net/gml#has_TimeTopologyPrimitive"/>
                  <owl:allValuesFrom rdf:resource="http://www.opengis.net/gml#_TimeTopologyPrimitive"/>
               </owl:Restriction>
            </owl:intersectionOf>
         </owl:Class>
      </rdfs:subClassOf>
   </owl:Class>
   <owl:Class rdf:about="http://www.opengis.net/gml#TimeNodeType">
      <rdfs:comment xml:lang="en">Type declaration of the element "TimeNode".</rdfs:comment>
      <rdfs:subClassOf>
         <owl:Class>
            <owl:intersectionOf rdf:parseType="Collection">
               <owl:Restriction>
                  <owl:onProperty rdf:resource="http://www.opengis.net/gml#previousEdge"/>
                  <owl:allValuesFrom rdf:resource="http://www.opengis.net/gml#TimeEdgePropertyType"/>
               </owl:Restriction>
               <owl:Restriction>
                  <owl:onProperty rdf:resource="http://www.opengis.net/gml#previousEdge"/>
                  <owl:minCardinality rdf:datatype="http://www.w3.org/2001/XMLSchema#nonNegativeInteger">0</owl:minCardinality>
               </owl:Restriction>
               <owl:Restriction>
                  <owl:onProperty rdf:resource="http://www.opengis.net/gml#nextEdge"/>
                  <owl:allValuesFrom rdf:resource="http://www.opengis.net/gml#TimeEdgePropertyType"/>
               </owl:Restriction>
               <owl:Restriction>
                  <owl:onProperty rdf:resource="http://www.opengis.net/gml#nextEdge"/>
                  <owl:minCardinality rdf:datatype="http://www.w3.org/2001/XMLSchema#nonNegativeInteger">0</owl:minCardinality>
               </owl:Restriction>
               <owl:Restriction>
                  <owl:onProperty rdf:resource="http://www.opengis.net/gml#position"/>
                  <owl:allValuesFrom rdf:resource="http://www.opengis.net/gml#TimeInstantPropertyType"/>
               </owl:Restriction>
               <owl:Restriction>
                  <owl:onProperty rdf:resource="http://www.opengis.net/gml#position"/>
                  <owl:minCardinality rdf:datatype="http://www.w3.org/2001/XMLSchema#nonNegativeInteger">0</owl:minCardinality>
               </owl:Restriction>
            </owl:intersectionOf>
         </owl:Class>
      </rdfs:subClassOf>
      <rdfs:subClassOf rdf:resource="http://www.opengis.net/gml#AbstractTimeTopologyPrimitiveType"/>
   </owl:Class>
   <owl:Class rdf:about="http://www.opengis.net/gml#TimeNodePropertyType">
      <rdfs:comment>A time node property can either be any time node element encapsulated in an element of this type 
      or an XLink reference to a remote time node element (where remote includes elements located elsewhere in the same document). 
      Note that either the reference or the contained element must be given, but not both or none.</rdfs:comment>
      <rdfs:subClassOf>
         <owl:Class>
            <owl:intersectionOf rdf:parseType="Collection">
               <owl:Restriction>
                  <owl:onProperty rdf:resource="http://www.opengis.net/gml#hasTimeNode"/>
                  <owl:allValuesFrom rdf:resource="http://www.opengis.net/gml#TimeNode"/>
               </owl:Restriction>
            </owl:intersectionOf>
         </owl:Class>
      </rdfs:subClassOf>
   </owl:Class>
   <owl:Class rdf:about="http://www.opengis.net/gml#TimeEdgeType">
      <rdfs:comment xml:lang="en">Type declaration of the element "TimeEdge".</rdfs:comment>
      <rdfs:subClassOf>
         <owl:Class>
            <owl:intersectionOf rdf:parseType="Collection">
               <owl:Restriction>
                  <owl:onProperty rdf:resource="http://www.opengis.net/gml#start"/>
                  <owl:allValuesFrom rdf:resource="http://www.opengis.net/gml#TimeNodePropertyType"/>
               </owl:Restriction>
               <owl:Restriction>
                  <owl:onProperty rdf:resource="http://www.opengis.net/gml#end"/>
                  <owl:allValuesFrom rdf:resource="http://www.opengis.net/gml#TimeNodePropertyType"/>
               </owl:Restriction>
               <owl:Restriction>
                  <owl:onProperty rdf:resource="http://www.opengis.net/gml#extent"/>
                  <owl:allValuesFrom rdf:resource="http://www.opengis.net/gml#TimePeriodPropertyType"/>
               </owl:Restriction>
               <owl:Restriction>
                  <owl:onProperty rdf:resource="http://www.opengis.net/gml#extent"/>
                  <owl:minCardinality rdf:datatype="http://www.w3.org/2001/XMLSchema#nonNegativeInteger">0</owl:minCardinality>
               </owl:Restriction>
            </owl:intersectionOf>
         </owl:Class>
      </rdfs:subClassOf>
      <rdfs:subClassOf rdf:resource="http://www.opengis.net/gml#AbstractTimeTopologyPrimitiveType"/>
   </owl:Class>
   <owl:Class rdf:about="http://www.opengis.net/gml#TimeEdgePropertyType">
      <rdfs:comment>A time edge property can either be any time edge element encapsulated in an element of this type 
      or an XLink reference to a remote time edge element (where remote includes elements located elsewhere in the same document). 
      Note that either the reference or the contained element must be given, but not both or none.</rdfs:comment>
      <rdfs:subClassOf>
         <owl:Class>
            <owl:intersectionOf rdf:parseType="Collection">
               <owl:Restriction>
                  <owl:onProperty rdf:resource="http://www.opengis.net/gml#hasTimeEdge"/>
                  <owl:allValuesFrom rdf:resource="http://www.opengis.net/gml#TimeEdge"/>
               </owl:Restriction>
            </owl:intersectionOf>
         </owl:Class>
      </rdfs:subClassOf>
   </owl:Class>
   <owl:Class rdf:about="http://www.opengis.net/gml#dynamicProperties">
      <rdfs:subClassOf>
         <owl:Class>
            <owl:intersectionOf rdf:parseType="Collection">
               <owl:Restriction>
                  <owl:onProperty rdf:resource="http://www.opengis.net/gml#hasvalidTime"/>
                  <owl:allValuesFrom rdf:resource="http://www.opengis.net/gml#validTime"/>
               </owl:Restriction>
               <owl:Restriction>
                  <owl:onProperty rdf:resource="http://www.opengis.net/gml#hasvalidTime"/>
                  <owl:minCardinality rdf:datatype="http://www.w3.org/2001/XMLSchema#nonNegativeInteger">0</owl:minCardinality>
               </owl:Restriction>
               <owl:Restriction>
                  <owl:onProperty rdf:resource="http://www.opengis.net/gml#hashistory"/>
                  <owl:allValuesFrom rdf:resource="http://www.opengis.net/gml#history"/>
               </owl:Restriction>
               <owl:Restriction>
                  <owl:onProperty rdf:resource="http://www.opengis.net/gml#hashistory"/>
                  <owl:minCardinality rdf:datatype="http://www.w3.org/2001/XMLSchema#nonNegativeInteger">0</owl:minCardinality>
               </owl:Restriction>
               <owl:Restriction>
                  <owl:onProperty rdf:resource="http://www.opengis.net/gml#hasdataSource"/>
                  <owl:allValuesFrom rdf:resource="http://www.opengis.net/gml#dataSource"/>
               </owl:Restriction>
               <owl:Restriction>
                  <owl:onProperty rdf:resource="http://www.opengis.net/gml#hasdataSource"/>
                  <owl:minCardinality rdf:datatype="http://www.w3.org/2001/XMLSchema#nonNegativeInteger">0</owl:minCardinality>
               </owl:Restriction>
            </owl:intersectionOf>
         </owl:Class>
      </rdfs:subClassOf>
   </owl:Class>
   <owl:Class rdf:about="http://www.opengis.net/gml#geometricPositionGroup">
      <owl:disjointUnionOf rdf:parseType="Collection">
         <owl:Restriction>
            <owl:onProperty rdf:resource="http://www.opengis.net/gml#haspos"/>
            <owl:someValuesFrom rdf:resource="http://www.opengis.net/gml#pos"/>
         </owl:Restriction>
         <owl:Restriction>
            <owl:onProperty rdf:resource="http://www.opengis.net/gml#haspointProperty"/>
            <owl:someValuesFrom rdf:resource="http://www.opengis.net/gml#pointProperty"/>
         </owl:Restriction>
      </owl:disjointUnionOf>
      <rdfs:comment>A geometric position represented either by a DirectPosition or a Point.</rdfs:comment>
   </owl:Class>
   <owl:Class rdf:about="http://www.opengis.net/gml#geometricPositionListGroup">
      <owl:disjointUnionOf rdf:parseType="Collection">
         <owl:Restriction>
            <owl:onProperty rdf:resource="http://www.opengis.net/gml#hasposList"/>
            <owl:someValuesFrom rdf:resource="http://www.opengis.net/gml#posList"/>
         </owl:Restriction>
         <owl:Restriction>
            <owl:onProperty rdf:resource="http://www.opengis.net/gml#hasgeometricPositionGroup"/>
            <owl:allValuesFrom rdf:resource="http://www.opengis.net/gml#geometricPositionGroup"/>
         </owl:Restriction>
      </owl:disjointUnionOf>
      <rdfs:comment>A list of geometric positions represented either by a DirectPosition or a Point.</rdfs:comment>
   </owl:Class>
   <owl:Class rdf:about="http://www.opengis.net/gml#StandardDefinitionProperties">
      <rdfs:subClassOf>
         <owl:Class>
            <owl:intersectionOf rdf:parseType="Collection">
               <owl:Restriction>
                  <owl:onProperty rdf:resource="http://www.opengis.net/gml#hasmetaDataProperty"/>
                  <owl:allValuesFrom rdf:resource="http://www.opengis.net/gml#metaDataProperty"/>
               </owl:Restriction>
               <owl:Restriction>
                  <owl:onProperty rdf:resource="http://www.opengis.net/gml#hasmetaDataProperty"/>
                  <owl:minCardinality rdf:datatype="http://www.w3.org/2001/XMLSchema#nonNegativeInteger">0</owl:minCardinality>
               </owl:Restriction>
               <owl:Restriction>
                  <owl:onProperty rdf:resource="http://www.opengis.net/gml#hasdescription"/>
                  <owl:allValuesFrom rdf:resource="http://www.opengis.net/gml#description"/>
               </owl:Restriction>
               <owl:Restriction>
                  <owl:onProperty rdf:resource="http://www.opengis.net/gml#hasdescription"/>
                  <owl:minCardinality rdf:datatype="http://www.w3.org/2001/XMLSchema#nonNegativeInteger">0</owl:minCardinality>
               </owl:Restriction>
               <owl:Restriction>
                  <owl:onProperty rdf:resource="http://www.opengis.net/gml#hasname"/>
                  <owl:allValuesFrom rdf:resource="http://www.opengis.net/gml#name"/>
               </owl:Restriction>
            </owl:intersectionOf>
         </owl:Class>
      </rdfs:subClassOf>
      <rdfs:comment>This content model group makes it easier to construct types that 
      derive from DefinitionType and its descendents "by restriction".  
      A reference to the group saves having to enumerate the standard definition properties. 
      See definition of StandardObjectProperties for more documentation</rdfs:comment>
   </owl:Class>
   <owl:Class rdf:about="http://www.opengis.net/gml#StandardObjectProperties">
      <rdfs:subClassOf>
         <owl:Class>
            <owl:intersectionOf rdf:parseType="Collection">
               <owl:Restriction>
                  <owl:onProperty rdf:resource="http://www.opengis.net/gml#hasmetaDataProperty"/>
                  <owl:allValuesFrom rdf:resource="http://www.opengis.net/gml#metaDataProperty"/>
               </owl:Restriction>
               <owl:Restriction>
                  <owl:onProperty rdf:resource="http://www.opengis.net/gml#hasmetaDataProperty"/>
                  <owl:minCardinality rdf:datatype="http://www.w3.org/2001/XMLSchema#nonNegativeInteger">0</owl:minCardinality>
               </owl:Restriction>
               <owl:Restriction>
                  <owl:onProperty rdf:resource="http://www.opengis.net/gml#hasdescription"/>
                  <owl:allValuesFrom rdf:resource="http://www.opengis.net/gml#description"/>
               </owl:Restriction>
               <owl:Restriction>
                  <owl:onProperty rdf:resource="http://www.opengis.net/gml#hasdescription"/>
                  <owl:minCardinality rdf:datatype="http://www.w3.org/2001/XMLSchema#nonNegativeInteger">0</owl:minCardinality>
               </owl:Restriction>
               <owl:Restriction>
                  <owl:onProperty rdf:resource="http://www.opengis.net/gml#hasname"/>
                  <owl:allValuesFrom rdf:resource="http://www.opengis.net/gml#name"/>
               </owl:Restriction>
               <owl:Restriction>
                  <owl:onProperty rdf:resource="http://www.opengis.net/gml#hasname"/>
                  <owl:minCardinality rdf:datatype="http://www.w3.org/2001/XMLSchema#nonNegativeInteger">0</owl:minCardinality>
               </owl:Restriction>
            </owl:intersectionOf>
         </owl:Class>
      </rdfs:subClassOf>
      <rdfs:comment>This content model group makes it easier to construct types that 
      derive from AbstractGMLType and its descendents "by restriction".  
      A reference to the group saves having to enumerate the standard object properties.</rdfs:comment>
   </owl:Class>
   <owl:Class rdf:about="http://www.opengis.net/gml#timeLength">
      <owl:disjointUnionOf rdf:parseType="Collection">
         <owl:Restriction>
            <owl:onProperty rdf:resource="http://www.opengis.net/gml#hasduration"/>
            <owl:someValuesFrom rdf:resource="http://www.opengis.net/gml#duration"/>
         </owl:Restriction>
         <owl:Restriction>
            <owl:onProperty rdf:resource="http://www.opengis.net/gml#hastimeInterval"/>
            <owl:someValuesFrom rdf:resource="http://www.opengis.net/gml#timeInterval"/>
         </owl:Restriction>
      </owl:disjointUnionOf>
      <rdfs:comment>This model group is provided as an alternative to the abstract susbstitutionGroup head _timeLength.
    ISO 19136 comment 411</rdfs:comment>
   </owl:Class>
   <owl:Class rdf:about="http://www.opengis.net/gml#PointGrid">
      <rdfs:subClassOf>
         <owl:Class>
            <owl:intersectionOf rdf:parseType="Collection">
               <owl:Restriction>
                  <owl:onProperty rdf:resource="http://www.opengis.net/gml#hasrow"/>
                  <owl:allValuesFrom rdf:resource="http://www.opengis.net/gml#row"/>
               </owl:Restriction>
            </owl:intersectionOf>
         </owl:Class>
      </rdfs:subClassOf>
      <rdfs:comment>Reference points which are organised
   into sequences or grids(sequences of equal length sequences).</rdfs:comment>
   </owl:Class>
   <owl:Class rdf:about="http://www.opengis.net/gml#Value">
      <owl:disjointUnionOf rdf:parseType="Collection">
         <owl:Restriction>
            <owl:onProperty rdf:resource="http://www.opengis.net/gml#has_Object"/>
            <owl:someValuesFrom rdf:resource="http://www.opengis.net/gml#_Object"/>
         </owl:Restriction>
         <owl:Restriction>
            <owl:onProperty rdf:resource="http://www.opengis.net/gml#hasNull"/>
            <owl:someValuesFrom rdf:resource="http://www.opengis.net/gml#Null"/>
         </owl:Restriction>
         <owl:Restriction>
            <owl:onProperty rdf:resource="http://www.opengis.net/gml#hasValueObject"/>
            <owl:allValuesFrom rdf:resource="http://www.opengis.net/gml#ValueObject"/>
         </owl:Restriction>
      </owl:disjointUnionOf>
      <rdfs:comment>Utility choice group which unifies generic Values defined in this schema document with 
      Geometry and Temporal objects and the Measures described above, 
      so that any of these may be used within aggregate Values.</rdfs:comment>
   </owl:Class>
   <owl:Class rdf:about="http://www.opengis.net/gml#ValueObject">
      <owl:disjointUnionOf rdf:parseType="Collection">
         <owl:Restriction>
            <owl:onProperty rdf:resource="http://www.opengis.net/gml#hasCompositeValue"/>
            <owl:someValuesFrom rdf:resource="http://www.opengis.net/gml#CompositeValue"/>
         </owl:Restriction>
         <owl:Restriction>
            <owl:onProperty rdf:resource="http://www.opengis.net/gml#hasScalarValue"/>
            <owl:allValuesFrom rdf:resource="http://www.opengis.net/gml#ScalarValue"/>
         </owl:Restriction>
         <owl:Restriction>
            <owl:onProperty rdf:resource="http://www.opengis.net/gml#hasScalarValueList"/>
            <owl:allValuesFrom rdf:resource="http://www.opengis.net/gml#ScalarValueList"/>
         </owl:Restriction>
         <owl:Restriction>
            <owl:onProperty rdf:resource="http://www.opengis.net/gml#hasValueExtent"/>
            <owl:allValuesFrom rdf:resource="http://www.opengis.net/gml#ValueExtent"/>
         </owl:Restriction>
      </owl:disjointUnionOf>
   </owl:Class>
   <owl:Class rdf:about="http://www.opengis.net/gml#ScalarValue">
      <owl:disjointUnionOf rdf:parseType="Collection">
         <owl:Restriction>
            <owl:onProperty rdf:resource="http://www.opengis.net/gml#hasBoolean"/>
            <owl:someValuesFrom rdf:resource="http://www.opengis.net/gml#Boolean"/>
         </owl:Restriction>
         <owl:Restriction>
            <owl:onProperty rdf:resource="http://www.opengis.net/gml#hasCategory"/>
            <owl:someValuesFrom rdf:resource="http://www.opengis.net/gml#Category"/>
         </owl:Restriction>
         <owl:Restriction>
            <owl:onProperty rdf:resource="http://www.opengis.net/gml#hasQuantity"/>
            <owl:someValuesFrom rdf:resource="http://www.opengis.net/gml#Quantity"/>
         </owl:Restriction>
         <owl:Restriction>
            <owl:onProperty rdf:resource="http://www.opengis.net/gml#hasCount"/>
            <owl:someValuesFrom rdf:resource="http://www.opengis.net/gml#Count"/>
         </owl:Restriction>
      </owl:disjointUnionOf>
   </owl:Class>
   <owl:Class rdf:about="http://www.opengis.net/gml#ScalarValueList">
      <owl:disjointUnionOf rdf:parseType="Collection">
         <owl:Restriction>
            <owl:onProperty rdf:resource="http://www.opengis.net/gml#hasBooleanList"/>
            <owl:someValuesFrom rdf:resource="http://www.opengis.net/gml#BooleanList"/>
         </owl:Restriction>
         <owl:Restriction>
            <owl:onProperty rdf:resource="http://www.opengis.net/gml#hasCategoryList"/>
            <owl:someValuesFrom rdf:resource="http://www.opengis.net/gml#CategoryList"/>
         </owl:Restriction>
         <owl:Restriction>
            <owl:onProperty rdf:resource="http://www.opengis.net/gml#hasQuantityList"/>
            <owl:someValuesFrom rdf:resource="http://www.opengis.net/gml#QuantityList"/>
         </owl:Restriction>
         <owl:Restriction>
            <owl:onProperty rdf:resource="http://www.opengis.net/gml#hasCountList"/>
            <owl:someValuesFrom rdf:resource="http://www.opengis.net/gml#CountList"/>
         </owl:Restriction>
      </owl:disjointUnionOf>
   </owl:Class>
   <owl:Class rdf:about="http://www.opengis.net/gml#ValueExtent">
      <owl:disjointUnionOf rdf:parseType="Collection">
         <owl:Restriction>
            <owl:onProperty rdf:resource="http://www.opengis.net/gml#hasCategoryExtent"/>
            <owl:someValuesFrom rdf:resource="http://www.opengis.net/gml#CategoryExtent"/>
         </owl:Restriction>
         <owl:Restriction>
            <owl:onProperty rdf:resource="http://www.opengis.net/gml#hasQuantityExtent"/>
            <owl:someValuesFrom rdf:resource="http://www.opengis.net/gml#QuantityExtent"/>
         </owl:Restriction>
         <owl:Restriction>
            <owl:onProperty rdf:resource="http://www.opengis.net/gml#hasCountExtent"/>
            <owl:someValuesFrom rdf:resource="http://www.opengis.net/gml#CountExtent"/>
         </owl:Restriction>
      </owl:disjointUnionOf>
   </owl:Class>
   <owl:Class rdf:about="http://www.opengis.net/gml#SRSReferenceGroup">
      <rdfs:subClassOf>
         <owl:Class>
            <owl:intersectionOf rdf:parseType="Collection">
               <owl:Restriction>
                  <owl:onProperty rdf:resource="http://www.opengis.net/gml#srsName"/>
                  <owl:allValuesFrom rdf:resource="http://www.w3.org/2001/XMLSchema#anyURI"/>
               </owl:Restriction>
               <owl:Restriction>
                  <owl:onProperty rdf:resource="http://www.opengis.net/gml#srsDimension"/>
                  <owl:allValuesFrom rdf:resource="http://www.w3.org/2001/XMLSchema#positiveInteger"/>
               </owl:Restriction>
            </owl:intersectionOf>
         </owl:Class>
      </rdfs:subClassOf>
      <rdfs:comment>Optional reference to the CRS used by this geometry, with optional additional information to simplify use when 
      a more complete definition of the CRS is not needed.</rdfs:comment>
   </owl:Class>
   <owl:Class rdf:about="http://www.opengis.net/gml#SRSInformationGroup">
      <rdfs:subClassOf>
         <owl:Class>
            <owl:intersectionOf rdf:parseType="Collection">
               <owl:Restriction>
                  <owl:onProperty rdf:resource="http://www.opengis.net/gml#axisLabels"/>
                  <owl:allValuesFrom rdf:resource="http://www.opengis.net/gml#NCNameList"/>
               </owl:Restriction>
               <owl:Restriction>
                  <owl:onProperty rdf:resource="http://www.opengis.net/gml#uomLabels"/>
                  <owl:allValuesFrom rdf:resource="http://www.opengis.net/gml#NCNameList"/>
               </owl:Restriction>
            </owl:intersectionOf>
         </owl:Class>
      </rdfs:subClassOf>
      <rdfs:comment>Optional additional and redundant information for a CRS to simplify use when a more complete definition of the 
      CRS is not needed. This information shall be the same as included in the more complete definition of the CRS, referenced by the 
      srsName attribute. When the srsName attribute is included, either both or neither of the axisLabels and uomLabels attributes 
      shall be included. When the srsName attribute is omitted, both of these attributes shall be omitted.</rdfs:comment>
   </owl:Class>
   <owl:Class rdf:about="http://www.opengis.net/gml#AssociationAttributeGroup">
      <rdfs:subClassOf>
         <owl:Class>
            <owl:intersectionOf rdf:parseType="Collection">
               <owl:Restriction>
                  <owl:onProperty rdf:resource="http://www.opengis.net/gml#hasremoteSchema"/>
                  <owl:allValuesFrom rdf:resource="http://www.opengis.net/gml#remoteSchema"/>
               </owl:Restriction>
            </owl:intersectionOf>
         </owl:Class>
      </rdfs:subClassOf>
      <rdfs:comment>Attribute group used to enable property elements to refer to their value remotely. It contains the simple link components from xlinks.xsd, with all members optional, and the remoteSchema attribute, which is also optional.  These attributes can be attached to any element, thus allowing it to act as a pointer. The 'remoteSchema' attribute allows an element  that carries link attributes to indicate that the element is declared  in a remote schema rather than by the schema that constrains the current document instance.</rdfs:comment>
   </owl:Class>
   <owl:Class rdf:about="http://www.opengis.net/gml#referenceSystem">
      <rdfs:subClassOf>
         <owl:Class>
            <owl:intersectionOf rdf:parseType="Collection">
               <owl:Restriction>
                  <owl:onProperty rdf:resource="http://www.opengis.net/gml#codeSpace"/>
                  <owl:allValuesFrom rdf:resource="http://www.w3.org/2001/XMLSchema#anyURI"/>
               </owl:Restriction>
               <owl:Restriction>
                  <owl:onProperty rdf:resource="http://www.opengis.net/gml#uom"/>
                  <owl:allValuesFrom rdf:resource="http://www.w3.org/2001/XMLSchema#anyURI"/>
               </owl:Restriction>
            </owl:intersectionOf>
         </owl:Class>
      </rdfs:subClassOf>
   </owl:Class>
   <rdfs:Datatype rdf:about="http://www.opengis.net/gml#direction">
      <owl:equivalentClass>
         <rdfs:Datatype>
            <owl:oneOf>
               <rdf:Description rdf:type="http://www.w3.org/1999/02/22-rdf-syntax-ns#List">
                  <rdf:first rdf:datatype="http://www.w3.org/2001/XMLSchema#string">N</rdf:first>
                  <rdf:rest>
                     <rdf:Description rdf:type="http://www.w3.org/1999/02/22-rdf-syntax-ns#List">
                        <rdf:first rdf:datatype="http://www.w3.org/2001/XMLSchema#string">E</rdf:first>
                        <rdf:rest>
                           <rdf:Description rdf:type="http://www.w3.org/1999/02/22-rdf-syntax-ns#List">
                              <rdf:first rdf:datatype="http://www.w3.org/2001/XMLSchema#string">S</rdf:first>
                              <rdf:rest>
                                 <rdf:Description rdf:type="http://www.w3.org/1999/02/22-rdf-syntax-ns#List">
                                    <rdf:first rdf:datatype="http://www.w3.org/2001/XMLSchema#string">W</rdf:first>
                                    <rdf:rest rdf:resource="http://www.w3.org/1999/02/22-rdf-syntax-ns#nil"/>
                                 </rdf:Description>
                              </rdf:rest>
                           </rdf:Description>
                        </rdf:rest>
                     </rdf:Description>
                  </rdf:rest>
               </rdf:Description>
            </owl:oneOf>
         </rdfs:Datatype>
      </owl:equivalentClass>
      <owl:equivalentClass rdf:resource="http://www.opengis.net/gml#SignType"/>
   </rdfs:Datatype>
   <rdfs:Datatype rdf:about="http://www.opengis.net/gml#DegreeValueType">
      <rdfs:comment>Integer number of degrees in a degree-minute-second or degree-minute angular value, without indication of direction.</rdfs:comment>
      <owl:equivalentClass>
         <rdfs:Datatype>
            <owl:onDatatype rdf:resource="http://www.w3.org/2001/XMLSchema#nonNegativeInteger"/>
            <owl:withRestrictions rdf:parseType="Collection">
               <rdf:Description>
                  <xs:maxInclusive rdf:datatype="http://www.w3.org/2001/XMLSchema#nonNegativeInteger">359</xs:maxInclusive>
               </rdf:Description>
            </owl:withRestrictions>
         </rdfs:Datatype>
      </owl:equivalentClass>
   </rdfs:Datatype>
   <rdfs:Datatype rdf:about="http://www.opengis.net/gml#DecimalMinutesType">
      <rdfs:comment>Decimal number of arc-minutes in a degree-minute angular value.</rdfs:comment>
      <owl:equivalentClass>
         <rdfs:Datatype>
            <owl:onDatatype rdf:resource="http://www.w3.org/2001/XMLSchema#decimal"/>
            <owl:withRestrictions rdf:parseType="Collection">
               <rdf:Description>
                  <xs:minInclusive rdf:datatype="http://www.w3.org/2001/XMLSchema#decimal">0.00</xs:minInclusive>
               </rdf:Description>
               <rdf:Description>
                  <xs:maxExclusive rdf:datatype="http://www.w3.org/2001/XMLSchema#decimal">60.00</xs:maxExclusive>
               </rdf:Description>
            </owl:withRestrictions>
         </rdfs:Datatype>
      </owl:equivalentClass>
   </rdfs:Datatype>
   <rdfs:Datatype rdf:about="http://www.opengis.net/gml#ArcMinutesType">
      <rdfs:comment>Integer number of arc-minutes in a degree-minute-second angular value.</rdfs:comment>
      <owl:equivalentClass>
         <rdfs:Datatype>
            <owl:onDatatype rdf:resource="http://www.w3.org/2001/XMLSchema#nonNegativeInteger"/>
            <owl:withRestrictions rdf:parseType="Collection">
               <rdf:Description>
                  <xs:maxInclusive rdf:datatype="http://www.w3.org/2001/XMLSchema#nonNegativeInteger">59</xs:maxInclusive>
               </rdf:Description>
            </owl:withRestrictions>
         </rdfs:Datatype>
      </owl:equivalentClass>
   </rdfs:Datatype>
   <rdfs:Datatype rdf:about="http://www.opengis.net/gml#ArcSecondsType">
      <rdfs:comment>Number of arc-seconds in a degree-minute-second angular value.</rdfs:comment>
      <owl:equivalentClass>
         <rdfs:Datatype>
            <owl:onDatatype rdf:resource="http://www.w3.org/2001/XMLSchema#decimal"/>
            <owl:withRestrictions rdf:parseType="Collection">
               <rdf:Description>
                  <xs:minInclusive rdf:datatype="http://www.w3.org/2001/XMLSchema#decimal">0.00</xs:minInclusive>
               </rdf:Description>
               <rdf:Description>
                  <xs:maxExclusive rdf:datatype="http://www.w3.org/2001/XMLSchema#decimal">60.00</xs:maxExclusive>
               </rdf:Description>
            </owl:withRestrictions>
         </rdfs:Datatype>
      </owl:equivalentClass>
   </rdfs:Datatype>
   <rdfs:Datatype rdf:about="http://www.opengis.net/gml#NullEnumeration">
      <rdfs:comment> Some common reasons for a null value:   
      
        innapplicable - the object does not have a value
        missing - The correct value is not readily available to the sender of this data.  
                           Furthermore, a correct value may not exist.
        template - the value will be available later
        unknown - The correct value is not known to, and not computable by, the sender of this data. 
                           However, a correct value probably exists.
        withheld - the value is not divulged 
        
        other:reason - as indicated by "reason" string
        
        Specific communities may agree to assign more strict semantics when these terms are used in a particular context.  
      </rdfs:comment>
      <owl:equivalentClass>
         <rdfs:Datatype>
            <owl:oneOf>
               <rdf:Description rdf:type="http://www.w3.org/1999/02/22-rdf-syntax-ns#List">
                  <rdf:first rdf:datatype="http://www.w3.org/2001/XMLSchema#string">inapplicable</rdf:first>
                  <rdf:rest>
                     <rdf:Description rdf:type="http://www.w3.org/1999/02/22-rdf-syntax-ns#List">
                        <rdf:first rdf:datatype="http://www.w3.org/2001/XMLSchema#string">missing</rdf:first>
                        <rdf:rest>
                           <rdf:Description rdf:type="http://www.w3.org/1999/02/22-rdf-syntax-ns#List">
                              <rdf:first rdf:datatype="http://www.w3.org/2001/XMLSchema#string">template</rdf:first>
                              <rdf:rest>
                                 <rdf:Description rdf:type="http://www.w3.org/1999/02/22-rdf-syntax-ns#List">
                                    <rdf:first rdf:datatype="http://www.w3.org/2001/XMLSchema#string">unknown</rdf:first>
                                    <rdf:rest>
                                       <rdf:Description rdf:type="http://www.w3.org/1999/02/22-rdf-syntax-ns#List">
                                          <rdf:first rdf:datatype="http://www.w3.org/2001/XMLSchema#string">withheld</rdf:first>
                                          <rdf:rest rdf:resource="http://www.w3.org/1999/02/22-rdf-syntax-ns#nil"/>
                                       </rdf:Description>
                                    </rdf:rest>
                                 </rdf:Description>
                              </rdf:rest>
                           </rdf:Description>
                        </rdf:rest>
                     </rdf:Description>
                  </rdf:rest>
               </rdf:Description>
            </owl:oneOf>
         </rdfs:Datatype>
      </owl:equivalentClass>
      <owl:equivalentClass rdf:resource="string"/>
   </rdfs:Datatype>
   <rdfs:Datatype rdf:about="http://www.opengis.net/gml#NullType">
      <rdfs:comment>Utility type for null elements.  The value may be selected from one of the enumerated tokens, or may be a URI in which case this should identify a resource which describes the reason for the null. </rdfs:comment>
      <owl:equivalentClass rdf:resource="http://www.opengis.net/gml#NullEnumeration"/>
      <owl:equivalentClass rdf:resource="http://www.w3.org/2001/XMLSchema#anyURI"/>
   </rdfs:Datatype>
   <rdfs:Datatype rdf:about="http://www.opengis.net/gml#SignType">
      <rdfs:comment>Utility type used in various places 
      - e.g. to indicate the direction of topological objects;
      "+" for forwards, or "-" for backwards.</rdfs:comment>
      <owl:equivalentClass>
         <rdfs:Datatype>
            <owl:oneOf>
               <rdf:Description rdf:type="http://www.w3.org/1999/02/22-rdf-syntax-ns#List">
                  <rdf:first rdf:datatype="http://www.w3.org/2001/XMLSchema#string">-</rdf:first>
                  <rdf:rest>
                     <rdf:Description rdf:type="http://www.w3.org/1999/02/22-rdf-syntax-ns#List">
                        <rdf:first rdf:datatype="http://www.w3.org/2001/XMLSchema#string">+</rdf:first>
                        <rdf:rest rdf:resource="http://www.w3.org/1999/02/22-rdf-syntax-ns#nil"/>
                     </rdf:Description>
                  </rdf:rest>
               </rdf:Description>
            </owl:oneOf>
         </rdfs:Datatype>
      </owl:equivalentClass>
   </rdfs:Datatype>
   <rdfs:Datatype rdf:about="http://www.opengis.net/gml#booleanOrNull">
      <rdfs:comment>Union of the XML Schema boolean type and the GML Nulltype.  An element which uses this type may have content which is either a boolean {0,1,true,false} or a value from Nulltype</rdfs:comment>
      <owl:equivalentClass rdf:resource="http://www.opengis.net/gml#NullEnumeration"/>
      <owl:equivalentClass rdf:resource="http://www.w3.org/2001/XMLSchema#boolean"/>
      <owl:equivalentClass rdf:resource="http://www.w3.org/2001/XMLSchema#anyURI"/>
   </rdfs:Datatype>
   <rdfs:Datatype rdf:about="http://www.opengis.net/gml#booleanOrNullList">
      <rdfs:comment>XML List based on the union type defined above.  An element declared with this type contains a space-separated list of boolean values {0,1,true,false} with null values interspersed as needed</rdfs:comment>
      <owl:equivalentClass rdf:resource="http://www.w3.org/2001/XMLSchema#string"/>
   </rdfs:Datatype>
   <rdfs:Datatype rdf:about="http://www.opengis.net/gml#booleanList">
      <rdfs:comment>XML List based on XML Schema boolean type.  An element of this type contains a space-separated list of boolean values {0,1,true,false}</rdfs:comment>
      <owl:equivalentClass rdf:resource="http://www.w3.org/2001/XMLSchema#string"/>
   </rdfs:Datatype>
   <rdfs:Datatype rdf:about="http://www.opengis.net/gml#stringOrNull">
      <rdfs:comment>Union of the XML Schema string type and the GML Nulltype.  An element which uses this type may have content which is either a string or a value from Nulltype.  Note that a "string" may contain whitespace.  </rdfs:comment>
      <owl:equivalentClass rdf:resource="http://www.opengis.net/gml#NullEnumeration"/>
      <owl:equivalentClass rdf:resource="http://www.w3.org/2001/XMLSchema#string"/>
      <owl:equivalentClass rdf:resource="http://www.w3.org/2001/XMLSchema#anyURI"/>
   </rdfs:Datatype>
   <rdfs:Datatype rdf:about="http://www.opengis.net/gml#NameOrNull">
      <rdfs:comment>Union of the XML Schema Name type and the GML Nulltype.  An element which uses this type may have content which is either a Name or a value from Nulltype.  Note that a "Name" may not contain whitespace.  </rdfs:comment>
      <owl:equivalentClass rdf:resource="http://www.opengis.net/gml#NullEnumeration"/>
      <owl:equivalentClass rdf:resource="http://www.w3.org/2001/XMLSchema#Name"/>
      <owl:equivalentClass rdf:resource="http://www.w3.org/2001/XMLSchema#anyURI"/>
   </rdfs:Datatype>
   <rdfs:Datatype rdf:about="http://www.opengis.net/gml#NameOrNullList">
      <rdfs:comment>XML List based on the union type defined above.  An element declared with this type contains a space-separated list of Name values with null values interspersed as needed</rdfs:comment>
      <owl:equivalentClass rdf:resource="http://www.w3.org/2001/XMLSchema#string"/>
   </rdfs:Datatype>
   <rdfs:Datatype rdf:about="http://www.opengis.net/gml#NameList">
      <rdfs:comment>XML List based on XML Schema Name type.  An element of this type contains a space-separated list of Name values</rdfs:comment>
      <owl:equivalentClass rdf:resource="http://www.w3.org/2001/XMLSchema#string"/>
   </rdfs:Datatype>
   <rdfs:Datatype rdf:about="http://www.opengis.net/gml#doubleOrNull">
      <rdfs:comment>Union of the XML Schema double type and the GML Nulltype.  An element which uses this type may have content which is either a double or a value from Nulltype</rdfs:comment>
      <owl:equivalentClass rdf:resource="http://www.opengis.net/gml#NullEnumeration"/>
      <owl:equivalentClass rdf:resource="http://www.w3.org/2001/XMLSchema#double"/>
      <owl:equivalentClass rdf:resource="http://www.w3.org/2001/XMLSchema#anyURI"/>
   </rdfs:Datatype>
   <rdfs:Datatype rdf:about="http://www.opengis.net/gml#doubleOrNullList">
      <rdfs:comment>XML List based on the union type defined above.  An element declared with this type contains a space-separated list of double values with null values interspersed as needed</rdfs:comment>
      <owl:equivalentClass rdf:resource="http://www.w3.org/2001/XMLSchema#string"/>
   </rdfs:Datatype>
   <rdfs:Datatype rdf:about="http://www.opengis.net/gml#doubleList">
      <rdfs:comment>XML List based on XML Schema double type.  An element of this type contains a space-separated list of double values</rdfs:comment>
      <owl:equivalentClass rdf:resource="http://www.w3.org/2001/XMLSchema#string"/>
   </rdfs:Datatype>
   <rdfs:Datatype rdf:about="http://www.opengis.net/gml#integerOrNull">
      <rdfs:comment>Union of the XML Schema integer type and the GML Nulltype.  An element which uses this type may have content which is either an integer or a value from Nulltype</rdfs:comment>
      <owl:equivalentClass rdf:resource="http://www.opengis.net/gml#NullEnumeration"/>
      <owl:equivalentClass rdf:resource="http://www.w3.org/2001/XMLSchema#integer"/>
      <owl:equivalentClass rdf:resource="http://www.w3.org/2001/XMLSchema#anyURI"/>
   </rdfs:Datatype>
   <rdfs:Datatype rdf:about="http://www.opengis.net/gml#integerOrNullList">
      <rdfs:comment>XML List based on the union type defined above.  An element declared with this type contains a space-separated list of integer values with null values interspersed as needed</rdfs:comment>
      <owl:equivalentClass rdf:resource="http://www.w3.org/2001/XMLSchema#string"/>
   </rdfs:Datatype>
   <rdfs:Datatype rdf:about="http://www.opengis.net/gml#integerList">
      <rdfs:comment>XML List based on XML Schema integer type.  An element of this type contains a space-separated list of integer values</rdfs:comment>
      <owl:equivalentClass rdf:resource="http://www.w3.org/2001/XMLSchema#string"/>
   </rdfs:Datatype>
   <rdfs:Datatype rdf:about="http://www.opengis.net/gml#NCNameList">
      <rdfs:comment>A set of values, representing a list of token with the lexical value space of NCName. The tokens are seperated by whitespace.</rdfs:comment>
      <owl:equivalentClass rdf:resource="http://www.w3.org/2001/XMLSchema#string"/>
   </rdfs:Datatype>
   <rdfs:Datatype rdf:about="http://www.opengis.net/gml#QNameList">
      <rdfs:comment>A set of values, representing a list of token with the lexical value space of QName. The tokens are seperated by whitespace.</rdfs:comment>
      <owl:equivalentClass rdf:resource="http://www.w3.org/2001/XMLSchema#string"/>
   </rdfs:Datatype>
   <rdfs:Datatype rdf:about="http://www.opengis.net/gml#relativePosition">
      <owl:equivalentClass>
         <rdfs:Datatype>
            <owl:oneOf>
               <rdf:Description rdf:type="http://www.w3.org/1999/02/22-rdf-syntax-ns#List">
                  <rdf:first rdf:datatype="http://www.w3.org/2001/XMLSchema#string">Before</rdf:first>
                  <rdf:rest>
                     <rdf:Description rdf:type="http://www.w3.org/1999/02/22-rdf-syntax-ns#List">
                        <rdf:first rdf:datatype="http://www.w3.org/2001/XMLSchema#string">After</rdf:first>
                        <rdf:rest>
                           <rdf:Description rdf:type="http://www.w3.org/1999/02/22-rdf-syntax-ns#List">
                              <rdf:first rdf:datatype="http://www.w3.org/2001/XMLSchema#string">Begins</rdf:first>
                              <rdf:rest>
                                 <rdf:Description rdf:type="http://www.w3.org/1999/02/22-rdf-syntax-ns#List">
                                    <rdf:first rdf:datatype="http://www.w3.org/2001/XMLSchema#string">Ends</rdf:first>
                                    <rdf:rest>
                                       <rdf:Description rdf:type="http://www.w3.org/1999/02/22-rdf-syntax-ns#List">
                                          <rdf:first rdf:datatype="http://www.w3.org/2001/XMLSchema#string">During</rdf:first>
                                          <rdf:rest>
                                             <rdf:Description rdf:type="http://www.w3.org/1999/02/22-rdf-syntax-ns#List">
                                                <rdf:first rdf:datatype="http://www.w3.org/2001/XMLSchema#string">Equals</rdf:first>
                                                <rdf:rest>
                                                   <rdf:Description rdf:type="http://www.w3.org/1999/02/22-rdf-syntax-ns#List">
                                                      <rdf:first rdf:datatype="http://www.w3.org/2001/XMLSchema#string">Contains</rdf:first>
                                                      <rdf:rest>
                                                         <rdf:Description rdf:type="http://www.w3.org/1999/02/22-rdf-syntax-ns#List">
                                                            <rdf:first rdf:datatype="http://www.w3.org/2001/XMLSchema#string">Overlaps</rdf:first>
                                                            <rdf:rest>
                                                               <rdf:Description rdf:type="http://www.w3.org/1999/02/22-rdf-syntax-ns#List">
                                                                  <rdf:first rdf:datatype="http://www.w3.org/2001/XMLSchema#string">Meets</rdf:first>
                                                                  <rdf:rest>
                                                                     <rdf:Description rdf:type="http://www.w3.org/1999/02/22-rdf-syntax-ns#List">
                                                                        <rdf:first rdf:datatype="http://www.w3.org/2001/XMLSchema#string">OverlappedBy</rdf:first>
                                                                        <rdf:rest>
                                                                           <rdf:Description rdf:type="http://www.w3.org/1999/02/22-rdf-syntax-ns#List">
                                                                              <rdf:first rdf:datatype="http://www.w3.org/2001/XMLSchema#string">MetBy</rdf:first>
                                                                              <rdf:rest>
                                                                                 <rdf:Description rdf:type="http://www.w3.org/1999/02/22-rdf-syntax-ns#List">
                                                                                    <rdf:first rdf:datatype="http://www.w3.org/2001/XMLSchema#string">BegunBy</rdf:first>
                                                                                    <rdf:rest>
                                                                                       <rdf:Description rdf:type="http://www.w3.org/1999/02/22-rdf-syntax-ns#List">
                                                                                          <rdf:first rdf:datatype="http://www.w3.org/2001/XMLSchema#string">EndedBy</rdf:first>
                                                                                          <rdf:rest rdf:resource="http://www.w3.org/1999/02/22-rdf-syntax-ns#nil"/>
                                                                                       </rdf:Description>
                                                                                    </rdf:rest>
                                                                                 </rdf:Description>
                                                                              </rdf:rest>
                                                                           </rdf:Description>
                                                                        </rdf:rest>
                                                                     </rdf:Description>
                                                                  </rdf:rest>
                                                               </rdf:Description>
                                                            </rdf:rest>
                                                         </rdf:Description>
                                                      </rdf:rest>
                                                   </rdf:Description>
                                                </rdf:rest>
                                             </rdf:Description>
                                          </rdf:rest>
                                       </rdf:Description>
                                    </rdf:rest>
                                 </rdf:Description>
                              </rdf:rest>
                           </rdf:Description>
                        </rdf:rest>
                     </rdf:Description>
                  </rdf:rest>
               </rdf:Description>
            </owl:oneOf>
         </rdfs:Datatype>
      </owl:equivalentClass>
   </rdfs:Datatype>
   <owl:DatatypeProperty rdf:about="http://www.opengis.net/gml#hasrelativePosition">
      <rdfs:range rdf:resource="http://www.opengis.net/gml#relativePosition"/>
   </owl:DatatypeProperty>
   <rdfs:Datatype rdf:about="http://www.opengis.net/gml#TimeUnitType">
      <rdfs:comment xml:lang="en">Standard units for measuring time intervals (see ISO 31-1).</rdfs:comment>
      <owl:equivalentClass>
         <rdfs:Datatype>
            <owl:oneOf>
               <rdf:Description rdf:type="http://www.w3.org/1999/02/22-rdf-syntax-ns#List">
                  <rdf:first rdf:datatype="http://www.w3.org/2001/XMLSchema#string">year</rdf:first>
                  <rdf:rest>
                     <rdf:Description rdf:type="http://www.w3.org/1999/02/22-rdf-syntax-ns#List">
                        <rdf:first rdf:datatype="http://www.w3.org/2001/XMLSchema#string">day</rdf:first>
                        <rdf:rest>
                           <rdf:Description rdf:type="http://www.w3.org/1999/02/22-rdf-syntax-ns#List">
                              <rdf:first rdf:datatype="http://www.w3.org/2001/XMLSchema#string">hour</rdf:first>
                              <rdf:rest>
                                 <rdf:Description rdf:type="http://www.w3.org/1999/02/22-rdf-syntax-ns#List">
                                    <rdf:first rdf:datatype="http://www.w3.org/2001/XMLSchema#string">minute</rdf:first>
                                    <rdf:rest>
                                       <rdf:Description rdf:type="http://www.w3.org/1999/02/22-rdf-syntax-ns#List">
                                          <rdf:first rdf:datatype="http://www.w3.org/2001/XMLSchema#string">second</rdf:first>
                                          <rdf:rest rdf:resource="http://www.w3.org/1999/02/22-rdf-syntax-ns#nil"/>
                                       </rdf:Description>
                                    </rdf:rest>
                                 </rdf:Description>
                              </rdf:rest>
                           </rdf:Description>
                        </rdf:rest>
                     </rdf:Description>
                  </rdf:rest>
               </rdf:Description>
            </owl:oneOf>
         </rdfs:Datatype>
      </owl:equivalentClass>
      <owl:equivalentClass rdf:resource="string"/>
   </rdfs:Datatype>
   <rdfs:Datatype rdf:about="http://www.opengis.net/gml#TimePositionUnion">
      <rdfs:comment xml:lang="en">The ISO 19108:2002 hierarchy of subtypes for temporal position are collapsed 
      by defining a union of XML Schema simple types for indicating temporal position relative 
      to a specific reference system. 
      
      Dates and dateTime may be indicated with varying degrees of precision.  
      dateTime by itself does not allow right-truncation, except for fractions of seconds. 
      When used with non-Gregorian calendars based on years, months, days, 
      the same lexical representation should still be used, with leading zeros added if the 
      year value would otherwise have fewer than four digits.  
      
      An ordinal position may be referenced via URI identifying the definition of an ordinal era.  
      
      A time coordinate value is indicated as a decimal (e.g. UNIX time, GPS calendar).</rdfs:comment>
      <owl:equivalentClass rdf:resource="http://www.opengis.net/gml#CalDate"/>
      <owl:equivalentClass rdf:resource="http://www.w3.org/2001/XMLSchema#time"/>
      <owl:equivalentClass rdf:resource="http://www.w3.org/2001/XMLSchema#dateTime"/>
      <owl:equivalentClass rdf:resource="http://www.w3.org/2001/XMLSchema#anyURI"/>
      <owl:equivalentClass rdf:resource="http://www.w3.org/2001/XMLSchema#decimal"/>
   </rdfs:Datatype>
   <rdfs:Datatype rdf:about="http://www.opengis.net/gml#CalDate">
      <rdfs:comment xml:lang="en">Calendar dates may be indicated with varying degrees of precision, 
      using year, year-month, date. 
      When used with non-Gregorian calendars based on years, months, days, 
      the same lexical representation should still be used, with leading zeros added if the 
      year value would otherwise have fewer than four digits.  
      time is used for a position that recurs daily (see clause 5.4.4.2 of ISO 19108:2002).</rdfs:comment>
      <owl:equivalentClass rdf:resource="http://www.w3.org/2001/XMLSchema#date"/>
      <owl:equivalentClass rdf:resource="http://www.w3.org/2001/XMLSchema#gYearMonth"/>
      <owl:equivalentClass rdf:resource="http://www.w3.org/2001/XMLSchema#gYear"/>
   </rdfs:Datatype>
   <rdfs:Datatype rdf:about="http://www.opengis.net/gml#TimeIndeterminateValueType">
      <rdfs:comment xml:lang="en">This enumerated data type specifies values for indeterminate positions.</rdfs:comment>
      <owl:equivalentClass>
         <rdfs:Datatype>
            <owl:oneOf>
               <rdf:Description rdf:type="http://www.w3.org/1999/02/22-rdf-syntax-ns#List">
                  <rdf:first rdf:datatype="http://www.w3.org/2001/XMLSchema#string">after</rdf:first>
                  <rdf:rest>
                     <rdf:Description rdf:type="http://www.w3.org/1999/02/22-rdf-syntax-ns#List">
                        <rdf:first rdf:datatype="http://www.w3.org/2001/XMLSchema#string">before</rdf:first>
                        <rdf:rest>
                           <rdf:Description rdf:type="http://www.w3.org/1999/02/22-rdf-syntax-ns#List">
                              <rdf:first rdf:datatype="http://www.w3.org/2001/XMLSchema#string">now</rdf:first>
                              <rdf:rest>
                                 <rdf:Description rdf:type="http://www.w3.org/1999/02/22-rdf-syntax-ns#List">
                                    <rdf:first rdf:datatype="http://www.w3.org/2001/XMLSchema#string">unknown</rdf:first>
                                    <rdf:rest rdf:resource="http://www.w3.org/1999/02/22-rdf-syntax-ns#nil"/>
                                 </rdf:Description>
                              </rdf:rest>
                           </rdf:Description>
                        </rdf:rest>
                     </rdf:Description>
                  </rdf:rest>
               </rdf:Description>
            </owl:oneOf>
         </rdfs:Datatype>
      </owl:equivalentClass>
   </rdfs:Datatype>
   <rdfs:Datatype rdf:about="http://www.opengis.net/gml#CompassPointEnumeration">
      <owl:equivalentClass>
         <rdfs:Datatype>
            <owl:oneOf>
               <rdf:Description rdf:type="http://www.w3.org/1999/02/22-rdf-syntax-ns#List">
                  <rdf:first rdf:datatype="http://www.w3.org/2001/XMLSchema#string">N</rdf:first>
                  <rdf:rest>
                     <rdf:Description rdf:type="http://www.w3.org/1999/02/22-rdf-syntax-ns#List">
                        <rdf:first rdf:datatype="http://www.w3.org/2001/XMLSchema#string">NNE</rdf:first>
                        <rdf:rest>
                           <rdf:Description rdf:type="http://www.w3.org/1999/02/22-rdf-syntax-ns#List">
                              <rdf:first rdf:datatype="http://www.w3.org/2001/XMLSchema#string">NE</rdf:first>
                              <rdf:rest>
                                 <rdf:Description rdf:type="http://www.w3.org/1999/02/22-rdf-syntax-ns#List">
                                    <rdf:first rdf:datatype="http://www.w3.org/2001/XMLSchema#string">ENE</rdf:first>
                                    <rdf:rest>
                                       <rdf:Description rdf:type="http://www.w3.org/1999/02/22-rdf-syntax-ns#List">
                                          <rdf:first rdf:datatype="http://www.w3.org/2001/XMLSchema#string">E</rdf:first>
                                          <rdf:rest>
                                             <rdf:Description rdf:type="http://www.w3.org/1999/02/22-rdf-syntax-ns#List">
                                                <rdf:first rdf:datatype="http://www.w3.org/2001/XMLSchema#string">ESE</rdf:first>
                                                <rdf:rest>
                                                   <rdf:Description rdf:type="http://www.w3.org/1999/02/22-rdf-syntax-ns#List">
                                                      <rdf:first rdf:datatype="http://www.w3.org/2001/XMLSchema#string">SE</rdf:first>
                                                      <rdf:rest>
                                                         <rdf:Description rdf:type="http://www.w3.org/1999/02/22-rdf-syntax-ns#List">
                                                            <rdf:first rdf:datatype="http://www.w3.org/2001/XMLSchema#string">SSE</rdf:first>
                                                            <rdf:rest>
                                                               <rdf:Description rdf:type="http://www.w3.org/1999/02/22-rdf-syntax-ns#List">
                                                                  <rdf:first rdf:datatype="http://www.w3.org/2001/XMLSchema#string">S</rdf:first>
                                                                  <rdf:rest>
                                                                     <rdf:Description rdf:type="http://www.w3.org/1999/02/22-rdf-syntax-ns#List">
                                                                        <rdf:first rdf:datatype="http://www.w3.org/2001/XMLSchema#string">SSW</rdf:first>
                                                                        <rdf:rest>
                                                                           <rdf:Description rdf:type="http://www.w3.org/1999/02/22-rdf-syntax-ns#List">
                                                                              <rdf:first rdf:datatype="http://www.w3.org/2001/XMLSchema#string">SW</rdf:first>
                                                                              <rdf:rest>
                                                                                 <rdf:Description rdf:type="http://www.w3.org/1999/02/22-rdf-syntax-ns#List">
                                                                                    <rdf:first rdf:datatype="http://www.w3.org/2001/XMLSchema#string">WSW</rdf:first>
                                                                                    <rdf:rest>
                                                                                       <rdf:Description rdf:type="http://www.w3.org/1999/02/22-rdf-syntax-ns#List">
                                                                                          <rdf:first rdf:datatype="http://www.w3.org/2001/XMLSchema#string">W</rdf:first>
                                                                                          <rdf:rest>
                                                                                             <rdf:Description rdf:type="http://www.w3.org/1999/02/22-rdf-syntax-ns#List">
                                                                                                <rdf:first rdf:datatype="http://www.w3.org/2001/XMLSchema#string">WNW</rdf:first>
                                                                                                <rdf:rest>
                                                                                                   <rdf:Description rdf:type="http://www.w3.org/1999/02/22-rdf-syntax-ns#List">
                                                                                                      <rdf:first rdf:datatype="http://www.w3.org/2001/XMLSchema#string">NW</rdf:first>
                                                                                                      <rdf:rest>
                                                                                                         <rdf:Description rdf:type="http://www.w3.org/1999/02/22-rdf-syntax-ns#List">
                                                                                                            <rdf:first rdf:datatype="http://www.w3.org/2001/XMLSchema#string">NNW</rdf:first>
                                                                                                            <rdf:rest rdf:resource="http://www.w3.org/1999/02/22-rdf-syntax-ns#nil"/>
                                                                                                         </rdf:Description>
                                                                                                      </rdf:rest>
                                                                                                   </rdf:Description>
                                                                                                </rdf:rest>
                                                                                             </rdf:Description>
                                                                                          </rdf:rest>
                                                                                       </rdf:Description>
                                                                                    </rdf:rest>
                                                                                 </rdf:Description>
                                                                              </rdf:rest>
                                                                           </rdf:Description>
                                                                        </rdf:rest>
                                                                     </rdf:Description>
                                                                  </rdf:rest>
                                                               </rdf:Description>
                                                            </rdf:rest>
                                                         </rdf:Description>
                                                      </rdf:rest>
                                                   </rdf:Description>
                                                </rdf:rest>
                                             </rdf:Description>
                                          </rdf:rest>
                                       </rdf:Description>
                                    </rdf:rest>
                                 </rdf:Description>
                              </rdf:rest>
                           </rdf:Description>
                        </rdf:rest>
                     </rdf:Description>
                  </rdf:rest>
               </rdf:Description>
            </owl:oneOf>
         </rdfs:Datatype>
      </owl:equivalentClass>
   </rdfs:Datatype>
   <rdfs:Datatype rdf:about="http://www.opengis.net/gml#CurveInterpolationType">
      <rdfs:comment>CurveInterpolationType is a list of codes that may be used to identify the interpolation mechanisms specified by an
application schema.</rdfs:comment>
      <owl:equivalentClass>
         <rdfs:Datatype>
            <owl:oneOf>
               <rdf:Description rdf:type="http://www.w3.org/1999/02/22-rdf-syntax-ns#List">
                  <rdf:first rdf:datatype="http://www.w3.org/2001/XMLSchema#string">linear</rdf:first>
                  <rdf:rest>
                     <rdf:Description rdf:type="http://www.w3.org/1999/02/22-rdf-syntax-ns#List">
                        <rdf:first rdf:datatype="http://www.w3.org/2001/XMLSchema#string">geodesic</rdf:first>
                        <rdf:rest>
                           <rdf:Description rdf:type="http://www.w3.org/1999/02/22-rdf-syntax-ns#List">
                              <rdf:first rdf:datatype="http://www.w3.org/2001/XMLSchema#string">circularArc3Points</rdf:first>
                              <rdf:rest>
                                 <rdf:Description rdf:type="http://www.w3.org/1999/02/22-rdf-syntax-ns#List">
                                    <rdf:first rdf:datatype="http://www.w3.org/2001/XMLSchema#string">circularArc2PointWithBulge</rdf:first>
                                    <rdf:rest>
                                       <rdf:Description rdf:type="http://www.w3.org/1999/02/22-rdf-syntax-ns#List">
                                          <rdf:first rdf:datatype="http://www.w3.org/2001/XMLSchema#string">circularArcCenterPointWithRadius</rdf:first>
                                          <rdf:rest>
                                             <rdf:Description rdf:type="http://www.w3.org/1999/02/22-rdf-syntax-ns#List">
                                                <rdf:first rdf:datatype="http://www.w3.org/2001/XMLSchema#string">elliptical</rdf:first>
                                                <rdf:rest>
                                                   <rdf:Description rdf:type="http://www.w3.org/1999/02/22-rdf-syntax-ns#List">
                                                      <rdf:first rdf:datatype="http://www.w3.org/2001/XMLSchema#string">clothoid</rdf:first>
                                                      <rdf:rest>
                                                         <rdf:Description rdf:type="http://www.w3.org/1999/02/22-rdf-syntax-ns#List">
                                                            <rdf:first rdf:datatype="http://www.w3.org/2001/XMLSchema#string">conic</rdf:first>
                                                            <rdf:rest>
                                                               <rdf:Description rdf:type="http://www.w3.org/1999/02/22-rdf-syntax-ns#List">
                                                                  <rdf:first rdf:datatype="http://www.w3.org/2001/XMLSchema#string">polynomialSpline</rdf:first>
                                                                  <rdf:rest>
                                                                     <rdf:Description rdf:type="http://www.w3.org/1999/02/22-rdf-syntax-ns#List">
                                                                        <rdf:first rdf:datatype="http://www.w3.org/2001/XMLSchema#string">cubicSpline</rdf:first>
                                                                        <rdf:rest>
                                                                           <rdf:Description rdf:type="http://www.w3.org/1999/02/22-rdf-syntax-ns#List">
                                                                              <rdf:first rdf:datatype="http://www.w3.org/2001/XMLSchema#string">rationalSpline</rdf:first>
                                                                              <rdf:rest rdf:resource="http://www.w3.org/1999/02/22-rdf-syntax-ns#nil"/>
                                                                           </rdf:Description>
                                                                        </rdf:rest>
                                                                     </rdf:Description>
                                                                  </rdf:rest>
                                                               </rdf:Description>
                                                            </rdf:rest>
                                                         </rdf:Description>
                                                      </rdf:rest>
                                                   </rdf:Description>
                                                </rdf:rest>
                                             </rdf:Description>
                                          </rdf:rest>
                                       </rdf:Description>
                                    </rdf:rest>
                                 </rdf:Description>
                              </rdf:rest>
                           </rdf:Description>
                        </rdf:rest>
                     </rdf:Description>
                  </rdf:rest>
               </rdf:Description>
            </owl:oneOf>
         </rdfs:Datatype>
      </owl:equivalentClass>
   </rdfs:Datatype>
   <rdfs:Datatype rdf:about="http://www.opengis.net/gml#SurfaceInterpolationType">
      <rdfs:comment>SurfaceInterpolationType is a list of codes that may be used to identify the interpolation mechanisms specified by an
application schema.</rdfs:comment>
      <owl:equivalentClass>
         <rdfs:Datatype>
            <owl:oneOf>
               <rdf:Description rdf:type="http://www.w3.org/1999/02/22-rdf-syntax-ns#List">
                  <rdf:first rdf:datatype="http://www.w3.org/2001/XMLSchema#string">none</rdf:first>
                  <rdf:rest>
                     <rdf:Description rdf:type="http://www.w3.org/1999/02/22-rdf-syntax-ns#List">
                        <rdf:first rdf:datatype="http://www.w3.org/2001/XMLSchema#string">planar</rdf:first>
                        <rdf:rest>
                           <rdf:Description rdf:type="http://www.w3.org/1999/02/22-rdf-syntax-ns#List">
                              <rdf:first rdf:datatype="http://www.w3.org/2001/XMLSchema#string">spherical</rdf:first>
                              <rdf:rest>
                                 <rdf:Description rdf:type="http://www.w3.org/1999/02/22-rdf-syntax-ns#List">
                                    <rdf:first rdf:datatype="http://www.w3.org/2001/XMLSchema#string">elliptical</rdf:first>
                                    <rdf:rest>
                                       <rdf:Description rdf:type="http://www.w3.org/1999/02/22-rdf-syntax-ns#List">
                                          <rdf:first rdf:datatype="http://www.w3.org/2001/XMLSchema#string">conic</rdf:first>
                                          <rdf:rest>
                                             <rdf:Description rdf:type="http://www.w3.org/1999/02/22-rdf-syntax-ns#List">
                                                <rdf:first rdf:datatype="http://www.w3.org/2001/XMLSchema#string">tin</rdf:first>
                                                <rdf:rest>
                                                   <rdf:Description rdf:type="http://www.w3.org/1999/02/22-rdf-syntax-ns#List">
                                                      <rdf:first rdf:datatype="http://www.w3.org/2001/XMLSchema#string">parametricCurve</rdf:first>
                                                      <rdf:rest>
                                                         <rdf:Description rdf:type="http://www.w3.org/1999/02/22-rdf-syntax-ns#List">
                                                            <rdf:first rdf:datatype="http://www.w3.org/2001/XMLSchema#string">polynomialSpline</rdf:first>
                                                            <rdf:rest>
                                                               <rdf:Description rdf:type="http://www.w3.org/1999/02/22-rdf-syntax-ns#List">
                                                                  <rdf:first rdf:datatype="http://www.w3.org/2001/XMLSchema#string">rationalSpline</rdf:first>
                                                                  <rdf:rest>
                                                                     <rdf:Description rdf:type="http://www.w3.org/1999/02/22-rdf-syntax-ns#List">
                                                                        <rdf:first rdf:datatype="http://www.w3.org/2001/XMLSchema#string">triangulatedSpline</rdf:first>
                                                                        <rdf:rest rdf:resource="http://www.w3.org/1999/02/22-rdf-syntax-ns#nil"/>
                                                                     </rdf:Description>
                                                                  </rdf:rest>
                                                               </rdf:Description>
                                                            </rdf:rest>
                                                         </rdf:Description>
                                                      </rdf:rest>
                                                   </rdf:Description>
                                                </rdf:rest>
                                             </rdf:Description>
                                          </rdf:rest>
                                       </rdf:Description>
                                    </rdf:rest>
                                 </rdf:Description>
                              </rdf:rest>
                           </rdf:Description>
                        </rdf:rest>
                     </rdf:Description>
                  </rdf:rest>
               </rdf:Description>
            </owl:oneOf>
         </rdfs:Datatype>
      </owl:equivalentClass>
   </rdfs:Datatype>
   <rdfs:Datatype rdf:about="http://www.opengis.net/gml#KnotTypesType">
      <rdfs:comment>Defines allowed values for the knots` type. Uniform knots implies that all knots are of multiplicity 1 and they differ by a positive constant from the preceding knot. Knots are quasi-uniform iff they are of multiplicity (degree + 1) at the ends, of multiplicity 1 elsewhere, and they differ by a positive constant from the preceding knot.</rdfs:comment>
      <owl:equivalentClass>
         <rdfs:Datatype>
            <owl:oneOf>
               <rdf:Description rdf:type="http://www.w3.org/1999/02/22-rdf-syntax-ns#List">
                  <rdf:first rdf:datatype="http://www.w3.org/2001/XMLSchema#string">uniform</rdf:first>
                  <rdf:rest>
                     <rdf:Description rdf:type="http://www.w3.org/1999/02/22-rdf-syntax-ns#List">
                        <rdf:first rdf:datatype="http://www.w3.org/2001/XMLSchema#string">quasiUniform</rdf:first>
                        <rdf:rest>
                           <rdf:Description rdf:type="http://www.w3.org/1999/02/22-rdf-syntax-ns#List">
                              <rdf:first rdf:datatype="http://www.w3.org/2001/XMLSchema#string">piecewiseBezier</rdf:first>
                              <rdf:rest rdf:resource="http://www.w3.org/1999/02/22-rdf-syntax-ns#nil"/>
                           </rdf:Description>
                        </rdf:rest>
                     </rdf:Description>
                  </rdf:rest>
               </rdf:Description>
            </owl:oneOf>
         </rdfs:Datatype>
      </owl:equivalentClass>
   </rdfs:Datatype>
   <rdfs:Datatype rdf:about="http://www.opengis.net/gml#FileValueModelType">
      <rdfs:comment>List of codes that identifies the file structure model for records stored in files.</rdfs:comment>
      <owl:equivalentClass>
         <rdfs:Datatype>
            <owl:oneOf>
               <rdf:Description rdf:type="http://www.w3.org/1999/02/22-rdf-syntax-ns#List">
                  <rdf:first rdf:datatype="http://www.w3.org/2001/XMLSchema#string">Record Interleaved</rdf:first>
                  <rdf:rest rdf:resource="http://www.w3.org/1999/02/22-rdf-syntax-ns#nil"/>
               </rdf:Description>
            </owl:oneOf>
         </rdfs:Datatype>
      </owl:equivalentClass>
   </rdfs:Datatype>
   <rdfs:Datatype rdf:about="http://www.opengis.net/gml#SequenceRuleNames">
      <rdfs:comment>List of codes (adopted from ISO 19123 Annex C) that identifies the rule for traversing a grid to correspond with the sequence of members of the rangeSet.</rdfs:comment>
      <owl:equivalentClass>
         <rdfs:Datatype>
            <owl:oneOf>
               <rdf:Description rdf:type="http://www.w3.org/1999/02/22-rdf-syntax-ns#List">
                  <rdf:first rdf:datatype="http://www.w3.org/2001/XMLSchema#string">Linear</rdf:first>
                  <rdf:rest>
                     <rdf:Description rdf:type="http://www.w3.org/1999/02/22-rdf-syntax-ns#List">
                        <rdf:first rdf:datatype="http://www.w3.org/2001/XMLSchema#string">Boustrophedonic</rdf:first>
                        <rdf:rest>
                           <rdf:Description rdf:type="http://www.w3.org/1999/02/22-rdf-syntax-ns#List">
                              <rdf:first rdf:datatype="http://www.w3.org/2001/XMLSchema#string">Cantor-diagonal</rdf:first>
                              <rdf:rest>
                                 <rdf:Description rdf:type="http://www.w3.org/1999/02/22-rdf-syntax-ns#List">
                                    <rdf:first rdf:datatype="http://www.w3.org/2001/XMLSchema#string">Spiral</rdf:first>
                                    <rdf:rest>
                                       <rdf:Description rdf:type="http://www.w3.org/1999/02/22-rdf-syntax-ns#List">
                                          <rdf:first rdf:datatype="http://www.w3.org/2001/XMLSchema#string">Morton</rdf:first>
                                          <rdf:rest>
                                             <rdf:Description rdf:type="http://www.w3.org/1999/02/22-rdf-syntax-ns#List">
                                                <rdf:first rdf:datatype="http://www.w3.org/2001/XMLSchema#string">Hilbert</rdf:first>
                                                <rdf:rest rdf:resource="http://www.w3.org/1999/02/22-rdf-syntax-ns#nil"/>
                                             </rdf:Description>
                                          </rdf:rest>
                                       </rdf:Description>
                                    </rdf:rest>
                                 </rdf:Description>
                              </rdf:rest>
                           </rdf:Description>
                        </rdf:rest>
                     </rdf:Description>
                  </rdf:rest>
               </rdf:Description>
            </owl:oneOf>
         </rdfs:Datatype>
      </owl:equivalentClass>
   </rdfs:Datatype>
   <rdfs:Datatype rdf:about="http://www.opengis.net/gml#IncrementOrder">
      <rdfs:comment>The enumeration value here indicates the incrementation order  to be used on the first 2 axes, i.e. "+x-y" means that the points on the first axis are to be traversed from lowest to highest and  the points on the second axis are to be traversed from highest to lowest. The points on all other axes (if any) beyond the first 2 are assumed to increment from lowest to highest.</rdfs:comment>
      <owl:equivalentClass>
         <rdfs:Datatype>
            <owl:oneOf>
               <rdf:Description rdf:type="http://www.w3.org/1999/02/22-rdf-syntax-ns#List">
                  <rdf:first rdf:datatype="http://www.w3.org/2001/XMLSchema#string">+x+y</rdf:first>
                  <rdf:rest>
                     <rdf:Description rdf:type="http://www.w3.org/1999/02/22-rdf-syntax-ns#List">
                        <rdf:first rdf:datatype="http://www.w3.org/2001/XMLSchema#string">+y+x</rdf:first>
                        <rdf:rest>
                           <rdf:Description rdf:type="http://www.w3.org/1999/02/22-rdf-syntax-ns#List">
                              <rdf:first rdf:datatype="http://www.w3.org/2001/XMLSchema#string">+x-y</rdf:first>
                              <rdf:rest>
                                 <rdf:Description rdf:type="http://www.w3.org/1999/02/22-rdf-syntax-ns#List">
                                    <rdf:first rdf:datatype="http://www.w3.org/2001/XMLSchema#string">-x-y</rdf:first>
                                    <rdf:rest rdf:resource="http://www.w3.org/1999/02/22-rdf-syntax-ns#nil"/>
                                 </rdf:Description>
                              </rdf:rest>
                           </rdf:Description>
                        </rdf:rest>
                     </rdf:Description>
                  </rdf:rest>
               </rdf:Description>
            </owl:oneOf>
         </rdfs:Datatype>
      </owl:equivalentClass>
   </rdfs:Datatype>
   <rdfs:Datatype rdf:about="http://www.opengis.net/gml#CountExtentType">
      <rdfs:comment>Restriction of list type to store a 2-point range of frequency values. If one member is a null, then this is a single ended interval.</rdfs:comment>
      <owl:equivalentClass rdf:resource="http://www.opengis.net/gml#integerOrNullList"/>
   </rdfs:Datatype>
   <rdfs:Datatype rdf:about="http://www.opengis.net/gml#isSphere">
      <owl:equivalentClass>
         <rdfs:Datatype>
            <owl:oneOf>
               <rdf:Description rdf:type="http://www.w3.org/1999/02/22-rdf-syntax-ns#List">
                  <rdf:first rdf:datatype="http://www.w3.org/2001/XMLSchema#string">sphere</rdf:first>
                  <rdf:rest rdf:resource="http://www.w3.org/1999/02/22-rdf-syntax-ns#nil"/>
               </rdf:Description>
            </owl:oneOf>
         </rdfs:Datatype>
      </owl:equivalentClass>
   </rdfs:Datatype>
   <owl:DatatypeProperty rdf:about="http://www.opengis.net/gml#hasisSphere">
      <rdfs:range rdf:resource="http://www.opengis.net/gml#isSphere"/>
   </owl:DatatypeProperty>
   <rdfs:Datatype rdf:about="http://www.opengis.net/gml#QueryGrammarEnumeration">
      <rdfs:comment>Used to specify the grammar of the feature query mechanism.</rdfs:comment>
      <owl:equivalentClass>
         <rdfs:Datatype>
            <owl:oneOf>
               <rdf:Description rdf:type="http://www.w3.org/1999/02/22-rdf-syntax-ns#List">
                  <rdf:first rdf:datatype="http://www.w3.org/2001/XMLSchema#string">xpath</rdf:first>
                  <rdf:rest>
                     <rdf:Description rdf:type="http://www.w3.org/1999/02/22-rdf-syntax-ns#List">
                        <rdf:first rdf:datatype="http://www.w3.org/2001/XMLSchema#string">xquery</rdf:first>
                        <rdf:rest>
                           <rdf:Description rdf:type="http://www.w3.org/1999/02/22-rdf-syntax-ns#List">
                              <rdf:first rdf:datatype="http://www.w3.org/2001/XMLSchema#string">other</rdf:first>
                              <rdf:rest rdf:resource="http://www.w3.org/1999/02/22-rdf-syntax-ns#nil"/>
                           </rdf:Description>
                        </rdf:rest>
                     </rdf:Description>
                  </rdf:rest>
               </rdf:Description>
            </owl:oneOf>
         </rdfs:Datatype>
      </owl:equivalentClass>
   </rdfs:Datatype>
   <rdfs:Datatype rdf:about="http://www.opengis.net/gml#SymbolTypeEnumeration">
      <rdfs:comment>Used to specify the type of the symbol used.</rdfs:comment>
      <owl:equivalentClass>
         <rdfs:Datatype>
            <owl:oneOf>
               <rdf:Description rdf:type="http://www.w3.org/1999/02/22-rdf-syntax-ns#List">
                  <rdf:first rdf:datatype="http://www.w3.org/2001/XMLSchema#string">svg</rdf:first>
                  <rdf:rest>
                     <rdf:Description rdf:type="http://www.w3.org/1999/02/22-rdf-syntax-ns#List">
                        <rdf:first rdf:datatype="http://www.w3.org/2001/XMLSchema#string">xpath</rdf:first>
                        <rdf:rest>
                           <rdf:Description rdf:type="http://www.w3.org/1999/02/22-rdf-syntax-ns#List">
                              <rdf:first rdf:datatype="http://www.w3.org/2001/XMLSchema#string">other</rdf:first>
                              <rdf:rest rdf:resource="http://www.w3.org/1999/02/22-rdf-syntax-ns#nil"/>
                           </rdf:Description>
                        </rdf:rest>
                     </rdf:Description>
                  </rdf:rest>
               </rdf:Description>
            </owl:oneOf>
         </rdfs:Datatype>
      </owl:equivalentClass>
   </rdfs:Datatype>
   <rdfs:Datatype rdf:about="http://www.opengis.net/gml#GraphTypeType">
      <rdfs:comment>Graph-specific styling property.</rdfs:comment>
      <owl:equivalentClass>
         <rdfs:Datatype>
            <owl:oneOf>
               <rdf:Description rdf:type="http://www.w3.org/1999/02/22-rdf-syntax-ns#List">
                  <rdf:first rdf:datatype="http://www.w3.org/2001/XMLSchema#string">TREE</rdf:first>
                  <rdf:rest>
                     <rdf:Description rdf:type="http://www.w3.org/1999/02/22-rdf-syntax-ns#List">
                        <rdf:first rdf:datatype="http://www.w3.org/2001/XMLSchema#string">BICONNECTED</rdf:first>
                        <rdf:rest rdf:resource="http://www.w3.org/1999/02/22-rdf-syntax-ns#nil"/>
                     </rdf:Description>
                  </rdf:rest>
               </rdf:Description>
            </owl:oneOf>
         </rdfs:Datatype>
      </owl:equivalentClass>
   </rdfs:Datatype>
   <rdfs:Datatype rdf:about="http://www.opengis.net/gml#DrawingTypeType">
      <rdfs:comment>Graph-specific styling property.</rdfs:comment>
      <owl:equivalentClass>
         <rdfs:Datatype>
            <owl:oneOf>
               <rdf:Description rdf:type="http://www.w3.org/1999/02/22-rdf-syntax-ns#List">
                  <rdf:first rdf:datatype="http://www.w3.org/2001/XMLSchema#string">POLYLINE</rdf:first>
                  <rdf:rest>
                     <rdf:Description rdf:type="http://www.w3.org/1999/02/22-rdf-syntax-ns#List">
                        <rdf:first rdf:datatype="http://www.w3.org/2001/XMLSchema#string">ORTHOGONAL</rdf:first>
                        <rdf:rest rdf:resource="http://www.w3.org/1999/02/22-rdf-syntax-ns#nil"/>
                     </rdf:Description>
                  </rdf:rest>
               </rdf:Description>
            </owl:oneOf>
         </rdfs:Datatype>
      </owl:equivalentClass>
   </rdfs:Datatype>
   <rdfs:Datatype rdf:about="http://www.opengis.net/gml#LineTypeType">
      <rdfs:comment>Graph-specific styling property.</rdfs:comment>
      <owl:equivalentClass>
         <rdfs:Datatype>
            <owl:oneOf>
               <rdf:Description rdf:type="http://www.w3.org/1999/02/22-rdf-syntax-ns#List">
                  <rdf:first rdf:datatype="http://www.w3.org/2001/XMLSchema#string">STRAIGHT</rdf:first>
                  <rdf:rest>
                     <rdf:Description rdf:type="http://www.w3.org/1999/02/22-rdf-syntax-ns#List">
                        <rdf:first rdf:datatype="http://www.w3.org/2001/XMLSchema#string">BENT</rdf:first>
                        <rdf:rest rdf:resource="http://www.w3.org/1999/02/22-rdf-syntax-ns#nil"/>
                     </rdf:Description>
                  </rdf:rest>
               </rdf:Description>
            </owl:oneOf>
         </rdfs:Datatype>
      </owl:equivalentClass>
   </rdfs:Datatype>
   <rdfs:Datatype rdf:about="http://www.opengis.net/gml#AesheticCriteriaType">
      <rdfs:comment>Graph-specific styling property.</rdfs:comment>
      <owl:equivalentClass>
         <rdfs:Datatype>
            <owl:oneOf>
               <rdf:Description rdf:type="http://www.w3.org/1999/02/22-rdf-syntax-ns#List">
                  <rdf:first rdf:datatype="http://www.w3.org/2001/XMLSchema#string">MIN_CROSSINGS</rdf:first>
                  <rdf:rest>
                     <rdf:Description rdf:type="http://www.w3.org/1999/02/22-rdf-syntax-ns#List">
                        <rdf:first rdf:datatype="http://www.w3.org/2001/XMLSchema#string">MIN_AREA</rdf:first>
                        <rdf:rest>
                           <rdf:Description rdf:type="http://www.w3.org/1999/02/22-rdf-syntax-ns#List">
                              <rdf:first rdf:datatype="http://www.w3.org/2001/XMLSchema#string">MIN_BENDS</rdf:first>
                              <rdf:rest>
                                 <rdf:Description rdf:type="http://www.w3.org/1999/02/22-rdf-syntax-ns#List">
                                    <rdf:first rdf:datatype="http://www.w3.org/2001/XMLSchema#string">MAX_BENDS</rdf:first>
                                    <rdf:rest>
                                       <rdf:Description rdf:type="http://www.w3.org/1999/02/22-rdf-syntax-ns#List">
                                          <rdf:first rdf:datatype="http://www.w3.org/2001/XMLSchema#string">UNIFORM_BENDS</rdf:first>
                                          <rdf:rest>
                                             <rdf:Description rdf:type="http://www.w3.org/1999/02/22-rdf-syntax-ns#List">
                                                <rdf:first rdf:datatype="http://www.w3.org/2001/XMLSchema#string">MIN_SLOPES</rdf:first>
                                                <rdf:rest>
                                                   <rdf:Description rdf:type="http://www.w3.org/1999/02/22-rdf-syntax-ns#List">
                                                      <rdf:first rdf:datatype="http://www.w3.org/2001/XMLSchema#string">MIN_EDGE_LENGTH</rdf:first>
                                                      <rdf:rest>
                                                         <rdf:Description rdf:type="http://www.w3.org/1999/02/22-rdf-syntax-ns#List">
                                                            <rdf:first rdf:datatype="http://www.w3.org/2001/XMLSchema#string">MAX_EDGE_LENGTH</rdf:first>
                                                            <rdf:rest>
                                                               <rdf:Description rdf:type="http://www.w3.org/1999/02/22-rdf-syntax-ns#List">
                                                                  <rdf:first rdf:datatype="http://www.w3.org/2001/XMLSchema#string">UNIFORM_EDGE_LENGTH</rdf:first>
                                                                  <rdf:rest>
                                                                     <rdf:Description rdf:type="http://www.w3.org/1999/02/22-rdf-syntax-ns#List">
                                                                        <rdf:first rdf:datatype="http://www.w3.org/2001/XMLSchema#string">MAX_ANGULAR_RESOLUTION</rdf:first>
                                                                        <rdf:rest>
                                                                           <rdf:Description rdf:type="http://www.w3.org/1999/02/22-rdf-syntax-ns#List">
                                                                              <rdf:first rdf:datatype="http://www.w3.org/2001/XMLSchema#string">MIN_ASPECT_RATIO</rdf:first>
                                                                              <rdf:rest>
                                                                                 <rdf:Description rdf:type="http://www.w3.org/1999/02/22-rdf-syntax-ns#List">
                                                                                    <rdf:first rdf:datatype="http://www.w3.org/2001/XMLSchema#string">MAX_SYMMETRIES</rdf:first>
                                                                                    <rdf:rest rdf:resource="http://www.w3.org/1999/02/22-rdf-syntax-ns#nil"/>
                                                                                 </rdf:Description>
                                                                              </rdf:rest>
                                                                           </rdf:Description>
                                                                        </rdf:rest>
                                                                     </rdf:Description>
                                                                  </rdf:rest>
                                                               </rdf:Description>
                                                            </rdf:rest>
                                                         </rdf:Description>
                                                      </rdf:rest>
                                                   </rdf:Description>
                                                </rdf:rest>
                                             </rdf:Description>
                                          </rdf:rest>
                                       </rdf:Description>
                                    </rdf:rest>
                                 </rdf:Description>
                              </rdf:rest>
                           </rdf:Description>
                        </rdf:rest>
                     </rdf:Description>
                  </rdf:rest>
               </rdf:Description>
            </owl:oneOf>
         </rdfs:Datatype>
      </owl:equivalentClass>
   </rdfs:Datatype>
   <rdfs:Datatype rdf:about="http://www.opengis.net/gml#SuccessionType">
      <rdfs:comment>Feature succession is a semantic relationship derived from evaluation of observer, and 
      Feature Substitution, Feature Division and Feature Fusion are defined as associations between 
      previous features and next features in the temporal context. 
      Successions shall be represented in either following two ways. 
      * define a temporal topological complex element as a feature element 
      * define an association same as temporal topological complex between features.</rdfs:comment>
      <owl:equivalentClass>
         <rdfs:Datatype>
            <owl:oneOf>
               <rdf:Description rdf:type="http://www.w3.org/1999/02/22-rdf-syntax-ns#List">
                  <rdf:first rdf:datatype="http://www.w3.org/2001/XMLSchema#string">substitution</rdf:first>
                  <rdf:rest>
                     <rdf:Description rdf:type="http://www.w3.org/1999/02/22-rdf-syntax-ns#List">
                        <rdf:first rdf:datatype="http://www.w3.org/2001/XMLSchema#string">division</rdf:first>
                        <rdf:rest>
                           <rdf:Description rdf:type="http://www.w3.org/1999/02/22-rdf-syntax-ns#List">
                              <rdf:first rdf:datatype="http://www.w3.org/2001/XMLSchema#string">fusion</rdf:first>
                              <rdf:rest>
                                 <rdf:Description rdf:type="http://www.w3.org/1999/02/22-rdf-syntax-ns#List">
                                    <rdf:first rdf:datatype="http://www.w3.org/2001/XMLSchema#string">initiation</rdf:first>
                                    <rdf:rest rdf:resource="http://www.w3.org/1999/02/22-rdf-syntax-ns#nil"/>
                                 </rdf:Description>
                              </rdf:rest>
                           </rdf:Description>
                        </rdf:rest>
                     </rdf:Description>
                  </rdf:rest>
               </rdf:Description>
            </owl:oneOf>
         </rdfs:Datatype>
      </owl:equivalentClass>
   </rdfs:Datatype>
   <owl:DatatypeProperty rdf:about="http://www.opengis.net/gml#frame">
      <rdfs:domain rdf:resource="http://www.opengis.net/gml#EnvelopeWithTimePeriodType"/>
      <rdfs:range rdf:resource="http://www.w3.org/2001/XMLSchema#anyURI"/>
   </owl:DatatypeProperty>
   <owl:DatatypeProperty rdf:about="http://www.opengis.net/gml#priority">
      <rdfs:domain rdf:resource="http://www.opengis.net/gml#PriorityLocationPropertyType"/>
      <rdfs:range rdf:resource="http://www.w3.org/2001/XMLSchema#string"/>
   </owl:DatatypeProperty>
   <owl:DatatypeProperty rdf:about="http://www.opengis.net/gml#gid">
      <rdfs:domain rdf:resource="http://www.opengis.net/gml#AbstractGeometryType"/>
      <rdfs:range rdf:resource="http://www.w3.org/2001/XMLSchema#string"/>
   </owl:DatatypeProperty>
   <owl:DatatypeProperty rdf:about="http://www.opengis.net/gml#srsName">
      <rdfs:domain rdf:resource="http://www.opengis.net/gml#SRSReferenceGroup"/>
      <rdfs:range rdf:resource="http://www.w3.org/2001/XMLSchema#anyURI"/>
   </owl:DatatypeProperty>
   <owl:DatatypeProperty rdf:about="http://www.opengis.net/gml#srsDimension">
      <rdfs:domain rdf:resource="http://www.opengis.net/gml#SRSReferenceGroup"/>
      <rdfs:range rdf:resource="http://www.w3.org/2001/XMLSchema#positiveInteger"/>
   </owl:DatatypeProperty>
   <owl:DatatypeProperty rdf:about="http://www.opengis.net/gml#axisLabels">
      <rdfs:domain rdf:resource="http://www.opengis.net/gml#SRSInformationGroup"/>
      <rdfs:range rdf:resource="http://www.opengis.net/gml#NCNameList"/>
   </owl:DatatypeProperty>
   <owl:DatatypeProperty rdf:about="http://www.opengis.net/gml#uomLabels">
      <rdfs:domain rdf:resource="http://www.opengis.net/gml#SRSInformationGroup"/>
      <rdfs:range rdf:resource="http://www.opengis.net/gml#NCNameList"/>
   </owl:DatatypeProperty>
   <owl:DatatypeProperty rdf:about="http://www.opengis.net/gml#count">
      <rdfs:domain rdf:resource="http://www.opengis.net/gml#DirectPositionListType"/>
      <rdfs:range rdf:resource="http://www.w3.org/2001/XMLSchema#positiveInteger"/>
   </owl:DatatypeProperty>
   <owl:DatatypeProperty rdf:about="http://www.opengis.net/gml#direction">
      <rdfs:domain rdf:resource="http://www.opengis.net/gml#DegreesType"/>
      <rdfs:range rdf:resource="http://www.w3.org/2001/XMLSchema#string"/>
   </owl:DatatypeProperty>
   <owl:DatatypeProperty rdf:about="http://www.opengis.net/gml#uom">
      <rdfs:domain rdf:resource="http://www.opengis.net/gml#UnitOfMeasureType"/>
      <rdfs:range rdf:resource="http://www.w3.org/2001/XMLSchema#anyURI"/>
   </owl:DatatypeProperty>
   <owl:DatatypeProperty rdf:about="http://www.opengis.net/gml#exponent">
      <rdfs:domain rdf:resource="http://www.opengis.net/gml#DerivationUnitTermType"/>
      <rdfs:range rdf:resource="http://www.w3.org/2001/XMLSchema#integer"/>
   </owl:DatatypeProperty>
   <owl:DatatypeProperty rdf:about="http://www.opengis.net/gml#hasid">
      <rdfs:domain rdf:resource="http://www.opengis.net/gml#DefinitionType"/>
      <rdfs:range rdf:resource="http://www.opengis.net/gml#id"/>
   </owl:DatatypeProperty>
   <owl:DatatypeProperty rdf:about="http://www.opengis.net/gml#hasid">
      <rdfs:domain rdf:resource="http://www.opengis.net/gml#AbstractGMLType"/>
      <rdfs:range rdf:resource="http://www.opengis.net/gml#id"/>
   </owl:DatatypeProperty>
   <owl:DatatypeProperty rdf:about="http://www.opengis.net/gml#hasid">
      <rdfs:domain rdf:resource="http://www.opengis.net/gml#AbstractMetaDataType"/>
      <rdfs:range rdf:resource="http://www.opengis.net/gml#id"/>
   </owl:DatatypeProperty>
   <owl:DatatypeProperty rdf:about="http://www.opengis.net/gml#about">
      <rdfs:domain rdf:resource="http://www.opengis.net/gml#MetaDataPropertyType"/>
      <rdfs:range rdf:resource="http://www.w3.org/2001/XMLSchema#anyURI"/>
   </owl:DatatypeProperty>
   <rdfs:Datatype rdf:about="http://www.opengis.net/gml#id">
      <rdfs:comment>Database handle for the object.  It is of XML type ID, so is constrained to be unique in the XML document within which it occurs.  An external identifier for the object in the form of a URI may be constructed using standard XML and XPointer methods.  This is done by concatenating the URI for the document, a fragment separator, and the value of the id attribute.</rdfs:comment>
      <owl:equivalentClass rdf:resource="http://www.w3.org/2001/XMLSchema#ID"/>
   </rdfs:Datatype>
   <rdfs:Datatype rdf:about="http://www.opengis.net/gml#remoteSchema">
      <rdfs:comment>Reference to an XML Schema fragment that specifies the content model of the propertys value. This is in conformance with the XML Schema Section 4.14 Referencing Schemas from Elsewhere.</rdfs:comment>
      <owl:equivalentClass rdf:resource="http://www.w3.org/2001/XMLSchema#anyURI"/>
   </rdfs:Datatype>
   <owl:DatatypeProperty rdf:about="http://www.opengis.net/gml#hasremoteSchema">
      <rdfs:domain rdf:resource="http://www.opengis.net/gml#AssociationAttributeGroup"/>
      <rdfs:range rdf:resource="http://www.opengis.net/gml#remoteSchema"/>
   </owl:DatatypeProperty>
   <owl:DatatypeProperty rdf:about="http://www.opengis.net/gml#codeSpace">
      <rdfs:domain rdf:resource="http://www.opengis.net/gml#CodeType"/>
      <rdfs:range rdf:resource="http://www.w3.org/2001/XMLSchema#anyURI"/>
   </owl:DatatypeProperty>
   <owl:DatatypeProperty rdf:about="http://www.opengis.net/gml#codeSpace">
      <rdfs:domain rdf:resource="http://www.opengis.net/gml#CodeListType"/>
      <rdfs:range rdf:resource="http://www.w3.org/2001/XMLSchema#anyURI"/>
   </owl:DatatypeProperty>
   <owl:DatatypeProperty rdf:about="http://www.opengis.net/gml#codeSpace">
      <rdfs:domain rdf:resource="http://www.opengis.net/gml#CodeOrNullListType"/>
      <rdfs:range rdf:resource="http://www.w3.org/2001/XMLSchema#anyURI"/>
   </owl:DatatypeProperty>
   <owl:DatatypeProperty rdf:about="http://www.opengis.net/gml#uom">
      <rdfs:domain rdf:resource="http://www.opengis.net/gml#MeasureType"/>
      <rdfs:range rdf:resource="http://www.w3.org/2001/XMLSchema#anyURI"/>
   </owl:DatatypeProperty>
   <owl:DatatypeProperty rdf:about="http://www.opengis.net/gml#uom">
      <rdfs:domain rdf:resource="http://www.opengis.net/gml#MeasureListType"/>
      <rdfs:range rdf:resource="http://www.w3.org/2001/XMLSchema#anyURI"/>
   </owl:DatatypeProperty>
   <owl:DatatypeProperty rdf:about="http://www.opengis.net/gml#uom">
      <rdfs:domain rdf:resource="http://www.opengis.net/gml#MeasureOrNullListType"/>
      <rdfs:range rdf:resource="http://www.w3.org/2001/XMLSchema#anyURI"/>
   </owl:DatatypeProperty>
   <owl:DatatypeProperty rdf:about="http://www.opengis.net/gml#decimal">
      <rdfs:domain rdf:resource="http://www.opengis.net/gml#CoordinatesType"/>
      <rdfs:range rdf:resource="http://www.w3.org/2001/XMLSchema#string"/>
   </owl:DatatypeProperty>
   <owl:DatatypeProperty rdf:about="http://www.opengis.net/gml#cs">
      <rdfs:domain rdf:resource="http://www.opengis.net/gml#CoordinatesType"/>
      <rdfs:range rdf:resource="http://www.w3.org/2001/XMLSchema#string"/>
   </owl:DatatypeProperty>
   <owl:DatatypeProperty rdf:about="http://www.opengis.net/gml#ts">
      <rdfs:domain rdf:resource="http://www.opengis.net/gml#CoordinatesType"/>
      <rdfs:range rdf:resource="http://www.w3.org/2001/XMLSchema#string"/>
   </owl:DatatypeProperty>
   <owl:DatatypeProperty rdf:about="http://www.opengis.net/gml#relativePosition">
      <rdfs:domain rdf:resource="http://www.opengis.net/gml#RelatedTimeType"/>
      <rdfs:range rdf:resource="http://www.w3.org/2001/XMLSchema#string"/>
   </owl:DatatypeProperty>
   <owl:DatatypeProperty rdf:about="http://www.opengis.net/gml#frame">
      <rdfs:domain rdf:resource="http://www.opengis.net/gml#AbstractTimeGeometricPrimitiveType"/>
      <rdfs:range rdf:resource="http://www.w3.org/2001/XMLSchema#anyURI"/>
   </owl:DatatypeProperty>
   <owl:DatatypeProperty rdf:about="http://www.opengis.net/gml#unit">
      <rdfs:domain rdf:resource="http://www.opengis.net/gml#TimeIntervalLengthType"/>
      <rdfs:range rdf:resource="http://www.opengis.net/gml#TimeUnitType"/>
   </owl:DatatypeProperty>
   <owl:DatatypeProperty rdf:about="http://www.opengis.net/gml#radix">
      <rdfs:domain rdf:resource="http://www.opengis.net/gml#TimeIntervalLengthType"/>
      <rdfs:range rdf:resource="http://www.w3.org/2001/XMLSchema#positiveInteger"/>
   </owl:DatatypeProperty>
   <owl:DatatypeProperty rdf:about="http://www.opengis.net/gml#factor">
      <rdfs:domain rdf:resource="http://www.opengis.net/gml#TimeIntervalLengthType"/>
      <rdfs:range rdf:resource="http://www.w3.org/2001/XMLSchema#integer"/>
   </owl:DatatypeProperty>
   <owl:DatatypeProperty rdf:about="http://www.opengis.net/gml#frame">
      <rdfs:domain rdf:resource="http://www.opengis.net/gml#TimePositionType"/>
      <rdfs:range rdf:resource="http://www.w3.org/2001/XMLSchema#anyURI"/>
   </owl:DatatypeProperty>
   <owl:DatatypeProperty rdf:about="http://www.opengis.net/gml#calendarEraName">
      <rdfs:domain rdf:resource="http://www.opengis.net/gml#TimePositionType"/>
      <rdfs:range rdf:resource="http://www.w3.org/2001/XMLSchema#string"/>
   </owl:DatatypeProperty>
   <owl:DatatypeProperty rdf:about="http://www.opengis.net/gml#indeterminatePosition">
      <rdfs:domain rdf:resource="http://www.opengis.net/gml#TimePositionType"/>
      <rdfs:range rdf:resource="http://www.opengis.net/gml#TimeIndeterminateValueType"/>
   </owl:DatatypeProperty>
   <owl:DatatypeProperty rdf:about="http://www.opengis.net/gml#orientation">
      <rdfs:domain rdf:resource="http://www.opengis.net/gml#DirectedNodePropertyType"/>
      <rdfs:range rdf:resource="http://www.opengis.net/gml#SignType"/>
   </owl:DatatypeProperty>
   <owl:DatatypeProperty rdf:about="http://www.opengis.net/gml#orientation">
      <rdfs:domain rdf:resource="http://www.opengis.net/gml#DirectedEdgePropertyType"/>
      <rdfs:range rdf:resource="http://www.opengis.net/gml#SignType"/>
   </owl:DatatypeProperty>
   <owl:DatatypeProperty rdf:about="http://www.opengis.net/gml#orientation">
      <rdfs:domain rdf:resource="http://www.opengis.net/gml#DirectedFacePropertyType"/>
      <rdfs:range rdf:resource="http://www.opengis.net/gml#SignType"/>
   </owl:DatatypeProperty>
   <owl:DatatypeProperty rdf:about="http://www.opengis.net/gml#orientation">
      <rdfs:domain rdf:resource="http://www.opengis.net/gml#DirectedTopoSolidPropertyType"/>
      <rdfs:range rdf:resource="http://www.opengis.net/gml#SignType"/>
   </owl:DatatypeProperty>
   <owl:DatatypeProperty rdf:about="http://www.opengis.net/gml#isMaximal">
      <rdfs:domain rdf:resource="http://www.opengis.net/gml#TopoComplexType"/>
      <rdfs:range rdf:resource="http://www.w3.org/2001/XMLSchema#boolean"/>
   </owl:DatatypeProperty>
   <owl:DatatypeProperty rdf:about="http://www.opengis.net/gml#orientation">
      <rdfs:domain rdf:resource="http://www.opengis.net/gml#OrientableCurveType"/>
      <rdfs:range rdf:resource="http://www.opengis.net/gml#SignType"/>
   </owl:DatatypeProperty>
   <owl:DatatypeProperty rdf:about="http://www.opengis.net/gml#numDerivativesAtStart">
      <rdfs:domain rdf:resource="http://www.opengis.net/gml#AbstractCurveSegmentType"/>
      <rdfs:range rdf:resource="http://www.w3.org/2001/XMLSchema#integer"/>
   </owl:DatatypeProperty>
   <owl:DatatypeProperty rdf:about="http://www.opengis.net/gml#numDerivativesAtEnd">
      <rdfs:domain rdf:resource="http://www.opengis.net/gml#AbstractCurveSegmentType"/>
      <rdfs:range rdf:resource="http://www.w3.org/2001/XMLSchema#integer"/>
   </owl:DatatypeProperty>
   <owl:DatatypeProperty rdf:about="http://www.opengis.net/gml#numDerivativeInterior">
      <rdfs:domain rdf:resource="http://www.opengis.net/gml#AbstractCurveSegmentType"/>
      <rdfs:range rdf:resource="http://www.w3.org/2001/XMLSchema#integer"/>
   </owl:DatatypeProperty>
   <owl:DatatypeProperty rdf:about="http://www.opengis.net/gml#interpolation">
      <rdfs:domain rdf:resource="http://www.opengis.net/gml#LineStringSegmentType"/>
      <rdfs:range rdf:resource="http://www.opengis.net/gml#CurveInterpolationType"/>
   </owl:DatatypeProperty>
   <owl:DatatypeProperty rdf:about="http://www.opengis.net/gml#interpolation">
      <rdfs:domain rdf:resource="http://www.opengis.net/gml#ArcStringType"/>
      <rdfs:range rdf:resource="http://www.opengis.net/gml#CurveInterpolationType"/>
   </owl:DatatypeProperty>
   <owl:DatatypeProperty rdf:about="http://www.opengis.net/gml#numArc">
      <rdfs:domain rdf:resource="http://www.opengis.net/gml#ArcStringType"/>
      <rdfs:range rdf:resource="http://www.w3.org/2001/XMLSchema#integer"/>
   </owl:DatatypeProperty>
   <owl:DatatypeProperty rdf:about="http://www.opengis.net/gml#numArc">
      <rdfs:domain rdf:resource="http://www.opengis.net/gml#ArcType"/>
      <rdfs:range rdf:resource="http://www.w3.org/2001/XMLSchema#integer"/>
   </owl:DatatypeProperty>
   <owl:DatatypeProperty rdf:about="http://www.opengis.net/gml#interpolation">
      <rdfs:domain rdf:resource="http://www.opengis.net/gml#ArcStringByBulgeType"/>
      <rdfs:range rdf:resource="http://www.opengis.net/gml#CurveInterpolationType"/>
   </owl:DatatypeProperty>
   <owl:DatatypeProperty rdf:about="http://www.opengis.net/gml#numArc">
      <rdfs:domain rdf:resource="http://www.opengis.net/gml#ArcStringByBulgeType"/>
      <rdfs:range rdf:resource="http://www.w3.org/2001/XMLSchema#integer"/>
   </owl:DatatypeProperty>
   <owl:DatatypeProperty rdf:about="http://www.opengis.net/gml#numArc">
      <rdfs:domain rdf:resource="http://www.opengis.net/gml#ArcByBulgeType"/>
      <rdfs:range rdf:resource="http://www.w3.org/2001/XMLSchema#integer"/>
   </owl:DatatypeProperty>
   <owl:DatatypeProperty rdf:about="http://www.opengis.net/gml#interpolation">
      <rdfs:domain rdf:resource="http://www.opengis.net/gml#ArcByCenterPointType"/>
      <rdfs:range rdf:resource="http://www.opengis.net/gml#CurveInterpolationType"/>
   </owl:DatatypeProperty>
   <owl:DatatypeProperty rdf:about="http://www.opengis.net/gml#numArc">
      <rdfs:domain rdf:resource="http://www.opengis.net/gml#ArcByCenterPointType"/>
      <rdfs:range rdf:resource="http://www.w3.org/2001/XMLSchema#integer"/>
   </owl:DatatypeProperty>
   <owl:DatatypeProperty rdf:about="http://www.opengis.net/gml#interpolation">
      <rdfs:domain rdf:resource="http://www.opengis.net/gml#GeodesicStringType"/>
      <rdfs:range rdf:resource="http://www.opengis.net/gml#CurveInterpolationType"/>
   </owl:DatatypeProperty>
   <owl:DatatypeProperty rdf:about="http://www.opengis.net/gml#interpolation">
      <rdfs:domain rdf:resource="http://www.opengis.net/gml#CubicSplineType"/>
      <rdfs:range rdf:resource="http://www.opengis.net/gml#CurveInterpolationType"/>
   </owl:DatatypeProperty>
   <owl:DatatypeProperty rdf:about="http://www.opengis.net/gml#degree">
      <rdfs:domain rdf:resource="http://www.opengis.net/gml#CubicSplineType"/>
      <rdfs:range rdf:resource="http://www.w3.org/2001/XMLSchema#integer"/>
   </owl:DatatypeProperty>
   <owl:DatatypeProperty rdf:about="http://www.opengis.net/gml#interpolation">
      <rdfs:domain rdf:resource="http://www.opengis.net/gml#BSplineType"/>
      <rdfs:range rdf:resource="http://www.opengis.net/gml#CurveInterpolationType"/>
   </owl:DatatypeProperty>
   <owl:DatatypeProperty rdf:about="http://www.opengis.net/gml#isPolynomial">
      <rdfs:domain rdf:resource="http://www.opengis.net/gml#BSplineType"/>
      <rdfs:range rdf:resource="http://www.w3.org/2001/XMLSchema#boolean"/>
   </owl:DatatypeProperty>
   <owl:DatatypeProperty rdf:about="http://www.opengis.net/gml#knotType">
      <rdfs:domain rdf:resource="http://www.opengis.net/gml#BSplineType"/>
      <rdfs:range rdf:resource="http://www.opengis.net/gml#KnotTypesType"/>
   </owl:DatatypeProperty>
   <owl:DatatypeProperty rdf:about="http://www.opengis.net/gml#interpolation">
      <rdfs:domain rdf:resource="http://www.opengis.net/gml#BezierType"/>
      <rdfs:range rdf:resource="http://www.opengis.net/gml#CurveInterpolationType"/>
   </owl:DatatypeProperty>
   <owl:DatatypeProperty rdf:about="http://www.opengis.net/gml#isPolynomial">
      <rdfs:domain rdf:resource="http://www.opengis.net/gml#BezierType"/>
      <rdfs:range rdf:resource="http://www.w3.org/2001/XMLSchema#boolean"/>
   </owl:DatatypeProperty>
   <owl:DatatypeProperty rdf:about="http://www.opengis.net/gml#knotType">
      <rdfs:domain rdf:resource="http://www.opengis.net/gml#BezierType"/>
      <rdfs:range rdf:resource="http://www.opengis.net/gml#KnotTypesType"/>
   </owl:DatatypeProperty>
   <owl:DatatypeProperty rdf:about="http://www.opengis.net/gml#orientation">
      <rdfs:domain rdf:resource="http://www.opengis.net/gml#OrientableSurfaceType"/>
      <rdfs:range rdf:resource="http://www.opengis.net/gml#SignType"/>
   </owl:DatatypeProperty>
   <owl:DatatypeProperty rdf:about="http://www.opengis.net/gml#interpolation">
      <rdfs:domain rdf:resource="http://www.opengis.net/gml#PolygonPatchType"/>
      <rdfs:range rdf:resource="http://www.opengis.net/gml#SurfaceInterpolationType"/>
   </owl:DatatypeProperty>
   <owl:DatatypeProperty rdf:about="http://www.opengis.net/gml#interpolation">
      <rdfs:domain rdf:resource="http://www.opengis.net/gml#TriangleType"/>
      <rdfs:range rdf:resource="http://www.opengis.net/gml#SurfaceInterpolationType"/>
   </owl:DatatypeProperty>
   <owl:DatatypeProperty rdf:about="http://www.opengis.net/gml#interpolation">
      <rdfs:domain rdf:resource="http://www.opengis.net/gml#RectangleType"/>
      <rdfs:range rdf:resource="http://www.opengis.net/gml#SurfaceInterpolationType"/>
   </owl:DatatypeProperty>
   <owl:DatatypeProperty rdf:about="http://www.opengis.net/gml#horizontalCurveType">
      <rdfs:domain rdf:resource="http://www.opengis.net/gml#ConeType"/>
      <rdfs:range rdf:resource="http://www.opengis.net/gml#CurveInterpolationType"/>
   </owl:DatatypeProperty>
   <owl:DatatypeProperty rdf:about="http://www.opengis.net/gml#verticalCurveType">
      <rdfs:domain rdf:resource="http://www.opengis.net/gml#ConeType"/>
      <rdfs:range rdf:resource="http://www.opengis.net/gml#CurveInterpolationType"/>
   </owl:DatatypeProperty>
   <owl:DatatypeProperty rdf:about="http://www.opengis.net/gml#horizontalCurveType">
      <rdfs:domain rdf:resource="http://www.opengis.net/gml#CylinderType"/>
      <rdfs:range rdf:resource="http://www.opengis.net/gml#CurveInterpolationType"/>
   </owl:DatatypeProperty>
   <owl:DatatypeProperty rdf:about="http://www.opengis.net/gml#verticalCurveType">
      <rdfs:domain rdf:resource="http://www.opengis.net/gml#CylinderType"/>
      <rdfs:range rdf:resource="http://www.opengis.net/gml#CurveInterpolationType"/>
   </owl:DatatypeProperty>
   <owl:DatatypeProperty rdf:about="http://www.opengis.net/gml#horizontalCurveType">
      <rdfs:domain rdf:resource="http://www.opengis.net/gml#SphereType"/>
      <rdfs:range rdf:resource="http://www.opengis.net/gml#CurveInterpolationType"/>
   </owl:DatatypeProperty>
   <owl:DatatypeProperty rdf:about="http://www.opengis.net/gml#verticalCurveType">
      <rdfs:domain rdf:resource="http://www.opengis.net/gml#SphereType"/>
      <rdfs:range rdf:resource="http://www.opengis.net/gml#CurveInterpolationType"/>
   </owl:DatatypeProperty>
   <owl:DatatypeProperty rdf:about="http://www.opengis.net/gml#dimension">
      <rdfs:domain rdf:resource="http://www.opengis.net/gml#AbstractCoverageType"/>
      <rdfs:range rdf:resource="http://www.w3.org/2001/XMLSchema#positiveInteger"/>
   </owl:DatatypeProperty>
   <owl:DatatypeProperty rdf:about="http://www.opengis.net/gml#order">
      <rdfs:domain rdf:resource="http://www.opengis.net/gml#SequenceRuleType"/>
      <rdfs:range rdf:resource="http://www.opengis.net/gml#IncrementOrder"/>
   </owl:DatatypeProperty>
   <owl:DatatypeProperty rdf:about="http://www.opengis.net/gml#codeSpace">
      <rdfs:domain rdf:resource="http://www.opengis.net/gml#referenceSystem"/>
      <rdfs:range rdf:resource="http://www.w3.org/2001/XMLSchema#anyURI"/>
   </owl:DatatypeProperty>
   <owl:DatatypeProperty rdf:about="http://www.opengis.net/gml#uom">
      <rdfs:domain rdf:resource="http://www.opengis.net/gml#referenceSystem"/>
      <rdfs:range rdf:resource="http://www.w3.org/2001/XMLSchema#anyURI"/>
   </owl:DatatypeProperty>
   <owl:DatatypeProperty rdf:about="http://www.opengis.net/gml#dimension">
      <rdfs:domain rdf:resource="http://www.opengis.net/gml#GridType"/>
      <rdfs:range rdf:resource="http://www.w3.org/2001/XMLSchema#positiveInteger"/>
   </owl:DatatypeProperty>
   <owl:DatatypeProperty rdf:about="http://www.opengis.net/gml#codeSpace">
      <rdfs:domain rdf:resource="http://www.opengis.net/gml#DerivedCRSTypeType"/>
      <rdfs:range rdf:resource="http://www.w3.org/2001/XMLSchema#anyURI"/>
   </owl:DatatypeProperty>
   <owl:DatatypeProperty rdf:about="http://www.opengis.net/gml#hasid">
      <rdfs:domain rdf:resource="http://www.opengis.net/gml#CoordinateSystemAxisBaseType"/>
      <rdfs:range rdf:resource="http://www.opengis.net/gml#id"/>
   </owl:DatatypeProperty>
   <owl:DatatypeProperty rdf:about="http://www.opengis.net/gml#hasuom">
      <rdfs:domain rdf:resource="http://www.opengis.net/gml#CoordinateSystemAxisType"/>
      <rdfs:range rdf:resource="http://www.opengis.net/gml#uom"/>
   </owl:DatatypeProperty>
   <rdfs:Datatype rdf:about="http://www.opengis.net/gml#uom">
      <rdfs:comment>Identifier of the unit of measure used for this coordinate system axis. The value of this coordinate in a coordinate tuple shall be recorded using this unit of measure, whenever those coordinates use a coordinate reference system that uses a coordinate system that uses this axis.</rdfs:comment>
      <owl:equivalentClass rdf:resource="http://www.w3.org/2001/XMLSchema#anyURI"/>
   </rdfs:Datatype>
   <owl:DatatypeProperty rdf:about="http://www.opengis.net/gml#hasid">
      <rdfs:domain rdf:resource="http://www.opengis.net/gml#AbstractCoordinateSystemBaseType"/>
      <rdfs:range rdf:resource="http://www.opengis.net/gml#id"/>
   </owl:DatatypeProperty>
   <owl:DatatypeProperty rdf:about="http://www.opengis.net/gml#hasid">
      <rdfs:domain rdf:resource="http://www.opengis.net/gml#AbstractReferenceSystemBaseType"/>
      <rdfs:range rdf:resource="http://www.opengis.net/gml#id"/>
   </owl:DatatypeProperty>
   <owl:DatatypeProperty rdf:about="http://www.opengis.net/gml#hasid">
      <rdfs:domain rdf:resource="http://www.opengis.net/gml#AbstractDatumBaseType"/>
      <rdfs:range rdf:resource="http://www.opengis.net/gml#id"/>
   </owl:DatatypeProperty>
   <owl:DatatypeProperty rdf:about="http://www.opengis.net/gml#codeSpace">
      <rdfs:domain rdf:resource="http://www.opengis.net/gml#PixelInCellType"/>
      <rdfs:range rdf:resource="http://www.w3.org/2001/XMLSchema#anyURI"/>
   </owl:DatatypeProperty>
   <owl:DatatypeProperty rdf:about="http://www.opengis.net/gml#codeSpace">
      <rdfs:domain rdf:resource="http://www.opengis.net/gml#VerticalDatumTypeType"/>
      <rdfs:range rdf:resource="http://www.w3.org/2001/XMLSchema#anyURI"/>
   </owl:DatatypeProperty>
   <owl:DatatypeProperty rdf:about="http://www.opengis.net/gml#hasid">
      <rdfs:domain rdf:resource="http://www.opengis.net/gml#TemporalDatumBaseType"/>
      <rdfs:range rdf:resource="http://www.opengis.net/gml#id"/>
   </owl:DatatypeProperty>
   <owl:DatatypeProperty rdf:about="http://www.opengis.net/gml#hasid">
      <rdfs:domain rdf:resource="http://www.opengis.net/gml#PrimeMeridianBaseType"/>
      <rdfs:range rdf:resource="http://www.opengis.net/gml#id"/>
   </owl:DatatypeProperty>
   <owl:DatatypeProperty rdf:about="http://www.opengis.net/gml#hasid">
      <rdfs:domain rdf:resource="http://www.opengis.net/gml#EllipsoidBaseType"/>
      <rdfs:range rdf:resource="http://www.opengis.net/gml#id"/>
   </owl:DatatypeProperty>
   <owl:DatatypeProperty rdf:about="http://www.opengis.net/gml#hasid">
      <rdfs:domain rdf:resource="http://www.opengis.net/gml#AbstractCoordinateOperationBaseType"/>
      <rdfs:range rdf:resource="http://www.opengis.net/gml#id"/>
   </owl:DatatypeProperty>
   <owl:DatatypeProperty rdf:about="http://www.opengis.net/gml#hasid">
      <rdfs:domain rdf:resource="http://www.opengis.net/gml#AbstractGeneralConversionType"/>
      <rdfs:range rdf:resource="http://www.opengis.net/gml#id"/>
   </owl:DatatypeProperty>
   <owl:DatatypeProperty rdf:about="http://www.opengis.net/gml#hasid">
      <rdfs:domain rdf:resource="http://www.opengis.net/gml#AbstractGeneralTransformationType"/>
      <rdfs:range rdf:resource="http://www.opengis.net/gml#id"/>
   </owl:DatatypeProperty>
   <owl:DatatypeProperty rdf:about="http://www.opengis.net/gml#hasid">
      <rdfs:domain rdf:resource="http://www.opengis.net/gml#OperationMethodBaseType"/>
      <rdfs:range rdf:resource="http://www.opengis.net/gml#id"/>
   </owl:DatatypeProperty>
   <owl:DatatypeProperty rdf:about="http://www.opengis.net/gml#hasid">
      <rdfs:domain rdf:resource="http://www.opengis.net/gml#OperationParameterBaseType"/>
      <rdfs:range rdf:resource="http://www.opengis.net/gml#id"/>
   </owl:DatatypeProperty>
   <owl:DatatypeProperty rdf:about="http://www.opengis.net/gml#hasid">
      <rdfs:domain rdf:resource="http://www.opengis.net/gml#OperationParameterGroupBaseType"/>
      <rdfs:range rdf:resource="http://www.opengis.net/gml#id"/>
   </owl:DatatypeProperty>
   <owl:DatatypeProperty rdf:about="http://www.opengis.net/gml#about">
      <rdfs:domain rdf:resource="http://www.opengis.net/gml#DefaultStylePropertyType"/>
      <rdfs:range rdf:resource="http://www.w3.org/2001/XMLSchema#anyURI"/>
   </owl:DatatypeProperty>
   <owl:DatatypeProperty rdf:about="http://www.opengis.net/gml#about">
      <rdfs:domain rdf:resource="http://www.opengis.net/gml#FeatureStylePropertyType"/>
      <rdfs:range rdf:resource="http://www.w3.org/2001/XMLSchema#anyURI"/>
   </owl:DatatypeProperty>
   <owl:DatatypeProperty rdf:about="http://www.opengis.net/gml#featureType">
      <rdfs:domain rdf:resource="http://www.opengis.net/gml#FeatureStyleType"/>
      <rdfs:range rdf:resource="http://www.w3.org/2001/XMLSchema#string"/>
   </owl:DatatypeProperty>
   <owl:DatatypeProperty rdf:about="http://www.opengis.net/gml#baseType">
      <rdfs:domain rdf:resource="http://www.opengis.net/gml#FeatureStyleType"/>
      <rdfs:range rdf:resource="http://www.w3.org/2001/XMLSchema#string"/>
   </owl:DatatypeProperty>
   <owl:DatatypeProperty rdf:about="http://www.opengis.net/gml#queryGrammar">
      <rdfs:domain rdf:resource="http://www.opengis.net/gml#FeatureStyleType"/>
      <rdfs:range rdf:resource="http://www.opengis.net/gml#QueryGrammarEnumeration"/>
   </owl:DatatypeProperty>
   <owl:DatatypeProperty rdf:about="http://www.opengis.net/gml#about">
      <rdfs:domain rdf:resource="http://www.opengis.net/gml#GeometryStylePropertyType"/>
      <rdfs:range rdf:resource="http://www.w3.org/2001/XMLSchema#anyURI"/>
   </owl:DatatypeProperty>
   <owl:DatatypeProperty rdf:about="http://www.opengis.net/gml#geometryProperty">
      <rdfs:domain rdf:resource="http://www.opengis.net/gml#GeometryStyleType"/>
      <rdfs:range rdf:resource="http://www.w3.org/2001/XMLSchema#string"/>
   </owl:DatatypeProperty>
   <owl:DatatypeProperty rdf:about="http://www.opengis.net/gml#geometryType">
      <rdfs:domain rdf:resource="http://www.opengis.net/gml#GeometryStyleType"/>
      <rdfs:range rdf:resource="http://www.w3.org/2001/XMLSchema#string"/>
   </owl:DatatypeProperty>
   <owl:DatatypeProperty rdf:about="http://www.opengis.net/gml#about">
      <rdfs:domain rdf:resource="http://www.opengis.net/gml#TopologyStylePropertyType"/>
      <rdfs:range rdf:resource="http://www.w3.org/2001/XMLSchema#anyURI"/>
   </owl:DatatypeProperty>
   <owl:DatatypeProperty rdf:about="http://www.opengis.net/gml#topologyProperty">
      <rdfs:domain rdf:resource="http://www.opengis.net/gml#TopologyStyleType"/>
      <rdfs:range rdf:resource="http://www.w3.org/2001/XMLSchema#string"/>
   </owl:DatatypeProperty>
   <owl:DatatypeProperty rdf:about="http://www.opengis.net/gml#topologyType">
      <rdfs:domain rdf:resource="http://www.opengis.net/gml#TopologyStyleType"/>
      <rdfs:range rdf:resource="http://www.w3.org/2001/XMLSchema#string"/>
   </owl:DatatypeProperty>
   <owl:DatatypeProperty rdf:about="http://www.opengis.net/gml#about">
      <rdfs:domain rdf:resource="http://www.opengis.net/gml#LabelStylePropertyType"/>
      <rdfs:range rdf:resource="http://www.w3.org/2001/XMLSchema#anyURI"/>
   </owl:DatatypeProperty>
   <owl:DatatypeProperty rdf:about="http://www.opengis.net/gml#about">
      <rdfs:domain rdf:resource="http://www.opengis.net/gml#GraphStylePropertyType"/>
      <rdfs:range rdf:resource="http://www.w3.org/2001/XMLSchema#anyURI"/>
   </owl:DatatypeProperty>
   <owl:DatatypeProperty rdf:about="http://www.opengis.net/gml#symbolType">
      <rdfs:domain rdf:resource="http://www.opengis.net/gml#SymbolType"/>
      <rdfs:range rdf:resource="http://www.opengis.net/gml#SymbolTypeEnumeration"/>
   </owl:DatatypeProperty>
   <owl:DatatypeProperty rdf:about="http://www.opengis.net/gml#hastransform">
      <rdfs:domain rdf:resource="http://www.opengis.net/gml#SymbolType"/>
      <rdfs:range rdf:resource="http://www.opengis.net/gml#transform"/>
   </owl:DatatypeProperty>
   <owl:DatatypeProperty rdf:about="http://www.opengis.net/gml#about">
      <rdfs:domain rdf:resource="http://www.opengis.net/gml#SymbolType"/>
      <rdfs:range rdf:resource="http://www.w3.org/2001/XMLSchema#anyURI"/>
   </owl:DatatypeProperty>
   <owl:DatatypeProperty rdf:about="http://www.opengis.net/gml#hastransform">
      <rdfs:domain rdf:resource="http://www.opengis.net/gml#LabelType"/>
      <rdfs:range rdf:resource="http://www.opengis.net/gml#transform"/>
   </owl:DatatypeProperty>
   <rdfs:Datatype rdf:about="http://www.opengis.net/gml#transform">
      <rdfs:comment>Defines the geometric transformation of entities. There is no particular grammar defined for this value.</rdfs:comment>
      <owl:equivalentClass rdf:resource="http://www.w3.org/2001/XMLSchema#string"/>
   </rdfs:Datatype>
   <owl:DatatypeProperty rdf:about="http://www.opengis.net/gml#styleProperty">
      <rdfs:domain rdf:resource="http://www.opengis.net/gml#StyleVariationType"/>
      <rdfs:range rdf:resource="http://www.w3.org/2001/XMLSchema#string"/>
   </owl:DatatypeProperty>
   <owl:DatatypeProperty rdf:about="http://www.opengis.net/gml#featurePropertyRange">
      <rdfs:domain rdf:resource="http://www.opengis.net/gml#StyleVariationType"/>
      <rdfs:range rdf:resource="http://www.w3.org/2001/XMLSchema#string"/>
   </owl:DatatypeProperty>
   <owl:Class rdf:about="http://www.opengis.net/gml#dataSource">
      <rdfs:subClassOf rdf:resource="http://www.opengis.net/gml#StringOrRefType"/>
   </owl:Class>
   <owl:Class rdf:about="http://www.opengis.net/gml#status">
      <rdfs:subClassOf rdf:resource="http://www.opengis.net/gml#StringOrRefType"/>
   </owl:Class>
   <owl:Class rdf:about="http://www.opengis.net/gml#_TimeSlice">
      <rdfs:subClassOf rdf:resource="http://www.opengis.net/gml#_GML"/>
      <rdfs:subClassOf rdf:resource="http://www.opengis.net/gml#AbstractTimeSliceType"/>
   </owl:Class>
   <owl:Class rdf:about="http://www.opengis.net/gml#MovingObjectStatus">
      <rdfs:subClassOf rdf:resource="http://www.opengis.net/gml#_TimeSlice"/>
      <rdfs:subClassOf rdf:resource="http://www.opengis.net/gml#MovingObjectStatusType"/>
   </owl:Class>
   <owl:Class rdf:about="http://www.opengis.net/gml#history">
      <rdfs:subClassOf rdf:resource="http://www.opengis.net/gml#HistoryPropertyType"/>
   </owl:Class>
   <owl:Class rdf:about="http://www.opengis.net/gml#track">
      <rdfs:subClassOf rdf:resource="http://www.opengis.net/gml#history"/>
      <rdfs:subClassOf rdf:resource="http://www.opengis.net/gml#TrackType"/>
   </owl:Class>
   <owl:Class rdf:about="http://www.opengis.net/gml#_Feature">
      <rdfs:subClassOf rdf:resource="http://www.opengis.net/gml#_GML"/>
      <rdfs:subClassOf rdf:resource="http://www.opengis.net/gml#AbstractFeatureType"/>
   </owl:Class>
   <owl:Class rdf:about="http://www.opengis.net/gml#boundedBy">
      <rdfs:subClassOf rdf:resource="http://www.opengis.net/gml#BoundingShapeType"/>
   </owl:Class>
   <owl:Class rdf:about="http://www.opengis.net/gml#EnvelopeWithTimePeriod">
      <rdfs:subClassOf rdf:resource="http://www.opengis.net/gml#Envelope"/>
      <rdfs:subClassOf rdf:resource="http://www.opengis.net/gml#EnvelopeWithTimePeriodType"/>
   </owl:Class>
   <owl:Class rdf:about="http://www.opengis.net/gml#featureMember">
      <rdfs:subClassOf rdf:resource="http://www.opengis.net/gml#FeaturePropertyType"/>
   </owl:Class>
   <owl:Class rdf:about="http://www.opengis.net/gml#featureProperty">
      <rdfs:subClassOf rdf:resource="http://www.opengis.net/gml#FeaturePropertyType"/>
   </owl:Class>
   <owl:Class rdf:about="http://www.opengis.net/gml#featureMembers">
      <rdfs:subClassOf rdf:resource="http://www.opengis.net/gml#FeatureArrayPropertyType"/>
   </owl:Class>
   <owl:Class rdf:about="http://www.opengis.net/gml#_FeatureCollection">
      <rdfs:subClassOf rdf:resource="http://www.opengis.net/gml#_Feature"/>
      <rdfs:subClassOf rdf:resource="http://www.opengis.net/gml#AbstractFeatureCollectionType"/>
   </owl:Class>
   <owl:Class rdf:about="http://www.opengis.net/gml#FeatureCollection">
      <rdfs:subClassOf rdf:resource="http://www.opengis.net/gml#_Feature"/>
      <rdfs:subClassOf rdf:resource="http://www.opengis.net/gml#FeatureCollectionType"/>
   </owl:Class>
   <owl:Class rdf:about="http://www.opengis.net/gml#LocationKeyWord">
      <rdfs:subClassOf rdf:resource="http://www.opengis.net/gml#CodeType"/>
   </owl:Class>
   <owl:Class rdf:about="http://www.opengis.net/gml#LocationString">
      <rdfs:subClassOf rdf:resource="http://www.opengis.net/gml#StringOrRefType"/>
   </owl:Class>
   <owl:Class rdf:about="http://www.opengis.net/gml#centerOf">
      <rdfs:subClassOf rdf:resource="http://www.opengis.net/gml#PointPropertyType"/>
   </owl:Class>
   <owl:Class rdf:about="http://www.opengis.net/gml#position">
      <rdfs:subClassOf rdf:resource="http://www.opengis.net/gml#PointPropertyType"/>
   </owl:Class>
   <owl:Class rdf:about="http://www.opengis.net/gml#edgeOf">
      <rdfs:subClassOf rdf:resource="http://www.opengis.net/gml#CurvePropertyType"/>
   </owl:Class>
   <owl:Class rdf:about="http://www.opengis.net/gml#centerLineOf">
      <rdfs:subClassOf rdf:resource="http://www.opengis.net/gml#CurvePropertyType"/>
   </owl:Class>
   <owl:Class rdf:about="http://www.opengis.net/gml#extentOf">
      <rdfs:subClassOf rdf:resource="http://www.opengis.net/gml#SurfacePropertyType"/>
   </owl:Class>
   <owl:Class rdf:about="http://www.opengis.net/gml#location">
      <rdfs:subClassOf rdf:resource="http://www.opengis.net/gml#LocationPropertyType"/>
   </owl:Class>
   <owl:Class rdf:about="http://www.opengis.net/gml#priorityLocation">
      <rdfs:subClassOf rdf:resource="http://www.opengis.net/gml#location"/>
      <rdfs:subClassOf rdf:resource="http://www.opengis.net/gml#PriorityLocationPropertyType"/>
   </owl:Class>
   <owl:Class rdf:about="http://www.opengis.net/gml#_Surface">
      <rdfs:subClassOf rdf:resource="http://www.opengis.net/gml#_GeometricPrimitive"/>
      <rdfs:subClassOf rdf:resource="http://www.opengis.net/gml#AbstractSurfaceType"/>
   </owl:Class>
   <owl:Class rdf:about="http://www.opengis.net/gml#surfaceProperty">
      <rdfs:subClassOf rdf:resource="http://www.opengis.net/gml#SurfacePropertyType"/>
   </owl:Class>
   <owl:Class rdf:about="http://www.opengis.net/gml#surfaceArrayProperty">
      <rdfs:subClassOf rdf:resource="http://www.opengis.net/gml#SurfaceArrayPropertyType"/>
   </owl:Class>
   <owl:Class rdf:about="http://www.opengis.net/gml#Polygon">
      <rdfs:subClassOf rdf:resource="http://www.opengis.net/gml#_Surface"/>
      <rdfs:subClassOf rdf:resource="http://www.opengis.net/gml#PolygonType"/>
   </owl:Class>
   <owl:Class rdf:about="http://www.opengis.net/gml#_Ring">
      <rdfs:subClassOf rdf:resource="http://www.opengis.net/gml#_Geometry"/>
      <rdfs:subClassOf rdf:resource="http://www.opengis.net/gml#AbstractRingType"/>
   </owl:Class>
   <owl:Class rdf:about="http://www.opengis.net/gml#exterior">
      <rdfs:subClassOf rdf:resource="http://www.opengis.net/gml#AbstractRingPropertyType"/>
   </owl:Class>
   <owl:Class rdf:about="http://www.opengis.net/gml#interior">
      <rdfs:subClassOf rdf:resource="http://www.opengis.net/gml#AbstractRingPropertyType"/>
   </owl:Class>
   <owl:Class rdf:about="http://www.opengis.net/gml#outerBoundaryIs">
      <rdfs:subClassOf rdf:resource="http://www.opengis.net/gml#exterior"/>
      <rdfs:subClassOf rdf:resource="http://www.opengis.net/gml#AbstractRingPropertyType"/>
   </owl:Class>
   <owl:Class rdf:about="http://www.opengis.net/gml#innerBoundaryIs">
      <rdfs:subClassOf rdf:resource="http://www.opengis.net/gml#interior"/>
      <rdfs:subClassOf rdf:resource="http://www.opengis.net/gml#AbstractRingPropertyType"/>
   </owl:Class>
   <owl:Class rdf:about="http://www.opengis.net/gml#LinearRing">
      <rdfs:subClassOf rdf:resource="http://www.opengis.net/gml#_Ring"/>
      <rdfs:subClassOf rdf:resource="http://www.opengis.net/gml#LinearRingType"/>
   </owl:Class>
   <owl:Class rdf:about="http://www.opengis.net/gml#polygonProperty">
      <rdfs:subClassOf rdf:resource="http://www.opengis.net/gml#PolygonPropertyType"/>
   </owl:Class>
   <owl:Class rdf:about="http://www.opengis.net/gml#_Geometry">
      <rdfs:subClassOf rdf:resource="http://www.opengis.net/gml#_GML"/>
      <rdfs:subClassOf rdf:resource="http://www.opengis.net/gml#AbstractGeometryType"/>
   </owl:Class>
   <owl:Class rdf:about="http://www.opengis.net/gml#_GeometricPrimitive">
      <rdfs:subClassOf rdf:resource="http://www.opengis.net/gml#_Geometry"/>
      <rdfs:subClassOf rdf:resource="http://www.opengis.net/gml#AbstractGeometricPrimitiveType"/>
   </owl:Class>
   <owl:Class rdf:about="http://www.opengis.net/gml#Point">
      <rdfs:subClassOf rdf:resource="http://www.opengis.net/gml#_GeometricPrimitive"/>
      <rdfs:subClassOf rdf:resource="http://www.opengis.net/gml#PointType"/>
   </owl:Class>
   <owl:Class rdf:about="http://www.opengis.net/gml#pointProperty">
      <rdfs:subClassOf rdf:resource="http://www.opengis.net/gml#PointPropertyType"/>
   </owl:Class>
   <owl:Class rdf:about="http://www.opengis.net/gml#pointRep">
      <rdfs:subClassOf rdf:resource="http://www.opengis.net/gml#PointPropertyType"/>
   </owl:Class>
   <owl:Class rdf:about="http://www.opengis.net/gml#pointArrayProperty">
      <rdfs:subClassOf rdf:resource="http://www.opengis.net/gml#PointArrayPropertyType"/>
   </owl:Class>
   <owl:Class rdf:about="http://www.opengis.net/gml#_Curve">
      <rdfs:subClassOf rdf:resource="http://www.opengis.net/gml#_GeometricPrimitive"/>
      <rdfs:subClassOf rdf:resource="http://www.opengis.net/gml#AbstractCurveType"/>
   </owl:Class>
   <owl:Class rdf:about="http://www.opengis.net/gml#curveProperty">
      <rdfs:subClassOf rdf:resource="http://www.opengis.net/gml#CurvePropertyType"/>
   </owl:Class>
   <owl:Class rdf:about="http://www.opengis.net/gml#curveArrayProperty">
      <rdfs:subClassOf rdf:resource="http://www.opengis.net/gml#CurveArrayPropertyType"/>
   </owl:Class>
   <owl:Class rdf:about="http://www.opengis.net/gml#LineString">
      <rdfs:subClassOf rdf:resource="http://www.opengis.net/gml#_Curve"/>
      <rdfs:subClassOf rdf:resource="http://www.opengis.net/gml#LineStringType"/>
   </owl:Class>
   <owl:Class rdf:about="http://www.opengis.net/gml#pos">
      <rdfs:subClassOf rdf:resource="http://www.opengis.net/gml#DirectPositionType"/>
   </owl:Class>
   <owl:Class rdf:about="http://www.opengis.net/gml#posList">
      <rdfs:subClassOf rdf:resource="http://www.opengis.net/gml#DirectPositionListType"/>
   </owl:Class>
   <owl:Class rdf:about="http://www.opengis.net/gml#vector">
      <rdfs:subClassOf rdf:resource="http://www.opengis.net/gml#VectorType"/>
   </owl:Class>
   <owl:Class rdf:about="http://www.opengis.net/gml#coordinates">
      <rdfs:subClassOf rdf:resource="http://www.opengis.net/gml#CoordinatesType"/>
   </owl:Class>
   <owl:Class rdf:about="http://www.opengis.net/gml#Envelope">
      <rdfs:subClassOf rdf:resource="http://www.opengis.net/gml#EnvelopeType"/>
   </owl:Class>
   <owl:Class rdf:about="http://www.opengis.net/gml#coord">
      <rdfs:subClassOf rdf:resource="http://www.opengis.net/gml#CoordType"/>
   </owl:Class>
   <owl:Class rdf:about="http://www.opengis.net/gml#lineStringProperty">
      <rdfs:subClassOf rdf:resource="http://www.opengis.net/gml#LineStringPropertyType"/>
   </owl:Class>
   <owl:Class rdf:about="http://www.opengis.net/gml#measure">
      <rdfs:subClassOf rdf:resource="http://www.opengis.net/gml#MeasureType"/>
   </owl:Class>
   <owl:Class rdf:about="http://www.opengis.net/gml#angle">
      <rdfs:subClassOf rdf:resource="http://www.opengis.net/gml#MeasureType"/>
   </owl:Class>
   <owl:Class rdf:about="http://www.opengis.net/gml#dmsAngle">
      <rdfs:subClassOf rdf:resource="http://www.opengis.net/gml#DMSAngleType"/>
   </owl:Class>
   <owl:Class rdf:about="http://www.opengis.net/gml#degrees">
      <rdfs:subClassOf rdf:resource="http://www.opengis.net/gml#DegreesType"/>
   </owl:Class>
   <rdfs:Datatype rdf:about="http://www.opengis.net/gml#decimalMinutes">
      <owl:equivalentClass rdf:resource="http://www.opengis.net/gml#DecimalMinutesType"/>
   </rdfs:Datatype>
   <rdfs:Datatype rdf:about="http://www.opengis.net/gml#minutes">
      <owl:equivalentClass rdf:resource="http://www.opengis.net/gml#ArcMinutesType"/>
   </rdfs:Datatype>
   <rdfs:Datatype rdf:about="http://www.opengis.net/gml#seconds">
      <owl:equivalentClass rdf:resource="http://www.opengis.net/gml#ArcSecondsType"/>
   </rdfs:Datatype>
   <owl:Class rdf:about="http://www.opengis.net/gml#unitOfMeasure">
      <rdfs:subClassOf rdf:resource="http://www.opengis.net/gml#UnitOfMeasureType"/>
   </owl:Class>
   <owl:Class rdf:about="http://www.opengis.net/gml#UnitDefinition">
      <rdfs:subClassOf rdf:resource="http://www.opengis.net/gml#Definition"/>
      <rdfs:subClassOf rdf:resource="http://www.opengis.net/gml#UnitDefinitionType"/>
   </owl:Class>
   <owl:Class rdf:about="http://www.opengis.net/gml#BaseUnit">
      <rdfs:subClassOf rdf:resource="http://www.opengis.net/gml#UnitDefinition"/>
      <rdfs:subClassOf rdf:resource="http://www.opengis.net/gml#BaseUnitType"/>
   </owl:Class>
   <owl:Class rdf:about="http://www.opengis.net/gml#DerivedUnit">
      <rdfs:subClassOf rdf:resource="http://www.opengis.net/gml#UnitDefinition"/>
      <rdfs:subClassOf rdf:resource="http://www.opengis.net/gml#DerivedUnitType"/>
   </owl:Class>
   <owl:Class rdf:about="http://www.opengis.net/gml#ConventionalUnit">
      <rdfs:subClassOf rdf:resource="http://www.opengis.net/gml#UnitDefinition"/>
      <rdfs:subClassOf rdf:resource="http://www.opengis.net/gml#ConventionalUnitType"/>
   </owl:Class>
   <owl:Class rdf:about="http://www.opengis.net/gml#quantityType">
      <rdfs:subClassOf rdf:resource="http://www.opengis.net/gml#StringOrRefType"/>
   </owl:Class>
   <owl:Class rdf:about="http://www.opengis.net/gml#catalogSymbol">
      <rdfs:subClassOf rdf:resource="http://www.opengis.net/gml#CodeType"/>
   </owl:Class>
   <owl:Class rdf:about="http://www.opengis.net/gml#derivationUnitTerm">
      <rdfs:subClassOf rdf:resource="http://www.opengis.net/gml#DerivationUnitTermType"/>
   </owl:Class>
   <owl:Class rdf:about="http://www.opengis.net/gml#conversionToPreferredUnit">
      <rdfs:subClassOf rdf:resource="http://www.opengis.net/gml#ConversionToPreferredUnitType"/>
   </owl:Class>
   <owl:Class rdf:about="http://www.opengis.net/gml#roughConversionToPreferredUnit">
      <rdfs:subClassOf rdf:resource="http://www.opengis.net/gml#ConversionToPreferredUnitType"/>
   </owl:Class>
   <owl:Class rdf:about="http://www.opengis.net/gml#Definition">
      <rdfs:subClassOf rdf:resource="http://www.opengis.net/gml#_GML"/>
      <rdfs:subClassOf rdf:resource="http://www.opengis.net/gml#DefinitionType"/>
   </owl:Class>
   <owl:Class rdf:about="http://www.opengis.net/gml#Dictionary">
      <rdfs:subClassOf rdf:resource="http://www.opengis.net/gml#Definition"/>
      <rdfs:subClassOf rdf:resource="http://www.opengis.net/gml#DictionaryType"/>
   </owl:Class>
   <owl:Class rdf:about="http://www.opengis.net/gml#DefinitionCollection">
      <rdfs:subClassOf rdf:resource="http://www.opengis.net/gml#Definition"/>
      <rdfs:subClassOf rdf:resource="http://www.opengis.net/gml#DictionaryType"/>
   </owl:Class>
   <owl:Class rdf:about="http://www.opengis.net/gml#dictionaryEntry">
      <rdfs:subClassOf rdf:resource="http://www.opengis.net/gml#DictionaryEntryType"/>
   </owl:Class>
   <owl:Class rdf:about="http://www.opengis.net/gml#definitionMember">
      <rdfs:subClassOf rdf:resource="http://www.opengis.net/gml#dictionaryEntry"/>
      <rdfs:subClassOf rdf:resource="http://www.opengis.net/gml#DictionaryEntryType"/>
   </owl:Class>
   <owl:Class rdf:about="http://www.opengis.net/gml#indirectEntry">
      <rdfs:subClassOf rdf:resource="http://www.opengis.net/gml#IndirectEntryType"/>
   </owl:Class>
   <owl:Class rdf:about="http://www.opengis.net/gml#DefinitionProxy">
      <rdfs:subClassOf rdf:resource="http://www.opengis.net/gml#Definition"/>
      <rdfs:subClassOf rdf:resource="http://www.opengis.net/gml#DefinitionProxyType"/>
   </owl:Class>
   <owl:Class rdf:about="http://www.opengis.net/gml#definitionRef">
      <rdfs:subClassOf rdf:resource="http://www.opengis.net/gml#ReferenceType"/>
   </owl:Class>
   <owl:Class rdf:about="http://www.opengis.net/gml#_GML">
      <rdfs:subClassOf rdf:resource="http://www.opengis.net/gml#_Object"/>
      <rdfs:subClassOf rdf:resource="http://www.opengis.net/gml#AbstractGMLType"/>
   </owl:Class>
   <owl:Class rdf:about="http://www.opengis.net/gml#Bag">
      <rdfs:subClassOf rdf:resource="http://www.opengis.net/gml#_GML"/>
      <rdfs:subClassOf rdf:resource="http://www.opengis.net/gml#BagType"/>
   </owl:Class>
   <owl:Class rdf:about="http://www.opengis.net/gml#Array">
      <rdfs:subClassOf rdf:resource="http://www.opengis.net/gml#_GML"/>
      <rdfs:subClassOf rdf:resource="http://www.opengis.net/gml#ArrayType"/>
   </owl:Class>
   <owl:Class rdf:about="http://www.opengis.net/gml#_MetaData">
      <rdfs:subClassOf rdf:resource="http://www.opengis.net/gml#_Object"/>
      <rdfs:subClassOf rdf:resource="http://www.opengis.net/gml#AbstractMetaDataType"/>
   </owl:Class>
   <owl:Class rdf:about="http://www.opengis.net/gml#GenericMetaData">
      <rdfs:subClassOf rdf:resource="http://www.opengis.net/gml#_MetaData"/>
      <rdfs:subClassOf rdf:resource="http://www.opengis.net/gml#GenericMetaDataType"/>
   </owl:Class>
   <owl:Class rdf:about="http://www.opengis.net/gml#_association">
      <rdfs:subClassOf rdf:resource="http://www.opengis.net/gml#AssociationType"/>
   </owl:Class>
   <owl:Class rdf:about="http://www.opengis.net/gml#_strictAssociation">
      <rdfs:subClassOf rdf:resource="http://www.opengis.net/gml#AssociationType"/>
   </owl:Class>
   <owl:Class rdf:about="http://www.opengis.net/gml#member">
      <rdfs:subClassOf rdf:resource="http://www.opengis.net/gml#AssociationType"/>
   </owl:Class>
   <owl:Class rdf:about="http://www.opengis.net/gml#_reference">
      <rdfs:subClassOf rdf:resource="http://www.opengis.net/gml#ReferenceType"/>
   </owl:Class>
   <owl:Class rdf:about="http://www.opengis.net/gml#members">
      <rdfs:subClassOf rdf:resource="http://www.opengis.net/gml#ArrayAssociationType"/>
   </owl:Class>
   <owl:Class rdf:about="http://www.opengis.net/gml#metaDataProperty">
      <rdfs:subClassOf rdf:resource="http://www.opengis.net/gml#MetaDataPropertyType"/>
   </owl:Class>
   <owl:Class rdf:about="http://www.opengis.net/gml#name">
      <rdfs:subClassOf rdf:resource="http://www.opengis.net/gml#CodeType"/>
   </owl:Class>
   <owl:Class rdf:about="http://www.opengis.net/gml#description">
      <rdfs:subClassOf rdf:resource="http://www.opengis.net/gml#StringOrRefType"/>
   </owl:Class>
   <rdfs:Datatype rdf:about="http://www.opengis.net/gml#Null">
      <owl:equivalentClass rdf:resource="http://www.opengis.net/gml#NullType"/>
   </rdfs:Datatype>
   <owl:Class rdf:about="http://www.opengis.net/gml#_TimeObject">
      <rdfs:subClassOf rdf:resource="http://www.opengis.net/gml#_GML"/>
      <rdfs:subClassOf rdf:resource="http://www.opengis.net/gml#AbstractTimeObjectType"/>
   </owl:Class>
   <owl:Class rdf:about="http://www.opengis.net/gml#_TimePrimitive">
      <rdfs:subClassOf rdf:resource="http://www.opengis.net/gml#_TimeObject"/>
      <rdfs:subClassOf rdf:resource="http://www.opengis.net/gml#AbstractTimePrimitiveType"/>
   </owl:Class>
   <owl:Class rdf:about="http://www.opengis.net/gml#_TimeComplex">
      <rdfs:subClassOf rdf:resource="http://www.opengis.net/gml#_TimeObject"/>
      <rdfs:subClassOf rdf:resource="http://www.opengis.net/gml#AbstractTimeComplexType"/>
   </owl:Class>
   <owl:Class rdf:about="http://www.opengis.net/gml#_TimeGeometricPrimitive">
      <rdfs:subClassOf rdf:resource="http://www.opengis.net/gml#_TimePrimitive"/>
      <rdfs:subClassOf rdf:resource="http://www.opengis.net/gml#AbstractTimeGeometricPrimitiveType"/>
   </owl:Class>
   <owl:Class rdf:about="http://www.opengis.net/gml#TimeInstant">
      <rdfs:subClassOf rdf:resource="http://www.opengis.net/gml#_TimeGeometricPrimitive"/>
      <rdfs:subClassOf rdf:resource="http://www.opengis.net/gml#TimeInstantType"/>
   </owl:Class>
   <owl:Class rdf:about="http://www.opengis.net/gml#TimePeriod">
      <rdfs:subClassOf rdf:resource="http://www.opengis.net/gml#_TimeGeometricPrimitive"/>
      <rdfs:subClassOf rdf:resource="http://www.opengis.net/gml#TimePeriodType"/>
   </owl:Class>
   <rdfs:Datatype rdf:about="http://www.opengis.net/gml#duration">
      <owl:equivalentClass rdf:resource="http://www.w3.org/2001/XMLSchema#duration"/>
   </rdfs:Datatype>
   <owl:Class rdf:about="http://www.opengis.net/gml#timeInterval">
      <rdfs:subClassOf rdf:resource="http://www.opengis.net/gml#TimeIntervalLengthType"/>
   </owl:Class>
   <owl:Class rdf:about="http://www.opengis.net/gml#timePosition">
      <rdfs:subClassOf rdf:resource="http://www.opengis.net/gml#TimePositionType"/>
   </owl:Class>
   <owl:Class rdf:about="http://www.opengis.net/gml#validTime">
      <rdfs:subClassOf rdf:resource="http://www.opengis.net/gml#TimePrimitivePropertyType"/>
   </owl:Class>
   <owl:Class rdf:about="http://www.opengis.net/gml#direction">
      <rdfs:subClassOf rdf:resource="http://www.opengis.net/gml#DirectionPropertyType"/>
   </owl:Class>
   <owl:Class rdf:about="http://www.opengis.net/gml#DirectionVector">
      <rdfs:subClassOf rdf:resource="http://www.opengis.net/gml#DirectionVectorType"/>
   </owl:Class>
   <rdfs:Datatype rdf:about="http://www.opengis.net/gml#CompassPoint">
      <owl:equivalentClass rdf:resource="http://www.opengis.net/gml#CompassPointEnumeration"/>
   </rdfs:Datatype>
   <owl:Class rdf:about="http://www.opengis.net/gml#_Topology">
      <rdfs:subClassOf rdf:resource="http://www.opengis.net/gml#_GML"/>
      <rdfs:subClassOf rdf:resource="http://www.opengis.net/gml#AbstractTopologyType"/>
   </owl:Class>
   <owl:Class rdf:about="http://www.opengis.net/gml#_TopoPrimitive">
      <rdfs:subClassOf rdf:resource="http://www.opengis.net/gml#_Topology"/>
      <rdfs:subClassOf rdf:resource="http://www.opengis.net/gml#AbstractTopoPrimitiveType"/>
   </owl:Class>
   <owl:Class rdf:about="http://www.opengis.net/gml#isolated">
      <rdfs:subClassOf rdf:resource="http://www.opengis.net/gml#IsolatedPropertyType"/>
   </owl:Class>
   <owl:Class rdf:about="http://www.opengis.net/gml#container">
      <rdfs:subClassOf rdf:resource="http://www.opengis.net/gml#ContainerPropertyType"/>
   </owl:Class>
   <owl:Class rdf:about="http://www.opengis.net/gml#Node">
      <rdfs:subClassOf rdf:resource="http://www.opengis.net/gml#_TopoPrimitive"/>
      <rdfs:subClassOf rdf:resource="http://www.opengis.net/gml#NodeType"/>
   </owl:Class>
   <owl:Class rdf:about="http://www.opengis.net/gml#directedNode">
      <rdfs:subClassOf rdf:resource="http://www.opengis.net/gml#DirectedNodePropertyType"/>
   </owl:Class>
   <owl:Class rdf:about="http://www.opengis.net/gml#Edge">
      <rdfs:subClassOf rdf:resource="http://www.opengis.net/gml#_TopoPrimitive"/>
      <rdfs:subClassOf rdf:resource="http://www.opengis.net/gml#EdgeType"/>
   </owl:Class>
   <owl:Class rdf:about="http://www.opengis.net/gml#directedEdge">
      <rdfs:subClassOf rdf:resource="http://www.opengis.net/gml#DirectedEdgePropertyType"/>
   </owl:Class>
   <owl:Class rdf:about="http://www.opengis.net/gml#Face">
      <rdfs:subClassOf rdf:resource="http://www.opengis.net/gml#_TopoPrimitive"/>
      <rdfs:subClassOf rdf:resource="http://www.opengis.net/gml#FaceType"/>
   </owl:Class>
   <owl:Class rdf:about="http://www.opengis.net/gml#directedFace">
      <rdfs:subClassOf rdf:resource="http://www.opengis.net/gml#DirectedFacePropertyType"/>
   </owl:Class>
   <owl:Class rdf:about="http://www.opengis.net/gml#TopoSolid">
      <rdfs:subClassOf rdf:resource="http://www.opengis.net/gml#_TopoPrimitive"/>
      <rdfs:subClassOf rdf:resource="http://www.opengis.net/gml#TopoSolidType"/>
   </owl:Class>
   <owl:Class rdf:about="http://www.opengis.net/gml#directedTopoSolid">
      <rdfs:subClassOf rdf:resource="http://www.opengis.net/gml#DirectedTopoSolidPropertyType"/>
   </owl:Class>
   <owl:Class rdf:about="http://www.opengis.net/gml#TopoPoint">
      <rdfs:subClassOf rdf:resource="http://www.opengis.net/gml#TopoPointType"/>
   </owl:Class>
   <owl:Class rdf:about="http://www.opengis.net/gml#topoPointProperty">
      <rdfs:subClassOf rdf:resource="http://www.opengis.net/gml#TopoPointPropertyType"/>
   </owl:Class>
   <owl:Class rdf:about="http://www.opengis.net/gml#TopoCurve">
      <rdfs:subClassOf rdf:resource="http://www.opengis.net/gml#TopoCurveType"/>
   </owl:Class>
   <owl:Class rdf:about="http://www.opengis.net/gml#topoCurveProperty">
      <rdfs:subClassOf rdf:resource="http://www.opengis.net/gml#TopoCurvePropertyType"/>
   </owl:Class>
   <owl:Class rdf:about="http://www.opengis.net/gml#TopoSurface">
      <rdfs:subClassOf rdf:resource="http://www.opengis.net/gml#TopoSurfaceType"/>
   </owl:Class>
   <owl:Class rdf:about="http://www.opengis.net/gml#topoSurfaceProperty">
      <rdfs:subClassOf rdf:resource="http://www.opengis.net/gml#TopoSurfacePropertyType"/>
   </owl:Class>
   <owl:Class rdf:about="http://www.opengis.net/gml#TopoVolume">
      <rdfs:subClassOf rdf:resource="http://www.opengis.net/gml#TopoVolumeType"/>
   </owl:Class>
   <owl:Class rdf:about="http://www.opengis.net/gml#topoVolumeProperty">
      <rdfs:subClassOf rdf:resource="http://www.opengis.net/gml#TopoVolumePropertyType"/>
   </owl:Class>
   <owl:Class rdf:about="http://www.opengis.net/gml#TopoComplex">
      <rdfs:subClassOf rdf:resource="http://www.opengis.net/gml#_Topology"/>
      <rdfs:subClassOf rdf:resource="http://www.opengis.net/gml#TopoComplexType"/>
   </owl:Class>
   <owl:Class rdf:about="http://www.opengis.net/gml#topoComplexProperty">
      <rdfs:subClassOf rdf:resource="http://www.opengis.net/gml#TopoComplexMemberType"/>
   </owl:Class>
   <owl:Class rdf:about="http://www.opengis.net/gml#subComplex">
      <rdfs:subClassOf rdf:resource="http://www.opengis.net/gml#TopoComplexMemberType"/>
   </owl:Class>
   <owl:Class rdf:about="http://www.opengis.net/gml#superComplex">
      <rdfs:subClassOf rdf:resource="http://www.opengis.net/gml#TopoComplexMemberType"/>
   </owl:Class>
   <owl:Class rdf:about="http://www.opengis.net/gml#maximalComplex">
      <rdfs:subClassOf rdf:resource="http://www.opengis.net/gml#TopoComplexMemberType"/>
   </owl:Class>
   <owl:Class rdf:about="http://www.opengis.net/gml#topoPrimitiveMember">
      <rdfs:subClassOf rdf:resource="http://www.opengis.net/gml#TopoPrimitiveMemberType"/>
   </owl:Class>
   <owl:Class rdf:about="http://www.opengis.net/gml#topoPrimitiveMembers">
      <rdfs:subClassOf rdf:resource="http://www.opengis.net/gml#TopoPrimitiveArrayAssociationType"/>
   </owl:Class>
   <owl:Class rdf:about="http://www.opengis.net/gml#CompositeCurve">
      <rdfs:subClassOf rdf:resource="http://www.opengis.net/gml#_Curve"/>
      <rdfs:subClassOf rdf:resource="http://www.opengis.net/gml#CompositeCurveType"/>
   </owl:Class>
   <owl:Class rdf:about="http://www.opengis.net/gml#CompositeSurface">
      <rdfs:subClassOf rdf:resource="http://www.opengis.net/gml#_Surface"/>
      <rdfs:subClassOf rdf:resource="http://www.opengis.net/gml#CompositeSurfaceType"/>
   </owl:Class>
   <owl:Class rdf:about="http://www.opengis.net/gml#CompositeSolid">
      <rdfs:subClassOf rdf:resource="http://www.opengis.net/gml#_Solid"/>
      <rdfs:subClassOf rdf:resource="http://www.opengis.net/gml#CompositeSolidType"/>
   </owl:Class>
   <owl:Class rdf:about="http://www.opengis.net/gml#GeometricComplex">
      <rdfs:subClassOf rdf:resource="http://www.opengis.net/gml#_Geometry"/>
      <rdfs:subClassOf rdf:resource="http://www.opengis.net/gml#GeometricComplexType"/>
   </owl:Class>
   <owl:Class rdf:about="http://www.opengis.net/gml#_GeometricAggregate">
      <rdfs:subClassOf rdf:resource="http://www.opengis.net/gml#_Geometry"/>
      <rdfs:subClassOf rdf:resource="http://www.opengis.net/gml#AbstractGeometricAggregateType"/>
   </owl:Class>
   <owl:Class rdf:about="http://www.opengis.net/gml#MultiGeometry">
      <rdfs:subClassOf rdf:resource="http://www.opengis.net/gml#_GeometricAggregate"/>
      <rdfs:subClassOf rdf:resource="http://www.opengis.net/gml#MultiGeometryType"/>
   </owl:Class>
   <owl:Class rdf:about="http://www.opengis.net/gml#multiGeometryProperty">
      <rdfs:subClassOf rdf:resource="http://www.opengis.net/gml#MultiGeometryPropertyType"/>
   </owl:Class>
   <owl:Class rdf:about="http://www.opengis.net/gml#MultiPoint">
      <rdfs:subClassOf rdf:resource="http://www.opengis.net/gml#_GeometricAggregate"/>
      <rdfs:subClassOf rdf:resource="http://www.opengis.net/gml#MultiPointType"/>
   </owl:Class>
   <owl:Class rdf:about="http://www.opengis.net/gml#multiPointProperty">
      <rdfs:subClassOf rdf:resource="http://www.opengis.net/gml#MultiPointPropertyType"/>
   </owl:Class>
   <owl:Class rdf:about="http://www.opengis.net/gml#MultiCurve">
      <rdfs:subClassOf rdf:resource="http://www.opengis.net/gml#_GeometricAggregate"/>
      <rdfs:subClassOf rdf:resource="http://www.opengis.net/gml#MultiCurveType"/>
   </owl:Class>
   <owl:Class rdf:about="http://www.opengis.net/gml#multiCurveProperty">
      <rdfs:subClassOf rdf:resource="http://www.opengis.net/gml#MultiCurvePropertyType"/>
   </owl:Class>
   <owl:Class rdf:about="http://www.opengis.net/gml#MultiSurface">
      <rdfs:subClassOf rdf:resource="http://www.opengis.net/gml#_GeometricAggregate"/>
      <rdfs:subClassOf rdf:resource="http://www.opengis.net/gml#MultiSurfaceType"/>
   </owl:Class>
   <owl:Class rdf:about="http://www.opengis.net/gml#multiSurfaceProperty">
      <rdfs:subClassOf rdf:resource="http://www.opengis.net/gml#MultiSurfacePropertyType"/>
   </owl:Class>
   <owl:Class rdf:about="http://www.opengis.net/gml#MultiSolid">
      <rdfs:subClassOf rdf:resource="http://www.opengis.net/gml#_GeometricAggregate"/>
      <rdfs:subClassOf rdf:resource="http://www.opengis.net/gml#MultiSolidType"/>
   </owl:Class>
   <owl:Class rdf:about="http://www.opengis.net/gml#multiSolidProperty">
      <rdfs:subClassOf rdf:resource="http://www.opengis.net/gml#MultiSolidPropertyType"/>
   </owl:Class>
   <owl:Class rdf:about="http://www.opengis.net/gml#MultiPolygon">
      <rdfs:subClassOf rdf:resource="http://www.opengis.net/gml#_GeometricAggregate"/>
      <rdfs:subClassOf rdf:resource="http://www.opengis.net/gml#MultiPolygonType"/>
   </owl:Class>
   <owl:Class rdf:about="http://www.opengis.net/gml#MultiLineString">
      <rdfs:subClassOf rdf:resource="http://www.opengis.net/gml#_GeometricAggregate"/>
      <rdfs:subClassOf rdf:resource="http://www.opengis.net/gml#MultiLineStringType"/>
   </owl:Class>
   <owl:Class rdf:about="http://www.opengis.net/gml#geometryMember">
      <rdfs:subClassOf rdf:resource="http://www.opengis.net/gml#GeometryPropertyType"/>
   </owl:Class>
   <owl:Class rdf:about="http://www.opengis.net/gml#geometryMembers">
      <rdfs:subClassOf rdf:resource="http://www.opengis.net/gml#GeometryArrayPropertyType"/>
   </owl:Class>
   <owl:Class rdf:about="http://www.opengis.net/gml#pointMember">
      <rdfs:subClassOf rdf:resource="http://www.opengis.net/gml#PointPropertyType"/>
   </owl:Class>
   <owl:Class rdf:about="http://www.opengis.net/gml#pointMembers">
      <rdfs:subClassOf rdf:resource="http://www.opengis.net/gml#PointArrayPropertyType"/>
   </owl:Class>
   <owl:Class rdf:about="http://www.opengis.net/gml#curveMembers">
      <rdfs:subClassOf rdf:resource="http://www.opengis.net/gml#CurveArrayPropertyType"/>
   </owl:Class>
   <owl:Class rdf:about="http://www.opengis.net/gml#surfaceMember">
      <rdfs:subClassOf rdf:resource="http://www.opengis.net/gml#SurfacePropertyType"/>
   </owl:Class>
   <owl:Class rdf:about="http://www.opengis.net/gml#surfaceMembers">
      <rdfs:subClassOf rdf:resource="http://www.opengis.net/gml#SurfaceArrayPropertyType"/>
   </owl:Class>
   <owl:Class rdf:about="http://www.opengis.net/gml#solidMember">
      <rdfs:subClassOf rdf:resource="http://www.opengis.net/gml#SolidPropertyType"/>
   </owl:Class>
   <owl:Class rdf:about="http://www.opengis.net/gml#solidMembers">
      <rdfs:subClassOf rdf:resource="http://www.opengis.net/gml#SolidArrayPropertyType"/>
   </owl:Class>
   <owl:Class rdf:about="http://www.opengis.net/gml#multiCenterOf">
      <rdfs:subClassOf rdf:resource="http://www.opengis.net/gml#MultiPointPropertyType"/>
   </owl:Class>
   <owl:Class rdf:about="http://www.opengis.net/gml#multiPosition">
      <rdfs:subClassOf rdf:resource="http://www.opengis.net/gml#MultiPointPropertyType"/>
   </owl:Class>
   <owl:Class rdf:about="http://www.opengis.net/gml#multiCenterLineOf">
      <rdfs:subClassOf rdf:resource="http://www.opengis.net/gml#MultiCurvePropertyType"/>
   </owl:Class>
   <owl:Class rdf:about="http://www.opengis.net/gml#multiEdgeOf">
      <rdfs:subClassOf rdf:resource="http://www.opengis.net/gml#MultiCurvePropertyType"/>
   </owl:Class>
   <owl:Class rdf:about="http://www.opengis.net/gml#multiCoverage">
      <rdfs:subClassOf rdf:resource="http://www.opengis.net/gml#MultiSurfacePropertyType"/>
   </owl:Class>
   <owl:Class rdf:about="http://www.opengis.net/gml#multiExtentOf">
      <rdfs:subClassOf rdf:resource="http://www.opengis.net/gml#MultiSurfacePropertyType"/>
   </owl:Class>
   <owl:Class rdf:about="http://www.opengis.net/gml#multiLocation">
      <rdfs:subClassOf rdf:resource="http://www.opengis.net/gml#MultiPointPropertyType"/>
   </owl:Class>
   <owl:Class rdf:about="http://www.opengis.net/gml#lineStringMember">
      <rdfs:subClassOf rdf:resource="http://www.opengis.net/gml#LineStringPropertyType"/>
   </owl:Class>
   <owl:Class rdf:about="http://www.opengis.net/gml#polygonMember">
      <rdfs:subClassOf rdf:resource="http://www.opengis.net/gml#PolygonPropertyType"/>
   </owl:Class>
   <owl:Class rdf:about="http://www.opengis.net/gml#Curve">
      <rdfs:subClassOf rdf:resource="http://www.opengis.net/gml#_Curve"/>
      <rdfs:subClassOf rdf:resource="http://www.opengis.net/gml#CurveType"/>
   </owl:Class>
   <owl:Class rdf:about="http://www.opengis.net/gml#baseCurve">
      <rdfs:subClassOf rdf:resource="http://www.opengis.net/gml#CurvePropertyType"/>
   </owl:Class>
   <owl:Class rdf:about="http://www.opengis.net/gml#OrientableCurve">
      <rdfs:subClassOf rdf:resource="http://www.opengis.net/gml#_Curve"/>
      <rdfs:subClassOf rdf:resource="http://www.opengis.net/gml#OrientableCurveType"/>
   </owl:Class>
   <owl:Class rdf:about="http://www.opengis.net/gml#_CurveSegment">
      <rdfs:subClassOf rdf:resource="http://www.opengis.net/gml#AbstractCurveSegmentType"/>
   </owl:Class>
   <owl:Class rdf:about="http://www.opengis.net/gml#segments">
      <rdfs:subClassOf rdf:resource="http://www.opengis.net/gml#CurveSegmentArrayPropertyType"/>
   </owl:Class>
   <owl:Class rdf:about="http://www.opengis.net/gml#LineStringSegment">
      <rdfs:subClassOf rdf:resource="http://www.opengis.net/gml#_CurveSegment"/>
      <rdfs:subClassOf rdf:resource="http://www.opengis.net/gml#LineStringSegmentType"/>
   </owl:Class>
   <owl:Class rdf:about="http://www.opengis.net/gml#ArcString">
      <rdfs:subClassOf rdf:resource="http://www.opengis.net/gml#_CurveSegment"/>
      <rdfs:subClassOf rdf:resource="http://www.opengis.net/gml#ArcStringType"/>
   </owl:Class>
   <owl:Class rdf:about="http://www.opengis.net/gml#Arc">
      <rdfs:subClassOf rdf:resource="http://www.opengis.net/gml#ArcString"/>
      <rdfs:subClassOf rdf:resource="http://www.opengis.net/gml#ArcType"/>
   </owl:Class>
   <owl:Class rdf:about="http://www.opengis.net/gml#Circle">
      <rdfs:subClassOf rdf:resource="http://www.opengis.net/gml#Arc"/>
      <rdfs:subClassOf rdf:resource="http://www.opengis.net/gml#CircleType"/>
   </owl:Class>
   <owl:Class rdf:about="http://www.opengis.net/gml#ArcStringByBulge">
      <rdfs:subClassOf rdf:resource="http://www.opengis.net/gml#_CurveSegment"/>
      <rdfs:subClassOf rdf:resource="http://www.opengis.net/gml#ArcStringByBulgeType"/>
   </owl:Class>
   <owl:Class rdf:about="http://www.opengis.net/gml#ArcByBulge">
      <rdfs:subClassOf rdf:resource="http://www.opengis.net/gml#ArcStringByBulge"/>
      <rdfs:subClassOf rdf:resource="http://www.opengis.net/gml#ArcByBulgeType"/>
   </owl:Class>
   <owl:Class rdf:about="http://www.opengis.net/gml#ArcByCenterPoint">
      <rdfs:subClassOf rdf:resource="http://www.opengis.net/gml#_CurveSegment"/>
      <rdfs:subClassOf rdf:resource="http://www.opengis.net/gml#ArcByCenterPointType"/>
   </owl:Class>
   <owl:Class rdf:about="http://www.opengis.net/gml#CircleByCenterPoint">
      <rdfs:subClassOf rdf:resource="http://www.opengis.net/gml#ArcByCenterPoint"/>
      <rdfs:subClassOf rdf:resource="http://www.opengis.net/gml#CircleByCenterPointType"/>
   </owl:Class>
   <owl:Class rdf:about="http://www.opengis.net/gml#OffsetCurve">
      <rdfs:subClassOf rdf:resource="http://www.opengis.net/gml#_CurveSegment"/>
      <rdfs:subClassOf rdf:resource="http://www.opengis.net/gml#OffsetCurveType"/>
   </owl:Class>
   <owl:Class rdf:about="http://www.opengis.net/gml#AffinePlacement">
      <rdfs:subClassOf rdf:resource="http://www.opengis.net/gml#AffinePlacementType"/>
   </owl:Class>
   <owl:Class rdf:about="http://www.opengis.net/gml#Clothoid">
      <rdfs:subClassOf rdf:resource="http://www.opengis.net/gml#_CurveSegment"/>
      <rdfs:subClassOf rdf:resource="http://www.opengis.net/gml#ClothoidType"/>
   </owl:Class>
   <owl:Class rdf:about="http://www.opengis.net/gml#GeodesicString">
      <rdfs:subClassOf rdf:resource="http://www.opengis.net/gml#_CurveSegment"/>
      <rdfs:subClassOf rdf:resource="http://www.opengis.net/gml#GeodesicStringType"/>
   </owl:Class>
   <owl:Class rdf:about="http://www.opengis.net/gml#Geodesic">
      <rdfs:subClassOf rdf:resource="http://www.opengis.net/gml#GeodesicString"/>
      <rdfs:subClassOf rdf:resource="http://www.opengis.net/gml#GeodesicType"/>
   </owl:Class>
   <owl:Class rdf:about="http://www.opengis.net/gml#CubicSpline">
      <rdfs:subClassOf rdf:resource="http://www.opengis.net/gml#_CurveSegment"/>
      <rdfs:subClassOf rdf:resource="http://www.opengis.net/gml#CubicSplineType"/>
   </owl:Class>
   <owl:Class rdf:about="http://www.opengis.net/gml#BSpline">
      <rdfs:subClassOf rdf:resource="http://www.opengis.net/gml#_CurveSegment"/>
      <rdfs:subClassOf rdf:resource="http://www.opengis.net/gml#BSplineType"/>
   </owl:Class>
   <owl:Class rdf:about="http://www.opengis.net/gml#Bezier">
      <rdfs:subClassOf rdf:resource="http://www.opengis.net/gml#BSpline"/>
      <rdfs:subClassOf rdf:resource="http://www.opengis.net/gml#BezierType"/>
   </owl:Class>
   <owl:Class rdf:about="http://www.opengis.net/gml#Surface">
      <rdfs:subClassOf rdf:resource="http://www.opengis.net/gml#_Surface"/>
      <rdfs:subClassOf rdf:resource="http://www.opengis.net/gml#SurfaceType"/>
   </owl:Class>
   <owl:Class rdf:about="http://www.opengis.net/gml#baseSurface">
      <rdfs:subClassOf rdf:resource="http://www.opengis.net/gml#SurfacePropertyType"/>
   </owl:Class>
   <owl:Class rdf:about="http://www.opengis.net/gml#OrientableSurface">
      <rdfs:subClassOf rdf:resource="http://www.opengis.net/gml#_Surface"/>
      <rdfs:subClassOf rdf:resource="http://www.opengis.net/gml#OrientableSurfaceType"/>
   </owl:Class>
   <owl:Class rdf:about="http://www.opengis.net/gml#_SurfacePatch">
      <rdfs:subClassOf rdf:resource="http://www.opengis.net/gml#AbstractSurfacePatchType"/>
   </owl:Class>
   <owl:Class rdf:about="http://www.opengis.net/gml#patches">
      <rdfs:subClassOf rdf:resource="http://www.opengis.net/gml#SurfacePatchArrayPropertyType"/>
   </owl:Class>
   <owl:Class rdf:about="http://www.opengis.net/gml#PolygonPatch">
      <rdfs:subClassOf rdf:resource="http://www.opengis.net/gml#_SurfacePatch"/>
      <rdfs:subClassOf rdf:resource="http://www.opengis.net/gml#PolygonPatchType"/>
   </owl:Class>
   <owl:Class rdf:about="http://www.opengis.net/gml#Triangle">
      <rdfs:subClassOf rdf:resource="http://www.opengis.net/gml#_SurfacePatch"/>
      <rdfs:subClassOf rdf:resource="http://www.opengis.net/gml#TriangleType"/>
   </owl:Class>
   <owl:Class rdf:about="http://www.opengis.net/gml#Rectangle">
      <rdfs:subClassOf rdf:resource="http://www.opengis.net/gml#_SurfacePatch"/>
      <rdfs:subClassOf rdf:resource="http://www.opengis.net/gml#RectangleType"/>
   </owl:Class>
   <owl:Class rdf:about="http://www.opengis.net/gml#curveMember">
      <rdfs:subClassOf rdf:resource="http://www.opengis.net/gml#CurvePropertyType"/>
   </owl:Class>
   <owl:Class rdf:about="http://www.opengis.net/gml#Ring">
      <rdfs:subClassOf rdf:resource="http://www.opengis.net/gml#_Ring"/>
      <rdfs:subClassOf rdf:resource="http://www.opengis.net/gml#RingType"/>
   </owl:Class>
   <owl:Class rdf:about="http://www.opengis.net/gml#_ParametricCurveSurface">
      <rdfs:subClassOf rdf:resource="http://www.opengis.net/gml#_SurfacePatch"/>
      <rdfs:subClassOf rdf:resource="http://www.opengis.net/gml#AbstractParametricCurveSurfaceType"/>
   </owl:Class>
   <owl:Class rdf:about="http://www.opengis.net/gml#_GriddedSurface">
      <rdfs:subClassOf rdf:resource="http://www.opengis.net/gml#_ParametricCurveSurface"/>
      <rdfs:subClassOf rdf:resource="http://www.opengis.net/gml#AbstractGriddedSurfaceType"/>
   </owl:Class>
   <owl:Class rdf:about="http://www.opengis.net/gml#Cone">
      <rdfs:subClassOf rdf:resource="http://www.opengis.net/gml#_GriddedSurface"/>
      <rdfs:subClassOf rdf:resource="http://www.opengis.net/gml#ConeType"/>
   </owl:Class>
   <owl:Class rdf:about="http://www.opengis.net/gml#Cylinder">
      <rdfs:subClassOf rdf:resource="http://www.opengis.net/gml#_GriddedSurface"/>
      <rdfs:subClassOf rdf:resource="http://www.opengis.net/gml#CylinderType"/>
   </owl:Class>
   <owl:Class rdf:about="http://www.opengis.net/gml#Sphere">
      <rdfs:subClassOf rdf:resource="http://www.opengis.net/gml#_GriddedSurface"/>
      <rdfs:subClassOf rdf:resource="http://www.opengis.net/gml#SphereType"/>
   </owl:Class>
   <owl:Class rdf:about="http://www.opengis.net/gml#PolyhedralSurface">
      <rdfs:subClassOf rdf:resource="http://www.opengis.net/gml#Surface"/>
      <rdfs:subClassOf rdf:resource="http://www.opengis.net/gml#PolyhedralSurfaceType"/>
   </owl:Class>
   <owl:Class rdf:about="http://www.opengis.net/gml#polygonPatches">
      <rdfs:subClassOf rdf:resource="http://www.opengis.net/gml#patches"/>
      <rdfs:subClassOf rdf:resource="http://www.opengis.net/gml#PolygonPatchArrayPropertyType"/>
   </owl:Class>
   <owl:Class rdf:about="http://www.opengis.net/gml#trianglePatches">
      <rdfs:subClassOf rdf:resource="http://www.opengis.net/gml#patches"/>
      <rdfs:subClassOf rdf:resource="http://www.opengis.net/gml#TrianglePatchArrayPropertyType"/>
   </owl:Class>
   <owl:Class rdf:about="http://www.opengis.net/gml#TriangulatedSurface">
      <rdfs:subClassOf rdf:resource="http://www.opengis.net/gml#Surface"/>
      <rdfs:subClassOf rdf:resource="http://www.opengis.net/gml#TriangulatedSurfaceType"/>
   </owl:Class>
   <owl:Class rdf:about="http://www.opengis.net/gml#Tin">
      <rdfs:subClassOf rdf:resource="http://www.opengis.net/gml#TriangulatedSurface"/>
      <rdfs:subClassOf rdf:resource="http://www.opengis.net/gml#TinType"/>
   </owl:Class>
   <owl:Class rdf:about="http://www.opengis.net/gml#_Solid">
      <rdfs:subClassOf rdf:resource="http://www.opengis.net/gml#_GeometricPrimitive"/>
      <rdfs:subClassOf rdf:resource="http://www.opengis.net/gml#AbstractSolidType"/>
   </owl:Class>
   <owl:Class rdf:about="http://www.opengis.net/gml#solidProperty">
      <rdfs:subClassOf rdf:resource="http://www.opengis.net/gml#SolidPropertyType"/>
   </owl:Class>
   <owl:Class rdf:about="http://www.opengis.net/gml#solidArrayProperty">
      <rdfs:subClassOf rdf:resource="http://www.opengis.net/gml#SolidArrayPropertyType"/>
   </owl:Class>
   <owl:Class rdf:about="http://www.opengis.net/gml#Solid">
      <rdfs:subClassOf rdf:resource="http://www.opengis.net/gml#_Solid"/>
      <rdfs:subClassOf rdf:resource="http://www.opengis.net/gml#SolidType"/>
   </owl:Class>
   <owl:Class rdf:about="http://www.opengis.net/gml#_Coverage">
      <rdfs:subClassOf rdf:resource="http://www.opengis.net/gml#_Feature"/>
      <rdfs:subClassOf rdf:resource="http://www.opengis.net/gml#AbstractCoverageType"/>
   </owl:Class>
   <owl:Class rdf:about="http://www.opengis.net/gml#_ContinuousCoverage">
      <rdfs:subClassOf rdf:resource="http://www.opengis.net/gml#_Coverage"/>
      <rdfs:subClassOf rdf:resource="http://www.opengis.net/gml#AbstractContinuousCoverageType"/>
   </owl:Class>
   <owl:Class rdf:about="http://www.opengis.net/gml#_DiscreteCoverage">
      <rdfs:subClassOf rdf:resource="http://www.opengis.net/gml#_Coverage"/>
      <rdfs:subClassOf rdf:resource="http://www.opengis.net/gml#AbstractDiscreteCoverageType"/>
   </owl:Class>
   <owl:Class rdf:about="http://www.opengis.net/gml#domainSet">
      <rdfs:subClassOf rdf:resource="http://www.opengis.net/gml#DomainSetType"/>
   </owl:Class>
   <owl:Class rdf:about="http://www.opengis.net/gml#rangeSet">
      <rdfs:subClassOf rdf:resource="http://www.opengis.net/gml#RangeSetType"/>
   </owl:Class>
   <owl:Class rdf:about="http://www.opengis.net/gml#coverageFunction">
      <rdfs:subClassOf rdf:resource="http://www.opengis.net/gml#CoverageFunctionType"/>
   </owl:Class>
   <owl:Class rdf:about="http://www.opengis.net/gml#DataBlock">
      <rdfs:subClassOf rdf:resource="http://www.opengis.net/gml#DataBlockType"/>
   </owl:Class>
   <owl:Class rdf:about="http://www.opengis.net/gml#tupleList">
      <rdfs:subClassOf rdf:resource="http://www.opengis.net/gml#CoordinatesType"/>
   </owl:Class>
   <rdfs:Datatype rdf:about="http://www.opengis.net/gml#doubleOrNullTupleList">
      <owl:equivalentClass rdf:resource="http://www.opengis.net/gml#doubleOrNullList"/>
   </rdfs:Datatype>
   <owl:Class rdf:about="http://www.opengis.net/gml#File">
      <rdfs:subClassOf rdf:resource="http://www.opengis.net/gml#FileType"/>
   </owl:Class>
   <owl:Class rdf:about="http://www.opengis.net/gml#rangeParameters">
      <rdfs:subClassOf rdf:resource="http://www.opengis.net/gml#RangeParametersType"/>
   </owl:Class>
   <owl:Class rdf:about="http://www.opengis.net/gml#MappingRule">
      <rdfs:subClassOf rdf:resource="http://www.opengis.net/gml#StringOrRefType"/>
   </owl:Class>
   <owl:Class rdf:about="http://www.opengis.net/gml#GridFunction">
      <rdfs:subClassOf rdf:resource="http://www.opengis.net/gml#GridFunctionType"/>
   </owl:Class>
   <owl:Class rdf:about="http://www.opengis.net/gml#IndexMap">
      <rdfs:subClassOf rdf:resource="http://www.opengis.net/gml#GridFunction"/>
      <rdfs:subClassOf rdf:resource="http://www.opengis.net/gml#IndexMapType"/>
   </owl:Class>
   <owl:Class rdf:about="http://www.opengis.net/gml#MultiPointCoverage">
      <rdfs:subClassOf rdf:resource="http://www.opengis.net/gml#_DiscreteCoverage"/>
      <rdfs:subClassOf rdf:resource="http://www.opengis.net/gml#MultiPointCoverageType"/>
   </owl:Class>
   <owl:Class rdf:about="http://www.opengis.net/gml#multiPointDomain">
      <rdfs:subClassOf rdf:resource="http://www.opengis.net/gml#domainSet"/>
      <rdfs:subClassOf rdf:resource="http://www.opengis.net/gml#MultiPointDomainType"/>
   </owl:Class>
   <owl:Class rdf:about="http://www.opengis.net/gml#MultiCurveCoverage">
      <rdfs:subClassOf rdf:resource="http://www.opengis.net/gml#_DiscreteCoverage"/>
      <rdfs:subClassOf rdf:resource="http://www.opengis.net/gml#MultiCurveCoverageType"/>
   </owl:Class>
   <owl:Class rdf:about="http://www.opengis.net/gml#multiCurveDomain">
      <rdfs:subClassOf rdf:resource="http://www.opengis.net/gml#domainSet"/>
      <rdfs:subClassOf rdf:resource="http://www.opengis.net/gml#MultiCurveDomainType"/>
   </owl:Class>
   <owl:Class rdf:about="http://www.opengis.net/gml#MultiSurfaceCoverage">
      <rdfs:subClassOf rdf:resource="http://www.opengis.net/gml#_DiscreteCoverage"/>
      <rdfs:subClassOf rdf:resource="http://www.opengis.net/gml#MultiSurfaceCoverageType"/>
   </owl:Class>
   <owl:Class rdf:about="http://www.opengis.net/gml#multiSurfaceDomain">
      <rdfs:subClassOf rdf:resource="http://www.opengis.net/gml#domainSet"/>
      <rdfs:subClassOf rdf:resource="http://www.opengis.net/gml#MultiSurfaceDomainType"/>
   </owl:Class>
   <owl:Class rdf:about="http://www.opengis.net/gml#MultiSolidCoverage">
      <rdfs:subClassOf rdf:resource="http://www.opengis.net/gml#_DiscreteCoverage"/>
      <rdfs:subClassOf rdf:resource="http://www.opengis.net/gml#MultiSolidCoverageType"/>
   </owl:Class>
   <owl:Class rdf:about="http://www.opengis.net/gml#multiSolidDomain">
      <rdfs:subClassOf rdf:resource="http://www.opengis.net/gml#domainSet"/>
      <rdfs:subClassOf rdf:resource="http://www.opengis.net/gml#MultiSolidDomainType"/>
   </owl:Class>
   <owl:Class rdf:about="http://www.opengis.net/gml#GridCoverage">
      <rdfs:subClassOf rdf:resource="http://www.opengis.net/gml#_DiscreteCoverage"/>
      <rdfs:subClassOf rdf:resource="http://www.opengis.net/gml#GridCoverageType"/>
   </owl:Class>
   <owl:Class rdf:about="http://www.opengis.net/gml#gridDomain">
      <rdfs:subClassOf rdf:resource="http://www.opengis.net/gml#domainSet"/>
      <rdfs:subClassOf rdf:resource="http://www.opengis.net/gml#GridDomainType"/>
   </owl:Class>
   <owl:Class rdf:about="http://www.opengis.net/gml#RectifiedGridCoverage">
      <rdfs:subClassOf rdf:resource="http://www.opengis.net/gml#_DiscreteCoverage"/>
      <rdfs:subClassOf rdf:resource="http://www.opengis.net/gml#RectifiedGridCoverageType"/>
   </owl:Class>
   <owl:Class rdf:about="http://www.opengis.net/gml#rectifiedGridDomain">
      <rdfs:subClassOf rdf:resource="http://www.opengis.net/gml#domainSet"/>
      <rdfs:subClassOf rdf:resource="http://www.opengis.net/gml#RectifiedGridDomainType"/>
   </owl:Class>
   <rdfs:Datatype rdf:about="http://www.opengis.net/gml#Boolean">
      <owl:equivalentClass rdf:resource="http://www.w3.org/2001/XMLSchema#boolean"/>
   </rdfs:Datatype>
   <rdfs:Datatype rdf:about="http://www.opengis.net/gml#BooleanList">
      <owl:equivalentClass rdf:resource="http://www.opengis.net/gml#booleanOrNullList"/>
   </rdfs:Datatype>
   <owl:Class rdf:about="http://www.opengis.net/gml#Category">
      <rdfs:subClassOf rdf:resource="http://www.opengis.net/gml#CodeType"/>
   </owl:Class>
   <owl:Class rdf:about="http://www.opengis.net/gml#CategoryList">
      <rdfs:subClassOf rdf:resource="http://www.opengis.net/gml#CodeOrNullListType"/>
   </owl:Class>
   <owl:Class rdf:about="http://www.opengis.net/gml#Quantity">
      <rdfs:subClassOf rdf:resource="http://www.opengis.net/gml#MeasureType"/>
   </owl:Class>
   <owl:Class rdf:about="http://www.opengis.net/gml#QuantityList">
      <rdfs:subClassOf rdf:resource="http://www.opengis.net/gml#MeasureOrNullListType"/>
   </owl:Class>
   <rdfs:Datatype rdf:about="http://www.opengis.net/gml#Count">
      <owl:equivalentClass rdf:resource="http://www.w3.org/2001/XMLSchema#integer"/>
   </rdfs:Datatype>
   <rdfs:Datatype rdf:about="http://www.opengis.net/gml#CountList">
      <owl:equivalentClass rdf:resource="http://www.opengis.net/gml#integerOrNullList"/>
   </rdfs:Datatype>
   <owl:Class rdf:about="http://www.opengis.net/gml#CompositeValue">
      <rdfs:subClassOf rdf:resource="http://www.opengis.net/gml#CompositeValueType"/>
   </owl:Class>
   <owl:Class rdf:about="http://www.opengis.net/gml#ValueArray">
      <rdfs:subClassOf rdf:resource="http://www.opengis.net/gml#CompositeValue"/>
      <rdfs:subClassOf rdf:resource="http://www.opengis.net/gml#ValueArrayType"/>
   </owl:Class>
   <owl:Class rdf:about="http://www.opengis.net/gml#QuantityExtent">
      <rdfs:subClassOf rdf:resource="http://www.opengis.net/gml#QuantityExtentType"/>
   </owl:Class>
   <owl:Class rdf:about="http://www.opengis.net/gml#CategoryExtent">
      <rdfs:subClassOf rdf:resource="http://www.opengis.net/gml#CategoryExtentType"/>
   </owl:Class>
   <rdfs:Datatype rdf:about="http://www.opengis.net/gml#CountExtent">
      <owl:equivalentClass rdf:resource="http://www.opengis.net/gml#CountExtentType"/>
   </rdfs:Datatype>
   <owl:Class rdf:about="http://www.opengis.net/gml#valueProperty">
      <rdfs:subClassOf rdf:resource="http://www.opengis.net/gml#ValuePropertyType"/>
   </owl:Class>
   <owl:Class rdf:about="http://www.opengis.net/gml#valueComponent">
      <rdfs:subClassOf rdf:resource="http://www.opengis.net/gml#ValuePropertyType"/>
   </owl:Class>
   <owl:Class rdf:about="http://www.opengis.net/gml#valueComponents">
      <rdfs:subClassOf rdf:resource="http://www.opengis.net/gml#ValueArrayPropertyType"/>
   </owl:Class>
   <owl:Class rdf:about="http://www.opengis.net/gml#_ImplicitGeometry">
      <rdfs:subClassOf rdf:resource="http://www.opengis.net/gml#_Geometry"/>
      <rdfs:subClassOf rdf:resource="http://www.opengis.net/gml#AbstractGeometryType"/>
   </owl:Class>
   <owl:Class rdf:about="http://www.opengis.net/gml#Grid">
      <rdfs:subClassOf rdf:resource="http://www.opengis.net/gml#_ImplicitGeometry"/>
      <rdfs:subClassOf rdf:resource="http://www.opengis.net/gml#GridType"/>
   </owl:Class>
   <owl:Class rdf:about="http://www.opengis.net/gml#RectifiedGrid">
      <rdfs:subClassOf rdf:resource="http://www.opengis.net/gml#_ImplicitGeometry"/>
      <rdfs:subClassOf rdf:resource="http://www.opengis.net/gml#RectifiedGridType"/>
   </owl:Class>
   <owl:Class rdf:about="http://www.opengis.net/gml#_CoordinateReferenceSystem">
      <rdfs:subClassOf rdf:resource="http://www.opengis.net/gml#_CRS"/>
      <rdfs:subClassOf rdf:resource="http://www.opengis.net/gml#AbstractReferenceSystemType"/>
   </owl:Class>
   <owl:Class rdf:about="http://www.opengis.net/gml#coordinateReferenceSystemRef">
      <rdfs:subClassOf rdf:resource="http://www.opengis.net/gml#CoordinateReferenceSystemRefType"/>
   </owl:Class>
   <owl:Class rdf:about="http://www.opengis.net/gml#CompoundCRS">
      <rdfs:subClassOf rdf:resource="http://www.opengis.net/gml#_CRS"/>
      <rdfs:subClassOf rdf:resource="http://www.opengis.net/gml#CompoundCRSType"/>
   </owl:Class>
   <owl:Class rdf:about="http://www.opengis.net/gml#includesCRS">
      <rdfs:subClassOf rdf:resource="http://www.opengis.net/gml#CoordinateReferenceSystemRefType"/>
   </owl:Class>
   <owl:Class rdf:about="http://www.opengis.net/gml#compoundCRSRef">
      <rdfs:subClassOf rdf:resource="http://www.opengis.net/gml#CompoundCRSRefType"/>
   </owl:Class>
   <owl:Class rdf:about="http://www.opengis.net/gml#GeographicCRS">
      <rdfs:subClassOf rdf:resource="http://www.opengis.net/gml#_CoordinateReferenceSystem"/>
      <rdfs:subClassOf rdf:resource="http://www.opengis.net/gml#GeographicCRSType"/>
   </owl:Class>
   <owl:Class rdf:about="http://www.opengis.net/gml#usesEllipsoidalCS">
      <rdfs:subClassOf rdf:resource="http://www.opengis.net/gml#EllipsoidalCSRefType"/>
   </owl:Class>
   <owl:Class rdf:about="http://www.opengis.net/gml#usesGeodeticDatum">
      <rdfs:subClassOf rdf:resource="http://www.opengis.net/gml#GeodeticDatumRefType"/>
   </owl:Class>
   <owl:Class rdf:about="http://www.opengis.net/gml#geographicCRSRef">
      <rdfs:subClassOf rdf:resource="http://www.opengis.net/gml#GeographicCRSRefType"/>
   </owl:Class>
   <owl:Class rdf:about="http://www.opengis.net/gml#VerticalCRS">
      <rdfs:subClassOf rdf:resource="http://www.opengis.net/gml#_CoordinateReferenceSystem"/>
      <rdfs:subClassOf rdf:resource="http://www.opengis.net/gml#VerticalCRSType"/>
   </owl:Class>
   <owl:Class rdf:about="http://www.opengis.net/gml#usesVerticalCS">
      <rdfs:subClassOf rdf:resource="http://www.opengis.net/gml#VerticalCSRefType"/>
   </owl:Class>
   <owl:Class rdf:about="http://www.opengis.net/gml#usesVerticalDatum">
      <rdfs:subClassOf rdf:resource="http://www.opengis.net/gml#VerticalDatumRefType"/>
   </owl:Class>
   <owl:Class rdf:about="http://www.opengis.net/gml#verticalCRSRef">
      <rdfs:subClassOf rdf:resource="http://www.opengis.net/gml#VerticalCRSRefType"/>
   </owl:Class>
   <owl:Class rdf:about="http://www.opengis.net/gml#GeocentricCRS">
      <rdfs:subClassOf rdf:resource="http://www.opengis.net/gml#_CoordinateReferenceSystem"/>
      <rdfs:subClassOf rdf:resource="http://www.opengis.net/gml#GeocentricCRSType"/>
   </owl:Class>
   <owl:Class rdf:about="http://www.opengis.net/gml#usesCartesianCS">
      <rdfs:subClassOf rdf:resource="http://www.opengis.net/gml#CartesianCSRefType"/>
   </owl:Class>
   <owl:Class rdf:about="http://www.opengis.net/gml#usesSphericalCS">
      <rdfs:subClassOf rdf:resource="http://www.opengis.net/gml#SphericalCSRefType"/>
   </owl:Class>
   <owl:Class rdf:about="http://www.opengis.net/gml#geocentricCRSRef">
      <rdfs:subClassOf rdf:resource="http://www.opengis.net/gml#GeocentricCRSRefType"/>
   </owl:Class>
   <owl:Class rdf:about="http://www.opengis.net/gml#_GeneralDerivedCRS">
      <rdfs:subClassOf rdf:resource="http://www.opengis.net/gml#_CoordinateReferenceSystem"/>
      <rdfs:subClassOf rdf:resource="http://www.opengis.net/gml#AbstractGeneralDerivedCRSType"/>
   </owl:Class>
   <owl:Class rdf:about="http://www.opengis.net/gml#baseCRS">
      <rdfs:subClassOf rdf:resource="http://www.opengis.net/gml#CoordinateReferenceSystemRefType"/>
   </owl:Class>
   <owl:Class rdf:about="http://www.opengis.net/gml#definedByConversion">
      <rdfs:subClassOf rdf:resource="http://www.opengis.net/gml#GeneralConversionRefType"/>
   </owl:Class>
   <owl:Class rdf:about="http://www.opengis.net/gml#ProjectedCRS">
      <rdfs:subClassOf rdf:resource="http://www.opengis.net/gml#_GeneralDerivedCRS"/>
      <rdfs:subClassOf rdf:resource="http://www.opengis.net/gml#ProjectedCRSType"/>
   </owl:Class>
   <owl:Class rdf:about="http://www.opengis.net/gml#projectedCRSRef">
      <rdfs:subClassOf rdf:resource="http://www.opengis.net/gml#ProjectedCRSRefType"/>
   </owl:Class>
   <owl:Class rdf:about="http://www.opengis.net/gml#DerivedCRS">
      <rdfs:subClassOf rdf:resource="http://www.opengis.net/gml#_GeneralDerivedCRS"/>
      <rdfs:subClassOf rdf:resource="http://www.opengis.net/gml#DerivedCRSType"/>
   </owl:Class>
   <owl:Class rdf:about="http://www.opengis.net/gml#derivedCRSType">
      <rdfs:subClassOf rdf:resource="http://www.opengis.net/gml#DerivedCRSTypeType"/>
   </owl:Class>
   <owl:Class rdf:about="http://www.opengis.net/gml#usesCS">
      <rdfs:subClassOf rdf:resource="http://www.opengis.net/gml#CoordinateSystemRefType"/>
   </owl:Class>
   <owl:Class rdf:about="http://www.opengis.net/gml#derivedCRSRef">
      <rdfs:subClassOf rdf:resource="http://www.opengis.net/gml#DerivedCRSRefType"/>
   </owl:Class>
   <owl:Class rdf:about="http://www.opengis.net/gml#EngineeringCRS">
      <rdfs:subClassOf rdf:resource="http://www.opengis.net/gml#_CoordinateReferenceSystem"/>
      <rdfs:subClassOf rdf:resource="http://www.opengis.net/gml#EngineeringCRSType"/>
   </owl:Class>
   <owl:Class rdf:about="http://www.opengis.net/gml#usesEngineeringDatum">
      <rdfs:subClassOf rdf:resource="http://www.opengis.net/gml#EngineeringDatumRefType"/>
   </owl:Class>
   <owl:Class rdf:about="http://www.opengis.net/gml#engineeringCRSRef">
      <rdfs:subClassOf rdf:resource="http://www.opengis.net/gml#EngineeringCRSRefType"/>
   </owl:Class>
   <owl:Class rdf:about="http://www.opengis.net/gml#ImageCRS">
      <rdfs:subClassOf rdf:resource="http://www.opengis.net/gml#_CoordinateReferenceSystem"/>
      <rdfs:subClassOf rdf:resource="http://www.opengis.net/gml#ImageCRSType"/>
   </owl:Class>
   <owl:Class rdf:about="http://www.opengis.net/gml#usesObliqueCartesianCS">
      <rdfs:subClassOf rdf:resource="http://www.opengis.net/gml#ObliqueCartesianCSRefType"/>
   </owl:Class>
   <owl:Class rdf:about="http://www.opengis.net/gml#usesImageDatum">
      <rdfs:subClassOf rdf:resource="http://www.opengis.net/gml#ImageDatumRefType"/>
   </owl:Class>
   <owl:Class rdf:about="http://www.opengis.net/gml#imageCRSRef">
      <rdfs:subClassOf rdf:resource="http://www.opengis.net/gml#ImageCRSRefType"/>
   </owl:Class>
   <owl:Class rdf:about="http://www.opengis.net/gml#TemporalCRS">
      <rdfs:subClassOf rdf:resource="http://www.opengis.net/gml#_CoordinateReferenceSystem"/>
      <rdfs:subClassOf rdf:resource="http://www.opengis.net/gml#TemporalCRSType"/>
   </owl:Class>
   <owl:Class rdf:about="http://www.opengis.net/gml#usesTemporalCS">
      <rdfs:subClassOf rdf:resource="http://www.opengis.net/gml#TemporalCSRefType"/>
   </owl:Class>
   <owl:Class rdf:about="http://www.opengis.net/gml#usesTemporalDatum">
      <rdfs:subClassOf rdf:resource="http://www.opengis.net/gml#TemporalDatumRefType"/>
   </owl:Class>
   <owl:Class rdf:about="http://www.opengis.net/gml#temporalCRSRef">
      <rdfs:subClassOf rdf:resource="http://www.opengis.net/gml#TemporalCRSRefType"/>
   </owl:Class>
   <owl:Class rdf:about="http://www.opengis.net/gml#CoordinateSystemAxis">
      <rdfs:subClassOf rdf:resource="http://www.opengis.net/gml#Definition"/>
      <rdfs:subClassOf rdf:resource="http://www.opengis.net/gml#CoordinateSystemAxisType"/>
   </owl:Class>
   <owl:Class rdf:about="http://www.opengis.net/gml#axisID">
      <rdfs:subClassOf rdf:resource="http://www.opengis.net/gml#IdentifierType"/>
   </owl:Class>
   <owl:Class rdf:about="http://www.opengis.net/gml#axisAbbrev">
      <rdfs:subClassOf rdf:resource="http://www.opengis.net/gml#CodeType"/>
   </owl:Class>
   <owl:Class rdf:about="http://www.opengis.net/gml#axisDirection">
      <rdfs:subClassOf rdf:resource="http://www.opengis.net/gml#CodeType"/>
   </owl:Class>
   <owl:Class rdf:about="http://www.opengis.net/gml#coordinateSystemAxisRef">
      <rdfs:subClassOf rdf:resource="http://www.opengis.net/gml#CoordinateSystemAxisRefType"/>
   </owl:Class>
   <owl:Class rdf:about="http://www.opengis.net/gml#_CoordinateSystem">
      <rdfs:subClassOf rdf:resource="http://www.opengis.net/gml#Definition"/>
      <rdfs:subClassOf rdf:resource="http://www.opengis.net/gml#AbstractCoordinateSystemType"/>
   </owl:Class>
   <owl:Class rdf:about="http://www.opengis.net/gml#csName">
      <rdfs:subClassOf rdf:resource="http://www.opengis.net/gml#name"/>
      <rdfs:subClassOf rdf:resource="http://www.opengis.net/gml#CodeType"/>
   </owl:Class>
   <owl:Class rdf:about="http://www.opengis.net/gml#csID">
      <rdfs:subClassOf rdf:resource="http://www.opengis.net/gml#IdentifierType"/>
   </owl:Class>
   <owl:Class rdf:about="http://www.opengis.net/gml#usesAxis">
      <rdfs:subClassOf rdf:resource="http://www.opengis.net/gml#CoordinateSystemAxisRefType"/>
   </owl:Class>
   <owl:Class rdf:about="http://www.opengis.net/gml#coordinateSystemRef">
      <rdfs:subClassOf rdf:resource="http://www.opengis.net/gml#CoordinateSystemRefType"/>
   </owl:Class>
   <owl:Class rdf:about="http://www.opengis.net/gml#EllipsoidalCS">
      <rdfs:subClassOf rdf:resource="http://www.opengis.net/gml#_CoordinateSystem"/>
      <rdfs:subClassOf rdf:resource="http://www.opengis.net/gml#EllipsoidalCSType"/>
   </owl:Class>
   <owl:Class rdf:about="http://www.opengis.net/gml#ellipsoidalCSRef">
      <rdfs:subClassOf rdf:resource="http://www.opengis.net/gml#EllipsoidalCSRefType"/>
   </owl:Class>
   <owl:Class rdf:about="http://www.opengis.net/gml#CartesianCS">
      <rdfs:subClassOf rdf:resource="http://www.opengis.net/gml#_CoordinateSystem"/>
      <rdfs:subClassOf rdf:resource="http://www.opengis.net/gml#CartesianCSType"/>
   </owl:Class>
   <owl:Class rdf:about="http://www.opengis.net/gml#cartesianCSRef">
      <rdfs:subClassOf rdf:resource="http://www.opengis.net/gml#CartesianCSRefType"/>
   </owl:Class>
   <owl:Class rdf:about="http://www.opengis.net/gml#VerticalCS">
      <rdfs:subClassOf rdf:resource="http://www.opengis.net/gml#_CoordinateSystem"/>
      <rdfs:subClassOf rdf:resource="http://www.opengis.net/gml#VerticalCSType"/>
   </owl:Class>
   <owl:Class rdf:about="http://www.opengis.net/gml#verticalCSRef">
      <rdfs:subClassOf rdf:resource="http://www.opengis.net/gml#VerticalCSRefType"/>
   </owl:Class>
   <owl:Class rdf:about="http://www.opengis.net/gml#TemporalCS">
      <rdfs:subClassOf rdf:resource="http://www.opengis.net/gml#_CoordinateSystem"/>
      <rdfs:subClassOf rdf:resource="http://www.opengis.net/gml#TemporalCSType"/>
   </owl:Class>
   <owl:Class rdf:about="http://www.opengis.net/gml#temporalCSRef">
      <rdfs:subClassOf rdf:resource="http://www.opengis.net/gml#TemporalCSRefType"/>
   </owl:Class>
   <owl:Class rdf:about="http://www.opengis.net/gml#LinearCS">
      <rdfs:subClassOf rdf:resource="http://www.opengis.net/gml#_CoordinateSystem"/>
      <rdfs:subClassOf rdf:resource="http://www.opengis.net/gml#LinearCSType"/>
   </owl:Class>
   <owl:Class rdf:about="http://www.opengis.net/gml#linearCSRef">
      <rdfs:subClassOf rdf:resource="http://www.opengis.net/gml#LinearCSRefType"/>
   </owl:Class>
   <owl:Class rdf:about="http://www.opengis.net/gml#UserDefinedCS">
      <rdfs:subClassOf rdf:resource="http://www.opengis.net/gml#_CoordinateSystem"/>
      <rdfs:subClassOf rdf:resource="http://www.opengis.net/gml#UserDefinedCSType"/>
   </owl:Class>
   <owl:Class rdf:about="http://www.opengis.net/gml#userDefinedCSRef">
      <rdfs:subClassOf rdf:resource="http://www.opengis.net/gml#UserDefinedCSRefType"/>
   </owl:Class>
   <owl:Class rdf:about="http://www.opengis.net/gml#SphericalCS">
      <rdfs:subClassOf rdf:resource="http://www.opengis.net/gml#_CoordinateSystem"/>
      <rdfs:subClassOf rdf:resource="http://www.opengis.net/gml#SphericalCSType"/>
   </owl:Class>
   <owl:Class rdf:about="http://www.opengis.net/gml#sphericalCSRef">
      <rdfs:subClassOf rdf:resource="http://www.opengis.net/gml#SphericalCSRefType"/>
   </owl:Class>
   <owl:Class rdf:about="http://www.opengis.net/gml#PolarCS">
      <rdfs:subClassOf rdf:resource="http://www.opengis.net/gml#_CoordinateSystem"/>
      <rdfs:subClassOf rdf:resource="http://www.opengis.net/gml#PolarCSType"/>
   </owl:Class>
   <owl:Class rdf:about="http://www.opengis.net/gml#polarCSRef">
      <rdfs:subClassOf rdf:resource="http://www.opengis.net/gml#PolarCSRefType"/>
   </owl:Class>
   <owl:Class rdf:about="http://www.opengis.net/gml#CylindricalCS">
      <rdfs:subClassOf rdf:resource="http://www.opengis.net/gml#_CoordinateSystem"/>
      <rdfs:subClassOf rdf:resource="http://www.opengis.net/gml#CylindricalCSType"/>
   </owl:Class>
   <owl:Class rdf:about="http://www.opengis.net/gml#cylindricalCSRef">
      <rdfs:subClassOf rdf:resource="http://www.opengis.net/gml#CylindricalCSRefType"/>
   </owl:Class>
   <owl:Class rdf:about="http://www.opengis.net/gml#ObliqueCartesianCS">
      <rdfs:subClassOf rdf:resource="http://www.opengis.net/gml#_CoordinateSystem"/>
      <rdfs:subClassOf rdf:resource="http://www.opengis.net/gml#ObliqueCartesianCSType"/>
   </owl:Class>
   <owl:Class rdf:about="http://www.opengis.net/gml#obliqueCartesianCSRef">
      <rdfs:subClassOf rdf:resource="http://www.opengis.net/gml#ObliqueCartesianCSRefType"/>
   </owl:Class>
   <owl:Class rdf:about="http://www.opengis.net/gml#_ReferenceSystem">
      <rdfs:subClassOf rdf:resource="http://www.opengis.net/gml#Definition"/>
      <rdfs:subClassOf rdf:resource="http://www.opengis.net/gml#AbstractReferenceSystemType"/>
   </owl:Class>
   <owl:Class rdf:about="http://www.opengis.net/gml#srsName">
      <rdfs:subClassOf rdf:resource="http://www.opengis.net/gml#name"/>
      <rdfs:subClassOf rdf:resource="http://www.opengis.net/gml#CodeType"/>
   </owl:Class>
   <owl:Class rdf:about="http://www.opengis.net/gml#srsID">
      <rdfs:subClassOf rdf:resource="http://www.opengis.net/gml#IdentifierType"/>
   </owl:Class>
   <owl:Class rdf:about="http://www.opengis.net/gml#referenceSystemRef">
      <rdfs:subClassOf rdf:resource="http://www.opengis.net/gml#ReferenceSystemRefType"/>
   </owl:Class>
   <owl:Class rdf:about="http://www.opengis.net/gml#_CRS">
      <rdfs:subClassOf rdf:resource="http://www.opengis.net/gml#_ReferenceSystem"/>
      <rdfs:subClassOf rdf:resource="http://www.opengis.net/gml#AbstractReferenceSystemType"/>
   </owl:Class>
   <owl:Class rdf:about="http://www.opengis.net/gml#crsRef">
      <rdfs:subClassOf rdf:resource="http://www.opengis.net/gml#CRSRefType"/>
   </owl:Class>
   <rdfs:Datatype rdf:about="http://www.opengis.net/gml#version">
      <owl:equivalentClass rdf:resource="http://www.w3.org/2001/XMLSchema#string"/>
   </rdfs:Datatype>
   <owl:Class rdf:about="http://www.opengis.net/gml#remarks">
      <rdfs:subClassOf rdf:resource="http://www.opengis.net/gml#StringOrRefType"/>
   </owl:Class>
   <rdfs:Datatype rdf:about="http://www.opengis.net/gml#scope">
      <owl:equivalentClass rdf:resource="http://www.w3.org/2001/XMLSchema#string"/>
   </rdfs:Datatype>
   <owl:Class rdf:about="http://www.opengis.net/gml#validArea">
      <rdfs:subClassOf rdf:resource="http://www.opengis.net/gml#ExtentType"/>
   </owl:Class>
   <owl:Class rdf:about="http://www.opengis.net/gml#boundingBox">
      <rdfs:subClassOf rdf:resource="http://www.opengis.net/gml#EnvelopeType"/>
   </owl:Class>
   <owl:Class rdf:about="http://www.opengis.net/gml#boundingPolygon">
      <rdfs:subClassOf rdf:resource="http://www.opengis.net/gml#PolygonType"/>
   </owl:Class>
   <owl:Class rdf:about="http://www.opengis.net/gml#verticalExtent">
      <rdfs:subClassOf rdf:resource="http://www.opengis.net/gml#EnvelopeType"/>
   </owl:Class>
   <owl:Class rdf:about="http://www.opengis.net/gml#temporalExtent">
      <rdfs:subClassOf rdf:resource="http://www.opengis.net/gml#TimePeriodType"/>
   </owl:Class>
   <owl:Class rdf:about="http://www.opengis.net/gml#_Datum">
      <rdfs:subClassOf rdf:resource="http://www.opengis.net/gml#Definition"/>
      <rdfs:subClassOf rdf:resource="http://www.opengis.net/gml#AbstractDatumType"/>
   </owl:Class>
   <owl:Class rdf:about="http://www.opengis.net/gml#datumName">
      <rdfs:subClassOf rdf:resource="http://www.opengis.net/gml#name"/>
      <rdfs:subClassOf rdf:resource="http://www.opengis.net/gml#CodeType"/>
   </owl:Class>
   <owl:Class rdf:about="http://www.opengis.net/gml#datumID">
      <rdfs:subClassOf rdf:resource="http://www.opengis.net/gml#IdentifierType"/>
   </owl:Class>
   <owl:Class rdf:about="http://www.opengis.net/gml#anchorPoint">
      <rdfs:subClassOf rdf:resource="http://www.opengis.net/gml#CodeType"/>
   </owl:Class>
   <rdfs:Datatype rdf:about="http://www.opengis.net/gml#realizationEpoch">
      <owl:equivalentClass rdf:resource="http://www.w3.org/2001/XMLSchema#date"/>
   </rdfs:Datatype>
   <owl:Class rdf:about="http://www.opengis.net/gml#datumRef">
      <rdfs:subClassOf rdf:resource="http://www.opengis.net/gml#DatumRefType"/>
   </owl:Class>
   <owl:Class rdf:about="http://www.opengis.net/gml#EngineeringDatum">
      <rdfs:subClassOf rdf:resource="http://www.opengis.net/gml#_Datum"/>
      <rdfs:subClassOf rdf:resource="http://www.opengis.net/gml#EngineeringDatumType"/>
   </owl:Class>
   <owl:Class rdf:about="http://www.opengis.net/gml#engineeringDatumRef">
      <rdfs:subClassOf rdf:resource="http://www.opengis.net/gml#EngineeringDatumRefType"/>
   </owl:Class>
   <owl:Class rdf:about="http://www.opengis.net/gml#ImageDatum">
      <rdfs:subClassOf rdf:resource="http://www.opengis.net/gml#_Datum"/>
      <rdfs:subClassOf rdf:resource="http://www.opengis.net/gml#ImageDatumType"/>
   </owl:Class>
   <owl:Class rdf:about="http://www.opengis.net/gml#pixelInCell">
      <rdfs:subClassOf rdf:resource="http://www.opengis.net/gml#PixelInCellType"/>
   </owl:Class>
   <owl:Class rdf:about="http://www.opengis.net/gml#imageDatumRef">
      <rdfs:subClassOf rdf:resource="http://www.opengis.net/gml#ImageDatumRefType"/>
   </owl:Class>
   <owl:Class rdf:about="http://www.opengis.net/gml#VerticalDatum">
      <rdfs:subClassOf rdf:resource="http://www.opengis.net/gml#_Datum"/>
      <rdfs:subClassOf rdf:resource="http://www.opengis.net/gml#VerticalDatumType"/>
   </owl:Class>
   <owl:Class rdf:about="http://www.opengis.net/gml#verticalDatumType">
      <rdfs:subClassOf rdf:resource="http://www.opengis.net/gml#VerticalDatumTypeType"/>
   </owl:Class>
   <owl:Class rdf:about="http://www.opengis.net/gml#verticalDatumRef">
      <rdfs:subClassOf rdf:resource="http://www.opengis.net/gml#VerticalDatumRefType"/>
   </owl:Class>
   <owl:Class rdf:about="http://www.opengis.net/gml#TemporalDatum">
      <rdfs:subClassOf rdf:resource="http://www.opengis.net/gml#_Datum"/>
      <rdfs:subClassOf rdf:resource="http://www.opengis.net/gml#TemporalDatumType"/>
   </owl:Class>
   <rdfs:Datatype rdf:about="http://www.opengis.net/gml#origin">
      <owl:equivalentClass rdf:resource="http://www.w3.org/2001/XMLSchema#dateTime"/>
   </rdfs:Datatype>
   <owl:Class rdf:about="http://www.opengis.net/gml#temporalDatumRef">
      <rdfs:subClassOf rdf:resource="http://www.opengis.net/gml#TemporalDatumRefType"/>
   </owl:Class>
   <owl:Class rdf:about="http://www.opengis.net/gml#GeodeticDatum">
      <rdfs:subClassOf rdf:resource="http://www.opengis.net/gml#_Datum"/>
      <rdfs:subClassOf rdf:resource="http://www.opengis.net/gml#GeodeticDatumType"/>
   </owl:Class>
   <owl:Class rdf:about="http://www.opengis.net/gml#usesPrimeMeridian">
      <rdfs:subClassOf rdf:resource="http://www.opengis.net/gml#PrimeMeridianRefType"/>
   </owl:Class>
   <owl:Class rdf:about="http://www.opengis.net/gml#usesEllipsoid">
      <rdfs:subClassOf rdf:resource="http://www.opengis.net/gml#EllipsoidRefType"/>
   </owl:Class>
   <owl:Class rdf:about="http://www.opengis.net/gml#geodeticDatumRef">
      <rdfs:subClassOf rdf:resource="http://www.opengis.net/gml#GeodeticDatumRefType"/>
   </owl:Class>
   <owl:Class rdf:about="http://www.opengis.net/gml#PrimeMeridian">
      <rdfs:subClassOf rdf:resource="http://www.opengis.net/gml#Definition"/>
      <rdfs:subClassOf rdf:resource="http://www.opengis.net/gml#PrimeMeridianType"/>
   </owl:Class>
   <owl:Class rdf:about="http://www.opengis.net/gml#meridianName">
      <rdfs:subClassOf rdf:resource="http://www.opengis.net/gml#name"/>
      <rdfs:subClassOf rdf:resource="http://www.opengis.net/gml#CodeType"/>
   </owl:Class>
   <owl:Class rdf:about="http://www.opengis.net/gml#meridianID">
      <rdfs:subClassOf rdf:resource="http://www.opengis.net/gml#IdentifierType"/>
   </owl:Class>
   <owl:Class rdf:about="http://www.opengis.net/gml#greenwichLongitude">
      <rdfs:subClassOf rdf:resource="http://www.opengis.net/gml#AngleChoiceType"/>
   </owl:Class>
   <owl:Class rdf:about="http://www.opengis.net/gml#primeMeridianRef">
      <rdfs:subClassOf rdf:resource="http://www.opengis.net/gml#PrimeMeridianRefType"/>
   </owl:Class>
   <owl:Class rdf:about="http://www.opengis.net/gml#Ellipsoid">
      <rdfs:subClassOf rdf:resource="http://www.opengis.net/gml#Definition"/>
      <rdfs:subClassOf rdf:resource="http://www.opengis.net/gml#EllipsoidType"/>
   </owl:Class>
   <owl:Class rdf:about="http://www.opengis.net/gml#ellipsoidName">
      <rdfs:subClassOf rdf:resource="http://www.opengis.net/gml#name"/>
      <rdfs:subClassOf rdf:resource="http://www.opengis.net/gml#CodeType"/>
   </owl:Class>
   <owl:Class rdf:about="http://www.opengis.net/gml#ellipsoidID">
      <rdfs:subClassOf rdf:resource="http://www.opengis.net/gml#IdentifierType"/>
   </owl:Class>
   <owl:Class rdf:about="http://www.opengis.net/gml#semiMajorAxis">
      <rdfs:subClassOf rdf:resource="http://www.opengis.net/gml#MeasureType"/>
   </owl:Class>
   <owl:Class rdf:about="http://www.opengis.net/gml#ellipsoidRef">
      <rdfs:subClassOf rdf:resource="http://www.opengis.net/gml#EllipsoidRefType"/>
   </owl:Class>
   <owl:Class rdf:about="http://www.opengis.net/gml#secondDefiningParameter">
      <rdfs:subClassOf rdf:resource="http://www.opengis.net/gml#SecondDefiningParameterType"/>
   </owl:Class>
   <owl:Class rdf:about="http://www.opengis.net/gml#inverseFlattening">
      <rdfs:subClassOf rdf:resource="http://www.opengis.net/gml#MeasureType"/>
   </owl:Class>
   <owl:Class rdf:about="http://www.opengis.net/gml#semiMinorAxis">
      <rdfs:subClassOf rdf:resource="http://www.opengis.net/gml#MeasureType"/>
   </owl:Class>
   <owl:Class rdf:about="http://www.opengis.net/gml#_CoordinateOperation">
      <rdfs:subClassOf rdf:resource="http://www.opengis.net/gml#Definition"/>
      <rdfs:subClassOf rdf:resource="http://www.opengis.net/gml#AbstractCoordinateOperationType"/>
   </owl:Class>
   <owl:Class rdf:about="http://www.opengis.net/gml#coordinateOperationName">
      <rdfs:subClassOf rdf:resource="http://www.opengis.net/gml#name"/>
      <rdfs:subClassOf rdf:resource="http://www.opengis.net/gml#CodeType"/>
   </owl:Class>
   <owl:Class rdf:about="http://www.opengis.net/gml#coordinateOperationID">
      <rdfs:subClassOf rdf:resource="http://www.opengis.net/gml#IdentifierType"/>
   </owl:Class>
   <rdfs:Datatype rdf:about="http://www.opengis.net/gml#operationVersion">
      <owl:equivalentClass rdf:resource="http://www.w3.org/2001/XMLSchema#string"/>
   </rdfs:Datatype>
   <owl:Class rdf:about="http://www.opengis.net/gml#sourceCRS">
      <rdfs:subClassOf rdf:resource="http://www.opengis.net/gml#CRSRefType"/>
   </owl:Class>
   <owl:Class rdf:about="http://www.opengis.net/gml#targetCRS">
      <rdfs:subClassOf rdf:resource="http://www.opengis.net/gml#CRSRefType"/>
   </owl:Class>
   <owl:Class rdf:about="http://www.opengis.net/gml#coordinateOperationRef">
      <rdfs:subClassOf rdf:resource="http://www.opengis.net/gml#CoordinateOperationRefType"/>
   </owl:Class>
   <owl:Class rdf:about="http://www.opengis.net/gml#ConcatenatedOperation">
      <rdfs:subClassOf rdf:resource="http://www.opengis.net/gml#_CoordinateOperation"/>
      <rdfs:subClassOf rdf:resource="http://www.opengis.net/gml#ConcatenatedOperationType"/>
   </owl:Class>
   <owl:Class rdf:about="http://www.opengis.net/gml#usesSingleOperation">
      <rdfs:subClassOf rdf:resource="http://www.opengis.net/gml#SingleOperationRefType"/>
   </owl:Class>
   <owl:Class rdf:about="http://www.opengis.net/gml#concatenatedOperationRef">
      <rdfs:subClassOf rdf:resource="http://www.opengis.net/gml#ConcatenatedOperationRefType"/>
   </owl:Class>
   <owl:Class rdf:about="http://www.opengis.net/gml#_SingleOperation">
      <rdfs:subClassOf rdf:resource="http://www.opengis.net/gml#_CoordinateOperation"/>
      <rdfs:subClassOf rdf:resource="http://www.opengis.net/gml#AbstractCoordinateOperationType"/>
   </owl:Class>
   <owl:Class rdf:about="http://www.opengis.net/gml#singleOperationRef">
      <rdfs:subClassOf rdf:resource="http://www.opengis.net/gml#SingleOperationRefType"/>
   </owl:Class>
   <owl:Class rdf:about="http://www.opengis.net/gml#PassThroughOperation">
      <rdfs:subClassOf rdf:resource="http://www.opengis.net/gml#_SingleOperation"/>
      <rdfs:subClassOf rdf:resource="http://www.opengis.net/gml#PassThroughOperationType"/>
   </owl:Class>
   <rdfs:Datatype rdf:about="http://www.opengis.net/gml#modifiedCoordinate">
      <owl:equivalentClass rdf:resource="http://www.w3.org/2001/XMLSchema#positiveInteger"/>
   </rdfs:Datatype>
   <owl:Class rdf:about="http://www.opengis.net/gml#usesOperation">
      <rdfs:subClassOf rdf:resource="http://www.opengis.net/gml#OperationRefType"/>
   </owl:Class>
   <owl:Class rdf:about="http://www.opengis.net/gml#passThroughOperationRef">
      <rdfs:subClassOf rdf:resource="http://www.opengis.net/gml#PassThroughOperationRefType"/>
   </owl:Class>
   <owl:Class rdf:about="http://www.opengis.net/gml#_Operation">
      <rdfs:subClassOf rdf:resource="http://www.opengis.net/gml#_SingleOperation"/>
      <rdfs:subClassOf rdf:resource="http://www.opengis.net/gml#AbstractCoordinateOperationType"/>
   </owl:Class>
   <owl:Class rdf:about="http://www.opengis.net/gml#operationRef">
      <rdfs:subClassOf rdf:resource="http://www.opengis.net/gml#OperationRefType"/>
   </owl:Class>
   <owl:Class rdf:about="http://www.opengis.net/gml#_GeneralConversion">
      <rdfs:subClassOf rdf:resource="http://www.opengis.net/gml#_Operation"/>
      <rdfs:subClassOf rdf:resource="http://www.opengis.net/gml#AbstractGeneralConversionType"/>
   </owl:Class>
   <owl:Class rdf:about="http://www.opengis.net/gml#generalConversionRef">
      <rdfs:subClassOf rdf:resource="http://www.opengis.net/gml#GeneralConversionRefType"/>
   </owl:Class>
   <owl:Class rdf:about="http://www.opengis.net/gml#Conversion">
      <rdfs:subClassOf rdf:resource="http://www.opengis.net/gml#_GeneralConversion"/>
      <rdfs:subClassOf rdf:resource="http://www.opengis.net/gml#ConversionType"/>
   </owl:Class>
   <owl:Class rdf:about="http://www.opengis.net/gml#usesMethod">
      <rdfs:subClassOf rdf:resource="http://www.opengis.net/gml#OperationMethodRefType"/>
   </owl:Class>
   <owl:Class rdf:about="http://www.opengis.net/gml#usesValue">
      <rdfs:subClassOf rdf:resource="http://www.opengis.net/gml#ParameterValueType"/>
   </owl:Class>
   <owl:Class rdf:about="http://www.opengis.net/gml#conversionRef">
      <rdfs:subClassOf rdf:resource="http://www.opengis.net/gml#ConversionRefType"/>
   </owl:Class>
   <owl:Class rdf:about="http://www.opengis.net/gml#_GeneralTransformation">
      <rdfs:subClassOf rdf:resource="http://www.opengis.net/gml#_Operation"/>
      <rdfs:subClassOf rdf:resource="http://www.opengis.net/gml#AbstractGeneralTransformationType"/>
   </owl:Class>
   <owl:Class rdf:about="http://www.opengis.net/gml#generalTransformationRef">
      <rdfs:subClassOf rdf:resource="http://www.opengis.net/gml#GeneralTransformationRefType"/>
   </owl:Class>
   <owl:Class rdf:about="http://www.opengis.net/gml#Transformation">
      <rdfs:subClassOf rdf:resource="http://www.opengis.net/gml#_GeneralTransformation"/>
      <rdfs:subClassOf rdf:resource="http://www.opengis.net/gml#TransformationType"/>
   </owl:Class>
   <owl:Class rdf:about="http://www.opengis.net/gml#transformationRef">
      <rdfs:subClassOf rdf:resource="http://www.opengis.net/gml#TransformationRefType"/>
   </owl:Class>
   <owl:Class rdf:about="http://www.opengis.net/gml#_generalParameterValue">
      <rdfs:subClassOf rdf:resource="http://www.opengis.net/gml#AbstractGeneralParameterValueType"/>
   </owl:Class>
   <owl:Class rdf:about="http://www.opengis.net/gml#parameterValue">
      <rdfs:subClassOf rdf:resource="http://www.opengis.net/gml#_generalParameterValue"/>
      <rdfs:subClassOf rdf:resource="http://www.opengis.net/gml#ParameterValueType"/>
   </owl:Class>
   <owl:Class rdf:about="http://www.opengis.net/gml#value">
      <rdfs:subClassOf rdf:resource="http://www.opengis.net/gml#MeasureType"/>
   </owl:Class>
   <owl:Class rdf:about="http://www.opengis.net/gml#dmsAngleValue">
      <rdfs:subClassOf rdf:resource="http://www.opengis.net/gml#DMSAngleType"/>
   </owl:Class>
   <rdfs:Datatype rdf:about="http://www.opengis.net/gml#stringValue">
      <owl:equivalentClass rdf:resource="http://www.w3.org/2001/XMLSchema#string"/>
   </rdfs:Datatype>
   <rdfs:Datatype rdf:about="http://www.opengis.net/gml#integerValue">
      <owl:equivalentClass rdf:resource="http://www.w3.org/2001/XMLSchema#positiveInteger"/>
   </rdfs:Datatype>
   <rdfs:Datatype rdf:about="http://www.opengis.net/gml#booleanValue">
      <owl:equivalentClass rdf:resource="http://www.w3.org/2001/XMLSchema#boolean"/>
   </rdfs:Datatype>
   <owl:Class rdf:about="http://www.opengis.net/gml#valueList">
      <rdfs:subClassOf rdf:resource="http://www.opengis.net/gml#MeasureListType"/>
   </owl:Class>
   <rdfs:Datatype rdf:about="http://www.opengis.net/gml#integerValueList">
      <owl:equivalentClass rdf:resource="http://www.opengis.net/gml#integerList"/>
   </rdfs:Datatype>
   <rdfs:Datatype rdf:about="http://www.opengis.net/gml#valueFile">
      <owl:equivalentClass rdf:resource="http://www.w3.org/2001/XMLSchema#anyURI"/>
   </rdfs:Datatype>
   <owl:Class rdf:about="http://www.opengis.net/gml#valueOfParameter">
      <rdfs:subClassOf rdf:resource="http://www.opengis.net/gml#OperationParameterRefType"/>
   </owl:Class>
   <owl:Class rdf:about="http://www.opengis.net/gml#parameterValueGroup">
      <rdfs:subClassOf rdf:resource="http://www.opengis.net/gml#_generalParameterValue"/>
      <rdfs:subClassOf rdf:resource="http://www.opengis.net/gml#ParameterValueGroupType"/>
   </owl:Class>
   <owl:Class rdf:about="http://www.opengis.net/gml#includesValue">
      <rdfs:subClassOf rdf:resource="http://www.opengis.net/gml#_generalParameterValue"/>
      <rdfs:subClassOf rdf:resource="http://www.opengis.net/gml#AbstractGeneralParameterValueType"/>
   </owl:Class>
   <owl:Class rdf:about="http://www.opengis.net/gml#valuesOfGroup">
      <rdfs:subClassOf rdf:resource="http://www.opengis.net/gml#OperationParameterGroupRefType"/>
   </owl:Class>
   <owl:Class rdf:about="http://www.opengis.net/gml#OperationMethod">
      <rdfs:subClassOf rdf:resource="http://www.opengis.net/gml#Definition"/>
      <rdfs:subClassOf rdf:resource="http://www.opengis.net/gml#OperationMethodType"/>
   </owl:Class>
   <owl:Class rdf:about="http://www.opengis.net/gml#methodName">
      <rdfs:subClassOf rdf:resource="http://www.opengis.net/gml#name"/>
      <rdfs:subClassOf rdf:resource="http://www.opengis.net/gml#CodeType"/>
   </owl:Class>
   <owl:Class rdf:about="http://www.opengis.net/gml#methodID">
      <rdfs:subClassOf rdf:resource="http://www.opengis.net/gml#IdentifierType"/>
   </owl:Class>
   <owl:Class rdf:about="http://www.opengis.net/gml#methodFormula">
      <rdfs:subClassOf rdf:resource="http://www.opengis.net/gml#CodeType"/>
   </owl:Class>
   <rdfs:Datatype rdf:about="http://www.opengis.net/gml#sourceDimensions">
      <owl:equivalentClass rdf:resource="http://www.w3.org/2001/XMLSchema#positiveInteger"/>
   </rdfs:Datatype>
   <rdfs:Datatype rdf:about="http://www.opengis.net/gml#targetDimensions">
      <owl:equivalentClass rdf:resource="http://www.w3.org/2001/XMLSchema#positiveInteger"/>
   </rdfs:Datatype>
   <owl:Class rdf:about="http://www.opengis.net/gml#usesParameter">
      <rdfs:subClassOf rdf:resource="http://www.opengis.net/gml#AbstractGeneralOperationParameterRefType"/>
   </owl:Class>
   <owl:Class rdf:about="http://www.opengis.net/gml#operationMethodRef">
      <rdfs:subClassOf rdf:resource="http://www.opengis.net/gml#OperationMethodRefType"/>
   </owl:Class>
   <owl:Class rdf:about="http://www.opengis.net/gml#_GeneralOperationParameter">
      <rdfs:subClassOf rdf:resource="http://www.opengis.net/gml#Definition"/>
      <rdfs:subClassOf rdf:resource="http://www.opengis.net/gml#AbstractGeneralOperationParameterType"/>
   </owl:Class>
   <rdfs:Datatype rdf:about="http://www.opengis.net/gml#minimumOccurs">
      <owl:equivalentClass rdf:resource="http://www.w3.org/2001/XMLSchema#nonNegativeInteger"/>
   </rdfs:Datatype>
   <owl:Class rdf:about="http://www.opengis.net/gml#abstractGeneralOperationParameterRef">
      <rdfs:subClassOf rdf:resource="http://www.opengis.net/gml#AbstractGeneralOperationParameterRefType"/>
   </owl:Class>
   <owl:Class rdf:about="http://www.opengis.net/gml#OperationParameter">
      <rdfs:subClassOf rdf:resource="http://www.opengis.net/gml#_GeneralOperationParameter"/>
      <rdfs:subClassOf rdf:resource="http://www.opengis.net/gml#OperationParameterType"/>
   </owl:Class>
   <owl:Class rdf:about="http://www.opengis.net/gml#parameterName">
      <rdfs:subClassOf rdf:resource="http://www.opengis.net/gml#name"/>
      <rdfs:subClassOf rdf:resource="http://www.opengis.net/gml#CodeType"/>
   </owl:Class>
   <owl:Class rdf:about="http://www.opengis.net/gml#parameterID">
      <rdfs:subClassOf rdf:resource="http://www.opengis.net/gml#IdentifierType"/>
   </owl:Class>
   <owl:Class rdf:about="http://www.opengis.net/gml#operationParameterRef">
      <rdfs:subClassOf rdf:resource="http://www.opengis.net/gml#OperationParameterRefType"/>
   </owl:Class>
   <owl:Class rdf:about="http://www.opengis.net/gml#OperationParameterGroup">
      <rdfs:subClassOf rdf:resource="http://www.opengis.net/gml#_GeneralOperationParameter"/>
      <rdfs:subClassOf rdf:resource="http://www.opengis.net/gml#OperationParameterGroupType"/>
   </owl:Class>
   <owl:Class rdf:about="http://www.opengis.net/gml#groupName">
      <rdfs:subClassOf rdf:resource="http://www.opengis.net/gml#name"/>
      <rdfs:subClassOf rdf:resource="http://www.opengis.net/gml#CodeType"/>
   </owl:Class>
   <owl:Class rdf:about="http://www.opengis.net/gml#groupID">
      <rdfs:subClassOf rdf:resource="http://www.opengis.net/gml#IdentifierType"/>
   </owl:Class>
   <rdfs:Datatype rdf:about="http://www.opengis.net/gml#maximumOccurs">
      <owl:equivalentClass rdf:resource="http://www.w3.org/2001/XMLSchema#positiveInteger"/>
   </rdfs:Datatype>
   <owl:Class rdf:about="http://www.opengis.net/gml#includesParameter">
      <rdfs:subClassOf rdf:resource="http://www.opengis.net/gml#AbstractGeneralOperationParameterRefType"/>
   </owl:Class>
   <owl:Class rdf:about="http://www.opengis.net/gml#operationParameterGroupRef">
      <rdfs:subClassOf rdf:resource="http://www.opengis.net/gml#OperationParameterRefType"/>
   </owl:Class>
   <owl:Class rdf:about="http://www.opengis.net/gml#_positionalAccuracy">
      <rdfs:subClassOf rdf:resource="http://www.opengis.net/gml#AbstractPositionalAccuracyType"/>
   </owl:Class>
   <owl:Class rdf:about="http://www.opengis.net/gml#measureDescription">
      <rdfs:subClassOf rdf:resource="http://www.opengis.net/gml#CodeType"/>
   </owl:Class>
   <owl:Class rdf:about="http://www.opengis.net/gml#absoluteExternalPositionalAccuracy">
      <rdfs:subClassOf rdf:resource="http://www.opengis.net/gml#_positionalAccuracy"/>
      <rdfs:subClassOf rdf:resource="http://www.opengis.net/gml#AbsoluteExternalPositionalAccuracyType"/>
   </owl:Class>
   <owl:Class rdf:about="http://www.opengis.net/gml#relativeInternalPositionalAccuracy">
      <rdfs:subClassOf rdf:resource="http://www.opengis.net/gml#_positionalAccuracy"/>
      <rdfs:subClassOf rdf:resource="http://www.opengis.net/gml#RelativeInternalPositionalAccuracyType"/>
   </owl:Class>
   <owl:Class rdf:about="http://www.opengis.net/gml#result">
      <rdfs:subClassOf rdf:resource="http://www.opengis.net/gml#MeasureType"/>
   </owl:Class>
   <owl:Class rdf:about="http://www.opengis.net/gml#covarianceMatrix">
      <rdfs:subClassOf rdf:resource="http://www.opengis.net/gml#_positionalAccuracy"/>
      <rdfs:subClassOf rdf:resource="http://www.opengis.net/gml#CovarianceMatrixType"/>
   </owl:Class>
   <owl:Class rdf:about="http://www.opengis.net/gml#includesElement">
      <rdfs:subClassOf rdf:resource="http://www.opengis.net/gml#CovarianceElementType"/>
   </owl:Class>
   <rdfs:Datatype rdf:about="http://www.opengis.net/gml#rowIndex">
      <owl:equivalentClass rdf:resource="http://www.w3.org/2001/XMLSchema#positiveInteger"/>
   </rdfs:Datatype>
   <rdfs:Datatype rdf:about="http://www.opengis.net/gml#columnIndex">
      <owl:equivalentClass rdf:resource="http://www.w3.org/2001/XMLSchema#positiveInteger"/>
   </rdfs:Datatype>
   <rdfs:Datatype rdf:about="http://www.opengis.net/gml#covariance">
      <owl:equivalentClass rdf:resource="http://www.w3.org/2001/XMLSchema#double"/>
   </rdfs:Datatype>
   <owl:Class rdf:about="http://www.opengis.net/gml#using">
      <rdfs:subClassOf rdf:resource="http://www.opengis.net/gml#FeaturePropertyType"/>
   </owl:Class>
   <owl:Class rdf:about="http://www.opengis.net/gml#target">
      <rdfs:subClassOf rdf:resource="http://www.opengis.net/gml#TargetPropertyType"/>
   </owl:Class>
   <owl:Class rdf:about="http://www.opengis.net/gml#subject">
      <rdfs:subClassOf rdf:resource="http://www.opengis.net/gml#target"/>
      <rdfs:subClassOf rdf:resource="http://www.opengis.net/gml#TargetPropertyType"/>
   </owl:Class>
   <owl:Class rdf:about="http://www.opengis.net/gml#resultOf">
      <rdfs:subClassOf rdf:resource="http://www.opengis.net/gml#AssociationType"/>
   </owl:Class>
   <owl:Class rdf:about="http://www.opengis.net/gml#Observation">
      <rdfs:subClassOf rdf:resource="http://www.opengis.net/gml#_Feature"/>
      <rdfs:subClassOf rdf:resource="http://www.opengis.net/gml#ObservationType"/>
   </owl:Class>
   <owl:Class rdf:about="http://www.opengis.net/gml#DirectedObservation">
      <rdfs:subClassOf rdf:resource="http://www.opengis.net/gml#Observation"/>
      <rdfs:subClassOf rdf:resource="http://www.opengis.net/gml#DirectedObservationType"/>
   </owl:Class>
   <owl:Class rdf:about="http://www.opengis.net/gml#DirectedObservationAtDistance">
      <rdfs:subClassOf rdf:resource="http://www.opengis.net/gml#DirectedObservation"/>
      <rdfs:subClassOf rdf:resource="http://www.opengis.net/gml#DirectedObservationAtDistanceType"/>
   </owl:Class>
   <owl:Class rdf:about="http://www.opengis.net/gml#defaultStyle">
      <rdfs:subClassOf rdf:resource="http://www.opengis.net/gml#DefaultStylePropertyType"/>
   </owl:Class>
   <owl:Class rdf:about="http://www.opengis.net/gml#_Style">
      <rdfs:subClassOf rdf:resource="http://www.opengis.net/gml#_GML"/>
      <rdfs:subClassOf rdf:resource="http://www.opengis.net/gml#AbstractStyleType"/>
   </owl:Class>
   <owl:Class rdf:about="http://www.opengis.net/gml#Style">
      <rdfs:subClassOf rdf:resource="http://www.opengis.net/gml#_Style"/>
      <rdfs:subClassOf rdf:resource="http://www.opengis.net/gml#StyleType"/>
   </owl:Class>
   <owl:Class rdf:about="http://www.opengis.net/gml#featureStyle">
      <rdfs:subClassOf rdf:resource="http://www.opengis.net/gml#FeatureStylePropertyType"/>
   </owl:Class>
   <owl:Class rdf:about="http://www.opengis.net/gml#FeatureStyle">
      <rdfs:subClassOf rdf:resource="http://www.opengis.net/gml#_GML"/>
      <rdfs:subClassOf rdf:resource="http://www.opengis.net/gml#FeatureStyleType"/>
   </owl:Class>
   <owl:Class rdf:about="http://www.opengis.net/gml#geometryStyle">
      <rdfs:subClassOf rdf:resource="http://www.opengis.net/gml#GeometryStylePropertyType"/>
   </owl:Class>
   <owl:Class rdf:about="http://www.opengis.net/gml#GeometryStyle">
      <rdfs:subClassOf rdf:resource="http://www.opengis.net/gml#_GML"/>
      <rdfs:subClassOf rdf:resource="http://www.opengis.net/gml#GeometryStyleType"/>
   </owl:Class>
   <owl:Class rdf:about="http://www.opengis.net/gml#topologyStyle">
      <rdfs:subClassOf rdf:resource="http://www.opengis.net/gml#TopologyStylePropertyType"/>
   </owl:Class>
   <owl:Class rdf:about="http://www.opengis.net/gml#TopologyStyle">
      <rdfs:subClassOf rdf:resource="http://www.opengis.net/gml#_GML"/>
      <rdfs:subClassOf rdf:resource="http://www.opengis.net/gml#TopologyStyleType"/>
   </owl:Class>
   <owl:Class rdf:about="http://www.opengis.net/gml#labelStyle">
      <rdfs:subClassOf rdf:resource="http://www.opengis.net/gml#LabelStylePropertyType"/>
   </owl:Class>
   <owl:Class rdf:about="http://www.opengis.net/gml#LabelStyle">
      <rdfs:subClassOf rdf:resource="http://www.opengis.net/gml#_GML"/>
      <rdfs:subClassOf rdf:resource="http://www.opengis.net/gml#LabelStyleType"/>
   </owl:Class>
   <owl:Class rdf:about="http://www.opengis.net/gml#graphStyle">
      <rdfs:subClassOf rdf:resource="http://www.opengis.net/gml#GraphStylePropertyType"/>
   </owl:Class>
   <owl:Class rdf:about="http://www.opengis.net/gml#GraphStyle">
      <rdfs:subClassOf rdf:resource="http://www.opengis.net/gml#_GML"/>
      <rdfs:subClassOf rdf:resource="http://www.opengis.net/gml#GraphStyleType"/>
   </owl:Class>
   <owl:Class rdf:about="http://www.opengis.net/gml#symbol">
      <rdfs:subClassOf rdf:resource="http://www.opengis.net/gml#SymbolType"/>
   </owl:Class>
   <owl:Class rdf:about="http://www.opengis.net/gml#_TimeReferenceSystem">
      <rdfs:subClassOf rdf:resource="http://www.opengis.net/gml#Definition"/>
      <rdfs:subClassOf rdf:resource="http://www.opengis.net/gml#AbstractTimeReferenceSystemType"/>
   </owl:Class>
   <owl:Class rdf:about="http://www.opengis.net/gml#TimeCoordinateSystem">
      <rdfs:subClassOf rdf:resource="http://www.opengis.net/gml#_TimeReferenceSystem"/>
      <rdfs:subClassOf rdf:resource="http://www.opengis.net/gml#TimeCoordinateSystemType"/>
   </owl:Class>
   <owl:Class rdf:about="http://www.opengis.net/gml#TimeOrdinalReferenceSystem">
      <rdfs:subClassOf rdf:resource="http://www.opengis.net/gml#_TimeReferenceSystem"/>
      <rdfs:subClassOf rdf:resource="http://www.opengis.net/gml#TimeOrdinalReferenceSystemType"/>
   </owl:Class>
   <owl:Class rdf:about="http://www.opengis.net/gml#TimeOrdinalEra">
      <rdfs:subClassOf rdf:resource="http://www.opengis.net/gml#TimeOrdinalEraType"/>
   </owl:Class>
   <owl:Class rdf:about="http://www.opengis.net/gml#TimeCalendar">
      <rdfs:subClassOf rdf:resource="http://www.opengis.net/gml#_TimeReferenceSystem"/>
      <rdfs:subClassOf rdf:resource="http://www.opengis.net/gml#TimeCalendarType"/>
   </owl:Class>
   <owl:Class rdf:about="http://www.opengis.net/gml#TimeCalendarEra">
      <rdfs:subClassOf rdf:resource="http://www.opengis.net/gml#Definition"/>
      <rdfs:subClassOf rdf:resource="http://www.opengis.net/gml#TimeCalendarEraType"/>
   </owl:Class>
   <owl:Class rdf:about="http://www.opengis.net/gml#TimeClock">
      <rdfs:subClassOf rdf:resource="http://www.opengis.net/gml#_TimeReferenceSystem"/>
      <rdfs:subClassOf rdf:resource="http://www.opengis.net/gml#TimeClockType"/>
   </owl:Class>
   <owl:Class rdf:about="http://www.opengis.net/gml#TimeTopologyComplex">
      <rdfs:subClassOf rdf:resource="http://www.opengis.net/gml#_TimeComplex"/>
      <rdfs:subClassOf rdf:resource="http://www.opengis.net/gml#TimeTopologyComplexType"/>
   </owl:Class>
   <owl:Class rdf:about="http://www.opengis.net/gml#_TimeTopologyPrimitive">
      <rdfs:subClassOf rdf:resource="http://www.opengis.net/gml#_TimePrimitive"/>
      <rdfs:subClassOf rdf:resource="http://www.opengis.net/gml#AbstractTimeTopologyPrimitiveType"/>
   </owl:Class>
   <owl:Class rdf:about="http://www.opengis.net/gml#TimeNode">
      <rdfs:subClassOf rdf:resource="http://www.opengis.net/gml#_TimeTopologyPrimitive"/>
      <rdfs:subClassOf rdf:resource="http://www.opengis.net/gml#TimeNodeType"/>
   </owl:Class>
   <owl:Class rdf:about="http://www.opengis.net/gml#TimeEdge">
      <rdfs:subClassOf rdf:resource="http://www.opengis.net/gml#_TimeTopologyPrimitive"/>
      <rdfs:subClassOf rdf:resource="http://www.opengis.net/gml#TimeEdgeType"/>
   </owl:Class>
   <owl:ObjectProperty rdf:about="http://www.opengis.net/gml#hasvalidTime">
      <rdfs:comment>Warning: This ObjectProperty reference was declared outside of its original schema. This ObjectProperty may be declared incorrectly.</rdfs:comment>
      <rdfs:domain rdf:resource="http://www.opengis.net/gml#AbstractTimeSliceType"/>
      <rdfs:range rdf:resource="http://www.opengis.net/gml#validTime"/>
   </owl:ObjectProperty>
   <owl:ObjectProperty rdf:about="http://www.opengis.net/gml#hasdataSource">
      <rdfs:comment>Warning: This ObjectProperty reference was declared outside of its original schema. This ObjectProperty may be declared incorrectly.</rdfs:comment>
      <rdfs:domain rdf:resource="http://www.opengis.net/gml#AbstractTimeSliceType"/>
      <rdfs:range rdf:resource="http://www.opengis.net/gml#dataSource"/>
   </owl:ObjectProperty>
   <owl:ObjectProperty rdf:about="http://www.opengis.net/gml#haslocation">
      <rdfs:comment>Warning: This ObjectProperty reference was declared outside of its original schema. This ObjectProperty may be declared incorrectly.</rdfs:comment>
      <rdfs:domain rdf:resource="http://www.opengis.net/gml#MovingObjectStatusType"/>
      <rdfs:range rdf:resource="http://www.opengis.net/gml#location"/>
   </owl:ObjectProperty>
   <owl:ObjectProperty rdf:about="http://www.opengis.net/gml#speed">
      <rdfs:domain rdf:resource="http://www.opengis.net/gml#MovingObjectStatusType"/>
      <rdfs:range rdf:resource="http://www.opengis.net/gml#MeasureType"/>
   </owl:ObjectProperty>
   <owl:ObjectProperty rdf:about="http://www.opengis.net/gml#bearing">
      <rdfs:domain rdf:resource="http://www.opengis.net/gml#MovingObjectStatusType"/>
      <rdfs:range rdf:resource="http://www.opengis.net/gml#DirectionPropertyType"/>
   </owl:ObjectProperty>
   <owl:ObjectProperty rdf:about="http://www.opengis.net/gml#acceleration">
      <rdfs:domain rdf:resource="http://www.opengis.net/gml#MovingObjectStatusType"/>
      <rdfs:range rdf:resource="http://www.opengis.net/gml#MeasureType"/>
   </owl:ObjectProperty>
   <owl:ObjectProperty rdf:about="http://www.opengis.net/gml#elevation">
      <rdfs:domain rdf:resource="http://www.opengis.net/gml#MovingObjectStatusType"/>
      <rdfs:range rdf:resource="http://www.opengis.net/gml#MeasureType"/>
   </owl:ObjectProperty>
   <owl:ObjectProperty rdf:about="http://www.opengis.net/gml#hasstatus">
      <rdfs:comment>Warning: This ObjectProperty reference was declared outside of its original schema. This ObjectProperty may be declared incorrectly.</rdfs:comment>
      <rdfs:domain rdf:resource="http://www.opengis.net/gml#MovingObjectStatusType"/>
      <rdfs:range rdf:resource="http://www.opengis.net/gml#status"/>
   </owl:ObjectProperty>
   <owl:ObjectProperty rdf:about="http://www.opengis.net/gml#has_TimeSlice">
      <rdfs:comment>Warning: This ObjectProperty reference was declared outside of its original schema. This ObjectProperty may be declared incorrectly.</rdfs:comment>
      <rdfs:domain rdf:resource="http://www.opengis.net/gml#HistoryPropertyType"/>
      <rdfs:range rdf:resource="http://www.opengis.net/gml#_TimeSlice"/>
   </owl:ObjectProperty>
   <owl:ObjectProperty rdf:about="http://www.opengis.net/gml#hasMovingObjectStatus">
      <rdfs:comment>Warning: This ObjectProperty reference was declared outside of its original schema. This ObjectProperty may be declared incorrectly.</rdfs:comment>
      <rdfs:domain rdf:resource="http://www.opengis.net/gml#TrackType"/>
      <rdfs:range rdf:resource="http://www.opengis.net/gml#MovingObjectStatus"/>
   </owl:ObjectProperty>
   <owl:ObjectProperty rdf:about="http://www.opengis.net/gml#hasvalidTime">
      <rdfs:comment>Warning: This ObjectProperty reference was declared outside of its original schema. This ObjectProperty may be declared incorrectly.</rdfs:comment>
      <rdfs:domain rdf:resource="http://www.opengis.net/gml#dynamicProperties"/>
      <rdfs:range rdf:resource="http://www.opengis.net/gml#validTime"/>
   </owl:ObjectProperty>
   <owl:ObjectProperty rdf:about="http://www.opengis.net/gml#hashistory">
      <rdfs:comment>Warning: This ObjectProperty reference was declared outside of its original schema. This ObjectProperty may be declared incorrectly.</rdfs:comment>
      <rdfs:domain rdf:resource="http://www.opengis.net/gml#dynamicProperties"/>
      <rdfs:range rdf:resource="http://www.opengis.net/gml#history"/>
   </owl:ObjectProperty>
   <owl:ObjectProperty rdf:about="http://www.opengis.net/gml#hasdataSource">
      <rdfs:comment>Warning: This ObjectProperty reference was declared outside of its original schema. This ObjectProperty may be declared incorrectly.</rdfs:comment>
      <rdfs:domain rdf:resource="http://www.opengis.net/gml#dynamicProperties"/>
      <rdfs:range rdf:resource="http://www.opengis.net/gml#dataSource"/>
   </owl:ObjectProperty>
   <owl:ObjectProperty rdf:about="http://www.opengis.net/gml#hasboundedBy">
      <rdfs:comment>Warning: This ObjectProperty reference was declared outside of its original schema. This ObjectProperty may be declared incorrectly.</rdfs:comment>
      <rdfs:domain rdf:resource="http://www.opengis.net/gml#AbstractFeatureType"/>
      <rdfs:range rdf:resource="http://www.opengis.net/gml#boundedBy"/>
   </owl:ObjectProperty>
   <owl:ObjectProperty rdf:about="http://www.opengis.net/gml#haslocation">
      <rdfs:comment>Warning: This ObjectProperty reference was declared outside of its original schema. This ObjectProperty may be declared incorrectly.</rdfs:comment>
      <rdfs:domain rdf:resource="http://www.opengis.net/gml#AbstractFeatureType"/>
      <rdfs:range rdf:resource="http://www.opengis.net/gml#location"/>
   </owl:ObjectProperty>
   <owl:ObjectProperty rdf:about="http://www.opengis.net/gml#hasEnvelope">
      <rdfs:comment>Warning: This ObjectProperty reference was declared outside of its original schema. This ObjectProperty may be declared incorrectly.</rdfs:comment>
      <rdfs:domain rdf:resource="http://www.opengis.net/gml#BoundingShapeType"/>
      <rdfs:range rdf:resource="http://www.opengis.net/gml#Envelope"/>
   </owl:ObjectProperty>
   <owl:ObjectProperty rdf:about="http://www.opengis.net/gml#hasNull">
      <rdfs:comment>Warning: This ObjectProperty reference was declared outside of its original schema. This ObjectProperty may be declared incorrectly.</rdfs:comment>
      <rdfs:domain rdf:resource="http://www.opengis.net/gml#BoundingShapeType"/>
      <rdfs:range rdf:resource="http://www.opengis.net/gml#Null"/>
   </owl:ObjectProperty>
   <owl:ObjectProperty rdf:about="http://www.opengis.net/gml#hastimePosition">
      <rdfs:comment>Warning: This ObjectProperty reference was declared outside of its original schema. This ObjectProperty may be declared incorrectly.</rdfs:comment>
      <rdfs:domain rdf:resource="http://www.opengis.net/gml#EnvelopeWithTimePeriodType"/>
      <rdfs:range rdf:resource="http://www.opengis.net/gml#timePosition"/>
   </owl:ObjectProperty>
   <owl:ObjectProperty rdf:about="http://www.opengis.net/gml#has_Feature">
      <rdfs:comment>Warning: This ObjectProperty reference was declared outside of its original schema. This ObjectProperty may be declared incorrectly.</rdfs:comment>
      <rdfs:domain rdf:resource="http://www.opengis.net/gml#FeaturePropertyType"/>
      <rdfs:range rdf:resource="http://www.opengis.net/gml#_Feature"/>
   </owl:ObjectProperty>
   <owl:ObjectProperty rdf:about="http://www.opengis.net/gml#has_Feature">
      <rdfs:comment>Warning: This ObjectProperty reference was declared outside of its original schema. This ObjectProperty may be declared incorrectly.</rdfs:comment>
      <rdfs:domain rdf:resource="http://www.opengis.net/gml#FeatureArrayPropertyType"/>
      <rdfs:range rdf:resource="http://www.opengis.net/gml#_Feature"/>
   </owl:ObjectProperty>
   <owl:ObjectProperty rdf:about="http://www.opengis.net/gml#hasfeatureMember">
      <rdfs:comment>Warning: This ObjectProperty reference was declared outside of its original schema. This ObjectProperty may be declared incorrectly.</rdfs:comment>
      <rdfs:domain rdf:resource="http://www.opengis.net/gml#AbstractFeatureCollectionType"/>
      <rdfs:range rdf:resource="http://www.opengis.net/gml#featureMember"/>
   </owl:ObjectProperty>
   <owl:ObjectProperty rdf:about="http://www.opengis.net/gml#hasfeatureMembers">
      <rdfs:comment>Warning: This ObjectProperty reference was declared outside of its original schema. This ObjectProperty may be declared incorrectly.</rdfs:comment>
      <rdfs:domain rdf:resource="http://www.opengis.net/gml#AbstractFeatureCollectionType"/>
      <rdfs:range rdf:resource="http://www.opengis.net/gml#featureMembers"/>
   </owl:ObjectProperty>
   <owl:ObjectProperty rdf:about="http://www.opengis.net/gml#hasboundedBy">
      <rdfs:comment>Warning: This ObjectProperty reference was declared outside of its original schema. This ObjectProperty may be declared incorrectly.</rdfs:comment>
      <rdfs:domain rdf:resource="http://www.opengis.net/gml#BoundedFeatureType"/>
      <rdfs:range rdf:resource="http://www.opengis.net/gml#boundedBy"/>
   </owl:ObjectProperty>
   <owl:ObjectProperty rdf:about="http://www.opengis.net/gml#haslocation">
      <rdfs:comment>Warning: This ObjectProperty reference was declared outside of its original schema. This ObjectProperty may be declared incorrectly.</rdfs:comment>
      <rdfs:domain rdf:resource="http://www.opengis.net/gml#BoundedFeatureType"/>
      <rdfs:range rdf:resource="http://www.opengis.net/gml#location"/>
   </owl:ObjectProperty>
   <owl:ObjectProperty rdf:about="http://www.opengis.net/gml#has_Geometry">
      <rdfs:comment>Warning: This ObjectProperty reference was declared outside of its original schema. This ObjectProperty may be declared incorrectly.</rdfs:comment>
      <rdfs:domain rdf:resource="http://www.opengis.net/gml#LocationPropertyType"/>
      <rdfs:range rdf:resource="http://www.opengis.net/gml#_Geometry"/>
   </owl:ObjectProperty>
   <owl:ObjectProperty rdf:about="http://www.opengis.net/gml#hasLocationKeyWord">
      <rdfs:comment>Warning: This ObjectProperty reference was declared outside of its original schema. This ObjectProperty may be declared incorrectly.</rdfs:comment>
      <rdfs:domain rdf:resource="http://www.opengis.net/gml#LocationPropertyType"/>
      <rdfs:range rdf:resource="http://www.opengis.net/gml#LocationKeyWord"/>
   </owl:ObjectProperty>
   <owl:ObjectProperty rdf:about="http://www.opengis.net/gml#hasLocationString">
      <rdfs:comment>Warning: This ObjectProperty reference was declared outside of its original schema. This ObjectProperty may be declared incorrectly.</rdfs:comment>
      <rdfs:domain rdf:resource="http://www.opengis.net/gml#LocationPropertyType"/>
      <rdfs:range rdf:resource="http://www.opengis.net/gml#LocationString"/>
   </owl:ObjectProperty>
   <owl:ObjectProperty rdf:about="http://www.opengis.net/gml#hasNull">
      <rdfs:comment>Warning: This ObjectProperty reference was declared outside of its original schema. This ObjectProperty may be declared incorrectly.</rdfs:comment>
      <rdfs:domain rdf:resource="http://www.opengis.net/gml#LocationPropertyType"/>
      <rdfs:range rdf:resource="http://www.opengis.net/gml#Null"/>
   </owl:ObjectProperty>
   <owl:ObjectProperty rdf:about="http://www.opengis.net/gml#has_Surface">
      <rdfs:comment>Warning: This ObjectProperty reference was declared outside of its original schema. This ObjectProperty may be declared incorrectly.</rdfs:comment>
      <rdfs:domain rdf:resource="http://www.opengis.net/gml#SurfacePropertyType"/>
      <rdfs:range rdf:resource="http://www.opengis.net/gml#_Surface"/>
   </owl:ObjectProperty>
   <owl:ObjectProperty rdf:about="http://www.opengis.net/gml#has_Surface">
      <rdfs:comment>Warning: This ObjectProperty reference was declared outside of its original schema. This ObjectProperty may be declared incorrectly.</rdfs:comment>
      <rdfs:domain rdf:resource="http://www.opengis.net/gml#SurfaceArrayPropertyType"/>
      <rdfs:range rdf:resource="http://www.opengis.net/gml#_Surface"/>
   </owl:ObjectProperty>
   <owl:ObjectProperty rdf:about="http://www.opengis.net/gml#hasexterior">
      <rdfs:comment>Warning: This ObjectProperty reference was declared outside of its original schema. This ObjectProperty may be declared incorrectly.</rdfs:comment>
      <rdfs:domain rdf:resource="http://www.opengis.net/gml#PolygonType"/>
      <rdfs:range rdf:resource="http://www.opengis.net/gml#exterior"/>
   </owl:ObjectProperty>
   <owl:ObjectProperty rdf:about="http://www.opengis.net/gml#hasinterior">
      <rdfs:comment>Warning: This ObjectProperty reference was declared outside of its original schema. This ObjectProperty may be declared incorrectly.</rdfs:comment>
      <rdfs:domain rdf:resource="http://www.opengis.net/gml#PolygonType"/>
      <rdfs:range rdf:resource="http://www.opengis.net/gml#interior"/>
   </owl:ObjectProperty>
   <owl:ObjectProperty rdf:about="http://www.opengis.net/gml#has_Ring">
      <rdfs:comment>Warning: This ObjectProperty reference was declared outside of its original schema. This ObjectProperty may be declared incorrectly.</rdfs:comment>
      <rdfs:domain rdf:resource="http://www.opengis.net/gml#AbstractRingPropertyType"/>
      <rdfs:range rdf:resource="http://www.opengis.net/gml#_Ring"/>
   </owl:ObjectProperty>
   <owl:ObjectProperty rdf:about="http://www.opengis.net/gml#haspos">
      <rdfs:comment>Warning: This ObjectProperty reference was declared outside of its original schema. This ObjectProperty may be declared incorrectly.</rdfs:comment>
      <rdfs:domain rdf:resource="http://www.opengis.net/gml#LinearRingType"/>
      <rdfs:range rdf:resource="http://www.opengis.net/gml#pos"/>
   </owl:ObjectProperty>
   <owl:ObjectProperty rdf:about="http://www.opengis.net/gml#haspointProperty">
      <rdfs:comment>Warning: This ObjectProperty reference was declared outside of its original schema. This ObjectProperty may be declared incorrectly.</rdfs:comment>
      <rdfs:domain rdf:resource="http://www.opengis.net/gml#LinearRingType"/>
      <rdfs:range rdf:resource="http://www.opengis.net/gml#pointProperty"/>
   </owl:ObjectProperty>
   <owl:ObjectProperty rdf:about="http://www.opengis.net/gml#haspointRep">
      <rdfs:comment>Warning: This ObjectProperty reference was declared outside of its original schema. This ObjectProperty may be declared incorrectly.</rdfs:comment>
      <rdfs:domain rdf:resource="http://www.opengis.net/gml#LinearRingType"/>
      <rdfs:range rdf:resource="http://www.opengis.net/gml#pointRep"/>
   </owl:ObjectProperty>
   <owl:ObjectProperty rdf:about="http://www.opengis.net/gml#hasposList">
      <rdfs:comment>Warning: This ObjectProperty reference was declared outside of its original schema. This ObjectProperty may be declared incorrectly.</rdfs:comment>
      <rdfs:domain rdf:resource="http://www.opengis.net/gml#LinearRingType"/>
      <rdfs:range rdf:resource="http://www.opengis.net/gml#posList"/>
   </owl:ObjectProperty>
   <owl:ObjectProperty rdf:about="http://www.opengis.net/gml#hascoordinates">
      <rdfs:comment>Warning: This ObjectProperty reference was declared outside of its original schema. This ObjectProperty may be declared incorrectly.</rdfs:comment>
      <rdfs:domain rdf:resource="http://www.opengis.net/gml#LinearRingType"/>
      <rdfs:range rdf:resource="http://www.opengis.net/gml#coordinates"/>
   </owl:ObjectProperty>
   <owl:ObjectProperty rdf:about="http://www.opengis.net/gml#hascoord">
      <rdfs:comment>Warning: This ObjectProperty reference was declared outside of its original schema. This ObjectProperty may be declared incorrectly.</rdfs:comment>
      <rdfs:domain rdf:resource="http://www.opengis.net/gml#LinearRingType"/>
      <rdfs:range rdf:resource="http://www.opengis.net/gml#coord"/>
   </owl:ObjectProperty>
   <owl:ObjectProperty rdf:about="http://www.opengis.net/gml#hasLinearRing">
      <rdfs:comment>Warning: This ObjectProperty reference was declared outside of its original schema. This ObjectProperty may be declared incorrectly.</rdfs:comment>
      <rdfs:domain rdf:resource="http://www.opengis.net/gml#LinearRingPropertyType"/>
      <rdfs:range rdf:resource="http://www.opengis.net/gml#LinearRing"/>
   </owl:ObjectProperty>
   <owl:ObjectProperty rdf:about="http://www.opengis.net/gml#hasPolygon">
      <rdfs:comment>Warning: This ObjectProperty reference was declared outside of its original schema. This ObjectProperty may be declared incorrectly.</rdfs:comment>
      <rdfs:domain rdf:resource="http://www.opengis.net/gml#PolygonPropertyType"/>
      <rdfs:range rdf:resource="http://www.opengis.net/gml#Polygon"/>
   </owl:ObjectProperty>
   <owl:ObjectProperty rdf:about="http://www.opengis.net/gml#has_Geometry">
      <rdfs:comment>Warning: This ObjectProperty reference was declared outside of its original schema. This ObjectProperty may be declared incorrectly.</rdfs:comment>
      <rdfs:domain rdf:resource="http://www.opengis.net/gml#GeometryPropertyType"/>
      <rdfs:range rdf:resource="http://www.opengis.net/gml#_Geometry"/>
   </owl:ObjectProperty>
   <owl:ObjectProperty rdf:about="http://www.opengis.net/gml#has_Geometry">
      <rdfs:comment>Warning: This ObjectProperty reference was declared outside of its original schema. This ObjectProperty may be declared incorrectly.</rdfs:comment>
      <rdfs:domain rdf:resource="http://www.opengis.net/gml#GeometryArrayPropertyType"/>
      <rdfs:range rdf:resource="http://www.opengis.net/gml#_Geometry"/>
   </owl:ObjectProperty>
   <owl:ObjectProperty rdf:about="http://www.opengis.net/gml#has_GeometricPrimitive">
      <rdfs:comment>Warning: This ObjectProperty reference was declared outside of its original schema. This ObjectProperty may be declared incorrectly.</rdfs:comment>
      <rdfs:domain rdf:resource="http://www.opengis.net/gml#GeometricPrimitivePropertyType"/>
      <rdfs:range rdf:resource="http://www.opengis.net/gml#_GeometricPrimitive"/>
   </owl:ObjectProperty>
   <owl:ObjectProperty rdf:about="http://www.opengis.net/gml#haspos">
      <rdfs:comment>Warning: This ObjectProperty reference was declared outside of its original schema. This ObjectProperty may be declared incorrectly.</rdfs:comment>
      <rdfs:domain rdf:resource="http://www.opengis.net/gml#PointType"/>
      <rdfs:range rdf:resource="http://www.opengis.net/gml#pos"/>
   </owl:ObjectProperty>
   <owl:ObjectProperty rdf:about="http://www.opengis.net/gml#hascoordinates">
      <rdfs:comment>Warning: This ObjectProperty reference was declared outside of its original schema. This ObjectProperty may be declared incorrectly.</rdfs:comment>
      <rdfs:domain rdf:resource="http://www.opengis.net/gml#PointType"/>
      <rdfs:range rdf:resource="http://www.opengis.net/gml#coordinates"/>
   </owl:ObjectProperty>
   <owl:ObjectProperty rdf:about="http://www.opengis.net/gml#hascoord">
      <rdfs:comment>Warning: This ObjectProperty reference was declared outside of its original schema. This ObjectProperty may be declared incorrectly.</rdfs:comment>
      <rdfs:domain rdf:resource="http://www.opengis.net/gml#PointType"/>
      <rdfs:range rdf:resource="http://www.opengis.net/gml#coord"/>
   </owl:ObjectProperty>
   <owl:ObjectProperty rdf:about="http://www.opengis.net/gml#hasPoint">
      <rdfs:comment>Warning: This ObjectProperty reference was declared outside of its original schema. This ObjectProperty may be declared incorrectly.</rdfs:comment>
      <rdfs:domain rdf:resource="http://www.opengis.net/gml#PointPropertyType"/>
      <rdfs:range rdf:resource="http://www.opengis.net/gml#Point"/>
   </owl:ObjectProperty>
   <owl:ObjectProperty rdf:about="http://www.opengis.net/gml#hasPoint">
      <rdfs:comment>Warning: This ObjectProperty reference was declared outside of its original schema. This ObjectProperty may be declared incorrectly.</rdfs:comment>
      <rdfs:domain rdf:resource="http://www.opengis.net/gml#PointArrayPropertyType"/>
      <rdfs:range rdf:resource="http://www.opengis.net/gml#Point"/>
   </owl:ObjectProperty>
   <owl:ObjectProperty rdf:about="http://www.opengis.net/gml#has_Curve">
      <rdfs:comment>Warning: This ObjectProperty reference was declared outside of its original schema. This ObjectProperty may be declared incorrectly.</rdfs:comment>
      <rdfs:domain rdf:resource="http://www.opengis.net/gml#CurvePropertyType"/>
      <rdfs:range rdf:resource="http://www.opengis.net/gml#_Curve"/>
   </owl:ObjectProperty>
   <owl:ObjectProperty rdf:about="http://www.opengis.net/gml#has_Curve">
      <rdfs:comment>Warning: This ObjectProperty reference was declared outside of its original schema. This ObjectProperty may be declared incorrectly.</rdfs:comment>
      <rdfs:domain rdf:resource="http://www.opengis.net/gml#CurveArrayPropertyType"/>
      <rdfs:range rdf:resource="http://www.opengis.net/gml#_Curve"/>
   </owl:ObjectProperty>
   <owl:ObjectProperty rdf:about="http://www.opengis.net/gml#haspos">
      <rdfs:comment>Warning: This ObjectProperty reference was declared outside of its original schema. This ObjectProperty may be declared incorrectly.</rdfs:comment>
      <rdfs:domain rdf:resource="http://www.opengis.net/gml#LineStringType"/>
      <rdfs:range rdf:resource="http://www.opengis.net/gml#pos"/>
   </owl:ObjectProperty>
   <owl:ObjectProperty rdf:about="http://www.opengis.net/gml#haspointProperty">
      <rdfs:comment>Warning: This ObjectProperty reference was declared outside of its original schema. This ObjectProperty may be declared incorrectly.</rdfs:comment>
      <rdfs:domain rdf:resource="http://www.opengis.net/gml#LineStringType"/>
      <rdfs:range rdf:resource="http://www.opengis.net/gml#pointProperty"/>
   </owl:ObjectProperty>
   <owl:ObjectProperty rdf:about="http://www.opengis.net/gml#haspointRep">
      <rdfs:comment>Warning: This ObjectProperty reference was declared outside of its original schema. This ObjectProperty may be declared incorrectly.</rdfs:comment>
      <rdfs:domain rdf:resource="http://www.opengis.net/gml#LineStringType"/>
      <rdfs:range rdf:resource="http://www.opengis.net/gml#pointRep"/>
   </owl:ObjectProperty>
   <owl:ObjectProperty rdf:about="http://www.opengis.net/gml#hascoord">
      <rdfs:comment>Warning: This ObjectProperty reference was declared outside of its original schema. This ObjectProperty may be declared incorrectly.</rdfs:comment>
      <rdfs:domain rdf:resource="http://www.opengis.net/gml#LineStringType"/>
      <rdfs:range rdf:resource="http://www.opengis.net/gml#coord"/>
   </owl:ObjectProperty>
   <owl:ObjectProperty rdf:about="http://www.opengis.net/gml#hasposList">
      <rdfs:comment>Warning: This ObjectProperty reference was declared outside of its original schema. This ObjectProperty may be declared incorrectly.</rdfs:comment>
      <rdfs:domain rdf:resource="http://www.opengis.net/gml#LineStringType"/>
      <rdfs:range rdf:resource="http://www.opengis.net/gml#posList"/>
   </owl:ObjectProperty>
   <owl:ObjectProperty rdf:about="http://www.opengis.net/gml#hascoordinates">
      <rdfs:comment>Warning: This ObjectProperty reference was declared outside of its original schema. This ObjectProperty may be declared incorrectly.</rdfs:comment>
      <rdfs:domain rdf:resource="http://www.opengis.net/gml#LineStringType"/>
      <rdfs:range rdf:resource="http://www.opengis.net/gml#coordinates"/>
   </owl:ObjectProperty>
   <owl:ObjectProperty rdf:about="http://www.opengis.net/gml#haspos">
      <rdfs:comment>Warning: This ObjectProperty reference was declared outside of its original schema. This ObjectProperty may be declared incorrectly.</rdfs:comment>
      <rdfs:domain rdf:resource="http://www.opengis.net/gml#geometricPositionGroup"/>
      <rdfs:range rdf:resource="http://www.opengis.net/gml#pos"/>
   </owl:ObjectProperty>
   <owl:ObjectProperty rdf:about="http://www.opengis.net/gml#haspointProperty">
      <rdfs:comment>Warning: This ObjectProperty reference was declared outside of its original schema. This ObjectProperty may be declared incorrectly.</rdfs:comment>
      <rdfs:domain rdf:resource="http://www.opengis.net/gml#geometricPositionGroup"/>
      <rdfs:range rdf:resource="http://www.opengis.net/gml#pointProperty"/>
   </owl:ObjectProperty>
   <owl:ObjectProperty rdf:about="http://www.opengis.net/gml#hasposList">
      <rdfs:comment>Warning: This ObjectProperty reference was declared outside of its original schema. This ObjectProperty may be declared incorrectly.</rdfs:comment>
      <rdfs:domain rdf:resource="http://www.opengis.net/gml#geometricPositionListGroup"/>
      <rdfs:range rdf:resource="http://www.opengis.net/gml#posList"/>
   </owl:ObjectProperty>
   <owl:ObjectProperty rdf:about="http://www.opengis.net/gml#lowerCorner">
      <rdfs:domain rdf:resource="http://www.opengis.net/gml#EnvelopeType"/>
      <rdfs:range rdf:resource="http://www.opengis.net/gml#DirectPositionType"/>
   </owl:ObjectProperty>
   <owl:ObjectProperty rdf:about="http://www.opengis.net/gml#upperCorner">
      <rdfs:domain rdf:resource="http://www.opengis.net/gml#EnvelopeType"/>
      <rdfs:range rdf:resource="http://www.opengis.net/gml#DirectPositionType"/>
   </owl:ObjectProperty>
   <owl:ObjectProperty rdf:about="http://www.opengis.net/gml#hascoord">
      <rdfs:comment>Warning: This ObjectProperty reference was declared outside of its original schema. This ObjectProperty may be declared incorrectly.</rdfs:comment>
      <rdfs:domain rdf:resource="http://www.opengis.net/gml#EnvelopeType"/>
      <rdfs:range rdf:resource="http://www.opengis.net/gml#coord"/>
   </owl:ObjectProperty>
   <owl:ObjectProperty rdf:about="http://www.opengis.net/gml#haspos">
      <rdfs:comment>Warning: This ObjectProperty reference was declared outside of its original schema. This ObjectProperty may be declared incorrectly.</rdfs:comment>
      <rdfs:domain rdf:resource="http://www.opengis.net/gml#EnvelopeType"/>
      <rdfs:range rdf:resource="http://www.opengis.net/gml#pos"/>
   </owl:ObjectProperty>
   <owl:ObjectProperty rdf:about="http://www.opengis.net/gml#hascoordinates">
      <rdfs:comment>Warning: This ObjectProperty reference was declared outside of its original schema. This ObjectProperty may be declared incorrectly.</rdfs:comment>
      <rdfs:domain rdf:resource="http://www.opengis.net/gml#EnvelopeType"/>
      <rdfs:range rdf:resource="http://www.opengis.net/gml#coordinates"/>
   </owl:ObjectProperty>
   <owl:DatatypeProperty rdf:about="http://www.opengis.net/gml#X">
      <rdfs:domain rdf:resource="http://www.opengis.net/gml#CoordType"/>
      <rdfs:range rdf:resource="http://www.w3.org/2001/XMLSchema#decimal"/>
   </owl:DatatypeProperty>
   <owl:DatatypeProperty rdf:about="http://www.opengis.net/gml#Y">
      <rdfs:domain rdf:resource="http://www.opengis.net/gml#CoordType"/>
      <rdfs:range rdf:resource="http://www.w3.org/2001/XMLSchema#decimal"/>
   </owl:DatatypeProperty>
   <owl:DatatypeProperty rdf:about="http://www.opengis.net/gml#Z">
      <rdfs:domain rdf:resource="http://www.opengis.net/gml#CoordType"/>
      <rdfs:range rdf:resource="http://www.w3.org/2001/XMLSchema#decimal"/>
   </owl:DatatypeProperty>
   <owl:ObjectProperty rdf:about="http://www.opengis.net/gml#hasLineString">
      <rdfs:comment>Warning: This ObjectProperty reference was declared outside of its original schema. This ObjectProperty may be declared incorrectly.</rdfs:comment>
      <rdfs:domain rdf:resource="http://www.opengis.net/gml#LineStringPropertyType"/>
      <rdfs:range rdf:resource="http://www.opengis.net/gml#LineString"/>
   </owl:ObjectProperty>
   <owl:ObjectProperty rdf:about="http://www.opengis.net/gml#hasangle">
      <rdfs:comment>Warning: This ObjectProperty reference was declared outside of its original schema. This ObjectProperty may be declared incorrectly.</rdfs:comment>
      <rdfs:domain rdf:resource="http://www.opengis.net/gml#AngleChoiceType"/>
      <rdfs:range rdf:resource="http://www.opengis.net/gml#angle"/>
   </owl:ObjectProperty>
   <owl:ObjectProperty rdf:about="http://www.opengis.net/gml#hasdmsAngle">
      <rdfs:comment>Warning: This ObjectProperty reference was declared outside of its original schema. This ObjectProperty may be declared incorrectly.</rdfs:comment>
      <rdfs:domain rdf:resource="http://www.opengis.net/gml#AngleChoiceType"/>
      <rdfs:range rdf:resource="http://www.opengis.net/gml#dmsAngle"/>
   </owl:ObjectProperty>
   <owl:ObjectProperty rdf:about="http://www.opengis.net/gml#hasdegrees">
      <rdfs:comment>Warning: This ObjectProperty reference was declared outside of its original schema. This ObjectProperty may be declared incorrectly.</rdfs:comment>
      <rdfs:domain rdf:resource="http://www.opengis.net/gml#DMSAngleType"/>
      <rdfs:range rdf:resource="http://www.opengis.net/gml#degrees"/>
   </owl:ObjectProperty>
   <owl:ObjectProperty rdf:about="http://www.opengis.net/gml#hasdecimalMinutes">
      <rdfs:comment>Warning: This ObjectProperty reference was declared outside of its original schema. This ObjectProperty may be declared incorrectly.</rdfs:comment>
      <rdfs:domain rdf:resource="http://www.opengis.net/gml#DMSAngleType"/>
      <rdfs:range rdf:resource="http://www.opengis.net/gml#decimalMinutes"/>
   </owl:ObjectProperty>
   <owl:ObjectProperty rdf:about="http://www.opengis.net/gml#hasminutes">
      <rdfs:comment>Warning: This ObjectProperty reference was declared outside of its original schema. This ObjectProperty may be declared incorrectly.</rdfs:comment>
      <rdfs:domain rdf:resource="http://www.opengis.net/gml#DMSAngleType"/>
      <rdfs:range rdf:resource="http://www.opengis.net/gml#minutes"/>
   </owl:ObjectProperty>
   <owl:ObjectProperty rdf:about="http://www.opengis.net/gml#hasseconds">
      <rdfs:comment>Warning: This ObjectProperty reference was declared outside of its original schema. This ObjectProperty may be declared incorrectly.</rdfs:comment>
      <rdfs:domain rdf:resource="http://www.opengis.net/gml#DMSAngleType"/>
      <rdfs:range rdf:resource="http://www.opengis.net/gml#seconds"/>
   </owl:ObjectProperty>
   <owl:ObjectProperty rdf:about="http://www.opengis.net/gml#hasquantityType">
      <rdfs:comment>Warning: This ObjectProperty reference was declared outside of its original schema. This ObjectProperty may be declared incorrectly.</rdfs:comment>
      <rdfs:domain rdf:resource="http://www.opengis.net/gml#UnitDefinitionType"/>
      <rdfs:range rdf:resource="http://www.opengis.net/gml#quantityType"/>
   </owl:ObjectProperty>
   <owl:ObjectProperty rdf:about="http://www.opengis.net/gml#hascatalogSymbol">
      <rdfs:comment>Warning: This ObjectProperty reference was declared outside of its original schema. This ObjectProperty may be declared incorrectly.</rdfs:comment>
      <rdfs:domain rdf:resource="http://www.opengis.net/gml#UnitDefinitionType"/>
      <rdfs:range rdf:resource="http://www.opengis.net/gml#catalogSymbol"/>
   </owl:ObjectProperty>
   <owl:ObjectProperty rdf:about="http://www.opengis.net/gml#unitsSystem">
      <rdfs:domain rdf:resource="http://www.opengis.net/gml#BaseUnitType"/>
      <rdfs:range rdf:resource="http://www.opengis.net/gml#ReferenceType"/>
   </owl:ObjectProperty>
   <owl:ObjectProperty rdf:about="http://www.opengis.net/gml#hasderivationUnitTerm">
      <rdfs:comment>Warning: This ObjectProperty reference was declared outside of its original schema. This ObjectProperty may be declared incorrectly.</rdfs:comment>
      <rdfs:domain rdf:resource="http://www.opengis.net/gml#DerivedUnitType"/>
      <rdfs:range rdf:resource="http://www.opengis.net/gml#derivationUnitTerm"/>
   </owl:ObjectProperty>
   <owl:ObjectProperty rdf:about="http://www.opengis.net/gml#hasconversionToPreferredUnit">
      <rdfs:comment>Warning: This ObjectProperty reference was declared outside of its original schema. This ObjectProperty may be declared incorrectly.</rdfs:comment>
      <rdfs:domain rdf:resource="http://www.opengis.net/gml#ConventionalUnitType"/>
      <rdfs:range rdf:resource="http://www.opengis.net/gml#conversionToPreferredUnit"/>
   </owl:ObjectProperty>
   <owl:ObjectProperty rdf:about="http://www.opengis.net/gml#hasroughConversionToPreferredUnit">
      <rdfs:comment>Warning: This ObjectProperty reference was declared outside of its original schema. This ObjectProperty may be declared incorrectly.</rdfs:comment>
      <rdfs:domain rdf:resource="http://www.opengis.net/gml#ConventionalUnitType"/>
      <rdfs:range rdf:resource="http://www.opengis.net/gml#roughConversionToPreferredUnit"/>
   </owl:ObjectProperty>
   <owl:ObjectProperty rdf:about="http://www.opengis.net/gml#hasderivationUnitTerm">
      <rdfs:comment>Warning: This ObjectProperty reference was declared outside of its original schema. This ObjectProperty may be declared incorrectly.</rdfs:comment>
      <rdfs:domain rdf:resource="http://www.opengis.net/gml#ConventionalUnitType"/>
      <rdfs:range rdf:resource="http://www.opengis.net/gml#derivationUnitTerm"/>
   </owl:ObjectProperty>
   <owl:DatatypeProperty rdf:about="http://www.opengis.net/gml#factor">
      <rdfs:domain rdf:resource="http://www.opengis.net/gml#ConversionToPreferredUnitType"/>
      <rdfs:range rdf:resource="http://www.w3.org/2001/XMLSchema#double"/>
   </owl:DatatypeProperty>
   <owl:ObjectProperty rdf:about="http://www.opengis.net/gml#formula">
      <rdfs:domain rdf:resource="http://www.opengis.net/gml#ConversionToPreferredUnitType"/>
      <rdfs:range rdf:resource="http://www.opengis.net/gml#FormulaType"/>
   </owl:ObjectProperty>
   <owl:DatatypeProperty rdf:about="http://www.opengis.net/gml#a">
      <rdfs:domain rdf:resource="http://www.opengis.net/gml#FormulaType"/>
      <rdfs:range rdf:resource="http://www.w3.org/2001/XMLSchema#double"/>
   </owl:DatatypeProperty>
   <owl:DatatypeProperty rdf:about="http://www.opengis.net/gml#b">
      <rdfs:domain rdf:resource="http://www.opengis.net/gml#FormulaType"/>
      <rdfs:range rdf:resource="http://www.w3.org/2001/XMLSchema#double"/>
   </owl:DatatypeProperty>
   <owl:DatatypeProperty rdf:about="http://www.opengis.net/gml#c">
      <rdfs:domain rdf:resource="http://www.opengis.net/gml#FormulaType"/>
      <rdfs:range rdf:resource="http://www.w3.org/2001/XMLSchema#double"/>
   </owl:DatatypeProperty>
   <owl:DatatypeProperty rdf:about="http://www.opengis.net/gml#d">
      <rdfs:domain rdf:resource="http://www.opengis.net/gml#FormulaType"/>
      <rdfs:range rdf:resource="http://www.w3.org/2001/XMLSchema#double"/>
   </owl:DatatypeProperty>
   <owl:ObjectProperty rdf:about="http://www.opengis.net/gml#hasmetaDataProperty">
      <rdfs:comment>Warning: This ObjectProperty reference was declared outside of its original schema. This ObjectProperty may be declared incorrectly.</rdfs:comment>
      <rdfs:domain rdf:resource="http://www.opengis.net/gml#StandardDefinitionProperties"/>
      <rdfs:range rdf:resource="http://www.opengis.net/gml#metaDataProperty"/>
   </owl:ObjectProperty>
   <owl:ObjectProperty rdf:about="http://www.opengis.net/gml#hasdescription">
      <rdfs:comment>Warning: This ObjectProperty reference was declared outside of its original schema. This ObjectProperty may be declared incorrectly.</rdfs:comment>
      <rdfs:domain rdf:resource="http://www.opengis.net/gml#StandardDefinitionProperties"/>
      <rdfs:range rdf:resource="http://www.opengis.net/gml#description"/>
   </owl:ObjectProperty>
   <owl:ObjectProperty rdf:about="http://www.opengis.net/gml#hasname">
      <rdfs:comment>Warning: This ObjectProperty reference was declared outside of its original schema. This ObjectProperty may be declared incorrectly.</rdfs:comment>
      <rdfs:domain rdf:resource="http://www.opengis.net/gml#StandardDefinitionProperties"/>
      <rdfs:range rdf:resource="http://www.opengis.net/gml#name"/>
   </owl:ObjectProperty>
   <owl:ObjectProperty rdf:about="http://www.opengis.net/gml#hasmetaDataProperty">
      <rdfs:comment>Warning: This ObjectProperty reference was declared outside of its original schema. This ObjectProperty may be declared incorrectly.</rdfs:comment>
      <rdfs:domain rdf:resource="http://www.opengis.net/gml#DefinitionType"/>
      <rdfs:range rdf:resource="http://www.opengis.net/gml#metaDataProperty"/>
   </owl:ObjectProperty>
   <owl:ObjectProperty rdf:about="http://www.opengis.net/gml#hasdescription">
      <rdfs:comment>Warning: This ObjectProperty reference was declared outside of its original schema. This ObjectProperty may be declared incorrectly.</rdfs:comment>
      <rdfs:domain rdf:resource="http://www.opengis.net/gml#DefinitionType"/>
      <rdfs:range rdf:resource="http://www.opengis.net/gml#description"/>
   </owl:ObjectProperty>
   <owl:ObjectProperty rdf:about="http://www.opengis.net/gml#hasname">
      <rdfs:comment>Warning: This ObjectProperty reference was declared outside of its original schema. This ObjectProperty may be declared incorrectly.</rdfs:comment>
      <rdfs:domain rdf:resource="http://www.opengis.net/gml#DefinitionType"/>
      <rdfs:range rdf:resource="http://www.opengis.net/gml#name"/>
   </owl:ObjectProperty>
   <owl:ObjectProperty rdf:about="http://www.opengis.net/gml#hasdictionaryEntry">
      <rdfs:comment>Warning: This ObjectProperty reference was declared outside of its original schema. This ObjectProperty may be declared incorrectly.</rdfs:comment>
      <rdfs:domain rdf:resource="http://www.opengis.net/gml#DictionaryType"/>
      <rdfs:range rdf:resource="http://www.opengis.net/gml#dictionaryEntry"/>
   </owl:ObjectProperty>
   <owl:ObjectProperty rdf:about="http://www.opengis.net/gml#hasindirectEntry">
      <rdfs:comment>Warning: This ObjectProperty reference was declared outside of its original schema. This ObjectProperty may be declared incorrectly.</rdfs:comment>
      <rdfs:domain rdf:resource="http://www.opengis.net/gml#DictionaryType"/>
      <rdfs:range rdf:resource="http://www.opengis.net/gml#indirectEntry"/>
   </owl:ObjectProperty>
   <owl:ObjectProperty rdf:about="http://www.opengis.net/gml#hasDefinition">
      <rdfs:comment>Warning: This ObjectProperty reference was declared outside of its original schema. This ObjectProperty may be declared incorrectly.</rdfs:comment>
      <rdfs:domain rdf:resource="http://www.opengis.net/gml#DictionaryEntryType"/>
      <rdfs:range rdf:resource="http://www.opengis.net/gml#Definition"/>
   </owl:ObjectProperty>
   <owl:ObjectProperty rdf:about="http://www.opengis.net/gml#hasDefinitionProxy">
      <rdfs:comment>Warning: This ObjectProperty reference was declared outside of its original schema. This ObjectProperty may be declared incorrectly.</rdfs:comment>
      <rdfs:domain rdf:resource="http://www.opengis.net/gml#IndirectEntryType"/>
      <rdfs:range rdf:resource="http://www.opengis.net/gml#DefinitionProxy"/>
   </owl:ObjectProperty>
   <owl:ObjectProperty rdf:about="http://www.opengis.net/gml#hasdefinitionRef">
      <rdfs:comment>Warning: This ObjectProperty reference was declared outside of its original schema. This ObjectProperty may be declared incorrectly.</rdfs:comment>
      <rdfs:domain rdf:resource="http://www.opengis.net/gml#DefinitionProxyType"/>
      <rdfs:range rdf:resource="http://www.opengis.net/gml#definitionRef"/>
   </owl:ObjectProperty>
   <owl:ObjectProperty rdf:about="http://www.opengis.net/gml#hasmetaDataProperty">
      <rdfs:comment>Warning: This ObjectProperty reference was declared outside of its original schema. This ObjectProperty may be declared incorrectly.</rdfs:comment>
      <rdfs:domain rdf:resource="http://www.opengis.net/gml#StandardObjectProperties"/>
      <rdfs:range rdf:resource="http://www.opengis.net/gml#metaDataProperty"/>
   </owl:ObjectProperty>
   <owl:ObjectProperty rdf:about="http://www.opengis.net/gml#hasdescription">
      <rdfs:comment>Warning: This ObjectProperty reference was declared outside of its original schema. This ObjectProperty may be declared incorrectly.</rdfs:comment>
      <rdfs:domain rdf:resource="http://www.opengis.net/gml#StandardObjectProperties"/>
      <rdfs:range rdf:resource="http://www.opengis.net/gml#description"/>
   </owl:ObjectProperty>
   <owl:ObjectProperty rdf:about="http://www.opengis.net/gml#hasname">
      <rdfs:comment>Warning: This ObjectProperty reference was declared outside of its original schema. This ObjectProperty may be declared incorrectly.</rdfs:comment>
      <rdfs:domain rdf:resource="http://www.opengis.net/gml#StandardObjectProperties"/>
      <rdfs:range rdf:resource="http://www.opengis.net/gml#name"/>
   </owl:ObjectProperty>
   <owl:ObjectProperty rdf:about="http://www.opengis.net/gml#hasmember">
      <rdfs:comment>Warning: This ObjectProperty reference was declared outside of its original schema. This ObjectProperty may be declared incorrectly.</rdfs:comment>
      <rdfs:domain rdf:resource="http://www.opengis.net/gml#BagType"/>
      <rdfs:range rdf:resource="http://www.opengis.net/gml#member"/>
   </owl:ObjectProperty>
   <owl:ObjectProperty rdf:about="http://www.opengis.net/gml#hasmembers">
      <rdfs:comment>Warning: This ObjectProperty reference was declared outside of its original schema. This ObjectProperty may be declared incorrectly.</rdfs:comment>
      <rdfs:domain rdf:resource="http://www.opengis.net/gml#BagType"/>
      <rdfs:range rdf:resource="http://www.opengis.net/gml#members"/>
   </owl:ObjectProperty>
   <owl:ObjectProperty rdf:about="http://www.opengis.net/gml#hasmembers">
      <rdfs:comment>Warning: This ObjectProperty reference was declared outside of its original schema. This ObjectProperty may be declared incorrectly.</rdfs:comment>
      <rdfs:domain rdf:resource="http://www.opengis.net/gml#ArrayType"/>
      <rdfs:range rdf:resource="http://www.opengis.net/gml#members"/>
   </owl:ObjectProperty>
   <owl:ObjectProperty rdf:about="http://www.opengis.net/gml#has_Object">
      <rdfs:comment>Warning: This ObjectProperty reference was declared outside of its original schema. This ObjectProperty may be declared incorrectly.</rdfs:comment>
      <rdfs:domain rdf:resource="http://www.opengis.net/gml#AssociationType"/>
      <rdfs:range rdf:resource="http://www.opengis.net/gml#_Object"/>
   </owl:ObjectProperty>
   <owl:ObjectProperty rdf:about="http://www.opengis.net/gml#has_Object">
      <rdfs:comment>Warning: This ObjectProperty reference was declared outside of its original schema. This ObjectProperty may be declared incorrectly.</rdfs:comment>
      <rdfs:domain rdf:resource="http://www.opengis.net/gml#ArrayAssociationType"/>
      <rdfs:range rdf:resource="http://www.opengis.net/gml#_Object"/>
   </owl:ObjectProperty>
   <owl:ObjectProperty rdf:about="http://www.opengis.net/gml#relatedTime">
      <rdfs:domain rdf:resource="http://www.opengis.net/gml#AbstractTimePrimitiveType"/>
      <rdfs:range rdf:resource="http://www.opengis.net/gml#RelatedTimeType"/>
   </owl:ObjectProperty>
   <owl:ObjectProperty rdf:about="http://www.opengis.net/gml#has_TimePrimitive">
      <rdfs:comment>Warning: This ObjectProperty reference was declared outside of its original schema. This ObjectProperty may be declared incorrectly.</rdfs:comment>
      <rdfs:domain rdf:resource="http://www.opengis.net/gml#TimePrimitivePropertyType"/>
      <rdfs:range rdf:resource="http://www.opengis.net/gml#_TimePrimitive"/>
   </owl:ObjectProperty>
   <owl:ObjectProperty rdf:about="http://www.opengis.net/gml#has_TimeGeometricPrimitive">
      <rdfs:comment>Warning: This ObjectProperty reference was declared outside of its original schema. This ObjectProperty may be declared incorrectly.</rdfs:comment>
      <rdfs:domain rdf:resource="http://www.opengis.net/gml#TimeGeometricPrimitivePropertyType"/>
      <rdfs:range rdf:resource="http://www.opengis.net/gml#_TimeGeometricPrimitive"/>
   </owl:ObjectProperty>
   <owl:ObjectProperty rdf:about="http://www.opengis.net/gml#hastimePosition">
      <rdfs:comment>Warning: This ObjectProperty reference was declared outside of its original schema. This ObjectProperty may be declared incorrectly.</rdfs:comment>
      <rdfs:domain rdf:resource="http://www.opengis.net/gml#TimeInstantType"/>
      <rdfs:range rdf:resource="http://www.opengis.net/gml#timePosition"/>
   </owl:ObjectProperty>
   <owl:ObjectProperty rdf:about="http://www.opengis.net/gml#hasTimeInstant">
      <rdfs:comment>Warning: This ObjectProperty reference was declared outside of its original schema. This ObjectProperty may be declared incorrectly.</rdfs:comment>
      <rdfs:domain rdf:resource="http://www.opengis.net/gml#TimeInstantPropertyType"/>
      <rdfs:range rdf:resource="http://www.opengis.net/gml#TimeInstant"/>
   </owl:ObjectProperty>
   <owl:ObjectProperty rdf:about="http://www.opengis.net/gml#beginPosition">
      <rdfs:domain rdf:resource="http://www.opengis.net/gml#TimePeriodType"/>
      <rdfs:range rdf:resource="http://www.opengis.net/gml#TimePositionType"/>
   </owl:ObjectProperty>
   <owl:ObjectProperty rdf:about="http://www.opengis.net/gml#begin">
      <rdfs:domain rdf:resource="http://www.opengis.net/gml#TimePeriodType"/>
      <rdfs:range rdf:resource="http://www.opengis.net/gml#TimeInstantPropertyType"/>
   </owl:ObjectProperty>
   <owl:ObjectProperty rdf:about="http://www.opengis.net/gml#endPosition">
      <rdfs:domain rdf:resource="http://www.opengis.net/gml#TimePeriodType"/>
      <rdfs:range rdf:resource="http://www.opengis.net/gml#TimePositionType"/>
   </owl:ObjectProperty>
   <owl:ObjectProperty rdf:about="http://www.opengis.net/gml#end">
      <rdfs:domain rdf:resource="http://www.opengis.net/gml#TimePeriodType"/>
      <rdfs:range rdf:resource="http://www.opengis.net/gml#TimeInstantPropertyType"/>
   </owl:ObjectProperty>
   <owl:ObjectProperty rdf:about="http://www.opengis.net/gml#hasTimePeriod">
      <rdfs:comment>Warning: This ObjectProperty reference was declared outside of its original schema. This ObjectProperty may be declared incorrectly.</rdfs:comment>
      <rdfs:domain rdf:resource="http://www.opengis.net/gml#TimePeriodPropertyType"/>
      <rdfs:range rdf:resource="http://www.opengis.net/gml#TimePeriod"/>
   </owl:ObjectProperty>
   <owl:ObjectProperty rdf:about="http://www.opengis.net/gml#hasduration">
      <rdfs:comment>Warning: This ObjectProperty reference was declared outside of its original schema. This ObjectProperty may be declared incorrectly.</rdfs:comment>
      <rdfs:domain rdf:resource="http://www.opengis.net/gml#timeLength"/>
      <rdfs:range rdf:resource="http://www.opengis.net/gml#duration"/>
   </owl:ObjectProperty>
   <owl:ObjectProperty rdf:about="http://www.opengis.net/gml#hastimeInterval">
      <rdfs:comment>Warning: This ObjectProperty reference was declared outside of its original schema. This ObjectProperty may be declared incorrectly.</rdfs:comment>
      <rdfs:domain rdf:resource="http://www.opengis.net/gml#timeLength"/>
      <rdfs:range rdf:resource="http://www.opengis.net/gml#timeInterval"/>
   </owl:ObjectProperty>
   <owl:ObjectProperty rdf:about="http://www.opengis.net/gml#hasDirectionVector">
      <rdfs:comment>Warning: This ObjectProperty reference was declared outside of its original schema. This ObjectProperty may be declared incorrectly.</rdfs:comment>
      <rdfs:domain rdf:resource="http://www.opengis.net/gml#DirectionPropertyType"/>
      <rdfs:range rdf:resource="http://www.opengis.net/gml#DirectionVector"/>
   </owl:ObjectProperty>
   <owl:ObjectProperty rdf:about="http://www.opengis.net/gml#hasCompassPoint">
      <rdfs:comment>Warning: This ObjectProperty reference was declared outside of its original schema. This ObjectProperty may be declared incorrectly.</rdfs:comment>
      <rdfs:domain rdf:resource="http://www.opengis.net/gml#DirectionPropertyType"/>
      <rdfs:range rdf:resource="http://www.opengis.net/gml#CompassPoint"/>
   </owl:ObjectProperty>
   <owl:ObjectProperty rdf:about="http://www.opengis.net/gml#DirectionKeyword">
      <rdfs:domain rdf:resource="http://www.opengis.net/gml#DirectionPropertyType"/>
      <rdfs:range rdf:resource="http://www.opengis.net/gml#CodeType"/>
   </owl:ObjectProperty>
   <owl:ObjectProperty rdf:about="http://www.opengis.net/gml#DirectionString">
      <rdfs:domain rdf:resource="http://www.opengis.net/gml#DirectionPropertyType"/>
      <rdfs:range rdf:resource="http://www.opengis.net/gml#StringOrRefType"/>
   </owl:ObjectProperty>
   <owl:ObjectProperty rdf:about="http://www.opengis.net/gml#hasvector">
      <rdfs:comment>Warning: This ObjectProperty reference was declared outside of its original schema. This ObjectProperty may be declared incorrectly.</rdfs:comment>
      <rdfs:domain rdf:resource="http://www.opengis.net/gml#DirectionVectorType"/>
      <rdfs:range rdf:resource="http://www.opengis.net/gml#vector"/>
   </owl:ObjectProperty>
   <owl:ObjectProperty rdf:about="http://www.opengis.net/gml#horizontalAngle">
      <rdfs:domain rdf:resource="http://www.opengis.net/gml#DirectionVectorType"/>
      <rdfs:range rdf:resource="http://www.opengis.net/gml#AngleType"/>
   </owl:ObjectProperty>
   <owl:ObjectProperty rdf:about="http://www.opengis.net/gml#verticalAngle">
      <rdfs:domain rdf:resource="http://www.opengis.net/gml#DirectionVectorType"/>
      <rdfs:range rdf:resource="http://www.opengis.net/gml#AngleType"/>
   </owl:ObjectProperty>
   <owl:ObjectProperty rdf:about="http://www.opengis.net/gml#hasisolated">
      <rdfs:comment>Warning: This ObjectProperty reference was declared outside of its original schema. This ObjectProperty may be declared incorrectly.</rdfs:comment>
      <rdfs:domain rdf:resource="http://www.opengis.net/gml#AbstractTopoPrimitiveType"/>
      <rdfs:range rdf:resource="http://www.opengis.net/gml#isolated"/>
   </owl:ObjectProperty>
   <owl:ObjectProperty rdf:about="http://www.opengis.net/gml#hascontainer">
      <rdfs:comment>Warning: This ObjectProperty reference was declared outside of its original schema. This ObjectProperty may be declared incorrectly.</rdfs:comment>
      <rdfs:domain rdf:resource="http://www.opengis.net/gml#AbstractTopoPrimitiveType"/>
      <rdfs:range rdf:resource="http://www.opengis.net/gml#container"/>
   </owl:ObjectProperty>
   <owl:ObjectProperty rdf:about="http://www.opengis.net/gml#hasNode">
      <rdfs:comment>Warning: This ObjectProperty reference was declared outside of its original schema. This ObjectProperty may be declared incorrectly.</rdfs:comment>
      <rdfs:domain rdf:resource="http://www.opengis.net/gml#IsolatedPropertyType"/>
      <rdfs:range rdf:resource="http://www.opengis.net/gml#Node"/>
   </owl:ObjectProperty>
   <owl:ObjectProperty rdf:about="http://www.opengis.net/gml#hasEdge">
      <rdfs:comment>Warning: This ObjectProperty reference was declared outside of its original schema. This ObjectProperty may be declared incorrectly.</rdfs:comment>
      <rdfs:domain rdf:resource="http://www.opengis.net/gml#IsolatedPropertyType"/>
      <rdfs:range rdf:resource="http://www.opengis.net/gml#Edge"/>
   </owl:ObjectProperty>
   <owl:ObjectProperty rdf:about="http://www.opengis.net/gml#hasFace">
      <rdfs:comment>Warning: This ObjectProperty reference was declared outside of its original schema. This ObjectProperty may be declared incorrectly.</rdfs:comment>
      <rdfs:domain rdf:resource="http://www.opengis.net/gml#ContainerPropertyType"/>
      <rdfs:range rdf:resource="http://www.opengis.net/gml#Face"/>
   </owl:ObjectProperty>
   <owl:ObjectProperty rdf:about="http://www.opengis.net/gml#hasTopoSolid">
      <rdfs:comment>Warning: This ObjectProperty reference was declared outside of its original schema. This ObjectProperty may be declared incorrectly.</rdfs:comment>
      <rdfs:domain rdf:resource="http://www.opengis.net/gml#ContainerPropertyType"/>
      <rdfs:range rdf:resource="http://www.opengis.net/gml#TopoSolid"/>
   </owl:ObjectProperty>
   <owl:ObjectProperty rdf:about="http://www.opengis.net/gml#hasdirectedEdge">
      <rdfs:comment>Warning: This ObjectProperty reference was declared outside of its original schema. This ObjectProperty may be declared incorrectly.</rdfs:comment>
      <rdfs:domain rdf:resource="http://www.opengis.net/gml#NodeType"/>
      <rdfs:range rdf:resource="http://www.opengis.net/gml#directedEdge"/>
   </owl:ObjectProperty>
   <owl:ObjectProperty rdf:about="http://www.opengis.net/gml#haspointProperty">
      <rdfs:comment>Warning: This ObjectProperty reference was declared outside of its original schema. This ObjectProperty may be declared incorrectly.</rdfs:comment>
      <rdfs:domain rdf:resource="http://www.opengis.net/gml#NodeType"/>
      <rdfs:range rdf:resource="http://www.opengis.net/gml#pointProperty"/>
   </owl:ObjectProperty>
   <owl:ObjectProperty rdf:about="http://www.opengis.net/gml#hasNode">
      <rdfs:comment>Warning: This ObjectProperty reference was declared outside of its original schema. This ObjectProperty may be declared incorrectly.</rdfs:comment>
      <rdfs:domain rdf:resource="http://www.opengis.net/gml#DirectedNodePropertyType"/>
      <rdfs:range rdf:resource="http://www.opengis.net/gml#Node"/>
   </owl:ObjectProperty>
   <owl:ObjectProperty rdf:about="http://www.opengis.net/gml#hasdirectedNode">
      <rdfs:comment>Warning: This ObjectProperty reference was declared outside of its original schema. This ObjectProperty may be declared incorrectly.</rdfs:comment>
      <rdfs:domain rdf:resource="http://www.opengis.net/gml#EdgeType"/>
      <rdfs:range rdf:resource="http://www.opengis.net/gml#directedNode"/>
   </owl:ObjectProperty>
   <owl:ObjectProperty rdf:about="http://www.opengis.net/gml#hasdirectedFace">
      <rdfs:comment>Warning: This ObjectProperty reference was declared outside of its original schema. This ObjectProperty may be declared incorrectly.</rdfs:comment>
      <rdfs:domain rdf:resource="http://www.opengis.net/gml#EdgeType"/>
      <rdfs:range rdf:resource="http://www.opengis.net/gml#directedFace"/>
   </owl:ObjectProperty>
   <owl:ObjectProperty rdf:about="http://www.opengis.net/gml#hascurveProperty">
      <rdfs:comment>Warning: This ObjectProperty reference was declared outside of its original schema. This ObjectProperty may be declared incorrectly.</rdfs:comment>
      <rdfs:domain rdf:resource="http://www.opengis.net/gml#EdgeType"/>
      <rdfs:range rdf:resource="http://www.opengis.net/gml#curveProperty"/>
   </owl:ObjectProperty>
   <owl:ObjectProperty rdf:about="http://www.opengis.net/gml#hasEdge">
      <rdfs:comment>Warning: This ObjectProperty reference was declared outside of its original schema. This ObjectProperty may be declared incorrectly.</rdfs:comment>
      <rdfs:domain rdf:resource="http://www.opengis.net/gml#DirectedEdgePropertyType"/>
      <rdfs:range rdf:resource="http://www.opengis.net/gml#Edge"/>
   </owl:ObjectProperty>
   <owl:ObjectProperty rdf:about="http://www.opengis.net/gml#hasdirectedEdge">
      <rdfs:comment>Warning: This ObjectProperty reference was declared outside of its original schema. This ObjectProperty may be declared incorrectly.</rdfs:comment>
      <rdfs:domain rdf:resource="http://www.opengis.net/gml#FaceType"/>
      <rdfs:range rdf:resource="http://www.opengis.net/gml#directedEdge"/>
   </owl:ObjectProperty>
   <owl:ObjectProperty rdf:about="http://www.opengis.net/gml#hasdirectedTopoSolid">
      <rdfs:comment>Warning: This ObjectProperty reference was declared outside of its original schema. This ObjectProperty may be declared incorrectly.</rdfs:comment>
      <rdfs:domain rdf:resource="http://www.opengis.net/gml#FaceType"/>
      <rdfs:range rdf:resource="http://www.opengis.net/gml#directedTopoSolid"/>
   </owl:ObjectProperty>
   <owl:ObjectProperty rdf:about="http://www.opengis.net/gml#hassurfaceProperty">
      <rdfs:comment>Warning: This ObjectProperty reference was declared outside of its original schema. This ObjectProperty may be declared incorrectly.</rdfs:comment>
      <rdfs:domain rdf:resource="http://www.opengis.net/gml#FaceType"/>
      <rdfs:range rdf:resource="http://www.opengis.net/gml#surfaceProperty"/>
   </owl:ObjectProperty>
   <owl:ObjectProperty rdf:about="http://www.opengis.net/gml#hasFace">
      <rdfs:comment>Warning: This ObjectProperty reference was declared outside of its original schema. This ObjectProperty may be declared incorrectly.</rdfs:comment>
      <rdfs:domain rdf:resource="http://www.opengis.net/gml#DirectedFacePropertyType"/>
      <rdfs:range rdf:resource="http://www.opengis.net/gml#Face"/>
   </owl:ObjectProperty>
   <owl:ObjectProperty rdf:about="http://www.opengis.net/gml#hasdirectedFace">
      <rdfs:comment>Warning: This ObjectProperty reference was declared outside of its original schema. This ObjectProperty may be declared incorrectly.</rdfs:comment>
      <rdfs:domain rdf:resource="http://www.opengis.net/gml#TopoSolidType"/>
      <rdfs:range rdf:resource="http://www.opengis.net/gml#directedFace"/>
   </owl:ObjectProperty>
   <owl:ObjectProperty rdf:about="http://www.opengis.net/gml#hasTopoSolid">
      <rdfs:comment>Warning: This ObjectProperty reference was declared outside of its original schema. This ObjectProperty may be declared incorrectly.</rdfs:comment>
      <rdfs:domain rdf:resource="http://www.opengis.net/gml#DirectedTopoSolidPropertyType"/>
      <rdfs:range rdf:resource="http://www.opengis.net/gml#TopoSolid"/>
   </owl:ObjectProperty>
   <owl:ObjectProperty rdf:about="http://www.opengis.net/gml#hasdirectedNode">
      <rdfs:comment>Warning: This ObjectProperty reference was declared outside of its original schema. This ObjectProperty may be declared incorrectly.</rdfs:comment>
      <rdfs:domain rdf:resource="http://www.opengis.net/gml#TopoPointType"/>
      <rdfs:range rdf:resource="http://www.opengis.net/gml#directedNode"/>
   </owl:ObjectProperty>
   <owl:ObjectProperty rdf:about="http://www.opengis.net/gml#hasTopoPoint">
      <rdfs:comment>Warning: This ObjectProperty reference was declared outside of its original schema. This ObjectProperty may be declared incorrectly.</rdfs:comment>
      <rdfs:domain rdf:resource="http://www.opengis.net/gml#TopoPointPropertyType"/>
      <rdfs:range rdf:resource="http://www.opengis.net/gml#TopoPoint"/>
   </owl:ObjectProperty>
   <owl:ObjectProperty rdf:about="http://www.opengis.net/gml#hasdirectedEdge">
      <rdfs:comment>Warning: This ObjectProperty reference was declared outside of its original schema. This ObjectProperty may be declared incorrectly.</rdfs:comment>
      <rdfs:domain rdf:resource="http://www.opengis.net/gml#TopoCurveType"/>
      <rdfs:range rdf:resource="http://www.opengis.net/gml#directedEdge"/>
   </owl:ObjectProperty>
   <owl:ObjectProperty rdf:about="http://www.opengis.net/gml#hasTopoCurve">
      <rdfs:comment>Warning: This ObjectProperty reference was declared outside of its original schema. This ObjectProperty may be declared incorrectly.</rdfs:comment>
      <rdfs:domain rdf:resource="http://www.opengis.net/gml#TopoCurvePropertyType"/>
      <rdfs:range rdf:resource="http://www.opengis.net/gml#TopoCurve"/>
   </owl:ObjectProperty>
   <owl:ObjectProperty rdf:about="http://www.opengis.net/gml#hasdirectedFace">
      <rdfs:comment>Warning: This ObjectProperty reference was declared outside of its original schema. This ObjectProperty may be declared incorrectly.</rdfs:comment>
      <rdfs:domain rdf:resource="http://www.opengis.net/gml#TopoSurfaceType"/>
      <rdfs:range rdf:resource="http://www.opengis.net/gml#directedFace"/>
   </owl:ObjectProperty>
   <owl:ObjectProperty rdf:about="http://www.opengis.net/gml#hasTopoSurface">
      <rdfs:comment>Warning: This ObjectProperty reference was declared outside of its original schema. This ObjectProperty may be declared incorrectly.</rdfs:comment>
      <rdfs:domain rdf:resource="http://www.opengis.net/gml#TopoSurfacePropertyType"/>
      <rdfs:range rdf:resource="http://www.opengis.net/gml#TopoSurface"/>
   </owl:ObjectProperty>
   <owl:ObjectProperty rdf:about="http://www.opengis.net/gml#hasdirectedTopoSolid">
      <rdfs:comment>Warning: This ObjectProperty reference was declared outside of its original schema. This ObjectProperty may be declared incorrectly.</rdfs:comment>
      <rdfs:domain rdf:resource="http://www.opengis.net/gml#TopoVolumeType"/>
      <rdfs:range rdf:resource="http://www.opengis.net/gml#directedTopoSolid"/>
   </owl:ObjectProperty>
   <owl:ObjectProperty rdf:about="http://www.opengis.net/gml#hasTopoVolume">
      <rdfs:comment>Warning: This ObjectProperty reference was declared outside of its original schema. This ObjectProperty may be declared incorrectly.</rdfs:comment>
      <rdfs:domain rdf:resource="http://www.opengis.net/gml#TopoVolumePropertyType"/>
      <rdfs:range rdf:resource="http://www.opengis.net/gml#TopoVolume"/>
   </owl:ObjectProperty>
   <owl:ObjectProperty rdf:about="http://www.opengis.net/gml#hasmaximalComplex">
      <rdfs:comment>Warning: This ObjectProperty reference was declared outside of its original schema. This ObjectProperty may be declared incorrectly.</rdfs:comment>
      <rdfs:domain rdf:resource="http://www.opengis.net/gml#TopoComplexType"/>
      <rdfs:range rdf:resource="http://www.opengis.net/gml#maximalComplex"/>
   </owl:ObjectProperty>
   <owl:ObjectProperty rdf:about="http://www.opengis.net/gml#hassuperComplex">
      <rdfs:comment>Warning: This ObjectProperty reference was declared outside of its original schema. This ObjectProperty may be declared incorrectly.</rdfs:comment>
      <rdfs:domain rdf:resource="http://www.opengis.net/gml#TopoComplexType"/>
      <rdfs:range rdf:resource="http://www.opengis.net/gml#superComplex"/>
   </owl:ObjectProperty>
   <owl:ObjectProperty rdf:about="http://www.opengis.net/gml#hassubComplex">
      <rdfs:comment>Warning: This ObjectProperty reference was declared outside of its original schema. This ObjectProperty may be declared incorrectly.</rdfs:comment>
      <rdfs:domain rdf:resource="http://www.opengis.net/gml#TopoComplexType"/>
      <rdfs:range rdf:resource="http://www.opengis.net/gml#subComplex"/>
   </owl:ObjectProperty>
   <owl:ObjectProperty rdf:about="http://www.opengis.net/gml#hastopoPrimitiveMember">
      <rdfs:comment>Warning: This ObjectProperty reference was declared outside of its original schema. This ObjectProperty may be declared incorrectly.</rdfs:comment>
      <rdfs:domain rdf:resource="http://www.opengis.net/gml#TopoComplexType"/>
      <rdfs:range rdf:resource="http://www.opengis.net/gml#topoPrimitiveMember"/>
   </owl:ObjectProperty>
   <owl:ObjectProperty rdf:about="http://www.opengis.net/gml#hastopoPrimitiveMembers">
      <rdfs:comment>Warning: This ObjectProperty reference was declared outside of its original schema. This ObjectProperty may be declared incorrectly.</rdfs:comment>
      <rdfs:domain rdf:resource="http://www.opengis.net/gml#TopoComplexType"/>
      <rdfs:range rdf:resource="http://www.opengis.net/gml#topoPrimitiveMembers"/>
   </owl:ObjectProperty>
   <owl:ObjectProperty rdf:about="http://www.opengis.net/gml#hasTopoComplex">
      <rdfs:comment>Warning: This ObjectProperty reference was declared outside of its original schema. This ObjectProperty may be declared incorrectly.</rdfs:comment>
      <rdfs:domain rdf:resource="http://www.opengis.net/gml#TopoComplexMemberType"/>
      <rdfs:range rdf:resource="http://www.opengis.net/gml#TopoComplex"/>
   </owl:ObjectProperty>
   <owl:ObjectProperty rdf:about="http://www.opengis.net/gml#has_TopoPrimitive">
      <rdfs:comment>Warning: This ObjectProperty reference was declared outside of its original schema. This ObjectProperty may be declared incorrectly.</rdfs:comment>
      <rdfs:domain rdf:resource="http://www.opengis.net/gml#TopoPrimitiveMemberType"/>
      <rdfs:range rdf:resource="http://www.opengis.net/gml#_TopoPrimitive"/>
   </owl:ObjectProperty>
   <owl:ObjectProperty rdf:about="http://www.opengis.net/gml#has_TopoPrimitive">
      <rdfs:comment>Warning: This ObjectProperty reference was declared outside of its original schema. This ObjectProperty may be declared incorrectly.</rdfs:comment>
      <rdfs:domain rdf:resource="http://www.opengis.net/gml#TopoPrimitiveArrayAssociationType"/>
      <rdfs:range rdf:resource="http://www.opengis.net/gml#_TopoPrimitive"/>
   </owl:ObjectProperty>
   <owl:ObjectProperty rdf:about="http://www.opengis.net/gml#hascurveMember">
      <rdfs:comment>Warning: This ObjectProperty reference was declared outside of its original schema. This ObjectProperty may be declared incorrectly.</rdfs:comment>
      <rdfs:domain rdf:resource="http://www.opengis.net/gml#CompositeCurveType"/>
      <rdfs:range rdf:resource="http://www.opengis.net/gml#curveMember"/>
   </owl:ObjectProperty>
   <owl:ObjectProperty rdf:about="http://www.opengis.net/gml#hasCompositeCurve">
      <rdfs:comment>Warning: This ObjectProperty reference was declared outside of its original schema. This ObjectProperty may be declared incorrectly.</rdfs:comment>
      <rdfs:domain rdf:resource="http://www.opengis.net/gml#CompositeCurvePropertyType"/>
      <rdfs:range rdf:resource="http://www.opengis.net/gml#CompositeCurve"/>
   </owl:ObjectProperty>
   <owl:ObjectProperty rdf:about="http://www.opengis.net/gml#hassurfaceMember">
      <rdfs:comment>Warning: This ObjectProperty reference was declared outside of its original schema. This ObjectProperty may be declared incorrectly.</rdfs:comment>
      <rdfs:domain rdf:resource="http://www.opengis.net/gml#CompositeSurfaceType"/>
      <rdfs:range rdf:resource="http://www.opengis.net/gml#surfaceMember"/>
   </owl:ObjectProperty>
   <owl:ObjectProperty rdf:about="http://www.opengis.net/gml#hasCompositeSurface">
      <rdfs:comment>Warning: This ObjectProperty reference was declared outside of its original schema. This ObjectProperty may be declared incorrectly.</rdfs:comment>
      <rdfs:domain rdf:resource="http://www.opengis.net/gml#CompositeSurfacePropertyType"/>
      <rdfs:range rdf:resource="http://www.opengis.net/gml#CompositeSurface"/>
   </owl:ObjectProperty>
   <owl:ObjectProperty rdf:about="http://www.opengis.net/gml#hassolidMember">
      <rdfs:comment>Warning: This ObjectProperty reference was declared outside of its original schema. This ObjectProperty may be declared incorrectly.</rdfs:comment>
      <rdfs:domain rdf:resource="http://www.opengis.net/gml#CompositeSolidType"/>
      <rdfs:range rdf:resource="http://www.opengis.net/gml#solidMember"/>
   </owl:ObjectProperty>
   <owl:ObjectProperty rdf:about="http://www.opengis.net/gml#hasCompositeSolid">
      <rdfs:comment>Warning: This ObjectProperty reference was declared outside of its original schema. This ObjectProperty may be declared incorrectly.</rdfs:comment>
      <rdfs:domain rdf:resource="http://www.opengis.net/gml#CompositeSolidPropertyType"/>
      <rdfs:range rdf:resource="http://www.opengis.net/gml#CompositeSolid"/>
   </owl:ObjectProperty>
   <owl:ObjectProperty rdf:about="http://www.opengis.net/gml#element">
      <rdfs:domain rdf:resource="http://www.opengis.net/gml#GeometricComplexType"/>
      <rdfs:range rdf:resource="http://www.opengis.net/gml#GeometricPrimitivePropertyType"/>
   </owl:ObjectProperty>
   <owl:ObjectProperty rdf:about="http://www.opengis.net/gml#hasGeometricComplex">
      <rdfs:comment>Warning: This ObjectProperty reference was declared outside of its original schema. This ObjectProperty may be declared incorrectly.</rdfs:comment>
      <rdfs:domain rdf:resource="http://www.opengis.net/gml#GeometricComplexPropertyType"/>
      <rdfs:range rdf:resource="http://www.opengis.net/gml#GeometricComplex"/>
   </owl:ObjectProperty>
   <owl:ObjectProperty rdf:about="http://www.opengis.net/gml#hasCompositeCurve">
      <rdfs:comment>Warning: This ObjectProperty reference was declared outside of its original schema. This ObjectProperty may be declared incorrectly.</rdfs:comment>
      <rdfs:domain rdf:resource="http://www.opengis.net/gml#GeometricComplexPropertyType"/>
      <rdfs:range rdf:resource="http://www.opengis.net/gml#CompositeCurve"/>
   </owl:ObjectProperty>
   <owl:ObjectProperty rdf:about="http://www.opengis.net/gml#hasCompositeSurface">
      <rdfs:comment>Warning: This ObjectProperty reference was declared outside of its original schema. This ObjectProperty may be declared incorrectly.</rdfs:comment>
      <rdfs:domain rdf:resource="http://www.opengis.net/gml#GeometricComplexPropertyType"/>
      <rdfs:range rdf:resource="http://www.opengis.net/gml#CompositeSurface"/>
   </owl:ObjectProperty>
   <owl:ObjectProperty rdf:about="http://www.opengis.net/gml#hasCompositeSolid">
      <rdfs:comment>Warning: This ObjectProperty reference was declared outside of its original schema. This ObjectProperty may be declared incorrectly.</rdfs:comment>
      <rdfs:domain rdf:resource="http://www.opengis.net/gml#GeometricComplexPropertyType"/>
      <rdfs:range rdf:resource="http://www.opengis.net/gml#CompositeSolid"/>
   </owl:ObjectProperty>
   <owl:ObjectProperty rdf:about="http://www.opengis.net/gml#hasgeometryMember">
      <rdfs:comment>Warning: This ObjectProperty reference was declared outside of its original schema. This ObjectProperty may be declared incorrectly.</rdfs:comment>
      <rdfs:domain rdf:resource="http://www.opengis.net/gml#MultiGeometryType"/>
      <rdfs:range rdf:resource="http://www.opengis.net/gml#geometryMember"/>
   </owl:ObjectProperty>
   <owl:ObjectProperty rdf:about="http://www.opengis.net/gml#hasgeometryMembers">
      <rdfs:comment>Warning: This ObjectProperty reference was declared outside of its original schema. This ObjectProperty may be declared incorrectly.</rdfs:comment>
      <rdfs:domain rdf:resource="http://www.opengis.net/gml#MultiGeometryType"/>
      <rdfs:range rdf:resource="http://www.opengis.net/gml#geometryMembers"/>
   </owl:ObjectProperty>
   <owl:ObjectProperty rdf:about="http://www.opengis.net/gml#has_GeometricAggregate">
      <rdfs:comment>Warning: This ObjectProperty reference was declared outside of its original schema. This ObjectProperty may be declared incorrectly.</rdfs:comment>
      <rdfs:domain rdf:resource="http://www.opengis.net/gml#MultiGeometryPropertyType"/>
      <rdfs:range rdf:resource="http://www.opengis.net/gml#_GeometricAggregate"/>
   </owl:ObjectProperty>
   <owl:ObjectProperty rdf:about="http://www.opengis.net/gml#haspointMember">
      <rdfs:comment>Warning: This ObjectProperty reference was declared outside of its original schema. This ObjectProperty may be declared incorrectly.</rdfs:comment>
      <rdfs:domain rdf:resource="http://www.opengis.net/gml#MultiPointType"/>
      <rdfs:range rdf:resource="http://www.opengis.net/gml#pointMember"/>
   </owl:ObjectProperty>
   <owl:ObjectProperty rdf:about="http://www.opengis.net/gml#haspointMembers">
      <rdfs:comment>Warning: This ObjectProperty reference was declared outside of its original schema. This ObjectProperty may be declared incorrectly.</rdfs:comment>
      <rdfs:domain rdf:resource="http://www.opengis.net/gml#MultiPointType"/>
      <rdfs:range rdf:resource="http://www.opengis.net/gml#pointMembers"/>
   </owl:ObjectProperty>
   <owl:ObjectProperty rdf:about="http://www.opengis.net/gml#hasMultiPoint">
      <rdfs:comment>Warning: This ObjectProperty reference was declared outside of its original schema. This ObjectProperty may be declared incorrectly.</rdfs:comment>
      <rdfs:domain rdf:resource="http://www.opengis.net/gml#MultiPointPropertyType"/>
      <rdfs:range rdf:resource="http://www.opengis.net/gml#MultiPoint"/>
   </owl:ObjectProperty>
   <owl:ObjectProperty rdf:about="http://www.opengis.net/gml#hascurveMember">
      <rdfs:comment>Warning: This ObjectProperty reference was declared outside of its original schema. This ObjectProperty may be declared incorrectly.</rdfs:comment>
      <rdfs:domain rdf:resource="http://www.opengis.net/gml#MultiCurveType"/>
      <rdfs:range rdf:resource="http://www.opengis.net/gml#curveMember"/>
   </owl:ObjectProperty>
   <owl:ObjectProperty rdf:about="http://www.opengis.net/gml#hascurveMembers">
      <rdfs:comment>Warning: This ObjectProperty reference was declared outside of its original schema. This ObjectProperty may be declared incorrectly.</rdfs:comment>
      <rdfs:domain rdf:resource="http://www.opengis.net/gml#MultiCurveType"/>
      <rdfs:range rdf:resource="http://www.opengis.net/gml#curveMembers"/>
   </owl:ObjectProperty>
   <owl:ObjectProperty rdf:about="http://www.opengis.net/gml#hasMultiCurve">
      <rdfs:comment>Warning: This ObjectProperty reference was declared outside of its original schema. This ObjectProperty may be declared incorrectly.</rdfs:comment>
      <rdfs:domain rdf:resource="http://www.opengis.net/gml#MultiCurvePropertyType"/>
      <rdfs:range rdf:resource="http://www.opengis.net/gml#MultiCurve"/>
   </owl:ObjectProperty>
   <owl:ObjectProperty rdf:about="http://www.opengis.net/gml#hassurfaceMember">
      <rdfs:comment>Warning: This ObjectProperty reference was declared outside of its original schema. This ObjectProperty may be declared incorrectly.</rdfs:comment>
      <rdfs:domain rdf:resource="http://www.opengis.net/gml#MultiSurfaceType"/>
      <rdfs:range rdf:resource="http://www.opengis.net/gml#surfaceMember"/>
   </owl:ObjectProperty>
   <owl:ObjectProperty rdf:about="http://www.opengis.net/gml#hassurfaceMembers">
      <rdfs:comment>Warning: This ObjectProperty reference was declared outside of its original schema. This ObjectProperty may be declared incorrectly.</rdfs:comment>
      <rdfs:domain rdf:resource="http://www.opengis.net/gml#MultiSurfaceType"/>
      <rdfs:range rdf:resource="http://www.opengis.net/gml#surfaceMembers"/>
   </owl:ObjectProperty>
   <owl:ObjectProperty rdf:about="http://www.opengis.net/gml#hasMultiSurface">
      <rdfs:comment>Warning: This ObjectProperty reference was declared outside of its original schema. This ObjectProperty may be declared incorrectly.</rdfs:comment>
      <rdfs:domain rdf:resource="http://www.opengis.net/gml#MultiSurfacePropertyType"/>
      <rdfs:range rdf:resource="http://www.opengis.net/gml#MultiSurface"/>
   </owl:ObjectProperty>
   <owl:ObjectProperty rdf:about="http://www.opengis.net/gml#hassolidMember">
      <rdfs:comment>Warning: This ObjectProperty reference was declared outside of its original schema. This ObjectProperty may be declared incorrectly.</rdfs:comment>
      <rdfs:domain rdf:resource="http://www.opengis.net/gml#MultiSolidType"/>
      <rdfs:range rdf:resource="http://www.opengis.net/gml#solidMember"/>
   </owl:ObjectProperty>
   <owl:ObjectProperty rdf:about="http://www.opengis.net/gml#hassolidMembers">
      <rdfs:comment>Warning: This ObjectProperty reference was declared outside of its original schema. This ObjectProperty may be declared incorrectly.</rdfs:comment>
      <rdfs:domain rdf:resource="http://www.opengis.net/gml#MultiSolidType"/>
      <rdfs:range rdf:resource="http://www.opengis.net/gml#solidMembers"/>
   </owl:ObjectProperty>
   <owl:ObjectProperty rdf:about="http://www.opengis.net/gml#hasMultiSolid">
      <rdfs:comment>Warning: This ObjectProperty reference was declared outside of its original schema. This ObjectProperty may be declared incorrectly.</rdfs:comment>
      <rdfs:domain rdf:resource="http://www.opengis.net/gml#MultiSolidPropertyType"/>
      <rdfs:range rdf:resource="http://www.opengis.net/gml#MultiSolid"/>
   </owl:ObjectProperty>
   <owl:ObjectProperty rdf:about="http://www.opengis.net/gml#haslineStringMember">
      <rdfs:comment>Warning: This ObjectProperty reference was declared outside of its original schema. This ObjectProperty may be declared incorrectly.</rdfs:comment>
      <rdfs:domain rdf:resource="http://www.opengis.net/gml#MultiLineStringType"/>
      <rdfs:range rdf:resource="http://www.opengis.net/gml#lineStringMember"/>
   </owl:ObjectProperty>
   <owl:ObjectProperty rdf:about="http://www.opengis.net/gml#hasMultiLineString">
      <rdfs:comment>Warning: This ObjectProperty reference was declared outside of its original schema. This ObjectProperty may be declared incorrectly.</rdfs:comment>
      <rdfs:domain rdf:resource="http://www.opengis.net/gml#MultiLineStringPropertyType"/>
      <rdfs:range rdf:resource="http://www.opengis.net/gml#MultiLineString"/>
   </owl:ObjectProperty>
   <owl:ObjectProperty rdf:about="http://www.opengis.net/gml#haspolygonMember">
      <rdfs:comment>Warning: This ObjectProperty reference was declared outside of its original schema. This ObjectProperty may be declared incorrectly.</rdfs:comment>
      <rdfs:domain rdf:resource="http://www.opengis.net/gml#MultiPolygonType"/>
      <rdfs:range rdf:resource="http://www.opengis.net/gml#polygonMember"/>
   </owl:ObjectProperty>
   <owl:ObjectProperty rdf:about="http://www.opengis.net/gml#hasMultiPolygon">
      <rdfs:comment>Warning: This ObjectProperty reference was declared outside of its original schema. This ObjectProperty may be declared incorrectly.</rdfs:comment>
      <rdfs:domain rdf:resource="http://www.opengis.net/gml#MultiPolygonPropertyType"/>
      <rdfs:range rdf:resource="http://www.opengis.net/gml#MultiPolygon"/>
   </owl:ObjectProperty>
   <owl:ObjectProperty rdf:about="http://www.opengis.net/gml#hassegments">
      <rdfs:comment>Warning: This ObjectProperty reference was declared outside of its original schema. This ObjectProperty may be declared incorrectly.</rdfs:comment>
      <rdfs:domain rdf:resource="http://www.opengis.net/gml#CurveType"/>
      <rdfs:range rdf:resource="http://www.opengis.net/gml#segments"/>
   </owl:ObjectProperty>
   <owl:ObjectProperty rdf:about="http://www.opengis.net/gml#hasbaseCurve">
      <rdfs:comment>Warning: This ObjectProperty reference was declared outside of its original schema. This ObjectProperty may be declared incorrectly.</rdfs:comment>
      <rdfs:domain rdf:resource="http://www.opengis.net/gml#OrientableCurveType"/>
      <rdfs:range rdf:resource="http://www.opengis.net/gml#baseCurve"/>
   </owl:ObjectProperty>
   <owl:ObjectProperty rdf:about="http://www.opengis.net/gml#has_CurveSegment">
      <rdfs:comment>Warning: This ObjectProperty reference was declared outside of its original schema. This ObjectProperty may be declared incorrectly.</rdfs:comment>
      <rdfs:domain rdf:resource="http://www.opengis.net/gml#CurveSegmentArrayPropertyType"/>
      <rdfs:range rdf:resource="http://www.opengis.net/gml#_CurveSegment"/>
   </owl:ObjectProperty>
   <owl:ObjectProperty rdf:about="http://www.opengis.net/gml#haspos">
      <rdfs:comment>Warning: This ObjectProperty reference was declared outside of its original schema. This ObjectProperty may be declared incorrectly.</rdfs:comment>
      <rdfs:domain rdf:resource="http://www.opengis.net/gml#LineStringSegmentType"/>
      <rdfs:range rdf:resource="http://www.opengis.net/gml#pos"/>
   </owl:ObjectProperty>
   <owl:ObjectProperty rdf:about="http://www.opengis.net/gml#haspointProperty">
      <rdfs:comment>Warning: This ObjectProperty reference was declared outside of its original schema. This ObjectProperty may be declared incorrectly.</rdfs:comment>
      <rdfs:domain rdf:resource="http://www.opengis.net/gml#LineStringSegmentType"/>
      <rdfs:range rdf:resource="http://www.opengis.net/gml#pointProperty"/>
   </owl:ObjectProperty>
   <owl:ObjectProperty rdf:about="http://www.opengis.net/gml#haspointRep">
      <rdfs:comment>Warning: This ObjectProperty reference was declared outside of its original schema. This ObjectProperty may be declared incorrectly.</rdfs:comment>
      <rdfs:domain rdf:resource="http://www.opengis.net/gml#LineStringSegmentType"/>
      <rdfs:range rdf:resource="http://www.opengis.net/gml#pointRep"/>
   </owl:ObjectProperty>
   <owl:ObjectProperty rdf:about="http://www.opengis.net/gml#hasposList">
      <rdfs:comment>Warning: This ObjectProperty reference was declared outside of its original schema. This ObjectProperty may be declared incorrectly.</rdfs:comment>
      <rdfs:domain rdf:resource="http://www.opengis.net/gml#LineStringSegmentType"/>
      <rdfs:range rdf:resource="http://www.opengis.net/gml#posList"/>
   </owl:ObjectProperty>
   <owl:ObjectProperty rdf:about="http://www.opengis.net/gml#hascoordinates">
      <rdfs:comment>Warning: This ObjectProperty reference was declared outside of its original schema. This ObjectProperty may be declared incorrectly.</rdfs:comment>
      <rdfs:domain rdf:resource="http://www.opengis.net/gml#LineStringSegmentType"/>
      <rdfs:range rdf:resource="http://www.opengis.net/gml#coordinates"/>
   </owl:ObjectProperty>
   <owl:ObjectProperty rdf:about="http://www.opengis.net/gml#haspos">
      <rdfs:comment>Warning: This ObjectProperty reference was declared outside of its original schema. This ObjectProperty may be declared incorrectly.</rdfs:comment>
      <rdfs:domain rdf:resource="http://www.opengis.net/gml#ArcStringType"/>
      <rdfs:range rdf:resource="http://www.opengis.net/gml#pos"/>
   </owl:ObjectProperty>
   <owl:ObjectProperty rdf:about="http://www.opengis.net/gml#haspointProperty">
      <rdfs:comment>Warning: This ObjectProperty reference was declared outside of its original schema. This ObjectProperty may be declared incorrectly.</rdfs:comment>
      <rdfs:domain rdf:resource="http://www.opengis.net/gml#ArcStringType"/>
      <rdfs:range rdf:resource="http://www.opengis.net/gml#pointProperty"/>
   </owl:ObjectProperty>
   <owl:ObjectProperty rdf:about="http://www.opengis.net/gml#haspointRep">
      <rdfs:comment>Warning: This ObjectProperty reference was declared outside of its original schema. This ObjectProperty may be declared incorrectly.</rdfs:comment>
      <rdfs:domain rdf:resource="http://www.opengis.net/gml#ArcStringType"/>
      <rdfs:range rdf:resource="http://www.opengis.net/gml#pointRep"/>
   </owl:ObjectProperty>
   <owl:ObjectProperty rdf:about="http://www.opengis.net/gml#hasposList">
      <rdfs:comment>Warning: This ObjectProperty reference was declared outside of its original schema. This ObjectProperty may be declared incorrectly.</rdfs:comment>
      <rdfs:domain rdf:resource="http://www.opengis.net/gml#ArcStringType"/>
      <rdfs:range rdf:resource="http://www.opengis.net/gml#posList"/>
   </owl:ObjectProperty>
   <owl:ObjectProperty rdf:about="http://www.opengis.net/gml#hascoordinates">
      <rdfs:comment>Warning: This ObjectProperty reference was declared outside of its original schema. This ObjectProperty may be declared incorrectly.</rdfs:comment>
      <rdfs:domain rdf:resource="http://www.opengis.net/gml#ArcStringType"/>
      <rdfs:range rdf:resource="http://www.opengis.net/gml#coordinates"/>
   </owl:ObjectProperty>
   <owl:ObjectProperty rdf:about="http://www.opengis.net/gml#haspos">
      <rdfs:comment>Warning: This ObjectProperty reference was declared outside of its original schema. This ObjectProperty may be declared incorrectly.</rdfs:comment>
      <rdfs:domain rdf:resource="http://www.opengis.net/gml#ArcType"/>
      <rdfs:range rdf:resource="http://www.opengis.net/gml#pos"/>
   </owl:ObjectProperty>
   <owl:ObjectProperty rdf:about="http://www.opengis.net/gml#haspointProperty">
      <rdfs:comment>Warning: This ObjectProperty reference was declared outside of its original schema. This ObjectProperty may be declared incorrectly.</rdfs:comment>
      <rdfs:domain rdf:resource="http://www.opengis.net/gml#ArcType"/>
      <rdfs:range rdf:resource="http://www.opengis.net/gml#pointProperty"/>
   </owl:ObjectProperty>
   <owl:ObjectProperty rdf:about="http://www.opengis.net/gml#haspointRep">
      <rdfs:comment>Warning: This ObjectProperty reference was declared outside of its original schema. This ObjectProperty may be declared incorrectly.</rdfs:comment>
      <rdfs:domain rdf:resource="http://www.opengis.net/gml#ArcType"/>
      <rdfs:range rdf:resource="http://www.opengis.net/gml#pointRep"/>
   </owl:ObjectProperty>
   <owl:ObjectProperty rdf:about="http://www.opengis.net/gml#hasposList">
      <rdfs:comment>Warning: This ObjectProperty reference was declared outside of its original schema. This ObjectProperty may be declared incorrectly.</rdfs:comment>
      <rdfs:domain rdf:resource="http://www.opengis.net/gml#ArcType"/>
      <rdfs:range rdf:resource="http://www.opengis.net/gml#posList"/>
   </owl:ObjectProperty>
   <owl:ObjectProperty rdf:about="http://www.opengis.net/gml#hascoordinates">
      <rdfs:comment>Warning: This ObjectProperty reference was declared outside of its original schema. This ObjectProperty may be declared incorrectly.</rdfs:comment>
      <rdfs:domain rdf:resource="http://www.opengis.net/gml#ArcType"/>
      <rdfs:range rdf:resource="http://www.opengis.net/gml#coordinates"/>
   </owl:ObjectProperty>
   <owl:ObjectProperty rdf:about="http://www.opengis.net/gml#haspos">
      <rdfs:comment>Warning: This ObjectProperty reference was declared outside of its original schema. This ObjectProperty may be declared incorrectly.</rdfs:comment>
      <rdfs:domain rdf:resource="http://www.opengis.net/gml#ArcStringByBulgeType"/>
      <rdfs:range rdf:resource="http://www.opengis.net/gml#pos"/>
   </owl:ObjectProperty>
   <owl:ObjectProperty rdf:about="http://www.opengis.net/gml#haspointProperty">
      <rdfs:comment>Warning: This ObjectProperty reference was declared outside of its original schema. This ObjectProperty may be declared incorrectly.</rdfs:comment>
      <rdfs:domain rdf:resource="http://www.opengis.net/gml#ArcStringByBulgeType"/>
      <rdfs:range rdf:resource="http://www.opengis.net/gml#pointProperty"/>
   </owl:ObjectProperty>
   <owl:ObjectProperty rdf:about="http://www.opengis.net/gml#haspointRep">
      <rdfs:comment>Warning: This ObjectProperty reference was declared outside of its original schema. This ObjectProperty may be declared incorrectly.</rdfs:comment>
      <rdfs:domain rdf:resource="http://www.opengis.net/gml#ArcStringByBulgeType"/>
      <rdfs:range rdf:resource="http://www.opengis.net/gml#pointRep"/>
   </owl:ObjectProperty>
   <owl:ObjectProperty rdf:about="http://www.opengis.net/gml#hasposList">
      <rdfs:comment>Warning: This ObjectProperty reference was declared outside of its original schema. This ObjectProperty may be declared incorrectly.</rdfs:comment>
      <rdfs:domain rdf:resource="http://www.opengis.net/gml#ArcStringByBulgeType"/>
      <rdfs:range rdf:resource="http://www.opengis.net/gml#posList"/>
   </owl:ObjectProperty>
   <owl:ObjectProperty rdf:about="http://www.opengis.net/gml#hascoordinates">
      <rdfs:comment>Warning: This ObjectProperty reference was declared outside of its original schema. This ObjectProperty may be declared incorrectly.</rdfs:comment>
      <rdfs:domain rdf:resource="http://www.opengis.net/gml#ArcStringByBulgeType"/>
      <rdfs:range rdf:resource="http://www.opengis.net/gml#coordinates"/>
   </owl:ObjectProperty>
   <owl:DatatypeProperty rdf:about="http://www.opengis.net/gml#bulge">
      <rdfs:domain rdf:resource="http://www.opengis.net/gml#ArcStringByBulgeType"/>
      <rdfs:range rdf:resource="http://www.w3.org/2001/XMLSchema#double"/>
   </owl:DatatypeProperty>
   <owl:ObjectProperty rdf:about="http://www.opengis.net/gml#normal">
      <rdfs:domain rdf:resource="http://www.opengis.net/gml#ArcStringByBulgeType"/>
      <rdfs:range rdf:resource="http://www.opengis.net/gml#VectorType"/>
   </owl:ObjectProperty>
   <owl:ObjectProperty rdf:about="http://www.opengis.net/gml#haspos">
      <rdfs:comment>Warning: This ObjectProperty reference was declared outside of its original schema. This ObjectProperty may be declared incorrectly.</rdfs:comment>
      <rdfs:domain rdf:resource="http://www.opengis.net/gml#ArcByBulgeType"/>
      <rdfs:range rdf:resource="http://www.opengis.net/gml#pos"/>
   </owl:ObjectProperty>
   <owl:ObjectProperty rdf:about="http://www.opengis.net/gml#haspointProperty">
      <rdfs:comment>Warning: This ObjectProperty reference was declared outside of its original schema. This ObjectProperty may be declared incorrectly.</rdfs:comment>
      <rdfs:domain rdf:resource="http://www.opengis.net/gml#ArcByBulgeType"/>
      <rdfs:range rdf:resource="http://www.opengis.net/gml#pointProperty"/>
   </owl:ObjectProperty>
   <owl:ObjectProperty rdf:about="http://www.opengis.net/gml#haspointRep">
      <rdfs:comment>Warning: This ObjectProperty reference was declared outside of its original schema. This ObjectProperty may be declared incorrectly.</rdfs:comment>
      <rdfs:domain rdf:resource="http://www.opengis.net/gml#ArcByBulgeType"/>
      <rdfs:range rdf:resource="http://www.opengis.net/gml#pointRep"/>
   </owl:ObjectProperty>
   <owl:ObjectProperty rdf:about="http://www.opengis.net/gml#hasposList">
      <rdfs:comment>Warning: This ObjectProperty reference was declared outside of its original schema. This ObjectProperty may be declared incorrectly.</rdfs:comment>
      <rdfs:domain rdf:resource="http://www.opengis.net/gml#ArcByBulgeType"/>
      <rdfs:range rdf:resource="http://www.opengis.net/gml#posList"/>
   </owl:ObjectProperty>
   <owl:ObjectProperty rdf:about="http://www.opengis.net/gml#hascoordinates">
      <rdfs:comment>Warning: This ObjectProperty reference was declared outside of its original schema. This ObjectProperty may be declared incorrectly.</rdfs:comment>
      <rdfs:domain rdf:resource="http://www.opengis.net/gml#ArcByBulgeType"/>
      <rdfs:range rdf:resource="http://www.opengis.net/gml#coordinates"/>
   </owl:ObjectProperty>
   <owl:DatatypeProperty rdf:about="http://www.opengis.net/gml#bulge">
      <rdfs:domain rdf:resource="http://www.opengis.net/gml#ArcByBulgeType"/>
      <rdfs:range rdf:resource="http://www.w3.org/2001/XMLSchema#double"/>
   </owl:DatatypeProperty>
   <owl:ObjectProperty rdf:about="http://www.opengis.net/gml#normal">
      <rdfs:domain rdf:resource="http://www.opengis.net/gml#ArcByBulgeType"/>
      <rdfs:range rdf:resource="http://www.opengis.net/gml#VectorType"/>
   </owl:ObjectProperty>
   <owl:ObjectProperty rdf:about="http://www.opengis.net/gml#haspos">
      <rdfs:comment>Warning: This ObjectProperty reference was declared outside of its original schema. This ObjectProperty may be declared incorrectly.</rdfs:comment>
      <rdfs:domain rdf:resource="http://www.opengis.net/gml#ArcByCenterPointType"/>
      <rdfs:range rdf:resource="http://www.opengis.net/gml#pos"/>
   </owl:ObjectProperty>
   <owl:ObjectProperty rdf:about="http://www.opengis.net/gml#haspointProperty">
      <rdfs:comment>Warning: This ObjectProperty reference was declared outside of its original schema. This ObjectProperty may be declared incorrectly.</rdfs:comment>
      <rdfs:domain rdf:resource="http://www.opengis.net/gml#ArcByCenterPointType"/>
      <rdfs:range rdf:resource="http://www.opengis.net/gml#pointProperty"/>
   </owl:ObjectProperty>
   <owl:ObjectProperty rdf:about="http://www.opengis.net/gml#haspointRep">
      <rdfs:comment>Warning: This ObjectProperty reference was declared outside of its original schema. This ObjectProperty may be declared incorrectly.</rdfs:comment>
      <rdfs:domain rdf:resource="http://www.opengis.net/gml#ArcByCenterPointType"/>
      <rdfs:range rdf:resource="http://www.opengis.net/gml#pointRep"/>
   </owl:ObjectProperty>
   <owl:ObjectProperty rdf:about="http://www.opengis.net/gml#hasposList">
      <rdfs:comment>Warning: This ObjectProperty reference was declared outside of its original schema. This ObjectProperty may be declared incorrectly.</rdfs:comment>
      <rdfs:domain rdf:resource="http://www.opengis.net/gml#ArcByCenterPointType"/>
      <rdfs:range rdf:resource="http://www.opengis.net/gml#posList"/>
   </owl:ObjectProperty>
   <owl:ObjectProperty rdf:about="http://www.opengis.net/gml#hascoordinates">
      <rdfs:comment>Warning: This ObjectProperty reference was declared outside of its original schema. This ObjectProperty may be declared incorrectly.</rdfs:comment>
      <rdfs:domain rdf:resource="http://www.opengis.net/gml#ArcByCenterPointType"/>
      <rdfs:range rdf:resource="http://www.opengis.net/gml#coordinates"/>
   </owl:ObjectProperty>
   <owl:ObjectProperty rdf:about="http://www.opengis.net/gml#radius">
      <rdfs:domain rdf:resource="http://www.opengis.net/gml#ArcByCenterPointType"/>
      <rdfs:range rdf:resource="http://www.opengis.net/gml#LengthType"/>
   </owl:ObjectProperty>
   <owl:ObjectProperty rdf:about="http://www.opengis.net/gml#startAngle">
      <rdfs:domain rdf:resource="http://www.opengis.net/gml#ArcByCenterPointType"/>
      <rdfs:range rdf:resource="http://www.opengis.net/gml#AngleType"/>
   </owl:ObjectProperty>
   <owl:ObjectProperty rdf:about="http://www.opengis.net/gml#endAngle">
      <rdfs:domain rdf:resource="http://www.opengis.net/gml#ArcByCenterPointType"/>
      <rdfs:range rdf:resource="http://www.opengis.net/gml#AngleType"/>
   </owl:ObjectProperty>
   <owl:ObjectProperty rdf:about="http://www.opengis.net/gml#offsetBase">
      <rdfs:domain rdf:resource="http://www.opengis.net/gml#OffsetCurveType"/>
      <rdfs:range rdf:resource="http://www.opengis.net/gml#CurvePropertyType"/>
   </owl:ObjectProperty>
   <owl:ObjectProperty rdf:about="http://www.opengis.net/gml#distance">
      <rdfs:domain rdf:resource="http://www.opengis.net/gml#OffsetCurveType"/>
      <rdfs:range rdf:resource="http://www.opengis.net/gml#LengthType"/>
   </owl:ObjectProperty>
   <owl:ObjectProperty rdf:about="http://www.opengis.net/gml#refDirection">
      <rdfs:domain rdf:resource="http://www.opengis.net/gml#OffsetCurveType"/>
      <rdfs:range rdf:resource="http://www.opengis.net/gml#VectorType"/>
   </owl:ObjectProperty>
   <owl:ObjectProperty rdf:about="http://www.opengis.net/gml#location">
      <rdfs:domain rdf:resource="http://www.opengis.net/gml#AffinePlacementType"/>
      <rdfs:range rdf:resource="http://www.opengis.net/gml#DirectPositionType"/>
   </owl:ObjectProperty>
   <owl:ObjectProperty rdf:about="http://www.opengis.net/gml#refDirection">
      <rdfs:domain rdf:resource="http://www.opengis.net/gml#AffinePlacementType"/>
      <rdfs:range rdf:resource="http://www.opengis.net/gml#VectorType"/>
   </owl:ObjectProperty>
   <owl:DatatypeProperty rdf:about="http://www.opengis.net/gml#inDimension">
      <rdfs:domain rdf:resource="http://www.opengis.net/gml#AffinePlacementType"/>
      <rdfs:range rdf:resource="http://www.w3.org/2001/XMLSchema#positiveInteger"/>
   </owl:DatatypeProperty>
   <owl:DatatypeProperty rdf:about="http://www.opengis.net/gml#outDimension">
      <rdfs:domain rdf:resource="http://www.opengis.net/gml#AffinePlacementType"/>
      <rdfs:range rdf:resource="http://www.w3.org/2001/XMLSchema#positiveInteger"/>
   </owl:DatatypeProperty>
   <owl:ObjectProperty rdf:about="http://www.opengis.net/gml#hasrefLocation">
      <rdfs:domain rdf:resource="http://www.opengis.net/gml#ClothoidType"/>
      <rdfs:range rdf:resource="http://www.opengis.net/gml#refLocation"/>
   </owl:ObjectProperty>
   <owl:ObjectProperty rdf:about="http://www.opengis.net/gml#hasAffinePlacement">
      <rdfs:comment>Warning: This ObjectProperty reference was declared outside of its original schema. This ObjectProperty may be declared incorrectly.</rdfs:comment>
      <rdfs:domain rdf:resource="http://www.opengis.net/gml#ClothoidType"/>
      <rdfs:range rdf:resource="http://www.opengis.net/gml#AffinePlacement"/>
   </owl:ObjectProperty>
   <owl:DatatypeProperty rdf:about="http://www.opengis.net/gml#scaleFactor">
      <rdfs:domain rdf:resource="http://www.opengis.net/gml#ClothoidType"/>
      <rdfs:range rdf:resource="http://www.w3.org/2001/XMLSchema#decimal"/>
   </owl:DatatypeProperty>
   <owl:DatatypeProperty rdf:about="http://www.opengis.net/gml#startParameter">
      <rdfs:domain rdf:resource="http://www.opengis.net/gml#ClothoidType"/>
      <rdfs:range rdf:resource="http://www.w3.org/2001/XMLSchema#double"/>
   </owl:DatatypeProperty>
   <owl:DatatypeProperty rdf:about="http://www.opengis.net/gml#endParameter">
      <rdfs:domain rdf:resource="http://www.opengis.net/gml#ClothoidType"/>
      <rdfs:range rdf:resource="http://www.w3.org/2001/XMLSchema#double"/>
   </owl:DatatypeProperty>
   <owl:ObjectProperty rdf:about="http://www.opengis.net/gml#hasposList">
      <rdfs:comment>Warning: This ObjectProperty reference was declared outside of its original schema. This ObjectProperty may be declared incorrectly.</rdfs:comment>
      <rdfs:domain rdf:resource="http://www.opengis.net/gml#GeodesicStringType"/>
      <rdfs:range rdf:resource="http://www.opengis.net/gml#posList"/>
   </owl:ObjectProperty>
   <owl:ObjectProperty rdf:about="http://www.opengis.net/gml#haspos">
      <rdfs:comment>Warning: This ObjectProperty reference was declared outside of its original schema. This ObjectProperty may be declared incorrectly.</rdfs:comment>
      <rdfs:domain rdf:resource="http://www.opengis.net/gml#CubicSplineType"/>
      <rdfs:range rdf:resource="http://www.opengis.net/gml#pos"/>
   </owl:ObjectProperty>
   <owl:ObjectProperty rdf:about="http://www.opengis.net/gml#haspointProperty">
      <rdfs:comment>Warning: This ObjectProperty reference was declared outside of its original schema. This ObjectProperty may be declared incorrectly.</rdfs:comment>
      <rdfs:domain rdf:resource="http://www.opengis.net/gml#CubicSplineType"/>
      <rdfs:range rdf:resource="http://www.opengis.net/gml#pointProperty"/>
   </owl:ObjectProperty>
   <owl:ObjectProperty rdf:about="http://www.opengis.net/gml#haspointRep">
      <rdfs:comment>Warning: This ObjectProperty reference was declared outside of its original schema. This ObjectProperty may be declared incorrectly.</rdfs:comment>
      <rdfs:domain rdf:resource="http://www.opengis.net/gml#CubicSplineType"/>
      <rdfs:range rdf:resource="http://www.opengis.net/gml#pointRep"/>
   </owl:ObjectProperty>
   <owl:ObjectProperty rdf:about="http://www.opengis.net/gml#hasposList">
      <rdfs:comment>Warning: This ObjectProperty reference was declared outside of its original schema. This ObjectProperty may be declared incorrectly.</rdfs:comment>
      <rdfs:domain rdf:resource="http://www.opengis.net/gml#CubicSplineType"/>
      <rdfs:range rdf:resource="http://www.opengis.net/gml#posList"/>
   </owl:ObjectProperty>
   <owl:ObjectProperty rdf:about="http://www.opengis.net/gml#hascoordinates">
      <rdfs:comment>Warning: This ObjectProperty reference was declared outside of its original schema. This ObjectProperty may be declared incorrectly.</rdfs:comment>
      <rdfs:domain rdf:resource="http://www.opengis.net/gml#CubicSplineType"/>
      <rdfs:range rdf:resource="http://www.opengis.net/gml#coordinates"/>
   </owl:ObjectProperty>
   <owl:ObjectProperty rdf:about="http://www.opengis.net/gml#vectorAtStart">
      <rdfs:domain rdf:resource="http://www.opengis.net/gml#CubicSplineType"/>
      <rdfs:range rdf:resource="http://www.opengis.net/gml#VectorType"/>
   </owl:ObjectProperty>
   <owl:ObjectProperty rdf:about="http://www.opengis.net/gml#vectorAtEnd">
      <rdfs:domain rdf:resource="http://www.opengis.net/gml#CubicSplineType"/>
      <rdfs:range rdf:resource="http://www.opengis.net/gml#VectorType"/>
   </owl:ObjectProperty>
   <owl:DatatypeProperty rdf:about="http://www.opengis.net/gml#value">
      <rdfs:domain rdf:resource="http://www.opengis.net/gml#KnotType"/>
      <rdfs:range rdf:resource="http://www.w3.org/2001/XMLSchema#double"/>
   </owl:DatatypeProperty>
   <owl:DatatypeProperty rdf:about="http://www.opengis.net/gml#multiplicity">
      <rdfs:domain rdf:resource="http://www.opengis.net/gml#KnotType"/>
      <rdfs:range rdf:resource="http://www.w3.org/2001/XMLSchema#nonNegativeInteger"/>
   </owl:DatatypeProperty>
   <owl:DatatypeProperty rdf:about="http://www.opengis.net/gml#weight">
      <rdfs:domain rdf:resource="http://www.opengis.net/gml#KnotType"/>
      <rdfs:range rdf:resource="http://www.w3.org/2001/XMLSchema#double"/>
   </owl:DatatypeProperty>
   <owl:ObjectProperty rdf:about="http://www.opengis.net/gml#Knot">
      <rdfs:domain rdf:resource="http://www.opengis.net/gml#KnotPropertyType"/>
      <rdfs:range rdf:resource="http://www.opengis.net/gml#KnotType"/>
   </owl:ObjectProperty>
   <owl:ObjectProperty rdf:about="http://www.opengis.net/gml#haspos">
      <rdfs:comment>Warning: This ObjectProperty reference was declared outside of its original schema. This ObjectProperty may be declared incorrectly.</rdfs:comment>
      <rdfs:domain rdf:resource="http://www.opengis.net/gml#BSplineType"/>
      <rdfs:range rdf:resource="http://www.opengis.net/gml#pos"/>
   </owl:ObjectProperty>
   <owl:ObjectProperty rdf:about="http://www.opengis.net/gml#haspointProperty">
      <rdfs:comment>Warning: This ObjectProperty reference was declared outside of its original schema. This ObjectProperty may be declared incorrectly.</rdfs:comment>
      <rdfs:domain rdf:resource="http://www.opengis.net/gml#BSplineType"/>
      <rdfs:range rdf:resource="http://www.opengis.net/gml#pointProperty"/>
   </owl:ObjectProperty>
   <owl:ObjectProperty rdf:about="http://www.opengis.net/gml#haspointRep">
      <rdfs:comment>Warning: This ObjectProperty reference was declared outside of its original schema. This ObjectProperty may be declared incorrectly.</rdfs:comment>
      <rdfs:domain rdf:resource="http://www.opengis.net/gml#BSplineType"/>
      <rdfs:range rdf:resource="http://www.opengis.net/gml#pointRep"/>
   </owl:ObjectProperty>
   <owl:ObjectProperty rdf:about="http://www.opengis.net/gml#hasposList">
      <rdfs:comment>Warning: This ObjectProperty reference was declared outside of its original schema. This ObjectProperty may be declared incorrectly.</rdfs:comment>
      <rdfs:domain rdf:resource="http://www.opengis.net/gml#BSplineType"/>
      <rdfs:range rdf:resource="http://www.opengis.net/gml#posList"/>
   </owl:ObjectProperty>
   <owl:ObjectProperty rdf:about="http://www.opengis.net/gml#hascoordinates">
      <rdfs:comment>Warning: This ObjectProperty reference was declared outside of its original schema. This ObjectProperty may be declared incorrectly.</rdfs:comment>
      <rdfs:domain rdf:resource="http://www.opengis.net/gml#BSplineType"/>
      <rdfs:range rdf:resource="http://www.opengis.net/gml#coordinates"/>
   </owl:ObjectProperty>
   <owl:DatatypeProperty rdf:about="http://www.opengis.net/gml#degree">
      <rdfs:domain rdf:resource="http://www.opengis.net/gml#BSplineType"/>
      <rdfs:range rdf:resource="http://www.w3.org/2001/XMLSchema#nonNegativeInteger"/>
   </owl:DatatypeProperty>
   <owl:ObjectProperty rdf:about="http://www.opengis.net/gml#knot">
      <rdfs:domain rdf:resource="http://www.opengis.net/gml#BSplineType"/>
      <rdfs:range rdf:resource="http://www.opengis.net/gml#KnotPropertyType"/>
   </owl:ObjectProperty>
   <owl:ObjectProperty rdf:about="http://www.opengis.net/gml#haspos">
      <rdfs:comment>Warning: This ObjectProperty reference was declared outside of its original schema. This ObjectProperty may be declared incorrectly.</rdfs:comment>
      <rdfs:domain rdf:resource="http://www.opengis.net/gml#BezierType"/>
      <rdfs:range rdf:resource="http://www.opengis.net/gml#pos"/>
   </owl:ObjectProperty>
   <owl:ObjectProperty rdf:about="http://www.opengis.net/gml#haspointProperty">
      <rdfs:comment>Warning: This ObjectProperty reference was declared outside of its original schema. This ObjectProperty may be declared incorrectly.</rdfs:comment>
      <rdfs:domain rdf:resource="http://www.opengis.net/gml#BezierType"/>
      <rdfs:range rdf:resource="http://www.opengis.net/gml#pointProperty"/>
   </owl:ObjectProperty>
   <owl:ObjectProperty rdf:about="http://www.opengis.net/gml#haspointRep">
      <rdfs:comment>Warning: This ObjectProperty reference was declared outside of its original schema. This ObjectProperty may be declared incorrectly.</rdfs:comment>
      <rdfs:domain rdf:resource="http://www.opengis.net/gml#BezierType"/>
      <rdfs:range rdf:resource="http://www.opengis.net/gml#pointRep"/>
   </owl:ObjectProperty>
   <owl:ObjectProperty rdf:about="http://www.opengis.net/gml#hasposList">
      <rdfs:comment>Warning: This ObjectProperty reference was declared outside of its original schema. This ObjectProperty may be declared incorrectly.</rdfs:comment>
      <rdfs:domain rdf:resource="http://www.opengis.net/gml#BezierType"/>
      <rdfs:range rdf:resource="http://www.opengis.net/gml#posList"/>
   </owl:ObjectProperty>
   <owl:ObjectProperty rdf:about="http://www.opengis.net/gml#hascoordinates">
      <rdfs:comment>Warning: This ObjectProperty reference was declared outside of its original schema. This ObjectProperty may be declared incorrectly.</rdfs:comment>
      <rdfs:domain rdf:resource="http://www.opengis.net/gml#BezierType"/>
      <rdfs:range rdf:resource="http://www.opengis.net/gml#coordinates"/>
   </owl:ObjectProperty>
   <owl:DatatypeProperty rdf:about="http://www.opengis.net/gml#degree">
      <rdfs:domain rdf:resource="http://www.opengis.net/gml#BezierType"/>
      <rdfs:range rdf:resource="http://www.w3.org/2001/XMLSchema#nonNegativeInteger"/>
   </owl:DatatypeProperty>
   <owl:ObjectProperty rdf:about="http://www.opengis.net/gml#knot">
      <rdfs:domain rdf:resource="http://www.opengis.net/gml#BezierType"/>
      <rdfs:range rdf:resource="http://www.opengis.net/gml#KnotPropertyType"/>
   </owl:ObjectProperty>
   <owl:ObjectProperty rdf:about="http://www.opengis.net/gml#haspatches">
      <rdfs:comment>Warning: This ObjectProperty reference was declared outside of its original schema. This ObjectProperty may be declared incorrectly.</rdfs:comment>
      <rdfs:domain rdf:resource="http://www.opengis.net/gml#SurfaceType"/>
      <rdfs:range rdf:resource="http://www.opengis.net/gml#patches"/>
   </owl:ObjectProperty>
   <owl:ObjectProperty rdf:about="http://www.opengis.net/gml#hasbaseSurface">
      <rdfs:comment>Warning: This ObjectProperty reference was declared outside of its original schema. This ObjectProperty may be declared incorrectly.</rdfs:comment>
      <rdfs:domain rdf:resource="http://www.opengis.net/gml#OrientableSurfaceType"/>
      <rdfs:range rdf:resource="http://www.opengis.net/gml#baseSurface"/>
   </owl:ObjectProperty>
   <owl:ObjectProperty rdf:about="http://www.opengis.net/gml#has_SurfacePatch">
      <rdfs:comment>Warning: This ObjectProperty reference was declared outside of its original schema. This ObjectProperty may be declared incorrectly.</rdfs:comment>
      <rdfs:domain rdf:resource="http://www.opengis.net/gml#SurfacePatchArrayPropertyType"/>
      <rdfs:range rdf:resource="http://www.opengis.net/gml#_SurfacePatch"/>
   </owl:ObjectProperty>
   <owl:ObjectProperty rdf:about="http://www.opengis.net/gml#hasexterior">
      <rdfs:comment>Warning: This ObjectProperty reference was declared outside of its original schema. This ObjectProperty may be declared incorrectly.</rdfs:comment>
      <rdfs:domain rdf:resource="http://www.opengis.net/gml#PolygonPatchType"/>
      <rdfs:range rdf:resource="http://www.opengis.net/gml#exterior"/>
   </owl:ObjectProperty>
   <owl:ObjectProperty rdf:about="http://www.opengis.net/gml#hasinterior">
      <rdfs:comment>Warning: This ObjectProperty reference was declared outside of its original schema. This ObjectProperty may be declared incorrectly.</rdfs:comment>
      <rdfs:domain rdf:resource="http://www.opengis.net/gml#PolygonPatchType"/>
      <rdfs:range rdf:resource="http://www.opengis.net/gml#interior"/>
   </owl:ObjectProperty>
   <owl:ObjectProperty rdf:about="http://www.opengis.net/gml#hasexterior">
      <rdfs:comment>Warning: This ObjectProperty reference was declared outside of its original schema. This ObjectProperty may be declared incorrectly.</rdfs:comment>
      <rdfs:domain rdf:resource="http://www.opengis.net/gml#TriangleType"/>
      <rdfs:range rdf:resource="http://www.opengis.net/gml#exterior"/>
   </owl:ObjectProperty>
   <owl:ObjectProperty rdf:about="http://www.opengis.net/gml#hasexterior">
      <rdfs:comment>Warning: This ObjectProperty reference was declared outside of its original schema. This ObjectProperty may be declared incorrectly.</rdfs:comment>
      <rdfs:domain rdf:resource="http://www.opengis.net/gml#RectangleType"/>
      <rdfs:range rdf:resource="http://www.opengis.net/gml#exterior"/>
   </owl:ObjectProperty>
   <owl:ObjectProperty rdf:about="http://www.opengis.net/gml#hascurveMember">
      <rdfs:comment>Warning: This ObjectProperty reference was declared outside of its original schema. This ObjectProperty may be declared incorrectly.</rdfs:comment>
      <rdfs:domain rdf:resource="http://www.opengis.net/gml#RingType"/>
      <rdfs:range rdf:resource="http://www.opengis.net/gml#curveMember"/>
   </owl:ObjectProperty>
   <owl:ObjectProperty rdf:about="http://www.opengis.net/gml#hasRing">
      <rdfs:comment>Warning: This ObjectProperty reference was declared outside of its original schema. This ObjectProperty may be declared incorrectly.</rdfs:comment>
      <rdfs:domain rdf:resource="http://www.opengis.net/gml#RingPropertyType"/>
      <rdfs:range rdf:resource="http://www.opengis.net/gml#Ring"/>
   </owl:ObjectProperty>
   <owl:ObjectProperty rdf:about="http://www.opengis.net/gml#hasrow">
      <rdfs:domain rdf:resource="http://www.opengis.net/gml#PointGrid"/>
      <rdfs:range rdf:resource="http://www.opengis.net/gml#row"/>
   </owl:ObjectProperty>
   <owl:DatatypeProperty rdf:about="http://www.opengis.net/gml#rows">
      <rdfs:domain rdf:resource="http://www.opengis.net/gml#AbstractGriddedSurfaceType"/>
      <rdfs:range rdf:resource="http://www.w3.org/2001/XMLSchema#integer"/>
   </owl:DatatypeProperty>
   <owl:DatatypeProperty rdf:about="http://www.opengis.net/gml#columns">
      <rdfs:domain rdf:resource="http://www.opengis.net/gml#AbstractGriddedSurfaceType"/>
      <rdfs:range rdf:resource="http://www.w3.org/2001/XMLSchema#integer"/>
   </owl:DatatypeProperty>
   <owl:ObjectProperty rdf:about="http://www.opengis.net/gml#haspolygonPatches">
      <rdfs:comment>Warning: This ObjectProperty reference was declared outside of its original schema. This ObjectProperty may be declared incorrectly.</rdfs:comment>
      <rdfs:domain rdf:resource="http://www.opengis.net/gml#PolyhedralSurfaceType"/>
      <rdfs:range rdf:resource="http://www.opengis.net/gml#polygonPatches"/>
   </owl:ObjectProperty>
   <owl:ObjectProperty rdf:about="http://www.opengis.net/gml#hasPolygonPatch">
      <rdfs:comment>Warning: This ObjectProperty reference was declared outside of its original schema. This ObjectProperty may be declared incorrectly.</rdfs:comment>
      <rdfs:domain rdf:resource="http://www.opengis.net/gml#PolygonPatchArrayPropertyType"/>
      <rdfs:range rdf:resource="http://www.opengis.net/gml#PolygonPatch"/>
   </owl:ObjectProperty>
   <owl:ObjectProperty rdf:about="http://www.opengis.net/gml#hasTriangle">
      <rdfs:comment>Warning: This ObjectProperty reference was declared outside of its original schema. This ObjectProperty may be declared incorrectly.</rdfs:comment>
      <rdfs:domain rdf:resource="http://www.opengis.net/gml#TrianglePatchArrayPropertyType"/>
      <rdfs:range rdf:resource="http://www.opengis.net/gml#Triangle"/>
   </owl:ObjectProperty>
   <owl:ObjectProperty rdf:about="http://www.opengis.net/gml#hastrianglePatches">
      <rdfs:comment>Warning: This ObjectProperty reference was declared outside of its original schema. This ObjectProperty may be declared incorrectly.</rdfs:comment>
      <rdfs:domain rdf:resource="http://www.opengis.net/gml#TriangulatedSurfaceType"/>
      <rdfs:range rdf:resource="http://www.opengis.net/gml#trianglePatches"/>
   </owl:ObjectProperty>
   <owl:ObjectProperty rdf:about="http://www.opengis.net/gml#stopLines">
      <rdfs:domain rdf:resource="http://www.opengis.net/gml#TinType"/>
      <rdfs:range rdf:resource="http://www.opengis.net/gml#LineStringSegmentArrayPropertyType"/>
   </owl:ObjectProperty>
   <owl:ObjectProperty rdf:about="http://www.opengis.net/gml#breakLines">
      <rdfs:domain rdf:resource="http://www.opengis.net/gml#TinType"/>
      <rdfs:range rdf:resource="http://www.opengis.net/gml#LineStringSegmentArrayPropertyType"/>
   </owl:ObjectProperty>
   <owl:ObjectProperty rdf:about="http://www.opengis.net/gml#maxLength">
      <rdfs:domain rdf:resource="http://www.opengis.net/gml#TinType"/>
      <rdfs:range rdf:resource="http://www.opengis.net/gml#LengthType"/>
   </owl:ObjectProperty>
   <owl:ObjectProperty rdf:about="http://www.opengis.net/gml#hascontrolPoint">
      <rdfs:domain rdf:resource="http://www.opengis.net/gml#TinType"/>
      <rdfs:range rdf:resource="http://www.opengis.net/gml#controlPoint"/>
   </owl:ObjectProperty>
   <owl:ObjectProperty rdf:about="http://www.opengis.net/gml#hasposList">
      <rdfs:comment>Warning: This ObjectProperty reference was declared outside of its original schema. This ObjectProperty may be declared incorrectly.</rdfs:comment>
      <rdfs:domain rdf:resource="http://www.opengis.net/gml#TinType"/>
      <rdfs:range rdf:resource="http://www.opengis.net/gml#posList"/>
   </owl:ObjectProperty>
   <owl:ObjectProperty rdf:about="http://www.opengis.net/gml#hasLineStringSegment">
      <rdfs:comment>Warning: This ObjectProperty reference was declared outside of its original schema. This ObjectProperty may be declared incorrectly.</rdfs:comment>
      <rdfs:domain rdf:resource="http://www.opengis.net/gml#LineStringSegmentArrayPropertyType"/>
      <rdfs:range rdf:resource="http://www.opengis.net/gml#LineStringSegment"/>
   </owl:ObjectProperty>
   <owl:ObjectProperty rdf:about="http://www.opengis.net/gml#has_Solid">
      <rdfs:comment>Warning: This ObjectProperty reference was declared outside of its original schema. This ObjectProperty may be declared incorrectly.</rdfs:comment>
      <rdfs:domain rdf:resource="http://www.opengis.net/gml#SolidPropertyType"/>
      <rdfs:range rdf:resource="http://www.opengis.net/gml#_Solid"/>
   </owl:ObjectProperty>
   <owl:ObjectProperty rdf:about="http://www.opengis.net/gml#has_Solid">
      <rdfs:comment>Warning: This ObjectProperty reference was declared outside of its original schema. This ObjectProperty may be declared incorrectly.</rdfs:comment>
      <rdfs:domain rdf:resource="http://www.opengis.net/gml#SolidArrayPropertyType"/>
      <rdfs:range rdf:resource="http://www.opengis.net/gml#_Solid"/>
   </owl:ObjectProperty>
   <owl:ObjectProperty rdf:about="http://www.opengis.net/gml#exterior">
      <rdfs:domain rdf:resource="http://www.opengis.net/gml#SolidType"/>
      <rdfs:range rdf:resource="http://www.opengis.net/gml#SurfacePropertyType"/>
   </owl:ObjectProperty>
   <owl:ObjectProperty rdf:about="http://www.opengis.net/gml#interior">
      <rdfs:domain rdf:resource="http://www.opengis.net/gml#SolidType"/>
      <rdfs:range rdf:resource="http://www.opengis.net/gml#SurfacePropertyType"/>
   </owl:ObjectProperty>
   <owl:ObjectProperty rdf:about="http://www.opengis.net/gml#hasdomainSet">
      <rdfs:comment>Warning: This ObjectProperty reference was declared outside of its original schema. This ObjectProperty may be declared incorrectly.</rdfs:comment>
      <rdfs:domain rdf:resource="http://www.opengis.net/gml#AbstractCoverageType"/>
      <rdfs:range rdf:resource="http://www.opengis.net/gml#domainSet"/>
   </owl:ObjectProperty>
   <owl:ObjectProperty rdf:about="http://www.opengis.net/gml#hasrangeSet">
      <rdfs:comment>Warning: This ObjectProperty reference was declared outside of its original schema. This ObjectProperty may be declared incorrectly.</rdfs:comment>
      <rdfs:domain rdf:resource="http://www.opengis.net/gml#AbstractCoverageType"/>
      <rdfs:range rdf:resource="http://www.opengis.net/gml#rangeSet"/>
   </owl:ObjectProperty>
   <owl:ObjectProperty rdf:about="http://www.opengis.net/gml#hascoverageFunction">
      <rdfs:comment>Warning: This ObjectProperty reference was declared outside of its original schema. This ObjectProperty may be declared incorrectly.</rdfs:comment>
      <rdfs:domain rdf:resource="http://www.opengis.net/gml#AbstractContinuousCoverageType"/>
      <rdfs:range rdf:resource="http://www.opengis.net/gml#coverageFunction"/>
   </owl:ObjectProperty>
   <owl:ObjectProperty rdf:about="http://www.opengis.net/gml#hascoverageFunction">
      <rdfs:comment>Warning: This ObjectProperty reference was declared outside of its original schema. This ObjectProperty may be declared incorrectly.</rdfs:comment>
      <rdfs:domain rdf:resource="http://www.opengis.net/gml#AbstractDiscreteCoverageType"/>
      <rdfs:range rdf:resource="http://www.opengis.net/gml#coverageFunction"/>
   </owl:ObjectProperty>
   <owl:ObjectProperty rdf:about="http://www.opengis.net/gml#has_Geometry">
      <rdfs:comment>Warning: This ObjectProperty reference was declared outside of its original schema. This ObjectProperty may be declared incorrectly.</rdfs:comment>
      <rdfs:domain rdf:resource="http://www.opengis.net/gml#DomainSetType"/>
      <rdfs:range rdf:resource="http://www.opengis.net/gml#_Geometry"/>
   </owl:ObjectProperty>
   <owl:ObjectProperty rdf:about="http://www.opengis.net/gml#has_TimeObject">
      <rdfs:comment>Warning: This ObjectProperty reference was declared outside of its original schema. This ObjectProperty may be declared incorrectly.</rdfs:comment>
      <rdfs:domain rdf:resource="http://www.opengis.net/gml#DomainSetType"/>
      <rdfs:range rdf:resource="http://www.opengis.net/gml#_TimeObject"/>
   </owl:ObjectProperty>
   <owl:ObjectProperty rdf:about="http://www.opengis.net/gml#hasValueArray">
      <rdfs:comment>Warning: This ObjectProperty reference was declared outside of its original schema. This ObjectProperty may be declared incorrectly.</rdfs:comment>
      <rdfs:domain rdf:resource="http://www.opengis.net/gml#RangeSetType"/>
      <rdfs:range rdf:resource="http://www.opengis.net/gml#ValueArray"/>
   </owl:ObjectProperty>
   <owl:ObjectProperty rdf:about="http://www.opengis.net/gml#hasDataBlock">
      <rdfs:comment>Warning: This ObjectProperty reference was declared outside of its original schema. This ObjectProperty may be declared incorrectly.</rdfs:comment>
      <rdfs:domain rdf:resource="http://www.opengis.net/gml#RangeSetType"/>
      <rdfs:range rdf:resource="http://www.opengis.net/gml#DataBlock"/>
   </owl:ObjectProperty>
   <owl:ObjectProperty rdf:about="http://www.opengis.net/gml#hasFile">
      <rdfs:comment>Warning: This ObjectProperty reference was declared outside of its original schema. This ObjectProperty may be declared incorrectly.</rdfs:comment>
      <rdfs:domain rdf:resource="http://www.opengis.net/gml#RangeSetType"/>
      <rdfs:range rdf:resource="http://www.opengis.net/gml#File"/>
   </owl:ObjectProperty>
   <owl:ObjectProperty rdf:about="http://www.opengis.net/gml#hasMappingRule">
      <rdfs:comment>Warning: This ObjectProperty reference was declared outside of its original schema. This ObjectProperty may be declared incorrectly.</rdfs:comment>
      <rdfs:domain rdf:resource="http://www.opengis.net/gml#CoverageFunctionType"/>
      <rdfs:range rdf:resource="http://www.opengis.net/gml#MappingRule"/>
   </owl:ObjectProperty>
   <owl:ObjectProperty rdf:about="http://www.opengis.net/gml#hasGridFunction">
      <rdfs:comment>Warning: This ObjectProperty reference was declared outside of its original schema. This ObjectProperty may be declared incorrectly.</rdfs:comment>
      <rdfs:domain rdf:resource="http://www.opengis.net/gml#CoverageFunctionType"/>
      <rdfs:range rdf:resource="http://www.opengis.net/gml#GridFunction"/>
   </owl:ObjectProperty>
   <owl:ObjectProperty rdf:about="http://www.opengis.net/gml#hasrangeParameters">
      <rdfs:comment>Warning: This ObjectProperty reference was declared outside of its original schema. This ObjectProperty may be declared incorrectly.</rdfs:comment>
      <rdfs:domain rdf:resource="http://www.opengis.net/gml#DataBlockType"/>
      <rdfs:range rdf:resource="http://www.opengis.net/gml#rangeParameters"/>
   </owl:ObjectProperty>
   <owl:ObjectProperty rdf:about="http://www.opengis.net/gml#hastupleList">
      <rdfs:comment>Warning: This ObjectProperty reference was declared outside of its original schema. This ObjectProperty may be declared incorrectly.</rdfs:comment>
      <rdfs:domain rdf:resource="http://www.opengis.net/gml#DataBlockType"/>
      <rdfs:range rdf:resource="http://www.opengis.net/gml#tupleList"/>
   </owl:ObjectProperty>
   <owl:ObjectProperty rdf:about="http://www.opengis.net/gml#hasdoubleOrNullTupleList">
      <rdfs:comment>Warning: This ObjectProperty reference was declared outside of its original schema. This ObjectProperty may be declared incorrectly.</rdfs:comment>
      <rdfs:domain rdf:resource="http://www.opengis.net/gml#DataBlockType"/>
      <rdfs:range rdf:resource="http://www.opengis.net/gml#doubleOrNullTupleList"/>
   </owl:ObjectProperty>
   <owl:ObjectProperty rdf:about="http://www.opengis.net/gml#hasrangeParameters">
      <rdfs:comment>Warning: This ObjectProperty reference was declared outside of its original schema. This ObjectProperty may be declared incorrectly.</rdfs:comment>
      <rdfs:domain rdf:resource="http://www.opengis.net/gml#FileType"/>
      <rdfs:range rdf:resource="http://www.opengis.net/gml#rangeParameters"/>
   </owl:ObjectProperty>
   <owl:DatatypeProperty rdf:about="http://www.opengis.net/gml#fileName">
      <rdfs:domain rdf:resource="http://www.opengis.net/gml#FileType"/>
      <rdfs:range rdf:resource="http://www.w3.org/2001/XMLSchema#anyURI"/>
   </owl:DatatypeProperty>
   <owl:DatatypeProperty rdf:about="http://www.opengis.net/gml#fileStructure">
      <rdfs:domain rdf:resource="http://www.opengis.net/gml#FileType"/>
      <rdfs:range rdf:resource="http://www.opengis.net/gml#FileValueModelType"/>
   </owl:DatatypeProperty>
   <owl:DatatypeProperty rdf:about="http://www.opengis.net/gml#mimeType">
      <rdfs:domain rdf:resource="http://www.opengis.net/gml#FileType"/>
      <rdfs:range rdf:resource="http://www.w3.org/2001/XMLSchema#anyURI"/>
   </owl:DatatypeProperty>
   <owl:DatatypeProperty rdf:about="http://www.opengis.net/gml#compression">
      <rdfs:domain rdf:resource="http://www.opengis.net/gml#FileType"/>
      <rdfs:range rdf:resource="http://www.w3.org/2001/XMLSchema#anyURI"/>
   </owl:DatatypeProperty>
   <owl:ObjectProperty rdf:about="http://www.opengis.net/gml#sequenceRule">
      <rdfs:domain rdf:resource="http://www.opengis.net/gml#GridFunctionType"/>
      <rdfs:range rdf:resource="http://www.opengis.net/gml#SequenceRuleType"/>
   </owl:ObjectProperty>
   <owl:DatatypeProperty rdf:about="http://www.opengis.net/gml#startPoint">
      <rdfs:domain rdf:resource="http://www.opengis.net/gml#GridFunctionType"/>
      <rdfs:range rdf:resource="http://www.opengis.net/gml#integerList"/>
   </owl:DatatypeProperty>
   <owl:DatatypeProperty rdf:about="http://www.opengis.net/gml#lookUpTable">
      <rdfs:domain rdf:resource="http://www.opengis.net/gml#IndexMapType"/>
      <rdfs:range rdf:resource="http://www.opengis.net/gml#integerList"/>
   </owl:DatatypeProperty>
   <owl:ObjectProperty rdf:about="http://www.opengis.net/gml#hasboundedBy">
      <rdfs:comment>Warning: This ObjectProperty reference was declared outside of its original schema. This ObjectProperty may be declared incorrectly.</rdfs:comment>
      <rdfs:domain rdf:resource="http://www.opengis.net/gml#MultiPointCoverageType"/>
      <rdfs:range rdf:resource="http://www.opengis.net/gml#boundedBy"/>
   </owl:ObjectProperty>
   <owl:ObjectProperty rdf:about="http://www.opengis.net/gml#hasmultiPointDomain">
      <rdfs:comment>Warning: This ObjectProperty reference was declared outside of its original schema. This ObjectProperty may be declared incorrectly.</rdfs:comment>
      <rdfs:domain rdf:resource="http://www.opengis.net/gml#MultiPointCoverageType"/>
      <rdfs:range rdf:resource="http://www.opengis.net/gml#multiPointDomain"/>
   </owl:ObjectProperty>
   <owl:ObjectProperty rdf:about="http://www.opengis.net/gml#hasrangeSet">
      <rdfs:comment>Warning: This ObjectProperty reference was declared outside of its original schema. This ObjectProperty may be declared incorrectly.</rdfs:comment>
      <rdfs:domain rdf:resource="http://www.opengis.net/gml#MultiPointCoverageType"/>
      <rdfs:range rdf:resource="http://www.opengis.net/gml#rangeSet"/>
   </owl:ObjectProperty>
   <owl:ObjectProperty rdf:about="http://www.opengis.net/gml#hascoverageFunction">
      <rdfs:comment>Warning: This ObjectProperty reference was declared outside of its original schema. This ObjectProperty may be declared incorrectly.</rdfs:comment>
      <rdfs:domain rdf:resource="http://www.opengis.net/gml#MultiPointCoverageType"/>
      <rdfs:range rdf:resource="http://www.opengis.net/gml#coverageFunction"/>
   </owl:ObjectProperty>
   <owl:ObjectProperty rdf:about="http://www.opengis.net/gml#hasMultiPoint">
      <rdfs:comment>Warning: This ObjectProperty reference was declared outside of its original schema. This ObjectProperty may be declared incorrectly.</rdfs:comment>
      <rdfs:domain rdf:resource="http://www.opengis.net/gml#MultiPointDomainType"/>
      <rdfs:range rdf:resource="http://www.opengis.net/gml#MultiPoint"/>
   </owl:ObjectProperty>
   <owl:ObjectProperty rdf:about="http://www.opengis.net/gml#hasboundedBy">
      <rdfs:comment>Warning: This ObjectProperty reference was declared outside of its original schema. This ObjectProperty may be declared incorrectly.</rdfs:comment>
      <rdfs:domain rdf:resource="http://www.opengis.net/gml#MultiCurveCoverageType"/>
      <rdfs:range rdf:resource="http://www.opengis.net/gml#boundedBy"/>
   </owl:ObjectProperty>
   <owl:ObjectProperty rdf:about="http://www.opengis.net/gml#hasmultiCurveDomain">
      <rdfs:comment>Warning: This ObjectProperty reference was declared outside of its original schema. This ObjectProperty may be declared incorrectly.</rdfs:comment>
      <rdfs:domain rdf:resource="http://www.opengis.net/gml#MultiCurveCoverageType"/>
      <rdfs:range rdf:resource="http://www.opengis.net/gml#multiCurveDomain"/>
   </owl:ObjectProperty>
   <owl:ObjectProperty rdf:about="http://www.opengis.net/gml#hasrangeSet">
      <rdfs:comment>Warning: This ObjectProperty reference was declared outside of its original schema. This ObjectProperty may be declared incorrectly.</rdfs:comment>
      <rdfs:domain rdf:resource="http://www.opengis.net/gml#MultiCurveCoverageType"/>
      <rdfs:range rdf:resource="http://www.opengis.net/gml#rangeSet"/>
   </owl:ObjectProperty>
   <owl:ObjectProperty rdf:about="http://www.opengis.net/gml#hascoverageFunction">
      <rdfs:comment>Warning: This ObjectProperty reference was declared outside of its original schema. This ObjectProperty may be declared incorrectly.</rdfs:comment>
      <rdfs:domain rdf:resource="http://www.opengis.net/gml#MultiCurveCoverageType"/>
      <rdfs:range rdf:resource="http://www.opengis.net/gml#coverageFunction"/>
   </owl:ObjectProperty>
   <owl:ObjectProperty rdf:about="http://www.opengis.net/gml#hasMultiCurve">
      <rdfs:comment>Warning: This ObjectProperty reference was declared outside of its original schema. This ObjectProperty may be declared incorrectly.</rdfs:comment>
      <rdfs:domain rdf:resource="http://www.opengis.net/gml#MultiCurveDomainType"/>
      <rdfs:range rdf:resource="http://www.opengis.net/gml#MultiCurve"/>
   </owl:ObjectProperty>
   <owl:ObjectProperty rdf:about="http://www.opengis.net/gml#hasboundedBy">
      <rdfs:comment>Warning: This ObjectProperty reference was declared outside of its original schema. This ObjectProperty may be declared incorrectly.</rdfs:comment>
      <rdfs:domain rdf:resource="http://www.opengis.net/gml#MultiSurfaceCoverageType"/>
      <rdfs:range rdf:resource="http://www.opengis.net/gml#boundedBy"/>
   </owl:ObjectProperty>
   <owl:ObjectProperty rdf:about="http://www.opengis.net/gml#hasmultiSurfaceDomain">
      <rdfs:comment>Warning: This ObjectProperty reference was declared outside of its original schema. This ObjectProperty may be declared incorrectly.</rdfs:comment>
      <rdfs:domain rdf:resource="http://www.opengis.net/gml#MultiSurfaceCoverageType"/>
      <rdfs:range rdf:resource="http://www.opengis.net/gml#multiSurfaceDomain"/>
   </owl:ObjectProperty>
   <owl:ObjectProperty rdf:about="http://www.opengis.net/gml#hasrangeSet">
      <rdfs:comment>Warning: This ObjectProperty reference was declared outside of its original schema. This ObjectProperty may be declared incorrectly.</rdfs:comment>
      <rdfs:domain rdf:resource="http://www.opengis.net/gml#MultiSurfaceCoverageType"/>
      <rdfs:range rdf:resource="http://www.opengis.net/gml#rangeSet"/>
   </owl:ObjectProperty>
   <owl:ObjectProperty rdf:about="http://www.opengis.net/gml#hascoverageFunction">
      <rdfs:comment>Warning: This ObjectProperty reference was declared outside of its original schema. This ObjectProperty may be declared incorrectly.</rdfs:comment>
      <rdfs:domain rdf:resource="http://www.opengis.net/gml#MultiSurfaceCoverageType"/>
      <rdfs:range rdf:resource="http://www.opengis.net/gml#coverageFunction"/>
   </owl:ObjectProperty>
   <owl:ObjectProperty rdf:about="http://www.opengis.net/gml#hasMultiSurface">
      <rdfs:comment>Warning: This ObjectProperty reference was declared outside of its original schema. This ObjectProperty may be declared incorrectly.</rdfs:comment>
      <rdfs:domain rdf:resource="http://www.opengis.net/gml#MultiSurfaceDomainType"/>
      <rdfs:range rdf:resource="http://www.opengis.net/gml#MultiSurface"/>
   </owl:ObjectProperty>
   <owl:ObjectProperty rdf:about="http://www.opengis.net/gml#hasboundedBy">
      <rdfs:comment>Warning: This ObjectProperty reference was declared outside of its original schema. This ObjectProperty may be declared incorrectly.</rdfs:comment>
      <rdfs:domain rdf:resource="http://www.opengis.net/gml#MultiSolidCoverageType"/>
      <rdfs:range rdf:resource="http://www.opengis.net/gml#boundedBy"/>
   </owl:ObjectProperty>
   <owl:ObjectProperty rdf:about="http://www.opengis.net/gml#hasmultiSolidDomain">
      <rdfs:comment>Warning: This ObjectProperty reference was declared outside of its original schema. This ObjectProperty may be declared incorrectly.</rdfs:comment>
      <rdfs:domain rdf:resource="http://www.opengis.net/gml#MultiSolidCoverageType"/>
      <rdfs:range rdf:resource="http://www.opengis.net/gml#multiSolidDomain"/>
   </owl:ObjectProperty>
   <owl:ObjectProperty rdf:about="http://www.opengis.net/gml#hasrangeSet">
      <rdfs:comment>Warning: This ObjectProperty reference was declared outside of its original schema. This ObjectProperty may be declared incorrectly.</rdfs:comment>
      <rdfs:domain rdf:resource="http://www.opengis.net/gml#MultiSolidCoverageType"/>
      <rdfs:range rdf:resource="http://www.opengis.net/gml#rangeSet"/>
   </owl:ObjectProperty>
   <owl:ObjectProperty rdf:about="http://www.opengis.net/gml#hascoverageFunction">
      <rdfs:comment>Warning: This ObjectProperty reference was declared outside of its original schema. This ObjectProperty may be declared incorrectly.</rdfs:comment>
      <rdfs:domain rdf:resource="http://www.opengis.net/gml#MultiSolidCoverageType"/>
      <rdfs:range rdf:resource="http://www.opengis.net/gml#coverageFunction"/>
   </owl:ObjectProperty>
   <owl:ObjectProperty rdf:about="http://www.opengis.net/gml#hasMultiSolid">
      <rdfs:comment>Warning: This ObjectProperty reference was declared outside of its original schema. This ObjectProperty may be declared incorrectly.</rdfs:comment>
      <rdfs:domain rdf:resource="http://www.opengis.net/gml#MultiSolidDomainType"/>
      <rdfs:range rdf:resource="http://www.opengis.net/gml#MultiSolid"/>
   </owl:ObjectProperty>
   <owl:ObjectProperty rdf:about="http://www.opengis.net/gml#hasboundedBy">
      <rdfs:comment>Warning: This ObjectProperty reference was declared outside of its original schema. This ObjectProperty may be declared incorrectly.</rdfs:comment>
      <rdfs:domain rdf:resource="http://www.opengis.net/gml#GridCoverageType"/>
      <rdfs:range rdf:resource="http://www.opengis.net/gml#boundedBy"/>
   </owl:ObjectProperty>
   <owl:ObjectProperty rdf:about="http://www.opengis.net/gml#hasgridDomain">
      <rdfs:comment>Warning: This ObjectProperty reference was declared outside of its original schema. This ObjectProperty may be declared incorrectly.</rdfs:comment>
      <rdfs:domain rdf:resource="http://www.opengis.net/gml#GridCoverageType"/>
      <rdfs:range rdf:resource="http://www.opengis.net/gml#gridDomain"/>
   </owl:ObjectProperty>
   <owl:ObjectProperty rdf:about="http://www.opengis.net/gml#hasrangeSet">
      <rdfs:comment>Warning: This ObjectProperty reference was declared outside of its original schema. This ObjectProperty may be declared incorrectly.</rdfs:comment>
      <rdfs:domain rdf:resource="http://www.opengis.net/gml#GridCoverageType"/>
      <rdfs:range rdf:resource="http://www.opengis.net/gml#rangeSet"/>
   </owl:ObjectProperty>
   <owl:ObjectProperty rdf:about="http://www.opengis.net/gml#hascoverageFunction">
      <rdfs:comment>Warning: This ObjectProperty reference was declared outside of its original schema. This ObjectProperty may be declared incorrectly.</rdfs:comment>
      <rdfs:domain rdf:resource="http://www.opengis.net/gml#GridCoverageType"/>
      <rdfs:range rdf:resource="http://www.opengis.net/gml#coverageFunction"/>
   </owl:ObjectProperty>
   <owl:ObjectProperty rdf:about="http://www.opengis.net/gml#hasGrid">
      <rdfs:comment>Warning: This ObjectProperty reference was declared outside of its original schema. This ObjectProperty may be declared incorrectly.</rdfs:comment>
      <rdfs:domain rdf:resource="http://www.opengis.net/gml#GridDomainType"/>
      <rdfs:range rdf:resource="http://www.opengis.net/gml#Grid"/>
   </owl:ObjectProperty>
   <owl:ObjectProperty rdf:about="http://www.opengis.net/gml#hasboundedBy">
      <rdfs:comment>Warning: This ObjectProperty reference was declared outside of its original schema. This ObjectProperty may be declared incorrectly.</rdfs:comment>
      <rdfs:domain rdf:resource="http://www.opengis.net/gml#RectifiedGridCoverageType"/>
      <rdfs:range rdf:resource="http://www.opengis.net/gml#boundedBy"/>
   </owl:ObjectProperty>
   <owl:ObjectProperty rdf:about="http://www.opengis.net/gml#hasrectifiedGridDomain">
      <rdfs:comment>Warning: This ObjectProperty reference was declared outside of its original schema. This ObjectProperty may be declared incorrectly.</rdfs:comment>
      <rdfs:domain rdf:resource="http://www.opengis.net/gml#RectifiedGridCoverageType"/>
      <rdfs:range rdf:resource="http://www.opengis.net/gml#rectifiedGridDomain"/>
   </owl:ObjectProperty>
   <owl:ObjectProperty rdf:about="http://www.opengis.net/gml#hasrangeSet">
      <rdfs:comment>Warning: This ObjectProperty reference was declared outside of its original schema. This ObjectProperty may be declared incorrectly.</rdfs:comment>
      <rdfs:domain rdf:resource="http://www.opengis.net/gml#RectifiedGridCoverageType"/>
      <rdfs:range rdf:resource="http://www.opengis.net/gml#rangeSet"/>
   </owl:ObjectProperty>
   <owl:ObjectProperty rdf:about="http://www.opengis.net/gml#hascoverageFunction">
      <rdfs:comment>Warning: This ObjectProperty reference was declared outside of its original schema. This ObjectProperty may be declared incorrectly.</rdfs:comment>
      <rdfs:domain rdf:resource="http://www.opengis.net/gml#RectifiedGridCoverageType"/>
      <rdfs:range rdf:resource="http://www.opengis.net/gml#coverageFunction"/>
   </owl:ObjectProperty>
   <owl:ObjectProperty rdf:about="http://www.opengis.net/gml#hasRectifiedGrid">
      <rdfs:comment>Warning: This ObjectProperty reference was declared outside of its original schema. This ObjectProperty may be declared incorrectly.</rdfs:comment>
      <rdfs:domain rdf:resource="http://www.opengis.net/gml#RectifiedGridDomainType"/>
      <rdfs:range rdf:resource="http://www.opengis.net/gml#RectifiedGrid"/>
   </owl:ObjectProperty>
   <owl:ObjectProperty rdf:about="http://www.opengis.net/gml#has_Object">
      <rdfs:comment>Warning: This ObjectProperty reference was declared outside of its original schema. This ObjectProperty may be declared incorrectly.</rdfs:comment>
      <rdfs:domain rdf:resource="http://www.opengis.net/gml#Value"/>
      <rdfs:range rdf:resource="http://www.opengis.net/gml#_Object"/>
   </owl:ObjectProperty>
   <owl:ObjectProperty rdf:about="http://www.opengis.net/gml#hasNull">
      <rdfs:comment>Warning: This ObjectProperty reference was declared outside of its original schema. This ObjectProperty may be declared incorrectly.</rdfs:comment>
      <rdfs:domain rdf:resource="http://www.opengis.net/gml#Value"/>
      <rdfs:range rdf:resource="http://www.opengis.net/gml#Null"/>
   </owl:ObjectProperty>
   <owl:ObjectProperty rdf:about="http://www.opengis.net/gml#hasCompositeValue">
      <rdfs:comment>Warning: This ObjectProperty reference was declared outside of its original schema. This ObjectProperty may be declared incorrectly.</rdfs:comment>
      <rdfs:domain rdf:resource="http://www.opengis.net/gml#ValueObject"/>
      <rdfs:range rdf:resource="http://www.opengis.net/gml#CompositeValue"/>
   </owl:ObjectProperty>
   <owl:ObjectProperty rdf:about="http://www.opengis.net/gml#hasBoolean">
      <rdfs:comment>Warning: This ObjectProperty reference was declared outside of its original schema. This ObjectProperty may be declared incorrectly.</rdfs:comment>
      <rdfs:domain rdf:resource="http://www.opengis.net/gml#ScalarValue"/>
      <rdfs:range rdf:resource="http://www.opengis.net/gml#Boolean"/>
   </owl:ObjectProperty>
   <owl:ObjectProperty rdf:about="http://www.opengis.net/gml#hasCategory">
      <rdfs:comment>Warning: This ObjectProperty reference was declared outside of its original schema. This ObjectProperty may be declared incorrectly.</rdfs:comment>
      <rdfs:domain rdf:resource="http://www.opengis.net/gml#ScalarValue"/>
      <rdfs:range rdf:resource="http://www.opengis.net/gml#Category"/>
   </owl:ObjectProperty>
   <owl:ObjectProperty rdf:about="http://www.opengis.net/gml#hasQuantity">
      <rdfs:comment>Warning: This ObjectProperty reference was declared outside of its original schema. This ObjectProperty may be declared incorrectly.</rdfs:comment>
      <rdfs:domain rdf:resource="http://www.opengis.net/gml#ScalarValue"/>
      <rdfs:range rdf:resource="http://www.opengis.net/gml#Quantity"/>
   </owl:ObjectProperty>
   <owl:ObjectProperty rdf:about="http://www.opengis.net/gml#hasCount">
      <rdfs:comment>Warning: This ObjectProperty reference was declared outside of its original schema. This ObjectProperty may be declared incorrectly.</rdfs:comment>
      <rdfs:domain rdf:resource="http://www.opengis.net/gml#ScalarValue"/>
      <rdfs:range rdf:resource="http://www.opengis.net/gml#Count"/>
   </owl:ObjectProperty>
   <owl:ObjectProperty rdf:about="http://www.opengis.net/gml#hasBooleanList">
      <rdfs:comment>Warning: This ObjectProperty reference was declared outside of its original schema. This ObjectProperty may be declared incorrectly.</rdfs:comment>
      <rdfs:domain rdf:resource="http://www.opengis.net/gml#ScalarValueList"/>
      <rdfs:range rdf:resource="http://www.opengis.net/gml#BooleanList"/>
   </owl:ObjectProperty>
   <owl:ObjectProperty rdf:about="http://www.opengis.net/gml#hasCategoryList">
      <rdfs:comment>Warning: This ObjectProperty reference was declared outside of its original schema. This ObjectProperty may be declared incorrectly.</rdfs:comment>
      <rdfs:domain rdf:resource="http://www.opengis.net/gml#ScalarValueList"/>
      <rdfs:range rdf:resource="http://www.opengis.net/gml#CategoryList"/>
   </owl:ObjectProperty>
   <owl:ObjectProperty rdf:about="http://www.opengis.net/gml#hasQuantityList">
      <rdfs:comment>Warning: This ObjectProperty reference was declared outside of its original schema. This ObjectProperty may be declared incorrectly.</rdfs:comment>
      <rdfs:domain rdf:resource="http://www.opengis.net/gml#ScalarValueList"/>
      <rdfs:range rdf:resource="http://www.opengis.net/gml#QuantityList"/>
   </owl:ObjectProperty>
   <owl:ObjectProperty rdf:about="http://www.opengis.net/gml#hasCountList">
      <rdfs:comment>Warning: This ObjectProperty reference was declared outside of its original schema. This ObjectProperty may be declared incorrectly.</rdfs:comment>
      <rdfs:domain rdf:resource="http://www.opengis.net/gml#ScalarValueList"/>
      <rdfs:range rdf:resource="http://www.opengis.net/gml#CountList"/>
   </owl:ObjectProperty>
   <owl:ObjectProperty rdf:about="http://www.opengis.net/gml#hasvalueComponent">
      <rdfs:comment>Warning: This ObjectProperty reference was declared outside of its original schema. This ObjectProperty may be declared incorrectly.</rdfs:comment>
      <rdfs:domain rdf:resource="http://www.opengis.net/gml#CompositeValueType"/>
      <rdfs:range rdf:resource="http://www.opengis.net/gml#valueComponent"/>
   </owl:ObjectProperty>
   <owl:ObjectProperty rdf:about="http://www.opengis.net/gml#hasvalueComponents">
      <rdfs:comment>Warning: This ObjectProperty reference was declared outside of its original schema. This ObjectProperty may be declared incorrectly.</rdfs:comment>
      <rdfs:domain rdf:resource="http://www.opengis.net/gml#CompositeValueType"/>
      <rdfs:range rdf:resource="http://www.opengis.net/gml#valueComponents"/>
   </owl:ObjectProperty>
   <owl:ObjectProperty rdf:about="http://www.opengis.net/gml#hasCategoryExtent">
      <rdfs:comment>Warning: This ObjectProperty reference was declared outside of its original schema. This ObjectProperty may be declared incorrectly.</rdfs:comment>
      <rdfs:domain rdf:resource="http://www.opengis.net/gml#ValueExtent"/>
      <rdfs:range rdf:resource="http://www.opengis.net/gml#CategoryExtent"/>
   </owl:ObjectProperty>
   <owl:ObjectProperty rdf:about="http://www.opengis.net/gml#hasQuantityExtent">
      <rdfs:comment>Warning: This ObjectProperty reference was declared outside of its original schema. This ObjectProperty may be declared incorrectly.</rdfs:comment>
      <rdfs:domain rdf:resource="http://www.opengis.net/gml#ValueExtent"/>
      <rdfs:range rdf:resource="http://www.opengis.net/gml#QuantityExtent"/>
   </owl:ObjectProperty>
   <owl:ObjectProperty rdf:about="http://www.opengis.net/gml#hasCountExtent">
      <rdfs:comment>Warning: This ObjectProperty reference was declared outside of its original schema. This ObjectProperty may be declared incorrectly.</rdfs:comment>
      <rdfs:domain rdf:resource="http://www.opengis.net/gml#ValueExtent"/>
      <rdfs:range rdf:resource="http://www.opengis.net/gml#CountExtent"/>
   </owl:ObjectProperty>
   <owl:ObjectProperty rdf:about="http://www.opengis.net/gml#hasBoolean">
      <rdfs:comment>Warning: This ObjectProperty reference was declared outside of its original schema. This ObjectProperty may be declared incorrectly.</rdfs:comment>
      <rdfs:domain rdf:resource="http://www.opengis.net/gml#BooleanPropertyType"/>
      <rdfs:range rdf:resource="http://www.opengis.net/gml#Boolean"/>
   </owl:ObjectProperty>
   <owl:ObjectProperty rdf:about="http://www.opengis.net/gml#hasCategory">
      <rdfs:comment>Warning: This ObjectProperty reference was declared outside of its original schema. This ObjectProperty may be declared incorrectly.</rdfs:comment>
      <rdfs:domain rdf:resource="http://www.opengis.net/gml#CategoryPropertyType"/>
      <rdfs:range rdf:resource="http://www.opengis.net/gml#Category"/>
   </owl:ObjectProperty>
   <owl:ObjectProperty rdf:about="http://www.opengis.net/gml#hasQuantity">
      <rdfs:comment>Warning: This ObjectProperty reference was declared outside of its original schema. This ObjectProperty may be declared incorrectly.</rdfs:comment>
      <rdfs:domain rdf:resource="http://www.opengis.net/gml#QuantityPropertyType"/>
      <rdfs:range rdf:resource="http://www.opengis.net/gml#Quantity"/>
   </owl:ObjectProperty>
   <owl:ObjectProperty rdf:about="http://www.opengis.net/gml#hasCount">
      <rdfs:comment>Warning: This ObjectProperty reference was declared outside of its original schema. This ObjectProperty may be declared incorrectly.</rdfs:comment>
      <rdfs:domain rdf:resource="http://www.opengis.net/gml#CountPropertyType"/>
      <rdfs:range rdf:resource="http://www.opengis.net/gml#Count"/>
   </owl:ObjectProperty>
   <owl:ObjectProperty rdf:about="http://www.opengis.net/gml#limits">
      <rdfs:domain rdf:resource="http://www.opengis.net/gml#GridType"/>
      <rdfs:range rdf:resource="http://www.opengis.net/gml#GridLimitsType"/>
   </owl:ObjectProperty>
   <owl:DatatypeProperty rdf:about="http://www.opengis.net/gml#axisName">
      <rdfs:domain rdf:resource="http://www.opengis.net/gml#GridType"/>
      <rdfs:range rdf:resource="http://www.w3.org/2001/XMLSchema#string"/>
   </owl:DatatypeProperty>
   <owl:ObjectProperty rdf:about="http://www.opengis.net/gml#GridEnvelope">
      <rdfs:domain rdf:resource="http://www.opengis.net/gml#GridLimitsType"/>
      <rdfs:range rdf:resource="http://www.opengis.net/gml#GridEnvelopeType"/>
   </owl:ObjectProperty>
   <owl:DatatypeProperty rdf:about="http://www.opengis.net/gml#low">
      <rdfs:domain rdf:resource="http://www.opengis.net/gml#GridEnvelopeType"/>
      <rdfs:range rdf:resource="http://www.opengis.net/gml#integerList"/>
   </owl:DatatypeProperty>
   <owl:DatatypeProperty rdf:about="http://www.opengis.net/gml#high">
      <rdfs:domain rdf:resource="http://www.opengis.net/gml#GridEnvelopeType"/>
      <rdfs:range rdf:resource="http://www.opengis.net/gml#integerList"/>
   </owl:DatatypeProperty>
   <owl:ObjectProperty rdf:about="http://www.opengis.net/gml#origin">
      <rdfs:domain rdf:resource="http://www.opengis.net/gml#RectifiedGridType"/>
      <rdfs:range rdf:resource="http://www.opengis.net/gml#PointPropertyType"/>
   </owl:ObjectProperty>
   <owl:ObjectProperty rdf:about="http://www.opengis.net/gml#offsetVector">
      <rdfs:domain rdf:resource="http://www.opengis.net/gml#RectifiedGridType"/>
      <rdfs:range rdf:resource="http://www.opengis.net/gml#VectorType"/>
   </owl:ObjectProperty>
   <owl:ObjectProperty rdf:about="http://www.opengis.net/gml#has_CoordinateReferenceSystem">
      <rdfs:comment>Warning: This ObjectProperty reference was declared outside of its original schema. This ObjectProperty may be declared incorrectly.</rdfs:comment>
      <rdfs:domain rdf:resource="http://www.opengis.net/gml#CoordinateReferenceSystemRefType"/>
      <rdfs:range rdf:resource="http://www.opengis.net/gml#_CoordinateReferenceSystem"/>
   </owl:ObjectProperty>
   <owl:ObjectProperty rdf:about="http://www.opengis.net/gml#hasincludesCRS">
      <rdfs:comment>Warning: This ObjectProperty reference was declared outside of its original schema. This ObjectProperty may be declared incorrectly.</rdfs:comment>
      <rdfs:domain rdf:resource="http://www.opengis.net/gml#CompoundCRSType"/>
      <rdfs:range rdf:resource="http://www.opengis.net/gml#includesCRS"/>
   </owl:ObjectProperty>
   <owl:ObjectProperty rdf:about="http://www.opengis.net/gml#hasCompoundCRS">
      <rdfs:comment>Warning: This ObjectProperty reference was declared outside of its original schema. This ObjectProperty may be declared incorrectly.</rdfs:comment>
      <rdfs:domain rdf:resource="http://www.opengis.net/gml#CompoundCRSRefType"/>
      <rdfs:range rdf:resource="http://www.opengis.net/gml#CompoundCRS"/>
   </owl:ObjectProperty>
   <owl:ObjectProperty rdf:about="http://www.opengis.net/gml#hasusesEllipsoidalCS">
      <rdfs:comment>Warning: This ObjectProperty reference was declared outside of its original schema. This ObjectProperty may be declared incorrectly.</rdfs:comment>
      <rdfs:domain rdf:resource="http://www.opengis.net/gml#GeographicCRSType"/>
      <rdfs:range rdf:resource="http://www.opengis.net/gml#usesEllipsoidalCS"/>
   </owl:ObjectProperty>
   <owl:ObjectProperty rdf:about="http://www.opengis.net/gml#hasusesGeodeticDatum">
      <rdfs:comment>Warning: This ObjectProperty reference was declared outside of its original schema. This ObjectProperty may be declared incorrectly.</rdfs:comment>
      <rdfs:domain rdf:resource="http://www.opengis.net/gml#GeographicCRSType"/>
      <rdfs:range rdf:resource="http://www.opengis.net/gml#usesGeodeticDatum"/>
   </owl:ObjectProperty>
   <owl:ObjectProperty rdf:about="http://www.opengis.net/gml#hasGeographicCRS">
      <rdfs:comment>Warning: This ObjectProperty reference was declared outside of its original schema. This ObjectProperty may be declared incorrectly.</rdfs:comment>
      <rdfs:domain rdf:resource="http://www.opengis.net/gml#GeographicCRSRefType"/>
      <rdfs:range rdf:resource="http://www.opengis.net/gml#GeographicCRS"/>
   </owl:ObjectProperty>
   <owl:ObjectProperty rdf:about="http://www.opengis.net/gml#hasusesVerticalCS">
      <rdfs:comment>Warning: This ObjectProperty reference was declared outside of its original schema. This ObjectProperty may be declared incorrectly.</rdfs:comment>
      <rdfs:domain rdf:resource="http://www.opengis.net/gml#VerticalCRSType"/>
      <rdfs:range rdf:resource="http://www.opengis.net/gml#usesVerticalCS"/>
   </owl:ObjectProperty>
   <owl:ObjectProperty rdf:about="http://www.opengis.net/gml#hasusesVerticalDatum">
      <rdfs:comment>Warning: This ObjectProperty reference was declared outside of its original schema. This ObjectProperty may be declared incorrectly.</rdfs:comment>
      <rdfs:domain rdf:resource="http://www.opengis.net/gml#VerticalCRSType"/>
      <rdfs:range rdf:resource="http://www.opengis.net/gml#usesVerticalDatum"/>
   </owl:ObjectProperty>
   <owl:ObjectProperty rdf:about="http://www.opengis.net/gml#hasVerticalCRS">
      <rdfs:comment>Warning: This ObjectProperty reference was declared outside of its original schema. This ObjectProperty may be declared incorrectly.</rdfs:comment>
      <rdfs:domain rdf:resource="http://www.opengis.net/gml#VerticalCRSRefType"/>
      <rdfs:range rdf:resource="http://www.opengis.net/gml#VerticalCRS"/>
   </owl:ObjectProperty>
   <owl:ObjectProperty rdf:about="http://www.opengis.net/gml#hasusesCartesianCS">
      <rdfs:comment>Warning: This ObjectProperty reference was declared outside of its original schema. This ObjectProperty may be declared incorrectly.</rdfs:comment>
      <rdfs:domain rdf:resource="http://www.opengis.net/gml#GeocentricCRSType"/>
      <rdfs:range rdf:resource="http://www.opengis.net/gml#usesCartesianCS"/>
   </owl:ObjectProperty>
   <owl:ObjectProperty rdf:about="http://www.opengis.net/gml#hasusesSphericalCS">
      <rdfs:comment>Warning: This ObjectProperty reference was declared outside of its original schema. This ObjectProperty may be declared incorrectly.</rdfs:comment>
      <rdfs:domain rdf:resource="http://www.opengis.net/gml#GeocentricCRSType"/>
      <rdfs:range rdf:resource="http://www.opengis.net/gml#usesSphericalCS"/>
   </owl:ObjectProperty>
   <owl:ObjectProperty rdf:about="http://www.opengis.net/gml#hasusesGeodeticDatum">
      <rdfs:comment>Warning: This ObjectProperty reference was declared outside of its original schema. This ObjectProperty may be declared incorrectly.</rdfs:comment>
      <rdfs:domain rdf:resource="http://www.opengis.net/gml#GeocentricCRSType"/>
      <rdfs:range rdf:resource="http://www.opengis.net/gml#usesGeodeticDatum"/>
   </owl:ObjectProperty>
   <owl:ObjectProperty rdf:about="http://www.opengis.net/gml#hasGeocentricCRS">
      <rdfs:comment>Warning: This ObjectProperty reference was declared outside of its original schema. This ObjectProperty may be declared incorrectly.</rdfs:comment>
      <rdfs:domain rdf:resource="http://www.opengis.net/gml#GeocentricCRSRefType"/>
      <rdfs:range rdf:resource="http://www.opengis.net/gml#GeocentricCRS"/>
   </owl:ObjectProperty>
   <owl:ObjectProperty rdf:about="http://www.opengis.net/gml#hasbaseCRS">
      <rdfs:comment>Warning: This ObjectProperty reference was declared outside of its original schema. This ObjectProperty may be declared incorrectly.</rdfs:comment>
      <rdfs:domain rdf:resource="http://www.opengis.net/gml#AbstractGeneralDerivedCRSType"/>
      <rdfs:range rdf:resource="http://www.opengis.net/gml#baseCRS"/>
   </owl:ObjectProperty>
   <owl:ObjectProperty rdf:about="http://www.opengis.net/gml#hasdefinedByConversion">
      <rdfs:comment>Warning: This ObjectProperty reference was declared outside of its original schema. This ObjectProperty may be declared incorrectly.</rdfs:comment>
      <rdfs:domain rdf:resource="http://www.opengis.net/gml#AbstractGeneralDerivedCRSType"/>
      <rdfs:range rdf:resource="http://www.opengis.net/gml#definedByConversion"/>
   </owl:ObjectProperty>
   <owl:ObjectProperty rdf:about="http://www.opengis.net/gml#hasusesCartesianCS">
      <rdfs:comment>Warning: This ObjectProperty reference was declared outside of its original schema. This ObjectProperty may be declared incorrectly.</rdfs:comment>
      <rdfs:domain rdf:resource="http://www.opengis.net/gml#ProjectedCRSType"/>
      <rdfs:range rdf:resource="http://www.opengis.net/gml#usesCartesianCS"/>
   </owl:ObjectProperty>
   <owl:ObjectProperty rdf:about="http://www.opengis.net/gml#hasProjectedCRS">
      <rdfs:comment>Warning: This ObjectProperty reference was declared outside of its original schema. This ObjectProperty may be declared incorrectly.</rdfs:comment>
      <rdfs:domain rdf:resource="http://www.opengis.net/gml#ProjectedCRSRefType"/>
      <rdfs:range rdf:resource="http://www.opengis.net/gml#ProjectedCRS"/>
   </owl:ObjectProperty>
   <owl:ObjectProperty rdf:about="http://www.opengis.net/gml#hasderivedCRSType">
      <rdfs:comment>Warning: This ObjectProperty reference was declared outside of its original schema. This ObjectProperty may be declared incorrectly.</rdfs:comment>
      <rdfs:domain rdf:resource="http://www.opengis.net/gml#DerivedCRSType"/>
      <rdfs:range rdf:resource="http://www.opengis.net/gml#derivedCRSType"/>
   </owl:ObjectProperty>
   <owl:ObjectProperty rdf:about="http://www.opengis.net/gml#hasusesCS">
      <rdfs:comment>Warning: This ObjectProperty reference was declared outside of its original schema. This ObjectProperty may be declared incorrectly.</rdfs:comment>
      <rdfs:domain rdf:resource="http://www.opengis.net/gml#DerivedCRSType"/>
      <rdfs:range rdf:resource="http://www.opengis.net/gml#usesCS"/>
   </owl:ObjectProperty>
   <owl:ObjectProperty rdf:about="http://www.opengis.net/gml#hasDerivedCRS">
      <rdfs:comment>Warning: This ObjectProperty reference was declared outside of its original schema. This ObjectProperty may be declared incorrectly.</rdfs:comment>
      <rdfs:domain rdf:resource="http://www.opengis.net/gml#DerivedCRSRefType"/>
      <rdfs:range rdf:resource="http://www.opengis.net/gml#DerivedCRS"/>
   </owl:ObjectProperty>
   <owl:ObjectProperty rdf:about="http://www.opengis.net/gml#hasusesCS">
      <rdfs:comment>Warning: This ObjectProperty reference was declared outside of its original schema. This ObjectProperty may be declared incorrectly.</rdfs:comment>
      <rdfs:domain rdf:resource="http://www.opengis.net/gml#EngineeringCRSType"/>
      <rdfs:range rdf:resource="http://www.opengis.net/gml#usesCS"/>
   </owl:ObjectProperty>
   <owl:ObjectProperty rdf:about="http://www.opengis.net/gml#hasusesEngineeringDatum">
      <rdfs:comment>Warning: This ObjectProperty reference was declared outside of its original schema. This ObjectProperty may be declared incorrectly.</rdfs:comment>
      <rdfs:domain rdf:resource="http://www.opengis.net/gml#EngineeringCRSType"/>
      <rdfs:range rdf:resource="http://www.opengis.net/gml#usesEngineeringDatum"/>
   </owl:ObjectProperty>
   <owl:ObjectProperty rdf:about="http://www.opengis.net/gml#hasEngineeringCRS">
      <rdfs:comment>Warning: This ObjectProperty reference was declared outside of its original schema. This ObjectProperty may be declared incorrectly.</rdfs:comment>
      <rdfs:domain rdf:resource="http://www.opengis.net/gml#EngineeringCRSRefType"/>
      <rdfs:range rdf:resource="http://www.opengis.net/gml#EngineeringCRS"/>
   </owl:ObjectProperty>
   <owl:ObjectProperty rdf:about="http://www.opengis.net/gml#hasusesCartesianCS">
      <rdfs:comment>Warning: This ObjectProperty reference was declared outside of its original schema. This ObjectProperty may be declared incorrectly.</rdfs:comment>
      <rdfs:domain rdf:resource="http://www.opengis.net/gml#ImageCRSType"/>
      <rdfs:range rdf:resource="http://www.opengis.net/gml#usesCartesianCS"/>
   </owl:ObjectProperty>
   <owl:ObjectProperty rdf:about="http://www.opengis.net/gml#hasusesObliqueCartesianCS">
      <rdfs:comment>Warning: This ObjectProperty reference was declared outside of its original schema. This ObjectProperty may be declared incorrectly.</rdfs:comment>
      <rdfs:domain rdf:resource="http://www.opengis.net/gml#ImageCRSType"/>
      <rdfs:range rdf:resource="http://www.opengis.net/gml#usesObliqueCartesianCS"/>
   </owl:ObjectProperty>
   <owl:ObjectProperty rdf:about="http://www.opengis.net/gml#hasusesImageDatum">
      <rdfs:comment>Warning: This ObjectProperty reference was declared outside of its original schema. This ObjectProperty may be declared incorrectly.</rdfs:comment>
      <rdfs:domain rdf:resource="http://www.opengis.net/gml#ImageCRSType"/>
      <rdfs:range rdf:resource="http://www.opengis.net/gml#usesImageDatum"/>
   </owl:ObjectProperty>
   <owl:ObjectProperty rdf:about="http://www.opengis.net/gml#hasImageCRS">
      <rdfs:comment>Warning: This ObjectProperty reference was declared outside of its original schema. This ObjectProperty may be declared incorrectly.</rdfs:comment>
      <rdfs:domain rdf:resource="http://www.opengis.net/gml#ImageCRSRefType"/>
      <rdfs:range rdf:resource="http://www.opengis.net/gml#ImageCRS"/>
   </owl:ObjectProperty>
   <owl:ObjectProperty rdf:about="http://www.opengis.net/gml#hasusesTemporalCS">
      <rdfs:comment>Warning: This ObjectProperty reference was declared outside of its original schema. This ObjectProperty may be declared incorrectly.</rdfs:comment>
      <rdfs:domain rdf:resource="http://www.opengis.net/gml#TemporalCRSType"/>
      <rdfs:range rdf:resource="http://www.opengis.net/gml#usesTemporalCS"/>
   </owl:ObjectProperty>
   <owl:ObjectProperty rdf:about="http://www.opengis.net/gml#hasusesTemporalDatum">
      <rdfs:comment>Warning: This ObjectProperty reference was declared outside of its original schema. This ObjectProperty may be declared incorrectly.</rdfs:comment>
      <rdfs:domain rdf:resource="http://www.opengis.net/gml#TemporalCRSType"/>
      <rdfs:range rdf:resource="http://www.opengis.net/gml#usesTemporalDatum"/>
   </owl:ObjectProperty>
   <owl:ObjectProperty rdf:about="http://www.opengis.net/gml#hasTemporalCRS">
      <rdfs:comment>Warning: This ObjectProperty reference was declared outside of its original schema. This ObjectProperty may be declared incorrectly.</rdfs:comment>
      <rdfs:domain rdf:resource="http://www.opengis.net/gml#TemporalCRSRefType"/>
      <rdfs:range rdf:resource="http://www.opengis.net/gml#TemporalCRS"/>
   </owl:ObjectProperty>
   <owl:ObjectProperty rdf:about="http://www.opengis.net/gml#hasmetaDataProperty">
      <rdfs:comment>Warning: This ObjectProperty reference was declared outside of its original schema. This ObjectProperty may be declared incorrectly.</rdfs:comment>
      <rdfs:domain rdf:resource="http://www.opengis.net/gml#CoordinateSystemAxisBaseType"/>
      <rdfs:range rdf:resource="http://www.opengis.net/gml#metaDataProperty"/>
   </owl:ObjectProperty>
   <owl:ObjectProperty rdf:about="http://www.opengis.net/gml#hasname">
      <rdfs:comment>Warning: This ObjectProperty reference was declared outside of its original schema. This ObjectProperty may be declared incorrectly.</rdfs:comment>
      <rdfs:domain rdf:resource="http://www.opengis.net/gml#CoordinateSystemAxisBaseType"/>
      <rdfs:range rdf:resource="http://www.opengis.net/gml#name"/>
   </owl:ObjectProperty>
   <owl:ObjectProperty rdf:about="http://www.opengis.net/gml#hasaxisID">
      <rdfs:comment>Warning: This ObjectProperty reference was declared outside of its original schema. This ObjectProperty may be declared incorrectly.</rdfs:comment>
      <rdfs:domain rdf:resource="http://www.opengis.net/gml#CoordinateSystemAxisType"/>
      <rdfs:range rdf:resource="http://www.opengis.net/gml#axisID"/>
   </owl:ObjectProperty>
   <owl:ObjectProperty rdf:about="http://www.opengis.net/gml#hasremarks">
      <rdfs:comment>Warning: This ObjectProperty reference was declared outside of its original schema. This ObjectProperty may be declared incorrectly.</rdfs:comment>
      <rdfs:domain rdf:resource="http://www.opengis.net/gml#CoordinateSystemAxisType"/>
      <rdfs:range rdf:resource="http://www.opengis.net/gml#remarks"/>
   </owl:ObjectProperty>
   <owl:ObjectProperty rdf:about="http://www.opengis.net/gml#hasaxisAbbrev">
      <rdfs:comment>Warning: This ObjectProperty reference was declared outside of its original schema. This ObjectProperty may be declared incorrectly.</rdfs:comment>
      <rdfs:domain rdf:resource="http://www.opengis.net/gml#CoordinateSystemAxisType"/>
      <rdfs:range rdf:resource="http://www.opengis.net/gml#axisAbbrev"/>
   </owl:ObjectProperty>
   <owl:ObjectProperty rdf:about="http://www.opengis.net/gml#hasaxisDirection">
      <rdfs:comment>Warning: This ObjectProperty reference was declared outside of its original schema. This ObjectProperty may be declared incorrectly.</rdfs:comment>
      <rdfs:domain rdf:resource="http://www.opengis.net/gml#CoordinateSystemAxisType"/>
      <rdfs:range rdf:resource="http://www.opengis.net/gml#axisDirection"/>
   </owl:ObjectProperty>
   <owl:ObjectProperty rdf:about="http://www.opengis.net/gml#hasCoordinateSystemAxis">
      <rdfs:comment>Warning: This ObjectProperty reference was declared outside of its original schema. This ObjectProperty may be declared incorrectly.</rdfs:comment>
      <rdfs:domain rdf:resource="http://www.opengis.net/gml#CoordinateSystemAxisRefType"/>
      <rdfs:range rdf:resource="http://www.opengis.net/gml#CoordinateSystemAxis"/>
   </owl:ObjectProperty>
   <owl:ObjectProperty rdf:about="http://www.opengis.net/gml#hasmetaDataProperty">
      <rdfs:comment>Warning: This ObjectProperty reference was declared outside of its original schema. This ObjectProperty may be declared incorrectly.</rdfs:comment>
      <rdfs:domain rdf:resource="http://www.opengis.net/gml#AbstractCoordinateSystemBaseType"/>
      <rdfs:range rdf:resource="http://www.opengis.net/gml#metaDataProperty"/>
   </owl:ObjectProperty>
   <owl:ObjectProperty rdf:about="http://www.opengis.net/gml#hascsName">
      <rdfs:comment>Warning: This ObjectProperty reference was declared outside of its original schema. This ObjectProperty may be declared incorrectly.</rdfs:comment>
      <rdfs:domain rdf:resource="http://www.opengis.net/gml#AbstractCoordinateSystemBaseType"/>
      <rdfs:range rdf:resource="http://www.opengis.net/gml#csName"/>
   </owl:ObjectProperty>
   <owl:ObjectProperty rdf:about="http://www.opengis.net/gml#hascsID">
      <rdfs:comment>Warning: This ObjectProperty reference was declared outside of its original schema. This ObjectProperty may be declared incorrectly.</rdfs:comment>
      <rdfs:domain rdf:resource="http://www.opengis.net/gml#AbstractCoordinateSystemType"/>
      <rdfs:range rdf:resource="http://www.opengis.net/gml#csID"/>
   </owl:ObjectProperty>
   <owl:ObjectProperty rdf:about="http://www.opengis.net/gml#hasremarks">
      <rdfs:comment>Warning: This ObjectProperty reference was declared outside of its original schema. This ObjectProperty may be declared incorrectly.</rdfs:comment>
      <rdfs:domain rdf:resource="http://www.opengis.net/gml#AbstractCoordinateSystemType"/>
      <rdfs:range rdf:resource="http://www.opengis.net/gml#remarks"/>
   </owl:ObjectProperty>
   <owl:ObjectProperty rdf:about="http://www.opengis.net/gml#hasusesAxis">
      <rdfs:comment>Warning: This ObjectProperty reference was declared outside of its original schema. This ObjectProperty may be declared incorrectly.</rdfs:comment>
      <rdfs:domain rdf:resource="http://www.opengis.net/gml#AbstractCoordinateSystemType"/>
      <rdfs:range rdf:resource="http://www.opengis.net/gml#usesAxis"/>
   </owl:ObjectProperty>
   <owl:ObjectProperty rdf:about="http://www.opengis.net/gml#has_CoordinateSystem">
      <rdfs:comment>Warning: This ObjectProperty reference was declared outside of its original schema. This ObjectProperty may be declared incorrectly.</rdfs:comment>
      <rdfs:domain rdf:resource="http://www.opengis.net/gml#CoordinateSystemRefType"/>
      <rdfs:range rdf:resource="http://www.opengis.net/gml#_CoordinateSystem"/>
   </owl:ObjectProperty>
   <owl:ObjectProperty rdf:about="http://www.opengis.net/gml#hasEllipsoidalCS">
      <rdfs:comment>Warning: This ObjectProperty reference was declared outside of its original schema. This ObjectProperty may be declared incorrectly.</rdfs:comment>
      <rdfs:domain rdf:resource="http://www.opengis.net/gml#EllipsoidalCSRefType"/>
      <rdfs:range rdf:resource="http://www.opengis.net/gml#EllipsoidalCS"/>
   </owl:ObjectProperty>
   <owl:ObjectProperty rdf:about="http://www.opengis.net/gml#hasCartesianCS">
      <rdfs:comment>Warning: This ObjectProperty reference was declared outside of its original schema. This ObjectProperty may be declared incorrectly.</rdfs:comment>
      <rdfs:domain rdf:resource="http://www.opengis.net/gml#CartesianCSRefType"/>
      <rdfs:range rdf:resource="http://www.opengis.net/gml#CartesianCS"/>
   </owl:ObjectProperty>
   <owl:ObjectProperty rdf:about="http://www.opengis.net/gml#hasVerticalCS">
      <rdfs:comment>Warning: This ObjectProperty reference was declared outside of its original schema. This ObjectProperty may be declared incorrectly.</rdfs:comment>
      <rdfs:domain rdf:resource="http://www.opengis.net/gml#VerticalCSRefType"/>
      <rdfs:range rdf:resource="http://www.opengis.net/gml#VerticalCS"/>
   </owl:ObjectProperty>
   <owl:ObjectProperty rdf:about="http://www.opengis.net/gml#hasTemporalCS">
      <rdfs:comment>Warning: This ObjectProperty reference was declared outside of its original schema. This ObjectProperty may be declared incorrectly.</rdfs:comment>
      <rdfs:domain rdf:resource="http://www.opengis.net/gml#TemporalCSRefType"/>
      <rdfs:range rdf:resource="http://www.opengis.net/gml#TemporalCS"/>
   </owl:ObjectProperty>
   <owl:ObjectProperty rdf:about="http://www.opengis.net/gml#hasLinearCS">
      <rdfs:comment>Warning: This ObjectProperty reference was declared outside of its original schema. This ObjectProperty may be declared incorrectly.</rdfs:comment>
      <rdfs:domain rdf:resource="http://www.opengis.net/gml#LinearCSRefType"/>
      <rdfs:range rdf:resource="http://www.opengis.net/gml#LinearCS"/>
   </owl:ObjectProperty>
   <owl:ObjectProperty rdf:about="http://www.opengis.net/gml#hasUserDefinedCS">
      <rdfs:comment>Warning: This ObjectProperty reference was declared outside of its original schema. This ObjectProperty may be declared incorrectly.</rdfs:comment>
      <rdfs:domain rdf:resource="http://www.opengis.net/gml#UserDefinedCSRefType"/>
      <rdfs:range rdf:resource="http://www.opengis.net/gml#UserDefinedCS"/>
   </owl:ObjectProperty>
   <owl:ObjectProperty rdf:about="http://www.opengis.net/gml#hasSphericalCS">
      <rdfs:comment>Warning: This ObjectProperty reference was declared outside of its original schema. This ObjectProperty may be declared incorrectly.</rdfs:comment>
      <rdfs:domain rdf:resource="http://www.opengis.net/gml#SphericalCSRefType"/>
      <rdfs:range rdf:resource="http://www.opengis.net/gml#SphericalCS"/>
   </owl:ObjectProperty>
   <owl:ObjectProperty rdf:about="http://www.opengis.net/gml#hasPolarCS">
      <rdfs:comment>Warning: This ObjectProperty reference was declared outside of its original schema. This ObjectProperty may be declared incorrectly.</rdfs:comment>
      <rdfs:domain rdf:resource="http://www.opengis.net/gml#PolarCSRefType"/>
      <rdfs:range rdf:resource="http://www.opengis.net/gml#PolarCS"/>
   </owl:ObjectProperty>
   <owl:ObjectProperty rdf:about="http://www.opengis.net/gml#hasCylindricalCS">
      <rdfs:comment>Warning: This ObjectProperty reference was declared outside of its original schema. This ObjectProperty may be declared incorrectly.</rdfs:comment>
      <rdfs:domain rdf:resource="http://www.opengis.net/gml#CylindricalCSRefType"/>
      <rdfs:range rdf:resource="http://www.opengis.net/gml#CylindricalCS"/>
   </owl:ObjectProperty>
   <owl:ObjectProperty rdf:about="http://www.opengis.net/gml#hasObliqueCartesianCS">
      <rdfs:comment>Warning: This ObjectProperty reference was declared outside of its original schema. This ObjectProperty may be declared incorrectly.</rdfs:comment>
      <rdfs:domain rdf:resource="http://www.opengis.net/gml#ObliqueCartesianCSRefType"/>
      <rdfs:range rdf:resource="http://www.opengis.net/gml#ObliqueCartesianCS"/>
   </owl:ObjectProperty>
   <owl:ObjectProperty rdf:about="http://www.opengis.net/gml#hasmetaDataProperty">
      <rdfs:comment>Warning: This ObjectProperty reference was declared outside of its original schema. This ObjectProperty may be declared incorrectly.</rdfs:comment>
      <rdfs:domain rdf:resource="http://www.opengis.net/gml#AbstractReferenceSystemBaseType"/>
      <rdfs:range rdf:resource="http://www.opengis.net/gml#metaDataProperty"/>
   </owl:ObjectProperty>
   <owl:ObjectProperty rdf:about="http://www.opengis.net/gml#hassrsName">
      <rdfs:comment>Warning: This ObjectProperty reference was declared outside of its original schema. This ObjectProperty may be declared incorrectly.</rdfs:comment>
      <rdfs:domain rdf:resource="http://www.opengis.net/gml#AbstractReferenceSystemBaseType"/>
      <rdfs:range rdf:resource="http://www.opengis.net/gml#srsName"/>
   </owl:ObjectProperty>
   <owl:ObjectProperty rdf:about="http://www.opengis.net/gml#hassrsID">
      <rdfs:comment>Warning: This ObjectProperty reference was declared outside of its original schema. This ObjectProperty may be declared incorrectly.</rdfs:comment>
      <rdfs:domain rdf:resource="http://www.opengis.net/gml#AbstractReferenceSystemType"/>
      <rdfs:range rdf:resource="http://www.opengis.net/gml#srsID"/>
   </owl:ObjectProperty>
   <owl:ObjectProperty rdf:about="http://www.opengis.net/gml#hasremarks">
      <rdfs:comment>Warning: This ObjectProperty reference was declared outside of its original schema. This ObjectProperty may be declared incorrectly.</rdfs:comment>
      <rdfs:domain rdf:resource="http://www.opengis.net/gml#AbstractReferenceSystemType"/>
      <rdfs:range rdf:resource="http://www.opengis.net/gml#remarks"/>
   </owl:ObjectProperty>
   <owl:ObjectProperty rdf:about="http://www.opengis.net/gml#hasvalidArea">
      <rdfs:comment>Warning: This ObjectProperty reference was declared outside of its original schema. This ObjectProperty may be declared incorrectly.</rdfs:comment>
      <rdfs:domain rdf:resource="http://www.opengis.net/gml#AbstractReferenceSystemType"/>
      <rdfs:range rdf:resource="http://www.opengis.net/gml#validArea"/>
   </owl:ObjectProperty>
   <owl:ObjectProperty rdf:about="http://www.opengis.net/gml#hasscope">
      <rdfs:comment>Warning: This ObjectProperty reference was declared outside of its original schema. This ObjectProperty may be declared incorrectly.</rdfs:comment>
      <rdfs:domain rdf:resource="http://www.opengis.net/gml#AbstractReferenceSystemType"/>
      <rdfs:range rdf:resource="http://www.opengis.net/gml#scope"/>
   </owl:ObjectProperty>
   <owl:ObjectProperty rdf:about="http://www.opengis.net/gml#has_ReferenceSystem">
      <rdfs:comment>Warning: This ObjectProperty reference was declared outside of its original schema. This ObjectProperty may be declared incorrectly.</rdfs:comment>
      <rdfs:domain rdf:resource="http://www.opengis.net/gml#ReferenceSystemRefType"/>
      <rdfs:range rdf:resource="http://www.opengis.net/gml#_ReferenceSystem"/>
   </owl:ObjectProperty>
   <owl:ObjectProperty rdf:about="http://www.opengis.net/gml#has_CRS">
      <rdfs:comment>Warning: This ObjectProperty reference was declared outside of its original schema. This ObjectProperty may be declared incorrectly.</rdfs:comment>
      <rdfs:domain rdf:resource="http://www.opengis.net/gml#CRSRefType"/>
      <rdfs:range rdf:resource="http://www.opengis.net/gml#_CRS"/>
   </owl:ObjectProperty>
   <owl:ObjectProperty rdf:about="http://www.opengis.net/gml#hasname">
      <rdfs:comment>Warning: This ObjectProperty reference was declared outside of its original schema. This ObjectProperty may be declared incorrectly.</rdfs:comment>
      <rdfs:domain rdf:resource="http://www.opengis.net/gml#IdentifierType"/>
      <rdfs:range rdf:resource="http://www.opengis.net/gml#name"/>
   </owl:ObjectProperty>
   <owl:ObjectProperty rdf:about="http://www.opengis.net/gml#hasversion">
      <rdfs:comment>Warning: This ObjectProperty reference was declared outside of its original schema. This ObjectProperty may be declared incorrectly.</rdfs:comment>
      <rdfs:domain rdf:resource="http://www.opengis.net/gml#IdentifierType"/>
      <rdfs:range rdf:resource="http://www.opengis.net/gml#version"/>
   </owl:ObjectProperty>
   <owl:ObjectProperty rdf:about="http://www.opengis.net/gml#hasremarks">
      <rdfs:comment>Warning: This ObjectProperty reference was declared outside of its original schema. This ObjectProperty may be declared incorrectly.</rdfs:comment>
      <rdfs:domain rdf:resource="http://www.opengis.net/gml#IdentifierType"/>
      <rdfs:range rdf:resource="http://www.opengis.net/gml#remarks"/>
   </owl:ObjectProperty>
   <owl:ObjectProperty rdf:about="http://www.opengis.net/gml#hasdescription">
      <rdfs:comment>Warning: This ObjectProperty reference was declared outside of its original schema. This ObjectProperty may be declared incorrectly.</rdfs:comment>
      <rdfs:domain rdf:resource="http://www.opengis.net/gml#ExtentType"/>
      <rdfs:range rdf:resource="http://www.opengis.net/gml#description"/>
   </owl:ObjectProperty>
   <owl:ObjectProperty rdf:about="http://www.opengis.net/gml#hasboundingBox">
      <rdfs:comment>Warning: This ObjectProperty reference was declared outside of its original schema. This ObjectProperty may be declared incorrectly.</rdfs:comment>
      <rdfs:domain rdf:resource="http://www.opengis.net/gml#ExtentType"/>
      <rdfs:range rdf:resource="http://www.opengis.net/gml#boundingBox"/>
   </owl:ObjectProperty>
   <owl:ObjectProperty rdf:about="http://www.opengis.net/gml#hasboundingPolygon">
      <rdfs:comment>Warning: This ObjectProperty reference was declared outside of its original schema. This ObjectProperty may be declared incorrectly.</rdfs:comment>
      <rdfs:domain rdf:resource="http://www.opengis.net/gml#ExtentType"/>
      <rdfs:range rdf:resource="http://www.opengis.net/gml#boundingPolygon"/>
   </owl:ObjectProperty>
   <owl:ObjectProperty rdf:about="http://www.opengis.net/gml#hasverticalExtent">
      <rdfs:comment>Warning: This ObjectProperty reference was declared outside of its original schema. This ObjectProperty may be declared incorrectly.</rdfs:comment>
      <rdfs:domain rdf:resource="http://www.opengis.net/gml#ExtentType"/>
      <rdfs:range rdf:resource="http://www.opengis.net/gml#verticalExtent"/>
   </owl:ObjectProperty>
   <owl:ObjectProperty rdf:about="http://www.opengis.net/gml#hastemporalExtent">
      <rdfs:comment>Warning: This ObjectProperty reference was declared outside of its original schema. This ObjectProperty may be declared incorrectly.</rdfs:comment>
      <rdfs:domain rdf:resource="http://www.opengis.net/gml#ExtentType"/>
      <rdfs:range rdf:resource="http://www.opengis.net/gml#temporalExtent"/>
   </owl:ObjectProperty>
   <owl:ObjectProperty rdf:about="http://www.opengis.net/gml#hasmetaDataProperty">
      <rdfs:comment>Warning: This ObjectProperty reference was declared outside of its original schema. This ObjectProperty may be declared incorrectly.</rdfs:comment>
      <rdfs:domain rdf:resource="http://www.opengis.net/gml#AbstractDatumBaseType"/>
      <rdfs:range rdf:resource="http://www.opengis.net/gml#metaDataProperty"/>
   </owl:ObjectProperty>
   <owl:ObjectProperty rdf:about="http://www.opengis.net/gml#hasdatumName">
      <rdfs:comment>Warning: This ObjectProperty reference was declared outside of its original schema. This ObjectProperty may be declared incorrectly.</rdfs:comment>
      <rdfs:domain rdf:resource="http://www.opengis.net/gml#AbstractDatumBaseType"/>
      <rdfs:range rdf:resource="http://www.opengis.net/gml#datumName"/>
   </owl:ObjectProperty>
   <owl:ObjectProperty rdf:about="http://www.opengis.net/gml#hasdatumID">
      <rdfs:comment>Warning: This ObjectProperty reference was declared outside of its original schema. This ObjectProperty may be declared incorrectly.</rdfs:comment>
      <rdfs:domain rdf:resource="http://www.opengis.net/gml#AbstractDatumType"/>
      <rdfs:range rdf:resource="http://www.opengis.net/gml#datumID"/>
   </owl:ObjectProperty>
   <owl:ObjectProperty rdf:about="http://www.opengis.net/gml#hasremarks">
      <rdfs:comment>Warning: This ObjectProperty reference was declared outside of its original schema. This ObjectProperty may be declared incorrectly.</rdfs:comment>
      <rdfs:domain rdf:resource="http://www.opengis.net/gml#AbstractDatumType"/>
      <rdfs:range rdf:resource="http://www.opengis.net/gml#remarks"/>
   </owl:ObjectProperty>
   <owl:ObjectProperty rdf:about="http://www.opengis.net/gml#hasanchorPoint">
      <rdfs:comment>Warning: This ObjectProperty reference was declared outside of its original schema. This ObjectProperty may be declared incorrectly.</rdfs:comment>
      <rdfs:domain rdf:resource="http://www.opengis.net/gml#AbstractDatumType"/>
      <rdfs:range rdf:resource="http://www.opengis.net/gml#anchorPoint"/>
   </owl:ObjectProperty>
   <owl:ObjectProperty rdf:about="http://www.opengis.net/gml#hasrealizationEpoch">
      <rdfs:comment>Warning: This ObjectProperty reference was declared outside of its original schema. This ObjectProperty may be declared incorrectly.</rdfs:comment>
      <rdfs:domain rdf:resource="http://www.opengis.net/gml#AbstractDatumType"/>
      <rdfs:range rdf:resource="http://www.opengis.net/gml#realizationEpoch"/>
   </owl:ObjectProperty>
   <owl:ObjectProperty rdf:about="http://www.opengis.net/gml#hasvalidArea">
      <rdfs:comment>Warning: This ObjectProperty reference was declared outside of its original schema. This ObjectProperty may be declared incorrectly.</rdfs:comment>
      <rdfs:domain rdf:resource="http://www.opengis.net/gml#AbstractDatumType"/>
      <rdfs:range rdf:resource="http://www.opengis.net/gml#validArea"/>
   </owl:ObjectProperty>
   <owl:ObjectProperty rdf:about="http://www.opengis.net/gml#hasscope">
      <rdfs:comment>Warning: This ObjectProperty reference was declared outside of its original schema. This ObjectProperty may be declared incorrectly.</rdfs:comment>
      <rdfs:domain rdf:resource="http://www.opengis.net/gml#AbstractDatumType"/>
      <rdfs:range rdf:resource="http://www.opengis.net/gml#scope"/>
   </owl:ObjectProperty>
   <owl:ObjectProperty rdf:about="http://www.opengis.net/gml#has_Datum">
      <rdfs:comment>Warning: This ObjectProperty reference was declared outside of its original schema. This ObjectProperty may be declared incorrectly.</rdfs:comment>
      <rdfs:domain rdf:resource="http://www.opengis.net/gml#DatumRefType"/>
      <rdfs:range rdf:resource="http://www.opengis.net/gml#_Datum"/>
   </owl:ObjectProperty>
   <owl:ObjectProperty rdf:about="http://www.opengis.net/gml#hasEngineeringDatum">
      <rdfs:comment>Warning: This ObjectProperty reference was declared outside of its original schema. This ObjectProperty may be declared incorrectly.</rdfs:comment>
      <rdfs:domain rdf:resource="http://www.opengis.net/gml#EngineeringDatumRefType"/>
      <rdfs:range rdf:resource="http://www.opengis.net/gml#EngineeringDatum"/>
   </owl:ObjectProperty>
   <owl:ObjectProperty rdf:about="http://www.opengis.net/gml#haspixelInCell">
      <rdfs:comment>Warning: This ObjectProperty reference was declared outside of its original schema. This ObjectProperty may be declared incorrectly.</rdfs:comment>
      <rdfs:domain rdf:resource="http://www.opengis.net/gml#ImageDatumType"/>
      <rdfs:range rdf:resource="http://www.opengis.net/gml#pixelInCell"/>
   </owl:ObjectProperty>
   <owl:ObjectProperty rdf:about="http://www.opengis.net/gml#hasImageDatum">
      <rdfs:comment>Warning: This ObjectProperty reference was declared outside of its original schema. This ObjectProperty may be declared incorrectly.</rdfs:comment>
      <rdfs:domain rdf:resource="http://www.opengis.net/gml#ImageDatumRefType"/>
      <rdfs:range rdf:resource="http://www.opengis.net/gml#ImageDatum"/>
   </owl:ObjectProperty>
   <owl:ObjectProperty rdf:about="http://www.opengis.net/gml#hasverticalDatumType">
      <rdfs:comment>Warning: This ObjectProperty reference was declared outside of its original schema. This ObjectProperty may be declared incorrectly.</rdfs:comment>
      <rdfs:domain rdf:resource="http://www.opengis.net/gml#VerticalDatumType"/>
      <rdfs:range rdf:resource="http://www.opengis.net/gml#verticalDatumType"/>
   </owl:ObjectProperty>
   <owl:ObjectProperty rdf:about="http://www.opengis.net/gml#hasVerticalDatum">
      <rdfs:comment>Warning: This ObjectProperty reference was declared outside of its original schema. This ObjectProperty may be declared incorrectly.</rdfs:comment>
      <rdfs:domain rdf:resource="http://www.opengis.net/gml#VerticalDatumRefType"/>
      <rdfs:range rdf:resource="http://www.opengis.net/gml#VerticalDatum"/>
   </owl:ObjectProperty>
   <owl:ObjectProperty rdf:about="http://www.opengis.net/gml#hasmetaDataProperty">
      <rdfs:comment>Warning: This ObjectProperty reference was declared outside of its original schema. This ObjectProperty may be declared incorrectly.</rdfs:comment>
      <rdfs:domain rdf:resource="http://www.opengis.net/gml#TemporalDatumBaseType"/>
      <rdfs:range rdf:resource="http://www.opengis.net/gml#metaDataProperty"/>
   </owl:ObjectProperty>
   <owl:ObjectProperty rdf:about="http://www.opengis.net/gml#hasdatumName">
      <rdfs:comment>Warning: This ObjectProperty reference was declared outside of its original schema. This ObjectProperty may be declared incorrectly.</rdfs:comment>
      <rdfs:domain rdf:resource="http://www.opengis.net/gml#TemporalDatumBaseType"/>
      <rdfs:range rdf:resource="http://www.opengis.net/gml#datumName"/>
   </owl:ObjectProperty>
   <owl:ObjectProperty rdf:about="http://www.opengis.net/gml#hasdatumID">
      <rdfs:comment>Warning: This ObjectProperty reference was declared outside of its original schema. This ObjectProperty may be declared incorrectly.</rdfs:comment>
      <rdfs:domain rdf:resource="http://www.opengis.net/gml#TemporalDatumBaseType"/>
      <rdfs:range rdf:resource="http://www.opengis.net/gml#datumID"/>
   </owl:ObjectProperty>
   <owl:ObjectProperty rdf:about="http://www.opengis.net/gml#hasvalidArea">
      <rdfs:comment>Warning: This ObjectProperty reference was declared outside of its original schema. This ObjectProperty may be declared incorrectly.</rdfs:comment>
      <rdfs:domain rdf:resource="http://www.opengis.net/gml#TemporalDatumBaseType"/>
      <rdfs:range rdf:resource="http://www.opengis.net/gml#validArea"/>
   </owl:ObjectProperty>
   <owl:ObjectProperty rdf:about="http://www.opengis.net/gml#hasscope">
      <rdfs:comment>Warning: This ObjectProperty reference was declared outside of its original schema. This ObjectProperty may be declared incorrectly.</rdfs:comment>
      <rdfs:domain rdf:resource="http://www.opengis.net/gml#TemporalDatumBaseType"/>
      <rdfs:range rdf:resource="http://www.opengis.net/gml#scope"/>
   </owl:ObjectProperty>
   <owl:ObjectProperty rdf:about="http://www.opengis.net/gml#hasorigin">
      <rdfs:comment>Warning: This ObjectProperty reference was declared outside of its original schema. This ObjectProperty may be declared incorrectly.</rdfs:comment>
      <rdfs:domain rdf:resource="http://www.opengis.net/gml#TemporalDatumType"/>
      <rdfs:range rdf:resource="http://www.opengis.net/gml#origin"/>
   </owl:ObjectProperty>
   <owl:ObjectProperty rdf:about="http://www.opengis.net/gml#hasTemporalDatum">
      <rdfs:comment>Warning: This ObjectProperty reference was declared outside of its original schema. This ObjectProperty may be declared incorrectly.</rdfs:comment>
      <rdfs:domain rdf:resource="http://www.opengis.net/gml#TemporalDatumRefType"/>
      <rdfs:range rdf:resource="http://www.opengis.net/gml#TemporalDatum"/>
   </owl:ObjectProperty>
   <owl:ObjectProperty rdf:about="http://www.opengis.net/gml#hasusesPrimeMeridian">
      <rdfs:comment>Warning: This ObjectProperty reference was declared outside of its original schema. This ObjectProperty may be declared incorrectly.</rdfs:comment>
      <rdfs:domain rdf:resource="http://www.opengis.net/gml#GeodeticDatumType"/>
      <rdfs:range rdf:resource="http://www.opengis.net/gml#usesPrimeMeridian"/>
   </owl:ObjectProperty>
   <owl:ObjectProperty rdf:about="http://www.opengis.net/gml#hasusesEllipsoid">
      <rdfs:comment>Warning: This ObjectProperty reference was declared outside of its original schema. This ObjectProperty may be declared incorrectly.</rdfs:comment>
      <rdfs:domain rdf:resource="http://www.opengis.net/gml#GeodeticDatumType"/>
      <rdfs:range rdf:resource="http://www.opengis.net/gml#usesEllipsoid"/>
   </owl:ObjectProperty>
   <owl:ObjectProperty rdf:about="http://www.opengis.net/gml#hasGeodeticDatum">
      <rdfs:comment>Warning: This ObjectProperty reference was declared outside of its original schema. This ObjectProperty may be declared incorrectly.</rdfs:comment>
      <rdfs:domain rdf:resource="http://www.opengis.net/gml#GeodeticDatumRefType"/>
      <rdfs:range rdf:resource="http://www.opengis.net/gml#GeodeticDatum"/>
   </owl:ObjectProperty>
   <owl:ObjectProperty rdf:about="http://www.opengis.net/gml#hasmetaDataProperty">
      <rdfs:comment>Warning: This ObjectProperty reference was declared outside of its original schema. This ObjectProperty may be declared incorrectly.</rdfs:comment>
      <rdfs:domain rdf:resource="http://www.opengis.net/gml#PrimeMeridianBaseType"/>
      <rdfs:range rdf:resource="http://www.opengis.net/gml#metaDataProperty"/>
   </owl:ObjectProperty>
   <owl:ObjectProperty rdf:about="http://www.opengis.net/gml#hasmeridianName">
      <rdfs:comment>Warning: This ObjectProperty reference was declared outside of its original schema. This ObjectProperty may be declared incorrectly.</rdfs:comment>
      <rdfs:domain rdf:resource="http://www.opengis.net/gml#PrimeMeridianBaseType"/>
      <rdfs:range rdf:resource="http://www.opengis.net/gml#meridianName"/>
   </owl:ObjectProperty>
   <owl:ObjectProperty rdf:about="http://www.opengis.net/gml#hasmeridianID">
      <rdfs:comment>Warning: This ObjectProperty reference was declared outside of its original schema. This ObjectProperty may be declared incorrectly.</rdfs:comment>
      <rdfs:domain rdf:resource="http://www.opengis.net/gml#PrimeMeridianType"/>
      <rdfs:range rdf:resource="http://www.opengis.net/gml#meridianID"/>
   </owl:ObjectProperty>
   <owl:ObjectProperty rdf:about="http://www.opengis.net/gml#hasremarks">
      <rdfs:comment>Warning: This ObjectProperty reference was declared outside of its original schema. This ObjectProperty may be declared incorrectly.</rdfs:comment>
      <rdfs:domain rdf:resource="http://www.opengis.net/gml#PrimeMeridianType"/>
      <rdfs:range rdf:resource="http://www.opengis.net/gml#remarks"/>
   </owl:ObjectProperty>
   <owl:ObjectProperty rdf:about="http://www.opengis.net/gml#hasgreenwichLongitude">
      <rdfs:comment>Warning: This ObjectProperty reference was declared outside of its original schema. This ObjectProperty may be declared incorrectly.</rdfs:comment>
      <rdfs:domain rdf:resource="http://www.opengis.net/gml#PrimeMeridianType"/>
      <rdfs:range rdf:resource="http://www.opengis.net/gml#greenwichLongitude"/>
   </owl:ObjectProperty>
   <owl:ObjectProperty rdf:about="http://www.opengis.net/gml#hasPrimeMeridian">
      <rdfs:comment>Warning: This ObjectProperty reference was declared outside of its original schema. This ObjectProperty may be declared incorrectly.</rdfs:comment>
      <rdfs:domain rdf:resource="http://www.opengis.net/gml#PrimeMeridianRefType"/>
      <rdfs:range rdf:resource="http://www.opengis.net/gml#PrimeMeridian"/>
   </owl:ObjectProperty>
   <owl:ObjectProperty rdf:about="http://www.opengis.net/gml#hasmetaDataProperty">
      <rdfs:comment>Warning: This ObjectProperty reference was declared outside of its original schema. This ObjectProperty may be declared incorrectly.</rdfs:comment>
      <rdfs:domain rdf:resource="http://www.opengis.net/gml#EllipsoidBaseType"/>
      <rdfs:range rdf:resource="http://www.opengis.net/gml#metaDataProperty"/>
   </owl:ObjectProperty>
   <owl:ObjectProperty rdf:about="http://www.opengis.net/gml#hasellipsoidName">
      <rdfs:comment>Warning: This ObjectProperty reference was declared outside of its original schema. This ObjectProperty may be declared incorrectly.</rdfs:comment>
      <rdfs:domain rdf:resource="http://www.opengis.net/gml#EllipsoidBaseType"/>
      <rdfs:range rdf:resource="http://www.opengis.net/gml#ellipsoidName"/>
   </owl:ObjectProperty>
   <owl:ObjectProperty rdf:about="http://www.opengis.net/gml#hasellipsoidID">
      <rdfs:comment>Warning: This ObjectProperty reference was declared outside of its original schema. This ObjectProperty may be declared incorrectly.</rdfs:comment>
      <rdfs:domain rdf:resource="http://www.opengis.net/gml#EllipsoidType"/>
      <rdfs:range rdf:resource="http://www.opengis.net/gml#ellipsoidID"/>
   </owl:ObjectProperty>
   <owl:ObjectProperty rdf:about="http://www.opengis.net/gml#hasremarks">
      <rdfs:comment>Warning: This ObjectProperty reference was declared outside of its original schema. This ObjectProperty may be declared incorrectly.</rdfs:comment>
      <rdfs:domain rdf:resource="http://www.opengis.net/gml#EllipsoidType"/>
      <rdfs:range rdf:resource="http://www.opengis.net/gml#remarks"/>
   </owl:ObjectProperty>
   <owl:ObjectProperty rdf:about="http://www.opengis.net/gml#hassemiMajorAxis">
      <rdfs:comment>Warning: This ObjectProperty reference was declared outside of its original schema. This ObjectProperty may be declared incorrectly.</rdfs:comment>
      <rdfs:domain rdf:resource="http://www.opengis.net/gml#EllipsoidType"/>
      <rdfs:range rdf:resource="http://www.opengis.net/gml#semiMajorAxis"/>
   </owl:ObjectProperty>
   <owl:ObjectProperty rdf:about="http://www.opengis.net/gml#hassecondDefiningParameter">
      <rdfs:comment>Warning: This ObjectProperty reference was declared outside of its original schema. This ObjectProperty may be declared incorrectly.</rdfs:comment>
      <rdfs:domain rdf:resource="http://www.opengis.net/gml#EllipsoidType"/>
      <rdfs:range rdf:resource="http://www.opengis.net/gml#secondDefiningParameter"/>
   </owl:ObjectProperty>
   <owl:ObjectProperty rdf:about="http://www.opengis.net/gml#hasEllipsoid">
      <rdfs:comment>Warning: This ObjectProperty reference was declared outside of its original schema. This ObjectProperty may be declared incorrectly.</rdfs:comment>
      <rdfs:domain rdf:resource="http://www.opengis.net/gml#EllipsoidRefType"/>
      <rdfs:range rdf:resource="http://www.opengis.net/gml#Ellipsoid"/>
   </owl:ObjectProperty>
   <owl:ObjectProperty rdf:about="http://www.opengis.net/gml#hasinverseFlattening">
      <rdfs:comment>Warning: This ObjectProperty reference was declared outside of its original schema. This ObjectProperty may be declared incorrectly.</rdfs:comment>
      <rdfs:domain rdf:resource="http://www.opengis.net/gml#SecondDefiningParameterType"/>
      <rdfs:range rdf:resource="http://www.opengis.net/gml#inverseFlattening"/>
   </owl:ObjectProperty>
   <owl:ObjectProperty rdf:about="http://www.opengis.net/gml#hassemiMinorAxis">
      <rdfs:comment>Warning: This ObjectProperty reference was declared outside of its original schema. This ObjectProperty may be declared incorrectly.</rdfs:comment>
      <rdfs:domain rdf:resource="http://www.opengis.net/gml#SecondDefiningParameterType"/>
      <rdfs:range rdf:resource="http://www.opengis.net/gml#semiMinorAxis"/>
   </owl:ObjectProperty>
   <owl:ObjectProperty rdf:about="http://www.opengis.net/gml#hasisSphere">
      <rdfs:comment>Warning: This ObjectProperty reference was declared outside of its original schema. This ObjectProperty may be declared incorrectly.</rdfs:comment>
      <rdfs:domain rdf:resource="http://www.opengis.net/gml#SecondDefiningParameterType"/>
      <rdfs:range rdf:resource="http://www.opengis.net/gml#isSphere"/>
   </owl:ObjectProperty>
   <owl:ObjectProperty rdf:about="http://www.opengis.net/gml#hasmetaDataProperty">
      <rdfs:comment>Warning: This ObjectProperty reference was declared outside of its original schema. This ObjectProperty may be declared incorrectly.</rdfs:comment>
      <rdfs:domain rdf:resource="http://www.opengis.net/gml#AbstractCoordinateOperationBaseType"/>
      <rdfs:range rdf:resource="http://www.opengis.net/gml#metaDataProperty"/>
   </owl:ObjectProperty>
   <owl:ObjectProperty rdf:about="http://www.opengis.net/gml#hascoordinateOperationName">
      <rdfs:comment>Warning: This ObjectProperty reference was declared outside of its original schema. This ObjectProperty may be declared incorrectly.</rdfs:comment>
      <rdfs:domain rdf:resource="http://www.opengis.net/gml#AbstractCoordinateOperationBaseType"/>
      <rdfs:range rdf:resource="http://www.opengis.net/gml#coordinateOperationName"/>
   </owl:ObjectProperty>
   <owl:ObjectProperty rdf:about="http://www.opengis.net/gml#hascoordinateOperationID">
      <rdfs:comment>Warning: This ObjectProperty reference was declared outside of its original schema. This ObjectProperty may be declared incorrectly.</rdfs:comment>
      <rdfs:domain rdf:resource="http://www.opengis.net/gml#AbstractCoordinateOperationType"/>
      <rdfs:range rdf:resource="http://www.opengis.net/gml#coordinateOperationID"/>
   </owl:ObjectProperty>
   <owl:ObjectProperty rdf:about="http://www.opengis.net/gml#hasremarks">
      <rdfs:comment>Warning: This ObjectProperty reference was declared outside of its original schema. This ObjectProperty may be declared incorrectly.</rdfs:comment>
      <rdfs:domain rdf:resource="http://www.opengis.net/gml#AbstractCoordinateOperationType"/>
      <rdfs:range rdf:resource="http://www.opengis.net/gml#remarks"/>
   </owl:ObjectProperty>
   <owl:ObjectProperty rdf:about="http://www.opengis.net/gml#hasoperationVersion">
      <rdfs:comment>Warning: This ObjectProperty reference was declared outside of its original schema. This ObjectProperty may be declared incorrectly.</rdfs:comment>
      <rdfs:domain rdf:resource="http://www.opengis.net/gml#AbstractCoordinateOperationType"/>
      <rdfs:range rdf:resource="http://www.opengis.net/gml#operationVersion"/>
   </owl:ObjectProperty>
   <owl:ObjectProperty rdf:about="http://www.opengis.net/gml#hasvalidArea">
      <rdfs:comment>Warning: This ObjectProperty reference was declared outside of its original schema. This ObjectProperty may be declared incorrectly.</rdfs:comment>
      <rdfs:domain rdf:resource="http://www.opengis.net/gml#AbstractCoordinateOperationType"/>
      <rdfs:range rdf:resource="http://www.opengis.net/gml#validArea"/>
   </owl:ObjectProperty>
   <owl:ObjectProperty rdf:about="http://www.opengis.net/gml#hasscope">
      <rdfs:comment>Warning: This ObjectProperty reference was declared outside of its original schema. This ObjectProperty may be declared incorrectly.</rdfs:comment>
      <rdfs:domain rdf:resource="http://www.opengis.net/gml#AbstractCoordinateOperationType"/>
      <rdfs:range rdf:resource="http://www.opengis.net/gml#scope"/>
   </owl:ObjectProperty>
   <owl:ObjectProperty rdf:about="http://www.opengis.net/gml#has_positionalAccuracy">
      <rdfs:comment>Warning: This ObjectProperty reference was declared outside of its original schema. This ObjectProperty may be declared incorrectly.</rdfs:comment>
      <rdfs:domain rdf:resource="http://www.opengis.net/gml#AbstractCoordinateOperationType"/>
      <rdfs:range rdf:resource="http://www.opengis.net/gml#_positionalAccuracy"/>
   </owl:ObjectProperty>
   <owl:ObjectProperty rdf:about="http://www.opengis.net/gml#hassourceCRS">
      <rdfs:comment>Warning: This ObjectProperty reference was declared outside of its original schema. This ObjectProperty may be declared incorrectly.</rdfs:comment>
      <rdfs:domain rdf:resource="http://www.opengis.net/gml#AbstractCoordinateOperationType"/>
      <rdfs:range rdf:resource="http://www.opengis.net/gml#sourceCRS"/>
   </owl:ObjectProperty>
   <owl:ObjectProperty rdf:about="http://www.opengis.net/gml#hastargetCRS">
      <rdfs:comment>Warning: This ObjectProperty reference was declared outside of its original schema. This ObjectProperty may be declared incorrectly.</rdfs:comment>
      <rdfs:domain rdf:resource="http://www.opengis.net/gml#AbstractCoordinateOperationType"/>
      <rdfs:range rdf:resource="http://www.opengis.net/gml#targetCRS"/>
   </owl:ObjectProperty>
   <owl:ObjectProperty rdf:about="http://www.opengis.net/gml#has_CoordinateOperation">
      <rdfs:comment>Warning: This ObjectProperty reference was declared outside of its original schema. This ObjectProperty may be declared incorrectly.</rdfs:comment>
      <rdfs:domain rdf:resource="http://www.opengis.net/gml#CoordinateOperationRefType"/>
      <rdfs:range rdf:resource="http://www.opengis.net/gml#_CoordinateOperation"/>
   </owl:ObjectProperty>
   <owl:ObjectProperty rdf:about="http://www.opengis.net/gml#hasusesSingleOperation">
      <rdfs:comment>Warning: This ObjectProperty reference was declared outside of its original schema. This ObjectProperty may be declared incorrectly.</rdfs:comment>
      <rdfs:domain rdf:resource="http://www.opengis.net/gml#ConcatenatedOperationType"/>
      <rdfs:range rdf:resource="http://www.opengis.net/gml#usesSingleOperation"/>
   </owl:ObjectProperty>
   <owl:ObjectProperty rdf:about="http://www.opengis.net/gml#hasConcatenatedOperation">
      <rdfs:comment>Warning: This ObjectProperty reference was declared outside of its original schema. This ObjectProperty may be declared incorrectly.</rdfs:comment>
      <rdfs:domain rdf:resource="http://www.opengis.net/gml#ConcatenatedOperationRefType"/>
      <rdfs:range rdf:resource="http://www.opengis.net/gml#ConcatenatedOperation"/>
   </owl:ObjectProperty>
   <owl:ObjectProperty rdf:about="http://www.opengis.net/gml#has_SingleOperation">
      <rdfs:comment>Warning: This ObjectProperty reference was declared outside of its original schema. This ObjectProperty may be declared incorrectly.</rdfs:comment>
      <rdfs:domain rdf:resource="http://www.opengis.net/gml#SingleOperationRefType"/>
      <rdfs:range rdf:resource="http://www.opengis.net/gml#_SingleOperation"/>
   </owl:ObjectProperty>
   <owl:ObjectProperty rdf:about="http://www.opengis.net/gml#hasmodifiedCoordinate">
      <rdfs:comment>Warning: This ObjectProperty reference was declared outside of its original schema. This ObjectProperty may be declared incorrectly.</rdfs:comment>
      <rdfs:domain rdf:resource="http://www.opengis.net/gml#PassThroughOperationType"/>
      <rdfs:range rdf:resource="http://www.opengis.net/gml#modifiedCoordinate"/>
   </owl:ObjectProperty>
   <owl:ObjectProperty rdf:about="http://www.opengis.net/gml#hasusesOperation">
      <rdfs:comment>Warning: This ObjectProperty reference was declared outside of its original schema. This ObjectProperty may be declared incorrectly.</rdfs:comment>
      <rdfs:domain rdf:resource="http://www.opengis.net/gml#PassThroughOperationType"/>
      <rdfs:range rdf:resource="http://www.opengis.net/gml#usesOperation"/>
   </owl:ObjectProperty>
   <owl:ObjectProperty rdf:about="http://www.opengis.net/gml#hasPassThroughOperation">
      <rdfs:comment>Warning: This ObjectProperty reference was declared outside of its original schema. This ObjectProperty may be declared incorrectly.</rdfs:comment>
      <rdfs:domain rdf:resource="http://www.opengis.net/gml#PassThroughOperationRefType"/>
      <rdfs:range rdf:resource="http://www.opengis.net/gml#PassThroughOperation"/>
   </owl:ObjectProperty>
   <owl:ObjectProperty rdf:about="http://www.opengis.net/gml#has_Operation">
      <rdfs:comment>Warning: This ObjectProperty reference was declared outside of its original schema. This ObjectProperty may be declared incorrectly.</rdfs:comment>
      <rdfs:domain rdf:resource="http://www.opengis.net/gml#OperationRefType"/>
      <rdfs:range rdf:resource="http://www.opengis.net/gml#_Operation"/>
   </owl:ObjectProperty>
   <owl:ObjectProperty rdf:about="http://www.opengis.net/gml#hasmetaDataProperty">
      <rdfs:comment>Warning: This ObjectProperty reference was declared outside of its original schema. This ObjectProperty may be declared incorrectly.</rdfs:comment>
      <rdfs:domain rdf:resource="http://www.opengis.net/gml#AbstractGeneralConversionType"/>
      <rdfs:range rdf:resource="http://www.opengis.net/gml#metaDataProperty"/>
   </owl:ObjectProperty>
   <owl:ObjectProperty rdf:about="http://www.opengis.net/gml#hascoordinateOperationName">
      <rdfs:comment>Warning: This ObjectProperty reference was declared outside of its original schema. This ObjectProperty may be declared incorrectly.</rdfs:comment>
      <rdfs:domain rdf:resource="http://www.opengis.net/gml#AbstractGeneralConversionType"/>
      <rdfs:range rdf:resource="http://www.opengis.net/gml#coordinateOperationName"/>
   </owl:ObjectProperty>
   <owl:ObjectProperty rdf:about="http://www.opengis.net/gml#hascoordinateOperationID">
      <rdfs:comment>Warning: This ObjectProperty reference was declared outside of its original schema. This ObjectProperty may be declared incorrectly.</rdfs:comment>
      <rdfs:domain rdf:resource="http://www.opengis.net/gml#AbstractGeneralConversionType"/>
      <rdfs:range rdf:resource="http://www.opengis.net/gml#coordinateOperationID"/>
   </owl:ObjectProperty>
   <owl:ObjectProperty rdf:about="http://www.opengis.net/gml#hasremarks">
      <rdfs:comment>Warning: This ObjectProperty reference was declared outside of its original schema. This ObjectProperty may be declared incorrectly.</rdfs:comment>
      <rdfs:domain rdf:resource="http://www.opengis.net/gml#AbstractGeneralConversionType"/>
      <rdfs:range rdf:resource="http://www.opengis.net/gml#remarks"/>
   </owl:ObjectProperty>
   <owl:ObjectProperty rdf:about="http://www.opengis.net/gml#hasvalidArea">
      <rdfs:comment>Warning: This ObjectProperty reference was declared outside of its original schema. This ObjectProperty may be declared incorrectly.</rdfs:comment>
      <rdfs:domain rdf:resource="http://www.opengis.net/gml#AbstractGeneralConversionType"/>
      <rdfs:range rdf:resource="http://www.opengis.net/gml#validArea"/>
   </owl:ObjectProperty>
   <owl:ObjectProperty rdf:about="http://www.opengis.net/gml#hasscope">
      <rdfs:comment>Warning: This ObjectProperty reference was declared outside of its original schema. This ObjectProperty may be declared incorrectly.</rdfs:comment>
      <rdfs:domain rdf:resource="http://www.opengis.net/gml#AbstractGeneralConversionType"/>
      <rdfs:range rdf:resource="http://www.opengis.net/gml#scope"/>
   </owl:ObjectProperty>
   <owl:ObjectProperty rdf:about="http://www.opengis.net/gml#has_positionalAccuracy">
      <rdfs:comment>Warning: This ObjectProperty reference was declared outside of its original schema. This ObjectProperty may be declared incorrectly.</rdfs:comment>
      <rdfs:domain rdf:resource="http://www.opengis.net/gml#AbstractGeneralConversionType"/>
      <rdfs:range rdf:resource="http://www.opengis.net/gml#_positionalAccuracy"/>
   </owl:ObjectProperty>
   <owl:ObjectProperty rdf:about="http://www.opengis.net/gml#has_GeneralConversion">
      <rdfs:comment>Warning: This ObjectProperty reference was declared outside of its original schema. This ObjectProperty may be declared incorrectly.</rdfs:comment>
      <rdfs:domain rdf:resource="http://www.opengis.net/gml#GeneralConversionRefType"/>
      <rdfs:range rdf:resource="http://www.opengis.net/gml#_GeneralConversion"/>
   </owl:ObjectProperty>
   <owl:ObjectProperty rdf:about="http://www.opengis.net/gml#hasusesMethod">
      <rdfs:comment>Warning: This ObjectProperty reference was declared outside of its original schema. This ObjectProperty may be declared incorrectly.</rdfs:comment>
      <rdfs:domain rdf:resource="http://www.opengis.net/gml#ConversionType"/>
      <rdfs:range rdf:resource="http://www.opengis.net/gml#usesMethod"/>
   </owl:ObjectProperty>
   <owl:ObjectProperty rdf:about="http://www.opengis.net/gml#hasusesValue">
      <rdfs:comment>Warning: This ObjectProperty reference was declared outside of its original schema. This ObjectProperty may be declared incorrectly.</rdfs:comment>
      <rdfs:domain rdf:resource="http://www.opengis.net/gml#ConversionType"/>
      <rdfs:range rdf:resource="http://www.opengis.net/gml#usesValue"/>
   </owl:ObjectProperty>
   <owl:ObjectProperty rdf:about="http://www.opengis.net/gml#hasConversion">
      <rdfs:comment>Warning: This ObjectProperty reference was declared outside of its original schema. This ObjectProperty may be declared incorrectly.</rdfs:comment>
      <rdfs:domain rdf:resource="http://www.opengis.net/gml#ConversionRefType"/>
      <rdfs:range rdf:resource="http://www.opengis.net/gml#Conversion"/>
   </owl:ObjectProperty>
   <owl:ObjectProperty rdf:about="http://www.opengis.net/gml#hasmetaDataProperty">
      <rdfs:comment>Warning: This ObjectProperty reference was declared outside of its original schema. This ObjectProperty may be declared incorrectly.</rdfs:comment>
      <rdfs:domain rdf:resource="http://www.opengis.net/gml#AbstractGeneralTransformationType"/>
      <rdfs:range rdf:resource="http://www.opengis.net/gml#metaDataProperty"/>
   </owl:ObjectProperty>
   <owl:ObjectProperty rdf:about="http://www.opengis.net/gml#hascoordinateOperationName">
      <rdfs:comment>Warning: This ObjectProperty reference was declared outside of its original schema. This ObjectProperty may be declared incorrectly.</rdfs:comment>
      <rdfs:domain rdf:resource="http://www.opengis.net/gml#AbstractGeneralTransformationType"/>
      <rdfs:range rdf:resource="http://www.opengis.net/gml#coordinateOperationName"/>
   </owl:ObjectProperty>
   <owl:ObjectProperty rdf:about="http://www.opengis.net/gml#hascoordinateOperationID">
      <rdfs:comment>Warning: This ObjectProperty reference was declared outside of its original schema. This ObjectProperty may be declared incorrectly.</rdfs:comment>
      <rdfs:domain rdf:resource="http://www.opengis.net/gml#AbstractGeneralTransformationType"/>
      <rdfs:range rdf:resource="http://www.opengis.net/gml#coordinateOperationID"/>
   </owl:ObjectProperty>
   <owl:ObjectProperty rdf:about="http://www.opengis.net/gml#hasremarks">
      <rdfs:comment>Warning: This ObjectProperty reference was declared outside of its original schema. This ObjectProperty may be declared incorrectly.</rdfs:comment>
      <rdfs:domain rdf:resource="http://www.opengis.net/gml#AbstractGeneralTransformationType"/>
      <rdfs:range rdf:resource="http://www.opengis.net/gml#remarks"/>
   </owl:ObjectProperty>
   <owl:ObjectProperty rdf:about="http://www.opengis.net/gml#hasoperationVersion">
      <rdfs:comment>Warning: This ObjectProperty reference was declared outside of its original schema. This ObjectProperty may be declared incorrectly.</rdfs:comment>
      <rdfs:domain rdf:resource="http://www.opengis.net/gml#AbstractGeneralTransformationType"/>
      <rdfs:range rdf:resource="http://www.opengis.net/gml#operationVersion"/>
   </owl:ObjectProperty>
   <owl:ObjectProperty rdf:about="http://www.opengis.net/gml#hasvalidArea">
      <rdfs:comment>Warning: This ObjectProperty reference was declared outside of its original schema. This ObjectProperty may be declared incorrectly.</rdfs:comment>
      <rdfs:domain rdf:resource="http://www.opengis.net/gml#AbstractGeneralTransformationType"/>
      <rdfs:range rdf:resource="http://www.opengis.net/gml#validArea"/>
   </owl:ObjectProperty>
   <owl:ObjectProperty rdf:about="http://www.opengis.net/gml#hasscope">
      <rdfs:comment>Warning: This ObjectProperty reference was declared outside of its original schema. This ObjectProperty may be declared incorrectly.</rdfs:comment>
      <rdfs:domain rdf:resource="http://www.opengis.net/gml#AbstractGeneralTransformationType"/>
      <rdfs:range rdf:resource="http://www.opengis.net/gml#scope"/>
   </owl:ObjectProperty>
   <owl:ObjectProperty rdf:about="http://www.opengis.net/gml#has_positionalAccuracy">
      <rdfs:comment>Warning: This ObjectProperty reference was declared outside of its original schema. This ObjectProperty may be declared incorrectly.</rdfs:comment>
      <rdfs:domain rdf:resource="http://www.opengis.net/gml#AbstractGeneralTransformationType"/>
      <rdfs:range rdf:resource="http://www.opengis.net/gml#_positionalAccuracy"/>
   </owl:ObjectProperty>
   <owl:ObjectProperty rdf:about="http://www.opengis.net/gml#hassourceCRS">
      <rdfs:comment>Warning: This ObjectProperty reference was declared outside of its original schema. This ObjectProperty may be declared incorrectly.</rdfs:comment>
      <rdfs:domain rdf:resource="http://www.opengis.net/gml#AbstractGeneralTransformationType"/>
      <rdfs:range rdf:resource="http://www.opengis.net/gml#sourceCRS"/>
   </owl:ObjectProperty>
   <owl:ObjectProperty rdf:about="http://www.opengis.net/gml#hastargetCRS">
      <rdfs:comment>Warning: This ObjectProperty reference was declared outside of its original schema. This ObjectProperty may be declared incorrectly.</rdfs:comment>
      <rdfs:domain rdf:resource="http://www.opengis.net/gml#AbstractGeneralTransformationType"/>
      <rdfs:range rdf:resource="http://www.opengis.net/gml#targetCRS"/>
   </owl:ObjectProperty>
   <owl:ObjectProperty rdf:about="http://www.opengis.net/gml#has_GeneralTransformation">
      <rdfs:comment>Warning: This ObjectProperty reference was declared outside of its original schema. This ObjectProperty may be declared incorrectly.</rdfs:comment>
      <rdfs:domain rdf:resource="http://www.opengis.net/gml#GeneralTransformationRefType"/>
      <rdfs:range rdf:resource="http://www.opengis.net/gml#_GeneralTransformation"/>
   </owl:ObjectProperty>
   <owl:ObjectProperty rdf:about="http://www.opengis.net/gml#hasusesMethod">
      <rdfs:comment>Warning: This ObjectProperty reference was declared outside of its original schema. This ObjectProperty may be declared incorrectly.</rdfs:comment>
      <rdfs:domain rdf:resource="http://www.opengis.net/gml#TransformationType"/>
      <rdfs:range rdf:resource="http://www.opengis.net/gml#usesMethod"/>
   </owl:ObjectProperty>
   <owl:ObjectProperty rdf:about="http://www.opengis.net/gml#hasusesValue">
      <rdfs:comment>Warning: This ObjectProperty reference was declared outside of its original schema. This ObjectProperty may be declared incorrectly.</rdfs:comment>
      <rdfs:domain rdf:resource="http://www.opengis.net/gml#TransformationType"/>
      <rdfs:range rdf:resource="http://www.opengis.net/gml#usesValue"/>
   </owl:ObjectProperty>
   <owl:ObjectProperty rdf:about="http://www.opengis.net/gml#hasTransformation">
      <rdfs:comment>Warning: This ObjectProperty reference was declared outside of its original schema. This ObjectProperty may be declared incorrectly.</rdfs:comment>
      <rdfs:domain rdf:resource="http://www.opengis.net/gml#TransformationRefType"/>
      <rdfs:range rdf:resource="http://www.opengis.net/gml#Transformation"/>
   </owl:ObjectProperty>
   <owl:ObjectProperty rdf:about="http://www.opengis.net/gml#hasvalue">
      <rdfs:comment>Warning: This ObjectProperty reference was declared outside of its original schema. This ObjectProperty may be declared incorrectly.</rdfs:comment>
      <rdfs:domain rdf:resource="http://www.opengis.net/gml#ParameterValueType"/>
      <rdfs:range rdf:resource="http://www.opengis.net/gml#value"/>
   </owl:ObjectProperty>
   <owl:ObjectProperty rdf:about="http://www.opengis.net/gml#hasdmsAngleValue">
      <rdfs:comment>Warning: This ObjectProperty reference was declared outside of its original schema. This ObjectProperty may be declared incorrectly.</rdfs:comment>
      <rdfs:domain rdf:resource="http://www.opengis.net/gml#ParameterValueType"/>
      <rdfs:range rdf:resource="http://www.opengis.net/gml#dmsAngleValue"/>
   </owl:ObjectProperty>
   <owl:ObjectProperty rdf:about="http://www.opengis.net/gml#hasstringValue">
      <rdfs:comment>Warning: This ObjectProperty reference was declared outside of its original schema. This ObjectProperty may be declared incorrectly.</rdfs:comment>
      <rdfs:domain rdf:resource="http://www.opengis.net/gml#ParameterValueType"/>
      <rdfs:range rdf:resource="http://www.opengis.net/gml#stringValue"/>
   </owl:ObjectProperty>
   <owl:ObjectProperty rdf:about="http://www.opengis.net/gml#hasintegerValue">
      <rdfs:comment>Warning: This ObjectProperty reference was declared outside of its original schema. This ObjectProperty may be declared incorrectly.</rdfs:comment>
      <rdfs:domain rdf:resource="http://www.opengis.net/gml#ParameterValueType"/>
      <rdfs:range rdf:resource="http://www.opengis.net/gml#integerValue"/>
   </owl:ObjectProperty>
   <owl:ObjectProperty rdf:about="http://www.opengis.net/gml#hasbooleanValue">
      <rdfs:comment>Warning: This ObjectProperty reference was declared outside of its original schema. This ObjectProperty may be declared incorrectly.</rdfs:comment>
      <rdfs:domain rdf:resource="http://www.opengis.net/gml#ParameterValueType"/>
      <rdfs:range rdf:resource="http://www.opengis.net/gml#booleanValue"/>
   </owl:ObjectProperty>
   <owl:ObjectProperty rdf:about="http://www.opengis.net/gml#hasvalueList">
      <rdfs:comment>Warning: This ObjectProperty reference was declared outside of its original schema. This ObjectProperty may be declared incorrectly.</rdfs:comment>
      <rdfs:domain rdf:resource="http://www.opengis.net/gml#ParameterValueType"/>
      <rdfs:range rdf:resource="http://www.opengis.net/gml#valueList"/>
   </owl:ObjectProperty>
   <owl:ObjectProperty rdf:about="http://www.opengis.net/gml#hasintegerValueList">
      <rdfs:comment>Warning: This ObjectProperty reference was declared outside of its original schema. This ObjectProperty may be declared incorrectly.</rdfs:comment>
      <rdfs:domain rdf:resource="http://www.opengis.net/gml#ParameterValueType"/>
      <rdfs:range rdf:resource="http://www.opengis.net/gml#integerValueList"/>
   </owl:ObjectProperty>
   <owl:ObjectProperty rdf:about="http://www.opengis.net/gml#hasvalueFile">
      <rdfs:comment>Warning: This ObjectProperty reference was declared outside of its original schema. This ObjectProperty may be declared incorrectly.</rdfs:comment>
      <rdfs:domain rdf:resource="http://www.opengis.net/gml#ParameterValueType"/>
      <rdfs:range rdf:resource="http://www.opengis.net/gml#valueFile"/>
   </owl:ObjectProperty>
   <owl:ObjectProperty rdf:about="http://www.opengis.net/gml#hasvalueOfParameter">
      <rdfs:comment>Warning: This ObjectProperty reference was declared outside of its original schema. This ObjectProperty may be declared incorrectly.</rdfs:comment>
      <rdfs:domain rdf:resource="http://www.opengis.net/gml#ParameterValueType"/>
      <rdfs:range rdf:resource="http://www.opengis.net/gml#valueOfParameter"/>
   </owl:ObjectProperty>
   <owl:ObjectProperty rdf:about="http://www.opengis.net/gml#hasincludesValue">
      <rdfs:comment>Warning: This ObjectProperty reference was declared outside of its original schema. This ObjectProperty may be declared incorrectly.</rdfs:comment>
      <rdfs:domain rdf:resource="http://www.opengis.net/gml#ParameterValueGroupType"/>
      <rdfs:range rdf:resource="http://www.opengis.net/gml#includesValue"/>
   </owl:ObjectProperty>
   <owl:ObjectProperty rdf:about="http://www.opengis.net/gml#hasvaluesOfGroup">
      <rdfs:comment>Warning: This ObjectProperty reference was declared outside of its original schema. This ObjectProperty may be declared incorrectly.</rdfs:comment>
      <rdfs:domain rdf:resource="http://www.opengis.net/gml#ParameterValueGroupType"/>
      <rdfs:range rdf:resource="http://www.opengis.net/gml#valuesOfGroup"/>
   </owl:ObjectProperty>
   <owl:ObjectProperty rdf:about="http://www.opengis.net/gml#hasmetaDataProperty">
      <rdfs:comment>Warning: This ObjectProperty reference was declared outside of its original schema. This ObjectProperty may be declared incorrectly.</rdfs:comment>
      <rdfs:domain rdf:resource="http://www.opengis.net/gml#OperationMethodBaseType"/>
      <rdfs:range rdf:resource="http://www.opengis.net/gml#metaDataProperty"/>
   </owl:ObjectProperty>
   <owl:ObjectProperty rdf:about="http://www.opengis.net/gml#hasmethodName">
      <rdfs:comment>Warning: This ObjectProperty reference was declared outside of its original schema. This ObjectProperty may be declared incorrectly.</rdfs:comment>
      <rdfs:domain rdf:resource="http://www.opengis.net/gml#OperationMethodBaseType"/>
      <rdfs:range rdf:resource="http://www.opengis.net/gml#methodName"/>
   </owl:ObjectProperty>
   <owl:ObjectProperty rdf:about="http://www.opengis.net/gml#hasmethodID">
      <rdfs:comment>Warning: This ObjectProperty reference was declared outside of its original schema. This ObjectProperty may be declared incorrectly.</rdfs:comment>
      <rdfs:domain rdf:resource="http://www.opengis.net/gml#OperationMethodType"/>
      <rdfs:range rdf:resource="http://www.opengis.net/gml#methodID"/>
   </owl:ObjectProperty>
   <owl:ObjectProperty rdf:about="http://www.opengis.net/gml#hasremarks">
      <rdfs:comment>Warning: This ObjectProperty reference was declared outside of its original schema. This ObjectProperty may be declared incorrectly.</rdfs:comment>
      <rdfs:domain rdf:resource="http://www.opengis.net/gml#OperationMethodType"/>
      <rdfs:range rdf:resource="http://www.opengis.net/gml#remarks"/>
   </owl:ObjectProperty>
   <owl:ObjectProperty rdf:about="http://www.opengis.net/gml#hasmethodFormula">
      <rdfs:comment>Warning: This ObjectProperty reference was declared outside of its original schema. This ObjectProperty may be declared incorrectly.</rdfs:comment>
      <rdfs:domain rdf:resource="http://www.opengis.net/gml#OperationMethodType"/>
      <rdfs:range rdf:resource="http://www.opengis.net/gml#methodFormula"/>
   </owl:ObjectProperty>
   <owl:ObjectProperty rdf:about="http://www.opengis.net/gml#hassourceDimensions">
      <rdfs:comment>Warning: This ObjectProperty reference was declared outside of its original schema. This ObjectProperty may be declared incorrectly.</rdfs:comment>
      <rdfs:domain rdf:resource="http://www.opengis.net/gml#OperationMethodType"/>
      <rdfs:range rdf:resource="http://www.opengis.net/gml#sourceDimensions"/>
   </owl:ObjectProperty>
   <owl:ObjectProperty rdf:about="http://www.opengis.net/gml#hastargetDimensions">
      <rdfs:comment>Warning: This ObjectProperty reference was declared outside of its original schema. This ObjectProperty may be declared incorrectly.</rdfs:comment>
      <rdfs:domain rdf:resource="http://www.opengis.net/gml#OperationMethodType"/>
      <rdfs:range rdf:resource="http://www.opengis.net/gml#targetDimensions"/>
   </owl:ObjectProperty>
   <owl:ObjectProperty rdf:about="http://www.opengis.net/gml#hasusesParameter">
      <rdfs:comment>Warning: This ObjectProperty reference was declared outside of its original schema. This ObjectProperty may be declared incorrectly.</rdfs:comment>
      <rdfs:domain rdf:resource="http://www.opengis.net/gml#OperationMethodType"/>
      <rdfs:range rdf:resource="http://www.opengis.net/gml#usesParameter"/>
   </owl:ObjectProperty>
   <owl:ObjectProperty rdf:about="http://www.opengis.net/gml#hasOperationMethod">
      <rdfs:comment>Warning: This ObjectProperty reference was declared outside of its original schema. This ObjectProperty may be declared incorrectly.</rdfs:comment>
      <rdfs:domain rdf:resource="http://www.opengis.net/gml#OperationMethodRefType"/>
      <rdfs:range rdf:resource="http://www.opengis.net/gml#OperationMethod"/>
   </owl:ObjectProperty>
   <owl:ObjectProperty rdf:about="http://www.opengis.net/gml#hasminimumOccurs">
      <rdfs:comment>Warning: This ObjectProperty reference was declared outside of its original schema. This ObjectProperty may be declared incorrectly.</rdfs:comment>
      <rdfs:domain rdf:resource="http://www.opengis.net/gml#AbstractGeneralOperationParameterType"/>
      <rdfs:range rdf:resource="http://www.opengis.net/gml#minimumOccurs"/>
   </owl:ObjectProperty>
   <owl:ObjectProperty rdf:about="http://www.opengis.net/gml#has_GeneralOperationParameter">
      <rdfs:comment>Warning: This ObjectProperty reference was declared outside of its original schema. This ObjectProperty may be declared incorrectly.</rdfs:comment>
      <rdfs:domain rdf:resource="http://www.opengis.net/gml#AbstractGeneralOperationParameterRefType"/>
      <rdfs:range rdf:resource="http://www.opengis.net/gml#_GeneralOperationParameter"/>
   </owl:ObjectProperty>
   <owl:ObjectProperty rdf:about="http://www.opengis.net/gml#hasmetaDataProperty">
      <rdfs:comment>Warning: This ObjectProperty reference was declared outside of its original schema. This ObjectProperty may be declared incorrectly.</rdfs:comment>
      <rdfs:domain rdf:resource="http://www.opengis.net/gml#OperationParameterBaseType"/>
      <rdfs:range rdf:resource="http://www.opengis.net/gml#metaDataProperty"/>
   </owl:ObjectProperty>
   <owl:ObjectProperty rdf:about="http://www.opengis.net/gml#hasparameterName">
      <rdfs:comment>Warning: This ObjectProperty reference was declared outside of its original schema. This ObjectProperty may be declared incorrectly.</rdfs:comment>
      <rdfs:domain rdf:resource="http://www.opengis.net/gml#OperationParameterBaseType"/>
      <rdfs:range rdf:resource="http://www.opengis.net/gml#parameterName"/>
   </owl:ObjectProperty>
   <owl:ObjectProperty rdf:about="http://www.opengis.net/gml#hasminimumOccurs">
      <rdfs:comment>Warning: This ObjectProperty reference was declared outside of its original schema. This ObjectProperty may be declared incorrectly.</rdfs:comment>
      <rdfs:domain rdf:resource="http://www.opengis.net/gml#OperationParameterBaseType"/>
      <rdfs:range rdf:resource="http://www.opengis.net/gml#minimumOccurs"/>
   </owl:ObjectProperty>
   <owl:ObjectProperty rdf:about="http://www.opengis.net/gml#hasparameterID">
      <rdfs:comment>Warning: This ObjectProperty reference was declared outside of its original schema. This ObjectProperty may be declared incorrectly.</rdfs:comment>
      <rdfs:domain rdf:resource="http://www.opengis.net/gml#OperationParameterType"/>
      <rdfs:range rdf:resource="http://www.opengis.net/gml#parameterID"/>
   </owl:ObjectProperty>
   <owl:ObjectProperty rdf:about="http://www.opengis.net/gml#hasremarks">
      <rdfs:comment>Warning: This ObjectProperty reference was declared outside of its original schema. This ObjectProperty may be declared incorrectly.</rdfs:comment>
      <rdfs:domain rdf:resource="http://www.opengis.net/gml#OperationParameterType"/>
      <rdfs:range rdf:resource="http://www.opengis.net/gml#remarks"/>
   </owl:ObjectProperty>
   <owl:ObjectProperty rdf:about="http://www.opengis.net/gml#hasOperationParameter">
      <rdfs:comment>Warning: This ObjectProperty reference was declared outside of its original schema. This ObjectProperty may be declared incorrectly.</rdfs:comment>
      <rdfs:domain rdf:resource="http://www.opengis.net/gml#OperationParameterRefType"/>
      <rdfs:range rdf:resource="http://www.opengis.net/gml#OperationParameter"/>
   </owl:ObjectProperty>
   <owl:ObjectProperty rdf:about="http://www.opengis.net/gml#hasmetaDataProperty">
      <rdfs:comment>Warning: This ObjectProperty reference was declared outside of its original schema. This ObjectProperty may be declared incorrectly.</rdfs:comment>
      <rdfs:domain rdf:resource="http://www.opengis.net/gml#OperationParameterGroupBaseType"/>
      <rdfs:range rdf:resource="http://www.opengis.net/gml#metaDataProperty"/>
   </owl:ObjectProperty>
   <owl:ObjectProperty rdf:about="http://www.opengis.net/gml#hasgroupName">
      <rdfs:comment>Warning: This ObjectProperty reference was declared outside of its original schema. This ObjectProperty may be declared incorrectly.</rdfs:comment>
      <rdfs:domain rdf:resource="http://www.opengis.net/gml#OperationParameterGroupBaseType"/>
      <rdfs:range rdf:resource="http://www.opengis.net/gml#groupName"/>
   </owl:ObjectProperty>
   <owl:ObjectProperty rdf:about="http://www.opengis.net/gml#hasminimumOccurs">
      <rdfs:comment>Warning: This ObjectProperty reference was declared outside of its original schema. This ObjectProperty may be declared incorrectly.</rdfs:comment>
      <rdfs:domain rdf:resource="http://www.opengis.net/gml#OperationParameterGroupBaseType"/>
      <rdfs:range rdf:resource="http://www.opengis.net/gml#minimumOccurs"/>
   </owl:ObjectProperty>
   <owl:ObjectProperty rdf:about="http://www.opengis.net/gml#hasgroupID">
      <rdfs:comment>Warning: This ObjectProperty reference was declared outside of its original schema. This ObjectProperty may be declared incorrectly.</rdfs:comment>
      <rdfs:domain rdf:resource="http://www.opengis.net/gml#OperationParameterGroupType"/>
      <rdfs:range rdf:resource="http://www.opengis.net/gml#groupID"/>
   </owl:ObjectProperty>
   <owl:ObjectProperty rdf:about="http://www.opengis.net/gml#hasremarks">
      <rdfs:comment>Warning: This ObjectProperty reference was declared outside of its original schema. This ObjectProperty may be declared incorrectly.</rdfs:comment>
      <rdfs:domain rdf:resource="http://www.opengis.net/gml#OperationParameterGroupType"/>
      <rdfs:range rdf:resource="http://www.opengis.net/gml#remarks"/>
   </owl:ObjectProperty>
   <owl:ObjectProperty rdf:about="http://www.opengis.net/gml#hasmaximumOccurs">
      <rdfs:comment>Warning: This ObjectProperty reference was declared outside of its original schema. This ObjectProperty may be declared incorrectly.</rdfs:comment>
      <rdfs:domain rdf:resource="http://www.opengis.net/gml#OperationParameterGroupType"/>
      <rdfs:range rdf:resource="http://www.opengis.net/gml#maximumOccurs"/>
   </owl:ObjectProperty>
   <owl:ObjectProperty rdf:about="http://www.opengis.net/gml#hasincludesParameter">
      <rdfs:comment>Warning: This ObjectProperty reference was declared outside of its original schema. This ObjectProperty may be declared incorrectly.</rdfs:comment>
      <rdfs:domain rdf:resource="http://www.opengis.net/gml#OperationParameterGroupType"/>
      <rdfs:range rdf:resource="http://www.opengis.net/gml#includesParameter"/>
   </owl:ObjectProperty>
   <owl:ObjectProperty rdf:about="http://www.opengis.net/gml#hasOperationParameterGroup">
      <rdfs:comment>Warning: This ObjectProperty reference was declared outside of its original schema. This ObjectProperty may be declared incorrectly.</rdfs:comment>
      <rdfs:domain rdf:resource="http://www.opengis.net/gml#OperationParameterGroupRefType"/>
      <rdfs:range rdf:resource="http://www.opengis.net/gml#OperationParameterGroup"/>
   </owl:ObjectProperty>
   <owl:ObjectProperty rdf:about="http://www.opengis.net/gml#hasmeasureDescription">
      <rdfs:comment>Warning: This ObjectProperty reference was declared outside of its original schema. This ObjectProperty may be declared incorrectly.</rdfs:comment>
      <rdfs:domain rdf:resource="http://www.opengis.net/gml#AbstractPositionalAccuracyType"/>
      <rdfs:range rdf:resource="http://www.opengis.net/gml#measureDescription"/>
   </owl:ObjectProperty>
   <owl:ObjectProperty rdf:about="http://www.opengis.net/gml#hasresult">
      <rdfs:comment>Warning: This ObjectProperty reference was declared outside of its original schema. This ObjectProperty may be declared incorrectly.</rdfs:comment>
      <rdfs:domain rdf:resource="http://www.opengis.net/gml#AbsoluteExternalPositionalAccuracyType"/>
      <rdfs:range rdf:resource="http://www.opengis.net/gml#result"/>
   </owl:ObjectProperty>
   <owl:ObjectProperty rdf:about="http://www.opengis.net/gml#hasresult">
      <rdfs:comment>Warning: This ObjectProperty reference was declared outside of its original schema. This ObjectProperty may be declared incorrectly.</rdfs:comment>
      <rdfs:domain rdf:resource="http://www.opengis.net/gml#RelativeInternalPositionalAccuracyType"/>
      <rdfs:range rdf:resource="http://www.opengis.net/gml#result"/>
   </owl:ObjectProperty>
   <owl:ObjectProperty rdf:about="http://www.opengis.net/gml#hasunitOfMeasure">
      <rdfs:comment>Warning: This ObjectProperty reference was declared outside of its original schema. This ObjectProperty may be declared incorrectly.</rdfs:comment>
      <rdfs:domain rdf:resource="http://www.opengis.net/gml#CovarianceMatrixType"/>
      <rdfs:range rdf:resource="http://www.opengis.net/gml#unitOfMeasure"/>
   </owl:ObjectProperty>
   <owl:ObjectProperty rdf:about="http://www.opengis.net/gml#hasincludesElement">
      <rdfs:comment>Warning: This ObjectProperty reference was declared outside of its original schema. This ObjectProperty may be declared incorrectly.</rdfs:comment>
      <rdfs:domain rdf:resource="http://www.opengis.net/gml#CovarianceMatrixType"/>
      <rdfs:range rdf:resource="http://www.opengis.net/gml#includesElement"/>
   </owl:ObjectProperty>
   <owl:ObjectProperty rdf:about="http://www.opengis.net/gml#hasrowIndex">
      <rdfs:comment>Warning: This ObjectProperty reference was declared outside of its original schema. This ObjectProperty may be declared incorrectly.</rdfs:comment>
      <rdfs:domain rdf:resource="http://www.opengis.net/gml#CovarianceElementType"/>
      <rdfs:range rdf:resource="http://www.opengis.net/gml#rowIndex"/>
   </owl:ObjectProperty>
   <owl:ObjectProperty rdf:about="http://www.opengis.net/gml#hascolumnIndex">
      <rdfs:comment>Warning: This ObjectProperty reference was declared outside of its original schema. This ObjectProperty may be declared incorrectly.</rdfs:comment>
      <rdfs:domain rdf:resource="http://www.opengis.net/gml#CovarianceElementType"/>
      <rdfs:range rdf:resource="http://www.opengis.net/gml#columnIndex"/>
   </owl:ObjectProperty>
   <owl:ObjectProperty rdf:about="http://www.opengis.net/gml#hascovariance">
      <rdfs:comment>Warning: This ObjectProperty reference was declared outside of its original schema. This ObjectProperty may be declared incorrectly.</rdfs:comment>
      <rdfs:domain rdf:resource="http://www.opengis.net/gml#CovarianceElementType"/>
      <rdfs:range rdf:resource="http://www.opengis.net/gml#covariance"/>
   </owl:ObjectProperty>
   <owl:ObjectProperty rdf:about="http://www.opengis.net/gml#has_Feature">
      <rdfs:comment>Warning: This ObjectProperty reference was declared outside of its original schema. This ObjectProperty may be declared incorrectly.</rdfs:comment>
      <rdfs:domain rdf:resource="http://www.opengis.net/gml#TargetPropertyType"/>
      <rdfs:range rdf:resource="http://www.opengis.net/gml#_Feature"/>
   </owl:ObjectProperty>
   <owl:ObjectProperty rdf:about="http://www.opengis.net/gml#has_Geometry">
      <rdfs:comment>Warning: This ObjectProperty reference was declared outside of its original schema. This ObjectProperty may be declared incorrectly.</rdfs:comment>
      <rdfs:domain rdf:resource="http://www.opengis.net/gml#TargetPropertyType"/>
      <rdfs:range rdf:resource="http://www.opengis.net/gml#_Geometry"/>
   </owl:ObjectProperty>
   <owl:ObjectProperty rdf:about="http://www.opengis.net/gml#hasvalidTime">
      <rdfs:comment>Warning: This ObjectProperty reference was declared outside of its original schema. This ObjectProperty may be declared incorrectly.</rdfs:comment>
      <rdfs:domain rdf:resource="http://www.opengis.net/gml#ObservationType"/>
      <rdfs:range rdf:resource="http://www.opengis.net/gml#validTime"/>
   </owl:ObjectProperty>
   <owl:ObjectProperty rdf:about="http://www.opengis.net/gml#hasusing">
      <rdfs:comment>Warning: This ObjectProperty reference was declared outside of its original schema. This ObjectProperty may be declared incorrectly.</rdfs:comment>
      <rdfs:domain rdf:resource="http://www.opengis.net/gml#ObservationType"/>
      <rdfs:range rdf:resource="http://www.opengis.net/gml#using"/>
   </owl:ObjectProperty>
   <owl:ObjectProperty rdf:about="http://www.opengis.net/gml#hastarget">
      <rdfs:comment>Warning: This ObjectProperty reference was declared outside of its original schema. This ObjectProperty may be declared incorrectly.</rdfs:comment>
      <rdfs:domain rdf:resource="http://www.opengis.net/gml#ObservationType"/>
      <rdfs:range rdf:resource="http://www.opengis.net/gml#target"/>
   </owl:ObjectProperty>
   <owl:ObjectProperty rdf:about="http://www.opengis.net/gml#hasresultOf">
      <rdfs:comment>Warning: This ObjectProperty reference was declared outside of its original schema. This ObjectProperty may be declared incorrectly.</rdfs:comment>
      <rdfs:domain rdf:resource="http://www.opengis.net/gml#ObservationType"/>
      <rdfs:range rdf:resource="http://www.opengis.net/gml#resultOf"/>
   </owl:ObjectProperty>
   <owl:ObjectProperty rdf:about="http://www.opengis.net/gml#hasdirection">
      <rdfs:comment>Warning: This ObjectProperty reference was declared outside of its original schema. This ObjectProperty may be declared incorrectly.</rdfs:comment>
      <rdfs:domain rdf:resource="http://www.opengis.net/gml#DirectedObservationType"/>
      <rdfs:range rdf:resource="http://www.opengis.net/gml#direction"/>
   </owl:ObjectProperty>
   <owl:ObjectProperty rdf:about="http://www.opengis.net/gml#distance">
      <rdfs:domain rdf:resource="http://www.opengis.net/gml#DirectedObservationAtDistanceType"/>
      <rdfs:range rdf:resource="http://www.opengis.net/gml#MeasureType"/>
   </owl:ObjectProperty>
   <owl:ObjectProperty rdf:about="http://www.opengis.net/gml#has_Style">
      <rdfs:comment>Warning: This ObjectProperty reference was declared outside of its original schema. This ObjectProperty may be declared incorrectly.</rdfs:comment>
      <rdfs:domain rdf:resource="http://www.opengis.net/gml#DefaultStylePropertyType"/>
      <rdfs:range rdf:resource="http://www.opengis.net/gml#_Style"/>
   </owl:ObjectProperty>
   <owl:ObjectProperty rdf:about="http://www.opengis.net/gml#hasfeatureStyle">
      <rdfs:comment>Warning: This ObjectProperty reference was declared outside of its original schema. This ObjectProperty may be declared incorrectly.</rdfs:comment>
      <rdfs:domain rdf:resource="http://www.opengis.net/gml#StyleType"/>
      <rdfs:range rdf:resource="http://www.opengis.net/gml#featureStyle"/>
   </owl:ObjectProperty>
   <owl:ObjectProperty rdf:about="http://www.opengis.net/gml#hasgraphStyle">
      <rdfs:comment>Warning: This ObjectProperty reference was declared outside of its original schema. This ObjectProperty may be declared incorrectly.</rdfs:comment>
      <rdfs:domain rdf:resource="http://www.opengis.net/gml#StyleType"/>
      <rdfs:range rdf:resource="http://www.opengis.net/gml#graphStyle"/>
   </owl:ObjectProperty>
   <owl:ObjectProperty rdf:about="http://www.opengis.net/gml#hasFeatureStyle">
      <rdfs:comment>Warning: This ObjectProperty reference was declared outside of its original schema. This ObjectProperty may be declared incorrectly.</rdfs:comment>
      <rdfs:domain rdf:resource="http://www.opengis.net/gml#FeatureStylePropertyType"/>
      <rdfs:range rdf:resource="http://www.opengis.net/gml#FeatureStyle"/>
   </owl:ObjectProperty>
   <owl:DatatypeProperty rdf:about="http://www.opengis.net/gml#featureConstraint">
      <rdfs:domain rdf:resource="http://www.opengis.net/gml#FeatureStyleType"/>
      <rdfs:range rdf:resource="http://www.w3.org/2001/XMLSchema#string"/>
   </owl:DatatypeProperty>
   <owl:ObjectProperty rdf:about="http://www.opengis.net/gml#hasgeometryStyle">
      <rdfs:comment>Warning: This ObjectProperty reference was declared outside of its original schema. This ObjectProperty may be declared incorrectly.</rdfs:comment>
      <rdfs:domain rdf:resource="http://www.opengis.net/gml#FeatureStyleType"/>
      <rdfs:range rdf:resource="http://www.opengis.net/gml#geometryStyle"/>
   </owl:ObjectProperty>
   <owl:ObjectProperty rdf:about="http://www.opengis.net/gml#hastopologyStyle">
      <rdfs:comment>Warning: This ObjectProperty reference was declared outside of its original schema. This ObjectProperty may be declared incorrectly.</rdfs:comment>
      <rdfs:domain rdf:resource="http://www.opengis.net/gml#FeatureStyleType"/>
      <rdfs:range rdf:resource="http://www.opengis.net/gml#topologyStyle"/>
   </owl:ObjectProperty>
   <owl:ObjectProperty rdf:about="http://www.opengis.net/gml#haslabelStyle">
      <rdfs:comment>Warning: This ObjectProperty reference was declared outside of its original schema. This ObjectProperty may be declared incorrectly.</rdfs:comment>
      <rdfs:domain rdf:resource="http://www.opengis.net/gml#FeatureStyleType"/>
      <rdfs:range rdf:resource="http://www.opengis.net/gml#labelStyle"/>
   </owl:ObjectProperty>
   <owl:ObjectProperty rdf:about="http://www.opengis.net/gml#spatialResolution">
      <rdfs:domain rdf:resource="http://www.opengis.net/gml#BaseStyleDescriptorType"/>
      <rdfs:range rdf:resource="http://www.opengis.net/gml#ScaleType"/>
   </owl:ObjectProperty>
   <owl:ObjectProperty rdf:about="http://www.opengis.net/gml#styleVariation">
      <rdfs:domain rdf:resource="http://www.opengis.net/gml#BaseStyleDescriptorType"/>
      <rdfs:range rdf:resource="http://www.opengis.net/gml#StyleVariationType"/>
   </owl:ObjectProperty>
   <owl:ObjectProperty rdf:about="smil20:hasanimate">
      <rdfs:comment>Warning: This ObjectProperty reference was declared outside of its original schema. This ObjectProperty may be declared incorrectly.</rdfs:comment>
      <rdfs:domain rdf:resource="http://www.opengis.net/gml#BaseStyleDescriptorType"/>
      <rdfs:range rdf:resource="smil20:animate"/>
   </owl:ObjectProperty>
   <owl:ObjectProperty rdf:about="smil20:hasanimateMotion">
      <rdfs:comment>Warning: This ObjectProperty reference was declared outside of its original schema. This ObjectProperty may be declared incorrectly.</rdfs:comment>
      <rdfs:domain rdf:resource="http://www.opengis.net/gml#BaseStyleDescriptorType"/>
      <rdfs:range rdf:resource="smil20:animateMotion"/>
   </owl:ObjectProperty>
   <owl:ObjectProperty rdf:about="smil20:hasanimateColor">
      <rdfs:comment>Warning: This ObjectProperty reference was declared outside of its original schema. This ObjectProperty may be declared incorrectly.</rdfs:comment>
      <rdfs:domain rdf:resource="http://www.opengis.net/gml#BaseStyleDescriptorType"/>
      <rdfs:range rdf:resource="smil20:animateColor"/>
   </owl:ObjectProperty>
   <owl:ObjectProperty rdf:about="smil20:hasset">
      <rdfs:comment>Warning: This ObjectProperty reference was declared outside of its original schema. This ObjectProperty may be declared incorrectly.</rdfs:comment>
      <rdfs:domain rdf:resource="http://www.opengis.net/gml#BaseStyleDescriptorType"/>
      <rdfs:range rdf:resource="smil20:set"/>
   </owl:ObjectProperty>
   <owl:ObjectProperty rdf:about="http://www.opengis.net/gml#hasGeometryStyle">
      <rdfs:comment>Warning: This ObjectProperty reference was declared outside of its original schema. This ObjectProperty may be declared incorrectly.</rdfs:comment>
      <rdfs:domain rdf:resource="http://www.opengis.net/gml#GeometryStylePropertyType"/>
      <rdfs:range rdf:resource="http://www.opengis.net/gml#GeometryStyle"/>
   </owl:ObjectProperty>
   <owl:ObjectProperty rdf:about="http://www.opengis.net/gml#hassymbol">
      <rdfs:comment>Warning: This ObjectProperty reference was declared outside of its original schema. This ObjectProperty may be declared incorrectly.</rdfs:comment>
      <rdfs:domain rdf:resource="http://www.opengis.net/gml#GeometryStyleType"/>
      <rdfs:range rdf:resource="http://www.opengis.net/gml#symbol"/>
   </owl:ObjectProperty>
   <owl:DatatypeProperty rdf:about="http://www.opengis.net/gml#style">
      <rdfs:domain rdf:resource="http://www.opengis.net/gml#GeometryStyleType"/>
      <rdfs:range rdf:resource="http://www.w3.org/2001/XMLSchema#string"/>
   </owl:DatatypeProperty>
   <owl:ObjectProperty rdf:about="http://www.opengis.net/gml#haslabelStyle">
      <rdfs:comment>Warning: This ObjectProperty reference was declared outside of its original schema. This ObjectProperty may be declared incorrectly.</rdfs:comment>
      <rdfs:domain rdf:resource="http://www.opengis.net/gml#GeometryStyleType"/>
      <rdfs:range rdf:resource="http://www.opengis.net/gml#labelStyle"/>
   </owl:ObjectProperty>
   <owl:ObjectProperty rdf:about="http://www.opengis.net/gml#hasTopologyStyle">
      <rdfs:comment>Warning: This ObjectProperty reference was declared outside of its original schema. This ObjectProperty may be declared incorrectly.</rdfs:comment>
      <rdfs:domain rdf:resource="http://www.opengis.net/gml#TopologyStylePropertyType"/>
      <rdfs:range rdf:resource="http://www.opengis.net/gml#TopologyStyle"/>
   </owl:ObjectProperty>
   <owl:ObjectProperty rdf:about="http://www.opengis.net/gml#hassymbol">
      <rdfs:comment>Warning: This ObjectProperty reference was declared outside of its original schema. This ObjectProperty may be declared incorrectly.</rdfs:comment>
      <rdfs:domain rdf:resource="http://www.opengis.net/gml#TopologyStyleType"/>
      <rdfs:range rdf:resource="http://www.opengis.net/gml#symbol"/>
   </owl:ObjectProperty>
   <owl:DatatypeProperty rdf:about="http://www.opengis.net/gml#style">
      <rdfs:domain rdf:resource="http://www.opengis.net/gml#TopologyStyleType"/>
      <rdfs:range rdf:resource="http://www.w3.org/2001/XMLSchema#string"/>
   </owl:DatatypeProperty>
   <owl:ObjectProperty rdf:about="http://www.opengis.net/gml#haslabelStyle">
      <rdfs:comment>Warning: This ObjectProperty reference was declared outside of its original schema. This ObjectProperty may be declared incorrectly.</rdfs:comment>
      <rdfs:domain rdf:resource="http://www.opengis.net/gml#TopologyStyleType"/>
      <rdfs:range rdf:resource="http://www.opengis.net/gml#labelStyle"/>
   </owl:ObjectProperty>
   <owl:ObjectProperty rdf:about="http://www.opengis.net/gml#hasLabelStyle">
      <rdfs:comment>Warning: This ObjectProperty reference was declared outside of its original schema. This ObjectProperty may be declared incorrectly.</rdfs:comment>
      <rdfs:domain rdf:resource="http://www.opengis.net/gml#LabelStylePropertyType"/>
      <rdfs:range rdf:resource="http://www.opengis.net/gml#LabelStyle"/>
   </owl:ObjectProperty>
   <owl:DatatypeProperty rdf:about="http://www.opengis.net/gml#style">
      <rdfs:domain rdf:resource="http://www.opengis.net/gml#LabelStyleType"/>
      <rdfs:range rdf:resource="http://www.w3.org/2001/XMLSchema#string"/>
   </owl:DatatypeProperty>
   <owl:ObjectProperty rdf:about="http://www.opengis.net/gml#label">
      <rdfs:domain rdf:resource="http://www.opengis.net/gml#LabelStyleType"/>
      <rdfs:range rdf:resource="http://www.opengis.net/gml#LabelType"/>
   </owl:ObjectProperty>
   <owl:ObjectProperty rdf:about="http://www.opengis.net/gml#hasGraphStyle">
      <rdfs:comment>Warning: This ObjectProperty reference was declared outside of its original schema. This ObjectProperty may be declared incorrectly.</rdfs:comment>
      <rdfs:domain rdf:resource="http://www.opengis.net/gml#GraphStylePropertyType"/>
      <rdfs:range rdf:resource="http://www.opengis.net/gml#GraphStyle"/>
   </owl:ObjectProperty>
   <owl:DatatypeProperty rdf:about="http://www.opengis.net/gml#planar">
      <rdfs:domain rdf:resource="http://www.opengis.net/gml#GraphStyleType"/>
      <rdfs:range rdf:resource="http://www.w3.org/2001/XMLSchema#boolean"/>
   </owl:DatatypeProperty>
   <owl:DatatypeProperty rdf:about="http://www.opengis.net/gml#directed">
      <rdfs:domain rdf:resource="http://www.opengis.net/gml#GraphStyleType"/>
      <rdfs:range rdf:resource="http://www.w3.org/2001/XMLSchema#boolean"/>
   </owl:DatatypeProperty>
   <owl:DatatypeProperty rdf:about="http://www.opengis.net/gml#grid">
      <rdfs:domain rdf:resource="http://www.opengis.net/gml#GraphStyleType"/>
      <rdfs:range rdf:resource="http://www.w3.org/2001/XMLSchema#boolean"/>
   </owl:DatatypeProperty>
   <owl:DatatypeProperty rdf:about="http://www.opengis.net/gml#minDistance">
      <rdfs:domain rdf:resource="http://www.opengis.net/gml#GraphStyleType"/>
      <rdfs:range rdf:resource="http://www.w3.org/2001/XMLSchema#double"/>
   </owl:DatatypeProperty>
   <owl:DatatypeProperty rdf:about="http://www.opengis.net/gml#minAngle">
      <rdfs:domain rdf:resource="http://www.opengis.net/gml#GraphStyleType"/>
      <rdfs:range rdf:resource="http://www.w3.org/2001/XMLSchema#double"/>
   </owl:DatatypeProperty>
   <owl:DatatypeProperty rdf:about="http://www.opengis.net/gml#graphType">
      <rdfs:domain rdf:resource="http://www.opengis.net/gml#GraphStyleType"/>
      <rdfs:range rdf:resource="http://www.opengis.net/gml#GraphTypeType"/>
   </owl:DatatypeProperty>
   <owl:DatatypeProperty rdf:about="http://www.opengis.net/gml#drawingType">
      <rdfs:domain rdf:resource="http://www.opengis.net/gml#GraphStyleType"/>
      <rdfs:range rdf:resource="http://www.opengis.net/gml#DrawingTypeType"/>
   </owl:DatatypeProperty>
   <owl:DatatypeProperty rdf:about="http://www.opengis.net/gml#lineType">
      <rdfs:domain rdf:resource="http://www.opengis.net/gml#GraphStyleType"/>
      <rdfs:range rdf:resource="http://www.opengis.net/gml#LineTypeType"/>
   </owl:DatatypeProperty>
   <owl:DatatypeProperty rdf:about="http://www.opengis.net/gml#aestheticCriteria">
      <rdfs:domain rdf:resource="http://www.opengis.net/gml#GraphStyleType"/>
      <rdfs:range rdf:resource="http://www.opengis.net/gml#AesheticCriteriaType"/>
   </owl:DatatypeProperty>
   <owl:DatatypeProperty rdf:about="http://www.opengis.net/gml#LabelExpression">
      <rdfs:domain rdf:resource="http://www.opengis.net/gml#LabelType"/>
      <rdfs:range rdf:resource="http://www.w3.org/2001/XMLSchema#string"/>
   </owl:DatatypeProperty>
   <owl:DatatypeProperty rdf:about="http://www.opengis.net/gml#domainOfValidity">
      <rdfs:domain rdf:resource="http://www.opengis.net/gml#AbstractTimeReferenceSystemType"/>
      <rdfs:range rdf:resource="http://www.w3.org/2001/XMLSchema#string"/>
   </owl:DatatypeProperty>
   <owl:ObjectProperty rdf:about="http://www.opengis.net/gml#originPosition">
      <rdfs:domain rdf:resource="http://www.opengis.net/gml#TimeCoordinateSystemType"/>
      <rdfs:range rdf:resource="http://www.opengis.net/gml#TimePositionType"/>
   </owl:ObjectProperty>
   <owl:ObjectProperty rdf:about="http://www.opengis.net/gml#origin">
      <rdfs:domain rdf:resource="http://www.opengis.net/gml#TimeCoordinateSystemType"/>
      <rdfs:range rdf:resource="http://www.opengis.net/gml#TimeInstantPropertyType"/>
   </owl:ObjectProperty>
   <owl:ObjectProperty rdf:about="http://www.opengis.net/gml#interval">
      <rdfs:domain rdf:resource="http://www.opengis.net/gml#TimeCoordinateSystemType"/>
      <rdfs:range rdf:resource="http://www.opengis.net/gml#TimeIntervalLengthType"/>
   </owl:ObjectProperty>
   <owl:ObjectProperty rdf:about="http://www.opengis.net/gml#component">
      <rdfs:domain rdf:resource="http://www.opengis.net/gml#TimeOrdinalReferenceSystemType"/>
      <rdfs:range rdf:resource="http://www.opengis.net/gml#TimeOrdinalEraPropertyType"/>
   </owl:ObjectProperty>
   <owl:ObjectProperty rdf:about="http://www.opengis.net/gml#relatedTime">
      <rdfs:domain rdf:resource="http://www.opengis.net/gml#TimeOrdinalEraType"/>
      <rdfs:range rdf:resource="http://www.opengis.net/gml#RelatedTimeType"/>
   </owl:ObjectProperty>
   <owl:ObjectProperty rdf:about="http://www.opengis.net/gml#start">
      <rdfs:domain rdf:resource="http://www.opengis.net/gml#TimeOrdinalEraType"/>
      <rdfs:range rdf:resource="http://www.opengis.net/gml#TimeNodePropertyType"/>
   </owl:ObjectProperty>
   <owl:ObjectProperty rdf:about="http://www.opengis.net/gml#end">
      <rdfs:domain rdf:resource="http://www.opengis.net/gml#TimeOrdinalEraType"/>
      <rdfs:range rdf:resource="http://www.opengis.net/gml#TimeNodePropertyType"/>
   </owl:ObjectProperty>
   <owl:ObjectProperty rdf:about="http://www.opengis.net/gml#extent">
      <rdfs:domain rdf:resource="http://www.opengis.net/gml#TimeOrdinalEraType"/>
      <rdfs:range rdf:resource="http://www.opengis.net/gml#TimePeriodPropertyType"/>
   </owl:ObjectProperty>
   <owl:ObjectProperty rdf:about="http://www.opengis.net/gml#member">
      <rdfs:domain rdf:resource="http://www.opengis.net/gml#TimeOrdinalEraType"/>
      <rdfs:range rdf:resource="http://www.opengis.net/gml#TimeOrdinalEraPropertyType"/>
   </owl:ObjectProperty>
   <owl:ObjectProperty rdf:about="http://www.opengis.net/gml#group">
      <rdfs:domain rdf:resource="http://www.opengis.net/gml#TimeOrdinalEraType"/>
      <rdfs:range rdf:resource="http://www.opengis.net/gml#ReferenceType"/>
   </owl:ObjectProperty>
   <owl:ObjectProperty rdf:about="http://www.opengis.net/gml#hasTimeOrdinalEra">
      <rdfs:comment>Warning: This ObjectProperty reference was declared outside of its original schema. This ObjectProperty may be declared incorrectly.</rdfs:comment>
      <rdfs:domain rdf:resource="http://www.opengis.net/gml#TimeOrdinalEraPropertyType"/>
      <rdfs:range rdf:resource="http://www.opengis.net/gml#TimeOrdinalEra"/>
   </owl:ObjectProperty>
   <owl:ObjectProperty rdf:about="http://www.opengis.net/gml#referenceFrame">
      <rdfs:domain rdf:resource="http://www.opengis.net/gml#TimeCalendarType"/>
      <rdfs:range rdf:resource="http://www.opengis.net/gml#TimeCalendarEraPropertyType"/>
   </owl:ObjectProperty>
   <owl:ObjectProperty rdf:about="http://www.opengis.net/gml#hasTimeCalendar">
      <rdfs:comment>Warning: This ObjectProperty reference was declared outside of its original schema. This ObjectProperty may be declared incorrectly.</rdfs:comment>
      <rdfs:domain rdf:resource="http://www.opengis.net/gml#TimeCalendarPropertyType"/>
      <rdfs:range rdf:resource="http://www.opengis.net/gml#TimeCalendar"/>
   </owl:ObjectProperty>
   <owl:ObjectProperty rdf:about="http://www.opengis.net/gml#referenceEvent">
      <rdfs:domain rdf:resource="http://www.opengis.net/gml#TimeCalendarEraType"/>
      <rdfs:range rdf:resource="http://www.opengis.net/gml#StringOrRefType"/>
   </owl:ObjectProperty>
   <owl:DatatypeProperty rdf:about="http://www.opengis.net/gml#referenceDate">
      <rdfs:domain rdf:resource="http://www.opengis.net/gml#TimeCalendarEraType"/>
      <rdfs:range rdf:resource="http://www.w3.org/2001/XMLSchema#date"/>
   </owl:DatatypeProperty>
   <owl:DatatypeProperty rdf:about="http://www.opengis.net/gml#julianReference">
      <rdfs:domain rdf:resource="http://www.opengis.net/gml#TimeCalendarEraType"/>
      <rdfs:range rdf:resource="http://www.w3.org/2001/XMLSchema#decimal"/>
   </owl:DatatypeProperty>
   <owl:ObjectProperty rdf:about="http://www.opengis.net/gml#epochOfUse">
      <rdfs:domain rdf:resource="http://www.opengis.net/gml#TimeCalendarEraType"/>
      <rdfs:range rdf:resource="http://www.opengis.net/gml#TimePeriodPropertyType"/>
   </owl:ObjectProperty>
   <owl:ObjectProperty rdf:about="http://www.opengis.net/gml#hasTimeCalendarEra">
      <rdfs:comment>Warning: This ObjectProperty reference was declared outside of its original schema. This ObjectProperty may be declared incorrectly.</rdfs:comment>
      <rdfs:domain rdf:resource="http://www.opengis.net/gml#TimeCalendarEraPropertyType"/>
      <rdfs:range rdf:resource="http://www.opengis.net/gml#TimeCalendarEra"/>
   </owl:ObjectProperty>
   <owl:ObjectProperty rdf:about="http://www.opengis.net/gml#referenceEvent">
      <rdfs:domain rdf:resource="http://www.opengis.net/gml#TimeClockType"/>
      <rdfs:range rdf:resource="http://www.opengis.net/gml#StringOrRefType"/>
   </owl:ObjectProperty>
   <owl:DatatypeProperty rdf:about="http://www.opengis.net/gml#referenceTime">
      <rdfs:domain rdf:resource="http://www.opengis.net/gml#TimeClockType"/>
      <rdfs:range rdf:resource="http://www.w3.org/2001/XMLSchema#time"/>
   </owl:DatatypeProperty>
   <owl:DatatypeProperty rdf:about="http://www.opengis.net/gml#utcReference">
      <rdfs:domain rdf:resource="http://www.opengis.net/gml#TimeClockType"/>
      <rdfs:range rdf:resource="http://www.w3.org/2001/XMLSchema#time"/>
   </owl:DatatypeProperty>
   <owl:ObjectProperty rdf:about="http://www.opengis.net/gml#dateBasis">
      <rdfs:domain rdf:resource="http://www.opengis.net/gml#TimeClockType"/>
      <rdfs:range rdf:resource="http://www.opengis.net/gml#TimeCalendarPropertyType"/>
   </owl:ObjectProperty>
   <owl:ObjectProperty rdf:about="http://www.opengis.net/gml#hasTimeClock">
      <rdfs:comment>Warning: This ObjectProperty reference was declared outside of its original schema. This ObjectProperty may be declared incorrectly.</rdfs:comment>
      <rdfs:domain rdf:resource="http://www.opengis.net/gml#TimeClockPropertyType"/>
      <rdfs:range rdf:resource="http://www.opengis.net/gml#TimeClock"/>
   </owl:ObjectProperty>
   <owl:ObjectProperty rdf:about="http://www.opengis.net/gml#primitive">
      <rdfs:domain rdf:resource="http://www.opengis.net/gml#TimeTopologyComplexType"/>
      <rdfs:range rdf:resource="http://www.opengis.net/gml#TimeTopologyPrimitivePropertyType"/>
   </owl:ObjectProperty>
   <owl:ObjectProperty rdf:about="http://www.opengis.net/gml#hasTimeTopologyComplex">
      <rdfs:comment>Warning: This ObjectProperty reference was declared outside of its original schema. This ObjectProperty may be declared incorrectly.</rdfs:comment>
      <rdfs:domain rdf:resource="http://www.opengis.net/gml#TimeTopologyComplexPropertyType"/>
      <rdfs:range rdf:resource="http://www.opengis.net/gml#TimeTopologyComplex"/>
   </owl:ObjectProperty>
   <owl:ObjectProperty rdf:about="http://www.opengis.net/gml#complex">
      <rdfs:domain rdf:resource="http://www.opengis.net/gml#AbstractTimeTopologyPrimitiveType"/>
      <rdfs:range rdf:resource="http://www.opengis.net/gml#ReferenceType"/>
   </owl:ObjectProperty>
   <owl:ObjectProperty rdf:about="http://www.opengis.net/gml#has_TimeTopologyPrimitive">
      <rdfs:comment>Warning: This ObjectProperty reference was declared outside of its original schema. This ObjectProperty may be declared incorrectly.</rdfs:comment>
      <rdfs:domain rdf:resource="http://www.opengis.net/gml#TimeTopologyPrimitivePropertyType"/>
      <rdfs:range rdf:resource="http://www.opengis.net/gml#_TimeTopologyPrimitive"/>
   </owl:ObjectProperty>
   <owl:ObjectProperty rdf:about="http://www.opengis.net/gml#previousEdge">
      <rdfs:domain rdf:resource="http://www.opengis.net/gml#TimeNodeType"/>
      <rdfs:range rdf:resource="http://www.opengis.net/gml#TimeEdgePropertyType"/>
   </owl:ObjectProperty>
   <owl:ObjectProperty rdf:about="http://www.opengis.net/gml#nextEdge">
      <rdfs:domain rdf:resource="http://www.opengis.net/gml#TimeNodeType"/>
      <rdfs:range rdf:resource="http://www.opengis.net/gml#TimeEdgePropertyType"/>
   </owl:ObjectProperty>
   <owl:ObjectProperty rdf:about="http://www.opengis.net/gml#position">
      <rdfs:domain rdf:resource="http://www.opengis.net/gml#TimeNodeType"/>
      <rdfs:range rdf:resource="http://www.opengis.net/gml#TimeInstantPropertyType"/>
   </owl:ObjectProperty>
   <owl:ObjectProperty rdf:about="http://www.opengis.net/gml#hasTimeNode">
      <rdfs:comment>Warning: This ObjectProperty reference was declared outside of its original schema. This ObjectProperty may be declared incorrectly.</rdfs:comment>
      <rdfs:domain rdf:resource="http://www.opengis.net/gml#TimeNodePropertyType"/>
      <rdfs:range rdf:resource="http://www.opengis.net/gml#TimeNode"/>
   </owl:ObjectProperty>
   <owl:ObjectProperty rdf:about="http://www.opengis.net/gml#start">
      <rdfs:domain rdf:resource="http://www.opengis.net/gml#TimeEdgeType"/>
      <rdfs:range rdf:resource="http://www.opengis.net/gml#TimeNodePropertyType"/>
   </owl:ObjectProperty>
   <owl:ObjectProperty rdf:about="http://www.opengis.net/gml#end">
      <rdfs:domain rdf:resource="http://www.opengis.net/gml#TimeEdgeType"/>
      <rdfs:range rdf:resource="http://www.opengis.net/gml#TimeNodePropertyType"/>
   </owl:ObjectProperty>
   <owl:ObjectProperty rdf:about="http://www.opengis.net/gml#extent">
      <rdfs:domain rdf:resource="http://www.opengis.net/gml#TimeEdgeType"/>
      <rdfs:range rdf:resource="http://www.opengis.net/gml#TimePeriodPropertyType"/>
   </owl:ObjectProperty>
   <owl:ObjectProperty rdf:about="http://www.opengis.net/gml#hasTimeEdge">
      <rdfs:comment>Warning: This ObjectProperty reference was declared outside of its original schema. This ObjectProperty may be declared incorrectly.</rdfs:comment>
      <rdfs:domain rdf:resource="http://www.opengis.net/gml#TimeEdgePropertyType"/>
      <rdfs:range rdf:resource="http://www.opengis.net/gml#TimeEdge"/>
   </owl:ObjectProperty>
</rdf:RDF>
