@prefix core:  <https://github.com/VCityTeam/UD-Graph/Ontologies/core#> .
@prefix iso19150-2: <http://def.isotc211.org/iso19150/-2/2012/base#> .
@prefix owl:   <http://www.w3.org/2002/07/owl#> .
@prefix rdf:   <http://www.w3.org/1999/02/22-rdf-syntax-ns#> .
@prefix gsp:   <http://www.opengis.net/ont/geosparql#> .
@prefix xsd:   <http://www.w3.org/2001/XMLSchema#> .
@prefix iso19136: <http://def.isotc211.org/iso19136/2007/GML> .
@prefix luse:  <https://github.com/VCityTeam/UD-Graph/Ontologies/landuse#> .
@prefix skos:  <http://www.w3.org/2004/02/skos/core#> .
@prefix rdfs:  <http://www.w3.org/2000/01/rdf-schema#> .

luse:LandUse  a          owl:Class ;
        rdfs:subClassOf  core:AbstractCityObject ;
        skos:definition  "SIG3D: Object describing an area of the earth's surface dedicated to a specific land use or having a specific land cover with or without vegetation, such as sand, rock, mud flats, forest, grasslands, etc (i.e. the physical appearance)."@en ;
        skos:prefLabel   "LandUse"@en .

<https://github.com/VCityTeam/UD-Graph/Ontologies/landuse>
        a                owl:Ontology ;
        owl:imports      <https://github.com/VCityTeam/UD-Graph/Ontologies/core> , <http://www.opengis.net/ont/geosparql> , <http://def.isotc211.org/iso19150/-2/2012/base> ;
        owl:versionIRI   "https://github.com/VCityTeam/UD-Graph/Ontologies/landuse/1.0" ;
        owl:versionInfo  "1.0" ;
        skos:prefLabel   "LandUse"@en .

luse:LandUse.lod2MultiSurface
        a                owl:ObjectProperty ;
        rdfs:domain      luse:LandUse ;
        rdfs:range       gsp:Geometry ;
        skos:definition  "SIG3D: Relation to a LOD2 multi surface geometry representing the Land Use area. The LOD concept for LandUse is defined in chapter ..."@en ;
        skos:prefLabel   "lod2MultiSurface"@en .

luse:LandUse.lod1MultiSurface
        a                owl:ObjectProperty ;
        rdfs:domain      luse:LandUse ;
        rdfs:range       gsp:Geometry ;
        skos:definition  "SIG3D: Relation to a LOD1 multi surface geometry representing the Land Use area. The LOD concept for LandUse is defined in chapter ..."@en ;
        skos:prefLabel   "lod1MultiSurface"@en .

luse:LandUse.lod4MultiSurface
        a                owl:ObjectProperty ;
        rdfs:domain      luse:LandUse ;
        rdfs:range       gsp:Geometry ;
        skos:definition  "SIG3D: Relation to a LOD4 multi surface geometry representing the Land Use area. The LOD concept for LandUse is defined in chapter ..."@en ;
        skos:prefLabel   "lod4MultiSurface"@en .

luse:LandUse.lod0MultiSurface
        a                owl:ObjectProperty ;
        rdfs:domain      luse:LandUse ;
        rdfs:range       gsp:Geometry ;
        skos:definition  "SIG3D: Relation to a LOD0 multi surface geometry representing the Land Use area. The LOD concept for LandUse is defined in chapter ..."@en ;
        skos:prefLabel   "lod0MultiSurface"@en .

luse:LandUse.usage  a    owl:ObjectProperty ;
        rdfs:domain      luse:LandUse ;
        rdfs:range       iso19136:Code ;
        skos:definition  "SIG3D: Actual usage of LandUse as given by the relevant national regulations, information communities or specific applications."@en ;
        skos:prefLabel   "usage"@en .

luse:LandUse.class  a    owl:ObjectProperty ;
        rdfs:domain      luse:LandUse ;
        rdfs:range       iso19136:Code ;
        skos:definition  "SIG3D: Classification of LandUse as given by the relevant national regulations, information communities or specific applications."@en ;
        skos:prefLabel   "class"@en .

luse:LandUse.lod3MultiSurface
        a                owl:ObjectProperty ;
        rdfs:domain      luse:LandUse ;
        rdfs:range       gsp:Geometry ;
        skos:definition  "SIG3D: Relation to a LOD3 multi surface geometry representing the Land Use area. The LOD concept for LandUse is defined in chapter ..."@en ;
        skos:prefLabel   "lod3MultiSurface"@en .

luse:LandUse.function
        a                owl:ObjectProperty ;
        rdfs:domain      luse:LandUse ;
        rdfs:range       iso19136:Code ;
        skos:definition  "SIG3D: Specified function of LandUse as given by the relevant national regulations, information communities or specific applications."@en ;
        skos:prefLabel   "function"@en .
