@prefix sc:    <http://shapechange.net/resources/ont/base#> .
@prefix core:  <https://github.com/VCityTeam/UD-Graph/Ontologies/core#> .
@prefix gen:   <https://github.com/VCityTeam/UD-Graph/Ontologies/generics#> .
@prefix iso19150-2: <http://def.isotc211.org/iso19150/-2/2012/base#> .
@prefix gsp:   <http://www.opengis.net/ont/geosparql#> .
@prefix rdf:   <http://www.w3.org/1999/02/22-rdf-syntax-ns#> .
@prefix owl:   <http://www.w3.org/2002/07/owl#> .
@prefix iso19136: <http://def.isotc211.org/iso19136/2007/GML> .
@prefix xsd:   <http://www.w3.org/2001/XMLSchema#> .
@prefix skos:  <http://www.w3.org/2004/02/skos/core#> .
@prefix rdfs:  <http://www.w3.org/2000/01/rdf-schema#> .

gen:GenericCityObject.class
        a                owl:ObjectProperty ;
        rdfs:domain      gen:GenericCityObject ;
        rdfs:range       iso19136:Code ;
        skos:definition  "SIG3D: Classification of the actual usage of GenericCityObject as given by the relevant national regulations, information communities or specific applications."@en ;
        skos:prefLabel   "class"@en .

gen:GenericCityObject.lod2TerrainIntersection
        a                owl:ObjectProperty ;
        rdfs:domain      gen:GenericCityObject ;
        rdfs:range       gsp:Geometry ;
        skos:definition  "SIG3D: Relation to Intersection curve(s) between a LOD2 generic city object and a terrain (LOD1 or LOD2 or LOD3 or LOD4). The LOD concepts forgeneric city objects and terrain are defined in chapter ..."@en ;
        skos:prefLabel   "lod2TerrainIntersection"@en .

gen:IntAttribute  a      owl:Class ;
        rdfs:subClassOf  gen:AbstractGenericAttribute ;
        skos:definition  "SIG3D: Generic Attribute of type \"integer\"."@en ;
        skos:prefLabel   "IntAttribute"@en .

gen:DateAttribute.value
        a                owl:DatatypeProperty ;
        rdfs:domain      gen:DateAttribute ;
        rdfs:range       xsd:date ;
        skos:definition  "SIG3D: Value of the Generic Attribute."@en ;
        skos:prefLabel   "value"@en .

gen:GenericCityObject.lod2Geometry
        a                owl:ObjectProperty ;
        rdfs:domain      gen:GenericCityObject ;
        rdfs:range       gsp:Geometry ;
        skos:definition  "SIG3D: Relation to a LOD2 geometry of a generic city object.The LOD concept for generic city objects is defined in chapter ..."@en ;
        skos:prefLabel   "lod2Geometry"@en .

gen:GenericCityObject.lod0Geometry
        a                owl:ObjectProperty ;
        rdfs:domain      gen:GenericCityObject ;
        rdfs:range       gsp:Geometry ;
        skos:definition  "SIG3D: Relation to a LOD0 geometry of a generic city object.The LOD concept for generic city objects is defined in chapter ..."@en ;
        skos:prefLabel   "lod0Geometry"@en .

gen:GenericCityObject.usage
        a                owl:ObjectProperty ;
        rdfs:domain      gen:GenericCityObject ;
        rdfs:range       iso19136:Code ;
        skos:definition  "SIG3D: Actual usage of GenericCityObject as given by the relevant national regulations, information communities or specific applications."@en ;
        skos:prefLabel   "usage"@en .

gen:AbstractGenericAttribute
        a                      owl:Class ;
        iso19150-2:isAbstract  true ;
        skos:definition        "SIG3D: Abstract superclass for all types of Generic Attributes. A Generic Attribute describes an additional property of an AbstractCityObject which cannot be expressed by a property provided by the schema."@en ;
        skos:prefLabel         "AbstractGenericAttribute"@en .

gen:GenericCityObject.lod1TerrainIntersection
        a                owl:ObjectProperty ;
        rdfs:domain      gen:GenericCityObject ;
        rdfs:range       gsp:Geometry ;
        skos:definition  "SIG3D: Relation to Intersection curve(s) between a LOD1 generic city object and a terrain (LOD1 or LOD2 or LOD3 or LOD4). The LOD concepts forgeneric city objects and terrain are defined in chapter ..."@en ;
        skos:prefLabel   "lod1TerrainIntersection"@en .

gen:GenericCityObject
        a                owl:Class ;
        rdfs:subClassOf  core:AbstractCityObject ;
        skos:definition  "SIG3D: Representation of a real wold city object which does not fit to any of the specific CityGML / ADE classes."@en ;
        skos:prefLabel   "GenericCityObject"@en .

gen:GenericCityObject.lod2ImplicitRepresentation
        a                owl:ObjectProperty ;
        rdfs:domain      gen:GenericCityObject ;
        rdfs:range       core:ImplicitGeometry ;
        skos:definition  "SIG3D:Relation to an implicit representation (ImplictGeometry) of a generic city object's LOD2 geometry. The LOD concept for generic city objects is defined in chapter ..."@en ;
        skos:prefLabel   "lod2ImplicitRepresentation"@en .

gen:DateAttribute  a     owl:Class ;
        rdfs:subClassOf  gen:AbstractGenericAttribute ;
        skos:definition  "SIG3D: Generic Attribute of type \"date\"."@en ;
        skos:prefLabel   "DateAttribute"@en .

gen:GenericCityObject.lod4TerrainIntersection
        a                owl:ObjectProperty ;
        rdfs:domain      gen:GenericCityObject ;
        rdfs:range       gsp:Geometry ;
        skos:definition  "SIG3D: Relation to Intersection curve(s) between a LOD4 generic city object and a terrain (LOD1 or LOD2 or LOD3 or LOD4). The LOD concepts forgeneric city objects and terrain are defined in chapter ..."@en ;
        skos:prefLabel   "lod4TerrainIntersection"@en .

gen:GenericCityObject.lod1Geometry
        a                owl:ObjectProperty ;
        rdfs:domain      gen:GenericCityObject ;
        rdfs:range       gsp:Geometry ;
        skos:definition  "SIG3D: Relation to a LOD1 geometry of a generic city object.The LOD concept for generic city objects is defined in chapter ..."@en ;
        skos:prefLabel   "lod1Geometry"@en .

gen:GenericCityObject.lod3Geometry
        a                owl:ObjectProperty ;
        rdfs:domain      gen:GenericCityObject ;
        rdfs:range       gsp:Geometry ;
        skos:definition  "SIG3D: Relation to a LOD3 geometry of a generic city object.The LOD concept for generic city objects is defined in chapter ..."@en ;
        skos:prefLabel   "lod3Geometry"@en .

gen:GenericAttributeSet.abstractGenericAttribute
        a                owl:ObjectProperty ;
        rdfs:domain      gen:GenericAttributeSet ;
        rdfs:range       gen:AbstractGenericAttribute ;
        skos:definition  "SIG3D: Aggregation of AbstractGenericAttributes by a GenericAttributeSet."@en ;
        skos:prefLabel   "abstractGenericAttribute"@en .

gen:UriAttribute  a      owl:Class ;
        rdfs:subClassOf  gen:AbstractGenericAttribute ;
        skos:definition  "SIG3D: Generic Attribute of type \"URI\"."@en ;
        skos:prefLabel   "UriAttribute"@en .

gen:GenericCityObject.lod3ImplicitRepresentation
        a                owl:ObjectProperty ;
        rdfs:domain      gen:GenericCityObject ;
        rdfs:range       core:ImplicitGeometry ;
        skos:definition  "SIG3D:Relation to an implicit representation (ImplictGeometry) of a generic city object's LOD3 geometry. The LOD concept for generic city objects is defined in chapter ..."@en ;
        skos:prefLabel   "lod3ImplicitRepresentation"@en .

gen:StringAttribute  a   owl:Class ;
        rdfs:subClassOf  gen:AbstractGenericAttribute ;
        skos:definition  "SIG3D: Generic Attribute of type \"string\"."@en ;
        skos:prefLabel   "StringAttribute"@en .

gen:MeasureAttribute  a  owl:Class ;
        rdfs:subClassOf  gen:AbstractGenericAttribute ;
        skos:definition  "SIG3D: Generic Attribute of type \"Measure\" (double-attribute with explicit specification of a unit-of-measurement)."@en ;
        skos:prefLabel   "MeasureAttribute"@en .

gen:GenericCityObject.lod0ImplicitRepresentation
        a                owl:ObjectProperty ;
        rdfs:domain      gen:GenericCityObject ;
        rdfs:range       core:ImplicitGeometry ;
        skos:definition  "SIG3D:Relation to an implicit representation (ImplictGeometry) of a generic city object's  LOD0 geometry. The LOD concept for generic city objects is defined in chapter ..."@en ;
        skos:prefLabel   "lod0ImplicitRepresentation"@en .

gen:GenericCityObject.function
        a                owl:ObjectProperty ;
        rdfs:domain      gen:GenericCityObject ;
        rdfs:range       iso19136:Code ;
        skos:definition  "SIG3D: Specified function of GenericCityObject as given by the relevant national regulations, information communities or specific applications."@en ;
        skos:prefLabel   "function"@en .

gen:GenericCityObject.lod3TerrainIntersection
        a                owl:ObjectProperty ;
        rdfs:domain      gen:GenericCityObject ;
        rdfs:range       gsp:Geometry ;
        skos:definition  "SIG3D: Relation to Intersection curve(s) between a LOD3 generic city object and a terrain (LOD1 or LOD2 or LOD3 or LOD4). The LOD concepts forgeneric city objects and terrain are defined in chapter ..."@en ;
        skos:prefLabel   "lod3TerrainIntersection"@en .

gen:GenericCityObject.lod4Geometry
        a                owl:ObjectProperty ;
        rdfs:domain      gen:GenericCityObject ;
        rdfs:range       gsp:Geometry ;
        skos:definition  "SIG3D: Relation to a LOD4 geometry of a generic city object.The LOD concept for generic city objects is defined in chapter ..."@en ;
        skos:prefLabel   "lod4Geometry"@en .

gen:GenericAttributeSet
        a                owl:Class ;
        rdfs:subClassOf  gen:AbstractGenericAttribute ;
        skos:definition  "SIG3D: Set of Generic Attributes."@en ;
        skos:prefLabel   "GenericAttributeSet"@en .

gen:GenericCityObject.lod0TerrainIntersection
        a                owl:ObjectProperty ;
        rdfs:domain      gen:GenericCityObject ;
        rdfs:range       gsp:Geometry ;
        skos:definition  "SIG3D: Relation to Intersection curve(s) between a LOD0 generic city object and a terrain (LOD1 or LOD2 or LOD3 or LOD4). The LOD concepts forgeneric city objects and terrain are defined in chapter ..."@en ;
        skos:prefLabel   "lod0TerrainIntersection"@en .

gen:GenericAttributeSet.codeSpace
        a                owl:DatatypeProperty ;
        rdfs:domain      gen:GenericAttributeSet ;
        rdfs:range       xsd:anyURI ;
        skos:definition  "SIG3D: Codespace idcentifier of the Generic AttributeSet."@en ;
        skos:prefLabel   "codeSpace"@en .

gen:IntAttribute.value
        a                owl:DatatypeProperty ;
        rdfs:domain      gen:IntAttribute ;
        rdfs:range       xsd:integer ;
        skos:definition  "SIG3D: Value of the Generic Attribute."@en ;
        skos:prefLabel   "value"@en .

gen:MeasureAttribute.value
        a                owl:DatatypeProperty ;
        rdfs:domain      gen:MeasureAttribute ;
        rdfs:range       sc:Measure ;
        skos:definition  "SIG3D: Value of the Generic Attribute."@en ;
        skos:prefLabel   "value"@en .

gen:UriAttribute.value
        a                owl:DatatypeProperty ;
        rdfs:domain      gen:UriAttribute ;
        rdfs:range       xsd:anyURI ;
        skos:definition  "SIG3D: Value of the Generic Attribute."@en ;
        skos:prefLabel   "value"@en .

gen:AbstractGenericAttribute.name
        a                owl:DatatypeProperty ;
        rdfs:domain      gen:AbstractGenericAttribute ;
        rdfs:range       xsd:string ;
        skos:definition  "SIG3D: Name of the Generic Attribute."@en ;
        skos:prefLabel   "name"@en .

gen:GenericCityObject.lod4ImplicitRepresentation
        a                owl:ObjectProperty ;
        rdfs:domain      gen:GenericCityObject ;
        rdfs:range       core:ImplicitGeometry ;
        skos:definition  "SIG3D:Relation to an implicit representation (ImplictGeometry) of a generic city object's LOD4 geometry. The LOD concept for generic city objects is defined in chapter ..."@en ;
        skos:prefLabel   "lod4ImplicitRepresentation"@en .

<https://github.com/VCityTeam/UD-Graph/Ontologies/generics>
        a                owl:Ontology ;
        owl:imports      <http://shapechange.net/resources/ont/base> , <https://github.com/VCityTeam/UD-Graph/Ontologies/core> , <http://www.opengis.net/ont/geosparql> , <http://def.isotc211.org/iso19150/-2/2012/base> ;
        owl:versionIRI   "https://github.com/VCityTeam/UD-Graph/Ontologies/generics/1.0" ;
        owl:versionInfo  "1.0" ;
        skos:definition  "\"SIG3D: Generic Attribute of type \"\"date\"\".\""@en ;
        skos:prefLabel   "Generics"@en .

gen:DoubleAttribute  a   owl:Class ;
        rdfs:subClassOf  gen:AbstractGenericAttribute ;
        skos:definition  "SIG3D: Generic Attribute of type \"double\"."@en ;
        skos:prefLabel   "DoubleAttribute"@en .

gen:StringAttribute.value
        a                owl:DatatypeProperty ;
        rdfs:domain      gen:StringAttribute ;
        rdfs:range       xsd:string ;
        skos:definition  "SIG3D: Value of the Generic Attribute."@en ;
        skos:prefLabel   "value"@en .

gen:DoubleAttribute.value
        a                owl:DatatypeProperty ;
        rdfs:domain      gen:DoubleAttribute ;
        rdfs:range       xsd:double ;
        skos:definition  "SIG3D: Value of the Generic Attribute."@en ;
        skos:prefLabel   "value"@en .

gen:GenericCityObject.lod1ImplicitRepresentation
        a                owl:ObjectProperty ;
        rdfs:domain      gen:GenericCityObject ;
        rdfs:range       core:ImplicitGeometry ;
        skos:definition  "SIG3D:Relation to an implicit representation (ImplictGeometry) of a generic city object's  LOD1 geometry. The LOD concept for generic city objects is defined in chapter ..."@en ;
        skos:prefLabel   "lod1ImplicitRepresentation"@en .
