@prefix core: <https://dataset-dl.liris.cnrs.fr/rdf-owl-urban-data-ontologies/Ontologies/CityGML/2.0/core#> .
@prefix gen: <https://dataset-dl.liris.cnrs.fr/rdf-owl-urban-data-ontologies/Ontologies/CityGML/2.0/generics#> .
@prefix gmlowl: <http://www.opengis.net/ont/gml#> .
@prefix iso19136-bt: <http://def.isotc211.org/iso19136/2007/BasicTypes#> .
@prefix iso19150-2: <http://def.isotc211.org/iso19150/-2/2012/base#> .
@prefix owl: <http://www.w3.org/2002/07/owl#> .
@prefix rdf: <http://www.w3.org/1999/02/22-rdf-syntax-ns#> .
@prefix rdfs: <http://www.w3.org/2000/01/rdf-schema#> .
@prefix sc: <http://shapechange.net/resources/ont/base#> .
@prefix skos: <http://www.w3.org/2004/02/skos/core#> .
@prefix xsd: <http://www.w3.org/2001/XMLSchema#> .

<https://dataset-dl.liris.cnrs.fr/rdf-owl-urban-data-ontologies/Ontologies/CityGML/2.0/generics> a owl:Ontology ;
    rdfs:label "Generics"@en ;
    owl:imports <http://def.isotc211.org/iso19150/-2/2012/base>,
        <http://shapechange.net/resources/ont/base>,
        <http://www.opengis.net/ont/gml>,
        <https://dataset-dl.liris.cnrs.fr/rdf-owl-urban-data-ontologies/Ontologies/CityGML/2.0/core.ttl> ;
    skos:definition "\"SIG3D: Generic Attribute of type \"\"date\"\".\""@en ;
    skos:prefLabel "Generics"@en .

gen:GenericCityObject.function a owl:ObjectProperty ;
    rdfs:label "function"@en ;
    rdfs:domain gen:GenericCityObject ;
    rdfs:range iso19136-bt:Code ;
    skos:definition "SIG3D: Specified function of GenericCityObject as given by the relevant national regulations, information communities or specific applications."@en ;
    skos:prefLabel "function"@en .

gen:GenericCityObject.usage a owl:ObjectProperty ;
    rdfs:label "usage"@en ;
    rdfs:domain gen:GenericCityObject ;
    rdfs:range iso19136-bt:Code ;
    skos:definition "SIG3D: Actual usage of GenericCityObject as given by the relevant national regulations, information communities or specific applications."@en ;
    skos:prefLabel "usage"@en .

gen:AbstractGenericAttribute.name a owl:DatatypeProperty ;
    rdfs:label "name"@en ;
    rdfs:domain gen:AbstractGenericAttribute ;
    rdfs:range xsd:string ;
    skos:definition "SIG3D: Name of the Generic Attribute."@en ;
    skos:prefLabel "name"@en .

gen:DateAttribute a owl:Class ;
    rdfs:label "DateAttribute"@en ;
    rdfs:subClassOf [ a owl:Restriction ;
            owl:allValuesFrom xsd:date ;
            owl:onProperty gen:DateAttribute.value ],
        [ a owl:Restriction ;
            owl:onDataRange xsd:date ;
            owl:onProperty gen:DateAttribute.value ;
            owl:qualifiedCardinality "1"^^xsd:nonNegativeInteger ],
        gen:AbstractGenericAttribute ;
    skos:definition "SIG3D: Generic Attribute of type \"date\"."@en ;
    skos:prefLabel "DateAttribute"@en .

gen:DateAttribute.value a owl:DatatypeProperty ;
    rdfs:label "value"@en ;
    rdfs:domain gen:DateAttribute ;
    rdfs:range xsd:date ;
    skos:definition "SIG3D: Value of the Generic Attribute."@en ;
    skos:prefLabel "value"@en .

gen:DoubleAttribute a owl:Class ;
    rdfs:label "DoubleAttribute"@en ;
    rdfs:subClassOf [ a owl:Restriction ;
            owl:allValuesFrom xsd:double ;
            owl:onProperty gen:DoubleAttribute.value ],
        [ a owl:Restriction ;
            owl:onDataRange xsd:double ;
            owl:onProperty gen:DoubleAttribute.value ;
            owl:qualifiedCardinality "1"^^xsd:nonNegativeInteger ],
        gen:AbstractGenericAttribute ;
    skos:definition "SIG3D: Generic Attribute of type \"double\"."@en ;
    skos:prefLabel "DoubleAttribute"@en .

gen:DoubleAttribute.value a owl:DatatypeProperty ;
    rdfs:label "value"@en ;
    rdfs:domain gen:DoubleAttribute ;
    rdfs:range xsd:double ;
    skos:definition "SIG3D: Value of the Generic Attribute."@en ;
    skos:prefLabel "value"@en .

gen:GenericAttributeSet.abstractGenericAttribute a owl:ObjectProperty ;
    rdfs:label "abstractGenericAttribute"@en ;
    rdfs:domain gen:GenericAttributeSet ;
    rdfs:range gen:AbstractGenericAttribute ;
    skos:definition "SIG3D: Aggregation of AbstractGenericAttributes by a GenericAttributeSet."@en ;
    skos:prefLabel "abstractGenericAttribute"@en .

gen:GenericAttributeSet.codeSpace a owl:DatatypeProperty ;
    rdfs:label "codeSpace"@en ;
    rdfs:domain gen:GenericAttributeSet ;
    rdfs:range xsd:anyURI ;
    skos:definition "SIG3D: Codespace idcentifier of the Generic AttributeSet."@en ;
    skos:prefLabel "codeSpace"@en .

gen:GenericCityObject.class a owl:ObjectProperty ;
    rdfs:label "class"@en ;
    rdfs:domain gen:GenericCityObject ;
    rdfs:range iso19136-bt:Code ;
    skos:definition "SIG3D: Classification of the actual usage of GenericCityObject as given by the relevant national regulations, information communities or specific applications."@en ;
    skos:prefLabel "class"@en .

gen:GenericCityObject.lod0Geometry a owl:ObjectProperty ;
    rdfs:label "lod0Geometry"@en ;
    rdfs:domain gen:GenericCityObject ;
    rdfs:range gmlowl:AbstractGeometry ;
    skos:definition "SIG3D: Relation to a LOD0 geometry of a generic city object.The LOD concept for generic city objects is defined in chapter ..."@en ;
    skos:prefLabel "lod0Geometry"@en .

gen:GenericCityObject.lod0ImplicitRepresentation a owl:ObjectProperty ;
    rdfs:label "lod0ImplicitRepresentation"@en ;
    rdfs:domain gen:GenericCityObject ;
    rdfs:range core:ImplicitGeometry ;
    skos:definition "SIG3D:Relation to an implicit representation (ImplictGeometry) of a generic city object's  LOD0 geometry. The LOD concept for generic city objects is defined in chapter ..."@en ;
    skos:prefLabel "lod0ImplicitRepresentation"@en .

gen:GenericCityObject.lod0TerrainIntersection a owl:ObjectProperty ;
    rdfs:label "lod0TerrainIntersection"@en ;
    rdfs:domain gen:GenericCityObject ;
    rdfs:range gmlowl:MultiCurve ;
    skos:definition "SIG3D: Relation to Intersection curve(s) between a LOD0 generic city object and a terrain (LOD1 or LOD2 or LOD3 or LOD4). The LOD concepts forgeneric city objects and terrain are defined in chapter ..."@en ;
    skos:prefLabel "lod0TerrainIntersection"@en .

gen:GenericCityObject.lod1Geometry a owl:ObjectProperty ;
    rdfs:label "lod1Geometry"@en ;
    rdfs:domain gen:GenericCityObject ;
    rdfs:range gmlowl:AbstractGeometry ;
    skos:definition "SIG3D: Relation to a LOD1 geometry of a generic city object.The LOD concept for generic city objects is defined in chapter ..."@en ;
    skos:prefLabel "lod1Geometry"@en .

gen:GenericCityObject.lod1ImplicitRepresentation a owl:ObjectProperty ;
    rdfs:label "lod1ImplicitRepresentation"@en ;
    rdfs:domain gen:GenericCityObject ;
    rdfs:range core:ImplicitGeometry ;
    skos:definition "SIG3D:Relation to an implicit representation (ImplictGeometry) of a generic city object's  LOD1 geometry. The LOD concept for generic city objects is defined in chapter ..."@en ;
    skos:prefLabel "lod1ImplicitRepresentation"@en .

gen:GenericCityObject.lod1TerrainIntersection a owl:ObjectProperty ;
    rdfs:label "lod1TerrainIntersection"@en ;
    rdfs:domain gen:GenericCityObject ;
    rdfs:range gmlowl:MultiCurve ;
    skos:definition "SIG3D: Relation to Intersection curve(s) between a LOD1 generic city object and a terrain (LOD1 or LOD2 or LOD3 or LOD4). The LOD concepts forgeneric city objects and terrain are defined in chapter ..."@en ;
    skos:prefLabel "lod1TerrainIntersection"@en .

gen:GenericCityObject.lod2Geometry a owl:ObjectProperty ;
    rdfs:label "lod2Geometry"@en ;
    rdfs:domain gen:GenericCityObject ;
    rdfs:range gmlowl:AbstractGeometry ;
    skos:definition "SIG3D: Relation to a LOD2 geometry of a generic city object.The LOD concept for generic city objects is defined in chapter ..."@en ;
    skos:prefLabel "lod2Geometry"@en .

gen:GenericCityObject.lod2ImplicitRepresentation a owl:ObjectProperty ;
    rdfs:label "lod2ImplicitRepresentation"@en ;
    rdfs:domain gen:GenericCityObject ;
    rdfs:range core:ImplicitGeometry ;
    skos:definition "SIG3D:Relation to an implicit representation (ImplictGeometry) of a generic city object's LOD2 geometry. The LOD concept for generic city objects is defined in chapter ..."@en ;
    skos:prefLabel "lod2ImplicitRepresentation"@en .

gen:GenericCityObject.lod2TerrainIntersection a owl:ObjectProperty ;
    rdfs:label "lod2TerrainIntersection"@en ;
    rdfs:domain gen:GenericCityObject ;
    rdfs:range gmlowl:MultiCurve ;
    skos:definition "SIG3D: Relation to Intersection curve(s) between a LOD2 generic city object and a terrain (LOD1 or LOD2 or LOD3 or LOD4). The LOD concepts forgeneric city objects and terrain are defined in chapter ..."@en ;
    skos:prefLabel "lod2TerrainIntersection"@en .

gen:GenericCityObject.lod3Geometry a owl:ObjectProperty ;
    rdfs:label "lod3Geometry"@en ;
    rdfs:domain gen:GenericCityObject ;
    rdfs:range gmlowl:AbstractGeometry ;
    skos:definition "SIG3D: Relation to a LOD3 geometry of a generic city object.The LOD concept for generic city objects is defined in chapter ..."@en ;
    skos:prefLabel "lod3Geometry"@en .

gen:GenericCityObject.lod3ImplicitRepresentation a owl:ObjectProperty ;
    rdfs:label "lod3ImplicitRepresentation"@en ;
    rdfs:domain gen:GenericCityObject ;
    rdfs:range core:ImplicitGeometry ;
    skos:definition "SIG3D:Relation to an implicit representation (ImplictGeometry) of a generic city object's LOD3 geometry. The LOD concept for generic city objects is defined in chapter ..."@en ;
    skos:prefLabel "lod3ImplicitRepresentation"@en .

gen:GenericCityObject.lod3TerrainIntersection a owl:ObjectProperty ;
    rdfs:label "lod3TerrainIntersection"@en ;
    rdfs:domain gen:GenericCityObject ;
    rdfs:range gmlowl:MultiCurve ;
    skos:definition "SIG3D: Relation to Intersection curve(s) between a LOD3 generic city object and a terrain (LOD1 or LOD2 or LOD3 or LOD4). The LOD concepts forgeneric city objects and terrain are defined in chapter ..."@en ;
    skos:prefLabel "lod3TerrainIntersection"@en .

gen:GenericCityObject.lod4Geometry a owl:ObjectProperty ;
    rdfs:label "lod4Geometry"@en ;
    rdfs:domain gen:GenericCityObject ;
    rdfs:range gmlowl:AbstractGeometry ;
    skos:definition "SIG3D: Relation to a LOD4 geometry of a generic city object.The LOD concept for generic city objects is defined in chapter ..."@en ;
    skos:prefLabel "lod4Geometry"@en .

gen:GenericCityObject.lod4ImplicitRepresentation a owl:ObjectProperty ;
    rdfs:label "lod4ImplicitRepresentation"@en ;
    rdfs:domain gen:GenericCityObject ;
    rdfs:range core:ImplicitGeometry ;
    skos:definition "SIG3D:Relation to an implicit representation (ImplictGeometry) of a generic city object's LOD4 geometry. The LOD concept for generic city objects is defined in chapter ..."@en ;
    skos:prefLabel "lod4ImplicitRepresentation"@en .

gen:GenericCityObject.lod4TerrainIntersection a owl:ObjectProperty ;
    rdfs:label "lod4TerrainIntersection"@en ;
    rdfs:domain gen:GenericCityObject ;
    rdfs:range gmlowl:MultiCurve ;
    skos:definition "SIG3D: Relation to Intersection curve(s) between a LOD4 generic city object and a terrain (LOD1 or LOD2 or LOD3 or LOD4). The LOD concepts forgeneric city objects and terrain are defined in chapter ..."@en ;
    skos:prefLabel "lod4TerrainIntersection"@en .

gen:IntAttribute a owl:Class ;
    rdfs:label "IntAttribute"@en ;
    rdfs:subClassOf [ a owl:Restriction ;
            owl:allValuesFrom xsd:integer ;
            owl:onProperty gen:IntAttribute.value ],
        [ a owl:Restriction ;
            owl:onDataRange xsd:integer ;
            owl:onProperty gen:IntAttribute.value ;
            owl:qualifiedCardinality "1"^^xsd:nonNegativeInteger ],
        gen:AbstractGenericAttribute ;
    skos:definition "SIG3D: Generic Attribute of type \"integer\"."@en ;
    skos:prefLabel "IntAttribute"@en .

gen:IntAttribute.value a owl:DatatypeProperty ;
    rdfs:label "value"@en ;
    rdfs:domain gen:IntAttribute ;
    rdfs:range xsd:integer ;
    skos:definition "SIG3D: Value of the Generic Attribute."@en ;
    skos:prefLabel "value"@en .

gen:MeasureAttribute a owl:Class ;
    rdfs:label "MeasureAttribute"@en ;
    rdfs:subClassOf [ a owl:Restriction ;
            owl:allValuesFrom sc:Measure ;
            owl:onProperty gen:MeasureAttribute.value ],
        [ a owl:Restriction ;
            owl:onDataRange sc:Measure ;
            owl:onProperty gen:MeasureAttribute.value ;
            owl:qualifiedCardinality "1"^^xsd:nonNegativeInteger ],
        gen:AbstractGenericAttribute ;
    skos:definition "SIG3D: Generic Attribute of type \"Measure\" (double-attribute with explicit specification of a unit-of-measurement)."@en ;
    skos:prefLabel "MeasureAttribute"@en .

gen:MeasureAttribute.value a owl:DatatypeProperty ;
    rdfs:label "value"@en ;
    rdfs:domain gen:MeasureAttribute ;
    rdfs:range sc:Measure ;
    skos:definition "SIG3D: Value of the Generic Attribute."@en ;
    skos:prefLabel "value"@en .

gen:StringAttribute a owl:Class ;
    rdfs:label "StringAttribute"@en ;
    rdfs:subClassOf [ a owl:Restriction ;
            owl:allValuesFrom xsd:string ;
            owl:onProperty gen:StringAttribute.value ],
        [ a owl:Restriction ;
            owl:onDataRange xsd:string ;
            owl:onProperty gen:StringAttribute.value ;
            owl:qualifiedCardinality "1"^^xsd:nonNegativeInteger ],
        gen:AbstractGenericAttribute ;
    skos:definition "SIG3D: Generic Attribute of type \"string\"."@en ;
    skos:prefLabel "StringAttribute"@en .

gen:StringAttribute.value a owl:DatatypeProperty ;
    rdfs:label "value"@en ;
    rdfs:domain gen:StringAttribute ;
    rdfs:range xsd:string ;
    skos:definition "SIG3D: Value of the Generic Attribute."@en ;
    skos:prefLabel "value"@en .

gen:UriAttribute a owl:Class ;
    rdfs:label "UriAttribute"@en ;
    rdfs:subClassOf [ a owl:Restriction ;
            owl:allValuesFrom xsd:anyURI ;
            owl:onProperty gen:UriAttribute.value ],
        [ a owl:Restriction ;
            owl:onDataRange xsd:anyURI ;
            owl:onProperty gen:UriAttribute.value ;
            owl:qualifiedCardinality "1"^^xsd:nonNegativeInteger ],
        gen:AbstractGenericAttribute ;
    skos:definition "SIG3D: Generic Attribute of type \"URI\"."@en ;
    skos:prefLabel "UriAttribute"@en .

gen:UriAttribute.value a owl:DatatypeProperty ;
    rdfs:label "value"@en ;
    rdfs:domain gen:UriAttribute ;
    rdfs:range xsd:anyURI ;
    skos:definition "SIG3D: Value of the Generic Attribute."@en ;
    skos:prefLabel "value"@en .

gen:GenericAttributeSet a owl:Class ;
    rdfs:label "GenericAttributeSet"@en ;
    rdfs:subClassOf [ a owl:Restriction ;
            owl:allValuesFrom xsd:anyURI ;
            owl:onProperty gen:GenericAttributeSet.codeSpace ],
        [ a owl:Restriction ;
            owl:maxQualifiedCardinality "1"^^xsd:nonNegativeInteger ;
            owl:onDataRange xsd:anyURI ;
            owl:onProperty gen:GenericAttributeSet.codeSpace ],
        [ a owl:Restriction ;
            owl:allValuesFrom gen:AbstractGenericAttribute ;
            owl:onProperty gen:GenericAttributeSet.abstractGenericAttribute ],
        [ a owl:Restriction ;
            owl:minQualifiedCardinality "1"^^xsd:nonNegativeInteger ;
            owl:onClass gen:AbstractGenericAttribute ;
            owl:onProperty gen:GenericAttributeSet.abstractGenericAttribute ],
        gen:AbstractGenericAttribute ;
    skos:definition "SIG3D: Set of Generic Attributes."@en ;
    skos:prefLabel "GenericAttributeSet"@en .

gen:AbstractGenericAttribute a owl:Class ;
    rdfs:label "AbstractGenericAttribute"@en ;
    iso19150-2:isAbstract true ;
    rdfs:subClassOf [ a owl:Restriction ;
            owl:allValuesFrom xsd:string ;
            owl:onProperty gen:AbstractGenericAttribute.name ],
        [ a owl:Restriction ;
            owl:onDataRange xsd:string ;
            owl:onProperty gen:AbstractGenericAttribute.name ;
            owl:qualifiedCardinality "1"^^xsd:nonNegativeInteger ] ;
    skos:definition "SIG3D: Abstract superclass for all types of Generic Attributes. A Generic Attribute describes an additional property of an AbstractCityObject which cannot be expressed by a property provided by the schema."@en ;
    skos:prefLabel "AbstractGenericAttribute"@en .

gen:GenericCityObject a owl:Class ;
    rdfs:label "GenericCityObject"@en ;
    rdfs:subClassOf [ a owl:Restriction ;
            owl:maxQualifiedCardinality "1"^^xsd:nonNegativeInteger ;
            owl:onClass gmlowl:MultiCurve ;
            owl:onProperty gen:GenericCityObject.lod2TerrainIntersection ],
        [ a owl:Restriction ;
            owl:allValuesFrom gmlowl:MultiCurve ;
            owl:onProperty gen:GenericCityObject.lod0TerrainIntersection ],
        [ a owl:Restriction ;
            owl:allValuesFrom gmlowl:AbstractGeometry ;
            owl:onProperty gen:GenericCityObject.lod4Geometry ],
        [ a owl:Restriction ;
            owl:maxQualifiedCardinality "1"^^xsd:nonNegativeInteger ;
            owl:onClass gmlowl:MultiCurve ;
            owl:onProperty gen:GenericCityObject.lod0TerrainIntersection ],
        [ a owl:Restriction ;
            owl:maxQualifiedCardinality "1"^^xsd:nonNegativeInteger ;
            owl:onClass iso19136-bt:Code ;
            owl:onProperty gen:GenericCityObject.class ],
        [ a owl:Restriction ;
            owl:maxQualifiedCardinality "1"^^xsd:nonNegativeInteger ;
            owl:onClass core:ImplicitGeometry ;
            owl:onProperty gen:GenericCityObject.lod3ImplicitRepresentation ],
        [ a owl:Restriction ;
            owl:allValuesFrom gmlowl:MultiCurve ;
            owl:onProperty gen:GenericCityObject.lod2TerrainIntersection ],
        [ a owl:Restriction ;
            owl:maxQualifiedCardinality "1"^^xsd:nonNegativeInteger ;
            owl:onClass gmlowl:AbstractGeometry ;
            owl:onProperty gen:GenericCityObject.lod3Geometry ],
        [ a owl:Restriction ;
            owl:allValuesFrom gmlowl:MultiCurve ;
            owl:onProperty gen:GenericCityObject.lod4TerrainIntersection ],
        [ a owl:Restriction ;
            owl:allValuesFrom gmlowl:AbstractGeometry ;
            owl:onProperty gen:GenericCityObject.lod2Geometry ],
        [ a owl:Restriction ;
            owl:allValuesFrom gmlowl:AbstractGeometry ;
            owl:onProperty gen:GenericCityObject.lod1Geometry ],
        [ a owl:Restriction ;
            owl:maxQualifiedCardinality "1"^^xsd:nonNegativeInteger ;
            owl:onClass gmlowl:AbstractGeometry ;
            owl:onProperty gen:GenericCityObject.lod4Geometry ],
        [ a owl:Restriction ;
            owl:maxQualifiedCardinality "1"^^xsd:nonNegativeInteger ;
            owl:onClass gmlowl:AbstractGeometry ;
            owl:onProperty gen:GenericCityObject.lod1Geometry ],
        [ a owl:Restriction ;
            owl:maxQualifiedCardinality "1"^^xsd:nonNegativeInteger ;
            owl:onClass core:ImplicitGeometry ;
            owl:onProperty gen:GenericCityObject.lod4ImplicitRepresentation ],
        [ a owl:Restriction ;
            owl:allValuesFrom iso19136-bt:Code ;
            owl:onProperty gen:GenericCityObject.class ],
        [ a owl:Restriction ;
            owl:allValuesFrom core:ImplicitGeometry ;
            owl:onProperty gen:GenericCityObject.lod4ImplicitRepresentation ],
        [ a owl:Restriction ;
            owl:maxQualifiedCardinality "1"^^xsd:nonNegativeInteger ;
            owl:onClass core:ImplicitGeometry ;
            owl:onProperty gen:GenericCityObject.lod1ImplicitRepresentation ],
        [ a owl:Restriction ;
            owl:allValuesFrom core:ImplicitGeometry ;
            owl:onProperty gen:GenericCityObject.lod3ImplicitRepresentation ],
        [ a owl:Restriction ;
            owl:maxQualifiedCardinality "1"^^xsd:nonNegativeInteger ;
            owl:onClass gmlowl:MultiCurve ;
            owl:onProperty gen:GenericCityObject.lod4TerrainIntersection ],
        [ a owl:Restriction ;
            owl:allValuesFrom gmlowl:AbstractGeometry ;
            owl:onProperty gen:GenericCityObject.lod3Geometry ],
        [ a owl:Restriction ;
            owl:maxQualifiedCardinality "1"^^xsd:nonNegativeInteger ;
            owl:onClass core:ImplicitGeometry ;
            owl:onProperty gen:GenericCityObject.lod2ImplicitRepresentation ],
        [ a owl:Restriction ;
            owl:allValuesFrom iso19136-bt:Code ;
            owl:onProperty gen:GenericCityObject.function ],
        [ a owl:Restriction ;
            owl:maxQualifiedCardinality "1"^^xsd:nonNegativeInteger ;
            owl:onClass core:ImplicitGeometry ;
            owl:onProperty gen:GenericCityObject.lod0ImplicitRepresentation ],
        [ a owl:Restriction ;
            owl:allValuesFrom gmlowl:MultiCurve ;
            owl:onProperty gen:GenericCityObject.lod1TerrainIntersection ],
        [ a owl:Restriction ;
            owl:maxQualifiedCardinality "1"^^xsd:nonNegativeInteger ;
            owl:onClass gmlowl:AbstractGeometry ;
            owl:onProperty gen:GenericCityObject.lod0Geometry ],
        [ a owl:Restriction ;
            owl:allValuesFrom core:ImplicitGeometry ;
            owl:onProperty gen:GenericCityObject.lod1ImplicitRepresentation ],
        [ a owl:Restriction ;
            owl:maxQualifiedCardinality "1"^^xsd:nonNegativeInteger ;
            owl:onClass gmlowl:AbstractGeometry ;
            owl:onProperty gen:GenericCityObject.lod2Geometry ],
        [ a owl:Restriction ;
            owl:allValuesFrom gmlowl:AbstractGeometry ;
            owl:onProperty gen:GenericCityObject.lod0Geometry ],
        [ a owl:Restriction ;
            owl:allValuesFrom gmlowl:MultiCurve ;
            owl:onProperty gen:GenericCityObject.lod3TerrainIntersection ],
        [ a owl:Restriction ;
            owl:allValuesFrom core:ImplicitGeometry ;
            owl:onProperty gen:GenericCityObject.lod2ImplicitRepresentation ],
        [ a owl:Restriction ;
            owl:allValuesFrom core:ImplicitGeometry ;
            owl:onProperty gen:GenericCityObject.lod0ImplicitRepresentation ],
        [ a owl:Restriction ;
            owl:allValuesFrom iso19136-bt:Code ;
            owl:onProperty gen:GenericCityObject.usage ],
        [ a owl:Restriction ;
            owl:maxQualifiedCardinality "1"^^xsd:nonNegativeInteger ;
            owl:onClass gmlowl:MultiCurve ;
            owl:onProperty gen:GenericCityObject.lod3TerrainIntersection ],
        [ a owl:Restriction ;
            owl:maxQualifiedCardinality "1"^^xsd:nonNegativeInteger ;
            owl:onClass gmlowl:MultiCurve ;
            owl:onProperty gen:GenericCityObject.lod1TerrainIntersection ],
        core:AbstractCityObject ;
    skos:definition "SIG3D: Representation of a real wold city object which does not fit to any of the specific CityGML / ADE classes."@en ;
    skos:prefLabel "GenericCityObject"@en .

[] a owl:AllDisjointClasses ;
    owl:members ( gen:DateAttribute gen:DoubleAttribute gen:GenericAttributeSet gen:IntAttribute gen:MeasureAttribute gen:StringAttribute gen:UriAttribute ) .

