@prefix core:  <https://github.com/VCityTeam/UD-Graph/Ontologies/core#> .
@prefix iso19150-2: <http://def.isotc211.org/iso19150/-2/2012/base#> .
@prefix owl:   <http://www.w3.org/2002/07/owl#> .
@prefix rdf:   <http://www.w3.org/1999/02/22-rdf-syntax-ns#> .
@prefix xsd:   <http://www.w3.org/2001/XMLSchema#> .
@prefix skos:  <http://www.w3.org/2004/02/skos/core#> .
@prefix rdfs:  <http://www.w3.org/2000/01/rdf-schema#> .
@prefix tran:  <https://github.com/VCityTeam/UD-Graph/Ontologies/transportation#> .

tran:Road.function  a    owl:ObjectProperty ;
        rdfs:domain      tran:Road ;
        rdfs:range       tran:RoadFunctionValue ;
        skos:definition  "Specifies the intended purposes of the Road."@en ;
        skos:prefLabel   "function"@en .

tran:Intersection  a     owl:Class ;
        rdfs:subClassOf  tran:AbstractTransportationSpace ;
        skos:definition  "An Intersection is a transportation space that is a shared segment of multiple Road, Track, Railway, or Waterway objects (e.g. a crossing of two roads or a level crossing of a road and a railway)."@en ;
        skos:prefLabel   "Intersection"@en .

tran:Road.usage  a       owl:ObjectProperty ;
        rdfs:domain      tran:Road ;
        rdfs:range       tran:RoadUsageValue ;
        skos:definition  "Specifies the actual uses of the Road."@en ;
        skos:prefLabel   "usage"@en .

tran:Hole  a             owl:Class ;
        rdfs:subClassOf  core:AbstractUnoccupiedSpace ;
        skos:definition  "A Hole is an opening in the surface of a Road, Track or Square such as road damages, manholes or drains. Holes can span multiple transportation objects."@en ;
        skos:prefLabel   "Hole"@en .

tran:AuxiliaryTrafficArea.adeOfAuxiliaryTrafficArea
        a                owl:ObjectProperty ;
        rdfs:domain      tran:AuxiliaryTrafficArea ;
        rdfs:range       tran:ADEOfAuxiliaryTrafficArea ;
        skos:definition  "Augments the AuxiliaryTrafficArea with properties defined in an ADE."@en ;
        skos:prefLabel   "adeOfAuxiliaryTrafficArea"@en .

tran:WaterwayFunctionValue
        a                owl:Class ;
        rdfs:subClassOf  skos:Concept ;
        skos:definition  "WaterwayFunctionValue is a code list that enumerates the different purposes of a Waterway."@en ;
        skos:prefLabel   "WaterwayFunctionValue"@en .

tran:TrafficSpace.predecessor
        a                owl:ObjectProperty ;
        rdfs:domain      tran:TrafficSpace ;
        rdfs:range       tran:TrafficSpace ;
        skos:definition  "Indicates the predecessor(s) of the TrafficSpace."@en ;
        skos:prefLabel   "predecessor"@en .

tran:AuxiliaryTrafficArea.class
        a                owl:ObjectProperty ;
        rdfs:domain      tran:AuxiliaryTrafficArea ;
        rdfs:range       tran:AuxiliaryTrafficAreaClassValue ;
        skos:definition  "Indicates the specific type of the AuxiliaryTrafficArea."@en ;
        skos:prefLabel   "class"@en .

tran:Road  a             owl:Class ;
        rdfs:subClassOf  tran:AbstractTransportationSpace ;
        skos:definition  "A Road is a transportation space used by vehicles, bicycles and/or pedestrians."@en ;
        skos:prefLabel   "Road"@en .

tran:ClearanceSpace.adeOfClearanceSpace
        a                owl:ObjectProperty ;
        rdfs:domain      tran:ClearanceSpace ;
        rdfs:range       tran:ADEOfClearanceSpace ;
        skos:definition  "Augments the ClearanceSpace with properties defined in an ADE."@en ;
        skos:prefLabel   "adeOfClearanceSpace"@en .

tran:TrafficArea.function
        a                owl:ObjectProperty ;
        rdfs:domain      tran:TrafficArea ;
        rdfs:range       tran:TrafficAreaFunctionValue ;
        skos:definition  "Specifies the intended purposes of the TrafficArea."@en ;
        skos:prefLabel   "function"@en .

tran:Railway.adeOfRailway
        a                owl:ObjectProperty ;
        rdfs:domain      tran:Railway ;
        rdfs:range       tran:ADEOfRailway ;
        skos:definition  "Augments the Railway with properties defined in an ADE."@en ;
        skos:prefLabel   "adeOfRailway"@en .

tran:Road.intersection
        a                owl:ObjectProperty ;
        rdfs:domain      tran:Road ;
        rdfs:range       tran:Intersection ;
        skos:definition  "Relates to the intersections that are part of the Road."@en ;
        skos:prefLabel   "intersection"@en .

tran:TrafficArea  a      owl:Class ;
        rdfs:subClassOf  core:AbstractThematicSurface ;
        skos:definition  "A TrafficArea is the ground surface of a TrafficSpace. Traffic areas are the surfaces upon which traffic actually takes place."@en ;
        skos:prefLabel   "TrafficArea"@en .

tran:Track.function  a   owl:ObjectProperty ;
        rdfs:domain      tran:Track ;
        rdfs:range       tran:TrackFunctionValue ;
        skos:definition  "Specifies the intended purposes of the Track."@en ;
        skos:prefLabel   "function"@en .

tran:TrafficArea.adeOfTrafficArea
        a                owl:ObjectProperty ;
        rdfs:domain      tran:TrafficArea ;
        rdfs:range       tran:ADEOfTrafficArea ;
        skos:definition  "Augments the TrafficArea with properties defined in an ADE."@en ;
        skos:prefLabel   "adeOfTrafficArea"@en .

tran:ClearanceSpaceClassValue
        a                owl:Class ;
        rdfs:subClassOf  skos:Concept ;
        skos:definition  "ClearanceSpaceClassValue is a code list used to further classify a ClearanceSpace."@en ;
        skos:prefLabel   "ClearanceSpaceClassValue"@en .

tran:TrafficSpace.clearanceSpace
        a                owl:ObjectProperty ;
        rdfs:domain      tran:TrafficSpace ;
        rdfs:range       tran:ClearanceSpace ;
        skos:definition  "Relates to the clearance spaces that are part of the TrafficSpace."@en ;
        skos:prefLabel   "clearanceSpace"@en .

tran:AbstractTransportationSpace
        a                      owl:Class ;
        rdfs:subClassOf        core:AbstractUnoccupiedSpace ;
        iso19150-2:isAbstract  true ;
        skos:definition        "AbstractTransportationSpace is the abstract superclass of transportation objects such as Roads, Tracks, Railways, Waterways or Squares."@en ;
        skos:prefLabel         "AbstractTransportationSpace"@en .

tran:Marking.class  a    owl:ObjectProperty ;
        rdfs:domain      tran:Marking ;
        rdfs:range       tran:MarkingClassValue ;
        skos:definition  "Indicates the specific type of the Marking."@en ;
        skos:prefLabel   "class"@en .

tran:Railway.section  a  owl:ObjectProperty ;
        rdfs:domain      tran:Railway ;
        rdfs:range       tran:Section ;
        skos:definition  "Relates to the sections that are part of the Railway."@en ;
        skos:prefLabel   "section"@en .

tran:RailwayUsageValue
        a                owl:Class ;
        rdfs:subClassOf  skos:Concept ;
        skos:definition  "RailwayUsageValue is a code list that enumerates the different uses of a Railway."@en ;
        skos:prefLabel   "RailwayUsageValue"@en .

tran:RoadClassValue  a   owl:Class ;
        rdfs:subClassOf  skos:Concept ;
        skos:definition  "RoadClassValue is a code list used to further classify a Road."@en ;
        skos:prefLabel   "RoadClassValue"@en .

tran:TrafficSpace.boundary
        a               owl:ObjectProperty ;
        rdfs:domain     tran:TrafficSpace ;
        rdfs:range      tran:TrafficArea ;
        skos:prefLabel  "boundary"@en .

tran:Track.adeOfTrack
        a                owl:ObjectProperty ;
        rdfs:domain      tran:Track ;
        rdfs:range       tran:ADEOfTrack ;
        skos:definition  "Augments the Track with properties defined in an ADE."@en ;
        skos:prefLabel   "adeOfTrack"@en .

tran:AuxiliaryTrafficAreaFunctionValue
        a                owl:Class ;
        rdfs:subClassOf  skos:Concept ;
        skos:definition  "AuxiliaryTrafficAreaFunctionValue is a code list that enumerates the different purposes of an AuxiliaryTrafficArea."@en ;
        skos:prefLabel   "AuxiliaryTrafficAreaFunctionValue"@en .

tran:TrafficSpaceFunctionValue
        a                owl:Class ;
        rdfs:subClassOf  skos:Concept ;
        skos:definition  "TrafficSpaceFunctionValue is a code list that enumerates the different purposes of a TrafficSpace."@en ;
        skos:prefLabel   "TrafficSpaceFunctionValue"@en .

tran:TrafficArea.usage
        a                owl:ObjectProperty ;
        rdfs:domain      tran:TrafficArea ;
        rdfs:range       tran:TrafficAreaUsageValue ;
        skos:definition  "Specifies the actual uses of the TrafficArea."@en ;
        skos:prefLabel   "usage"@en .

tran:HoleSurface  a      owl:Class ;
        rdfs:subClassOf  core:AbstractThematicSurface ;
        skos:definition  "A HoleSurface is a representation of the ground surface of a hole."@en ;
        skos:prefLabel   "HoleSurface"@en .

tran:Railway.intersection
        a                owl:ObjectProperty ;
        rdfs:domain      tran:Railway ;
        rdfs:range       tran:Intersection ;
        skos:definition  "Relates to the intersections that are part of the Railway."@en ;
        skos:prefLabel   "intersection"@en .

tran:TransportationSpaceFunctionValue
        a                owl:Class ;
        rdfs:subClassOf  skos:Concept ;
        skos:definition  "TransportationSpaceFunctionValue is a code list that enumerates the different purposes of a TransportationSpace."@en ;
        skos:prefLabel   "TransportationSpaceFunctionValue"@en .

tran:Railway.function
        a                owl:ObjectProperty ;
        rdfs:domain      tran:Railway ;
        rdfs:range       tran:RailwayFunctionValue ;
        skos:definition  "Specifies the intended purposes of the Railway."@en ;
        skos:prefLabel   "function"@en .

tran:AuxiliaryTrafficSpaceFunctionValue
        a                owl:Class ;
        rdfs:subClassOf  skos:Concept ;
        skos:definition  "AuxiliaryTrafficSpaceFunctionValue is a code list that enumerates the different purposes of an AuxiliaryTrafficSpace."@en ;
        skos:prefLabel   "AuxiliaryTrafficSpaceFunctionValue"@en .

tran:Square  a           owl:Class ;
        rdfs:subClassOf  tran:AbstractTransportationSpace ;
        skos:definition  "A Square is a transportation space for unrestricted movement for vehicles, bicycles and/or pedestrians. This includes plazas as well as large sealed surfaces such as parking lots."@en ;
        skos:prefLabel   "Square"@en .

tran:ClearanceSpace.class
        a                owl:ObjectProperty ;
        rdfs:domain      tran:ClearanceSpace ;
        rdfs:range       tran:ClearanceSpaceClassValue ;
        skos:definition  "Indicates the specific type of the ClearanceSpace."@en ;
        skos:prefLabel   "class"@en .

tran:Railway.usage  a    owl:ObjectProperty ;
        rdfs:domain      tran:Railway ;
        rdfs:range       tran:RailwayUsageValue ;
        skos:definition  "Specifies the actual uses of the Railway."@en ;
        skos:prefLabel   "usage"@en .

tran:TrafficSpaceClassValue
        a                owl:Class ;
        rdfs:subClassOf  skos:Concept ;
        skos:definition  "TrafficSpaceClassValue is a code list used to further classify a TrafficSpace."@en ;
        skos:prefLabel   "TrafficSpaceClassValue"@en .

tran:AbstractTransportationSpace.trafficDirection
        a                owl:ObjectProperty ;
        rdfs:domain      tran:AbstractTransportationSpace ;
        rdfs:range       tran:TrafficDirectionValue ;
        skos:definition  "Indicates the direction of traffic flow relative to the corresponding linear geometry representation."@en ;
        skos:prefLabel   "trafficDirection"@en .

tran:WaterwayUsageValue
        a                owl:Class ;
        rdfs:subClassOf  skos:Concept ;
        skos:definition  "WaterwayUsageValue is a code list that enumerates the different uses of a Waterway."@en ;
        skos:prefLabel   "WaterwayUsageValue"@en .

tran:Waterway.section
        a                owl:ObjectProperty ;
        rdfs:domain      tran:Waterway ;
        rdfs:range       tran:Section ;
        skos:definition  "Relates to the sections that are part of the Waterway."@en ;
        skos:prefLabel   "section"@en .

tran:Waterway.class  a   owl:ObjectProperty ;
        rdfs:domain      tran:Waterway ;
        rdfs:range       tran:WaterwayClassValue ;
        skos:definition  "Indicates the specific type of the Waterway."@en ;
        skos:prefLabel   "class"@en .

tran:TrafficSpace.function
        a                owl:ObjectProperty ;
        rdfs:domain      tran:TrafficSpace ;
        rdfs:range       tran:TrafficSpaceFunctionValue ;
        skos:definition  "Specifies the intended purposes of the TrafficSpace."@en ;
        skos:prefLabel   "function"@en .

tran:AuxiliaryTrafficSpace.granularity
        a                owl:ObjectProperty ;
        rdfs:domain      tran:AuxiliaryTrafficSpace ;
        rdfs:range       tran:GranularityValue ;
        skos:definition  "Defines whether auxiliary traffic spaces are represented by individual ways or by individual lanes, depending on the desired level of detail."@en ;
        skos:prefLabel   "granularity"@en .

tran:AuxiliaryTrafficArea.usage
        a                owl:ObjectProperty ;
        rdfs:domain      tran:AuxiliaryTrafficArea ;
        rdfs:range       tran:AuxiliaryTrafficAreaUsageValue ;
        skos:definition  "Specifies the actual uses of the AuxiliaryTrafficArea."@en ;
        skos:prefLabel   "usage"@en .

tran:TransportationSpaceUsageValue
        a                owl:Class ;
        rdfs:subClassOf  skos:Concept ;
        skos:definition  "TransportationSpaceUsageValue is a code list that enumerates the different uses of a TransportationSpace."@en ;
        skos:prefLabel   "TransportationSpaceUsageValue"@en .

tran:ADEOfTrafficArea
        a                      owl:Class ;
        iso19150-2:isAbstract  true ;
        skos:definition        "ADEOfTrafficArea acts as a hook to define properties within an ADE that are to be added to a TrafficArea."@en ;
        skos:prefLabel         "ADEOfTrafficArea"@en .

tran:Railway  a          owl:Class ;
        rdfs:subClassOf  tran:AbstractTransportationSpace ;
        skos:definition  "A Railway is a transportation space used by wheeled vehicles on rails."@en ;
        skos:prefLabel   "Railway"@en .

tran:Track.intersection
        a                owl:ObjectProperty ;
        rdfs:domain      tran:Track ;
        rdfs:range       tran:Intersection ;
        skos:definition  "Relates to the intersections that are part of the Track."@en ;
        skos:prefLabel   "intersection"@en .

tran:Square.adeOfSquare
        a                owl:ObjectProperty ;
        rdfs:domain      tran:Square ;
        rdfs:range       tran:ADEOfSquare ;
        skos:definition  "Augments the Square with properties defined in an ADE."@en ;
        skos:prefLabel   "adeOfSquare"@en .

tran:ADEOfSquare  a            owl:Class ;
        iso19150-2:isAbstract  true ;
        skos:definition        "ADEOfSquare acts as a hook to define properties within an ADE that are to be added to a Square."@en ;
        skos:prefLabel         "ADEOfSquare"@en .

tran:TrafficSpace.adeOfTrafficSpace
        a                owl:ObjectProperty ;
        rdfs:domain      tran:TrafficSpace ;
        rdfs:range       tran:ADEOfTrafficSpace ;
        skos:definition  "Augments the TrafficSpace with properties defined in an ADE."@en ;
        skos:prefLabel   "adeOfTrafficSpace"@en .

tran:TrafficSpace.occupancy
        a                owl:ObjectProperty ;
        rdfs:domain      tran:TrafficSpace ;
        rdfs:range       core:Occupancy ;
        skos:definition  "Provides information on the residency of persons, vehicles, or other moving features in the TrafficSpace."@en ;
        skos:prefLabel   "occupancy"@en .

tran:TrafficDirectionValue
        a                rdfs:Datatype ;
        owl:oneOf        ( "forwards" "backwards" "both" ) ;
        skos:definition  "TrafficDirectionValue enumerates the allowed directions of travel of a mobile object."@en ;
        skos:prefLabel   "TrafficDirectionValue"@en .

tran:AuxiliaryTrafficSpace.adeOfAuxiliaryTrafficSpace
        a                owl:ObjectProperty ;
        rdfs:domain      tran:AuxiliaryTrafficSpace ;
        rdfs:range       tran:ADEOfAuxiliaryTrafficSpace ;
        skos:definition  "Augments the AuxiliaryTrafficSpace with properties defined in an ADE."@en ;
        skos:prefLabel   "adeOfAuxiliaryTrafficSpace"@en .

tran:TrafficArea.surfaceMaterial
        a                owl:ObjectProperty ;
        rdfs:domain      tran:TrafficArea ;
        rdfs:range       tran:SurfaceMaterialValue ;
        skos:definition  "Specifies the type of pavement of the TrafficArea."@en ;
        skos:prefLabel   "surfaceMaterial"@en .

tran:ADEOfHoleSurface
        a                      owl:Class ;
        iso19150-2:isAbstract  true ;
        skos:definition        "ADEOfHoleSurface acts as a hook to define properties within an ADE that are to be added to a HoleSurface."@en ;
        skos:prefLabel         "ADEOfHoleSurface"@en .

tran:AuxiliaryTrafficArea
        a                owl:Class ;
        rdfs:subClassOf  core:AbstractThematicSurface ;
        skos:definition  "An AuxiliaryTrafficArea is the ground surface of an AuxiliaryTrafficSpace."@en ;
        skos:prefLabel   "AuxiliaryTrafficArea"@en .

tran:AuxiliaryTrafficSpace.boundary
        a               owl:ObjectProperty ;
        rdfs:domain     tran:AuxiliaryTrafficSpace ;
        rdfs:range      tran:AuxiliaryTrafficArea ;
        skos:prefLabel  "boundary"@en .

tran:AbstractTransportationSpace.marking
        a                owl:ObjectProperty ;
        rdfs:domain      tran:AbstractTransportationSpace ;
        rdfs:range       tran:Marking ;
        skos:definition  "Relates to the markings that are part of the transportation space."@en ;
        skos:prefLabel   "marking"@en .

tran:SectionClassValue
        a                owl:Class ;
        rdfs:subClassOf  skos:Concept ;
        skos:definition  "SectionClassValue is a code list used to further classify a Section."@en ;
        skos:prefLabel   "SectionClassValue"@en .

tran:AbstractTransportationSpace.auxiliaryTrafficSpace
        a                owl:ObjectProperty ;
        rdfs:domain      tran:AbstractTransportationSpace ;
        rdfs:range       tran:AuxiliaryTrafficSpace ;
        skos:definition  "Relates to the auxiliary traffic spaces that are part of the transportation space."@en ;
        skos:prefLabel   "auxiliaryTrafficSpace"@en .

tran:ADEOfAbstractTransportationSpace
        a                      owl:Class ;
        iso19150-2:isAbstract  true ;
        skos:definition        "ADEOfAbstractTransportationSpace acts as a hook to define properties within an ADE that are to be added to AbstractTransportationSpace."@en ;
        skos:prefLabel         "ADEOfAbstractTransportationSpace"@en .

tran:ADEOfTrafficSpace
        a                      owl:Class ;
        iso19150-2:isAbstract  true ;
        skos:definition        "ADEOfTrafficSpace acts as a hook to define properties within an ADE that are to be added to a TrafficSpace."@en ;
        skos:prefLabel         "ADEOfTrafficSpace"@en .

tran:RoadFunctionValue
        a                owl:Class ;
        rdfs:subClassOf  skos:Concept ;
        skos:definition  "RoadFunctionValue is a code list that enumerates the different purposes of a Road."@en ;
        skos:prefLabel   "RoadFunctionValue"@en .

tran:Section.adeOfSection
        a                owl:ObjectProperty ;
        rdfs:domain      tran:Section ;
        rdfs:range       tran:ADEOfSection ;
        skos:definition  "Augments the Section with properties defined in an ADE."@en ;
        skos:prefLabel   "adeOfSection"@en .

tran:Track.class  a      owl:ObjectProperty ;
        rdfs:domain      tran:Track ;
        rdfs:range       tran:TrackClassValue ;
        skos:definition  "Indicates the specific type of the Track."@en ;
        skos:prefLabel   "class"@en .

tran:SquareClassValue
        a                owl:Class ;
        rdfs:subClassOf  skos:Concept ;
        skos:definition  "SquareClassValue is a code list used to further classify a Square."@en ;
        skos:prefLabel   "SquareClassValue"@en .

tran:TrafficSpace  a     owl:Class ;
        rdfs:subClassOf  core:AbstractUnoccupiedSpace ;
        skos:definition  "A TrafficSpace is a space in which traffic takes place. Traffic includes the movement of entities such as trains, vehicles, pedestrians, ships, or other transportation types."@en ;
        skos:prefLabel   "TrafficSpace"@en .

tran:Marking  a          owl:Class ;
        rdfs:subClassOf  core:AbstractThematicSurface ;
        skos:definition  "A Marking is a visible pattern on a transportation area relevant to the structuring or restriction of traffic. Examples are road markings and markings related to railway or waterway traffic."@en ;
        skos:prefLabel   "Marking"@en .

tran:ADEOfAuxiliaryTrafficArea
        a                      owl:Class ;
        iso19150-2:isAbstract  true ;
        skos:definition        "ADEOfAuxiliaryTrafficAra acts as a hook to define properties within an ADE that are to be added to an AuxiliaryTrafficArea."@en ;
        skos:prefLabel         "ADEOfAuxiliaryTrafficArea"@en .

tran:TrafficSpaceUsageValue
        a                owl:Class ;
        rdfs:subClassOf  skos:Concept ;
        skos:definition  "TrafficSpaceUsageValue is a code list that enumerates the different uses of a TrafficSpace."@en ;
        skos:prefLabel   "TrafficSpaceUsageValue"@en .

tran:Marking.adeOfMarking
        a                owl:ObjectProperty ;
        rdfs:domain      tran:Marking ;
        rdfs:range       tran:ADEOfMarking ;
        skos:definition  "Augments the Marking with properties defined in an ADE."@en ;
        skos:prefLabel   "adeOfMarking"@en .

tran:Section.class  a    owl:ObjectProperty ;
        rdfs:domain      tran:Section ;
        rdfs:range       tran:SectionClassValue ;
        skos:definition  "Indicates the specific type of the Section."@en ;
        skos:prefLabel   "class"@en .

tran:ADEOfRailway  a           owl:Class ;
        iso19150-2:isAbstract  true ;
        skos:definition        "ADEOfRailway acts as a hook to define properties within an ADE that are to be added to a Railway."@en ;
        skos:prefLabel         "ADEOfRailway"@en .

tran:Section  a          owl:Class ;
        rdfs:subClassOf  tran:AbstractTransportationSpace ;
        skos:definition  "A Section is a transportation space that is a segment of a Road, Railway, Track, or Waterway."@en ;
        skos:prefLabel   "Section"@en .

tran:AuxiliaryTrafficSpace.class
        a                owl:ObjectProperty ;
        rdfs:domain      tran:AuxiliaryTrafficSpace ;
        rdfs:range       tran:AuxiliaryTrafficSpaceClassValue ;
        skos:definition  "Indicates the specific type of the AuxiliaryTrafficSpace."@en ;
        skos:prefLabel   "class"@en .

tran:TrafficAreaClassValue
        a                owl:Class ;
        rdfs:subClassOf  skos:Concept ;
        skos:definition  "TrafficAreaClassValue is a code list used to further classify a TrafficArea."@en ;
        skos:prefLabel   "TrafficAreaClassValue"@en .

tran:Road.adeOfRoad  a   owl:ObjectProperty ;
        rdfs:domain      tran:Road ;
        rdfs:range       tran:ADEOfRoad ;
        skos:definition  "Augments the Road with properties defined in an ADE."@en ;
        skos:prefLabel   "adeOfRoad"@en .

tran:ADEOfWaterway  a          owl:Class ;
        iso19150-2:isAbstract  true ;
        skos:definition        "ADEOfWaterway acts as a hook to define properties within an ADE that are to be added to a Waterway."@en ;
        skos:prefLabel         "ADEOfWaterway"@en .

tran:AuxiliaryTrafficSpace.function
        a                owl:ObjectProperty ;
        rdfs:domain      tran:AuxiliaryTrafficSpace ;
        rdfs:range       tran:AuxiliaryTrafficSpaceFunctionValue ;
        skos:definition  "Specifies the intended purposes of the AuxiliaryTrafficSpace."@en ;
        skos:prefLabel   "function"@en .

tran:AuxiliaryTrafficSpaceClassValue
        a                owl:Class ;
        rdfs:subClassOf  skos:Concept ;
        skos:definition  "AuxiliaryTrafficSpaceClassValue is a code list used to further classify an AuxiliaryTrafficSpace."@en ;
        skos:prefLabel   "AuxiliaryTrafficSpaceClassValue"@en .

tran:Waterway.usage  a   owl:ObjectProperty ;
        rdfs:domain      tran:Waterway ;
        rdfs:range       tran:WaterwayUsageValue ;
        skos:definition  "Specifies the actual uses of the Waterway."@en ;
        skos:prefLabel   "usage"@en .

tran:Square.class  a     owl:ObjectProperty ;
        rdfs:domain      tran:Square ;
        rdfs:range       tran:SquareClassValue ;
        skos:definition  "Indicates the specific type of the Square."@en ;
        skos:prefLabel   "class"@en .

tran:ADEOfHole  a              owl:Class ;
        iso19150-2:isAbstract  true ;
        skos:definition        "ADEOfHole acts as a hook to define properties within an ADE that are to be added to a Hole."@en ;
        skos:prefLabel         "ADEOfHole"@en .

tran:TrafficSpace.class
        a                owl:ObjectProperty ;
        rdfs:domain      tran:TrafficSpace ;
        rdfs:range       tran:TrafficSpaceClassValue ;
        skos:definition  "Indicates the specific type of the TrafficSpace."@en ;
        skos:prefLabel   "class"@en .

tran:Waterway  a         owl:Class ;
        rdfs:subClassOf  tran:AbstractTransportationSpace ;
        skos:definition  "A Waterway is a transportation space used for the movement of vessels upon or within a water body."@en ;
        skos:prefLabel   "Waterway"@en .

tran:Road.section  a     owl:ObjectProperty ;
        rdfs:domain      tran:Road ;
        rdfs:range       tran:Section ;
        skos:definition  "Relates to the sections that are part of the Road."@en ;
        skos:prefLabel   "section"@en .

tran:TrackClassValue  a  owl:Class ;
        rdfs:subClassOf  skos:Concept ;
        skos:definition  "TrackClassValue is a code list used to further classify a Track."@en ;
        skos:prefLabel   "TrackClassValue"@en .

tran:SurfaceMaterialValue
        a                owl:Class ;
        rdfs:subClassOf  skos:Concept ;
        skos:definition  "SurfaceMaterialValue is a code list that enumerates the different surface materials."@en ;
        skos:prefLabel   "SurfaceMaterialValue"@en .

tran:ADEOfMarking  a           owl:Class ;
        iso19150-2:isAbstract  true ;
        skos:definition        "ADEOfMarking acts as a hook to define properties within an ADE that are to be added to a Marking."@en ;
        skos:prefLabel         "ADEOfMarking"@en .

tran:ClearanceSpace  a   owl:Class ;
        rdfs:subClassOf  core:AbstractUnoccupiedSpace ;
        skos:definition  "A ClearanceSpace represents the actual free space above a TrafficArea within which a mobile object can move without contacting an obstruction."@en ;
        skos:prefLabel   "ClearanceSpace"@en .

tran:RoadUsageValue  a   owl:Class ;
        rdfs:subClassOf  skos:Concept ;
        skos:definition  "RoadUsageValue is a code list that enumerates the different uses of a Road."@en ;
        skos:prefLabel   "RoadUsageValue"@en .

tran:HoleClassValue  a   owl:Class ;
        rdfs:subClassOf  skos:Concept ;
        skos:definition  "HoleClassValue is a code list used to further classify a Hole."@en ;
        skos:prefLabel   "HoleClassValue"@en .

tran:ADEOfTrack  a             owl:Class ;
        iso19150-2:isAbstract  true ;
        skos:definition        "ADEOfTrack acts as a hook to define properties within an ADE that are to be added to a Track."@en ;
        skos:prefLabel         "ADEOfTrack"@en .

tran:ADEOfRoad  a              owl:Class ;
        iso19150-2:isAbstract  true ;
        skos:definition        "ADEOfRoad acts as a hook to define properties within an ADE that are to be added to a Road."@en ;
        skos:prefLabel         "ADEOfRoad"@en .

tran:Track  a            owl:Class ;
        rdfs:subClassOf  tran:AbstractTransportationSpace ;
        skos:definition  "A Track is a small path mainly used by pedestrians. Tracks can be segmented into Sections and Intersections."@en ;
        skos:prefLabel   "Track"@en .

tran:ADEOfSection  a           owl:Class ;
        iso19150-2:isAbstract  true ;
        skos:definition        "ADEOfSection acts as a hook to define properties within an ADE that are to be added to a Section."@en ;
        skos:prefLabel         "ADEOfSection"@en .

tran:Waterway.intersection
        a                owl:ObjectProperty ;
        rdfs:domain      tran:Waterway ;
        rdfs:range       tran:Intersection ;
        skos:definition  "Relates to the intersections that are part of the Waterway."@en ;
        skos:prefLabel   "intersection"@en .

tran:ADEOfAuxiliaryTrafficSpace
        a                      owl:Class ;
        iso19150-2:isAbstract  true ;
        skos:definition        "ADEOfAuxiliaryTrafficSpace acts as a hook to define properties within an ADE that are to be added to an AuxiliaryTrafficSpace."@en ;
        skos:prefLabel         "ADEOfAuxiliaryTrafficSpace"@en .

tran:SquareUsageValue
        a                owl:Class ;
        rdfs:subClassOf  skos:Concept ;
        skos:definition  "SquareUsageValue is a code list that enumerates the different uses of a Square."@en ;
        skos:prefLabel   "SquareUsageValue"@en .

tran:Square.function  a  owl:ObjectProperty ;
        rdfs:domain      tran:Square ;
        rdfs:range       tran:SquareFunctionValue ;
        skos:definition  "Specifies the intended purposes of the Square."@en ;
        skos:prefLabel   "function"@en .

tran:TrackFunctionValue
        a                owl:Class ;
        rdfs:subClassOf  skos:Concept ;
        skos:definition  "TrackFunctionValue is a code list that enumerates the different purposes of a Track."@en ;
        skos:prefLabel   "TrackFunctionValue"@en .

tran:Hole.adeOfHole  a   owl:ObjectProperty ;
        rdfs:domain      tran:Hole ;
        rdfs:range       tran:ADEOfHole ;
        skos:definition  "Augments the Hole with properties defined in an ADE."@en ;
        skos:prefLabel   "adeOfHole"@en .

tran:Road.class  a       owl:ObjectProperty ;
        rdfs:domain      tran:Road ;
        rdfs:range       tran:RoadClassValue ;
        skos:definition  "Indicates the specific type of the Road."@en ;
        skos:prefLabel   "class"@en .

tran:TrafficAreaFunctionValue
        a                owl:Class ;
        rdfs:subClassOf  skos:Concept ;
        skos:definition  "TrafficAreaFunctionValue is a code list that enumerates the different purposes of a TrafficArea."@en ;
        skos:prefLabel   "TrafficAreaFunctionValue"@en .

tran:IntersectionClassValue
        a                owl:Class ;
        rdfs:subClassOf  skos:Concept ;
        skos:definition  "IntersectionClassValue is a code list used to further classify an Intersection."@en ;
        skos:prefLabel   "IntersectionClassValue"@en .

tran:TrafficAreaUsageValue
        a                owl:Class ;
        rdfs:subClassOf  skos:Concept ;
        skos:definition  "TrafficAreaUsageValue is a code list that enumerates the different uses of a TrafficArea."@en ;
        skos:prefLabel   "TrafficAreaUsageValue"@en .

tran:Track.section  a    owl:ObjectProperty ;
        rdfs:domain      tran:Track ;
        rdfs:range       tran:Section ;
        skos:definition  "Relates to the sections that are part of the Track."@en ;
        skos:prefLabel   "section"@en .

tran:Waterway.function
        a                owl:ObjectProperty ;
        rdfs:domain      tran:Waterway ;
        rdfs:range       tran:WaterwayFunctionValue ;
        skos:definition  "Specifies the intended purposes of the Waterway."@en ;
        skos:prefLabel   "function"@en .

tran:Waterway.adeOfWaterway
        a                owl:ObjectProperty ;
        rdfs:domain      tran:Waterway ;
        rdfs:range       tran:ADEOfWaterway ;
        skos:definition  "Augments the Waterway with properties defined in an ADE."@en ;
        skos:prefLabel   "adeOfWaterway"@en .

tran:AuxiliaryTrafficArea.function
        a                owl:ObjectProperty ;
        rdfs:domain      tran:AuxiliaryTrafficArea ;
        rdfs:range       tran:AuxiliaryTrafficAreaFunctionValue ;
        skos:definition  "Specifies the intended purposes of the AuxiliaryTrafficArea."@en ;
        skos:prefLabel   "function"@en .

tran:Track.usage  a      owl:ObjectProperty ;
        rdfs:domain      tran:Track ;
        rdfs:range       tran:TrackUsageValue ;
        skos:definition  "Specifies the actual uses of the Track."@en ;
        skos:prefLabel   "usage"@en .

tran:AuxiliaryTrafficAreaClassValue
        a                owl:Class ;
        rdfs:subClassOf  skos:Concept ;
        skos:definition  "AuxiliaryTrafficAreaClassValue is a code list used to further classify an AuxiliaryTrafficArea."@en ;
        skos:prefLabel   "AuxiliaryTrafficAreaClassValue"@en .

tran:MarkingClassValue
        a                owl:Class ;
        rdfs:subClassOf  skos:Concept ;
        skos:definition  "MarkingClassValue is a code list used to further classify a Marking."@en ;
        skos:prefLabel   "MarkingClassValue"@en .

tran:AuxiliaryTrafficSpaceUsageValue
        a                owl:Class ;
        rdfs:subClassOf  skos:Concept ;
        skos:definition  "AuxiliaryTrafficSpaceUsageValue is a code list that enumerates the different uses of an AuxiliaryTrafficSpace."@en ;
        skos:prefLabel   "AuxiliaryTrafficSpaceUsageValue"@en .

tran:RailwayFunctionValue
        a                owl:Class ;
        rdfs:subClassOf  skos:Concept ;
        skos:definition  "RailwayFunctionValue is a code list that enumerates the different purposes of a Railway."@en ;
        skos:prefLabel   "RailwayFunctionValue"@en .

tran:AuxiliaryTrafficSpace.usage
        a                owl:ObjectProperty ;
        rdfs:domain      tran:AuxiliaryTrafficSpace ;
        rdfs:range       tran:AuxiliaryTrafficSpaceUsageValue ;
        skos:definition  "Specifies the actual uses of the AuxiliaryTrafficSpace."@en ;
        skos:prefLabel   "usage"@en .

tran:TrafficSpace.successor
        a                owl:ObjectProperty ;
        rdfs:domain      tran:TrafficSpace ;
        rdfs:range       tran:TrafficSpace ;
        skos:definition  "Indicates the successor(s) of the TrafficSpace."@en ;
        skos:prefLabel   "successor"@en .

tran:WaterwayClassValue
        a                owl:Class ;
        rdfs:subClassOf  skos:Concept ;
        skos:definition  "WaterwayClassValue is a code list used to further classify a Waterway."@en ;
        skos:prefLabel   "WaterwayClassValue"@en .

tran:AbstractTransportationSpace.trafficSpace
        a                owl:ObjectProperty ;
        rdfs:domain      tran:AbstractTransportationSpace ;
        rdfs:range       tran:TrafficSpace ;
        skos:definition  "Relates to the traffic spaces that are part of the transportation space."@en ;
        skos:prefLabel   "trafficSpace"@en .

tran:GranularityValue
        a                rdfs:Datatype ;
        owl:oneOf        ( "lane" "way" ) ;
        skos:definition  "GranularityValue enumerates the different levels of granularity in which transportation objects are represented."@en ;
        skos:prefLabel   "GranularityValue"@en .

tran:ADEOfClearanceSpace
        a                      owl:Class ;
        iso19150-2:isAbstract  true ;
        skos:definition        "ADEOfClearanceSpace acts as a hook to define properties within an ADE that are to be added to a ClearanceSpace."@en ;
        skos:prefLabel         "ADEOfClearanceSpace"@en .

tran:TrackUsageValue  a  owl:Class ;
        rdfs:subClassOf  skos:Concept ;
        skos:definition  "TrackUsageValue is a code list that enumerates the different uses of a Track."@en ;
        skos:prefLabel   "TrackUsageValue"@en .

<https://github.com/VCityTeam/UD-Graph/Ontologies/transportation>
        a                owl:Ontology ;
        owl:imports      <https://github.com/VCityTeam/UD-Graph/Ontologies/core> , <http://def.isotc211.org/iso19150/-2/2012/base> ;
        owl:versionIRI   "https://github.com/VCityTeam/UD-Graph/Ontologies/transportation/3.0.0" ;
        owl:versionInfo  "3.0.0" ;
        skos:definition  "The Transportation module supports representation of the transportation infrastructure. Transportation features include roads, tracks, waterways, railways, and squares. Transportation features may be represented as a network and/or as a collection of spaces or surface elements embedded in a three-dimensional space."@en ;
        skos:prefLabel   "Transportation"@en .

tran:TransportationSpaceClassValue
        a                owl:Class ;
        rdfs:subClassOf  skos:Concept ;
        skos:definition  "TransportationSpaceClassValue is a code list used to further classify a TransportationSpace."@en ;
        skos:prefLabel   "TransportationSpaceClassValue"@en .

tran:TrafficSpace.granularity
        a                owl:ObjectProperty ;
        rdfs:domain      tran:TrafficSpace ;
        rdfs:range       tran:GranularityValue ;
        skos:definition  "Defines whether traffic spaces are represented by individual ways or by individual lanes, depending on the desired level of detail."@en ;
        skos:prefLabel   "granularity"@en .

tran:AuxiliaryTrafficArea.surfaceMaterial
        a                owl:ObjectProperty ;
        rdfs:domain      tran:AuxiliaryTrafficArea ;
        rdfs:range       tran:SurfaceMaterialValue ;
        skos:definition  "Specifies the type of pavement of the AuxiliaryTrafficArea."@en ;
        skos:prefLabel   "surfaceMaterial"@en .

tran:AuxiliaryTrafficSpace
        a                owl:Class ;
        rdfs:subClassOf  core:AbstractUnoccupiedSpace ;
        skos:definition  "An AuxiliaryTrafficSpace is a space within the transportation space not intended for traffic purposes."@en ;
        skos:prefLabel   "AuxiliaryTrafficSpace"@en .

tran:Intersection.class
        a                owl:ObjectProperty ;
        rdfs:domain      tran:Intersection ;
        rdfs:range       tran:IntersectionClassValue ;
        skos:definition  "Indicates the specific type of the Intersection."@en ;
        skos:prefLabel   "class"@en .

tran:TrafficArea.class
        a                owl:ObjectProperty ;
        rdfs:domain      tran:TrafficArea ;
        rdfs:range       tran:TrafficAreaClassValue ;
        skos:definition  "Indicates the specific type of the TrafficArea."@en ;
        skos:prefLabel   "class"@en .

tran:SquareFunctionValue
        a                owl:Class ;
        rdfs:subClassOf  skos:Concept ;
        skos:definition  "SquareFunctionValue is a code list that enumerates the different purposes of a Square."@en ;
        skos:prefLabel   "SquareFunctionValue"@en .

tran:TrafficSpace.usage
        a                owl:ObjectProperty ;
        rdfs:domain      tran:TrafficSpace ;
        rdfs:range       tran:TrafficSpaceUsageValue ;
        skos:definition  "Specifies the actual uses of the TrafficSpace."@en ;
        skos:prefLabel   "usage"@en .

tran:AbstractTransportationSpace.hole
        a                owl:ObjectProperty ;
        rdfs:domain      tran:AbstractTransportationSpace ;
        rdfs:range       tran:Hole ;
        skos:definition  "Relates to the holes that are part of the transportation space."@en ;
        skos:prefLabel   "hole"@en .

tran:Square.usage  a     owl:ObjectProperty ;
        rdfs:domain      tran:Square ;
        rdfs:range       tran:SquareUsageValue ;
        skos:definition  "Specifies the actual uses of the Square."@en ;
        skos:prefLabel   "usage"@en .

tran:RailwayClassValue
        a                owl:Class ;
        rdfs:subClassOf  skos:Concept ;
        skos:definition  "RailwayClassValue is a code list used to further classify a Railway."@en ;
        skos:prefLabel   "RailwayClassValue"@en .

tran:AbstractTransportationSpace.occupancy
        a                owl:ObjectProperty ;
        rdfs:domain      tran:AbstractTransportationSpace ;
        rdfs:range       core:Occupancy ;
        skos:definition  "Provides information on the residency of persons, vehicles, or other moving features in the transportation space."@en ;
        skos:prefLabel   "occupancy"@en .

tran:Railway.class  a    owl:ObjectProperty ;
        rdfs:domain      tran:Railway ;
        rdfs:range       tran:RailwayClassValue ;
        skos:definition  "Indicates the specific type of the Railway."@en ;
        skos:prefLabel   "class"@en .

tran:HoleSurface.adeOfHoleSurface
        a                owl:ObjectProperty ;
        rdfs:domain      tran:HoleSurface ;
        rdfs:range       tran:ADEOfHoleSurface ;
        skos:definition  "Augments the HoleSurface with properties defined in an ADE."@en ;
        skos:prefLabel   "adeOfHoleSurface"@en .

tran:TrafficSpace.trafficDirection
        a                owl:ObjectProperty ;
        rdfs:domain      tran:TrafficSpace ;
        rdfs:range       tran:TrafficDirectionValue ;
        skos:definition  "Indicates the direction of traffic flow relative to the corresponding linear geometry representation."@en ;
        skos:prefLabel   "trafficDirection"@en .

tran:Intersection.adeOfIntersection
        a                owl:ObjectProperty ;
        rdfs:domain      tran:Intersection ;
        rdfs:range       tran:ADEOfIntersection ;
        skos:definition  "Augments the Intersection with properties defined in an ADE."@en ;
        skos:prefLabel   "adeOfIntersection"@en .

tran:AuxiliaryTrafficAreaUsageValue
        a                owl:Class ;
        rdfs:subClassOf  skos:Concept ;
        skos:definition  "AuxiliaryTrafficAreaUsageValue is a code list that enumerates the different uses of an AuxiliaryTrafficArea."@en ;
        skos:prefLabel   "AuxiliaryTrafficAreaUsageValue"@en .

tran:ADEOfIntersection
        a                      owl:Class ;
        iso19150-2:isAbstract  true ;
        skos:definition        "ADEOfIntersection acts as a hook to define properties within an ADE that are to be added to an Intersection."@en ;
        skos:prefLabel         "ADEOfIntersection"@en .

tran:Hole.class  a       owl:ObjectProperty ;
        rdfs:domain      tran:Hole ;
        rdfs:range       tran:HoleClassValue ;
        skos:definition  "Indicates the specific type of the Hole."@en ;
        skos:prefLabel   "class"@en .

tran:AbstractTransportationSpace.adeOfAbstractTransportationSpace
        a                owl:ObjectProperty ;
        rdfs:domain      tran:AbstractTransportationSpace ;
        rdfs:range       tran:ADEOfAbstractTransportationSpace ;
        skos:definition  "Augments AbstractTransportationSpace with properties defined in an ADE."@en ;
        skos:prefLabel   "adeOfAbstractTransportationSpace"@en .
